<?xml version="1.0" encoding="utf-8"?>
<processDataSet xmlns:epd="http://www.iai.kit.edu/EPD/2013" xmlns:epd2="http://www.indata.network/EPD/2019" xmlns:common="http://lca.jrc.it/ILCD/Common" xsi:schemaLocation="http://lca.jrc.it/ILCD/Process ../../schemas/EPD_DataSet.xsd" epd2:epd-version="1.2" version="1.1" locations="../ILCDLocations.xml" xmlns:xsi="http://www.w3.org/2001/XMLSchema-instance" xmlns="http://lca.jrc.it/ILCD/Process">
<processInformation>
<dataSetInformation>
<common:UUID>0cd9a40d-dc97-4ca8-92ba-9dd80a68b579</common:UUID>
<name>
<baseName xml:lang="en">Mineral pre-made mortar: rendering and plastering mortar – normal/finishing render or plaster</baseName>
<functionalUnitFlowProperties xml:lang="en" />
</name>
<classificationInformation>
<common:classification name="OEKOBAU.DAT">
<common:class level="0" classId="1">Mineralische Baustoffe</common:class>
<common:class level="1" classId="1.4">Mörtel und Beton</common:class>
<common:class level="2" classId="1.4.04">Putz und Putzmörtel</common:class>
</common:classification>
<common:classification name="IBUCategories">
<common:class level="0">02 Building products</common:class>
<common:class level="1">Masonry and related products</common:class>
<common:class level="2">Mineral factory-made mortar</common:class>
</common:classification>
</classificationInformation>
<common:generalComment xml:lang="en">Mineral pre-made mortars are mortars whose components are mixed at the factory and not on the construction site. They are divided into three different types – masonry mortar, rendering and plastering mortar, and screed material – depending on the type of application.  Mineral rendering and plastering mortars are mixtures of one or more mineral binders, aggregates, water, and – if applicable – additions or admixtures for the manufacture of renders or plasters. Rendering and plastering mortars are applied to walls and ceilings in one or more layers as required. Alongside the aesthetic design of the surface, they protect against effects of the weather when used as external renders and provide an even substrate for paint coats and wallpaper when used as internal plasters. In the case of reinforced concrete ceilings and stairs, renders/plasters also serve as fire protection; when porous aggregates are added, they serve as thermal protection. Depending on the technical data, the base materials and processing aids used, and the practical application, rendering and plastering mortars are divided into the following product groups: normal/finishing render or plaster, normal/finishing render, or plaster with special properties, lightweight render, reinforcement fibre plaster, and insulating render with an especially high proportion of lightweight aggregates.  Placing normal/finishing render or plaster on the market in the EU/EFTA (with the exception of Switzerland) is subject to Regulation (EU) No. 305/2011 (CPR). Normal/finishing render or plaster requires a declaration of performance – taking into consideration DIN EN 998-1:2017-02, Specification for mortar for masonry - Part 1: Rendering and plastering mortar – and the CE marking. The relevant national regulations apply with regard to usage.</common:generalComment>
</dataSetInformation>
<quantitativeReference>
<referenceToReferenceFlow>0</referenceToReferenceFlow>
</quantitativeReference>
<time>
<common:referenceYear>2021</common:referenceYear>
<common:dataSetValidUntil>2026</common:dataSetValidUntil>
<common:other>
<epd2:publicationDateOfEPD>2021-07-07</epd2:publicationDateOfEPD>
</common:other>
</time>
<geography>
<locationOfOperationSupplyOrProduction location="RER" />
</geography>
<technology>
<technologyDescriptionAndIncludedProcesses xml:lang="en">The graphic shows the manufacturing process. Mineral rendering and plastering mortars are made in mixing plants in the following steps: Filling of the storage or weighing containers Conveyance of ingredients and substances being mixed into the mixer Mixing Conveyance of finished products Packaging Loading and shipping of the finished product The raw materials – sand, binder, lightweight aggregates, processing aids, admixtures, and additions (see base materials) – are stored at the manufacturing plant in silos. From the silos, the raw materials are gravimetrically dosed and intensely mixed according to the respective formulation. The mixture is then packaged and shipped dry as pre-made dry mortar in containers or silos. Graphic 1: Manufacturing process (green: input; blue: unit process) 
Declared unit: 
This declaration refers to the production of one kilogram of typical rendering mortar of the normal/finishing render product group. Only dry mortars are taken into consideration.</technologyDescriptionAndIncludedProcesses>
<technologicalApplicability xml:lang="en">Rendering and plastering mortars produced in the factory for use as a base coat or finishing render/plaster on walls, ceilings, piers, and separating walls of structures which comply with the applicable standards or on similar backgrounds (e.g. in the case of existing buildings).  Normal render for the production of internal plaster and external render without special properties.</technologicalApplicability>
</technology>
</processInformation>
<modellingAndValidation>
<LCIMethodAndAllocation>
<typeOfDataSet>EPD</typeOfDataSet>
<referenceToLCAMethodDetails type="source data set" refObjectId="cd66dab2-6ff4-49ba-8701-afc1d7ca8986">
<common:shortDescription xml:lang="en">Mineral factory-made mortar.pdf</common:shortDescription>
</referenceToLCAMethodDetails>
<common:other>
<epd:subType xmlns="http://www.iai.kit.edu/EPD/2013">average dataset</epd:subType>
</common:other>
</LCIMethodAndAllocation>
<dataSourcesTreatmentAndRepresentativeness>
<referenceToDataSource type="source data set" refObjectId="28d74cc0-db8b-4d7e-bc44-5f6d56ce0c4a">
<common:shortDescription xml:lang="en">GaBi Database (all versions)</common:shortDescription>
</referenceToDataSource>
<referenceToDataSource type="source data set" refObjectId="dad5023c-8d97-4656-b82a-2fc6480b33a7">
<common:shortDescription xml:lang="en">GaBi database SP36 2018</common:shortDescription>
</referenceToDataSource>
<useAdviceForDataSet xml:lang="en">Scope: 
This document is a model EPD. When calculating the Life Cycle Assessment, the product selected to represent the group in question was the product with the highest environmental impact in that group. This EPD applies exclusively to rendering and plastering mortar – normal/finishing render or plaster as mineral pre-made mortars for association members; these can be found on the association’s website. Any numerical values – e.g. for constructional data or concentration specifications – are average values that are customary in practice for this product group. 
System boundary: 
The lifecycle analysis of the products being examined encompasses the production of the mortar including raw material extraction and the provision of energy sources up to the packaged, finished product (module A1-A3), the application of the product including transportation to the construction site (module A4-A5), the usage phase (module B1), and disposal of the mortar (module C4). For silo-based goods, the proportionate expenditure for transportation and manufacturing of the silo is taken into account. Credit for packaging including energy recovery (module D) is also incorporated into the Life Cycle Assessment.</useAdviceForDataSet>
<common:other>
<epd2:referenceToOriginalEPD type="source data set" refObjectId="fa91645d-0b47-40ec-b811-6f1ff27e5db5">
<common:shortDescription xml:lang="en">Mineral pre-made mortar: rendering and plastering mortar – normal/finishing render or plaster.pdf</common:shortDescription>
</epd2:referenceToOriginalEPD>
</common:other>
</dataSourcesTreatmentAndRepresentativeness>
<validation>
<review type="Accredited third party review">
<common:referenceToNameOfReviewerAndInstitution uri="../contacts/d111dbec-b024-4be5-86c5-752d6eb2cf95.xml" type="contact data set" refObjectId="d111dbec-b024-4be5-86c5-752d6eb2cf95">
<common:shortDescription xml:lang="en">Institut Bauen und Umwelt e. V.</common:shortDescription>
</common:referenceToNameOfReviewerAndInstitution>
</review>
</validation>
<complianceDeclarations>
<compliance>
<common:referenceToComplianceSystem uri="../sources/b00f9ec0-7874-11e3-981f-0800200c9a66.xml" type="source data set" refObjectId="b00f9ec0-7874-11e3-981f-0800200c9a66">
<common:shortDescription xml:lang="en">DIN EN 15804</common:shortDescription>
</common:referenceToComplianceSystem>
</compliance>
<compliance>
<common:referenceToComplianceSystem uri="../sources/4f2eb655-6e44-4874-a95a-e28f5442cd4d.xml" type="source data set" refObjectId="4f2eb655-6e44-4874-a95a-e28f5442cd4d">
<common:shortDescription xml:lang="en">ISO 14025</common:shortDescription>
</common:referenceToComplianceSystem>
</compliance>
</complianceDeclarations>
</modellingAndValidation>
<administrativeInformation>
<common:commissionerAndGoal>
<common:referenceToCommissioner uri="../contacts/d1f9cf21-554b-41a8-976f-83ff8dfe6987.xml" type="contact data set" refObjectId="d1f9cf21-554b-41a8-976f-83ff8dfe6987">
<common:shortDescription xml:lang="en">Sto SE &amp; Co. KGaA</common:shortDescription>
</common:referenceToCommissioner>
</common:commissionerAndGoal>
<dataGenerator>
<common:referenceToPersonOrEntityGeneratingTheDataSet uri="../contacts/623edf96-39d1-4e6f-9892-674c7228546b.xml" type="contact data set" refObjectId="623edf96-39d1-4e6f-9892-674c7228546b">
<common:shortDescription xml:lang="en">Sphera Solutions GmbH</common:shortDescription>
</common:referenceToPersonOrEntityGeneratingTheDataSet>
</dataGenerator>
<dataEntryBy>
<common:timeStamp>2021-07-07T17:55:56.774</common:timeStamp>
<common:referenceToDataSetFormat uri="../sources/a97a0155-0234-4b87-b4ce-a45da52f2a40.xml" type="source data set" refObjectId="a97a0155-0234-4b87-b4ce-a45da52f2a40">
<common:shortDescription xml:lang="en">ILCD Format</common:shortDescription>
</common:referenceToDataSetFormat>
<common:referenceToDataSetFormat uri="../sources/a29449fd-aa2f-4de8-b5d7-4b06b43c6fde.xml" type="source data set" refObjectId="a29449fd-aa2f-4de8-b5d7-4b06b43c6fde">
<common:shortDescription xml:lang="de">EPD-Datenformaterweiterungen v1.2</common:shortDescription>
<common:shortDescription xml:lang="en">EPD Data Format Extensions v1.2</common:shortDescription>
</common:referenceToDataSetFormat>
</dataEntryBy>
<publicationAndOwnership>
<common:dataSetVersion>00.01.000</common:dataSetVersion>
<common:referenceToPrecedingDataSetVersion uri="../processes/7c040c63-505d-4970-9333-d6bbdf425ea9.xml" type="process data set" refObjectId="7c040c63-505d-4970-9333-d6bbdf425ea9">
<common:shortDescription xml:lang="en">Rendering mortar – normal/finishing render</common:shortDescription>
</common:referenceToPrecedingDataSetVersion>
<common:referenceToRegistrationAuthority uri="../contacts/d111dbec-b024-4be5-86c5-752d6eb2cf95.xml" type="contact data set" refObjectId="d111dbec-b024-4be5-86c5-752d6eb2cf95">
<common:shortDescription xml:lang="en">Institut Bauen und Umwelt e. V.</common:shortDescription>
</common:referenceToRegistrationAuthority>
<common:registrationNumber>EPD-IWM-STO-20210128-IBG1-DE</common:registrationNumber>
<common:referenceToOwnershipOfDataSet uri="../contacts/d1f9cf21-554b-41a8-976f-83ff8dfe6987.xml" type="contact data set" refObjectId="d1f9cf21-554b-41a8-976f-83ff8dfe6987">
<common:shortDescription xml:lang="en">Sto SE &amp; Co. KGaA</common:shortDescription>
</common:referenceToOwnershipOfDataSet>
<common:copyright>true</common:copyright>
<common:licenseType>Free of charge for all users and uses</common:licenseType>
<common:accessRestrictions xml:lang="en">None</common:accessRestrictions>
<common:other>
<epd2:referenceToPublisher type="contact data set" refObjectId="d111dbec-b024-4be5-86c5-752d6eb2cf95" uri="../contacts/d111dbec-b024-4be5-86c5-752d6eb2cf95.xml">
<common:shortDescription xml:lang="en">Institut Bauen und Umwelt e. V.</common:shortDescription>
</epd2:referenceToPublisher>
</common:other>
</publicationAndOwnership>
</administrativeInformation>
<exchanges>
<exchange dataSetInternalID="0">
<referenceToFlowDataSet uri="../flows/0d173a1f-72f4-49e8-9145-efec9a6bdb03.xml" type="flow data set" refObjectId="0d173a1f-72f4-49e8-9145-efec9a6bdb03">
<common:shortDescription xml:lang="en">1 kg Rendering mortar – normal/finishing render (1 kg rendering mortar – normal/finishing render)</common:shortDescription>
</referenceToFlowDataSet>
<meanAmount>1</meanAmount>
<referencesToDataSource />
</exchange>
<exchange dataSetInternalID="1">
<referenceToFlowDataSet uri="../flows/20f32be5-0398-4288-9b6d-accddd195317.xml" type="flow data set" refObjectId="20f32be5-0398-4288-9b6d-accddd195317">
<common:shortDescription xml:lang="en">Renewable primary energy as energy carrier (PERE)</common:shortDescription>
</referenceToFlowDataSet>
<functionType>General reminder flow</functionType>
<exchangeDirection>Input</exchangeDirection>
<common:other>
<epd:referenceToUnitGroupDataSet uri="../unitgroups/93a60a57-a3c8-11da-a746-0800200c9a66.xml" type="unit group data set" refObjectId="93a60a57-a3c8-11da-a746-0800200c9a66">
<common:shortDescription xml:lang="en">MJ</common:shortDescription>
</epd:referenceToUnitGroupDataSet>
<epd:amount epd:module="A1-A3">0.396</epd:amount>
<epd:amount epd:module="A4">0.0197</epd:amount>
<epd:amount epd:module="A5">0.28837</epd:amount>
<epd:amount epd:module="B1">0</epd:amount>
<epd:amount epd:module="C4">0.0276</epd:amount>
<epd:amount epd:module="D">-0.0523</epd:amount>
</common:other>
</exchange>
<exchange dataSetInternalID="2">
<referenceToFlowDataSet uri="../flows/fb3ec0de-548d-4508-aea5-00b73bf6f702.xml" type="flow data set" refObjectId="fb3ec0de-548d-4508-aea5-00b73bf6f702">
<common:shortDescription xml:lang="en">Renewable primary energy resources as material utilization (PERM)</common:shortDescription>
</referenceToFlowDataSet>
<functionType>General reminder flow</functionType>
<exchangeDirection>Input</exchangeDirection>
<common:other>
<epd:referenceToUnitGroupDataSet uri="../unitgroups/93a60a57-a3c8-11da-a746-0800200c9a66.xml" type="unit group data set" refObjectId="93a60a57-a3c8-11da-a746-0800200c9a66">
<common:shortDescription xml:lang="en">MJ</common:shortDescription>
</epd:referenceToUnitGroupDataSet>
<epd:amount epd:module="A1-A3">0.286</epd:amount>
<epd:amount epd:module="A4">0</epd:amount>
<epd:amount epd:module="A5">-0.286</epd:amount>
<epd:amount epd:module="B1">0</epd:amount>
<epd:amount epd:module="C4">0</epd:amount>
<epd:amount epd:module="D">0</epd:amount>
</common:other>
</exchange>
<exchange dataSetInternalID="3">
<referenceToFlowDataSet uri="../flows/53f97275-fa8a-4cdd-9024-65936002acd0.xml" type="flow data set" refObjectId="53f97275-fa8a-4cdd-9024-65936002acd0">
<common:shortDescription xml:lang="en">Total use of renewable primary energy resources (PERT)</common:shortDescription>
</referenceToFlowDataSet>
<functionType>General reminder flow</functionType>
<exchangeDirection>Input</exchangeDirection>
<common:other>
<epd:referenceToUnitGroupDataSet uri="../unitgroups/93a60a57-a3c8-11da-a746-0800200c9a66.xml" type="unit group data set" refObjectId="93a60a57-a3c8-11da-a746-0800200c9a66">
<common:shortDescription xml:lang="en">MJ</common:shortDescription>
</epd:referenceToUnitGroupDataSet>
<epd:amount epd:module="A1-A3">0.682</epd:amount>
<epd:amount epd:module="A4">0.0197</epd:amount>
<epd:amount epd:module="A5">0.00237</epd:amount>
<epd:amount epd:module="B1">0</epd:amount>
<epd:amount epd:module="C4">0.0276</epd:amount>
<epd:amount epd:module="D">-0.0523</epd:amount>
</common:other>
</exchange>
<exchange dataSetInternalID="4">
<referenceToFlowDataSet uri="../flows/ac857178-2b45-46ec-892a-a9a4332f0372.xml" type="flow data set" refObjectId="ac857178-2b45-46ec-892a-a9a4332f0372">
<common:shortDescription xml:lang="en">Non renewable primary energy as energy carrier (PENRE)</common:shortDescription>
</referenceToFlowDataSet>
<functionType>General reminder flow</functionType>
<exchangeDirection>Input</exchangeDirection>
<common:other>
<epd:referenceToUnitGroupDataSet uri="../unitgroups/93a60a57-a3c8-11da-a746-0800200c9a66.xml" type="unit group data set" refObjectId="93a60a57-a3c8-11da-a746-0800200c9a66">
<common:shortDescription xml:lang="en">MJ</common:shortDescription>
</epd:referenceToUnitGroupDataSet>
<epd:amount epd:module="A1-A3">1.503</epd:amount>
<epd:amount epd:module="A4">0.293</epd:amount>
<epd:amount epd:module="A5">0.0493</epd:amount>
<epd:amount epd:module="B1">0</epd:amount>
<epd:amount epd:module="C4">0.222</epd:amount>
<epd:amount epd:module="D">-0.253</epd:amount>
</common:other>
</exchange>
<exchange dataSetInternalID="5">
<referenceToFlowDataSet uri="../flows/1421caa0-679d-4bf4-b282-0eb850ccae27.xml" type="flow data set" refObjectId="1421caa0-679d-4bf4-b282-0eb850ccae27">
<common:shortDescription xml:lang="en">Non renewable primary energy as material utilization (PENRM)</common:shortDescription>
</referenceToFlowDataSet>
<functionType>General reminder flow</functionType>
<exchangeDirection>Input</exchangeDirection>
<common:other>
<epd:referenceToUnitGroupDataSet uri="../unitgroups/93a60a57-a3c8-11da-a746-0800200c9a66.xml" type="unit group data set" refObjectId="93a60a57-a3c8-11da-a746-0800200c9a66">
<common:shortDescription xml:lang="en">MJ</common:shortDescription>
</epd:referenceToUnitGroupDataSet>
<epd:amount epd:module="A1-A3">0.037</epd:amount>
<epd:amount epd:module="A4">0</epd:amount>
<epd:amount epd:module="A5">-0.037</epd:amount>
<epd:amount epd:module="B1">0</epd:amount>
<epd:amount epd:module="C4">0</epd:amount>
<epd:amount epd:module="D">0</epd:amount>
</common:other>
</exchange>
<exchange dataSetInternalID="6">
<referenceToFlowDataSet uri="../flows/06159210-646b-4c8d-8583-da9b3b95a6c1.xml" type="flow data set" refObjectId="06159210-646b-4c8d-8583-da9b3b95a6c1">
<common:shortDescription xml:lang="en">Total use of non renewable primary energy resources (PENRT)</common:shortDescription>
</referenceToFlowDataSet>
<functionType>General reminder flow</functionType>
<exchangeDirection>Input</exchangeDirection>
<common:other>
<epd:referenceToUnitGroupDataSet uri="../unitgroups/93a60a57-a3c8-11da-a746-0800200c9a66.xml" type="unit group data set" refObjectId="93a60a57-a3c8-11da-a746-0800200c9a66">
<common:shortDescription xml:lang="en">MJ</common:shortDescription>
</epd:referenceToUnitGroupDataSet>
<epd:amount epd:module="A1-A3">1.54</epd:amount>
<epd:amount epd:module="A4">0.293</epd:amount>
<epd:amount epd:module="A5">0.0123</epd:amount>
<epd:amount epd:module="B1">0</epd:amount>
<epd:amount epd:module="C4">0.222</epd:amount>
<epd:amount epd:module="D">-0.253</epd:amount>
</common:other>
</exchange>
<exchange dataSetInternalID="7">
<referenceToFlowDataSet uri="../flows/c6a1f35f-2d09-4f54-8dfb-97e502e1ce92.xml" type="flow data set" refObjectId="c6a1f35f-2d09-4f54-8dfb-97e502e1ce92">
<common:shortDescription xml:lang="en">Use of secondary material (SM)</common:shortDescription>
</referenceToFlowDataSet>
<functionType>General reminder flow</functionType>
<exchangeDirection>Input</exchangeDirection>
<common:other>
<epd:referenceToUnitGroupDataSet uri="../unitgroups/ad38d542-3fe9-439d-9b95-2f5f7752acaf.xml" type="unit group data set" refObjectId="ad38d542-3fe9-439d-9b95-2f5f7752acaf">
<common:shortDescription xml:lang="en">kg</common:shortDescription>
</epd:referenceToUnitGroupDataSet>
<epd:amount epd:module="A1-A3">0</epd:amount>
<epd:amount epd:module="A4">0</epd:amount>
<epd:amount epd:module="A5">0</epd:amount>
<epd:amount epd:module="B1">0</epd:amount>
<epd:amount epd:module="C4">0</epd:amount>
<epd:amount epd:module="D">0</epd:amount>
</common:other>
</exchange>
<exchange dataSetInternalID="8">
<referenceToFlowDataSet uri="../flows/64333088-a55f-4aa2-9a31-c10b07816787.xml" type="flow data set" refObjectId="64333088-a55f-4aa2-9a31-c10b07816787">
<common:shortDescription xml:lang="en">Use of renewable secondary fuels (RSF)</common:shortDescription>
</referenceToFlowDataSet>
<functionType>General reminder flow</functionType>
<exchangeDirection>Input</exchangeDirection>
<common:other>
<epd:referenceToUnitGroupDataSet uri="../unitgroups/93a60a57-a3c8-11da-a746-0800200c9a66.xml" type="unit group data set" refObjectId="93a60a57-a3c8-11da-a746-0800200c9a66">
<common:shortDescription xml:lang="en">MJ</common:shortDescription>
</epd:referenceToUnitGroupDataSet>
<epd:amount epd:module="A1-A3">0</epd:amount>
<epd:amount epd:module="A4">0</epd:amount>
<epd:amount epd:module="A5">0</epd:amount>
<epd:amount epd:module="B1">0</epd:amount>
<epd:amount epd:module="C4">0</epd:amount>
<epd:amount epd:module="D">0</epd:amount>
</common:other>
</exchange>
<exchange dataSetInternalID="9">
<referenceToFlowDataSet uri="../flows/89def144-d39a-4287-b86f-efde453ddcb2.xml" type="flow data set" refObjectId="89def144-d39a-4287-b86f-efde453ddcb2">
<common:shortDescription xml:lang="en">Use of non renewable secondary fuels (NRSF)</common:shortDescription>
</referenceToFlowDataSet>
<functionType>General reminder flow</functionType>
<exchangeDirection>Input</exchangeDirection>
<common:other>
<epd:referenceToUnitGroupDataSet uri="../unitgroups/93a60a57-a3c8-11da-a746-0800200c9a66.xml" type="unit group data set" refObjectId="93a60a57-a3c8-11da-a746-0800200c9a66">
<common:shortDescription xml:lang="en">MJ</common:shortDescription>
</epd:referenceToUnitGroupDataSet>
<epd:amount epd:module="A1-A3">0</epd:amount>
<epd:amount epd:module="A4">0</epd:amount>
<epd:amount epd:module="A5">0</epd:amount>
<epd:amount epd:module="B1">0</epd:amount>
<epd:amount epd:module="C4">0</epd:amount>
<epd:amount epd:module="D">0</epd:amount>
</common:other>
</exchange>
<exchange dataSetInternalID="10">
<referenceToFlowDataSet uri="../flows/3cf952c8-f3a4-461d-8c96-96456ca62246.xml" type="flow data set" refObjectId="3cf952c8-f3a4-461d-8c96-96456ca62246">
<common:shortDescription xml:lang="en">Use of net fresh water (FW)</common:shortDescription>
</referenceToFlowDataSet>
<functionType>General reminder flow</functionType>
<exchangeDirection>Input</exchangeDirection>
<common:other>
<epd:referenceToUnitGroupDataSet uri="../unitgroups/cd950537-0a98-4044-9ba7-9f9a68d0a504.xml" type="unit group data set" refObjectId="cd950537-0a98-4044-9ba7-9f9a68d0a504">
<common:shortDescription xml:lang="en">m^3</common:shortDescription>
</epd:referenceToUnitGroupDataSet>
<epd:amount epd:module="A1-A3">0.00444</epd:amount>
<epd:amount epd:module="A4">2.29E-05</epd:amount>
<epd:amount epd:module="A5">0.000402</epd:amount>
<epd:amount epd:module="B1">0</epd:amount>
<epd:amount epd:module="C4">4.23E-05</epd:amount>
<epd:amount epd:module="D">-3.33E-05</epd:amount>
</common:other>
</exchange>
<exchange dataSetInternalID="11">
<referenceToFlowDataSet uri="../flows/430f9e0f-59b2-46a0-8e0d-55e0e84948fc.xml" type="flow data set" refObjectId="430f9e0f-59b2-46a0-8e0d-55e0e84948fc">
<common:shortDescription xml:lang="en">Hazardous waste disposed (HWD)</common:shortDescription>
</referenceToFlowDataSet>
<functionType>General reminder flow</functionType>
<exchangeDirection>Output</exchangeDirection>
<common:other>
<epd:referenceToUnitGroupDataSet uri="../unitgroups/ad38d542-3fe9-439d-9b95-2f5f7752acaf.xml" type="unit group data set" refObjectId="ad38d542-3fe9-439d-9b95-2f5f7752acaf">
<common:shortDescription xml:lang="en">kg</common:shortDescription>
</epd:referenceToUnitGroupDataSet>
<epd:amount epd:module="A1-A3">1.23E-08</epd:amount>
<epd:amount epd:module="A4">1.88E-08</epd:amount>
<epd:amount epd:module="A5">1.19E-11</epd:amount>
<epd:amount epd:module="B1">0</epd:amount>
<epd:amount epd:module="C4">3.82E-09</epd:amount>
<epd:amount epd:module="D">-1.42E-10</epd:amount>
</common:other>
</exchange>
<exchange dataSetInternalID="12">
<referenceToFlowDataSet uri="../flows/b29ef66b-e286-4afa-949f-62f1a7b4d7fa.xml" type="flow data set" refObjectId="b29ef66b-e286-4afa-949f-62f1a7b4d7fa">
<common:shortDescription xml:lang="en">Non hazardous waste disposed (NHWD)</common:shortDescription>
</referenceToFlowDataSet>
<functionType>General reminder flow</functionType>
<exchangeDirection>Output</exchangeDirection>
<common:other>
<epd:referenceToUnitGroupDataSet uri="../unitgroups/ad38d542-3fe9-439d-9b95-2f5f7752acaf.xml" type="unit group data set" refObjectId="ad38d542-3fe9-439d-9b95-2f5f7752acaf">
<common:shortDescription xml:lang="en">kg</common:shortDescription>
</epd:referenceToUnitGroupDataSet>
<epd:amount epd:module="A1-A3">0.00522</epd:amount>
<epd:amount epd:module="A4">2.18E-05</epd:amount>
<epd:amount epd:module="A5">0.00018</epd:amount>
<epd:amount epd:module="B1">0</epd:amount>
<epd:amount epd:module="C4">1.04</epd:amount>
<epd:amount epd:module="D">-0.000139</epd:amount>
</common:other>
</exchange>
<exchange dataSetInternalID="13">
<referenceToFlowDataSet uri="../flows/3449546e-52ad-4b39-b809-9fb77cea8ff6.xml" type="flow data set" refObjectId="3449546e-52ad-4b39-b809-9fb77cea8ff6">
<common:shortDescription xml:lang="en">Radioactive waste disposed (RWD)</common:shortDescription>
</referenceToFlowDataSet>
<functionType>General reminder flow</functionType>
<exchangeDirection>Output</exchangeDirection>
<common:other>
<epd:referenceToUnitGroupDataSet uri="../unitgroups/ad38d542-3fe9-439d-9b95-2f5f7752acaf.xml" type="unit group data set" refObjectId="ad38d542-3fe9-439d-9b95-2f5f7752acaf">
<common:shortDescription xml:lang="en">kg</common:shortDescription>
</epd:referenceToUnitGroupDataSet>
<epd:amount epd:module="A1-A3">4.91E-05</epd:amount>
<epd:amount epd:module="A4">3.54E-07</epd:amount>
<epd:amount epd:module="A5">4.99E-07</epd:amount>
<epd:amount epd:module="B1">0</epd:amount>
<epd:amount epd:module="C4">3.18E-06</epd:amount>
<epd:amount epd:module="D">-1.1E-05</epd:amount>
</common:other>
</exchange>
<exchange dataSetInternalID="14">
<referenceToFlowDataSet uri="../flows/a2b32f97-3fc7-4af2-b209-525bc6426f33.xml" type="flow data set" refObjectId="a2b32f97-3fc7-4af2-b209-525bc6426f33">
<common:shortDescription xml:lang="en">Components for re-use (CRU)</common:shortDescription>
</referenceToFlowDataSet>
<functionType>General reminder flow</functionType>
<exchangeDirection>Output</exchangeDirection>
<common:other>
<epd:referenceToUnitGroupDataSet uri="../unitgroups/ad38d542-3fe9-439d-9b95-2f5f7752acaf.xml" type="unit group data set" refObjectId="ad38d542-3fe9-439d-9b95-2f5f7752acaf">
<common:shortDescription xml:lang="en">kg</common:shortDescription>
</epd:referenceToUnitGroupDataSet>
<epd:amount epd:module="A1-A3">0</epd:amount>
<epd:amount epd:module="A4">0</epd:amount>
<epd:amount epd:module="A5">0</epd:amount>
<epd:amount epd:module="B1">0</epd:amount>
<epd:amount epd:module="C4">0</epd:amount>
<epd:amount epd:module="D">0</epd:amount>
</common:other>
</exchange>
<exchange dataSetInternalID="15">
<referenceToFlowDataSet uri="../flows/d7fe48a5-4103-49c8-9aae-b0b5dfdbd6ae.xml" type="flow data set" refObjectId="d7fe48a5-4103-49c8-9aae-b0b5dfdbd6ae">
<common:shortDescription xml:lang="en">Materials for recycling (MFR)</common:shortDescription>
</referenceToFlowDataSet>
<functionType>General reminder flow</functionType>
<exchangeDirection>Output</exchangeDirection>
<common:other>
<epd:referenceToUnitGroupDataSet uri="../unitgroups/ad38d542-3fe9-439d-9b95-2f5f7752acaf.xml" type="unit group data set" refObjectId="ad38d542-3fe9-439d-9b95-2f5f7752acaf">
<common:shortDescription xml:lang="en">kg</common:shortDescription>
</epd:referenceToUnitGroupDataSet>
<epd:amount epd:module="A1-A3">0</epd:amount>
<epd:amount epd:module="A4">0</epd:amount>
<epd:amount epd:module="A5">0.000187</epd:amount>
<epd:amount epd:module="B1">0</epd:amount>
<epd:amount epd:module="C4">0</epd:amount>
<epd:amount epd:module="D">0</epd:amount>
</common:other>
</exchange>
<exchange dataSetInternalID="16">
<referenceToFlowDataSet uri="../flows/59a9181c-3aaf-46ee-8b13-2b3723b6e447.xml" type="flow data set" refObjectId="59a9181c-3aaf-46ee-8b13-2b3723b6e447">
<common:shortDescription xml:lang="en">Materials for energy recovery (MER)</common:shortDescription>
</referenceToFlowDataSet>
<functionType>General reminder flow</functionType>
<exchangeDirection>Output</exchangeDirection>
<common:other>
<epd:referenceToUnitGroupDataSet uri="../unitgroups/ad38d542-3fe9-439d-9b95-2f5f7752acaf.xml" type="unit group data set" refObjectId="ad38d542-3fe9-439d-9b95-2f5f7752acaf">
<common:shortDescription xml:lang="en">kg</common:shortDescription>
</epd:referenceToUnitGroupDataSet>
<epd:amount epd:module="A1-A3">0</epd:amount>
<epd:amount epd:module="A4">0</epd:amount>
<epd:amount epd:module="A5">0.0226</epd:amount>
<epd:amount epd:module="B1">0</epd:amount>
<epd:amount epd:module="C4">0</epd:amount>
<epd:amount epd:module="D">0</epd:amount>
</common:other>
</exchange>
<exchange dataSetInternalID="17">
<referenceToFlowDataSet uri="../flows/4da0c987-2b76-40d6-9e9e-82a017aaaf29.xml" type="flow data set" refObjectId="4da0c987-2b76-40d6-9e9e-82a017aaaf29">
<common:shortDescription xml:lang="en">Exported electrical energy (EEE)</common:shortDescription>
</referenceToFlowDataSet>
<functionType>General reminder flow</functionType>
<exchangeDirection>Output</exchangeDirection>
<common:other>
<epd:referenceToUnitGroupDataSet uri="../unitgroups/93a60a57-a3c8-11da-a746-0800200c9a66.xml" type="unit group data set" refObjectId="93a60a57-a3c8-11da-a746-0800200c9a66">
<common:shortDescription xml:lang="en">MJ</common:shortDescription>
</epd:referenceToUnitGroupDataSet>
<epd:amount epd:module="A1-A3">0</epd:amount>
<epd:amount epd:module="A4">0</epd:amount>
<epd:amount epd:module="A5">0.0522</epd:amount>
<epd:amount epd:module="B1">0</epd:amount>
<epd:amount epd:module="C4">0</epd:amount>
<epd:amount epd:module="D">0</epd:amount>
</common:other>
</exchange>
<exchange dataSetInternalID="18">
<referenceToFlowDataSet uri="../flows/98daf38a-7a79-46d3-9a37-2b7bd0955810.xml" type="flow data set" refObjectId="98daf38a-7a79-46d3-9a37-2b7bd0955810">
<common:shortDescription xml:lang="en">Exported thermal energy (EET)</common:shortDescription>
</referenceToFlowDataSet>
<functionType>General reminder flow</functionType>
<exchangeDirection>Output</exchangeDirection>
<common:other>
<epd:referenceToUnitGroupDataSet uri="../unitgroups/93a60a57-a3c8-11da-a746-0800200c9a66.xml" type="unit group data set" refObjectId="93a60a57-a3c8-11da-a746-0800200c9a66">
<common:shortDescription xml:lang="en">MJ</common:shortDescription>
</epd:referenceToUnitGroupDataSet>
<epd:amount epd:module="A1-A3">0</epd:amount>
<epd:amount epd:module="A4">0</epd:amount>
<epd:amount epd:module="A5">0.122</epd:amount>
<epd:amount epd:module="B1">0</epd:amount>
<epd:amount epd:module="C4">0</epd:amount>
<epd:amount epd:module="D">0</epd:amount>
</common:other>
</exchange>
</exchanges>
<LCIAResults>
<LCIAResult>
<referenceToLCIAMethodDataSet uri="../lciamethods/77e416eb-a363-4258-a04e-171d843a6460.xml" type="LCIA method data set" refObjectId="77e416eb-a363-4258-a04e-171d843a6460">
<common:shortDescription xml:lang="en">Global warming potential (GWP)</common:shortDescription>
</referenceToLCIAMethodDataSet>
<common:other>
<epd:referenceToUnitGroupDataSet uri="../unitgroups/1ebf3012-d0db-4de2-aefd-ef30cedb0be1.xml" type="unit group data set" refObjectId="1ebf3012-d0db-4de2-aefd-ef30cedb0be1">
<common:shortDescription xml:lang="en">kg CO_(2)-Äq.</common:shortDescription>
</epd:referenceToUnitGroupDataSet>
<epd:amount epd:module="A1-A3">0.208</epd:amount>
<epd:amount epd:module="A4">0.0218</epd:amount>
<epd:amount epd:module="A5">0.0417</epd:amount>
<epd:amount epd:module="B1">-0.108</epd:amount>
<epd:amount epd:module="C4">0.0166</epd:amount>
<epd:amount epd:module="D">-0.0175</epd:amount>
</common:other>
</LCIAResult>
<LCIAResult>
<referenceToLCIAMethodDataSet uri="../lciamethods/06dcd26f-025f-401a-a7c1-5e457eb54637.xml" type="LCIA method data set" refObjectId="06dcd26f-025f-401a-a7c1-5e457eb54637">
<common:shortDescription xml:lang="en">Depletion potential of the stratospheric ozone layer (ODP)</common:shortDescription>
</referenceToLCIAMethodDataSet>
<common:other>
<epd:referenceToUnitGroupDataSet uri="../unitgroups/88054749-b0a6-47ea-a82b-dc5b29326512.xml" type="unit group data set" refObjectId="88054749-b0a6-47ea-a82b-dc5b29326512">
<common:shortDescription xml:lang="en">kg CFC11-Äq.</common:shortDescription>
</epd:referenceToUnitGroupDataSet>
<epd:amount epd:module="A1-A3">4.97E-10</epd:amount>
<epd:amount epd:module="A4">4.58E-16</epd:amount>
<epd:amount epd:module="A5">5.71E-16</epd:amount>
<epd:amount epd:module="B1">0</epd:amount>
<epd:amount epd:module="C4">3.69E-15</epd:amount>
<epd:amount epd:module="D">-1.27E-14</epd:amount>
</common:other>
</LCIAResult>
<LCIAResult>
<referenceToLCIAMethodDataSet uri="../lciamethods/b4274add-93b7-4905-a5e4-2e878c4e4216.xml" type="LCIA method data set" refObjectId="b4274add-93b7-4905-a5e4-2e878c4e4216">
<common:shortDescription xml:lang="en">Acidification potential of land and water (AP)</common:shortDescription>
</referenceToLCIAMethodDataSet>
<common:other>
<epd:referenceToUnitGroupDataSet uri="../unitgroups/bc50c624-a9bc-45b1-a9b0-e6b10d00476f.xml" type="unit group data set" refObjectId="bc50c624-a9bc-45b1-a9b0-e6b10d00476f">
<common:shortDescription xml:lang="en">kg SO_(2)-Äq.</common:shortDescription>
</epd:referenceToUnitGroupDataSet>
<epd:amount epd:module="A1-A3">0.000278</epd:amount>
<epd:amount epd:module="A4">1.66E-05</epd:amount>
<epd:amount epd:module="A5">5.46E-06</epd:amount>
<epd:amount epd:module="B1">0</epd:amount>
<epd:amount epd:module="C4">9.8E-05</epd:amount>
<epd:amount epd:module="D">-1.91E-05</epd:amount>
</common:other>
</LCIAResult>
<LCIAResult>
<referenceToLCIAMethodDataSet uri="../lciamethods/f58827d0-b407-4ec6-be75-8b69efb98a0f.xml" type="LCIA method data set" refObjectId="f58827d0-b407-4ec6-be75-8b69efb98a0f">
<common:shortDescription xml:lang="en">Eutrophication potential (EP)</common:shortDescription>
</referenceToLCIAMethodDataSet>
<common:other>
<epd:referenceToUnitGroupDataSet uri="../unitgroups/67b5401d-873c-485f-bcf3-6ae83b918822.xml" type="unit group data set" refObjectId="67b5401d-873c-485f-bcf3-6ae83b918822">
<common:shortDescription xml:lang="en">kg PO_(4)^(3)-Äq.</common:shortDescription>
</epd:referenceToUnitGroupDataSet>
<epd:amount epd:module="A1-A3">6.25E-05</epd:amount>
<epd:amount epd:module="A4">3.74E-06</epd:amount>
<epd:amount epd:module="A5">1.21E-06</epd:amount>
<epd:amount epd:module="B1">0</epd:amount>
<epd:amount epd:module="C4">1.35E-05</epd:amount>
<epd:amount epd:module="D">-3.12E-06</epd:amount>
</common:other>
</LCIAResult>
<LCIAResult>
<referenceToLCIAMethodDataSet uri="../lciamethods/1e84a202-dae6-42aa-9e9d-71ea48b8be00.xml" type="LCIA method data set" refObjectId="1e84a202-dae6-42aa-9e9d-71ea48b8be00">
<common:shortDescription xml:lang="en">Formation potential of tropospheric ozone photochemical oxidants (POCP)</common:shortDescription>
</referenceToLCIAMethodDataSet>
<common:other>
<epd:referenceToUnitGroupDataSet uri="../unitgroups/01c26c17-9a76-406e-8295-f17b55fd909e.xml" type="unit group data set" refObjectId="01c26c17-9a76-406e-8295-f17b55fd909e">
<common:shortDescription xml:lang="en">kg Ethen-Äq.</common:shortDescription>
</epd:referenceToUnitGroupDataSet>
<epd:amount epd:module="A1-A3">2.79E-05</epd:amount>
<epd:amount epd:module="A4">-2.35E-07</epd:amount>
<epd:amount epd:module="A5">3.65E-07</epd:amount>
<epd:amount epd:module="B1">0</epd:amount>
<epd:amount epd:module="C4">7.62E-06</epd:amount>
<epd:amount epd:module="D">-1.68E-06</epd:amount>
</common:other>
</LCIAResult>
<LCIAResult>
<referenceToLCIAMethodDataSet uri="../lciamethods/f7c73bb9-ab1a-4249-9c6d-379a0de6f67e.xml" type="LCIA method data set" refObjectId="f7c73bb9-ab1a-4249-9c6d-379a0de6f67e">
<common:shortDescription xml:lang="en">Abiotic depletion potential for non fossil resources (ADPE)</common:shortDescription>
</referenceToLCIAMethodDataSet>
<common:other>
<epd:referenceToUnitGroupDataSet uri="../unitgroups/54ccd2d9-a32a-4fc2-923d-f2c8c93e89d4.xml" type="unit group data set" refObjectId="54ccd2d9-a32a-4fc2-923d-f2c8c93e89d4">
<common:shortDescription xml:lang="en">kg Sb-Äq.</common:shortDescription>
</epd:referenceToUnitGroupDataSet>
<epd:amount epd:module="A1-A3">9.43E-07</epd:amount>
<epd:amount epd:module="A4">2.26E-09</epd:amount>
<epd:amount epd:module="A5">7.3E-10</epd:amount>
<epd:amount epd:module="B1">0</epd:amount>
<epd:amount epd:module="C4">6.37E-09</epd:amount>
<epd:amount epd:module="D">-4.04E-08</epd:amount>
</common:other>
</LCIAResult>
<LCIAResult>
<referenceToLCIAMethodDataSet uri="../lciamethods/804ebcdf-309d-4098-8ed8-fdaf2f389981.xml" type="LCIA method data set" refObjectId="804ebcdf-309d-4098-8ed8-fdaf2f389981">
<common:shortDescription xml:lang="en">Abiotic depletion potential for fossil resources (ADPF)</common:shortDescription>
</referenceToLCIAMethodDataSet>
<common:other>
<epd:referenceToUnitGroupDataSet uri="../unitgroups/93a60a57-a3c8-11da-a746-0800200c9a66.xml" type="unit group data set" refObjectId="93a60a57-a3c8-11da-a746-0800200c9a66">
<common:shortDescription xml:lang="en">MJ</common:shortDescription>
</epd:referenceToUnitGroupDataSet>
<epd:amount epd:module="A1-A3">1.4</epd:amount>
<epd:amount epd:module="A4">0.292</epd:amount>
<epd:amount epd:module="A5">0.0111</epd:amount>
<epd:amount epd:module="B1">0</epd:amount>
<epd:amount epd:module="C4">0.214</epd:amount>
<epd:amount epd:module="D">-0.225</epd:amount>
</common:other>
</LCIAResult>
</LCIAResults>
</processDataSet>