<?xml version="1.0" encoding="utf-8"?>
<processDataSet xmlns:epd="http://www.iai.kit.edu/EPD/2013" xmlns:epd2="http://www.indata.network/EPD/2019" xmlns:common="http://lca.jrc.it/ILCD/Common" xsi:schemaLocation="http://lca.jrc.it/ILCD/Process ../../schemas/EPD_DataSet.xsd" epd2:epd-version="1.2" version="1.1" locations="../ILCDLocations.xml" xmlns:xsi="http://www.w3.org/2001/XMLSchema-instance" xmlns="http://lca.jrc.it/ILCD/Process">
<processInformation>
<dataSetInformation>
<common:UUID>16fcd034-c658-4353-985b-bac75ca86099</common:UUID>
<name>
<baseName xml:lang="en">Bioguard Acoustic (17mm)</baseName>
<functionalUnitFlowProperties xml:lang="en" />
</name>
<classificationInformation>
<common:classification name="OEKOBAU.DAT">
<common:class level="0" classId="1">Mineralische Baustoffe</common:class>
<common:class level="1" classId="1.3">Steine und Elemente</common:class>
<common:class level="2" classId="1.3.15">Deckenplatten</common:class>
</common:classification>
<common:classification name="IBUCategories">
<common:class level="0">02 Building products</common:class>
<common:class level="1">Internal and external wall and ceiling finishes</common:class>
<common:class level="2">Mineral panels</common:class>
</common:classification>
</classificationInformation>
<common:generalComment xml:lang="en">Mineral ceiling tiles and planks are factory produced using the wet felt process. They meet the requirements of /DIN 18177/ and are placed on the market in accordance with /EN 13964/ as well as German legislation on hazardous substances. Mineral tiles and planks consist of mineral wool(s), fillers and binders. The Bioguard Acoustic (17mm) combines a cleanable surface and resistance to disinfectants as well as an antimicrobial performance and is available in a range of different edge details; Board, Tegular, and MicroLook.</common:generalComment>
</dataSetInformation>
<quantitativeReference>
<referenceToReferenceFlow>0</referenceToReferenceFlow>
</quantitativeReference>
<time>
<common:referenceYear>2020</common:referenceYear>
<common:dataSetValidUntil>2025</common:dataSetValidUntil>
<common:other>
<epd2:publicationDateOfEPD>2020-01-08</epd2:publicationDateOfEPD>
</common:other>
</time>
<geography>
<locationOfOperationSupplyOrProduction location="DE" />
</geography>
<technology>
<technologyDescriptionAndIncludedProcesses xml:lang="en">The described mineral products are produced using the wet-felt process. The initial materials are mixed with water to a homogenous suspension that is then pumped onto a belt conveyor (Fourdrinier). The water is removed both mechanically (gravity and vacuum) and by evaporation in a drying oven. The process water is reused as much as possible. It is treated and re-fed into the process water circuit. Production waste and dust are reused in the production process. Armstrong World Industries is ISO 9001 certified. Raw material Proportion (M - %) Binding agent (mainly starch) 0-10 % Mineral fibre 20 - 70 % Cellulose fibre 0 - 10 % Fillers (clay, talcum, limestone) 20 - 50 % Perlite 10 - 50 % Other &lt; 1 % Dispersion paint and mineral coatings are additionally used for the surface finish as well as water during the production process. Flame retardants are not used. Isothiazolinone based products are used as biocides. 
Declared unit: 
The declared unit for this EPD is 1m2 of Sierra OP (15mm) ceiling panel for use over 50 years</technologyDescriptionAndIncludedProcesses>
<technologicalApplicability xml:lang="en">Wet felt mineral suspended ceiling products are used as aesthetic internal ceiling linings and offer concealment of building services as well as providing sound absorption, sound insulation, fire resistance and very low Volatile Organic Compound (VOC) emissions. Typical applications are in offices, schools, healthcare premises, retail, leisure and transport sectors.</technologicalApplicability>
</technology>
</processInformation>
<modellingAndValidation>
<LCIMethodAndAllocation>
<typeOfDataSet>EPD</typeOfDataSet>
<referenceToLCAMethodDetails type="source data set" refObjectId="0024925d-0678-425b-a0c8-6d1fa13fb20a">
<common:shortDescription xml:lang="en">Mineral panels.pdf</common:shortDescription>
</referenceToLCAMethodDetails>
<common:other>
<epd:subType xmlns="http://www.iai.kit.edu/EPD/2013">specific dataset</epd:subType>
</common:other>
</LCIMethodAndAllocation>
<dataSourcesTreatmentAndRepresentativeness>
<referenceToDataSource type="source data set" refObjectId="b497a91f-e14b-4b69-8f28-f50eb1576766">
<common:shortDescription xml:lang="en">ecoinvent database (all versions)</common:shortDescription>
</referenceToDataSource>
<referenceToDataSource type="source data set" refObjectId="c667cc42-12a7-4d92-9d7b-5e4e90a7a274">
<common:shortDescription xml:lang="en">ecoinvent 3.3 database</common:shortDescription>
</referenceToDataSource>
<useAdviceForDataSet xml:lang="en">Scope: 
This declaration and its LCA study are based on 2016 production data for ceiling products manufactured at the Armstrong Munster plant  in Germany. 
System boundary: 
The system boundaries studied as part of this cradle to grave LCA include the following information modules as per /EN15804/. The Cradle to Grave Assessment Includes: A1: Raw materials production including substrate, coating, and packaging materials for ceiling panelsA2: Transportation of raw materials to Armstrong manufacturing facility A3: Manufacturing of the ceiling panels at an Armstrong facilityA3: Packaging of finished product including energy to operate packaging equipmentA4: Transportation from manufacturing facility to distribution centres, retailers, job site (assumed to be 1200 km)A5: Installation into the building including 7% construction waste.B1-7: Use and maintenance (0 emissions as the ceiling tiles do not require maintenance during life)C1: Deconstruction  (0 emissions as is done by manual labour)C2: Transportation to landfill (assumed to be 100 km)C3: Waste processing (0 emissions)C4: End of life includes disposal of ceiling panel (54.5% landfill, 44.5% incineration and 1% recycled)D: Benefits and loads beyond the system boundaryThe Assessment Excludes: Steel suspension systems that are used for most installationsOverhead energy usage (heating, the lighting of manufacturing facility)</useAdviceForDataSet>
<common:other>
<epd2:referenceToOriginalEPD type="source data set" refObjectId="472e0f60-4be7-40bb-99a6-39bb676bfaea">
<common:shortDescription xml:lang="en">Bioguard Acoustic (17mm).pdf</common:shortDescription>
</epd2:referenceToOriginalEPD>
</common:other>
</dataSourcesTreatmentAndRepresentativeness>
<validation>
<review type="Accredited third party review">
<common:referenceToNameOfReviewerAndInstitution uri="../contacts/d111dbec-b024-4be5-86c5-752d6eb2cf95.xml" type="contact data set" refObjectId="d111dbec-b024-4be5-86c5-752d6eb2cf95">
<common:shortDescription xml:lang="en">Institut Bauen und Umwelt e. V.</common:shortDescription>
</common:referenceToNameOfReviewerAndInstitution>
</review>
</validation>
<complianceDeclarations>
<compliance>
<common:referenceToComplianceSystem uri="../sources/b00f9ec0-7874-11e3-981f-0800200c9a66.xml" type="source data set" refObjectId="b00f9ec0-7874-11e3-981f-0800200c9a66">
<common:shortDescription xml:lang="en">DIN EN 15804</common:shortDescription>
</common:referenceToComplianceSystem>
</compliance>
<compliance>
<common:referenceToComplianceSystem uri="../sources/4f2eb655-6e44-4874-a95a-e28f5442cd4d.xml" type="source data set" refObjectId="4f2eb655-6e44-4874-a95a-e28f5442cd4d">
<common:shortDescription xml:lang="en">ISO 14025</common:shortDescription>
</common:referenceToComplianceSystem>
</compliance>
</complianceDeclarations>
</modellingAndValidation>
<administrativeInformation>
<common:commissionerAndGoal>
<common:referenceToCommissioner uri="../contacts/5c027db1-b832-4395-9cfd-075fb56a4d23.xml" type="contact data set" refObjectId="5c027db1-b832-4395-9cfd-075fb56a4d23">
<common:shortDescription xml:lang="en">Armstrong World Industries Limited</common:shortDescription>
</common:referenceToCommissioner>
</common:commissionerAndGoal>
<dataGenerator>
<common:referenceToPersonOrEntityGeneratingTheDataSet uri="../contacts/585e969a-614a-4757-bbc5-6e9261aa888b.xml" type="contact data set" refObjectId="585e969a-614a-4757-bbc5-6e9261aa888b">
<common:shortDescription xml:lang="en">SGS Search</common:shortDescription>
</common:referenceToPersonOrEntityGeneratingTheDataSet>
</dataGenerator>
<dataEntryBy>
<common:timeStamp>2020-01-08T00:00:00</common:timeStamp>
<common:referenceToDataSetFormat uri="../sources/a97a0155-0234-4b87-b4ce-a45da52f2a40.xml" type="source data set" refObjectId="a97a0155-0234-4b87-b4ce-a45da52f2a40">
<common:shortDescription xml:lang="en">ILCD Format</common:shortDescription>
</common:referenceToDataSetFormat>
<common:referenceToDataSetFormat uri="../sources/a29449fd-aa2f-4de8-b5d7-4b06b43c6fde.xml" type="source data set" refObjectId="a29449fd-aa2f-4de8-b5d7-4b06b43c6fde">
<common:shortDescription xml:lang="de">EPD-Datenformaterweiterungen v1.2</common:shortDescription>
<common:shortDescription xml:lang="en">EPD Data Format Extensions v1.2</common:shortDescription>
</common:referenceToDataSetFormat>
</dataEntryBy>
<publicationAndOwnership>
<common:dataSetVersion>00.01.000</common:dataSetVersion>
<common:referenceToRegistrationAuthority uri="../contacts/d111dbec-b024-4be5-86c5-752d6eb2cf95.xml" type="contact data set" refObjectId="d111dbec-b024-4be5-86c5-752d6eb2cf95">
<common:shortDescription xml:lang="en">Institut Bauen und Umwelt e. V.</common:shortDescription>
</common:referenceToRegistrationAuthority>
<common:registrationNumber>EPD-AWI-20200044-ICA1-EN</common:registrationNumber>
<common:referenceToOwnershipOfDataSet uri="../contacts/5c027db1-b832-4395-9cfd-075fb56a4d23.xml" type="contact data set" refObjectId="5c027db1-b832-4395-9cfd-075fb56a4d23">
<common:shortDescription xml:lang="en">Armstrong World Industries Limited</common:shortDescription>
</common:referenceToOwnershipOfDataSet>
<common:copyright>true</common:copyright>
<common:licenseType>Free of charge for all users and uses</common:licenseType>
<common:accessRestrictions xml:lang="en">None</common:accessRestrictions>
<common:other>
<epd2:referenceToPublisher type="contact data set" refObjectId="d111dbec-b024-4be5-86c5-752d6eb2cf95" uri="../contacts/d111dbec-b024-4be5-86c5-752d6eb2cf95.xml">
<common:shortDescription xml:lang="en">Institut Bauen und Umwelt e. V.</common:shortDescription>
</epd2:referenceToPublisher>
</common:other>
</publicationAndOwnership>
</administrativeInformation>
<exchanges>
<exchange dataSetInternalID="0">
<referenceToFlowDataSet uri="../flows/89ab9da4-cc8c-8650-add6-256cb397ac12.xml" type="flow data set" refObjectId="89ab9da4-cc8c-8650-add6-256cb397ac12">
<common:shortDescription xml:lang="en">Bioguard Acoustic (17mm) ()</common:shortDescription>
</referenceToFlowDataSet>
<meanAmount>1</meanAmount>
<referencesToDataSource />
</exchange>
<exchange dataSetInternalID="1">
<referenceToFlowDataSet uri="../flows/20f32be5-0398-4288-9b6d-accddd195317.xml" type="flow data set" refObjectId="20f32be5-0398-4288-9b6d-accddd195317">
<common:shortDescription xml:lang="en">Renewable primary energy as energy carrier (PERE)</common:shortDescription>
</referenceToFlowDataSet>
<functionType>General reminder flow</functionType>
<exchangeDirection>Input</exchangeDirection>
<common:other>
<epd:referenceToUnitGroupDataSet uri="../unitgroups/93a60a57-a3c8-11da-a746-0800200c9a66.xml" type="unit group data set" refObjectId="93a60a57-a3c8-11da-a746-0800200c9a66">
<common:shortDescription xml:lang="en">MJ</common:shortDescription>
</epd:referenceToUnitGroupDataSet>
<epd:amount epd:module="A1-A3">12.160149</epd:amount>
<epd:amount epd:module="A4">0.14972693</epd:amount>
<epd:amount epd:module="A5">0.8544075</epd:amount>
<epd:amount epd:module="B1">0</epd:amount>
<epd:amount epd:module="B2">0</epd:amount>
<epd:amount epd:module="B3">0</epd:amount>
<epd:amount epd:module="B4">0</epd:amount>
<epd:amount epd:module="B5">0</epd:amount>
<epd:amount epd:module="B6">0</epd:amount>
<epd:amount epd:module="B7">0</epd:amount>
<epd:amount epd:module="C1">0</epd:amount>
<epd:amount epd:module="C2">0.013849741</epd:amount>
<epd:amount epd:module="C3">0</epd:amount>
<epd:amount epd:module="C4">0.027608384</epd:amount>
<epd:amount epd:module="D">-5.3320479</epd:amount>
</common:other>
</exchange>
<exchange dataSetInternalID="2">
<referenceToFlowDataSet uri="../flows/fb3ec0de-548d-4508-aea5-00b73bf6f702.xml" type="flow data set" refObjectId="fb3ec0de-548d-4508-aea5-00b73bf6f702">
<common:shortDescription xml:lang="en">Renewable primary energy resources as material utilization (PERM)</common:shortDescription>
</referenceToFlowDataSet>
<functionType>General reminder flow</functionType>
<exchangeDirection>Input</exchangeDirection>
<common:other>
<epd:referenceToUnitGroupDataSet uri="../unitgroups/93a60a57-a3c8-11da-a746-0800200c9a66.xml" type="unit group data set" refObjectId="93a60a57-a3c8-11da-a746-0800200c9a66">
<common:shortDescription xml:lang="en">MJ</common:shortDescription>
</epd:referenceToUnitGroupDataSet>
<epd:amount epd:module="A1-A3">6.1323</epd:amount>
<epd:amount epd:module="A4">0</epd:amount>
<epd:amount epd:module="A5">0.4293</epd:amount>
<epd:amount epd:module="B1">0</epd:amount>
<epd:amount epd:module="B2">0</epd:amount>
<epd:amount epd:module="B3">0</epd:amount>
<epd:amount epd:module="B4">0</epd:amount>
<epd:amount epd:module="B5">0</epd:amount>
<epd:amount epd:module="B6">0</epd:amount>
<epd:amount epd:module="B7">0</epd:amount>
<epd:amount epd:module="C1">0</epd:amount>
<epd:amount epd:module="C2">0</epd:amount>
<epd:amount epd:module="C3">0</epd:amount>
<epd:amount epd:module="C4">0</epd:amount>
<epd:amount epd:module="D">0</epd:amount>
</common:other>
</exchange>
<exchange dataSetInternalID="3">
<referenceToFlowDataSet uri="../flows/53f97275-fa8a-4cdd-9024-65936002acd0.xml" type="flow data set" refObjectId="53f97275-fa8a-4cdd-9024-65936002acd0">
<common:shortDescription xml:lang="en">Total use of renewable primary energy resources (PERT)</common:shortDescription>
</referenceToFlowDataSet>
<functionType>General reminder flow</functionType>
<exchangeDirection>Input</exchangeDirection>
<common:other>
<epd:referenceToUnitGroupDataSet uri="../unitgroups/93a60a57-a3c8-11da-a746-0800200c9a66.xml" type="unit group data set" refObjectId="93a60a57-a3c8-11da-a746-0800200c9a66">
<common:shortDescription xml:lang="en">MJ</common:shortDescription>
</epd:referenceToUnitGroupDataSet>
<epd:amount epd:module="A1-A3">18.292449</epd:amount>
<epd:amount epd:module="A4">0.14972693</epd:amount>
<epd:amount epd:module="A5">1.2837075</epd:amount>
<epd:amount epd:module="B1">0</epd:amount>
<epd:amount epd:module="B2">0</epd:amount>
<epd:amount epd:module="B3">0</epd:amount>
<epd:amount epd:module="B4">0</epd:amount>
<epd:amount epd:module="B5">0</epd:amount>
<epd:amount epd:module="B6">0</epd:amount>
<epd:amount epd:module="B7">0</epd:amount>
<epd:amount epd:module="C1">0</epd:amount>
<epd:amount epd:module="C2">0.013849741</epd:amount>
<epd:amount epd:module="C3">0</epd:amount>
<epd:amount epd:module="C4">0.027608384</epd:amount>
<epd:amount epd:module="D">-5.3320479</epd:amount>
</common:other>
</exchange>
<exchange dataSetInternalID="4">
<referenceToFlowDataSet uri="../flows/ac857178-2b45-46ec-892a-a9a4332f0372.xml" type="flow data set" refObjectId="ac857178-2b45-46ec-892a-a9a4332f0372">
<common:shortDescription xml:lang="en">Non renewable primary energy as energy carrier (PENRE)</common:shortDescription>
</referenceToFlowDataSet>
<functionType>General reminder flow</functionType>
<exchangeDirection>Input</exchangeDirection>
<common:other>
<epd:referenceToUnitGroupDataSet uri="../unitgroups/93a60a57-a3c8-11da-a746-0800200c9a66.xml" type="unit group data set" refObjectId="93a60a57-a3c8-11da-a746-0800200c9a66">
<common:shortDescription xml:lang="en">MJ</common:shortDescription>
</epd:referenceToUnitGroupDataSet>
<epd:amount epd:module="A1-A3">82.866192</epd:amount>
<epd:amount epd:module="A4">11.60549</epd:amount>
<epd:amount epd:module="A5">5.9619811</epd:amount>
<epd:amount epd:module="B1">0</epd:amount>
<epd:amount epd:module="B2">0</epd:amount>
<epd:amount epd:module="B3">0</epd:amount>
<epd:amount epd:module="B4">0</epd:amount>
<epd:amount epd:module="B5">0</epd:amount>
<epd:amount epd:module="B6">0</epd:amount>
<epd:amount epd:module="B7">0</epd:amount>
<epd:amount epd:module="C1">0</epd:amount>
<epd:amount epd:module="C2">1.0735078</epd:amount>
<epd:amount epd:module="C3">0</epd:amount>
<epd:amount epd:module="C4">1.0809026</epd:amount>
<epd:amount epd:module="D">2.0975347</epd:amount>
</common:other>
</exchange>
<exchange dataSetInternalID="5">
<referenceToFlowDataSet uri="../flows/1421caa0-679d-4bf4-b282-0eb850ccae27.xml" type="flow data set" refObjectId="1421caa0-679d-4bf4-b282-0eb850ccae27">
<common:shortDescription xml:lang="en">Non renewable primary energy as material utilization (PENRM)</common:shortDescription>
</referenceToFlowDataSet>
<functionType>General reminder flow</functionType>
<exchangeDirection>Input</exchangeDirection>
<common:other>
<epd:referenceToUnitGroupDataSet uri="../unitgroups/93a60a57-a3c8-11da-a746-0800200c9a66.xml" type="unit group data set" refObjectId="93a60a57-a3c8-11da-a746-0800200c9a66">
<common:shortDescription xml:lang="en">MJ</common:shortDescription>
</epd:referenceToUnitGroupDataSet>
<epd:amount epd:module="A1-A3">0.0791</epd:amount>
<epd:amount epd:module="A4">0</epd:amount>
<epd:amount epd:module="A5">0.0055</epd:amount>
<epd:amount epd:module="B1">0</epd:amount>
<epd:amount epd:module="B2">0</epd:amount>
<epd:amount epd:module="B3">0</epd:amount>
<epd:amount epd:module="B4">0</epd:amount>
<epd:amount epd:module="B5">0</epd:amount>
<epd:amount epd:module="B6">0</epd:amount>
<epd:amount epd:module="B7">0</epd:amount>
<epd:amount epd:module="C1">0</epd:amount>
<epd:amount epd:module="C2">0</epd:amount>
<epd:amount epd:module="C3">0</epd:amount>
<epd:amount epd:module="C4">0</epd:amount>
<epd:amount epd:module="D">0</epd:amount>
</common:other>
</exchange>
<exchange dataSetInternalID="6">
<referenceToFlowDataSet uri="../flows/06159210-646b-4c8d-8583-da9b3b95a6c1.xml" type="flow data set" refObjectId="06159210-646b-4c8d-8583-da9b3b95a6c1">
<common:shortDescription xml:lang="en">Total use of non renewable primary energy resources (PENRT)</common:shortDescription>
</referenceToFlowDataSet>
<functionType>General reminder flow</functionType>
<exchangeDirection>Input</exchangeDirection>
<common:other>
<epd:referenceToUnitGroupDataSet uri="../unitgroups/93a60a57-a3c8-11da-a746-0800200c9a66.xml" type="unit group data set" refObjectId="93a60a57-a3c8-11da-a746-0800200c9a66">
<common:shortDescription xml:lang="en">MJ</common:shortDescription>
</epd:referenceToUnitGroupDataSet>
<epd:amount epd:module="A1-A3">82.945292</epd:amount>
<epd:amount epd:module="A4">11.60549</epd:amount>
<epd:amount epd:module="A5">5.9674811</epd:amount>
<epd:amount epd:module="B1">0</epd:amount>
<epd:amount epd:module="B2">0</epd:amount>
<epd:amount epd:module="B3">0</epd:amount>
<epd:amount epd:module="B4">0</epd:amount>
<epd:amount epd:module="B5">0</epd:amount>
<epd:amount epd:module="B6">0</epd:amount>
<epd:amount epd:module="B7">0</epd:amount>
<epd:amount epd:module="C1">0</epd:amount>
<epd:amount epd:module="C2">1.0735078</epd:amount>
<epd:amount epd:module="C3">0</epd:amount>
<epd:amount epd:module="C4">1.0809026</epd:amount>
<epd:amount epd:module="D">2.0975347</epd:amount>
</common:other>
</exchange>
<exchange dataSetInternalID="7">
<referenceToFlowDataSet uri="../flows/c6a1f35f-2d09-4f54-8dfb-97e502e1ce92.xml" type="flow data set" refObjectId="c6a1f35f-2d09-4f54-8dfb-97e502e1ce92">
<common:shortDescription xml:lang="en">Use of secondary material (SM)</common:shortDescription>
</referenceToFlowDataSet>
<functionType>General reminder flow</functionType>
<exchangeDirection>Input</exchangeDirection>
<common:other>
<epd:referenceToUnitGroupDataSet uri="../unitgroups/ad38d542-3fe9-439d-9b95-2f5f7752acaf.xml" type="unit group data set" refObjectId="ad38d542-3fe9-439d-9b95-2f5f7752acaf">
<common:shortDescription xml:lang="en">kg</common:shortDescription>
</epd:referenceToUnitGroupDataSet>
<epd:amount epd:module="A1-A3">0.5789</epd:amount>
<epd:amount epd:module="A4">0</epd:amount>
<epd:amount epd:module="A5">0.0405</epd:amount>
<epd:amount epd:module="B1">0</epd:amount>
<epd:amount epd:module="B2">0</epd:amount>
<epd:amount epd:module="B3">0</epd:amount>
<epd:amount epd:module="B4">0</epd:amount>
<epd:amount epd:module="B5">0</epd:amount>
<epd:amount epd:module="B6">0</epd:amount>
<epd:amount epd:module="B7">0</epd:amount>
<epd:amount epd:module="C1">0</epd:amount>
<epd:amount epd:module="C2">0</epd:amount>
<epd:amount epd:module="C3">0</epd:amount>
<epd:amount epd:module="C4">0</epd:amount>
<epd:amount epd:module="D">0</epd:amount>
</common:other>
</exchange>
<exchange dataSetInternalID="8">
<referenceToFlowDataSet uri="../flows/64333088-a55f-4aa2-9a31-c10b07816787.xml" type="flow data set" refObjectId="64333088-a55f-4aa2-9a31-c10b07816787">
<common:shortDescription xml:lang="en">Use of renewable secondary fuels (RSF)</common:shortDescription>
</referenceToFlowDataSet>
<functionType>General reminder flow</functionType>
<exchangeDirection>Input</exchangeDirection>
<common:other>
<epd:referenceToUnitGroupDataSet uri="../unitgroups/93a60a57-a3c8-11da-a746-0800200c9a66.xml" type="unit group data set" refObjectId="93a60a57-a3c8-11da-a746-0800200c9a66">
<common:shortDescription xml:lang="en">MJ</common:shortDescription>
</epd:referenceToUnitGroupDataSet>
<epd:amount epd:module="A1-A3"></epd:amount>
<epd:amount epd:module="A4"></epd:amount>
<epd:amount epd:module="A5"></epd:amount>
<epd:amount epd:module="B1"></epd:amount>
<epd:amount epd:module="B2"></epd:amount>
<epd:amount epd:module="B3"></epd:amount>
<epd:amount epd:module="B4"></epd:amount>
<epd:amount epd:module="B5"></epd:amount>
<epd:amount epd:module="B6"></epd:amount>
<epd:amount epd:module="B7"></epd:amount>
<epd:amount epd:module="C1"></epd:amount>
<epd:amount epd:module="C2"></epd:amount>
<epd:amount epd:module="C3"></epd:amount>
<epd:amount epd:module="C4"></epd:amount>
<epd:amount epd:module="D"></epd:amount>
</common:other>
</exchange>
<exchange dataSetInternalID="9">
<referenceToFlowDataSet uri="../flows/89def144-d39a-4287-b86f-efde453ddcb2.xml" type="flow data set" refObjectId="89def144-d39a-4287-b86f-efde453ddcb2">
<common:shortDescription xml:lang="en">Use of non renewable secondary fuels (NRSF)</common:shortDescription>
</referenceToFlowDataSet>
<functionType>General reminder flow</functionType>
<exchangeDirection>Input</exchangeDirection>
<common:other>
<epd:referenceToUnitGroupDataSet uri="../unitgroups/93a60a57-a3c8-11da-a746-0800200c9a66.xml" type="unit group data set" refObjectId="93a60a57-a3c8-11da-a746-0800200c9a66">
<common:shortDescription xml:lang="en">MJ</common:shortDescription>
</epd:referenceToUnitGroupDataSet>
<epd:amount epd:module="A1-A3"></epd:amount>
<epd:amount epd:module="A4"></epd:amount>
<epd:amount epd:module="A5"></epd:amount>
<epd:amount epd:module="B1"></epd:amount>
<epd:amount epd:module="B2"></epd:amount>
<epd:amount epd:module="B3"></epd:amount>
<epd:amount epd:module="B4"></epd:amount>
<epd:amount epd:module="B5"></epd:amount>
<epd:amount epd:module="B6"></epd:amount>
<epd:amount epd:module="B7"></epd:amount>
<epd:amount epd:module="C1"></epd:amount>
<epd:amount epd:module="C2"></epd:amount>
<epd:amount epd:module="C3"></epd:amount>
<epd:amount epd:module="C4"></epd:amount>
<epd:amount epd:module="D"></epd:amount>
</common:other>
</exchange>
<exchange dataSetInternalID="10">
<referenceToFlowDataSet uri="../flows/3cf952c8-f3a4-461d-8c96-96456ca62246.xml" type="flow data set" refObjectId="3cf952c8-f3a4-461d-8c96-96456ca62246">
<common:shortDescription xml:lang="en">Use of net fresh water (FW)</common:shortDescription>
</referenceToFlowDataSet>
<functionType>General reminder flow</functionType>
<exchangeDirection>Input</exchangeDirection>
<common:other>
<epd:referenceToUnitGroupDataSet uri="../unitgroups/cd950537-0a98-4044-9ba7-9f9a68d0a504.xml" type="unit group data set" refObjectId="cd950537-0a98-4044-9ba7-9f9a68d0a504">
<common:shortDescription xml:lang="en">m^3</common:shortDescription>
</epd:referenceToUnitGroupDataSet>
<epd:amount epd:module="A1-A3">0.034128099</epd:amount>
<epd:amount epd:module="A4">0.0021169411</epd:amount>
<epd:amount epd:module="A5">0.0024673855</epd:amount>
<epd:amount epd:module="B1">0</epd:amount>
<epd:amount epd:module="B2">0</epd:amount>
<epd:amount epd:module="B3">0</epd:amount>
<epd:amount epd:module="B4">0</epd:amount>
<epd:amount epd:module="B5">0</epd:amount>
<epd:amount epd:module="B6">0</epd:amount>
<epd:amount epd:module="B7">0</epd:amount>
<epd:amount epd:module="C1">0</epd:amount>
<epd:amount epd:module="C2">0.00019581705</epd:amount>
<epd:amount epd:module="C3">0</epd:amount>
<epd:amount epd:module="C4">0.00043084522</epd:amount>
<epd:amount epd:module="D">0.0012786685</epd:amount>
</common:other>
</exchange>
<exchange dataSetInternalID="11">
<referenceToFlowDataSet uri="../flows/430f9e0f-59b2-46a0-8e0d-55e0e84948fc.xml" type="flow data set" refObjectId="430f9e0f-59b2-46a0-8e0d-55e0e84948fc">
<common:shortDescription xml:lang="en">Hazardous waste disposed (HWD)</common:shortDescription>
</referenceToFlowDataSet>
<functionType>General reminder flow</functionType>
<exchangeDirection>Output</exchangeDirection>
<common:other>
<epd:referenceToUnitGroupDataSet uri="../unitgroups/ad38d542-3fe9-439d-9b95-2f5f7752acaf.xml" type="unit group data set" refObjectId="ad38d542-3fe9-439d-9b95-2f5f7752acaf">
<common:shortDescription xml:lang="en">kg</common:shortDescription>
</epd:referenceToUnitGroupDataSet>
<epd:amount epd:module="A1-A3">0.00010595823</epd:amount>
<epd:amount epd:module="A4">6.5151006E-06</epd:amount>
<epd:amount epd:module="A5">7.5866409E-06</epd:amount>
<epd:amount epd:module="B1">0</epd:amount>
<epd:amount epd:module="B2">0</epd:amount>
<epd:amount epd:module="B3">0</epd:amount>
<epd:amount epd:module="B4">0</epd:amount>
<epd:amount epd:module="B5">0</epd:amount>
<epd:amount epd:module="B6">0</epd:amount>
<epd:amount epd:module="B7">0</epd:amount>
<epd:amount epd:module="C1">0</epd:amount>
<epd:amount epd:module="C2">6.026468E-07</epd:amount>
<epd:amount epd:module="C3">0</epd:amount>
<epd:amount epd:module="C4">9.8885029E-07</epd:amount>
<epd:amount epd:module="D">-6.3976694E-06</epd:amount>
</common:other>
</exchange>
<exchange dataSetInternalID="12">
<referenceToFlowDataSet uri="../flows/b29ef66b-e286-4afa-949f-62f1a7b4d7fa.xml" type="flow data set" refObjectId="b29ef66b-e286-4afa-949f-62f1a7b4d7fa">
<common:shortDescription xml:lang="en">Non hazardous waste disposed (NHWD)</common:shortDescription>
</referenceToFlowDataSet>
<functionType>General reminder flow</functionType>
<exchangeDirection>Output</exchangeDirection>
<common:other>
<epd:referenceToUnitGroupDataSet uri="../unitgroups/ad38d542-3fe9-439d-9b95-2f5f7752acaf.xml" type="unit group data set" refObjectId="ad38d542-3fe9-439d-9b95-2f5f7752acaf">
<common:shortDescription xml:lang="en">kg</common:shortDescription>
</epd:referenceToUnitGroupDataSet>
<epd:amount epd:module="A1-A3">0.91753614</epd:amount>
<epd:amount epd:module="A4">0.66280621</epd:amount>
<epd:amount epd:module="A5">0.23537703</epd:amount>
<epd:amount epd:module="B1">0</epd:amount>
<epd:amount epd:module="B2">0</epd:amount>
<epd:amount epd:module="B3">0</epd:amount>
<epd:amount epd:module="B4">0</epd:amount>
<epd:amount epd:module="B5">0</epd:amount>
<epd:amount epd:module="B6">0</epd:amount>
<epd:amount epd:module="B7">0</epd:amount>
<epd:amount epd:module="C1">0</epd:amount>
<epd:amount epd:module="C2">0.061309575</epd:amount>
<epd:amount epd:module="C3">0</epd:amount>
<epd:amount epd:module="C4">2.373032</epd:amount>
<epd:amount epd:module="D">-0.0025498585</epd:amount>
</common:other>
</exchange>
<exchange dataSetInternalID="13">
<referenceToFlowDataSet uri="../flows/3449546e-52ad-4b39-b809-9fb77cea8ff6.xml" type="flow data set" refObjectId="3449546e-52ad-4b39-b809-9fb77cea8ff6">
<common:shortDescription xml:lang="en">Radioactive waste disposed (RWD)</common:shortDescription>
</referenceToFlowDataSet>
<functionType>General reminder flow</functionType>
<exchangeDirection>Output</exchangeDirection>
<common:other>
<epd:referenceToUnitGroupDataSet uri="../unitgroups/ad38d542-3fe9-439d-9b95-2f5f7752acaf.xml" type="unit group data set" refObjectId="ad38d542-3fe9-439d-9b95-2f5f7752acaf">
<common:shortDescription xml:lang="en">kg</common:shortDescription>
</epd:referenceToUnitGroupDataSet>
<epd:amount epd:module="A1-A3">0.00020992785</epd:amount>
<epd:amount epd:module="A4">7.4836563E-05</epd:amount>
<epd:amount epd:module="A5">1.5638547E-05</epd:amount>
<epd:amount epd:module="B1">0</epd:amount>
<epd:amount epd:module="B2">0</epd:amount>
<epd:amount epd:module="B3">0</epd:amount>
<epd:amount epd:module="B4">0</epd:amount>
<epd:amount epd:module="B5">0</epd:amount>
<epd:amount epd:module="B6">0</epd:amount>
<epd:amount epd:module="B7">0</epd:amount>
<epd:amount epd:module="C1">0</epd:amount>
<epd:amount epd:module="C2">6.9223821E-06</epd:amount>
<epd:amount epd:module="C3">0</epd:amount>
<epd:amount epd:module="C4">6.1232128E-06</epd:amount>
<epd:amount epd:module="D">1.0766969E-05</epd:amount>
</common:other>
</exchange>
<exchange dataSetInternalID="14">
<referenceToFlowDataSet uri="../flows/a2b32f97-3fc7-4af2-b209-525bc6426f33.xml" type="flow data set" refObjectId="a2b32f97-3fc7-4af2-b209-525bc6426f33">
<common:shortDescription xml:lang="en">Components for re-use (CRU)</common:shortDescription>
</referenceToFlowDataSet>
<functionType>General reminder flow</functionType>
<exchangeDirection>Output</exchangeDirection>
<common:other>
<epd:referenceToUnitGroupDataSet uri="../unitgroups/ad38d542-3fe9-439d-9b95-2f5f7752acaf.xml" type="unit group data set" refObjectId="ad38d542-3fe9-439d-9b95-2f5f7752acaf">
<common:shortDescription xml:lang="en">kg</common:shortDescription>
</epd:referenceToUnitGroupDataSet>
<epd:amount epd:module="A1-A3">0</epd:amount>
<epd:amount epd:module="A4">0</epd:amount>
<epd:amount epd:module="A5">0.0659</epd:amount>
<epd:amount epd:module="B1">0</epd:amount>
<epd:amount epd:module="B2">0</epd:amount>
<epd:amount epd:module="B3">0</epd:amount>
<epd:amount epd:module="B4">0</epd:amount>
<epd:amount epd:module="B5">0</epd:amount>
<epd:amount epd:module="B6">0</epd:amount>
<epd:amount epd:module="B7">0</epd:amount>
<epd:amount epd:module="C1">0</epd:amount>
<epd:amount epd:module="C2">0</epd:amount>
<epd:amount epd:module="C3">0</epd:amount>
<epd:amount epd:module="C4">0</epd:amount>
<epd:amount epd:module="D">0</epd:amount>
</common:other>
</exchange>
<exchange dataSetInternalID="15">
<referenceToFlowDataSet uri="../flows/d7fe48a5-4103-49c8-9aae-b0b5dfdbd6ae.xml" type="flow data set" refObjectId="d7fe48a5-4103-49c8-9aae-b0b5dfdbd6ae">
<common:shortDescription xml:lang="en">Materials for recycling (MFR)</common:shortDescription>
</referenceToFlowDataSet>
<functionType>General reminder flow</functionType>
<exchangeDirection>Output</exchangeDirection>
<common:other>
<epd:referenceToUnitGroupDataSet uri="../unitgroups/ad38d542-3fe9-439d-9b95-2f5f7752acaf.xml" type="unit group data set" refObjectId="ad38d542-3fe9-439d-9b95-2f5f7752acaf">
<common:shortDescription xml:lang="en">kg</common:shortDescription>
</epd:referenceToUnitGroupDataSet>
<epd:amount epd:module="A1-A3">0</epd:amount>
<epd:amount epd:module="A4">0</epd:amount>
<epd:amount epd:module="A5">0.0043</epd:amount>
<epd:amount epd:module="B1">0</epd:amount>
<epd:amount epd:module="B2">0</epd:amount>
<epd:amount epd:module="B3">0</epd:amount>
<epd:amount epd:module="B4">0</epd:amount>
<epd:amount epd:module="B5">0</epd:amount>
<epd:amount epd:module="B6">0</epd:amount>
<epd:amount epd:module="B7">0</epd:amount>
<epd:amount epd:module="C1">0</epd:amount>
<epd:amount epd:module="C2">0</epd:amount>
<epd:amount epd:module="C3">0</epd:amount>
<epd:amount epd:module="C4">0</epd:amount>
<epd:amount epd:module="D">0.0614</epd:amount>
</common:other>
</exchange>
<exchange dataSetInternalID="16">
<referenceToFlowDataSet uri="../flows/59a9181c-3aaf-46ee-8b13-2b3723b6e447.xml" type="flow data set" refObjectId="59a9181c-3aaf-46ee-8b13-2b3723b6e447">
<common:shortDescription xml:lang="en">Materials for energy recovery (MER)</common:shortDescription>
</referenceToFlowDataSet>
<functionType>General reminder flow</functionType>
<exchangeDirection>Output</exchangeDirection>
<common:other>
<epd:referenceToUnitGroupDataSet uri="../unitgroups/ad38d542-3fe9-439d-9b95-2f5f7752acaf.xml" type="unit group data set" refObjectId="ad38d542-3fe9-439d-9b95-2f5f7752acaf">
<common:shortDescription xml:lang="en">kg</common:shortDescription>
</epd:referenceToUnitGroupDataSet>
<epd:amount epd:module="A1-A3">0</epd:amount>
<epd:amount epd:module="A4">0</epd:amount>
<epd:amount epd:module="A5">0.0711</epd:amount>
<epd:amount epd:module="B1">0</epd:amount>
<epd:amount epd:module="B2">0</epd:amount>
<epd:amount epd:module="B3">0</epd:amount>
<epd:amount epd:module="B4">0</epd:amount>
<epd:amount epd:module="B5">0</epd:amount>
<epd:amount epd:module="B6">0</epd:amount>
<epd:amount epd:module="B7">0</epd:amount>
<epd:amount epd:module="C1">0</epd:amount>
<epd:amount epd:module="C2">0</epd:amount>
<epd:amount epd:module="C3">0</epd:amount>
<epd:amount epd:module="C4">0</epd:amount>
<epd:amount epd:module="D">0</epd:amount>
</common:other>
</exchange>
<exchange dataSetInternalID="17">
<referenceToFlowDataSet uri="../flows/4da0c987-2b76-40d6-9e9e-82a017aaaf29.xml" type="flow data set" refObjectId="4da0c987-2b76-40d6-9e9e-82a017aaaf29">
<common:shortDescription xml:lang="en">Exported electrical energy (EEE)</common:shortDescription>
</referenceToFlowDataSet>
<functionType>General reminder flow</functionType>
<exchangeDirection>Output</exchangeDirection>
<common:other>
<epd:referenceToUnitGroupDataSet uri="../unitgroups/93a60a57-a3c8-11da-a746-0800200c9a66.xml" type="unit group data set" refObjectId="93a60a57-a3c8-11da-a746-0800200c9a66">
<common:shortDescription xml:lang="en">MJ</common:shortDescription>
</epd:referenceToUnitGroupDataSet>
<epd:amount epd:module="A1-A3">0</epd:amount>
<epd:amount epd:module="A4">0</epd:amount>
<epd:amount epd:module="A5">0.2401</epd:amount>
<epd:amount epd:module="B1">0</epd:amount>
<epd:amount epd:module="B2">0</epd:amount>
<epd:amount epd:module="B3">0</epd:amount>
<epd:amount epd:module="B4">0</epd:amount>
<epd:amount epd:module="B5">0</epd:amount>
<epd:amount epd:module="B6">0</epd:amount>
<epd:amount epd:module="B7">0</epd:amount>
<epd:amount epd:module="C1">0</epd:amount>
<epd:amount epd:module="C2">0</epd:amount>
<epd:amount epd:module="C3">0</epd:amount>
<epd:amount epd:module="C4">15.3389</epd:amount>
<epd:amount epd:module="D">0</epd:amount>
</common:other>
</exchange>
<exchange dataSetInternalID="18">
<referenceToFlowDataSet uri="../flows/98daf38a-7a79-46d3-9a37-2b7bd0955810.xml" type="flow data set" refObjectId="98daf38a-7a79-46d3-9a37-2b7bd0955810">
<common:shortDescription xml:lang="en">Exported thermal energy (EET)</common:shortDescription>
</referenceToFlowDataSet>
<functionType>General reminder flow</functionType>
<exchangeDirection>Output</exchangeDirection>
<common:other>
<epd:referenceToUnitGroupDataSet uri="../unitgroups/93a60a57-a3c8-11da-a746-0800200c9a66.xml" type="unit group data set" refObjectId="93a60a57-a3c8-11da-a746-0800200c9a66">
<common:shortDescription xml:lang="en">MJ</common:shortDescription>
</epd:referenceToUnitGroupDataSet>
<epd:amount epd:module="A1-A3">0</epd:amount>
<epd:amount epd:module="A4">0</epd:amount>
<epd:amount epd:module="A5">0.3708</epd:amount>
<epd:amount epd:module="B1">0</epd:amount>
<epd:amount epd:module="B2">0</epd:amount>
<epd:amount epd:module="B3">0</epd:amount>
<epd:amount epd:module="B4">0</epd:amount>
<epd:amount epd:module="B5">0</epd:amount>
<epd:amount epd:module="B6">0</epd:amount>
<epd:amount epd:module="B7">0</epd:amount>
<epd:amount epd:module="C1">0</epd:amount>
<epd:amount epd:module="C2">0</epd:amount>
<epd:amount epd:module="C3">0</epd:amount>
<epd:amount epd:module="C4">26.417</epd:amount>
<epd:amount epd:module="D">0</epd:amount>
</common:other>
</exchange>
</exchanges>
<LCIAResults>
<LCIAResult>
<referenceToLCIAMethodDataSet uri="../lciamethods/77e416eb-a363-4258-a04e-171d843a6460.xml" type="LCIA method data set" refObjectId="77e416eb-a363-4258-a04e-171d843a6460">
<common:shortDescription xml:lang="en">Global warming potential (GWP)</common:shortDescription>
</referenceToLCIAMethodDataSet>
<common:other>
<epd:referenceToUnitGroupDataSet uri="../unitgroups/1ebf3012-d0db-4de2-aefd-ef30cedb0be1.xml" type="unit group data set" refObjectId="1ebf3012-d0db-4de2-aefd-ef30cedb0be1">
<common:shortDescription xml:lang="en">kg CO_(2)-Äq.</common:shortDescription>
</epd:referenceToUnitGroupDataSet>
<epd:amount epd:module="A1-A3">5.1571741</epd:amount>
<epd:amount epd:module="A4">0.70626841</epd:amount>
<epd:amount epd:module="A5">0.41645967</epd:amount>
<epd:amount epd:module="B1">0</epd:amount>
<epd:amount epd:module="B2">0</epd:amount>
<epd:amount epd:module="B3">0</epd:amount>
<epd:amount epd:module="B4">0</epd:amount>
<epd:amount epd:module="B5">0</epd:amount>
<epd:amount epd:module="B6">0</epd:amount>
<epd:amount epd:module="B7">0</epd:amount>
<epd:amount epd:module="C1">0</epd:amount>
<epd:amount epd:module="C2">0.065329828</epd:amount>
<epd:amount epd:module="C3">0</epd:amount>
<epd:amount epd:module="C4">0.11422076</epd:amount>
<epd:amount epd:module="D">0.24617551</epd:amount>
</common:other>
</LCIAResult>
<LCIAResult>
<referenceToLCIAMethodDataSet uri="../lciamethods/06dcd26f-025f-401a-a7c1-5e457eb54637.xml" type="LCIA method data set" refObjectId="06dcd26f-025f-401a-a7c1-5e457eb54637">
<common:shortDescription xml:lang="en">Depletion potential of the stratospheric ozone layer (ODP)</common:shortDescription>
</referenceToLCIAMethodDataSet>
<common:other>
<epd:referenceToUnitGroupDataSet uri="../unitgroups/88054749-b0a6-47ea-a82b-dc5b29326512.xml" type="unit group data set" refObjectId="88054749-b0a6-47ea-a82b-dc5b29326512">
<common:shortDescription xml:lang="en">kg CFC11-Äq.</common:shortDescription>
</epd:referenceToUnitGroupDataSet>
<epd:amount epd:module="A1-A3">6.006916E-07</epd:amount>
<epd:amount epd:module="A4">1.3154198E-07</epd:amount>
<epd:amount epd:module="A5">4.3778158E-08</epd:amount>
<epd:amount epd:module="B1">0</epd:amount>
<epd:amount epd:module="B2">0</epd:amount>
<epd:amount epd:module="B3">0</epd:amount>
<epd:amount epd:module="B4">0</epd:amount>
<epd:amount epd:module="B5">0</epd:amount>
<epd:amount epd:module="B6">0</epd:amount>
<epd:amount epd:module="B7">0</epd:amount>
<epd:amount epd:module="C1">0</epd:amount>
<epd:amount epd:module="C2">1.2167633E-08</epd:amount>
<epd:amount epd:module="C3">0</epd:amount>
<epd:amount epd:module="C4">1.1017836E-08</epd:amount>
<epd:amount epd:module="D">-9.0158988E-09</epd:amount>
</common:other>
</LCIAResult>
<LCIAResult>
<referenceToLCIAMethodDataSet uri="../lciamethods/b4274add-93b7-4905-a5e4-2e878c4e4216.xml" type="LCIA method data set" refObjectId="b4274add-93b7-4905-a5e4-2e878c4e4216">
<common:shortDescription xml:lang="en">Acidification potential of land and water (AP)</common:shortDescription>
</referenceToLCIAMethodDataSet>
<common:other>
<epd:referenceToUnitGroupDataSet uri="../unitgroups/bc50c624-a9bc-45b1-a9b0-e6b10d00476f.xml" type="unit group data set" refObjectId="bc50c624-a9bc-45b1-a9b0-e6b10d00476f">
<common:shortDescription xml:lang="en">kg SO_(2)-Äq.</common:shortDescription>
</epd:referenceToUnitGroupDataSet>
<epd:amount epd:module="A1-A3">0.014340172</epd:amount>
<epd:amount epd:module="A4">0.0031088205</epd:amount>
<epd:amount epd:module="A5">0.0010641935</epd:amount>
<epd:amount epd:module="B1">0</epd:amount>
<epd:amount epd:module="B2">0</epd:amount>
<epd:amount epd:module="B3">0</epd:amount>
<epd:amount epd:module="B4">0</epd:amount>
<epd:amount epd:module="B5">0</epd:amount>
<epd:amount epd:module="B6">0</epd:amount>
<epd:amount epd:module="B7">0</epd:amount>
<epd:amount epd:module="C1">0</epd:amount>
<epd:amount epd:module="C2">0.00028756589</epd:amount>
<epd:amount epd:module="C3">0</epd:amount>
<epd:amount epd:module="C4">0.00031750926</epd:amount>
<epd:amount epd:module="D">0.0022541418</epd:amount>
</common:other>
</LCIAResult>
<LCIAResult>
<referenceToLCIAMethodDataSet uri="../lciamethods/f58827d0-b407-4ec6-be75-8b69efb98a0f.xml" type="LCIA method data set" refObjectId="f58827d0-b407-4ec6-be75-8b69efb98a0f">
<common:shortDescription xml:lang="en">Eutrophication potential (EP)</common:shortDescription>
</referenceToLCIAMethodDataSet>
<common:other>
<epd:referenceToUnitGroupDataSet uri="../unitgroups/67b5401d-873c-485f-bcf3-6ae83b918822.xml" type="unit group data set" refObjectId="67b5401d-873c-485f-bcf3-6ae83b918822">
<common:shortDescription xml:lang="en">kg PO_(4)^(3)-Äq.</common:shortDescription>
</epd:referenceToUnitGroupDataSet>
<epd:amount epd:module="A1-A3">0.0040524363</epd:amount>
<epd:amount epd:module="A4">0.00056248391</epd:amount>
<epd:amount epd:module="A5">0.00029659678</epd:amount>
<epd:amount epd:module="B1">0</epd:amount>
<epd:amount epd:module="B2">0</epd:amount>
<epd:amount epd:module="B3">0</epd:amount>
<epd:amount epd:module="B4">0</epd:amount>
<epd:amount epd:module="B5">0</epd:amount>
<epd:amount epd:module="B6">0</epd:amount>
<epd:amount epd:module="B7">0</epd:amount>
<epd:amount epd:module="C1">0</epd:amount>
<epd:amount epd:module="C2">5.2029762E-05</epd:amount>
<epd:amount epd:module="C3">0</epd:amount>
<epd:amount epd:module="C4">6.3051691E-05</epd:amount>
<epd:amount epd:module="D">1.0941243E-05</epd:amount>
</common:other>
</LCIAResult>
<LCIAResult>
<referenceToLCIAMethodDataSet uri="../lciamethods/1e84a202-dae6-42aa-9e9d-71ea48b8be00.xml" type="LCIA method data set" refObjectId="1e84a202-dae6-42aa-9e9d-71ea48b8be00">
<common:shortDescription xml:lang="en">Formation potential of tropospheric ozone photochemical oxidants (POCP)</common:shortDescription>
</referenceToLCIAMethodDataSet>
<common:other>
<epd:referenceToUnitGroupDataSet uri="../unitgroups/01c26c17-9a76-406e-8295-f17b55fd909e.xml" type="unit group data set" refObjectId="01c26c17-9a76-406e-8295-f17b55fd909e">
<common:shortDescription xml:lang="en">kg Ethen-Äq.</common:shortDescription>
</epd:referenceToUnitGroupDataSet>
<epd:amount epd:module="A1-A3">0.00079487444</epd:amount>
<epd:amount epd:module="A4">0.00012581929</epd:amount>
<epd:amount epd:module="A5">5.8771042E-05</epd:amount>
<epd:amount epd:module="B1">0</epd:amount>
<epd:amount epd:module="B2">0</epd:amount>
<epd:amount epd:module="B3">0</epd:amount>
<epd:amount epd:module="B4">0</epd:amount>
<epd:amount epd:module="B5">0</epd:amount>
<epd:amount epd:module="B6">0</epd:amount>
<epd:amount epd:module="B7">0</epd:amount>
<epd:amount epd:module="C1">0</epd:amount>
<epd:amount epd:module="C2">1.1638284E-05</epd:amount>
<epd:amount epd:module="C3">0</epd:amount>
<epd:amount epd:module="C4">2.3747884E-05</epd:amount>
<epd:amount epd:module="D">0.00011405336</epd:amount>
</common:other>
</LCIAResult>
<LCIAResult>
<referenceToLCIAMethodDataSet uri="../lciamethods/f7c73bb9-ab1a-4249-9c6d-379a0de6f67e.xml" type="LCIA method data set" refObjectId="f7c73bb9-ab1a-4249-9c6d-379a0de6f67e">
<common:shortDescription xml:lang="en">Abiotic depletion potential for non fossil resources (ADPE)</common:shortDescription>
</referenceToLCIAMethodDataSet>
<common:other>
<epd:referenceToUnitGroupDataSet uri="../unitgroups/54ccd2d9-a32a-4fc2-923d-f2c8c93e89d4.xml" type="unit group data set" refObjectId="54ccd2d9-a32a-4fc2-923d-f2c8c93e89d4">
<common:shortDescription xml:lang="en">kg Sb-Äq.</common:shortDescription>
</epd:referenceToUnitGroupDataSet>
<epd:amount epd:module="A1-A3">5.511919E-06</epd:amount>
<epd:amount epd:module="A4">1.9943468E-06</epd:amount>
<epd:amount epd:module="A5">4.0658059E-07</epd:amount>
<epd:amount epd:module="B1">0</epd:amount>
<epd:amount epd:module="B2">0</epd:amount>
<epd:amount epd:module="B3">0</epd:amount>
<epd:amount epd:module="B4">0</epd:amount>
<epd:amount epd:module="B5">0</epd:amount>
<epd:amount epd:module="B6">0</epd:amount>
<epd:amount epd:module="B7">0</epd:amount>
<epd:amount epd:module="C1">0</epd:amount>
<epd:amount epd:module="C2">1.8447708E-07</epd:amount>
<epd:amount epd:module="C3">0</epd:amount>
<epd:amount epd:module="C4">8.7154094E-08</epd:amount>
<epd:amount epd:module="D">5.2288202E-07</epd:amount>
</common:other>
</LCIAResult>
<LCIAResult>
<referenceToLCIAMethodDataSet uri="../lciamethods/804ebcdf-309d-4098-8ed8-fdaf2f389981.xml" type="LCIA method data set" refObjectId="804ebcdf-309d-4098-8ed8-fdaf2f389981">
<common:shortDescription xml:lang="en">Abiotic depletion potential for fossil resources (ADPF)</common:shortDescription>
</referenceToLCIAMethodDataSet>
<common:other>
<epd:referenceToUnitGroupDataSet uri="../unitgroups/93a60a57-a3c8-11da-a746-0800200c9a66.xml" type="unit group data set" refObjectId="93a60a57-a3c8-11da-a746-0800200c9a66">
<common:shortDescription xml:lang="en">MJ</common:shortDescription>
</epd:referenceToUnitGroupDataSet>
<epd:amount epd:module="A1-A3">68.264985</epd:amount>
<epd:amount epd:module="A4">10.72383</epd:amount>
<epd:amount epd:module="A5">4.9267638</epd:amount>
<epd:amount epd:module="B1">0</epd:amount>
<epd:amount epd:module="B2">0</epd:amount>
<epd:amount epd:module="B3">0</epd:amount>
<epd:amount epd:module="B4">0</epd:amount>
<epd:amount epd:module="B5">0</epd:amount>
<epd:amount epd:module="B6">0</epd:amount>
<epd:amount epd:module="B7">0</epd:amount>
<epd:amount epd:module="C1">0</epd:amount>
<epd:amount epd:module="C2">0.9919543</epd:amount>
<epd:amount epd:module="C3">0</epd:amount>
<epd:amount epd:module="C4">0.99334857</epd:amount>
<epd:amount epd:module="D">1.2643821</epd:amount>
</common:other>
</LCIAResult>
</LCIAResults>
</processDataSet>