<?xml-stylesheet type='text/xsl' href='../../stylesheets/epd2html.xsl'?>
<processDataSet xmlns:xsi="http://www.w3.org/2001/XMLSchema-instance" xmlns="http://lca.jrc.it/ILCD/Process" xsi:schemaLocation="http://lca.jrc.it/ILCD/Process ../../schemas/EPD_DataSet.xsd" locations="../ILCDLocations.xml" version="1.1">
  <processInformation>
    <dataSetInformation>
      <common:UUID xmlns:common="http://lca.jrc.it/ILCD/Common">1b978129-dd5e-45ea-9c82-1c3510e9c965</common:UUID>
      <name>
        <baseName xmlns:epd="http://www.iai.kit.edu/EPD/2013" xmlns:common="http://lca.jrc.it/ILCD/Common" xml:lang="en">Expanded clay concrete block inner wall</baseName>
        <baseName xmlns:epd="http://www.iai.kit.edu/EPD/2013" xmlns:common="http://lca.jrc.it/ILCD/Common" xml:lang="de">Blähton LB Planstein Innenwand</baseName>
        <functionalUnitFlowProperties xmlns:epd="http://www.iai.kit.edu/EPD/2013" xmlns:common="http://lca.jrc.it/ILCD/Common" xml:lang="en">Plan stone interior wall, density class 0,7, 700 kg/m3</functionalUnitFlowProperties>
      </name>
      <classificationInformation>
        <common:classification xmlns:common="http://lca.jrc.it/ILCD/Common" name="oekobau.dat">
          <common:class level="0" classId="1">Mineralische Baustoffe</common:class>
          <common:class level="1" classId="1.3">Steine und Elemente</common:class>
          <common:class level="2" classId="1.3.04">Leichtbeton</common:class>
        </common:classification>
      </classificationInformation>
      <common:generalComment xmlns:common="http://lca.jrc.it/ILCD/Common" xmlns:epd="http://www.iai.kit.edu/EPD/2013" xml:lang="en">This data set has been modeled according to the European Standard EN 15804 for Sustainable Building. Results are depicted in modules that allow the structured expression of results over the entire life cycle.</common:generalComment>
      <common:generalComment xmlns:common="http://lca.jrc.it/ILCD/Common" xmlns:epd="http://www.iai.kit.edu/EPD/2013" xml:lang="de">Dieser Datensatz wurde nach dem European Standard EN 15804 für Nachhaltiges Bauen modelliert. Ergebnisse werden in Modulen abgebildet, die den strukturierten Ausdruck von Ergebnissen über den gesamten Lebenszyklus zulassen.</common:generalComment>
      <common:other xmlns:common="http://lca.jrc.it/ILCD/Common">
        <epd:safetyMargins xmlns:epd="http://www.iai.kit.edu/EPD/2013">
          <epd:margins>10</epd:margins>
          <epd:description xml:lang="en">Product system almost completely covered. Good technological, temporal and geographic representativeness.</epd:description>
          <epd:description xml:lang="de">Produktsystem weitgehend vollständig abgebildet. Gute technologische, zeitliche und geographische Repräsentativität.</epd:description>
        </epd:safetyMargins>
      </common:other>
    </dataSetInformation>
    <quantitativeReference type="Reference flow(s)">
      <referenceToReferenceFlow>100076</referenceToReferenceFlow>
    </quantitativeReference>
    <time>
      <common:referenceYear xmlns:common="http://lca.jrc.it/ILCD/Common">2018</common:referenceYear>
      <common:dataSetValidUntil xmlns:common="http://lca.jrc.it/ILCD/Common">2022</common:dataSetValidUntil>
      <common:timeRepresentativenessDescription xmlns:common="http://lca.jrc.it/ILCD/Common" xmlns:epd="http://www.iai.kit.edu/EPD/2013" xml:lang="en">Annual average</common:timeRepresentativenessDescription>
      <common:timeRepresentativenessDescription xmlns:common="http://lca.jrc.it/ILCD/Common" xmlns:epd="http://www.iai.kit.edu/EPD/2013" xml:lang="de">Jährlicher Durchschnitt</common:timeRepresentativenessDescription>
    </time>
    <geography>
      <locationOfOperationSupplyOrProduction location="DE">
        <descriptionOfRestrictions xmlns:epd="http://www.iai.kit.edu/EPD/2013" xmlns:common="http://lca.jrc.it/ILCD/Common" xml:lang="en">The data set represents the country specific situation in Germany, focusing on the main technologies, the region specific characteristics and / or import statistics.</descriptionOfRestrictions>
        <descriptionOfRestrictions xmlns:epd="http://www.iai.kit.edu/EPD/2013" xmlns:common="http://lca.jrc.it/ILCD/Common" xml:lang="de">Der Datensatz bildet die länderspezifische Situation in Deutschland ab. Dabei werden Haupttechnologien, spezifische regionale Charakteristiken und ggf. Importstatistiken berücksichtigt.</descriptionOfRestrictions>
      </locationOfOperationSupplyOrProduction>
    </geography>
    <technology>
      <technologyDescriptionAndIncludedProcesses xmlns:common="http://lca.jrc.it/ILCD/Common" xmlns:epd="http://www.iai.kit.edu/EPD/2013" xml:lang="en">The light concrete mix is produced in a mixer from washed pumice and exactly dosed quantities of water and bonding agents. The mixture arrives in the filling chest of the stone moulding machine which feeds the charging car. The charging car then goes over to the metallic mould (which is set on a board) and fills it up. The stone moulds contain enough cores (for the particular type of stone) for grooves or chambers.  With extra loading and vibration the mixture is compacted and the stone is pushed out of the mould. The stones on the underlying boards are taken to a high bay racking where they set for 24 to 36 hours. They are stored for 6 weeks, longer than the required standard of 28 days, in the yard.       
Background system:
Electricity: Electricity is modelled according to the individual country-specific situations. The country-specific modelling is achieved on multiple levels. Firstly, individual energy carrier specific power plants and plants for renewable energy sources are modelled according to the current national electricity grid mix. Modelling the electricity consumption mix includes transmission / distribution losses and the own use by energy producers (own consumption of power plants and "other" own consumption e.g. due to pumped storage hydro power etc.), as well as imported electricity. Secondly, the national emission and efficiency standards of the power plants are modelled as well as the share of electricity plants and combined heat and power plants (CHP). Thirdly, the country-specific energy carrier supply (share of imports and / or domestic supply) including the country-specific energy carrier properties (e.g. element and energy content) are accounted for. Fourthly, the exploration, mining/production, processing and transport processes of the energy carrier supply chains are modelled according to the specific situation of each electricity producing country. The different production and processing techniques (emissions and efficiencies) in the different energy producing countries are considered, e.g. different crude oil production technologies or different flaring rates at the oil platforms.
Thermal energy, process steam: The thermal energy and process steam supply is modelled according to the individual country-specific situation with regard to emission standards and considered energy carriers. The thermal energy and process steam are produced at heat plants. Efficiencies for thermal energy production are by definition 100% in relation to the corresponding energy carrier input. For process steam the efficiency ranges from 85%, 90% to 95%. The energy carriers used for the generation of thermal energy and process steam are modelled according to the specific import situation (see electricity above).
Transports: All relevant and known transport processes are included. Ocean-going and inland ship transport as well as rail, truck and pipeline transport of bulk commodities are considered.
Energy carriers: The energy carriers are modelled according to the specific supply situation (see electricity above).
Refinery products: Diesel fuel, gasoline, technical gases, fuel oils, lubricants and residues such as bitumen are modelled with a parameterised country-specific refinery model. The refinery model represents the current national standard in refining techniques (e.g. emission level, internal energy consumption, etc.) as well as the individual country-specific product output spectrum, which can be quite different from country to country. The supply of crude oil is modelled, again, according to the country-specific situation with the respective properties of the resources.</technologyDescriptionAndIncludedProcesses>
      <technologyDescriptionAndIncludedProcesses xmlns:common="http://lca.jrc.it/ILCD/Common" xmlns:epd="http://www.iai.kit.edu/EPD/2013" xml:lang="de">Der Leichtbeton-Mix wird in einem Mischer aus gewaschenem Bimsstein und genau dosierten Mengen von Wasser und Bindemitteln produziert. Die Mixtur kommt in den Tank der Steingussmaschine, welche die Ofenbatterie auflädt. Die Ofenbatterie geht über in die Metallform (die auf einem Brett befestigt ist), und füllt diese auf. Die Steinformen enthalten genug Cores (für die spezielle Steinform) für Rillen und Kammern. Durch zusätzliche Belastung und Vibration wird die Mixtur verdichtet und der Stein aus der Form gedrückt. Die Steine auf den darunterliegenden Brettern werden in ein Hochregallager gebracht wo sie für 24 bis 36 Stunden verbleiben. Sie werden für 6 Wochen an einem Lagerplatz eingelagert, länger als der erforderliche Standard von 28 Tagen. 



Hintergrundsystem:

Strom: Die Stromerzeugung wird entsprechend der länderspezifischen Randbedingungen modelliert. Die landesspezifische Analyse beinhaltet:
1.: Spezifische Kraftwerke der verschiedenen fossilen Energieträger und der Einsatz erneuerbarer Energien sind entsprechend der länderspezifischen Energieträgermixe modelliert. Die Analyse bezieht Stromimporte aus den Nachbarländern, Transmissions-und Verteilungsverluste und den Eigenverbrauch im Kraftwerk und bei der Verteilung bzw. Speicherung, z. B. durch Pumpspeicherwerke, ein.
2.: Die landes-/regionalspezifischen Technologiestandards sowie die Erzeugung in Elektrizitätskraftwerken und/oder in speziellen Kraftwerken mit Kraft-Wärme-Kopplung (KWK) sind berücksichtigt. 
3.: Die länderspezifische Energieträgerbereitstellung (mit Anteil der Importe und/oder Eigenversorgung) einschließlich der Energieträger-Eigenschaften (z. B. Elementar- und Energiegehalte) werden berücksichtigt. 
4.: Die Förderung, Produktion, Verarbeitung und Transportprozesse werden entsprechend der Situation im jeweiligen Stromerzeugerland modelliert. Die unterschiedlichen Produktions- und Verarbeitungsverfahren (Emissionen und Wirkungsgrade) in den verschiedenen Energieerzeugerländern werden einbezogen, z. B. Rohöl-Veredelungsverfahren oder Abfackel-Raten an den Ölplattformen.
Thermische Energie, Prozessdampf: Die Erzeugung von Dampf und thermischer Energie in Heizkraftwerken wird entsprechend der landesspezifischen Situation (Emissionsgrenzwerte, Energieträgerbasis) modelliert.
Der Wirkungsgrad für die thermische Energieerzeugung beträgt per Definition 100% des Energieträgereinsatzes. Für Prozessdampf liegt der Wirkungsgrad im Bereich von 85-95%. Die zur Heizenergie-Erzeugung verwendeten Energieträger werden entsprechend der nationalen Situation modelliert (siehe Kapitel Strom oben).
Transporte: Alle relevanten und bekannten Transportprozesse in Form von See- und Binnenschiffsverkehr sowie Bahn-, Lkw- und der Leitungstransport sind enthalten.
Energieträger: Die Energieträger werden entsprechend der spezifischen Versorgungslage modelliert (siehe Kapitel Strom oben). 
Raffinerieprodukte: Diesel, Benzin, technische Gase, Heizöl, Schmierstoffe und Rückstände, wie Bitumen, werden mit einem parametrierten länderspezifische Raffineriemodell modelliert. Das Raffinerie-Modell bezieht die länderspezifischen Veredelungsverfahren (z. B. Emissionspegel, interner Energieverbrauch etc.) und das länderspezifische Produktspektrum ein, das sich je nach Land stark unterscheiden kann. Die Rohöl-Förderung wird gemäß der länderspezifischen Situation mit den jeweiligen Energieträger-Eigenschaften modelliert.
"</technologyDescriptionAndIncludedProcesses>
      <technologicalApplicability xmlns:common="http://lca.jrc.it/ILCD/Common" xmlns:epd="http://www.iai.kit.edu/EPD/2013" xml:lang="en">This product can be used in construction.</technologicalApplicability>
      <technologicalApplicability xmlns:common="http://lca.jrc.it/ILCD/Common" xmlns:epd="http://www.iai.kit.edu/EPD/2013" xml:lang="de">Dieses Produkt kann im Baubereich verwendet werden.</technologicalApplicability>
      <referenceToTechnologyFlowDiagrammOrPicture refObjectId="1b77affe-1d7d-409a-ab02-fe6f0031682c" version="39.00.000" type="source data set" uri="../sources/1b77affe-1d7d-409a-ab02-fe6f0031682c.xml">
        <common:shortDescription xmlns:common="http://lca.jrc.it/ILCD/Common" xmlns:epd="http://www.iai.kit.edu/EPD/2013" xml:lang="en">construction_raw density classes.jpg</common:shortDescription>
      </referenceToTechnologyFlowDiagrammOrPicture>
      <referenceToTechnologyFlowDiagrammOrPicture refObjectId="b47cf4aa-e57f-4966-8bc0-0d6f059d0d4f" version="39.00.000" type="source data set" uri="../sources/b47cf4aa-e57f-4966-8bc0-0d6f059d0d4f.xml">
        <common:shortDescription xmlns:common="http://lca.jrc.it/ILCD/Common" xmlns:epd="http://www.iai.kit.edu/EPD/2013" xml:lang="en">construction_20_lightconcrete_ingred.pdf</common:shortDescription>
      </referenceToTechnologyFlowDiagrammOrPicture>
    </technology>
  </processInformation>
  <modellingAndValidation>
    <LCIMethodAndAllocation>
      <typeOfDataSet>EPD</typeOfDataSet>
      <common:other xmlns:common="http://lca.jrc.it/ILCD/Common">
        <epd:subType xmlns:epd="http://www.iai.kit.edu/EPD/2013">generic dataset</epd:subType>
      </common:other>
    </LCIMethodAndAllocation>
    <dataSourcesTreatmentAndRepresentativeness>
      <referenceToDataSource refObjectId="0b1ac3d3-3960-11dd-ae16-0800200c9a66" version="39.00.000" type="source data set" uri="../sources/0b1ac3d3-3960-11dd-ae16-0800200c9a66.xml">
        <common:shortDescription xmlns:common="http://lca.jrc.it/ILCD/Common" xmlns:epd="http://www.iai.kit.edu/EPD/2013" xml:lang="en">LEICHTBETON, 2008</common:shortDescription>
        <common:shortDescription xmlns:common="http://lca.jrc.it/ILCD/Common" xmlns:epd="http://www.iai.kit.edu/EPD/2013" xml:lang="de">GaBi Database Edition 2020, SP40</common:shortDescription>
      </referenceToDataSource>
      <referenceToDataSource refObjectId="0b1aeae0-3960-11dd-ae16-0800200c9a66" version="39.00.000" type="source data set" uri="../sources/0b1aeae0-3960-11dd-ae16-0800200c9a66.xml">
        <common:shortDescription xmlns:common="http://lca.jrc.it/ILCD/Common" xmlns:epd="http://www.iai.kit.edu/EPD/2013" xml:lang="en">Leichtbeton Handbuch, 2006</common:shortDescription>
        <common:shortDescription xmlns:common="http://lca.jrc.it/ILCD/Common" xmlns:epd="http://www.iai.kit.edu/EPD/2013" xml:lang="de">GaBi database (all versions)</common:shortDescription>
      </referenceToDataSource>
      <referenceToDataSource refObjectId="d2732220-5fbd-11db-b0de-0800200c9a66" version="39.00.000" type="source data set" uri="../sources/d2732220-5fbd-11db-b0de-0800200c9a66.xml">
        <common:shortDescription xmlns:common="http://lca.jrc.it/ILCD/Common" xmlns:epd="http://www.iai.kit.edu/EPD/2013" xml:lang="en">Ökologische Bilanzierung von Baustoffen und Gebäuden, 2000</common:shortDescription>
      </referenceToDataSource>
      <referenceToDataSource refObjectId="cb50c596-16b4-44e4-b1aa-319319a79fb5" version="39.00.000" type="source data set" uri="../sources/cb50c596-16b4-44e4-b1aa-319319a79fb5.xml">
        <common:shortDescription xmlns:common="http://lca.jrc.it/ILCD/Common" xmlns:epd="http://www.iai.kit.edu/EPD/2013" xml:lang="en">GaBi Database Edition 2020, SP40</common:shortDescription>
      </referenceToDataSource>
      <referenceToDataSource refObjectId="28d74cc0-db8b-4d7e-bc44-5f6d56ce0c4a" version="39.00.000" type="source data set" uri="../sources/28d74cc0-db8b-4d7e-bc44-5f6d56ce0c4a.xml">
        <common:shortDescription xmlns:common="http://lca.jrc.it/ILCD/Common" xmlns:epd="http://www.iai.kit.edu/EPD/2013" xml:lang="en">GaBi database (all versions)</common:shortDescription>
      </referenceToDataSource>
      <useAdviceForDataSet xmlns:common="http://lca.jrc.it/ILCD/Common" xmlns:epd="http://www.iai.kit.edu/EPD/2013" xml:lang="en">The data set represents a cradle to gate inventory. It can be used to characterise the supply chain situation of the respective commodity in a representative manner. Combination with individual unit processes using this commodity enables the generation of user-specific (product) LCAs.</useAdviceForDataSet>
      <useAdviceForDataSet xmlns:common="http://lca.jrc.it/ILCD/Common" xmlns:epd="http://www.iai.kit.edu/EPD/2013" xml:lang="de">Der Datensatz repräsentiert ein Cradle to Gate Inventar. Er kann verwendet werden, um die Lieferkette des jeweiligen Produktes in einer repräsentativen Weise zu charakterisieren. Die Kombination mit einzelnen Einheitenprozessen und diesem Produkt ermöglicht die Erstellung von anwenderspezifischen (Produkt-) LCAs.</useAdviceForDataSet>
    </dataSourcesTreatmentAndRepresentativeness>
    <validation>
      <review type="Dependent internal review">
        <common:referenceToNameOfReviewerAndInstitution xmlns:common="http://lca.jrc.it/ILCD/Common" refObjectId="d7fa0337-f279-430d-becf-7f3111a85010" version="39.00.000" type="contact data set" uri="../contacts/d7fa0337-f279-430d-becf-7f3111a85010.xml">
          <common:shortDescription xmlns:epd="http://www.iai.kit.edu/EPD/2013" xml:lang="en">thinkstep</common:shortDescription>
          <common:shortDescription xmlns:epd="http://www.iai.kit.edu/EPD/2013" xml:lang="de">thinkstep</common:shortDescription>
        </common:referenceToNameOfReviewerAndInstitution>
        <common:referenceToNameOfReviewerAndInstitution xmlns:common="http://lca.jrc.it/ILCD/Common" refObjectId="de53c560-d6a9-11da-a94d-0800200c9a66" version="39.00.000" type="contact data set" uri="../contacts/de53c560-d6a9-11da-a94d-0800200c9a66.xml">
          <common:shortDescription xmlns:epd="http://www.iai.kit.edu/EPD/2013" xml:lang="en">IABP-GaBi</common:shortDescription>
          <common:shortDescription xmlns:epd="http://www.iai.kit.edu/EPD/2013" xml:lang="de">IABP-GaBi</common:shortDescription>
        </common:referenceToNameOfReviewerAndInstitution>
        <common:referenceToNameOfReviewerAndInstitution xmlns:common="http://lca.jrc.it/ILCD/Common" refObjectId="c0a9feeb-48d1-4c8f-9e8f-3ada7c0294c7" version="39.00.000" type="contact data set" uri="../contacts/c0a9feeb-48d1-4c8f-9e8f-3ada7c0294c7.xml">
          <common:shortDescription xmlns:epd="http://www.iai.kit.edu/EPD/2013" xml:lang="en">IBP-GaBi</common:shortDescription>
          <common:shortDescription xmlns:epd="http://www.iai.kit.edu/EPD/2013" xml:lang="de">IBP-GaBi</common:shortDescription>
        </common:referenceToNameOfReviewerAndInstitution>
      </review>
      <review type="Independent external review">
        <common:referenceToNameOfReviewerAndInstitution xmlns:common="http://lca.jrc.it/ILCD/Common" refObjectId="8f1306f0-7b83-4f36-a537-aa83f0498266" version="39.00.000" type="contact data set" uri="../contacts/8f1306f0-7b83-4f36-a537-aa83f0498266.xml">
          <common:shortDescription xmlns:epd="http://www.iai.kit.edu/EPD/2013" xml:lang="en">GaBi user forum</common:shortDescription>
          <common:shortDescription xmlns:epd="http://www.iai.kit.edu/EPD/2013" xml:lang="de">GaBi user forum</common:shortDescription>
        </common:referenceToNameOfReviewerAndInstitution>
        <common:referenceToNameOfReviewerAndInstitution xmlns:common="http://lca.jrc.it/ILCD/Common" refObjectId="851d996c-b88d-45ce-983a-b00ed0393ffb" version="39.00.000" type="contact data set" uri="../contacts/851d996c-b88d-45ce-983a-b00ed0393ffb.xml">
          <common:shortDescription xmlns:epd="http://www.iai.kit.edu/EPD/2013" xml:lang="en">GaBi bug forum</common:shortDescription>
          <common:shortDescription xmlns:epd="http://www.iai.kit.edu/EPD/2013" xml:lang="de">GaBi bug forum</common:shortDescription>
        </common:referenceToNameOfReviewerAndInstitution>
        <common:referenceToNameOfReviewerAndInstitution xmlns:common="http://lca.jrc.it/ILCD/Common" refObjectId="47511c41-5096-4dcf-be4f-dbb0c1c5cffc" version="39.00.000" type="contact data set" uri="../contacts/47511c41-5096-4dcf-be4f-dbb0c1c5cffc.xml">
          <common:shortDescription xmlns:epd="http://www.iai.kit.edu/EPD/2013" xml:lang="en">GaBi user community</common:shortDescription>
          <common:shortDescription xmlns:epd="http://www.iai.kit.edu/EPD/2013" xml:lang="de">GaBi user community</common:shortDescription>
        </common:referenceToNameOfReviewerAndInstitution>
      </review>
    </validation>
    <complianceDeclarations>
      <compliance>
        <common:referenceToComplianceSystem xmlns:common="http://lca.jrc.it/ILCD/Common" refObjectId="b00f9ec0-7874-11e3-981f-0800200c9a66" version="02.00.000" type="source data set" uri="../sources/b00f9ec0-7874-11e3-981f-0800200c9a66.xml">
          <common:shortDescription xmlns:epd="http://www.iai.kit.edu/EPD/2013" xml:lang="en">DIN EN 15804</common:shortDescription>
          <common:shortDescription xmlns:epd="http://www.iai.kit.edu/EPD/2013" xml:lang="de">DIN EN 15804</common:shortDescription>
        </common:referenceToComplianceSystem>
        <common:approvalOfOverallCompliance xmlns:common="http://lca.jrc.it/ILCD/Common">Fully compliant</common:approvalOfOverallCompliance>
      </compliance>
    </complianceDeclarations>
  </modellingAndValidation>
  <administrativeInformation>
    <dataEntryBy>
      <common:timeStamp xmlns:common="http://lca.jrc.it/ILCD/Common">2019-12-04T10:06:49+01:00</common:timeStamp>
      <common:referenceToDataSetFormat xmlns:common="http://lca.jrc.it/ILCD/Common" refObjectId="a97a0155-0234-4b87-b4ce-a45da52f2a40" version="03.00.000" type="source data set" uri="../sources/a97a0155-0234-4b87-b4ce-a45da52f2a40.xml">
        <common:shortDescription xmlns:epd="http://www.iai.kit.edu/EPD/2013" xml:lang="en">ILCD format 1.1</common:shortDescription>
        <common:shortDescription xmlns:epd="http://www.iai.kit.edu/EPD/2013" xml:lang="de">ILCD format 1.1</common:shortDescription>
      </common:referenceToDataSetFormat>
      <common:referenceToDataSetFormat xmlns:common="http://lca.jrc.it/ILCD/Common" refObjectId="cba73800-7874-11e3-981f-0800200c9a66" version="02.00.000" type="source data set" uri="../sources/cba73800-7874-11e3-981f-0800200c9a66.xml">
        <common:shortDescription xmlns:epd="http://www.iai.kit.edu/EPD/2013" xml:lang="en">EPD Data Format Extensions</common:shortDescription>
        <common:shortDescription xmlns:epd="http://www.iai.kit.edu/EPD/2013" xml:lang="de">EPD-Datenformaterweiterungen</common:shortDescription>
      </common:referenceToDataSetFormat>
      <common:referenceToPersonOrEntityEnteringTheData xmlns:common="http://lca.jrc.it/ILCD/Common" refObjectId="d7fa0337-f279-430d-becf-7f3111a85010" version="39.00.000" type="contact data set" uri="../contacts/d7fa0337-f279-430d-becf-7f3111a85010.xml">
        <common:shortDescription xmlns:epd="http://www.iai.kit.edu/EPD/2013" xml:lang="en">thinkstep</common:shortDescription>
        <common:shortDescription xmlns:epd="http://www.iai.kit.edu/EPD/2013" xml:lang="de">thinkstep</common:shortDescription>
      </common:referenceToPersonOrEntityEnteringTheData>
    </dataEntryBy>
    <publicationAndOwnership>
      <common:dataSetVersion xmlns:common="http://lca.jrc.it/ILCD/Common">20.20.020</common:dataSetVersion>
      <common:permanentDataSetURI xmlns:common="http://lca.jrc.it/ILCD/Common"/>
      <common:referenceToOwnershipOfDataSet xmlns:common="http://lca.jrc.it/ILCD/Common" refObjectId="d7fa0337-f279-430d-becf-7f3111a85010" version="39.00.000" type="contact data set" uri="../contacts/d7fa0337-f279-430d-becf-7f3111a85010.xml">
        <common:shortDescription xmlns:epd="http://www.iai.kit.edu/EPD/2013" xml:lang="en">thinkstep</common:shortDescription>
        <common:shortDescription xmlns:epd="http://www.iai.kit.edu/EPD/2013" xml:lang="de">thinkstep</common:shortDescription>
      </common:referenceToOwnershipOfDataSet>
      <common:copyright xmlns:common="http://lca.jrc.it/ILCD/Common">true</common:copyright>
    </publicationAndOwnership>
  </administrativeInformation>
  <exchanges>
    <exchange dataSetInternalID="100076">
      <referenceToFlowDataSet refObjectId="b6509ee0-6753-4818-b960-000ac93c6739" version="39.00.000" type="flow data set" uri="../flows/b6509ee0-6753-4818-b960-000ac93c6739.xml">
        <common:shortDescription xmlns:common="http://lca.jrc.it/ILCD/Common" xmlns:epd="http://www.iai.kit.edu/EPD/2013" xml:lang="en">Expanded clay LB precision building block IW (m3)</common:shortDescription>
        <common:shortDescription xmlns:common="http://lca.jrc.it/ILCD/Common" xmlns:epd="http://www.iai.kit.edu/EPD/2013" xml:lang="de">Blähton LB Planstein Innenwand (m3)</common:shortDescription>
      </referenceToFlowDataSet>
      <meanAmount>1</meanAmount>
    </exchange>
    <exchange dataSetInternalID="100077">
      <referenceToFlowDataSet refObjectId="20f32be5-0398-4288-9b6d-accddd195317" version="39.00.000" type="flow data set" uri="../flows/20f32be5-0398-4288-9b6d-accddd195317.xml">
        <common:shortDescription xmlns:common="http://lca.jrc.it/ILCD/Common" xmlns:epd="http://www.iai.kit.edu/EPD/2013" xml:lang="en">Erneuerbare Primärenergie als Energieträger (PERE)</common:shortDescription>
        <common:shortDescription xmlns:common="http://lca.jrc.it/ILCD/Common" xmlns:epd="http://www.iai.kit.edu/EPD/2013" xml:lang="de">Erneuerbare Primärenergie als Energieträger (PERE)</common:shortDescription>
      </referenceToFlowDataSet>
      <functionType>General reminder flow</functionType>
      <exchangeDirection>Input</exchangeDirection>
      <common:other xmlns:common="http://lca.jrc.it/ILCD/Common">
        <epd:amount xmlns:epd="http://www.iai.kit.edu/EPD/2013" epd:module="A1-A3">405.271130221155</epd:amount>
        <epd:referenceToUnitGroupDataSet xmlns:epd="http://www.iai.kit.edu/EPD/2013" refObjectId="93a60a57-a3c8-11da-a746-0800200c9a66" version="03.00.000" type="unit group data set" uri="../unitgroups/93a60a57-a3c8-11da-a746-0800200c9a66.xml">
          <common:shortDescription xml:lang="en">MJ</common:shortDescription>
          <common:shortDescription xml:lang="de">MJ</common:shortDescription>
        </epd:referenceToUnitGroupDataSet>
        <epd:amount xmlns:epd="http://www.iai.kit.edu/EPD/2013" epd:module="C1">0.363474223311921</epd:amount>
        <epd:amount xmlns:epd="http://www.iai.kit.edu/EPD/2013" epd:module="C2">1.3983202047092</epd:amount>
        <epd:amount xmlns:epd="http://www.iai.kit.edu/EPD/2013" epd:module="C3">8.43841571602314</epd:amount>
        <epd:amount xmlns:epd="http://www.iai.kit.edu/EPD/2013" epd:module="D">-5.47234038638987</epd:amount>
      </common:other>
    </exchange>
    <exchange dataSetInternalID="100078">
      <referenceToFlowDataSet refObjectId="fb3ec0de-548d-4508-aea5-00b73bf6f702" version="39.00.000" type="flow data set" uri="../flows/fb3ec0de-548d-4508-aea5-00b73bf6f702.xml">
        <common:shortDescription xmlns:common="http://lca.jrc.it/ILCD/Common" xmlns:epd="http://www.iai.kit.edu/EPD/2013" xml:lang="en">Erneuerbare Primärenergie zur stofflichen Nutzung (PERM)</common:shortDescription>
        <common:shortDescription xmlns:common="http://lca.jrc.it/ILCD/Common" xmlns:epd="http://www.iai.kit.edu/EPD/2013" xml:lang="de">Erneuerbare Primärenergie zur stofflichen Nutzung (PERM)</common:shortDescription>
      </referenceToFlowDataSet>
      <functionType>General reminder flow</functionType>
      <exchangeDirection>Input</exchangeDirection>
      <common:other xmlns:common="http://lca.jrc.it/ILCD/Common">
        <epd:amount xmlns:epd="http://www.iai.kit.edu/EPD/2013" epd:module="A1-A3">0</epd:amount>
        <epd:referenceToUnitGroupDataSet xmlns:epd="http://www.iai.kit.edu/EPD/2013" refObjectId="93a60a57-a3c8-11da-a746-0800200c9a66" version="03.00.000" type="unit group data set" uri="../unitgroups/93a60a57-a3c8-11da-a746-0800200c9a66.xml">
          <common:shortDescription xml:lang="en">MJ</common:shortDescription>
          <common:shortDescription xml:lang="de">MJ</common:shortDescription>
        </epd:referenceToUnitGroupDataSet>
        <epd:amount xmlns:epd="http://www.iai.kit.edu/EPD/2013" epd:module="C1">0</epd:amount>
        <epd:amount xmlns:epd="http://www.iai.kit.edu/EPD/2013" epd:module="C2">0</epd:amount>
        <epd:amount xmlns:epd="http://www.iai.kit.edu/EPD/2013" epd:module="C3">0</epd:amount>
        <epd:amount xmlns:epd="http://www.iai.kit.edu/EPD/2013" epd:module="D">0</epd:amount>
      </common:other>
    </exchange>
    <exchange dataSetInternalID="100079">
      <referenceToFlowDataSet refObjectId="53f97275-fa8a-4cdd-9024-65936002acd0" version="39.00.000" type="flow data set" uri="../flows/53f97275-fa8a-4cdd-9024-65936002acd0.xml">
        <common:shortDescription xmlns:common="http://lca.jrc.it/ILCD/Common" xmlns:epd="http://www.iai.kit.edu/EPD/2013" xml:lang="en">Total use of renewable primary energy resources (PERT)</common:shortDescription>
        <common:shortDescription xmlns:common="http://lca.jrc.it/ILCD/Common" xmlns:epd="http://www.iai.kit.edu/EPD/2013" xml:lang="de">Total erneuerbare Primärenergie (PERT)</common:shortDescription>
      </referenceToFlowDataSet>
      <functionType>General reminder flow</functionType>
      <exchangeDirection>Input</exchangeDirection>
      <common:other xmlns:common="http://lca.jrc.it/ILCD/Common">
        <epd:amount xmlns:epd="http://www.iai.kit.edu/EPD/2013" epd:module="A1-A3">405.271130221155</epd:amount>
        <epd:referenceToUnitGroupDataSet xmlns:epd="http://www.iai.kit.edu/EPD/2013" refObjectId="93a60a57-a3c8-11da-a746-0800200c9a66" version="03.00.000" type="unit group data set" uri="../unitgroups/93a60a57-a3c8-11da-a746-0800200c9a66.xml">
          <common:shortDescription xml:lang="en">MJ</common:shortDescription>
          <common:shortDescription xml:lang="de">MJ</common:shortDescription>
        </epd:referenceToUnitGroupDataSet>
        <epd:amount xmlns:epd="http://www.iai.kit.edu/EPD/2013" epd:module="C1">0.363474223311921</epd:amount>
        <epd:amount xmlns:epd="http://www.iai.kit.edu/EPD/2013" epd:module="C2">1.3983202047092</epd:amount>
        <epd:amount xmlns:epd="http://www.iai.kit.edu/EPD/2013" epd:module="C3">8.43841571602314</epd:amount>
        <epd:amount xmlns:epd="http://www.iai.kit.edu/EPD/2013" epd:module="D">-5.47234038638987</epd:amount>
      </common:other>
    </exchange>
    <exchange dataSetInternalID="100080">
      <referenceToFlowDataSet refObjectId="ac857178-2b45-46ec-892a-a9a4332f0372" version="39.00.000" type="flow data set" uri="../flows/ac857178-2b45-46ec-892a-a9a4332f0372.xml">
        <common:shortDescription xmlns:common="http://lca.jrc.it/ILCD/Common" xmlns:epd="http://www.iai.kit.edu/EPD/2013" xml:lang="en">Nicht-erneuerbare Primärenergie als Energieträger (PENRE)</common:shortDescription>
        <common:shortDescription xmlns:common="http://lca.jrc.it/ILCD/Common" xmlns:epd="http://www.iai.kit.edu/EPD/2013" xml:lang="de">Nicht-erneuerbare Primärenergie als Energieträger (PENRE)</common:shortDescription>
      </referenceToFlowDataSet>
      <functionType>General reminder flow</functionType>
      <exchangeDirection>Input</exchangeDirection>
      <common:other xmlns:common="http://lca.jrc.it/ILCD/Common">
        <epd:amount xmlns:epd="http://www.iai.kit.edu/EPD/2013" epd:module="A1-A3">2018.52090456673</epd:amount>
        <epd:referenceToUnitGroupDataSet xmlns:epd="http://www.iai.kit.edu/EPD/2013" refObjectId="93a60a57-a3c8-11da-a746-0800200c9a66" version="03.00.000" type="unit group data set" uri="../unitgroups/93a60a57-a3c8-11da-a746-0800200c9a66.xml">
          <common:shortDescription xml:lang="en">MJ</common:shortDescription>
          <common:shortDescription xml:lang="de">MJ</common:shortDescription>
        </epd:referenceToUnitGroupDataSet>
        <epd:amount xmlns:epd="http://www.iai.kit.edu/EPD/2013" epd:module="C1">6.24354344775955</epd:amount>
        <epd:amount xmlns:epd="http://www.iai.kit.edu/EPD/2013" epd:module="C2">24.0195105788553</epd:amount>
        <epd:amount xmlns:epd="http://www.iai.kit.edu/EPD/2013" epd:module="C3">78.1765288816641</epd:amount>
        <epd:amount xmlns:epd="http://www.iai.kit.edu/EPD/2013" epd:module="D">-19.1865911407486</epd:amount>
      </common:other>
    </exchange>
    <exchange dataSetInternalID="100081">
      <referenceToFlowDataSet refObjectId="1421caa0-679d-4bf4-b282-0eb850ccae27" version="39.00.000" type="flow data set" uri="../flows/1421caa0-679d-4bf4-b282-0eb850ccae27.xml">
        <common:shortDescription xmlns:common="http://lca.jrc.it/ILCD/Common" xmlns:epd="http://www.iai.kit.edu/EPD/2013" xml:lang="en">Nicht-erneuerbare Primärenergie zur stofflichen Nutzung (PENRM)</common:shortDescription>
        <common:shortDescription xmlns:common="http://lca.jrc.it/ILCD/Common" xmlns:epd="http://www.iai.kit.edu/EPD/2013" xml:lang="de">Nicht-erneuerbare Primärenergie zur stofflichen Nutzung (PENRM)</common:shortDescription>
      </referenceToFlowDataSet>
      <functionType>General reminder flow</functionType>
      <exchangeDirection>Input</exchangeDirection>
      <common:other xmlns:common="http://lca.jrc.it/ILCD/Common">
        <epd:amount xmlns:epd="http://www.iai.kit.edu/EPD/2013" epd:module="A1-A3">0</epd:amount>
        <epd:referenceToUnitGroupDataSet xmlns:epd="http://www.iai.kit.edu/EPD/2013" refObjectId="93a60a57-a3c8-11da-a746-0800200c9a66" version="03.00.000" type="unit group data set" uri="../unitgroups/93a60a57-a3c8-11da-a746-0800200c9a66.xml">
          <common:shortDescription xml:lang="en">MJ</common:shortDescription>
          <common:shortDescription xml:lang="de">MJ</common:shortDescription>
        </epd:referenceToUnitGroupDataSet>
        <epd:amount xmlns:epd="http://www.iai.kit.edu/EPD/2013" epd:module="C1">0</epd:amount>
        <epd:amount xmlns:epd="http://www.iai.kit.edu/EPD/2013" epd:module="C2">0</epd:amount>
        <epd:amount xmlns:epd="http://www.iai.kit.edu/EPD/2013" epd:module="C3">0</epd:amount>
        <epd:amount xmlns:epd="http://www.iai.kit.edu/EPD/2013" epd:module="D">0</epd:amount>
      </common:other>
    </exchange>
    <exchange dataSetInternalID="100082">
      <referenceToFlowDataSet refObjectId="06159210-646b-4c8d-8583-da9b3b95a6c1" version="39.00.000" type="flow data set" uri="../flows/06159210-646b-4c8d-8583-da9b3b95a6c1.xml">
        <common:shortDescription xmlns:common="http://lca.jrc.it/ILCD/Common" xmlns:epd="http://www.iai.kit.edu/EPD/2013" xml:lang="en">Total use of non-renewable primary energy resources (PENRT)</common:shortDescription>
        <common:shortDescription xmlns:common="http://lca.jrc.it/ILCD/Common" xmlns:epd="http://www.iai.kit.edu/EPD/2013" xml:lang="de">Total nicht erneuerbare Primärenergie (PENRT)</common:shortDescription>
      </referenceToFlowDataSet>
      <functionType>General reminder flow</functionType>
      <exchangeDirection>Input</exchangeDirection>
      <common:other xmlns:common="http://lca.jrc.it/ILCD/Common">
        <epd:amount xmlns:epd="http://www.iai.kit.edu/EPD/2013" epd:module="A1-A3">2018.52090456673</epd:amount>
        <epd:referenceToUnitGroupDataSet xmlns:epd="http://www.iai.kit.edu/EPD/2013" refObjectId="93a60a57-a3c8-11da-a746-0800200c9a66" version="03.00.000" type="unit group data set" uri="../unitgroups/93a60a57-a3c8-11da-a746-0800200c9a66.xml">
          <common:shortDescription xml:lang="en">MJ</common:shortDescription>
          <common:shortDescription xml:lang="de">MJ</common:shortDescription>
        </epd:referenceToUnitGroupDataSet>
        <epd:amount xmlns:epd="http://www.iai.kit.edu/EPD/2013" epd:module="C1">6.24354344775955</epd:amount>
        <epd:amount xmlns:epd="http://www.iai.kit.edu/EPD/2013" epd:module="C2">24.0195105788553</epd:amount>
        <epd:amount xmlns:epd="http://www.iai.kit.edu/EPD/2013" epd:module="C3">78.1765288816641</epd:amount>
        <epd:amount xmlns:epd="http://www.iai.kit.edu/EPD/2013" epd:module="D">-19.1865911407486</epd:amount>
      </common:other>
    </exchange>
    <exchange dataSetInternalID="100083">
      <referenceToFlowDataSet refObjectId="c6a1f35f-2d09-4f54-8dfb-97e502e1ce92" version="39.00.000" type="flow data set" uri="../flows/c6a1f35f-2d09-4f54-8dfb-97e502e1ce92.xml">
        <common:shortDescription xmlns:common="http://lca.jrc.it/ILCD/Common" xmlns:epd="http://www.iai.kit.edu/EPD/2013" xml:lang="en">Input of secondary material (SM)</common:shortDescription>
        <common:shortDescription xmlns:common="http://lca.jrc.it/ILCD/Common" xmlns:epd="http://www.iai.kit.edu/EPD/2013" xml:lang="de">Einsatz von Sekundärstoffen (SM)</common:shortDescription>
      </referenceToFlowDataSet>
      <functionType>General reminder flow</functionType>
      <exchangeDirection>Input</exchangeDirection>
      <common:other xmlns:common="http://lca.jrc.it/ILCD/Common">
        <epd:amount xmlns:epd="http://www.iai.kit.edu/EPD/2013" epd:module="A1-A3">0</epd:amount>
        <epd:referenceToUnitGroupDataSet xmlns:epd="http://www.iai.kit.edu/EPD/2013" refObjectId="93a60a57-a4c8-11da-a746-0800200c9a66" version="03.00.000" type="unit group data set" uri="../unitgroups/93a60a57-a4c8-11da-a746-0800200c9a66.xml">
          <common:shortDescription xml:lang="en">kg</common:shortDescription>
          <common:shortDescription xml:lang="de">kg</common:shortDescription>
        </epd:referenceToUnitGroupDataSet>
        <epd:amount xmlns:epd="http://www.iai.kit.edu/EPD/2013" epd:module="C1">0</epd:amount>
        <epd:amount xmlns:epd="http://www.iai.kit.edu/EPD/2013" epd:module="C2">0</epd:amount>
        <epd:amount xmlns:epd="http://www.iai.kit.edu/EPD/2013" epd:module="C3">0</epd:amount>
        <epd:amount xmlns:epd="http://www.iai.kit.edu/EPD/2013" epd:module="D">0</epd:amount>
      </common:other>
    </exchange>
    <exchange dataSetInternalID="100084">
      <referenceToFlowDataSet refObjectId="64333088-a55f-4aa2-9a31-c10b07816787" version="39.00.000" type="flow data set" uri="../flows/64333088-a55f-4aa2-9a31-c10b07816787.xml">
        <common:shortDescription xmlns:common="http://lca.jrc.it/ILCD/Common" xmlns:epd="http://www.iai.kit.edu/EPD/2013" xml:lang="en">Use of renewable secondary fuels (RSF)</common:shortDescription>
        <common:shortDescription xmlns:common="http://lca.jrc.it/ILCD/Common" xmlns:epd="http://www.iai.kit.edu/EPD/2013" xml:lang="de">Erneuerbare Sekundärbrennstoffe (RSF)</common:shortDescription>
      </referenceToFlowDataSet>
      <functionType>General reminder flow</functionType>
      <exchangeDirection>Input</exchangeDirection>
      <common:other xmlns:common="http://lca.jrc.it/ILCD/Common">
        <epd:amount xmlns:epd="http://www.iai.kit.edu/EPD/2013" epd:module="A1-A3">0.976724679029957</epd:amount>
        <epd:referenceToUnitGroupDataSet xmlns:epd="http://www.iai.kit.edu/EPD/2013" refObjectId="93a60a57-a3c8-11da-a746-0800200c9a66" version="03.00.000" type="unit group data set" uri="../unitgroups/93a60a57-a3c8-11da-a746-0800200c9a66.xml">
          <common:shortDescription xml:lang="en">MJ</common:shortDescription>
          <common:shortDescription xml:lang="de">MJ</common:shortDescription>
        </epd:referenceToUnitGroupDataSet>
        <epd:amount xmlns:epd="http://www.iai.kit.edu/EPD/2013" epd:module="C1">0</epd:amount>
        <epd:amount xmlns:epd="http://www.iai.kit.edu/EPD/2013" epd:module="C2">0</epd:amount>
        <epd:amount xmlns:epd="http://www.iai.kit.edu/EPD/2013" epd:module="C3">0</epd:amount>
        <epd:amount xmlns:epd="http://www.iai.kit.edu/EPD/2013" epd:module="D">0</epd:amount>
      </common:other>
    </exchange>
    <exchange dataSetInternalID="100085">
      <referenceToFlowDataSet refObjectId="89def144-d39a-4287-b86f-efde453ddcb2" version="39.00.000" type="flow data set" uri="../flows/89def144-d39a-4287-b86f-efde453ddcb2.xml">
        <common:shortDescription xmlns:common="http://lca.jrc.it/ILCD/Common" xmlns:epd="http://www.iai.kit.edu/EPD/2013" xml:lang="en">Use of non renewable secondary fuels (NRSF)</common:shortDescription>
        <common:shortDescription xmlns:common="http://lca.jrc.it/ILCD/Common" xmlns:epd="http://www.iai.kit.edu/EPD/2013" xml:lang="de">Nicht erneuerbare Sekundärbrennstoffe (NRSF)</common:shortDescription>
      </referenceToFlowDataSet>
      <functionType>General reminder flow</functionType>
      <exchangeDirection>Input</exchangeDirection>
      <common:other xmlns:common="http://lca.jrc.it/ILCD/Common">
        <epd:amount xmlns:epd="http://www.iai.kit.edu/EPD/2013" epd:module="A1-A3">10.274392296719</epd:amount>
        <epd:referenceToUnitGroupDataSet xmlns:epd="http://www.iai.kit.edu/EPD/2013" refObjectId="93a60a57-a3c8-11da-a746-0800200c9a66" version="03.00.000" type="unit group data set" uri="../unitgroups/93a60a57-a3c8-11da-a746-0800200c9a66.xml">
          <common:shortDescription xml:lang="en">MJ</common:shortDescription>
          <common:shortDescription xml:lang="de">MJ</common:shortDescription>
        </epd:referenceToUnitGroupDataSet>
        <epd:amount xmlns:epd="http://www.iai.kit.edu/EPD/2013" epd:module="C1">0</epd:amount>
        <epd:amount xmlns:epd="http://www.iai.kit.edu/EPD/2013" epd:module="C2">0</epd:amount>
        <epd:amount xmlns:epd="http://www.iai.kit.edu/EPD/2013" epd:module="C3">0</epd:amount>
        <epd:amount xmlns:epd="http://www.iai.kit.edu/EPD/2013" epd:module="D">0</epd:amount>
      </common:other>
    </exchange>
    <exchange dataSetInternalID="100086">
      <referenceToFlowDataSet refObjectId="3cf952c8-f3a4-461d-8c96-96456ca62246" version="39.00.000" type="flow data set" uri="../flows/3cf952c8-f3a4-461d-8c96-96456ca62246.xml">
        <common:shortDescription xmlns:common="http://lca.jrc.it/ILCD/Common" xmlns:epd="http://www.iai.kit.edu/EPD/2013" xml:lang="en">Use of net fresh water (FW)</common:shortDescription>
        <common:shortDescription xmlns:common="http://lca.jrc.it/ILCD/Common" xmlns:epd="http://www.iai.kit.edu/EPD/2013" xml:lang="de">Einsatz von Süßwasserressourcen (FW)</common:shortDescription>
      </referenceToFlowDataSet>
      <functionType>General reminder flow</functionType>
      <exchangeDirection>Input</exchangeDirection>
      <common:other xmlns:common="http://lca.jrc.it/ILCD/Common">
        <epd:amount xmlns:epd="http://www.iai.kit.edu/EPD/2013" epd:module="A1-A3">0.444560972257769</epd:amount>
        <epd:referenceToUnitGroupDataSet xmlns:epd="http://www.iai.kit.edu/EPD/2013" refObjectId="93a60a57-a3c8-12da-a746-0800200c9a66" version="03.00.000" type="unit group data set" uri="../unitgroups/93a60a57-a3c8-12da-a746-0800200c9a66.xml">
          <common:shortDescription xml:lang="en">m3</common:shortDescription>
          <common:shortDescription xml:lang="de">m3</common:shortDescription>
        </epd:referenceToUnitGroupDataSet>
        <epd:amount xmlns:epd="http://www.iai.kit.edu/EPD/2013" epd:module="C1">0.000325521668997333</epd:amount>
        <epd:amount xmlns:epd="http://www.iai.kit.edu/EPD/2013" epd:module="C2">0.00125231308751984</epd:amount>
        <epd:amount xmlns:epd="http://www.iai.kit.edu/EPD/2013" epd:module="C3">0.0200578969030086</epd:amount>
        <epd:amount xmlns:epd="http://www.iai.kit.edu/EPD/2013" epd:module="D">-0.00354881982213959</epd:amount>
      </common:other>
    </exchange>
    <exchange dataSetInternalID="100087">
      <referenceToFlowDataSet refObjectId="430f9e0f-59b2-46a0-8e0d-55e0e84948fc" version="39.00.000" type="flow data set" uri="../flows/430f9e0f-59b2-46a0-8e0d-55e0e84948fc.xml">
        <common:shortDescription xmlns:common="http://lca.jrc.it/ILCD/Common" xmlns:epd="http://www.iai.kit.edu/EPD/2013" xml:lang="en">Hazardous waste disposed (HWD)</common:shortDescription>
        <common:shortDescription xmlns:common="http://lca.jrc.it/ILCD/Common" xmlns:epd="http://www.iai.kit.edu/EPD/2013" xml:lang="de">Gefährlicher Abfall zur Deponie (HWD)</common:shortDescription>
      </referenceToFlowDataSet>
      <functionType>General reminder flow</functionType>
      <exchangeDirection>Output</exchangeDirection>
      <common:other xmlns:common="http://lca.jrc.it/ILCD/Common">
        <epd:amount xmlns:epd="http://www.iai.kit.edu/EPD/2013" epd:module="A1-A3">8.17881783334828E-6</epd:amount>
        <epd:referenceToUnitGroupDataSet xmlns:epd="http://www.iai.kit.edu/EPD/2013" refObjectId="93a60a57-a4c8-11da-a746-0800200c9a66" version="03.00.000" type="unit group data set" uri="../unitgroups/93a60a57-a4c8-11da-a746-0800200c9a66.xml">
          <common:shortDescription xml:lang="en">kg</common:shortDescription>
          <common:shortDescription xml:lang="de">kg</common:shortDescription>
        </epd:referenceToUnitGroupDataSet>
        <epd:amount xmlns:epd="http://www.iai.kit.edu/EPD/2013" epd:module="C1">2.33314706473154E-7</epd:amount>
        <epd:amount xmlns:epd="http://www.iai.kit.edu/EPD/2013" epd:module="C2">8.97584057390588E-7</epd:amount>
        <epd:amount xmlns:epd="http://www.iai.kit.edu/EPD/2013" epd:module="C3">1.41606760115646E-6</epd:amount>
        <epd:amount xmlns:epd="http://www.iai.kit.edu/EPD/2013" epd:module="D">-3.61635583220129E-7</epd:amount>
      </common:other>
    </exchange>
    <exchange dataSetInternalID="100088">
      <referenceToFlowDataSet refObjectId="b29ef66b-e286-4afa-949f-62f1a7b4d7fa" version="39.00.000" type="flow data set" uri="../flows/b29ef66b-e286-4afa-949f-62f1a7b4d7fa.xml">
        <common:shortDescription xmlns:common="http://lca.jrc.it/ILCD/Common" xmlns:epd="http://www.iai.kit.edu/EPD/2013" xml:lang="en">Non-hazardous waste disposed (NHWD)</common:shortDescription>
        <common:shortDescription xmlns:common="http://lca.jrc.it/ILCD/Common" xmlns:epd="http://www.iai.kit.edu/EPD/2013" xml:lang="de">Entsorgter nicht gefährlicher Abfall (NHWD)</common:shortDescription>
      </referenceToFlowDataSet>
      <functionType>General reminder flow</functionType>
      <exchangeDirection>Output</exchangeDirection>
      <common:other xmlns:common="http://lca.jrc.it/ILCD/Common">
        <epd:amount xmlns:epd="http://www.iai.kit.edu/EPD/2013" epd:module="A1-A3">3.71905272885172</epd:amount>
        <epd:referenceToUnitGroupDataSet xmlns:epd="http://www.iai.kit.edu/EPD/2013" refObjectId="93a60a57-a4c8-11da-a746-0800200c9a66" version="03.00.000" type="unit group data set" uri="../unitgroups/93a60a57-a4c8-11da-a746-0800200c9a66.xml">
          <common:shortDescription xml:lang="en">kg</common:shortDescription>
          <common:shortDescription xml:lang="de">kg</common:shortDescription>
        </epd:referenceToUnitGroupDataSet>
        <epd:amount xmlns:epd="http://www.iai.kit.edu/EPD/2013" epd:module="C1">0.00109585098601902</epd:amount>
        <epd:amount xmlns:epd="http://www.iai.kit.edu/EPD/2013" epd:module="C2">0.00421584386683146</epd:amount>
        <epd:amount xmlns:epd="http://www.iai.kit.edu/EPD/2013" epd:module="C3">198.661263714075</epd:amount>
        <epd:amount xmlns:epd="http://www.iai.kit.edu/EPD/2013" epd:module="D">-11.2777673457207</epd:amount>
      </common:other>
    </exchange>
    <exchange dataSetInternalID="100089">
      <referenceToFlowDataSet refObjectId="3449546e-52ad-4b39-b809-9fb77cea8ff6" version="39.00.000" type="flow data set" uri="../flows/3449546e-52ad-4b39-b809-9fb77cea8ff6.xml">
        <common:shortDescription xmlns:common="http://lca.jrc.it/ILCD/Common" xmlns:epd="http://www.iai.kit.edu/EPD/2013" xml:lang="en">Radioactive waste disposed (RWD)</common:shortDescription>
        <common:shortDescription xmlns:common="http://lca.jrc.it/ILCD/Common" xmlns:epd="http://www.iai.kit.edu/EPD/2013" xml:lang="de">Entsorgter radioaktiver Abfall (RWD)</common:shortDescription>
      </referenceToFlowDataSet>
      <functionType>General reminder flow</functionType>
      <exchangeDirection>Output</exchangeDirection>
      <common:other xmlns:common="http://lca.jrc.it/ILCD/Common">
        <epd:amount xmlns:epd="http://www.iai.kit.edu/EPD/2013" epd:module="A1-A3">0.0354649521785423</epd:amount>
        <epd:referenceToUnitGroupDataSet xmlns:epd="http://www.iai.kit.edu/EPD/2013" refObjectId="93a60a57-a4c8-11da-a746-0800200c9a66" version="03.00.000" type="unit group data set" uri="../unitgroups/93a60a57-a4c8-11da-a746-0800200c9a66.xml">
          <common:shortDescription xml:lang="en">kg</common:shortDescription>
          <common:shortDescription xml:lang="de">kg</common:shortDescription>
        </epd:referenceToUnitGroupDataSet>
        <epd:amount xmlns:epd="http://www.iai.kit.edu/EPD/2013" epd:module="C1">6.57316842115322E-6</epd:amount>
        <epd:amount xmlns:epd="http://www.iai.kit.edu/EPD/2013" epd:module="C2">2.52876094720127E-5</epd:amount>
        <epd:amount xmlns:epd="http://www.iai.kit.edu/EPD/2013" epd:module="C3">0.000753424228948066</epd:amount>
        <epd:amount xmlns:epd="http://www.iai.kit.edu/EPD/2013" epd:module="D">-0.000714387096067933</epd:amount>
      </common:other>
    </exchange>
    <exchange dataSetInternalID="100090">
      <referenceToFlowDataSet refObjectId="a2b32f97-3fc7-4af2-b209-525bc6426f33" version="39.00.000" type="flow data set" uri="../flows/a2b32f97-3fc7-4af2-b209-525bc6426f33.xml">
        <common:shortDescription xmlns:common="http://lca.jrc.it/ILCD/Common" xmlns:epd="http://www.iai.kit.edu/EPD/2013" xml:lang="en">Components for re-use (CRU)</common:shortDescription>
        <common:shortDescription xmlns:common="http://lca.jrc.it/ILCD/Common" xmlns:epd="http://www.iai.kit.edu/EPD/2013" xml:lang="de">Komponenten für die Wiederverwendung (CRU)</common:shortDescription>
      </referenceToFlowDataSet>
      <functionType>General reminder flow</functionType>
      <exchangeDirection>Output</exchangeDirection>
      <common:other xmlns:common="http://lca.jrc.it/ILCD/Common">
        <epd:amount xmlns:epd="http://www.iai.kit.edu/EPD/2013" epd:module="A1-A3">0</epd:amount>
        <epd:referenceToUnitGroupDataSet xmlns:epd="http://www.iai.kit.edu/EPD/2013" refObjectId="93a60a57-a4c8-11da-a746-0800200c9a66" version="03.00.000" type="unit group data set" uri="../unitgroups/93a60a57-a4c8-11da-a746-0800200c9a66.xml">
          <common:shortDescription xml:lang="en">kg</common:shortDescription>
          <common:shortDescription xml:lang="de">kg</common:shortDescription>
        </epd:referenceToUnitGroupDataSet>
        <epd:amount xmlns:epd="http://www.iai.kit.edu/EPD/2013" epd:module="C1">0</epd:amount>
        <epd:amount xmlns:epd="http://www.iai.kit.edu/EPD/2013" epd:module="C2">0</epd:amount>
        <epd:amount xmlns:epd="http://www.iai.kit.edu/EPD/2013" epd:module="C3">0</epd:amount>
        <epd:amount xmlns:epd="http://www.iai.kit.edu/EPD/2013" epd:module="D">0</epd:amount>
      </common:other>
    </exchange>
    <exchange dataSetInternalID="100091">
      <referenceToFlowDataSet refObjectId="d7fe48a5-4103-49c8-9aae-b0b5dfdbd6ae" version="39.00.000" type="flow data set" uri="../flows/d7fe48a5-4103-49c8-9aae-b0b5dfdbd6ae.xml">
        <common:shortDescription xmlns:common="http://lca.jrc.it/ILCD/Common" xmlns:epd="http://www.iai.kit.edu/EPD/2013" xml:lang="en">Materials for Recycling (MFR)</common:shortDescription>
        <common:shortDescription xmlns:common="http://lca.jrc.it/ILCD/Common" xmlns:epd="http://www.iai.kit.edu/EPD/2013" xml:lang="de">Stoffe zum Recycling (MFR)</common:shortDescription>
      </referenceToFlowDataSet>
      <functionType>General reminder flow</functionType>
      <exchangeDirection>Output</exchangeDirection>
      <common:other xmlns:common="http://lca.jrc.it/ILCD/Common">
        <epd:amount xmlns:epd="http://www.iai.kit.edu/EPD/2013" epd:module="A1-A3">0</epd:amount>
        <epd:referenceToUnitGroupDataSet xmlns:epd="http://www.iai.kit.edu/EPD/2013" refObjectId="93a60a57-a4c8-11da-a746-0800200c9a66" version="03.00.000" type="unit group data set" uri="../unitgroups/93a60a57-a4c8-11da-a746-0800200c9a66.xml">
          <common:shortDescription xml:lang="en">kg</common:shortDescription>
          <common:shortDescription xml:lang="de">kg</common:shortDescription>
        </epd:referenceToUnitGroupDataSet>
        <epd:amount xmlns:epd="http://www.iai.kit.edu/EPD/2013" epd:module="C1">0</epd:amount>
        <epd:amount xmlns:epd="http://www.iai.kit.edu/EPD/2013" epd:module="C2">0</epd:amount>
        <epd:amount xmlns:epd="http://www.iai.kit.edu/EPD/2013" epd:module="C3">595.360824742268</epd:amount>
        <epd:amount xmlns:epd="http://www.iai.kit.edu/EPD/2013" epd:module="D">0</epd:amount>
      </common:other>
    </exchange>
    <exchange dataSetInternalID="100092">
      <referenceToFlowDataSet refObjectId="59a9181c-3aaf-46ee-8b13-2b3723b6e447" version="39.00.000" type="flow data set" uri="../flows/59a9181c-3aaf-46ee-8b13-2b3723b6e447.xml">
        <common:shortDescription xmlns:common="http://lca.jrc.it/ILCD/Common" xmlns:epd="http://www.iai.kit.edu/EPD/2013" xml:lang="en">Material for Energy Recovery (MER)</common:shortDescription>
        <common:shortDescription xmlns:common="http://lca.jrc.it/ILCD/Common" xmlns:epd="http://www.iai.kit.edu/EPD/2013" xml:lang="de">Stoffe für die Energierückgewinnung (MER)</common:shortDescription>
      </referenceToFlowDataSet>
      <functionType>General reminder flow</functionType>
      <exchangeDirection>Output</exchangeDirection>
      <common:other xmlns:common="http://lca.jrc.it/ILCD/Common">
        <epd:amount xmlns:epd="http://www.iai.kit.edu/EPD/2013" epd:module="A1-A3">0</epd:amount>
        <epd:referenceToUnitGroupDataSet xmlns:epd="http://www.iai.kit.edu/EPD/2013" refObjectId="93a60a57-a4c8-11da-a746-0800200c9a66" version="03.00.000" type="unit group data set" uri="../unitgroups/93a60a57-a4c8-11da-a746-0800200c9a66.xml">
          <common:shortDescription xml:lang="en">kg</common:shortDescription>
          <common:shortDescription xml:lang="de">kg</common:shortDescription>
        </epd:referenceToUnitGroupDataSet>
        <epd:amount xmlns:epd="http://www.iai.kit.edu/EPD/2013" epd:module="C1">0</epd:amount>
        <epd:amount xmlns:epd="http://www.iai.kit.edu/EPD/2013" epd:module="C2">0</epd:amount>
        <epd:amount xmlns:epd="http://www.iai.kit.edu/EPD/2013" epd:module="C3">0</epd:amount>
        <epd:amount xmlns:epd="http://www.iai.kit.edu/EPD/2013" epd:module="D">0</epd:amount>
      </common:other>
    </exchange>
    <exchange dataSetInternalID="100093">
      <referenceToFlowDataSet refObjectId="4da0c987-2b76-40d6-9e9e-82a017aaaf29" version="39.00.000" type="flow data set" uri="../flows/4da0c987-2b76-40d6-9e9e-82a017aaaf29.xml">
        <common:shortDescription xmlns:common="http://lca.jrc.it/ILCD/Common" xmlns:epd="http://www.iai.kit.edu/EPD/2013" xml:lang="en">Exported electrical energy (EEE)</common:shortDescription>
        <common:shortDescription xmlns:common="http://lca.jrc.it/ILCD/Common" xmlns:epd="http://www.iai.kit.edu/EPD/2013" xml:lang="de">Exportierte elektrische Energie (EEE)</common:shortDescription>
      </referenceToFlowDataSet>
      <functionType>General reminder flow</functionType>
      <exchangeDirection>Output</exchangeDirection>
      <common:other xmlns:common="http://lca.jrc.it/ILCD/Common">
        <epd:amount xmlns:epd="http://www.iai.kit.edu/EPD/2013" epd:module="A1-A3">0</epd:amount>
        <epd:referenceToUnitGroupDataSet xmlns:epd="http://www.iai.kit.edu/EPD/2013" refObjectId="93a60a57-a3c8-11da-a746-0800200c9a66" version="03.00.000" type="unit group data set" uri="../unitgroups/93a60a57-a3c8-11da-a746-0800200c9a66.xml">
          <common:shortDescription xml:lang="en">MJ</common:shortDescription>
          <common:shortDescription xml:lang="de">MJ</common:shortDescription>
        </epd:referenceToUnitGroupDataSet>
        <epd:amount xmlns:epd="http://www.iai.kit.edu/EPD/2013" epd:module="C1">0</epd:amount>
        <epd:amount xmlns:epd="http://www.iai.kit.edu/EPD/2013" epd:module="C2">0</epd:amount>
        <epd:amount xmlns:epd="http://www.iai.kit.edu/EPD/2013" epd:module="C3">0</epd:amount>
        <epd:amount xmlns:epd="http://www.iai.kit.edu/EPD/2013" epd:module="D">0</epd:amount>
      </common:other>
    </exchange>
    <exchange dataSetInternalID="100094">
      <referenceToFlowDataSet refObjectId="98daf38a-7a79-46d3-9a37-2b7bd0955810" version="39.00.000" type="flow data set" uri="../flows/98daf38a-7a79-46d3-9a37-2b7bd0955810.xml">
        <common:shortDescription xmlns:common="http://lca.jrc.it/ILCD/Common" xmlns:epd="http://www.iai.kit.edu/EPD/2013" xml:lang="en">Exported thermal energy (EET)</common:shortDescription>
        <common:shortDescription xmlns:common="http://lca.jrc.it/ILCD/Common" xmlns:epd="http://www.iai.kit.edu/EPD/2013" xml:lang="de">Exportierte thermische Energie (EET)</common:shortDescription>
      </referenceToFlowDataSet>
      <functionType>General reminder flow</functionType>
      <exchangeDirection>Output</exchangeDirection>
      <common:other xmlns:common="http://lca.jrc.it/ILCD/Common">
        <epd:amount xmlns:epd="http://www.iai.kit.edu/EPD/2013" epd:module="A1-A3">0</epd:amount>
        <epd:referenceToUnitGroupDataSet xmlns:epd="http://www.iai.kit.edu/EPD/2013" refObjectId="93a60a57-a3c8-11da-a746-0800200c9a66" version="03.00.000" type="unit group data set" uri="../unitgroups/93a60a57-a3c8-11da-a746-0800200c9a66.xml">
          <common:shortDescription xml:lang="en">MJ</common:shortDescription>
          <common:shortDescription xml:lang="de">MJ</common:shortDescription>
        </epd:referenceToUnitGroupDataSet>
        <epd:amount xmlns:epd="http://www.iai.kit.edu/EPD/2013" epd:module="C1">0</epd:amount>
        <epd:amount xmlns:epd="http://www.iai.kit.edu/EPD/2013" epd:module="C2">0</epd:amount>
        <epd:amount xmlns:epd="http://www.iai.kit.edu/EPD/2013" epd:module="C3">0</epd:amount>
        <epd:amount xmlns:epd="http://www.iai.kit.edu/EPD/2013" epd:module="D">0</epd:amount>
      </common:other>
    </exchange>
  </exchanges>
  <LCIAResults>
    <LCIAResult>
      <referenceToLCIAMethodDataSet refObjectId="77e416eb-a363-4258-a04e-171d843a6460" version="39.00.000" type="LCIA method data set" uri="../lciamethods/77e416eb-a363-4258-a04e-171d843a6460.xml">
        <common:shortDescription xmlns:common="http://lca.jrc.it/ILCD/Common" xmlns:epd="http://www.iai.kit.edu/EPD/2013" xml:lang="en">Global warming potential (GWP)</common:shortDescription>
        <common:shortDescription xmlns:common="http://lca.jrc.it/ILCD/Common" xmlns:epd="http://www.iai.kit.edu/EPD/2013" xml:lang="de">Globales Erwärmungspotenzial (GWP)</common:shortDescription>
      </referenceToLCIAMethodDataSet>
      <common:other xmlns:common="http://lca.jrc.it/ILCD/Common">
        <epd:amount xmlns:epd="http://www.iai.kit.edu/EPD/2013" epd:module="A1-A3">212.643300775782</epd:amount>
        <epd:amount xmlns:epd="http://www.iai.kit.edu/EPD/2013" epd:module="C1">0.46127527026048</epd:amount>
        <epd:amount xmlns:epd="http://www.iai.kit.edu/EPD/2013" epd:module="C2">1.78708143423231</epd:amount>
        <epd:amount xmlns:epd="http://www.iai.kit.edu/EPD/2013" epd:module="C3">4.7080487589761</epd:amount>
        <epd:amount xmlns:epd="http://www.iai.kit.edu/EPD/2013" epd:module="D">-1.43778679290098</epd:amount>
        <epd:referenceToUnitGroupDataSet xmlns:epd="http://www.iai.kit.edu/EPD/2013" refObjectId="1ebf3012-d0db-4de2-aefd-ef30cedb0be1" version="39.00.000" type="unit group data set" uri="../unitgroups/1ebf3012-d0db-4de2-aefd-ef30cedb0be1.xml">
          <common:shortDescription xml:lang="en">kg CO2 eq.</common:shortDescription>
          <common:shortDescription xml:lang="de">kg CO2 Äquiv.</common:shortDescription>
        </epd:referenceToUnitGroupDataSet>
      </common:other>
    </LCIAResult>
    <LCIAResult>
      <referenceToLCIAMethodDataSet refObjectId="06dcd26f-025f-401a-a7c1-5e457eb54637" version="39.00.000" type="LCIA method data set" uri="../lciamethods/06dcd26f-025f-401a-a7c1-5e457eb54637.xml">
        <common:shortDescription xmlns:common="http://lca.jrc.it/ILCD/Common" xmlns:epd="http://www.iai.kit.edu/EPD/2013" xml:lang="en">Ozone Depletion Potential (ODP)</common:shortDescription>
        <common:shortDescription xmlns:common="http://lca.jrc.it/ILCD/Common" xmlns:epd="http://www.iai.kit.edu/EPD/2013" xml:lang="de">Abbaupotenzial der stratosphärischen Ozonschicht (ODP)</common:shortDescription>
      </referenceToLCIAMethodDataSet>
      <common:other xmlns:common="http://lca.jrc.it/ILCD/Common">
        <epd:amount xmlns:epd="http://www.iai.kit.edu/EPD/2013" epd:module="A1-A3">1.43755756847261E-12</epd:amount>
        <epd:amount xmlns:epd="http://www.iai.kit.edu/EPD/2013" epd:module="C1">1.53760401686362E-16</epd:amount>
        <epd:amount xmlns:epd="http://www.iai.kit.edu/EPD/2013" epd:module="C2">5.91531015330711E-16</epd:amount>
        <epd:amount xmlns:epd="http://www.iai.kit.edu/EPD/2013" epd:module="C3">2.66696907324711E-14</epd:amount>
        <epd:amount xmlns:epd="http://www.iai.kit.edu/EPD/2013" epd:module="D">-2.77492678072127E-14</epd:amount>
        <epd:referenceToUnitGroupDataSet xmlns:epd="http://www.iai.kit.edu/EPD/2013" refObjectId="88054749-b0a6-47ea-a82b-dc5b29326512" version="39.00.000" type="unit group data set" uri="../unitgroups/88054749-b0a6-47ea-a82b-dc5b29326512.xml">
          <common:shortDescription xml:lang="en">kg R11 eq.</common:shortDescription>
          <common:shortDescription xml:lang="de">kg R11 Äquiv.</common:shortDescription>
        </epd:referenceToUnitGroupDataSet>
      </common:other>
    </LCIAResult>
    <LCIAResult>
      <referenceToLCIAMethodDataSet refObjectId="b4274add-93b7-4905-a5e4-2e878c4e4216" version="39.00.000" type="LCIA method data set" uri="../lciamethods/b4274add-93b7-4905-a5e4-2e878c4e4216.xml">
        <common:shortDescription xmlns:common="http://lca.jrc.it/ILCD/Common" xmlns:epd="http://www.iai.kit.edu/EPD/2013" xml:lang="en">Acidification potential (AP)</common:shortDescription>
        <common:shortDescription xmlns:common="http://lca.jrc.it/ILCD/Common" xmlns:epd="http://www.iai.kit.edu/EPD/2013" xml:lang="de">Versauerungspotential (AP)</common:shortDescription>
      </referenceToLCIAMethodDataSet>
      <common:other xmlns:common="http://lca.jrc.it/ILCD/Common">
        <epd:amount xmlns:epd="http://www.iai.kit.edu/EPD/2013" epd:module="A1-A3">0.842774495206643</epd:amount>
        <epd:amount xmlns:epd="http://www.iai.kit.edu/EPD/2013" epd:module="C1">0.00160890323799915</epd:amount>
        <epd:amount xmlns:epd="http://www.iai.kit.edu/EPD/2013" epd:module="C2">0.00360971188560073</epd:amount>
        <epd:amount xmlns:epd="http://www.iai.kit.edu/EPD/2013" epd:module="C3">0.0304471719255847</epd:amount>
        <epd:amount xmlns:epd="http://www.iai.kit.edu/EPD/2013" epd:module="D">-0.00339529197689463</epd:amount>
        <epd:referenceToUnitGroupDataSet xmlns:epd="http://www.iai.kit.edu/EPD/2013" refObjectId="bc50c624-a9bc-45b1-a9b0-e6b10d00476f" version="39.00.000" type="unit group data set" uri="../unitgroups/bc50c624-a9bc-45b1-a9b0-e6b10d00476f.xml">
          <common:shortDescription xml:lang="en">kg SO2 eq.</common:shortDescription>
          <common:shortDescription xml:lang="de">kg SO2 Äquiv.</common:shortDescription>
        </epd:referenceToUnitGroupDataSet>
      </common:other>
    </LCIAResult>
    <LCIAResult>
      <referenceToLCIAMethodDataSet refObjectId="f58827d0-b407-4ec6-be75-8b69efb98a0f" version="39.00.000" type="LCIA method data set" uri="../lciamethods/f58827d0-b407-4ec6-be75-8b69efb98a0f.xml">
        <common:shortDescription xmlns:common="http://lca.jrc.it/ILCD/Common" xmlns:epd="http://www.iai.kit.edu/EPD/2013" xml:lang="en">Eutrophication potential (EP)</common:shortDescription>
        <common:shortDescription xmlns:common="http://lca.jrc.it/ILCD/Common" xmlns:epd="http://www.iai.kit.edu/EPD/2013" xml:lang="de">Eutrophierungspotential (EP)</common:shortDescription>
      </referenceToLCIAMethodDataSet>
      <common:other xmlns:common="http://lca.jrc.it/ILCD/Common">
        <epd:amount xmlns:epd="http://www.iai.kit.edu/EPD/2013" epd:module="A1-A3">0.0646069309247934</epd:amount>
        <epd:amount xmlns:epd="http://www.iai.kit.edu/EPD/2013" epd:module="C1">0.000379613103872203</epd:amount>
        <epd:amount xmlns:epd="http://www.iai.kit.edu/EPD/2013" epd:module="C2">0.000858128311713464</epd:amount>
        <epd:amount xmlns:epd="http://www.iai.kit.edu/EPD/2013" epd:module="C3">0.00518070238166062</epd:amount>
        <epd:amount xmlns:epd="http://www.iai.kit.edu/EPD/2013" epd:module="D">-0.000660669270481837</epd:amount>
        <epd:referenceToUnitGroupDataSet xmlns:epd="http://www.iai.kit.edu/EPD/2013" refObjectId="67b5401d-873c-485f-bcf3-6ae83b918822" version="39.00.000" type="unit group data set" uri="../unitgroups/67b5401d-873c-485f-bcf3-6ae83b918822.xml">
          <common:shortDescription xml:lang="en">kg Phosphate eq.</common:shortDescription>
          <common:shortDescription xml:lang="de">kg Phosphat Äquiv.</common:shortDescription>
        </epd:referenceToUnitGroupDataSet>
      </common:other>
    </LCIAResult>
    <LCIAResult>
      <referenceToLCIAMethodDataSet refObjectId="1e84a202-dae6-42aa-9e9d-71ea48b8be00" version="39.00.000" type="LCIA method data set" uri="../lciamethods/1e84a202-dae6-42aa-9e9d-71ea48b8be00.xml">
        <common:shortDescription xmlns:common="http://lca.jrc.it/ILCD/Common" xmlns:epd="http://www.iai.kit.edu/EPD/2013" xml:lang="en">Photochemical Ozone Creation Potential (POCP)</common:shortDescription>
        <common:shortDescription xmlns:common="http://lca.jrc.it/ILCD/Common" xmlns:epd="http://www.iai.kit.edu/EPD/2013" xml:lang="de">Bildungspotenzial für troposphärisches Ozon (POCP)</common:shortDescription>
      </referenceToLCIAMethodDataSet>
      <common:other xmlns:common="http://lca.jrc.it/ILCD/Common">
        <epd:amount xmlns:epd="http://www.iai.kit.edu/EPD/2013" epd:module="A1-A3">0.0290456571565047</epd:amount>
        <epd:amount xmlns:epd="http://www.iai.kit.edu/EPD/2013" epd:module="C1">0.000158976257705422</epd:amount>
        <epd:amount xmlns:epd="http://www.iai.kit.edu/EPD/2013" epd:module="C2">-0.00117978322332452</epd:amount>
        <epd:amount xmlns:epd="http://www.iai.kit.edu/EPD/2013" epd:module="C3">0.00276311430157004</epd:amount>
        <epd:amount xmlns:epd="http://www.iai.kit.edu/EPD/2013" epd:module="D">0.000312110400498809</epd:amount>
        <epd:referenceToUnitGroupDataSet xmlns:epd="http://www.iai.kit.edu/EPD/2013" refObjectId="01c26c17-9a76-406e-8295-f17b55fd909e" version="39.00.000" type="unit group data set" uri="../unitgroups/01c26c17-9a76-406e-8295-f17b55fd909e.xml">
          <common:shortDescription xml:lang="en">kg Ethene eq.</common:shortDescription>
          <common:shortDescription xml:lang="de">kg Ethen Äquiv.</common:shortDescription>
        </epd:referenceToUnitGroupDataSet>
      </common:other>
    </LCIAResult>
    <LCIAResult>
      <referenceToLCIAMethodDataSet refObjectId="f7c73bb9-ab1a-4249-9c6d-379a0de6f67e" version="39.00.000" type="LCIA method data set" uri="../lciamethods/f7c73bb9-ab1a-4249-9c6d-379a0de6f67e.xml">
        <common:shortDescription xmlns:common="http://lca.jrc.it/ILCD/Common" xmlns:epd="http://www.iai.kit.edu/EPD/2013" xml:lang="en">Abiotic depletion potential for non fossil resources (ADPE)</common:shortDescription>
        <common:shortDescription xmlns:common="http://lca.jrc.it/ILCD/Common" xmlns:epd="http://www.iai.kit.edu/EPD/2013" xml:lang="de">Potenzial für den abiotischen Abbau nicht fossiler Ressourcen (ADPE)</common:shortDescription>
      </referenceToLCIAMethodDataSet>
      <common:other xmlns:common="http://lca.jrc.it/ILCD/Common">
        <epd:amount xmlns:epd="http://www.iai.kit.edu/EPD/2013" epd:module="A1-A3">1.97680776959441E-5</epd:amount>
        <epd:amount xmlns:epd="http://www.iai.kit.edu/EPD/2013" epd:module="C1">3.90903705372772E-8</epd:amount>
        <epd:amount xmlns:epd="http://www.iai.kit.edu/EPD/2013" epd:module="C2">1.50384405347324E-7</epd:amount>
        <epd:amount xmlns:epd="http://www.iai.kit.edu/EPD/2013" epd:module="C3">2.52983363361583E-6</epd:amount>
        <epd:amount xmlns:epd="http://www.iai.kit.edu/EPD/2013" epd:module="D">-3.19548132286828E-7</epd:amount>
        <epd:referenceToUnitGroupDataSet xmlns:epd="http://www.iai.kit.edu/EPD/2013" refObjectId="54ccd2d9-a32a-4fc2-923d-f2c8c93e89d4" version="39.00.000" type="unit group data set" uri="../unitgroups/54ccd2d9-a32a-4fc2-923d-f2c8c93e89d4.xml">
          <common:shortDescription xml:lang="en">kg Sb eq.</common:shortDescription>
          <common:shortDescription xml:lang="de">kg Sb Äquiv.</common:shortDescription>
        </epd:referenceToUnitGroupDataSet>
      </common:other>
    </LCIAResult>
    <LCIAResult>
      <referenceToLCIAMethodDataSet refObjectId="804ebcdf-309d-4098-8ed8-fdaf2f389981" version="39.00.000" type="LCIA method data set" uri="../lciamethods/804ebcdf-309d-4098-8ed8-fdaf2f389981.xml">
        <common:shortDescription xmlns:common="http://lca.jrc.it/ILCD/Common" xmlns:epd="http://www.iai.kit.edu/EPD/2013" xml:lang="en">Abiotic depletion potential for fossil resources (ADPF)</common:shortDescription>
        <common:shortDescription xmlns:common="http://lca.jrc.it/ILCD/Common" xmlns:epd="http://www.iai.kit.edu/EPD/2013" xml:lang="de">Potenzial für den abiotischen Abbau fossiler Brennstoffe (ADPF)</common:shortDescription>
      </referenceToLCIAMethodDataSet>
      <common:other xmlns:common="http://lca.jrc.it/ILCD/Common">
        <epd:amount xmlns:epd="http://www.iai.kit.edu/EPD/2013" epd:module="A1-A3">1928.96741871454</epd:amount>
        <epd:amount xmlns:epd="http://www.iai.kit.edu/EPD/2013" epd:module="C1">6.22674399295628</epd:amount>
        <epd:amount xmlns:epd="http://www.iai.kit.edu/EPD/2013" epd:module="C2">23.9548814646764</epd:amount>
        <epd:amount xmlns:epd="http://www.iai.kit.edu/EPD/2013" epd:module="C3">76.2733245253551</epd:amount>
        <epd:amount xmlns:epd="http://www.iai.kit.edu/EPD/2013" epd:module="D">-17.3830796225213</epd:amount>
        <epd:referenceToUnitGroupDataSet xmlns:epd="http://www.iai.kit.edu/EPD/2013" refObjectId="93a60a57-a3c8-11da-a746-0800200c9a66" version="03.00.000" type="unit group data set" uri="../unitgroups/93a60a57-a3c8-11da-a746-0800200c9a66.xml">
          <common:shortDescription xml:lang="en">MJ</common:shortDescription>
          <common:shortDescription xml:lang="de">MJ</common:shortDescription>
        </epd:referenceToUnitGroupDataSet>
      </common:other>
    </LCIAResult>
  </LCIAResults>
</processDataSet>