<?xml version="1.0" encoding="UTF-8" standalone="yes"?>
<processDataSet xmlns:m="http://lca.jrc.it/ILCD/LCIAMethod" xmlns:common="http://lca.jrc.it/ILCD/Common" xmlns:s="http://lca.jrc.it/ILCD/Source" xmlns:c="http://lca.jrc.it/ILCD/Contact" xmlns:f="http://lca.jrc.it/ILCD/Flow" xmlns="http://lca.jrc.it/ILCD/Process" xmlns:fp="http://lca.jrc.it/ILCD/FlowProperty" xmlns:u="http://lca.jrc.it/ILCD/UnitGroup" xmlns:epd2="http://www.indata.network/EPD/2019" xmlns:ns10="http://www.okworx.com/ILCD/Extensions/2018/Profile" version="1.1" epd2:epd-version="1.2" ns10:profile="EN_15804_A2">
    <processInformation>
        <dataSetInformation>
            <common:UUID>1d0124d4-5a30-4501-a8dd-dbddbb1f8ec7</common:UUID>
            <name>
                <baseName xml:lang="en">eLCA Luftschicht (gemäß EN 15804+A2)</baseName>
            </name>
            <classificationInformation>
                <common:classification name="oekobau.dat">
                    <common:class level="0" classId="9">Sonstige</common:class>
                    <common:class level="1" classId="9.99">eLCA Intern</common:class>
                    <common:class level="2" classId="9.99.01">eLCA Intern</common:class>
                </common:classification>
            </classificationInformation>
            <common:generalComment xml:lang="en">Dieser Datensatz dient der Modellierung von Bauteilen und geht lastenfrei in die Bilanzierung ein.</common:generalComment>
        </dataSetInformation>
        <quantitativeReference type="Reference flow(s)">
            <referenceToReferenceFlow>1</referenceToReferenceFlow>
        </quantitativeReference>
    </processInformation>
    <modellingAndValidation>
        <LCIMethodAndAllocation>
            <typeOfDataSet>EPD</typeOfDataSet>
            <common:other>
                <epd:subType xmlns:epd="http://www.iai.kit.edu/EPD/2013">generic dataset</epd:subType>
            </common:other>
        </LCIMethodAndAllocation>
        <dataSourcesTreatmentAndRepresentativeness/>
        <validation/>
        <complianceDeclarations>
            <compliance>
                <common:referenceToComplianceSystem type="source data set" refObjectId="c0016b33-8cf7-415c-ac6e-deba0d21440d" version="00.01.000">
                    <common:shortDescription xml:lang="de">EN 15804+A2</common:shortDescription>
                    <common:shortDescription xml:lang="en">EN 15804+A2</common:shortDescription>
                </common:referenceToComplianceSystem>
            </compliance>
        </complianceDeclarations>
    </modellingAndValidation>
    <administrativeInformation>
        <dataGenerator>
            <common:referenceToPersonOrEntityGeneratingTheDataSet type="contact data set" refObjectId="c59d4649-4b5c-4df1-a6f5-374923f0df63" version="00.00.002">
                <common:shortDescription xml:lang="en">Marc-William Siegert</common:shortDescription>
            </common:referenceToPersonOrEntityGeneratingTheDataSet>
        </dataGenerator>
        <dataEntryBy>
            <common:timeStamp>2021-06-24T11:00:50.291+02:00</common:timeStamp>
        </dataEntryBy>
        <publicationAndOwnership>
            <common:dataSetVersion>00.00.023</common:dataSetVersion>
            <common:referenceToPrecedingDataSetVersion type="process data set" refObjectId="41c5627a-4a1d-4e12-ac62-c1d4f1560fb9" version="00.00.017">
                <common:shortDescription xml:lang="en">eLCA Luftschicht (gemäß EN 15804+A1)</common:shortDescription>
            </common:referenceToPrecedingDataSetVersion>
            <common:referenceToOwnershipOfDataSet type="contact data set" refObjectId="f11651e0-7877-11e3-981f-0800200c9a66" version="00.01.000">
                <common:shortDescription xml:lang="en">The Federal Institute for Research on Building, Urban Affairs and Spatial Development (BBSR) within the Federal Office for Building and Regional Planning (BBR)</common:shortDescription>
                <common:shortDescription xml:lang="de">Bundesinstitut für Bau-, Stadt- und Raumforschung (BBSR) im Bundesamt für Bauwesen und Raumordnung (BBR)</common:shortDescription>
            </common:referenceToOwnershipOfDataSet>
            <common:licenseType>Free of charge for all users and uses</common:licenseType>
            <common:other>
                <ns9:referenceToPublisher xmlns:ns9="http://www.indata.network/EPD/2019" refObjectId="f11651e0-7877-11e3-981f-0800200c9a66" type="contact data set" version="00.01.000">
                    <common:shortDescription xml:lang="en">The Federal Institute for Research on Building, Urban Affairs and Spatial Development (BBSR) within the Federal Office for Building and Regional Planning (BBR)</common:shortDescription>
                    <common:shortDescription xml:lang="de">Bundesinstitut für Bau-, Stadt- und Raumforschung (BBSR) im Bundesamt für Bauwesen und Raumordnung (BBR)</common:shortDescription>
                </ns9:referenceToPublisher>
            </common:other>
        </publicationAndOwnership>
    </administrativeInformation>
    <exchanges>
        <exchange dataSetInternalID="1">
            <referenceToFlowDataSet type="flow data set" refObjectId="99d9eea1-583c-467b-9210-5e808a78586e" version="00.00.007">
                <common:shortDescription xml:lang="en">eLCA Luftschicht</common:shortDescription>
            </referenceToFlowDataSet>
            <meanAmount>1.0</meanAmount>
            <resultingAmount>1.0</resultingAmount>
        </exchange>
        <exchange dataSetInternalID="2">
            <referenceToFlowDataSet type="flow data set" refObjectId="a2b32f97-3fc7-4af2-b209-525bc6426f33" version="30.00.000">
                <common:shortDescription xml:lang="en">Components for re-use (CRU)</common:shortDescription>
                <common:shortDescription xml:lang="de">Komponenten für die Wiederverwendung (CRU)</common:shortDescription>
                <common:shortDescription xml:lang="es">Componentes para su reutilización (CRU)</common:shortDescription>
            </referenceToFlowDataSet>
            <functionType>General reminder flow</functionType>
            <exchangeDirection>Output</exchangeDirection>
            <meanAmount>0.0</meanAmount>
            <common:other>
                <epd:amount xmlns:epd="http://www.iai.kit.edu/EPD/2013" epd:module="C3">0.0</epd:amount>
                <epd:amount xmlns:epd="http://www.iai.kit.edu/EPD/2013" epd:module="A1-A3">0.0</epd:amount>
                <epd:amount xmlns:epd="http://www.iai.kit.edu/EPD/2013" epd:module="C4">0.0</epd:amount>
                <epd:referenceToUnitGroupDataSet xmlns:epd="http://www.iai.kit.edu/EPD/2013" refObjectId="ad38d542-3fe9-439d-9b95-2f5f7752acaf" type="unit group data set" uri="../unitgroups/ad38d542-3fe9-439d-9b95-2f5f7752acaf">
                    <common:shortDescription>kg</common:shortDescription>
                </epd:referenceToUnitGroupDataSet>
            </common:other>
        </exchange>
        <exchange dataSetInternalID="3">
            <referenceToFlowDataSet type="flow data set" refObjectId="4da0c987-2b76-40d6-9e9e-82a017aaaf29" version="30.00.000">
                <common:shortDescription xml:lang="en">Exported electrical energy (EEE)</common:shortDescription>
                <common:shortDescription xml:lang="de">Exportierte elektrische Energie (EEE)</common:shortDescription>
                <common:shortDescription xml:lang="es">Energía exportada electrica (EEE)</common:shortDescription>
            </referenceToFlowDataSet>
            <functionType>General reminder flow</functionType>
            <exchangeDirection>Output</exchangeDirection>
            <meanAmount>0.0</meanAmount>
            <common:other>
                <epd:amount xmlns:epd="http://www.iai.kit.edu/EPD/2013" epd:module="C3">0.0</epd:amount>
                <epd:amount xmlns:epd="http://www.iai.kit.edu/EPD/2013" epd:module="A1-A3">0.0</epd:amount>
                <epd:amount xmlns:epd="http://www.iai.kit.edu/EPD/2013" epd:module="C4">0.0</epd:amount>
                <epd:referenceToUnitGroupDataSet xmlns:epd="http://www.iai.kit.edu/EPD/2013" refObjectId="93a60a57-a3c8-11da-a746-0800200c9a66" type="unit group data set" uri="../unitgroups/93a60a57-a3c8-11da-a746-0800200c9a66">
                    <common:shortDescription>MJ</common:shortDescription>
                </epd:referenceToUnitGroupDataSet>
            </common:other>
        </exchange>
        <exchange dataSetInternalID="4">
            <referenceToFlowDataSet type="flow data set" refObjectId="98daf38a-7a79-46d3-9a37-2b7bd0955810" version="30.00.000">
                <common:shortDescription xml:lang="en">Exported thermal energy (EET)</common:shortDescription>
                <common:shortDescription xml:lang="de">Exportierte thermische Energie (EET)</common:shortDescription>
                <common:shortDescription xml:lang="es">Energía exportada termal (EET)</common:shortDescription>
            </referenceToFlowDataSet>
            <functionType>General reminder flow</functionType>
            <exchangeDirection>Output</exchangeDirection>
            <meanAmount>0.0</meanAmount>
            <common:other>
                <epd:amount xmlns:epd="http://www.iai.kit.edu/EPD/2013" epd:module="C3">0.0</epd:amount>
                <epd:amount xmlns:epd="http://www.iai.kit.edu/EPD/2013" epd:module="A1-A3">0.0</epd:amount>
                <epd:amount xmlns:epd="http://www.iai.kit.edu/EPD/2013" epd:module="C4">0.0</epd:amount>
                <epd:referenceToUnitGroupDataSet xmlns:epd="http://www.iai.kit.edu/EPD/2013" refObjectId="93a60a57-a3c8-11da-a746-0800200c9a66" type="unit group data set" uri="../unitgroups/93a60a57-a3c8-11da-a746-0800200c9a66">
                    <common:shortDescription>MJ</common:shortDescription>
                </epd:referenceToUnitGroupDataSet>
            </common:other>
        </exchange>
        <exchange dataSetInternalID="5">
            <referenceToFlowDataSet type="flow data set" refObjectId="430f9e0f-59b2-46a0-8e0d-55e0e84948fc" version="30.00.000">
                <common:shortDescription xml:lang="en">Hazardous waste disposed (HWD)</common:shortDescription>
                <common:shortDescription xml:lang="de">Gefährlicher Abfall zur Deponie (HWD)</common:shortDescription>
                <common:shortDescription xml:lang="es">Residuos peligrosos eliminados (HWD)</common:shortDescription>
            </referenceToFlowDataSet>
            <functionType>General reminder flow</functionType>
            <exchangeDirection>Output</exchangeDirection>
            <meanAmount>0.0</meanAmount>
            <common:other>
                <epd:amount xmlns:epd="http://www.iai.kit.edu/EPD/2013" epd:module="C3">0.0</epd:amount>
                <epd:amount xmlns:epd="http://www.iai.kit.edu/EPD/2013" epd:module="A1-A3">0.0</epd:amount>
                <epd:amount xmlns:epd="http://www.iai.kit.edu/EPD/2013" epd:module="C4">0.0</epd:amount>
                <epd:referenceToUnitGroupDataSet xmlns:epd="http://www.iai.kit.edu/EPD/2013" refObjectId="ad38d542-3fe9-439d-9b95-2f5f7752acaf" type="unit group data set" uri="../unitgroups/ad38d542-3fe9-439d-9b95-2f5f7752acaf">
                    <common:shortDescription>kg</common:shortDescription>
                </epd:referenceToUnitGroupDataSet>
            </common:other>
        </exchange>
        <exchange dataSetInternalID="6">
            <referenceToFlowDataSet type="flow data set" refObjectId="59a9181c-3aaf-46ee-8b13-2b3723b6e447" version="30.00.000">
                <common:shortDescription xml:lang="en">Materials for energy recovery (MER)</common:shortDescription>
                <common:shortDescription xml:lang="de">Stoffe für die Energierückgewinnung (MER)</common:shortDescription>
                <common:shortDescription xml:lang="es">Materiales para valorización energética (recuperación de energía) (MER)</common:shortDescription>
            </referenceToFlowDataSet>
            <functionType>General reminder flow</functionType>
            <exchangeDirection>Output</exchangeDirection>
            <meanAmount>0.0</meanAmount>
            <common:other>
                <epd:amount xmlns:epd="http://www.iai.kit.edu/EPD/2013" epd:module="C3">0.0</epd:amount>
                <epd:amount xmlns:epd="http://www.iai.kit.edu/EPD/2013" epd:module="A1-A3">0.0</epd:amount>
                <epd:amount xmlns:epd="http://www.iai.kit.edu/EPD/2013" epd:module="C4">0.0</epd:amount>
                <epd:referenceToUnitGroupDataSet xmlns:epd="http://www.iai.kit.edu/EPD/2013" refObjectId="ad38d542-3fe9-439d-9b95-2f5f7752acaf" type="unit group data set" uri="../unitgroups/ad38d542-3fe9-439d-9b95-2f5f7752acaf">
                    <common:shortDescription>kg</common:shortDescription>
                </epd:referenceToUnitGroupDataSet>
            </common:other>
        </exchange>
        <exchange dataSetInternalID="7">
            <referenceToFlowDataSet type="flow data set" refObjectId="d7fe48a5-4103-49c8-9aae-b0b5dfdbd6ae" version="30.00.000">
                <common:shortDescription xml:lang="en">Materials for recycling (MFR)</common:shortDescription>
                <common:shortDescription xml:lang="de">Stoffe zum Recycling (MFR)</common:shortDescription>
                <common:shortDescription xml:lang="es">Materiales para el reciclaje (MFR)</common:shortDescription>
            </referenceToFlowDataSet>
            <functionType>General reminder flow</functionType>
            <exchangeDirection>Output</exchangeDirection>
            <meanAmount>0.0</meanAmount>
            <common:other>
                <epd:amount xmlns:epd="http://www.iai.kit.edu/EPD/2013" epd:module="C3">0.0</epd:amount>
                <epd:amount xmlns:epd="http://www.iai.kit.edu/EPD/2013" epd:module="A1-A3">0.0</epd:amount>
                <epd:amount xmlns:epd="http://www.iai.kit.edu/EPD/2013" epd:module="C4">0.0</epd:amount>
                <epd:referenceToUnitGroupDataSet xmlns:epd="http://www.iai.kit.edu/EPD/2013" refObjectId="ad38d542-3fe9-439d-9b95-2f5f7752acaf" type="unit group data set" uri="../unitgroups/ad38d542-3fe9-439d-9b95-2f5f7752acaf">
                    <common:shortDescription>kg</common:shortDescription>
                </epd:referenceToUnitGroupDataSet>
            </common:other>
        </exchange>
        <exchange dataSetInternalID="8">
            <referenceToFlowDataSet type="flow data set" refObjectId="3cf952c8-f3a4-461d-8c96-96456ca62246" version="30.00.000">
                <common:shortDescription xml:lang="en">Use of net fresh water (FW)</common:shortDescription>
                <common:shortDescription xml:lang="de">Einsatz von Süßwasserressourcen (FW)</common:shortDescription>
                <common:shortDescription xml:lang="es">Uso neto de recursos de agua dulce (FW)</common:shortDescription>
            </referenceToFlowDataSet>
            <functionType>General reminder flow</functionType>
            <exchangeDirection>Input</exchangeDirection>
            <meanAmount>0.0</meanAmount>
            <common:other>
                <epd:amount xmlns:epd="http://www.iai.kit.edu/EPD/2013" epd:module="C3">0.0</epd:amount>
                <epd:amount xmlns:epd="http://www.iai.kit.edu/EPD/2013" epd:module="A1-A3">0.0</epd:amount>
                <epd:amount xmlns:epd="http://www.iai.kit.edu/EPD/2013" epd:module="C4">0.0</epd:amount>
                <epd:referenceToUnitGroupDataSet xmlns:epd="http://www.iai.kit.edu/EPD/2013" refObjectId="cd950537-0a98-4044-9ba7-9f9a68d0a504" type="unit group data set" uri="../unitgroups/cd950537-0a98-4044-9ba7-9f9a68d0a504">
                    <common:shortDescription>m3</common:shortDescription>
                </epd:referenceToUnitGroupDataSet>
            </common:other>
        </exchange>
        <exchange dataSetInternalID="9">
            <referenceToFlowDataSet type="flow data set" refObjectId="b29ef66b-e286-4afa-949f-62f1a7b4d7fa" version="30.00.000">
                <common:shortDescription xml:lang="en">Non hazardous waste dispose (NHWD)</common:shortDescription>
                <common:shortDescription xml:lang="de">Entsorgter nicht gefährlicher Abfall (NHWD)</common:shortDescription>
                <common:shortDescription xml:lang="es">Residuos no peligrosos eliminados (NHWD)</common:shortDescription>
            </referenceToFlowDataSet>
            <functionType>General reminder flow</functionType>
            <exchangeDirection>Output</exchangeDirection>
            <meanAmount>0.0</meanAmount>
            <common:other>
                <epd:amount xmlns:epd="http://www.iai.kit.edu/EPD/2013" epd:module="C3">0.0</epd:amount>
                <epd:amount xmlns:epd="http://www.iai.kit.edu/EPD/2013" epd:module="A1-A3">0.0</epd:amount>
                <epd:amount xmlns:epd="http://www.iai.kit.edu/EPD/2013" epd:module="C4">0.0</epd:amount>
                <epd:referenceToUnitGroupDataSet xmlns:epd="http://www.iai.kit.edu/EPD/2013" refObjectId="ad38d542-3fe9-439d-9b95-2f5f7752acaf" type="unit group data set" uri="../unitgroups/ad38d542-3fe9-439d-9b95-2f5f7752acaf">
                    <common:shortDescription>kg</common:shortDescription>
                </epd:referenceToUnitGroupDataSet>
            </common:other>
        </exchange>
        <exchange dataSetInternalID="10">
            <referenceToFlowDataSet type="flow data set" refObjectId="ac857178-2b45-46ec-892a-a9a4332f0372" version="30.00.000">
                <common:shortDescription xml:lang="en">Use of non renewable primary energy (PENRE)</common:shortDescription>
                <common:shortDescription xml:lang="de">Nicht-erneuerbare Primärenergie als Energieträger (PENRE)</common:shortDescription>
                <common:shortDescription xml:lang="es">Uso de energía primaria no renovable, excluyendo los recursos de energía primaria no renovable utilizada como materia prima (PENRE)</common:shortDescription>
            </referenceToFlowDataSet>
            <functionType>General reminder flow</functionType>
            <exchangeDirection>Input</exchangeDirection>
            <meanAmount>0.0</meanAmount>
            <common:other>
                <epd:amount xmlns:epd="http://www.iai.kit.edu/EPD/2013" epd:module="C3">0.0</epd:amount>
                <epd:amount xmlns:epd="http://www.iai.kit.edu/EPD/2013" epd:module="A1-A3">0.0</epd:amount>
                <epd:amount xmlns:epd="http://www.iai.kit.edu/EPD/2013" epd:module="C4">0.0</epd:amount>
                <epd:referenceToUnitGroupDataSet xmlns:epd="http://www.iai.kit.edu/EPD/2013" refObjectId="93a60a57-a3c8-11da-a746-0800200c9a66" type="unit group data set" uri="../unitgroups/93a60a57-a3c8-11da-a746-0800200c9a66">
                    <common:shortDescription>MJ</common:shortDescription>
                </epd:referenceToUnitGroupDataSet>
            </common:other>
        </exchange>
        <exchange dataSetInternalID="11">
            <referenceToFlowDataSet type="flow data set" refObjectId="1421caa0-679d-4bf4-b282-0eb850ccae27" version="30.00.000">
                <common:shortDescription xml:lang="en">Use of non renewable primary energy resources used as raw materials (PENRM)</common:shortDescription>
                <common:shortDescription xml:lang="de">Nicht-erneuerbare Primärenergie zur stofflichen Nutzung (PENRM)</common:shortDescription>
                <common:shortDescription xml:lang="es">Uso de la energía primaria no renovable utilizada como materia prima (PENRM)</common:shortDescription>
            </referenceToFlowDataSet>
            <functionType>General reminder flow</functionType>
            <exchangeDirection>Input</exchangeDirection>
            <meanAmount>0.0</meanAmount>
            <common:other>
                <epd:amount xmlns:epd="http://www.iai.kit.edu/EPD/2013" epd:module="C3">0.0</epd:amount>
                <epd:amount xmlns:epd="http://www.iai.kit.edu/EPD/2013" epd:module="A1-A3">0.0</epd:amount>
                <epd:amount xmlns:epd="http://www.iai.kit.edu/EPD/2013" epd:module="C4">0.0</epd:amount>
                <epd:referenceToUnitGroupDataSet xmlns:epd="http://www.iai.kit.edu/EPD/2013" refObjectId="93a60a57-a3c8-11da-a746-0800200c9a66" type="unit group data set" uri="../unitgroups/93a60a57-a3c8-11da-a746-0800200c9a66">
                    <common:shortDescription>MJ</common:shortDescription>
                </epd:referenceToUnitGroupDataSet>
            </common:other>
        </exchange>
        <exchange dataSetInternalID="12">
            <referenceToFlowDataSet type="flow data set" refObjectId="89def144-d39a-4287-b86f-efde453ddcb2" version="30.00.000">
                <common:shortDescription xml:lang="en">Use of non renewable secondary fuels (NRSF)</common:shortDescription>
                <common:shortDescription xml:lang="de">Nicht erneuerbare Sekundärbrennstoffe (NRSF)</common:shortDescription>
                <common:shortDescription xml:lang="es">Uso de combustibles secundarios no renovables (NRSF)</common:shortDescription>
            </referenceToFlowDataSet>
            <functionType>General reminder flow</functionType>
            <exchangeDirection>Input</exchangeDirection>
            <meanAmount>0.0</meanAmount>
            <common:other>
                <epd:amount xmlns:epd="http://www.iai.kit.edu/EPD/2013" epd:module="C3">0.0</epd:amount>
                <epd:amount xmlns:epd="http://www.iai.kit.edu/EPD/2013" epd:module="A1-A3">0.0</epd:amount>
                <epd:amount xmlns:epd="http://www.iai.kit.edu/EPD/2013" epd:module="C4">0.0</epd:amount>
                <epd:referenceToUnitGroupDataSet xmlns:epd="http://www.iai.kit.edu/EPD/2013" refObjectId="93a60a57-a3c8-11da-a746-0800200c9a66" type="unit group data set" uri="../unitgroups/93a60a57-a3c8-11da-a746-0800200c9a66">
                    <common:shortDescription>MJ</common:shortDescription>
                </epd:referenceToUnitGroupDataSet>
            </common:other>
        </exchange>
        <exchange dataSetInternalID="13">
            <referenceToFlowDataSet type="flow data set" refObjectId="3449546e-52ad-4b39-b809-9fb77cea8ff6" version="30.00.000">
                <common:shortDescription xml:lang="en">Radioactive waste disposed (RWD)</common:shortDescription>
                <common:shortDescription xml:lang="de">Entsorgter radioaktiver Abfall (RWD)</common:shortDescription>
                <common:shortDescription xml:lang="es">Residuos radiactivos eliminados (RWD)</common:shortDescription>
            </referenceToFlowDataSet>
            <functionType>General reminder flow</functionType>
            <exchangeDirection>Output</exchangeDirection>
            <meanAmount>0.0</meanAmount>
            <common:other>
                <epd:amount xmlns:epd="http://www.iai.kit.edu/EPD/2013" epd:module="C3">0.0</epd:amount>
                <epd:amount xmlns:epd="http://www.iai.kit.edu/EPD/2013" epd:module="A1-A3">0.0</epd:amount>
                <epd:amount xmlns:epd="http://www.iai.kit.edu/EPD/2013" epd:module="C4">0.0</epd:amount>
                <epd:referenceToUnitGroupDataSet xmlns:epd="http://www.iai.kit.edu/EPD/2013" refObjectId="ad38d542-3fe9-439d-9b95-2f5f7752acaf" type="unit group data set" uri="../unitgroups/ad38d542-3fe9-439d-9b95-2f5f7752acaf">
                    <common:shortDescription>kg</common:shortDescription>
                </epd:referenceToUnitGroupDataSet>
            </common:other>
        </exchange>
        <exchange dataSetInternalID="14">
            <referenceToFlowDataSet type="flow data set" refObjectId="20f32be5-0398-4288-9b6d-accddd195317" version="30.00.000">
                <common:shortDescription xml:lang="en">Use of renewable primary energy (PERE)</common:shortDescription>
                <common:shortDescription xml:lang="de">Erneuerbare Primärenergie als Energieträger (PERE)</common:shortDescription>
                <common:shortDescription xml:lang="es">Uso de energía primaria renovable excluyendo los recursos de energía primaria renovable utilizada como materia prima (PERE)</common:shortDescription>
            </referenceToFlowDataSet>
            <functionType>General reminder flow</functionType>
            <exchangeDirection>Input</exchangeDirection>
            <meanAmount>0.0</meanAmount>
            <common:other>
                <epd:amount xmlns:epd="http://www.iai.kit.edu/EPD/2013" epd:module="C3">0.0</epd:amount>
                <epd:amount xmlns:epd="http://www.iai.kit.edu/EPD/2013" epd:module="A1-A3">0.0</epd:amount>
                <epd:amount xmlns:epd="http://www.iai.kit.edu/EPD/2013" epd:module="C4">0.0</epd:amount>
                <epd:referenceToUnitGroupDataSet xmlns:epd="http://www.iai.kit.edu/EPD/2013" refObjectId="93a60a57-a3c8-11da-a746-0800200c9a66" type="unit group data set" uri="../unitgroups/93a60a57-a3c8-11da-a746-0800200c9a66">
                    <common:shortDescription>MJ</common:shortDescription>
                </epd:referenceToUnitGroupDataSet>
            </common:other>
        </exchange>
        <exchange dataSetInternalID="15">
            <referenceToFlowDataSet type="flow data set" refObjectId="fb3ec0de-548d-4508-aea5-00b73bf6f702" version="30.00.000">
                <common:shortDescription xml:lang="en">Use of renewable primary energy resources used as raw materials (PERM)</common:shortDescription>
                <common:shortDescription xml:lang="de">Erneuerbare Primärenergie zur stofflichen Nutzung (PERM)</common:shortDescription>
                <common:shortDescription xml:lang="es">Uso de energía primaria renovable utilizada como materia prima (PERM)</common:shortDescription>
            </referenceToFlowDataSet>
            <functionType>General reminder flow</functionType>
            <exchangeDirection>Input</exchangeDirection>
            <meanAmount>0.0</meanAmount>
            <common:other>
                <epd:amount xmlns:epd="http://www.iai.kit.edu/EPD/2013" epd:module="C3">0.0</epd:amount>
                <epd:amount xmlns:epd="http://www.iai.kit.edu/EPD/2013" epd:module="A1-A3">0.0</epd:amount>
                <epd:amount xmlns:epd="http://www.iai.kit.edu/EPD/2013" epd:module="C4">0.0</epd:amount>
                <epd:referenceToUnitGroupDataSet xmlns:epd="http://www.iai.kit.edu/EPD/2013" refObjectId="93a60a57-a3c8-11da-a746-0800200c9a66" type="unit group data set" uri="../unitgroups/93a60a57-a3c8-11da-a746-0800200c9a66">
                    <common:shortDescription>MJ</common:shortDescription>
                </epd:referenceToUnitGroupDataSet>
            </common:other>
        </exchange>
        <exchange dataSetInternalID="16">
            <referenceToFlowDataSet type="flow data set" refObjectId="64333088-a55f-4aa2-9a31-c10b07816787" version="30.00.000">
                <common:shortDescription xml:lang="en">Use of renewable secondary fuels (RSF)</common:shortDescription>
                <common:shortDescription xml:lang="de">Erneuerbare Sekundärbrennstoffe (RSF)</common:shortDescription>
                <common:shortDescription xml:lang="es">Uso de combustibles secundarios renovables (RSF)</common:shortDescription>
            </referenceToFlowDataSet>
            <functionType>General reminder flow</functionType>
            <exchangeDirection>Input</exchangeDirection>
            <meanAmount>0.0</meanAmount>
            <common:other>
                <epd:amount xmlns:epd="http://www.iai.kit.edu/EPD/2013" epd:module="C3">0.0</epd:amount>
                <epd:amount xmlns:epd="http://www.iai.kit.edu/EPD/2013" epd:module="A1-A3">0.0</epd:amount>
                <epd:amount xmlns:epd="http://www.iai.kit.edu/EPD/2013" epd:module="C4">0.0</epd:amount>
                <epd:referenceToUnitGroupDataSet xmlns:epd="http://www.iai.kit.edu/EPD/2013" refObjectId="93a60a57-a3c8-11da-a746-0800200c9a66" type="unit group data set" uri="../unitgroups/93a60a57-a3c8-11da-a746-0800200c9a66">
                    <common:shortDescription>MJ</common:shortDescription>
                </epd:referenceToUnitGroupDataSet>
            </common:other>
        </exchange>
        <exchange dataSetInternalID="17">
            <referenceToFlowDataSet type="flow data set" refObjectId="c6a1f35f-2d09-4f54-8dfb-97e502e1ce92" version="30.00.000">
                <common:shortDescription xml:lang="en">Use of secondary material (SM)</common:shortDescription>
                <common:shortDescription xml:lang="de">Einsatz von Sekundärstoffen (SM)</common:shortDescription>
                <common:shortDescription xml:lang="es">Uso de materiales secundarios (SM)</common:shortDescription>
            </referenceToFlowDataSet>
            <functionType>General reminder flow</functionType>
            <exchangeDirection>Input</exchangeDirection>
            <meanAmount>0.0</meanAmount>
            <common:other>
                <epd:amount xmlns:epd="http://www.iai.kit.edu/EPD/2013" epd:module="C3">0.0</epd:amount>
                <epd:amount xmlns:epd="http://www.iai.kit.edu/EPD/2013" epd:module="A1-A3">0.0</epd:amount>
                <epd:amount xmlns:epd="http://www.iai.kit.edu/EPD/2013" epd:module="C4">0.0</epd:amount>
                <epd:referenceToUnitGroupDataSet xmlns:epd="http://www.iai.kit.edu/EPD/2013" refObjectId="ad38d542-3fe9-439d-9b95-2f5f7752acaf" type="unit group data set" uri="../unitgroups/ad38d542-3fe9-439d-9b95-2f5f7752acaf">
                    <common:shortDescription>kg</common:shortDescription>
                </epd:referenceToUnitGroupDataSet>
            </common:other>
        </exchange>
        <exchange dataSetInternalID="18">
            <referenceToFlowDataSet type="flow data set" refObjectId="06159210-646b-4c8d-8583-da9b3b95a6c1" version="30.00.000">
                <common:shortDescription xml:lang="en">Total use of non renewable primary energy resource (PENRT)</common:shortDescription>
                <common:shortDescription xml:lang="de">Total nicht erneuerbare Primärenergie (PENRT)</common:shortDescription>
                <common:shortDescription xml:lang="es">Uso total de la energía primaria no renovable (energía primaria y recursos de energía primaria renovable utilizada como materia prima) (PENRT)</common:shortDescription>
            </referenceToFlowDataSet>
            <functionType>General reminder flow</functionType>
            <exchangeDirection>Input</exchangeDirection>
            <meanAmount>0.0</meanAmount>
            <common:other>
                <epd:amount xmlns:epd="http://www.iai.kit.edu/EPD/2013" epd:module="C3">0.0</epd:amount>
                <epd:amount xmlns:epd="http://www.iai.kit.edu/EPD/2013" epd:module="A1-A3">0.0</epd:amount>
                <epd:amount xmlns:epd="http://www.iai.kit.edu/EPD/2013" epd:module="C4">0.0</epd:amount>
                <epd:referenceToUnitGroupDataSet xmlns:epd="http://www.iai.kit.edu/EPD/2013" refObjectId="93a60a57-a3c8-11da-a746-0800200c9a66" type="unit group data set" uri="../unitgroups/93a60a57-a3c8-11da-a746-0800200c9a66">
                    <common:shortDescription>MJ</common:shortDescription>
                </epd:referenceToUnitGroupDataSet>
            </common:other>
        </exchange>
        <exchange dataSetInternalID="19">
            <referenceToFlowDataSet type="flow data set" refObjectId="53f97275-fa8a-4cdd-9024-65936002acd0" version="30.00.000">
                <common:shortDescription xml:lang="en">Total use of renewable primary energy resources (PERT)</common:shortDescription>
                <common:shortDescription xml:lang="de">Total erneuerbare Primärenergie (PERT)</common:shortDescription>
                <common:shortDescription xml:lang="es">Uso total de la energía primaria renovable (energía primaria y recursos de energía primaria renovable utilizada como materia prima) (PERT)</common:shortDescription>
            </referenceToFlowDataSet>
            <functionType>General reminder flow</functionType>
            <exchangeDirection>Input</exchangeDirection>
            <meanAmount>0.0</meanAmount>
            <common:other>
                <epd:amount xmlns:epd="http://www.iai.kit.edu/EPD/2013" epd:module="C3">0.0</epd:amount>
                <epd:amount xmlns:epd="http://www.iai.kit.edu/EPD/2013" epd:module="A1-A3">0.0</epd:amount>
                <epd:amount xmlns:epd="http://www.iai.kit.edu/EPD/2013" epd:module="C4">0.0</epd:amount>
                <epd:referenceToUnitGroupDataSet xmlns:epd="http://www.iai.kit.edu/EPD/2013" refObjectId="93a60a57-a3c8-11da-a746-0800200c9a66" type="unit group data set" uri="../unitgroups/93a60a57-a3c8-11da-a746-0800200c9a66">
                    <common:shortDescription>MJ</common:shortDescription>
                </epd:referenceToUnitGroupDataSet>
            </common:other>
        </exchange>
    </exchanges>
    <LCIAResults>
        <LCIAResult>
            <referenceToLCIAMethodDataSet type="LCIA method data set" refObjectId="b2ad6494-c78d-11e6-9d9d-cec0c932ce01" version="01.00.011" uri="">
                <common:shortDescription xml:lang="en">Abiotic depletion potential - non-fossil resources (ADPE)</common:shortDescription>
                <common:shortDescription xml:lang="de">Potenzial für die Verknappung abiotischer Ressourcen – nicht fossile Ressourcen (ADPE)</common:shortDescription>
            </referenceToLCIAMethodDataSet>
            <meanAmount>0.0</meanAmount>
            <common:other>
                <epd:amount xmlns:epd="http://www.iai.kit.edu/EPD/2013" epd:module="A1-A3">0.0</epd:amount>
                <epd:amount xmlns:epd="http://www.iai.kit.edu/EPD/2013" epd:module="C3">0.0</epd:amount>
                <epd:amount xmlns:epd="http://www.iai.kit.edu/EPD/2013" epd:module="C4">0.0</epd:amount>
                <epd:referenceToUnitGroupDataSet xmlns:epd="http://www.iai.kit.edu/EPD/2013" refObjectId="54ccd2d9-a32a-4fc2-923d-f2c8c93e89d4" type="unit group data set" uri="../unitgroups/54ccd2d9-a32a-4fc2-923d-f2c8c93e89d4">
                    <common:shortDescription>kg Sb-Äqv.</common:shortDescription>
                </epd:referenceToUnitGroupDataSet>
            </common:other>
        </LCIAResult>
        <LCIAResult>
            <referenceToLCIAMethodDataSet type="LCIA method data set" refObjectId="b2ad6110-c78d-11e6-9d9d-cec0c932ce01" version="01.00.011" uri="">
                <common:shortDescription xml:lang="en">Abiotic depletion potential - fossil resources (ADPF)</common:shortDescription>
                <common:shortDescription xml:lang="de">Potenzial für die Verknappung abiotischer Ressourcen – fossile Brennstoffe (ADPF)</common:shortDescription>
            </referenceToLCIAMethodDataSet>
            <meanAmount>0.0</meanAmount>
            <common:other>
                <epd:amount xmlns:epd="http://www.iai.kit.edu/EPD/2013" epd:module="A1-A3">0.0</epd:amount>
                <epd:amount xmlns:epd="http://www.iai.kit.edu/EPD/2013" epd:module="C3">0.0</epd:amount>
                <epd:amount xmlns:epd="http://www.iai.kit.edu/EPD/2013" epd:module="C4">0.0</epd:amount>
                <epd:referenceToUnitGroupDataSet xmlns:epd="http://www.iai.kit.edu/EPD/2013" refObjectId="93a60a57-a3c8-11da-a746-0800200c9a66" type="unit group data set" uri="../unitgroups/93a60a57-a3c8-11da-a746-0800200c9a66">
                    <common:shortDescription>MJ</common:shortDescription>
                </epd:referenceToUnitGroupDataSet>
            </common:other>
        </LCIAResult>
        <LCIAResult>
            <referenceToLCIAMethodDataSet type="LCIA method data set" refObjectId="b5c611c6-def3-11e6-bf01-fe55135034f3" version="01.03.010" uri="http://lca.jrc.ec.europa.eu/lcainfohub/datasets/elcd/lciamethods/f6cbd466-253f-4145-a4bb-8dae7d266e89.xml">
                <common:shortDescription xml:lang="en">Acidification potential, Accumulated Exceedance (AP)</common:shortDescription>
                <common:shortDescription xml:lang="de">Versauerungspotenzial, kumulierte Überschreitung (AP)</common:shortDescription>
            </referenceToLCIAMethodDataSet>
            <meanAmount>0.0</meanAmount>
            <common:other>
                <epd:amount xmlns:epd="http://www.iai.kit.edu/EPD/2013" epd:module="A1-A3">0.0</epd:amount>
                <epd:amount xmlns:epd="http://www.iai.kit.edu/EPD/2013" epd:module="C3">0.0</epd:amount>
                <epd:amount xmlns:epd="http://www.iai.kit.edu/EPD/2013" epd:module="C4">0.0</epd:amount>
                <epd:referenceToUnitGroupDataSet xmlns:epd="http://www.iai.kit.edu/EPD/2013" refObjectId="42e089ac-92bf-4bf2-8ca1-5fc40d18f2ed" type="unit group data set" uri="../unitgroups/42e089ac-92bf-4bf2-8ca1-5fc40d18f2ed">
                    <common:shortDescription>mol H+ eqv.</common:shortDescription>
                </epd:referenceToUnitGroupDataSet>
            </common:other>
        </LCIAResult>
        <LCIAResult>
            <referenceToLCIAMethodDataSet type="LCIA method data set" refObjectId="b53ec18f-7377-4ad3-86eb-cc3f4f276b2b" version="01.00.011" uri="http://lca.jrc.ec.europa.eu/lcainfohub/datasets/elcd/lciamethods/a4630d5b-df2f-48ae-b3f2-5e5257606d68.xml">
                <common:shortDescription xml:lang="en">Eutrophication potential - freshwater (EP-freshwater)</common:shortDescription>
                <common:shortDescription xml:lang="de">Eutrophierungspotenzial - Süßwasser (EP-freshwater)</common:shortDescription>
            </referenceToLCIAMethodDataSet>
            <meanAmount>0.0</meanAmount>
            <common:other>
                <epd:amount xmlns:epd="http://www.iai.kit.edu/EPD/2013" epd:module="A1-A3">0.0</epd:amount>
                <epd:amount xmlns:epd="http://www.iai.kit.edu/EPD/2013" epd:module="C3">0.0</epd:amount>
                <epd:amount xmlns:epd="http://www.iai.kit.edu/EPD/2013" epd:module="C4">0.0</epd:amount>
                <epd:referenceToUnitGroupDataSet xmlns:epd="http://www.iai.kit.edu/EPD/2013" refObjectId="0429039d-a61d-4590-ba67-aa4a20a810a1" type="unit group data set" uri="../unitgroups/0429039d-a61d-4590-ba67-aa4a20a810a1">
                    <common:shortDescription>kg P eqv.</common:shortDescription>
                </epd:referenceToUnitGroupDataSet>
            </common:other>
        </LCIAResult>
        <LCIAResult>
            <referenceToLCIAMethodDataSet type="LCIA method data set" refObjectId="b5c619fa-def3-11e6-bf01-fe55135034f3" version="02.00.011" uri="http://lca.jrc.ec.europa.eu/lcainfohub/datasets/elcd/lciamethods/5296e2be-060b-4e50-b033-d45f85f6ac92.xml">
                <common:shortDescription xml:lang="en">Eutrophication potential - marine (EP-marine)</common:shortDescription>
                <common:shortDescription xml:lang="de">Eutrophierungspotenzial - Salzwasser (EP-marine)</common:shortDescription>
            </referenceToLCIAMethodDataSet>
            <meanAmount>0.0</meanAmount>
            <common:other>
                <epd:amount xmlns:epd="http://www.iai.kit.edu/EPD/2013" epd:module="A1-A3">0.0</epd:amount>
                <epd:amount xmlns:epd="http://www.iai.kit.edu/EPD/2013" epd:module="C3">0.0</epd:amount>
                <epd:amount xmlns:epd="http://www.iai.kit.edu/EPD/2013" epd:module="C4">0.0</epd:amount>
                <epd:referenceToUnitGroupDataSet xmlns:epd="http://www.iai.kit.edu/EPD/2013" refObjectId="d05bb823-ecdf-4686-8c40-bf1d9257859f" type="unit group data set" uri="../unitgroups/d05bb823-ecdf-4686-8c40-bf1d9257859f">
                    <common:shortDescription>kg N eqv.</common:shortDescription>
                </epd:referenceToUnitGroupDataSet>
            </common:other>
        </LCIAResult>
        <LCIAResult>
            <referenceToLCIAMethodDataSet type="LCIA method data set" refObjectId="b5c614d2-def3-11e6-bf01-fe55135034f3" version="01.02.010" uri="http://lca.jrc.ec.europa.eu/lcainfohub/datasets/elcd/lciamethods/40054970-5936-477c-9bec-29fa23b1cb77.xml">
                <common:shortDescription xml:lang="en">Eutrophication potential - terrestrial (EP-terrestrial)</common:shortDescription>
                <common:shortDescription xml:lang="de">Eutrophierungspotenzial - Land (EP-terrestrial)</common:shortDescription>
            </referenceToLCIAMethodDataSet>
            <meanAmount>0.0</meanAmount>
            <common:other>
                <epd:amount xmlns:epd="http://www.iai.kit.edu/EPD/2013" epd:module="A1-A3">0.0</epd:amount>
                <epd:amount xmlns:epd="http://www.iai.kit.edu/EPD/2013" epd:module="C3">0.0</epd:amount>
                <epd:amount xmlns:epd="http://www.iai.kit.edu/EPD/2013" epd:module="C4">0.0</epd:amount>
                <epd:referenceToUnitGroupDataSet xmlns:epd="http://www.iai.kit.edu/EPD/2013" refObjectId="71b4d617-0ec9-4d3f-b65e-e438940c2401" type="unit group data set" uri="../unitgroups/71b4d617-0ec9-4d3f-b65e-e438940c2401">
                    <common:shortDescription>mol N eqv.</common:shortDescription>
                </epd:referenceToUnitGroupDataSet>
            </common:other>
        </LCIAResult>
        <LCIAResult>
            <referenceToLCIAMethodDataSet type="LCIA method data set" refObjectId="6a37f984-a4b3-458a-a20a-64418c145fa2" version="04.00.017" uri="">
                <common:shortDescription xml:lang="en">Global Warming Potential - total (GWP-total)</common:shortDescription>
                <common:shortDescription xml:lang="de">Globales Erwärmungspotenzial - total (GWP-total)</common:shortDescription>
            </referenceToLCIAMethodDataSet>
            <meanAmount>0.0</meanAmount>
            <common:other>
                <epd:amount xmlns:epd="http://www.iai.kit.edu/EPD/2013" epd:module="A1-A3">0.0</epd:amount>
                <epd:amount xmlns:epd="http://www.iai.kit.edu/EPD/2013" epd:module="C3">0.0</epd:amount>
                <epd:amount xmlns:epd="http://www.iai.kit.edu/EPD/2013" epd:module="C4">0.0</epd:amount>
                <epd:referenceToUnitGroupDataSet xmlns:epd="http://www.iai.kit.edu/EPD/2013" refObjectId="1ebf3012-d0db-4de2-aefd-ef30cedb0be1" type="unit group data set" uri="../unitgroups/1ebf3012-d0db-4de2-aefd-ef30cedb0be1">
                    <common:shortDescription>kg CO2-Äqv.</common:shortDescription>
                </epd:referenceToUnitGroupDataSet>
            </common:other>
        </LCIAResult>
        <LCIAResult>
            <referenceToLCIAMethodDataSet type="LCIA method data set" refObjectId="5f635281-343e-44fb-83df-1971b155e6b6" version="01.00.009" uri="">
                <common:shortDescription xml:lang="en">Global Warming Potential - fossil fuels (GWP-fossil)</common:shortDescription>
                <common:shortDescription xml:lang="de">Globales Erwärmungspotenzial - fossil (GWP-fossil)</common:shortDescription>
            </referenceToLCIAMethodDataSet>
            <meanAmount>0.0</meanAmount>
            <common:other>
                <epd:amount xmlns:epd="http://www.iai.kit.edu/EPD/2013" epd:module="A1-A3">0.0</epd:amount>
                <epd:amount xmlns:epd="http://www.iai.kit.edu/EPD/2013" epd:module="C3">0.0</epd:amount>
                <epd:amount xmlns:epd="http://www.iai.kit.edu/EPD/2013" epd:module="C4">0.0</epd:amount>
                <epd:referenceToUnitGroupDataSet xmlns:epd="http://www.iai.kit.edu/EPD/2013" refObjectId="1ebf3012-d0db-4de2-aefd-ef30cedb0be1" type="unit group data set" uri="../unitgroups/1ebf3012-d0db-4de2-aefd-ef30cedb0be1">
                    <common:shortDescription>kg CO2-Äqv.</common:shortDescription>
                </epd:referenceToUnitGroupDataSet>
            </common:other>
        </LCIAResult>
        <LCIAResult>
            <referenceToLCIAMethodDataSet type="LCIA method data set" refObjectId="2356e1ab-0185-4db5-86e5-16de51c7485c" version="01.00.006" uri="">
                <common:shortDescription xml:lang="en">Global Warming Potential - biogenic (GWP-biogenic)</common:shortDescription>
                <common:shortDescription xml:lang="de">Globales Erwärmungspotenzial - biogen (GWP-biogenic)</common:shortDescription>
            </referenceToLCIAMethodDataSet>
            <meanAmount>0.0</meanAmount>
            <common:other>
                <epd:amount xmlns:epd="http://www.iai.kit.edu/EPD/2013" epd:module="A1-A3">0.0</epd:amount>
                <epd:amount xmlns:epd="http://www.iai.kit.edu/EPD/2013" epd:module="C3">0.0</epd:amount>
                <epd:amount xmlns:epd="http://www.iai.kit.edu/EPD/2013" epd:module="C4">0.0</epd:amount>
                <epd:referenceToUnitGroupDataSet xmlns:epd="http://www.iai.kit.edu/EPD/2013" refObjectId="1ebf3012-d0db-4de2-aefd-ef30cedb0be1" type="unit group data set" uri="../unitgroups/1ebf3012-d0db-4de2-aefd-ef30cedb0be1">
                    <common:shortDescription>kg CO2-Äqv.</common:shortDescription>
                </epd:referenceToUnitGroupDataSet>
            </common:other>
        </LCIAResult>
        <LCIAResult>
            <referenceToLCIAMethodDataSet type="LCIA method data set" refObjectId="4331bbdb-978a-490d-8707-eeb047f01a55" version="01.00.006" uri="">
                <common:shortDescription xml:lang="en">Global Warming Potential - land use and land use change (GWP-luluc)</common:shortDescription>
                <common:shortDescription xml:lang="de">Globales Erwärmungspotenzial - luluc (GWP-luluc)</common:shortDescription>
            </referenceToLCIAMethodDataSet>
            <meanAmount>0.0</meanAmount>
            <common:other>
                <epd:amount xmlns:epd="http://www.iai.kit.edu/EPD/2013" epd:module="A1-A3">0.0</epd:amount>
                <epd:amount xmlns:epd="http://www.iai.kit.edu/EPD/2013" epd:module="C3">0.0</epd:amount>
                <epd:amount xmlns:epd="http://www.iai.kit.edu/EPD/2013" epd:module="C4">0.0</epd:amount>
                <epd:referenceToUnitGroupDataSet xmlns:epd="http://www.iai.kit.edu/EPD/2013" refObjectId="1ebf3012-d0db-4de2-aefd-ef30cedb0be1" type="unit group data set" uri="../unitgroups/1ebf3012-d0db-4de2-aefd-ef30cedb0be1">
                    <common:shortDescription>kg CO2-Äqv.</common:shortDescription>
                </epd:referenceToUnitGroupDataSet>
            </common:other>
        </LCIAResult>
        <LCIAResult>
            <referenceToLCIAMethodDataSet type="LCIA method data set" refObjectId="b5c629d6-def3-11e6-bf01-fe55135034f3" version="02.00.013" uri="http://lca.jrc.ec.europa.eu/lcainfohub/datasets/elcd/lciamethods/8b723200-3d8f-4eec-9e10-444edb029476.xml">
                <common:shortDescription xml:lang="en">Depletion potential of the stratospheric ozone layer (ODP)</common:shortDescription>
                <common:shortDescription xml:lang="de">Abbaupotenzial der stratosphärischen Ozonschicht (ODP)</common:shortDescription>
            </referenceToLCIAMethodDataSet>
            <meanAmount>0.0</meanAmount>
            <common:other>
                <epd:amount xmlns:epd="http://www.iai.kit.edu/EPD/2013" epd:module="A1-A3">0.0</epd:amount>
                <epd:amount xmlns:epd="http://www.iai.kit.edu/EPD/2013" epd:module="C3">0.0</epd:amount>
                <epd:amount xmlns:epd="http://www.iai.kit.edu/EPD/2013" epd:module="C4">0.0</epd:amount>
                <epd:referenceToUnitGroupDataSet xmlns:epd="http://www.iai.kit.edu/EPD/2013" refObjectId="d9e957c9-7309-4474-bf3a-7777df6c4e5b" type="unit group data set" uri="../unitgroups/d9e957c9-7309-4474-bf3a-7777df6c4e5b">
                    <common:shortDescription>kg CFC 11-Äquiv.</common:shortDescription>
                </epd:referenceToUnitGroupDataSet>
            </common:other>
        </LCIAResult>
        <LCIAResult>
            <referenceToLCIAMethodDataSet type="LCIA method data set" refObjectId="b5c610fe-def3-11e6-bf01-fe55135034f3" version="02.00.014" uri="http://lca.jrc.ec.europa.eu/lcainfohub/datasets/elcd/lciamethods/ec7836be-83eb-41da-bcda-1a6a3fe2d149.xml">
                <common:shortDescription xml:lang="en">Versauerungspotenzial, kumulierte Überschreitung (AP)</common:shortDescription>
                <common:shortDescription xml:lang="de">Bildungspotenzial für troposphärisches Ozon (POCP)</common:shortDescription>
            </referenceToLCIAMethodDataSet>
            <meanAmount>0.0</meanAmount>
            <common:other>
                <epd:amount xmlns:epd="http://www.iai.kit.edu/EPD/2013" epd:module="A1-A3">0.0</epd:amount>
                <epd:amount xmlns:epd="http://www.iai.kit.edu/EPD/2013" epd:module="C3">0.0</epd:amount>
                <epd:amount xmlns:epd="http://www.iai.kit.edu/EPD/2013" epd:module="C4">0.0</epd:amount>
                <epd:referenceToUnitGroupDataSet xmlns:epd="http://www.iai.kit.edu/EPD/2013" refObjectId="d27c25f8-fbc1-44c6-b47b-4adbae4199c6" type="unit group data set" uri="../unitgroups/d27c25f8-fbc1-44c6-b47b-4adbae4199c6">
                    <common:shortDescription>kg NMVOC eqv.</common:shortDescription>
                </epd:referenceToUnitGroupDataSet>
            </common:other>
        </LCIAResult>
        <LCIAResult>
            <referenceToLCIAMethodDataSet type="LCIA method data set" refObjectId="b2ad66ce-c78d-11e6-9d9d-cec0c932ce01" version="03.00.015" uri="">
                <common:shortDescription xml:lang="en">Water (user) deprivation potential (WDP)</common:shortDescription>
                <common:shortDescription xml:lang="de">Wasser-Entzugspotenzial (Benutzer) (WDP)</common:shortDescription>
            </referenceToLCIAMethodDataSet>
            <meanAmount>0.0</meanAmount>
            <common:other>
                <epd:amount xmlns:epd="http://www.iai.kit.edu/EPD/2013" epd:module="A1-A3">0.0</epd:amount>
                <epd:amount xmlns:epd="http://www.iai.kit.edu/EPD/2013" epd:module="C3">0.0</epd:amount>
                <epd:amount xmlns:epd="http://www.iai.kit.edu/EPD/2013" epd:module="C4">0.0</epd:amount>
                <epd:referenceToUnitGroupDataSet xmlns:epd="http://www.iai.kit.edu/EPD/2013" refObjectId="6ae2df01-888e-46c8-b17d-49fa3869b476" type="unit group data set" uri="../unitgroups/6ae2df01-888e-46c8-b17d-49fa3869b476">
                    <common:shortDescription>m3 world eqv.</common:shortDescription>
                </epd:referenceToUnitGroupDataSet>
            </common:other>
        </LCIAResult>
        <LCIAResult>
            <referenceToLCIAMethodDataSet type="LCIA method data set" refObjectId="b5c602c6-def3-11e6-bf01-fe55135034f3" version="02.00.012" uri="http://lca.jrc.ec.europa.eu/lcainfohub/datasets/elcd/lciamethods/72ce3013-f678-4c6a-935b-f4752ff8901b.xml">
                <common:shortDescription xml:lang="en">Potential incidence of disease due to PM emissions (PM)</common:shortDescription>
                <common:shortDescription xml:lang="de">Potenzielles Auftreten von Krankheiten aufgrund von Feinstaubemissionen (PM)</common:shortDescription>
            </referenceToLCIAMethodDataSet>
            <meanAmount>0.0</meanAmount>
            <common:other>
                <epd:amount xmlns:epd="http://www.iai.kit.edu/EPD/2013" epd:module="A1-A3">0.0</epd:amount>
                <epd:amount xmlns:epd="http://www.iai.kit.edu/EPD/2013" epd:module="C3">0.0</epd:amount>
                <epd:amount xmlns:epd="http://www.iai.kit.edu/EPD/2013" epd:module="C4">0.0</epd:amount>
                <epd:referenceToUnitGroupDataSet xmlns:epd="http://www.iai.kit.edu/EPD/2013" refObjectId="3883559b-648f-4afc-8ba2-0bd24f3affa3" type="unit group data set" uri="../unitgroups/3883559b-648f-4afc-8ba2-0bd24f3affa3">
                    <common:shortDescription>disease incidence</common:shortDescription>
                </epd:referenceToUnitGroupDataSet>
            </common:other>
        </LCIAResult>
        <LCIAResult>
            <referenceToLCIAMethodDataSet type="LCIA method data set" refObjectId="b5c632be-def3-11e6-bf01-fe55135034f3" version="01.00.012" uri="http://lca.jrc.ec.europa.eu/lcainfohub/datasets/elcd/lciamethods/a6f4cbc8-5388-44d6-9a67-53d05684f93e.xml">
                <common:shortDescription xml:lang="en">Potential Human exposure efficiency relative to U235 (IRP)</common:shortDescription>
                <common:shortDescription xml:lang="de">Potenzielle Wirkung durch Exposition des Menschen mit U235 (IRP)</common:shortDescription>
            </referenceToLCIAMethodDataSet>
            <meanAmount>0.0</meanAmount>
            <common:other>
                <epd:amount xmlns:epd="http://www.iai.kit.edu/EPD/2013" epd:module="A1-A3">0.0</epd:amount>
                <epd:amount xmlns:epd="http://www.iai.kit.edu/EPD/2013" epd:module="C3">0.0</epd:amount>
                <epd:amount xmlns:epd="http://www.iai.kit.edu/EPD/2013" epd:module="C4">0.0</epd:amount>
                <epd:referenceToUnitGroupDataSet xmlns:epd="http://www.iai.kit.edu/EPD/2013" refObjectId="456b05bf-1415-44a9-9993-02452f554c09" type="unit group data set" uri="../unitgroups/456b05bf-1415-44a9-9993-02452f554c09">
                    <common:shortDescription>kBq U235 eqv.</common:shortDescription>
                </epd:referenceToUnitGroupDataSet>
            </common:other>
        </LCIAResult>
        <LCIAResult>
            <referenceToLCIAMethodDataSet type="LCIA method data set" refObjectId="ee1082d1-b0f7-43ca-a1f0-21e2a4a74511" version="01.00.003" uri="http://lca.jrc.ec.europa.eu/lcainfohub/datasets/elcd/lciamethods/ee1082d1-b0f7-43ca-a1f0-21e2a4a74511.xml">
                <common:shortDescription xml:lang="en">Potential Comparative Toxic Unit for ecosystems (ETP-fw)</common:shortDescription>
                <common:shortDescription xml:lang="de">Potenzielle Toxizitätsvergleichseinheit für Ökosysteme (ETP-fw)</common:shortDescription>
            </referenceToLCIAMethodDataSet>
            <meanAmount>0.0</meanAmount>
            <common:other>
                <epd:amount xmlns:epd="http://www.iai.kit.edu/EPD/2013" epd:module="A1-A3">0.0</epd:amount>
                <epd:amount xmlns:epd="http://www.iai.kit.edu/EPD/2013" epd:module="C3">0.0</epd:amount>
                <epd:amount xmlns:epd="http://www.iai.kit.edu/EPD/2013" epd:module="C4">0.0</epd:amount>
                <epd:referenceToUnitGroupDataSet xmlns:epd="http://www.iai.kit.edu/EPD/2013" refObjectId="aa959ded-f1eb-4efb-9c5c-2d60be36b3e6" type="unit group data set" uri="../unitgroups/aa959ded-f1eb-4efb-9c5c-2d60be36b3e6">
                    <common:shortDescription>CTUe</common:shortDescription>
                </epd:referenceToUnitGroupDataSet>
            </common:other>
        </LCIAResult>
        <LCIAResult>
            <referenceToLCIAMethodDataSet type="LCIA method data set" refObjectId="2299222a-bbd8-474f-9d4f-4dd1f18aea7c" version="01.00.004" uri="http://lca.jrc.ec.europa.eu/lcainfohub/datasets/elcd/lciamethods/2299222a-bbd8-474f-9d4f-4dd1f18aea7c.xml">
                <common:shortDescription xml:lang="en">Potential Comparative Toxic Unit for humans - cancer effects (HTP-c)</common:shortDescription>
                <common:shortDescription xml:lang="de">Potenzielle Toxizitätsvergleichseinheit für den Menschen - kanzerogene Wirkung (HTP-c)</common:shortDescription>
            </referenceToLCIAMethodDataSet>
            <meanAmount>0.0</meanAmount>
            <common:other>
                <epd:amount xmlns:epd="http://www.iai.kit.edu/EPD/2013" epd:module="A1-A3">0.0</epd:amount>
                <epd:amount xmlns:epd="http://www.iai.kit.edu/EPD/2013" epd:module="C3">0.0</epd:amount>
                <epd:amount xmlns:epd="http://www.iai.kit.edu/EPD/2013" epd:module="C4">0.0</epd:amount>
                <epd:referenceToUnitGroupDataSet xmlns:epd="http://www.iai.kit.edu/EPD/2013" refObjectId="d4c9523e-2d7e-49fd-8469-998f547d3a70" type="unit group data set" uri="../unitgroups/d4c9523e-2d7e-49fd-8469-998f547d3a70">
                    <common:shortDescription>CTUh</common:shortDescription>
                </epd:referenceToUnitGroupDataSet>
            </common:other>
        </LCIAResult>
        <LCIAResult>
            <referenceToLCIAMethodDataSet type="LCIA method data set" refObjectId="3af763a5-b7a1-48c9-9cee-1f223481fcef" version="01.00.003" uri="http://lca.jrc.ec.europa.eu/lcainfohub/datasets/elcd/lciamethods/3af763a5-b7a1-48c9-9cee-1f223481fcef.xml">
                <common:shortDescription xml:lang="en">Potential Comparative Toxic Unit for humans - non-cancer effects (HTP-nc)</common:shortDescription>
                <common:shortDescription xml:lang="de">Potenzielle Toxizitätsvergleichseinheit für den Menschen - nicht kanzerogene Wirkung (HTP-nc)</common:shortDescription>
            </referenceToLCIAMethodDataSet>
            <meanAmount>0.0</meanAmount>
            <common:other>
                <epd:amount xmlns:epd="http://www.iai.kit.edu/EPD/2013" epd:module="A1-A3">0.0</epd:amount>
                <epd:amount xmlns:epd="http://www.iai.kit.edu/EPD/2013" epd:module="C3">0.0</epd:amount>
                <epd:amount xmlns:epd="http://www.iai.kit.edu/EPD/2013" epd:module="C4">0.0</epd:amount>
                <epd:referenceToUnitGroupDataSet xmlns:epd="http://www.iai.kit.edu/EPD/2013" refObjectId="d4c9523e-2d7e-49fd-8469-998f547d3a70" type="unit group data set" uri="../unitgroups/d4c9523e-2d7e-49fd-8469-998f547d3a70">
                    <common:shortDescription>CTUh</common:shortDescription>
                </epd:referenceToUnitGroupDataSet>
            </common:other>
        </LCIAResult>
        <LCIAResult>
            <referenceToLCIAMethodDataSet type="LCIA method data set" refObjectId="b2ad6890-c78d-11e6-9d9d-cec0c932ce01" version="01.00.011" uri="">
                <common:shortDescription xml:lang="en">Potential Soil quality index (SQP)</common:shortDescription>
                <common:shortDescription xml:lang="de">Potenzieller Bodenqualitätsindex (SQP)</common:shortDescription>
            </referenceToLCIAMethodDataSet>
            <meanAmount>0.0</meanAmount>
            <common:other>
                <epd:amount xmlns:epd="http://www.iai.kit.edu/EPD/2013" epd:module="A1-A3">0.0</epd:amount>
                <epd:amount xmlns:epd="http://www.iai.kit.edu/EPD/2013" epd:module="C3">0.0</epd:amount>
                <epd:amount xmlns:epd="http://www.iai.kit.edu/EPD/2013" epd:module="C4">0.0</epd:amount>
                <epd:referenceToUnitGroupDataSet xmlns:epd="http://www.iai.kit.edu/EPD/2013" refObjectId="f130951c-e67f-4f7f-8dd4-665de3974e18" type="unit group data set" uri="../unitgroups/f130951c-e67f-4f7f-8dd4-665de3974e18">
                    <common:shortDescription>dimensionless</common:shortDescription>
                </epd:referenceToUnitGroupDataSet>
            </common:other>
        </LCIAResult>
    </LCIAResults>
</processDataSet>
