<?xml version="1.0" encoding="utf-8"?>
<processDataSet xmlns:epd="http://www.iai.kit.edu/EPD/2013" xmlns:epd2="http://www.indata.network/EPD/2019" xmlns:common="http://lca.jrc.it/ILCD/Common" xsi:schemaLocation="http://lca.jrc.it/ILCD/Process ../../schemas/EPD_DataSet.xsd" epd2:epd-version="1.2" version="1.1" locations="../ILCDLocations.xml" xmlns:xsi="http://www.w3.org/2001/XMLSchema-instance" xmlns="http://lca.jrc.it/ILCD/Process">
<processInformation>
<dataSetInformation>
<common:UUID>25295071-852e-4b85-be91-f9901c0a4f7b</common:UUID>
<name>
<baseName xml:lang="de">Befestigungssysteme für vorgehängte hinterlüftete Fassaden (VHF)</baseName>
<baseName xml:lang="en">Fastening systems for rear-ventilated curtain wall facades</baseName>
<functionalUnitFlowProperties xml:lang="de" />
</name>
<classificationInformation>
<common:classification name="OEKOBAU.DAT">
<common:class level="0" classId="7">Komponenten von Fenstern und Vorhangfassaden</common:class>
<common:class level="1" classId="7.4">Beschläge</common:class>
<common:class level="2" classId="7.4.06">Befestigungen</common:class>
</common:classification>
<common:classification name="IBUCategories">
<common:class level="0">02 Bauprodukte</common:class>
<common:class level="1">Befestigungen</common:class>
<common:class level="2">Dübel aus Kunststoff und Metall</common:class>
</common:classification>
</classificationInformation>
<common:generalComment xml:lang="de">Verbindungs-, Befestigungs-, und Verankerungselemente der EJOT Baubefestigungen GmbH sind Fertigerzeugnisse, die aus einer Kunststoffhülse und einem Spreizelement aus Stahl oder Edelstahl, nur aus einem Kunststoffelement oder nur aus einem oder aus mehreren Stahlteilen bestehen. Die Deklaration gilt für alle nachfolgend genannten Verankerungs-, Verbindungs- und Befestigungselemente, die vorzugsweise im VHF-System oder in Verbindung mit dem VHF-System eingesetzt werden.</common:generalComment>
<common:generalComment xml:lang="en">Connecting, fastening and anchoring elements of EJOT Baubefestigungen GmbH are finished products consisting of a plastic sleeve and an expansion element made of steel or stainless steel, only a plastic element or only one or more steel parts.The declaration applies to all anchoring, connecting and fastening elements mentioned below, which preferably can be used in the rear-ventilated facades system or in conjunction with the rear-ventilated facades system.</common:generalComment>
</dataSetInformation>
<quantitativeReference>
<referenceToReferenceFlow>0</referenceToReferenceFlow>
</quantitativeReference>
<time>
<common:referenceYear>2021</common:referenceYear>
<common:dataSetValidUntil>2026</common:dataSetValidUntil>
<common:other>
<epd2:publicationDateOfEPD>2021-07-09</epd2:publicationDateOfEPD>
</common:other>
</time>
<geography>
<locationOfOperationSupplyOrProduction location="RER" />
</geography>
<technology>
<technologyDescriptionAndIncludedProcesses xml:lang="de">Die Dübelhülsen aus Kunststoff werden nach konventionellen Spritzgusstechniken hergestellt. Dazu wird mit einer Spritzgießmaschine der jeweilige Kunststoff in einer Spritzeinheit plastifiziert und in ein Spritzgießwerkzeug eingespritzt. Der Hohlraum (die Kavität) des Werkzeugs bestimmt die Form und die Oberflächenstruktur des fertigen Teils (hier Kunststoffdübel). Schrauben: Der weitaus größte Teil von Schrauben und Verbindungselementen wird durch spanlose Kaltumformung hergestellt. Das Kaltfließpressverfahren: Das Ausgangsmaterial wird als „Draht“ auf Spulen aufgewickelt angeliefert und in den Pressen vorgeschalteten Anlagen abgehaspelt, gerichtet und gegebenenfalls auf den gewünschten Durchmesser reduziert. Moderne Kaltfließpressen arbeiten mehrstufig, d. h. pro Hub sind mehrere Operationen hintereinander verkettet, bspw. Schraubenkopf vorformen, stauchen, abgraten und Gewindeteil reduzieren. Im nachfolgenden Prozess werden die Gewinde durch Gewindewalzmaschinen mit Flachbacken oder Roll- und Segmentwerkzeugen spanlos auf die reduzierten Gewindeteile aufgerollt. Vorzugsweise verwendet man Kaltfließpressen mit integrierter Gewinderollmaschine. Die EJOT Baubefestigungen GmbH ist gemäß ISO 9001 zertifiziert. 
Technische Daten: 
Die technischen Daten sind beispielhaft und repräsentativ für jedes der 3 durchschnittlich deklarierten Produkte gegeben. 
Deklarierte Einheit: 
Die deklarierte Einheit ist ein durchschnittliches Dübelsystem für den Einsatz in 1 m2 VHF mit einer spezifischen Länge von 120 mm, das aus vier einzelnen Systemen besteht. „Durchschnittlich“ beschreibt sämtliche produzierte Dübeltypen des Systems im Durchschnitt gemäß Produktionsanteilen gewichtet auf Basis einer Parameteranalyse gerechnet. Das bedeutet, dass ein hypothetisches Dübelsystem berechnet wird, welches das gesamte VHF-System repräsentiert. Um die deklarierte Einheit auf kg umrechnen zu können wird das Gewicht pro System angeführt.</technologyDescriptionAndIncludedProcesses>
<technologyDescriptionAndIncludedProcesses xml:lang="en">Raw materials/ Ancillary materials: The main basic materials or primary products for the anchoring and fastening products from the ventilated curtain wall system are: - Steel (mass 75-80 %) - PE HD Polyethylene high density (mass 15-17 %) - PA polyamide (3-6 %) Dyes (&lt; 1 %). The auxiliary materials and additives are contained in the plastic granulate. In the EJOT production companies, no auxiliary materials and additives are used in production. Production: The plastic anchor sleeves are manufactured using conventional injection moulding techniques. For this purpose, an injection moulding machine is used to plasticise the respective plastic in an injection unit and inject it into an injection mould.The cavity of the mould determines the shape and surface structure of the finished part (here plastic anchor). Screws: The vast majority of screws and fasteners are produced by non-cutting cold forming. The cold extrusion process: The starting material is delivered as &quot;wire&quot; wound on spools and uncoiled, straightened and, if necessary, reduced to the desired diameter in equipment upstream of the presses. Modern cold extrusion presses work in several stages, i.e. several operations are linked in succession per stroke, e.g. preforming the screw head, upsetting, deburring and reducing the threaded part. In the subsequent process, the threads are rolled onto the reduced threaded parts by thread rolling machines with flat dies or rolling and segment tools without cutting. Preferably cold extrusion presses with integrated thread rolling machines are used. Technical data: The technical data are given as examples and representative for each of the 3 average declared products. Declared unit: The declared unit is an average anchor system for use in 1 m²rear-ventilated facades with a specific length of 120 mm, consisting of four individual systems. &quot;Average&quot; describes all produced anchor types of the system on average according to production shares weighted on the basis of a parameter analysis. This means that a hypothetical anchor system is calculated, which represents the entire rear-ventilated facades system. To convert the declared unit to kg, the weight per system is given. 
Technical data: 
The technical data are given as examples and representative for each of the 3 average declared products. 
Declared unit: 
The declared unit is an average anchor system for use in 1 m² rear-ventilated facades with a specific length of 120 mm, consisting of four individual systems. &quot;Average&quot; describes all produced anchor types of the system on average according to production shares weighted on the basis of a parameter analysis. This means that a hypothetical anchor system is calculated, which represents the entire rear-ventilated facades system. To convert the declared unit to kg, the weight per system is given.</technologyDescriptionAndIncludedProcesses>
<technologicalApplicability xml:lang="de">1.) Folgende Produkte werden vorzugsweise zur Verankerung, Verbindung und / oder Befestigung von Fassadenbekleidungen verwendet:  - Dämmhalter: DH - Dämmstoffmetallhalter / -halteteller: DMH, DMT - Verbindungsmittel Schrauben: JT3 &amp; JT4 (Edelstahl A2) JT6 &amp; JT9 (Edelstahl A4) - Fassadendübel 8 mm, 10 mm und 14 mm: SDF, SDP 2.) Folgende Produkte werden vorzugsweise zur Sanierung von Außenwandelementen verwendet: - Verblendsanierdübel: VSD - Wetterschalen-Sanieranker: WSS - KERI-Anker 3.) Folgende Produkte werden zur Verankerung von tragenden Bauteilen in Beton verwendet: - EJOT Bolzenanker BA und BA-Plus</technologicalApplicability>
<technologicalApplicability xml:lang="en">1.) The following products are preferably used for anchoring, connecting and / or fastening facade cladding: -Insulation holder: DH -Insulation metal holder / stress plate: DMH, DMT -Fasteners Screws: JT3 &amp; JT4 (stainless steel A2) JT6 &amp; JT9 (stainless steel A4) -Facade anchors 8 mm, 10 mm and 14 mm: SDF, SDP 2.) The following products are preferably used for the renovation of exterior wall elements: -cavity wall repair anchor: VSD -Pre-cast panel anchor: WSS -KERI anchor 3.) The following products are used for anchoring load-bearing components in concrete: -EJOT Through Bolts BA and BA-Plus</technologicalApplicability>
</technology>
</processInformation>
<modellingAndValidation>
<LCIMethodAndAllocation>
<typeOfDataSet>EPD</typeOfDataSet>
<referenceToLCAMethodDetails type="source data set" refObjectId="934e3f45-b8d6-49f0-b8ec-606c2a3df49d">
<common:shortDescription xml:lang="de">Dübel aus Kunststoff und Metall.pdf</common:shortDescription>
</referenceToLCAMethodDetails>
<common:other>
<epd:subType xmlns="http://www.iai.kit.edu/EPD/2013">average dataset</epd:subType>
</common:other>
</LCIMethodAndAllocation>
<dataSourcesTreatmentAndRepresentativeness>
<referenceToDataSource type="source data set" refObjectId="28d74cc0-db8b-4d7e-bc44-5f6d56ce0c4a">
<common:shortDescription xml:lang="de">GaBi Database (all versions)</common:shortDescription>
</referenceToDataSource>
<referenceToDataSource type="source data set" refObjectId="0115289e-52f0-4920-bc7e-57b1c96aec8d">
<common:shortDescription xml:lang="de">GaBi database SP40 2020</common:shortDescription>
</referenceToDataSource>
<useAdviceForDataSet xml:lang="de">Gültigkeitsbereich: 
Die EPD bezieht sich auf alle Produkte im EJOT Portfolio, welche in vorgehängten, hinterlüfteten Fassadensystemen zum Einsatz kommen. Das deklarierte Produkt wird in den Werken Ciasna in Polen, Tambach in Deutschland und Dozwil in der Schweiz hergestellt. Die Datenbasis ist das Jahr 2012. Die deklarierten Ergebnisse gelten für eine Länge von 120 mm, für alle weiteren Längen können die Ergebnisse mit der angegebenen Formel extrapoliert werden. 
Systemgrenze: 
Typ der EPD: Wiege bis Werkstor - mit Optionen. Die Umweltproduktdeklaration bezieht sich auf das Produktionsstadium (Modul A1–A3), das Entsorgungsstadium (Module C1–C4) sowie Gutschriften und Lasten außerhalb der Systemgrenze (Modul D). In dem Produktionsstadium wird die Beschaffung der Rohstoffe inklusive der entsprechenden Vorketten, die notwendigen Beschaffungstransporte zu den Werken sowie die für die Produktion der Dübelsysteme werden notwendigen Energien betrachtet.Für die Werke wurde jeweils der länderspezifische Strommix modelliert. Die Materialzusammensetzung und der Energiebedarf der deklarierten Dübelsysteme wurde gemäß ihrer Produktionsanteile in jedem Werk berechnet.In der Entsorgungsphase wird der Rückbau der Dübelsysteme (Modul C1), der Transport zur Abfallbehandlung (Modul C2), die Abfallaufbereitung (Modul C3) sowie die Deponierung der Kunststoffe (Modul C4) betrachtet. Vermiedene Lasten aus dem Recycling der Metalle werden in Modul D ausgewiesen. Hierfür werden lediglich die Nettoschrottmengen betrachtet.</useAdviceForDataSet>
<useAdviceForDataSet xml:lang="en">Scope: 
The EPD refers to all products in the EJOT portfolio that are used in rear-ventilated facade systems. The declared product is manufactured in the plants Ciasna in Poland, Tambach in Germany and Dozwil in Switzerland. The data basis is the year 2012. The declared results apply to a length of 120 mm, for all other lengths the results can be extrapolated using the formula given. 
System boundary: 
Type of EPD: Cradle to factory gate - with options. The environmental product declaration refers to the production stage (module A1-A3), the disposal stage (modules C1-C4) as well as Credits and loads outside the system boundary (module D). In the production stage, the procurement of raw materials including the corresponding upstream chains, the necessary procurement transports to the plants as well as the energies required for the production of the anchor systems are considered. The country-specific electricity mix was modelled for each of the plants. The material composition and the energy demand of the declared anchor systems were calculated according to their production shares in each plant. In the disposal phase, the dismantling of the anchor systems (Module C1), the transport to waste treatment (Module C2), the waste treatment (Module C3) and the landfilling of the plastics (Module C4) are considered. Avoided burdens from the recycling of metals are reported in Module D. For this purpose, only the net scrap quantities are considered.</useAdviceForDataSet>
<common:other>
<epd2:referenceToOriginalEPD type="source data set" refObjectId="7e60edbe-24b0-4d94-88ff-7b40323690f9">
<common:shortDescription xml:lang="de">Befestigungssysteme für vorgehängte hinterlüftete Fassaden (VHF).pdf</common:shortDescription>
</epd2:referenceToOriginalEPD>
</common:other>
</dataSourcesTreatmentAndRepresentativeness>
<validation>
<review type="Accredited third party review">
<common:referenceToNameOfReviewerAndInstitution uri="../contacts/d111dbec-b024-4be5-86c5-752d6eb2cf95.xml" type="contact data set" refObjectId="d111dbec-b024-4be5-86c5-752d6eb2cf95">
<common:shortDescription xml:lang="de">Institut Bauen und Umwelt e. V.</common:shortDescription>
</common:referenceToNameOfReviewerAndInstitution>
</review>
</validation>
<complianceDeclarations>
<compliance>
<common:referenceToComplianceSystem uri="../sources/c0016b33-8cf7-415c-ac6e-deba0d21440d.xml" type="source data set" refObjectId="c0016b33-8cf7-415c-ac6e-deba0d21440d">
<common:shortDescription xml:lang="de">DIN EN 15804+A2</common:shortDescription>
</common:referenceToComplianceSystem>
</compliance>
<compliance>
<common:referenceToComplianceSystem uri="../sources/4f2eb655-6e44-4874-a95a-e28f5442cd4d.xml" type="source data set" refObjectId="4f2eb655-6e44-4874-a95a-e28f5442cd4d">
<common:shortDescription xml:lang="de">ISO 14025</common:shortDescription>
</common:referenceToComplianceSystem>
</compliance>
</complianceDeclarations>
</modellingAndValidation>
<administrativeInformation>
<common:commissionerAndGoal>
<common:referenceToCommissioner uri="../contacts/23f45e6a-f4d2-409b-afaf-7f0ca4e180d9.xml" type="contact data set" refObjectId="23f45e6a-f4d2-409b-afaf-7f0ca4e180d9">
<common:shortDescription xml:lang="de">EJOT BAUBEFESTIGUNGEN GmbH</common:shortDescription>
</common:referenceToCommissioner>
</common:commissionerAndGoal>
<dataGenerator>
<common:referenceToPersonOrEntityGeneratingTheDataSet uri="../contacts/6b539b8a-10e3-4004-8ccc-a79f169aa339.xml" type="contact data set" refObjectId="6b539b8a-10e3-4004-8ccc-a79f169aa339">
<common:shortDescription xml:lang="de">brands and values GmbH</common:shortDescription>
</common:referenceToPersonOrEntityGeneratingTheDataSet>
</dataGenerator>
<dataEntryBy>
<common:timeStamp>2021-07-09T11:17:23.604</common:timeStamp>
<common:referenceToDataSetFormat uri="../sources/a97a0155-0234-4b87-b4ce-a45da52f2a40.xml" type="source data set" refObjectId="a97a0155-0234-4b87-b4ce-a45da52f2a40">
<common:shortDescription xml:lang="de">ILCD Format</common:shortDescription>
</common:referenceToDataSetFormat>
<common:referenceToDataSetFormat uri="../sources/a29449fd-aa2f-4de8-b5d7-4b06b43c6fde.xml" type="source data set" refObjectId="a29449fd-aa2f-4de8-b5d7-4b06b43c6fde">
<common:shortDescription xml:lang="de">EPD-Datenformaterweiterungen v1.2</common:shortDescription>
<common:shortDescription xml:lang="en">EPD Data Format Extensions v1.2</common:shortDescription>
</common:referenceToDataSetFormat>
</dataEntryBy>
<publicationAndOwnership>
<common:dataSetVersion>00.01.000</common:dataSetVersion>
<common:referenceToPrecedingDataSetVersion uri="../processes/0d8e151e-6436-406e-a394-dc2da2e1aa67.xml" type="process data set" refObjectId="0d8e151e-6436-406e-a394-dc2da2e1aa67">
<common:shortDescription xml:lang="de">Befestigungssysteme für vorgehängte hinterlüftete Fassaden (VHF)</common:shortDescription>
</common:referenceToPrecedingDataSetVersion>
<common:referenceToRegistrationAuthority uri="../contacts/d111dbec-b024-4be5-86c5-752d6eb2cf95.xml" type="contact data set" refObjectId="d111dbec-b024-4be5-86c5-752d6eb2cf95">
<common:shortDescription xml:lang="de">Institut Bauen und Umwelt e. V.</common:shortDescription>
</common:referenceToRegistrationAuthority>
<common:registrationNumber>EPD-EJO-20210061-IBD1-DE</common:registrationNumber>
<common:referenceToOwnershipOfDataSet uri="../contacts/23f45e6a-f4d2-409b-afaf-7f0ca4e180d9.xml" type="contact data set" refObjectId="23f45e6a-f4d2-409b-afaf-7f0ca4e180d9">
<common:shortDescription xml:lang="de">EJOT BAUBEFESTIGUNGEN GmbH</common:shortDescription>
</common:referenceToOwnershipOfDataSet>
<common:copyright>true</common:copyright>
<common:licenseType>Free of charge for all users and uses</common:licenseType>
<common:accessRestrictions xml:lang="en">None</common:accessRestrictions>
<common:other>
<epd2:referenceToPublisher type="contact data set" refObjectId="d111dbec-b024-4be5-86c5-752d6eb2cf95" uri="../contacts/d111dbec-b024-4be5-86c5-752d6eb2cf95.xml">
<common:shortDescription xml:lang="de">Institut Bauen und Umwelt e. V.</common:shortDescription>
</epd2:referenceToPublisher>
</common:other>
</publicationAndOwnership>
</administrativeInformation>
<exchanges>
<exchange dataSetInternalID="0">
<referenceToFlowDataSet uri="../flows/f7836637-3c35-12db-6045-a19e1c62ea58.xml" type="flow data set" refObjectId="f7836637-3c35-12db-6045-a19e1c62ea58">
<common:shortDescription xml:lang="de">durchschnittliche Dübelsysteme für VHF von 120 mm Länge ()</common:shortDescription>
</referenceToFlowDataSet>
<meanAmount>1</meanAmount>
<referencesToDataSource />
</exchange>
<exchange dataSetInternalID="1">
<referenceToFlowDataSet uri="../flows/20f32be5-0398-4288-9b6d-accddd195317.xml" type="flow data set" refObjectId="20f32be5-0398-4288-9b6d-accddd195317">
<common:shortDescription xml:lang="de">Erneuerbare Primärenergie als Energieträger (PERE)</common:shortDescription>
<common:shortDescription xml:lang="en">Renewable primary energy as energy carrier (PERE)</common:shortDescription>
</referenceToFlowDataSet>
<functionType>General reminder flow</functionType>
<exchangeDirection>Input</exchangeDirection>
<common:other>
<epd:referenceToUnitGroupDataSet uri="../unitgroups/93a60a57-a3c8-11da-a746-0800200c9a66.xml" type="unit group data set" refObjectId="93a60a57-a3c8-11da-a746-0800200c9a66">
<common:shortDescription xml:lang="de">MJ</common:shortDescription>
</epd:referenceToUnitGroupDataSet>
<epd:amount epd:module="A1-A3">1.81302972800887</epd:amount>
<epd:amount epd:module="C1">0.00198</epd:amount>
<epd:amount epd:module="C2">0.000691</epd:amount>
<epd:amount epd:module="C3">0.000477</epd:amount>
<epd:amount epd:module="C4">0.00222</epd:amount>
<epd:amount epd:module="D">0.0974</epd:amount>
</common:other>
</exchange>
<exchange dataSetInternalID="2">
<referenceToFlowDataSet uri="../flows/fb3ec0de-548d-4508-aea5-00b73bf6f702.xml" type="flow data set" refObjectId="fb3ec0de-548d-4508-aea5-00b73bf6f702">
<common:shortDescription xml:lang="de">Erneuerbare Primärenergie zur stofflichen Nutzung (PERM)</common:shortDescription>
<common:shortDescription xml:lang="en">Renewable primary energy resources as material utilization (PERM)</common:shortDescription>
</referenceToFlowDataSet>
<functionType>General reminder flow</functionType>
<exchangeDirection>Input</exchangeDirection>
<common:other>
<epd:referenceToUnitGroupDataSet uri="../unitgroups/93a60a57-a3c8-11da-a746-0800200c9a66.xml" type="unit group data set" refObjectId="93a60a57-a3c8-11da-a746-0800200c9a66">
<common:shortDescription xml:lang="de">MJ</common:shortDescription>
</epd:referenceToUnitGroupDataSet>
<epd:amount epd:module="A1-A3">0.306970271991133</epd:amount>
<epd:amount epd:module="C1">0</epd:amount>
<epd:amount epd:module="C2">0</epd:amount>
<epd:amount epd:module="C3">0</epd:amount>
<epd:amount epd:module="C4">0</epd:amount>
<epd:amount epd:module="D">0</epd:amount>
</common:other>
</exchange>
<exchange dataSetInternalID="3">
<referenceToFlowDataSet uri="../flows/53f97275-fa8a-4cdd-9024-65936002acd0.xml" type="flow data set" refObjectId="53f97275-fa8a-4cdd-9024-65936002acd0">
<common:shortDescription xml:lang="de">Total erneuerbare Primärenergie (PERT)</common:shortDescription>
<common:shortDescription xml:lang="en">Total use of renewable primary energy resources (PERT)</common:shortDescription>
</referenceToFlowDataSet>
<functionType>General reminder flow</functionType>
<exchangeDirection>Input</exchangeDirection>
<common:other>
<epd:referenceToUnitGroupDataSet uri="../unitgroups/93a60a57-a3c8-11da-a746-0800200c9a66.xml" type="unit group data set" refObjectId="93a60a57-a3c8-11da-a746-0800200c9a66">
<common:shortDescription xml:lang="de">MJ</common:shortDescription>
</epd:referenceToUnitGroupDataSet>
<epd:amount epd:module="A1-A3">2.12</epd:amount>
<epd:amount epd:module="C1">0.00198</epd:amount>
<epd:amount epd:module="C2">0.000691</epd:amount>
<epd:amount epd:module="C3">0.000477</epd:amount>
<epd:amount epd:module="C4">0.00222</epd:amount>
<epd:amount epd:module="D">0.0974</epd:amount>
</common:other>
</exchange>
<exchange dataSetInternalID="4">
<referenceToFlowDataSet uri="../flows/ac857178-2b45-46ec-892a-a9a4332f0372.xml" type="flow data set" refObjectId="ac857178-2b45-46ec-892a-a9a4332f0372">
<common:shortDescription xml:lang="de">Nicht-erneuerbare Primärenergie als Energieträger (PENRE)</common:shortDescription>
<common:shortDescription xml:lang="en">Non renewable primary energy as energy carrier (PENRE)</common:shortDescription>
</referenceToFlowDataSet>
<functionType>General reminder flow</functionType>
<exchangeDirection>Input</exchangeDirection>
<common:other>
<epd:referenceToUnitGroupDataSet uri="../unitgroups/93a60a57-a3c8-11da-a746-0800200c9a66.xml" type="unit group data set" refObjectId="93a60a57-a3c8-11da-a746-0800200c9a66">
<common:shortDescription xml:lang="de">MJ</common:shortDescription>
</epd:referenceToUnitGroupDataSet>
<epd:amount epd:module="A1-A3">8.16232802671139</epd:amount>
<epd:amount epd:module="C1">0.0343</epd:amount>
<epd:amount epd:module="C2">0.012</epd:amount>
<epd:amount epd:module="C3">1.11429197328861</epd:amount>
<epd:amount epd:module="C4">0.0316</epd:amount>
<epd:amount epd:module="D">-1.26</epd:amount>
</common:other>
</exchange>
<exchange dataSetInternalID="5">
<referenceToFlowDataSet uri="../flows/1421caa0-679d-4bf4-b282-0eb850ccae27.xml" type="flow data set" refObjectId="1421caa0-679d-4bf4-b282-0eb850ccae27">
<common:shortDescription xml:lang="de">Nicht-erneuerbare Primärenergie zur stofflichen Nutzung (PENRM)</common:shortDescription>
<common:shortDescription xml:lang="en">Non renewable primary energy as material utilization (PENRM)</common:shortDescription>
</referenceToFlowDataSet>
<functionType>General reminder flow</functionType>
<exchangeDirection>Input</exchangeDirection>
<common:other>
<epd:referenceToUnitGroupDataSet uri="../unitgroups/93a60a57-a3c8-11da-a746-0800200c9a66.xml" type="unit group data set" refObjectId="93a60a57-a3c8-11da-a746-0800200c9a66">
<common:shortDescription xml:lang="de">MJ</common:shortDescription>
</epd:referenceToUnitGroupDataSet>
<epd:amount epd:module="A1-A3">1.10767197328861</epd:amount>
<epd:amount epd:module="C1">0</epd:amount>
<epd:amount epd:module="C2">0</epd:amount>
<epd:amount epd:module="C3">-1.10767197328861</epd:amount>
<epd:amount epd:module="C4">0</epd:amount>
<epd:amount epd:module="D">0</epd:amount>
</common:other>
</exchange>
<exchange dataSetInternalID="6">
<referenceToFlowDataSet uri="../flows/06159210-646b-4c8d-8583-da9b3b95a6c1.xml" type="flow data set" refObjectId="06159210-646b-4c8d-8583-da9b3b95a6c1">
<common:shortDescription xml:lang="de">Total nicht erneuerbare Primärenergie (PENRT)</common:shortDescription>
<common:shortDescription xml:lang="en">Total use of non renewable primary energy resources (PENRT)</common:shortDescription>
</referenceToFlowDataSet>
<functionType>General reminder flow</functionType>
<exchangeDirection>Input</exchangeDirection>
<common:other>
<epd:referenceToUnitGroupDataSet uri="../unitgroups/93a60a57-a3c8-11da-a746-0800200c9a66.xml" type="unit group data set" refObjectId="93a60a57-a3c8-11da-a746-0800200c9a66">
<common:shortDescription xml:lang="de">MJ</common:shortDescription>
</epd:referenceToUnitGroupDataSet>
<epd:amount epd:module="A1-A3">9.27</epd:amount>
<epd:amount epd:module="C1">0.0343</epd:amount>
<epd:amount epd:module="C2">0.012</epd:amount>
<epd:amount epd:module="C3">0.00662</epd:amount>
<epd:amount epd:module="C4">0.0316</epd:amount>
<epd:amount epd:module="D">-1.26</epd:amount>
</common:other>
</exchange>
<exchange dataSetInternalID="7">
<referenceToFlowDataSet uri="../flows/c6a1f35f-2d09-4f54-8dfb-97e502e1ce92.xml" type="flow data set" refObjectId="c6a1f35f-2d09-4f54-8dfb-97e502e1ce92">
<common:shortDescription xml:lang="de">Einsatz von Sekundärstoffen (SM)</common:shortDescription>
<common:shortDescription xml:lang="en">Use of secondary material (SM)</common:shortDescription>
</referenceToFlowDataSet>
<functionType>General reminder flow</functionType>
<exchangeDirection>Input</exchangeDirection>
<common:other>
<epd:referenceToUnitGroupDataSet uri="../unitgroups/ad38d542-3fe9-439d-9b95-2f5f7752acaf.xml" type="unit group data set" refObjectId="ad38d542-3fe9-439d-9b95-2f5f7752acaf">
<common:shortDescription xml:lang="de">kg</common:shortDescription>
</epd:referenceToUnitGroupDataSet>
<epd:amount epd:module="A1-A3">0.0544334267115518</epd:amount>
<epd:amount epd:module="C1">0</epd:amount>
<epd:amount epd:module="C2">0</epd:amount>
<epd:amount epd:module="C3">0</epd:amount>
<epd:amount epd:module="C4">0</epd:amount>
<epd:amount epd:module="D">0.0864942671125976</epd:amount>
</common:other>
</exchange>
<exchange dataSetInternalID="8">
<referenceToFlowDataSet uri="../flows/64333088-a55f-4aa2-9a31-c10b07816787.xml" type="flow data set" refObjectId="64333088-a55f-4aa2-9a31-c10b07816787">
<common:shortDescription xml:lang="de">Erneuerbare Sekundärbrennstoffe (RSF)</common:shortDescription>
<common:shortDescription xml:lang="en">Use of renewable secondary fuels (RSF)</common:shortDescription>
</referenceToFlowDataSet>
<functionType>General reminder flow</functionType>
<exchangeDirection>Input</exchangeDirection>
<common:other>
<epd:referenceToUnitGroupDataSet uri="../unitgroups/93a60a57-a3c8-11da-a746-0800200c9a66.xml" type="unit group data set" refObjectId="93a60a57-a3c8-11da-a746-0800200c9a66">
<common:shortDescription xml:lang="de">MJ</common:shortDescription>
</epd:referenceToUnitGroupDataSet>
<epd:amount epd:module="A1-A3">0</epd:amount>
<epd:amount epd:module="C1">0</epd:amount>
<epd:amount epd:module="C2">0</epd:amount>
<epd:amount epd:module="C3">0</epd:amount>
<epd:amount epd:module="C4">0</epd:amount>
<epd:amount epd:module="D">0</epd:amount>
</common:other>
</exchange>
<exchange dataSetInternalID="9">
<referenceToFlowDataSet uri="../flows/89def144-d39a-4287-b86f-efde453ddcb2.xml" type="flow data set" refObjectId="89def144-d39a-4287-b86f-efde453ddcb2">
<common:shortDescription xml:lang="de">Nicht erneuerbare Sekundärbrennstoffe (NRSF)</common:shortDescription>
<common:shortDescription xml:lang="en">Use of non renewable secondary fuels (NRSF)</common:shortDescription>
</referenceToFlowDataSet>
<functionType>General reminder flow</functionType>
<exchangeDirection>Input</exchangeDirection>
<common:other>
<epd:referenceToUnitGroupDataSet uri="../unitgroups/93a60a57-a3c8-11da-a746-0800200c9a66.xml" type="unit group data set" refObjectId="93a60a57-a3c8-11da-a746-0800200c9a66">
<common:shortDescription xml:lang="de">MJ</common:shortDescription>
</epd:referenceToUnitGroupDataSet>
<epd:amount epd:module="A1-A3">0</epd:amount>
<epd:amount epd:module="C1">0</epd:amount>
<epd:amount epd:module="C2">0</epd:amount>
<epd:amount epd:module="C3">0</epd:amount>
<epd:amount epd:module="C4">0</epd:amount>
<epd:amount epd:module="D">0</epd:amount>
</common:other>
</exchange>
<exchange dataSetInternalID="10">
<referenceToFlowDataSet uri="../flows/3cf952c8-f3a4-461d-8c96-96456ca62246.xml" type="flow data set" refObjectId="3cf952c8-f3a4-461d-8c96-96456ca62246">
<common:shortDescription xml:lang="de">Einsatz von Süßwasserressourcen (FW)</common:shortDescription>
<common:shortDescription xml:lang="en">Use of net fresh water (FW)</common:shortDescription>
</referenceToFlowDataSet>
<functionType>General reminder flow</functionType>
<exchangeDirection>Input</exchangeDirection>
<common:other>
<epd:referenceToUnitGroupDataSet uri="../unitgroups/cd950537-0a98-4044-9ba7-9f9a68d0a504.xml" type="unit group data set" refObjectId="cd950537-0a98-4044-9ba7-9f9a68d0a504">
<common:shortDescription xml:lang="de">m^3</common:shortDescription>
</epd:referenceToUnitGroupDataSet>
<epd:amount epd:module="A1-A3">0.0024</epd:amount>
<epd:amount epd:module="C1">2.3E-06</epd:amount>
<epd:amount epd:module="C2">8.05E-07</epd:amount>
<epd:amount epd:module="C3">1.86E-06</epd:amount>
<epd:amount epd:module="C4">3.88E-07</epd:amount>
<epd:amount epd:module="D">-0.000258</epd:amount>
</common:other>
</exchange>
<exchange dataSetInternalID="11">
<referenceToFlowDataSet uri="../flows/430f9e0f-59b2-46a0-8e0d-55e0e84948fc.xml" type="flow data set" refObjectId="430f9e0f-59b2-46a0-8e0d-55e0e84948fc">
<common:shortDescription xml:lang="de">Gefährlicher Abfall zur Deponie (HWD)</common:shortDescription>
<common:shortDescription xml:lang="en">Hazardous waste disposed (HWD)</common:shortDescription>
</referenceToFlowDataSet>
<functionType>General reminder flow</functionType>
<exchangeDirection>Output</exchangeDirection>
<common:other>
<epd:referenceToUnitGroupDataSet uri="../unitgroups/ad38d542-3fe9-439d-9b95-2f5f7752acaf.xml" type="unit group data set" refObjectId="ad38d542-3fe9-439d-9b95-2f5f7752acaf">
<common:shortDescription xml:lang="de">kg</common:shortDescription>
</epd:referenceToUnitGroupDataSet>
<epd:amount epd:module="A1-A3">2.03E-08</epd:amount>
<epd:amount epd:module="C1">1.59E-09</epd:amount>
<epd:amount epd:module="C2">5.54E-10</epd:amount>
<epd:amount epd:module="C3">1.73E-10</epd:amount>
<epd:amount epd:module="C4">1.15E-10</epd:amount>
<epd:amount epd:module="D">-1.61E-07</epd:amount>
</common:other>
</exchange>
<exchange dataSetInternalID="12">
<referenceToFlowDataSet uri="../flows/b29ef66b-e286-4afa-949f-62f1a7b4d7fa.xml" type="flow data set" refObjectId="b29ef66b-e286-4afa-949f-62f1a7b4d7fa">
<common:shortDescription xml:lang="de">Entsorgter nicht gefährlicher Abfall (NHWD)</common:shortDescription>
<common:shortDescription xml:lang="en">Non hazardous waste disposed (NHWD)</common:shortDescription>
</referenceToFlowDataSet>
<functionType>General reminder flow</functionType>
<exchangeDirection>Output</exchangeDirection>
<common:other>
<epd:referenceToUnitGroupDataSet uri="../unitgroups/ad38d542-3fe9-439d-9b95-2f5f7752acaf.xml" type="unit group data set" refObjectId="ad38d542-3fe9-439d-9b95-2f5f7752acaf">
<common:shortDescription xml:lang="de">kg</common:shortDescription>
</epd:referenceToUnitGroupDataSet>
<epd:amount epd:module="A1-A3">0.04</epd:amount>
<epd:amount epd:module="C1">5.44E-06</epd:amount>
<epd:amount epd:module="C2">1.9E-06</epd:amount>
<epd:amount epd:module="C3">1.79E-06</epd:amount>
<epd:amount epd:module="C4">0.0304</epd:amount>
<epd:amount epd:module="D">0.015</epd:amount>
</common:other>
</exchange>
<exchange dataSetInternalID="13">
<referenceToFlowDataSet uri="../flows/3449546e-52ad-4b39-b809-9fb77cea8ff6.xml" type="flow data set" refObjectId="3449546e-52ad-4b39-b809-9fb77cea8ff6">
<common:shortDescription xml:lang="de">Entsorgter radioaktiver Abfall (RWD)</common:shortDescription>
<common:shortDescription xml:lang="en">Radioactive waste disposed (RWD)</common:shortDescription>
</referenceToFlowDataSet>
<functionType>General reminder flow</functionType>
<exchangeDirection>Output</exchangeDirection>
<common:other>
<epd:referenceToUnitGroupDataSet uri="../unitgroups/ad38d542-3fe9-439d-9b95-2f5f7752acaf.xml" type="unit group data set" refObjectId="ad38d542-3fe9-439d-9b95-2f5f7752acaf">
<common:shortDescription xml:lang="de">kg</common:shortDescription>
</epd:referenceToUnitGroupDataSet>
<epd:amount epd:module="A1-A3">0.000235</epd:amount>
<epd:amount epd:module="C1">6.32E-08</epd:amount>
<epd:amount epd:module="C2">2.21E-08</epd:amount>
<epd:amount epd:module="C3">8.74E-08</epd:amount>
<epd:amount epd:module="C4">3.82E-07</epd:amount>
<epd:amount epd:module="D">4.46E-08</epd:amount>
</common:other>
</exchange>
<exchange dataSetInternalID="14">
<referenceToFlowDataSet uri="../flows/a2b32f97-3fc7-4af2-b209-525bc6426f33.xml" type="flow data set" refObjectId="a2b32f97-3fc7-4af2-b209-525bc6426f33">
<common:shortDescription xml:lang="de">Komponenten für die Wiederverwendung (CRU)</common:shortDescription>
<common:shortDescription xml:lang="en">Components for re-use (CRU)</common:shortDescription>
</referenceToFlowDataSet>
<functionType>General reminder flow</functionType>
<exchangeDirection>Output</exchangeDirection>
<common:other>
<epd:referenceToUnitGroupDataSet uri="../unitgroups/ad38d542-3fe9-439d-9b95-2f5f7752acaf.xml" type="unit group data set" refObjectId="ad38d542-3fe9-439d-9b95-2f5f7752acaf">
<common:shortDescription xml:lang="de">kg</common:shortDescription>
</epd:referenceToUnitGroupDataSet>
<epd:amount epd:module="A1-A3">0</epd:amount>
<epd:amount epd:module="C1">0</epd:amount>
<epd:amount epd:module="C2">0</epd:amount>
<epd:amount epd:module="C3">0</epd:amount>
<epd:amount epd:module="C4">0</epd:amount>
<epd:amount epd:module="D">0</epd:amount>
</common:other>
</exchange>
<exchange dataSetInternalID="15">
<referenceToFlowDataSet uri="../flows/d7fe48a5-4103-49c8-9aae-b0b5dfdbd6ae.xml" type="flow data set" refObjectId="d7fe48a5-4103-49c8-9aae-b0b5dfdbd6ae">
<common:shortDescription xml:lang="de">Stoffe zum Recycling (MFR)</common:shortDescription>
<common:shortDescription xml:lang="en">Materials for recycling (MFR)</common:shortDescription>
</referenceToFlowDataSet>
<functionType>General reminder flow</functionType>
<exchangeDirection>Output</exchangeDirection>
<common:other>
<epd:referenceToUnitGroupDataSet uri="../unitgroups/ad38d542-3fe9-439d-9b95-2f5f7752acaf.xml" type="unit group data set" refObjectId="ad38d542-3fe9-439d-9b95-2f5f7752acaf">
<common:shortDescription xml:lang="de">kg</common:shortDescription>
</epd:referenceToUnitGroupDataSet>
<epd:amount epd:module="A1-A3">0.00529892350733332</epd:amount>
<epd:amount epd:module="C1">0</epd:amount>
<epd:amount epd:module="C2">0</epd:amount>
<epd:amount epd:module="C3">0.098884</epd:amount>
<epd:amount epd:module="C4">0</epd:amount>
<epd:amount epd:module="D">0</epd:amount>
</common:other>
</exchange>
<exchange dataSetInternalID="16">
<referenceToFlowDataSet uri="../flows/59a9181c-3aaf-46ee-8b13-2b3723b6e447.xml" type="flow data set" refObjectId="59a9181c-3aaf-46ee-8b13-2b3723b6e447">
<common:shortDescription xml:lang="de">Stoffe für die Energierückgewinnung (MER)</common:shortDescription>
<common:shortDescription xml:lang="en">Materials for energy recovery (MER)</common:shortDescription>
</referenceToFlowDataSet>
<functionType>General reminder flow</functionType>
<exchangeDirection>Output</exchangeDirection>
<common:other>
<epd:referenceToUnitGroupDataSet uri="../unitgroups/ad38d542-3fe9-439d-9b95-2f5f7752acaf.xml" type="unit group data set" refObjectId="ad38d542-3fe9-439d-9b95-2f5f7752acaf">
<common:shortDescription xml:lang="de">kg</common:shortDescription>
</epd:referenceToUnitGroupDataSet>
<epd:amount epd:module="A1-A3">0.0128172666265383</epd:amount>
<epd:amount epd:module="C1">0</epd:amount>
<epd:amount epd:module="C2">0</epd:amount>
<epd:amount epd:module="C3">0</epd:amount>
<epd:amount epd:module="C4">0</epd:amount>
<epd:amount epd:module="D">0</epd:amount>
</common:other>
</exchange>
<exchange dataSetInternalID="17">
<referenceToFlowDataSet uri="../flows/4da0c987-2b76-40d6-9e9e-82a017aaaf29.xml" type="flow data set" refObjectId="4da0c987-2b76-40d6-9e9e-82a017aaaf29">
<common:shortDescription xml:lang="de">Exportierte elektrische Energie (EEE)</common:shortDescription>
<common:shortDescription xml:lang="en">Exported electrical energy (EEE)</common:shortDescription>
</referenceToFlowDataSet>
<functionType>General reminder flow</functionType>
<exchangeDirection>Output</exchangeDirection>
<common:other>
<epd:referenceToUnitGroupDataSet uri="../unitgroups/93a60a57-a3c8-11da-a746-0800200c9a66.xml" type="unit group data set" refObjectId="93a60a57-a3c8-11da-a746-0800200c9a66">
<common:shortDescription xml:lang="de">MJ</common:shortDescription>
</epd:referenceToUnitGroupDataSet>
<epd:amount epd:module="A1-A3">0</epd:amount>
<epd:amount epd:module="C1">0</epd:amount>
<epd:amount epd:module="C2">0</epd:amount>
<epd:amount epd:module="C3">0</epd:amount>
<epd:amount epd:module="C4">0</epd:amount>
<epd:amount epd:module="D">0</epd:amount>
</common:other>
</exchange>
<exchange dataSetInternalID="18">
<referenceToFlowDataSet uri="../flows/98daf38a-7a79-46d3-9a37-2b7bd0955810.xml" type="flow data set" refObjectId="98daf38a-7a79-46d3-9a37-2b7bd0955810">
<common:shortDescription xml:lang="de">Exportierte thermische Energie (EET)</common:shortDescription>
<common:shortDescription xml:lang="en">Exported thermal energy (EET)</common:shortDescription>
</referenceToFlowDataSet>
<functionType>General reminder flow</functionType>
<exchangeDirection>Output</exchangeDirection>
<common:other>
<epd:referenceToUnitGroupDataSet uri="../unitgroups/93a60a57-a3c8-11da-a746-0800200c9a66.xml" type="unit group data set" refObjectId="93a60a57-a3c8-11da-a746-0800200c9a66">
<common:shortDescription xml:lang="de">MJ</common:shortDescription>
</epd:referenceToUnitGroupDataSet>
<epd:amount epd:module="A1-A3">0</epd:amount>
<epd:amount epd:module="C1">0</epd:amount>
<epd:amount epd:module="C2">0</epd:amount>
<epd:amount epd:module="C3">0</epd:amount>
<epd:amount epd:module="C4">0</epd:amount>
<epd:amount epd:module="D">0</epd:amount>
</common:other>
</exchange>
</exchanges>
<LCIAResults>
<LCIAResult>
<referenceToLCIAMethodDataSet uri="../lciamethods/6a37f984-a4b3-458a-a20a-64418c145fa2.xml" type="LCIA method data set" refObjectId="6a37f984-a4b3-458a-a20a-64418c145fa2">
<common:shortDescription xml:lang="de">Globales Erwärmungspotenzial total (GWP-total)</common:shortDescription>
<common:shortDescription xml:lang="en">Global Warming Potential total (GWP-total)</common:shortDescription>
</referenceToLCIAMethodDataSet>
<common:other>
<epd:referenceToUnitGroupDataSet uri="../unitgroups/1ebf3012-d0db-4de2-aefd-ef30cedb0be1.xml" type="unit group data set" refObjectId="1ebf3012-d0db-4de2-aefd-ef30cedb0be1">
<common:shortDescription xml:lang="de">kg CO_(2)-Äq.</common:shortDescription>
</epd:referenceToUnitGroupDataSet>
<epd:amount epd:module="A1-A3">0.671</epd:amount>
<epd:amount epd:module="C1">0.00256</epd:amount>
<epd:amount epd:module="C2">0.000895</epd:amount>
<epd:amount epd:module="C3">0.000341</epd:amount>
<epd:amount epd:module="C4">0.00221</epd:amount>
<epd:amount epd:module="D">-0.146</epd:amount>
</common:other>
</LCIAResult>
<LCIAResult>
<referenceToLCIAMethodDataSet uri="../lciamethods/5f635281-343e-44fb-83df-1971b155e6b6.xml" type="LCIA method data set" refObjectId="5f635281-343e-44fb-83df-1971b155e6b6">
<common:shortDescription xml:lang="de">Globales Erwärmungspotenzial fossil (GWP-fossil)</common:shortDescription>
<common:shortDescription xml:lang="en">Global Warming Potential fossil fuels (GWP-fossil)</common:shortDescription>
</referenceToLCIAMethodDataSet>
<common:other>
<epd:referenceToUnitGroupDataSet uri="../unitgroups/1ebf3012-d0db-4de2-aefd-ef30cedb0be1.xml" type="unit group data set" refObjectId="1ebf3012-d0db-4de2-aefd-ef30cedb0be1">
<common:shortDescription xml:lang="de">kg CO_(2)-Äq.</common:shortDescription>
</epd:referenceToUnitGroupDataSet>
<epd:amount epd:module="A1-A3">0.67</epd:amount>
<epd:amount epd:module="C1">0.00254</epd:amount>
<epd:amount epd:module="C2">0.000888</epd:amount>
<epd:amount epd:module="C3">0.000338</epd:amount>
<epd:amount epd:module="C4">0.00221</epd:amount>
<epd:amount epd:module="D">-0.146</epd:amount>
</common:other>
</LCIAResult>
<LCIAResult>
<referenceToLCIAMethodDataSet uri="../lciamethods/2356e1ab-0185-4db5-86e5-16de51c7485c.xml" type="LCIA method data set" refObjectId="2356e1ab-0185-4db5-86e5-16de51c7485c">
<common:shortDescription xml:lang="de">Globales Erwärmungspotenzial biogen (GWP-biogenic)</common:shortDescription>
<common:shortDescription xml:lang="en">Global Warming Potential biogenic (GWP-biogenic)</common:shortDescription>
</referenceToLCIAMethodDataSet>
<common:other>
<epd:referenceToUnitGroupDataSet uri="../unitgroups/1ebf3012-d0db-4de2-aefd-ef30cedb0be1.xml" type="unit group data set" refObjectId="1ebf3012-d0db-4de2-aefd-ef30cedb0be1">
<common:shortDescription xml:lang="de">kg CO_(2)-Äq.</common:shortDescription>
</epd:referenceToUnitGroupDataSet>
<epd:amount epd:module="A1-A3">0</epd:amount>
<epd:amount epd:module="C1">0</epd:amount>
<epd:amount epd:module="C2">0</epd:amount>
<epd:amount epd:module="C3">0</epd:amount>
<epd:amount epd:module="C4">0</epd:amount>
<epd:amount epd:module="D">0</epd:amount>
</common:other>
</LCIAResult>
<LCIAResult>
<referenceToLCIAMethodDataSet uri="../lciamethods/4331bbdb-978a-490d-8707-eeb047f01a55.xml" type="LCIA method data set" refObjectId="4331bbdb-978a-490d-8707-eeb047f01a55">
<common:shortDescription xml:lang="de">Globales Erwärmungspotenzial luluc (GWP-luluc)</common:shortDescription>
<common:shortDescription xml:lang="en">Global Warming Potential luluc (GWP-luluc)</common:shortDescription>
</referenceToLCIAMethodDataSet>
<common:other>
<epd:referenceToUnitGroupDataSet uri="../unitgroups/1ebf3012-d0db-4de2-aefd-ef30cedb0be1.xml" type="unit group data set" refObjectId="1ebf3012-d0db-4de2-aefd-ef30cedb0be1">
<common:shortDescription xml:lang="de">kg CO_(2)-Äq.</common:shortDescription>
</epd:referenceToUnitGroupDataSet>
<epd:amount epd:module="A1-A3">0.000548</epd:amount>
<epd:amount epd:module="C1">2.07E-05</epd:amount>
<epd:amount epd:module="C2">7.25E-06</epd:amount>
<epd:amount epd:module="C3">2.31E-06</epd:amount>
<epd:amount epd:module="C4">1.79E-06</epd:amount>
<epd:amount epd:module="D">4.17E-06</epd:amount>
</common:other>
</LCIAResult>
<LCIAResult>
<referenceToLCIAMethodDataSet uri="../lciamethods/b5c629d6-def3-11e6-bf01-fe55135034f3.xml" type="LCIA method data set" refObjectId="b5c629d6-def3-11e6-bf01-fe55135034f3">
<common:shortDescription xml:lang="de">Abbau Potential der stratosphärischen Ozonschicht (ODP)</common:shortDescription>
<common:shortDescription xml:lang="en">Depletion potential of the stratospheric ozone layer (ODP)</common:shortDescription>
</referenceToLCIAMethodDataSet>
<common:other>
<epd:referenceToUnitGroupDataSet uri="../unitgroups/d9e957c9-7309-4474-bf3a-7777df6c4e5b.xml" type="unit group data set" refObjectId="d9e957c9-7309-4474-bf3a-7777df6c4e5b">
<common:shortDescription xml:lang="de">kg CFC11-Äq.</common:shortDescription>
</epd:referenceToUnitGroupDataSet>
<epd:amount epd:module="A1-A3">3.87E-11</epd:amount>
<epd:amount epd:module="C1">4.7E-19</epd:amount>
<epd:amount epd:module="C2">1.64E-19</epd:amount>
<epd:amount epd:module="C3">8.21E-19</epd:amount>
<epd:amount epd:module="C4">5E-18</epd:amount>
<epd:amount epd:module="D">3.19E-16</epd:amount>
</common:other>
</LCIAResult>
<LCIAResult>
<referenceToLCIAMethodDataSet uri="../lciamethods/b5c611c6-def3-11e6-bf01-fe55135034f3.xml" type="LCIA method data set" refObjectId="b5c611c6-def3-11e6-bf01-fe55135034f3">
<common:shortDescription xml:lang="de">Versauerungspotenzial von Boden und Wasser (AP)</common:shortDescription>
<common:shortDescription xml:lang="en">Acidification potential of land and water (AP)</common:shortDescription>
</referenceToLCIAMethodDataSet>
<common:other>
<epd:referenceToUnitGroupDataSet uri="../unitgroups/42e089ac-92bf-4bf2-8ca1-5fc40d18f2ed.xml" type="unit group data set" refObjectId="42e089ac-92bf-4bf2-8ca1-5fc40d18f2ed">
<common:shortDescription xml:lang="de">mol H^(+)-Äq.</common:shortDescription>
</epd:referenceToUnitGroupDataSet>
<epd:amount epd:module="A1-A3">0.00243</epd:amount>
<epd:amount epd:module="C1">1.29E-05</epd:amount>
<epd:amount epd:module="C2">5.46E-06</epd:amount>
<epd:amount epd:module="C3">3.32E-06</epd:amount>
<epd:amount epd:module="C4">6.68E-06</epd:amount>
<epd:amount epd:module="D">-0.000325</epd:amount>
</common:other>
</LCIAResult>
<LCIAResult>
<referenceToLCIAMethodDataSet uri="../lciamethods/b53ec18f-7377-4ad3-86eb-cc3f4f276b2b.xml" type="LCIA method data set" refObjectId="b53ec18f-7377-4ad3-86eb-cc3f4f276b2b">
<common:shortDescription xml:lang="de">Eutrophierungspotenzial Süßwasser (EP-freshwater)</common:shortDescription>
<common:shortDescription xml:lang="en">Eutrophication potential aquatic freshwater (EP-freshwater)</common:shortDescription>
</referenceToLCIAMethodDataSet>
<common:other>
<epd:referenceToUnitGroupDataSet uri="../unitgroups/0429039d-a61d-4590-ba67-aa4a20a810a1.xml" type="unit group data set" refObjectId="0429039d-a61d-4590-ba67-aa4a20a810a1">
<common:shortDescription xml:lang="de">kg PO_(4)-Äq.</common:shortDescription>
</epd:referenceToUnitGroupDataSet>
<epd:amount epd:module="A1-A3">1.76E-06</epd:amount>
<epd:amount epd:module="C1">7.8E-09</epd:amount>
<epd:amount epd:module="C2">2.73E-09</epd:amount>
<epd:amount epd:module="C3">9.87E-10</epd:amount>
<epd:amount epd:module="C4">4.03E-07</epd:amount>
<epd:amount epd:module="D">-8.27E-08</epd:amount>
</common:other>
</LCIAResult>
<LCIAResult>
<referenceToLCIAMethodDataSet uri="../lciamethods/b5c619fa-def3-11e6-bf01-fe55135034f3.xml" type="LCIA method data set" refObjectId="b5c619fa-def3-11e6-bf01-fe55135034f3">
<common:shortDescription xml:lang="de">Eutrophierungspotenzial Salzwasser (EP-marine)</common:shortDescription>
<common:shortDescription xml:lang="en">Eutrophication potential aquatic marine (EP-marine)</common:shortDescription>
</referenceToLCIAMethodDataSet>
<common:other>
<epd:referenceToUnitGroupDataSet uri="../unitgroups/d05bb823-ecdf-4686-8c40-bf1d9257859f.xml" type="unit group data set" refObjectId="d05bb823-ecdf-4686-8c40-bf1d9257859f">
<common:shortDescription xml:lang="de">kg N-Äq.</common:shortDescription>
</epd:referenceToUnitGroupDataSet>
<epd:amount epd:module="A1-A3">0.000464</epd:amount>
<epd:amount epd:module="C1">6.14E-06</epd:amount>
<epd:amount epd:module="C2">2.64E-06</epd:amount>
<epd:amount epd:module="C3">1.61E-06</epd:amount>
<epd:amount epd:module="C4">1.48E-06</epd:amount>
<epd:amount epd:module="D">-5.93E-05</epd:amount>
</common:other>
</LCIAResult>
<LCIAResult>
<referenceToLCIAMethodDataSet uri="../lciamethods/b5c614d2-def3-11e6-bf01-fe55135034f3.xml" type="LCIA method data set" refObjectId="b5c614d2-def3-11e6-bf01-fe55135034f3">
<common:shortDescription xml:lang="de">Eutrophierungspotenzial Land (EP-terrestrial)</common:shortDescription>
<common:shortDescription xml:lang="en">Eutrophication potential terrestrial (EP-terrestrial)</common:shortDescription>
</referenceToLCIAMethodDataSet>
<common:other>
<epd:referenceToUnitGroupDataSet uri="../unitgroups/71b4d617-0ec9-4d3f-b65e-e438940c2401.xml" type="unit group data set" refObjectId="71b4d617-0ec9-4d3f-b65e-e438940c2401">
<common:shortDescription xml:lang="de">mol N-Äq.</common:shortDescription>
</epd:referenceToUnitGroupDataSet>
<epd:amount epd:module="A1-A3">0.00482</epd:amount>
<epd:amount epd:module="C1">6.82E-05</epd:amount>
<epd:amount epd:module="C2">2.93E-05</epd:amount>
<epd:amount epd:module="C3">1.77E-05</epd:amount>
<epd:amount epd:module="C4">1.62E-05</epd:amount>
<epd:amount epd:module="D">-0.000601</epd:amount>
</common:other>
</LCIAResult>
<LCIAResult>
<referenceToLCIAMethodDataSet uri="../lciamethods/b5c610fe-def3-11e6-bf01-fe55135034f3.xml" type="LCIA method data set" refObjectId="b5c610fe-def3-11e6-bf01-fe55135034f3">
<common:shortDescription xml:lang="de">Bildungspotential für troposphärisches Ozon (POCP)</common:shortDescription>
<common:shortDescription xml:lang="en">Formation potential of tropospheric ozone photochemical oxidants (POCP)</common:shortDescription>
</referenceToLCIAMethodDataSet>
<common:other>
<epd:referenceToUnitGroupDataSet uri="../unitgroups/d27c25f8-fbc1-44c6-b47b-4adbae4199c6.xml" type="unit group data set" refObjectId="d27c25f8-fbc1-44c6-b47b-4adbae4199c6">
<common:shortDescription xml:lang="de">kg NMVOC-Äq.</common:shortDescription>
</epd:referenceToUnitGroupDataSet>
<epd:amount epd:module="A1-A3">0.00136</epd:amount>
<epd:amount epd:module="C1">1.25E-05</epd:amount>
<epd:amount epd:module="C2">5.1E-06</epd:amount>
<epd:amount epd:module="C3">4.7E-06</epd:amount>
<epd:amount epd:module="C4">4.82E-06</epd:amount>
<epd:amount epd:module="D">-0.000245</epd:amount>
</common:other>
</LCIAResult>
<LCIAResult>
<referenceToLCIAMethodDataSet uri="../lciamethods/b2ad6494-c78d-11e6-9d9d-cec0c932ce01.xml" type="LCIA method data set" refObjectId="b2ad6494-c78d-11e6-9d9d-cec0c932ce01">
<common:shortDescription xml:lang="de">Potenzial für den abiotischen Abbau nicht fossiler Ressourcen (ADPE)</common:shortDescription>
<common:shortDescription xml:lang="en">Abiotic depletion potential for non fossil resources (ADPE)</common:shortDescription>
</referenceToLCIAMethodDataSet>
<common:other>
<epd:referenceToUnitGroupDataSet uri="../unitgroups/54ccd2d9-a32a-4fc2-923d-f2c8c93e89d4.xml" type="unit group data set" refObjectId="54ccd2d9-a32a-4fc2-923d-f2c8c93e89d4">
<common:shortDescription xml:lang="de">kg Sb-Äq.</common:shortDescription>
</epd:referenceToUnitGroupDataSet>
<epd:amount epd:module="A1-A3">9.11E-05</epd:amount>
<epd:amount epd:module="C1">2.07E-10</epd:amount>
<epd:amount epd:module="C2">7.24E-11</epd:amount>
<epd:amount epd:module="C3">3.71E-10</epd:amount>
<epd:amount epd:module="C4">1.49E-10</epd:amount>
<epd:amount epd:module="D">-2.37E-06</epd:amount>
</common:other>
</LCIAResult>
<LCIAResult>
<referenceToLCIAMethodDataSet uri="../lciamethods/b2ad6110-c78d-11e6-9d9d-cec0c932ce01.xml" type="LCIA method data set" refObjectId="b2ad6110-c78d-11e6-9d9d-cec0c932ce01">
<common:shortDescription xml:lang="de">Potenzial für den abiotischen Abbau fossiler Brennstoffe (ADPF)</common:shortDescription>
<common:shortDescription xml:lang="en">Abiotic depletion potential for fossil resources (ADPF)</common:shortDescription>
</referenceToLCIAMethodDataSet>
<common:other>
<epd:referenceToUnitGroupDataSet uri="../unitgroups/93a60a57-a3c8-11da-a746-0800200c9a66.xml" type="unit group data set" refObjectId="93a60a57-a3c8-11da-a746-0800200c9a66">
<common:shortDescription xml:lang="de">MJ</common:shortDescription>
</epd:referenceToUnitGroupDataSet>
<epd:amount epd:module="A1-A3">9.26</epd:amount>
<epd:amount epd:module="C1">0.0342</epd:amount>
<epd:amount epd:module="C2">0.0119</epd:amount>
<epd:amount epd:module="C3">0.00661</epd:amount>
<epd:amount epd:module="C4">0.0316</epd:amount>
<epd:amount epd:module="D">-1.26</epd:amount>
</common:other>
</LCIAResult>
<LCIAResult>
<referenceToLCIAMethodDataSet uri="../lciamethods/b2ad66ce-c78d-11e6-9d9d-cec0c932ce01.xml" type="LCIA method data set" refObjectId="b2ad66ce-c78d-11e6-9d9d-cec0c932ce01">
<common:shortDescription xml:lang="de">Wassernutzung (WDP)</common:shortDescription>
<common:shortDescription xml:lang="en">Water use (WDP)</common:shortDescription>
</referenceToLCIAMethodDataSet>
<common:other>
<epd:referenceToUnitGroupDataSet uri="../unitgroups/6ae2df01-888e-46c8-b17d-49fa3869b476.xml" type="unit group data set" refObjectId="6ae2df01-888e-46c8-b17d-49fa3869b476">
<common:shortDescription xml:lang="de">m^(3) Welt-Äq. entzogen</common:shortDescription>
</epd:referenceToUnitGroupDataSet>
<epd:amount epd:module="A1-A3">0.0716</epd:amount>
<epd:amount epd:module="C1">2.5E-05</epd:amount>
<epd:amount epd:module="C2">8.73E-06</epd:amount>
<epd:amount epd:module="C3">6.52E-05</epd:amount>
<epd:amount epd:module="C4">-2.48E-05</epd:amount>
<epd:amount epd:module="D">-0.011</epd:amount>
</common:other>
</LCIAResult>
<LCIAResult>
<referenceToLCIAMethodDataSet uri="../lciamethods/b5c602c6-def3-11e6-bf01-fe55135034f3.xml" type="LCIA method data set" refObjectId="b5c602c6-def3-11e6-bf01-fe55135034f3">
<common:shortDescription xml:lang="de">Auftreten von Krankheiten aufgrund von Feinstaubemissionen (PM)</common:shortDescription>
<common:shortDescription xml:lang="en">Incidence of disease due to PM emissions (PM)</common:shortDescription>
</referenceToLCIAMethodDataSet>
<common:other>
<epd:referenceToUnitGroupDataSet uri="../unitgroups/3883559b-648f-4afc-8ba2-0bd24f3affa3.xml" type="unit group data set" refObjectId="3883559b-648f-4afc-8ba2-0bd24f3affa3">
<common:shortDescription xml:lang="de">Krankheitsfälle</common:shortDescription>
</epd:referenceToUnitGroupDataSet>
<epd:amount epd:module="A1-A3"></epd:amount>
<epd:amount epd:module="C1"></epd:amount>
<epd:amount epd:module="C2"></epd:amount>
<epd:amount epd:module="C3"></epd:amount>
<epd:amount epd:module="C4"></epd:amount>
<epd:amount epd:module="D"></epd:amount>
</common:other>
</LCIAResult>
<LCIAResult>
<referenceToLCIAMethodDataSet uri="../lciamethods/b5c632be-def3-11e6-bf01-fe55135034f3.xml" type="LCIA method data set" refObjectId="b5c632be-def3-11e6-bf01-fe55135034f3">
<common:shortDescription xml:lang="de">Wirkung durch Exposition des Menschen mit U235 (IR)</common:shortDescription>
<common:shortDescription xml:lang="en">Human exposure efficiency relative to U235 (IR)</common:shortDescription>
</referenceToLCIAMethodDataSet>
<common:other>
<epd:referenceToUnitGroupDataSet uri="../unitgroups/456b05bf-1415-44a9-9993-02452f554c09.xml" type="unit group data set" refObjectId="456b05bf-1415-44a9-9993-02452f554c09">
<common:shortDescription xml:lang="de">kBq U235-Äq.</common:shortDescription>
</epd:referenceToUnitGroupDataSet>
<epd:amount epd:module="A1-A3"></epd:amount>
<epd:amount epd:module="C1"></epd:amount>
<epd:amount epd:module="C2"></epd:amount>
<epd:amount epd:module="C3"></epd:amount>
<epd:amount epd:module="C4"></epd:amount>
<epd:amount epd:module="D"></epd:amount>
</common:other>
</LCIAResult>
<LCIAResult>
<referenceToLCIAMethodDataSet uri="../lciamethods/ee1082d1-b0f7-43ca-a1f0-21e2a4a74511.xml" type="LCIA method data set" refObjectId="ee1082d1-b0f7-43ca-a1f0-21e2a4a74511">
<common:shortDescription xml:lang="de">Toxizitätsvergleichseinheit für Ökosysteme (ETP-fw)</common:shortDescription>
<common:shortDescription xml:lang="en">Comparative toxic unit for ecosystems (ETP-fw)</common:shortDescription>
</referenceToLCIAMethodDataSet>
<common:other>
<epd:referenceToUnitGroupDataSet uri="../unitgroups/aa959ded-f1eb-4efb-9c5c-2d60be36b3e6.xml" type="unit group data set" refObjectId="aa959ded-f1eb-4efb-9c5c-2d60be36b3e6">
<common:shortDescription xml:lang="de">CTUe</common:shortDescription>
</epd:referenceToUnitGroupDataSet>
<epd:amount epd:module="A1-A3"></epd:amount>
<epd:amount epd:module="C1"></epd:amount>
<epd:amount epd:module="C2"></epd:amount>
<epd:amount epd:module="C3"></epd:amount>
<epd:amount epd:module="C4"></epd:amount>
<epd:amount epd:module="D"></epd:amount>
</common:other>
</LCIAResult>
<LCIAResult>
<referenceToLCIAMethodDataSet uri="../lciamethods/2299222a-bbd8-474f-9d4f-4dd1f18aea7c.xml" type="LCIA method data set" refObjectId="2299222a-bbd8-474f-9d4f-4dd1f18aea7c">
<common:shortDescription xml:lang="de">Toxizitätsvergleichseinheit für Menschen (krebserregend) (HTP-c)</common:shortDescription>
<common:shortDescription xml:lang="en">Comparative toxic unit for humans (carcinogenic) (HTP-c)</common:shortDescription>
</referenceToLCIAMethodDataSet>
<common:other>
<epd:referenceToUnitGroupDataSet uri="../unitgroups/d4c9523e-2d7e-49fd-8469-998f547d3a70.xml" type="unit group data set" refObjectId="d4c9523e-2d7e-49fd-8469-998f547d3a70">
<common:shortDescription xml:lang="de">CTUh</common:shortDescription>
</epd:referenceToUnitGroupDataSet>
<epd:amount epd:module="A1-A3"></epd:amount>
<epd:amount epd:module="C1"></epd:amount>
<epd:amount epd:module="C2"></epd:amount>
<epd:amount epd:module="C3"></epd:amount>
<epd:amount epd:module="C4"></epd:amount>
<epd:amount epd:module="D"></epd:amount>
</common:other>
</LCIAResult>
<LCIAResult>
<referenceToLCIAMethodDataSet uri="../lciamethods/3af763a5-b7a1-48c9-9cee-1f223481fcef.xml" type="LCIA method data set" refObjectId="3af763a5-b7a1-48c9-9cee-1f223481fcef">
<common:shortDescription xml:lang="de">Toxizitätsvergleichseinheit für Menschen (nicht krebserregend) (HTP-nc)</common:shortDescription>
<common:shortDescription xml:lang="en">Comparative toxic unit for humans (noncarcinogenic) (HTP-nc)</common:shortDescription>
</referenceToLCIAMethodDataSet>
<common:other>
<epd:referenceToUnitGroupDataSet uri="../unitgroups/d4c9523e-2d7e-49fd-8469-998f547d3a70.xml" type="unit group data set" refObjectId="d4c9523e-2d7e-49fd-8469-998f547d3a70">
<common:shortDescription xml:lang="de">CTUh</common:shortDescription>
</epd:referenceToUnitGroupDataSet>
<epd:amount epd:module="A1-A3"></epd:amount>
<epd:amount epd:module="C1"></epd:amount>
<epd:amount epd:module="C2"></epd:amount>
<epd:amount epd:module="C3"></epd:amount>
<epd:amount epd:module="C4"></epd:amount>
<epd:amount epd:module="D"></epd:amount>
</common:other>
</LCIAResult>
<LCIAResult>
<referenceToLCIAMethodDataSet uri="../lciamethods/b2ad6890-c78d-11e6-9d9d-cec0c932ce01.xml" type="LCIA method data set" refObjectId="b2ad6890-c78d-11e6-9d9d-cec0c932ce01">
<common:shortDescription xml:lang="de">Bodenqualitätsindex (SQP)</common:shortDescription>
<common:shortDescription xml:lang="en">Soil quality index (SQP)</common:shortDescription>
</referenceToLCIAMethodDataSet>
<common:other>
<epd:referenceToUnitGroupDataSet uri="../unitgroups/f130951c-e67f-4f7f-8dd4-665de3974e18.xml" type="unit group data set" refObjectId="f130951c-e67f-4f7f-8dd4-665de3974e18">
<common:shortDescription xml:lang="de">SQP</common:shortDescription>
</epd:referenceToUnitGroupDataSet>
<epd:amount epd:module="A1-A3"></epd:amount>
<epd:amount epd:module="C1"></epd:amount>
<epd:amount epd:module="C2"></epd:amount>
<epd:amount epd:module="C3"></epd:amount>
<epd:amount epd:module="C4"></epd:amount>
<epd:amount epd:module="D"></epd:amount>
</common:other>
</LCIAResult>
</LCIAResults>
</processDataSet>