<?xml version="1.0" encoding="utf-8"?>
<processDataSet xmlns:epd="http://www.iai.kit.edu/EPD/2013" xmlns:epd2="http://www.indata.network/EPD/2019" xmlns:common="http://lca.jrc.it/ILCD/Common" xsi:schemaLocation="http://lca.jrc.it/ILCD/Process ../../schemas/EPD_DataSet.xsd" epd2:epd-version="1.2" version="1.1" locations="../ILCDLocations.xml" xmlns:xsi="http://www.w3.org/2001/XMLSchema-instance" xmlns="http://lca.jrc.it/ILCD/Process">
<processInformation>
<dataSetInformation>
<common:UUID>3000c0cd-b0f0-454e-ab47-6b27937bb7dd</common:UUID>
<name>
<baseName xml:lang="en">TOURNIKET - All options included</baseName>
<functionalUnitFlowProperties xml:lang="en" />
</name>
<classificationInformation>
<common:classification name="OEKOBAU.DAT">
<common:class level="0" classId="7">Komponenten von Fenstern und Vorhangfassaden</common:class>
<common:class level="1" classId="7.6">Türen und Tore</common:class>
<common:class level="2" classId="7.6.02">Aluminium</common:class>
</common:classification>
<common:classification name="IBUCategories">
<common:class level="0">02 Building products</common:class>
<common:class level="1">Doors, windows, shutters, and related products</common:class>
<common:class level="2">Automatic doors, automatic gates, and revolving door systems</common:class>
</common:classification>
</classificationInformation>
<common:generalComment xml:lang="en">The Tourniket is Boon Edam’s most versatile entry solution. Available in virtually every colour or finish, with three or four door wings, manual or automatic operation, and with a variety of door set options, it is the ultimate solution for many different types of buildings.For the product studied in this document, all options available for a Tourniket TQ were selected:Maximum diameter (3800 mm) and height under canopy (2300mm) available for the range, 4 Collapsible door leaves with thickened-glass windows, Thickened-glass windows curved walls, Automated drive positioned in the canopy (hence a higher canopy), Motion detector control and idle speed control, External manual control panel, Automatic night locking, including monitoring, with thickened-glass windows, Protective aluminium strips on all windows, Lighting, with 4 low energy lamps, Increased thickness floor mat.</common:generalComment>
</dataSetInformation>
<quantitativeReference>
<referenceToReferenceFlow>0</referenceToReferenceFlow>
</quantitativeReference>
<time>
<common:referenceYear>2018</common:referenceYear>
<common:dataSetValidUntil>2023</common:dataSetValidUntil>
<common:other>
<epd2:publicationDateOfEPD>2018-09-03</epd2:publicationDateOfEPD>
</common:other>
</time>
<geography>
<locationOfOperationSupplyOrProduction location="RER" />
</geography>
<technology>
<technologyDescriptionAndIncludedProcesses xml:lang="en">All materials are shipped from suppliers to Boon Edam Manufacturing EMEA site in Edam, The Netherlands. Steel and aluminium profiles are cut to shape and size on site, and are assembled with the rest of the materials by Boon Edam. The manufacturing site in Edam is /ISO 9001/ certified. 
Declared unit: 
The LCA study used to draft this EPD is based on 1 Boon Edam Tourniket TQ-04, used in Europe for 20 years.Declared Unit: 1 piece (1 revolving door), with a 3800mm diameter, 2300mm height under canopy and 3500mm height.It is fitted with a 220V AC motor of 180W.This is the maximum possible size for this range, with all potential options included, in effect presenting the &apos;worst-case scenario&apos; for a product of the TQ range.</technologyDescriptionAndIncludedProcesses>
<technologicalApplicability xml:lang="en">Automatic revolving doors are intended to be used in commercial buildings, in particular in:Airports RetailBanksCorporate HeadquartersGovernmental buildingsHealthcareHotels &amp; Restaurants</technologicalApplicability>
</technology>
</processInformation>
<modellingAndValidation>
<LCIMethodAndAllocation>
<typeOfDataSet>EPD</typeOfDataSet>
<referenceToLCAMethodDetails type="source data set" refObjectId="d83d5033-265f-44e8-8c17-0fea4c2d16e7">
<common:shortDescription xml:lang="en">Automatic doors, automatic gates, and revolving door systems.pdf</common:shortDescription>
</referenceToLCAMethodDetails>
<common:other>
<epd:subType xmlns="http://www.iai.kit.edu/EPD/2013">average dataset</epd:subType>
</common:other>
</LCIMethodAndAllocation>
<dataSourcesTreatmentAndRepresentativeness>
<referenceToDataSource type="source data set" refObjectId="b497a91f-e14b-4b69-8f28-f50eb1576766">
<common:shortDescription xml:lang="en">ecoinvent database (all versions)</common:shortDescription>
</referenceToDataSource>
<referenceToDataSource type="source data set" refObjectId="c667cc42-12a7-4d92-9d7b-5e4e90a7a274">
<common:shortDescription xml:lang="en">ecoinvent 3.3 database</common:shortDescription>
</referenceToDataSource>
<useAdviceForDataSet xml:lang="en">Scope: 
The declaration and background LCA report represent an automatic revolving door Boon Edam Tourniket, type TQ.Raw materials and components are provided by suppliers from around the globe and shipped to Boon Edam, where the doors are manufactured and assembled before being shipped and installed on a construction site in Europe.The energy use on site and maintenance during the 20 years of use are taken in account. 
System boundary: 
The present EPD is declared as a &quot;cradle-to-gate - with options&quot;The modules declared are:Production stageA1 - Raw material extraction and processing: All materials and parts that are constituents of the final product are considered. All pre-processing that are applied to the material, prior to handling by Boon Edam, are part of A1. Additional raw material quantities that are needed to cover-up for the production losses and metal cuttings that are sent back to suppliers are also accounted in A1.A2 - Transport to the manufacturer: Transports of all raw materials (incl. quantities needed to cover-up for the production losses) and packaging materials are accounted for. A3 - Manufacturing: All processes performed at Boon Edam are accounted for (incl. use of energy), as well as raw material extraction and pre-processing of packaging materials. Waste generated are accounted in A3, excepted for recycled metal cutting (included in A1)Construction stageA4 - Transport to building site: Transport from Boon Edam Distribution &amp; Support centre to a theoretical building in Europe is modelled, including the door and its packaging. A5 - Installation in the building: The effort for installation is minimal since the main parts of the doors are supplied pre-assembled, and (depending on the dimensions and option of the product) consist only in a couple of hours of use of electric screwdrivers and power drills. Disposal of packaging is also accounted for.Use stage modules related to the building fabricB2- Maintenance: For the door to be functional over a period of 20 years, some parts need to be replaced as preventive maintenance (mainly sensors and wear parts). The material needed for production of these parts, and the production effort in the upstream chain are included, as well as the transport to the construction site. When it comes to the replaced elements, their transport from the installation site back to Boon Edam and end of life treatment are taken into account. Use stage modules related to operation of the buildingB6 - operational energy use: The electricity use for powering the electric drive is computed in the model. End-of-life stage C1 - Deconstruction: Electricity needed for the use of power drills is included. C2 - Transport to waste processing: Transport of the complete door is computed. C3 - Waste processing: The processing of components which reach end of waste state and need conversion to secondary materials, and those which are incinerated, is included.C4 - Disposal: End of life of all the materials is considered. Some of the materials used in the product - steel, aluminium and glass - present a value and reach the end of waste state (see detail of the ratios used in §4.1.4). The remaining components are incinerated and landfilled</useAdviceForDataSet>
<common:other>
<epd2:referenceToOriginalEPD type="source data set" refObjectId="7bb23ebc-0a41-4af1-b66d-d348287abf03">
<common:shortDescription xml:lang="en">TOURNIKET - All options included.pdf</common:shortDescription>
</epd2:referenceToOriginalEPD>
</common:other>
</dataSourcesTreatmentAndRepresentativeness>
<validation>
<review type="Accredited third party review">
<common:referenceToNameOfReviewerAndInstitution uri="../contacts/d111dbec-b024-4be5-86c5-752d6eb2cf95.xml" type="contact data set" refObjectId="d111dbec-b024-4be5-86c5-752d6eb2cf95">
<common:shortDescription xml:lang="en">Institut Bauen und Umwelt e. V.</common:shortDescription>
</common:referenceToNameOfReviewerAndInstitution>
</review>
</validation>
<complianceDeclarations>
<compliance>
<common:referenceToComplianceSystem uri="../sources/b00f9ec0-7874-11e3-981f-0800200c9a66.xml" type="source data set" refObjectId="b00f9ec0-7874-11e3-981f-0800200c9a66">
<common:shortDescription xml:lang="en">DIN EN 15804</common:shortDescription>
</common:referenceToComplianceSystem>
</compliance>
<compliance>
<common:referenceToComplianceSystem uri="../sources/4f2eb655-6e44-4874-a95a-e28f5442cd4d.xml" type="source data set" refObjectId="4f2eb655-6e44-4874-a95a-e28f5442cd4d">
<common:shortDescription xml:lang="en">ISO 14025</common:shortDescription>
</common:referenceToComplianceSystem>
</compliance>
</complianceDeclarations>
</modellingAndValidation>
<administrativeInformation>
<common:commissionerAndGoal>
<common:referenceToCommissioner uri="../contacts/bc40a500-bc56-46fe-9d67-440a571be25a.xml" type="contact data set" refObjectId="bc40a500-bc56-46fe-9d67-440a571be25a">
<common:shortDescription xml:lang="en">Royal Boon Edam International B.V.</common:shortDescription>
</common:referenceToCommissioner>
</common:commissionerAndGoal>
<dataGenerator>
<common:referenceToPersonOrEntityGeneratingTheDataSet uri="../contacts/bbbbdfdd-3471-40ba-9688-852d3eaeb853.xml" type="contact data set" refObjectId="bbbbdfdd-3471-40ba-9688-852d3eaeb853">
<common:shortDescription xml:lang="en">PRé Sustainability</common:shortDescription>
</common:referenceToPersonOrEntityGeneratingTheDataSet>
</dataGenerator>
<dataEntryBy>
<common:timeStamp>2018-09-03T11:24:51.855</common:timeStamp>
<common:referenceToDataSetFormat uri="../sources/a97a0155-0234-4b87-b4ce-a45da52f2a40.xml" type="source data set" refObjectId="a97a0155-0234-4b87-b4ce-a45da52f2a40">
<common:shortDescription xml:lang="en">ILCD Format</common:shortDescription>
</common:referenceToDataSetFormat>
<common:referenceToDataSetFormat uri="../sources/a29449fd-aa2f-4de8-b5d7-4b06b43c6fde.xml" type="source data set" refObjectId="a29449fd-aa2f-4de8-b5d7-4b06b43c6fde">
<common:shortDescription xml:lang="de">EPD-Datenformaterweiterungen v1.2</common:shortDescription>
<common:shortDescription xml:lang="en">EPD Data Format Extensions v1.2</common:shortDescription>
</common:referenceToDataSetFormat>
</dataEntryBy>
<publicationAndOwnership>
<common:dataSetVersion>00.01.000</common:dataSetVersion>
<common:referenceToRegistrationAuthority uri="../contacts/d111dbec-b024-4be5-86c5-752d6eb2cf95.xml" type="contact data set" refObjectId="d111dbec-b024-4be5-86c5-752d6eb2cf95">
<common:shortDescription xml:lang="en">Institut Bauen und Umwelt e. V.</common:shortDescription>
</common:referenceToRegistrationAuthority>
<common:registrationNumber>EPD-RBE-20180009-IBD1-EN</common:registrationNumber>
<common:referenceToOwnershipOfDataSet uri="../contacts/bc40a500-bc56-46fe-9d67-440a571be25a.xml" type="contact data set" refObjectId="bc40a500-bc56-46fe-9d67-440a571be25a">
<common:shortDescription xml:lang="en">Royal Boon Edam International B.V.</common:shortDescription>
</common:referenceToOwnershipOfDataSet>
<common:copyright>true</common:copyright>
<common:licenseType>Free of charge for all users and uses</common:licenseType>
<common:accessRestrictions xml:lang="en">None</common:accessRestrictions>
<common:other>
<epd2:referenceToPublisher type="contact data set" refObjectId="d111dbec-b024-4be5-86c5-752d6eb2cf95" uri="../contacts/d111dbec-b024-4be5-86c5-752d6eb2cf95.xml">
<common:shortDescription xml:lang="en">Institut Bauen und Umwelt e. V.</common:shortDescription>
</epd2:referenceToPublisher>
</common:other>
</publicationAndOwnership>
</administrativeInformation>
<exchanges>
<exchange dataSetInternalID="0">
<referenceToFlowDataSet uri="../flows/dd3c732f-048e-9f7b-e76f-b829ec5d2a1a.xml" type="flow data set" refObjectId="dd3c732f-048e-9f7b-e76f-b829ec5d2a1a">
<common:shortDescription xml:lang="en">1 Tourniket TQ, all options included ()</common:shortDescription>
</referenceToFlowDataSet>
<meanAmount>1</meanAmount>
<referencesToDataSource />
</exchange>
<exchange dataSetInternalID="1">
<referenceToFlowDataSet uri="../flows/20f32be5-0398-4288-9b6d-accddd195317.xml" type="flow data set" refObjectId="20f32be5-0398-4288-9b6d-accddd195317">
<common:shortDescription xml:lang="en">Renewable primary energy as energy carrier (PERE)</common:shortDescription>
</referenceToFlowDataSet>
<functionType>General reminder flow</functionType>
<exchangeDirection>Input</exchangeDirection>
<common:other>
<epd:referenceToUnitGroupDataSet uri="../unitgroups/93a60a57-a3c8-11da-a746-0800200c9a66.xml" type="unit group data set" refObjectId="93a60a57-a3c8-11da-a746-0800200c9a66">
<common:shortDescription xml:lang="en">MJ</common:shortDescription>
</epd:referenceToUnitGroupDataSet>
<epd:amount epd:module="A1-A3">31600</epd:amount>
<epd:amount epd:module="A4">37.7</epd:amount>
<epd:amount epd:module="A5">5420</epd:amount>
<epd:amount epd:module="B2">1060</epd:amount>
<epd:amount epd:module="B6">15800</epd:amount>
<epd:amount epd:module="C1">10.1</epd:amount>
<epd:amount epd:module="C2">7.96</epd:amount>
<epd:amount epd:module="C3">3920</epd:amount>
<epd:amount epd:module="C4">1.38</epd:amount>
</common:other>
</exchange>
<exchange dataSetInternalID="2">
<referenceToFlowDataSet uri="../flows/fb3ec0de-548d-4508-aea5-00b73bf6f702.xml" type="flow data set" refObjectId="fb3ec0de-548d-4508-aea5-00b73bf6f702">
<common:shortDescription xml:lang="en">Renewable primary energy resources as material utilization (PERM)</common:shortDescription>
</referenceToFlowDataSet>
<functionType>General reminder flow</functionType>
<exchangeDirection>Input</exchangeDirection>
<common:other>
<epd:referenceToUnitGroupDataSet uri="../unitgroups/93a60a57-a3c8-11da-a746-0800200c9a66.xml" type="unit group data set" refObjectId="93a60a57-a3c8-11da-a746-0800200c9a66">
<common:shortDescription xml:lang="en">MJ</common:shortDescription>
</epd:referenceToUnitGroupDataSet>
<epd:amount epd:module="A1-A3">9310</epd:amount>
<epd:amount epd:module="A4">0</epd:amount>
<epd:amount epd:module="A5">-5410</epd:amount>
<epd:amount epd:module="B2">0</epd:amount>
<epd:amount epd:module="B6">0</epd:amount>
<epd:amount epd:module="C1">0</epd:amount>
<epd:amount epd:module="C2">0</epd:amount>
<epd:amount epd:module="C3">-3900</epd:amount>
<epd:amount epd:module="C4">0</epd:amount>
</common:other>
</exchange>
<exchange dataSetInternalID="3">
<referenceToFlowDataSet uri="../flows/53f97275-fa8a-4cdd-9024-65936002acd0.xml" type="flow data set" refObjectId="53f97275-fa8a-4cdd-9024-65936002acd0">
<common:shortDescription xml:lang="en">Total use of renewable primary energy resources (PERT)</common:shortDescription>
</referenceToFlowDataSet>
<functionType>General reminder flow</functionType>
<exchangeDirection>Input</exchangeDirection>
<common:other>
<epd:referenceToUnitGroupDataSet uri="../unitgroups/93a60a57-a3c8-11da-a746-0800200c9a66.xml" type="unit group data set" refObjectId="93a60a57-a3c8-11da-a746-0800200c9a66">
<common:shortDescription xml:lang="en">MJ</common:shortDescription>
</epd:referenceToUnitGroupDataSet>
<epd:amount epd:module="A1-A3">40900</epd:amount>
<epd:amount epd:module="A4">37.7</epd:amount>
<epd:amount epd:module="A5">10.6</epd:amount>
<epd:amount epd:module="B2">1060</epd:amount>
<epd:amount epd:module="B6">15800</epd:amount>
<epd:amount epd:module="C1">10.1</epd:amount>
<epd:amount epd:module="C2">7.96</epd:amount>
<epd:amount epd:module="C3">19.8</epd:amount>
<epd:amount epd:module="C4">1.38</epd:amount>
</common:other>
</exchange>
<exchange dataSetInternalID="4">
<referenceToFlowDataSet uri="../flows/ac857178-2b45-46ec-892a-a9a4332f0372.xml" type="flow data set" refObjectId="ac857178-2b45-46ec-892a-a9a4332f0372">
<common:shortDescription xml:lang="en">Non renewable primary energy as energy carrier (PENRE)</common:shortDescription>
</referenceToFlowDataSet>
<functionType>General reminder flow</functionType>
<exchangeDirection>Input</exchangeDirection>
<common:other>
<epd:referenceToUnitGroupDataSet uri="../unitgroups/93a60a57-a3c8-11da-a746-0800200c9a66.xml" type="unit group data set" refObjectId="93a60a57-a3c8-11da-a746-0800200c9a66">
<common:shortDescription xml:lang="en">MJ</common:shortDescription>
</epd:referenceToUnitGroupDataSet>
<epd:amount epd:module="A1-A3">197000</epd:amount>
<epd:amount epd:module="A4">2590</epd:amount>
<epd:amount epd:module="A5">238</epd:amount>
<epd:amount epd:module="B2">9190</epd:amount>
<epd:amount epd:module="B6">83700</epd:amount>
<epd:amount epd:module="C1">53.6</epd:amount>
<epd:amount epd:module="C2">547</epd:amount>
<epd:amount epd:module="C3">2800</epd:amount>
<epd:amount epd:module="C4">29</epd:amount>
</common:other>
</exchange>
<exchange dataSetInternalID="5">
<referenceToFlowDataSet uri="../flows/1421caa0-679d-4bf4-b282-0eb850ccae27.xml" type="flow data set" refObjectId="1421caa0-679d-4bf4-b282-0eb850ccae27">
<common:shortDescription xml:lang="en">Non renewable primary energy as material utilization (PENRM)</common:shortDescription>
</referenceToFlowDataSet>
<functionType>General reminder flow</functionType>
<exchangeDirection>Input</exchangeDirection>
<common:other>
<epd:referenceToUnitGroupDataSet uri="../unitgroups/93a60a57-a3c8-11da-a746-0800200c9a66.xml" type="unit group data set" refObjectId="93a60a57-a3c8-11da-a746-0800200c9a66">
<common:shortDescription xml:lang="en">MJ</common:shortDescription>
</epd:referenceToUnitGroupDataSet>
<epd:amount epd:module="A1-A3">2570</epd:amount>
<epd:amount epd:module="A4">0</epd:amount>
<epd:amount epd:module="A5">-169</epd:amount>
<epd:amount epd:module="B2">0</epd:amount>
<epd:amount epd:module="B6">0</epd:amount>
<epd:amount epd:module="C1">0</epd:amount>
<epd:amount epd:module="C2">0</epd:amount>
<epd:amount epd:module="C3">-2400</epd:amount>
<epd:amount epd:module="C4">0</epd:amount>
</common:other>
</exchange>
<exchange dataSetInternalID="6">
<referenceToFlowDataSet uri="../flows/06159210-646b-4c8d-8583-da9b3b95a6c1.xml" type="flow data set" refObjectId="06159210-646b-4c8d-8583-da9b3b95a6c1">
<common:shortDescription xml:lang="en">Total use of non renewable primary energy resources (PENRT)</common:shortDescription>
</referenceToFlowDataSet>
<functionType>General reminder flow</functionType>
<exchangeDirection>Input</exchangeDirection>
<common:other>
<epd:referenceToUnitGroupDataSet uri="../unitgroups/93a60a57-a3c8-11da-a746-0800200c9a66.xml" type="unit group data set" refObjectId="93a60a57-a3c8-11da-a746-0800200c9a66">
<common:shortDescription xml:lang="en">MJ</common:shortDescription>
</epd:referenceToUnitGroupDataSet>
<epd:amount epd:module="A1-A3">199000</epd:amount>
<epd:amount epd:module="A4">2590</epd:amount>
<epd:amount epd:module="A5">68.8</epd:amount>
<epd:amount epd:module="B2">9190</epd:amount>
<epd:amount epd:module="B6">83700</epd:amount>
<epd:amount epd:module="C1">53.6</epd:amount>
<epd:amount epd:module="C2">547</epd:amount>
<epd:amount epd:module="C3">402</epd:amount>
<epd:amount epd:module="C4">29</epd:amount>
</common:other>
</exchange>
<exchange dataSetInternalID="7">
<referenceToFlowDataSet uri="../flows/c6a1f35f-2d09-4f54-8dfb-97e502e1ce92.xml" type="flow data set" refObjectId="c6a1f35f-2d09-4f54-8dfb-97e502e1ce92">
<common:shortDescription xml:lang="en">Use of secondary material (SM)</common:shortDescription>
</referenceToFlowDataSet>
<functionType>General reminder flow</functionType>
<exchangeDirection>Input</exchangeDirection>
<common:other>
<epd:referenceToUnitGroupDataSet uri="../unitgroups/ad38d542-3fe9-439d-9b95-2f5f7752acaf.xml" type="unit group data set" refObjectId="ad38d542-3fe9-439d-9b95-2f5f7752acaf">
<common:shortDescription xml:lang="en">kg</common:shortDescription>
</epd:referenceToUnitGroupDataSet>
<epd:amount epd:module="A1-A3">173</epd:amount>
<epd:amount epd:module="A4">0</epd:amount>
<epd:amount epd:module="A5">0</epd:amount>
<epd:amount epd:module="B2">17.7</epd:amount>
<epd:amount epd:module="B6">0</epd:amount>
<epd:amount epd:module="C1">0</epd:amount>
<epd:amount epd:module="C2">0</epd:amount>
<epd:amount epd:module="C3">0</epd:amount>
<epd:amount epd:module="C4">0</epd:amount>
</common:other>
</exchange>
<exchange dataSetInternalID="8">
<referenceToFlowDataSet uri="../flows/64333088-a55f-4aa2-9a31-c10b07816787.xml" type="flow data set" refObjectId="64333088-a55f-4aa2-9a31-c10b07816787">
<common:shortDescription xml:lang="en">Use of renewable secondary fuels (RSF)</common:shortDescription>
</referenceToFlowDataSet>
<functionType>General reminder flow</functionType>
<exchangeDirection>Input</exchangeDirection>
<common:other>
<epd:referenceToUnitGroupDataSet uri="../unitgroups/93a60a57-a3c8-11da-a746-0800200c9a66.xml" type="unit group data set" refObjectId="93a60a57-a3c8-11da-a746-0800200c9a66">
<common:shortDescription xml:lang="en">MJ</common:shortDescription>
</epd:referenceToUnitGroupDataSet>
<epd:amount epd:module="A1-A3">0</epd:amount>
<epd:amount epd:module="A4">0</epd:amount>
<epd:amount epd:module="A5">0</epd:amount>
<epd:amount epd:module="B2">0</epd:amount>
<epd:amount epd:module="B6">0</epd:amount>
<epd:amount epd:module="C1">0</epd:amount>
<epd:amount epd:module="C2">0</epd:amount>
<epd:amount epd:module="C3">0</epd:amount>
<epd:amount epd:module="C4">0</epd:amount>
</common:other>
</exchange>
<exchange dataSetInternalID="9">
<referenceToFlowDataSet uri="../flows/89def144-d39a-4287-b86f-efde453ddcb2.xml" type="flow data set" refObjectId="89def144-d39a-4287-b86f-efde453ddcb2">
<common:shortDescription xml:lang="en">Use of non renewable secondary fuels (NRSF)</common:shortDescription>
</referenceToFlowDataSet>
<functionType>General reminder flow</functionType>
<exchangeDirection>Input</exchangeDirection>
<common:other>
<epd:referenceToUnitGroupDataSet uri="../unitgroups/93a60a57-a3c8-11da-a746-0800200c9a66.xml" type="unit group data set" refObjectId="93a60a57-a3c8-11da-a746-0800200c9a66">
<common:shortDescription xml:lang="en">MJ</common:shortDescription>
</epd:referenceToUnitGroupDataSet>
<epd:amount epd:module="A1-A3">0</epd:amount>
<epd:amount epd:module="A4">0</epd:amount>
<epd:amount epd:module="A5">0</epd:amount>
<epd:amount epd:module="B2">0</epd:amount>
<epd:amount epd:module="B6">0</epd:amount>
<epd:amount epd:module="C1">0</epd:amount>
<epd:amount epd:module="C2">0</epd:amount>
<epd:amount epd:module="C3">0</epd:amount>
<epd:amount epd:module="C4">0</epd:amount>
</common:other>
</exchange>
<exchange dataSetInternalID="10">
<referenceToFlowDataSet uri="../flows/3cf952c8-f3a4-461d-8c96-96456ca62246.xml" type="flow data set" refObjectId="3cf952c8-f3a4-461d-8c96-96456ca62246">
<common:shortDescription xml:lang="en">Use of net fresh water (FW)</common:shortDescription>
</referenceToFlowDataSet>
<functionType>General reminder flow</functionType>
<exchangeDirection>Input</exchangeDirection>
<common:other>
<epd:referenceToUnitGroupDataSet uri="../unitgroups/cd950537-0a98-4044-9ba7-9f9a68d0a504.xml" type="unit group data set" refObjectId="cd950537-0a98-4044-9ba7-9f9a68d0a504">
<common:shortDescription xml:lang="en">m^3</common:shortDescription>
</epd:referenceToUnitGroupDataSet>
<epd:amount epd:module="A1-A3">181</epd:amount>
<epd:amount epd:module="A4">0.532</epd:amount>
<epd:amount epd:module="A5">0.0776</epd:amount>
<epd:amount epd:module="B2">6.93</epd:amount>
<epd:amount epd:module="B6">72</epd:amount>
<epd:amount epd:module="C1">0.0461</epd:amount>
<epd:amount epd:module="C2">0.112</epd:amount>
<epd:amount epd:module="C3">0.0934</epd:amount>
<epd:amount epd:module="C4">0.0258</epd:amount>
</common:other>
</exchange>
<exchange dataSetInternalID="11">
<referenceToFlowDataSet uri="../flows/430f9e0f-59b2-46a0-8e0d-55e0e84948fc.xml" type="flow data set" refObjectId="430f9e0f-59b2-46a0-8e0d-55e0e84948fc">
<common:shortDescription xml:lang="en">Hazardous waste disposed (HWD)</common:shortDescription>
</referenceToFlowDataSet>
<functionType>General reminder flow</functionType>
<exchangeDirection>Output</exchangeDirection>
<common:other>
<epd:referenceToUnitGroupDataSet uri="../unitgroups/ad38d542-3fe9-439d-9b95-2f5f7752acaf.xml" type="unit group data set" refObjectId="ad38d542-3fe9-439d-9b95-2f5f7752acaf">
<common:shortDescription xml:lang="en">kg</common:shortDescription>
</epd:referenceToUnitGroupDataSet>
<epd:amount epd:module="A1-A3">0.527</epd:amount>
<epd:amount epd:module="A4">0.00152</epd:amount>
<epd:amount epd:module="A5">0.0001</epd:amount>
<epd:amount epd:module="B2">0.0483</epd:amount>
<epd:amount epd:module="B6">0.127</epd:amount>
<epd:amount epd:module="C1">8.15E-05</epd:amount>
<epd:amount epd:module="C2">0.00032</epd:amount>
<epd:amount epd:module="C3">0.000577</epd:amount>
<epd:amount epd:module="C4">2.81E-05</epd:amount>
</common:other>
</exchange>
<exchange dataSetInternalID="12">
<referenceToFlowDataSet uri="../flows/b29ef66b-e286-4afa-949f-62f1a7b4d7fa.xml" type="flow data set" refObjectId="b29ef66b-e286-4afa-949f-62f1a7b4d7fa">
<common:shortDescription xml:lang="en">Non hazardous waste disposed (NHWD)</common:shortDescription>
</referenceToFlowDataSet>
<functionType>General reminder flow</functionType>
<exchangeDirection>Output</exchangeDirection>
<common:other>
<epd:referenceToUnitGroupDataSet uri="../unitgroups/ad38d542-3fe9-439d-9b95-2f5f7752acaf.xml" type="unit group data set" refObjectId="ad38d542-3fe9-439d-9b95-2f5f7752acaf">
<common:shortDescription xml:lang="en">kg</common:shortDescription>
</epd:referenceToUnitGroupDataSet>
<epd:amount epd:module="A1-A3">5870</epd:amount>
<epd:amount epd:module="A4">123</epd:amount>
<epd:amount epd:module="A5">75.6</epd:amount>
<epd:amount epd:module="B2">148</epd:amount>
<epd:amount epd:module="B6">277</epd:amount>
<epd:amount epd:module="C1">0.178</epd:amount>
<epd:amount epd:module="C2">26</epd:amount>
<epd:amount epd:module="C3">17.2</epd:amount>
<epd:amount epd:module="C4">95.1</epd:amount>
</common:other>
</exchange>
<exchange dataSetInternalID="13">
<referenceToFlowDataSet uri="../flows/3449546e-52ad-4b39-b809-9fb77cea8ff6.xml" type="flow data set" refObjectId="3449546e-52ad-4b39-b809-9fb77cea8ff6">
<common:shortDescription xml:lang="en">Radioactive waste disposed (RWD)</common:shortDescription>
</referenceToFlowDataSet>
<functionType>General reminder flow</functionType>
<exchangeDirection>Output</exchangeDirection>
<common:other>
<epd:referenceToUnitGroupDataSet uri="../unitgroups/ad38d542-3fe9-439d-9b95-2f5f7752acaf.xml" type="unit group data set" refObjectId="ad38d542-3fe9-439d-9b95-2f5f7752acaf">
<common:shortDescription xml:lang="en">kg</common:shortDescription>
</epd:referenceToUnitGroupDataSet>
<epd:amount epd:module="A1-A3">0.386</epd:amount>
<epd:amount epd:module="A4">0.0178</epd:amount>
<epd:amount epd:module="A5">0.000466</epd:amount>
<epd:amount epd:module="B2">0.0201</epd:amount>
<epd:amount epd:module="B6">0.593</epd:amount>
<epd:amount epd:module="C1">0.00038</epd:amount>
<epd:amount epd:module="C2">0.00376</epd:amount>
<epd:amount epd:module="C3">0.00226</epd:amount>
<epd:amount epd:module="C4">0.000144</epd:amount>
</common:other>
</exchange>
<exchange dataSetInternalID="14">
<referenceToFlowDataSet uri="../flows/a2b32f97-3fc7-4af2-b209-525bc6426f33.xml" type="flow data set" refObjectId="a2b32f97-3fc7-4af2-b209-525bc6426f33">
<common:shortDescription xml:lang="en">Components for re-use (CRU)</common:shortDescription>
</referenceToFlowDataSet>
<functionType>General reminder flow</functionType>
<exchangeDirection>Output</exchangeDirection>
<common:other>
<epd:referenceToUnitGroupDataSet uri="../unitgroups/ad38d542-3fe9-439d-9b95-2f5f7752acaf.xml" type="unit group data set" refObjectId="ad38d542-3fe9-439d-9b95-2f5f7752acaf">
<common:shortDescription xml:lang="en">kg</common:shortDescription>
</epd:referenceToUnitGroupDataSet>
<epd:amount epd:module="A1-A3">0</epd:amount>
<epd:amount epd:module="A4">0</epd:amount>
<epd:amount epd:module="A5">0</epd:amount>
<epd:amount epd:module="B2">0</epd:amount>
<epd:amount epd:module="B6">0</epd:amount>
<epd:amount epd:module="C1">0</epd:amount>
<epd:amount epd:module="C2">0</epd:amount>
<epd:amount epd:module="C3">0</epd:amount>
<epd:amount epd:module="C4">0</epd:amount>
</common:other>
</exchange>
<exchange dataSetInternalID="15">
<referenceToFlowDataSet uri="../flows/d7fe48a5-4103-49c8-9aae-b0b5dfdbd6ae.xml" type="flow data set" refObjectId="d7fe48a5-4103-49c8-9aae-b0b5dfdbd6ae">
<common:shortDescription xml:lang="en">Materials for recycling (MFR)</common:shortDescription>
</referenceToFlowDataSet>
<functionType>General reminder flow</functionType>
<exchangeDirection>Output</exchangeDirection>
<common:other>
<epd:referenceToUnitGroupDataSet uri="../unitgroups/ad38d542-3fe9-439d-9b95-2f5f7752acaf.xml" type="unit group data set" refObjectId="ad38d542-3fe9-439d-9b95-2f5f7752acaf">
<common:shortDescription xml:lang="en">kg</common:shortDescription>
</epd:referenceToUnitGroupDataSet>
<epd:amount epd:module="A1-A3">109</epd:amount>
<epd:amount epd:module="A4">0</epd:amount>
<epd:amount epd:module="A5">0</epd:amount>
<epd:amount epd:module="B2">40.8</epd:amount>
<epd:amount epd:module="B6">0</epd:amount>
<epd:amount epd:module="C1">0</epd:amount>
<epd:amount epd:module="C2">0</epd:amount>
<epd:amount epd:module="C3">0</epd:amount>
<epd:amount epd:module="C4">889</epd:amount>
</common:other>
</exchange>
<exchange dataSetInternalID="16">
<referenceToFlowDataSet uri="../flows/59a9181c-3aaf-46ee-8b13-2b3723b6e447.xml" type="flow data set" refObjectId="59a9181c-3aaf-46ee-8b13-2b3723b6e447">
<common:shortDescription xml:lang="en">Materials for energy recovery (MER)</common:shortDescription>
</referenceToFlowDataSet>
<functionType>General reminder flow</functionType>
<exchangeDirection>Output</exchangeDirection>
<common:other>
<epd:referenceToUnitGroupDataSet uri="../unitgroups/ad38d542-3fe9-439d-9b95-2f5f7752acaf.xml" type="unit group data set" refObjectId="ad38d542-3fe9-439d-9b95-2f5f7752acaf">
<common:shortDescription xml:lang="en">kg</common:shortDescription>
</epd:referenceToUnitGroupDataSet>
<epd:amount epd:module="A1-A3">0</epd:amount>
<epd:amount epd:module="A4">0</epd:amount>
<epd:amount epd:module="A5">0</epd:amount>
<epd:amount epd:module="B2">0</epd:amount>
<epd:amount epd:module="B6">0</epd:amount>
<epd:amount epd:module="C1">0</epd:amount>
<epd:amount epd:module="C2">0</epd:amount>
<epd:amount epd:module="C3">0</epd:amount>
<epd:amount epd:module="C4">0</epd:amount>
</common:other>
</exchange>
<exchange dataSetInternalID="17">
<referenceToFlowDataSet uri="../flows/4da0c987-2b76-40d6-9e9e-82a017aaaf29.xml" type="flow data set" refObjectId="4da0c987-2b76-40d6-9e9e-82a017aaaf29">
<common:shortDescription xml:lang="en">Exported electrical energy (EEE)</common:shortDescription>
</referenceToFlowDataSet>
<functionType>General reminder flow</functionType>
<exchangeDirection>Output</exchangeDirection>
<common:other>
<epd:referenceToUnitGroupDataSet uri="../unitgroups/93a60a57-a3c8-11da-a746-0800200c9a66.xml" type="unit group data set" refObjectId="93a60a57-a3c8-11da-a746-0800200c9a66">
<common:shortDescription xml:lang="en">MJ</common:shortDescription>
</epd:referenceToUnitGroupDataSet>
<epd:amount epd:module="A1-A3">56.9</epd:amount>
<epd:amount epd:module="A4">0</epd:amount>
<epd:amount epd:module="A5">52</epd:amount>
<epd:amount epd:module="B2">43</epd:amount>
<epd:amount epd:module="B6">0</epd:amount>
<epd:amount epd:module="C1">0</epd:amount>
<epd:amount epd:module="C2">0</epd:amount>
<epd:amount epd:module="C3">297</epd:amount>
<epd:amount epd:module="C4">0</epd:amount>
</common:other>
</exchange>
<exchange dataSetInternalID="18">
<referenceToFlowDataSet uri="../flows/98daf38a-7a79-46d3-9a37-2b7bd0955810.xml" type="flow data set" refObjectId="98daf38a-7a79-46d3-9a37-2b7bd0955810">
<common:shortDescription xml:lang="en">Exported thermal energy (EET)</common:shortDescription>
</referenceToFlowDataSet>
<functionType>General reminder flow</functionType>
<exchangeDirection>Output</exchangeDirection>
<common:other>
<epd:referenceToUnitGroupDataSet uri="../unitgroups/93a60a57-a3c8-11da-a746-0800200c9a66.xml" type="unit group data set" refObjectId="93a60a57-a3c8-11da-a746-0800200c9a66">
<common:shortDescription xml:lang="en">MJ</common:shortDescription>
</epd:referenceToUnitGroupDataSet>
<epd:amount epd:module="A1-A3">119</epd:amount>
<epd:amount epd:module="A4">0</epd:amount>
<epd:amount epd:module="A5">110</epd:amount>
<epd:amount epd:module="B2">883</epd:amount>
<epd:amount epd:module="B6">0</epd:amount>
<epd:amount epd:module="C1">0</epd:amount>
<epd:amount epd:module="C2">0</epd:amount>
<epd:amount epd:module="C3">613</epd:amount>
<epd:amount epd:module="C4">0</epd:amount>
</common:other>
</exchange>
</exchanges>
<LCIAResults>
<LCIAResult>
<referenceToLCIAMethodDataSet uri="../lciamethods/77e416eb-a363-4258-a04e-171d843a6460.xml" type="LCIA method data set" refObjectId="77e416eb-a363-4258-a04e-171d843a6460">
<common:shortDescription xml:lang="en">Global warming potential (GWP)</common:shortDescription>
</referenceToLCIAMethodDataSet>
<common:other>
<epd:referenceToUnitGroupDataSet uri="../unitgroups/1ebf3012-d0db-4de2-aefd-ef30cedb0be1.xml" type="unit group data set" refObjectId="1ebf3012-d0db-4de2-aefd-ef30cedb0be1">
<common:shortDescription xml:lang="en">kg CO_(2)-Äq.</common:shortDescription>
</epd:referenceToUnitGroupDataSet>
<epd:amount epd:module="A1-A3">19900</epd:amount>
<epd:amount epd:module="A4">167</epd:amount>
<epd:amount epd:module="A5">3.45</epd:amount>
<epd:amount epd:module="B2">906</epd:amount>
<epd:amount epd:module="B6">4200</epd:amount>
<epd:amount epd:module="C1">2.69</epd:amount>
<epd:amount epd:module="C2">35.3</epd:amount>
<epd:amount epd:module="C3">127</epd:amount>
<epd:amount epd:module="C4">5.68</epd:amount>
</common:other>
</LCIAResult>
<LCIAResult>
<referenceToLCIAMethodDataSet uri="../lciamethods/06dcd26f-025f-401a-a7c1-5e457eb54637.xml" type="LCIA method data set" refObjectId="06dcd26f-025f-401a-a7c1-5e457eb54637">
<common:shortDescription xml:lang="en">Depletion potential of the stratospheric ozone layer (ODP)</common:shortDescription>
</referenceToLCIAMethodDataSet>
<common:other>
<epd:referenceToUnitGroupDataSet uri="../unitgroups/88054749-b0a6-47ea-a82b-dc5b29326512.xml" type="unit group data set" refObjectId="88054749-b0a6-47ea-a82b-dc5b29326512">
<common:shortDescription xml:lang="en">kg CFC11-Äq.</common:shortDescription>
</epd:referenceToUnitGroupDataSet>
<epd:amount epd:module="A1-A3">0.000916</epd:amount>
<epd:amount epd:module="A4">3.12E-05</epd:amount>
<epd:amount epd:module="A5">4.43E-07</epd:amount>
<epd:amount epd:module="B2">4.16E-05</epd:amount>
<epd:amount epd:module="B6">0.00042</epd:amount>
<epd:amount epd:module="C1">2.69E-07</epd:amount>
<epd:amount epd:module="C2">6.59E-06</epd:amount>
<epd:amount epd:module="C3">3.87E-06</epd:amount>
<epd:amount epd:module="C4">2.44E-07</epd:amount>
</common:other>
</LCIAResult>
<LCIAResult>
<referenceToLCIAMethodDataSet uri="../lciamethods/b4274add-93b7-4905-a5e4-2e878c4e4216.xml" type="LCIA method data set" refObjectId="b4274add-93b7-4905-a5e4-2e878c4e4216">
<common:shortDescription xml:lang="en">Acidification potential of land and water (AP)</common:shortDescription>
</referenceToLCIAMethodDataSet>
<common:other>
<epd:referenceToUnitGroupDataSet uri="../unitgroups/bc50c624-a9bc-45b1-a9b0-e6b10d00476f.xml" type="unit group data set" refObjectId="bc50c624-a9bc-45b1-a9b0-e6b10d00476f">
<common:shortDescription xml:lang="en">kg SO_(2)-Äq.</common:shortDescription>
</epd:referenceToUnitGroupDataSet>
<epd:amount epd:module="A1-A3">119</epd:amount>
<epd:amount epd:module="A4">0.754</epd:amount>
<epd:amount epd:module="A5">0.0284</epd:amount>
<epd:amount epd:module="B2">5.36</epd:amount>
<epd:amount epd:module="B6">21.2</epd:amount>
<epd:amount epd:module="C1">0.0136</epd:amount>
<epd:amount epd:module="C2">0.159</epd:amount>
<epd:amount epd:module="C3">0.162</epd:amount>
<epd:amount epd:module="C4">0.0128</epd:amount>
</common:other>
</LCIAResult>
<LCIAResult>
<referenceToLCIAMethodDataSet uri="../lciamethods/f58827d0-b407-4ec6-be75-8b69efb98a0f.xml" type="LCIA method data set" refObjectId="f58827d0-b407-4ec6-be75-8b69efb98a0f">
<common:shortDescription xml:lang="en">Eutrophication potential (EP)</common:shortDescription>
</referenceToLCIAMethodDataSet>
<common:other>
<epd:referenceToUnitGroupDataSet uri="../unitgroups/67b5401d-873c-485f-bcf3-6ae83b918822.xml" type="unit group data set" refObjectId="67b5401d-873c-485f-bcf3-6ae83b918822">
<common:shortDescription xml:lang="en">kg PO_(4)^(3)-Äq.</common:shortDescription>
</epd:referenceToUnitGroupDataSet>
<epd:amount epd:module="A1-A3">10.3</epd:amount>
<epd:amount epd:module="A4">0.117</epd:amount>
<epd:amount epd:module="A5">0.00473</epd:amount>
<epd:amount epd:module="B2">0.799</epd:amount>
<epd:amount epd:module="B6">3.16</epd:amount>
<epd:amount epd:module="C1">0.00202</epd:amount>
<epd:amount epd:module="C2">0.0247</epd:amount>
<epd:amount epd:module="C3">0.0276</epd:amount>
<epd:amount epd:module="C4">0.00469</epd:amount>
</common:other>
</LCIAResult>
<LCIAResult>
<referenceToLCIAMethodDataSet uri="../lciamethods/1e84a202-dae6-42aa-9e9d-71ea48b8be00.xml" type="LCIA method data set" refObjectId="1e84a202-dae6-42aa-9e9d-71ea48b8be00">
<common:shortDescription xml:lang="en">Formation potential of tropospheric ozone photochemical oxidants (POCP)</common:shortDescription>
</referenceToLCIAMethodDataSet>
<common:other>
<epd:referenceToUnitGroupDataSet uri="../unitgroups/01c26c17-9a76-406e-8295-f17b55fd909e.xml" type="unit group data set" refObjectId="01c26c17-9a76-406e-8295-f17b55fd909e">
<common:shortDescription xml:lang="en">kg Ethen-Äq.</common:shortDescription>
</epd:referenceToUnitGroupDataSet>
<epd:amount epd:module="A1-A3">7.18</epd:amount>
<epd:amount epd:module="A4">0.0274</epd:amount>
<epd:amount epd:module="A5">0.00101</epd:amount>
<epd:amount epd:module="B2">0.534</epd:amount>
<epd:amount epd:module="B6">0.79</epd:amount>
<epd:amount epd:module="C1">0.000506</epd:amount>
<epd:amount epd:module="C2">0.00578</epd:amount>
<epd:amount epd:module="C3">0.00911</epd:amount>
<epd:amount epd:module="C4">0.00145</epd:amount>
</common:other>
</LCIAResult>
<LCIAResult>
<referenceToLCIAMethodDataSet uri="../lciamethods/f7c73bb9-ab1a-4249-9c6d-379a0de6f67e.xml" type="LCIA method data set" refObjectId="f7c73bb9-ab1a-4249-9c6d-379a0de6f67e">
<common:shortDescription xml:lang="en">Abiotic depletion potential for non fossil resources (ADPE)</common:shortDescription>
</referenceToLCIAMethodDataSet>
<common:other>
<epd:referenceToUnitGroupDataSet uri="../unitgroups/54ccd2d9-a32a-4fc2-923d-f2c8c93e89d4.xml" type="unit group data set" refObjectId="54ccd2d9-a32a-4fc2-923d-f2c8c93e89d4">
<common:shortDescription xml:lang="en">kg Sb-Äq.</common:shortDescription>
</epd:referenceToUnitGroupDataSet>
<epd:amount epd:module="A1-A3">0.281</epd:amount>
<epd:amount epd:module="A4">0.000513</epd:amount>
<epd:amount epd:module="A5">5.28E-06</epd:amount>
<epd:amount epd:module="B2">0.033</epd:amount>
<epd:amount epd:module="B6">0.00636</epd:amount>
<epd:amount epd:module="C1">4.07E-06</epd:amount>
<epd:amount epd:module="C2">0.000108</epd:amount>
<epd:amount epd:module="C3">4.53E-05</epd:amount>
<epd:amount epd:module="C4">1.22E-06</epd:amount>
</common:other>
</LCIAResult>
<LCIAResult>
<referenceToLCIAMethodDataSet uri="../lciamethods/804ebcdf-309d-4098-8ed8-fdaf2f389981.xml" type="LCIA method data set" refObjectId="804ebcdf-309d-4098-8ed8-fdaf2f389981">
<common:shortDescription xml:lang="en">Abiotic depletion potential for fossil resources (ADPF)</common:shortDescription>
</referenceToLCIAMethodDataSet>
<common:other>
<epd:referenceToUnitGroupDataSet uri="../unitgroups/93a60a57-a3c8-11da-a746-0800200c9a66.xml" type="unit group data set" refObjectId="93a60a57-a3c8-11da-a746-0800200c9a66">
<common:shortDescription xml:lang="en">MJ</common:shortDescription>
</epd:referenceToUnitGroupDataSet>
<epd:amount epd:module="A1-A3">188000</epd:amount>
<epd:amount epd:module="A4">2530</epd:amount>
<epd:amount epd:module="A5">43.3</epd:amount>
<epd:amount epd:module="B2">8450</epd:amount>
<epd:amount epd:module="B6">44400</epd:amount>
<epd:amount epd:module="C1">28.5</epd:amount>
<epd:amount epd:module="C2">535</epd:amount>
<epd:amount epd:module="C3">368</epd:amount>
<epd:amount epd:module="C4">27.3</epd:amount>
</common:other>
</LCIAResult>
</LCIAResults>
</processDataSet>