<?xml-stylesheet type='text/xsl' href='../../stylesheets/epd2html.xsl'?>
<processDataSet xmlns:xsi="http://www.w3.org/2001/XMLSchema-instance" xmlns="http://lca.jrc.it/ILCD/Process" xsi:schemaLocation="http://lca.jrc.it/ILCD/Process ../../schemas/EPD_DataSet.xsd" locations="../ILCDLocations.xml" version="1.1">
  <processInformation>
    <dataSetInformation>
      <common:UUID xmlns:common="http://lca.jrc.it/ILCD/Common">38051c22-fbd1-4b0e-944a-ae348b8c7695</common:UUID>
      <name>
        <baseName xmlns:epd="http://www.iai.kit.edu/EPD/2013" xmlns:common="http://lca.jrc.it/ILCD/Common" xml:lang="en">Steel section</baseName>
        <baseName xmlns:epd="http://www.iai.kit.edu/EPD/2013" xmlns:common="http://lca.jrc.it/ILCD/Common" xml:lang="de">Stahlprofil</baseName>
        <functionalUnitFlowProperties xmlns:epd="http://www.iai.kit.edu/EPD/2013" xmlns:common="http://lca.jrc.it/ILCD/Common" xml:lang="en">Steel sections</functionalUnitFlowProperties>
      </name>
      <classificationInformation>
        <common:classification xmlns:common="http://lca.jrc.it/ILCD/Common" name="oekobau.dat">
          <common:class level="0" classId="4">Metalle</common:class>
          <common:class level="1" classId="4.1">Stahl und Eisen</common:class>
          <common:class level="2" classId="4.1.03">Stahlprofile</common:class>
        </common:classification>
      </classificationInformation>
      <common:generalComment xmlns:common="http://lca.jrc.it/ILCD/Common" xmlns:epd="http://www.iai.kit.edu/EPD/2013" xml:lang="en">This data set has been modeled according to the European Standard EN 15804 for Sustainable Building. Results are depicted in modules that allow the structured expression of results over the entire life cycle.</common:generalComment>
      <common:generalComment xmlns:common="http://lca.jrc.it/ILCD/Common" xmlns:epd="http://www.iai.kit.edu/EPD/2013" xml:lang="de">Dieser Datensatz wurde nach dem European Standard EN 15804 für Nachhaltiges Bauen modelliert. Ergebnisse werden in Modulen abgebildet, die den strukturierten Ausdruck von Ergebnissen über den gesamten Lebenszyklus zulassen.</common:generalComment>
      <common:other xmlns:common="http://lca.jrc.it/ILCD/Common">
        <epd:safetyMargins xmlns:epd="http://www.iai.kit.edu/EPD/2013">
          <epd:margins>10</epd:margins>
          <epd:description xml:lang="en">Product system almost completely covered. Good technological, temporal and geographic representativeness.</epd:description>
          <epd:description xml:lang="de">Produktsystem weitgehend vollständig abgebildet. Gute technologische, zeitliche und geographische Repräsentativität.</epd:description>
        </epd:safetyMargins>
      </common:other>
    </dataSetInformation>
    <quantitativeReference type="Reference flow(s)">
      <referenceToReferenceFlow>107068</referenceToReferenceFlow>
    </quantitativeReference>
    <time>
      <common:referenceYear xmlns:common="http://lca.jrc.it/ILCD/Common">2018</common:referenceYear>
      <common:dataSetValidUntil xmlns:common="http://lca.jrc.it/ILCD/Common">2022</common:dataSetValidUntil>
      <common:timeRepresentativenessDescription xmlns:common="http://lca.jrc.it/ILCD/Common" xmlns:epd="http://www.iai.kit.edu/EPD/2013" xml:lang="en">Annual average</common:timeRepresentativenessDescription>
      <common:timeRepresentativenessDescription xmlns:common="http://lca.jrc.it/ILCD/Common" xmlns:epd="http://www.iai.kit.edu/EPD/2013" xml:lang="de">Jährlicher Durchschnitt</common:timeRepresentativenessDescription>
    </time>
    <geography>
      <locationOfOperationSupplyOrProduction location="DE">
        <descriptionOfRestrictions xmlns:epd="http://www.iai.kit.edu/EPD/2013" xmlns:common="http://lca.jrc.it/ILCD/Common" xml:lang="en">The data set represents the country specific situation in Germany, focusing on the main technologies, the region specific characteristics and / or import statistics.</descriptionOfRestrictions>
        <descriptionOfRestrictions xmlns:epd="http://www.iai.kit.edu/EPD/2013" xmlns:common="http://lca.jrc.it/ILCD/Common" xml:lang="de">Der Datensatz bildet die länderspezifische Situation in Deutschland ab. Dabei werden Haupttechnologien, spezifische regionale Charakteristiken und ggf. Importstatistiken berücksichtigt.</descriptionOfRestrictions>
      </locationOfOperationSupplyOrProduction>
    </geography>
    <technology>
      <technologyDescriptionAndIncludedProcesses xmlns:common="http://lca.jrc.it/ILCD/Common" xmlns:epd="http://www.iai.kit.edu/EPD/2013" xml:lang="en">The steel profile is manufactured with primary and secondary steel. 20% comes from the blast furnace route (primary) and 80% from the electric arc furnace route (secondary). The models of the primary and secondary route represents the country specific material and energy consumption according to their shares. Description of the EAF route:  The major feed stock for the EAF is ferrous scrap, which may comprise of scrap from inside the steelworks (e.g. cut-offs), cut-offs from steel product manufacturers (e.g. vehicle builders) and post-consumer scrap (e.g. end of life products). As in the integrated steel plant including blast furnaces and converters, a slag is formed from lime to collect undesirable components in the steel. Thus lime is an additive as well as coal (carbon) as reducing agent. Oxygen lances and / or oxy-fuel burners are used to assist in the early stages of melting.  For every material fraction the transport is considered in the data set.   For the production of carbon steel and low alloyed steels, following main operations are performed: raw material handling and storage, furnace charging with/without scrap preheating, EAF scrap melting, steel and slag tapping, ladle furnace treatments for quality adjustment, slag handling and finally continuous casting. The output of the continuous casting is the steel slab.   
Background system:
Electricity: Electricity is modelled according to the individual country-specific situations. The country-specific modelling is achieved on multiple levels. Firstly, individual energy carrier specific power plants and plants for renewable energy sources are modelled according to the current national electricity grid mix. Modelling the electricity consumption mix includes transmission / distribution losses and the own use by energy producers (own consumption of power plants and "other" own consumption e.g. due to pumped storage hydro power etc.), as well as imported electricity. Secondly, the national emission and efficiency standards of the power plants are modelled as well as the share of electricity plants and combined heat and power plants (CHP). Thirdly, the country-specific energy carrier supply (share of imports and / or domestic supply) including the country-specific energy carrier properties (e.g. element and energy content) are accounted for. Fourthly, the exploration, mining/production, processing and transport processes of the energy carrier supply chains are modelled according to the specific situation of each electricity producing country. The different production and processing techniques (emissions and efficiencies) in the different energy producing countries are considered, e.g. different crude oil production technologies or different flaring rates at the oil platforms.
Thermal energy, process steam: The thermal energy and process steam supply is modelled according to the individual country-specific situation with regard to emission standards and considered energy carriers. The thermal energy and process steam are produced at heat plants. Efficiencies for thermal energy production are by definition 100% in relation to the corresponding energy carrier input. For process steam the efficiency ranges from 85%, 90% to 95%. The energy carriers used for the generation of thermal energy and process steam are modelled according to the specific import situation (see electricity above).
Transports: All relevant and known transport processes are included. Ocean-going and inland ship transport as well as rail, truck and pipeline transport of bulk commodities are considered.
Energy carriers: The energy carriers are modelled according to the specific supply situation (see electricity above).
Refinery products: Diesel fuel, gasoline, technical gases, fuel oils, lubricants and residues such as bitumen are modelled with a parameterised country-specific refinery model. The refinery model represents the current national standard in refining techniques (e.g. emission level, internal energy consumption, etc.) as well as the individual country-specific product output spectrum, which can be quite different from country to country. The supply of crude oil is modelled, again, according to the country-specific situation with the respective properties of the resources.
 </technologyDescriptionAndIncludedProcesses>
      <technologyDescriptionAndIncludedProcesses xmlns:common="http://lca.jrc.it/ILCD/Common" xmlns:epd="http://www.iai.kit.edu/EPD/2013" xml:lang="de">Das Stahlprofil wird mittels Primär- und Sekundärstahl hergestellt.20 % stammen aus Hochöfen (primär) und 80 % aus Lichtbögenöfen (sekundär). 
Beschreibung des Elektrostahlwerks: Das Hauptausgangsmaterial für die Lichtbögenöfen  sind  Eisenmetallschrott, der den Schrott innerhalb der Stahlwerke (z. B. Ausschuss), Ausschuss von Stahlproduktherstellern (z. B. Fahrzeugbauer) und Verbraucherschrott (z. B. Altprodukte) einschließt. Wie in dem integrierten Hütten-/Stahlwerk inklusive  Hochöfen und Konvertern, wird Schlacke aus Kalk gebildet, um unerwünschte Komponenten im Stahl zu sammeln. Dementsprechend ist Kalk ein Zusatzstoff, ebenso wie  Kohle  (Kohlenstoff) ein Reduktionsmittel ist. Sauerstofflanzen und/oder Sauerstoffbrenner  werden zur Unterstützung in frühen Stadien des Schmelzens verwendet. Für jede Metallfraktion wird der Transport im Datensatz berücksichtigt. Für die Herstellung  von Karbonstahl  und niedriglegierten Stahlen, werden die folgenden Operationen durchgeführt: Rohmaterial-Handling und -Lagerung, Hochofenbeschickung mit/ohne Schrottvorwärmung, Lichtbogenofen-Schrott-Einschmelzung, Stahl- und Schlacken-Abstechen, Stahlbehandlung zur Qualitätsanpassung, Schlacketransporte und schließlich Strangguss. Der Output des Stranggusses sind Brammen. 

Es wird nur der Primäranteil an Stahl als Gutschrift vergeben. Der primäre Stahlanteil im Stahlprofil beträgt 12,7%, 87,3% sind Stahlschrott.
Bei den Recyclingpropzessen dieses Datensatzes wurden 5% Verluste angenommen, die deponiert werden (s. Werte in Modul C4). Die restlichen 95% werden stofflich recycled (siehe Gutschriften in Modul D), es werden also 0,12kg Primärstahl gutgeschrieben.</technologyDescriptionAndIncludedProcesses>
      <technologicalApplicability xmlns:common="http://lca.jrc.it/ILCD/Common" xmlns:epd="http://www.iai.kit.edu/EPD/2013" xml:lang="en">This product can be used in construction.</technologicalApplicability>
      <technologicalApplicability xmlns:common="http://lca.jrc.it/ILCD/Common" xmlns:epd="http://www.iai.kit.edu/EPD/2013" xml:lang="de">Dieses Produkt kann im Baubereich verwendet werden.</technologicalApplicability>
      <referenceToTechnologyPictogramme refObjectId="f41936f0-ca74-4586-9a60-06297e770d05" version="39.00.000" type="source data set" uri="../sources/f41936f0-ca74-4586-9a60-06297e770d05.xml">
        <common:shortDescription xmlns:common="http://lca.jrc.it/ILCD/Common" xmlns:epd="http://www.iai.kit.edu/EPD/2013" xml:lang="en">metals_glo_carbon steel production - eaf route.jpg</common:shortDescription>
        <common:shortDescription xmlns:common="http://lca.jrc.it/ILCD/Common" xmlns:epd="http://www.iai.kit.edu/EPD/2013" xml:lang="de">metals_glo_carbon steel production - eaf route.jpg</common:shortDescription>
      </referenceToTechnologyPictogramme>
    </technology>
  </processInformation>
  <modellingAndValidation>
    <LCIMethodAndAllocation>
      <typeOfDataSet>EPD</typeOfDataSet>
      <common:other xmlns:common="http://lca.jrc.it/ILCD/Common">
        <epd:subType xmlns:epd="http://www.iai.kit.edu/EPD/2013">generic dataset</epd:subType>
      </common:other>
    </LCIMethodAndAllocation>
    <dataSourcesTreatmentAndRepresentativeness>
      <referenceToDataSource refObjectId="cb50c596-16b4-44e4-b1aa-319319a79fb5" version="39.00.000" type="source data set" uri="../sources/cb50c596-16b4-44e4-b1aa-319319a79fb5.xml">
        <common:shortDescription xmlns:common="http://lca.jrc.it/ILCD/Common" xmlns:epd="http://www.iai.kit.edu/EPD/2013" xml:lang="en">GaBi Database Edition 2020, SP40</common:shortDescription>
        <common:shortDescription xmlns:common="http://lca.jrc.it/ILCD/Common" xmlns:epd="http://www.iai.kit.edu/EPD/2013" xml:lang="de">GaBi Database Edition 2020, SP40</common:shortDescription>
      </referenceToDataSource>
      <referenceToDataSource refObjectId="28d74cc0-db8b-4d7e-bc44-5f6d56ce0c4a" version="39.00.000" type="source data set" uri="../sources/28d74cc0-db8b-4d7e-bc44-5f6d56ce0c4a.xml">
        <common:shortDescription xmlns:common="http://lca.jrc.it/ILCD/Common" xmlns:epd="http://www.iai.kit.edu/EPD/2013" xml:lang="en">GaBi database (all versions)</common:shortDescription>
        <common:shortDescription xmlns:common="http://lca.jrc.it/ILCD/Common" xmlns:epd="http://www.iai.kit.edu/EPD/2013" xml:lang="de">GaBi database (all versions)</common:shortDescription>
      </referenceToDataSource>
      <useAdviceForDataSet xmlns:common="http://lca.jrc.it/ILCD/Common" xmlns:epd="http://www.iai.kit.edu/EPD/2013" xml:lang="en">The data set represents a cradle to gate inventory. It can be used to characterise the supply chain situation of the respective commodity in a representative manner. Combination with individual unit processes using this commodity enables the generation of user-specific (product) LCAs.</useAdviceForDataSet>
      <useAdviceForDataSet xmlns:common="http://lca.jrc.it/ILCD/Common" xmlns:epd="http://www.iai.kit.edu/EPD/2013" xml:lang="de">Der Datensatz repräsentiert ein Cradle to Gate Inventar. Er kann verwendet werden, um die Lieferkette des jeweiligen Produktes in einer repräsentativen Weise zu charakterisieren. Die Kombination mit einzelnen Einheitenprozessen und diesem Produkt ermöglicht die Erstellung von anwenderspezifischen (Produkt-) LCAs.</useAdviceForDataSet>
    </dataSourcesTreatmentAndRepresentativeness>
    <validation>
      <review type="Dependent internal review">
        <common:referenceToNameOfReviewerAndInstitution xmlns:common="http://lca.jrc.it/ILCD/Common" refObjectId="d7fa0337-f279-430d-becf-7f3111a85010" version="39.00.000" type="contact data set" uri="../contacts/d7fa0337-f279-430d-becf-7f3111a85010.xml">
          <common:shortDescription xmlns:epd="http://www.iai.kit.edu/EPD/2013" xml:lang="en">thinkstep</common:shortDescription>
          <common:shortDescription xmlns:epd="http://www.iai.kit.edu/EPD/2013" xml:lang="de">thinkstep</common:shortDescription>
        </common:referenceToNameOfReviewerAndInstitution>
        <common:referenceToNameOfReviewerAndInstitution xmlns:common="http://lca.jrc.it/ILCD/Common" refObjectId="de53c560-d6a9-11da-a94d-0800200c9a66" version="39.00.000" type="contact data set" uri="../contacts/de53c560-d6a9-11da-a94d-0800200c9a66.xml">
          <common:shortDescription xmlns:epd="http://www.iai.kit.edu/EPD/2013" xml:lang="en">IABP-GaBi</common:shortDescription>
          <common:shortDescription xmlns:epd="http://www.iai.kit.edu/EPD/2013" xml:lang="de">IABP-GaBi</common:shortDescription>
        </common:referenceToNameOfReviewerAndInstitution>
        <common:referenceToNameOfReviewerAndInstitution xmlns:common="http://lca.jrc.it/ILCD/Common" refObjectId="c0a9feeb-48d1-4c8f-9e8f-3ada7c0294c7" version="39.00.000" type="contact data set" uri="../contacts/c0a9feeb-48d1-4c8f-9e8f-3ada7c0294c7.xml">
          <common:shortDescription xmlns:epd="http://www.iai.kit.edu/EPD/2013" xml:lang="en">IBP-GaBi</common:shortDescription>
          <common:shortDescription xmlns:epd="http://www.iai.kit.edu/EPD/2013" xml:lang="de">IBP-GaBi</common:shortDescription>
        </common:referenceToNameOfReviewerAndInstitution>
      </review>
      <review type="Independent external review">
        <common:referenceToNameOfReviewerAndInstitution xmlns:common="http://lca.jrc.it/ILCD/Common" refObjectId="8f1306f0-7b83-4f36-a537-aa83f0498266" version="39.00.000" type="contact data set" uri="../contacts/8f1306f0-7b83-4f36-a537-aa83f0498266.xml">
          <common:shortDescription xmlns:epd="http://www.iai.kit.edu/EPD/2013" xml:lang="en">GaBi user forum</common:shortDescription>
          <common:shortDescription xmlns:epd="http://www.iai.kit.edu/EPD/2013" xml:lang="de">GaBi user forum</common:shortDescription>
        </common:referenceToNameOfReviewerAndInstitution>
        <common:referenceToNameOfReviewerAndInstitution xmlns:common="http://lca.jrc.it/ILCD/Common" refObjectId="851d996c-b88d-45ce-983a-b00ed0393ffb" version="39.00.000" type="contact data set" uri="../contacts/851d996c-b88d-45ce-983a-b00ed0393ffb.xml">
          <common:shortDescription xmlns:epd="http://www.iai.kit.edu/EPD/2013" xml:lang="en">GaBi bug forum</common:shortDescription>
          <common:shortDescription xmlns:epd="http://www.iai.kit.edu/EPD/2013" xml:lang="de">GaBi bug forum</common:shortDescription>
        </common:referenceToNameOfReviewerAndInstitution>
        <common:referenceToNameOfReviewerAndInstitution xmlns:common="http://lca.jrc.it/ILCD/Common" refObjectId="47511c41-5096-4dcf-be4f-dbb0c1c5cffc" version="39.00.000" type="contact data set" uri="../contacts/47511c41-5096-4dcf-be4f-dbb0c1c5cffc.xml">
          <common:shortDescription xmlns:epd="http://www.iai.kit.edu/EPD/2013" xml:lang="en">GaBi user community</common:shortDescription>
          <common:shortDescription xmlns:epd="http://www.iai.kit.edu/EPD/2013" xml:lang="de">GaBi user community</common:shortDescription>
        </common:referenceToNameOfReviewerAndInstitution>
      </review>
    </validation>
    <complianceDeclarations>
      <compliance>
        <common:referenceToComplianceSystem xmlns:common="http://lca.jrc.it/ILCD/Common" refObjectId="b00f9ec0-7874-11e3-981f-0800200c9a66" version="02.00.000" type="source data set" uri="../sources/b00f9ec0-7874-11e3-981f-0800200c9a66.xml">
          <common:shortDescription xmlns:epd="http://www.iai.kit.edu/EPD/2013" xml:lang="en">DIN EN 15804</common:shortDescription>
          <common:shortDescription xmlns:epd="http://www.iai.kit.edu/EPD/2013" xml:lang="de">DIN EN 15804</common:shortDescription>
        </common:referenceToComplianceSystem>
        <common:approvalOfOverallCompliance xmlns:common="http://lca.jrc.it/ILCD/Common">Fully compliant</common:approvalOfOverallCompliance>
      </compliance>
    </complianceDeclarations>
  </modellingAndValidation>
  <administrativeInformation>
    <dataEntryBy>
      <common:timeStamp xmlns:common="http://lca.jrc.it/ILCD/Common">2019-12-04T10:06:02+01:00</common:timeStamp>
      <common:referenceToDataSetFormat xmlns:common="http://lca.jrc.it/ILCD/Common" refObjectId="a97a0155-0234-4b87-b4ce-a45da52f2a40" version="03.00.000" type="source data set" uri="../sources/a97a0155-0234-4b87-b4ce-a45da52f2a40.xml">
        <common:shortDescription xmlns:epd="http://www.iai.kit.edu/EPD/2013" xml:lang="en">ILCD format 1.1</common:shortDescription>
        <common:shortDescription xmlns:epd="http://www.iai.kit.edu/EPD/2013" xml:lang="de">ILCD format 1.1</common:shortDescription>
      </common:referenceToDataSetFormat>
      <common:referenceToDataSetFormat xmlns:common="http://lca.jrc.it/ILCD/Common" refObjectId="cba73800-7874-11e3-981f-0800200c9a66" version="02.00.000" type="source data set" uri="../sources/cba73800-7874-11e3-981f-0800200c9a66.xml">
        <common:shortDescription xmlns:epd="http://www.iai.kit.edu/EPD/2013" xml:lang="en">EPD Data Format Extensions</common:shortDescription>
        <common:shortDescription xmlns:epd="http://www.iai.kit.edu/EPD/2013" xml:lang="de">EPD-Datenformaterweiterungen</common:shortDescription>
      </common:referenceToDataSetFormat>
      <common:referenceToPersonOrEntityEnteringTheData xmlns:common="http://lca.jrc.it/ILCD/Common" refObjectId="d7fa0337-f279-430d-becf-7f3111a85010" version="39.00.000" type="contact data set" uri="../contacts/d7fa0337-f279-430d-becf-7f3111a85010.xml">
        <common:shortDescription xmlns:epd="http://www.iai.kit.edu/EPD/2013" xml:lang="en">thinkstep</common:shortDescription>
        <common:shortDescription xmlns:epd="http://www.iai.kit.edu/EPD/2013" xml:lang="de">thinkstep</common:shortDescription>
      </common:referenceToPersonOrEntityEnteringTheData>
    </dataEntryBy>
    <publicationAndOwnership>
      <common:dataSetVersion xmlns:common="http://lca.jrc.it/ILCD/Common">20.19.120</common:dataSetVersion>
      <common:permanentDataSetURI xmlns:common="http://lca.jrc.it/ILCD/Common"/>
      <common:referenceToOwnershipOfDataSet xmlns:common="http://lca.jrc.it/ILCD/Common" refObjectId="d7fa0337-f279-430d-becf-7f3111a85010" version="39.00.000" type="contact data set" uri="../contacts/d7fa0337-f279-430d-becf-7f3111a85010.xml">
        <common:shortDescription xmlns:epd="http://www.iai.kit.edu/EPD/2013" xml:lang="en">thinkstep</common:shortDescription>
        <common:shortDescription xmlns:epd="http://www.iai.kit.edu/EPD/2013" xml:lang="de">thinkstep</common:shortDescription>
      </common:referenceToOwnershipOfDataSet>
      <common:copyright xmlns:common="http://lca.jrc.it/ILCD/Common">true</common:copyright>
    </publicationAndOwnership>
  </administrativeInformation>
  <exchanges>
    <exchange dataSetInternalID="107068">
      <referenceToFlowDataSet refObjectId="9eb8145d-d035-4d9f-a1dc-1006c45cb818" version="39.00.000" type="flow data set" uri="../flows/9eb8145d-d035-4d9f-a1dc-1006c45cb818.xml">
        <common:shortDescription xmlns:common="http://lca.jrc.it/ILCD/Common" xmlns:epd="http://www.iai.kit.edu/EPD/2013" xml:lang="en">Steel profile</common:shortDescription>
        <common:shortDescription xmlns:common="http://lca.jrc.it/ILCD/Common" xmlns:epd="http://www.iai.kit.edu/EPD/2013" xml:lang="de">Stahlprofil</common:shortDescription>
      </referenceToFlowDataSet>
      <meanAmount>1</meanAmount>
    </exchange>
    <exchange dataSetInternalID="107069">
      <referenceToFlowDataSet refObjectId="20f32be5-0398-4288-9b6d-accddd195317" version="39.00.000" type="flow data set" uri="../flows/20f32be5-0398-4288-9b6d-accddd195317.xml">
        <common:shortDescription xmlns:common="http://lca.jrc.it/ILCD/Common" xmlns:epd="http://www.iai.kit.edu/EPD/2013" xml:lang="en">Use of renewable primary energy (PERE)</common:shortDescription>
        <common:shortDescription xmlns:common="http://lca.jrc.it/ILCD/Common" xmlns:epd="http://www.iai.kit.edu/EPD/2013" xml:lang="de">Erneuerbare Primärenergie als Energieträger (PERE)</common:shortDescription>
      </referenceToFlowDataSet>
      <functionType>General reminder flow</functionType>
      <exchangeDirection>Input</exchangeDirection>
      <common:other xmlns:common="http://lca.jrc.it/ILCD/Common">
        <epd:amount xmlns:epd="http://www.iai.kit.edu/EPD/2013" epd:module="A1-A3">3.14562210314066</epd:amount>
        <epd:referenceToUnitGroupDataSet xmlns:epd="http://www.iai.kit.edu/EPD/2013" refObjectId="93a60a57-a3c8-11da-a746-0800200c9a66" version="03.00.000" type="unit group data set" uri="../unitgroups/93a60a57-a3c8-11da-a746-0800200c9a66.xml">
          <common:shortDescription xml:lang="en">MJ</common:shortDescription>
          <common:shortDescription xml:lang="de">MJ</common:shortDescription>
        </epd:referenceToUnitGroupDataSet>
        <epd:amount xmlns:epd="http://www.iai.kit.edu/EPD/2013" epd:module="C1">0.000519248890445602</epd:amount>
        <epd:amount xmlns:epd="http://www.iai.kit.edu/EPD/2013" epd:module="C2">0.00199760029244171</epd:amount>
        <epd:amount xmlns:epd="http://www.iai.kit.edu/EPD/2013" epd:module="D">0.192416775537167</epd:amount>
      </common:other>
    </exchange>
    <exchange dataSetInternalID="107070">
      <referenceToFlowDataSet refObjectId="fb3ec0de-548d-4508-aea5-00b73bf6f702" version="39.00.000" type="flow data set" uri="../flows/fb3ec0de-548d-4508-aea5-00b73bf6f702.xml">
        <common:shortDescription xmlns:common="http://lca.jrc.it/ILCD/Common" xmlns:epd="http://www.iai.kit.edu/EPD/2013" xml:lang="en">Primary energy resources used as raw materials (PERM)</common:shortDescription>
        <common:shortDescription xmlns:common="http://lca.jrc.it/ILCD/Common" xmlns:epd="http://www.iai.kit.edu/EPD/2013" xml:lang="de">Erneuerbare Primärenergie zur stofflichen Nutzung (PERM)</common:shortDescription>
      </referenceToFlowDataSet>
      <functionType>General reminder flow</functionType>
      <exchangeDirection>Input</exchangeDirection>
      <common:other xmlns:common="http://lca.jrc.it/ILCD/Common">
        <epd:amount xmlns:epd="http://www.iai.kit.edu/EPD/2013" epd:module="A1-A3">0</epd:amount>
        <epd:referenceToUnitGroupDataSet xmlns:epd="http://www.iai.kit.edu/EPD/2013" refObjectId="93a60a57-a3c8-11da-a746-0800200c9a66" version="03.00.000" type="unit group data set" uri="../unitgroups/93a60a57-a3c8-11da-a746-0800200c9a66.xml">
          <common:shortDescription xml:lang="en">MJ</common:shortDescription>
          <common:shortDescription xml:lang="de">MJ</common:shortDescription>
        </epd:referenceToUnitGroupDataSet>
        <epd:amount xmlns:epd="http://www.iai.kit.edu/EPD/2013" epd:module="C1">0</epd:amount>
        <epd:amount xmlns:epd="http://www.iai.kit.edu/EPD/2013" epd:module="C2">0</epd:amount>
        <epd:amount xmlns:epd="http://www.iai.kit.edu/EPD/2013" epd:module="D">0</epd:amount>
      </common:other>
    </exchange>
    <exchange dataSetInternalID="107071">
      <referenceToFlowDataSet refObjectId="53f97275-fa8a-4cdd-9024-65936002acd0" version="39.00.000" type="flow data set" uri="../flows/53f97275-fa8a-4cdd-9024-65936002acd0.xml">
        <common:shortDescription xmlns:common="http://lca.jrc.it/ILCD/Common" xmlns:epd="http://www.iai.kit.edu/EPD/2013" xml:lang="en">Total use of renewable primary energy resources (PERT)</common:shortDescription>
        <common:shortDescription xmlns:common="http://lca.jrc.it/ILCD/Common" xmlns:epd="http://www.iai.kit.edu/EPD/2013" xml:lang="de">Total erneuerbare Primärenergie (PERT)</common:shortDescription>
      </referenceToFlowDataSet>
      <functionType>General reminder flow</functionType>
      <exchangeDirection>Input</exchangeDirection>
      <common:other xmlns:common="http://lca.jrc.it/ILCD/Common">
        <epd:amount xmlns:epd="http://www.iai.kit.edu/EPD/2013" epd:module="A1-A3">3.14562210314066</epd:amount>
        <epd:referenceToUnitGroupDataSet xmlns:epd="http://www.iai.kit.edu/EPD/2013" refObjectId="93a60a57-a3c8-11da-a746-0800200c9a66" version="03.00.000" type="unit group data set" uri="../unitgroups/93a60a57-a3c8-11da-a746-0800200c9a66.xml">
          <common:shortDescription xml:lang="en">MJ</common:shortDescription>
          <common:shortDescription xml:lang="de">MJ</common:shortDescription>
        </epd:referenceToUnitGroupDataSet>
        <epd:amount xmlns:epd="http://www.iai.kit.edu/EPD/2013" epd:module="C1">0.000519248890445602</epd:amount>
        <epd:amount xmlns:epd="http://www.iai.kit.edu/EPD/2013" epd:module="C2">0.00199760029244171</epd:amount>
        <epd:amount xmlns:epd="http://www.iai.kit.edu/EPD/2013" epd:module="D">0.192416775537167</epd:amount>
      </common:other>
    </exchange>
    <exchange dataSetInternalID="107072">
      <referenceToFlowDataSet refObjectId="ac857178-2b45-46ec-892a-a9a4332f0372" version="39.00.000" type="flow data set" uri="../flows/ac857178-2b45-46ec-892a-a9a4332f0372.xml">
        <common:shortDescription xmlns:common="http://lca.jrc.it/ILCD/Common" xmlns:epd="http://www.iai.kit.edu/EPD/2013" xml:lang="en">Use of non-renewable primary energy (PENRE)</common:shortDescription>
        <common:shortDescription xmlns:common="http://lca.jrc.it/ILCD/Common" xmlns:epd="http://www.iai.kit.edu/EPD/2013" xml:lang="de">Nicht-erneuerbare Primärenergie als Energieträger (PENRE)</common:shortDescription>
      </referenceToFlowDataSet>
      <functionType>General reminder flow</functionType>
      <exchangeDirection>Input</exchangeDirection>
      <common:other xmlns:common="http://lca.jrc.it/ILCD/Common">
        <epd:amount xmlns:epd="http://www.iai.kit.edu/EPD/2013" epd:module="A1-A3">10.9902922094</epd:amount>
        <epd:referenceToUnitGroupDataSet xmlns:epd="http://www.iai.kit.edu/EPD/2013" refObjectId="93a60a57-a3c8-11da-a746-0800200c9a66" version="03.00.000" type="unit group data set" uri="../unitgroups/93a60a57-a3c8-11da-a746-0800200c9a66.xml">
          <common:shortDescription xml:lang="en">MJ</common:shortDescription>
          <common:shortDescription xml:lang="de">MJ</common:shortDescription>
        </epd:referenceToUnitGroupDataSet>
        <epd:amount xmlns:epd="http://www.iai.kit.edu/EPD/2013" epd:module="C1">0.00891934778251364</epd:amount>
        <epd:amount xmlns:epd="http://www.iai.kit.edu/EPD/2013" epd:module="C2">0.0343135865412218</epd:amount>
        <epd:amount xmlns:epd="http://www.iai.kit.edu/EPD/2013" epd:module="D">-1.68634991445539</epd:amount>
      </common:other>
    </exchange>
    <exchange dataSetInternalID="107073">
      <referenceToFlowDataSet refObjectId="1421caa0-679d-4bf4-b282-0eb850ccae27" version="39.00.000" type="flow data set" uri="../flows/1421caa0-679d-4bf4-b282-0eb850ccae27.xml">
        <common:shortDescription xmlns:common="http://lca.jrc.it/ILCD/Common" xmlns:epd="http://www.iai.kit.edu/EPD/2013" xml:lang="en">Non-renewable primary energy resources used as raw materials (PENRM)</common:shortDescription>
        <common:shortDescription xmlns:common="http://lca.jrc.it/ILCD/Common" xmlns:epd="http://www.iai.kit.edu/EPD/2013" xml:lang="de">Nicht-erneuerbare Primärenergie zur stofflichen Nutzung (PENRM)</common:shortDescription>
      </referenceToFlowDataSet>
      <functionType>General reminder flow</functionType>
      <exchangeDirection>Input</exchangeDirection>
      <common:other xmlns:common="http://lca.jrc.it/ILCD/Common">
        <epd:amount xmlns:epd="http://www.iai.kit.edu/EPD/2013" epd:module="A1-A3">0</epd:amount>
        <epd:referenceToUnitGroupDataSet xmlns:epd="http://www.iai.kit.edu/EPD/2013" refObjectId="93a60a57-a3c8-11da-a746-0800200c9a66" version="03.00.000" type="unit group data set" uri="../unitgroups/93a60a57-a3c8-11da-a746-0800200c9a66.xml">
          <common:shortDescription xml:lang="en">MJ</common:shortDescription>
          <common:shortDescription xml:lang="de">MJ</common:shortDescription>
        </epd:referenceToUnitGroupDataSet>
        <epd:amount xmlns:epd="http://www.iai.kit.edu/EPD/2013" epd:module="C1">0</epd:amount>
        <epd:amount xmlns:epd="http://www.iai.kit.edu/EPD/2013" epd:module="C2">0</epd:amount>
        <epd:amount xmlns:epd="http://www.iai.kit.edu/EPD/2013" epd:module="D">0</epd:amount>
      </common:other>
    </exchange>
    <exchange dataSetInternalID="107074">
      <referenceToFlowDataSet refObjectId="06159210-646b-4c8d-8583-da9b3b95a6c1" version="39.00.000" type="flow data set" uri="../flows/06159210-646b-4c8d-8583-da9b3b95a6c1.xml">
        <common:shortDescription xmlns:common="http://lca.jrc.it/ILCD/Common" xmlns:epd="http://www.iai.kit.edu/EPD/2013" xml:lang="en">Total use of non-renewable primary energy resources (PENRT)</common:shortDescription>
        <common:shortDescription xmlns:common="http://lca.jrc.it/ILCD/Common" xmlns:epd="http://www.iai.kit.edu/EPD/2013" xml:lang="de">Total nicht erneuerbare Primärenergie (PENRT)</common:shortDescription>
      </referenceToFlowDataSet>
      <functionType>General reminder flow</functionType>
      <exchangeDirection>Input</exchangeDirection>
      <common:other xmlns:common="http://lca.jrc.it/ILCD/Common">
        <epd:amount xmlns:epd="http://www.iai.kit.edu/EPD/2013" epd:module="A1-A3">10.9902922094</epd:amount>
        <epd:referenceToUnitGroupDataSet xmlns:epd="http://www.iai.kit.edu/EPD/2013" refObjectId="93a60a57-a3c8-11da-a746-0800200c9a66" version="03.00.000" type="unit group data set" uri="../unitgroups/93a60a57-a3c8-11da-a746-0800200c9a66.xml">
          <common:shortDescription xml:lang="en">MJ</common:shortDescription>
          <common:shortDescription xml:lang="de">MJ</common:shortDescription>
        </epd:referenceToUnitGroupDataSet>
        <epd:amount xmlns:epd="http://www.iai.kit.edu/EPD/2013" epd:module="C1">0.00891934778251364</epd:amount>
        <epd:amount xmlns:epd="http://www.iai.kit.edu/EPD/2013" epd:module="C2">0.0343135865412218</epd:amount>
        <epd:amount xmlns:epd="http://www.iai.kit.edu/EPD/2013" epd:module="D">-1.68634991445539</epd:amount>
      </common:other>
    </exchange>
    <exchange dataSetInternalID="107075">
      <referenceToFlowDataSet refObjectId="c6a1f35f-2d09-4f54-8dfb-97e502e1ce92" version="39.00.000" type="flow data set" uri="../flows/c6a1f35f-2d09-4f54-8dfb-97e502e1ce92.xml">
        <common:shortDescription xmlns:common="http://lca.jrc.it/ILCD/Common" xmlns:epd="http://www.iai.kit.edu/EPD/2013" xml:lang="en">Input of secondary material (SM)</common:shortDescription>
        <common:shortDescription xmlns:common="http://lca.jrc.it/ILCD/Common" xmlns:epd="http://www.iai.kit.edu/EPD/2013" xml:lang="de">Einsatz von Sekundärstoffen (SM)</common:shortDescription>
      </referenceToFlowDataSet>
      <functionType>General reminder flow</functionType>
      <exchangeDirection>Input</exchangeDirection>
      <common:other xmlns:common="http://lca.jrc.it/ILCD/Common">
        <epd:amount xmlns:epd="http://www.iai.kit.edu/EPD/2013" epd:module="A1-A3">0.971036</epd:amount>
        <epd:referenceToUnitGroupDataSet xmlns:epd="http://www.iai.kit.edu/EPD/2013" refObjectId="93a60a57-a4c8-11da-a746-0800200c9a66" version="03.00.000" type="unit group data set" uri="../unitgroups/93a60a57-a4c8-11da-a746-0800200c9a66.xml">
          <common:shortDescription xml:lang="en">kg</common:shortDescription>
          <common:shortDescription xml:lang="de">kg</common:shortDescription>
        </epd:referenceToUnitGroupDataSet>
        <epd:amount xmlns:epd="http://www.iai.kit.edu/EPD/2013" epd:module="C1">0</epd:amount>
        <epd:amount xmlns:epd="http://www.iai.kit.edu/EPD/2013" epd:module="C2">0</epd:amount>
        <epd:amount xmlns:epd="http://www.iai.kit.edu/EPD/2013" epd:module="D">0</epd:amount>
      </common:other>
    </exchange>
    <exchange dataSetInternalID="107076">
      <referenceToFlowDataSet refObjectId="64333088-a55f-4aa2-9a31-c10b07816787" version="39.00.000" type="flow data set" uri="../flows/64333088-a55f-4aa2-9a31-c10b07816787.xml">
        <common:shortDescription xmlns:common="http://lca.jrc.it/ILCD/Common" xmlns:epd="http://www.iai.kit.edu/EPD/2013" xml:lang="en">Use of renewable secondary fuels (RSF)</common:shortDescription>
        <common:shortDescription xmlns:common="http://lca.jrc.it/ILCD/Common" xmlns:epd="http://www.iai.kit.edu/EPD/2013" xml:lang="de">Erneuerbare Sekundärbrennstoffe (RSF)</common:shortDescription>
      </referenceToFlowDataSet>
      <functionType>General reminder flow</functionType>
      <exchangeDirection>Input</exchangeDirection>
      <common:other xmlns:common="http://lca.jrc.it/ILCD/Common">
        <epd:amount xmlns:epd="http://www.iai.kit.edu/EPD/2013" epd:module="A1-A3">0</epd:amount>
        <epd:referenceToUnitGroupDataSet xmlns:epd="http://www.iai.kit.edu/EPD/2013" refObjectId="93a60a57-a3c8-11da-a746-0800200c9a66" version="03.00.000" type="unit group data set" uri="../unitgroups/93a60a57-a3c8-11da-a746-0800200c9a66.xml">
          <common:shortDescription xml:lang="en">MJ</common:shortDescription>
          <common:shortDescription xml:lang="de">MJ</common:shortDescription>
        </epd:referenceToUnitGroupDataSet>
        <epd:amount xmlns:epd="http://www.iai.kit.edu/EPD/2013" epd:module="C1">0</epd:amount>
        <epd:amount xmlns:epd="http://www.iai.kit.edu/EPD/2013" epd:module="C2">0</epd:amount>
        <epd:amount xmlns:epd="http://www.iai.kit.edu/EPD/2013" epd:module="D">0</epd:amount>
      </common:other>
    </exchange>
    <exchange dataSetInternalID="107077">
      <referenceToFlowDataSet refObjectId="89def144-d39a-4287-b86f-efde453ddcb2" version="39.00.000" type="flow data set" uri="../flows/89def144-d39a-4287-b86f-efde453ddcb2.xml">
        <common:shortDescription xmlns:common="http://lca.jrc.it/ILCD/Common" xmlns:epd="http://www.iai.kit.edu/EPD/2013" xml:lang="en">Use of non renewable secondary fuels (NRSF)</common:shortDescription>
        <common:shortDescription xmlns:common="http://lca.jrc.it/ILCD/Common" xmlns:epd="http://www.iai.kit.edu/EPD/2013" xml:lang="de">Nicht erneuerbare Sekundärbrennstoffe (NRSF)</common:shortDescription>
      </referenceToFlowDataSet>
      <functionType>General reminder flow</functionType>
      <exchangeDirection>Input</exchangeDirection>
      <common:other xmlns:common="http://lca.jrc.it/ILCD/Common">
        <epd:amount xmlns:epd="http://www.iai.kit.edu/EPD/2013" epd:module="A1-A3">0</epd:amount>
        <epd:referenceToUnitGroupDataSet xmlns:epd="http://www.iai.kit.edu/EPD/2013" refObjectId="93a60a57-a3c8-11da-a746-0800200c9a66" version="03.00.000" type="unit group data set" uri="../unitgroups/93a60a57-a3c8-11da-a746-0800200c9a66.xml">
          <common:shortDescription xml:lang="en">MJ</common:shortDescription>
          <common:shortDescription xml:lang="de">MJ</common:shortDescription>
        </epd:referenceToUnitGroupDataSet>
        <epd:amount xmlns:epd="http://www.iai.kit.edu/EPD/2013" epd:module="C1">0</epd:amount>
        <epd:amount xmlns:epd="http://www.iai.kit.edu/EPD/2013" epd:module="C2">0</epd:amount>
        <epd:amount xmlns:epd="http://www.iai.kit.edu/EPD/2013" epd:module="D">0</epd:amount>
      </common:other>
    </exchange>
    <exchange dataSetInternalID="107078">
      <referenceToFlowDataSet refObjectId="3cf952c8-f3a4-461d-8c96-96456ca62246" version="39.00.000" type="flow data set" uri="../flows/3cf952c8-f3a4-461d-8c96-96456ca62246.xml">
        <common:shortDescription xmlns:common="http://lca.jrc.it/ILCD/Common" xmlns:epd="http://www.iai.kit.edu/EPD/2013" xml:lang="en">Use of net fresh water (FW)</common:shortDescription>
        <common:shortDescription xmlns:common="http://lca.jrc.it/ILCD/Common" xmlns:epd="http://www.iai.kit.edu/EPD/2013" xml:lang="de">Einsatz von Süßwasserressourcen (FW)</common:shortDescription>
      </referenceToFlowDataSet>
      <functionType>General reminder flow</functionType>
      <exchangeDirection>Input</exchangeDirection>
      <common:other xmlns:common="http://lca.jrc.it/ILCD/Common">
        <epd:amount xmlns:epd="http://www.iai.kit.edu/EPD/2013" epd:module="A1-A3">0.00231412893156495</epd:amount>
        <epd:referenceToUnitGroupDataSet xmlns:epd="http://www.iai.kit.edu/EPD/2013" refObjectId="93a60a57-a3c8-12da-a746-0800200c9a66" version="03.00.000" type="unit group data set" uri="../unitgroups/93a60a57-a3c8-12da-a746-0800200c9a66.xml">
          <common:shortDescription xml:lang="en">m3</common:shortDescription>
          <common:shortDescription xml:lang="de">m3</common:shortDescription>
        </epd:referenceToUnitGroupDataSet>
        <epd:amount xmlns:epd="http://www.iai.kit.edu/EPD/2013" epd:module="C1">4.65030955710469E-7</epd:amount>
        <epd:amount xmlns:epd="http://www.iai.kit.edu/EPD/2013" epd:module="C2">1.78901869645694E-6</epd:amount>
        <epd:amount xmlns:epd="http://www.iai.kit.edu/EPD/2013" epd:module="D">-0.000151911150893355</epd:amount>
      </common:other>
    </exchange>
    <exchange dataSetInternalID="107079">
      <referenceToFlowDataSet refObjectId="430f9e0f-59b2-46a0-8e0d-55e0e84948fc" version="39.00.000" type="flow data set" uri="../flows/430f9e0f-59b2-46a0-8e0d-55e0e84948fc.xml">
        <common:shortDescription xmlns:common="http://lca.jrc.it/ILCD/Common" xmlns:epd="http://www.iai.kit.edu/EPD/2013" xml:lang="en">Hazardous waste disposed (HWD)</common:shortDescription>
        <common:shortDescription xmlns:common="http://lca.jrc.it/ILCD/Common" xmlns:epd="http://www.iai.kit.edu/EPD/2013" xml:lang="de">Gefährlicher Abfall zur Deponie (HWD)</common:shortDescription>
      </referenceToFlowDataSet>
      <functionType>General reminder flow</functionType>
      <exchangeDirection>Output</exchangeDirection>
      <common:other xmlns:common="http://lca.jrc.it/ILCD/Common">
        <epd:amount xmlns:epd="http://www.iai.kit.edu/EPD/2013" epd:module="A1-A3">7.26498156120683E-9</epd:amount>
        <epd:referenceToUnitGroupDataSet xmlns:epd="http://www.iai.kit.edu/EPD/2013" refObjectId="93a60a57-a4c8-11da-a746-0800200c9a66" version="03.00.000" type="unit group data set" uri="../unitgroups/93a60a57-a4c8-11da-a746-0800200c9a66.xml">
          <common:shortDescription xml:lang="en">kg</common:shortDescription>
          <common:shortDescription xml:lang="de">kg</common:shortDescription>
        </epd:referenceToUnitGroupDataSet>
        <epd:amount xmlns:epd="http://www.iai.kit.edu/EPD/2013" epd:module="C1">3.33306723533077E-10</epd:amount>
        <epd:amount xmlns:epd="http://www.iai.kit.edu/EPD/2013" epd:module="C2">1.28226293912941E-9</epd:amount>
        <epd:amount xmlns:epd="http://www.iai.kit.edu/EPD/2013" epd:module="D">-1.42826244281399E-9</epd:amount>
      </common:other>
    </exchange>
    <exchange dataSetInternalID="107080">
      <referenceToFlowDataSet refObjectId="b29ef66b-e286-4afa-949f-62f1a7b4d7fa" version="39.00.000" type="flow data set" uri="../flows/b29ef66b-e286-4afa-949f-62f1a7b4d7fa.xml">
        <common:shortDescription xmlns:common="http://lca.jrc.it/ILCD/Common" xmlns:epd="http://www.iai.kit.edu/EPD/2013" xml:lang="en">Non-hazardous waste disposed (NHWD)</common:shortDescription>
        <common:shortDescription xmlns:common="http://lca.jrc.it/ILCD/Common" xmlns:epd="http://www.iai.kit.edu/EPD/2013" xml:lang="de">Entsorgter nicht gefährlicher Abfall (NHWD)</common:shortDescription>
      </referenceToFlowDataSet>
      <functionType>General reminder flow</functionType>
      <exchangeDirection>Output</exchangeDirection>
      <common:other xmlns:common="http://lca.jrc.it/ILCD/Common">
        <epd:amount xmlns:epd="http://www.iai.kit.edu/EPD/2013" epd:module="A1-A3">0.00693792511044756</epd:amount>
        <epd:referenceToUnitGroupDataSet xmlns:epd="http://www.iai.kit.edu/EPD/2013" refObjectId="93a60a57-a4c8-11da-a746-0800200c9a66" version="03.00.000" type="unit group data set" uri="../unitgroups/93a60a57-a4c8-11da-a746-0800200c9a66.xml">
          <common:shortDescription xml:lang="en">kg</common:shortDescription>
          <common:shortDescription xml:lang="de">kg</common:shortDescription>
        </epd:referenceToUnitGroupDataSet>
        <epd:amount xmlns:epd="http://www.iai.kit.edu/EPD/2013" epd:module="C1">1.5655014085986E-6</epd:amount>
        <epd:amount xmlns:epd="http://www.iai.kit.edu/EPD/2013" epd:module="C2">6.02263409547351E-6</epd:amount>
        <epd:amount xmlns:epd="http://www.iai.kit.edu/EPD/2013" epd:module="D">-0.00321158301521316</epd:amount>
      </common:other>
    </exchange>
    <exchange dataSetInternalID="107081">
      <referenceToFlowDataSet refObjectId="3449546e-52ad-4b39-b809-9fb77cea8ff6" version="39.00.000" type="flow data set" uri="../flows/3449546e-52ad-4b39-b809-9fb77cea8ff6.xml">
        <common:shortDescription xmlns:common="http://lca.jrc.it/ILCD/Common" xmlns:epd="http://www.iai.kit.edu/EPD/2013" xml:lang="en">Radioactive waste disposed (RWD)</common:shortDescription>
        <common:shortDescription xmlns:common="http://lca.jrc.it/ILCD/Common" xmlns:epd="http://www.iai.kit.edu/EPD/2013" xml:lang="de">Entsorgter radioaktiver Abfall (RWD)</common:shortDescription>
      </referenceToFlowDataSet>
      <functionType>General reminder flow</functionType>
      <exchangeDirection>Output</exchangeDirection>
      <common:other xmlns:common="http://lca.jrc.it/ILCD/Common">
        <epd:amount xmlns:epd="http://www.iai.kit.edu/EPD/2013" epd:module="A1-A3">0.000384148205341613</epd:amount>
        <epd:referenceToUnitGroupDataSet xmlns:epd="http://www.iai.kit.edu/EPD/2013" refObjectId="93a60a57-a4c8-11da-a746-0800200c9a66" version="03.00.000" type="unit group data set" uri="../unitgroups/93a60a57-a4c8-11da-a746-0800200c9a66.xml">
          <common:shortDescription xml:lang="en">kg</common:shortDescription>
          <common:shortDescription xml:lang="de">kg</common:shortDescription>
        </epd:referenceToUnitGroupDataSet>
        <epd:amount xmlns:epd="http://www.iai.kit.edu/EPD/2013" epd:module="C1">9.39024060164747E-9</epd:amount>
        <epd:amount xmlns:epd="http://www.iai.kit.edu/EPD/2013" epd:module="C2">3.61251563885896E-8</epd:amount>
        <epd:amount xmlns:epd="http://www.iai.kit.edu/EPD/2013" epd:module="D">3.05985038558626E-5</epd:amount>
      </common:other>
    </exchange>
    <exchange dataSetInternalID="107082">
      <referenceToFlowDataSet refObjectId="a2b32f97-3fc7-4af2-b209-525bc6426f33" version="39.00.000" type="flow data set" uri="../flows/a2b32f97-3fc7-4af2-b209-525bc6426f33.xml">
        <common:shortDescription xmlns:common="http://lca.jrc.it/ILCD/Common" xmlns:epd="http://www.iai.kit.edu/EPD/2013" xml:lang="en">Components for re-use (CRU)</common:shortDescription>
        <common:shortDescription xmlns:common="http://lca.jrc.it/ILCD/Common" xmlns:epd="http://www.iai.kit.edu/EPD/2013" xml:lang="de">Komponenten für die Wiederverwendung (CRU)</common:shortDescription>
      </referenceToFlowDataSet>
      <functionType>General reminder flow</functionType>
      <exchangeDirection>Output</exchangeDirection>
      <common:other xmlns:common="http://lca.jrc.it/ILCD/Common">
        <epd:amount xmlns:epd="http://www.iai.kit.edu/EPD/2013" epd:module="A1-A3">0</epd:amount>
        <epd:referenceToUnitGroupDataSet xmlns:epd="http://www.iai.kit.edu/EPD/2013" refObjectId="93a60a57-a4c8-11da-a746-0800200c9a66" version="03.00.000" type="unit group data set" uri="../unitgroups/93a60a57-a4c8-11da-a746-0800200c9a66.xml">
          <common:shortDescription xml:lang="en">kg</common:shortDescription>
          <common:shortDescription xml:lang="de">kg</common:shortDescription>
        </epd:referenceToUnitGroupDataSet>
        <epd:amount xmlns:epd="http://www.iai.kit.edu/EPD/2013" epd:module="C1">0</epd:amount>
        <epd:amount xmlns:epd="http://www.iai.kit.edu/EPD/2013" epd:module="C2">0</epd:amount>
        <epd:amount xmlns:epd="http://www.iai.kit.edu/EPD/2013" epd:module="D">0</epd:amount>
      </common:other>
    </exchange>
    <exchange dataSetInternalID="107083">
      <referenceToFlowDataSet refObjectId="d7fe48a5-4103-49c8-9aae-b0b5dfdbd6ae" version="39.00.000" type="flow data set" uri="../flows/d7fe48a5-4103-49c8-9aae-b0b5dfdbd6ae.xml">
        <common:shortDescription xmlns:common="http://lca.jrc.it/ILCD/Common" xmlns:epd="http://www.iai.kit.edu/EPD/2013" xml:lang="en">Materials for Recycling (MFR)</common:shortDescription>
        <common:shortDescription xmlns:common="http://lca.jrc.it/ILCD/Common" xmlns:epd="http://www.iai.kit.edu/EPD/2013" xml:lang="de">Stoffe zum Recycling (MFR)</common:shortDescription>
      </referenceToFlowDataSet>
      <functionType>General reminder flow</functionType>
      <exchangeDirection>Output</exchangeDirection>
      <common:other xmlns:common="http://lca.jrc.it/ILCD/Common">
        <epd:amount xmlns:epd="http://www.iai.kit.edu/EPD/2013" epd:module="A1-A3">0</epd:amount>
        <epd:referenceToUnitGroupDataSet xmlns:epd="http://www.iai.kit.edu/EPD/2013" refObjectId="93a60a57-a4c8-11da-a746-0800200c9a66" version="03.00.000" type="unit group data set" uri="../unitgroups/93a60a57-a4c8-11da-a746-0800200c9a66.xml">
          <common:shortDescription xml:lang="en">kg</common:shortDescription>
          <common:shortDescription xml:lang="de">kg</common:shortDescription>
        </epd:referenceToUnitGroupDataSet>
        <epd:amount xmlns:epd="http://www.iai.kit.edu/EPD/2013" epd:module="C1">1.1</epd:amount>
        <epd:amount xmlns:epd="http://www.iai.kit.edu/EPD/2013" epd:module="C2">0</epd:amount>
        <epd:amount xmlns:epd="http://www.iai.kit.edu/EPD/2013" epd:module="D">0</epd:amount>
      </common:other>
    </exchange>
    <exchange dataSetInternalID="107084">
      <referenceToFlowDataSet refObjectId="59a9181c-3aaf-46ee-8b13-2b3723b6e447" version="39.00.000" type="flow data set" uri="../flows/59a9181c-3aaf-46ee-8b13-2b3723b6e447.xml">
        <common:shortDescription xmlns:common="http://lca.jrc.it/ILCD/Common" xmlns:epd="http://www.iai.kit.edu/EPD/2013" xml:lang="en">Material for Energy Recovery (MER)</common:shortDescription>
        <common:shortDescription xmlns:common="http://lca.jrc.it/ILCD/Common" xmlns:epd="http://www.iai.kit.edu/EPD/2013" xml:lang="de">Stoffe für die Energierückgewinnung (MER)</common:shortDescription>
      </referenceToFlowDataSet>
      <functionType>General reminder flow</functionType>
      <exchangeDirection>Output</exchangeDirection>
      <common:other xmlns:common="http://lca.jrc.it/ILCD/Common">
        <epd:amount xmlns:epd="http://www.iai.kit.edu/EPD/2013" epd:module="A1-A3">0</epd:amount>
        <epd:referenceToUnitGroupDataSet xmlns:epd="http://www.iai.kit.edu/EPD/2013" refObjectId="93a60a57-a4c8-11da-a746-0800200c9a66" version="03.00.000" type="unit group data set" uri="../unitgroups/93a60a57-a4c8-11da-a746-0800200c9a66.xml">
          <common:shortDescription xml:lang="en">kg</common:shortDescription>
          <common:shortDescription xml:lang="de">kg</common:shortDescription>
        </epd:referenceToUnitGroupDataSet>
        <epd:amount xmlns:epd="http://www.iai.kit.edu/EPD/2013" epd:module="C1">0</epd:amount>
        <epd:amount xmlns:epd="http://www.iai.kit.edu/EPD/2013" epd:module="C2">0</epd:amount>
        <epd:amount xmlns:epd="http://www.iai.kit.edu/EPD/2013" epd:module="D">0</epd:amount>
      </common:other>
    </exchange>
    <exchange dataSetInternalID="107085">
      <referenceToFlowDataSet refObjectId="4da0c987-2b76-40d6-9e9e-82a017aaaf29" version="39.00.000" type="flow data set" uri="../flows/4da0c987-2b76-40d6-9e9e-82a017aaaf29.xml">
        <common:shortDescription xmlns:common="http://lca.jrc.it/ILCD/Common" xmlns:epd="http://www.iai.kit.edu/EPD/2013" xml:lang="en">Exported electrical energy (EEE)</common:shortDescription>
        <common:shortDescription xmlns:common="http://lca.jrc.it/ILCD/Common" xmlns:epd="http://www.iai.kit.edu/EPD/2013" xml:lang="de">Exportierte elektrische Energie (EEE)</common:shortDescription>
      </referenceToFlowDataSet>
      <functionType>General reminder flow</functionType>
      <exchangeDirection>Output</exchangeDirection>
      <common:other xmlns:common="http://lca.jrc.it/ILCD/Common">
        <epd:amount xmlns:epd="http://www.iai.kit.edu/EPD/2013" epd:module="A1-A3">0</epd:amount>
        <epd:referenceToUnitGroupDataSet xmlns:epd="http://www.iai.kit.edu/EPD/2013" refObjectId="93a60a57-a3c8-11da-a746-0800200c9a66" version="03.00.000" type="unit group data set" uri="../unitgroups/93a60a57-a3c8-11da-a746-0800200c9a66.xml">
          <common:shortDescription xml:lang="en">MJ</common:shortDescription>
          <common:shortDescription xml:lang="de">MJ</common:shortDescription>
        </epd:referenceToUnitGroupDataSet>
        <epd:amount xmlns:epd="http://www.iai.kit.edu/EPD/2013" epd:module="C1">0</epd:amount>
        <epd:amount xmlns:epd="http://www.iai.kit.edu/EPD/2013" epd:module="C2">0</epd:amount>
        <epd:amount xmlns:epd="http://www.iai.kit.edu/EPD/2013" epd:module="D">0</epd:amount>
      </common:other>
    </exchange>
    <exchange dataSetInternalID="107086">
      <referenceToFlowDataSet refObjectId="98daf38a-7a79-46d3-9a37-2b7bd0955810" version="39.00.000" type="flow data set" uri="../flows/98daf38a-7a79-46d3-9a37-2b7bd0955810.xml">
        <common:shortDescription xmlns:common="http://lca.jrc.it/ILCD/Common" xmlns:epd="http://www.iai.kit.edu/EPD/2013" xml:lang="en">Exported thermal energy (EET)</common:shortDescription>
        <common:shortDescription xmlns:common="http://lca.jrc.it/ILCD/Common" xmlns:epd="http://www.iai.kit.edu/EPD/2013" xml:lang="de">Exportierte thermische Energie (EET)</common:shortDescription>
      </referenceToFlowDataSet>
      <functionType>General reminder flow</functionType>
      <exchangeDirection>Output</exchangeDirection>
      <common:other xmlns:common="http://lca.jrc.it/ILCD/Common">
        <epd:amount xmlns:epd="http://www.iai.kit.edu/EPD/2013" epd:module="A1-A3">0</epd:amount>
        <epd:referenceToUnitGroupDataSet xmlns:epd="http://www.iai.kit.edu/EPD/2013" refObjectId="93a60a57-a3c8-11da-a746-0800200c9a66" version="03.00.000" type="unit group data set" uri="../unitgroups/93a60a57-a3c8-11da-a746-0800200c9a66.xml">
          <common:shortDescription xml:lang="en">MJ</common:shortDescription>
          <common:shortDescription xml:lang="de">MJ</common:shortDescription>
        </epd:referenceToUnitGroupDataSet>
        <epd:amount xmlns:epd="http://www.iai.kit.edu/EPD/2013" epd:module="C1">0</epd:amount>
        <epd:amount xmlns:epd="http://www.iai.kit.edu/EPD/2013" epd:module="C2">0</epd:amount>
        <epd:amount xmlns:epd="http://www.iai.kit.edu/EPD/2013" epd:module="D">0</epd:amount>
      </common:other>
    </exchange>
  </exchanges>
  <LCIAResults>
    <LCIAResult>
      <referenceToLCIAMethodDataSet refObjectId="77e416eb-a363-4258-a04e-171d843a6460" version="39.00.000" type="LCIA method data set" uri="../lciamethods/77e416eb-a363-4258-a04e-171d843a6460.xml">
        <common:shortDescription xmlns:common="http://lca.jrc.it/ILCD/Common" xmlns:epd="http://www.iai.kit.edu/EPD/2013" xml:lang="en">Global warming potential (GWP)</common:shortDescription>
        <common:shortDescription xmlns:common="http://lca.jrc.it/ILCD/Common" xmlns:epd="http://www.iai.kit.edu/EPD/2013" xml:lang="de">Globales Erwärmungspotenzial (GWP)</common:shortDescription>
      </referenceToLCIAMethodDataSet>
      <common:other xmlns:common="http://lca.jrc.it/ILCD/Common">
        <epd:amount xmlns:epd="http://www.iai.kit.edu/EPD/2013" epd:module="A1-A3">0.994443589117387</epd:amount>
        <epd:amount xmlns:epd="http://www.iai.kit.edu/EPD/2013" epd:module="C1">0.000658964671800686</epd:amount>
        <epd:amount xmlns:epd="http://www.iai.kit.edu/EPD/2013" epd:module="C2">0.00255297347747473</epd:amount>
        <epd:amount xmlns:epd="http://www.iai.kit.edu/EPD/2013" epd:module="D">-0.222992169057188</epd:amount>
        <epd:referenceToUnitGroupDataSet xmlns:epd="http://www.iai.kit.edu/EPD/2013" refObjectId="1ebf3012-d0db-4de2-aefd-ef30cedb0be1" version="39.00.000" type="unit group data set" uri="../unitgroups/1ebf3012-d0db-4de2-aefd-ef30cedb0be1.xml">
          <common:shortDescription xml:lang="en">kg CO2 eq.</common:shortDescription>
          <common:shortDescription xml:lang="de">kg CO2 Äquiv.</common:shortDescription>
        </epd:referenceToUnitGroupDataSet>
      </common:other>
    </LCIAResult>
    <LCIAResult>
      <referenceToLCIAMethodDataSet refObjectId="06dcd26f-025f-401a-a7c1-5e457eb54637" version="39.00.000" type="LCIA method data set" uri="../lciamethods/06dcd26f-025f-401a-a7c1-5e457eb54637.xml">
        <common:shortDescription xmlns:common="http://lca.jrc.it/ILCD/Common" xmlns:epd="http://www.iai.kit.edu/EPD/2013" xml:lang="en">Ozone Depletion Potential (ODP)</common:shortDescription>
        <common:shortDescription xmlns:common="http://lca.jrc.it/ILCD/Common" xmlns:epd="http://www.iai.kit.edu/EPD/2013" xml:lang="de">Abbaupotenzial der stratosphärischen Ozonschicht (ODP)</common:shortDescription>
      </referenceToLCIAMethodDataSet>
      <common:other xmlns:common="http://lca.jrc.it/ILCD/Common">
        <epd:amount xmlns:epd="http://www.iai.kit.edu/EPD/2013" epd:module="A1-A3">1.69162677960518E-14</epd:amount>
        <epd:amount xmlns:epd="http://www.iai.kit.edu/EPD/2013" epd:module="C1">2.19657716694803E-19</epd:amount>
        <epd:amount xmlns:epd="http://www.iai.kit.edu/EPD/2013" epd:module="C2">8.45044307615301E-19</epd:amount>
        <epd:amount xmlns:epd="http://www.iai.kit.edu/EPD/2013" epd:module="D">1.36978564100407E-15</epd:amount>
        <epd:referenceToUnitGroupDataSet xmlns:epd="http://www.iai.kit.edu/EPD/2013" refObjectId="88054749-b0a6-47ea-a82b-dc5b29326512" version="39.00.000" type="unit group data set" uri="../unitgroups/88054749-b0a6-47ea-a82b-dc5b29326512.xml">
          <common:shortDescription xml:lang="en">kg R11 eq.</common:shortDescription>
          <common:shortDescription xml:lang="de">kg R11 Äquiv.</common:shortDescription>
        </epd:referenceToUnitGroupDataSet>
      </common:other>
    </LCIAResult>
    <LCIAResult>
      <referenceToLCIAMethodDataSet refObjectId="b4274add-93b7-4905-a5e4-2e878c4e4216" version="39.00.000" type="LCIA method data set" uri="../lciamethods/b4274add-93b7-4905-a5e4-2e878c4e4216.xml">
        <common:shortDescription xmlns:common="http://lca.jrc.it/ILCD/Common" xmlns:epd="http://www.iai.kit.edu/EPD/2013" xml:lang="en">Acidification potential (AP)</common:shortDescription>
        <common:shortDescription xmlns:common="http://lca.jrc.it/ILCD/Common" xmlns:epd="http://www.iai.kit.edu/EPD/2013" xml:lang="de">Versauerungspotential (AP)</common:shortDescription>
      </referenceToLCIAMethodDataSet>
      <common:other xmlns:common="http://lca.jrc.it/ILCD/Common">
        <epd:amount xmlns:epd="http://www.iai.kit.edu/EPD/2013" epd:module="A1-A3">0.0019496923322709</epd:amount>
        <epd:amount xmlns:epd="http://www.iai.kit.edu/EPD/2013" epd:module="C1">2.29843319714164E-6</epd:amount>
        <epd:amount xmlns:epd="http://www.iai.kit.edu/EPD/2013" epd:module="C2">5.1567312651439E-6</epd:amount>
        <epd:amount xmlns:epd="http://www.iai.kit.edu/EPD/2013" epd:module="D">-0.000514369885866408</epd:amount>
        <epd:referenceToUnitGroupDataSet xmlns:epd="http://www.iai.kit.edu/EPD/2013" refObjectId="bc50c624-a9bc-45b1-a9b0-e6b10d00476f" version="39.00.000" type="unit group data set" uri="../unitgroups/bc50c624-a9bc-45b1-a9b0-e6b10d00476f.xml">
          <common:shortDescription xml:lang="en">kg SO2 eq.</common:shortDescription>
          <common:shortDescription xml:lang="de">kg SO2 Äquiv.</common:shortDescription>
        </epd:referenceToUnitGroupDataSet>
      </common:other>
    </LCIAResult>
    <LCIAResult>
      <referenceToLCIAMethodDataSet refObjectId="f58827d0-b407-4ec6-be75-8b69efb98a0f" version="39.00.000" type="LCIA method data set" uri="../lciamethods/f58827d0-b407-4ec6-be75-8b69efb98a0f.xml">
        <common:shortDescription xmlns:common="http://lca.jrc.it/ILCD/Common" xmlns:epd="http://www.iai.kit.edu/EPD/2013" xml:lang="en">Eutrophication potential (EP)</common:shortDescription>
        <common:shortDescription xmlns:common="http://lca.jrc.it/ILCD/Common" xmlns:epd="http://www.iai.kit.edu/EPD/2013" xml:lang="de">Eutrophierungspotential (EP)</common:shortDescription>
      </referenceToLCIAMethodDataSet>
      <common:other xmlns:common="http://lca.jrc.it/ILCD/Common">
        <epd:amount xmlns:epd="http://www.iai.kit.edu/EPD/2013" epd:module="A1-A3">0.000219206765157236</epd:amount>
        <epd:amount xmlns:epd="http://www.iai.kit.edu/EPD/2013" epd:module="C1">5.42304434103147E-7</epd:amount>
        <epd:amount xmlns:epd="http://www.iai.kit.edu/EPD/2013" epd:module="C2">1.22589758816209E-6</epd:amount>
        <epd:amount xmlns:epd="http://www.iai.kit.edu/EPD/2013" epd:module="D">-4.27274870157544E-5</epd:amount>
        <epd:referenceToUnitGroupDataSet xmlns:epd="http://www.iai.kit.edu/EPD/2013" refObjectId="67b5401d-873c-485f-bcf3-6ae83b918822" version="39.00.000" type="unit group data set" uri="../unitgroups/67b5401d-873c-485f-bcf3-6ae83b918822.xml">
          <common:shortDescription xml:lang="en">kg Phosphate eq.</common:shortDescription>
          <common:shortDescription xml:lang="de">kg Phosphat Äquiv.</common:shortDescription>
        </epd:referenceToUnitGroupDataSet>
      </common:other>
    </LCIAResult>
    <LCIAResult>
      <referenceToLCIAMethodDataSet refObjectId="1e84a202-dae6-42aa-9e9d-71ea48b8be00" version="39.00.000" type="LCIA method data set" uri="../lciamethods/1e84a202-dae6-42aa-9e9d-71ea48b8be00.xml">
        <common:shortDescription xmlns:common="http://lca.jrc.it/ILCD/Common" xmlns:epd="http://www.iai.kit.edu/EPD/2013" xml:lang="en">Photochemical Ozone Creation Potential (POCP)</common:shortDescription>
        <common:shortDescription xmlns:common="http://lca.jrc.it/ILCD/Common" xmlns:epd="http://www.iai.kit.edu/EPD/2013" xml:lang="de">Bildungspotenzial für troposphärisches Ozon (POCP)</common:shortDescription>
      </referenceToLCIAMethodDataSet>
      <common:other xmlns:common="http://lca.jrc.it/ILCD/Common">
        <epd:amount xmlns:epd="http://www.iai.kit.edu/EPD/2013" epd:module="A1-A3">0.000352839723041945</epd:amount>
        <epd:amount xmlns:epd="http://www.iai.kit.edu/EPD/2013" epd:module="C1">2.27108939579174E-7</epd:amount>
        <epd:amount xmlns:epd="http://www.iai.kit.edu/EPD/2013" epd:module="C2">-1.68540460474931E-6</epd:amount>
        <epd:amount xmlns:epd="http://www.iai.kit.edu/EPD/2013" epd:module="D">-6.71773402349625E-5</epd:amount>
        <epd:referenceToUnitGroupDataSet xmlns:epd="http://www.iai.kit.edu/EPD/2013" refObjectId="01c26c17-9a76-406e-8295-f17b55fd909e" version="39.00.000" type="unit group data set" uri="../unitgroups/01c26c17-9a76-406e-8295-f17b55fd909e.xml">
          <common:shortDescription xml:lang="en">kg Ethene eq.</common:shortDescription>
          <common:shortDescription xml:lang="de">kg Ethen Äquiv.</common:shortDescription>
        </epd:referenceToUnitGroupDataSet>
      </common:other>
    </LCIAResult>
    <LCIAResult>
      <referenceToLCIAMethodDataSet refObjectId="f7c73bb9-ab1a-4249-9c6d-379a0de6f67e" version="39.00.000" type="LCIA method data set" uri="../lciamethods/f7c73bb9-ab1a-4249-9c6d-379a0de6f67e.xml">
        <common:shortDescription xmlns:common="http://lca.jrc.it/ILCD/Common" xmlns:epd="http://www.iai.kit.edu/EPD/2013" xml:lang="en">Abiotic depletion potential for non fossil resources (ADPE)</common:shortDescription>
        <common:shortDescription xmlns:common="http://lca.jrc.it/ILCD/Common" xmlns:epd="http://www.iai.kit.edu/EPD/2013" xml:lang="de">Potenzial für den abiotischen Abbau nicht fossiler Ressourcen (ADPE)</common:shortDescription>
      </referenceToLCIAMethodDataSet>
      <common:other xmlns:common="http://lca.jrc.it/ILCD/Common">
        <epd:amount xmlns:epd="http://www.iai.kit.edu/EPD/2013" epd:module="A1-A3">2.01492953640174E-7</epd:amount>
        <epd:amount xmlns:epd="http://www.iai.kit.edu/EPD/2013" epd:module="C1">5.58433864818246E-11</epd:amount>
        <epd:amount xmlns:epd="http://www.iai.kit.edu/EPD/2013" epd:module="C2">2.14834864781892E-10</epd:amount>
        <epd:amount xmlns:epd="http://www.iai.kit.edu/EPD/2013" epd:module="D">5.30754726861462E-9</epd:amount>
        <epd:referenceToUnitGroupDataSet xmlns:epd="http://www.iai.kit.edu/EPD/2013" refObjectId="54ccd2d9-a32a-4fc2-923d-f2c8c93e89d4" version="39.00.000" type="unit group data set" uri="../unitgroups/54ccd2d9-a32a-4fc2-923d-f2c8c93e89d4.xml">
          <common:shortDescription xml:lang="en">kg Sb eq.</common:shortDescription>
          <common:shortDescription xml:lang="de">kg Sb Äquiv.</common:shortDescription>
        </epd:referenceToUnitGroupDataSet>
      </common:other>
    </LCIAResult>
    <LCIAResult>
      <referenceToLCIAMethodDataSet refObjectId="804ebcdf-309d-4098-8ed8-fdaf2f389981" version="39.00.000" type="LCIA method data set" uri="../lciamethods/804ebcdf-309d-4098-8ed8-fdaf2f389981.xml">
        <common:shortDescription xmlns:common="http://lca.jrc.it/ILCD/Common" xmlns:epd="http://www.iai.kit.edu/EPD/2013" xml:lang="en">Abiotic depletion potential for fossil resources (ADPF)</common:shortDescription>
        <common:shortDescription xmlns:common="http://lca.jrc.it/ILCD/Common" xmlns:epd="http://www.iai.kit.edu/EPD/2013" xml:lang="de">Potenzial für den abiotischen Abbau fossiler Brennstoffe (ADPF)</common:shortDescription>
      </referenceToLCIAMethodDataSet>
      <common:other xmlns:common="http://lca.jrc.it/ILCD/Common">
        <epd:amount xmlns:epd="http://www.iai.kit.edu/EPD/2013" epd:module="A1-A3">10.0204089386643</epd:amount>
        <epd:amount xmlns:epd="http://www.iai.kit.edu/EPD/2013" epd:module="C1">0.00889534856136612</epd:amount>
        <epd:amount xmlns:epd="http://www.iai.kit.edu/EPD/2013" epd:module="C2">0.034221259235252</epd:amount>
        <epd:amount xmlns:epd="http://www.iai.kit.edu/EPD/2013" epd:module="D">-1.76385661905841</epd:amount>
        <epd:referenceToUnitGroupDataSet xmlns:epd="http://www.iai.kit.edu/EPD/2013" refObjectId="93a60a57-a3c8-11da-a746-0800200c9a66" version="03.00.000" type="unit group data set" uri="../unitgroups/93a60a57-a3c8-11da-a746-0800200c9a66.xml">
          <common:shortDescription xml:lang="en">MJ</common:shortDescription>
          <common:shortDescription xml:lang="de">MJ</common:shortDescription>
        </epd:referenceToUnitGroupDataSet>
      </common:other>
    </LCIAResult>
  </LCIAResults>
</processDataSet>