<?xml version="1.0" encoding="UTF-8" standalone="yes"?>
<processDataSet xmlns:m="http://lca.jrc.it/ILCD/LCIAMethod" xmlns:common="http://lca.jrc.it/ILCD/Common" xmlns:s="http://lca.jrc.it/ILCD/Source" xmlns:c="http://lca.jrc.it/ILCD/Contact" xmlns:f="http://lca.jrc.it/ILCD/Flow" xmlns="http://lca.jrc.it/ILCD/Process" xmlns:fp="http://lca.jrc.it/ILCD/FlowProperty" xmlns:u="http://lca.jrc.it/ILCD/UnitGroup" xmlns:ns9="http://www.okworx.com/ILCD/Extensions/2018/Profile" xmlns:epd2="http://www.indata.network/EPD/2019" version="1.1" ns9:profile="EN_15804" epd2:epd-version="1.2">
    <processInformation>
        <dataSetInformation>
            <common:UUID>3ffff149-0e31-47e9-a411-b406daf75394</common:UUID>
            <name>
                <baseName xml:lang="de">Tor - Theo Schröders Entwicklung &amp; Beratung GmbH - Feuerschutz-Schiebetore</baseName>
                <baseName xml:lang="en">Door - Theo Schröders Entwicklung &amp; Beratung GmbH - Sliding fire doors</baseName>
            </name>
            <common:synonyms xml:lang="de">Rauchschutz-Schiebetor; Teleskopschiebetor; Rauchschutztor; Mehrzwecktor; ST-11; ST-12; TST-11; TST-12; ST-1; ST-2; TST-1; TST-2; RST-1; RST-2; MST-1; MST-2</common:synonyms>
            <common:synonyms xml:lang="en">Smoke protection sliding door; fire protection sliding door; Telescopic sliding door; Smoke protection door; Multi-purpose door; ST-11; ST-12; TST-11; TST-12; ST-1; ST-2; TST-1; TST-2; RST-1; RST-2; MST-1; MST-2</common:synonyms>
            <classificationInformation>
                <common:classification name="OEKOBAU.DAT">
                    <common:class level="0" classId="7">Komponenten von Fenstern und Vorhangfassaden</common:class>
                    <common:class level="1" classId="7.6">Türen und Tore</common:class>
                    <common:class level="2" classId="7.6.01">Stahl</common:class>
                </common:classification>
            </classificationInformation>
            <common:generalComment xml:lang="de">Dieser Datensatz beinhaltet die Ergebnisse für die Module A1-A3 sowie die Module B2, B3, B4, B5, B6, B7, C1, C2, C3, C4, und D gemäß EN 15804. Ein Vergleich mit anderen Produkten ist nur mit einer vergleichbaren Anwendung im Gebäude zulässig. Grundsätzlich ist eine Gegenüberstellung oder die Bewertung von EPD Daten nur möglich, wenn alle zu vergleichenden Datensätze nach EN 15804 erstellt wurden und der Gebäudekontext, bzw. die produktspezifischen Leistungsmerkmale berücksichtigt werden.</common:generalComment>
            <common:generalComment xml:lang="en">This data set contains the results for modules A1-A3 as well as modules B2, B3, B4, B5, B6, B7, C1, C2, C3, C4, and D according to EN 15804. A comparison with other products is only permissible with a comparable application in the building. In principle, a comparison or the evaluation of EPD data is only possible if all data sets to be compared were created according to EN 15804 and the building context or the product-specific performance characteristics are taken into account.</common:generalComment>
        </dataSetInformation>
        <quantitativeReference type="Reference flow(s)">
            <referenceToReferenceFlow>1</referenceToReferenceFlow>
        </quantitativeReference>
        <time>
            <common:referenceYear>2020</common:referenceYear>
            <common:dataSetValidUntil>2026</common:dataSetValidUntil>
            <common:timeRepresentativenessDescription xml:lang="de">jährlicher Durchschnitt</common:timeRepresentativenessDescription>
            <common:timeRepresentativenessDescription xml:lang="en">anual average</common:timeRepresentativenessDescription>
            <common:other>
                <epd2:publicationDateOfEPD>2021-08-10</epd2:publicationDateOfEPD>
            </common:other>
        </time>
        <geography>
            <locationOfOperationSupplyOrProduction location="RER">
                <descriptionOfRestrictions xml:lang="de">Dieser Datensatz repräsentiert die Situation von Unternehmen, die Produkte entsprechend den Systemen von System Schröders produzieren, im Hinblick auf die wichtigsten Technologien und die gesetzlichen Rahmenbedingungen.</descriptionOfRestrictions>
                <descriptionOfRestrictions xml:lang="en">This dataset represents the situation of companies producing products according to System Schröders' systems with regard to the most important technologies and the legal framework.</descriptionOfRestrictions>
            </locationOfOperationSupplyOrProduction>
        </geography>
        <technology>
            <technologyDescriptionAndIncludedProcesses xml:lang="de">Die Ökobilanzergebnisse umfassen die Lebenszyklusstadien der Herstellung der Vorprodukte bis hin zur Rohstoffgewinnung und Verarbeitungsprozesse von als Input dienenden Sekundärstoffen (z.B. Recyclingprozesse), deren Transporte zum Werk sowie die Produktion selbst, einschließlich der Bereitstellung von allen Hilfs- und Betriebsstoffen, Energie, sowie die vollständige Abfallbehandlung oder die Deponierung der Restabfälle während des Stadiums der Produktion. Die Module A1, A2 und A3 sind hier als ein aggregiertes Modul A1-A3 ausgewiesen. Falls für diesen Datensatz weitere Module berechnet wurden, sind diese separat zu finden und können für eine Betrachtung des gesamten Lebenszyklus zusammengeführt werden.</technologyDescriptionAndIncludedProcesses>
            <technologyDescriptionAndIncludedProcesses xml:lang="en">The LCA results cover the life cycle stages of the manufacture of intermediate products up to raw material extraction and processing operations of secondary materials serving as input (e.g. recycling processes), their transports to the plant as well as the production itself, including the provision of all auxiliary and operating materials, energy, and the complete waste treatment or landfilling of residual waste during the stage of production. Modules A1, A2, and A3 are shown here as one aggregated module A1-A3. If further modules were calculated for this data set, they can be found separately and can be combined for a consideration of the entire life cycle.&#13;
&#13;
</technologyDescriptionAndIncludedProcesses>
            <technologicalApplicability xml:lang="de">Innen- und Außenbereich.</technologicalApplicability>
            <technologicalApplicability xml:lang="en">Indoor and outdoor.</technologicalApplicability>
        </technology>
    </processInformation>
    <modellingAndValidation>
        <LCIMethodAndAllocation>
            <typeOfDataSet>EPD</typeOfDataSet>
            <referenceToLCAMethodDetails type="source data set" refObjectId="c6e986be-62a9-4f2f-b486-27aa9129eaeb" version="00.00.002">
                <common:shortDescription xml:lang="de">Produktkategorieregeln Teil A</common:shortDescription>
            </referenceToLCAMethodDetails>
            <referenceToLCAMethodDetails type="source data set" refObjectId="673a73ac-5e03-4cd7-bdff-03be304bdf5a" version="00.00.001">
                <common:shortDescription xml:lang="de">Produktkategorieregeln Teil B – für Türen und Tore</common:shortDescription>
            </referenceToLCAMethodDetails>
            <referenceToLCAMethodDetails type="source data set" refObjectId="e584ff64-c11b-40e5-9979-6d93ed8caa0a" version="00.00.001">
                <common:shortDescription xml:lang="de">EPD Türen, Tore und Klappen aus Stahl des System Schröders</common:shortDescription>
            </referenceToLCAMethodDetails>
            <common:other>
                <epd:subType xmlns:epd="http://www.iai.kit.edu/EPD/2013">template dataset</epd:subType>
            </common:other>
        </LCIMethodAndAllocation>
        <dataSourcesTreatmentAndRepresentativeness>
            <referenceToDataSource type="source data set" refObjectId="28d74cc0-db8b-4d7e-bc44-5f6d56ce0c4a" version="00.03.002">
                <common:shortDescription xml:lang="en">GaBi database (general)</common:shortDescription>
            </referenceToDataSource>
            <useAdviceForDataSet xml:lang="de">Dieser Datensatz beinhaltet die Ergebnisse für die Module A1-A3 sowie die Module A4, A5, B2, B3, B4, B5, B6, B7, C1, C2, C3, C4, D gemäß EN 15804.&#13;
Ein Vergleich mit anderen Produkten ist nur mit einer vergleichbaren Anwendung im Gebäude zulässig. Grundsätzlich ist eine Gegenüberstellung oder die Bewertung von EPD Daten nur möglich, wenn alle zu vergleichenden Datensätze nach EN 15804 erstellt wurden und der Gebäudekontext, bzw. die produktspezifischen Leistungsmerkmale berücksichtigt werden.&#13;
&#13;
Die Muster-EPD erlangt Gültigkeit durch die Übertragung an den Hersteller durch das ift. Aktuell gültige EPDs sind der nachfolgenden Liste zu entehmen und auf www.ift-service.de/epd veröffentlicht.&#13;
EPD-Nummer und Deklarationsinhaber:&#13;
- -	M-EPD-TTS-102&#13;
HODAPP GmbH &amp; Co. KG&#13;
Großweierer Str.77&#13;
77855 Achern&#13;
-	M-EPD-TTS-103&#13;
MTS Brandschutzsysteme GmbH&#13;
Bruchweg 3&#13;
14550 Groß Kreutz&#13;
-	M-EPD-TTS-104&#13;
Wiedemann GmbH&#13;
Siemensstr.16-18&#13;
25813 Husum&#13;
- M-EPD-TTS-105, Metall- u. Anlagenbau Erfurt GmbH, 99091 Erfurt&#13;
- M-EPD-TTS-106, Körner Stahltore GmbH &amp; Co. KG, 21335 Lüneburg-Oedeme&#13;
- M-EPD-TTS-107, Georg Brüggemann GmbH, 59757 Arnsberg&#13;
- M-EPD-TTS-108, Metallbau Ebeling GmbH, 31699 Reckedorf</useAdviceForDataSet>
            <useAdviceForDataSet xml:lang="en">This data set includes the results for modules A1-A3 as well as modules A4, A5, B2, B3, B4, B5, B6, B7, C1, C2, C3, C4, D according to EN 15804.&#13;
A comparison with other products is only permissible with a comparable application in the building. In principle, a comparison or the evaluation of EPD data is only possible if all data sets to be compared were created according to EN 15804 and the building context, or the product-specific performance characteristics are taken into account.&#13;&#13;
&#13;&#13;
&#13;
&#13;
The sample EPD becomes valid when it is transferred to the manufacturer by ift. Currently valid EPDs can be found in the following list and are published on www.ift-service.de/epd.&#13;
EPD number and declaration holder:&#13;
- -	M-EPD-TTS-102&#13;
HODAPP GmbH &amp; Co. KG&#13;
Großweierer Str.77&#13;
77855 Achern&#13;
-	M-EPD-TTS-103&#13;
MTS Brandschutzsysteme GmbH&#13;
Bruchweg 3&#13;
14550 Groß Kreutz&#13;
-	M-EPD-TTS-104&#13;
Wiedemann GmbH&#13;
Siemensstr.16-18&#13;
25813 Husum&#13;
- M-EPD-TTS-105, Metall- u. Anlagenbau Erfurt GmbH, 99091 Erfurt&#13;
- M-EPD-TTS-106, Körner Stahltore GmbH &amp; Co. KG, 21335 Lüneburg-Oedeme&#13;
- M-EPD-TTS-107, Georg Brüggemann GmbH, 59757 Arnsberg&#13;
- M-EPD-TTS-108, Metallbau Ebeling GmbH, 31699 Reckedorf</useAdviceForDataSet>
            <common:other>
                <ns9:referenceToOriginalEPD xmlns:ns9="http://www.indata.network/EPD/2019" refObjectId="e584ff64-c11b-40e5-9979-6d93ed8caa0a" type="source data set" version="00.00.001">
                    <common:shortDescription xml:lang="de">EPD Türen, Tore und Klappen aus Stahl des System Schröders</common:shortDescription>
                </ns9:referenceToOriginalEPD>
            </common:other>
        </dataSourcesTreatmentAndRepresentativeness>
        <validation>
            <review type="Independent external review">
                <common:reviewDetails xml:lang="de">Die angewendete LCI Methode ist in Übereinstimmung mit ISO 14040 und 14044. Die Dokumentation enthält alle relevanten Informationen im Hinblick auf die Datenqualität und den Umfang der Anwendung der jeweiligen LCI Ergebnisse bzw. der Datensätze. Der Datensatz repräsentiert den Stand der Technik bezogen auf die funktionelle Einheit.</common:reviewDetails>
                <common:reviewDetails xml:lang="en">The applied LCI method is in accordance with ISO 14040 and 14044. The documentation contains all relevant information with regard to the data quality and the scope of application of the respective LCI results or data sets. The data set represents the state of the art related to the functional unit.</common:reviewDetails>
                <common:referenceToNameOfReviewerAndInstitution type="contact data set" refObjectId="4ca8370d-bd95-4619-9fe3-8c74f628b623" version="00.00.003" uri="http://openlca.org/ilcd/resource/contacts/4ca8370d-bd95-4619-9fe3-8c74f628b623">
                    <common:shortDescription xml:lang="de">Patrick Wortner</common:shortDescription>
                    <common:shortDescription xml:lang="en">Patrick Wortner</common:shortDescription>
                </common:referenceToNameOfReviewerAndInstitution>
            </review>
        </validation>
        <complianceDeclarations>
            <compliance>
                <common:referenceToComplianceSystem type="source data set" refObjectId="b00f9ec0-7874-11e3-981f-0800200c9a66" version="00.02.001">
                    <common:shortDescription xml:lang="de">EN 15804</common:shortDescription>
                    <common:shortDescription xml:lang="en">EN 15804</common:shortDescription>
                </common:referenceToComplianceSystem>
            </compliance>
        </complianceDeclarations>
    </modellingAndValidation>
    <administrativeInformation>
        <dataGenerator>
            <common:referenceToPersonOrEntityGeneratingTheDataSet type="contact data set" refObjectId="e4e77c13-c6e7-437a-8b76-826e43bb5a95" version="00.00.001" uri="http://openlca.org/ilcd/resource/contacts/e4e77c13-c6e7-437a-8b76-826e43bb5a95">
                <common:shortDescription xml:lang="en">ift Rosenheim</common:shortDescription>
            </common:referenceToPersonOrEntityGeneratingTheDataSet>
        </dataGenerator>
        <dataEntryBy>
            <common:timeStamp>2022-04-19T13:35:41.335+02:00</common:timeStamp>
            <common:referenceToDataSetFormat type="source data set" refObjectId="a97a0155-0234-4b87-b4ce-a45da52f2a40" version="03.00.000" uri="http://lca.jrc.ec.europa.eu/lcainfohub/datasets/ilcd/sources/a97a0155-0234-4b87-b4ce-a45da52f2a40.xml">
                <common:shortDescription xml:lang="en">ILCD format</common:shortDescription>
            </common:referenceToDataSetFormat>
            <common:referenceToDataSetFormat type="source data set" refObjectId="cba73800-7874-11e3-981f-0800200c9a66" version="00.01.001">
                <common:shortDescription xml:lang="de">EPD Data Format Extension</common:shortDescription>
            </common:referenceToDataSetFormat>
            <common:referenceToDataSetFormat type="source data set" refObjectId="a29449fd-aa2f-4de8-b5d7-4b06b43c6fde" version="00.01.000">
                <common:shortDescription xml:lang="en">EPD Data Format Extensions v1.2</common:shortDescription>
                <common:shortDescription xml:lang="de">EPD-Datenformaterweiterungen v1.2</common:shortDescription>
            </common:referenceToDataSetFormat>
            <common:referenceToPersonOrEntityEnteringTheData type="contact data set" refObjectId="e4e77c13-c6e7-437a-8b76-826e43bb5a95" version="00.00.001" uri="http://openlca.org/ilcd/resource/contacts/e4e77c13-c6e7-437a-8b76-826e43bb5a95">
                <common:shortDescription xml:lang="en">ift Rosenheim</common:shortDescription>
            </common:referenceToPersonOrEntityEnteringTheData>
        </dataEntryBy>
        <publicationAndOwnership>
            <common:dataSetVersion>00.00.009</common:dataSetVersion>
            <common:referenceToRegistrationAuthority type="contact data set" refObjectId="e4e77c13-c6e7-437a-8b76-826e43bb5a95" version="00.00.001" uri="http://openlca.org/ilcd/resource/contacts/e4e77c13-c6e7-437a-8b76-826e43bb5a95">
                <common:shortDescription xml:lang="en">ift Rosenheim</common:shortDescription>
            </common:referenceToRegistrationAuthority>
            <common:registrationNumber>M-EPD-TTS-100</common:registrationNumber>
            <common:referenceToOwnershipOfDataSet type="contact data set" refObjectId="fc4e6f4f-4d13-47c5-9b6d-d80d90a276eb" version="00.00.001">
                <common:shortDescription xml:lang="de">Theo Schröders Entwicklung &amp; Beratung GmbH</common:shortDescription>
            </common:referenceToOwnershipOfDataSet>
            <common:copyright>true</common:copyright>
            <common:licenseType>Free of charge for all users and uses</common:licenseType>
            <common:accessRestrictions xml:lang="de">None</common:accessRestrictions>
            <common:other>
                <ns9:referenceToPublisher xmlns:ns9="http://www.indata.network/EPD/2019" refObjectId="f11651e0-7877-11e3-981f-0800200c9a66" type="contact data set" version="00.01.000">
                    <common:shortDescription xml:lang="en">The Federal Institute for Research on Building, Urban Affairs and Spatial Development (BBSR) within the Federal Office for Building and Regional Planning (BBR)</common:shortDescription>
                    <common:shortDescription xml:lang="de">Bundesinstitut für Bau-, Stadt- und Raumforschung (BBSR) im Bundesamt für Bauwesen und Raumordnung (BBR) </common:shortDescription>
                </ns9:referenceToPublisher>
            </common:other>
        </publicationAndOwnership>
    </administrativeInformation>
    <exchanges>
        <exchange dataSetInternalID="1">
            <referenceToFlowDataSet type="flow data set" refObjectId="a62280bf-f500-4e9b-b42c-5c4836171001" version="00.00.005">
                <common:shortDescription xml:lang="de">Tor - Theo Schröders Entwicklung &amp; Beratung GmbH - Feuerschutz-Schiebetore</common:shortDescription>
            </referenceToFlowDataSet>
            <meanAmount>1.0</meanAmount>
            <resultingAmount>1.0</resultingAmount>
        </exchange>
        <exchange dataSetInternalID="2">
            <referenceToFlowDataSet type="flow data set" refObjectId="a2b32f97-3fc7-4af2-b209-525bc6426f33" version="38.00.000">
                <common:shortDescription xml:lang="en">Components for re-use (CRU)</common:shortDescription>
                <common:shortDescription xml:lang="de">Komponenten für die Wiederverwendung (CRU)</common:shortDescription>
            </referenceToFlowDataSet>
            <functionType>General reminder flow</functionType>
            <exchangeDirection>Output</exchangeDirection>
            <meanAmount>0.0</meanAmount>
            <common:other>
                <epd:amount xmlns:epd="http://www.iai.kit.edu/EPD/2013" epd:module="A1-A3">0.0</epd:amount>
                <epd:amount xmlns:epd="http://www.iai.kit.edu/EPD/2013" epd:module="A4">0.0</epd:amount>
                <epd:amount xmlns:epd="http://www.iai.kit.edu/EPD/2013" epd:module="A5">0.0</epd:amount>
                <epd:amount xmlns:epd="http://www.iai.kit.edu/EPD/2013" epd:module="B2">0.0</epd:amount>
                <epd:amount xmlns:epd="http://www.iai.kit.edu/EPD/2013" epd:module="B3">0.0</epd:amount>
                <epd:amount xmlns:epd="http://www.iai.kit.edu/EPD/2013" epd:module="B4">0.0</epd:amount>
                <epd:amount xmlns:epd="http://www.iai.kit.edu/EPD/2013" epd:module="B5">0.0</epd:amount>
                <epd:amount xmlns:epd="http://www.iai.kit.edu/EPD/2013" epd:module="B6">0.0</epd:amount>
                <epd:amount xmlns:epd="http://www.iai.kit.edu/EPD/2013" epd:module="B7">0.0</epd:amount>
                <epd:amount xmlns:epd="http://www.iai.kit.edu/EPD/2013" epd:module="C1">0.0</epd:amount>
                <epd:amount xmlns:epd="http://www.iai.kit.edu/EPD/2013" epd:module="C2">0.0</epd:amount>
                <epd:amount xmlns:epd="http://www.iai.kit.edu/EPD/2013" epd:module="C3">0.0</epd:amount>
                <epd:amount xmlns:epd="http://www.iai.kit.edu/EPD/2013" epd:module="C4">0.0</epd:amount>
                <epd:amount xmlns:epd="http://www.iai.kit.edu/EPD/2013" epd:module="D">0.0</epd:amount>
                <epd:referenceToUnitGroupDataSet xmlns:epd="http://www.iai.kit.edu/EPD/2013" refObjectId="ad38d542-3fe9-439d-9b95-2f5f7752acaf" type="unit group data set" uri="../unitgroups/ad38d542-3fe9-439d-9b95-2f5f7752acaf">
                    <common:shortDescription>kg</common:shortDescription>
                </epd:referenceToUnitGroupDataSet>
            </common:other>
        </exchange>
        <exchange dataSetInternalID="3">
            <referenceToFlowDataSet type="flow data set" refObjectId="4da0c987-2b76-40d6-9e9e-82a017aaaf29" version="38.00.000">
                <common:shortDescription xml:lang="en">Exported electrical energy (EEE)</common:shortDescription>
                <common:shortDescription xml:lang="de">Exportierte elektrische Energie (EEE)</common:shortDescription>
            </referenceToFlowDataSet>
            <functionType>General reminder flow</functionType>
            <exchangeDirection>Output</exchangeDirection>
            <meanAmount>0.0</meanAmount>
            <common:other>
                <epd:amount xmlns:epd="http://www.iai.kit.edu/EPD/2013" epd:module="A1-A3">1.37</epd:amount>
                <epd:amount xmlns:epd="http://www.iai.kit.edu/EPD/2013" epd:module="A4">0.0</epd:amount>
                <epd:amount xmlns:epd="http://www.iai.kit.edu/EPD/2013" epd:module="A5">3.17</epd:amount>
                <epd:amount xmlns:epd="http://www.iai.kit.edu/EPD/2013" epd:module="B2">0.0</epd:amount>
                <epd:amount xmlns:epd="http://www.iai.kit.edu/EPD/2013" epd:module="B3">0.0</epd:amount>
                <epd:amount xmlns:epd="http://www.iai.kit.edu/EPD/2013" epd:module="B4">4.54</epd:amount>
                <epd:amount xmlns:epd="http://www.iai.kit.edu/EPD/2013" epd:module="B5">0.0</epd:amount>
                <epd:amount xmlns:epd="http://www.iai.kit.edu/EPD/2013" epd:module="B6">0.0</epd:amount>
                <epd:amount xmlns:epd="http://www.iai.kit.edu/EPD/2013" epd:module="B7">0.0</epd:amount>
                <epd:amount xmlns:epd="http://www.iai.kit.edu/EPD/2013" epd:module="C1">0.0</epd:amount>
                <epd:amount xmlns:epd="http://www.iai.kit.edu/EPD/2013" epd:module="C2">0.0</epd:amount>
                <epd:amount xmlns:epd="http://www.iai.kit.edu/EPD/2013" epd:module="C3">0.0</epd:amount>
                <epd:amount xmlns:epd="http://www.iai.kit.edu/EPD/2013" epd:module="C4">0.0</epd:amount>
                <epd:amount xmlns:epd="http://www.iai.kit.edu/EPD/2013" epd:module="D">0.0</epd:amount>
                <epd:referenceToUnitGroupDataSet xmlns:epd="http://www.iai.kit.edu/EPD/2013" refObjectId="93a60a57-a3c8-11da-a746-0800200c9a66" type="unit group data set" uri="../unitgroups/93a60a57-a3c8-11da-a746-0800200c9a66">
                    <common:shortDescription>MJ</common:shortDescription>
                </epd:referenceToUnitGroupDataSet>
            </common:other>
        </exchange>
        <exchange dataSetInternalID="4">
            <referenceToFlowDataSet type="flow data set" refObjectId="98daf38a-7a79-46d3-9a37-2b7bd0955810" version="38.00.000">
                <common:shortDescription xml:lang="en">Exported thermal energy (EET)</common:shortDescription>
                <common:shortDescription xml:lang="de">Exportierte thermische Energie (EET)</common:shortDescription>
            </referenceToFlowDataSet>
            <functionType>General reminder flow</functionType>
            <exchangeDirection>Output</exchangeDirection>
            <meanAmount>0.0</meanAmount>
            <common:other>
                <epd:amount xmlns:epd="http://www.iai.kit.edu/EPD/2013" epd:module="A1-A3">2.84</epd:amount>
                <epd:amount xmlns:epd="http://www.iai.kit.edu/EPD/2013" epd:module="A4">0.0</epd:amount>
                <epd:amount xmlns:epd="http://www.iai.kit.edu/EPD/2013" epd:module="A5">7.27</epd:amount>
                <epd:amount xmlns:epd="http://www.iai.kit.edu/EPD/2013" epd:module="B2">0.0</epd:amount>
                <epd:amount xmlns:epd="http://www.iai.kit.edu/EPD/2013" epd:module="B3">0.0</epd:amount>
                <epd:amount xmlns:epd="http://www.iai.kit.edu/EPD/2013" epd:module="B4">10.1</epd:amount>
                <epd:amount xmlns:epd="http://www.iai.kit.edu/EPD/2013" epd:module="B5">0.0</epd:amount>
                <epd:amount xmlns:epd="http://www.iai.kit.edu/EPD/2013" epd:module="B6">0.0</epd:amount>
                <epd:amount xmlns:epd="http://www.iai.kit.edu/EPD/2013" epd:module="B7">0.0</epd:amount>
                <epd:amount xmlns:epd="http://www.iai.kit.edu/EPD/2013" epd:module="C1">0.0</epd:amount>
                <epd:amount xmlns:epd="http://www.iai.kit.edu/EPD/2013" epd:module="C2">0.0</epd:amount>
                <epd:amount xmlns:epd="http://www.iai.kit.edu/EPD/2013" epd:module="C3">0.0</epd:amount>
                <epd:amount xmlns:epd="http://www.iai.kit.edu/EPD/2013" epd:module="C4">0.0</epd:amount>
                <epd:amount xmlns:epd="http://www.iai.kit.edu/EPD/2013" epd:module="D">0.0</epd:amount>
                <epd:referenceToUnitGroupDataSet xmlns:epd="http://www.iai.kit.edu/EPD/2013" refObjectId="93a60a57-a3c8-11da-a746-0800200c9a66" type="unit group data set" uri="../unitgroups/93a60a57-a3c8-11da-a746-0800200c9a66">
                    <common:shortDescription>MJ</common:shortDescription>
                </epd:referenceToUnitGroupDataSet>
            </common:other>
        </exchange>
        <exchange dataSetInternalID="5">
            <referenceToFlowDataSet type="flow data set" refObjectId="430f9e0f-59b2-46a0-8e0d-55e0e84948fc" version="38.00.000">
                <common:shortDescription xml:lang="en">Hazardous waste disposed (HWD)</common:shortDescription>
                <common:shortDescription xml:lang="de">Gefährlicher Abfall zur Beseitigung (HWD)</common:shortDescription>
            </referenceToFlowDataSet>
            <functionType>General reminder flow</functionType>
            <exchangeDirection>Output</exchangeDirection>
            <meanAmount>0.0</meanAmount>
            <common:other>
                <epd:amount xmlns:epd="http://www.iai.kit.edu/EPD/2013" epd:module="A1-A3">6.61E-6</epd:amount>
                <epd:amount xmlns:epd="http://www.iai.kit.edu/EPD/2013" epd:module="A4">8.68E-9</epd:amount>
                <epd:amount xmlns:epd="http://www.iai.kit.edu/EPD/2013" epd:module="A5">1.59E-10</epd:amount>
                <epd:amount xmlns:epd="http://www.iai.kit.edu/EPD/2013" epd:module="B2">3.3E-10</epd:amount>
                <epd:amount xmlns:epd="http://www.iai.kit.edu/EPD/2013" epd:module="B3">0.0</epd:amount>
                <epd:amount xmlns:epd="http://www.iai.kit.edu/EPD/2013" epd:module="B4">6.28E-6</epd:amount>
                <epd:amount xmlns:epd="http://www.iai.kit.edu/EPD/2013" epd:module="B5">0.0</epd:amount>
                <epd:amount xmlns:epd="http://www.iai.kit.edu/EPD/2013" epd:module="B6">0.0</epd:amount>
                <epd:amount xmlns:epd="http://www.iai.kit.edu/EPD/2013" epd:module="B7">0.0</epd:amount>
                <epd:amount xmlns:epd="http://www.iai.kit.edu/EPD/2013" epd:module="C1">0.0</epd:amount>
                <epd:amount xmlns:epd="http://www.iai.kit.edu/EPD/2013" epd:module="C2">1.2E-10</epd:amount>
                <epd:amount xmlns:epd="http://www.iai.kit.edu/EPD/2013" epd:module="C3">5.83E-9</epd:amount>
                <epd:amount xmlns:epd="http://www.iai.kit.edu/EPD/2013" epd:module="C4">8.53E-10</epd:amount>
                <epd:amount xmlns:epd="http://www.iai.kit.edu/EPD/2013" epd:module="D">-3.45E-7</epd:amount>
                <epd:referenceToUnitGroupDataSet xmlns:epd="http://www.iai.kit.edu/EPD/2013" refObjectId="ad38d542-3fe9-439d-9b95-2f5f7752acaf" type="unit group data set" uri="../unitgroups/ad38d542-3fe9-439d-9b95-2f5f7752acaf">
                    <common:shortDescription>kg</common:shortDescription>
                </epd:referenceToUnitGroupDataSet>
            </common:other>
        </exchange>
        <exchange dataSetInternalID="6">
            <referenceToFlowDataSet type="flow data set" refObjectId="59a9181c-3aaf-46ee-8b13-2b3723b6e447" version="38.00.000">
                <common:shortDescription xml:lang="en">Material for Energy Recovery (MER)</common:shortDescription>
                <common:shortDescription xml:lang="de">Stoff für die Energierückgewinnung (MER)</common:shortDescription>
            </referenceToFlowDataSet>
            <functionType>General reminder flow</functionType>
            <exchangeDirection>Output</exchangeDirection>
            <meanAmount>0.0</meanAmount>
            <common:other>
                <epd:amount xmlns:epd="http://www.iai.kit.edu/EPD/2013" epd:module="A1-A3">0.0</epd:amount>
                <epd:amount xmlns:epd="http://www.iai.kit.edu/EPD/2013" epd:module="A4">0.0</epd:amount>
                <epd:amount xmlns:epd="http://www.iai.kit.edu/EPD/2013" epd:module="A5">0.0</epd:amount>
                <epd:amount xmlns:epd="http://www.iai.kit.edu/EPD/2013" epd:module="B2">0.0</epd:amount>
                <epd:amount xmlns:epd="http://www.iai.kit.edu/EPD/2013" epd:module="B3">0.0</epd:amount>
                <epd:amount xmlns:epd="http://www.iai.kit.edu/EPD/2013" epd:module="B4">0.0</epd:amount>
                <epd:amount xmlns:epd="http://www.iai.kit.edu/EPD/2013" epd:module="B5">0.0</epd:amount>
                <epd:amount xmlns:epd="http://www.iai.kit.edu/EPD/2013" epd:module="B6">0.0</epd:amount>
                <epd:amount xmlns:epd="http://www.iai.kit.edu/EPD/2013" epd:module="B7">0.0</epd:amount>
                <epd:amount xmlns:epd="http://www.iai.kit.edu/EPD/2013" epd:module="C1">0.0</epd:amount>
                <epd:amount xmlns:epd="http://www.iai.kit.edu/EPD/2013" epd:module="C2">0.0</epd:amount>
                <epd:amount xmlns:epd="http://www.iai.kit.edu/EPD/2013" epd:module="C3">0.0</epd:amount>
                <epd:amount xmlns:epd="http://www.iai.kit.edu/EPD/2013" epd:module="C4">0.0</epd:amount>
                <epd:amount xmlns:epd="http://www.iai.kit.edu/EPD/2013" epd:module="D">0.0</epd:amount>
                <epd:referenceToUnitGroupDataSet xmlns:epd="http://www.iai.kit.edu/EPD/2013" refObjectId="ad38d542-3fe9-439d-9b95-2f5f7752acaf" type="unit group data set" uri="../unitgroups/ad38d542-3fe9-439d-9b95-2f5f7752acaf">
                    <common:shortDescription>kg</common:shortDescription>
                </epd:referenceToUnitGroupDataSet>
            </common:other>
        </exchange>
        <exchange dataSetInternalID="7">
            <referenceToFlowDataSet type="flow data set" refObjectId="d7fe48a5-4103-49c8-9aae-b0b5dfdbd6ae" version="38.00.000">
                <common:shortDescription xml:lang="en">Materials for Recycling (MFR)</common:shortDescription>
                <common:shortDescription xml:lang="de">Stoffe zum Recycling (MFR)</common:shortDescription>
            </referenceToFlowDataSet>
            <functionType>General reminder flow</functionType>
            <exchangeDirection>Output</exchangeDirection>
            <meanAmount>0.0</meanAmount>
            <common:other>
                <epd:amount xmlns:epd="http://www.iai.kit.edu/EPD/2013" epd:module="A1-A3">5.63</epd:amount>
                <epd:amount xmlns:epd="http://www.iai.kit.edu/EPD/2013" epd:module="A4">0.0</epd:amount>
                <epd:amount xmlns:epd="http://www.iai.kit.edu/EPD/2013" epd:module="A5">0.0</epd:amount>
                <epd:amount xmlns:epd="http://www.iai.kit.edu/EPD/2013" epd:module="B2">0.0</epd:amount>
                <epd:amount xmlns:epd="http://www.iai.kit.edu/EPD/2013" epd:module="B3">0.0</epd:amount>
                <epd:amount xmlns:epd="http://www.iai.kit.edu/EPD/2013" epd:module="B4">33.6</epd:amount>
                <epd:amount xmlns:epd="http://www.iai.kit.edu/EPD/2013" epd:module="B5">0.0</epd:amount>
                <epd:amount xmlns:epd="http://www.iai.kit.edu/EPD/2013" epd:module="B6">0.0</epd:amount>
                <epd:amount xmlns:epd="http://www.iai.kit.edu/EPD/2013" epd:module="B7">0.0</epd:amount>
                <epd:amount xmlns:epd="http://www.iai.kit.edu/EPD/2013" epd:module="C1">0.0</epd:amount>
                <epd:amount xmlns:epd="http://www.iai.kit.edu/EPD/2013" epd:module="C2">0.0</epd:amount>
                <epd:amount xmlns:epd="http://www.iai.kit.edu/EPD/2013" epd:module="C3">28.0</epd:amount>
                <epd:amount xmlns:epd="http://www.iai.kit.edu/EPD/2013" epd:module="C4">0.0</epd:amount>
                <epd:amount xmlns:epd="http://www.iai.kit.edu/EPD/2013" epd:module="D">0.0</epd:amount>
                <epd:referenceToUnitGroupDataSet xmlns:epd="http://www.iai.kit.edu/EPD/2013" refObjectId="ad38d542-3fe9-439d-9b95-2f5f7752acaf" type="unit group data set" uri="../unitgroups/ad38d542-3fe9-439d-9b95-2f5f7752acaf">
                    <common:shortDescription>kg</common:shortDescription>
                </epd:referenceToUnitGroupDataSet>
            </common:other>
        </exchange>
        <exchange dataSetInternalID="8">
            <referenceToFlowDataSet type="flow data set" refObjectId="3cf952c8-f3a4-461d-8c96-96456ca62246" version="38.00.000">
                <common:shortDescription xml:lang="en">Use of net fresh water (FW)</common:shortDescription>
                <common:shortDescription xml:lang="de">Frischwasserverbrauch (FW)</common:shortDescription>
            </referenceToFlowDataSet>
            <functionType>General reminder flow</functionType>
            <exchangeDirection>Input</exchangeDirection>
            <meanAmount>0.0</meanAmount>
            <common:other>
                <epd:amount xmlns:epd="http://www.iai.kit.edu/EPD/2013" epd:module="A1-A3">0.77</epd:amount>
                <epd:amount xmlns:epd="http://www.iai.kit.edu/EPD/2013" epd:module="A4">0.011</epd:amount>
                <epd:amount xmlns:epd="http://www.iai.kit.edu/EPD/2013" epd:module="A5">0.00729</epd:amount>
                <epd:amount xmlns:epd="http://www.iai.kit.edu/EPD/2013" epd:module="B2">2.5E-4</epd:amount>
                <epd:amount xmlns:epd="http://www.iai.kit.edu/EPD/2013" epd:module="B3">0.0</epd:amount>
                <epd:amount xmlns:epd="http://www.iai.kit.edu/EPD/2013" epd:module="B4">0.17</epd:amount>
                <epd:amount xmlns:epd="http://www.iai.kit.edu/EPD/2013" epd:module="B5">0.0</epd:amount>
                <epd:amount xmlns:epd="http://www.iai.kit.edu/EPD/2013" epd:module="B6">0.0</epd:amount>
                <epd:amount xmlns:epd="http://www.iai.kit.edu/EPD/2013" epd:module="B7">0.0</epd:amount>
                <epd:amount xmlns:epd="http://www.iai.kit.edu/EPD/2013" epd:module="C1">0.0</epd:amount>
                <epd:amount xmlns:epd="http://www.iai.kit.edu/EPD/2013" epd:module="C2">1.52E-4</epd:amount>
                <epd:amount xmlns:epd="http://www.iai.kit.edu/EPD/2013" epd:module="C3">0.00493</epd:amount>
                <epd:amount xmlns:epd="http://www.iai.kit.edu/EPD/2013" epd:module="C4">0.00198</epd:amount>
                <epd:amount xmlns:epd="http://www.iai.kit.edu/EPD/2013" epd:module="D">-0.63</epd:amount>
                <epd:referenceToUnitGroupDataSet xmlns:epd="http://www.iai.kit.edu/EPD/2013" refObjectId="cd950537-0a98-4044-9ba7-9f9a68d0a504" type="unit group data set" uri="../unitgroups/cd950537-0a98-4044-9ba7-9f9a68d0a504">
                    <common:shortDescription>m3</common:shortDescription>
                </epd:referenceToUnitGroupDataSet>
            </common:other>
        </exchange>
        <exchange dataSetInternalID="9">
            <referenceToFlowDataSet type="flow data set" refObjectId="b29ef66b-e286-4afa-949f-62f1a7b4d7fa" version="38.00.000">
                <common:shortDescription xml:lang="en">Non-hazardous waste disposed (NHWD)</common:shortDescription>
                <common:shortDescription xml:lang="de">Ungefährlicher Abfall zur Beseitigung (NHWD)</common:shortDescription>
            </referenceToFlowDataSet>
            <functionType>General reminder flow</functionType>
            <exchangeDirection>Output</exchangeDirection>
            <meanAmount>0.0</meanAmount>
            <common:other>
                <epd:amount xmlns:epd="http://www.iai.kit.edu/EPD/2013" epd:module="A1-A3">3.46</epd:amount>
                <epd:amount xmlns:epd="http://www.iai.kit.edu/EPD/2013" epd:module="A4">0.0256</epd:amount>
                <epd:amount xmlns:epd="http://www.iai.kit.edu/EPD/2013" epd:module="A5">0.0219</epd:amount>
                <epd:amount xmlns:epd="http://www.iai.kit.edu/EPD/2013" epd:module="B2">0.00176</epd:amount>
                <epd:amount xmlns:epd="http://www.iai.kit.edu/EPD/2013" epd:module="B3">0.0</epd:amount>
                <epd:amount xmlns:epd="http://www.iai.kit.edu/EPD/2013" epd:module="B4">41.8</epd:amount>
                <epd:amount xmlns:epd="http://www.iai.kit.edu/EPD/2013" epd:module="B5">0.0</epd:amount>
                <epd:amount xmlns:epd="http://www.iai.kit.edu/EPD/2013" epd:module="B6">0.0</epd:amount>
                <epd:amount xmlns:epd="http://www.iai.kit.edu/EPD/2013" epd:module="B7">0.0</epd:amount>
                <epd:amount xmlns:epd="http://www.iai.kit.edu/EPD/2013" epd:module="C1">0.0</epd:amount>
                <epd:amount xmlns:epd="http://www.iai.kit.edu/EPD/2013" epd:module="C2">3.54E-4</epd:amount>
                <epd:amount xmlns:epd="http://www.iai.kit.edu/EPD/2013" epd:module="C3">0.0125</epd:amount>
                <epd:amount xmlns:epd="http://www.iai.kit.edu/EPD/2013" epd:module="C4">40.1</epd:amount>
                <epd:amount xmlns:epd="http://www.iai.kit.edu/EPD/2013" epd:module="D">-1.82</epd:amount>
                <epd:referenceToUnitGroupDataSet xmlns:epd="http://www.iai.kit.edu/EPD/2013" refObjectId="ad38d542-3fe9-439d-9b95-2f5f7752acaf" type="unit group data set" uri="../unitgroups/ad38d542-3fe9-439d-9b95-2f5f7752acaf">
                    <common:shortDescription>kg</common:shortDescription>
                </epd:referenceToUnitGroupDataSet>
            </common:other>
        </exchange>
        <exchange dataSetInternalID="10">
            <referenceToFlowDataSet type="flow data set" refObjectId="ac857178-2b45-46ec-892a-a9a4332f0372" version="38.00.000">
                <common:shortDescription xml:lang="en">Nicht-erneuerbare Primärenergie als Energieträger (PENRE)</common:shortDescription>
                <common:shortDescription xml:lang="de">Nicht-erneuerbare Primärenergie als Energieträger (PENRE)</common:shortDescription>
            </referenceToFlowDataSet>
            <functionType>General reminder flow</functionType>
            <exchangeDirection>Input</exchangeDirection>
            <meanAmount>0.0</meanAmount>
            <common:other>
                <epd:amount xmlns:epd="http://www.iai.kit.edu/EPD/2013" epd:module="A1-A3">2350.0</epd:amount>
                <epd:amount xmlns:epd="http://www.iai.kit.edu/EPD/2013" epd:module="A4">172.0</epd:amount>
                <epd:amount xmlns:epd="http://www.iai.kit.edu/EPD/2013" epd:module="A5">1.5</epd:amount>
                <epd:amount xmlns:epd="http://www.iai.kit.edu/EPD/2013" epd:module="B2">15.5</epd:amount>
                <epd:amount xmlns:epd="http://www.iai.kit.edu/EPD/2013" epd:module="B3">0.0</epd:amount>
                <epd:amount xmlns:epd="http://www.iai.kit.edu/EPD/2013" epd:module="B4">2020.0</epd:amount>
                <epd:amount xmlns:epd="http://www.iai.kit.edu/EPD/2013" epd:module="B5">0.0</epd:amount>
                <epd:amount xmlns:epd="http://www.iai.kit.edu/EPD/2013" epd:module="B6">0.0</epd:amount>
                <epd:amount xmlns:epd="http://www.iai.kit.edu/EPD/2013" epd:module="B7">0.0</epd:amount>
                <epd:amount xmlns:epd="http://www.iai.kit.edu/EPD/2013" epd:module="C1">0.0</epd:amount>
                <epd:amount xmlns:epd="http://www.iai.kit.edu/EPD/2013" epd:module="C2">2.38</epd:amount>
                <epd:amount xmlns:epd="http://www.iai.kit.edu/EPD/2013" epd:module="C3">16.1</epd:amount>
                <epd:amount xmlns:epd="http://www.iai.kit.edu/EPD/2013" epd:module="C4">8.04</epd:amount>
                <epd:amount xmlns:epd="http://www.iai.kit.edu/EPD/2013" epd:module="D">-529.0</epd:amount>
                <epd:referenceToUnitGroupDataSet xmlns:epd="http://www.iai.kit.edu/EPD/2013" refObjectId="93a60a57-a3c8-11da-a746-0800200c9a66" type="unit group data set" uri="../unitgroups/93a60a57-a3c8-11da-a746-0800200c9a66">
                    <common:shortDescription>MJ</common:shortDescription>
                </epd:referenceToUnitGroupDataSet>
            </common:other>
        </exchange>
        <exchange dataSetInternalID="11">
            <referenceToFlowDataSet type="flow data set" refObjectId="1421caa0-679d-4bf4-b282-0eb850ccae27" version="38.00.000">
                <common:shortDescription xml:lang="en">Nicht-erneuerbare Primärenergie zur stofflichen Nutzung (PENRM)</common:shortDescription>
                <common:shortDescription xml:lang="de">Nicht-erneuerbare Primärenergie zur stofflichen Nutzung (PENRM)</common:shortDescription>
            </referenceToFlowDataSet>
            <functionType>General reminder flow</functionType>
            <exchangeDirection>Input</exchangeDirection>
            <meanAmount>0.0</meanAmount>
            <common:other>
                <epd:amount xmlns:epd="http://www.iai.kit.edu/EPD/2013" epd:module="A1-A3">0.65</epd:amount>
                <epd:amount xmlns:epd="http://www.iai.kit.edu/EPD/2013" epd:module="A4">0.0</epd:amount>
                <epd:amount xmlns:epd="http://www.iai.kit.edu/EPD/2013" epd:module="A5">-0.65</epd:amount>
                <epd:amount xmlns:epd="http://www.iai.kit.edu/EPD/2013" epd:module="B2">0.0</epd:amount>
                <epd:amount xmlns:epd="http://www.iai.kit.edu/EPD/2013" epd:module="B3">0.0</epd:amount>
                <epd:amount xmlns:epd="http://www.iai.kit.edu/EPD/2013" epd:module="B4">0.0</epd:amount>
                <epd:amount xmlns:epd="http://www.iai.kit.edu/EPD/2013" epd:module="B5">0.0</epd:amount>
                <epd:amount xmlns:epd="http://www.iai.kit.edu/EPD/2013" epd:module="B6">0.0</epd:amount>
                <epd:amount xmlns:epd="http://www.iai.kit.edu/EPD/2013" epd:module="B7">0.0</epd:amount>
                <epd:amount xmlns:epd="http://www.iai.kit.edu/EPD/2013" epd:module="C1">0.0</epd:amount>
                <epd:amount xmlns:epd="http://www.iai.kit.edu/EPD/2013" epd:module="C2">0.0</epd:amount>
                <epd:amount xmlns:epd="http://www.iai.kit.edu/EPD/2013" epd:module="C3">0.0</epd:amount>
                <epd:amount xmlns:epd="http://www.iai.kit.edu/EPD/2013" epd:module="C4">0.0</epd:amount>
                <epd:amount xmlns:epd="http://www.iai.kit.edu/EPD/2013" epd:module="D">0.0</epd:amount>
                <epd:referenceToUnitGroupDataSet xmlns:epd="http://www.iai.kit.edu/EPD/2013" refObjectId="93a60a57-a3c8-11da-a746-0800200c9a66" type="unit group data set" uri="../unitgroups/93a60a57-a3c8-11da-a746-0800200c9a66">
                    <common:shortDescription>MJ</common:shortDescription>
                </epd:referenceToUnitGroupDataSet>
            </common:other>
        </exchange>
        <exchange dataSetInternalID="12">
            <referenceToFlowDataSet type="flow data set" refObjectId="89def144-d39a-4287-b86f-efde453ddcb2" version="38.00.000">
                <common:shortDescription xml:lang="en">Use of non renewable secondary fuels (NRSF)</common:shortDescription>
                <common:shortDescription xml:lang="de">Verbrauch nicht erneuerbarer Sekundärbrennstoffe (NRSF)</common:shortDescription>
            </referenceToFlowDataSet>
            <functionType>General reminder flow</functionType>
            <exchangeDirection>Input</exchangeDirection>
            <meanAmount>0.0</meanAmount>
            <common:other>
                <epd:amount xmlns:epd="http://www.iai.kit.edu/EPD/2013" epd:module="A1-A3">0.0</epd:amount>
                <epd:amount xmlns:epd="http://www.iai.kit.edu/EPD/2013" epd:module="A4">0.0</epd:amount>
                <epd:amount xmlns:epd="http://www.iai.kit.edu/EPD/2013" epd:module="A5">0.0</epd:amount>
                <epd:amount xmlns:epd="http://www.iai.kit.edu/EPD/2013" epd:module="B2">0.0</epd:amount>
                <epd:amount xmlns:epd="http://www.iai.kit.edu/EPD/2013" epd:module="B3">0.0</epd:amount>
                <epd:amount xmlns:epd="http://www.iai.kit.edu/EPD/2013" epd:module="B4">0.0</epd:amount>
                <epd:amount xmlns:epd="http://www.iai.kit.edu/EPD/2013" epd:module="B5">0.0</epd:amount>
                <epd:amount xmlns:epd="http://www.iai.kit.edu/EPD/2013" epd:module="B6">0.0</epd:amount>
                <epd:amount xmlns:epd="http://www.iai.kit.edu/EPD/2013" epd:module="B7">0.0</epd:amount>
                <epd:amount xmlns:epd="http://www.iai.kit.edu/EPD/2013" epd:module="C1">0.0</epd:amount>
                <epd:amount xmlns:epd="http://www.iai.kit.edu/EPD/2013" epd:module="C2">0.0</epd:amount>
                <epd:amount xmlns:epd="http://www.iai.kit.edu/EPD/2013" epd:module="C3">0.0</epd:amount>
                <epd:amount xmlns:epd="http://www.iai.kit.edu/EPD/2013" epd:module="C4">0.0</epd:amount>
                <epd:amount xmlns:epd="http://www.iai.kit.edu/EPD/2013" epd:module="D">0.0</epd:amount>
                <epd:referenceToUnitGroupDataSet xmlns:epd="http://www.iai.kit.edu/EPD/2013" refObjectId="93a60a57-a3c8-11da-a746-0800200c9a66" type="unit group data set" uri="../unitgroups/93a60a57-a3c8-11da-a746-0800200c9a66">
                    <common:shortDescription>MJ</common:shortDescription>
                </epd:referenceToUnitGroupDataSet>
            </common:other>
        </exchange>
        <exchange dataSetInternalID="13">
            <referenceToFlowDataSet type="flow data set" refObjectId="3449546e-52ad-4b39-b809-9fb77cea8ff6" version="38.00.000">
                <common:shortDescription xml:lang="en">Radioactive waste disposed (RWD)</common:shortDescription>
                <common:shortDescription xml:lang="de">Entsorgter radioaktiver Abfall (RWD)</common:shortDescription>
            </referenceToFlowDataSet>
            <functionType>General reminder flow</functionType>
            <exchangeDirection>Output</exchangeDirection>
            <meanAmount>0.0</meanAmount>
            <common:other>
                <epd:amount xmlns:epd="http://www.iai.kit.edu/EPD/2013" epd:module="A1-A3">0.0606</epd:amount>
                <epd:amount xmlns:epd="http://www.iai.kit.edu/EPD/2013" epd:module="A4">2.08E-4</epd:amount>
                <epd:amount xmlns:epd="http://www.iai.kit.edu/EPD/2013" epd:module="A5">2.12E-5</epd:amount>
                <epd:amount xmlns:epd="http://www.iai.kit.edu/EPD/2013" epd:module="B2">6.24E-5</epd:amount>
                <epd:amount xmlns:epd="http://www.iai.kit.edu/EPD/2013" epd:module="B3">0.0</epd:amount>
                <epd:amount xmlns:epd="http://www.iai.kit.edu/EPD/2013" epd:module="B4">0.0611</epd:amount>
                <epd:amount xmlns:epd="http://www.iai.kit.edu/EPD/2013" epd:module="B5">0.0</epd:amount>
                <epd:amount xmlns:epd="http://www.iai.kit.edu/EPD/2013" epd:module="B6">0.0</epd:amount>
                <epd:amount xmlns:epd="http://www.iai.kit.edu/EPD/2013" epd:module="B7">0.0</epd:amount>
                <epd:amount xmlns:epd="http://www.iai.kit.edu/EPD/2013" epd:module="C1">0.0</epd:amount>
                <epd:amount xmlns:epd="http://www.iai.kit.edu/EPD/2013" epd:module="C2">2.88E-6</epd:amount>
                <epd:amount xmlns:epd="http://www.iai.kit.edu/EPD/2013" epd:module="C3">0.00129</epd:amount>
                <epd:amount xmlns:epd="http://www.iai.kit.edu/EPD/2013" epd:module="C4">8.44E-5</epd:amount>
                <epd:amount xmlns:epd="http://www.iai.kit.edu/EPD/2013" epd:module="D">-0.00113</epd:amount>
                <epd:referenceToUnitGroupDataSet xmlns:epd="http://www.iai.kit.edu/EPD/2013" refObjectId="ad38d542-3fe9-439d-9b95-2f5f7752acaf" type="unit group data set" uri="../unitgroups/ad38d542-3fe9-439d-9b95-2f5f7752acaf">
                    <common:shortDescription>kg</common:shortDescription>
                </epd:referenceToUnitGroupDataSet>
            </common:other>
        </exchange>
        <exchange dataSetInternalID="14">
            <referenceToFlowDataSet type="flow data set" refObjectId="20f32be5-0398-4288-9b6d-accddd195317" version="38.00.000">
                <common:shortDescription xml:lang="en">Erneuerbare Primärenergie als Energieträger (PERE)</common:shortDescription>
                <common:shortDescription xml:lang="de">Erneuerbare Primärenergie als Energieträger (PERE)</common:shortDescription>
            </referenceToFlowDataSet>
            <functionType>General reminder flow</functionType>
            <exchangeDirection>Input</exchangeDirection>
            <meanAmount>0.0</meanAmount>
            <common:other>
                <epd:amount xmlns:epd="http://www.iai.kit.edu/EPD/2013" epd:module="A1-A3">119.0</epd:amount>
                <epd:amount xmlns:epd="http://www.iai.kit.edu/EPD/2013" epd:module="A4">9.6</epd:amount>
                <epd:amount xmlns:epd="http://www.iai.kit.edu/EPD/2013" epd:module="A5">25.9</epd:amount>
                <epd:amount xmlns:epd="http://www.iai.kit.edu/EPD/2013" epd:module="B2">0.19</epd:amount>
                <epd:amount xmlns:epd="http://www.iai.kit.edu/EPD/2013" epd:module="B3">0.0</epd:amount>
                <epd:amount xmlns:epd="http://www.iai.kit.edu/EPD/2013" epd:module="B4">147.0</epd:amount>
                <epd:amount xmlns:epd="http://www.iai.kit.edu/EPD/2013" epd:module="B5">0.0</epd:amount>
                <epd:amount xmlns:epd="http://www.iai.kit.edu/EPD/2013" epd:module="B6">0.0</epd:amount>
                <epd:amount xmlns:epd="http://www.iai.kit.edu/EPD/2013" epd:module="B7">0.0</epd:amount>
                <epd:amount xmlns:epd="http://www.iai.kit.edu/EPD/2013" epd:module="C1">0.0</epd:amount>
                <epd:amount xmlns:epd="http://www.iai.kit.edu/EPD/2013" epd:module="C2">0.13</epd:amount>
                <epd:amount xmlns:epd="http://www.iai.kit.edu/EPD/2013" epd:module="C3">10.5</epd:amount>
                <epd:amount xmlns:epd="http://www.iai.kit.edu/EPD/2013" epd:module="C4">1.08</epd:amount>
                <epd:amount xmlns:epd="http://www.iai.kit.edu/EPD/2013" epd:module="D">-19.3</epd:amount>
                <epd:referenceToUnitGroupDataSet xmlns:epd="http://www.iai.kit.edu/EPD/2013" refObjectId="93a60a57-a3c8-11da-a746-0800200c9a66" type="unit group data set" uri="../unitgroups/93a60a57-a3c8-11da-a746-0800200c9a66">
                    <common:shortDescription>MJ</common:shortDescription>
                </epd:referenceToUnitGroupDataSet>
            </common:other>
        </exchange>
        <exchange dataSetInternalID="15">
            <referenceToFlowDataSet type="flow data set" refObjectId="fb3ec0de-548d-4508-aea5-00b73bf6f702" version="38.00.000">
                <common:shortDescription xml:lang="en">Erneuerbare Primärenergie zur stofflichen Nutzung (PERM)</common:shortDescription>
                <common:shortDescription xml:lang="de">Erneuerbare Primärenergie zur stofflichen Nutzung (PERM)</common:shortDescription>
            </referenceToFlowDataSet>
            <functionType>General reminder flow</functionType>
            <exchangeDirection>Input</exchangeDirection>
            <meanAmount>0.0</meanAmount>
            <common:other>
                <epd:amount xmlns:epd="http://www.iai.kit.edu/EPD/2013" epd:module="A1-A3">21.4</epd:amount>
                <epd:amount xmlns:epd="http://www.iai.kit.edu/EPD/2013" epd:module="A4">0.0</epd:amount>
                <epd:amount xmlns:epd="http://www.iai.kit.edu/EPD/2013" epd:module="A5">-21.4</epd:amount>
                <epd:amount xmlns:epd="http://www.iai.kit.edu/EPD/2013" epd:module="B2">0.0</epd:amount>
                <epd:amount xmlns:epd="http://www.iai.kit.edu/EPD/2013" epd:module="B3">0.0</epd:amount>
                <epd:amount xmlns:epd="http://www.iai.kit.edu/EPD/2013" epd:module="B4">0.0</epd:amount>
                <epd:amount xmlns:epd="http://www.iai.kit.edu/EPD/2013" epd:module="B5">0.0</epd:amount>
                <epd:amount xmlns:epd="http://www.iai.kit.edu/EPD/2013" epd:module="B6">0.0</epd:amount>
                <epd:amount xmlns:epd="http://www.iai.kit.edu/EPD/2013" epd:module="B7">0.0</epd:amount>
                <epd:amount xmlns:epd="http://www.iai.kit.edu/EPD/2013" epd:module="C1">0.0</epd:amount>
                <epd:amount xmlns:epd="http://www.iai.kit.edu/EPD/2013" epd:module="C2">0.0</epd:amount>
                <epd:amount xmlns:epd="http://www.iai.kit.edu/EPD/2013" epd:module="C3">0.0</epd:amount>
                <epd:amount xmlns:epd="http://www.iai.kit.edu/EPD/2013" epd:module="C4">0.0</epd:amount>
                <epd:amount xmlns:epd="http://www.iai.kit.edu/EPD/2013" epd:module="D">0.0</epd:amount>
                <epd:referenceToUnitGroupDataSet xmlns:epd="http://www.iai.kit.edu/EPD/2013" refObjectId="93a60a57-a3c8-11da-a746-0800200c9a66" type="unit group data set" uri="../unitgroups/93a60a57-a3c8-11da-a746-0800200c9a66">
                    <common:shortDescription>MJ</common:shortDescription>
                </epd:referenceToUnitGroupDataSet>
            </common:other>
        </exchange>
        <exchange dataSetInternalID="16">
            <referenceToFlowDataSet type="flow data set" refObjectId="64333088-a55f-4aa2-9a31-c10b07816787" version="38.00.000">
                <common:shortDescription xml:lang="en">Use of renewable secondary fuels (RSF)</common:shortDescription>
                <common:shortDescription xml:lang="de">Erneuerbare Sekundärbrennstoffe (RSF)</common:shortDescription>
            </referenceToFlowDataSet>
            <functionType>General reminder flow</functionType>
            <exchangeDirection>Input</exchangeDirection>
            <meanAmount>0.0</meanAmount>
            <common:other>
                <epd:amount xmlns:epd="http://www.iai.kit.edu/EPD/2013" epd:module="A1-A3">0.0</epd:amount>
                <epd:amount xmlns:epd="http://www.iai.kit.edu/EPD/2013" epd:module="A4">0.0</epd:amount>
                <epd:amount xmlns:epd="http://www.iai.kit.edu/EPD/2013" epd:module="A5">0.0</epd:amount>
                <epd:amount xmlns:epd="http://www.iai.kit.edu/EPD/2013" epd:module="B2">0.0</epd:amount>
                <epd:amount xmlns:epd="http://www.iai.kit.edu/EPD/2013" epd:module="B3">0.0</epd:amount>
                <epd:amount xmlns:epd="http://www.iai.kit.edu/EPD/2013" epd:module="B4">0.0</epd:amount>
                <epd:amount xmlns:epd="http://www.iai.kit.edu/EPD/2013" epd:module="B5">0.0</epd:amount>
                <epd:amount xmlns:epd="http://www.iai.kit.edu/EPD/2013" epd:module="B6">0.0</epd:amount>
                <epd:amount xmlns:epd="http://www.iai.kit.edu/EPD/2013" epd:module="B7">0.0</epd:amount>
                <epd:amount xmlns:epd="http://www.iai.kit.edu/EPD/2013" epd:module="C1">0.0</epd:amount>
                <epd:amount xmlns:epd="http://www.iai.kit.edu/EPD/2013" epd:module="C2">0.0</epd:amount>
                <epd:amount xmlns:epd="http://www.iai.kit.edu/EPD/2013" epd:module="C3">0.0</epd:amount>
                <epd:amount xmlns:epd="http://www.iai.kit.edu/EPD/2013" epd:module="C4">0.0</epd:amount>
                <epd:amount xmlns:epd="http://www.iai.kit.edu/EPD/2013" epd:module="D">0.0</epd:amount>
                <epd:referenceToUnitGroupDataSet xmlns:epd="http://www.iai.kit.edu/EPD/2013" refObjectId="93a60a57-a3c8-11da-a746-0800200c9a66" type="unit group data set" uri="../unitgroups/93a60a57-a3c8-11da-a746-0800200c9a66">
                    <common:shortDescription>MJ</common:shortDescription>
                </epd:referenceToUnitGroupDataSet>
            </common:other>
        </exchange>
        <exchange dataSetInternalID="17">
            <referenceToFlowDataSet type="flow data set" refObjectId="c6a1f35f-2d09-4f54-8dfb-97e502e1ce92" version="38.00.000">
                <common:shortDescription xml:lang="en">Input of secondary material (SM)</common:shortDescription>
                <common:shortDescription xml:lang="de">Einsatz von Sekundärstoffen (SM)</common:shortDescription>
            </referenceToFlowDataSet>
            <functionType>General reminder flow</functionType>
            <exchangeDirection>Input</exchangeDirection>
            <meanAmount>0.0</meanAmount>
            <common:other>
                <epd:amount xmlns:epd="http://www.iai.kit.edu/EPD/2013" epd:module="A1-A3">0.0</epd:amount>
                <epd:amount xmlns:epd="http://www.iai.kit.edu/EPD/2013" epd:module="A4">0.0</epd:amount>
                <epd:amount xmlns:epd="http://www.iai.kit.edu/EPD/2013" epd:module="A5">0.0</epd:amount>
                <epd:amount xmlns:epd="http://www.iai.kit.edu/EPD/2013" epd:module="B2">0.0</epd:amount>
                <epd:amount xmlns:epd="http://www.iai.kit.edu/EPD/2013" epd:module="B3">0.0</epd:amount>
                <epd:amount xmlns:epd="http://www.iai.kit.edu/EPD/2013" epd:module="B4">0.0</epd:amount>
                <epd:amount xmlns:epd="http://www.iai.kit.edu/EPD/2013" epd:module="B5">0.0</epd:amount>
                <epd:amount xmlns:epd="http://www.iai.kit.edu/EPD/2013" epd:module="B6">0.0</epd:amount>
                <epd:amount xmlns:epd="http://www.iai.kit.edu/EPD/2013" epd:module="B7">0.0</epd:amount>
                <epd:amount xmlns:epd="http://www.iai.kit.edu/EPD/2013" epd:module="C1">0.0</epd:amount>
                <epd:amount xmlns:epd="http://www.iai.kit.edu/EPD/2013" epd:module="C2">0.0</epd:amount>
                <epd:amount xmlns:epd="http://www.iai.kit.edu/EPD/2013" epd:module="C3">0.0</epd:amount>
                <epd:amount xmlns:epd="http://www.iai.kit.edu/EPD/2013" epd:module="C4">0.0</epd:amount>
                <epd:amount xmlns:epd="http://www.iai.kit.edu/EPD/2013" epd:module="D">0.0</epd:amount>
                <epd:referenceToUnitGroupDataSet xmlns:epd="http://www.iai.kit.edu/EPD/2013" refObjectId="ad38d542-3fe9-439d-9b95-2f5f7752acaf" type="unit group data set" uri="../unitgroups/ad38d542-3fe9-439d-9b95-2f5f7752acaf">
                    <common:shortDescription>kg</common:shortDescription>
                </epd:referenceToUnitGroupDataSet>
            </common:other>
        </exchange>
        <exchange dataSetInternalID="18">
            <referenceToFlowDataSet type="flow data set" refObjectId="06159210-646b-4c8d-8583-da9b3b95a6c1" version="38.00.000">
                <common:shortDescription xml:lang="en">Total use of non-renewable primary energy resources (PENRT)</common:shortDescription>
                <common:shortDescription xml:lang="de">Total nicht erneuerbare Primärenergie (PENRT)</common:shortDescription>
            </referenceToFlowDataSet>
            <functionType>General reminder flow</functionType>
            <exchangeDirection>Input</exchangeDirection>
            <meanAmount>0.0</meanAmount>
            <common:other>
                <epd:amount xmlns:epd="http://www.iai.kit.edu/EPD/2013" epd:module="A1-A3">2350.0</epd:amount>
                <epd:amount xmlns:epd="http://www.iai.kit.edu/EPD/2013" epd:module="A4">172.0</epd:amount>
                <epd:amount xmlns:epd="http://www.iai.kit.edu/EPD/2013" epd:module="A5">0.85</epd:amount>
                <epd:amount xmlns:epd="http://www.iai.kit.edu/EPD/2013" epd:module="B2">15.5</epd:amount>
                <epd:amount xmlns:epd="http://www.iai.kit.edu/EPD/2013" epd:module="B3">0.0</epd:amount>
                <epd:amount xmlns:epd="http://www.iai.kit.edu/EPD/2013" epd:module="B4">2020.0</epd:amount>
                <epd:amount xmlns:epd="http://www.iai.kit.edu/EPD/2013" epd:module="B5">0.0</epd:amount>
                <epd:amount xmlns:epd="http://www.iai.kit.edu/EPD/2013" epd:module="B6">0.0</epd:amount>
                <epd:amount xmlns:epd="http://www.iai.kit.edu/EPD/2013" epd:module="B7">0.0</epd:amount>
                <epd:amount xmlns:epd="http://www.iai.kit.edu/EPD/2013" epd:module="C1">0.0</epd:amount>
                <epd:amount xmlns:epd="http://www.iai.kit.edu/EPD/2013" epd:module="C2">2.38</epd:amount>
                <epd:amount xmlns:epd="http://www.iai.kit.edu/EPD/2013" epd:module="C3">16.1</epd:amount>
                <epd:amount xmlns:epd="http://www.iai.kit.edu/EPD/2013" epd:module="C4">8.04</epd:amount>
                <epd:amount xmlns:epd="http://www.iai.kit.edu/EPD/2013" epd:module="D">-529.0</epd:amount>
                <epd:referenceToUnitGroupDataSet xmlns:epd="http://www.iai.kit.edu/EPD/2013" refObjectId="93a60a57-a3c8-11da-a746-0800200c9a66" type="unit group data set" uri="../unitgroups/93a60a57-a3c8-11da-a746-0800200c9a66">
                    <common:shortDescription>MJ</common:shortDescription>
                </epd:referenceToUnitGroupDataSet>
            </common:other>
        </exchange>
        <exchange dataSetInternalID="19">
            <referenceToFlowDataSet type="flow data set" refObjectId="53f97275-fa8a-4cdd-9024-65936002acd0" version="38.00.000">
                <common:shortDescription xml:lang="en">Total use of renewable primary energy resources (PERT)</common:shortDescription>
                <common:shortDescription xml:lang="de">Gesamtverbrauch von erneuerbarer Primärenergie (PERT)</common:shortDescription>
            </referenceToFlowDataSet>
            <functionType>General reminder flow</functionType>
            <exchangeDirection>Input</exchangeDirection>
            <meanAmount>0.0</meanAmount>
            <common:other>
                <epd:amount xmlns:epd="http://www.iai.kit.edu/EPD/2013" epd:module="A1-A3">141.0</epd:amount>
                <epd:amount xmlns:epd="http://www.iai.kit.edu/EPD/2013" epd:module="A4">9.6</epd:amount>
                <epd:amount xmlns:epd="http://www.iai.kit.edu/EPD/2013" epd:module="A5">4.44</epd:amount>
                <epd:amount xmlns:epd="http://www.iai.kit.edu/EPD/2013" epd:module="B2">0.19</epd:amount>
                <epd:amount xmlns:epd="http://www.iai.kit.edu/EPD/2013" epd:module="B3">0.0</epd:amount>
                <epd:amount xmlns:epd="http://www.iai.kit.edu/EPD/2013" epd:module="B4">147.0</epd:amount>
                <epd:amount xmlns:epd="http://www.iai.kit.edu/EPD/2013" epd:module="B5">0.0</epd:amount>
                <epd:amount xmlns:epd="http://www.iai.kit.edu/EPD/2013" epd:module="B6">0.0</epd:amount>
                <epd:amount xmlns:epd="http://www.iai.kit.edu/EPD/2013" epd:module="B7">0.0</epd:amount>
                <epd:amount xmlns:epd="http://www.iai.kit.edu/EPD/2013" epd:module="C1">0.0</epd:amount>
                <epd:amount xmlns:epd="http://www.iai.kit.edu/EPD/2013" epd:module="C2">0.13</epd:amount>
                <epd:amount xmlns:epd="http://www.iai.kit.edu/EPD/2013" epd:module="C3">10.5</epd:amount>
                <epd:amount xmlns:epd="http://www.iai.kit.edu/EPD/2013" epd:module="C4">1.08</epd:amount>
                <epd:amount xmlns:epd="http://www.iai.kit.edu/EPD/2013" epd:module="D">-19.3</epd:amount>
                <epd:referenceToUnitGroupDataSet xmlns:epd="http://www.iai.kit.edu/EPD/2013" refObjectId="93a60a57-a3c8-11da-a746-0800200c9a66" type="unit group data set" uri="../unitgroups/93a60a57-a3c8-11da-a746-0800200c9a66">
                    <common:shortDescription>MJ</common:shortDescription>
                </epd:referenceToUnitGroupDataSet>
            </common:other>
        </exchange>
    </exchanges>
    <LCIAResults>
        <LCIAResult>
            <referenceToLCIAMethodDataSet type="LCIA method data set" refObjectId="f7c73bb9-ab1a-4249-9c6d-379a0de6f67e" version="00.01.000">
                <common:shortDescription xml:lang="en">Abiotic depletion potential for non fossil resources (ADPE)</common:shortDescription>
                <common:shortDescription xml:lang="de">Potenzial für den abiotischen Abbau nicht fossiler Ressourcen (ADPE)</common:shortDescription>
                <common:shortDescription xml:lang="es">Potencial de agotamiento de recursos abióticos para recursos no fósiles (ADPE)</common:shortDescription>
            </referenceToLCIAMethodDataSet>
            <meanAmount>0.0</meanAmount>
            <common:other>
                <epd:amount xmlns:epd="http://www.iai.kit.edu/EPD/2013" epd:module="A1-A3">5.17E-4</epd:amount>
                <epd:amount xmlns:epd="http://www.iai.kit.edu/EPD/2013" epd:module="A4">1.1E-6</epd:amount>
                <epd:amount xmlns:epd="http://www.iai.kit.edu/EPD/2013" epd:module="A5">3.66E-8</epd:amount>
                <epd:amount xmlns:epd="http://www.iai.kit.edu/EPD/2013" epd:module="B2">4.53E-8</epd:amount>
                <epd:amount xmlns:epd="http://www.iai.kit.edu/EPD/2013" epd:module="B3">0.0</epd:amount>
                <epd:amount xmlns:epd="http://www.iai.kit.edu/EPD/2013" epd:module="B4">2.53E-4</epd:amount>
                <epd:amount xmlns:epd="http://www.iai.kit.edu/EPD/2013" epd:module="B5">0.0</epd:amount>
                <epd:amount xmlns:epd="http://www.iai.kit.edu/EPD/2013" epd:module="B6">0.0</epd:amount>
                <epd:amount xmlns:epd="http://www.iai.kit.edu/EPD/2013" epd:module="B7">0.0</epd:amount>
                <epd:amount xmlns:epd="http://www.iai.kit.edu/EPD/2013" epd:module="C1">0.0</epd:amount>
                <epd:amount xmlns:epd="http://www.iai.kit.edu/EPD/2013" epd:module="C2">1.52E-8</epd:amount>
                <epd:amount xmlns:epd="http://www.iai.kit.edu/EPD/2013" epd:module="C3">5.62E-7</epd:amount>
                <epd:amount xmlns:epd="http://www.iai.kit.edu/EPD/2013" epd:module="C4">2.11E-7</epd:amount>
                <epd:amount xmlns:epd="http://www.iai.kit.edu/EPD/2013" epd:module="D">-2.65E-4</epd:amount>
                <epd:referenceToUnitGroupDataSet xmlns:epd="http://www.iai.kit.edu/EPD/2013" refObjectId="54ccd2d9-a32a-4fc2-923d-f2c8c93e89d4" type="unit group data set" uri="../unitgroups/54ccd2d9-a32a-4fc2-923d-f2c8c93e89d4">
                    <common:shortDescription>kg Sb-Äqv.</common:shortDescription>
                </epd:referenceToUnitGroupDataSet>
            </common:other>
        </LCIAResult>
        <LCIAResult>
            <referenceToLCIAMethodDataSet type="LCIA method data set" refObjectId="804ebcdf-309d-4098-8ed8-fdaf2f389981" version="00.01.000">
                <common:shortDescription xml:lang="en">Abiotic depletion potential for fossil resources (ADPF)</common:shortDescription>
                <common:shortDescription xml:lang="de">Potenzial für den abiotischen Abbau fossiler Brennstoffe (ADPF)</common:shortDescription>
                <common:shortDescription xml:lang="es">Potencial de agotamiento de recursos abióticos para recursos fósiles (ADPF)</common:shortDescription>
            </referenceToLCIAMethodDataSet>
            <meanAmount>0.0</meanAmount>
            <common:other>
                <epd:amount xmlns:epd="http://www.iai.kit.edu/EPD/2013" epd:module="A1-A3">2110.0</epd:amount>
                <epd:amount xmlns:epd="http://www.iai.kit.edu/EPD/2013" epd:module="A4">172.0</epd:amount>
                <epd:amount xmlns:epd="http://www.iai.kit.edu/EPD/2013" epd:module="A5">0.66</epd:amount>
                <epd:amount xmlns:epd="http://www.iai.kit.edu/EPD/2013" epd:module="B2">15.4</epd:amount>
                <epd:amount xmlns:epd="http://www.iai.kit.edu/EPD/2013" epd:module="B3">0.0</epd:amount>
                <epd:amount xmlns:epd="http://www.iai.kit.edu/EPD/2013" epd:module="B4">1790.0</epd:amount>
                <epd:amount xmlns:epd="http://www.iai.kit.edu/EPD/2013" epd:module="B5">0.0</epd:amount>
                <epd:amount xmlns:epd="http://www.iai.kit.edu/EPD/2013" epd:module="B6">0.0</epd:amount>
                <epd:amount xmlns:epd="http://www.iai.kit.edu/EPD/2013" epd:module="B7">0.0</epd:amount>
                <epd:amount xmlns:epd="http://www.iai.kit.edu/EPD/2013" epd:module="C1">0.0</epd:amount>
                <epd:amount xmlns:epd="http://www.iai.kit.edu/EPD/2013" epd:module="C2">2.37</epd:amount>
                <epd:amount xmlns:epd="http://www.iai.kit.edu/EPD/2013" epd:module="C3">12.8</epd:amount>
                <epd:amount xmlns:epd="http://www.iai.kit.edu/EPD/2013" epd:module="C4">7.83</epd:amount>
                <epd:amount xmlns:epd="http://www.iai.kit.edu/EPD/2013" epd:module="D">-516.0</epd:amount>
                <epd:referenceToUnitGroupDataSet xmlns:epd="http://www.iai.kit.edu/EPD/2013" refObjectId="93a60a57-a3c8-11da-a746-0800200c9a66" type="unit group data set" uri="../unitgroups/93a60a57-a3c8-11da-a746-0800200c9a66">
                    <common:shortDescription>MJ</common:shortDescription>
                </epd:referenceToUnitGroupDataSet>
            </common:other>
        </LCIAResult>
        <LCIAResult>
            <referenceToLCIAMethodDataSet type="LCIA method data set" refObjectId="b4274add-93b7-4905-a5e4-2e878c4e4216" version="00.01.000">
                <common:shortDescription xml:lang="en">Acidification potential of soil and water (AP)</common:shortDescription>
                <common:shortDescription xml:lang="de">Versauerungspotenzial von Boden und Wasser (AP)</common:shortDescription>
                <common:shortDescription xml:lang="es">Potencial de acidificación del suelo y de los recursos de agua (AP)</common:shortDescription>
            </referenceToLCIAMethodDataSet>
            <meanAmount>0.0</meanAmount>
            <common:other>
                <epd:amount xmlns:epd="http://www.iai.kit.edu/EPD/2013" epd:module="A1-A3">0.49</epd:amount>
                <epd:amount xmlns:epd="http://www.iai.kit.edu/EPD/2013" epd:module="A4">0.0207</epd:amount>
                <epd:amount xmlns:epd="http://www.iai.kit.edu/EPD/2013" epd:module="A5">3.5E-4</epd:amount>
                <epd:amount xmlns:epd="http://www.iai.kit.edu/EPD/2013" epd:module="B2">8.79E-4</epd:amount>
                <epd:amount xmlns:epd="http://www.iai.kit.edu/EPD/2013" epd:module="B3">0.0</epd:amount>
                <epd:amount xmlns:epd="http://www.iai.kit.edu/EPD/2013" epd:module="B4">0.41</epd:amount>
                <epd:amount xmlns:epd="http://www.iai.kit.edu/EPD/2013" epd:module="B5">0.0</epd:amount>
                <epd:amount xmlns:epd="http://www.iai.kit.edu/EPD/2013" epd:module="B6">0.0</epd:amount>
                <epd:amount xmlns:epd="http://www.iai.kit.edu/EPD/2013" epd:module="B7">0.0</epd:amount>
                <epd:amount xmlns:epd="http://www.iai.kit.edu/EPD/2013" epd:module="C1">0.0</epd:amount>
                <epd:amount xmlns:epd="http://www.iai.kit.edu/EPD/2013" epd:module="C2">6.92E-4</epd:amount>
                <epd:amount xmlns:epd="http://www.iai.kit.edu/EPD/2013" epd:module="C3">0.00164</epd:amount>
                <epd:amount xmlns:epd="http://www.iai.kit.edu/EPD/2013" epd:module="C4">0.00346</epd:amount>
                <epd:amount xmlns:epd="http://www.iai.kit.edu/EPD/2013" epd:module="D">-0.11</epd:amount>
                <epd:referenceToUnitGroupDataSet xmlns:epd="http://www.iai.kit.edu/EPD/2013" refObjectId="bc50c624-a9bc-45b1-a9b0-e6b10d00476f" type="unit group data set" uri="../unitgroups/bc50c624-a9bc-45b1-a9b0-e6b10d00476f">
                    <common:shortDescription>kg SO2-Äqv.</common:shortDescription>
                </epd:referenceToUnitGroupDataSet>
            </common:other>
        </LCIAResult>
        <LCIAResult>
            <referenceToLCIAMethodDataSet type="LCIA method data set" refObjectId="f58827d0-b407-4ec6-be75-8b69efb98a0f" version="00.01.000">
                <common:shortDescription xml:lang="en">Eutrophication potential (EP)</common:shortDescription>
                <common:shortDescription xml:lang="de">Eutrophierungspotenzial (EP)</common:shortDescription>
                <common:shortDescription xml:lang="es">Potencial de eutrofización (EP)</common:shortDescription>
            </referenceToLCIAMethodDataSet>
            <meanAmount>0.0</meanAmount>
            <common:other>
                <epd:amount xmlns:epd="http://www.iai.kit.edu/EPD/2013" epd:module="A1-A3">0.071</epd:amount>
                <epd:amount xmlns:epd="http://www.iai.kit.edu/EPD/2013" epd:module="A4">0.00505</epd:amount>
                <epd:amount xmlns:epd="http://www.iai.kit.edu/EPD/2013" epd:module="A5">7.84E-5</epd:amount>
                <epd:amount xmlns:epd="http://www.iai.kit.edu/EPD/2013" epd:module="B2">7.34E-5</epd:amount>
                <epd:amount xmlns:epd="http://www.iai.kit.edu/EPD/2013" epd:module="B3">0.0</epd:amount>
                <epd:amount xmlns:epd="http://www.iai.kit.edu/EPD/2013" epd:module="B4">0.0666</epd:amount>
                <epd:amount xmlns:epd="http://www.iai.kit.edu/EPD/2013" epd:module="B5">0.0</epd:amount>
                <epd:amount xmlns:epd="http://www.iai.kit.edu/EPD/2013" epd:module="B6">0.0</epd:amount>
                <epd:amount xmlns:epd="http://www.iai.kit.edu/EPD/2013" epd:module="B7">0.0</epd:amount>
                <epd:amount xmlns:epd="http://www.iai.kit.edu/EPD/2013" epd:module="C1">0.0</epd:amount>
                <epd:amount xmlns:epd="http://www.iai.kit.edu/EPD/2013" epd:module="C2">1.75E-4</epd:amount>
                <epd:amount xmlns:epd="http://www.iai.kit.edu/EPD/2013" epd:module="C3">3.05E-4</epd:amount>
                <epd:amount xmlns:epd="http://www.iai.kit.edu/EPD/2013" epd:module="C4">3.93E-4</epd:amount>
                <epd:amount xmlns:epd="http://www.iai.kit.edu/EPD/2013" epd:module="D">-0.0104</epd:amount>
                <epd:referenceToUnitGroupDataSet xmlns:epd="http://www.iai.kit.edu/EPD/2013" refObjectId="67b5401d-873c-485f-bcf3-6ae83b918822" type="unit group data set" uri="../unitgroups/67b5401d-873c-485f-bcf3-6ae83b918822">
                    <common:shortDescription>kg Phosphat-Äqv.</common:shortDescription>
                </epd:referenceToUnitGroupDataSet>
            </common:other>
        </LCIAResult>
        <LCIAResult>
            <referenceToLCIAMethodDataSet type="LCIA method data set" refObjectId="77e416eb-a363-4258-a04e-171d843a6460" version="00.01.000">
                <common:shortDescription xml:lang="en">Global warming potential (GWP)</common:shortDescription>
                <common:shortDescription xml:lang="de">Globales Erwärmungspotenzial (GWP)</common:shortDescription>
                <common:shortDescription xml:lang="es">Potencial de calentamiento global (GWP)</common:shortDescription>
            </referenceToLCIAMethodDataSet>
            <meanAmount>0.0</meanAmount>
            <common:other>
                <epd:amount xmlns:epd="http://www.iai.kit.edu/EPD/2013" epd:module="A1-A3">172.0</epd:amount>
                <epd:amount xmlns:epd="http://www.iai.kit.edu/EPD/2013" epd:module="A4">12.6</epd:amount>
                <epd:amount xmlns:epd="http://www.iai.kit.edu/EPD/2013" epd:module="A5">3.03</epd:amount>
                <epd:amount xmlns:epd="http://www.iai.kit.edu/EPD/2013" epd:module="B2">0.31</epd:amount>
                <epd:amount xmlns:epd="http://www.iai.kit.edu/EPD/2013" epd:module="B3">0.0</epd:amount>
                <epd:amount xmlns:epd="http://www.iai.kit.edu/EPD/2013" epd:module="B4">140.0</epd:amount>
                <epd:amount xmlns:epd="http://www.iai.kit.edu/EPD/2013" epd:module="B5">0.0</epd:amount>
                <epd:amount xmlns:epd="http://www.iai.kit.edu/EPD/2013" epd:module="B6">0.0</epd:amount>
                <epd:amount xmlns:epd="http://www.iai.kit.edu/EPD/2013" epd:module="B7">0.0</epd:amount>
                <epd:amount xmlns:epd="http://www.iai.kit.edu/EPD/2013" epd:module="C1">0.0</epd:amount>
                <epd:amount xmlns:epd="http://www.iai.kit.edu/EPD/2013" epd:module="C2">0.17</epd:amount>
                <epd:amount xmlns:epd="http://www.iai.kit.edu/EPD/2013" epd:module="C3">1.26</epd:amount>
                <epd:amount xmlns:epd="http://www.iai.kit.edu/EPD/2013" epd:module="C4">0.57</epd:amount>
                <epd:amount xmlns:epd="http://www.iai.kit.edu/EPD/2013" epd:module="D">-50.3</epd:amount>
                <epd:referenceToUnitGroupDataSet xmlns:epd="http://www.iai.kit.edu/EPD/2013" refObjectId="1ebf3012-d0db-4de2-aefd-ef30cedb0be1" type="unit group data set" uri="../unitgroups/1ebf3012-d0db-4de2-aefd-ef30cedb0be1">
                    <common:shortDescription>kg CO2-Äqv.</common:shortDescription>
                </epd:referenceToUnitGroupDataSet>
            </common:other>
        </LCIAResult>
        <LCIAResult>
            <referenceToLCIAMethodDataSet type="LCIA method data set" refObjectId="06dcd26f-025f-401a-a7c1-5e457eb54637" version="00.01.000">
                <common:shortDescription xml:lang="en">Depletion potential of the stratospheric ozone layer (ODP)</common:shortDescription>
                <common:shortDescription xml:lang="de">Abbau Potential der stratosphärischen Ozonschicht (ODP)</common:shortDescription>
                <common:shortDescription xml:lang="es">Potencial de agotamiento de la capa de ozono estratosférico (ODP)</common:shortDescription>
            </referenceToLCIAMethodDataSet>
            <meanAmount>0.0</meanAmount>
            <common:other>
                <epd:amount xmlns:epd="http://www.iai.kit.edu/EPD/2013" epd:module="A1-A3">3.96E-6</epd:amount>
                <epd:amount xmlns:epd="http://www.iai.kit.edu/EPD/2013" epd:module="A4">2.2E-15</epd:amount>
                <epd:amount xmlns:epd="http://www.iai.kit.edu/EPD/2013" epd:module="A5">8.88E-16</epd:amount>
                <epd:amount xmlns:epd="http://www.iai.kit.edu/EPD/2013" epd:module="B2">7.22E-16</epd:amount>
                <epd:amount xmlns:epd="http://www.iai.kit.edu/EPD/2013" epd:module="B3">0.0</epd:amount>
                <epd:amount xmlns:epd="http://www.iai.kit.edu/EPD/2013" epd:module="B4">3.96E-6</epd:amount>
                <epd:amount xmlns:epd="http://www.iai.kit.edu/EPD/2013" epd:module="B5">0.0</epd:amount>
                <epd:amount xmlns:epd="http://www.iai.kit.edu/EPD/2013" epd:module="B6">0.0</epd:amount>
                <epd:amount xmlns:epd="http://www.iai.kit.edu/EPD/2013" epd:module="B7">0.0</epd:amount>
                <epd:amount xmlns:epd="http://www.iai.kit.edu/EPD/2013" epd:module="C1">0.0</epd:amount>
                <epd:amount xmlns:epd="http://www.iai.kit.edu/EPD/2013" epd:module="C2">3.04E-17</epd:amount>
                <epd:amount xmlns:epd="http://www.iai.kit.edu/EPD/2013" epd:module="C3">5.77E-14</epd:amount>
                <epd:amount xmlns:epd="http://www.iai.kit.edu/EPD/2013" epd:module="C4">3.14E-15</epd:amount>
                <epd:amount xmlns:epd="http://www.iai.kit.edu/EPD/2013" epd:module="D">-6.54E-13</epd:amount>
                <epd:referenceToUnitGroupDataSet xmlns:epd="http://www.iai.kit.edu/EPD/2013" refObjectId="88054749-b0a6-47ea-a82b-dc5b29326512" type="unit group data set" uri="../unitgroups/88054749-b0a6-47ea-a82b-dc5b29326512">
                    <common:shortDescription>kg R11 eq.</common:shortDescription>
                </epd:referenceToUnitGroupDataSet>
            </common:other>
        </LCIAResult>
        <LCIAResult>
            <referenceToLCIAMethodDataSet type="LCIA method data set" refObjectId="1e84a202-dae6-42aa-9e9d-71ea48b8be00" version="00.01.000">
                <common:shortDescription xml:lang="en">Formation potential of tropospheric ozone (POCP)</common:shortDescription>
                <common:shortDescription xml:lang="de">Bildungspotential für troposphärisches Ozon (POCP)</common:shortDescription>
                <common:shortDescription xml:lang="es">Potencial de formación de ozono troposférico (POCP)</common:shortDescription>
            </referenceToLCIAMethodDataSet>
            <meanAmount>0.0</meanAmount>
            <common:other>
                <epd:amount xmlns:epd="http://www.iai.kit.edu/EPD/2013" epd:module="A1-A3">0.045</epd:amount>
                <epd:amount xmlns:epd="http://www.iai.kit.edu/EPD/2013" epd:module="A4">-0.006</epd:amount>
                <epd:amount xmlns:epd="http://www.iai.kit.edu/EPD/2013" epd:module="A5">2.43E-5</epd:amount>
                <epd:amount xmlns:epd="http://www.iai.kit.edu/EPD/2013" epd:module="B2">1.4E-4</epd:amount>
                <epd:amount xmlns:epd="http://www.iai.kit.edu/EPD/2013" epd:module="B3">0.0</epd:amount>
                <epd:amount xmlns:epd="http://www.iai.kit.edu/EPD/2013" epd:module="B4">0.0218</epd:amount>
                <epd:amount xmlns:epd="http://www.iai.kit.edu/EPD/2013" epd:module="B5">0.0</epd:amount>
                <epd:amount xmlns:epd="http://www.iai.kit.edu/EPD/2013" epd:module="B6">0.0</epd:amount>
                <epd:amount xmlns:epd="http://www.iai.kit.edu/EPD/2013" epd:module="B7">0.0</epd:amount>
                <epd:amount xmlns:epd="http://www.iai.kit.edu/EPD/2013" epd:module="C1">0.0</epd:amount>
                <epd:amount xmlns:epd="http://www.iai.kit.edu/EPD/2013" epd:module="C2">-2.65E-4</epd:amount>
                <epd:amount xmlns:epd="http://www.iai.kit.edu/EPD/2013" epd:module="C3">1.16E-4</epd:amount>
                <epd:amount xmlns:epd="http://www.iai.kit.edu/EPD/2013" epd:module="C4">2.63E-4</epd:amount>
                <epd:amount xmlns:epd="http://www.iai.kit.edu/EPD/2013" epd:module="D">-0.0174</epd:amount>
                <epd:referenceToUnitGroupDataSet xmlns:epd="http://www.iai.kit.edu/EPD/2013" refObjectId="01c26c17-9a76-406e-8295-f17b55fd909e" type="unit group data set" uri="../unitgroups/01c26c17-9a76-406e-8295-f17b55fd909e">
                    <common:shortDescription>kg Ethen-Äqv.</common:shortDescription>
                </epd:referenceToUnitGroupDataSet>
            </common:other>
        </LCIAResult>
    </LCIAResults>
</processDataSet>
