<?xml version="1.0" encoding="UTF-8" standalone="yes"?>
<processDataSet xmlns:m="http://lca.jrc.it/ILCD/LCIAMethod" xmlns:common="http://lca.jrc.it/ILCD/Common" xmlns:s="http://lca.jrc.it/ILCD/Source" xmlns:c="http://lca.jrc.it/ILCD/Contact" xmlns:f="http://lca.jrc.it/ILCD/Flow" xmlns="http://lca.jrc.it/ILCD/Process" xmlns:fp="http://lca.jrc.it/ILCD/FlowProperty" xmlns:u="http://lca.jrc.it/ILCD/UnitGroup" xmlns:epd2="http://www.indata.network/EPD/2019" xmlns:ns10="http://www.okworx.com/ILCD/Extensions/2018/Profile" version="1.1" epd2:epd-version="1.2" ns10:profile="EN_15804">
    <processInformation>
        <dataSetInformation>
            <common:UUID>41c5627a-4a1d-4e12-ac62-c1d4f1560fb9</common:UUID>
            <name>
                <baseName xml:lang="en">eLCA Luftschicht (gemäß EN 15804+A1)</baseName>
            </name>
            <classificationInformation>
                <common:classification name="oekobau.dat">
                    <common:class level="0" classId="9">Sonstige</common:class>
                    <common:class level="1" classId="9.99">eLCA Intern</common:class>
                    <common:class level="2" classId="9.99.01">eLCA Intern</common:class>
                </common:classification>
            </classificationInformation>
            <common:generalComment xml:lang="en">Dieser Datensatz dient der Modellierung von Bauteilen und geht lastenfrei in die Bilanzierung ein.</common:generalComment>
        </dataSetInformation>
        <quantitativeReference type="Reference flow(s)">
            <referenceToReferenceFlow>1</referenceToReferenceFlow>
        </quantitativeReference>
    </processInformation>
    <modellingAndValidation>
        <LCIMethodAndAllocation>
            <typeOfDataSet>EPD</typeOfDataSet>
            <common:other>
                <epd:subType xmlns:epd="http://www.iai.kit.edu/EPD/2013">generic dataset</epd:subType>
            </common:other>
        </LCIMethodAndAllocation>
        <dataSourcesTreatmentAndRepresentativeness/>
        <validation/>
        <complianceDeclarations>
            <compliance>
                <common:referenceToComplianceSystem type="source data set" refObjectId="b00f9ec0-7874-11e3-981f-0800200c9a66" version="00.02.000">
                    <common:shortDescription xml:lang="de">EN 15804</common:shortDescription>
                    <common:shortDescription xml:lang="en">EN 15804</common:shortDescription>
                </common:referenceToComplianceSystem>
            </compliance>
        </complianceDeclarations>
    </modellingAndValidation>
    <administrativeInformation>
        <dataGenerator>
            <common:referenceToPersonOrEntityGeneratingTheDataSet type="contact data set" refObjectId="c59d4649-4b5c-4df1-a6f5-374923f0df63" version="00.00.002">
                <common:shortDescription xml:lang="en">Marc-William Siegert</common:shortDescription>
            </common:referenceToPersonOrEntityGeneratingTheDataSet>
        </dataGenerator>
        <dataEntryBy>
            <common:timeStamp>2021-06-24T11:00:35.876+02:00</common:timeStamp>
        </dataEntryBy>
        <publicationAndOwnership>
            <common:dataSetVersion>00.00.017</common:dataSetVersion>
            <common:referenceToOwnershipOfDataSet type="contact data set" refObjectId="f11651e0-7877-11e3-981f-0800200c9a66" version="00.01.000">
                <common:shortDescription xml:lang="en">The Federal Institute for Research on Building, Urban Affairs and Spatial Development (BBSR) within the Federal Office for Building and Regional Planning (BBR)</common:shortDescription>
                <common:shortDescription xml:lang="de">Bundesinstitut für Bau-, Stadt- und Raumforschung (BBSR) im Bundesamt für Bauwesen und Raumordnung (BBR)</common:shortDescription>
            </common:referenceToOwnershipOfDataSet>
            <common:licenseType>Free of charge for all users and uses</common:licenseType>
            <common:other>
                <ns9:referenceToPublisher xmlns:ns9="http://www.indata.network/EPD/2019" refObjectId="f11651e0-7877-11e3-981f-0800200c9a66" type="contact data set" version="00.01.000">
                    <common:shortDescription xml:lang="en">The Federal Institute for Research on Building, Urban Affairs and Spatial Development (BBSR) within the Federal Office for Building and Regional Planning (BBR)</common:shortDescription>
                    <common:shortDescription xml:lang="de">Bundesinstitut für Bau-, Stadt- und Raumforschung (BBSR) im Bundesamt für Bauwesen und Raumordnung (BBR)</common:shortDescription>
                </ns9:referenceToPublisher>
            </common:other>
        </publicationAndOwnership>
    </administrativeInformation>
    <exchanges>
        <exchange dataSetInternalID="1">
            <referenceToFlowDataSet type="flow data set" refObjectId="99d9eea1-583c-467b-9210-5e808a78586e" version="00.00.007">
                <common:shortDescription xml:lang="en">eLCA Luftschicht</common:shortDescription>
            </referenceToFlowDataSet>
            <meanAmount>1.0</meanAmount>
            <resultingAmount>1.0</resultingAmount>
        </exchange>
        <exchange dataSetInternalID="2">
            <referenceToFlowDataSet type="flow data set" refObjectId="a2b32f97-3fc7-4af2-b209-525bc6426f33" version="30.00.000">
                <common:shortDescription xml:lang="en">Components for re-use (CRU)</common:shortDescription>
                <common:shortDescription xml:lang="de">Komponenten für die Wiederverwendung (CRU)</common:shortDescription>
                <common:shortDescription xml:lang="es">Componentes para su reutilización (CRU)</common:shortDescription>
            </referenceToFlowDataSet>
            <functionType>General reminder flow</functionType>
            <exchangeDirection>Output</exchangeDirection>
            <meanAmount>0.0</meanAmount>
            <common:other>
                <epd:amount xmlns:epd="http://www.iai.kit.edu/EPD/2013" epd:module="C3">0.0</epd:amount>
                <epd:amount xmlns:epd="http://www.iai.kit.edu/EPD/2013" epd:module="A1-A3">0.0</epd:amount>
                <epd:amount xmlns:epd="http://www.iai.kit.edu/EPD/2013" epd:module="C4">0.0</epd:amount>
                <epd:referenceToUnitGroupDataSet xmlns:epd="http://www.iai.kit.edu/EPD/2013" refObjectId="ad38d542-3fe9-439d-9b95-2f5f7752acaf" type="unit group data set" uri="../unitgroups/ad38d542-3fe9-439d-9b95-2f5f7752acaf">
                    <common:shortDescription>kg</common:shortDescription>
                </epd:referenceToUnitGroupDataSet>
            </common:other>
        </exchange>
        <exchange dataSetInternalID="3">
            <referenceToFlowDataSet type="flow data set" refObjectId="4da0c987-2b76-40d6-9e9e-82a017aaaf29" version="30.00.000">
                <common:shortDescription xml:lang="en">Exported electrical energy (EEE)</common:shortDescription>
                <common:shortDescription xml:lang="de">Exportierte elektrische Energie (EEE)</common:shortDescription>
                <common:shortDescription xml:lang="es">Energía exportada electrica (EEE)</common:shortDescription>
            </referenceToFlowDataSet>
            <functionType>General reminder flow</functionType>
            <exchangeDirection>Output</exchangeDirection>
            <meanAmount>0.0</meanAmount>
            <common:other>
                <epd:amount xmlns:epd="http://www.iai.kit.edu/EPD/2013" epd:module="C3">0.0</epd:amount>
                <epd:amount xmlns:epd="http://www.iai.kit.edu/EPD/2013" epd:module="A1-A3">0.0</epd:amount>
                <epd:amount xmlns:epd="http://www.iai.kit.edu/EPD/2013" epd:module="C4">0.0</epd:amount>
                <epd:referenceToUnitGroupDataSet xmlns:epd="http://www.iai.kit.edu/EPD/2013" refObjectId="93a60a57-a3c8-11da-a746-0800200c9a66" type="unit group data set" uri="../unitgroups/93a60a57-a3c8-11da-a746-0800200c9a66">
                    <common:shortDescription>MJ</common:shortDescription>
                </epd:referenceToUnitGroupDataSet>
            </common:other>
        </exchange>
        <exchange dataSetInternalID="4">
            <referenceToFlowDataSet type="flow data set" refObjectId="98daf38a-7a79-46d3-9a37-2b7bd0955810" version="30.00.000">
                <common:shortDescription xml:lang="en">Exported thermal energy (EET)</common:shortDescription>
                <common:shortDescription xml:lang="de">Exportierte thermische Energie (EET)</common:shortDescription>
                <common:shortDescription xml:lang="es">Energía exportada termal (EET)</common:shortDescription>
            </referenceToFlowDataSet>
            <functionType>General reminder flow</functionType>
            <exchangeDirection>Output</exchangeDirection>
            <meanAmount>0.0</meanAmount>
            <common:other>
                <epd:amount xmlns:epd="http://www.iai.kit.edu/EPD/2013" epd:module="C3">0.0</epd:amount>
                <epd:amount xmlns:epd="http://www.iai.kit.edu/EPD/2013" epd:module="A1-A3">0.0</epd:amount>
                <epd:amount xmlns:epd="http://www.iai.kit.edu/EPD/2013" epd:module="C4">0.0</epd:amount>
                <epd:referenceToUnitGroupDataSet xmlns:epd="http://www.iai.kit.edu/EPD/2013" refObjectId="93a60a57-a3c8-11da-a746-0800200c9a66" type="unit group data set" uri="../unitgroups/93a60a57-a3c8-11da-a746-0800200c9a66">
                    <common:shortDescription>MJ</common:shortDescription>
                </epd:referenceToUnitGroupDataSet>
            </common:other>
        </exchange>
        <exchange dataSetInternalID="5">
            <referenceToFlowDataSet type="flow data set" refObjectId="430f9e0f-59b2-46a0-8e0d-55e0e84948fc" version="30.00.000">
                <common:shortDescription xml:lang="en">Hazardous waste disposed (HWD)</common:shortDescription>
                <common:shortDescription xml:lang="de">Gefährlicher Abfall zur Deponie (HWD)</common:shortDescription>
                <common:shortDescription xml:lang="es">Residuos peligrosos eliminados (HWD)</common:shortDescription>
            </referenceToFlowDataSet>
            <functionType>General reminder flow</functionType>
            <exchangeDirection>Output</exchangeDirection>
            <meanAmount>0.0</meanAmount>
            <common:other>
                <epd:amount xmlns:epd="http://www.iai.kit.edu/EPD/2013" epd:module="C3">0.0</epd:amount>
                <epd:amount xmlns:epd="http://www.iai.kit.edu/EPD/2013" epd:module="A1-A3">0.0</epd:amount>
                <epd:amount xmlns:epd="http://www.iai.kit.edu/EPD/2013" epd:module="C4">0.0</epd:amount>
                <epd:referenceToUnitGroupDataSet xmlns:epd="http://www.iai.kit.edu/EPD/2013" refObjectId="ad38d542-3fe9-439d-9b95-2f5f7752acaf" type="unit group data set" uri="../unitgroups/ad38d542-3fe9-439d-9b95-2f5f7752acaf">
                    <common:shortDescription>kg</common:shortDescription>
                </epd:referenceToUnitGroupDataSet>
            </common:other>
        </exchange>
        <exchange dataSetInternalID="6">
            <referenceToFlowDataSet type="flow data set" refObjectId="59a9181c-3aaf-46ee-8b13-2b3723b6e447" version="30.00.000">
                <common:shortDescription xml:lang="en">Materials for energy recovery (MER)</common:shortDescription>
                <common:shortDescription xml:lang="de">Stoffe für die Energierückgewinnung (MER)</common:shortDescription>
                <common:shortDescription xml:lang="es">Materiales para valorización energética (recuperación de energía) (MER)</common:shortDescription>
            </referenceToFlowDataSet>
            <functionType>General reminder flow</functionType>
            <exchangeDirection>Output</exchangeDirection>
            <meanAmount>0.0</meanAmount>
            <common:other>
                <epd:amount xmlns:epd="http://www.iai.kit.edu/EPD/2013" epd:module="C3">0.0</epd:amount>
                <epd:amount xmlns:epd="http://www.iai.kit.edu/EPD/2013" epd:module="A1-A3">0.0</epd:amount>
                <epd:amount xmlns:epd="http://www.iai.kit.edu/EPD/2013" epd:module="C4">0.0</epd:amount>
                <epd:referenceToUnitGroupDataSet xmlns:epd="http://www.iai.kit.edu/EPD/2013" refObjectId="ad38d542-3fe9-439d-9b95-2f5f7752acaf" type="unit group data set" uri="../unitgroups/ad38d542-3fe9-439d-9b95-2f5f7752acaf">
                    <common:shortDescription>kg</common:shortDescription>
                </epd:referenceToUnitGroupDataSet>
            </common:other>
        </exchange>
        <exchange dataSetInternalID="7">
            <referenceToFlowDataSet type="flow data set" refObjectId="d7fe48a5-4103-49c8-9aae-b0b5dfdbd6ae" version="30.00.000">
                <common:shortDescription xml:lang="en">Materials for recycling (MFR)</common:shortDescription>
                <common:shortDescription xml:lang="de">Stoffe zum Recycling (MFR)</common:shortDescription>
                <common:shortDescription xml:lang="es">Materiales para el reciclaje (MFR)</common:shortDescription>
            </referenceToFlowDataSet>
            <functionType>General reminder flow</functionType>
            <exchangeDirection>Output</exchangeDirection>
            <meanAmount>0.0</meanAmount>
            <common:other>
                <epd:amount xmlns:epd="http://www.iai.kit.edu/EPD/2013" epd:module="C3">0.0</epd:amount>
                <epd:amount xmlns:epd="http://www.iai.kit.edu/EPD/2013" epd:module="A1-A3">0.0</epd:amount>
                <epd:amount xmlns:epd="http://www.iai.kit.edu/EPD/2013" epd:module="C4">0.0</epd:amount>
                <epd:referenceToUnitGroupDataSet xmlns:epd="http://www.iai.kit.edu/EPD/2013" refObjectId="ad38d542-3fe9-439d-9b95-2f5f7752acaf" type="unit group data set" uri="../unitgroups/ad38d542-3fe9-439d-9b95-2f5f7752acaf">
                    <common:shortDescription>kg</common:shortDescription>
                </epd:referenceToUnitGroupDataSet>
            </common:other>
        </exchange>
        <exchange dataSetInternalID="8">
            <referenceToFlowDataSet type="flow data set" refObjectId="3cf952c8-f3a4-461d-8c96-96456ca62246" version="30.00.000">
                <common:shortDescription xml:lang="en">Use of net fresh water (FW)</common:shortDescription>
                <common:shortDescription xml:lang="de">Einsatz von Süßwasserressourcen (FW)</common:shortDescription>
                <common:shortDescription xml:lang="es">Uso neto de recursos de agua dulce (FW)</common:shortDescription>
            </referenceToFlowDataSet>
            <functionType>General reminder flow</functionType>
            <exchangeDirection>Input</exchangeDirection>
            <meanAmount>0.0</meanAmount>
            <common:other>
                <epd:amount xmlns:epd="http://www.iai.kit.edu/EPD/2013" epd:module="C3">0.0</epd:amount>
                <epd:amount xmlns:epd="http://www.iai.kit.edu/EPD/2013" epd:module="A1-A3">0.0</epd:amount>
                <epd:amount xmlns:epd="http://www.iai.kit.edu/EPD/2013" epd:module="C4">0.0</epd:amount>
                <epd:referenceToUnitGroupDataSet xmlns:epd="http://www.iai.kit.edu/EPD/2013" refObjectId="cd950537-0a98-4044-9ba7-9f9a68d0a504" type="unit group data set" uri="../unitgroups/cd950537-0a98-4044-9ba7-9f9a68d0a504">
                    <common:shortDescription>m3</common:shortDescription>
                </epd:referenceToUnitGroupDataSet>
            </common:other>
        </exchange>
        <exchange dataSetInternalID="9">
            <referenceToFlowDataSet type="flow data set" refObjectId="b29ef66b-e286-4afa-949f-62f1a7b4d7fa" version="30.00.000">
                <common:shortDescription xml:lang="en">Non hazardous waste dispose (NHWD)</common:shortDescription>
                <common:shortDescription xml:lang="de">Entsorgter nicht gefährlicher Abfall (NHWD)</common:shortDescription>
                <common:shortDescription xml:lang="es">Residuos no peligrosos eliminados (NHWD)</common:shortDescription>
            </referenceToFlowDataSet>
            <functionType>General reminder flow</functionType>
            <exchangeDirection>Output</exchangeDirection>
            <meanAmount>0.0</meanAmount>
            <common:other>
                <epd:amount xmlns:epd="http://www.iai.kit.edu/EPD/2013" epd:module="C3">0.0</epd:amount>
                <epd:amount xmlns:epd="http://www.iai.kit.edu/EPD/2013" epd:module="A1-A3">0.0</epd:amount>
                <epd:amount xmlns:epd="http://www.iai.kit.edu/EPD/2013" epd:module="C4">0.0</epd:amount>
                <epd:referenceToUnitGroupDataSet xmlns:epd="http://www.iai.kit.edu/EPD/2013" refObjectId="ad38d542-3fe9-439d-9b95-2f5f7752acaf" type="unit group data set" uri="../unitgroups/ad38d542-3fe9-439d-9b95-2f5f7752acaf">
                    <common:shortDescription>kg</common:shortDescription>
                </epd:referenceToUnitGroupDataSet>
            </common:other>
        </exchange>
        <exchange dataSetInternalID="10">
            <referenceToFlowDataSet type="flow data set" refObjectId="ac857178-2b45-46ec-892a-a9a4332f0372" version="30.00.000">
                <common:shortDescription xml:lang="en">Use of non renewable primary energy (PENRE)</common:shortDescription>
                <common:shortDescription xml:lang="de">Nicht-erneuerbare Primärenergie als Energieträger (PENRE)</common:shortDescription>
                <common:shortDescription xml:lang="es">Uso de energía primaria no renovable, excluyendo los recursos de energía primaria no renovable utilizada como materia prima (PENRE)</common:shortDescription>
            </referenceToFlowDataSet>
            <functionType>General reminder flow</functionType>
            <exchangeDirection>Input</exchangeDirection>
            <meanAmount>0.0</meanAmount>
            <common:other>
                <epd:amount xmlns:epd="http://www.iai.kit.edu/EPD/2013" epd:module="C3">0.0</epd:amount>
                <epd:amount xmlns:epd="http://www.iai.kit.edu/EPD/2013" epd:module="A1-A3">0.0</epd:amount>
                <epd:amount xmlns:epd="http://www.iai.kit.edu/EPD/2013" epd:module="C4">0.0</epd:amount>
                <epd:referenceToUnitGroupDataSet xmlns:epd="http://www.iai.kit.edu/EPD/2013" refObjectId="93a60a57-a3c8-11da-a746-0800200c9a66" type="unit group data set" uri="../unitgroups/93a60a57-a3c8-11da-a746-0800200c9a66">
                    <common:shortDescription>MJ</common:shortDescription>
                </epd:referenceToUnitGroupDataSet>
            </common:other>
        </exchange>
        <exchange dataSetInternalID="11">
            <referenceToFlowDataSet type="flow data set" refObjectId="1421caa0-679d-4bf4-b282-0eb850ccae27" version="30.00.000">
                <common:shortDescription xml:lang="en">Use of non renewable primary energy resources used as raw materials (PENRM)</common:shortDescription>
                <common:shortDescription xml:lang="de">Nicht-erneuerbare Primärenergie zur stofflichen Nutzung (PENRM)</common:shortDescription>
                <common:shortDescription xml:lang="es">Uso de la energía primaria no renovable utilizada como materia prima (PENRM)</common:shortDescription>
            </referenceToFlowDataSet>
            <functionType>General reminder flow</functionType>
            <exchangeDirection>Input</exchangeDirection>
            <meanAmount>0.0</meanAmount>
            <common:other>
                <epd:amount xmlns:epd="http://www.iai.kit.edu/EPD/2013" epd:module="C3">0.0</epd:amount>
                <epd:amount xmlns:epd="http://www.iai.kit.edu/EPD/2013" epd:module="A1-A3">0.0</epd:amount>
                <epd:amount xmlns:epd="http://www.iai.kit.edu/EPD/2013" epd:module="C4">0.0</epd:amount>
                <epd:referenceToUnitGroupDataSet xmlns:epd="http://www.iai.kit.edu/EPD/2013" refObjectId="93a60a57-a3c8-11da-a746-0800200c9a66" type="unit group data set" uri="../unitgroups/93a60a57-a3c8-11da-a746-0800200c9a66">
                    <common:shortDescription>MJ</common:shortDescription>
                </epd:referenceToUnitGroupDataSet>
            </common:other>
        </exchange>
        <exchange dataSetInternalID="12">
            <referenceToFlowDataSet type="flow data set" refObjectId="89def144-d39a-4287-b86f-efde453ddcb2" version="30.00.000">
                <common:shortDescription xml:lang="en">Use of non renewable secondary fuels (NRSF)</common:shortDescription>
                <common:shortDescription xml:lang="de">Nicht erneuerbare Sekundärbrennstoffe (NRSF)</common:shortDescription>
                <common:shortDescription xml:lang="es">Uso de combustibles secundarios no renovables (NRSF)</common:shortDescription>
            </referenceToFlowDataSet>
            <functionType>General reminder flow</functionType>
            <exchangeDirection>Input</exchangeDirection>
            <meanAmount>0.0</meanAmount>
            <common:other>
                <epd:amount xmlns:epd="http://www.iai.kit.edu/EPD/2013" epd:module="C3">0.0</epd:amount>
                <epd:amount xmlns:epd="http://www.iai.kit.edu/EPD/2013" epd:module="A1-A3">0.0</epd:amount>
                <epd:amount xmlns:epd="http://www.iai.kit.edu/EPD/2013" epd:module="C4">0.0</epd:amount>
                <epd:referenceToUnitGroupDataSet xmlns:epd="http://www.iai.kit.edu/EPD/2013" refObjectId="93a60a57-a3c8-11da-a746-0800200c9a66" type="unit group data set" uri="../unitgroups/93a60a57-a3c8-11da-a746-0800200c9a66">
                    <common:shortDescription>MJ</common:shortDescription>
                </epd:referenceToUnitGroupDataSet>
            </common:other>
        </exchange>
        <exchange dataSetInternalID="13">
            <referenceToFlowDataSet type="flow data set" refObjectId="3449546e-52ad-4b39-b809-9fb77cea8ff6" version="30.00.000">
                <common:shortDescription xml:lang="en">Radioactive waste disposed (RWD)</common:shortDescription>
                <common:shortDescription xml:lang="de">Entsorgter radioaktiver Abfall (RWD)</common:shortDescription>
                <common:shortDescription xml:lang="es">Residuos radiactivos eliminados (RWD)</common:shortDescription>
            </referenceToFlowDataSet>
            <functionType>General reminder flow</functionType>
            <exchangeDirection>Output</exchangeDirection>
            <meanAmount>0.0</meanAmount>
            <common:other>
                <epd:amount xmlns:epd="http://www.iai.kit.edu/EPD/2013" epd:module="C3">0.0</epd:amount>
                <epd:amount xmlns:epd="http://www.iai.kit.edu/EPD/2013" epd:module="A1-A3">0.0</epd:amount>
                <epd:amount xmlns:epd="http://www.iai.kit.edu/EPD/2013" epd:module="C4">0.0</epd:amount>
                <epd:referenceToUnitGroupDataSet xmlns:epd="http://www.iai.kit.edu/EPD/2013" refObjectId="ad38d542-3fe9-439d-9b95-2f5f7752acaf" type="unit group data set" uri="../unitgroups/ad38d542-3fe9-439d-9b95-2f5f7752acaf">
                    <common:shortDescription>kg</common:shortDescription>
                </epd:referenceToUnitGroupDataSet>
            </common:other>
        </exchange>
        <exchange dataSetInternalID="14">
            <referenceToFlowDataSet type="flow data set" refObjectId="20f32be5-0398-4288-9b6d-accddd195317" version="30.00.000">
                <common:shortDescription xml:lang="en">Use of renewable primary energy (PERE)</common:shortDescription>
                <common:shortDescription xml:lang="de">Erneuerbare Primärenergie als Energieträger (PERE)</common:shortDescription>
                <common:shortDescription xml:lang="es">Uso de energía primaria renovable excluyendo los recursos de energía primaria renovable utilizada como materia prima (PERE)</common:shortDescription>
            </referenceToFlowDataSet>
            <functionType>General reminder flow</functionType>
            <exchangeDirection>Input</exchangeDirection>
            <meanAmount>0.0</meanAmount>
            <common:other>
                <epd:amount xmlns:epd="http://www.iai.kit.edu/EPD/2013" epd:module="C3">0.0</epd:amount>
                <epd:amount xmlns:epd="http://www.iai.kit.edu/EPD/2013" epd:module="A1-A3">0.0</epd:amount>
                <epd:amount xmlns:epd="http://www.iai.kit.edu/EPD/2013" epd:module="C4">0.0</epd:amount>
                <epd:referenceToUnitGroupDataSet xmlns:epd="http://www.iai.kit.edu/EPD/2013" refObjectId="93a60a57-a3c8-11da-a746-0800200c9a66" type="unit group data set" uri="../unitgroups/93a60a57-a3c8-11da-a746-0800200c9a66">
                    <common:shortDescription>MJ</common:shortDescription>
                </epd:referenceToUnitGroupDataSet>
            </common:other>
        </exchange>
        <exchange dataSetInternalID="15">
            <referenceToFlowDataSet type="flow data set" refObjectId="fb3ec0de-548d-4508-aea5-00b73bf6f702" version="30.00.000">
                <common:shortDescription xml:lang="en">Use of renewable primary energy resources used as raw materials (PERM)</common:shortDescription>
                <common:shortDescription xml:lang="de">Erneuerbare Primärenergie zur stofflichen Nutzung (PERM)</common:shortDescription>
                <common:shortDescription xml:lang="es">Uso de energía primaria renovable utilizada como materia prima (PERM)</common:shortDescription>
            </referenceToFlowDataSet>
            <functionType>General reminder flow</functionType>
            <exchangeDirection>Input</exchangeDirection>
            <meanAmount>0.0</meanAmount>
            <common:other>
                <epd:amount xmlns:epd="http://www.iai.kit.edu/EPD/2013" epd:module="C3">0.0</epd:amount>
                <epd:amount xmlns:epd="http://www.iai.kit.edu/EPD/2013" epd:module="A1-A3">0.0</epd:amount>
                <epd:amount xmlns:epd="http://www.iai.kit.edu/EPD/2013" epd:module="C4">0.0</epd:amount>
                <epd:referenceToUnitGroupDataSet xmlns:epd="http://www.iai.kit.edu/EPD/2013" refObjectId="93a60a57-a3c8-11da-a746-0800200c9a66" type="unit group data set" uri="../unitgroups/93a60a57-a3c8-11da-a746-0800200c9a66">
                    <common:shortDescription>MJ</common:shortDescription>
                </epd:referenceToUnitGroupDataSet>
            </common:other>
        </exchange>
        <exchange dataSetInternalID="16">
            <referenceToFlowDataSet type="flow data set" refObjectId="64333088-a55f-4aa2-9a31-c10b07816787" version="30.00.000">
                <common:shortDescription xml:lang="en">Use of renewable secondary fuels (RSF)</common:shortDescription>
                <common:shortDescription xml:lang="de">Erneuerbare Sekundärbrennstoffe (RSF)</common:shortDescription>
                <common:shortDescription xml:lang="es">Uso de combustibles secundarios renovables (RSF)</common:shortDescription>
            </referenceToFlowDataSet>
            <functionType>General reminder flow</functionType>
            <exchangeDirection>Input</exchangeDirection>
            <meanAmount>0.0</meanAmount>
            <common:other>
                <epd:amount xmlns:epd="http://www.iai.kit.edu/EPD/2013" epd:module="C3">0.0</epd:amount>
                <epd:amount xmlns:epd="http://www.iai.kit.edu/EPD/2013" epd:module="A1-A3">0.0</epd:amount>
                <epd:amount xmlns:epd="http://www.iai.kit.edu/EPD/2013" epd:module="C4">0.0</epd:amount>
                <epd:referenceToUnitGroupDataSet xmlns:epd="http://www.iai.kit.edu/EPD/2013" refObjectId="93a60a57-a3c8-11da-a746-0800200c9a66" type="unit group data set" uri="../unitgroups/93a60a57-a3c8-11da-a746-0800200c9a66">
                    <common:shortDescription>MJ</common:shortDescription>
                </epd:referenceToUnitGroupDataSet>
            </common:other>
        </exchange>
        <exchange dataSetInternalID="17">
            <referenceToFlowDataSet type="flow data set" refObjectId="c6a1f35f-2d09-4f54-8dfb-97e502e1ce92" version="30.00.000">
                <common:shortDescription xml:lang="en">Use of secondary material (SM)</common:shortDescription>
                <common:shortDescription xml:lang="de">Einsatz von Sekundärstoffen (SM)</common:shortDescription>
                <common:shortDescription xml:lang="es">Uso de materiales secundarios (SM)</common:shortDescription>
            </referenceToFlowDataSet>
            <functionType>General reminder flow</functionType>
            <exchangeDirection>Input</exchangeDirection>
            <meanAmount>0.0</meanAmount>
            <common:other>
                <epd:amount xmlns:epd="http://www.iai.kit.edu/EPD/2013" epd:module="C3">0.0</epd:amount>
                <epd:amount xmlns:epd="http://www.iai.kit.edu/EPD/2013" epd:module="A1-A3">0.0</epd:amount>
                <epd:amount xmlns:epd="http://www.iai.kit.edu/EPD/2013" epd:module="C4">0.0</epd:amount>
                <epd:referenceToUnitGroupDataSet xmlns:epd="http://www.iai.kit.edu/EPD/2013" refObjectId="ad38d542-3fe9-439d-9b95-2f5f7752acaf" type="unit group data set" uri="../unitgroups/ad38d542-3fe9-439d-9b95-2f5f7752acaf">
                    <common:shortDescription>kg</common:shortDescription>
                </epd:referenceToUnitGroupDataSet>
            </common:other>
        </exchange>
        <exchange dataSetInternalID="18">
            <referenceToFlowDataSet type="flow data set" refObjectId="06159210-646b-4c8d-8583-da9b3b95a6c1" version="30.00.000">
                <common:shortDescription xml:lang="en">Total use of non renewable primary energy resource (PENRT)</common:shortDescription>
                <common:shortDescription xml:lang="de">Total nicht erneuerbare Primärenergie (PENRT)</common:shortDescription>
                <common:shortDescription xml:lang="es">Uso total de la energía primaria no renovable (energía primaria y recursos de energía primaria renovable utilizada como materia prima) (PENRT)</common:shortDescription>
            </referenceToFlowDataSet>
            <functionType>General reminder flow</functionType>
            <exchangeDirection>Input</exchangeDirection>
            <meanAmount>0.0</meanAmount>
            <common:other>
                <epd:amount xmlns:epd="http://www.iai.kit.edu/EPD/2013" epd:module="C3">0.0</epd:amount>
                <epd:amount xmlns:epd="http://www.iai.kit.edu/EPD/2013" epd:module="A1-A3">0.0</epd:amount>
                <epd:amount xmlns:epd="http://www.iai.kit.edu/EPD/2013" epd:module="C4">0.0</epd:amount>
                <epd:referenceToUnitGroupDataSet xmlns:epd="http://www.iai.kit.edu/EPD/2013" refObjectId="93a60a57-a3c8-11da-a746-0800200c9a66" type="unit group data set" uri="../unitgroups/93a60a57-a3c8-11da-a746-0800200c9a66">
                    <common:shortDescription>MJ</common:shortDescription>
                </epd:referenceToUnitGroupDataSet>
            </common:other>
        </exchange>
        <exchange dataSetInternalID="19">
            <referenceToFlowDataSet type="flow data set" refObjectId="53f97275-fa8a-4cdd-9024-65936002acd0" version="30.00.000">
                <common:shortDescription xml:lang="en">Total use of renewable primary energy resources (PERT)</common:shortDescription>
                <common:shortDescription xml:lang="de">Total erneuerbare Primärenergie (PERT)</common:shortDescription>
                <common:shortDescription xml:lang="es">Uso total de la energía primaria renovable (energía primaria y recursos de energía primaria renovable utilizada como materia prima) (PERT)</common:shortDescription>
            </referenceToFlowDataSet>
            <functionType>General reminder flow</functionType>
            <exchangeDirection>Input</exchangeDirection>
            <meanAmount>0.0</meanAmount>
            <common:other>
                <epd:amount xmlns:epd="http://www.iai.kit.edu/EPD/2013" epd:module="C3">0.0</epd:amount>
                <epd:amount xmlns:epd="http://www.iai.kit.edu/EPD/2013" epd:module="A1-A3">0.0</epd:amount>
                <epd:amount xmlns:epd="http://www.iai.kit.edu/EPD/2013" epd:module="C4">0.0</epd:amount>
                <epd:referenceToUnitGroupDataSet xmlns:epd="http://www.iai.kit.edu/EPD/2013" refObjectId="93a60a57-a3c8-11da-a746-0800200c9a66" type="unit group data set" uri="../unitgroups/93a60a57-a3c8-11da-a746-0800200c9a66">
                    <common:shortDescription>MJ</common:shortDescription>
                </epd:referenceToUnitGroupDataSet>
            </common:other>
        </exchange>
    </exchanges>
</processDataSet>
