<?xml version="1.0" encoding="utf-8"?>
<processDataSet xmlns:epd="http://www.iai.kit.edu/EPD/2013" xmlns:epd2="http://www.indata.network/EPD/2019" xmlns:common="http://lca.jrc.it/ILCD/Common" xsi:schemaLocation="http://lca.jrc.it/ILCD/Process ../../schemas/EPD_DataSet.xsd" epd2:epd-version="1.2" version="1.1" locations="../ILCDLocations.xml" xmlns:xsi="http://www.w3.org/2001/XMLSchema-instance" xmlns="http://lca.jrc.it/ILCD/Process">
<processInformation>
<dataSetInformation>
<common:UUID>454fd5d6-5637-4881-ad4f-7925fd784d3a</common:UUID>
<name>
<baseName xml:lang="de">Sarnafil TS 77-E</baseName>
<baseName xml:lang="en">Sarnafil TS 77-E</baseName>
<functionalUnitFlowProperties xml:lang="de" />
</name>
<classificationInformation>
<common:classification name="OEKOBAU.DAT">
<common:class level="0" classId="6">Kunststoffe</common:class>
<common:class level="1" classId="6.3">Dachbahnen</common:class>
<common:class level="2" classId="6.3.05">TPO-Dachbahnen (FPO)</common:class>
</common:classification>
<common:classification name="IBUCategories">
<common:class level="0">02 Bauprodukte</common:class>
<common:class level="1">Abdichtungen</common:class>
<common:class level="2">Dach- und Dichtungsbahnsysteme aus Kunststoffen und Elastomeren</common:class>
</common:classification>
</classificationInformation>
<common:generalComment xml:lang="de">Sarnafil® TS 77-E Kunststoffabdichtungsbahnen beste-hen aus flexiblen Polyolefinen (FPO) und werden zu-sätzlich mit UV-Lichtschutzmittel und Flammschutz-mittel ausgerüstet. Als Verstärkung dient eine innen-liegende Kombination aus Glasvlies und Polyester-gelege. Die Sarnafil® TS 77-E Kunststoffabdichtungs-bahnen sind in den Dicken 1,5 mm (TS 77-15 E), 1,8 mm (TS 77-18 E) und 2,0 mm (TS 77-20 E) erhältlich.</common:generalComment>
<common:generalComment xml:lang="en">Sarnafil® TS 77-E polymeric waterproofing membrane is made of flexible polyolefin (FPO) and is treated with flame retardant and stabilizers against UV radiation. An inlay of glass non-woven and polyester reinforcement is encapsulated within the sheet. Sarnafil® TS 77-E polymeric waterproofing membrane is available in the following thicknesses: 1.5 mm (TS 77-15 E), 1.8 mm (TS 77-18 E) and 2.0 mm (TS 77-20 E).</common:generalComment>
<common:other>
<epd:scenarios>
<epd:scenario epd:default="true" epd:name="S0">
<epd:description xml:lang="de">Szenario 0</epd:description>
<epd:description xml:lang="en">Scenario 0</epd:description>
</epd:scenario>
<epd:scenario epd:name="S1">
<epd:description xml:lang="de">100 % Recycling</epd:description>
<epd:description xml:lang="en">100% recycling</epd:description>
</epd:scenario>
<epd:scenario epd:name="S2">
<epd:description xml:lang="de">100 % thermische Verwertung</epd:description>
<epd:description xml:lang="en">100% thermal energy recovery</epd:description>
</epd:scenario>
</epd:scenarios>
</common:other>
</dataSetInformation>
<quantitativeReference>
<referenceToReferenceFlow>0</referenceToReferenceFlow>
</quantitativeReference>
<time>
<common:referenceYear>2020</common:referenceYear>
<common:dataSetValidUntil>2025</common:dataSetValidUntil>
<common:other>
<epd2:publicationDateOfEPD>2020-04-24</epd2:publicationDateOfEPD>
</common:other>
</time>
<geography>
<locationOfOperationSupplyOrProduction location="DE" />
</geography>
<technology>
<technologyDescriptionAndIncludedProcesses xml:lang="de">Der Herstellungsprozess der Sarnafil® TS 77-E Kunst-stoffabdichtungsbahnen verläuft auf eigens entwickel-ten Produktionsanlagen in folgenden Schritten: Aufschmelzen der Kunststoffkomponenten sowie ihrer Additive in ExtrudernDispergieren der aufgeschmolzenen MaterialienAufbringen der Schichten auf den Träger bzw. die Armierung, so dass eine homogene Einbettung erfolgtKühlen der KunststoffabdichtungsbahnAufwickeln der Kunststoffabdichtungsbahn auf Rollenkerne aus AltpapierkartonageVerpacken der einzelnen Rollen mit einer PE-Folie Das Werk Sarnen verfügt seit 1993 über ein zertifizier-tes Qualitätsmanagementsystem nach /ISO 9001/. 
Deklarierte Einheit: 
Diese Deklaration bezieht sich auf 1 m2 verlegte Sarnafil® TS 77-E Kunststoffabdichtungsbahn mit der Dicke 2,0 mm.  Für andere Dicken wird in Kapitel 5 eine Formel zur eigenständigen Berechnung der Werte angegeben.</technologyDescriptionAndIncludedProcesses>
<technologyDescriptionAndIncludedProcesses xml:lang="en">Sarnafil® TS 77-E polymeric waterproofing sheets are manufactured on production lines developed in-house in the following stages: Melting of the polymeric components and additives in extruders Dispersing of the molten materials Coating of the carrier or the reinforcing in layers, producing homogenous encapsulation Cooling of the polymeric waterproofing sheet Winding of the sheets onto cardboard spools made of recycled paper Individually wrapping each roll The quality management system of the Sarnen plant has been ISO 9001 certified since 1993. 
Declared unit: 
This declaration applies to 1 m2 of installed Sarnafil® TS 77-E polymeric waterproofing membrane, thickness 2.0 mm. A formula is given in Chapter 5 for independent calculation of the values for other thicknesses.</technologyDescriptionAndIncludedProcesses>
<technologicalApplicability xml:lang="de">Sarnafil® TS 77-E Kunststoffabdichtungsbahnen dienen ausschließlich der Abdichtung von Flach-dächern ohne Auflast. Die Dachbahnen werden vorzugsweise auf Dächern mit einer Dachneigung ≥ 20° lose verlegt und mechanisch befestigt. Die Sarnafil® TS 77-E Dachabdichtungsbahnen bieten im Vergleich zu den Sarnafil® TS 77 Dachabdichtungs-bahnen einen erhöhten Brandschutz.</technologicalApplicability>
<technologicalApplicability xml:lang="en">Sarnafil® TS 77-E polymeric waterproofing membrane is used exclusively to seal unballasted flat roofs. On roofs with a slope of ≥ 20°, the roofing sheets should be loose laid and mechanically fastened. Sarnafil® TS 77-E polymeric waterproofing membrane provides greater protection against fire than does Sarnafil® TS 77 polymeric waterproofing membrane.</technologicalApplicability>
</technology>
</processInformation>
<modellingAndValidation>
<LCIMethodAndAllocation>
<typeOfDataSet>EPD</typeOfDataSet>
<referenceToLCAMethodDetails type="source data set" refObjectId="2f91f7a3-95c7-4c43-9c35-62c37d4e539b">
<common:shortDescription xml:lang="de">Dach- und Dichtungsbahnsysteme aus Kunststoffen und Elastomeren.pdf</common:shortDescription>
</referenceToLCAMethodDetails>
<common:other>
<epd:subType xmlns="http://www.iai.kit.edu/EPD/2013">specific dataset</epd:subType>
</common:other>
</LCIMethodAndAllocation>
<dataSourcesTreatmentAndRepresentativeness>
<referenceToDataSource type="source data set" refObjectId="28d74cc0-db8b-4d7e-bc44-5f6d56ce0c4a">
<common:shortDescription xml:lang="de">GaBi Database (all versions)</common:shortDescription>
</referenceToDataSource>
<referenceToDataSource type="source data set" refObjectId="07d9b8a7-e0fc-408f-a95e-c90735f843ce">
<common:shortDescription xml:lang="de">GaBi database SP39 2019</common:shortDescription>
</referenceToDataSource>
<useAdviceForDataSet xml:lang="de">Gültigkeitsbereich: 
Dieses Dokument bezieht sich auf die von der Sika AG in CH-6060 Sarnen (Schweiz) hergestellten Sarnafil® TS 77-E Kunststoffabdichtungsbahnen in den Dicken 1,5, 1,8 und 2,0 mm. Die EPD umfasst die Produktion der Dachbahn, den Transport des Produkts zur Baustelle, die Installation der Dachbahn, die Entsorgung sowie Potenziale und Lasten außerhalb der Systemgrenze. Das Modell wurde auf Basis der Produktionsdaten aus dem Jahr 2018 von der Sika Services AG für die Dicke 2,0 mm modelliert. 
Systemgrenze: 
Typ der EPD: Wiege bis Werkstor - mit OptionenDie Systemgrenze der EPD folgt dem modularen Auf-bau gemäß EN 15804. In der Ökobilanz werden die folgenden Module berücksichtigt:A1–A3: Gewinnung, Verarbeitung und Transport von Rohstoffen (u.a. Polymere, Pigmente, Verar-beitungshilfsmittel, Stabilisatoren, Füllstoffe, Flammschutzmittel und Trägermaterialien), die für die Herstellung der Vorprodukte und der Dach-bahnen verwendet werden sowie der Verpack-ungsmaterialien, die zum Verpacken der Dach-bahnen verwendet werden, wie z. B. Holzpalet-ten, Karton und PE-Folie, zum Werk. Abfallverarbeitung von Produktionsabfällen (Randbeschnitt), die bei der Herstellung der Dachbahnen anfallen.A4: Transport der Kunststoffabdichtungs-bahnen zur BaustelleA5: Einbau der Kunststoffabdichtungsbahnen ins Gebäude mittels Heißluftschweißen (inkl. Schweißenergie und Wasserverbrauch), Entsorgung bzw. stoffliches Recycling von Verpackung und Verschnitt der DachbahnC1: Manueller Rückbau der DachabdichtungC2: Transport der rückgebauten Abdichtungs-bahnen zur AbfallbewirtschaftungC3: Abfallverarbeitung der rückgebauten Abdichtungsbahnen über stoffliches Recyc-ling (Szenario 1 - C3/1) oder thermische Verwertung (Szenario 2 - C3/2)C4: Abfallentsorgung der rückgebauten Abdichtungsbahnen auf DeponienD: Wiederverwendungs-, Rückgewinnungs- und Recyclingpotenziale (aus der thermi-schen Verwertung und dem stofflichen Recyc-ling der Kunststoffabdichtungsbahnen sowie der Wiederverwendung der Holzpaletten)</useAdviceForDataSet>
<useAdviceForDataSet xml:lang="en">Scope: 
This document applies to Sarnafil® TS 77-E polymeric waterproofing membrane in thicknesses of 1.5, 1.8, 2.0 and 2.5 mm manufactured by Sika Services AG in CH-6060 Sarnen (Switzerland). The EPD covers the production of the waterproofing membrane, transport of the product to the construction site, installation of the waterproofing membrane, disposal, as well as benefits and loads outside the system limits. The model was calculated on the basis of production data for the thickness 2.0 mm provided by Sika Services AG from the year 2018. 
System boundary: 
Type of EPD: Cradle to gate with optionsThe system boundaries of the EPD follow the modular structure set forth by EN 15804. The LCA takes into account the following modules: A1-A3: Extraction, processing and transport of raw materials (e.g. polymers, pigments, processing aids, stabilizers, fillers, flame retardants and carrier materials) used for the production of intermediate products and the waterproofing membrane and the packaging materials used to package the waterproofing membranes, such as wooden pallets, cardboard and PE film, for transport to the plant. Waste processing of production waste (edge trim), which occurs during the production of the waterproofing membrane. A4: Transport of the waterproofing membrane to the building site A5: Installation of the waterproofing membrane into the building by means of hot-air welding (including welding energy and water consumption), disposal or recycling of packaging, and waterproofing membrane scraps C1: Manual deconstruction and removal of the waterproofing membrane (recovery) C2: Transport of the recovered waterproofing membrane to waste-processing facility C3: Processing of the recovered waterproofing membrane for material recycling (Scenario 1 – C3/1) or thermal energy recovery (Scenario 2 – C3/2)  C4: Disposal of the recovered waterproofing membrane in landfill D: Benefits for reuse, recovery and/or recycling (through thermal energy recovery, recycling of the recovered waterproofing membrane and reuse of the wooden pallets)</useAdviceForDataSet>
<common:other>
<epd2:referenceToOriginalEPD type="source data set" refObjectId="9a6d407e-ee78-455e-af17-5548469adfc4">
<common:shortDescription xml:lang="de">Sarnafil TS 77-E.pdf</common:shortDescription>
</epd2:referenceToOriginalEPD>
</common:other>
</dataSourcesTreatmentAndRepresentativeness>
<validation>
<review type="Accredited third party review">
<common:referenceToNameOfReviewerAndInstitution uri="../contacts/d111dbec-b024-4be5-86c5-752d6eb2cf95.xml" type="contact data set" refObjectId="d111dbec-b024-4be5-86c5-752d6eb2cf95">
<common:shortDescription xml:lang="de">Institut Bauen und Umwelt e. V.</common:shortDescription>
</common:referenceToNameOfReviewerAndInstitution>
</review>
</validation>
<complianceDeclarations>
<compliance>
<common:referenceToComplianceSystem uri="../sources/b00f9ec0-7874-11e3-981f-0800200c9a66.xml" type="source data set" refObjectId="b00f9ec0-7874-11e3-981f-0800200c9a66">
<common:shortDescription xml:lang="de">DIN EN 15804</common:shortDescription>
</common:referenceToComplianceSystem>
</compliance>
<compliance>
<common:referenceToComplianceSystem uri="../sources/4f2eb655-6e44-4874-a95a-e28f5442cd4d.xml" type="source data set" refObjectId="4f2eb655-6e44-4874-a95a-e28f5442cd4d">
<common:shortDescription xml:lang="de">ISO 14025</common:shortDescription>
</common:referenceToComplianceSystem>
</compliance>
</complianceDeclarations>
</modellingAndValidation>
<administrativeInformation>
<common:commissionerAndGoal>
<common:referenceToCommissioner uri="../contacts/3d99c862-ca4d-4bff-9241-8a83668bd310.xml" type="contact data set" refObjectId="3d99c862-ca4d-4bff-9241-8a83668bd310">
<common:shortDescription xml:lang="de">Sika Deutschland GmbH</common:shortDescription>
</common:referenceToCommissioner>
</common:commissionerAndGoal>
<dataGenerator>
<common:referenceToPersonOrEntityGeneratingTheDataSet uri="../contacts/e6e310ee-d48d-41ec-b502-68ec650bae28.xml" type="contact data set" refObjectId="e6e310ee-d48d-41ec-b502-68ec650bae28">
<common:shortDescription xml:lang="de">Sika Services AG</common:shortDescription>
</common:referenceToPersonOrEntityGeneratingTheDataSet>
</dataGenerator>
<dataEntryBy>
<common:timeStamp>2020-04-24T15:35:30.997</common:timeStamp>
<common:referenceToDataSetFormat uri="../sources/a97a0155-0234-4b87-b4ce-a45da52f2a40.xml" type="source data set" refObjectId="a97a0155-0234-4b87-b4ce-a45da52f2a40">
<common:shortDescription xml:lang="de">ILCD Format</common:shortDescription>
</common:referenceToDataSetFormat>
<common:referenceToDataSetFormat uri="../sources/a29449fd-aa2f-4de8-b5d7-4b06b43c6fde.xml" type="source data set" refObjectId="a29449fd-aa2f-4de8-b5d7-4b06b43c6fde">
<common:shortDescription xml:lang="de">EPD-Datenformaterweiterungen v1.2</common:shortDescription>
<common:shortDescription xml:lang="en">EPD Data Format Extensions v1.2</common:shortDescription>
</common:referenceToDataSetFormat>
</dataEntryBy>
<publicationAndOwnership>
<common:dataSetVersion>00.02.000</common:dataSetVersion>
<common:referenceToPrecedingDataSetVersion uri="../processes/8a43146c-6b9e-4bf4-967f-84a198ff93d8.xml" type="process data set" refObjectId="8a43146c-6b9e-4bf4-967f-84a198ff93d8">
<common:shortDescription xml:lang="de">Sarnafil TS 77-E</common:shortDescription>
</common:referenceToPrecedingDataSetVersion>
<common:referenceToRegistrationAuthority uri="../contacts/d111dbec-b024-4be5-86c5-752d6eb2cf95.xml" type="contact data set" refObjectId="d111dbec-b024-4be5-86c5-752d6eb2cf95">
<common:shortDescription xml:lang="de">Institut Bauen und Umwelt e. V.</common:shortDescription>
</common:referenceToRegistrationAuthority>
<common:registrationNumber>EPD-SIK-20190187-IBA1-DE</common:registrationNumber>
<common:referenceToOwnershipOfDataSet uri="../contacts/3d99c862-ca4d-4bff-9241-8a83668bd310.xml" type="contact data set" refObjectId="3d99c862-ca4d-4bff-9241-8a83668bd310">
<common:shortDescription xml:lang="de">Sika Deutschland GmbH</common:shortDescription>
</common:referenceToOwnershipOfDataSet>
<common:copyright>true</common:copyright>
<common:licenseType>Free of charge for all users and uses</common:licenseType>
<common:accessRestrictions xml:lang="en">None</common:accessRestrictions>
<common:other>
<epd2:referenceToPublisher type="contact data set" refObjectId="d111dbec-b024-4be5-86c5-752d6eb2cf95" uri="../contacts/d111dbec-b024-4be5-86c5-752d6eb2cf95.xml">
<common:shortDescription xml:lang="de">Institut Bauen und Umwelt e. V.</common:shortDescription>
</epd2:referenceToPublisher>
</common:other>
</publicationAndOwnership>
</administrativeInformation>
<exchanges>
<exchange dataSetInternalID="0">
<referenceToFlowDataSet uri="../flows/247102bf-8eda-d79f-8b39-3f1e2408c1b1.xml" type="flow data set" refObjectId="247102bf-8eda-d79f-8b39-3f1e2408c1b1">
<common:shortDescription xml:lang="de">1 m² Dachbahn ()</common:shortDescription>
</referenceToFlowDataSet>
<meanAmount>1</meanAmount>
<referencesToDataSource />
</exchange>
<exchange dataSetInternalID="1">
<referenceToFlowDataSet uri="../flows/20f32be5-0398-4288-9b6d-accddd195317.xml" type="flow data set" refObjectId="20f32be5-0398-4288-9b6d-accddd195317">
<common:shortDescription xml:lang="de">Erneuerbare Primärenergie als Energieträger (PERE)</common:shortDescription>
<common:shortDescription xml:lang="en">Renewable primary energy as energy carrier (PERE)</common:shortDescription>
</referenceToFlowDataSet>
<functionType>General reminder flow</functionType>
<exchangeDirection>Input</exchangeDirection>
<common:other>
<epd:referenceToUnitGroupDataSet uri="../unitgroups/93a60a57-a3c8-11da-a746-0800200c9a66.xml" type="unit group data set" refObjectId="93a60a57-a3c8-11da-a746-0800200c9a66">
<common:shortDescription xml:lang="de">MJ</common:shortDescription>
</epd:referenceToUnitGroupDataSet>
<epd:amount epd:module="A1-A3">8.38</epd:amount>
<epd:amount epd:module="A4">0.0902</epd:amount>
<epd:amount epd:module="A5">1.06</epd:amount>
<epd:amount epd:module="C1">0</epd:amount>
<epd:amount epd:module="C2" epd:scenario="S1">0.0369</epd:amount>
<epd:amount epd:module="C2" epd:scenario="S2">0.00737</epd:amount>
<epd:amount epd:module="C3" epd:scenario="S1">0.929</epd:amount>
<epd:amount epd:module="C3" epd:scenario="S2">0.178</epd:amount>
<epd:amount epd:module="C4">0</epd:amount>
<epd:amount epd:module="D" epd:scenario="S1">-6.71</epd:amount>
<epd:amount epd:module="D" epd:scenario="S2">-18.6</epd:amount>
</common:other>
</exchange>
<exchange dataSetInternalID="2">
<referenceToFlowDataSet uri="../flows/fb3ec0de-548d-4508-aea5-00b73bf6f702.xml" type="flow data set" refObjectId="fb3ec0de-548d-4508-aea5-00b73bf6f702">
<common:shortDescription xml:lang="de">Erneuerbare Primärenergie zur stofflichen Nutzung (PERM)</common:shortDescription>
<common:shortDescription xml:lang="en">Renewable primary energy resources as material utilization (PERM)</common:shortDescription>
</referenceToFlowDataSet>
<functionType>General reminder flow</functionType>
<exchangeDirection>Input</exchangeDirection>
<common:other>
<epd:referenceToUnitGroupDataSet uri="../unitgroups/93a60a57-a3c8-11da-a746-0800200c9a66.xml" type="unit group data set" refObjectId="93a60a57-a3c8-11da-a746-0800200c9a66">
<common:shortDescription xml:lang="de">MJ</common:shortDescription>
</epd:referenceToUnitGroupDataSet>
<epd:amount epd:module="A1-A3">1.99</epd:amount>
<epd:amount epd:module="A4">0</epd:amount>
<epd:amount epd:module="A5">-0.159</epd:amount>
<epd:amount epd:module="C1">0</epd:amount>
<epd:amount epd:module="C2" epd:scenario="S1">0</epd:amount>
<epd:amount epd:module="C2" epd:scenario="S2">0</epd:amount>
<epd:amount epd:module="C3" epd:scenario="S1">0</epd:amount>
<epd:amount epd:module="C3" epd:scenario="S2">0</epd:amount>
<epd:amount epd:module="C4">0</epd:amount>
<epd:amount epd:module="D" epd:scenario="S1">0</epd:amount>
<epd:amount epd:module="D" epd:scenario="S2">0</epd:amount>
</common:other>
</exchange>
<exchange dataSetInternalID="3">
<referenceToFlowDataSet uri="../flows/53f97275-fa8a-4cdd-9024-65936002acd0.xml" type="flow data set" refObjectId="53f97275-fa8a-4cdd-9024-65936002acd0">
<common:shortDescription xml:lang="de">Total erneuerbare Primärenergie (PERT)</common:shortDescription>
<common:shortDescription xml:lang="en">Total use of renewable primary energy resources (PERT)</common:shortDescription>
</referenceToFlowDataSet>
<functionType>General reminder flow</functionType>
<exchangeDirection>Input</exchangeDirection>
<common:other>
<epd:referenceToUnitGroupDataSet uri="../unitgroups/93a60a57-a3c8-11da-a746-0800200c9a66.xml" type="unit group data set" refObjectId="93a60a57-a3c8-11da-a746-0800200c9a66">
<common:shortDescription xml:lang="de">MJ</common:shortDescription>
</epd:referenceToUnitGroupDataSet>
<epd:amount epd:module="A1-A3">10.4</epd:amount>
<epd:amount epd:module="A4">0.0902</epd:amount>
<epd:amount epd:module="A5">0.905</epd:amount>
<epd:amount epd:module="C1">0</epd:amount>
<epd:amount epd:module="C2" epd:scenario="S1">0.0369</epd:amount>
<epd:amount epd:module="C2" epd:scenario="S2">0.00737</epd:amount>
<epd:amount epd:module="C3" epd:scenario="S1">0.929</epd:amount>
<epd:amount epd:module="C3" epd:scenario="S2">0.178</epd:amount>
<epd:amount epd:module="C4">0</epd:amount>
<epd:amount epd:module="D" epd:scenario="S1">-6.71</epd:amount>
<epd:amount epd:module="D" epd:scenario="S2">-18.6</epd:amount>
</common:other>
</exchange>
<exchange dataSetInternalID="4">
<referenceToFlowDataSet uri="../flows/ac857178-2b45-46ec-892a-a9a4332f0372.xml" type="flow data set" refObjectId="ac857178-2b45-46ec-892a-a9a4332f0372">
<common:shortDescription xml:lang="de">Nicht-erneuerbare Primärenergie als Energieträger (PENRE)</common:shortDescription>
<common:shortDescription xml:lang="en">Non renewable primary energy as energy carrier (PENRE)</common:shortDescription>
</referenceToFlowDataSet>
<functionType>General reminder flow</functionType>
<exchangeDirection>Input</exchangeDirection>
<common:other>
<epd:referenceToUnitGroupDataSet uri="../unitgroups/93a60a57-a3c8-11da-a746-0800200c9a66.xml" type="unit group data set" refObjectId="93a60a57-a3c8-11da-a746-0800200c9a66">
<common:shortDescription xml:lang="de">MJ</common:shortDescription>
</epd:referenceToUnitGroupDataSet>
<epd:amount epd:module="A1-A3">49.5</epd:amount>
<epd:amount epd:module="A4">1.48</epd:amount>
<epd:amount epd:module="A5">4.26</epd:amount>
<epd:amount epd:module="C1">0</epd:amount>
<epd:amount epd:module="C2" epd:scenario="S1">0.636</epd:amount>
<epd:amount epd:module="C2" epd:scenario="S2">0.127</epd:amount>
<epd:amount epd:module="C3" epd:scenario="S1">62</epd:amount>
<epd:amount epd:module="C3" epd:scenario="S2">61.2</epd:amount>
<epd:amount epd:module="C4">0</epd:amount>
<epd:amount epd:module="D" epd:scenario="S1">-142</epd:amount>
<epd:amount epd:module="D" epd:scenario="S2">-59.9</epd:amount>
</common:other>
</exchange>
<exchange dataSetInternalID="5">
<referenceToFlowDataSet uri="../flows/1421caa0-679d-4bf4-b282-0eb850ccae27.xml" type="flow data set" refObjectId="1421caa0-679d-4bf4-b282-0eb850ccae27">
<common:shortDescription xml:lang="de">Nicht-erneuerbare Primärenergie zur stofflichen Nutzung (PENRM)</common:shortDescription>
<common:shortDescription xml:lang="en">Non renewable primary energy as material utilization (PENRM)</common:shortDescription>
</referenceToFlowDataSet>
<functionType>General reminder flow</functionType>
<exchangeDirection>Input</exchangeDirection>
<common:other>
<epd:referenceToUnitGroupDataSet uri="../unitgroups/93a60a57-a3c8-11da-a746-0800200c9a66.xml" type="unit group data set" refObjectId="93a60a57-a3c8-11da-a746-0800200c9a66">
<common:shortDescription xml:lang="de">MJ</common:shortDescription>
</epd:referenceToUnitGroupDataSet>
<epd:amount epd:module="A1-A3">57</epd:amount>
<epd:amount epd:module="A4">0</epd:amount>
<epd:amount epd:module="A5">4.53</epd:amount>
<epd:amount epd:module="C1">0</epd:amount>
<epd:amount epd:module="C2" epd:scenario="S1">0</epd:amount>
<epd:amount epd:module="C2" epd:scenario="S2">0</epd:amount>
<epd:amount epd:module="C3" epd:scenario="S1">-60.2</epd:amount>
<epd:amount epd:module="C3" epd:scenario="S2">-60.2</epd:amount>
<epd:amount epd:module="C4">0</epd:amount>
<epd:amount epd:module="D" epd:scenario="S1">0</epd:amount>
<epd:amount epd:module="D" epd:scenario="S2">0</epd:amount>
</common:other>
</exchange>
<exchange dataSetInternalID="6">
<referenceToFlowDataSet uri="../flows/06159210-646b-4c8d-8583-da9b3b95a6c1.xml" type="flow data set" refObjectId="06159210-646b-4c8d-8583-da9b3b95a6c1">
<common:shortDescription xml:lang="de">Total nicht erneuerbare Primärenergie (PENRT)</common:shortDescription>
<common:shortDescription xml:lang="en">Total use of non renewable primary energy resources (PENRT)</common:shortDescription>
</referenceToFlowDataSet>
<functionType>General reminder flow</functionType>
<exchangeDirection>Input</exchangeDirection>
<common:other>
<epd:referenceToUnitGroupDataSet uri="../unitgroups/93a60a57-a3c8-11da-a746-0800200c9a66.xml" type="unit group data set" refObjectId="93a60a57-a3c8-11da-a746-0800200c9a66">
<common:shortDescription xml:lang="de">MJ</common:shortDescription>
</epd:referenceToUnitGroupDataSet>
<epd:amount epd:module="A1-A3">106</epd:amount>
<epd:amount epd:module="A4">1.48</epd:amount>
<epd:amount epd:module="A5">8.8</epd:amount>
<epd:amount epd:module="C1">0</epd:amount>
<epd:amount epd:module="C2" epd:scenario="S1">0.636</epd:amount>
<epd:amount epd:module="C2" epd:scenario="S2">0.127</epd:amount>
<epd:amount epd:module="C3" epd:scenario="S1">1.78</epd:amount>
<epd:amount epd:module="C3" epd:scenario="S2">1</epd:amount>
<epd:amount epd:module="C4">0</epd:amount>
<epd:amount epd:module="D" epd:scenario="S1">-142</epd:amount>
<epd:amount epd:module="D" epd:scenario="S2">-59.9</epd:amount>
</common:other>
</exchange>
<exchange dataSetInternalID="7">
<referenceToFlowDataSet uri="../flows/c6a1f35f-2d09-4f54-8dfb-97e502e1ce92.xml" type="flow data set" refObjectId="c6a1f35f-2d09-4f54-8dfb-97e502e1ce92">
<common:shortDescription xml:lang="de">Einsatz von Sekundärstoffen (SM)</common:shortDescription>
<common:shortDescription xml:lang="en">Use of secondary material (SM)</common:shortDescription>
</referenceToFlowDataSet>
<functionType>General reminder flow</functionType>
<exchangeDirection>Input</exchangeDirection>
<common:other>
<epd:referenceToUnitGroupDataSet uri="../unitgroups/ad38d542-3fe9-439d-9b95-2f5f7752acaf.xml" type="unit group data set" refObjectId="ad38d542-3fe9-439d-9b95-2f5f7752acaf">
<common:shortDescription xml:lang="de">kg</common:shortDescription>
</epd:referenceToUnitGroupDataSet>
<epd:amount epd:module="A1-A3">0.0687</epd:amount>
<epd:amount epd:module="A4">0</epd:amount>
<epd:amount epd:module="A5">0.0055</epd:amount>
<epd:amount epd:module="C1">0</epd:amount>
<epd:amount epd:module="C2" epd:scenario="S1">0</epd:amount>
<epd:amount epd:module="C2" epd:scenario="S2">0</epd:amount>
<epd:amount epd:module="C3" epd:scenario="S1">0</epd:amount>
<epd:amount epd:module="C3" epd:scenario="S2">0</epd:amount>
<epd:amount epd:module="C4">0</epd:amount>
<epd:amount epd:module="D" epd:scenario="S1">-2.43</epd:amount>
<epd:amount epd:module="D" epd:scenario="S2">0</epd:amount>
</common:other>
</exchange>
<exchange dataSetInternalID="8">
<referenceToFlowDataSet uri="../flows/64333088-a55f-4aa2-9a31-c10b07816787.xml" type="flow data set" refObjectId="64333088-a55f-4aa2-9a31-c10b07816787">
<common:shortDescription xml:lang="de">Erneuerbare Sekundärbrennstoffe (RSF)</common:shortDescription>
<common:shortDescription xml:lang="en">Use of renewable secondary fuels (RSF)</common:shortDescription>
</referenceToFlowDataSet>
<functionType>General reminder flow</functionType>
<exchangeDirection>Input</exchangeDirection>
<common:other>
<epd:referenceToUnitGroupDataSet uri="../unitgroups/93a60a57-a3c8-11da-a746-0800200c9a66.xml" type="unit group data set" refObjectId="93a60a57-a3c8-11da-a746-0800200c9a66">
<common:shortDescription xml:lang="de">MJ</common:shortDescription>
</epd:referenceToUnitGroupDataSet>
<epd:amount epd:module="A1-A3">1.78E-21</epd:amount>
<epd:amount epd:module="A4">0</epd:amount>
<epd:amount epd:module="A5">1.42E-22</epd:amount>
<epd:amount epd:module="C1">0</epd:amount>
<epd:amount epd:module="C2" epd:scenario="S1">0</epd:amount>
<epd:amount epd:module="C2" epd:scenario="S2">0</epd:amount>
<epd:amount epd:module="C3" epd:scenario="S1">0</epd:amount>
<epd:amount epd:module="C3" epd:scenario="S2">0</epd:amount>
<epd:amount epd:module="C4">0</epd:amount>
<epd:amount epd:module="D" epd:scenario="S1">0</epd:amount>
<epd:amount epd:module="D" epd:scenario="S2">0</epd:amount>
</common:other>
</exchange>
<exchange dataSetInternalID="9">
<referenceToFlowDataSet uri="../flows/89def144-d39a-4287-b86f-efde453ddcb2.xml" type="flow data set" refObjectId="89def144-d39a-4287-b86f-efde453ddcb2">
<common:shortDescription xml:lang="de">Nicht erneuerbare Sekundärbrennstoffe (NRSF)</common:shortDescription>
<common:shortDescription xml:lang="en">Use of non renewable secondary fuels (NRSF)</common:shortDescription>
</referenceToFlowDataSet>
<functionType>General reminder flow</functionType>
<exchangeDirection>Input</exchangeDirection>
<common:other>
<epd:referenceToUnitGroupDataSet uri="../unitgroups/93a60a57-a3c8-11da-a746-0800200c9a66.xml" type="unit group data set" refObjectId="93a60a57-a3c8-11da-a746-0800200c9a66">
<common:shortDescription xml:lang="de">MJ</common:shortDescription>
</epd:referenceToUnitGroupDataSet>
<epd:amount epd:module="A1-A3">2.08E-20</epd:amount>
<epd:amount epd:module="A4">0</epd:amount>
<epd:amount epd:module="A5">1.67E-21</epd:amount>
<epd:amount epd:module="C1">0</epd:amount>
<epd:amount epd:module="C2" epd:scenario="S1">0</epd:amount>
<epd:amount epd:module="C2" epd:scenario="S2">0</epd:amount>
<epd:amount epd:module="C3" epd:scenario="S1">0</epd:amount>
<epd:amount epd:module="C3" epd:scenario="S2">0</epd:amount>
<epd:amount epd:module="C4">0</epd:amount>
<epd:amount epd:module="D" epd:scenario="S1">0</epd:amount>
<epd:amount epd:module="D" epd:scenario="S2">0</epd:amount>
</common:other>
</exchange>
<exchange dataSetInternalID="10">
<referenceToFlowDataSet uri="../flows/3cf952c8-f3a4-461d-8c96-96456ca62246.xml" type="flow data set" refObjectId="3cf952c8-f3a4-461d-8c96-96456ca62246">
<common:shortDescription xml:lang="de">Einsatz von Süßwasserressourcen (FW)</common:shortDescription>
<common:shortDescription xml:lang="en">Use of net fresh water (FW)</common:shortDescription>
</referenceToFlowDataSet>
<functionType>General reminder flow</functionType>
<exchangeDirection>Input</exchangeDirection>
<common:other>
<epd:referenceToUnitGroupDataSet uri="../unitgroups/cd950537-0a98-4044-9ba7-9f9a68d0a504.xml" type="unit group data set" refObjectId="cd950537-0a98-4044-9ba7-9f9a68d0a504">
<common:shortDescription xml:lang="de">m^3</common:shortDescription>
</epd:referenceToUnitGroupDataSet>
<epd:amount epd:module="A1-A3">0.0187</epd:amount>
<epd:amount epd:module="A4">0.000104</epd:amount>
<epd:amount epd:module="A5">0.00204</epd:amount>
<epd:amount epd:module="C1">0</epd:amount>
<epd:amount epd:module="C2" epd:scenario="S1">6.23E-05</epd:amount>
<epd:amount epd:module="C2" epd:scenario="S2">1.25E-05</epd:amount>
<epd:amount epd:module="C3" epd:scenario="S1">0.000971</epd:amount>
<epd:amount epd:module="C3" epd:scenario="S2">0.0173</epd:amount>
<epd:amount epd:module="C4">0</epd:amount>
<epd:amount epd:module="D" epd:scenario="S1">-0.0163</epd:amount>
<epd:amount epd:module="D" epd:scenario="S2">-0.0195</epd:amount>
</common:other>
</exchange>
<exchange dataSetInternalID="11">
<referenceToFlowDataSet uri="../flows/430f9e0f-59b2-46a0-8e0d-55e0e84948fc.xml" type="flow data set" refObjectId="430f9e0f-59b2-46a0-8e0d-55e0e84948fc">
<common:shortDescription xml:lang="de">Gefährlicher Abfall zur Deponie (HWD)</common:shortDescription>
<common:shortDescription xml:lang="en">Hazardous waste disposed (HWD)</common:shortDescription>
</referenceToFlowDataSet>
<functionType>General reminder flow</functionType>
<exchangeDirection>Output</exchangeDirection>
<common:other>
<epd:referenceToUnitGroupDataSet uri="../unitgroups/ad38d542-3fe9-439d-9b95-2f5f7752acaf.xml" type="unit group data set" refObjectId="ad38d542-3fe9-439d-9b95-2f5f7752acaf">
<common:shortDescription xml:lang="de">kg</common:shortDescription>
</epd:referenceToUnitGroupDataSet>
<epd:amount epd:module="A1-A3">2.42E-06</epd:amount>
<epd:amount epd:module="A4">8.44E-08</epd:amount>
<epd:amount epd:module="A5">2.01E-07</epd:amount>
<epd:amount epd:module="C1">0</epd:amount>
<epd:amount epd:module="C2" epd:scenario="S1">3.55E-08</epd:amount>
<epd:amount epd:module="C2" epd:scenario="S2">7.1E-09</epd:amount>
<epd:amount epd:module="C3" epd:scenario="S1">1.72E-09</epd:amount>
<epd:amount epd:module="C3" epd:scenario="S2">7.98E-10</epd:amount>
<epd:amount epd:module="C4">0</epd:amount>
<epd:amount epd:module="D" epd:scenario="S1">-3.54E-08</epd:amount>
<epd:amount epd:module="D" epd:scenario="S2">-2.59E-08</epd:amount>
</common:other>
</exchange>
<exchange dataSetInternalID="12">
<referenceToFlowDataSet uri="../flows/b29ef66b-e286-4afa-949f-62f1a7b4d7fa.xml" type="flow data set" refObjectId="b29ef66b-e286-4afa-949f-62f1a7b4d7fa">
<common:shortDescription xml:lang="de">Entsorgter nicht gefährlicher Abfall (NHWD)</common:shortDescription>
<common:shortDescription xml:lang="en">Non hazardous waste disposed (NHWD)</common:shortDescription>
</referenceToFlowDataSet>
<functionType>General reminder flow</functionType>
<exchangeDirection>Output</exchangeDirection>
<common:other>
<epd:referenceToUnitGroupDataSet uri="../unitgroups/ad38d542-3fe9-439d-9b95-2f5f7752acaf.xml" type="unit group data set" refObjectId="ad38d542-3fe9-439d-9b95-2f5f7752acaf">
<common:shortDescription xml:lang="de">kg</common:shortDescription>
</epd:referenceToUnitGroupDataSet>
<epd:amount epd:module="A1-A3">0.254</epd:amount>
<epd:amount epd:module="A4">9.91E-05</epd:amount>
<epd:amount epd:module="A5">0.0224</epd:amount>
<epd:amount epd:module="C1">0</epd:amount>
<epd:amount epd:module="C2" epd:scenario="S1">5.17E-05</epd:amount>
<epd:amount epd:module="C2" epd:scenario="S2">1.03E-05</epd:amount>
<epd:amount epd:module="C3" epd:scenario="S1">0.0238</epd:amount>
<epd:amount epd:module="C3" epd:scenario="S2">0.0317</epd:amount>
<epd:amount epd:module="C4">0</epd:amount>
<epd:amount epd:module="D" epd:scenario="S1">-0.0188</epd:amount>
<epd:amount epd:module="D" epd:scenario="S2">-0.0413</epd:amount>
</common:other>
</exchange>
<exchange dataSetInternalID="13">
<referenceToFlowDataSet uri="../flows/3449546e-52ad-4b39-b809-9fb77cea8ff6.xml" type="flow data set" refObjectId="3449546e-52ad-4b39-b809-9fb77cea8ff6">
<common:shortDescription xml:lang="de">Entsorgter radioaktiver Abfall (RWD)</common:shortDescription>
<common:shortDescription xml:lang="en">Radioactive waste disposed (RWD)</common:shortDescription>
</referenceToFlowDataSet>
<functionType>General reminder flow</functionType>
<exchangeDirection>Output</exchangeDirection>
<common:other>
<epd:referenceToUnitGroupDataSet uri="../unitgroups/ad38d542-3fe9-439d-9b95-2f5f7752acaf.xml" type="unit group data set" refObjectId="ad38d542-3fe9-439d-9b95-2f5f7752acaf">
<common:shortDescription xml:lang="de">kg</common:shortDescription>
</epd:referenceToUnitGroupDataSet>
<epd:amount epd:module="A1-A3">0.00227</epd:amount>
<epd:amount epd:module="A4">1.76E-06</epd:amount>
<epd:amount epd:module="A5">0.000195</epd:amount>
<epd:amount epd:module="C1">0</epd:amount>
<epd:amount epd:module="C2" epd:scenario="S1">8.62E-07</epd:amount>
<epd:amount epd:module="C2" epd:scenario="S2">1.72E-07</epd:amount>
<epd:amount epd:module="C3" epd:scenario="S1">0.000164</epd:amount>
<epd:amount epd:module="C3" epd:scenario="S2">6.43E-05</epd:amount>
<epd:amount epd:module="C4">0</epd:amount>
<epd:amount epd:module="D" epd:scenario="S1">-0.00138</epd:amount>
<epd:amount epd:module="D" epd:scenario="S2">-0.00697</epd:amount>
</common:other>
</exchange>
<exchange dataSetInternalID="14">
<referenceToFlowDataSet uri="../flows/a2b32f97-3fc7-4af2-b209-525bc6426f33.xml" type="flow data set" refObjectId="a2b32f97-3fc7-4af2-b209-525bc6426f33">
<common:shortDescription xml:lang="de">Komponenten für die Wiederverwendung (CRU)</common:shortDescription>
<common:shortDescription xml:lang="en">Components for re-use (CRU)</common:shortDescription>
</referenceToFlowDataSet>
<functionType>General reminder flow</functionType>
<exchangeDirection>Output</exchangeDirection>
<common:other>
<epd:referenceToUnitGroupDataSet uri="../unitgroups/ad38d542-3fe9-439d-9b95-2f5f7752acaf.xml" type="unit group data set" refObjectId="ad38d542-3fe9-439d-9b95-2f5f7752acaf">
<common:shortDescription xml:lang="de">kg</common:shortDescription>
</epd:referenceToUnitGroupDataSet>
<epd:amount epd:module="A1-A3">0</epd:amount>
<epd:amount epd:module="A4">0</epd:amount>
<epd:amount epd:module="A5">0</epd:amount>
<epd:amount epd:module="C1">0</epd:amount>
<epd:amount epd:module="C2" epd:scenario="S1">0</epd:amount>
<epd:amount epd:module="C2" epd:scenario="S2">0</epd:amount>
<epd:amount epd:module="C3" epd:scenario="S1">0</epd:amount>
<epd:amount epd:module="C3" epd:scenario="S2">0</epd:amount>
<epd:amount epd:module="C4">0</epd:amount>
<epd:amount epd:module="D" epd:scenario="S1">0</epd:amount>
<epd:amount epd:module="D" epd:scenario="S2">0</epd:amount>
</common:other>
</exchange>
<exchange dataSetInternalID="15">
<referenceToFlowDataSet uri="../flows/d7fe48a5-4103-49c8-9aae-b0b5dfdbd6ae.xml" type="flow data set" refObjectId="d7fe48a5-4103-49c8-9aae-b0b5dfdbd6ae">
<common:shortDescription xml:lang="de">Stoffe zum Recycling (MFR)</common:shortDescription>
<common:shortDescription xml:lang="en">Materials for recycling (MFR)</common:shortDescription>
</referenceToFlowDataSet>
<functionType>General reminder flow</functionType>
<exchangeDirection>Output</exchangeDirection>
<common:other>
<epd:referenceToUnitGroupDataSet uri="../unitgroups/ad38d542-3fe9-439d-9b95-2f5f7752acaf.xml" type="unit group data set" refObjectId="ad38d542-3fe9-439d-9b95-2f5f7752acaf">
<common:shortDescription xml:lang="de">kg</common:shortDescription>
</epd:referenceToUnitGroupDataSet>
<epd:amount epd:module="A1-A3">0</epd:amount>
<epd:amount epd:module="A4">0</epd:amount>
<epd:amount epd:module="A5">0</epd:amount>
<epd:amount epd:module="C1">0</epd:amount>
<epd:amount epd:module="C2" epd:scenario="S1">0</epd:amount>
<epd:amount epd:module="C2" epd:scenario="S2">0</epd:amount>
<epd:amount epd:module="C3" epd:scenario="S1">2.43</epd:amount>
<epd:amount epd:module="C3" epd:scenario="S2">0</epd:amount>
<epd:amount epd:module="C4">0</epd:amount>
<epd:amount epd:module="D" epd:scenario="S1">0</epd:amount>
<epd:amount epd:module="D" epd:scenario="S2">0</epd:amount>
</common:other>
</exchange>
<exchange dataSetInternalID="16">
<referenceToFlowDataSet uri="../flows/59a9181c-3aaf-46ee-8b13-2b3723b6e447.xml" type="flow data set" refObjectId="59a9181c-3aaf-46ee-8b13-2b3723b6e447">
<common:shortDescription xml:lang="de">Stoffe für die Energierückgewinnung (MER)</common:shortDescription>
<common:shortDescription xml:lang="en">Materials for energy recovery (MER)</common:shortDescription>
</referenceToFlowDataSet>
<functionType>General reminder flow</functionType>
<exchangeDirection>Output</exchangeDirection>
<common:other>
<epd:referenceToUnitGroupDataSet uri="../unitgroups/ad38d542-3fe9-439d-9b95-2f5f7752acaf.xml" type="unit group data set" refObjectId="ad38d542-3fe9-439d-9b95-2f5f7752acaf">
<common:shortDescription xml:lang="de">kg</common:shortDescription>
</epd:referenceToUnitGroupDataSet>
<epd:amount epd:module="A1-A3">0</epd:amount>
<epd:amount epd:module="A4">0</epd:amount>
<epd:amount epd:module="A5">0</epd:amount>
<epd:amount epd:module="C1">0</epd:amount>
<epd:amount epd:module="C2" epd:scenario="S1">0</epd:amount>
<epd:amount epd:module="C2" epd:scenario="S2">0</epd:amount>
<epd:amount epd:module="C3" epd:scenario="S1">0</epd:amount>
<epd:amount epd:module="C3" epd:scenario="S2">0</epd:amount>
<epd:amount epd:module="C4">0</epd:amount>
<epd:amount epd:module="D" epd:scenario="S1">0</epd:amount>
<epd:amount epd:module="D" epd:scenario="S2">0</epd:amount>
</common:other>
</exchange>
<exchange dataSetInternalID="17">
<referenceToFlowDataSet uri="../flows/4da0c987-2b76-40d6-9e9e-82a017aaaf29.xml" type="flow data set" refObjectId="4da0c987-2b76-40d6-9e9e-82a017aaaf29">
<common:shortDescription xml:lang="de">Exportierte elektrische Energie (EEE)</common:shortDescription>
<common:shortDescription xml:lang="en">Exported electrical energy (EEE)</common:shortDescription>
</referenceToFlowDataSet>
<functionType>General reminder flow</functionType>
<exchangeDirection>Output</exchangeDirection>
<common:other>
<epd:referenceToUnitGroupDataSet uri="../unitgroups/93a60a57-a3c8-11da-a746-0800200c9a66.xml" type="unit group data set" refObjectId="93a60a57-a3c8-11da-a746-0800200c9a66">
<common:shortDescription xml:lang="de">MJ</common:shortDescription>
</epd:referenceToUnitGroupDataSet>
<epd:amount epd:module="A1-A3">0</epd:amount>
<epd:amount epd:module="A4">0</epd:amount>
<epd:amount epd:module="A5">0.426</epd:amount>
<epd:amount epd:module="C1">0</epd:amount>
<epd:amount epd:module="C2" epd:scenario="S1">0</epd:amount>
<epd:amount epd:module="C2" epd:scenario="S2">0</epd:amount>
<epd:amount epd:module="C3" epd:scenario="S1">0.605</epd:amount>
<epd:amount epd:module="C3" epd:scenario="S2">17.5</epd:amount>
<epd:amount epd:module="C4">0</epd:amount>
<epd:amount epd:module="D" epd:scenario="S1">0</epd:amount>
<epd:amount epd:module="D" epd:scenario="S2">0</epd:amount>
</common:other>
</exchange>
<exchange dataSetInternalID="18">
<referenceToFlowDataSet uri="../flows/98daf38a-7a79-46d3-9a37-2b7bd0955810.xml" type="flow data set" refObjectId="98daf38a-7a79-46d3-9a37-2b7bd0955810">
<common:shortDescription xml:lang="de">Exportierte thermische Energie (EET)</common:shortDescription>
<common:shortDescription xml:lang="en">Exported thermal energy (EET)</common:shortDescription>
</referenceToFlowDataSet>
<functionType>General reminder flow</functionType>
<exchangeDirection>Output</exchangeDirection>
<common:other>
<epd:referenceToUnitGroupDataSet uri="../unitgroups/93a60a57-a3c8-11da-a746-0800200c9a66.xml" type="unit group data set" refObjectId="93a60a57-a3c8-11da-a746-0800200c9a66">
<common:shortDescription xml:lang="de">MJ</common:shortDescription>
</epd:referenceToUnitGroupDataSet>
<epd:amount epd:module="A1-A3">0</epd:amount>
<epd:amount epd:module="A4">0</epd:amount>
<epd:amount epd:module="A5">0.759</epd:amount>
<epd:amount epd:module="C1">0</epd:amount>
<epd:amount epd:module="C2" epd:scenario="S1">0</epd:amount>
<epd:amount epd:module="C2" epd:scenario="S2">0</epd:amount>
<epd:amount epd:module="C3" epd:scenario="S1">1.1</epd:amount>
<epd:amount epd:module="C3" epd:scenario="S2">31.1</epd:amount>
<epd:amount epd:module="C4">0</epd:amount>
<epd:amount epd:module="D" epd:scenario="S1">0</epd:amount>
<epd:amount epd:module="D" epd:scenario="S2">0</epd:amount>
</common:other>
</exchange>
</exchanges>
<LCIAResults>
<LCIAResult>
<referenceToLCIAMethodDataSet uri="../lciamethods/77e416eb-a363-4258-a04e-171d843a6460.xml" type="LCIA method data set" refObjectId="77e416eb-a363-4258-a04e-171d843a6460">
<common:shortDescription xml:lang="de">Globales Erwärmungspotenzial (GWP)</common:shortDescription>
<common:shortDescription xml:lang="en">Global warming potential (GWP)</common:shortDescription>
</referenceToLCIAMethodDataSet>
<common:other>
<epd:referenceToUnitGroupDataSet uri="../unitgroups/1ebf3012-d0db-4de2-aefd-ef30cedb0be1.xml" type="unit group data set" refObjectId="1ebf3012-d0db-4de2-aefd-ef30cedb0be1">
<common:shortDescription xml:lang="de">kg CO_(2)-Äq.</common:shortDescription>
</epd:referenceToUnitGroupDataSet>
<epd:amount epd:module="A1-A3">3.72</epd:amount>
<epd:amount epd:module="A4">0.111</epd:amount>
<epd:amount epd:module="A5">0.532</epd:amount>
<epd:amount epd:module="C1">0</epd:amount>
<epd:amount epd:module="C2" epd:scenario="S1">0.0468</epd:amount>
<epd:amount epd:module="C2" epd:scenario="S2">0.00936</epd:amount>
<epd:amount epd:module="C3" epd:scenario="S1">0.294</epd:amount>
<epd:amount epd:module="C3" epd:scenario="S2">8</epd:amount>
<epd:amount epd:module="C4">0</epd:amount>
<epd:amount epd:module="D" epd:scenario="S1">-3.41</epd:amount>
<epd:amount epd:module="D" epd:scenario="S2">-2.89</epd:amount>
</common:other>
</LCIAResult>
<LCIAResult>
<referenceToLCIAMethodDataSet uri="../lciamethods/06dcd26f-025f-401a-a7c1-5e457eb54637.xml" type="LCIA method data set" refObjectId="06dcd26f-025f-401a-a7c1-5e457eb54637">
<common:shortDescription xml:lang="de">Abbau Potential der stratosphärischen Ozonschicht (ODP)</common:shortDescription>
<common:shortDescription xml:lang="en">Depletion potential of the stratospheric ozone layer (ODP)</common:shortDescription>
</referenceToLCIAMethodDataSet>
<common:other>
<epd:referenceToUnitGroupDataSet uri="../unitgroups/88054749-b0a6-47ea-a82b-dc5b29326512.xml" type="unit group data set" refObjectId="88054749-b0a6-47ea-a82b-dc5b29326512">
<common:shortDescription xml:lang="de">kg CFC11-Äq.</common:shortDescription>
</epd:referenceToUnitGroupDataSet>
<epd:amount epd:module="A1-A3">1.5E-08</epd:amount>
<epd:amount epd:module="A4">3.77E-17</epd:amount>
<epd:amount epd:module="A5">1.2E-09</epd:amount>
<epd:amount epd:module="C1">0</epd:amount>
<epd:amount epd:module="C2" epd:scenario="S1">7.72E-18</epd:amount>
<epd:amount epd:module="C2" epd:scenario="S2">1.54E-18</epd:amount>
<epd:amount epd:module="C3" epd:scenario="S1">5.61E-15</epd:amount>
<epd:amount epd:module="C3" epd:scenario="S2">7.43E-16</epd:amount>
<epd:amount epd:module="C4">0</epd:amount>
<epd:amount epd:module="D" epd:scenario="S1">-2.4E-09</epd:amount>
<epd:amount epd:module="D" epd:scenario="S2">-2.4E-09</epd:amount>
</common:other>
</LCIAResult>
<LCIAResult>
<referenceToLCIAMethodDataSet uri="../lciamethods/b4274add-93b7-4905-a5e4-2e878c4e4216.xml" type="LCIA method data set" refObjectId="b4274add-93b7-4905-a5e4-2e878c4e4216">
<common:shortDescription xml:lang="de">Versauerungspotenzial von Boden und Wasser (AP)</common:shortDescription>
<common:shortDescription xml:lang="en">Acidification potential of land and water (AP)</common:shortDescription>
</referenceToLCIAMethodDataSet>
<common:other>
<epd:referenceToUnitGroupDataSet uri="../unitgroups/bc50c624-a9bc-45b1-a9b0-e6b10d00476f.xml" type="unit group data set" refObjectId="bc50c624-a9bc-45b1-a9b0-e6b10d00476f">
<common:shortDescription xml:lang="de">kg SO_(2)-Äq.</common:shortDescription>
</epd:referenceToUnitGroupDataSet>
<epd:amount epd:module="A1-A3">0.00825</epd:amount>
<epd:amount epd:module="A4">0.000245</epd:amount>
<epd:amount epd:module="A5">0.000715</epd:amount>
<epd:amount epd:module="C1">0</epd:amount>
<epd:amount epd:module="C2" epd:scenario="S1">0.000109</epd:amount>
<epd:amount epd:module="C2" epd:scenario="S2">2.18E-05</epd:amount>
<epd:amount epd:module="C3" epd:scenario="S1">0.00027</epd:amount>
<epd:amount epd:module="C3" epd:scenario="S2">0.000515</epd:amount>
<epd:amount epd:module="C4">0</epd:amount>
<epd:amount epd:module="D" epd:scenario="S1">-0.00541</epd:amount>
<epd:amount epd:module="D" epd:scenario="S2">-0.00408</epd:amount>
</common:other>
</LCIAResult>
<LCIAResult>
<referenceToLCIAMethodDataSet uri="../lciamethods/f58827d0-b407-4ec6-be75-8b69efb98a0f.xml" type="LCIA method data set" refObjectId="f58827d0-b407-4ec6-be75-8b69efb98a0f">
<common:shortDescription xml:lang="de">Eutrophierungspotenzial (EP)</common:shortDescription>
<common:shortDescription xml:lang="en">Eutrophication potential (EP)</common:shortDescription>
</referenceToLCIAMethodDataSet>
<common:other>
<epd:referenceToUnitGroupDataSet uri="../unitgroups/67b5401d-873c-485f-bcf3-6ae83b918822.xml" type="unit group data set" refObjectId="67b5401d-873c-485f-bcf3-6ae83b918822">
<common:shortDescription xml:lang="de">kg PO_(4)^(3)-Äq.</common:shortDescription>
</epd:referenceToUnitGroupDataSet>
<epd:amount epd:module="A1-A3">0.0017</epd:amount>
<epd:amount epd:module="A4">6.12E-05</epd:amount>
<epd:amount epd:module="A5">0.000148</epd:amount>
<epd:amount epd:module="C1">0</epd:amount>
<epd:amount epd:module="C2" epd:scenario="S1">2.72E-05</epd:amount>
<epd:amount epd:module="C2" epd:scenario="S2">5.45E-06</epd:amount>
<epd:amount epd:module="C3" epd:scenario="S1">4.53E-05</epd:amount>
<epd:amount epd:module="C3" epd:scenario="S2">0.000109</epd:amount>
<epd:amount epd:module="C4">0</epd:amount>
<epd:amount epd:module="D" epd:scenario="S1">-0.000729</epd:amount>
<epd:amount epd:module="D" epd:scenario="S2">-0.000434</epd:amount>
</common:other>
</LCIAResult>
<LCIAResult>
<referenceToLCIAMethodDataSet uri="../lciamethods/1e84a202-dae6-42aa-9e9d-71ea48b8be00.xml" type="LCIA method data set" refObjectId="1e84a202-dae6-42aa-9e9d-71ea48b8be00">
<common:shortDescription xml:lang="de">Bildungspotential für troposphärisches Ozon (POCP)</common:shortDescription>
<common:shortDescription xml:lang="en">Formation potential of tropospheric ozone photochemical oxidants (POCP)</common:shortDescription>
</referenceToLCIAMethodDataSet>
<common:other>
<epd:referenceToUnitGroupDataSet uri="../unitgroups/01c26c17-9a76-406e-8295-f17b55fd909e.xml" type="unit group data set" refObjectId="01c26c17-9a76-406e-8295-f17b55fd909e">
<common:shortDescription xml:lang="de">kg Ethen-Äq.</common:shortDescription>
</epd:referenceToUnitGroupDataSet>
<epd:amount epd:module="A1-A3">0.000991</epd:amount>
<epd:amount epd:module="A4">-8.7E-05</epd:amount>
<epd:amount epd:module="A5">7.43E-05</epd:amount>
<epd:amount epd:module="C1">0</epd:amount>
<epd:amount epd:module="C2" epd:scenario="S1">-3.64E-05</epd:amount>
<epd:amount epd:module="C2" epd:scenario="S2">-7.28E-06</epd:amount>
<epd:amount epd:module="C3" epd:scenario="S1">1.74E-05</epd:amount>
<epd:amount epd:module="C3" epd:scenario="S2">5.28E-05</epd:amount>
<epd:amount epd:module="C4">0</epd:amount>
<epd:amount epd:module="D" epd:scenario="S1">-0.00098</epd:amount>
<epd:amount epd:module="D" epd:scenario="S2">-0.000436</epd:amount>
</common:other>
</LCIAResult>
<LCIAResult>
<referenceToLCIAMethodDataSet uri="../lciamethods/f7c73bb9-ab1a-4249-9c6d-379a0de6f67e.xml" type="LCIA method data set" refObjectId="f7c73bb9-ab1a-4249-9c6d-379a0de6f67e">
<common:shortDescription xml:lang="de">Potenzial für den abiotischen Abbau nicht fossiler Ressourcen (ADPE)</common:shortDescription>
<common:shortDescription xml:lang="en">Abiotic depletion potential for non fossil resources (ADPE)</common:shortDescription>
</referenceToLCIAMethodDataSet>
<common:other>
<epd:referenceToUnitGroupDataSet uri="../unitgroups/54ccd2d9-a32a-4fc2-923d-f2c8c93e89d4.xml" type="unit group data set" refObjectId="54ccd2d9-a32a-4fc2-923d-f2c8c93e89d4">
<common:shortDescription xml:lang="de">kg Sb-Äq.</common:shortDescription>
</epd:referenceToUnitGroupDataSet>
<epd:amount epd:module="A1-A3">7.48E-06</epd:amount>
<epd:amount epd:module="A4">1.05E-08</epd:amount>
<epd:amount epd:module="A5">6.05E-07</epd:amount>
<epd:amount epd:module="C1">0</epd:amount>
<epd:amount epd:module="C2" epd:scenario="S1">3.6E-09</epd:amount>
<epd:amount epd:module="C2" epd:scenario="S2">7.2E-10</epd:amount>
<epd:amount epd:module="C3" epd:scenario="S1">6.27E-08</epd:amount>
<epd:amount epd:module="C3" epd:scenario="S2">4.38E-08</epd:amount>
<epd:amount epd:module="C4">0</epd:amount>
<epd:amount epd:module="D" epd:scenario="S1">-8.66E-07</epd:amount>
<epd:amount epd:module="D" epd:scenario="S2">-7.76E-07</epd:amount>
</common:other>
</LCIAResult>
<LCIAResult>
<referenceToLCIAMethodDataSet uri="../lciamethods/804ebcdf-309d-4098-8ed8-fdaf2f389981.xml" type="LCIA method data set" refObjectId="804ebcdf-309d-4098-8ed8-fdaf2f389981">
<common:shortDescription xml:lang="de">Potenzial für den abiotischen Abbau fossiler Brennstoffe (ADPF)</common:shortDescription>
<common:shortDescription xml:lang="en">Abiotic depletion potential for fossil resources (ADPF)</common:shortDescription>
</referenceToLCIAMethodDataSet>
<common:other>
<epd:referenceToUnitGroupDataSet uri="../unitgroups/93a60a57-a3c8-11da-a746-0800200c9a66.xml" type="unit group data set" refObjectId="93a60a57-a3c8-11da-a746-0800200c9a66">
<common:shortDescription xml:lang="de">MJ</common:shortDescription>
</epd:referenceToUnitGroupDataSet>
<epd:amount epd:module="A1-A3">100</epd:amount>
<epd:amount epd:module="A4">1.47</epd:amount>
<epd:amount epd:module="A5">8.25</epd:amount>
<epd:amount epd:module="C1">0</epd:amount>
<epd:amount epd:module="C2" epd:scenario="S1">0.633</epd:amount>
<epd:amount epd:module="C2" epd:scenario="S2">0.127</epd:amount>
<epd:amount epd:module="C3" epd:scenario="S1">1.36</epd:amount>
<epd:amount epd:module="C3" epd:scenario="S2">0.841</epd:amount>
<epd:amount epd:module="C4">0</epd:amount>
<epd:amount epd:module="D" epd:scenario="S1">-138</epd:amount>
<epd:amount epd:module="D" epd:scenario="S2">-41.9</epd:amount>
</common:other>
</LCIAResult>
</LCIAResults>
</processDataSet>