<?xml version="1.0" encoding="utf-8"?>
<processDataSet xmlns:epd="http://www.iai.kit.edu/EPD/2013" xmlns:epd2="http://www.indata.network/EPD/2019" xmlns:common="http://lca.jrc.it/ILCD/Common" xsi:schemaLocation="http://lca.jrc.it/ILCD/Process ../../schemas/EPD_DataSet.xsd" epd2:epd-version="1.2" version="1.1" locations="../ILCDLocations.xml" xmlns:xsi="http://www.w3.org/2001/XMLSchema-instance" xmlns="http://lca.jrc.it/ILCD/Process">
<processInformation>
<dataSetInformation>
<common:UUID>4d3bcf18-9a74-4f4e-93d8-dabd48a73f19</common:UUID>
<name>
<baseName xml:lang="de">StoVentec R</baseName>
<baseName xml:lang="en">StoVentec R</baseName>
<functionalUnitFlowProperties xml:lang="de" />
</name>
<classificationInformation>
<common:classification name="OEKOBAU.DAT">
<common:class level="0" classId="10">Komposite</common:class>
<common:class level="1" classId="10.1">Systembauteile</common:class>
<common:class level="2" classId="10.1.03">Aussenwände</common:class>
</common:classification>
<common:classification name="IBUCategories">
<common:class level="0">02 Bauprodukte</common:class>
<common:class level="1">Fassaden</common:class>
<common:class level="2">Vorhangfassaden</common:class>
</common:classification>
</classificationInformation>
<common:generalComment xml:lang="de">Sto SE &amp; Co. KGaA ist ein international führender Hersteller von Produkten und Systemen für Gebäudebeschichtungen mit mehr als 5.500 Mitarbeitern. Der Umsatz 2019 betrug 1,39 Milliarden Euro. Zum Kernsortiment gehören Fassadensysteme in Form von Wärmedämm-Verbundsystemen (WDVS) sowie vorgehängten hinterlüfteten Fassadensystemen (VHF). Sto Scandinavia AB operiert in Nordeuropa (Schweden, Norwegen, Dänemark und Finnland) als vollständige Tochtergesellschaft von Sto SE &amp; Co KGaA. Die geschäftlichen Aktivitäten umfassen die Entwicklung, Produktion und Vermarktung sowie den Vertrieb von Produkten, Systemen und Lösungen für Fassaden, Beton, Innenräume und Böden.  Produktbeschreibung/Produktdefinition StoVentec R ist eine hinterlüftete Vorhangfassade mit fugenloser Putzoberfläche, die die Wände atmen lässt und Unebenheiten des Untergrunds ausgleicht. StoVentec R kann auf verschiedenen Unterkonstruktionen montiert werden. Die Unterkonstruktion sowie die Dämmung werden in dieser Deklaration nicht berücksichtigt. Die Deklaration umfasst die folgenden Komponenten. Dabei können die speziellen (Sto-)Produkte einiger Komponenten variieren: StoVentec R organisch: - StoVentec Trägerplatte/StoVentec Trägerplatte A - Befestigungsschrauben für StoVentec Trägerplatte (Verwendung für diese EPD: StoVentec Schraube/  Sto-Fassadenschraube) - Unterputz (Verwendung für diese EPD: StoArmat Classic Plus) - Komprimiertes Dichtband aus imprägniertem Weichschaum (Verwendung für diese EPD:  StoVentec Dichtband 10/3-7) - Schutzprofil für Abschlusskanten der Putzträgerplatte (Verwendung für diese EPD:  Sto-Kantenschutzprofil G) - Abschlussprofil mit Tropfkante  (Verwendung für diese EPD: Sto-Regenabweisprofil G)   - Kantenprofil mit integriertem Glasfasergewebe  (Verwendung für diese EPD:  Sto-Gewebewinkel Standard 11/13 cm) - Alkalibeständiges Armierungsgewebe  (Verwendung für diese EPD: Sto-Glasfasergewebe F) - Schlussbeschichtung (Verwendung für diese EPD: StoLotusan K) StoVentec R mineralisch: - StoVentec Trägerplatte/StoVentec Trägerplatte A - Befestigungsschrauben für StoVentec Trägerplatte (Verwendung für diese EPD: StoVentec Schraube/  Sto-Schraube) - Grundbeschichtung  (Verwendung für diese EPD: Sto-Putzgrund) - Unterputz (Verwendung für diese EPD: StoLevell Evo) - Komprimiertes Dichtband aus imprägniertem Weichschaum (Verwendung für diese EPD:  StoVentec Dichtband 10/3-7) - Schutzprofil für Abschlusskanten der Putzträgerplatte (Verwendung für diese EPD:  Sto-Kantenschutzprofil G) - Abschlussprofil mit Tropfkante  (Verwendung für diese EPD: Sto-Regenabweisprofil G)  - Kantenprofil mit integriertem Glasfasergewebe  (Verwendung für diese EPD:  Sto-Gewebewinkel Standard 11/13 cm) - Alkalibeständiges Armierungsgewebe  (Verwendung für diese EPD: Sto-Glasfasergewebe) - Zwischenbeschichtung  (Verwendung: StoPrep Miral) - Schlussbeschichtung (Verwendung für diese EPD: StoLotusan K) Für das Inverkehrbringen des Produkts in der EU/EFTA (mit Ausnahme der Schweiz) gilt die Verordnung (EU) Nr. 305/2011 (CPR).  Das Produkt benötigt eine Leistungserklärung unter Berücksichtigung der Europäischen Technischen Zulassung Nr. ETA-17/0406, Datum: 13.6.2017, Titel: StoVentec R, und die CE-Kennzeichnung.    Für die Verarbeitung und Verwendung gelten die jeweiligen nationalen Bestimmungen.</common:generalComment>
<common:generalComment xml:lang="en">StoVentec R is a ventilated rainscreen cladding system with a seamless render finish, allowing walls to breathe and levelling uneven substrates. StoVentec R can be mounted on different types of substructures. The substructure or the insulation is not included in this declaration. The declaration includes the following components. The specific (Sto-)products of some components can vary:StoVentec R organic: - StoVentec Carrier Board / StoVentec Carrier Board A - Fixing screws for StoVentec Carrier Board  (used for this declaration: StoVentec Screw /  Sto-Façade Screw) - Basecoat  (used for this declaration: StoArmat Classic Plus) - Compressed sealing tape made of impregnated flexible foam (used for this declaration:  StoVentec Waterproofing Joint 10/3-7) - Protective profile for the outer edges of the render carrier board (used for this declaration:  Sto-Edge Protection Profile G) - Stop profile with drip edge  (used for this declaration: Sto-Rain Guard Profile G)  - Edge profile with integrated glass fibre mesh  (used for this declaration:  Sto-Mesh Angle Bead Standard 11/13 cm) - Alkali-resistant reinforcing mesh  (used for this declaration: Sto-Glass Fibre Mesh F) - Finish (used for this declaration: StoLotusan K) StoVentec R mineralic: - StoVentec Carrier Board / StoVentec Carrier Board A - Fixing screws for StoVentec Carrier Board  (used for this declaration: StoVentec Screw) - Substrate coating  (used for this declaration: Sto Primer) - Basecoat (used for this declaration: StoLevell Evo) - Compressed sealing tape made of impregnated flexible foam (used for this declaration:  StoVentec Waterproofing Joint 10/3-7) - Protective profile for the outer edges of the render carrier board (used for this declaration:  Sto-Edge Protection Profile G) - Stop profile with drip edge  (used for this declaration: Sto-Rain Guard Profile G) - Edge profile with integrated glass fibre mesh  (used for this declaration:  Sto-Mesh Angle Bead Standard 11/13 cm) - Alkali-resistant reinforcing mesh  (used for this declaration: Sto Glass Fibre Mesh) - Intermediate coat  (used for this declaration: StoPrep Miral) - Finish (used for this declaration: StoLotusan K) For the placing of the product on the market in the European Union/European Free Trade Association /EU/EFTA) (with the exception of Switzerland) the Regulation (EU) No. 305/2011 (CPR) applies.  The product needs a declaration of performance taking into consideration ETA no. ETA-17/0406 :date 13/6-2017, title StoVentec R  and the CE-marking. For the application and use the respective national provisions apply.</common:generalComment>
</dataSetInformation>
<quantitativeReference>
<referenceToReferenceFlow>0</referenceToReferenceFlow>
</quantitativeReference>
<time>
<common:referenceYear>2021</common:referenceYear>
<common:dataSetValidUntil>2025</common:dataSetValidUntil>
<common:other>
<epd2:publicationDateOfEPD>2021-06-08</epd2:publicationDateOfEPD>
</common:other>
</time>
<geography>
<locationOfOperationSupplyOrProduction location="RER" />
</geography>
<technology>
<technologyDescriptionAndIncludedProcesses xml:lang="de">This dataset represents one squaremeter (1 m²) StoVentec R ventilated facade system (13,287 kg/m²), based on organic plasters. The composition of the system is: Carrier Board (StoVentec Carrier Board): 6,000 kg/m2 (1 pc/m2) Fixing screws (Stainless steel screws): 0,049 kg/m2 (12 pc/m2) Basecoat (StoArmat Classic Plus): 4,500 kg/m2 Compressed sealing tape made of impregnated flexible foam (StoVentec Waterproofing Joint 10/3-7): 0,005 kg/m2 Protective profile for the outer edges of the render carrier board (Sto-Edge Protection Profile G): 0,058 kg/m2 Profile with drip edge (Sto-Rain Guard Profile G): 0,063 kg/m2 Edge profile with integrated glass fibre mesh (Sto-Mesh Angle Bead Standard 11/3 cm): 0,040 kg/m2 Alkali-resistant reinforcing mesh (Glass Reinforcement mesh): 0,174 kg/m2 Finish (StoLotusan K): 2,400 kg/m2 For further details, and LCA results for a mineral based ventilated facade system, see the EPD document and it´s public annexe. 
Deklarierte Einheit: 
Die Deklaration bezieht sich auf 1 m² Fassadensystem StoVentec R (1) mit einer Oberflächenmasse von 13,287 kg/m² und einer Dicke von 16 mm. Die Deklaration bezieht sich auf 1 m² Fassadensystem StoVentec R (2) (siehe öffentlicher Anhang der EPD) mit einer Oberflächenmasse von 19,504 kg/m² und einer Dicke von 20 mm.</technologyDescriptionAndIncludedProcesses>
<technologyDescriptionAndIncludedProcesses xml:lang="en">This dataset represents one squaremeter (1 m²) StoVentec R ventilated facade system (13,287 kg/m²), based on organic plasters. The composition of the system is: Carrier Board (StoVentec Carrier Board): 6,000 kg/m2 (1 pc/m2) Fixing screws (Stainless steel screws): 0,049 kg/m2 (12 pc/m2) Basecoat (StoArmat Classic Plus): 4,500 kg/m2 Compressed sealing tape made of impregnated flexible foam (StoVentec Waterproofing Joint 10/3-7): 0,005 kg/m2 Protective profile for the outer edges of the render carrier board (Sto-Edge Protection Profile G): 0,058 kg/m2 Profile with drip edge (Sto-Rain Guard Profile G): 0,063 kg/m2 Edge profile with integrated glass fibre mesh (Sto-Mesh Angle Bead Standard 11/3 cm): 0,040 kg/m2 Alkali-resistant reinforcing mesh (Glass Reinforcement mesh): 0,174 kg/m2 Finish (StoLotusan K): 2,400 kg/m2 For further details, and LCA results for a mineral based ventilated facade system, see the EPD document and it´s public annexe. 
Declared unit: 
The declared unit for the StoVentec R (1) facade system is 1 m² with a surface weight of 13,287 kg/m² and a thickness of 16mm.The declared unit for the StoVentec R (2) facade system (see public annex to the EPD)  is 1 m² with a surface weight of 19,504 kg/m² and a thickness of 20mm.</technologyDescriptionAndIncludedProcesses>
<technologicalApplicability xml:lang="de">Das deklarierte Produkt StoVentec R wird als fugenloses Putzsystem mit vorgehängter hinterlüfteter Fassade (VHF) verwendet. Für die Verarbeitung und Anwendung gelten die jeweiligen nationalen Bestimmungen. In Deutschland ist dies beispielsweise die Allgemeine bauaufsichtliche Zulassung Z-10.3-717 des Deutschen Instituts für Bautechnik (DiBt), Berlin.</technologicalApplicability>
<technologicalApplicability xml:lang="en">The declared product StoVentec R is being used as a seamless plaster system within an RSC (Rainscreen cladding) system. For the application and use national regulations apply. For example, in Germany the “Allgemeine bauaufsichtliche Zulassung Z-10.3-717” issued by the Deutsches Institut für Bautechnik (DiBt), Berlin, applies.</technologicalApplicability>
</technology>
</processInformation>
<modellingAndValidation>
<LCIMethodAndAllocation>
<typeOfDataSet>EPD</typeOfDataSet>
<referenceToLCAMethodDetails type="source data set" refObjectId="55c881f9-aa14-4fc5-aa28-ae9ca592d7a2">
<common:shortDescription xml:lang="de">Vorhangfassaden.pdf</common:shortDescription>
</referenceToLCAMethodDetails>
<common:other>
<epd:subType xmlns="http://www.iai.kit.edu/EPD/2013">average dataset</epd:subType>
</common:other>
</LCIMethodAndAllocation>
<dataSourcesTreatmentAndRepresentativeness>
<referenceToDataSource type="source data set" refObjectId="28d74cc0-db8b-4d7e-bc44-5f6d56ce0c4a">
<common:shortDescription xml:lang="de">GaBi Database (all versions)</common:shortDescription>
</referenceToDataSource>
<referenceToDataSource type="source data set" refObjectId="4467e22f-78e4-4e21-ae4a-b8ffeda7d795">
<common:shortDescription xml:lang="de">GaBi database SP38 2019</common:shortDescription>
</referenceToDataSource>
<useAdviceForDataSet xml:lang="de">Gültigkeitsbereich: 
Diese Deklaration bezieht sich auf hinterlüftete Fassadensysteme StoVentec R ohne Unterkonstruktion und Dämmung. Es werden zwei Fassadenvarianten betrachtet: - StoVentec R (1) auf organischem Unterputz, Deklaration im vorliegenden Dokument. - StoVentec R (2) auf mineralischem Unterputz, Deklaration im öffentlichen Anhang zu dieser EPD. Die Produktkomponenten werden von Sto SE &amp; Co. KGaA (Standort in Stühlingen, Deutschland), Sto Scandinavia AB (Standort Linköping, Schweden) und externen Lieferanten hergestellt. 
Systemgrenze: 
Cradle to gate - mit Optionen. Beschreibung der Systemgrenzen: Modul A1 bis A3: Dieses Modul berücksichtigt die Herstellung der Systemkomponenten (z. B. Trägerplatte, Befestigungen, Putz usw.), ihren Transport zur Baustelle in Schweden sowie die Herstellung/Zusammenstellung der Komponenten des Fassadensystems. Auch die Auswirkungen für die Herstellung des Verpackungsmaterials wurden berücksichtigt. Modul A4: Dieses Modul berücksichtigt eine Transportstrecke von 100 km per Lkw zur Baustelle. Die Transportstrecke kann projektspezifisch angepasst werden. Modul A5: Verwertung und Entsorgung des Verpackungsmaterials. Gutschriften für die potenzielle Vermeidung von Lasten für die Strom- und Wärmeenergieerzeugung werden im Modul D deklariert und betreffen nur den Anteil der neuen Materialien. In A5 werden 10 % Überlappung mit Glasfasergewebe berücksichtigt (Herstellung der Überlappung im Rahmen des Moduls A1–A3, „Bausatz-Ansatz“). Der Stromverbrauch für Bohrarbeiten und den Mörtelauftrag wird berücksichtigt. Montageverluste wurden nicht berücksichtigt, da solche Verluste in hohem Maße von der jeweiligen Gebäudegeometrie und weiteren standortspezifischen Faktoren abhängig sind. Schätzwerte für Montageverluste können anhand der Ergebnisse aus der Ökobilanz für die Herstellung und Entsorgung beispielsweise mittels Skalierung bestimmt werden. Modul C1 bis C4: C1: Manueller Rückbau, keine Umweltlasten. C2: 50 km Lkw-Transport zur Abfallaufbereitung (je nach Gebäude anpassbar). C3: Keine zusätzliche Abfallbehandlung, keine Umweltlasten.   C4: Deklariert wird das europäische Szenario für durchschnittliche Emissionen bei der Deponierung. Modul D: Gutschriften und Lasten für Metallkomponenten und vermiedene Lasten aus der Verpackungsverwertung.</useAdviceForDataSet>
<useAdviceForDataSet xml:lang="en">Scope: 
This declaration covers the StoVentec R ventilated façade systems without subconstruction and insulation. Two specific façade variations are covered:- StoVentec R (1), based on organic plaster, declared in this document.- StoVentec R (2), based on mineral plaster, LCA results can be found in the public annexe to this EPD.Product components are produced by Sto SE &amp; Co. KGaA (site at Stühlingen, Germany), Sto Scandinavia AB (site at Linköping, Sweden), and external suppliers. 
System boundary: 
Cradle to gate - with options. Description of the system boundaries:Module A1 to A3: This module considers the manufacturing of system components (e.g. carrier board, fastening, plaster etc.), the transport to the site in Sweden and the manufacturing/compiling of the façade system components. The impact for producing packaging materials is included as well.Module A4: This module considers 100 km truck transport to site. The transport distance can be modified project-specific.Module A5: Treatment and disposal of packaging material. Credits for potential avoided burdens on electricity and thermal energy generation are declared in module D and affects only the rate of virgin material.An overlap of 10% with glass fibre mesh is considered in A5 (production of overlap within module A1-A3, “kit-approach”).Electricity consumption for drilling and mortar application is considered.Installation losses have not been accounted for, since such losses highly depend on the specific building geometry and other site-specific factors. Installation losses may be estimated based on the LCA results for manufacturing and End-Of-Life (EoL), e.g. via scaling.Module C1 to C4: C1: Manual dismantling, no environmental burdens.C2: 50 km transport to waste treatment by truck (may be adapted on building level).C3: No additional waste processing, no environmental burdens.   C4: European scenario for average landfill emissions is declared.Module D: Benefits and loads for metal components and avoided burdens from packaging treatment.</useAdviceForDataSet>
<common:other>
<epd2:referenceToOriginalEPD type="source data set" refObjectId="f8fdc00a-39c0-4d0e-9a79-948cf0ee3cb8">
<common:shortDescription xml:lang="de">StoVentec R.pdf</common:shortDescription>
</epd2:referenceToOriginalEPD>
</common:other>
</dataSourcesTreatmentAndRepresentativeness>
<validation>
<review type="Accredited third party review">
<common:referenceToNameOfReviewerAndInstitution uri="../contacts/d111dbec-b024-4be5-86c5-752d6eb2cf95.xml" type="contact data set" refObjectId="d111dbec-b024-4be5-86c5-752d6eb2cf95">
<common:shortDescription xml:lang="de">Institut Bauen und Umwelt e. V.</common:shortDescription>
</common:referenceToNameOfReviewerAndInstitution>
</review>
</validation>
<complianceDeclarations>
<compliance>
<common:referenceToComplianceSystem uri="../sources/b00f9ec0-7874-11e3-981f-0800200c9a66.xml" type="source data set" refObjectId="b00f9ec0-7874-11e3-981f-0800200c9a66">
<common:shortDescription xml:lang="de">DIN EN 15804</common:shortDescription>
</common:referenceToComplianceSystem>
</compliance>
<compliance>
<common:referenceToComplianceSystem uri="../sources/4f2eb655-6e44-4874-a95a-e28f5442cd4d.xml" type="source data set" refObjectId="4f2eb655-6e44-4874-a95a-e28f5442cd4d">
<common:shortDescription xml:lang="de">ISO 14025</common:shortDescription>
</common:referenceToComplianceSystem>
</compliance>
</complianceDeclarations>
</modellingAndValidation>
<administrativeInformation>
<common:commissionerAndGoal>
<common:referenceToCommissioner uri="../contacts/d1f9cf21-554b-41a8-976f-83ff8dfe6987.xml" type="contact data set" refObjectId="d1f9cf21-554b-41a8-976f-83ff8dfe6987">
<common:shortDescription xml:lang="de">Sto SE &amp; Co. KGaA</common:shortDescription>
</common:referenceToCommissioner>
</common:commissionerAndGoal>
<dataGenerator>
<common:referenceToPersonOrEntityGeneratingTheDataSet uri="../contacts/623edf96-39d1-4e6f-9892-674c7228546b.xml" type="contact data set" refObjectId="623edf96-39d1-4e6f-9892-674c7228546b">
<common:shortDescription xml:lang="de">Sphera Solutions GmbH</common:shortDescription>
</common:referenceToPersonOrEntityGeneratingTheDataSet>
</dataGenerator>
<dataEntryBy>
<common:timeStamp>2021-06-08T17:19:47.076</common:timeStamp>
<common:referenceToDataSetFormat uri="../sources/a97a0155-0234-4b87-b4ce-a45da52f2a40.xml" type="source data set" refObjectId="a97a0155-0234-4b87-b4ce-a45da52f2a40">
<common:shortDescription xml:lang="de">ILCD Format</common:shortDescription>
</common:referenceToDataSetFormat>
<common:referenceToDataSetFormat uri="../sources/a29449fd-aa2f-4de8-b5d7-4b06b43c6fde.xml" type="source data set" refObjectId="a29449fd-aa2f-4de8-b5d7-4b06b43c6fde">
<common:shortDescription xml:lang="de">EPD-Datenformaterweiterungen v1.2</common:shortDescription>
<common:shortDescription xml:lang="en">EPD Data Format Extensions v1.2</common:shortDescription>
</common:referenceToDataSetFormat>
</dataEntryBy>
<publicationAndOwnership>
<common:dataSetVersion>00.06.000</common:dataSetVersion>
<common:referenceToPrecedingDataSetVersion uri="../processes/4d3bcf18-9a74-4f4e-93d8-dabd48a73f19.xml" type="process data set" refObjectId="4d3bcf18-9a74-4f4e-93d8-dabd48a73f19">
<common:shortDescription xml:lang="de">StoVentec R</common:shortDescription>
</common:referenceToPrecedingDataSetVersion>
<common:referenceToRegistrationAuthority uri="../contacts/d111dbec-b024-4be5-86c5-752d6eb2cf95.xml" type="contact data set" refObjectId="d111dbec-b024-4be5-86c5-752d6eb2cf95">
<common:shortDescription xml:lang="de">Institut Bauen und Umwelt e. V.</common:shortDescription>
</common:referenceToRegistrationAuthority>
<common:registrationNumber>EPD-STO-20200207-CBD1-DE</common:registrationNumber>
<common:referenceToOwnershipOfDataSet uri="../contacts/d1f9cf21-554b-41a8-976f-83ff8dfe6987.xml" type="contact data set" refObjectId="d1f9cf21-554b-41a8-976f-83ff8dfe6987">
<common:shortDescription xml:lang="de">Sto SE &amp; Co. KGaA</common:shortDescription>
</common:referenceToOwnershipOfDataSet>
<common:copyright>true</common:copyright>
<common:licenseType>Free of charge for all users and uses</common:licenseType>
<common:accessRestrictions xml:lang="en">None</common:accessRestrictions>
<common:other>
<epd2:referenceToPublisher type="contact data set" refObjectId="d111dbec-b024-4be5-86c5-752d6eb2cf95" uri="../contacts/d111dbec-b024-4be5-86c5-752d6eb2cf95.xml">
<common:shortDescription xml:lang="de">Institut Bauen und Umwelt e. V.</common:shortDescription>
</epd2:referenceToPublisher>
</common:other>
</publicationAndOwnership>
</administrativeInformation>
<exchanges>
<exchange dataSetInternalID="0">
<referenceToFlowDataSet uri="../flows/ae6c2e62-e50c-2c74-2431-966f0a3089da.xml" type="flow data set" refObjectId="ae6c2e62-e50c-2c74-2431-966f0a3089da">
<common:shortDescription xml:lang="de">StoVentec R (StoVentec R)</common:shortDescription>
</referenceToFlowDataSet>
<meanAmount>1</meanAmount>
<referencesToDataSource />
</exchange>
<exchange dataSetInternalID="1">
<referenceToFlowDataSet uri="../flows/20f32be5-0398-4288-9b6d-accddd195317.xml" type="flow data set" refObjectId="20f32be5-0398-4288-9b6d-accddd195317">
<common:shortDescription xml:lang="de">Erneuerbare Primärenergie als Energieträger (PERE)</common:shortDescription>
<common:shortDescription xml:lang="en">Renewable primary energy as energy carrier (PERE)</common:shortDescription>
</referenceToFlowDataSet>
<functionType>General reminder flow</functionType>
<exchangeDirection>Input</exchangeDirection>
<common:other>
<epd:referenceToUnitGroupDataSet uri="../unitgroups/93a60a57-a3c8-11da-a746-0800200c9a66.xml" type="unit group data set" refObjectId="93a60a57-a3c8-11da-a746-0800200c9a66">
<common:shortDescription xml:lang="de">MJ</common:shortDescription>
</epd:referenceToUnitGroupDataSet>
<epd:amount epd:module="A1-A3">34.497</epd:amount>
<epd:amount epd:module="A4">0.0694</epd:amount>
<epd:amount epd:module="A5">7.66</epd:amount>
<epd:amount epd:module="C1">0</epd:amount>
<epd:amount epd:module="C2">0.0347</epd:amount>
<epd:amount epd:module="C4">1.13</epd:amount>
<epd:amount epd:module="D">-2.95</epd:amount>
</common:other>
</exchange>
<exchange dataSetInternalID="2">
<referenceToFlowDataSet uri="../flows/fb3ec0de-548d-4508-aea5-00b73bf6f702.xml" type="flow data set" refObjectId="fb3ec0de-548d-4508-aea5-00b73bf6f702">
<common:shortDescription xml:lang="de">Erneuerbare Primärenergie zur stofflichen Nutzung (PERM)</common:shortDescription>
<common:shortDescription xml:lang="en">Renewable primary energy resources as material utilization (PERM)</common:shortDescription>
</referenceToFlowDataSet>
<functionType>General reminder flow</functionType>
<exchangeDirection>Input</exchangeDirection>
<common:other>
<epd:referenceToUnitGroupDataSet uri="../unitgroups/93a60a57-a3c8-11da-a746-0800200c9a66.xml" type="unit group data set" refObjectId="93a60a57-a3c8-11da-a746-0800200c9a66">
<common:shortDescription xml:lang="de">MJ</common:shortDescription>
</epd:referenceToUnitGroupDataSet>
<epd:amount epd:module="A1-A3">8.173</epd:amount>
<epd:amount epd:module="A4">0</epd:amount>
<epd:amount epd:module="A5">-7.39</epd:amount>
<epd:amount epd:module="C1">0</epd:amount>
<epd:amount epd:module="C2">0</epd:amount>
<epd:amount epd:module="C4">-0.786</epd:amount>
<epd:amount epd:module="D">0</epd:amount>
</common:other>
</exchange>
<exchange dataSetInternalID="3">
<referenceToFlowDataSet uri="../flows/53f97275-fa8a-4cdd-9024-65936002acd0.xml" type="flow data set" refObjectId="53f97275-fa8a-4cdd-9024-65936002acd0">
<common:shortDescription xml:lang="de">Total erneuerbare Primärenergie (PERT)</common:shortDescription>
<common:shortDescription xml:lang="en">Total use of renewable primary energy resources (PERT)</common:shortDescription>
</referenceToFlowDataSet>
<functionType>General reminder flow</functionType>
<exchangeDirection>Input</exchangeDirection>
<common:other>
<epd:referenceToUnitGroupDataSet uri="../unitgroups/93a60a57-a3c8-11da-a746-0800200c9a66.xml" type="unit group data set" refObjectId="93a60a57-a3c8-11da-a746-0800200c9a66">
<common:shortDescription xml:lang="de">MJ</common:shortDescription>
</epd:referenceToUnitGroupDataSet>
<epd:amount epd:module="A1-A3">42.667</epd:amount>
<epd:amount epd:module="A4">0.0694</epd:amount>
<epd:amount epd:module="A5">0.272</epd:amount>
<epd:amount epd:module="C1">0</epd:amount>
<epd:amount epd:module="C2">0.0347</epd:amount>
<epd:amount epd:module="C4">0.346</epd:amount>
<epd:amount epd:module="D">-2.95</epd:amount>
</common:other>
</exchange>
<exchange dataSetInternalID="4">
<referenceToFlowDataSet uri="../flows/ac857178-2b45-46ec-892a-a9a4332f0372.xml" type="flow data set" refObjectId="ac857178-2b45-46ec-892a-a9a4332f0372">
<common:shortDescription xml:lang="de">Nicht-erneuerbare Primärenergie als Energieträger (PENRE)</common:shortDescription>
<common:shortDescription xml:lang="en">Non renewable primary energy as energy carrier (PENRE)</common:shortDescription>
</referenceToFlowDataSet>
<functionType>General reminder flow</functionType>
<exchangeDirection>Input</exchangeDirection>
<common:other>
<epd:referenceToUnitGroupDataSet uri="../unitgroups/93a60a57-a3c8-11da-a746-0800200c9a66.xml" type="unit group data set" refObjectId="93a60a57-a3c8-11da-a746-0800200c9a66">
<common:shortDescription xml:lang="de">MJ</common:shortDescription>
</epd:referenceToUnitGroupDataSet>
<epd:amount epd:module="A1-A3">270.1</epd:amount>
<epd:amount epd:module="A4">1.24</epd:amount>
<epd:amount epd:module="A5">9.5</epd:amount>
<epd:amount epd:module="C1">0</epd:amount>
<epd:amount epd:module="C2">0.618</epd:amount>
<epd:amount epd:module="C4">24.1</epd:amount>
<epd:amount epd:module="D">-13.5</epd:amount>
</common:other>
</exchange>
<exchange dataSetInternalID="5">
<referenceToFlowDataSet uri="../flows/1421caa0-679d-4bf4-b282-0eb850ccae27.xml" type="flow data set" refObjectId="1421caa0-679d-4bf4-b282-0eb850ccae27">
<common:shortDescription xml:lang="de">Nicht-erneuerbare Primärenergie zur stofflichen Nutzung (PENRM)</common:shortDescription>
<common:shortDescription xml:lang="en">Non renewable primary energy as material utilization (PENRM)</common:shortDescription>
</referenceToFlowDataSet>
<functionType>General reminder flow</functionType>
<exchangeDirection>Input</exchangeDirection>
<common:other>
<epd:referenceToUnitGroupDataSet uri="../unitgroups/93a60a57-a3c8-11da-a746-0800200c9a66.xml" type="unit group data set" refObjectId="93a60a57-a3c8-11da-a746-0800200c9a66">
<common:shortDescription xml:lang="de">MJ</common:shortDescription>
</epd:referenceToUnitGroupDataSet>
<epd:amount epd:module="A1-A3">30.19</epd:amount>
<epd:amount epd:module="A4">0</epd:amount>
<epd:amount epd:module="A5">-8.69</epd:amount>
<epd:amount epd:module="C1">0</epd:amount>
<epd:amount epd:module="C2">0</epd:amount>
<epd:amount epd:module="C4">-21.5</epd:amount>
<epd:amount epd:module="D">0</epd:amount>
</common:other>
</exchange>
<exchange dataSetInternalID="6">
<referenceToFlowDataSet uri="../flows/06159210-646b-4c8d-8583-da9b3b95a6c1.xml" type="flow data set" refObjectId="06159210-646b-4c8d-8583-da9b3b95a6c1">
<common:shortDescription xml:lang="de">Total nicht erneuerbare Primärenergie (PENRT)</common:shortDescription>
<common:shortDescription xml:lang="en">Total use of non renewable primary energy resources (PENRT)</common:shortDescription>
</referenceToFlowDataSet>
<functionType>General reminder flow</functionType>
<exchangeDirection>Input</exchangeDirection>
<common:other>
<epd:referenceToUnitGroupDataSet uri="../unitgroups/93a60a57-a3c8-11da-a746-0800200c9a66.xml" type="unit group data set" refObjectId="93a60a57-a3c8-11da-a746-0800200c9a66">
<common:shortDescription xml:lang="de">MJ</common:shortDescription>
</epd:referenceToUnitGroupDataSet>
<epd:amount epd:module="A1-A3">300.8</epd:amount>
<epd:amount epd:module="A4">1.24</epd:amount>
<epd:amount epd:module="A5">0.809</epd:amount>
<epd:amount epd:module="C1">0</epd:amount>
<epd:amount epd:module="C2">0.618</epd:amount>
<epd:amount epd:module="C4">2.64</epd:amount>
<epd:amount epd:module="D">-13.5</epd:amount>
</common:other>
</exchange>
<exchange dataSetInternalID="7">
<referenceToFlowDataSet uri="../flows/c6a1f35f-2d09-4f54-8dfb-97e502e1ce92.xml" type="flow data set" refObjectId="c6a1f35f-2d09-4f54-8dfb-97e502e1ce92">
<common:shortDescription xml:lang="de">Einsatz von Sekundärstoffen (SM)</common:shortDescription>
<common:shortDescription xml:lang="en">Use of secondary material (SM)</common:shortDescription>
</referenceToFlowDataSet>
<functionType>General reminder flow</functionType>
<exchangeDirection>Input</exchangeDirection>
<common:other>
<epd:referenceToUnitGroupDataSet uri="../unitgroups/ad38d542-3fe9-439d-9b95-2f5f7752acaf.xml" type="unit group data set" refObjectId="ad38d542-3fe9-439d-9b95-2f5f7752acaf">
<common:shortDescription xml:lang="de">kg</common:shortDescription>
</epd:referenceToUnitGroupDataSet>
<epd:amount epd:module="A1-A3">5.11</epd:amount>
<epd:amount epd:module="A4">0</epd:amount>
<epd:amount epd:module="A5">0</epd:amount>
<epd:amount epd:module="C1">0</epd:amount>
<epd:amount epd:module="C2">0</epd:amount>
<epd:amount epd:module="C4">0</epd:amount>
<epd:amount epd:module="D">0</epd:amount>
</common:other>
</exchange>
<exchange dataSetInternalID="8">
<referenceToFlowDataSet uri="../flows/64333088-a55f-4aa2-9a31-c10b07816787.xml" type="flow data set" refObjectId="64333088-a55f-4aa2-9a31-c10b07816787">
<common:shortDescription xml:lang="de">Erneuerbare Sekundärbrennstoffe (RSF)</common:shortDescription>
<common:shortDescription xml:lang="en">Use of renewable secondary fuels (RSF)</common:shortDescription>
</referenceToFlowDataSet>
<functionType>General reminder flow</functionType>
<exchangeDirection>Input</exchangeDirection>
<common:other>
<epd:referenceToUnitGroupDataSet uri="../unitgroups/93a60a57-a3c8-11da-a746-0800200c9a66.xml" type="unit group data set" refObjectId="93a60a57-a3c8-11da-a746-0800200c9a66">
<common:shortDescription xml:lang="de">MJ</common:shortDescription>
</epd:referenceToUnitGroupDataSet>
<epd:amount epd:module="A1-A3">0</epd:amount>
<epd:amount epd:module="A4">0</epd:amount>
<epd:amount epd:module="A5">0</epd:amount>
<epd:amount epd:module="C1">0</epd:amount>
<epd:amount epd:module="C2">0</epd:amount>
<epd:amount epd:module="C4">0</epd:amount>
<epd:amount epd:module="D">0</epd:amount>
</common:other>
</exchange>
<exchange dataSetInternalID="9">
<referenceToFlowDataSet uri="../flows/89def144-d39a-4287-b86f-efde453ddcb2.xml" type="flow data set" refObjectId="89def144-d39a-4287-b86f-efde453ddcb2">
<common:shortDescription xml:lang="de">Nicht erneuerbare Sekundärbrennstoffe (NRSF)</common:shortDescription>
<common:shortDescription xml:lang="en">Use of non renewable secondary fuels (NRSF)</common:shortDescription>
</referenceToFlowDataSet>
<functionType>General reminder flow</functionType>
<exchangeDirection>Input</exchangeDirection>
<common:other>
<epd:referenceToUnitGroupDataSet uri="../unitgroups/93a60a57-a3c8-11da-a746-0800200c9a66.xml" type="unit group data set" refObjectId="93a60a57-a3c8-11da-a746-0800200c9a66">
<common:shortDescription xml:lang="de">MJ</common:shortDescription>
</epd:referenceToUnitGroupDataSet>
<epd:amount epd:module="A1-A3">0</epd:amount>
<epd:amount epd:module="A4">0</epd:amount>
<epd:amount epd:module="A5">0</epd:amount>
<epd:amount epd:module="C1">0</epd:amount>
<epd:amount epd:module="C2">0</epd:amount>
<epd:amount epd:module="C4">0</epd:amount>
<epd:amount epd:module="D">0</epd:amount>
</common:other>
</exchange>
<exchange dataSetInternalID="10">
<referenceToFlowDataSet uri="../flows/3cf952c8-f3a4-461d-8c96-96456ca62246.xml" type="flow data set" refObjectId="3cf952c8-f3a4-461d-8c96-96456ca62246">
<common:shortDescription xml:lang="de">Einsatz von Süßwasserressourcen (FW)</common:shortDescription>
<common:shortDescription xml:lang="en">Use of net fresh water (FW)</common:shortDescription>
</referenceToFlowDataSet>
<functionType>General reminder flow</functionType>
<exchangeDirection>Input</exchangeDirection>
<common:other>
<epd:referenceToUnitGroupDataSet uri="../unitgroups/cd950537-0a98-4044-9ba7-9f9a68d0a504.xml" type="unit group data set" refObjectId="cd950537-0a98-4044-9ba7-9f9a68d0a504">
<common:shortDescription xml:lang="de">m^3</common:shortDescription>
</epd:referenceToUnitGroupDataSet>
<epd:amount epd:module="A1-A3">0.05826</epd:amount>
<epd:amount epd:module="A4">8.04E-05</epd:amount>
<epd:amount epd:module="A5">0.00453</epd:amount>
<epd:amount epd:module="C1">0</epd:amount>
<epd:amount epd:module="C2">4.02E-05</epd:amount>
<epd:amount epd:module="C4">0.000665</epd:amount>
<epd:amount epd:module="D">-0.0049</epd:amount>
</common:other>
</exchange>
<exchange dataSetInternalID="11">
<referenceToFlowDataSet uri="../flows/430f9e0f-59b2-46a0-8e0d-55e0e84948fc.xml" type="flow data set" refObjectId="430f9e0f-59b2-46a0-8e0d-55e0e84948fc">
<common:shortDescription xml:lang="de">Gefährlicher Abfall zur Deponie (HWD)</common:shortDescription>
<common:shortDescription xml:lang="en">Hazardous waste disposed (HWD)</common:shortDescription>
</referenceToFlowDataSet>
<functionType>General reminder flow</functionType>
<exchangeDirection>Output</exchangeDirection>
<common:other>
<epd:referenceToUnitGroupDataSet uri="../unitgroups/ad38d542-3fe9-439d-9b95-2f5f7752acaf.xml" type="unit group data set" refObjectId="ad38d542-3fe9-439d-9b95-2f5f7752acaf">
<common:shortDescription xml:lang="de">kg</common:shortDescription>
</epd:referenceToUnitGroupDataSet>
<epd:amount epd:module="A1-A3">1.4385E-06</epd:amount>
<epd:amount epd:module="A4">5.75E-08</epd:amount>
<epd:amount epd:module="A5">4.28E-10</epd:amount>
<epd:amount epd:module="C1">0</epd:amount>
<epd:amount epd:module="C2">2.88E-08</epd:amount>
<epd:amount epd:module="C4">4.02E-08</epd:amount>
<epd:amount epd:module="D">-1.21E-05</epd:amount>
</common:other>
</exchange>
<exchange dataSetInternalID="12">
<referenceToFlowDataSet uri="../flows/b29ef66b-e286-4afa-949f-62f1a7b4d7fa.xml" type="flow data set" refObjectId="b29ef66b-e286-4afa-949f-62f1a7b4d7fa">
<common:shortDescription xml:lang="de">Entsorgter nicht gefährlicher Abfall (NHWD)</common:shortDescription>
<common:shortDescription xml:lang="en">Non hazardous waste disposed (NHWD)</common:shortDescription>
</referenceToFlowDataSet>
<functionType>General reminder flow</functionType>
<exchangeDirection>Output</exchangeDirection>
<common:other>
<epd:referenceToUnitGroupDataSet uri="../unitgroups/ad38d542-3fe9-439d-9b95-2f5f7752acaf.xml" type="unit group data set" refObjectId="ad38d542-3fe9-439d-9b95-2f5f7752acaf">
<common:shortDescription xml:lang="de">kg</common:shortDescription>
</epd:referenceToUnitGroupDataSet>
<epd:amount epd:module="A1-A3">1.00036</epd:amount>
<epd:amount epd:module="A4">0.000189</epd:amount>
<epd:amount epd:module="A5">0.0115</epd:amount>
<epd:amount epd:module="C1">0</epd:amount>
<epd:amount epd:module="C2">9.46E-05</epd:amount>
<epd:amount epd:module="C4">13.3</epd:amount>
<epd:amount epd:module="D">-0.0059</epd:amount>
</common:other>
</exchange>
<exchange dataSetInternalID="13">
<referenceToFlowDataSet uri="../flows/3449546e-52ad-4b39-b809-9fb77cea8ff6.xml" type="flow data set" refObjectId="3449546e-52ad-4b39-b809-9fb77cea8ff6">
<common:shortDescription xml:lang="de">Entsorgter radioaktiver Abfall (RWD)</common:shortDescription>
<common:shortDescription xml:lang="en">Radioactive waste disposed (RWD)</common:shortDescription>
</referenceToFlowDataSet>
<functionType>General reminder flow</functionType>
<exchangeDirection>Output</exchangeDirection>
<common:other>
<epd:referenceToUnitGroupDataSet uri="../unitgroups/ad38d542-3fe9-439d-9b95-2f5f7752acaf.xml" type="unit group data set" refObjectId="ad38d542-3fe9-439d-9b95-2f5f7752acaf">
<common:shortDescription xml:lang="de">kg</common:shortDescription>
</epd:referenceToUnitGroupDataSet>
<epd:amount epd:module="A1-A3">0.0055413</epd:amount>
<epd:amount epd:module="A4">1.53E-06</epd:amount>
<epd:amount epd:module="A5">9.1E-05</epd:amount>
<epd:amount epd:module="C1">0</epd:amount>
<epd:amount epd:module="C2">7.65E-07</epd:amount>
<epd:amount epd:module="C4">3E-05</epd:amount>
<epd:amount epd:module="D">-0.000927</epd:amount>
</common:other>
</exchange>
<exchange dataSetInternalID="14">
<referenceToFlowDataSet uri="../flows/a2b32f97-3fc7-4af2-b209-525bc6426f33.xml" type="flow data set" refObjectId="a2b32f97-3fc7-4af2-b209-525bc6426f33">
<common:shortDescription xml:lang="de">Komponenten für die Wiederverwendung (CRU)</common:shortDescription>
<common:shortDescription xml:lang="en">Components for re-use (CRU)</common:shortDescription>
</referenceToFlowDataSet>
<functionType>General reminder flow</functionType>
<exchangeDirection>Output</exchangeDirection>
<common:other>
<epd:referenceToUnitGroupDataSet uri="../unitgroups/ad38d542-3fe9-439d-9b95-2f5f7752acaf.xml" type="unit group data set" refObjectId="ad38d542-3fe9-439d-9b95-2f5f7752acaf">
<common:shortDescription xml:lang="de">kg</common:shortDescription>
</epd:referenceToUnitGroupDataSet>
<epd:amount epd:module="A1-A3">0</epd:amount>
<epd:amount epd:module="A4">0</epd:amount>
<epd:amount epd:module="A5">0</epd:amount>
<epd:amount epd:module="C1">0</epd:amount>
<epd:amount epd:module="C2">0</epd:amount>
<epd:amount epd:module="C4">0</epd:amount>
<epd:amount epd:module="D">0</epd:amount>
</common:other>
</exchange>
<exchange dataSetInternalID="15">
<referenceToFlowDataSet uri="../flows/d7fe48a5-4103-49c8-9aae-b0b5dfdbd6ae.xml" type="flow data set" refObjectId="d7fe48a5-4103-49c8-9aae-b0b5dfdbd6ae">
<common:shortDescription xml:lang="de">Stoffe zum Recycling (MFR)</common:shortDescription>
<common:shortDescription xml:lang="en">Materials for recycling (MFR)</common:shortDescription>
</referenceToFlowDataSet>
<functionType>General reminder flow</functionType>
<exchangeDirection>Output</exchangeDirection>
<common:other>
<epd:referenceToUnitGroupDataSet uri="../unitgroups/ad38d542-3fe9-439d-9b95-2f5f7752acaf.xml" type="unit group data set" refObjectId="ad38d542-3fe9-439d-9b95-2f5f7752acaf">
<common:shortDescription xml:lang="de">kg</common:shortDescription>
</epd:referenceToUnitGroupDataSet>
<epd:amount epd:module="A1-A3">0</epd:amount>
<epd:amount epd:module="A4">0</epd:amount>
<epd:amount epd:module="A5">0</epd:amount>
<epd:amount epd:module="C1">0.0113</epd:amount>
<epd:amount epd:module="C2">0</epd:amount>
<epd:amount epd:module="C4">0</epd:amount>
<epd:amount epd:module="D">0</epd:amount>
</common:other>
</exchange>
<exchange dataSetInternalID="16">
<referenceToFlowDataSet uri="../flows/59a9181c-3aaf-46ee-8b13-2b3723b6e447.xml" type="flow data set" refObjectId="59a9181c-3aaf-46ee-8b13-2b3723b6e447">
<common:shortDescription xml:lang="de">Stoffe für die Energierückgewinnung (MER)</common:shortDescription>
<common:shortDescription xml:lang="en">Materials for energy recovery (MER)</common:shortDescription>
</referenceToFlowDataSet>
<functionType>General reminder flow</functionType>
<exchangeDirection>Output</exchangeDirection>
<common:other>
<epd:referenceToUnitGroupDataSet uri="../unitgroups/ad38d542-3fe9-439d-9b95-2f5f7752acaf.xml" type="unit group data set" refObjectId="ad38d542-3fe9-439d-9b95-2f5f7752acaf">
<common:shortDescription xml:lang="de">kg</common:shortDescription>
</epd:referenceToUnitGroupDataSet>
<epd:amount epd:module="A1-A3">0</epd:amount>
<epd:amount epd:module="A4">0</epd:amount>
<epd:amount epd:module="A5">0</epd:amount>
<epd:amount epd:module="C1">0</epd:amount>
<epd:amount epd:module="C2">0</epd:amount>
<epd:amount epd:module="C4">0</epd:amount>
<epd:amount epd:module="D">0</epd:amount>
</common:other>
</exchange>
<exchange dataSetInternalID="17">
<referenceToFlowDataSet uri="../flows/4da0c987-2b76-40d6-9e9e-82a017aaaf29.xml" type="flow data set" refObjectId="4da0c987-2b76-40d6-9e9e-82a017aaaf29">
<common:shortDescription xml:lang="de">Exportierte elektrische Energie (EEE)</common:shortDescription>
<common:shortDescription xml:lang="en">Exported electrical energy (EEE)</common:shortDescription>
</referenceToFlowDataSet>
<functionType>General reminder flow</functionType>
<exchangeDirection>Output</exchangeDirection>
<common:other>
<epd:referenceToUnitGroupDataSet uri="../unitgroups/93a60a57-a3c8-11da-a746-0800200c9a66.xml" type="unit group data set" refObjectId="93a60a57-a3c8-11da-a746-0800200c9a66">
<common:shortDescription xml:lang="de">MJ</common:shortDescription>
</epd:referenceToUnitGroupDataSet>
<epd:amount epd:module="A1-A3">0</epd:amount>
<epd:amount epd:module="A4">0</epd:amount>
<epd:amount epd:module="A5">3.07</epd:amount>
<epd:amount epd:module="C1">0</epd:amount>
<epd:amount epd:module="C2">0</epd:amount>
<epd:amount epd:module="C4">0</epd:amount>
<epd:amount epd:module="D">0</epd:amount>
</common:other>
</exchange>
<exchange dataSetInternalID="18">
<referenceToFlowDataSet uri="../flows/98daf38a-7a79-46d3-9a37-2b7bd0955810.xml" type="flow data set" refObjectId="98daf38a-7a79-46d3-9a37-2b7bd0955810">
<common:shortDescription xml:lang="de">Exportierte thermische Energie (EET)</common:shortDescription>
<common:shortDescription xml:lang="en">Exported thermal energy (EET)</common:shortDescription>
</referenceToFlowDataSet>
<functionType>General reminder flow</functionType>
<exchangeDirection>Output</exchangeDirection>
<common:other>
<epd:referenceToUnitGroupDataSet uri="../unitgroups/93a60a57-a3c8-11da-a746-0800200c9a66.xml" type="unit group data set" refObjectId="93a60a57-a3c8-11da-a746-0800200c9a66">
<common:shortDescription xml:lang="de">MJ</common:shortDescription>
</epd:referenceToUnitGroupDataSet>
<epd:amount epd:module="A1-A3">0</epd:amount>
<epd:amount epd:module="A4">0</epd:amount>
<epd:amount epd:module="A5">5.49</epd:amount>
<epd:amount epd:module="C1">0</epd:amount>
<epd:amount epd:module="C2">0</epd:amount>
<epd:amount epd:module="C4">0</epd:amount>
<epd:amount epd:module="D">0</epd:amount>
</common:other>
</exchange>
</exchanges>
<LCIAResults>
<LCIAResult>
<referenceToLCIAMethodDataSet uri="../lciamethods/77e416eb-a363-4258-a04e-171d843a6460.xml" type="LCIA method data set" refObjectId="77e416eb-a363-4258-a04e-171d843a6460">
<common:shortDescription xml:lang="de">Globales Erwärmungspotenzial (GWP)</common:shortDescription>
<common:shortDescription xml:lang="en">Global warming potential (GWP)</common:shortDescription>
</referenceToLCIAMethodDataSet>
<common:other>
<epd:referenceToUnitGroupDataSet uri="../unitgroups/1ebf3012-d0db-4de2-aefd-ef30cedb0be1.xml" type="unit group data set" refObjectId="1ebf3012-d0db-4de2-aefd-ef30cedb0be1">
<common:shortDescription xml:lang="de">kg CO_(2)-Äq.</common:shortDescription>
</epd:referenceToUnitGroupDataSet>
<epd:amount epd:module="A1-A3">15.744</epd:amount>
<epd:amount epd:module="A4">0.091</epd:amount>
<epd:amount epd:module="A5">1.86</epd:amount>
<epd:amount epd:module="C1">0</epd:amount>
<epd:amount epd:module="C2">0.0455</epd:amount>
<epd:amount epd:module="C4">0.181</epd:amount>
<epd:amount epd:module="D">-0.798</epd:amount>
</common:other>
</LCIAResult>
<LCIAResult>
<referenceToLCIAMethodDataSet uri="../lciamethods/06dcd26f-025f-401a-a7c1-5e457eb54637.xml" type="LCIA method data set" refObjectId="06dcd26f-025f-401a-a7c1-5e457eb54637">
<common:shortDescription xml:lang="de">Abbau Potential der stratosphärischen Ozonschicht (ODP)</common:shortDescription>
<common:shortDescription xml:lang="en">Depletion potential of the stratospheric ozone layer (ODP)</common:shortDescription>
</referenceToLCIAMethodDataSet>
<common:other>
<epd:referenceToUnitGroupDataSet uri="../unitgroups/88054749-b0a6-47ea-a82b-dc5b29326512.xml" type="unit group data set" refObjectId="88054749-b0a6-47ea-a82b-dc5b29326512">
<common:shortDescription xml:lang="de">kg CFC11-Äq.</common:shortDescription>
</epd:referenceToUnitGroupDataSet>
<epd:amount epd:module="A1-A3">2.4127207E-11</epd:amount>
<epd:amount epd:module="A4">1.49E-17</epd:amount>
<epd:amount epd:module="A5">1.04E-15</epd:amount>
<epd:amount epd:module="C1">0</epd:amount>
<epd:amount epd:module="C2">7.43E-18</epd:amount>
<epd:amount epd:module="C4">9.94E-16</epd:amount>
<epd:amount epd:module="D">-1.02E-14</epd:amount>
</common:other>
</LCIAResult>
<LCIAResult>
<referenceToLCIAMethodDataSet uri="../lciamethods/b4274add-93b7-4905-a5e4-2e878c4e4216.xml" type="LCIA method data set" refObjectId="b4274add-93b7-4905-a5e4-2e878c4e4216">
<common:shortDescription xml:lang="de">Versauerungspotenzial von Boden und Wasser (AP)</common:shortDescription>
<common:shortDescription xml:lang="en">Acidification potential of land and water (AP)</common:shortDescription>
</referenceToLCIAMethodDataSet>
<common:other>
<epd:referenceToUnitGroupDataSet uri="../unitgroups/bc50c624-a9bc-45b1-a9b0-e6b10d00476f.xml" type="unit group data set" refObjectId="bc50c624-a9bc-45b1-a9b0-e6b10d00476f">
<common:shortDescription xml:lang="de">kg SO_(2)-Äq.</common:shortDescription>
</epd:referenceToUnitGroupDataSet>
<epd:amount epd:module="A1-A3">0.03094</epd:amount>
<epd:amount epd:module="A4">7.11E-05</epd:amount>
<epd:amount epd:module="A5">0.000201</epd:amount>
<epd:amount epd:module="C1">0</epd:amount>
<epd:amount epd:module="C2">3.55E-05</epd:amount>
<epd:amount epd:module="C4">0.00115</epd:amount>
<epd:amount epd:module="D">-0.00134</epd:amount>
</common:other>
</LCIAResult>
<LCIAResult>
<referenceToLCIAMethodDataSet uri="../lciamethods/f58827d0-b407-4ec6-be75-8b69efb98a0f.xml" type="LCIA method data set" refObjectId="f58827d0-b407-4ec6-be75-8b69efb98a0f">
<common:shortDescription xml:lang="de">Eutrophierungspotenzial (EP)</common:shortDescription>
<common:shortDescription xml:lang="en">Eutrophication potential (EP)</common:shortDescription>
</referenceToLCIAMethodDataSet>
<common:other>
<epd:referenceToUnitGroupDataSet uri="../unitgroups/67b5401d-873c-485f-bcf3-6ae83b918822.xml" type="unit group data set" refObjectId="67b5401d-873c-485f-bcf3-6ae83b918822">
<common:shortDescription xml:lang="de">kg PO_(4)^(3)-Äq.</common:shortDescription>
</epd:referenceToUnitGroupDataSet>
<epd:amount epd:module="A1-A3">0.004645</epd:amount>
<epd:amount epd:module="A4">1.31E-05</epd:amount>
<epd:amount epd:module="A5">3.9E-05</epd:amount>
<epd:amount epd:module="C1">0</epd:amount>
<epd:amount epd:module="C2">6.54E-06</epd:amount>
<epd:amount epd:module="C4">0.000129</epd:amount>
<epd:amount epd:module="D">-0.00014</epd:amount>
</common:other>
</LCIAResult>
<LCIAResult>
<referenceToLCIAMethodDataSet uri="../lciamethods/1e84a202-dae6-42aa-9e9d-71ea48b8be00.xml" type="LCIA method data set" refObjectId="1e84a202-dae6-42aa-9e9d-71ea48b8be00">
<common:shortDescription xml:lang="de">Bildungspotential für troposphärisches Ozon (POCP)</common:shortDescription>
<common:shortDescription xml:lang="en">Formation potential of tropospheric ozone photochemical oxidants (POCP)</common:shortDescription>
</referenceToLCIAMethodDataSet>
<common:other>
<epd:referenceToUnitGroupDataSet uri="../unitgroups/01c26c17-9a76-406e-8295-f17b55fd909e.xml" type="unit group data set" refObjectId="01c26c17-9a76-406e-8295-f17b55fd909e">
<common:shortDescription xml:lang="de">kg Ethen-Äq.</common:shortDescription>
</epd:referenceToUnitGroupDataSet>
<epd:amount epd:module="A1-A3">0.00282422</epd:amount>
<epd:amount epd:module="A4">-3.22E-07</epd:amount>
<epd:amount epd:module="A5">1.75E-05</epd:amount>
<epd:amount epd:module="C1">0</epd:amount>
<epd:amount epd:module="C2">-1.61E-07</epd:amount>
<epd:amount epd:module="C4">8.71E-05</epd:amount>
<epd:amount epd:module="D">-0.000111</epd:amount>
</common:other>
</LCIAResult>
<LCIAResult>
<referenceToLCIAMethodDataSet uri="../lciamethods/f7c73bb9-ab1a-4249-9c6d-379a0de6f67e.xml" type="LCIA method data set" refObjectId="f7c73bb9-ab1a-4249-9c6d-379a0de6f67e">
<common:shortDescription xml:lang="de">Potenzial für den abiotischen Abbau nicht fossiler Ressourcen (ADPE)</common:shortDescription>
<common:shortDescription xml:lang="en">Abiotic depletion potential for non fossil resources (ADPE)</common:shortDescription>
</referenceToLCIAMethodDataSet>
<common:other>
<epd:referenceToUnitGroupDataSet uri="../unitgroups/54ccd2d9-a32a-4fc2-923d-f2c8c93e89d4.xml" type="unit group data set" refObjectId="54ccd2d9-a32a-4fc2-923d-f2c8c93e89d4">
<common:shortDescription xml:lang="de">kg Sb-Äq.</common:shortDescription>
</epd:referenceToUnitGroupDataSet>
<epd:amount epd:module="A1-A3">5.48751E-05</epd:amount>
<epd:amount epd:module="A4">6.66E-09</epd:amount>
<epd:amount epd:module="A5">1.14E-08</epd:amount>
<epd:amount epd:module="C1">0</epd:amount>
<epd:amount epd:module="C2">3.33E-09</epd:amount>
<epd:amount epd:module="C4">1.82E-08</epd:amount>
<epd:amount epd:module="D">-3.36E-06</epd:amount>
</common:other>
</LCIAResult>
<LCIAResult>
<referenceToLCIAMethodDataSet uri="../lciamethods/804ebcdf-309d-4098-8ed8-fdaf2f389981.xml" type="LCIA method data set" refObjectId="804ebcdf-309d-4098-8ed8-fdaf2f389981">
<common:shortDescription xml:lang="de">Potenzial für den abiotischen Abbau fossiler Brennstoffe (ADPF)</common:shortDescription>
<common:shortDescription xml:lang="en">Abiotic depletion potential for fossil resources (ADPF)</common:shortDescription>
</referenceToLCIAMethodDataSet>
<common:other>
<epd:referenceToUnitGroupDataSet uri="../unitgroups/93a60a57-a3c8-11da-a746-0800200c9a66.xml" type="unit group data set" refObjectId="93a60a57-a3c8-11da-a746-0800200c9a66">
<common:shortDescription xml:lang="de">MJ</common:shortDescription>
</epd:referenceToUnitGroupDataSet>
<epd:amount epd:module="A1-A3">286.1</epd:amount>
<epd:amount epd:module="A4">1.23</epd:amount>
<epd:amount epd:module="A5">0.58</epd:amount>
<epd:amount epd:module="C1">0</epd:amount>
<epd:amount epd:module="C2">0.616</epd:amount>
<epd:amount epd:module="C4">2.56</epd:amount>
<epd:amount epd:module="D">-11.1</epd:amount>
</common:other>
</LCIAResult>
</LCIAResults>
</processDataSet>