<?xml version="1.0" encoding="utf-8"?>
<?xml-stylesheet version="1.0" href="../../stylesheets/epd2html.xsl" type="text/xsl"?>
<processDataSet xmlns="http://lca.jrc.it/ILCD/Process" xmlns:common="http://lca.jrc.it/ILCD/Common" xmlns:epd="http://www.iai.kit.edu/EPD/2013" xmlns:epd2="http://www.indata.network/EPD/2019" xmlns:xsi="http://www.w3.org/2001/XMLSchema-instance" xsi:schemaLocation="http://lca.jrc.it/ILCD/Process ../../schemas/EPD_DataSet.xsd" locations="../ILCDLocations.xml" epd2:epd-version="1.2" version="1.1">
  <processInformation>
    <dataSetInformation>
      <common:UUID>5331890a-9fd2-4388-bc6f-9776f9552848</common:UUID>
      <name>
        <baseName xml:lang="en">Electricity grid mix scenario 2050</baseName>
        <baseName xml:lang="de">Strom-Mix-Szenario 2050</baseName>
        <functionalUnitFlowProperties xml:lang="en">&lt;1kV</functionalUnitFlowProperties>
        <functionalUnitFlowProperties xml:lang="de">&lt;1kV</functionalUnitFlowProperties>
      </name>
      <classificationInformation>
        <common:classification name="oekobau.dat">
          <common:class level="0" classId="9">Sonstige</common:class>
          <common:class level="1" classId="9.2">Energieträger - Bereitstellung frei Verbraucher</common:class>
          <common:class level="2" classId="9.2.05">Strom</common:class>
        </common:classification>
      </classificationInformation>
      <common:generalComment xml:lang="en">This data set has been modeled according to the European Standard EN 15804+A2 for Sustainable Building. Results are depicted in modules that allow the structured expression of results over the entire life cycle.</common:generalComment>
      <common:generalComment xml:lang="de">Dieser Datensatz wurde nach dem European Standard EN 15804+A2 für Nachhaltiges Bauen modelliert. Ergebnisse werden in Modulen abgebildet, die den strukturierten Ausdruck von Ergebnissen über den gesamten Lebenszyklus zulassen.</common:generalComment>
      <common:other>
        <epd:safetyMargins>
          <epd:margins>0</epd:margins>
          <epd:description xml:lang="en"></epd:description>
          <epd:description xml:lang="de"></epd:description>
        </epd:safetyMargins>
      </common:other>
    </dataSetInformation>
    <quantitativeReference type="Reference flow(s)">
      <referenceToReferenceFlow>107885</referenceToReferenceFlow>
    </quantitativeReference>
    <time>
      <common:referenceYear>2021</common:referenceYear>
      <common:dataSetValidUntil>2022</common:dataSetValidUntil>
      <common:timeRepresentativenessDescription xml:lang="en">Annual average</common:timeRepresentativenessDescription>
      <common:timeRepresentativenessDescription xml:lang="de">Jährlicher Durchschnitt</common:timeRepresentativenessDescription>
    </time>
    <geography>
      <locationOfOperationSupplyOrProduction location="DE">
        <descriptionOfRestrictions xml:lang="en">The data set represents the country specific situation in Germany, focusing on the main technologies, the region specific characteristics and / or import statistics.</descriptionOfRestrictions>
        <descriptionOfRestrictions xml:lang="de">Der Datensatz bildet die länderspezifische Situation in Deutschland ab. Dabei werden Haupttechnologien, spezifische regionale Charakteristiken und ggf. Importstatistiken berücksichtigt.</descriptionOfRestrictions>
      </locationOfOperationSupplyOrProduction>
    </geography>
    <technology>
      <technologyDescriptionAndIncludedProcesses xml:lang="en">Foreground system:
The national or regional specific electricity consumption mix is provided by the conversion of the different energy carriers to electricity and imports from neighbouring countries, as illustrated in the pie chart "Electricity Mix".
The electricity is either produced in energy carrier specific power plants and/or combined heat and power plants (CHP). Also considered are the national and regional specific technology standards of the power plants in regard to efficiency, firing technology, flue-gas desulphurisation, NOx removal and de-dusting. The electricity provided by non-combustible renewable energy sources also considers the national or regional situation, such as solar radiation (photovoltaic), annual full load hours (wind power), and share of hydro power stations by type (run-of-river, storage and pumped storage).
The fossil power plant models combine emission data from literature with calculated values for non-measured emissions e.g. organics or heavy metals. For the emissions CO2, SO2, NOx, CO, CH4, N2O, NMVOC and particulate matter (PM) measured/calculated data are used, taken from national inventory reports, emission inventory data bases, utility companies and other sources. The calculation of other emissions within the models are based on energy carrier properties, transfer coefficients and power plant thermodynamics representing the applied flue gas treatment technologies and standards (flue gas desulphurisation, dust filter etc.). Combustion residues from solid fuels, such as gypsum, bottom ash or fly ash are assumed  to be reused e.g. in construction work. Waste treatment for these substances is therefore not considered. Radioactive emissions from ashes are not considered in the coal power plant model.
The energy carrier supply considers the whole supply chain of the energy carrier from exploration, production, processing and transport of the fuels to the power plants. The supply chain is modelled in specific national / regional energy carrier consumption mixes (i.e. domestic production and imports), and considers national / regional average energy carrier properties (e.g. elemental composition and energy content).
The electricity grid mix includes imported electricity from neighbouring countries, transmission / distribution losses of low voltage electricity supply and the own use of electricity by energy producers (own consumption of power plants, and "other" own consumption e.g. due to pumped storage hydro power etc.). The logic of modelling the electricity consumption mix is represented in the flow diagram "Modelling of Electricity Consumption Mixes".
Background system:
Electricity: Electricity is modelled according to the individual country-specific situations. The country-specific modelling is achieved on multiple levels. Firstly, individual energy carrier specific power plants and plants for renewable energy sources are modelled according to the current national electricity grid mix. Modelling the electricity consumption mix includes transmission / distribution losses and the own use by energy producers (own consumption of power plants and "other" own consumption e.g. due to pumped storage hydro power etc.), as well as imported electricity. Secondly, the national emission and efficiency standards of the power plants are modelled as well as the share of electricity plants and combined heat and power plants (CHP). Thirdly, the country-specific energy carrier supply (share of imports and / or domestic supply) including the country-specific energy carrier properties (e.g. element and energy content) are accounted for. Fourthly, the exploration, mining/production, processing and transport processes of the energy carrier supply chains are modelled according to the specific situation of each electricity producing country. The different production and processing techniques (emissions and efficiencies) in the different energy producing countries are considered, e.g. different crude oil production technologies or different flaring rates at the oil platforms.
Thermal energy, process steam: The thermal energy and process steam supply is modelled according to the individual country-specific situation with regard to emission standards and considered energy carriers. The thermal energy and process steam are produced at heat plants. Efficiencies for thermal energy production are by definition 100% in relation to the corresponding energy carrier input. For process steam the efficiency ranges from 85%, 90% to 95%. The energy carriers used for the generation of thermal energy and process steam are modelled according to the specific import situation (see electricity above).
Transports: All relevant and known transport processes are included. Ocean-going and inland ship transport as well as rail, truck and pipeline transport of bulk commodities are considered.
Energy carriers: The energy carriers are modelled according to the specific supply situation (see electricity above).
Refinery products: Diesel fuel, gasoline, technical gases, fuel oils, lubricants and residues such as bitumen are modelled with a parameterised country-specific refinery model. The refinery model represents the current national standard in refining techniques (e.g. emission level, internal energy consumption, etc.) as well as the individual country-specific product output spectrum, which can be quite different from country to country. The supply of crude oil is modelled, again, according to the country-specific situation with the respective properties of the resources.</technologyDescriptionAndIncludedProcesses>
      <technologyDescriptionAndIncludedProcesses xml:lang="de">Foreground system:
The national or regional specific electricity consumption mix is provided by the conversion of the different energy carriers to electricity and imports from neighbouring countries, as illustrated in the pie chart "Electricity Mix".
The electricity is either produced in energy carrier specific power plants and/or combined heat and power plants (CHP). Also considered are the national and regional specific technology standards of the power plants in regard to efficiency, firing technology, flue-gas desulphurisation, NOx removal and de-dusting. The electricity provided by non-combustible renewable energy sources also considers the national or regional situation, such as solar radiation (photovoltaic), annual full load hours (wind power), and share of hydro power stations by type (run-of-river, storage and pumped storage).
The fossil power plant models combine emission data from literature with calculated values for non-measured emissions e.g. organics or heavy metals. For the emissions CO2, SO2, NOx, CO, CH4, N2O, NMVOC and particulate matter (PM) measured/calculated data are used, taken from national inventory reports, emission inventory data bases, utility companies and other sources. The calculation of other emissions within the models are based on energy carrier properties, transfer coefficients and power plant thermodynamics representing the applied flue gas treatment technologies and standards (flue gas desulphurisation, dust filter etc.). Combustion residues from solid fuels, such as gypsum, bottom ash or fly ash are assumed  to be reused e.g. in construction work. Waste treatment for these substances is therefore not considered. Radioactive emissions from ashes are not considered in the coal power plant model.
The energy carrier supply considers the whole supply chain of the energy carrier from exploration, production, processing and transport of the fuels to the power plants. The supply chain is modelled in specific national / regional energy carrier consumption mixes (i.e. domestic production and imports), and considers national / regional average energy carrier properties (e.g. elemental composition and energy content).
The electricity grid mix includes imported electricity from neighbouring countries, transmission / distribution losses of low voltage electricity supply and the own use of electricity by energy producers (own consumption of power plants, and "other" own consumption e.g. due to pumped storage hydro power etc.). The logic of modelling the electricity consumption mix is represented in the flow diagram "Modelling of Electricity Consumption Mixes".
Background system:
Electricity: Electricity is modelled according to the individual country-specific situations. The country-specific modelling is achieved on multiple levels. Firstly, individual energy carrier specific power plants and plants for renewable energy sources are modelled according to the current national electricity grid mix. Modelling the electricity consumption mix includes transmission / distribution losses and the own use by energy producers (own consumption of power plants and "other" own consumption e.g. due to pumped storage hydro power etc.), as well as imported electricity. Secondly, the national emission and efficiency standards of the power plants are modelled as well as the share of electricity plants and combined heat and power plants (CHP). Thirdly, the country-specific energy carrier supply (share of imports and / or domestic supply) including the country-specific energy carrier properties (e.g. element and energy content) are accounted for. Fourthly, the exploration, mining/production, processing and transport processes of the energy carrier supply chains are modelled according to the specific situation of each electricity producing country. The different production and processing techniques (emissions and efficiencies) in the different energy producing countries are considered, e.g. different crude oil production technologies or different flaring rates at the oil platforms.
Thermal energy, process steam: The thermal energy and process steam supply is modelled according to the individual country-specific situation with regard to emission standards and considered energy carriers. The thermal energy and process steam are produced at heat plants. Efficiencies for thermal energy production are by definition 100% in relation to the corresponding energy carrier input. For process steam the efficiency ranges from 85%, 90% to 95%. The energy carriers used for the generation of thermal energy and process steam are modelled according to the specific import situation (see electricity above).
Transports: All relevant and known transport processes are included. Ocean-going and inland ship transport as well as rail, truck and pipeline transport of bulk commodities are considered.
Energy carriers: The energy carriers are modelled according to the specific supply situation (see electricity above).
Refinery products: Diesel fuel, gasoline, technical gases, fuel oils, lubricants and residues such as bitumen are modelled with a parameterised country-specific refinery model. The refinery model represents the current national standard in refining techniques (e.g. emission level, internal energy consumption, etc.) as well as the individual country-specific product output spectrum, which can be quite different from country to country. The supply of crude oil is modelled, again, according to the country-specific situation with the respective properties of the resources.</technologyDescriptionAndIncludedProcesses>
      <technologicalApplicability xml:lang="en">Supply of 1 kWh low voltage (&lt;1kV) electricity to final consumers.</technologicalApplicability>
      <technologicalApplicability xml:lang="de">Supply of 1 kWh low voltage (&lt;1kV) electricity to final consumers.</technologicalApplicability>
      <referenceToTechnologyPictogramme refObjectId="36980b3c-2db5-48d7-83ee-5a5bdfecae99" version="21.01.000" type="source data set" uri="../sources/36980b3c-2db5-48d7-83ee-5a5bdfecae99.xml">
        <common:shortDescription xml:lang="en">energy_electricity_modelling_of_electricity_consumption_mixes.jpg</common:shortDescription>
      </referenceToTechnologyPictogramme>
      <referenceToTechnologyFlowDiagrammOrPicture refObjectId="6c1888e9-d92f-494d-a887-99104a2ea1f2" version="21.01.000" type="source data set" uri="../sources/6c1888e9-d92f-494d-a887-99104a2ea1f2.xml">
        <common:shortDescription xml:lang="en">energy_projection electricity mix de (eu energy trends 2013).jpg</common:shortDescription>
      </referenceToTechnologyFlowDiagrammOrPicture>
    </technology>
  </processInformation>
  <modellingAndValidation>
    <LCIMethodAndAllocation>
      <typeOfDataSet>EPD</typeOfDataSet>
      <common:other>
        <epd:subType>generic dataset</epd:subType>
      </common:other>
    </LCIMethodAndAllocation>
    <dataSourcesTreatmentAndRepresentativeness>
      <referenceToDataSource refObjectId="6de1e618-4960-4b0e-aa2c-7f561a1b6f03" version="21.01.000" type="source data set" uri="../sources/6de1e618-4960-4b0e-aa2c-7f561a1b6f03.xml">
        <common:shortDescription xml:lang="en">K.Weissermel, H.- J. Arpe: Industrial organic chemistry</common:shortDescription>
      </referenceToDataSource>
      <referenceToDataSource refObjectId="2b041bb8-adea-4fab-9e28-8abfe409033a" version="21.01.000" type="source data set" uri="../sources/2b041bb8-adea-4fab-9e28-8abfe409033a.xml">
        <common:shortDescription xml:lang="en">Copper development association: Overview of Recycled Copper</common:shortDescription>
      </referenceToDataSource>
      <referenceToDataSource refObjectId="b2012fa6-b2f7-4151-b781-aadfaacf4136" version="21.01.000" type="source data set" uri="../sources/b2012fa6-b2f7-4151-b781-aadfaacf4136.xml">
        <common:shortDescription xml:lang="en">Smelter Tech: The Reverberatory Furnace </common:shortDescription>
      </referenceToDataSource>
      <referenceToDataSource refObjectId="9b8971e3-b693-49f0-a0ef-2353e4cfb60b" version="21.01.000" type="source data set" uri="../sources/9b8971e3-b693-49f0-a0ef-2353e4cfb60b.xml">
        <common:shortDescription xml:lang="en">Process for the production of a plasticized polyvinyl butyral for gluing a base onto a glazing</common:shortDescription>
      </referenceToDataSource>
      <referenceToDataSource refObjectId="2ea4220d-0ba7-4351-b99b-545de2232365" version="21.01.000" type="source data set" uri="../sources/2ea4220d-0ba7-4351-b99b-545de2232365.xml">
        <common:shortDescription xml:lang="en">LookChem: Manufacture of 1.12-Dodecanedioic Acid</common:shortDescription>
      </referenceToDataSource>
      <referenceToDataSource refObjectId="4a1fd634-a5ff-4bd1-a08e-95750cda3a35" version="21.01.000" type="source data set" uri="../sources/4a1fd634-a5ff-4bd1-a08e-95750cda3a35.xml">
        <common:shortDescription xml:lang="en">Methods of making cyclododecatriene and</common:shortDescription>
      </referenceToDataSource>
      <referenceToDataSource refObjectId="56c9aae6-4e0b-4b66-b898-d59cc485198b" version="21.01.000" type="source data set" uri="../sources/56c9aae6-4e0b-4b66-b898-d59cc485198b.xml">
        <common:shortDescription xml:lang="en">EPA - Health and Environmental Effects Profile for 2-Chloro-1,3-Butadiene, 1984</common:shortDescription>
      </referenceToDataSource>
      <referenceToDataSource refObjectId="7e35dd34-81c9-488b-9a69-2b525bfe2999" version="21.01.000" type="source data set" uri="../sources/7e35dd34-81c9-488b-9a69-2b525bfe2999.xml">
        <common:shortDescription xml:lang="en">Chlorpropanes, Chlorobutanes, and Chlorobutenes: Chapter in Ullmann's, 2011</common:shortDescription>
      </referenceToDataSource>
      <referenceToDataSource refObjectId="d54f049a-2ece-4140-ac8d-caa694d1d1e9" version="21.01.000" type="source data set" uri="../sources/d54f049a-2ece-4140-ac8d-caa694d1d1e9.xml">
        <common:shortDescription xml:lang="en">Chloroprene  - Données technico-économiques sur les substances chimiques en France - 2006</common:shortDescription>
      </referenceToDataSource>
      <referenceToDataSource refObjectId="47b981ff-8e4a-4973-8aab-d88611ff3a06" version="21.01.000" type="source data set" uri="../sources/47b981ff-8e4a-4973-8aab-d88611ff3a06.xml">
        <common:shortDescription xml:lang="en">Renewables Information 2011</common:shortDescription>
      </referenceToDataSource>
      <referenceToDataSource refObjectId="3ebd4e78-289a-4b3a-ba90-1071b2ea1a3e" version="21.01.000" type="source data set" uri="../sources/3ebd4e78-289a-4b3a-ba90-1071b2ea1a3e.xml">
        <common:shortDescription xml:lang="en">eGrid2012 Version 1.0</common:shortDescription>
      </referenceToDataSource>
      <referenceToDataSource refObjectId="acb3a6c1-d206-46ed-8b68-1067eb388a90" version="21.01.000" type="source data set" uri="../sources/acb3a6c1-d206-46ed-8b68-1067eb388a90.xml">
        <common:shortDescription xml:lang="en">Update of the Environmental Indicators and Energy Payback Time of CIS Modules in Europe, 2010</common:shortDescription>
      </referenceToDataSource>
      <referenceToDataSource refObjectId="e831a684-0b46-4c3a-b754-009dd58883ae" version="21.01.000" type="source data set" uri="../sources/e831a684-0b46-4c3a-b754-009dd58883ae.xml">
        <common:shortDescription xml:lang="en">Sustainability Evaluation of Solar Energy Systems: LCA Analysis (LCA of Thin Film Technologies)</common:shortDescription>
      </referenceToDataSource>
      <referenceToDataSource refObjectId="58b86392-5559-43b1-9d76-7e7a33134051" version="21.01.000" type="source data set" uri="../sources/58b86392-5559-43b1-9d76-7e7a33134051.xml">
        <common:shortDescription xml:lang="en">Life Cycle Inventories and Life Cycle Assessments of Photovoltaic Systems, 2011</common:shortDescription>
      </referenceToDataSource>
      <referenceToDataSource refObjectId="6b29835e-9afe-410d-a650-c8eb7cedf7a3" version="21.01.000" type="source data set" uri="../sources/6b29835e-9afe-410d-a650-c8eb7cedf7a3.xml">
        <common:shortDescription xml:lang="en">Environmental Life Cycle Inventory of Crystalline Silicon Photovoltaic System Production, 2006</common:shortDescription>
      </referenceToDataSource>
      <referenceToDataSource refObjectId="41603ac1-427a-4b74-a6d2-07124c811a06" version="21.01.000" type="source data set" uri="../sources/41603ac1-427a-4b74-a6d2-07124c811a06.xml">
        <common:shortDescription xml:lang="en">Update of environmental indicators and energy payback time of CdTe PV systems in Europe, 2011</common:shortDescription>
      </referenceToDataSource>
      <referenceToDataSource refObjectId="db43ce49-69ff-436b-b2ba-0d711ee292d2" version="21.01.000" type="source data set" uri="../sources/db43ce49-69ff-436b-b2ba-0d711ee292d2.xml">
        <common:shortDescription xml:lang="en">Energy payback, life cycle CO2 emissions of the BOS in optimized 3.5 MW PV installation</common:shortDescription>
      </referenceToDataSource>
      <referenceToDataSource refObjectId="83c23f89-16d9-4687-9fb5-b46e5632c594" version="21.01.000" type="source data set" uri="../sources/83c23f89-16d9-4687-9fb5-b46e5632c594.xml">
        <common:shortDescription xml:lang="en">Methodology Guidelines on Life Cycle Assessment of Photovoltaic Electricity, 2009</common:shortDescription>
      </referenceToDataSource>
      <referenceToDataSource refObjectId="d19e0017-9ce6-41f6-80d8-1ddcba714d92" version="21.01.000" type="source data set" uri="../sources/d19e0017-9ce6-41f6-80d8-1ddcba714d92.xml">
        <common:shortDescription xml:lang="en">Annual European Union greenhouse gas inventory 1990 - 2008 and inventory report 2010</common:shortDescription>
      </referenceToDataSource>
      <referenceToDataSource refObjectId="4d0b4cd8-ef1e-4b9f-9cc0-a15164f1f1c6" version="21.01.000" type="source data set" uri="../sources/4d0b4cd8-ef1e-4b9f-9cc0-a15164f1f1c6.xml">
        <common:shortDescription xml:lang="en">Air pollutant emissions in Finland 1990-2008 Informative Inventory report</common:shortDescription>
      </referenceToDataSource>
      <referenceToDataSource refObjectId="63ab79ca-79b8-480a-93ff-23b6e10f3301" version="21.01.000" type="source data set" uri="../sources/63ab79ca-79b8-480a-93ff-23b6e10f3301.xml">
        <common:shortDescription xml:lang="en">Air pollutant emissions from stationary installations using bioenergy in the NLs BOLK Phase 2</common:shortDescription>
      </referenceToDataSource>
      <referenceToDataSource refObjectId="4d9277ae-6882-4704-9da8-d864fe7035a6" version="21.01.000" type="source data set" uri="../sources/4d9277ae-6882-4704-9da8-d864fe7035a6.xml">
        <common:shortDescription xml:lang="en">2da Comunicacion Nacional de la Republica Argentina</common:shortDescription>
      </referenceToDataSource>
      <referenceToDataSource refObjectId="676b2a43-4d64-47d3-939d-17361afd74df" version="21.01.000" type="source data set" uri="../sources/676b2a43-4d64-47d3-939d-17361afd74df.xml">
        <common:shortDescription xml:lang="en">2006 IPCC Guidelines for National Greenhouse Gas Inventories</common:shortDescription>
      </referenceToDataSource>
      <referenceToDataSource refObjectId="d2743393-5fbd-11db-b0de-0800200c9a66" version="21.01.000" type="source data set" uri="../sources/d2743393-5fbd-11db-b0de-0800200c9a66.xml">
        <common:shortDescription xml:lang="en">13. Verordnung zur Durchführung des Bundes-Immissionsschutzgesetzes</common:shortDescription>
      </referenceToDataSource>
      <referenceToDataSource refObjectId="fdf1a71b-fde9-4939-b14e-164ff0f4d094" version="21.01.000" type="source data set" uri="../sources/fdf1a71b-fde9-4939-b14e-164ff0f4d094.xml">
        <common:shortDescription xml:lang="en">Auswertung PV-Leistung</common:shortDescription>
      </referenceToDataSource>
      <referenceToDataSource refObjectId="c175a776-a82f-4739-a0cf-1ac02966df7a" version="21.01.000" type="source data set" uri="../sources/c175a776-a82f-4739-a0cf-1ac02966df7a.xml">
        <common:shortDescription xml:lang="en">Austria's National Inventory Report 2010</common:shortDescription>
      </referenceToDataSource>
      <referenceToDataSource refObjectId="1f692183-8c45-4d9a-87d0-2cb0cdadaf9c" version="21.01.000" type="source data set" uri="../sources/1f692183-8c45-4d9a-87d0-2cb0cdadaf9c.xml">
        <common:shortDescription xml:lang="en">Austria's Informative Inventory Report (IIR) 2010</common:shortDescription>
      </referenceToDataSource>
      <referenceToDataSource refObjectId="6b02aa13-02c4-4f89-b418-51c46249cd74" version="21.01.000" type="source data set" uri="../sources/6b02aa13-02c4-4f89-b418-51c46249cd74.xml">
        <common:shortDescription xml:lang="en">Australian National Greenhouse Accounts (NIR)</common:shortDescription>
      </referenceToDataSource>
      <referenceToDataSource refObjectId="13f3c0d9-2cd1-40d6-a887-8132d168ce49" version="21.01.000" type="source data set" uri="../sources/13f3c0d9-2cd1-40d6-a887-8132d168ce49.xml">
        <common:shortDescription xml:lang="en">Australian electricity generation report 2008</common:shortDescription>
      </referenceToDataSource>
      <referenceToDataSource refObjectId="af10f2b3-4618-47f0-bae4-57e2ba035a5b" version="21.01.000" type="source data set" uri="../sources/af10f2b3-4618-47f0-bae4-57e2ba035a5b.xml">
        <common:shortDescription xml:lang="en">Appendix H: Calorific Value, Price, and Emission Coefficients of Energy Kinds</common:shortDescription>
      </referenceToDataSource>
      <referenceToDataSource refObjectId="b61ddd50-66c1-4b57-a62b-1b3eff1d5c88" version="21.01.000" type="source data set" uri="../sources/b61ddd50-66c1-4b57-a62b-1b3eff1d5c88.xml">
        <common:shortDescription xml:lang="en">Appendix 17 Thermal values and Emission factors energy.xls GWP conversion factors 2006</common:shortDescription>
      </referenceToDataSource>
      <referenceToDataSource refObjectId="074971c8-93ee-41ec-b368-d04410a29499" version="21.01.000" type="source data set" uri="../sources/074971c8-93ee-41ec-b368-d04410a29499.xml">
        <common:shortDescription xml:lang="en">Anthropogenic Emissions from Energy Activities in India</common:shortDescription>
      </referenceToDataSource>
      <referenceToDataSource refObjectId="45ebaf6b-1827-40ab-afc8-5cdf4adbe55f" version="21.01.000" type="source data set" uri="../sources/45ebaf6b-1827-40ab-afc8-5cdf4adbe55f.xml">
        <common:shortDescription xml:lang="en">Emission Estimation Technique Manual for Fossil Fuel Electric Power Generation Version 2.3</common:shortDescription>
      </referenceToDataSource>
      <referenceToDataSource refObjectId="c400ff58-c292-41cf-9b9b-2ae4efe728be" version="21.01.000" type="source data set" uri="../sources/c400ff58-c292-41cf-9b9b-2ae4efe728be.xml">
        <common:shortDescription xml:lang="en">Emisiones atmosféricas de las centrales eléctricas en América del Norte</common:shortDescription>
      </referenceToDataSource>
      <referenceToDataSource refObjectId="9049ae1c-8dc6-4452-bdda-9a0fd0dabef6" version="21.01.000" type="source data set" uri="../sources/9049ae1c-8dc6-4452-bdda-9a0fd0dabef6.xml">
        <common:shortDescription xml:lang="en">EMEP/EEA air pollutant emission inventory guidebook - 2009</common:shortDescription>
      </referenceToDataSource>
      <referenceToDataSource refObjectId="ed37667c-d18a-4745-bdc3-2d1907a758c5" version="21.01.000" type="source data set" uri="../sources/ed37667c-d18a-4745-bdc3-2d1907a758c5.xml">
        <common:shortDescription xml:lang="en">EMEP/CORINAIR  Emission Inventory Guidebook - 2006</common:shortDescription>
      </referenceToDataSource>
      <referenceToDataSource refObjectId="09f34c8b-3240-4a63-ab33-1aca513c5b0a" version="21.01.000" type="source data set" uri="../sources/09f34c8b-3240-4a63-ab33-1aca513c5b0a.xml">
        <common:shortDescription xml:lang="en">Electricity Gas Australia</common:shortDescription>
      </referenceToDataSource>
      <referenceToDataSource refObjectId="8b23bb67-fbe3-48e4-9191-bdb52c8fbb28" version="21.01.000" type="source data set" uri="../sources/8b23bb67-fbe3-48e4-9191-bdb52c8fbb28.xml">
        <common:shortDescription xml:lang="en">Electric Power Industry 2009: Year in Review</common:shortDescription>
      </referenceToDataSource>
      <referenceToDataSource refObjectId="f3323ac4-38f6-4bff-95b9-0cc97275e91e" version="21.01.000" type="source data set" uri="../sources/f3323ac4-38f6-4bff-95b9-0cc97275e91e.xml">
        <common:shortDescription xml:lang="en">Directive 2009/28/EC of the European Parliament and of the Council of 23 April 2009</common:shortDescription>
      </referenceToDataSource>
      <referenceToDataSource refObjectId="c524c263-6f87-41a1-9998-10806f915e4f" version="21.01.000" type="source data set" uri="../sources/c524c263-6f87-41a1-9998-10806f915e4f.xml">
        <common:shortDescription xml:lang="en">Digest of United Kingdom Energy Statistics 2010</common:shortDescription>
      </referenceToDataSource>
      <referenceToDataSource refObjectId="95fbb395-92f4-4993-b88d-5a4cd3ff5471" version="21.01.000" type="source data set" uri="../sources/95fbb395-92f4-4993-b88d-5a4cd3ff5471.xml">
        <common:shortDescription xml:lang="en">Denmark's National Inventory report 2010</common:shortDescription>
      </referenceToDataSource>
      <referenceToDataSource refObjectId="3b917ad4-fb71-43b1-be0b-806537efbfeb" version="21.01.000" type="source data set" uri="../sources/3b917ad4-fb71-43b1-be0b-806537efbfeb.xml">
        <common:shortDescription xml:lang="en">Danish Emission inventories for stationary combustion plants</common:shortDescription>
      </referenceToDataSource>
      <referenceToDataSource refObjectId="02564626-8de7-43b0-b671-8dfa43044be8" version="21.01.000" type="source data set" uri="../sources/02564626-8de7-43b0-b671-8dfa43044be8.xml">
        <common:shortDescription xml:lang="en">Compilation of Air Pollutant Emission Factors</common:shortDescription>
      </referenceToDataSource>
      <referenceToDataSource refObjectId="5f5d9711-aa38-4ca5-9c43-0b6737d7c48b" version="21.01.000" type="source data set" uri="../sources/5f5d9711-aa38-4ca5-9c43-0b6737d7c48b.xml">
        <common:shortDescription xml:lang="en">Climate change - Immision Inventory</common:shortDescription>
      </referenceToDataSource>
      <referenceToDataSource refObjectId="d7d8f94e-c30b-47f4-aadb-b64a0134cc33" version="21.01.000" type="source data set" uri="../sources/d7d8f94e-c30b-47f4-aadb-b64a0134cc33.xml">
        <common:shortDescription xml:lang="en">BVT - Festlegung in ausgewählten industriellen Bereichen als Beitrag zur Erfüllung der Klimasch...</common:shortDescription>
      </referenceToDataSource>
      <referenceToDataSource refObjectId="a719ff4c-3b16-4090-b9bc-aac600d7a690" version="21.01.000" type="source data set" uri="../sources/a719ff4c-3b16-4090-b9bc-aac600d7a690.xml">
        <common:shortDescription xml:lang="en">Brennstoffe und Verbrennungsrechnung, 2. Auflage</common:shortDescription>
      </referenceToDataSource>
      <referenceToDataSource refObjectId="cf5a4784-0372-43d0-a814-a2b52132ff11" version="21.01.000" type="source data set" uri="../sources/cf5a4784-0372-43d0-a814-a2b52132ff11.xml">
        <common:shortDescription xml:lang="en">Brennstoffe und Verbrennungsrechnung</common:shortDescription>
      </referenceToDataSource>
      <referenceToDataSource refObjectId="14a1e369-d2e8-4054-a4c9-c20f14be6195" version="21.01.000" type="source data set" uri="../sources/14a1e369-d2e8-4054-a4c9-c20f14be6195.xml">
        <common:shortDescription xml:lang="en">Belgium's Greenhouse Gas Inventory (1990-2008)</common:shortDescription>
      </referenceToDataSource>
      <referenceToDataSource refObjectId="a5806d02-3a7d-4ebc-9edb-d82d4a254625" version="21.01.000" type="source data set" uri="../sources/a5806d02-3a7d-4ebc-9edb-d82d4a254625.xml">
        <common:shortDescription xml:lang="en">Greenhouse Gas Emissions in the Netherlands 1990-2008</common:shortDescription>
      </referenceToDataSource>
      <referenceToDataSource refObjectId="952089a6-fdba-406f-ac7f-c0c3b2286a65" version="21.01.000" type="source data set" uri="../sources/952089a6-fdba-406f-ac7f-c0c3b2286a65.xml">
        <common:shortDescription xml:lang="en">Greenhouse Gas Emissions in Finland 1990-2008</common:shortDescription>
      </referenceToDataSource>
      <referenceToDataSource refObjectId="d83bb703-1ab5-4306-b324-c6b61e0951a7" version="21.01.000" type="source data set" uri="../sources/d83bb703-1ab5-4306-b324-c6b61e0951a7.xml">
        <common:shortDescription xml:lang="en">Greenhouse Gas Emissions in Estonia 1990-2008</common:shortDescription>
      </referenceToDataSource>
      <referenceToDataSource refObjectId="a2bb6096-1c77-46a8-8fe5-59b1b3590c83" version="21.01.000" type="source data set" uri="../sources/a2bb6096-1c77-46a8-8fe5-59b1b3590c83.xml">
        <common:shortDescription xml:lang="en">Greenhouse Gas Emission in Estonia</common:shortDescription>
      </referenceToDataSource>
      <referenceToDataSource refObjectId="cd6f1cfc-f0f8-4270-aa6d-69bdec0e8a7d" version="21.01.000" type="source data set" uri="../sources/cd6f1cfc-f0f8-4270-aa6d-69bdec0e8a7d.xml">
        <common:shortDescription xml:lang="en">GHG Inventories 2008 - Common Reporting Format (CRF)</common:shortDescription>
      </referenceToDataSource>
      <referenceToDataSource refObjectId="4cf7f11b-29ea-482a-acc2-9014aef4e870" version="21.01.000" type="source data set" uri="../sources/4cf7f11b-29ea-482a-acc2-9014aef4e870.xml">
        <common:shortDescription xml:lang="en">Full fuel cycle greenhouse gas emission analysis for proposed Kwinana CCGT power station</common:shortDescription>
      </referenceToDataSource>
      <referenceToDataSource refObjectId="580c3724-d564-4c28-bacd-297a8a10ef60" version="21.01.000" type="source data set" uri="../sources/580c3724-d564-4c28-bacd-297a8a10ef60.xml">
        <common:shortDescription xml:lang="en">Ermittlung und Evaluierung von Emissionsfaktoren für Feuerungsanlagen in Deutschland</common:shortDescription>
      </referenceToDataSource>
      <referenceToDataSource refObjectId="8f9004d8-69bc-4bfb-ae2c-ec49304abc8d" version="21.01.000" type="source data set" uri="../sources/8f9004d8-69bc-4bfb-ae2c-ec49304abc8d.xml">
        <common:shortDescription xml:lang="en">Erarbeitung der Grundlagen für das BVT - Merkblatt Großfeuerungsanlagen</common:shortDescription>
      </referenceToDataSource>
      <referenceToDataSource refObjectId="010e303b-7e52-4a01-b176-4ac26f4b7eac" version="21.01.000" type="source data set" uri="../sources/010e303b-7e52-4a01-b176-4ac26f4b7eac.xml">
        <common:shortDescription xml:lang="en">Environmental Report 2008</common:shortDescription>
      </referenceToDataSource>
      <referenceToDataSource refObjectId="debe5c14-a3c5-4ae1-8f00-ac91dbdcc12d" version="21.01.000" type="source data set" uri="../sources/debe5c14-a3c5-4ae1-8f00-ac91dbdcc12d.xml">
        <common:shortDescription xml:lang="en">Energy Statistics  Imports Electricity</common:shortDescription>
      </referenceToDataSource>
      <referenceToDataSource refObjectId="39c74932-1b36-41ed-9ed7-2e8fc678b95a" version="21.01.000" type="source data set" uri="../sources/39c74932-1b36-41ed-9ed7-2e8fc678b95a.xml">
        <common:shortDescription xml:lang="en">Energy Futures and Urban Air Pollution: Challenges for China and the United States</common:shortDescription>
      </referenceToDataSource>
      <referenceToDataSource refObjectId="6961baea-190f-4bc4-9aed-c7231f20f128" version="21.01.000" type="source data set" uri="../sources/6961baea-190f-4bc4-9aed-c7231f20f128.xml">
        <common:shortDescription xml:lang="en">Energy Consumption, Energy Savings and Emission Analysis for Industrial Motors</common:shortDescription>
      </referenceToDataSource>
      <referenceToDataSource refObjectId="1a433db5-054d-4795-adc2-1618b790eca2" version="21.01.000" type="source data set" uri="../sources/1a433db5-054d-4795-adc2-1618b790eca2.xml">
        <common:shortDescription xml:lang="en">Emissoes dos Gases Geradores do Efeito Estufa por Termelctricas no Periodo 2000 a 2020</common:shortDescription>
      </referenceToDataSource>
      <referenceToDataSource refObjectId="78626e1d-4507-4562-8c0d-18d84f8bcfe4" version="21.01.000" type="source data set" uri="../sources/78626e1d-4507-4562-8c0d-18d84f8bcfe4.xml">
        <common:shortDescription xml:lang="en">Emissionsschätzungen für SO2, NO2, NMVOC und NH3 in Deutschland 2000-2020</common:shortDescription>
      </referenceToDataSource>
      <referenceToDataSource refObjectId="a648a855-48d6-4dfa-a65f-7ef376c077b0" version="21.01.000" type="source data set" uri="../sources/a648a855-48d6-4dfa-a65f-7ef376c077b0.xml">
        <common:shortDescription xml:lang="en">Emissionsfaktoren und Kohlenstoffgehalte</common:shortDescription>
      </referenceToDataSource>
      <referenceToDataSource refObjectId="4300d477-7d2e-46ed-bcc4-226e1877565c" version="21.01.000" type="source data set" uri="../sources/4300d477-7d2e-46ed-bcc4-226e1877565c.xml">
        <common:shortDescription xml:lang="en">Emissions of greenhouse gases in Iceland from 1990 to 2008</common:shortDescription>
      </referenceToDataSource>
      <referenceToDataSource refObjectId="37800c0d-0dbc-436e-99eb-d3790e3c8d1c" version="21.01.000" type="source data set" uri="../sources/37800c0d-0dbc-436e-99eb-d3790e3c8d1c.xml">
        <common:shortDescription xml:lang="en">Evaluation Criteria Investment Proposals (translated from hellenic)</common:shortDescription>
      </referenceToDataSource>
      <referenceToDataSource refObjectId="308acd86-30a4-42c9-b68c-6ed6a2931877" version="21.01.000" type="source data set" uri="../sources/308acd86-30a4-42c9-b68c-6ed6a2931877.xml">
        <common:shortDescription xml:lang="en">Greenhouse Gas Emissions Inventory Reports of Spain 1990-2008</common:shortDescription>
      </referenceToDataSource>
      <referenceToDataSource refObjectId="4560b4c3-bf00-470f-b5ed-140cc4d5a3e7" version="21.01.000" type="source data set" uri="../sources/4560b4c3-bf00-470f-b5ed-140cc4d5a3e7.xml">
        <common:shortDescription xml:lang="en">Life Cycle Inventory for Electricity Generation in China</common:shortDescription>
      </referenceToDataSource>
      <referenceToDataSource refObjectId="d1047ccd-64b4-4f5e-b403-1887547c55d2" version="21.01.000" type="source data set" uri="../sources/d1047ccd-64b4-4f5e-b403-1887547c55d2.xml">
        <common:shortDescription xml:lang="en">Liechtenstein`s Greenhouse Gas Inventory Report 1990 -2008</common:shortDescription>
      </referenceToDataSource>
      <referenceToDataSource refObjectId="2ce438a9-0284-4c06-aaab-9cd27962125d" version="21.01.000" type="source data set" uri="../sources/2ce438a9-0284-4c06-aaab-9cd27962125d.xml">
        <common:shortDescription xml:lang="en">Latvia's Informative Inventory 1990- 2008</common:shortDescription>
      </referenceToDataSource>
      <referenceToDataSource refObjectId="7a9db98c-5b25-49b9-ace6-ea693b1e1f6d" version="21.01.000" type="source data set" uri="../sources/7a9db98c-5b25-49b9-ace6-ea693b1e1f6d.xml">
        <common:shortDescription xml:lang="en">Italian Greenhouse Gas Inventory 1990-2008</common:shortDescription>
      </referenceToDataSource>
      <referenceToDataSource refObjectId="20b6f41e-6725-4deb-8d68-dd5cd3447cc0" version="21.01.000" type="source data set" uri="../sources/20b6f41e-6725-4deb-8d68-dd5cd3447cc0.xml">
        <common:shortDescription xml:lang="en">Ireland - Informative Inventory Report 2010</common:shortDescription>
      </referenceToDataSource>
      <referenceToDataSource refObjectId="0508ea86-19b8-4557-ad52-10bc9f73452f" version="21.01.000" type="source data set" uri="../sources/0508ea86-19b8-4557-ad52-10bc9f73452f.xml">
        <common:shortDescription xml:lang="en">Inventory of the U.S. Greenhouse Gas Emissions and Sinks (1990 -2008)</common:shortDescription>
      </referenceToDataSource>
      <referenceToDataSource refObjectId="72d46923-91d3-4d2e-8565-0c4be7e8f543" version="21.01.000" type="source data set" uri="../sources/72d46923-91d3-4d2e-8565-0c4be7e8f543.xml">
        <common:shortDescription xml:lang="en">Inventaire des emissions des grandes installations de combustion en France</common:shortDescription>
      </referenceToDataSource>
      <referenceToDataSource refObjectId="f99161e2-1e5e-4d6a-8c9a-4164b8ee87b5" version="21.01.000" type="source data set" uri="../sources/f99161e2-1e5e-4d6a-8c9a-4164b8ee87b5.xml">
        <common:shortDescription xml:lang="en">Integrated Report 2010</common:shortDescription>
      </referenceToDataSource>
      <referenceToDataSource refObjectId="1a8ea509-dbfd-4ba5-805c-e9ba64d6b0cb" version="21.01.000" type="source data set" uri="../sources/1a8ea509-dbfd-4ba5-805c-e9ba64d6b0cb.xml">
        <common:shortDescription xml:lang="en">Integrated Pollution Prevention and Control (IPPC) - Ref. Doc. on the BAT for Large Combustion Plant</common:shortDescription>
      </referenceToDataSource>
      <referenceToDataSource refObjectId="e2e153a9-0d09-4447-a398-f9995717eee9" version="21.01.000" type="source data set" uri="../sources/e2e153a9-0d09-4447-a398-f9995717eee9.xml">
        <common:shortDescription xml:lang="en">Integrated Pollution Prevention and Control</common:shortDescription>
      </referenceToDataSource>
      <referenceToDataSource refObjectId="6e2d42b4-545d-4450-b5c4-0963dc5a2e59" version="21.01.000" type="source data set" uri="../sources/6e2d42b4-545d-4450-b5c4-0963dc5a2e59.xml">
        <common:shortDescription xml:lang="en">Informative Inventory Report</common:shortDescription>
      </referenceToDataSource>
      <referenceToDataSource refObjectId="8ddabeaf-59ca-45e0-b661-5c29be4427f6" version="21.01.000" type="source data set" uri="../sources/8ddabeaf-59ca-45e0-b661-5c29be4427f6.xml">
        <common:shortDescription xml:lang="en">India's Initial National Communication to the United Nations Framework Convention on Climate Change</common:shortDescription>
      </referenceToDataSource>
      <referenceToDataSource refObjectId="1a1829ef-6948-485d-b545-3b72db17264c" version="21.01.000" type="source data set" uri="../sources/1a1829ef-6948-485d-b545-3b72db17264c.xml">
        <common:shortDescription xml:lang="en">Organisation et methodes des inventaires nationaux des emission atmospheriques en France</common:shortDescription>
      </referenceToDataSource>
      <referenceToDataSource refObjectId="bbc58da8-15bb-4025-90dc-64ae4caed98f" version="21.01.000" type="source data set" uri="../sources/bbc58da8-15bb-4025-90dc-64ae4caed98f.xml">
        <common:shortDescription xml:lang="en">NIR pour la France au titre de la convention cadre des Nations Unies sur les changements climatiques</common:shortDescription>
      </referenceToDataSource>
      <referenceToDataSource refObjectId="516c7b37-100e-4481-9f93-00ed916d4541" version="21.01.000" type="source data set" uri="../sources/516c7b37-100e-4481-9f93-00ed916d4541.xml">
        <common:shortDescription xml:lang="en">New Zealand's Greenhouse Gas Inventory 1990 - 2007</common:shortDescription>
      </referenceToDataSource>
      <referenceToDataSource refObjectId="ccdc8729-d723-4a89-a1a2-60b6cab0c0bb" version="21.01.000" type="source data set" uri="../sources/ccdc8729-d723-4a89-a1a2-60b6cab0c0bb.xml">
        <common:shortDescription xml:lang="en">National Inventory Report for 1985-2008 - Hungary</common:shortDescription>
      </referenceToDataSource>
      <referenceToDataSource refObjectId="15b19a42-6441-4394-bcda-2e49ff1e0fd4" version="21.01.000" type="source data set" uri="../sources/15b19a42-6441-4394-bcda-2e49ff1e0fd4.xml">
        <common:shortDescription xml:lang="en">National Inventory Report 2010 Sweden</common:shortDescription>
      </referenceToDataSource>
      <referenceToDataSource refObjectId="4b36b132-4a68-431c-bc8b-45d2f5f21fab" version="21.01.000" type="source data set" uri="../sources/4b36b132-4a68-431c-bc8b-45d2f5f21fab.xml">
        <common:shortDescription xml:lang="en">National Inventory Report 2010 Norway</common:shortDescription>
      </referenceToDataSource>
      <referenceToDataSource refObjectId="23897ee3-ae1e-4a7b-85ea-5c8906d89269" version="21.01.000" type="source data set" uri="../sources/23897ee3-ae1e-4a7b-85ea-5c8906d89269.xml">
        <common:shortDescription xml:lang="en">National Inventory Report 2010 for Greenhouse Gas Emissions</common:shortDescription>
      </referenceToDataSource>
      <referenceToDataSource refObjectId="95d3a90d-512b-4b85-8458-f6a859a33d5a" version="21.01.000" type="source data set" uri="../sources/95d3a90d-512b-4b85-8458-f6a859a33d5a.xml">
        <common:shortDescription xml:lang="en">National Inventory Report 2010</common:shortDescription>
      </referenceToDataSource>
      <referenceToDataSource refObjectId="ab9a284c-a89e-4f6a-b507-60e0c0b5b551" version="21.01.000" type="source data set" uri="../sources/ab9a284c-a89e-4f6a-b507-60e0c0b5b551.xml">
        <common:shortDescription xml:lang="en">National Inventory Report 2010</common:shortDescription>
      </referenceToDataSource>
      <referenceToDataSource refObjectId="8892c020-5266-4d9e-828f-cdf47015d2bb" version="21.01.000" type="source data set" uri="../sources/8892c020-5266-4d9e-828f-cdf47015d2bb.xml">
        <common:shortDescription xml:lang="en">National Inventory Report</common:shortDescription>
      </referenceToDataSource>
      <referenceToDataSource refObjectId="b73a174c-74ad-4949-ae92-8e6f321c46b2" version="21.01.000" type="source data set" uri="../sources/b73a174c-74ad-4949-ae92-8e6f321c46b2.xml">
        <common:shortDescription xml:lang="en">National Greenhouse Gas Inventory Report of the Czech Republic, NIR</common:shortDescription>
      </referenceToDataSource>
      <referenceToDataSource refObjectId="9eeb0e0e-b628-4562-afb5-ddc20f317972" version="21.01.000" type="source data set" uri="../sources/9eeb0e0e-b628-4562-afb5-ddc20f317972.xml">
        <common:shortDescription xml:lang="en">National Greenhouse Gas Inventory Report of Japan</common:shortDescription>
      </referenceToDataSource>
      <referenceToDataSource refObjectId="44b3c207-ff56-4f71-9045-165718811601" version="21.01.000" type="source data set" uri="../sources/44b3c207-ff56-4f71-9045-165718811601.xml">
        <common:shortDescription xml:lang="en">National Greenhouse Gas Emission Inventory Report 2009 of the Republic of Lithuania</common:shortDescription>
      </referenceToDataSource>
      <referenceToDataSource refObjectId="ff68e8d0-7dde-4614-ba27-cf5262b7859c" version="21.01.000" type="source data set" uri="../sources/ff68e8d0-7dde-4614-ba27-cf5262b7859c.xml">
        <common:shortDescription xml:lang="en">Luxembourg´s National Inventory Report 2010 (1990 -2008)</common:shortDescription>
      </referenceToDataSource>
      <referenceToDataSource refObjectId="68dd4a61-7521-4dfc-91fe-13513bb38ca1" version="21.01.000" type="source data set" uri="../sources/68dd4a61-7521-4dfc-91fe-13513bb38ca1.xml">
        <common:shortDescription xml:lang="en">Lithuanians's Informative Inventory 2008</common:shortDescription>
      </referenceToDataSource>
      <referenceToDataSource refObjectId="555d4c66-852f-4743-a1f6-5a47a5a7dc23" version="21.01.000" type="source data set" uri="../sources/555d4c66-852f-4743-a1f6-5a47a5a7dc23.xml">
        <common:shortDescription xml:lang="en">Switzerland's Greenhouse Gas Inventory 1990-2008</common:shortDescription>
      </referenceToDataSource>
      <referenceToDataSource refObjectId="ef9503bc-edf6-4910-8e93-933446348e4f" version="21.01.000" type="source data set" uri="../sources/ef9503bc-edf6-4910-8e93-933446348e4f.xml">
        <common:shortDescription xml:lang="en">Sumas Energy 2 Generation Facility Air Quality Issue Summary</common:shortDescription>
      </referenceToDataSource>
      <referenceToDataSource refObjectId="f711df00-97d3-47c4-b180-5594b3ebe201" version="21.01.000" type="source data set" uri="../sources/f711df00-97d3-47c4-b180-5594b3ebe201.xml">
        <common:shortDescription xml:lang="en">Submission under the UN Framework Convention on Climate Change and under the Kyoto Protocol 2010</common:shortDescription>
      </referenceToDataSource>
      <referenceToDataSource refObjectId="975b5607-1824-4b62-b16d-cd44b9427522" version="21.01.000" type="source data set" uri="../sources/975b5607-1824-4b62-b16d-cd44b9427522.xml">
        <common:shortDescription xml:lang="en">Slovenia's National Inventory Report 2010</common:shortDescription>
      </referenceToDataSource>
      <referenceToDataSource refObjectId="7ed2df76-c25a-428b-870f-bb116cc4ba12" version="21.01.000" type="source data set" uri="../sources/7ed2df76-c25a-428b-870f-bb116cc4ba12.xml">
        <common:shortDescription xml:lang="en">Slovak Republic National Inventory Report 2010</common:shortDescription>
      </referenceToDataSource>
      <referenceToDataSource refObjectId="648eabe1-6171-481e-9385-0aa23ca08a9a" version="21.01.000" type="source data set" uri="../sources/648eabe1-6171-481e-9385-0aa23ca08a9a.xml">
        <common:shortDescription xml:lang="en">Romania's Greenhouse Gas Inventory 1989-2008</common:shortDescription>
      </referenceToDataSource>
      <referenceToDataSource refObjectId="fef1f400-2e11-4dbe-88eb-459269290154" version="21.01.000" type="source data set" uri="../sources/fef1f400-2e11-4dbe-88eb-459269290154.xml">
        <common:shortDescription xml:lang="en">Romanian Informative Inventory 2008</common:shortDescription>
      </referenceToDataSource>
      <referenceToDataSource refObjectId="f494c11e-737c-4b1b-a911-1d511177b5e3" version="21.01.000" type="source data set" uri="../sources/f494c11e-737c-4b1b-a911-1d511177b5e3.xml">
        <common:shortDescription xml:lang="en">Richtlinie 2009/28/EG des Europäischen Parlaments und des Rates vom 23. April 2009</common:shortDescription>
      </referenceToDataSource>
      <referenceToDataSource refObjectId="b431a232-fe5b-41c5-87b0-94fdb402a733" version="21.01.000" type="source data set" uri="../sources/b431a232-fe5b-41c5-87b0-94fdb402a733.xml">
        <common:shortDescription xml:lang="en">Renewables 2010</common:shortDescription>
      </referenceToDataSource>
      <referenceToDataSource refObjectId="e8f646de-4e1f-40ab-8294-46f81ad67fd1" version="21.01.000" type="source data set" uri="../sources/e8f646de-4e1f-40ab-8294-46f81ad67fd1.xml">
        <common:shortDescription xml:lang="en">Power Hungry: Reinventing The U.S. Electric Grid</common:shortDescription>
      </referenceToDataSource>
      <referenceToDataSource refObjectId="15fec28d-cbbc-42a8-aed9-4140a217c74e" version="21.01.000" type="source data set" uri="../sources/15fec28d-cbbc-42a8-aed9-4140a217c74e.xml">
        <common:shortDescription xml:lang="en">Power Connections: Canadian Electricity Trade and Foreign Policy</common:shortDescription>
      </referenceToDataSource>
      <referenceToDataSource refObjectId="a25eb4da-f802-4e7b-b8f9-5db9d9d59fc2" version="21.01.000" type="source data set" uri="../sources/a25eb4da-f802-4e7b-b8f9-5db9d9d59fc2.xml">
        <common:shortDescription xml:lang="en">Portuguese National Inventory Report on Grennhouse Gases, 1990-2008</common:shortDescription>
      </referenceToDataSource>
      <referenceToDataSource refObjectId="0aadf465-cc80-4843-93aa-1d2fc5a16263" version="21.01.000" type="source data set" uri="../sources/0aadf465-cc80-4843-93aa-1d2fc5a16263.xml">
        <common:shortDescription xml:lang="en">Portuguese Informative Inventory 1990-2008</common:shortDescription>
      </referenceToDataSource>
      <referenceToDataSource refObjectId="2e7f9df2-2d00-4ed3-a366-001dc03e43db" version="21.01.000" type="source data set" uri="../sources/2e7f9df2-2d00-4ed3-a366-001dc03e43db.xml">
        <common:shortDescription xml:lang="en">Poland's Informative Inventory 2010</common:shortDescription>
      </referenceToDataSource>
      <referenceToDataSource refObjectId="71fd4cb6-d468-4dca-8b65-b5b35ad6f80c" version="21.01.000" type="source data set" uri="../sources/71fd4cb6-d468-4dca-8b65-b5b35ad6f80c.xml">
        <common:shortDescription xml:lang="en">Verhaltenes Lächeln auf langen Gesichtern</common:shortDescription>
      </referenceToDataSource>
      <referenceToDataSource refObjectId="34a298be-4daa-457f-bd8f-075755d1d42d" version="21.01.000" type="source data set" uri="../sources/34a298be-4daa-457f-bd8f-075755d1d42d.xml">
        <common:shortDescription xml:lang="en">UK Greenhouse gas inventory, 1990 to 2008</common:shortDescription>
      </referenceToDataSource>
      <referenceToDataSource refObjectId="6c59444d-2cf1-426d-9df7-93e60364c955" version="21.01.000" type="source data set" uri="../sources/6c59444d-2cf1-426d-9df7-93e60364c955.xml">
        <common:shortDescription xml:lang="en">Turkey Greenhouse gas Inventory, 1990 to 2008</common:shortDescription>
      </referenceToDataSource>
      <referenceToDataSource refObjectId="68570e54-3d75-4c1f-b88d-df2a66c2ba30" version="21.01.000" type="source data set" uri="../sources/68570e54-3d75-4c1f-b88d-df2a66c2ba30.xml">
        <common:shortDescription xml:lang="en">The European Pollutant Release and Transfer Register</common:shortDescription>
      </referenceToDataSource>
      <referenceToDataSource refObjectId="3b65ee48-c719-40f4-ab73-7f0383584712" version="21.01.000" type="source data set" uri="../sources/3b65ee48-c719-40f4-ab73-7f0383584712.xml">
        <common:shortDescription xml:lang="en">The CEA Mercury program</common:shortDescription>
      </referenceToDataSource>
      <referenceToDataSource refObjectId="cbede9c2-03b5-457c-a947-6e944f9d39fc" version="21.01.000" type="source data set" uri="../sources/cbede9c2-03b5-457c-a947-6e944f9d39fc.xml">
        <common:shortDescription xml:lang="en">Telefonische Recherche - Preis Kraftwerksnebenprodukte</common:shortDescription>
      </referenceToDataSource>
      <referenceToDataSource refObjectId="fd4d74a3-6fe7-4227-9d91-83bcc4fbd80b" version="21.01.000" type="source data set" uri="../sources/fd4d74a3-6fe7-4227-9d91-83bcc4fbd80b.xml">
        <common:shortDescription xml:lang="en">EU Energy Trends to 2050</common:shortDescription>
      </referenceToDataSource>
      <referenceToDataSource refObjectId="4ba1c4d7-d4cd-4dbd-9d52-d66e65917097" version="21.01.000" type="source data set" uri="../sources/4ba1c4d7-d4cd-4dbd-9d52-d66e65917097.xml">
        <common:shortDescription xml:lang="en">Plant-by-Plant emissions reported under LCP directive </common:shortDescription>
      </referenceToDataSource>
      <referenceToDataSource refObjectId="f0a58cb7-9486-4458-a6a5-4dbef32d871b" version="21.01.000" type="source data set" uri="../sources/f0a58cb7-9486-4458-a6a5-4dbef32d871b.xml">
        <common:shortDescription xml:lang="en">The European offshore wind industry - key trends and statistics 2014</common:shortDescription>
      </referenceToDataSource>
      <referenceToDataSource refObjectId="3875965d-fb85-4dc4-94ef-3372b30d7ef9" version="21.01.000" type="source data set" uri="../sources/3875965d-fb85-4dc4-94ef-3372b30d7ef9.xml">
        <common:shortDescription xml:lang="en">China Electric Power Yearbook 2015</common:shortDescription>
      </referenceToDataSource>
      <referenceToDataSource refObjectId="038ede2d-0650-4acf-89c4-623cad30bbb9" version="21.01.000" type="source data set" uri="../sources/038ede2d-0650-4acf-89c4-623cad30bbb9.xml">
        <common:shortDescription xml:lang="en">Wind in power 2016 - European statistics  </common:shortDescription>
      </referenceToDataSource>
      <referenceToDataSource refObjectId="d5cfdcc8-52ec-4fdb-8180-4150014ed370" version="21.01.000" type="source data set" uri="../sources/d5cfdcc8-52ec-4fdb-8180-4150014ed370.xml">
        <common:shortDescription xml:lang="en">The European offshore wind industry - key trends and statistics 2015</common:shortDescription>
      </referenceToDataSource>
      <referenceToDataSource refObjectId="2593f5d7-97c7-415c-8b5e-035d7178abce" version="21.01.000" type="source data set" uri="../sources/2593f5d7-97c7-415c-8b5e-035d7178abce.xml">
        <common:shortDescription xml:lang="en">IEA Wind - 2016 Annual report   </common:shortDescription>
      </referenceToDataSource>
      <referenceToDataSource refObjectId="888c15fe-6986-4434-a7e2-39f2b06d0d8e" version="21.01.000" type="source data set" uri="../sources/888c15fe-6986-4434-a7e2-39f2b06d0d8e.xml">
        <common:shortDescription xml:lang="en">Statistical Yearbook 2015</common:shortDescription>
      </referenceToDataSource>
      <referenceToDataSource refObjectId="931e99ab-e2b5-4667-bfd6-d8517f702997" version="21.01.000" type="source data set" uri="../sources/931e99ab-e2b5-4667-bfd6-d8517f702997.xml">
        <common:shortDescription xml:lang="en">Energy Balances of OECD Countries 2017</common:shortDescription>
      </referenceToDataSource>
      <referenceToDataSource refObjectId="fc9d620f-c3b9-46b6-a592-099cdede9eca" version="21.01.000" type="source data set" uri="../sources/fc9d620f-c3b9-46b6-a592-099cdede9eca.xml">
        <common:shortDescription xml:lang="en">Energy Statistics of OECD Countries 2017</common:shortDescription>
      </referenceToDataSource>
      <referenceToDataSource refObjectId="cf73d907-7766-432e-84f7-73bde6bd0e18" version="21.01.000" type="source data set" uri="../sources/cf73d907-7766-432e-84f7-73bde6bd0e18.xml">
        <common:shortDescription xml:lang="en">Energy Balances of Non-OECD Countries 2017 </common:shortDescription>
      </referenceToDataSource>
      <referenceToDataSource refObjectId="df41463a-39bb-4787-a194-c676ba6f8523" version="21.01.000" type="source data set" uri="../sources/df41463a-39bb-4787-a194-c676ba6f8523.xml">
        <common:shortDescription xml:lang="en">Energy Statistics of Non-OECD Countries 2017</common:shortDescription>
      </referenceToDataSource>
      <referenceToDataSource refObjectId="f8733bf1-8713-445d-9f5c-511452ed6e9c" version="21.01.000" type="source data set" uri="../sources/f8733bf1-8713-445d-9f5c-511452ed6e9c.xml">
        <common:shortDescription xml:lang="en">World Energy Statistics 2017</common:shortDescription>
      </referenceToDataSource>
      <referenceToDataSource refObjectId="f3bbd3d5-6143-400c-ba0c-4d36b745ef9d" version="21.01.000" type="source data set" uri="../sources/f3bbd3d5-6143-400c-ba0c-4d36b745ef9d.xml">
        <common:shortDescription xml:lang="en">Electricity Information 2017</common:shortDescription>
      </referenceToDataSource>
      <referenceToDataSource refObjectId="e3bd9bbf-2c3c-42aa-8892-fd13f1065ca5" version="21.01.000" type="source data set" uri="../sources/e3bd9bbf-2c3c-42aa-8892-fd13f1065ca5.xml">
        <common:shortDescription xml:lang="en">Documentation of data quality management</common:shortDescription>
      </referenceToDataSource>
      <referenceToDataSource refObjectId="1cece811-7501-44d4-8067-9259bd5cb835" version="00.01.000" type="source data set" uri="../sources/1cece811-7501-44d4-8067-9259bd5cb835.xml">
        <common:shortDescription xml:lang="en">GaBi Database Edition 2021, CUP2021.01</common:shortDescription>
      </referenceToDataSource>
      <referenceToDataSource refObjectId="28d74cc0-db8b-4d7e-bc44-5f6d56ce0c4a" version="00.03.002" type="source data set" uri="../sources/28d74cc0-db8b-4d7e-bc44-5f6d56ce0c4a.xml">
        <common:shortDescription xml:lang="en">GaBi database (all versions)</common:shortDescription>
      </referenceToDataSource>
      <useAdviceForDataSet xml:lang="en">The data set represents a projected electricity supply in the future. The projection includes changes from policies that have been already implemented but also planned policies and policies that are needed to fullfill certain mitigation targets (especially primary energy consumption and GHG emissions). The data set can be used for all LCA/CF studies where low voltage electricity is needed. Combination with individual unit processes using this commodity enables the generation of user-specific (product) LCAs.</useAdviceForDataSet>
      <useAdviceForDataSet xml:lang="de">The data set represents a projected electricity supply in the future. The projection includes changes from policies that have been already implemented but also planned policies and policies that are needed to fullfill certain mitigation targets (especially primary energy consumption and GHG emissions). The data set can be used for all LCA/CF studies where low voltage electricity is needed. Combination with individual unit processes using this commodity enables the generation of user-specific (product) LCAs.</useAdviceForDataSet>
    </dataSourcesTreatmentAndRepresentativeness>
    <validation>
      <review type="Dependent internal review">
        <common:referenceToNameOfReviewerAndInstitution refObjectId="d7fa0337-f279-430d-becf-7f3111a85010" version="21.01.000" type="contact data set" uri="../contacts/d7fa0337-f279-430d-becf-7f3111a85010.xml">
          <common:shortDescription xml:lang="en">Sphera Solutions GmbH</common:shortDescription>
        </common:referenceToNameOfReviewerAndInstitution>
      </review>
      <review type="Independent external review">
        <common:referenceToNameOfReviewerAndInstitution refObjectId="8f1306f0-7b83-4f36-a537-aa83f0498266" version="21.01.000" type="contact data set" uri="../contacts/8f1306f0-7b83-4f36-a537-aa83f0498266.xml">
          <common:shortDescription xml:lang="en">GaBi user forum</common:shortDescription>
        </common:referenceToNameOfReviewerAndInstitution>
      </review>
    </validation>
    <complianceDeclarations>
      <compliance>
        <common:referenceToComplianceSystem refObjectId="c0016b33-8cf7-415c-ac6e-deba0d21440d" version="00.01.000" type="source data set" uri="../sources/c0016b33-8cf7-415c-ac6e-deba0d21440d.xml">
          <common:shortDescription xml:lang="de">EN 15804+A2</common:shortDescription>
          <common:shortDescription xml:lang="en">EN 15804+A2</common:shortDescription>
        </common:referenceToComplianceSystem>
        <common:approvalOfOverallCompliance>Fully compliant</common:approvalOfOverallCompliance>
      </compliance>
    </complianceDeclarations>
  </modellingAndValidation>
  <administrativeInformation>
    <dataEntryBy>
      <common:timeStamp>2021-04-28T21:03:15+01:00</common:timeStamp>
      <common:referenceToDataSetFormat refObjectId="a97a0155-0234-4b87-b4ce-a45da52f2a40" version="01.00.000" type="source data set" uri="../sources/a97a0155-0234-4b87-b4ce-a45da52f2a40.xml">
        <common:shortDescription xml:lang="de">ILCD format 1.1</common:shortDescription>
        <common:shortDescription xml:lang="en">ILCD format 1.1</common:shortDescription>
      </common:referenceToDataSetFormat>
      <common:referenceToDataSetFormat refObjectId="a29449fd-aa2f-4de8-b5d7-4b06b43c6fde" version="00.01.000" type="source data set" uri="../sources/a29449fd-aa2f-4de8-b5d7-4b06b43c6fde.xml">
        <common:shortDescription xml:lang="de">EPD-Datenformaterweiterungen v1.2</common:shortDescription>
        <common:shortDescription xml:lang="en">EPD Data Format Extensions v1.2</common:shortDescription>
      </common:referenceToDataSetFormat>
      <common:referenceToPersonOrEntityEnteringTheData refObjectId="d7fa0337-f279-430d-becf-7f3111a85010" version="21.01.000" type="contact data set" uri="../contacts/d7fa0337-f279-430d-becf-7f3111a85010.xml">
        <common:shortDescription xml:lang="en">Sphera Solutions GmbH</common:shortDescription>
      </common:referenceToPersonOrEntityEnteringTheData>
    </dataEntryBy>
    <publicationAndOwnership>
      <common:dataSetVersion>20.21.060</common:dataSetVersion>
      <common:referenceToPrecedingDataSetVersion refObjectId="5331890a-9fd2-4388-bc6f-9776f9552848" type="process data set" uri="https://www.oekobaudat.de/OEKOBAU.DAT/datasetdetail/process.xhtml?uuid=5331890a-9fd2-4388-bc6f-9776f9552848&amp;stock=OBD_2020_II&amp;lang=de">
        <common:shortDescription xml:lang="en">Electricity grid mix scenario 2050</common:shortDescription>
      </common:referenceToPrecedingDataSetVersion>
      <common:referenceToOwnershipOfDataSet refObjectId="d7fa0337-f279-430d-becf-7f3111a85010" version="21.01.000" type="contact data set" uri="../contacts/d7fa0337-f279-430d-becf-7f3111a85010.xml">
        <common:shortDescription xml:lang="en">Sphera Solutions GmbH</common:shortDescription>
      </common:referenceToOwnershipOfDataSet>
      <common:copyright>true</common:copyright>
      <common:licenseType>Free of charge for all users and uses</common:licenseType>
      <common:accessRestrictions xml:lang="en">The license conditions as stated on https://www.oekobaudat.de/ apply.</common:accessRestrictions>
      <common:accessRestrictions xml:lang="de">Es gelten die Lizenzbedingungen wie sie auf https://www.oekobaudat.de/ genannt sind.</common:accessRestrictions>
      <common:other>
        <epd2:referenceToPublisher refObjectId="f11651e0-7877-11e3-981f-0800200c9a66" version="00.01.000" type="contact data set" uri="../contacts/f11651e0-7877-11e3-981f-0800200c9a66.xml">
          <common:shortDescription xml:lang="en">BBSR</common:shortDescription>
        </epd2:referenceToPublisher>
      </common:other>
    </publicationAndOwnership>
  </administrativeInformation>
  <exchanges>
    <exchange dataSetInternalID="107885">
      <referenceToFlowDataSet refObjectId="890a70b7-b677-4e2a-8a1b-7d017e0a10ae" version="21.01.000" type="flow data set" uri="../flows/890a70b7-b677-4e2a-8a1b-7d017e0a10ae.xml">
        <common:shortDescription xml:lang="en">Electricity grid mix scenario 2050</common:shortDescription>
        <common:shortDescription xml:lang="de">Strom-Mix-Szenario 2050</common:shortDescription>
      </referenceToFlowDataSet>
      <meanAmount>3.6</meanAmount>
    </exchange>
    <exchange dataSetInternalID="107886">
      <referenceToFlowDataSet refObjectId="20f32be5-0398-4288-9b6d-accddd195317" version="21.01.000" type="flow data set" uri="../flows/20f32be5-0398-4288-9b6d-accddd195317.xml">
        <common:shortDescription xml:lang="en">Use of renewable primary energy as energy carrier (PERE)</common:shortDescription>
        <common:shortDescription xml:lang="de">Erneuerbare Primärenergie als Energieträger (PERE)</common:shortDescription>
      </referenceToFlowDataSet>
      <functionType>General reminder flow</functionType>
      <exchangeDirection>Input</exchangeDirection>
      <common:other>
        <epd:amount epd:module="B6">7.57835882270437</epd:amount>
        <epd:referenceToUnitGroupDataSet refObjectId="93a60a57-a3c8-11da-a746-0800200c9a66" version="03.00.000" type="unit group data set" uri="../unitgroups/93a60a57-a3c8-11da-a746-0800200c9a66.xml">
          <common:shortDescription xml:lang="en">MJ</common:shortDescription>
        </epd:referenceToUnitGroupDataSet>
      </common:other>
    </exchange>
    <exchange dataSetInternalID="107887">
      <referenceToFlowDataSet refObjectId="fb3ec0de-548d-4508-aea5-00b73bf6f702" version="21.01.000" type="flow data set" uri="../flows/fb3ec0de-548d-4508-aea5-00b73bf6f702.xml">
        <common:shortDescription xml:lang="en">Use of renewable primary energy resources used as raw materials (PERM)</common:shortDescription>
        <common:shortDescription xml:lang="de">Erneuerbare Primärenergie zur stofflichen Nutzung (PERM)</common:shortDescription>
      </referenceToFlowDataSet>
      <functionType>General reminder flow</functionType>
      <exchangeDirection>Input</exchangeDirection>
      <common:other>
        <epd:amount epd:module="B6">0</epd:amount>
        <epd:referenceToUnitGroupDataSet refObjectId="93a60a57-a3c8-11da-a746-0800200c9a66" version="03.00.000" type="unit group data set" uri="../unitgroups/93a60a57-a3c8-11da-a746-0800200c9a66.xml">
          <common:shortDescription xml:lang="en">MJ</common:shortDescription>
        </epd:referenceToUnitGroupDataSet>
      </common:other>
    </exchange>
    <exchange dataSetInternalID="107888">
      <referenceToFlowDataSet refObjectId="53f97275-fa8a-4cdd-9024-65936002acd0" version="21.01.000" type="flow data set" uri="../flows/53f97275-fa8a-4cdd-9024-65936002acd0.xml">
        <common:shortDescription xml:lang="en">Total use of renewable primary energy (PERT)</common:shortDescription>
        <common:shortDescription xml:lang="de">Total erneuerbare Primärenergie (PERT)</common:shortDescription>
      </referenceToFlowDataSet>
      <functionType>General reminder flow</functionType>
      <exchangeDirection>Input</exchangeDirection>
      <common:other>
        <epd:amount epd:module="B6">7.57835882270437</epd:amount>
        <epd:referenceToUnitGroupDataSet refObjectId="93a60a57-a3c8-11da-a746-0800200c9a66" version="03.00.000" type="unit group data set" uri="../unitgroups/93a60a57-a3c8-11da-a746-0800200c9a66.xml">
          <common:shortDescription xml:lang="en">MJ</common:shortDescription>
        </epd:referenceToUnitGroupDataSet>
      </common:other>
    </exchange>
    <exchange dataSetInternalID="107889">
      <referenceToFlowDataSet refObjectId="ac857178-2b45-46ec-892a-a9a4332f0372" version="21.01.000" type="flow data set" uri="../flows/ac857178-2b45-46ec-892a-a9a4332f0372.xml">
        <common:shortDescription xml:lang="en">Use of non renewable primary energy as energy carrier (PENRE)</common:shortDescription>
        <common:shortDescription xml:lang="de">Nicht-erneuerbare Primärenergie als Energieträger (PENRE)</common:shortDescription>
      </referenceToFlowDataSet>
      <functionType>General reminder flow</functionType>
      <exchangeDirection>Input</exchangeDirection>
      <common:other>
        <epd:amount epd:module="B6">4.14543367662597</epd:amount>
        <epd:referenceToUnitGroupDataSet refObjectId="93a60a57-a3c8-11da-a746-0800200c9a66" version="03.00.000" type="unit group data set" uri="../unitgroups/93a60a57-a3c8-11da-a746-0800200c9a66.xml">
          <common:shortDescription xml:lang="en">MJ</common:shortDescription>
        </epd:referenceToUnitGroupDataSet>
      </common:other>
    </exchange>
    <exchange dataSetInternalID="107890">
      <referenceToFlowDataSet refObjectId="1421caa0-679d-4bf4-b282-0eb850ccae27" version="21.01.000" type="flow data set" uri="../flows/1421caa0-679d-4bf4-b282-0eb850ccae27.xml">
        <common:shortDescription xml:lang="en">Use of non renewable primary energy resources used as raw materials (PENRM)</common:shortDescription>
        <common:shortDescription xml:lang="de">Nicht-erneuerbare Primärenergie zur stofflichen Nutzung (PENRM)</common:shortDescription>
      </referenceToFlowDataSet>
      <functionType>General reminder flow</functionType>
      <exchangeDirection>Input</exchangeDirection>
      <common:other>
        <epd:amount epd:module="B6">0</epd:amount>
        <epd:referenceToUnitGroupDataSet refObjectId="93a60a57-a3c8-11da-a746-0800200c9a66" version="03.00.000" type="unit group data set" uri="../unitgroups/93a60a57-a3c8-11da-a746-0800200c9a66.xml">
          <common:shortDescription xml:lang="en">MJ</common:shortDescription>
        </epd:referenceToUnitGroupDataSet>
      </common:other>
    </exchange>
    <exchange dataSetInternalID="107891">
      <referenceToFlowDataSet refObjectId="06159210-646b-4c8d-8583-da9b3b95a6c1" version="21.01.000" type="flow data set" uri="../flows/06159210-646b-4c8d-8583-da9b3b95a6c1.xml">
        <common:shortDescription xml:lang="en">Total use of non renewable primary energy resource (PENRT)</common:shortDescription>
        <common:shortDescription xml:lang="de">Total nicht-erneuerbare Primärenergie (PENRT)</common:shortDescription>
      </referenceToFlowDataSet>
      <functionType>General reminder flow</functionType>
      <exchangeDirection>Input</exchangeDirection>
      <common:other>
        <epd:amount epd:module="B6">4.14543367662597</epd:amount>
        <epd:referenceToUnitGroupDataSet refObjectId="93a60a57-a3c8-11da-a746-0800200c9a66" version="03.00.000" type="unit group data set" uri="../unitgroups/93a60a57-a3c8-11da-a746-0800200c9a66.xml">
          <common:shortDescription xml:lang="en">MJ</common:shortDescription>
        </epd:referenceToUnitGroupDataSet>
      </common:other>
    </exchange>
    <exchange dataSetInternalID="107892">
      <referenceToFlowDataSet refObjectId="c6a1f35f-2d09-4f54-8dfb-97e502e1ce92" version="21.01.000" type="flow data set" uri="../flows/c6a1f35f-2d09-4f54-8dfb-97e502e1ce92.xml">
        <common:shortDescription xml:lang="en">Use of secondary material (SM)</common:shortDescription>
        <common:shortDescription xml:lang="de">Einsatz von Sekundärstoffen (SM)</common:shortDescription>
      </referenceToFlowDataSet>
      <functionType>General reminder flow</functionType>
      <exchangeDirection>Input</exchangeDirection>
      <common:other>
        <epd:amount epd:module="B6">0</epd:amount>
        <epd:referenceToUnitGroupDataSet refObjectId="93a60a57-a4c8-11da-a746-0800200c9a66" version="03.00.000" type="unit group data set" uri="../unitgroups/93a60a57-a4c8-11da-a746-0800200c9a66.xml">
          <common:shortDescription xml:lang="en">kg</common:shortDescription>
        </epd:referenceToUnitGroupDataSet>
      </common:other>
    </exchange>
    <exchange dataSetInternalID="107893">
      <referenceToFlowDataSet refObjectId="64333088-a55f-4aa2-9a31-c10b07816787" version="21.01.000" type="flow data set" uri="../flows/64333088-a55f-4aa2-9a31-c10b07816787.xml">
        <common:shortDescription xml:lang="en">Use of renewable secondary fuels (SF)</common:shortDescription>
        <common:shortDescription xml:lang="de">Erneuerbare Sekundärbrennstoffe (SF)</common:shortDescription>
      </referenceToFlowDataSet>
      <functionType>General reminder flow</functionType>
      <exchangeDirection>Input</exchangeDirection>
      <common:other>
        <epd:amount epd:module="B6">0</epd:amount>
        <epd:referenceToUnitGroupDataSet refObjectId="93a60a57-a3c8-11da-a746-0800200c9a66" version="03.00.000" type="unit group data set" uri="../unitgroups/93a60a57-a3c8-11da-a746-0800200c9a66.xml">
          <common:shortDescription xml:lang="en">MJ</common:shortDescription>
        </epd:referenceToUnitGroupDataSet>
      </common:other>
    </exchange>
    <exchange dataSetInternalID="107894">
      <referenceToFlowDataSet refObjectId="89def144-d39a-4287-b86f-efde453ddcb2" version="21.01.000" type="flow data set" uri="../flows/89def144-d39a-4287-b86f-efde453ddcb2.xml">
        <common:shortDescription xml:lang="en">Use of non renewable secondary fuels (NRSF)</common:shortDescription>
        <common:shortDescription xml:lang="de">Nicht erneuerbare Sekundärbrennstoffe (NRSF)</common:shortDescription>
      </referenceToFlowDataSet>
      <functionType>General reminder flow</functionType>
      <exchangeDirection>Input</exchangeDirection>
      <common:other>
        <epd:amount epd:module="B6">0</epd:amount>
        <epd:referenceToUnitGroupDataSet refObjectId="93a60a57-a3c8-11da-a746-0800200c9a66" version="03.00.000" type="unit group data set" uri="../unitgroups/93a60a57-a3c8-11da-a746-0800200c9a66.xml">
          <common:shortDescription xml:lang="en">MJ</common:shortDescription>
        </epd:referenceToUnitGroupDataSet>
      </common:other>
    </exchange>
    <exchange dataSetInternalID="107895">
      <referenceToFlowDataSet refObjectId="3cf952c8-f3a4-461d-8c96-96456ca62246" version="21.01.000" type="flow data set" uri="../flows/3cf952c8-f3a4-461d-8c96-96456ca62246.xml">
        <common:shortDescription xml:lang="en">Net use of fresh water (FW)</common:shortDescription>
        <common:shortDescription xml:lang="de">Nettoeinsatz von Süßwasserressourcen (FW)</common:shortDescription>
      </referenceToFlowDataSet>
      <functionType>General reminder flow</functionType>
      <exchangeDirection>Input</exchangeDirection>
      <common:other>
        <epd:amount epd:module="B6">0.00151451400280991</epd:amount>
        <epd:referenceToUnitGroupDataSet refObjectId="93a60a57-a3c8-12da-a746-0800200c9a66" version="03.00.000" type="unit group data set" uri="../unitgroups/93a60a57-a3c8-12da-a746-0800200c9a66.xml">
          <common:shortDescription xml:lang="en">m3</common:shortDescription>
        </epd:referenceToUnitGroupDataSet>
      </common:other>
    </exchange>
    <exchange dataSetInternalID="107896">
      <referenceToFlowDataSet refObjectId="430f9e0f-59b2-46a0-8e0d-55e0e84948fc" version="21.01.000" type="flow data set" uri="../flows/430f9e0f-59b2-46a0-8e0d-55e0e84948fc.xml">
        <common:shortDescription xml:lang="en">Hazardous waste disposed (HWD)</common:shortDescription>
        <common:shortDescription xml:lang="de">Gefährlicher Abfall zur Deponie (HWD)</common:shortDescription>
      </referenceToFlowDataSet>
      <functionType>General reminder flow</functionType>
      <exchangeDirection>Output</exchangeDirection>
      <common:other>
        <epd:amount epd:module="B6">3.82067809958865E-9</epd:amount>
        <epd:referenceToUnitGroupDataSet refObjectId="93a60a57-a4c8-11da-a746-0800200c9a66" version="03.00.000" type="unit group data set" uri="../unitgroups/93a60a57-a4c8-11da-a746-0800200c9a66.xml">
          <common:shortDescription xml:lang="en">kg</common:shortDescription>
        </epd:referenceToUnitGroupDataSet>
      </common:other>
    </exchange>
    <exchange dataSetInternalID="107897">
      <referenceToFlowDataSet refObjectId="b29ef66b-e286-4afa-949f-62f1a7b4d7fa" version="21.01.000" type="flow data set" uri="../flows/b29ef66b-e286-4afa-949f-62f1a7b4d7fa.xml">
        <common:shortDescription xml:lang="en">Non harzardous waste disposed (NHWD)</common:shortDescription>
        <common:shortDescription xml:lang="de">Entsorgter nicht gefährlicher Abfall (NHWD)</common:shortDescription>
      </referenceToFlowDataSet>
      <functionType>General reminder flow</functionType>
      <exchangeDirection>Output</exchangeDirection>
      <common:other>
        <epd:amount epd:module="B6">0.00549209184516188</epd:amount>
        <epd:referenceToUnitGroupDataSet refObjectId="93a60a57-a4c8-11da-a746-0800200c9a66" version="03.00.000" type="unit group data set" uri="../unitgroups/93a60a57-a4c8-11da-a746-0800200c9a66.xml">
          <common:shortDescription xml:lang="en">kg</common:shortDescription>
        </epd:referenceToUnitGroupDataSet>
      </common:other>
    </exchange>
    <exchange dataSetInternalID="107898">
      <referenceToFlowDataSet refObjectId="3449546e-52ad-4b39-b809-9fb77cea8ff6" version="21.01.000" type="flow data set" uri="../flows/3449546e-52ad-4b39-b809-9fb77cea8ff6.xml">
        <common:shortDescription xml:lang="en">Radioactive waste disposed (RWD)</common:shortDescription>
        <common:shortDescription xml:lang="de">Entsorgter radioaktiver Abfall (RWD)</common:shortDescription>
      </referenceToFlowDataSet>
      <functionType>General reminder flow</functionType>
      <exchangeDirection>Output</exchangeDirection>
      <common:other>
        <epd:amount epd:module="B6">7.76977543552647E-5</epd:amount>
        <epd:referenceToUnitGroupDataSet refObjectId="93a60a57-a4c8-11da-a746-0800200c9a66" version="03.00.000" type="unit group data set" uri="../unitgroups/93a60a57-a4c8-11da-a746-0800200c9a66.xml">
          <common:shortDescription xml:lang="en">kg</common:shortDescription>
        </epd:referenceToUnitGroupDataSet>
      </common:other>
    </exchange>
    <exchange dataSetInternalID="107899">
      <referenceToFlowDataSet refObjectId="a2b32f97-3fc7-4af2-b209-525bc6426f33" version="21.01.000" type="flow data set" uri="../flows/a2b32f97-3fc7-4af2-b209-525bc6426f33.xml">
        <common:shortDescription xml:lang="en">Components for re-use (CRU)</common:shortDescription>
        <common:shortDescription xml:lang="de">Komponenten für die Wiederverwendung (CRU)</common:shortDescription>
      </referenceToFlowDataSet>
      <functionType>General reminder flow</functionType>
      <exchangeDirection>Output</exchangeDirection>
      <common:other>
        <epd:amount epd:module="B6">0</epd:amount>
        <epd:referenceToUnitGroupDataSet refObjectId="93a60a57-a4c8-11da-a746-0800200c9a66" version="03.00.000" type="unit group data set" uri="../unitgroups/93a60a57-a4c8-11da-a746-0800200c9a66.xml">
          <common:shortDescription xml:lang="en">kg</common:shortDescription>
        </epd:referenceToUnitGroupDataSet>
      </common:other>
    </exchange>
    <exchange dataSetInternalID="107900">
      <referenceToFlowDataSet refObjectId="d7fe48a5-4103-49c8-9aae-b0b5dfdbd6ae" version="21.01.000" type="flow data set" uri="../flows/d7fe48a5-4103-49c8-9aae-b0b5dfdbd6ae.xml">
        <common:shortDescription xml:lang="en">Materials for recycling  (MFR)</common:shortDescription>
        <common:shortDescription xml:lang="de">Stoffe zum Recycling (MFR)</common:shortDescription>
      </referenceToFlowDataSet>
      <functionType>General reminder flow</functionType>
      <exchangeDirection>Output</exchangeDirection>
      <common:other>
        <epd:amount epd:module="B6">0</epd:amount>
        <epd:referenceToUnitGroupDataSet refObjectId="93a60a57-a4c8-11da-a746-0800200c9a66" version="03.00.000" type="unit group data set" uri="../unitgroups/93a60a57-a4c8-11da-a746-0800200c9a66.xml">
          <common:shortDescription xml:lang="en">kg</common:shortDescription>
        </epd:referenceToUnitGroupDataSet>
      </common:other>
    </exchange>
    <exchange dataSetInternalID="107901">
      <referenceToFlowDataSet refObjectId="59a9181c-3aaf-46ee-8b13-2b3723b6e447" version="21.01.000" type="flow data set" uri="../flows/59a9181c-3aaf-46ee-8b13-2b3723b6e447.xml">
        <common:shortDescription xml:lang="en">Materials for energy recovery (MER)</common:shortDescription>
        <common:shortDescription xml:lang="de">Stoffe für die Energierückgewinnung (MER)</common:shortDescription>
      </referenceToFlowDataSet>
      <functionType>General reminder flow</functionType>
      <exchangeDirection>Output</exchangeDirection>
      <common:other>
        <epd:amount epd:module="B6">0</epd:amount>
        <epd:referenceToUnitGroupDataSet refObjectId="93a60a57-a4c8-11da-a746-0800200c9a66" version="03.00.000" type="unit group data set" uri="../unitgroups/93a60a57-a4c8-11da-a746-0800200c9a66.xml">
          <common:shortDescription xml:lang="en">kg</common:shortDescription>
        </epd:referenceToUnitGroupDataSet>
      </common:other>
    </exchange>
    <exchange dataSetInternalID="107902">
      <referenceToFlowDataSet refObjectId="4da0c987-2b76-40d6-9e9e-82a017aaaf29" version="21.01.000" type="flow data set" uri="../flows/4da0c987-2b76-40d6-9e9e-82a017aaaf29.xml">
        <common:shortDescription xml:lang="en">Exported electrical energy (EEE)</common:shortDescription>
        <common:shortDescription xml:lang="de">Exportierte elektrische Energie (EEE)</common:shortDescription>
      </referenceToFlowDataSet>
      <functionType>General reminder flow</functionType>
      <exchangeDirection>Output</exchangeDirection>
      <common:other>
        <epd:amount epd:module="B6">0</epd:amount>
        <epd:referenceToUnitGroupDataSet refObjectId="93a60a57-a3c8-11da-a746-0800200c9a66" version="03.00.000" type="unit group data set" uri="../unitgroups/93a60a57-a3c8-11da-a746-0800200c9a66.xml">
          <common:shortDescription xml:lang="en">MJ</common:shortDescription>
        </epd:referenceToUnitGroupDataSet>
      </common:other>
    </exchange>
    <exchange dataSetInternalID="107903">
      <referenceToFlowDataSet refObjectId="98daf38a-7a79-46d3-9a37-2b7bd0955810" version="21.01.000" type="flow data set" uri="../flows/98daf38a-7a79-46d3-9a37-2b7bd0955810.xml">
        <common:shortDescription xml:lang="en">Exported thermal energy (EET)</common:shortDescription>
        <common:shortDescription xml:lang="de">Exportierte thermische Energie (EET)</common:shortDescription>
      </referenceToFlowDataSet>
      <functionType>General reminder flow</functionType>
      <exchangeDirection>Output</exchangeDirection>
      <common:other>
        <epd:amount epd:module="B6">0</epd:amount>
        <epd:referenceToUnitGroupDataSet refObjectId="93a60a57-a3c8-11da-a746-0800200c9a66" version="03.00.000" type="unit group data set" uri="../unitgroups/93a60a57-a3c8-11da-a746-0800200c9a66.xml">
          <common:shortDescription xml:lang="en">MJ</common:shortDescription>
        </epd:referenceToUnitGroupDataSet>
      </common:other>
    </exchange>
  </exchanges>
  <LCIAResults>
    <LCIAResult>
      <referenceToLCIAMethodDataSet refObjectId="6a37f984-a4b3-458a-a20a-64418c145fa2" version="21.01.000" type="LCIA method data set" uri="../lciamethods/6a37f984-a4b3-458a-a20a-64418c145fa2.xml">
        <common:shortDescription xml:lang="en">Global Warming Potential - total (GWP-total)</common:shortDescription>
        <common:shortDescription xml:lang="de">Globales Erwärmungspotenzial - total (GWP-total)</common:shortDescription>
      </referenceToLCIAMethodDataSet>
      <common:other>
        <epd:amount epd:module="B6">0.369757848787261</epd:amount>
        <epd:referenceToUnitGroupDataSet refObjectId="1ebf3012-d0db-4de2-aefd-ef30cedb0be1" version="25.00.000" type="unit group data set" uri="../unitgroups/1ebf3012-d0db-4de2-aefd-ef30cedb0be1.xml">
          <common:shortDescription xml:lang="en">kg CO2 eq.</common:shortDescription>
        </epd:referenceToUnitGroupDataSet>
      </common:other>
    </LCIAResult>
    <LCIAResult>
      <referenceToLCIAMethodDataSet refObjectId="5f635281-343e-44fb-83df-1971b155e6b6" version="21.01.000" type="LCIA method data set" uri="../lciamethods/5f635281-343e-44fb-83df-1971b155e6b6.xml">
        <common:shortDescription xml:lang="en">Global Warming Potential - fossil fuels (GWP-fossil)</common:shortDescription>
        <common:shortDescription xml:lang="de">Globales Erwärmungspotenzial - fossil (GWP-fossil)</common:shortDescription>
      </referenceToLCIAMethodDataSet>
      <common:other>
        <epd:amount epd:module="B6">0.362808242559218</epd:amount>
        <epd:referenceToUnitGroupDataSet refObjectId="1ebf3012-d0db-4de2-aefd-ef30cedb0be1" version="25.00.000" type="unit group data set" uri="../unitgroups/1ebf3012-d0db-4de2-aefd-ef30cedb0be1.xml">
          <common:shortDescription xml:lang="en">kg CO2 eq.</common:shortDescription>
        </epd:referenceToUnitGroupDataSet>
      </common:other>
    </LCIAResult>
    <LCIAResult>
      <referenceToLCIAMethodDataSet refObjectId="2356e1ab-0185-4db5-86e5-16de51c7485c" version="21.01.000" type="LCIA method data set" uri="../lciamethods/2356e1ab-0185-4db5-86e5-16de51c7485c.xml">
        <common:shortDescription xml:lang="en">Global Warming Potential - biogenic (GWP-biogenic)</common:shortDescription>
        <common:shortDescription xml:lang="de">Globales Erwärmungspotenzial - biogen (GWP-biogenic)</common:shortDescription>
      </referenceToLCIAMethodDataSet>
      <common:other>
        <epd:amount epd:module="B6">0.00542005531306656</epd:amount>
        <epd:referenceToUnitGroupDataSet refObjectId="1ebf3012-d0db-4de2-aefd-ef30cedb0be1" version="25.00.000" type="unit group data set" uri="../unitgroups/1ebf3012-d0db-4de2-aefd-ef30cedb0be1.xml">
          <common:shortDescription xml:lang="en">kg CO2 eq.</common:shortDescription>
        </epd:referenceToUnitGroupDataSet>
      </common:other>
    </LCIAResult>
    <LCIAResult>
      <referenceToLCIAMethodDataSet refObjectId="4331bbdb-978a-490d-8707-eeb047f01a55" version="21.01.000" type="LCIA method data set" uri="../lciamethods/4331bbdb-978a-490d-8707-eeb047f01a55.xml">
        <common:shortDescription xml:lang="en">Global Warming Potential - land use and land use change (GWP-luluc)</common:shortDescription>
        <common:shortDescription xml:lang="de">Globales Erwärmungspotenzial - luluc (GWP-luluc)</common:shortDescription>
      </referenceToLCIAMethodDataSet>
      <common:other>
        <epd:amount epd:module="B6">0.00152955091497613</epd:amount>
        <epd:referenceToUnitGroupDataSet refObjectId="1ebf3012-d0db-4de2-aefd-ef30cedb0be1" version="25.00.000" type="unit group data set" uri="../unitgroups/1ebf3012-d0db-4de2-aefd-ef30cedb0be1.xml">
          <common:shortDescription xml:lang="en">kg CO2 eq.</common:shortDescription>
        </epd:referenceToUnitGroupDataSet>
      </common:other>
    </LCIAResult>
    <LCIAResult>
      <referenceToLCIAMethodDataSet refObjectId="b5c629d6-def3-11e6-bf01-fe55135034f3" version="21.01.000" type="LCIA method data set" uri="../lciamethods/b5c629d6-def3-11e6-bf01-fe55135034f3.xml">
        <common:shortDescription xml:lang="en">Depletion potenzial of the stratospheric ozone layer (ODP)</common:shortDescription>
        <common:shortDescription xml:lang="de">Abbaupotenzial der stratosphärischen Ozonschicht (ODP)</common:shortDescription>
      </referenceToLCIAMethodDataSet>
      <common:other>
        <epd:amount epd:module="B6">3.81333539531788E-14</epd:amount>
        <epd:referenceToUnitGroupDataSet refObjectId="d9e957c9-7309-4474-bf3a-7777df6c4e5b" version="25.00.000" type="unit group data set" uri="../unitgroups/d9e957c9-7309-4474-bf3a-7777df6c4e5b.xml">
          <common:shortDescription xml:lang="en">kg CFC-11 eq.</common:shortDescription>
        </epd:referenceToUnitGroupDataSet>
      </common:other>
    </LCIAResult>
    <LCIAResult>
      <referenceToLCIAMethodDataSet refObjectId="b5c611c6-def3-11e6-bf01-fe55135034f3" version="21.01.000" type="LCIA method data set" uri="../lciamethods/b5c611c6-def3-11e6-bf01-fe55135034f3.xml">
        <common:shortDescription xml:lang="en">Acidifcation potential, Accumulated Exceedance (AP)</common:shortDescription>
        <common:shortDescription xml:lang="de">Versauerungspotenzial, kumulierte Überschreitung (AP)</common:shortDescription>
      </referenceToLCIAMethodDataSet>
      <common:other>
        <epd:amount epd:module="B6">0.000605764587568383</epd:amount>
        <epd:referenceToUnitGroupDataSet refObjectId="42e089ac-92bf-4bf2-8ca1-5fc40d18f2ed" version="00.01.000" type="unit group data set" uri="../unitgroups/42e089ac-92bf-4bf2-8ca1-5fc40d18f2ed.xml">
          <common:shortDescription xml:lang="en">Mole of H+ eq.</common:shortDescription>
        </epd:referenceToUnitGroupDataSet>
      </common:other>
    </LCIAResult>
    <LCIAResult>
      <referenceToLCIAMethodDataSet refObjectId="b53ec18f-7377-4ad3-86eb-cc3f4f276b2b" version="21.01.000" type="LCIA method data set" uri="../lciamethods/b53ec18f-7377-4ad3-86eb-cc3f4f276b2b.xml">
        <common:shortDescription xml:lang="en">Eutrophication potential - freshwater (EP-freshwater)</common:shortDescription>
        <common:shortDescription xml:lang="de">Eutrophierungspotenzial - Süßwasser (EP-freshwater)</common:shortDescription>
      </referenceToLCIAMethodDataSet>
      <common:other>
        <epd:amount epd:module="B6">2.65103617667578E-6</epd:amount>
        <epd:referenceToUnitGroupDataSet refObjectId="0429039d-a61d-4590-ba67-aa4a20a810a1" version="25.00.000" type="unit group data set" uri="../unitgroups/0429039d-a61d-4590-ba67-aa4a20a810a1.xml">
          <common:shortDescription xml:lang="en">kg P eq.</common:shortDescription>
        </epd:referenceToUnitGroupDataSet>
      </common:other>
    </LCIAResult>
    <LCIAResult>
      <referenceToLCIAMethodDataSet refObjectId="b5c619fa-def3-11e6-bf01-fe55135034f3" version="21.01.000" type="LCIA method data set" uri="../lciamethods/b5c619fa-def3-11e6-bf01-fe55135034f3.xml">
        <common:shortDescription xml:lang="en">Eutrophication potential - marine (EP-marine)</common:shortDescription>
        <common:shortDescription xml:lang="de">Eutrophierungspotenzial - Salzwasser (EP-marine)</common:shortDescription>
      </referenceToLCIAMethodDataSet>
      <common:other>
        <epd:amount epd:module="B6">0.000196668422580086</epd:amount>
        <epd:referenceToUnitGroupDataSet refObjectId="d05bb823-ecdf-4686-8c40-bf1d9257859f" version="00.00.003" type="unit group data set" uri="../unitgroups/d05bb823-ecdf-4686-8c40-bf1d9257859f.xml">
          <common:shortDescription xml:lang="en">kg N eq.</common:shortDescription>
        </epd:referenceToUnitGroupDataSet>
      </common:other>
    </LCIAResult>
    <LCIAResult>
      <referenceToLCIAMethodDataSet refObjectId="b5c614d2-def3-11e6-bf01-fe55135034f3" version="21.01.000" type="LCIA method data set" uri="../lciamethods/b5c614d2-def3-11e6-bf01-fe55135034f3.xml">
        <common:shortDescription xml:lang="en">Eutrophication potential - terrestrial (EP-terrestrial)</common:shortDescription>
        <common:shortDescription xml:lang="de">Eutrophierungspotenzial - Land (EP-terrestrial)</common:shortDescription>
      </referenceToLCIAMethodDataSet>
      <common:other>
        <epd:amount epd:module="B6">0.00202213765075914</epd:amount>
        <epd:referenceToUnitGroupDataSet refObjectId="71b4d617-0ec9-4d3f-b65e-e438940c2401" version="00.00.003" type="unit group data set" uri="../unitgroups/71b4d617-0ec9-4d3f-b65e-e438940c2401.xml">
          <common:shortDescription xml:lang="en">Mole of N eq.</common:shortDescription>
        </epd:referenceToUnitGroupDataSet>
      </common:other>
    </LCIAResult>
    <LCIAResult>
      <referenceToLCIAMethodDataSet refObjectId="b5c610fe-def3-11e6-bf01-fe55135034f3" version="21.01.000" type="LCIA method data set" uri="../lciamethods/b5c610fe-def3-11e6-bf01-fe55135034f3.xml">
        <common:shortDescription xml:lang="en">Photochemical Ozone Creation Potential  (POCP)</common:shortDescription>
        <common:shortDescription xml:lang="de">Bildungspotenzial für troposphärisches Ozon (POCP)</common:shortDescription>
      </referenceToLCIAMethodDataSet>
      <common:other>
        <epd:amount epd:module="B6">0.000472345846867001</epd:amount>
        <epd:referenceToUnitGroupDataSet refObjectId="d27c25f8-fbc1-44c6-b47b-4adbae4199c6" version="00.00.003" type="unit group data set" uri="../unitgroups/d27c25f8-fbc1-44c6-b47b-4adbae4199c6.xml">
          <common:shortDescription xml:lang="en">kg NMVOC eq.</common:shortDescription>
        </epd:referenceToUnitGroupDataSet>
      </common:other>
    </LCIAResult>
    <LCIAResult>
      <referenceToLCIAMethodDataSet refObjectId="b2ad6494-c78d-11e6-9d9d-cec0c932ce01" version="21.01.000" type="LCIA method data set" uri="../lciamethods/b2ad6494-c78d-11e6-9d9d-cec0c932ce01.xml">
        <common:shortDescription xml:lang="en">Abiotic depletion potential - non-fossil resources (ADPE)</common:shortDescription>
        <common:shortDescription xml:lang="de">Potenzial für die Verknappung abiotischer Ressourcen  nicht fossile Ressourcen (ADPE)</common:shortDescription>
      </referenceToLCIAMethodDataSet>
      <common:other>
        <epd:amount epd:module="B6">4.1499432810449E-7</epd:amount>
        <epd:referenceToUnitGroupDataSet refObjectId="54ccd2d9-a32a-4fc2-923d-f2c8c93e89d4" version="25.00.000" type="unit group data set" uri="../unitgroups/54ccd2d9-a32a-4fc2-923d-f2c8c93e89d4.xml">
          <common:shortDescription xml:lang="en">kg Sb eq.</common:shortDescription>
        </epd:referenceToUnitGroupDataSet>
      </common:other>
    </LCIAResult>
    <LCIAResult>
      <referenceToLCIAMethodDataSet refObjectId="b2ad6110-c78d-11e6-9d9d-cec0c932ce01" version="21.01.000" type="LCIA method data set" uri="../lciamethods/b2ad6110-c78d-11e6-9d9d-cec0c932ce01.xml">
        <common:shortDescription xml:lang="en">Abiotic depletion potential - fossil resources (ADPF)</common:shortDescription>
        <common:shortDescription xml:lang="de">Potenzial für die Verknappung abiotischer Ressourcen  fossile Brennstoffe (ADPF)</common:shortDescription>
      </referenceToLCIAMethodDataSet>
      <common:other>
        <epd:amount epd:module="B6">4.14358834215642</epd:amount>
        <epd:referenceToUnitGroupDataSet refObjectId="93a60a57-a3c8-11da-a746-0800200c9a66" version="02.00.000" type="unit group data set" uri="../unitgroups/93a60a57-a3c8-11da-a746-0800200c9a66.xml">
          <common:shortDescription xml:lang="en">MJ</common:shortDescription>
        </epd:referenceToUnitGroupDataSet>
      </common:other>
    </LCIAResult>
    <LCIAResult>
      <referenceToLCIAMethodDataSet refObjectId="b2ad66ce-c78d-11e6-9d9d-cec0c932ce01" version="21.01.000" type="LCIA method data set" uri="../lciamethods/b2ad66ce-c78d-11e6-9d9d-cec0c932ce01.xml">
        <common:shortDescription xml:lang="en">Water (user) deprivation potential (WDP)</common:shortDescription>
        <common:shortDescription xml:lang="de">Wasser-Entzugspotenzial (Benutzer) (WDP)</common:shortDescription>
      </referenceToLCIAMethodDataSet>
      <common:other>
        <epd:amount epd:module="B6">0.0123494509477067</epd:amount>
        <epd:referenceToUnitGroupDataSet refObjectId="6ae2df01-888e-46c8-b17d-49fa3869b476" version="00.00.003" type="unit group data set" uri="../unitgroups/6ae2df01-888e-46c8-b17d-49fa3869b476.xml">
          <common:shortDescription xml:lang="en">m³ world equiv.</common:shortDescription>
        </epd:referenceToUnitGroupDataSet>
      </common:other>
    </LCIAResult>
  </LCIAResults>
</processDataSet>
