<?xml version="1.0" encoding="utf-8"?>
<processDataSet xmlns:epd="http://www.iai.kit.edu/EPD/2013" xmlns:epd2="http://www.indata.network/EPD/2019" xmlns:common="http://lca.jrc.it/ILCD/Common" xsi:schemaLocation="http://lca.jrc.it/ILCD/Process ../../schemas/EPD_DataSet.xsd" epd2:epd-version="1.2" version="1.1" locations="../ILCDLocations.xml" xmlns:xsi="http://www.w3.org/2001/XMLSchema-instance" xmlns="http://lca.jrc.it/ILCD/Process">
<processInformation>
<dataSetInformation>
<common:UUID>53c6478d-357b-4933-947a-46e70babd100</common:UUID>
<name>
<baseName xml:lang="en">PROMATECT®-L / PROMATECT®-L500 / PROMATECT®-AD / VERMICULUX-S</baseName>
<functionalUnitFlowProperties xml:lang="en" />
</name>
<classificationInformation>
<common:classification name="OEKOBAU.DAT">
<common:class level="0" classId="10">Komposite</common:class>
<common:class level="1" classId="10.1">Systembauteile</common:class>
<common:class level="2" classId="10.1.04">Innenwände</common:class>
</common:classification>
<common:classification name="IBUCategories">
<common:class level="0">02 Building products</common:class>
<common:class level="1">Thermal insulation products</common:class>
<common:class level="2">Calcium silicate insulating materials</common:class>
</common:classification>
</classificationInformation>
<common:generalComment xml:lang="en">PROMATECT®-L/-L500/-AD and VERMICULUX-S are lightweight, non-combustible, fire-resisting calcium silicate boards, not sensitive to moisture. All boards are manufactured in the same plant, using the same production technology and similar raw materials though in different quantities.The functional unit refers to a weighted average product based on the ratio of tons produced of the products in the reference year 2019.</common:generalComment>
</dataSetInformation>
<quantitativeReference>
<referenceToReferenceFlow>0</referenceToReferenceFlow>
</quantitativeReference>
<time>
<common:referenceYear>2021</common:referenceYear>
<common:dataSetValidUntil>2026</common:dataSetValidUntil>
<common:other>
<epd2:publicationDateOfEPD>2021-09-06</epd2:publicationDateOfEPD>
</common:other>
</time>
<geography>
<locationOfOperationSupplyOrProduction location="GLO" />
</geography>
<technology>
<technologyDescriptionAndIncludedProcesses xml:lang="en">Sand, water and lime are mixed and blended in a reactor to form calcium silicate. This is combined in a mixer with the other raw materials to form a thick slurry. The slurry is formed to a board in a filter press. Boards are dried, edges are trimmed and the upper surface is sanded to the specific thickness. All material which is cut off or sanded away is fully recycled within the process. The quality management system of the company and the production facility are certified according to ISO 9001:2015. 
Declared unit: 
The functional unit is 1 m² of PROMATECT®-L/-L500/-AD and VERMICULUX-S with a thickness of 30mm. The results for other thicknesses can be obtained by multiplying the presented results by the corresponding adjustment factor as included in the table.This unit refers to a weighted average product based on the ratio of tons produced of all products in the reference year 2019.</technologyDescriptionAndIncludedProcesses>
<technologicalApplicability xml:lang="en">PROMATECT®-L/-L500/-AD and VERMICULUX-S are primarily used in interior building applications where normal to high levels of fire resistance are required. The boards are intended to protect elements or to be used in technical services assemblies.Main application areas are the fire protection of ducts such as cable, ventilation and smoke extraction ducts, fire protection to structural steel and fire protection of mechanical and electrical service enclosures.</technologicalApplicability>
</technology>
</processInformation>
<modellingAndValidation>
<LCIMethodAndAllocation>
<typeOfDataSet>EPD</typeOfDataSet>
<referenceToLCAMethodDetails type="source data set" refObjectId="c6559591-e26c-472f-b872-31b8e24660e7">
<common:shortDescription xml:lang="en">Calcium silicate insulating materials.pdf</common:shortDescription>
</referenceToLCAMethodDetails>
<common:other>
<epd:subType xmlns="http://www.iai.kit.edu/EPD/2013">average dataset</epd:subType>
</common:other>
</LCIMethodAndAllocation>
<dataSourcesTreatmentAndRepresentativeness>
<referenceToDataSource type="source data set" refObjectId="28d74cc0-db8b-4d7e-bc44-5f6d56ce0c4a">
<common:shortDescription xml:lang="en">GaBi Database (all versions)</common:shortDescription>
</referenceToDataSource>
<referenceToDataSource type="source data set" refObjectId="1cece811-7501-44d4-8067-9259bd5cb835">
<common:shortDescription xml:lang="en">GaBi Database Edition 2021, CUP 2021.01</common:shortDescription>
</referenceToDataSource>
<useAdviceForDataSet xml:lang="en">Scope: 
The life cycle assessment is based on production data of PROMATECT®-L/-L500/-AD and VERMICULUX-S of the year 2019 at the production site Tisselt, Belgium. 
System boundary: 
Type of the EPD: cradle to grave.The following life cycle stages and modules are included:Production stage (A1-A3):pre-chains of the raw materials and their transportation to the manufacturing siteenergy consumption during productionrecycling and disposal of production wastesproduction of packagingConstruction stage (A4-A5):transportation of product to the construction sitedisposal of installation wastesincineration of packaging materials (potential benefits from energy substitution within the incineration process are declared in module D)Use stage (B1-B7):efforts for the use of the product, maintenance and operational effortsmodules B3, B4, B5 are declared as MNR (module not relevant) according to the IBU requirement. These modules are defined on building level in generalEnd-of-life stage (C1-C4):transport to disposal of the materiallandfill end-of-life scenario was consideredLoads and benefits beyond system boundary (D):loads and benefits from the recycling of production waste and incineration of packaging waste</useAdviceForDataSet>
<common:other>
<epd2:referenceToOriginalEPD type="source data set" refObjectId="703881bd-8c94-4742-96bd-047effd51ab0">
<common:shortDescription xml:lang="en">PROMATECT®-L / PROMATECT®-L500 / PROMATECT®-AD / VERMICULUX-S.pdf</common:shortDescription>
</epd2:referenceToOriginalEPD>
</common:other>
</dataSourcesTreatmentAndRepresentativeness>
<validation>
<review type="Accredited third party review">
<common:referenceToNameOfReviewerAndInstitution uri="../contacts/d111dbec-b024-4be5-86c5-752d6eb2cf95.xml" type="contact data set" refObjectId="d111dbec-b024-4be5-86c5-752d6eb2cf95">
<common:shortDescription xml:lang="en">Institut Bauen und Umwelt e. V.</common:shortDescription>
</common:referenceToNameOfReviewerAndInstitution>
</review>
</validation>
<complianceDeclarations>
<compliance>
<common:referenceToComplianceSystem uri="../sources/c0016b33-8cf7-415c-ac6e-deba0d21440d.xml" type="source data set" refObjectId="c0016b33-8cf7-415c-ac6e-deba0d21440d">
<common:shortDescription xml:lang="en">DIN EN 15804+A2</common:shortDescription>
</common:referenceToComplianceSystem>
</compliance>
<compliance>
<common:referenceToComplianceSystem uri="../sources/4f2eb655-6e44-4874-a95a-e28f5442cd4d.xml" type="source data set" refObjectId="4f2eb655-6e44-4874-a95a-e28f5442cd4d">
<common:shortDescription xml:lang="en">ISO 14025</common:shortDescription>
</common:referenceToComplianceSystem>
</compliance>
</complianceDeclarations>
</modellingAndValidation>
<administrativeInformation>
<common:commissionerAndGoal>
<common:referenceToCommissioner uri="../contacts/9f15c029-1fb0-467d-8dd1-92b013e91ca8.xml" type="contact data set" refObjectId="9f15c029-1fb0-467d-8dd1-92b013e91ca8">
<common:shortDescription xml:lang="en">Etex Building Performance International</common:shortDescription>
</common:referenceToCommissioner>
</common:commissionerAndGoal>
<dataGenerator>
<common:referenceToPersonOrEntityGeneratingTheDataSet uri="../contacts/119f4128-cc6a-43d5-98e4-aa527a77d939.xml" type="contact data set" refObjectId="119f4128-cc6a-43d5-98e4-aa527a77d939">
<common:shortDescription xml:lang="en">Peggy Van De Velde</common:shortDescription>
</common:referenceToPersonOrEntityGeneratingTheDataSet>
</dataGenerator>
<dataEntryBy>
<common:timeStamp>2021-09-06T17:46:13.499</common:timeStamp>
<common:referenceToDataSetFormat uri="../sources/a97a0155-0234-4b87-b4ce-a45da52f2a40.xml" type="source data set" refObjectId="a97a0155-0234-4b87-b4ce-a45da52f2a40">
<common:shortDescription xml:lang="en">ILCD Format</common:shortDescription>
</common:referenceToDataSetFormat>
<common:referenceToDataSetFormat uri="../sources/a29449fd-aa2f-4de8-b5d7-4b06b43c6fde.xml" type="source data set" refObjectId="a29449fd-aa2f-4de8-b5d7-4b06b43c6fde">
<common:shortDescription xml:lang="de">EPD-Datenformaterweiterungen v1.2</common:shortDescription>
<common:shortDescription xml:lang="en">EPD Data Format Extensions v1.2</common:shortDescription>
</common:referenceToDataSetFormat>
</dataEntryBy>
<publicationAndOwnership>
<common:dataSetVersion>00.05.000</common:dataSetVersion>
<common:referenceToPrecedingDataSetVersion uri="../processes/d25d716b-100e-4b26-9d70-596c7b240f61.xml" type="process data set" refObjectId="d25d716b-100e-4b26-9d70-596c7b240f61">
<common:shortDescription xml:lang="en">PROMATECT®-L / PROMATECT®-L500</common:shortDescription>
</common:referenceToPrecedingDataSetVersion>
<common:referenceToRegistrationAuthority uri="../contacts/d111dbec-b024-4be5-86c5-752d6eb2cf95.xml" type="contact data set" refObjectId="d111dbec-b024-4be5-86c5-752d6eb2cf95">
<common:shortDescription xml:lang="en">Institut Bauen und Umwelt e. V.</common:shortDescription>
</common:referenceToRegistrationAuthority>
<common:registrationNumber>EPD-PMT-20210153-IBC1-EN</common:registrationNumber>
<common:referenceToOwnershipOfDataSet uri="../contacts/9f15c029-1fb0-467d-8dd1-92b013e91ca8.xml" type="contact data set" refObjectId="9f15c029-1fb0-467d-8dd1-92b013e91ca8">
<common:shortDescription xml:lang="en">Etex Building Performance International</common:shortDescription>
</common:referenceToOwnershipOfDataSet>
<common:copyright>true</common:copyright>
<common:licenseType>Free of charge for all users and uses</common:licenseType>
<common:accessRestrictions xml:lang="en">None</common:accessRestrictions>
<common:other>
<epd2:referenceToPublisher type="contact data set" refObjectId="d111dbec-b024-4be5-86c5-752d6eb2cf95" uri="../contacts/d111dbec-b024-4be5-86c5-752d6eb2cf95.xml">
<common:shortDescription xml:lang="en">Institut Bauen und Umwelt e. V.</common:shortDescription>
</epd2:referenceToPublisher>
</common:other>
</publicationAndOwnership>
</administrativeInformation>
<exchanges>
<exchange dataSetInternalID="0">
<referenceToFlowDataSet uri="../flows/25905b1c-c27f-27e3-5168-4bd1b0f9cac6.xml" type="flow data set" refObjectId="25905b1c-c27f-27e3-5168-4bd1b0f9cac6">
<common:shortDescription xml:lang="en">30mm PROMATECT®-L/-L500/-AD and VERMICULUX S (30mm PROMATECT®-L/-L500/-AD and VERMICULUX S)</common:shortDescription>
</referenceToFlowDataSet>
<meanAmount>1</meanAmount>
<referencesToDataSource />
</exchange>
<exchange dataSetInternalID="1">
<referenceToFlowDataSet uri="../flows/20f32be5-0398-4288-9b6d-accddd195317.xml" type="flow data set" refObjectId="20f32be5-0398-4288-9b6d-accddd195317">
<common:shortDescription xml:lang="en">Renewable primary energy as energy carrier (PERE)</common:shortDescription>
</referenceToFlowDataSet>
<functionType>General reminder flow</functionType>
<exchangeDirection>Input</exchangeDirection>
<common:other>
<epd:referenceToUnitGroupDataSet uri="../unitgroups/93a60a57-a3c8-11da-a746-0800200c9a66.xml" type="unit group data set" refObjectId="93a60a57-a3c8-11da-a746-0800200c9a66">
<common:shortDescription xml:lang="en">MJ</common:shortDescription>
</epd:referenceToUnitGroupDataSet>
<epd:amount epd:module="A1">17.2165090101377</epd:amount>
<epd:amount epd:module="A2">0.0499765734792531</epd:amount>
<epd:amount epd:module="A3">15.4225116929377</epd:amount>
<epd:amount epd:module="A4">0.0777708232974478</epd:amount>
<epd:amount epd:module="A5">13.5442473837812</epd:amount>
<epd:amount epd:module="B1">0</epd:amount>
<epd:amount epd:module="B2">0</epd:amount>
<epd:amount epd:module="B6">0</epd:amount>
<epd:amount epd:module="B7">0</epd:amount>
<epd:amount epd:module="C1">0</epd:amount>
<epd:amount epd:module="C2">0.0744293989737253</epd:amount>
<epd:amount epd:module="C3">0</epd:amount>
<epd:amount epd:module="C4">2.64619388505229</epd:amount>
<epd:amount epd:module="D">-1.61993171582342</epd:amount>
</common:other>
</exchange>
<exchange dataSetInternalID="2">
<referenceToFlowDataSet uri="../flows/fb3ec0de-548d-4508-aea5-00b73bf6f702.xml" type="flow data set" refObjectId="fb3ec0de-548d-4508-aea5-00b73bf6f702">
<common:shortDescription xml:lang="en">Renewable primary energy resources as material utilization (PERM)</common:shortDescription>
</referenceToFlowDataSet>
<functionType>General reminder flow</functionType>
<exchangeDirection>Input</exchangeDirection>
<common:other>
<epd:referenceToUnitGroupDataSet uri="../unitgroups/93a60a57-a3c8-11da-a746-0800200c9a66.xml" type="unit group data set" refObjectId="93a60a57-a3c8-11da-a746-0800200c9a66">
<common:shortDescription xml:lang="en">MJ</common:shortDescription>
</epd:referenceToUnitGroupDataSet>
<epd:amount epd:module="A1">3.0573574762634</epd:amount>
<epd:amount epd:module="A2">0</epd:amount>
<epd:amount epd:module="A3">10.9910248392037</epd:amount>
<epd:amount epd:module="A4">0</epd:amount>
<epd:amount epd:module="A5">-11.1299888842266</epd:amount>
<epd:amount epd:module="B1">0</epd:amount>
<epd:amount epd:module="B2">0</epd:amount>
<epd:amount epd:module="B6">0</epd:amount>
<epd:amount epd:module="B7">0</epd:amount>
<epd:amount epd:module="C1">0</epd:amount>
<epd:amount epd:module="C2">0</epd:amount>
<epd:amount epd:module="C3">0</epd:amount>
<epd:amount epd:module="C4">-2.2491</epd:amount>
<epd:amount epd:module="D">0</epd:amount>
</common:other>
</exchange>
<exchange dataSetInternalID="3">
<referenceToFlowDataSet uri="../flows/53f97275-fa8a-4cdd-9024-65936002acd0.xml" type="flow data set" refObjectId="53f97275-fa8a-4cdd-9024-65936002acd0">
<common:shortDescription xml:lang="en">Total use of renewable primary energy resources (PERT)</common:shortDescription>
</referenceToFlowDataSet>
<functionType>General reminder flow</functionType>
<exchangeDirection>Input</exchangeDirection>
<common:other>
<epd:referenceToUnitGroupDataSet uri="../unitgroups/93a60a57-a3c8-11da-a746-0800200c9a66.xml" type="unit group data set" refObjectId="93a60a57-a3c8-11da-a746-0800200c9a66">
<common:shortDescription xml:lang="en">MJ</common:shortDescription>
</epd:referenceToUnitGroupDataSet>
<epd:amount epd:module="A1">20.2738664864011</epd:amount>
<epd:amount epd:module="A2">0.0499765734792531</epd:amount>
<epd:amount epd:module="A3">26.4135365321414</epd:amount>
<epd:amount epd:module="A4">0.0777708232974478</epd:amount>
<epd:amount epd:module="A5">2.41425849955453</epd:amount>
<epd:amount epd:module="B1">0</epd:amount>
<epd:amount epd:module="B2">0</epd:amount>
<epd:amount epd:module="B6">0</epd:amount>
<epd:amount epd:module="B7">0</epd:amount>
<epd:amount epd:module="C1">0</epd:amount>
<epd:amount epd:module="C2">0.0744293989737253</epd:amount>
<epd:amount epd:module="C3">0</epd:amount>
<epd:amount epd:module="C4">0.39709388505229</epd:amount>
<epd:amount epd:module="D">-1.61993171582342</epd:amount>
</common:other>
</exchange>
<exchange dataSetInternalID="4">
<referenceToFlowDataSet uri="../flows/ac857178-2b45-46ec-892a-a9a4332f0372.xml" type="flow data set" refObjectId="ac857178-2b45-46ec-892a-a9a4332f0372">
<common:shortDescription xml:lang="en">Non renewable primary energy as energy carrier (PENRE)</common:shortDescription>
</referenceToFlowDataSet>
<functionType>General reminder flow</functionType>
<exchangeDirection>Input</exchangeDirection>
<common:other>
<epd:referenceToUnitGroupDataSet uri="../unitgroups/93a60a57-a3c8-11da-a746-0800200c9a66.xml" type="unit group data set" refObjectId="93a60a57-a3c8-11da-a746-0800200c9a66">
<common:shortDescription xml:lang="en">MJ</common:shortDescription>
</epd:referenceToUnitGroupDataSet>
<epd:amount epd:module="A1">65.1332207519764</epd:amount>
<epd:amount epd:module="A2">1.48769627838391</epd:amount>
<epd:amount epd:module="A3">198.265547898623</epd:amount>
<epd:amount epd:module="A4">1.35645896985338</epd:amount>
<epd:amount epd:module="A5">13.8398221338075</epd:amount>
<epd:amount epd:module="B1">0</epd:amount>
<epd:amount epd:module="B2">0</epd:amount>
<epd:amount epd:module="B6">0</epd:amount>
<epd:amount epd:module="B7">0</epd:amount>
<epd:amount epd:module="C1">0</epd:amount>
<epd:amount epd:module="C2">1.29817869450302</epd:amount>
<epd:amount epd:module="C3">0</epd:amount>
<epd:amount epd:module="C4">2.9504181092041</epd:amount>
<epd:amount epd:module="D">-7.14420333624457</epd:amount>
</common:other>
</exchange>
<exchange dataSetInternalID="5">
<referenceToFlowDataSet uri="../flows/1421caa0-679d-4bf4-b282-0eb850ccae27.xml" type="flow data set" refObjectId="1421caa0-679d-4bf4-b282-0eb850ccae27">
<common:shortDescription xml:lang="en">Non renewable primary energy as material utilization (PENRM)</common:shortDescription>
</referenceToFlowDataSet>
<functionType>General reminder flow</functionType>
<exchangeDirection>Input</exchangeDirection>
<common:other>
<epd:referenceToUnitGroupDataSet uri="../unitgroups/93a60a57-a3c8-11da-a746-0800200c9a66.xml" type="unit group data set" refObjectId="93a60a57-a3c8-11da-a746-0800200c9a66">
<common:shortDescription xml:lang="en">MJ</common:shortDescription>
</epd:referenceToUnitGroupDataSet>
<epd:amount epd:module="A1">0</epd:amount>
<epd:amount epd:module="A2">0</epd:amount>
<epd:amount epd:module="A3">0.09744</epd:amount>
<epd:amount epd:module="A4">0</epd:amount>
<epd:amount epd:module="A5">-0.09744</epd:amount>
<epd:amount epd:module="B1">0</epd:amount>
<epd:amount epd:module="B2">0</epd:amount>
<epd:amount epd:module="B6">0</epd:amount>
<epd:amount epd:module="B7">0</epd:amount>
<epd:amount epd:module="C1">0</epd:amount>
<epd:amount epd:module="C2">0</epd:amount>
<epd:amount epd:module="C3">0</epd:amount>
<epd:amount epd:module="C4">0</epd:amount>
<epd:amount epd:module="D">0</epd:amount>
</common:other>
</exchange>
<exchange dataSetInternalID="6">
<referenceToFlowDataSet uri="../flows/06159210-646b-4c8d-8583-da9b3b95a6c1.xml" type="flow data set" refObjectId="06159210-646b-4c8d-8583-da9b3b95a6c1">
<common:shortDescription xml:lang="en">Total use of non renewable primary energy resources (PENRT)</common:shortDescription>
</referenceToFlowDataSet>
<functionType>General reminder flow</functionType>
<exchangeDirection>Input</exchangeDirection>
<common:other>
<epd:referenceToUnitGroupDataSet uri="../unitgroups/93a60a57-a3c8-11da-a746-0800200c9a66.xml" type="unit group data set" refObjectId="93a60a57-a3c8-11da-a746-0800200c9a66">
<common:shortDescription xml:lang="en">MJ</common:shortDescription>
</epd:referenceToUnitGroupDataSet>
<epd:amount epd:module="A1">65.1332207519824</epd:amount>
<epd:amount epd:module="A2">1.48769627838392</epd:amount>
<epd:amount epd:module="A3">198.362987898628</epd:amount>
<epd:amount epd:module="A4">1.35645896985339</epd:amount>
<epd:amount epd:module="A5">13.742382133808</epd:amount>
<epd:amount epd:module="B1">0</epd:amount>
<epd:amount epd:module="B2">0</epd:amount>
<epd:amount epd:module="B6">0</epd:amount>
<epd:amount epd:module="B7">0</epd:amount>
<epd:amount epd:module="C1">0</epd:amount>
<epd:amount epd:module="C2">1.29817869450303</epd:amount>
<epd:amount epd:module="C3">0</epd:amount>
<epd:amount epd:module="C4">2.95041810920415</epd:amount>
<epd:amount epd:module="D">-7.14420333624482</epd:amount>
</common:other>
</exchange>
<exchange dataSetInternalID="7">
<referenceToFlowDataSet uri="../flows/c6a1f35f-2d09-4f54-8dfb-97e502e1ce92.xml" type="flow data set" refObjectId="c6a1f35f-2d09-4f54-8dfb-97e502e1ce92">
<common:shortDescription xml:lang="en">Use of secondary material (SM)</common:shortDescription>
</referenceToFlowDataSet>
<functionType>General reminder flow</functionType>
<exchangeDirection>Input</exchangeDirection>
<common:other>
<epd:referenceToUnitGroupDataSet uri="../unitgroups/ad38d542-3fe9-439d-9b95-2f5f7752acaf.xml" type="unit group data set" refObjectId="ad38d542-3fe9-439d-9b95-2f5f7752acaf">
<common:shortDescription xml:lang="en">kg</common:shortDescription>
</epd:referenceToUnitGroupDataSet>
<epd:amount epd:module="A1">1.92806370597243</epd:amount>
<epd:amount epd:module="A2">0</epd:amount>
<epd:amount epd:module="A3">0</epd:amount>
<epd:amount epd:module="A4">0</epd:amount>
<epd:amount epd:module="A5">0.0964031852986217</epd:amount>
<epd:amount epd:module="B1">0</epd:amount>
<epd:amount epd:module="B2">0</epd:amount>
<epd:amount epd:module="B6">0</epd:amount>
<epd:amount epd:module="B7">0</epd:amount>
<epd:amount epd:module="C1">0</epd:amount>
<epd:amount epd:module="C2">0</epd:amount>
<epd:amount epd:module="C3">0</epd:amount>
<epd:amount epd:module="C4">0</epd:amount>
<epd:amount epd:module="D">0</epd:amount>
</common:other>
</exchange>
<exchange dataSetInternalID="8">
<referenceToFlowDataSet uri="../flows/64333088-a55f-4aa2-9a31-c10b07816787.xml" type="flow data set" refObjectId="64333088-a55f-4aa2-9a31-c10b07816787">
<common:shortDescription xml:lang="en">Use of renewable secondary fuels (RSF)</common:shortDescription>
</referenceToFlowDataSet>
<functionType>General reminder flow</functionType>
<exchangeDirection>Input</exchangeDirection>
<common:other>
<epd:referenceToUnitGroupDataSet uri="../unitgroups/93a60a57-a3c8-11da-a746-0800200c9a66.xml" type="unit group data set" refObjectId="93a60a57-a3c8-11da-a746-0800200c9a66">
<common:shortDescription xml:lang="en">MJ</common:shortDescription>
</epd:referenceToUnitGroupDataSet>
<epd:amount epd:module="A1">0</epd:amount>
<epd:amount epd:module="A2">0</epd:amount>
<epd:amount epd:module="A3">0</epd:amount>
<epd:amount epd:module="A4">0</epd:amount>
<epd:amount epd:module="A5">0</epd:amount>
<epd:amount epd:module="B1">0</epd:amount>
<epd:amount epd:module="B2">0</epd:amount>
<epd:amount epd:module="B6">0</epd:amount>
<epd:amount epd:module="B7">0</epd:amount>
<epd:amount epd:module="C1">0</epd:amount>
<epd:amount epd:module="C2">0</epd:amount>
<epd:amount epd:module="C3">0</epd:amount>
<epd:amount epd:module="C4">0</epd:amount>
<epd:amount epd:module="D">0</epd:amount>
</common:other>
</exchange>
<exchange dataSetInternalID="9">
<referenceToFlowDataSet uri="../flows/89def144-d39a-4287-b86f-efde453ddcb2.xml" type="flow data set" refObjectId="89def144-d39a-4287-b86f-efde453ddcb2">
<common:shortDescription xml:lang="en">Use of non renewable secondary fuels (NRSF)</common:shortDescription>
</referenceToFlowDataSet>
<functionType>General reminder flow</functionType>
<exchangeDirection>Input</exchangeDirection>
<common:other>
<epd:referenceToUnitGroupDataSet uri="../unitgroups/93a60a57-a3c8-11da-a746-0800200c9a66.xml" type="unit group data set" refObjectId="93a60a57-a3c8-11da-a746-0800200c9a66">
<common:shortDescription xml:lang="en">MJ</common:shortDescription>
</epd:referenceToUnitGroupDataSet>
<epd:amount epd:module="A1">0</epd:amount>
<epd:amount epd:module="A2">0</epd:amount>
<epd:amount epd:module="A3">0</epd:amount>
<epd:amount epd:module="A4">0</epd:amount>
<epd:amount epd:module="A5">0</epd:amount>
<epd:amount epd:module="B1">0</epd:amount>
<epd:amount epd:module="B2">0</epd:amount>
<epd:amount epd:module="B6">0</epd:amount>
<epd:amount epd:module="B7">0</epd:amount>
<epd:amount epd:module="C1">0</epd:amount>
<epd:amount epd:module="C2">0</epd:amount>
<epd:amount epd:module="C3">0</epd:amount>
<epd:amount epd:module="C4">0</epd:amount>
<epd:amount epd:module="D">0</epd:amount>
</common:other>
</exchange>
<exchange dataSetInternalID="10">
<referenceToFlowDataSet uri="../flows/3cf952c8-f3a4-461d-8c96-96456ca62246.xml" type="flow data set" refObjectId="3cf952c8-f3a4-461d-8c96-96456ca62246">
<common:shortDescription xml:lang="en">Use of net fresh water (FW)</common:shortDescription>
</referenceToFlowDataSet>
<functionType>General reminder flow</functionType>
<exchangeDirection>Input</exchangeDirection>
<common:other>
<epd:referenceToUnitGroupDataSet uri="../unitgroups/cd950537-0a98-4044-9ba7-9f9a68d0a504.xml" type="unit group data set" refObjectId="cd950537-0a98-4044-9ba7-9f9a68d0a504">
<common:shortDescription xml:lang="en">m^3</common:shortDescription>
</epd:referenceToUnitGroupDataSet>
<epd:amount epd:module="A1">0.0136849229777392</epd:amount>
<epd:amount epd:module="A2">5.83247071758945E-05</epd:amount>
<epd:amount epd:module="A3">0.0712227859767896</epd:amount>
<epd:amount epd:module="A4">8.90727774936675E-05</epd:amount>
<epd:amount epd:module="A5">0.00731734381283938</epd:amount>
<epd:amount epd:module="B1">0</epd:amount>
<epd:amount epd:module="B2">0</epd:amount>
<epd:amount epd:module="B6">0</epd:amount>
<epd:amount epd:module="B7">0</epd:amount>
<epd:amount epd:module="C1">0</epd:amount>
<epd:amount epd:module="C2">8.52457645769958E-05</epd:amount>
<epd:amount epd:module="C3">0</epd:amount>
<epd:amount epd:module="C4">0.0007276975953803</epd:amount>
<epd:amount epd:module="D">-0.00158094045637391</epd:amount>
</common:other>
</exchange>
<exchange dataSetInternalID="11">
<referenceToFlowDataSet uri="../flows/430f9e0f-59b2-46a0-8e0d-55e0e84948fc.xml" type="flow data set" refObjectId="430f9e0f-59b2-46a0-8e0d-55e0e84948fc">
<common:shortDescription xml:lang="en">Hazardous waste disposed (HWD)</common:shortDescription>
</referenceToFlowDataSet>
<functionType>General reminder flow</functionType>
<exchangeDirection>Output</exchangeDirection>
<common:other>
<epd:referenceToUnitGroupDataSet uri="../unitgroups/ad38d542-3fe9-439d-9b95-2f5f7752acaf.xml" type="unit group data set" refObjectId="ad38d542-3fe9-439d-9b95-2f5f7752acaf">
<common:shortDescription xml:lang="en">kg</common:shortDescription>
</epd:referenceToUnitGroupDataSet>
<epd:amount epd:module="A1">0.00112</epd:amount>
<epd:amount epd:module="A2">4.89E-11</epd:amount>
<epd:amount epd:module="A3">4.76E-08</epd:amount>
<epd:amount epd:module="A4">7.15E-11</epd:amount>
<epd:amount epd:module="A5">5.6E-05</epd:amount>
<epd:amount epd:module="B1">0</epd:amount>
<epd:amount epd:module="B2">0</epd:amount>
<epd:amount epd:module="B6">0</epd:amount>
<epd:amount epd:module="B7">0</epd:amount>
<epd:amount epd:module="C1">0</epd:amount>
<epd:amount epd:module="C2">6.84E-11</epd:amount>
<epd:amount epd:module="C3">0</epd:amount>
<epd:amount epd:module="C4">3.13E-10</epd:amount>
<epd:amount epd:module="D">-1.61E-09</epd:amount>
</common:other>
</exchange>
<exchange dataSetInternalID="12">
<referenceToFlowDataSet uri="../flows/b29ef66b-e286-4afa-949f-62f1a7b4d7fa.xml" type="flow data set" refObjectId="b29ef66b-e286-4afa-949f-62f1a7b4d7fa">
<common:shortDescription xml:lang="en">Non hazardous waste disposed (NHWD)</common:shortDescription>
</referenceToFlowDataSet>
<functionType>General reminder flow</functionType>
<exchangeDirection>Output</exchangeDirection>
<common:other>
<epd:referenceToUnitGroupDataSet uri="../unitgroups/ad38d542-3fe9-439d-9b95-2f5f7752acaf.xml" type="unit group data set" refObjectId="ad38d542-3fe9-439d-9b95-2f5f7752acaf">
<common:shortDescription xml:lang="en">kg</common:shortDescription>
</epd:referenceToUnitGroupDataSet>
<epd:amount epd:module="A1">0.35</epd:amount>
<epd:amount epd:module="A2">0.000196</epd:amount>
<epd:amount epd:module="A3">1.07</epd:amount>
<epd:amount epd:module="A4">0.000213</epd:amount>
<epd:amount epd:module="A5">0.819</epd:amount>
<epd:amount epd:module="B1">0</epd:amount>
<epd:amount epd:module="B2">0</epd:amount>
<epd:amount epd:module="B6">0</epd:amount>
<epd:amount epd:module="B7">0</epd:amount>
<epd:amount epd:module="C1">0</epd:amount>
<epd:amount epd:module="C2">0.000204</epd:amount>
<epd:amount epd:module="C3">0</epd:amount>
<epd:amount epd:module="C4">14.7</epd:amount>
<epd:amount epd:module="D">-0.00336</epd:amount>
</common:other>
</exchange>
<exchange dataSetInternalID="13">
<referenceToFlowDataSet uri="../flows/3449546e-52ad-4b39-b809-9fb77cea8ff6.xml" type="flow data set" refObjectId="3449546e-52ad-4b39-b809-9fb77cea8ff6">
<common:shortDescription xml:lang="en">Radioactive waste disposed (RWD)</common:shortDescription>
</referenceToFlowDataSet>
<functionType>General reminder flow</functionType>
<exchangeDirection>Output</exchangeDirection>
<common:other>
<epd:referenceToUnitGroupDataSet uri="../unitgroups/ad38d542-3fe9-439d-9b95-2f5f7752acaf.xml" type="unit group data set" refObjectId="ad38d542-3fe9-439d-9b95-2f5f7752acaf">
<common:shortDescription xml:lang="en">kg</common:shortDescription>
</epd:referenceToUnitGroupDataSet>
<epd:amount epd:module="A1">0.00233</epd:amount>
<epd:amount epd:module="A2">2.24E-06</epd:amount>
<epd:amount epd:module="A3">0.00114</epd:amount>
<epd:amount epd:module="A4">2.46E-06</epd:amount>
<epd:amount epd:module="A5">0.00019</epd:amount>
<epd:amount epd:module="B1">0</epd:amount>
<epd:amount epd:module="B2">0</epd:amount>
<epd:amount epd:module="B6">0</epd:amount>
<epd:amount epd:module="B7">0</epd:amount>
<epd:amount epd:module="C1">0</epd:amount>
<epd:amount epd:module="C2">2.35E-06</epd:amount>
<epd:amount epd:module="C3">0</epd:amount>
<epd:amount epd:module="C4">3.09E-05</epd:amount>
<epd:amount epd:module="D">-0.000521</epd:amount>
</common:other>
</exchange>
<exchange dataSetInternalID="14">
<referenceToFlowDataSet uri="../flows/a2b32f97-3fc7-4af2-b209-525bc6426f33.xml" type="flow data set" refObjectId="a2b32f97-3fc7-4af2-b209-525bc6426f33">
<common:shortDescription xml:lang="en">Components for re-use (CRU)</common:shortDescription>
</referenceToFlowDataSet>
<functionType>General reminder flow</functionType>
<exchangeDirection>Output</exchangeDirection>
<common:other>
<epd:referenceToUnitGroupDataSet uri="../unitgroups/ad38d542-3fe9-439d-9b95-2f5f7752acaf.xml" type="unit group data set" refObjectId="ad38d542-3fe9-439d-9b95-2f5f7752acaf">
<common:shortDescription xml:lang="en">kg</common:shortDescription>
</epd:referenceToUnitGroupDataSet>
<epd:amount epd:module="A1">0</epd:amount>
<epd:amount epd:module="A2">0</epd:amount>
<epd:amount epd:module="A3">0</epd:amount>
<epd:amount epd:module="A4">0</epd:amount>
<epd:amount epd:module="A5">0</epd:amount>
<epd:amount epd:module="B1">0</epd:amount>
<epd:amount epd:module="B2">0</epd:amount>
<epd:amount epd:module="B6">0</epd:amount>
<epd:amount epd:module="B7">0</epd:amount>
<epd:amount epd:module="C1">0</epd:amount>
<epd:amount epd:module="C2">0</epd:amount>
<epd:amount epd:module="C3">0</epd:amount>
<epd:amount epd:module="C4">0</epd:amount>
<epd:amount epd:module="D">0</epd:amount>
</common:other>
</exchange>
<exchange dataSetInternalID="15">
<referenceToFlowDataSet uri="../flows/d7fe48a5-4103-49c8-9aae-b0b5dfdbd6ae.xml" type="flow data set" refObjectId="d7fe48a5-4103-49c8-9aae-b0b5dfdbd6ae">
<common:shortDescription xml:lang="en">Materials for recycling (MFR)</common:shortDescription>
</referenceToFlowDataSet>
<functionType>General reminder flow</functionType>
<exchangeDirection>Output</exchangeDirection>
<common:other>
<epd:referenceToUnitGroupDataSet uri="../unitgroups/ad38d542-3fe9-439d-9b95-2f5f7752acaf.xml" type="unit group data set" refObjectId="ad38d542-3fe9-439d-9b95-2f5f7752acaf">
<common:shortDescription xml:lang="en">kg</common:shortDescription>
</epd:referenceToUnitGroupDataSet>
<epd:amount epd:module="A1">0</epd:amount>
<epd:amount epd:module="A2">0</epd:amount>
<epd:amount epd:module="A3">0.144</epd:amount>
<epd:amount epd:module="A4">0</epd:amount>
<epd:amount epd:module="A5">0.0072</epd:amount>
<epd:amount epd:module="B1">0</epd:amount>
<epd:amount epd:module="B2">0</epd:amount>
<epd:amount epd:module="B6">0</epd:amount>
<epd:amount epd:module="B7">0</epd:amount>
<epd:amount epd:module="C1">0</epd:amount>
<epd:amount epd:module="C2">0</epd:amount>
<epd:amount epd:module="C3">0</epd:amount>
<epd:amount epd:module="C4">0</epd:amount>
<epd:amount epd:module="D">0</epd:amount>
</common:other>
</exchange>
<exchange dataSetInternalID="16">
<referenceToFlowDataSet uri="../flows/59a9181c-3aaf-46ee-8b13-2b3723b6e447.xml" type="flow data set" refObjectId="59a9181c-3aaf-46ee-8b13-2b3723b6e447">
<common:shortDescription xml:lang="en">Materials for energy recovery (MER)</common:shortDescription>
</referenceToFlowDataSet>
<functionType>General reminder flow</functionType>
<exchangeDirection>Output</exchangeDirection>
<common:other>
<epd:referenceToUnitGroupDataSet uri="../unitgroups/ad38d542-3fe9-439d-9b95-2f5f7752acaf.xml" type="unit group data set" refObjectId="ad38d542-3fe9-439d-9b95-2f5f7752acaf">
<common:shortDescription xml:lang="en">kg</common:shortDescription>
</epd:referenceToUnitGroupDataSet>
<epd:amount epd:module="A1">0</epd:amount>
<epd:amount epd:module="A2">0</epd:amount>
<epd:amount epd:module="A3">0</epd:amount>
<epd:amount epd:module="A4">0</epd:amount>
<epd:amount epd:module="A5">0</epd:amount>
<epd:amount epd:module="B1">0</epd:amount>
<epd:amount epd:module="B2">0</epd:amount>
<epd:amount epd:module="B6">0</epd:amount>
<epd:amount epd:module="B7">0</epd:amount>
<epd:amount epd:module="C1">0</epd:amount>
<epd:amount epd:module="C2">0</epd:amount>
<epd:amount epd:module="C3">0</epd:amount>
<epd:amount epd:module="C4">0</epd:amount>
<epd:amount epd:module="D">0</epd:amount>
</common:other>
</exchange>
<exchange dataSetInternalID="17">
<referenceToFlowDataSet uri="../flows/4da0c987-2b76-40d6-9e9e-82a017aaaf29.xml" type="flow data set" refObjectId="4da0c987-2b76-40d6-9e9e-82a017aaaf29">
<common:shortDescription xml:lang="en">Exported electrical energy (EEE)</common:shortDescription>
</referenceToFlowDataSet>
<functionType>General reminder flow</functionType>
<exchangeDirection>Output</exchangeDirection>
<common:other>
<epd:referenceToUnitGroupDataSet uri="../unitgroups/93a60a57-a3c8-11da-a746-0800200c9a66.xml" type="unit group data set" refObjectId="93a60a57-a3c8-11da-a746-0800200c9a66">
<common:shortDescription xml:lang="en">MJ</common:shortDescription>
</epd:referenceToUnitGroupDataSet>
<epd:amount epd:module="A1">0</epd:amount>
<epd:amount epd:module="A2">0</epd:amount>
<epd:amount epd:module="A3">0.000211</epd:amount>
<epd:amount epd:module="A4">0</epd:amount>
<epd:amount epd:module="A5">1.77</epd:amount>
<epd:amount epd:module="B1">0</epd:amount>
<epd:amount epd:module="B2">0</epd:amount>
<epd:amount epd:module="B6">0</epd:amount>
<epd:amount epd:module="B7">0</epd:amount>
<epd:amount epd:module="C1">0</epd:amount>
<epd:amount epd:module="C2">0</epd:amount>
<epd:amount epd:module="C3">0</epd:amount>
<epd:amount epd:module="C4">0</epd:amount>
<epd:amount epd:module="D">0</epd:amount>
</common:other>
</exchange>
<exchange dataSetInternalID="18">
<referenceToFlowDataSet uri="../flows/98daf38a-7a79-46d3-9a37-2b7bd0955810.xml" type="flow data set" refObjectId="98daf38a-7a79-46d3-9a37-2b7bd0955810">
<common:shortDescription xml:lang="en">Exported thermal energy (EET)</common:shortDescription>
</referenceToFlowDataSet>
<functionType>General reminder flow</functionType>
<exchangeDirection>Output</exchangeDirection>
<common:other>
<epd:referenceToUnitGroupDataSet uri="../unitgroups/93a60a57-a3c8-11da-a746-0800200c9a66.xml" type="unit group data set" refObjectId="93a60a57-a3c8-11da-a746-0800200c9a66">
<common:shortDescription xml:lang="en">MJ</common:shortDescription>
</epd:referenceToUnitGroupDataSet>
<epd:amount epd:module="A1">0</epd:amount>
<epd:amount epd:module="A2">0</epd:amount>
<epd:amount epd:module="A3">0.000487</epd:amount>
<epd:amount epd:module="A4">0</epd:amount>
<epd:amount epd:module="A5">3.2</epd:amount>
<epd:amount epd:module="B1">0</epd:amount>
<epd:amount epd:module="B2">0</epd:amount>
<epd:amount epd:module="B6">0</epd:amount>
<epd:amount epd:module="B7">0</epd:amount>
<epd:amount epd:module="C1">0</epd:amount>
<epd:amount epd:module="C2">0</epd:amount>
<epd:amount epd:module="C3">0</epd:amount>
<epd:amount epd:module="C4">0</epd:amount>
<epd:amount epd:module="D">0</epd:amount>
</common:other>
</exchange>
</exchanges>
<LCIAResults>
<LCIAResult>
<referenceToLCIAMethodDataSet uri="../lciamethods/6a37f984-a4b3-458a-a20a-64418c145fa2.xml" type="LCIA method data set" refObjectId="6a37f984-a4b3-458a-a20a-64418c145fa2">
<common:shortDescription xml:lang="en">Global Warming Potential total (GWP-total)</common:shortDescription>
</referenceToLCIAMethodDataSet>
<common:other>
<epd:referenceToUnitGroupDataSet uri="../unitgroups/1ebf3012-d0db-4de2-aefd-ef30cedb0be1.xml" type="unit group data set" refObjectId="1ebf3012-d0db-4de2-aefd-ef30cedb0be1">
<common:shortDescription xml:lang="en">kg CO_(2)-Äq.</common:shortDescription>
</epd:referenceToUnitGroupDataSet>
<epd:amount epd:module="A1">9.58691629805337</epd:amount>
<epd:amount epd:module="A2">0.116841625624031</epd:amount>
<epd:amount epd:module="A3">11.0203806797841</epd:amount>
<epd:amount epd:module="A4">0.102278212331828</epd:amount>
<epd:amount epd:module="A5">2.27899176173866</epd:amount>
<epd:amount epd:module="B1">0</epd:amount>
<epd:amount epd:module="B2">0</epd:amount>
<epd:amount epd:module="B6">0</epd:amount>
<epd:amount epd:module="B7">0</epd:amount>
<epd:amount epd:module="C1">0</epd:amount>
<epd:amount epd:module="C2">0.0978838277543967</epd:amount>
<epd:amount epd:module="C3">0</epd:amount>
<epd:amount epd:module="C4">0.216472175840232</epd:amount>
<epd:amount epd:module="D">-0.41408257624149</epd:amount>
</common:other>
</LCIAResult>
<LCIAResult>
<referenceToLCIAMethodDataSet uri="../lciamethods/5f635281-343e-44fb-83df-1971b155e6b6.xml" type="LCIA method data set" refObjectId="5f635281-343e-44fb-83df-1971b155e6b6">
<common:shortDescription xml:lang="en">Global Warming Potential fossil fuels (GWP-fossil)</common:shortDescription>
</referenceToLCIAMethodDataSet>
<common:other>
<epd:referenceToUnitGroupDataSet uri="../unitgroups/1ebf3012-d0db-4de2-aefd-ef30cedb0be1.xml" type="unit group data set" refObjectId="1ebf3012-d0db-4de2-aefd-ef30cedb0be1">
<common:shortDescription xml:lang="en">kg CO_(2)-Äq.</common:shortDescription>
</epd:referenceToUnitGroupDataSet>
<epd:amount epd:module="A1">9.77998943361015</epd:amount>
<epd:amount epd:module="A2">0.116334627432829</epd:amount>
<epd:amount epd:module="A3">12.0146215268875</epd:amount>
<epd:amount epd:module="A4">0.101569680396667</epd:amount>
<epd:amount epd:module="A5">1.13985137056866</epd:amount>
<epd:amount epd:module="B1">0</epd:amount>
<epd:amount epd:module="B2">0</epd:amount>
<epd:amount epd:module="B6">0</epd:amount>
<epd:amount epd:module="B7">0</epd:amount>
<epd:amount epd:module="C1">0</epd:amount>
<epd:amount epd:module="C2">0.0972057379020361</epd:amount>
<epd:amount epd:module="C3">0</epd:amount>
<epd:amount epd:module="C4">0.222278408371024</epd:amount>
<epd:amount epd:module="D">-0.411756428801807</epd:amount>
</common:other>
</LCIAResult>
<LCIAResult>
<referenceToLCIAMethodDataSet uri="../lciamethods/2356e1ab-0185-4db5-86e5-16de51c7485c.xml" type="LCIA method data set" refObjectId="2356e1ab-0185-4db5-86e5-16de51c7485c">
<common:shortDescription xml:lang="en">Global Warming Potential biogenic (GWP-biogenic)</common:shortDescription>
</referenceToLCIAMethodDataSet>
<common:other>
<epd:referenceToUnitGroupDataSet uri="../unitgroups/1ebf3012-d0db-4de2-aefd-ef30cedb0be1.xml" type="unit group data set" refObjectId="1ebf3012-d0db-4de2-aefd-ef30cedb0be1">
<common:shortDescription xml:lang="en">kg CO_(2)-Äq.</common:shortDescription>
</epd:referenceToUnitGroupDataSet>
<epd:amount epd:module="A1">-0.197864433352997</epd:amount>
<epd:amount epd:module="A2">-3.12416474546051E-06</epd:amount>
<epd:amount epd:module="A3">-0.995812470690095</epd:amount>
<epd:amount epd:module="A4">-0.000120856844218336</epd:amount>
<epd:amount epd:module="A5">1.13871018471056</epd:amount>
<epd:amount epd:module="B1">0</epd:amount>
<epd:amount epd:module="B2">0</epd:amount>
<epd:amount epd:module="B6">0</epd:amount>
<epd:amount epd:module="B7">0</epd:amount>
<epd:amount epd:module="C1">0</epd:amount>
<epd:amount epd:module="C2">-0.000115664228506722</epd:amount>
<epd:amount epd:module="C3">0</epd:amount>
<epd:amount epd:module="C4">-0.00645938341945963</epd:amount>
<epd:amount epd:module="D">-0.00203829911335646</epd:amount>
</common:other>
</LCIAResult>
<LCIAResult>
<referenceToLCIAMethodDataSet uri="../lciamethods/4331bbdb-978a-490d-8707-eeb047f01a55.xml" type="LCIA method data set" refObjectId="4331bbdb-978a-490d-8707-eeb047f01a55">
<common:shortDescription xml:lang="en">Global Warming Potential luluc (GWP-luluc)</common:shortDescription>
</referenceToLCIAMethodDataSet>
<common:other>
<epd:referenceToUnitGroupDataSet uri="../unitgroups/1ebf3012-d0db-4de2-aefd-ef30cedb0be1.xml" type="unit group data set" refObjectId="1ebf3012-d0db-4de2-aefd-ef30cedb0be1">
<common:shortDescription xml:lang="en">kg CO_(2)-Äq.</common:shortDescription>
</epd:referenceToUnitGroupDataSet>
<epd:amount epd:module="A1">0.00479129779621385</epd:amount>
<epd:amount epd:module="A2">0.000510122355947634</epd:amount>
<epd:amount epd:module="A3">0.00157162358659696</epd:amount>
<epd:amount epd:module="A4">0.000829388779379447</epd:amount>
<epd:amount epd:module="A5">0.000430206459438806</epd:amount>
<epd:amount epd:module="B1">0</epd:amount>
<epd:amount epd:module="B2">0</epd:amount>
<epd:amount epd:module="B6">0</epd:amount>
<epd:amount epd:module="B7">0</epd:amount>
<epd:amount epd:module="C1">0</epd:amount>
<epd:amount epd:module="C2">0.000793754080867365</epd:amount>
<epd:amount epd:module="C3">0</epd:amount>
<epd:amount epd:module="C4">0.000653150888667683</epd:amount>
<epd:amount epd:module="D">-0.000287848326325898</epd:amount>
</common:other>
</LCIAResult>
<LCIAResult>
<referenceToLCIAMethodDataSet uri="../lciamethods/b5c629d6-def3-11e6-bf01-fe55135034f3.xml" type="LCIA method data set" refObjectId="b5c629d6-def3-11e6-bf01-fe55135034f3">
<common:shortDescription xml:lang="en">Depletion potential of the stratospheric ozone layer (ODP)</common:shortDescription>
</referenceToLCIAMethodDataSet>
<common:other>
<epd:referenceToUnitGroupDataSet uri="../unitgroups/d9e957c9-7309-4474-bf3a-7777df6c4e5b.xml" type="unit group data set" refObjectId="d9e957c9-7309-4474-bf3a-7777df6c4e5b">
<common:shortDescription xml:lang="en">kg CFC11-Äq.</common:shortDescription>
</epd:referenceToUnitGroupDataSet>
<epd:amount epd:module="A1">8.65466827029359E-09</epd:amount>
<epd:amount epd:module="A2">1.78493756576795E-17</epd:amount>
<epd:amount epd:module="A3">1.03636383198992E-12</epd:amount>
<epd:amount epd:module="A4">2.0032881920733E-17</epd:amount>
<epd:amount epd:module="A5">4.32785444494975E-10</epd:amount>
<epd:amount epd:module="B1">0</epd:amount>
<epd:amount epd:module="B2">0</epd:amount>
<epd:amount epd:module="B6">0</epd:amount>
<epd:amount epd:module="B7">0</epd:amount>
<epd:amount epd:module="C1">0</epd:amount>
<epd:amount epd:module="C2">1.91721689169864E-17</epd:amount>
<epd:amount epd:module="C3">0</epd:amount>
<epd:amount epd:module="C4">8.63322953892699E-16</epd:amount>
<epd:amount epd:module="D">-4.71567652906964E-15</epd:amount>
</common:other>
</LCIAResult>
<LCIAResult>
<referenceToLCIAMethodDataSet uri="../lciamethods/b5c611c6-def3-11e6-bf01-fe55135034f3.xml" type="LCIA method data set" refObjectId="b5c611c6-def3-11e6-bf01-fe55135034f3">
<common:shortDescription xml:lang="en">Acidification potential of land and water (AP)</common:shortDescription>
</referenceToLCIAMethodDataSet>
<common:other>
<epd:referenceToUnitGroupDataSet uri="../unitgroups/42e089ac-92bf-4bf2-8ca1-5fc40d18f2ed.xml" type="unit group data set" refObjectId="42e089ac-92bf-4bf2-8ca1-5fc40d18f2ed">
<common:shortDescription xml:lang="en">mol H^(+)-Äq.</common:shortDescription>
</epd:referenceToUnitGroupDataSet>
<epd:amount epd:module="A1">0.0194250220595148</epd:amount>
<epd:amount epd:module="A2">0.00212054951886048</epd:amount>
<epd:amount epd:module="A3">0.00879370250850818</epd:amount>
<epd:amount epd:module="A4">0.000107903861301523</epd:amount>
<epd:amount epd:module="A5">0.00179217474919128</epd:amount>
<epd:amount epd:module="B1">0</epd:amount>
<epd:amount epd:module="B2">0</epd:amount>
<epd:amount epd:module="B6">0</epd:amount>
<epd:amount epd:module="B7">0</epd:amount>
<epd:amount epd:module="C1">0</epd:amount>
<epd:amount epd:module="C2">0.000103267770650952</epd:amount>
<epd:amount epd:module="C3">0</epd:amount>
<epd:amount epd:module="C4">0.00158337497971427</epd:amount>
<epd:amount epd:module="D">-0.000542873829938874</epd:amount>
</common:other>
</LCIAResult>
<LCIAResult>
<referenceToLCIAMethodDataSet uri="../lciamethods/b53ec18f-7377-4ad3-86eb-cc3f4f276b2b.xml" type="LCIA method data set" refObjectId="b53ec18f-7377-4ad3-86eb-cc3f4f276b2b">
<common:shortDescription xml:lang="en">Eutrophication potential aquatic freshwater (EP-freshwater)</common:shortDescription>
</referenceToLCIAMethodDataSet>
<common:other>
<epd:referenceToUnitGroupDataSet uri="../unitgroups/0429039d-a61d-4590-ba67-aa4a20a810a1.xml" type="unit group data set" refObjectId="0429039d-a61d-4590-ba67-aa4a20a810a1">
<common:shortDescription xml:lang="en">kg PO_(4)-Äq.</common:shortDescription>
</epd:referenceToUnitGroupDataSet>
<epd:amount epd:module="A1">0.000102021166333917</epd:amount>
<epd:amount epd:module="A2">1.97132054556153E-07</epd:amount>
<epd:amount epd:module="A3">5.62520103782213E-05</epd:amount>
<epd:amount epd:module="A4">3.01453592274017E-07</epd:amount>
<epd:amount epd:module="A5">7.98111055563161E-06</epd:amount>
<epd:amount epd:module="B1">0</epd:amount>
<epd:amount epd:module="B2">0</epd:amount>
<epd:amount epd:module="B6">0</epd:amount>
<epd:amount epd:module="B7">0</epd:amount>
<epd:amount epd:module="C1">0</epd:amount>
<epd:amount epd:module="C2">2.88501635190506E-07</epd:amount>
<epd:amount epd:module="C3">0</epd:amount>
<epd:amount epd:module="C4">3.73131065206824E-07</epd:amount>
<epd:amount epd:module="D">-5.43819760863017E-07</epd:amount>
</common:other>
</LCIAResult>
<LCIAResult>
<referenceToLCIAMethodDataSet uri="../lciamethods/b5c619fa-def3-11e6-bf01-fe55135034f3.xml" type="LCIA method data set" refObjectId="b5c619fa-def3-11e6-bf01-fe55135034f3">
<common:shortDescription xml:lang="en">Eutrophication potential aquatic marine (EP-marine)</common:shortDescription>
</referenceToLCIAMethodDataSet>
<common:other>
<epd:referenceToUnitGroupDataSet uri="../unitgroups/d05bb823-ecdf-4686-8c40-bf1d9257859f.xml" type="unit group data set" refObjectId="d05bb823-ecdf-4686-8c40-bf1d9257859f">
<common:shortDescription xml:lang="en">kg N-Äq.</common:shortDescription>
</epd:referenceToUnitGroupDataSet>
<epd:amount epd:module="A1">0.00498940726500359</epd:amount>
<epd:amount epd:module="A2">0.000582130646783652</epd:amount>
<epd:amount epd:module="A3">0.00396660878160847</epd:amount>
<epd:amount epd:module="A4">3.44402380669669E-05</epd:amount>
<epd:amount epd:module="A5">0.000562852369977391</epd:amount>
<epd:amount epd:module="B1">0</epd:amount>
<epd:amount epd:module="B2">0</epd:amount>
<epd:amount epd:module="B6">0</epd:amount>
<epd:amount epd:module="B7">0</epd:amount>
<epd:amount epd:module="C1">0</epd:amount>
<epd:amount epd:module="C2">3.29605128395302E-05</epd:amount>
<epd:amount epd:module="C3">0</epd:amount>
<epd:amount epd:module="C4">0.000410990265082963</epd:amount>
<epd:amount epd:module="D">-0.000155298660524205</epd:amount>
</common:other>
</LCIAResult>
<LCIAResult>
<referenceToLCIAMethodDataSet uri="../lciamethods/b5c614d2-def3-11e6-bf01-fe55135034f3.xml" type="LCIA method data set" refObjectId="b5c614d2-def3-11e6-bf01-fe55135034f3">
<common:shortDescription xml:lang="en">Eutrophication potential terrestrial (EP-terrestrial)</common:shortDescription>
</referenceToLCIAMethodDataSet>
<common:other>
<epd:referenceToUnitGroupDataSet uri="../unitgroups/71b4d617-0ec9-4d3f-b65e-e438940c2401.xml" type="unit group data set" refObjectId="71b4d617-0ec9-4d3f-b65e-e438940c2401">
<common:shortDescription xml:lang="en">mol N-Äq.</common:shortDescription>
</epd:referenceToUnitGroupDataSet>
<epd:amount epd:module="A1">0.0541458243951714</epd:amount>
<epd:amount epd:module="A2">0.00639463169309022</epd:amount>
<epd:amount epd:module="A3">0.0415919031322674</epd:amount>
<epd:amount epd:module="A4">0.000409246405349062</epd:amount>
<epd:amount epd:module="A5">0.00625321577321776</epd:amount>
<epd:amount epd:module="B1">0</epd:amount>
<epd:amount epd:module="B2">0</epd:amount>
<epd:amount epd:module="B6">0</epd:amount>
<epd:amount epd:module="B7">0</epd:amount>
<epd:amount epd:module="C1">0</epd:amount>
<epd:amount epd:module="C2">0.000391663128803316</epd:amount>
<epd:amount epd:module="C3">0</epd:amount>
<epd:amount epd:module="C4">0.00451547018984874</epd:amount>
<epd:amount epd:module="D">-0.00166428605686476</epd:amount>
</common:other>
</LCIAResult>
<LCIAResult>
<referenceToLCIAMethodDataSet uri="../lciamethods/b5c610fe-def3-11e6-bf01-fe55135034f3.xml" type="LCIA method data set" refObjectId="b5c610fe-def3-11e6-bf01-fe55135034f3">
<common:shortDescription xml:lang="en">Formation potential of tropospheric ozone photochemical oxidants (POCP)</common:shortDescription>
</referenceToLCIAMethodDataSet>
<common:other>
<epd:referenceToUnitGroupDataSet uri="../unitgroups/d27c25f8-fbc1-44c6-b47b-4adbae4199c6.xml" type="unit group data set" refObjectId="d27c25f8-fbc1-44c6-b47b-4adbae4199c6">
<common:shortDescription xml:lang="en">kg NMVOC-Äq.</common:shortDescription>
</epd:referenceToUnitGroupDataSet>
<epd:amount epd:module="A1">0.0164582340926144</epd:amount>
<epd:amount epd:module="A2">0.00163013591598696</epd:amount>
<epd:amount epd:module="A3">0.0111136981117272</epd:amount>
<epd:amount epd:module="A4">9.36564934842971E-05</epd:amount>
<epd:amount epd:module="A5">0.00169914460668004</epd:amount>
<epd:amount epd:module="B1">0</epd:amount>
<epd:amount epd:module="B2">0</epd:amount>
<epd:amount epd:module="B6">0</epd:amount>
<epd:amount epd:module="B7">0</epd:amount>
<epd:amount epd:module="C1">0</epd:amount>
<epd:amount epd:module="C2">8.96325411570076E-05</epd:amount>
<epd:amount epd:module="C3">0</epd:amount>
<epd:amount epd:module="C4">0.00124541607421517</epd:amount>
<epd:amount epd:module="D">-0.000435841370723553</epd:amount>
</common:other>
</LCIAResult>
<LCIAResult>
<referenceToLCIAMethodDataSet uri="../lciamethods/b2ad6494-c78d-11e6-9d9d-cec0c932ce01.xml" type="LCIA method data set" refObjectId="b2ad6494-c78d-11e6-9d9d-cec0c932ce01">
<common:shortDescription xml:lang="en">Abiotic depletion potential for non fossil resources (ADPE)</common:shortDescription>
</referenceToLCIAMethodDataSet>
<common:other>
<epd:referenceToUnitGroupDataSet uri="../unitgroups/54ccd2d9-a32a-4fc2-923d-f2c8c93e89d4.xml" type="unit group data set" refObjectId="54ccd2d9-a32a-4fc2-923d-f2c8c93e89d4">
<common:shortDescription xml:lang="en">kg Sb-Äq.</common:shortDescription>
</epd:referenceToUnitGroupDataSet>
<epd:amount epd:module="A1">1.00162818674452E-06</epd:amount>
<epd:amount epd:module="A2">7.13877443416993E-09</epd:amount>
<epd:amount epd:module="A3">1.42635915971215E-06</epd:amount>
<epd:amount epd:module="A4">8.99375103059325E-09</epd:amount>
<epd:amount epd:module="A5">1.25809930258482E-07</epd:amount>
<epd:amount epd:module="B1">0</epd:amount>
<epd:amount epd:module="B2">0</epd:amount>
<epd:amount epd:module="B6">0</epd:amount>
<epd:amount epd:module="B7">0</epd:amount>
<epd:amount epd:module="C1">0</epd:amount>
<epd:amount epd:module="C2">8.6073344133975E-09</epd:amount>
<epd:amount epd:module="C3">0</epd:amount>
<epd:amount epd:module="C4">2.09731915757562E-08</epd:amount>
<epd:amount epd:module="D">-6.86424891038059E-08</epd:amount>
</common:other>
</LCIAResult>
<LCIAResult>
<referenceToLCIAMethodDataSet uri="../lciamethods/b2ad6110-c78d-11e6-9d9d-cec0c932ce01.xml" type="LCIA method data set" refObjectId="b2ad6110-c78d-11e6-9d9d-cec0c932ce01">
<common:shortDescription xml:lang="en">Abiotic depletion potential for fossil resources (ADPF)</common:shortDescription>
</referenceToLCIAMethodDataSet>
<common:other>
<epd:referenceToUnitGroupDataSet uri="../unitgroups/93a60a57-a3c8-11da-a746-0800200c9a66.xml" type="unit group data set" refObjectId="93a60a57-a3c8-11da-a746-0800200c9a66">
<common:shortDescription xml:lang="en">MJ</common:shortDescription>
</epd:referenceToUnitGroupDataSet>
<epd:amount epd:module="A1">65.1127940917828</epd:amount>
<epd:amount epd:module="A2">1.48382406961703</epd:amount>
<epd:amount epd:module="A3">198.35703767699</epd:amount>
<epd:amount epd:module="A4">1.35153629587689</epd:amount>
<epd:amount epd:module="A5">13.7404196308939</epd:amount>
<epd:amount epd:module="B1">0</epd:amount>
<epd:amount epd:module="B2">0</epd:amount>
<epd:amount epd:module="B6">0</epd:amount>
<epd:amount epd:module="B7">0</epd:amount>
<epd:amount epd:module="C1">0</epd:amount>
<epd:amount epd:module="C2">1.29346752327094</epd:amount>
<epd:amount epd:module="C3">0</epd:amount>
<epd:amount epd:module="C4">2.9488619475852</epd:amount>
<epd:amount epd:module="D">-7.14333418142</epd:amount>
</common:other>
</LCIAResult>
<LCIAResult>
<referenceToLCIAMethodDataSet uri="../lciamethods/b2ad66ce-c78d-11e6-9d9d-cec0c932ce01.xml" type="LCIA method data set" refObjectId="b2ad66ce-c78d-11e6-9d9d-cec0c932ce01">
<common:shortDescription xml:lang="en">Water use (WDP)</common:shortDescription>
</referenceToLCIAMethodDataSet>
<common:other>
<epd:referenceToUnitGroupDataSet uri="../unitgroups/6ae2df01-888e-46c8-b17d-49fa3869b476.xml" type="unit group data set" refObjectId="6ae2df01-888e-46c8-b17d-49fa3869b476">
<common:shortDescription xml:lang="en">m^(3) world-Äq. deprived</common:shortDescription>
</epd:referenceToUnitGroupDataSet>
<epd:amount epd:module="A1">0.401755475785965</epd:amount>
<epd:amount epd:module="A2">0.000660662965822505</epd:amount>
<epd:amount epd:module="A3">2.84284862885433</epd:amount>
<epd:amount epd:module="A4">0.0009416051881736</epd:amount>
<epd:amount epd:module="A5">0.292266330910183</epd:amount>
<epd:amount epd:module="B1">0</epd:amount>
<epd:amount epd:module="B2">0</epd:amount>
<epd:amount epd:module="B6">0</epd:amount>
<epd:amount epd:module="B7">0</epd:amount>
<epd:amount epd:module="C1">0</epd:amount>
<epd:amount epd:module="C2">0.000901149110358011</epd:amount>
<epd:amount epd:module="C3">0</epd:amount>
<epd:amount epd:module="C4">0.0238551973359026</epd:amount>
<epd:amount epd:module="D">-0.0315912165168859</epd:amount>
</common:other>
</LCIAResult>
<LCIAResult>
<referenceToLCIAMethodDataSet uri="../lciamethods/b5c602c6-def3-11e6-bf01-fe55135034f3.xml" type="LCIA method data set" refObjectId="b5c602c6-def3-11e6-bf01-fe55135034f3">
<common:shortDescription xml:lang="en">Incidence of disease due to PM emissions (PM)</common:shortDescription>
</referenceToLCIAMethodDataSet>
<common:other>
<epd:referenceToUnitGroupDataSet uri="../unitgroups/3883559b-648f-4afc-8ba2-0bd24f3affa3.xml" type="unit group data set" refObjectId="3883559b-648f-4afc-8ba2-0bd24f3affa3">
<common:shortDescription xml:lang="en">Disease incidence</common:shortDescription>
</epd:referenceToUnitGroupDataSet>
<epd:amount epd:module="A1">2.56E-07</epd:amount>
<epd:amount epd:module="A2">3.68E-08</epd:amount>
<epd:amount epd:module="A3">2.16E-07</epd:amount>
<epd:amount epd:module="A4">7.4E-10</epd:amount>
<epd:amount epd:module="A5">2.74E-08</epd:amount>
<epd:amount epd:module="B1">0</epd:amount>
<epd:amount epd:module="B2">0</epd:amount>
<epd:amount epd:module="B6">0</epd:amount>
<epd:amount epd:module="B7">0</epd:amount>
<epd:amount epd:module="C1">0</epd:amount>
<epd:amount epd:module="C2">7.08E-10</epd:amount>
<epd:amount epd:module="C3">0</epd:amount>
<epd:amount epd:module="C4">1.97E-08</epd:amount>
<epd:amount epd:module="D">-5.82E-09</epd:amount>
</common:other>
</LCIAResult>
<LCIAResult>
<referenceToLCIAMethodDataSet uri="../lciamethods/b5c632be-def3-11e6-bf01-fe55135034f3.xml" type="LCIA method data set" refObjectId="b5c632be-def3-11e6-bf01-fe55135034f3">
<common:shortDescription xml:lang="en">Human exposure efficiency relative to U235 (IR)</common:shortDescription>
</referenceToLCIAMethodDataSet>
<common:other>
<epd:referenceToUnitGroupDataSet uri="../unitgroups/456b05bf-1415-44a9-9993-02452f554c09.xml" type="unit group data set" refObjectId="456b05bf-1415-44a9-9993-02452f554c09">
<common:shortDescription xml:lang="en">kBq U235-Äq.</common:shortDescription>
</epd:referenceToUnitGroupDataSet>
<epd:amount epd:module="A1">0.328</epd:amount>
<epd:amount epd:module="A2">0.000325</epd:amount>
<epd:amount epd:module="A3">0.133</epd:amount>
<epd:amount epd:module="A4">0.00036</epd:amount>
<epd:amount epd:module="A5">0.0257</epd:amount>
<epd:amount epd:module="B1">0</epd:amount>
<epd:amount epd:module="B2">0</epd:amount>
<epd:amount epd:module="B6">0</epd:amount>
<epd:amount epd:module="B7">0</epd:amount>
<epd:amount epd:module="C1">0</epd:amount>
<epd:amount epd:module="C2">0.000344</epd:amount>
<epd:amount epd:module="C3">0</epd:amount>
<epd:amount epd:module="C4">0.00325</epd:amount>
<epd:amount epd:module="D">-0.0854</epd:amount>
</common:other>
</LCIAResult>
<LCIAResult>
<referenceToLCIAMethodDataSet uri="../lciamethods/ee1082d1-b0f7-43ca-a1f0-21e2a4a74511.xml" type="LCIA method data set" refObjectId="ee1082d1-b0f7-43ca-a1f0-21e2a4a74511">
<common:shortDescription xml:lang="en">Comparative toxic unit for ecosystems (ETP-fw)</common:shortDescription>
</referenceToLCIAMethodDataSet>
<common:other>
<epd:referenceToUnitGroupDataSet uri="../unitgroups/aa959ded-f1eb-4efb-9c5c-2d60be36b3e6.xml" type="unit group data set" refObjectId="aa959ded-f1eb-4efb-9c5c-2d60be36b3e6">
<common:shortDescription xml:lang="en">CTUe</common:shortDescription>
</epd:referenceToUnitGroupDataSet>
<epd:amount epd:module="A1">28.1</epd:amount>
<epd:amount epd:module="A2">1.09</epd:amount>
<epd:amount epd:module="A3">13.8</epd:amount>
<epd:amount epd:module="A4">1</epd:amount>
<epd:amount epd:module="A5">2.4</epd:amount>
<epd:amount epd:module="B1">0</epd:amount>
<epd:amount epd:module="B2">0</epd:amount>
<epd:amount epd:module="B6">0</epd:amount>
<epd:amount epd:module="B7">0</epd:amount>
<epd:amount epd:module="C1">0</epd:amount>
<epd:amount epd:module="C2">0.96</epd:amount>
<epd:amount epd:module="C3">0</epd:amount>
<epd:amount epd:module="C4">1.68</epd:amount>
<epd:amount epd:module="D">-1.5</epd:amount>
</common:other>
</LCIAResult>
<LCIAResult>
<referenceToLCIAMethodDataSet uri="../lciamethods/2299222a-bbd8-474f-9d4f-4dd1f18aea7c.xml" type="LCIA method data set" refObjectId="2299222a-bbd8-474f-9d4f-4dd1f18aea7c">
<common:shortDescription xml:lang="en">Comparative toxic unit for humans (carcinogenic) (HTP-c)</common:shortDescription>
</referenceToLCIAMethodDataSet>
<common:other>
<epd:referenceToUnitGroupDataSet uri="../unitgroups/d4c9523e-2d7e-49fd-8469-998f547d3a70.xml" type="unit group data set" refObjectId="d4c9523e-2d7e-49fd-8469-998f547d3a70">
<common:shortDescription xml:lang="en">CTUh</common:shortDescription>
</epd:referenceToUnitGroupDataSet>
<epd:amount epd:module="A1">6.2E-09</epd:amount>
<epd:amount epd:module="A2">2.13E-11</epd:amount>
<epd:amount epd:module="A3">1.84E-09</epd:amount>
<epd:amount epd:module="A4">2.03E-11</epd:amount>
<epd:amount epd:module="A5">4.24E-10</epd:amount>
<epd:amount epd:module="B1">0</epd:amount>
<epd:amount epd:module="B2">0</epd:amount>
<epd:amount epd:module="B6">0</epd:amount>
<epd:amount epd:module="B7">0</epd:amount>
<epd:amount epd:module="C1">0</epd:amount>
<epd:amount epd:module="C2">1.94E-11</epd:amount>
<epd:amount epd:module="C3">0</epd:amount>
<epd:amount epd:module="C4">2.48E-10</epd:amount>
<epd:amount epd:module="D">-6.82E-11</epd:amount>
</common:other>
</LCIAResult>
<LCIAResult>
<referenceToLCIAMethodDataSet uri="../lciamethods/3af763a5-b7a1-48c9-9cee-1f223481fcef.xml" type="LCIA method data set" refObjectId="3af763a5-b7a1-48c9-9cee-1f223481fcef">
<common:shortDescription xml:lang="en">Comparative toxic unit for humans (noncarcinogenic) (HTP-nc)</common:shortDescription>
</referenceToLCIAMethodDataSet>
<common:other>
<epd:referenceToUnitGroupDataSet uri="../unitgroups/d4c9523e-2d7e-49fd-8469-998f547d3a70.xml" type="unit group data set" refObjectId="d4c9523e-2d7e-49fd-8469-998f547d3a70">
<common:shortDescription xml:lang="en">CTUh</common:shortDescription>
</epd:referenceToUnitGroupDataSet>
<epd:amount epd:module="A1">1.01E-07</epd:amount>
<epd:amount epd:module="A2">1.08E-09</epd:amount>
<epd:amount epd:module="A3">4.06E-08</epd:amount>
<epd:amount epd:module="A4">1.05E-09</epd:amount>
<epd:amount epd:module="A5">8.82E-09</epd:amount>
<epd:amount epd:module="B1">0</epd:amount>
<epd:amount epd:module="B2">0</epd:amount>
<epd:amount epd:module="B6">0</epd:amount>
<epd:amount epd:module="B7">0</epd:amount>
<epd:amount epd:module="C1">0</epd:amount>
<epd:amount epd:module="C2">1.01E-09</epd:amount>
<epd:amount epd:module="C3">0</epd:amount>
<epd:amount epd:module="C4">2.74E-08</epd:amount>
<epd:amount epd:module="D">-2.7E-09</epd:amount>
</common:other>
</LCIAResult>
<LCIAResult>
<referenceToLCIAMethodDataSet uri="../lciamethods/b2ad6890-c78d-11e6-9d9d-cec0c932ce01.xml" type="LCIA method data set" refObjectId="b2ad6890-c78d-11e6-9d9d-cec0c932ce01">
<common:shortDescription xml:lang="en">Soil quality index (SQP)</common:shortDescription>
</referenceToLCIAMethodDataSet>
<common:other>
<epd:referenceToUnitGroupDataSet uri="../unitgroups/f130951c-e67f-4f7f-8dd4-665de3974e18.xml" type="unit group data set" refObjectId="f130951c-e67f-4f7f-8dd4-665de3974e18">
<common:shortDescription xml:lang="en">SQP</common:shortDescription>
</epd:referenceToUnitGroupDataSet>
<epd:amount epd:module="A1">99.6</epd:amount>
<epd:amount epd:module="A2">0.287</epd:amount>
<epd:amount epd:module="A3">217</epd:amount>
<epd:amount epd:module="A4">0.465</epd:amount>
<epd:amount epd:module="A5">16</epd:amount>
<epd:amount epd:module="B1">0</epd:amount>
<epd:amount epd:module="B2">0</epd:amount>
<epd:amount epd:module="B6">0</epd:amount>
<epd:amount epd:module="B7">0</epd:amount>
<epd:amount epd:module="C1">0</epd:amount>
<epd:amount epd:module="C2">0.445</epd:amount>
<epd:amount epd:module="C3">0</epd:amount>
<epd:amount epd:module="C4">0.595</epd:amount>
<epd:amount epd:module="D">-1.11</epd:amount>
</common:other>
</LCIAResult>
</LCIAResults>
</processDataSet>