<?xml version="1.0" encoding="utf-8"?>
<?xml-stylesheet version="1.0" href="../../stylesheets/epd2html.xsl" type="text/xsl"?>
<processDataSet xmlns="http://lca.jrc.it/ILCD/Process" xmlns:common="http://lca.jrc.it/ILCD/Common" xmlns:epd="http://www.iai.kit.edu/EPD/2013" xmlns:epd2="http://www.indata.network/EPD/2019" xmlns:xsi="http://www.w3.org/2001/XMLSchema-instance" xsi:schemaLocation="http://lca.jrc.it/ILCD/Process ../../schemas/EPD_DataSet.xsd" locations="../ILCDLocations.xml" epd2:epd-version="1.2" version="1.1">
  <processInformation>
    <dataSetInformation>
      <common:UUID>5b90a086-26c7-41dc-82fa-3b04fe7e36c2</common:UUID>
      <name>
        <baseName xml:lang="en">Gas Combined heat and power unit (500 kW)</baseName>
        <baseName xml:lang="de">Gas Blockheizkraftwerk (500 kW)</baseName>
        <functionalUnitFlowProperties xml:lang="en">1 piece</functionalUnitFlowProperties>
      </name>
      <classificationInformation>
        <common:classification name="oekobau.dat">
          <common:class level="0" classId="8">Gebäudetechnik</common:class>
          <common:class level="1" classId="8.1">Heizung</common:class>
          <common:class level="2" classId="8.1.01">Wärmeerzeuger</common:class>
        </common:classification>
      </classificationInformation>
      <common:generalComment xml:lang="en">This data set has been modeled according to the European Standard EN 15804+A2 for Sustainable Building. Results are depicted in modules that allow the structured expression of results over the entire life cycle.</common:generalComment>
      <common:generalComment xml:lang="de">Dieser Datensatz wurde nach dem European Standard EN 15804+A2 für Nachhaltiges Bauen modelliert. Ergebnisse werden in Modulen abgebildet, die den strukturierten Ausdruck von Ergebnissen über den gesamten Lebenszyklus zulassen.</common:generalComment>
      <common:other>
        <epd:safetyMargins>
          <epd:margins>20</epd:margins>
          <epd:description xml:lang="en">Product system depicted except for a few missing processes / flows. Technological, temporal and geographic representativeness partly given.</epd:description>
          <epd:description xml:lang="de">Produktsystem bis auf wenige Prozesse/Flüsse abgebildet. Technologische, zeitliche und geographische Repräsentativität teilweise gegeben.</epd:description>
        </epd:safetyMargins>
      </common:other>
    </dataSetInformation>
    <quantitativeReference type="Reference flow(s)">
      <referenceToReferenceFlow>108873</referenceToReferenceFlow>
    </quantitativeReference>
    <time>
      <common:referenceYear>2021</common:referenceYear>
      <common:dataSetValidUntil>2022</common:dataSetValidUntil>
      <common:timeRepresentativenessDescription xml:lang="en">Annual average</common:timeRepresentativenessDescription>
      <common:timeRepresentativenessDescription xml:lang="de">Jährlicher Durchschnitt</common:timeRepresentativenessDescription>
    </time>
    <geography>
      <locationOfOperationSupplyOrProduction location="DE">
        <descriptionOfRestrictions xml:lang="en">The data set represents the country specific situation in Germany, focusing on the main technologies, the region specific characteristics and / or import statistics.</descriptionOfRestrictions>
        <descriptionOfRestrictions xml:lang="de">Der Datensatz bildet die länderspezifische Situation in Deutschland ab. Dabei werden Haupttechnologien, spezifische regionale Charakteristiken und ggf. Importstatistiken berücksichtigt.</descriptionOfRestrictions>
      </locationOfOperationSupplyOrProduction>
    </geography>
    <technology>
      <technologyDescriptionAndIncludedProcesses xml:lang="en">The data set only includes the manufacture and disposal of the combined heat and power unit, not its operation. The main raw materials of the plant are steel (approx. 47 m.%), stainless steel (approx. 19 m.%), aluminum (approx. 17 m.%) and copper (approx. 5 m.%).
For these metals (steel, stainless steel, aluminum and copper), the primary upstream chains were used in the sense of a coservative approach (e.g. the blast furnace route in the case of steel). The life cycle assessment is dominated by steel production. Stainless steel, aluminum and copper also make relevant contributions. 

In module C1, a dismantling with machinery is assumed, collecting losses are neglected.
The transport in module C2 to the recycling plant takes place with a truck (50km).

Tratment of metal components:
Collecting losses are neglected. It is assumed that all metals reach the end of the waste status immediately after dismantling. This means that the loads for processing and the credits for the substitution of primary material are shown in Module D.
Module D includes loads for sorting, remelting, slag treatment, landfill, filtration of dusts and dross treatment. Credits are given for the net scrap amount (amount returned minus secondary material content, minus processing losses) for the average material mix (from different alloys).

Treatment of plastic components:
Module C3 takes into account the grinding and thermal treatment (combustion) of the material. When calculating combustion emissions and credits, the specific calorific value of each material and the material composition are taken into account.
In module D credits for the substitution of electricity (German electricity mix) and thermal energy (from natural gas) are given.</technologyDescriptionAndIncludedProcesses>
      <technologyDescriptionAndIncludedProcesses xml:lang="de">Der Datensatz beinhaltet ausschließlich die Herstellung und Entsorgung des Blockheizkraftwerks, nicht dessen Betrieb. Hauptrohstoffe der Anlage sind Stahl (ca. 47 M.%), Edelstahl (ca. 19 M.%), Aluminium (ca. 17 M.%) und Kupfer (ca. 5 M.%). 
Für diese Metalle (Stahl, Edelstahl, Aluminium und Kupfer) wurden im Sinne eines koservativen Ansatzes die Primärvorketten verwendet (z.B. im Falle von Stahl die Hochofenroute). Die Ökobilanz wird von der Stahlherstellung dominiert. Edelstahl, Aluminium und Kupfer liefern ebenfalls relevante Beiträge.

Beschreibung EoL Prozesse:
In Modul C1 wird ein maschineller Rückbau angenommen. Sammelverluste werden vernachlässigt.
Der Transport in Modul C2 zur Verwertungsanlage erfolgt mit einem LKW (50km). 

Behandlung Metallkomponenten:
Es wird angenommen, dass alle Metalle das Ende der Abfalleigenschaft direkt nach dem Ausbau erreichen. Das heißt die Lasten für die Aufbereitung und die Gutschriften für die Substitution von Primärmaterial werden in Modul D ausgewiesen.
In Modul D sind die Lasten für die Sortierung, Umschmelzen, Schlackebehandlung, Deponierung von Reststoffen, Behandlung von Filterstäuben und Krätzebehandlung enthalten. Die Gutschriften werden für die Nettoschrottmenge (zurückgebaute Menge abzüglich ggfs. enthaltenes Sekundärmaterial, abzüglich Aufbereitungsverluste) für den durchschnittlich vorhandenen Materialmix (aus verschiedenen Legierungen) vergeben.

Kunststoffkomponten:
In Modul C3 wird die Zerkleinerung und thermische Behandlung (Verbrennung) des Materials berücksichtigt. Bei der Berechnung der Verbrennungsemissionen und Gutschriften wird der spezifische Heizwert des jeweiligen Materials sowie die Materialzusammensetzung berücksichtigt.
In Modul D erfolgen Gutschriften für die Substitution von Strom (deutscher Strommix) und thermischer Energie (aus Erdgas).</technologyDescriptionAndIncludedProcesses>
      <technologicalApplicability xml:lang="en">Combined heat and power plants are used to generate electrical and thermal energy.</technologicalApplicability>
      <technologicalApplicability xml:lang="de">Blockheizkraftwerke werden für die Erzeugung von elektrischer und thermischer Energie verwendet.</technologicalApplicability>
    </technology>
  </processInformation>
  <modellingAndValidation>
    <LCIMethodAndAllocation>
      <typeOfDataSet>EPD</typeOfDataSet>
      <common:other>
        <epd:subType>generic dataset</epd:subType>
      </common:other>
    </LCIMethodAndAllocation>
    <dataSourcesTreatmentAndRepresentativeness>
      <referenceToDataSource refObjectId="fe5b9b2f-38c9-430a-b331-c7e9d70fca9d" version="21.01.000" type="source data set" uri="../sources/fe5b9b2f-38c9-430a-b331-c7e9d70fca9d.xml">
        <common:shortDescription xml:lang="en">VDI 2067</common:shortDescription>
      </referenceToDataSource>
      <referenceToDataSource refObjectId="7fd798d8-6216-4bc0-a9cf-6614fe359f97" version="21.01.000" type="source data set" uri="../sources/7fd798d8-6216-4bc0-a9cf-6614fe359f97.xml">
        <common:shortDescription xml:lang="en">HUTTER 2001</common:shortDescription>
      </referenceToDataSource>
      <referenceToDataSource refObjectId="acbfacd6-f9a7-40ed-9fbc-0e520867eb9e" version="21.01.000" type="source data set" uri="../sources/acbfacd6-f9a7-40ed-9fbc-0e520867eb9e.xml">
        <common:shortDescription xml:lang="en">MEEUP  2005</common:shortDescription>
      </referenceToDataSource>
      <referenceToDataSource refObjectId="339584a7-5d2b-49d1-a2b7-775c38786639" version="21.01.000" type="source data set" uri="../sources/339584a7-5d2b-49d1-a2b7-775c38786639.xml">
        <common:shortDescription xml:lang="en">BUDERUS 2008</common:shortDescription>
      </referenceToDataSource>
      <referenceToDataSource refObjectId="96353542-ff08-4323-8bdd-d09a27871a70" version="21.01.000" type="source data set" uri="../sources/96353542-ff08-4323-8bdd-d09a27871a70.xml">
        <common:shortDescription xml:lang="en">BRÖNTJE 2006</common:shortDescription>
      </referenceToDataSource>
      <referenceToDataSource refObjectId="4713dca3-5f73-4b9d-bf9f-8dd95aba5574" version="21.01.000" type="source data set" uri="../sources/4713dca3-5f73-4b9d-bf9f-8dd95aba5574.xml">
        <common:shortDescription xml:lang="en">EVA 2003</common:shortDescription>
      </referenceToDataSource>
      <referenceToDataSource refObjectId="e3bd9bbf-2c3c-42aa-8892-fd13f1065ca5" version="21.01.000" type="source data set" uri="../sources/e3bd9bbf-2c3c-42aa-8892-fd13f1065ca5.xml">
        <common:shortDescription xml:lang="en">Documentation of data quality management</common:shortDescription>
      </referenceToDataSource>
      <referenceToDataSource refObjectId="1cece811-7501-44d4-8067-9259bd5cb835" version="00.01.000" type="source data set" uri="../sources/1cece811-7501-44d4-8067-9259bd5cb835.xml">
        <common:shortDescription xml:lang="en">GaBi Database Edition 2021, CUP2021.01</common:shortDescription>
      </referenceToDataSource>
      <referenceToDataSource refObjectId="28d74cc0-db8b-4d7e-bc44-5f6d56ce0c4a" version="00.03.002" type="source data set" uri="../sources/28d74cc0-db8b-4d7e-bc44-5f6d56ce0c4a.xml">
        <common:shortDescription xml:lang="en">GaBi database (all versions)</common:shortDescription>
      </referenceToDataSource>
      <useAdviceForDataSet xml:lang="en">This data set refers to the production of a combined heat and power (CHP) unit with an electrical output of 500 kW. The total weight of the system is 7,500 kg. The data set can be used to estimate other unit weights between 5,000 and 10,000 kg.</useAdviceForDataSet>
      <useAdviceForDataSet xml:lang="de">Dieser Datensatz bezieht sich auf die Herstellung eines Blockheizkraftwerks mit einer elektrischen Leistung von 500 kW. Das Gesamtgewicht der Anlage beträgt 7.500 kg. Der Datensatz kann näherungsweise für die Abschätzung anderer Anlagengewichte zwischen 5.000 und 10.000 kg verwendet werden.</useAdviceForDataSet>
    </dataSourcesTreatmentAndRepresentativeness>
    <validation>
      <review type="Dependent internal review">
        <common:referenceToNameOfReviewerAndInstitution refObjectId="d7fa0337-f279-430d-becf-7f3111a85010" version="21.01.000" type="contact data set" uri="../contacts/d7fa0337-f279-430d-becf-7f3111a85010.xml">
          <common:shortDescription xml:lang="en">Sphera Solutions GmbH</common:shortDescription>
        </common:referenceToNameOfReviewerAndInstitution>
      </review>
      <review type="Independent external review">
        <common:referenceToNameOfReviewerAndInstitution refObjectId="8f1306f0-7b83-4f36-a537-aa83f0498266" version="21.01.000" type="contact data set" uri="../contacts/8f1306f0-7b83-4f36-a537-aa83f0498266.xml">
          <common:shortDescription xml:lang="en">GaBi user forum</common:shortDescription>
        </common:referenceToNameOfReviewerAndInstitution>
      </review>
    </validation>
    <complianceDeclarations>
      <compliance>
        <common:referenceToComplianceSystem refObjectId="c0016b33-8cf7-415c-ac6e-deba0d21440d" version="00.01.000" type="source data set" uri="../sources/c0016b33-8cf7-415c-ac6e-deba0d21440d.xml">
          <common:shortDescription xml:lang="de">EN 15804+A2</common:shortDescription>
          <common:shortDescription xml:lang="en">EN 15804+A2</common:shortDescription>
        </common:referenceToComplianceSystem>
        <common:approvalOfOverallCompliance>Fully compliant</common:approvalOfOverallCompliance>
      </compliance>
    </complianceDeclarations>
  </modellingAndValidation>
  <administrativeInformation>
    <dataEntryBy>
      <common:timeStamp>2021-04-28T21:02:58+01:00</common:timeStamp>
      <common:referenceToDataSetFormat refObjectId="a97a0155-0234-4b87-b4ce-a45da52f2a40" version="01.00.000" type="source data set" uri="../sources/a97a0155-0234-4b87-b4ce-a45da52f2a40.xml">
        <common:shortDescription xml:lang="de">ILCD format 1.1</common:shortDescription>
        <common:shortDescription xml:lang="en">ILCD format 1.1</common:shortDescription>
      </common:referenceToDataSetFormat>
      <common:referenceToDataSetFormat refObjectId="a29449fd-aa2f-4de8-b5d7-4b06b43c6fde" version="00.01.000" type="source data set" uri="../sources/a29449fd-aa2f-4de8-b5d7-4b06b43c6fde.xml">
        <common:shortDescription xml:lang="de">EPD-Datenformaterweiterungen v1.2</common:shortDescription>
        <common:shortDescription xml:lang="en">EPD Data Format Extensions v1.2</common:shortDescription>
      </common:referenceToDataSetFormat>
      <common:referenceToPersonOrEntityEnteringTheData refObjectId="d7fa0337-f279-430d-becf-7f3111a85010" version="21.01.000" type="contact data set" uri="../contacts/d7fa0337-f279-430d-becf-7f3111a85010.xml">
        <common:shortDescription xml:lang="en">Sphera Solutions GmbH</common:shortDescription>
      </common:referenceToPersonOrEntityEnteringTheData>
    </dataEntryBy>
    <publicationAndOwnership>
      <common:dataSetVersion>20.21.060</common:dataSetVersion>
      <common:referenceToPrecedingDataSetVersion refObjectId="5b90a086-26c7-41dc-82fa-3b04fe7e36c2" type="process data set" uri="https://www.oekobaudat.de/OEKOBAU.DAT/datasetdetail/process.xhtml?uuid=5b90a086-26c7-41dc-82fa-3b04fe7e36c2&amp;stock=OBD_2020_II&amp;lang=de">
        <common:shortDescription xml:lang="en">Gas Combined heat and power unit (500 kW)</common:shortDescription>
      </common:referenceToPrecedingDataSetVersion>
      <common:referenceToOwnershipOfDataSet refObjectId="d7fa0337-f279-430d-becf-7f3111a85010" version="21.01.000" type="contact data set" uri="../contacts/d7fa0337-f279-430d-becf-7f3111a85010.xml">
        <common:shortDescription xml:lang="en">Sphera Solutions GmbH</common:shortDescription>
      </common:referenceToOwnershipOfDataSet>
      <common:copyright>true</common:copyright>
      <common:licenseType>Free of charge for all users and uses</common:licenseType>
      <common:accessRestrictions xml:lang="en">The license conditions as stated on https://www.oekobaudat.de/ apply.</common:accessRestrictions>
      <common:accessRestrictions xml:lang="de">Es gelten die Lizenzbedingungen wie sie auf https://www.oekobaudat.de/ genannt sind.</common:accessRestrictions>
      <common:other>
        <epd2:referenceToPublisher refObjectId="f11651e0-7877-11e3-981f-0800200c9a66" version="00.01.000" type="contact data set" uri="../contacts/f11651e0-7877-11e3-981f-0800200c9a66.xml">
          <common:shortDescription xml:lang="en">BBSR</common:shortDescription>
        </epd2:referenceToPublisher>
      </common:other>
    </publicationAndOwnership>
  </administrativeInformation>
  <exchanges>
    <exchange dataSetInternalID="108873">
      <referenceToFlowDataSet refObjectId="bbe01ed0-2509-4023-87ee-569764831561" version="21.01.000" type="flow data set" uri="../flows/bbe01ed0-2509-4023-87ee-569764831561.xml">
        <common:shortDescription xml:lang="en">Gas Combined heat and power unit (500 kW)</common:shortDescription>
        <common:shortDescription xml:lang="de">Gas Blockheizkraftwerk (500 kW)</common:shortDescription>
      </referenceToFlowDataSet>
      <meanAmount>1</meanAmount>
    </exchange>
    <exchange dataSetInternalID="108874">
      <referenceToFlowDataSet refObjectId="20f32be5-0398-4288-9b6d-accddd195317" version="21.01.000" type="flow data set" uri="../flows/20f32be5-0398-4288-9b6d-accddd195317.xml">
        <common:shortDescription xml:lang="en">Use of renewable primary energy as energy carrier (PERE)</common:shortDescription>
        <common:shortDescription xml:lang="de">Erneuerbare Primärenergie als Energieträger (PERE)</common:shortDescription>
      </referenceToFlowDataSet>
      <functionType>General reminder flow</functionType>
      <exchangeDirection>Input</exchangeDirection>
      <common:other>
        <epd:amount epd:module="A1-A3">112253.514918611</epd:amount>
        <epd:referenceToUnitGroupDataSet refObjectId="93a60a57-a3c8-11da-a746-0800200c9a66" version="03.00.000" type="unit group data set" uri="../unitgroups/93a60a57-a3c8-11da-a746-0800200c9a66.xml">
          <common:shortDescription xml:lang="en">MJ</common:shortDescription>
        </epd:referenceToUnitGroupDataSet>
        <epd:amount epd:module="C1">0.918882092074404</epd:amount>
        <epd:amount epd:module="C2">16.4268380033628</epd:amount>
        <epd:amount epd:module="C3">62.9541198726882</epd:amount>
        <epd:amount epd:module="D">-55220.2634766046</epd:amount>
      </common:other>
    </exchange>
    <exchange dataSetInternalID="108875">
      <referenceToFlowDataSet refObjectId="fb3ec0de-548d-4508-aea5-00b73bf6f702" version="21.01.000" type="flow data set" uri="../flows/fb3ec0de-548d-4508-aea5-00b73bf6f702.xml">
        <common:shortDescription xml:lang="en">Use of renewable primary energy resources used as raw materials (PERM)</common:shortDescription>
        <common:shortDescription xml:lang="de">Erneuerbare Primärenergie zur stofflichen Nutzung (PERM)</common:shortDescription>
      </referenceToFlowDataSet>
      <functionType>General reminder flow</functionType>
      <exchangeDirection>Input</exchangeDirection>
      <common:other>
        <epd:amount epd:module="A1-A3">0</epd:amount>
        <epd:referenceToUnitGroupDataSet refObjectId="93a60a57-a3c8-11da-a746-0800200c9a66" version="03.00.000" type="unit group data set" uri="../unitgroups/93a60a57-a3c8-11da-a746-0800200c9a66.xml">
          <common:shortDescription xml:lang="en">MJ</common:shortDescription>
        </epd:referenceToUnitGroupDataSet>
        <epd:amount epd:module="C1">0</epd:amount>
        <epd:amount epd:module="C2">0</epd:amount>
        <epd:amount epd:module="C3">0</epd:amount>
        <epd:amount epd:module="D">0</epd:amount>
      </common:other>
    </exchange>
    <exchange dataSetInternalID="108876">
      <referenceToFlowDataSet refObjectId="53f97275-fa8a-4cdd-9024-65936002acd0" version="21.01.000" type="flow data set" uri="../flows/53f97275-fa8a-4cdd-9024-65936002acd0.xml">
        <common:shortDescription xml:lang="en">Total use of renewable primary energy (PERT)</common:shortDescription>
        <common:shortDescription xml:lang="de">Total erneuerbare Primärenergie (PERT)</common:shortDescription>
      </referenceToFlowDataSet>
      <functionType>General reminder flow</functionType>
      <exchangeDirection>Input</exchangeDirection>
      <common:other>
        <epd:amount epd:module="A1-A3">112253.514918611</epd:amount>
        <epd:referenceToUnitGroupDataSet refObjectId="93a60a57-a3c8-11da-a746-0800200c9a66" version="03.00.000" type="unit group data set" uri="../unitgroups/93a60a57-a3c8-11da-a746-0800200c9a66.xml">
          <common:shortDescription xml:lang="en">MJ</common:shortDescription>
        </epd:referenceToUnitGroupDataSet>
        <epd:amount epd:module="C1">0.918882092074404</epd:amount>
        <epd:amount epd:module="C2">16.4268380033628</epd:amount>
        <epd:amount epd:module="C3">62.9541198726882</epd:amount>
        <epd:amount epd:module="D">-55220.2634766046</epd:amount>
      </common:other>
    </exchange>
    <exchange dataSetInternalID="108877">
      <referenceToFlowDataSet refObjectId="ac857178-2b45-46ec-892a-a9a4332f0372" version="21.01.000" type="flow data set" uri="../flows/ac857178-2b45-46ec-892a-a9a4332f0372.xml">
        <common:shortDescription xml:lang="en">Use of non renewable primary energy as energy carrier (PENRE)</common:shortDescription>
        <common:shortDescription xml:lang="de">Nicht-erneuerbare Primärenergie als Energieträger (PENRE)</common:shortDescription>
      </referenceToFlowDataSet>
      <functionType>General reminder flow</functionType>
      <exchangeDirection>Input</exchangeDirection>
      <common:other>
        <epd:amount epd:module="A1-A3">511537.991897082</epd:amount>
        <epd:referenceToUnitGroupDataSet refObjectId="93a60a57-a3c8-11da-a746-0800200c9a66" version="03.00.000" type="unit group data set" uri="../unitgroups/93a60a57-a3c8-11da-a746-0800200c9a66.xml">
          <common:shortDescription xml:lang="en">MJ</common:shortDescription>
        </epd:referenceToUnitGroupDataSet>
        <epd:amount epd:module="C1">15.8323693299927</epd:amount>
        <epd:amount epd:module="C2">283.034970902602</epd:amount>
        <epd:amount epd:module="C3">285.433682434836</epd:amount>
        <epd:amount epd:module="D">-250713.569082614</epd:amount>
      </common:other>
    </exchange>
    <exchange dataSetInternalID="108878">
      <referenceToFlowDataSet refObjectId="1421caa0-679d-4bf4-b282-0eb850ccae27" version="21.01.000" type="flow data set" uri="../flows/1421caa0-679d-4bf4-b282-0eb850ccae27.xml">
        <common:shortDescription xml:lang="en">Use of non renewable primary energy resources used as raw materials (PENRM)</common:shortDescription>
        <common:shortDescription xml:lang="de">Nicht-erneuerbare Primärenergie zur stofflichen Nutzung (PENRM)</common:shortDescription>
      </referenceToFlowDataSet>
      <functionType>General reminder flow</functionType>
      <exchangeDirection>Input</exchangeDirection>
      <common:other>
        <epd:amount epd:module="A1-A3">0</epd:amount>
        <epd:referenceToUnitGroupDataSet refObjectId="93a60a57-a3c8-11da-a746-0800200c9a66" version="03.00.000" type="unit group data set" uri="../unitgroups/93a60a57-a3c8-11da-a746-0800200c9a66.xml">
          <common:shortDescription xml:lang="en">MJ</common:shortDescription>
        </epd:referenceToUnitGroupDataSet>
        <epd:amount epd:module="C1">0</epd:amount>
        <epd:amount epd:module="C2">0</epd:amount>
        <epd:amount epd:module="C3">0</epd:amount>
        <epd:amount epd:module="D">0</epd:amount>
      </common:other>
    </exchange>
    <exchange dataSetInternalID="108879">
      <referenceToFlowDataSet refObjectId="06159210-646b-4c8d-8583-da9b3b95a6c1" version="21.01.000" type="flow data set" uri="../flows/06159210-646b-4c8d-8583-da9b3b95a6c1.xml">
        <common:shortDescription xml:lang="en">Total use of non renewable primary energy resource (PENRT)</common:shortDescription>
        <common:shortDescription xml:lang="de">Total nicht-erneuerbare Primärenergie (PENRT)</common:shortDescription>
      </referenceToFlowDataSet>
      <functionType>General reminder flow</functionType>
      <exchangeDirection>Input</exchangeDirection>
      <common:other>
        <epd:amount epd:module="A1-A3">511537.991897082</epd:amount>
        <epd:referenceToUnitGroupDataSet refObjectId="93a60a57-a3c8-11da-a746-0800200c9a66" version="03.00.000" type="unit group data set" uri="../unitgroups/93a60a57-a3c8-11da-a746-0800200c9a66.xml">
          <common:shortDescription xml:lang="en">MJ</common:shortDescription>
        </epd:referenceToUnitGroupDataSet>
        <epd:amount epd:module="C1">15.8323693299927</epd:amount>
        <epd:amount epd:module="C2">283.034970902602</epd:amount>
        <epd:amount epd:module="C3">285.433682434836</epd:amount>
        <epd:amount epd:module="D">-250713.569082614</epd:amount>
      </common:other>
    </exchange>
    <exchange dataSetInternalID="108880">
      <referenceToFlowDataSet refObjectId="c6a1f35f-2d09-4f54-8dfb-97e502e1ce92" version="21.01.000" type="flow data set" uri="../flows/c6a1f35f-2d09-4f54-8dfb-97e502e1ce92.xml">
        <common:shortDescription xml:lang="en">Use of secondary material (SM)</common:shortDescription>
        <common:shortDescription xml:lang="de">Einsatz von Sekundärstoffen (SM)</common:shortDescription>
      </referenceToFlowDataSet>
      <functionType>General reminder flow</functionType>
      <exchangeDirection>Input</exchangeDirection>
      <common:other>
        <epd:amount epd:module="A1-A3">1098.95127469838</epd:amount>
        <epd:referenceToUnitGroupDataSet refObjectId="93a60a57-a4c8-11da-a746-0800200c9a66" version="03.00.000" type="unit group data set" uri="../unitgroups/93a60a57-a4c8-11da-a746-0800200c9a66.xml">
          <common:shortDescription xml:lang="en">kg</common:shortDescription>
        </epd:referenceToUnitGroupDataSet>
        <epd:amount epd:module="C1">0</epd:amount>
        <epd:amount epd:module="C2">0</epd:amount>
        <epd:amount epd:module="C3">0</epd:amount>
        <epd:amount epd:module="D">0</epd:amount>
      </common:other>
    </exchange>
    <exchange dataSetInternalID="108881">
      <referenceToFlowDataSet refObjectId="64333088-a55f-4aa2-9a31-c10b07816787" version="21.01.000" type="flow data set" uri="../flows/64333088-a55f-4aa2-9a31-c10b07816787.xml">
        <common:shortDescription xml:lang="en">Use of renewable secondary fuels (SF)</common:shortDescription>
        <common:shortDescription xml:lang="de">Erneuerbare Sekundärbrennstoffe (SF)</common:shortDescription>
      </referenceToFlowDataSet>
      <functionType>General reminder flow</functionType>
      <exchangeDirection>Input</exchangeDirection>
      <common:other>
        <epd:amount epd:module="A1-A3">0</epd:amount>
        <epd:referenceToUnitGroupDataSet refObjectId="93a60a57-a3c8-11da-a746-0800200c9a66" version="03.00.000" type="unit group data set" uri="../unitgroups/93a60a57-a3c8-11da-a746-0800200c9a66.xml">
          <common:shortDescription xml:lang="en">MJ</common:shortDescription>
        </epd:referenceToUnitGroupDataSet>
        <epd:amount epd:module="C1">0</epd:amount>
        <epd:amount epd:module="C2">0</epd:amount>
        <epd:amount epd:module="C3">0</epd:amount>
        <epd:amount epd:module="D">0</epd:amount>
      </common:other>
    </exchange>
    <exchange dataSetInternalID="108882">
      <referenceToFlowDataSet refObjectId="89def144-d39a-4287-b86f-efde453ddcb2" version="21.01.000" type="flow data set" uri="../flows/89def144-d39a-4287-b86f-efde453ddcb2.xml">
        <common:shortDescription xml:lang="en">Use of non renewable secondary fuels (NRSF)</common:shortDescription>
        <common:shortDescription xml:lang="de">Nicht erneuerbare Sekundärbrennstoffe (NRSF)</common:shortDescription>
      </referenceToFlowDataSet>
      <functionType>General reminder flow</functionType>
      <exchangeDirection>Input</exchangeDirection>
      <common:other>
        <epd:amount epd:module="A1-A3">0</epd:amount>
        <epd:referenceToUnitGroupDataSet refObjectId="93a60a57-a3c8-11da-a746-0800200c9a66" version="03.00.000" type="unit group data set" uri="../unitgroups/93a60a57-a3c8-11da-a746-0800200c9a66.xml">
          <common:shortDescription xml:lang="en">MJ</common:shortDescription>
        </epd:referenceToUnitGroupDataSet>
        <epd:amount epd:module="C1">0</epd:amount>
        <epd:amount epd:module="C2">0</epd:amount>
        <epd:amount epd:module="C3">0</epd:amount>
        <epd:amount epd:module="D">0</epd:amount>
      </common:other>
    </exchange>
    <exchange dataSetInternalID="108883">
      <referenceToFlowDataSet refObjectId="3cf952c8-f3a4-461d-8c96-96456ca62246" version="21.01.000" type="flow data set" uri="../flows/3cf952c8-f3a4-461d-8c96-96456ca62246.xml">
        <common:shortDescription xml:lang="en">Net use of fresh water (FW)</common:shortDescription>
        <common:shortDescription xml:lang="de">Nettoeinsatz von Süßwasserressourcen (FW)</common:shortDescription>
      </referenceToFlowDataSet>
      <functionType>General reminder flow</functionType>
      <exchangeDirection>Input</exchangeDirection>
      <common:other>
        <epd:amount epd:module="A1-A3">288.953641552713</epd:amount>
        <epd:referenceToUnitGroupDataSet refObjectId="93a60a57-a3c8-12da-a746-0800200c9a66" version="03.00.000" type="unit group data set" uri="../unitgroups/93a60a57-a3c8-12da-a746-0800200c9a66.xml">
          <common:shortDescription xml:lang="en">m3</common:shortDescription>
        </epd:referenceToUnitGroupDataSet>
        <epd:amount epd:module="C1">0.000816656781936826</epd:amount>
        <epd:amount epd:module="C2">0.0145993580427045</epd:amount>
        <epd:amount epd:module="C3">3.75914817842785</epd:amount>
        <epd:amount epd:module="D">-201.591358203953</epd:amount>
      </common:other>
    </exchange>
    <exchange dataSetInternalID="108884">
      <referenceToFlowDataSet refObjectId="430f9e0f-59b2-46a0-8e0d-55e0e84948fc" version="21.01.000" type="flow data set" uri="../flows/430f9e0f-59b2-46a0-8e0d-55e0e84948fc.xml">
        <common:shortDescription xml:lang="en">Hazardous waste disposed (HWD)</common:shortDescription>
        <common:shortDescription xml:lang="de">Gefährlicher Abfall zur Deponie (HWD)</common:shortDescription>
      </referenceToFlowDataSet>
      <functionType>General reminder flow</functionType>
      <exchangeDirection>Output</exchangeDirection>
      <common:other>
        <epd:amount epd:module="A1-A3">5.2831792429471E-5</epd:amount>
        <epd:referenceToUnitGroupDataSet refObjectId="93a60a57-a4c8-11da-a746-0800200c9a66" version="03.00.000" type="unit group data set" uri="../unitgroups/93a60a57-a4c8-11da-a746-0800200c9a66.xml">
          <common:shortDescription xml:lang="en">kg</common:shortDescription>
        </epd:referenceToUnitGroupDataSet>
        <epd:amount epd:module="C1">6.61741812699845E-10</epd:amount>
        <epd:amount epd:module="C2">1.1829946030107E-8</epd:amount>
        <epd:amount epd:module="C3">6.0076020881475E-8</epd:amount>
        <epd:amount epd:module="D">2.38574126922031E-6</epd:amount>
      </common:other>
    </exchange>
    <exchange dataSetInternalID="108885">
      <referenceToFlowDataSet refObjectId="b29ef66b-e286-4afa-949f-62f1a7b4d7fa" version="21.01.000" type="flow data set" uri="../flows/b29ef66b-e286-4afa-949f-62f1a7b4d7fa.xml">
        <common:shortDescription xml:lang="en">Non harzardous waste disposed (NHWD)</common:shortDescription>
        <common:shortDescription xml:lang="de">Entsorgter nicht gefährlicher Abfall (NHWD)</common:shortDescription>
      </referenceToFlowDataSet>
      <functionType>General reminder flow</functionType>
      <exchangeDirection>Output</exchangeDirection>
      <common:other>
        <epd:amount epd:module="A1-A3">5673.51575182376</epd:amount>
        <epd:referenceToUnitGroupDataSet refObjectId="93a60a57-a4c8-11da-a746-0800200c9a66" version="03.00.000" type="unit group data set" uri="../unitgroups/93a60a57-a4c8-11da-a746-0800200c9a66.xml">
          <common:shortDescription xml:lang="en">kg</common:shortDescription>
        </epd:referenceToUnitGroupDataSet>
        <epd:amount epd:module="C1">0.00255570621873345</epd:amount>
        <epd:amount epd:module="C2">0.0456883123541403</epd:amount>
        <epd:amount epd:module="C3">7.06852988892534</epd:amount>
        <epd:amount epd:module="D">-3090.30020417778</epd:amount>
      </common:other>
    </exchange>
    <exchange dataSetInternalID="108886">
      <referenceToFlowDataSet refObjectId="3449546e-52ad-4b39-b809-9fb77cea8ff6" version="21.01.000" type="flow data set" uri="../flows/3449546e-52ad-4b39-b809-9fb77cea8ff6.xml">
        <common:shortDescription xml:lang="en">Radioactive waste disposed (RWD)</common:shortDescription>
        <common:shortDescription xml:lang="de">Entsorgter radioaktiver Abfall (RWD)</common:shortDescription>
      </referenceToFlowDataSet>
      <functionType>General reminder flow</functionType>
      <exchangeDirection>Output</exchangeDirection>
      <common:other>
        <epd:amount epd:module="A1-A3">18.2091503603418</epd:amount>
        <epd:referenceToUnitGroupDataSet refObjectId="93a60a57-a4c8-11da-a746-0800200c9a66" version="03.00.000" type="unit group data set" uri="../unitgroups/93a60a57-a4c8-11da-a746-0800200c9a66.xml">
          <common:shortDescription xml:lang="en">kg</common:shortDescription>
        </epd:referenceToUnitGroupDataSet>
        <epd:amount epd:module="C1">1.51932266772247E-5</epd:amount>
        <epd:amount epd:module="C2">0.000271609029632642</epd:amount>
        <epd:amount epd:module="C3">0.00772948813712817</epd:amount>
        <epd:amount epd:module="D">-8.88240234243746</epd:amount>
      </common:other>
    </exchange>
    <exchange dataSetInternalID="108887">
      <referenceToFlowDataSet refObjectId="a2b32f97-3fc7-4af2-b209-525bc6426f33" version="21.01.000" type="flow data set" uri="../flows/a2b32f97-3fc7-4af2-b209-525bc6426f33.xml">
        <common:shortDescription xml:lang="en">Components for re-use (CRU)</common:shortDescription>
        <common:shortDescription xml:lang="de">Komponenten für die Wiederverwendung (CRU)</common:shortDescription>
      </referenceToFlowDataSet>
      <functionType>General reminder flow</functionType>
      <exchangeDirection>Output</exchangeDirection>
      <common:other>
        <epd:amount epd:module="A1-A3">0</epd:amount>
        <epd:referenceToUnitGroupDataSet refObjectId="93a60a57-a4c8-11da-a746-0800200c9a66" version="03.00.000" type="unit group data set" uri="../unitgroups/93a60a57-a4c8-11da-a746-0800200c9a66.xml">
          <common:shortDescription xml:lang="en">kg</common:shortDescription>
        </epd:referenceToUnitGroupDataSet>
        <epd:amount epd:module="C1">0</epd:amount>
        <epd:amount epd:module="C2">0</epd:amount>
        <epd:amount epd:module="C3">0</epd:amount>
        <epd:amount epd:module="D">0</epd:amount>
      </common:other>
    </exchange>
    <exchange dataSetInternalID="108888">
      <referenceToFlowDataSet refObjectId="d7fe48a5-4103-49c8-9aae-b0b5dfdbd6ae" version="21.01.000" type="flow data set" uri="../flows/d7fe48a5-4103-49c8-9aae-b0b5dfdbd6ae.xml">
        <common:shortDescription xml:lang="en">Materials for recycling  (MFR)</common:shortDescription>
        <common:shortDescription xml:lang="de">Stoffe zum Recycling (MFR)</common:shortDescription>
      </referenceToFlowDataSet>
      <functionType>General reminder flow</functionType>
      <exchangeDirection>Output</exchangeDirection>
      <common:other>
        <epd:amount epd:module="A1-A3">0</epd:amount>
        <epd:referenceToUnitGroupDataSet refObjectId="93a60a57-a4c8-11da-a746-0800200c9a66" version="03.00.000" type="unit group data set" uri="../unitgroups/93a60a57-a4c8-11da-a746-0800200c9a66.xml">
          <common:shortDescription xml:lang="en">kg</common:shortDescription>
        </epd:referenceToUnitGroupDataSet>
        <epd:amount epd:module="C1">7050</epd:amount>
        <epd:amount epd:module="C2">0</epd:amount>
        <epd:amount epd:module="C3">0</epd:amount>
        <epd:amount epd:module="D">0</epd:amount>
      </common:other>
    </exchange>
    <exchange dataSetInternalID="108889">
      <referenceToFlowDataSet refObjectId="59a9181c-3aaf-46ee-8b13-2b3723b6e447" version="21.01.000" type="flow data set" uri="../flows/59a9181c-3aaf-46ee-8b13-2b3723b6e447.xml">
        <common:shortDescription xml:lang="en">Materials for energy recovery (MER)</common:shortDescription>
        <common:shortDescription xml:lang="de">Stoffe für die Energierückgewinnung (MER)</common:shortDescription>
      </referenceToFlowDataSet>
      <functionType>General reminder flow</functionType>
      <exchangeDirection>Output</exchangeDirection>
      <common:other>
        <epd:amount epd:module="A1-A3">0</epd:amount>
        <epd:referenceToUnitGroupDataSet refObjectId="93a60a57-a4c8-11da-a746-0800200c9a66" version="03.00.000" type="unit group data set" uri="../unitgroups/93a60a57-a4c8-11da-a746-0800200c9a66.xml">
          <common:shortDescription xml:lang="en">kg</common:shortDescription>
        </epd:referenceToUnitGroupDataSet>
        <epd:amount epd:module="C1">0</epd:amount>
        <epd:amount epd:module="C2">0</epd:amount>
        <epd:amount epd:module="C3">464</epd:amount>
        <epd:amount epd:module="D">0</epd:amount>
      </common:other>
    </exchange>
    <exchange dataSetInternalID="108890">
      <referenceToFlowDataSet refObjectId="4da0c987-2b76-40d6-9e9e-82a017aaaf29" version="21.01.000" type="flow data set" uri="../flows/4da0c987-2b76-40d6-9e9e-82a017aaaf29.xml">
        <common:shortDescription xml:lang="en">Exported electrical energy (EEE)</common:shortDescription>
        <common:shortDescription xml:lang="de">Exportierte elektrische Energie (EEE)</common:shortDescription>
      </referenceToFlowDataSet>
      <functionType>General reminder flow</functionType>
      <exchangeDirection>Output</exchangeDirection>
      <common:other>
        <epd:amount epd:module="A1-A3">0</epd:amount>
        <epd:referenceToUnitGroupDataSet refObjectId="93a60a57-a3c8-11da-a746-0800200c9a66" version="03.00.000" type="unit group data set" uri="../unitgroups/93a60a57-a3c8-11da-a746-0800200c9a66.xml">
          <common:shortDescription xml:lang="en">MJ</common:shortDescription>
        </epd:referenceToUnitGroupDataSet>
        <epd:amount epd:module="C1">0</epd:amount>
        <epd:amount epd:module="C2">0</epd:amount>
        <epd:amount epd:module="C3">2646.47425328916</epd:amount>
        <epd:amount epd:module="D">0</epd:amount>
      </common:other>
    </exchange>
    <exchange dataSetInternalID="108891">
      <referenceToFlowDataSet refObjectId="98daf38a-7a79-46d3-9a37-2b7bd0955810" version="21.01.000" type="flow data set" uri="../flows/98daf38a-7a79-46d3-9a37-2b7bd0955810.xml">
        <common:shortDescription xml:lang="en">Exported thermal energy (EET)</common:shortDescription>
        <common:shortDescription xml:lang="de">Exportierte thermische Energie (EET)</common:shortDescription>
      </referenceToFlowDataSet>
      <functionType>General reminder flow</functionType>
      <exchangeDirection>Output</exchangeDirection>
      <common:other>
        <epd:amount epd:module="A1-A3">0</epd:amount>
        <epd:referenceToUnitGroupDataSet refObjectId="93a60a57-a3c8-11da-a746-0800200c9a66" version="03.00.000" type="unit group data set" uri="../unitgroups/93a60a57-a3c8-11da-a746-0800200c9a66.xml">
          <common:shortDescription xml:lang="en">MJ</common:shortDescription>
        </epd:referenceToUnitGroupDataSet>
        <epd:amount epd:module="C1">0</epd:amount>
        <epd:amount epd:module="C2">0</epd:amount>
        <epd:amount epd:module="C3">6095.22003235328</epd:amount>
        <epd:amount epd:module="D">0</epd:amount>
      </common:other>
    </exchange>
  </exchanges>
  <LCIAResults>
    <LCIAResult>
      <referenceToLCIAMethodDataSet refObjectId="6a37f984-a4b3-458a-a20a-64418c145fa2" version="21.01.000" type="LCIA method data set" uri="../lciamethods/6a37f984-a4b3-458a-a20a-64418c145fa2.xml">
        <common:shortDescription xml:lang="en">Global Warming Potential - total (GWP-total)</common:shortDescription>
        <common:shortDescription xml:lang="de">Globales Erwärmungspotenzial - total (GWP-total)</common:shortDescription>
      </referenceToLCIAMethodDataSet>
      <common:other>
        <epd:amount epd:module="A1-A3">41496.5874360262</epd:amount>
        <epd:amount epd:module="C1">1.18447264532431</epd:amount>
        <epd:amount epd:module="C2">21.4987591981623</epd:amount>
        <epd:amount epd:module="C3">1749.10763025289</epd:amount>
        <epd:amount epd:module="D">-22134.9755800489</epd:amount>
        <epd:referenceToUnitGroupDataSet refObjectId="1ebf3012-d0db-4de2-aefd-ef30cedb0be1" version="25.00.000" type="unit group data set" uri="../unitgroups/1ebf3012-d0db-4de2-aefd-ef30cedb0be1.xml">
          <common:shortDescription xml:lang="en">kg CO2 eq.</common:shortDescription>
        </epd:referenceToUnitGroupDataSet>
      </common:other>
    </LCIAResult>
    <LCIAResult>
      <referenceToLCIAMethodDataSet refObjectId="5f635281-343e-44fb-83df-1971b155e6b6" version="21.01.000" type="LCIA method data set" uri="../lciamethods/5f635281-343e-44fb-83df-1971b155e6b6.xml">
        <common:shortDescription xml:lang="en">Global Warming Potential - fossil fuels (GWP-fossil)</common:shortDescription>
        <common:shortDescription xml:lang="de">Globales Erwärmungspotenzial - fossil (GWP-fossil)</common:shortDescription>
      </referenceToLCIAMethodDataSet>
      <common:other>
        <epd:amount epd:module="A1-A3">41444.1534306472</epd:amount>
        <epd:amount epd:module="C1">1.17654675643175</epd:amount>
        <epd:amount epd:module="C2">21.3527806773543</epd:amount>
        <epd:amount epd:module="C3">1748.99292316658</epd:amount>
        <epd:amount epd:module="D">-22139.8144176848</epd:amount>
        <epd:referenceToUnitGroupDataSet refObjectId="1ebf3012-d0db-4de2-aefd-ef30cedb0be1" version="25.00.000" type="unit group data set" uri="../unitgroups/1ebf3012-d0db-4de2-aefd-ef30cedb0be1.xml">
          <common:shortDescription xml:lang="en">kg CO2 eq.</common:shortDescription>
        </epd:referenceToUnitGroupDataSet>
      </common:other>
    </LCIAResult>
    <LCIAResult>
      <referenceToLCIAMethodDataSet refObjectId="2356e1ab-0185-4db5-86e5-16de51c7485c" version="21.01.000" type="LCIA method data set" uri="../lciamethods/2356e1ab-0185-4db5-86e5-16de51c7485c.xml">
        <common:shortDescription xml:lang="en">Global Warming Potential - biogenic (GWP-biogenic)</common:shortDescription>
        <common:shortDescription xml:lang="de">Globales Erwärmungspotenzial - biogen (GWP-biogenic)</common:shortDescription>
      </referenceToLCIAMethodDataSet>
      <common:other>
        <epd:amount epd:module="A1-A3">11.6564734698944</epd:amount>
        <epd:amount epd:module="C1">0.000254942861814057</epd:amount>
        <epd:amount epd:module="C2">0.00884516184227696</epd:amount>
        <epd:amount epd:module="C3">0.0937525598460442</epd:amount>
        <epd:amount epd:module="D">27.1935403205152</epd:amount>
        <epd:referenceToUnitGroupDataSet refObjectId="1ebf3012-d0db-4de2-aefd-ef30cedb0be1" version="25.00.000" type="unit group data set" uri="../unitgroups/1ebf3012-d0db-4de2-aefd-ef30cedb0be1.xml">
          <common:shortDescription xml:lang="en">kg CO2 eq.</common:shortDescription>
        </epd:referenceToUnitGroupDataSet>
      </common:other>
    </LCIAResult>
    <LCIAResult>
      <referenceToLCIAMethodDataSet refObjectId="4331bbdb-978a-490d-8707-eeb047f01a55" version="21.01.000" type="LCIA method data set" uri="../lciamethods/4331bbdb-978a-490d-8707-eeb047f01a55.xml">
        <common:shortDescription xml:lang="en">Global Warming Potential - land use and land use change (GWP-luluc)</common:shortDescription>
        <common:shortDescription xml:lang="de">Globales Erwärmungspotenzial - luluc (GWP-luluc)</common:shortDescription>
      </referenceToLCIAMethodDataSet>
      <common:other>
        <epd:amount epd:module="A1-A3">40.7775319091463</epd:amount>
        <epd:amount epd:module="C1">0.00767094603074982</epd:amount>
        <epd:amount epd:module="C2">0.13713335896578</epd:amount>
        <epd:amount epd:module="C3">0.0209545264579518</epd:amount>
        <epd:amount epd:module="D">-22.3547026845556</epd:amount>
        <epd:referenceToUnitGroupDataSet refObjectId="1ebf3012-d0db-4de2-aefd-ef30cedb0be1" version="25.00.000" type="unit group data set" uri="../unitgroups/1ebf3012-d0db-4de2-aefd-ef30cedb0be1.xml">
          <common:shortDescription xml:lang="en">kg CO2 eq.</common:shortDescription>
        </epd:referenceToUnitGroupDataSet>
      </common:other>
    </LCIAResult>
    <LCIAResult>
      <referenceToLCIAMethodDataSet refObjectId="b5c629d6-def3-11e6-bf01-fe55135034f3" version="21.01.000" type="LCIA method data set" uri="../lciamethods/b5c629d6-def3-11e6-bf01-fe55135034f3.xml">
        <common:shortDescription xml:lang="en">Depletion potenzial of the stratospheric ozone layer (ODP)</common:shortDescription>
        <common:shortDescription xml:lang="de">Abbaupotenzial der stratosphärischen Ozonschicht (ODP)</common:shortDescription>
      </referenceToLCIAMethodDataSet>
      <common:other>
        <epd:amount epd:module="A1-A3">1.73772961272712E-10</epd:amount>
        <epd:amount epd:module="C1">3.05623195946085E-16</epd:amount>
        <epd:amount epd:module="C2">5.4636201675697E-15</epd:amount>
        <epd:amount epd:module="C3">2.58595861972979E-13</epd:amount>
        <epd:amount epd:module="D">2.81756367126951E-9</epd:amount>
        <epd:referenceToUnitGroupDataSet refObjectId="d9e957c9-7309-4474-bf3a-7777df6c4e5b" version="25.00.000" type="unit group data set" uri="../unitgroups/d9e957c9-7309-4474-bf3a-7777df6c4e5b.xml">
          <common:shortDescription xml:lang="en">kg CFC-11 eq.</common:shortDescription>
        </epd:referenceToUnitGroupDataSet>
      </common:other>
    </LCIAResult>
    <LCIAResult>
      <referenceToLCIAMethodDataSet refObjectId="b5c611c6-def3-11e6-bf01-fe55135034f3" version="21.01.000" type="LCIA method data set" uri="../lciamethods/b5c611c6-def3-11e6-bf01-fe55135034f3.xml">
        <common:shortDescription xml:lang="en">Acidifcation potential, Accumulated Exceedance (AP)</common:shortDescription>
        <common:shortDescription xml:lang="de">Versauerungspotenzial, kumulierte Überschreitung (AP)</common:shortDescription>
      </referenceToLCIAMethodDataSet>
      <common:other>
        <epd:amount epd:module="A1-A3">184.438315146836</epd:amount>
        <epd:amount epd:module="C1">0.0158408136907005</epd:amount>
        <epd:amount epd:module="C2">0.0605400251520379</epd:amount>
        <epd:amount epd:module="C3">0.2699015570859</epd:amount>
        <epd:amount epd:module="D">-96.998714773029</epd:amount>
        <epd:referenceToUnitGroupDataSet refObjectId="42e089ac-92bf-4bf2-8ca1-5fc40d18f2ed" version="00.01.000" type="unit group data set" uri="../unitgroups/42e089ac-92bf-4bf2-8ca1-5fc40d18f2ed.xml">
          <common:shortDescription xml:lang="en">Mole of H+ eq.</common:shortDescription>
        </epd:referenceToUnitGroupDataSet>
      </common:other>
    </LCIAResult>
    <LCIAResult>
      <referenceToLCIAMethodDataSet refObjectId="b53ec18f-7377-4ad3-86eb-cc3f4f276b2b" version="21.01.000" type="LCIA method data set" uri="../lciamethods/b53ec18f-7377-4ad3-86eb-cc3f4f276b2b.xml">
        <common:shortDescription xml:lang="en">Eutrophication potential - freshwater (EP-freshwater)</common:shortDescription>
        <common:shortDescription xml:lang="de">Eutrophierungspotenzial - Süßwasser (EP-freshwater)</common:shortDescription>
      </referenceToLCIAMethodDataSet>
      <common:other>
        <epd:amount epd:module="A1-A3">0.0387400793466807</epd:amount>
        <epd:amount epd:module="C1">2.45648065114927E-6</epd:amount>
        <epd:amount epd:module="C2">4.39144587351005E-5</epd:amount>
        <epd:amount epd:module="C3">3.52857306310519E-5</epd:amount>
        <epd:amount epd:module="D">-0.0132428904913793</epd:amount>
        <epd:referenceToUnitGroupDataSet refObjectId="0429039d-a61d-4590-ba67-aa4a20a810a1" version="25.00.000" type="unit group data set" uri="../unitgroups/0429039d-a61d-4590-ba67-aa4a20a810a1.xml">
          <common:shortDescription xml:lang="en">kg P eq.</common:shortDescription>
        </epd:referenceToUnitGroupDataSet>
      </common:other>
    </LCIAResult>
    <LCIAResult>
      <referenceToLCIAMethodDataSet refObjectId="b5c619fa-def3-11e6-bf01-fe55135034f3" version="21.01.000" type="LCIA method data set" uri="../lciamethods/b5c619fa-def3-11e6-bf01-fe55135034f3.xml">
        <common:shortDescription xml:lang="en">Eutrophication potential - marine (EP-marine)</common:shortDescription>
        <common:shortDescription xml:lang="de">Eutrophierungspotenzial - Salzwasser (EP-marine)</common:shortDescription>
      </referenceToLCIAMethodDataSet>
      <common:other>
        <epd:amount epd:module="A1-A3">26.369585428175</epd:amount>
        <epd:amount epd:module="C1">0.00720656394044638</epd:amount>
        <epd:amount epd:module="C2">0.0278895098517641</epd:amount>
        <epd:amount epd:module="C3">0.0434473073305514</epd:amount>
        <epd:amount epd:module="D">-13.6756624484037</epd:amount>
        <epd:referenceToUnitGroupDataSet refObjectId="d05bb823-ecdf-4686-8c40-bf1d9257859f" version="00.00.003" type="unit group data set" uri="../unitgroups/d05bb823-ecdf-4686-8c40-bf1d9257859f.xml">
          <common:shortDescription xml:lang="en">kg N eq.</common:shortDescription>
        </epd:referenceToUnitGroupDataSet>
      </common:other>
    </LCIAResult>
    <LCIAResult>
      <referenceToLCIAMethodDataSet refObjectId="b5c614d2-def3-11e6-bf01-fe55135034f3" version="21.01.000" type="LCIA method data set" uri="../lciamethods/b5c614d2-def3-11e6-bf01-fe55135034f3.xml">
        <common:shortDescription xml:lang="en">Eutrophication potential - terrestrial (EP-terrestrial)</common:shortDescription>
        <common:shortDescription xml:lang="de">Eutrophierungspotenzial - Land (EP-terrestrial)</common:shortDescription>
      </referenceToLCIAMethodDataSet>
      <common:other>
        <epd:amount epd:module="A1-A3">285.360814708974</epd:amount>
        <epd:amount epd:module="C1">0.0792370263992148</epd:amount>
        <epd:amount epd:module="C2">0.312032905346964</epd:amount>
        <epd:amount epd:module="C3">1.25660165987817</epd:amount>
        <epd:amount epd:module="D">-147.755339615603</epd:amount>
        <epd:referenceToUnitGroupDataSet refObjectId="71b4d617-0ec9-4d3f-b65e-e438940c2401" version="00.00.003" type="unit group data set" uri="../unitgroups/71b4d617-0ec9-4d3f-b65e-e438940c2401.xml">
          <common:shortDescription xml:lang="en">Mole of N eq.</common:shortDescription>
        </epd:referenceToUnitGroupDataSet>
      </common:other>
    </LCIAResult>
    <LCIAResult>
      <referenceToLCIAMethodDataSet refObjectId="b5c610fe-def3-11e6-bf01-fe55135034f3" version="21.01.000" type="LCIA method data set" uri="../lciamethods/b5c610fe-def3-11e6-bf01-fe55135034f3.xml">
        <common:shortDescription xml:lang="en">Photochemical Ozone Creation Potential  (POCP)</common:shortDescription>
        <common:shortDescription xml:lang="de">Bildungspotenzial für troposphärisches Ozon (POCP)</common:shortDescription>
      </referenceToLCIAMethodDataSet>
      <common:other>
        <epd:amount epd:module="A1-A3">82.3811734586499</epd:amount>
        <epd:amount epd:module="C1">0.0215828243738646</epd:amount>
        <epd:amount epd:module="C2">0.0543852004788982</epd:amount>
        <epd:amount epd:module="C3">0.117743864577456</epd:amount>
        <epd:amount epd:module="D">-42.5282494482376</epd:amount>
        <epd:referenceToUnitGroupDataSet refObjectId="d27c25f8-fbc1-44c6-b47b-4adbae4199c6" version="00.00.003" type="unit group data set" uri="../unitgroups/d27c25f8-fbc1-44c6-b47b-4adbae4199c6.xml">
          <common:shortDescription xml:lang="en">kg NMVOC eq.</common:shortDescription>
        </epd:referenceToUnitGroupDataSet>
      </common:other>
    </LCIAResult>
    <LCIAResult>
      <referenceToLCIAMethodDataSet refObjectId="b2ad6494-c78d-11e6-9d9d-cec0c932ce01" version="21.01.000" type="LCIA method data set" uri="../lciamethods/b2ad6494-c78d-11e6-9d9d-cec0c932ce01.xml">
        <common:shortDescription xml:lang="en">Abiotic depletion potential - non-fossil resources (ADPE)</common:shortDescription>
        <common:shortDescription xml:lang="de">Potenzial für die Verknappung abiotischer Ressourcen  nicht fossile Ressourcen (ADPE)</common:shortDescription>
      </referenceToLCIAMethodDataSet>
      <common:other>
        <epd:amount epd:module="A1-A3">2.04347810409298</epd:amount>
        <epd:amount epd:module="C1">1.03898675365841E-7</epd:amount>
        <epd:amount epd:module="C2">1.85739467959994E-6</epd:amount>
        <epd:amount epd:module="C3">3.67715920711767E-6</epd:amount>
        <epd:amount epd:module="D">-1.15733050584516</epd:amount>
        <epd:referenceToUnitGroupDataSet refObjectId="54ccd2d9-a32a-4fc2-923d-f2c8c93e89d4" version="25.00.000" type="unit group data set" uri="../unitgroups/54ccd2d9-a32a-4fc2-923d-f2c8c93e89d4.xml">
          <common:shortDescription xml:lang="en">kg Sb eq.</common:shortDescription>
        </epd:referenceToUnitGroupDataSet>
      </common:other>
    </LCIAResult>
    <LCIAResult>
      <referenceToLCIAMethodDataSet refObjectId="b2ad6110-c78d-11e6-9d9d-cec0c932ce01" version="21.01.000" type="LCIA method data set" uri="../lciamethods/b2ad6110-c78d-11e6-9d9d-cec0c932ce01.xml">
        <common:shortDescription xml:lang="en">Abiotic depletion potential - fossil resources (ADPF)</common:shortDescription>
        <common:shortDescription xml:lang="de">Potenzial für die Verknappung abiotischer Ressourcen  fossile Brennstoffe (ADPF)</common:shortDescription>
      </referenceToLCIAMethodDataSet>
      <common:other>
        <epd:amount epd:module="A1-A3">510536.276564372</epd:amount>
        <epd:amount epd:module="C1">15.8317085875633</epd:amount>
        <epd:amount epd:module="C2">283.023158822527</epd:amount>
        <epd:amount epd:module="C3">285.332619325573</epd:amount>
        <epd:amount epd:module="D">-250066.585108234</epd:amount>
        <epd:referenceToUnitGroupDataSet refObjectId="93a60a57-a3c8-11da-a746-0800200c9a66" version="02.00.000" type="unit group data set" uri="../unitgroups/93a60a57-a3c8-11da-a746-0800200c9a66.xml">
          <common:shortDescription xml:lang="en">MJ</common:shortDescription>
        </epd:referenceToUnitGroupDataSet>
      </common:other>
    </LCIAResult>
    <LCIAResult>
      <referenceToLCIAMethodDataSet refObjectId="b2ad66ce-c78d-11e6-9d9d-cec0c932ce01" version="21.01.000" type="LCIA method data set" uri="../lciamethods/b2ad66ce-c78d-11e6-9d9d-cec0c932ce01.xml">
        <common:shortDescription xml:lang="en">Water (user) deprivation potential (WDP)</common:shortDescription>
        <common:shortDescription xml:lang="de">Wasser-Entzugspotenzial (Benutzer) (WDP)</common:shortDescription>
      </referenceToLCIAMethodDataSet>
      <common:other>
        <epd:amount epd:module="A1-A3">5498.52457684328</epd:amount>
        <epd:amount epd:module="C1">0.0046431543978455</epd:amount>
        <epd:amount epd:module="C2">0.0830055844769166</epd:amount>
        <epd:amount epd:module="C3">160.199948799245</epd:amount>
        <epd:amount epd:module="D">-3940.26610747195</epd:amount>
        <epd:referenceToUnitGroupDataSet refObjectId="6ae2df01-888e-46c8-b17d-49fa3869b476" version="00.00.003" type="unit group data set" uri="../unitgroups/6ae2df01-888e-46c8-b17d-49fa3869b476.xml">
          <common:shortDescription xml:lang="en">m³ world equiv.</common:shortDescription>
        </epd:referenceToUnitGroupDataSet>
      </common:other>
    </LCIAResult>
  </LCIAResults>
</processDataSet>
