<?xml version="1.0" encoding="UTF-8" standalone="yes"?>
<processDataSet xmlns:m="http://lca.jrc.it/ILCD/LCIAMethod" xmlns:common="http://lca.jrc.it/ILCD/Common" xmlns:s="http://lca.jrc.it/ILCD/Source" xmlns:c="http://lca.jrc.it/ILCD/Contact" xmlns:f="http://lca.jrc.it/ILCD/Flow" xmlns="http://lca.jrc.it/ILCD/Process" xmlns:fp="http://lca.jrc.it/ILCD/FlowProperty" xmlns:u="http://lca.jrc.it/ILCD/UnitGroup" xmlns:ns9="http://www.okworx.com/ILCD/Extensions/2018/Profile" xmlns:epd2="http://www.indata.network/EPD/2019" version="1.1" ns9:profile="EN_15804" epd2:epd-version="1.2">
    <processInformation>
        <dataSetInformation>
            <common:UUID>67c0a87a-0750-4439-8b29-3035198d32f9</common:UUID>
            <name>
                <baseName xml:lang="de">Schüco AWS 70.HI Fenstersystem Rahmenprofil (ohne Dreifachverglasung)</baseName>
                <baseName xml:lang="en">Schüco AWS 70.HI frame profile for windows without triple glazing</baseName>
                <functionalUnitFlowProperties xml:lang="de">42,6 kg/m²</functionalUnitFlowProperties>
            </name>
            <common:synonyms xml:lang="de">Fenster, Profil</common:synonyms>
            <classificationInformation>
                <common:classification name="OEKOBAU.DAT">
                    <common:class level="0" classId="7">Komponenten von Fenstern und Vorhangfassaden</common:class>
                    <common:class level="1" classId="7.1">Rahmen / Profile</common:class>
                    <common:class level="2" classId="7.1.05">Aluminium</common:class>
                </common:classification>
            </classificationInformation>
            <common:generalComment xml:lang="de">Aluminium-Rahmenprofil für Fenster (konzipiert für Dreifachverglasung) im Format 1,23 x 1,48 m². &#13;
Als funktionale Einheit wurde ein (virtueller) m² Rahmen festgelegt. Es handelt sich dabei nicht um die Menge &#13;
Rahmen pro m² Produkt, sondern um 1 m² Verglasung bzw. um einen (virtuellen) m² Rahmen, d.h. ein beispielsweise 10 cm breiter und 1 m langer Rahmen wird mit dem Faktor 10 auf 1 m² Rahmen umgerechnet.</common:generalComment>
            <common:generalComment xml:lang="en">Aluminum frame profile for windows (designed for triple glazing) in the format 1.23 x 1.48 m².&#13;
A (virtual) m² frame was defined as a functional unit. It's not about the quantity&#13;
frame per m² of product, but by 1 m² of glazing or a (virtual) m² frame, i.e. a 10 cm wide and 1 m long frame, for example, is converted to 1 m² frame by a factor of 10.</common:generalComment>
            <common:other>
                <epd:scenarios xmlns:epd="http://www.iai.kit.edu/EPD/2013">
                    <epd:scenario epd:name="Recycling">
                        <epd:description>100% Recycling</epd:description>
                    </epd:scenario>
                </epd:scenarios>
            </common:other>
        </dataSetInformation>
        <quantitativeReference type="Reference flow(s)">
            <referenceToReferenceFlow>1</referenceToReferenceFlow>
        </quantitativeReference>
        <time>
            <common:referenceYear>2020</common:referenceYear>
            <common:dataSetValidUntil>2025</common:dataSetValidUntil>
            <common:timeRepresentativenessDescription xml:lang="de">Die Sachbilanzdaten repräsentieren die Produktion der betrachteten &#13;
Schüco Fenstersysteme in Österreich zum Zeitpunkt der &#13;
Deklarationserstellung im Jahr 2020</common:timeRepresentativenessDescription>
            <common:other>
                <epd2:publicationDateOfEPD>2020-05-26</epd2:publicationDateOfEPD>
            </common:other>
        </time>
        <geography>
            <locationOfOperationSupplyOrProduction location="AT"/>
        </geography>
        <technology>
            <technologyDescriptionAndIncludedProcesses xml:lang="de">Rahmenprofil aus Aluminium für Fenster (konzipiert für Dreifach-Verglasung im Format 1,23 x 1,48 m². &#13;
Als funktionale Einheit wurde ein (virtueller m² Rahmen) festgelegt. </technologyDescriptionAndIncludedProcesses>
            <technologyDescriptionAndIncludedProcesses xml:lang="en">Aluminum frame profile for windows (designed for triple glazing in the format 1.23 x 1.48 m².&#13;
A (virtual m² frame) was defined as a functional unit.&#13;
&#13;
&#13;
</technologyDescriptionAndIncludedProcesses>
            <technologicalApplicability xml:lang="en">The products are used in single and multi-storey residential buildings and in non-residential buildings, both indoors and outdoors&#13;
use.</technologicalApplicability>
            <technologicalApplicability xml:lang="de">Die Produkte kommen im ein- und mehrgeschossigen Wohnbau und in Nichtwohngebäuden im Innen- und Außenbereich zur Anwendung. </technologicalApplicability>
        </technology>
    </processInformation>
    <modellingAndValidation>
        <LCIMethodAndAllocation>
            <typeOfDataSet>EPD</typeOfDataSet>
            <referenceToLCAMethodDetails type="source data set" refObjectId="e88110d6-d80e-466e-9ab6-e62ca1aebc79" version="00.00.007">
                <common:shortDescription xml:lang="de">PKR Bau EPD GmbH PKR-Code: 2.21.1 Stand 07.06.2019 "Fenster Tueren Glasfassadenelemente"</common:shortDescription>
            </referenceToLCAMethodDetails>
            <common:other>
                <epd:subType xmlns:epd="http://www.iai.kit.edu/EPD/2013">specific dataset</epd:subType>
            </common:other>
        </LCIMethodAndAllocation>
        <dataSourcesTreatmentAndRepresentativeness>
            <referenceToDataSource type="source data set" refObjectId="ca0da4f4-c837-4005-9c17-e77b9bd09d8b" version="00.00.000">
                <common:shortDescription xml:lang="en">ecoinvent 3.5 database</common:shortDescription>
            </referenceToDataSource>
            <referenceToDataSource type="source data set" refObjectId="b497a91f-e14b-4b69-8f28-f50eb1576766" version="00.03.002">
                <common:shortDescription xml:lang="en">ecoinvent database (general)</common:shortDescription>
            </referenceToDataSource>
            <referenceToDataSource type="source data set" refObjectId="c0cdb43c-2590-411d-8979-5105bab8a373" version="00.00.001">
                <common:shortDescription xml:lang="de">Software: SimaPro 9.0</common:shortDescription>
            </referenceToDataSource>
            <common:other>
                <ns9:referenceToOriginalEPD xmlns:ns9="http://www.indata.network/EPD/2019" refObjectId="2bcdf90a-5f58-4709-80a1-15b2b9ca8530" type="source data set" version="00.00.012">
                    <common:shortDescription xml:lang="de">Bau EPD GmbH EPD Ecoinvent-Schüco AWS Fenstersysteme</common:shortDescription>
                </ns9:referenceToOriginalEPD>
            </common:other>
        </dataSourcesTreatmentAndRepresentativeness>
        <validation>
            <review type="Independent external review">
                <common:referenceToNameOfReviewerAndInstitution type="contact data set" refObjectId="42398bec-0af8-444e-9221-d40be4c4f553" version="00.00.006" uri="http://openlca.org/ilcd/resource/contacts/42398bec-0af8-444e-9221-d40be4c4f553">
                    <common:shortDescription xml:lang="de">Bau EPD GmbH</common:shortDescription>
                    <common:shortDescription xml:lang="en">Richter Sarah</common:shortDescription>
                </common:referenceToNameOfReviewerAndInstitution>
            </review>
        </validation>
        <complianceDeclarations>
            <compliance>
                <common:referenceToComplianceSystem type="source data set" refObjectId="b00f9ec0-7874-11e3-981f-0800200c9a66" version="00.02.000">
                    <common:shortDescription xml:lang="de">EN 15804</common:shortDescription>
                    <common:shortDescription xml:lang="en">EN 15804</common:shortDescription>
                </common:referenceToComplianceSystem>
            </compliance>
            <compliance>
                <common:referenceToComplianceSystem type="source data set" refObjectId="4f2eb655-6e44-4874-a95a-e28f5442cd4d" version="00.00.001">
                    <common:shortDescription xml:lang="en">ISO 14025</common:shortDescription>
                </common:referenceToComplianceSystem>
            </compliance>
        </complianceDeclarations>
        <common:other>
            <norreq:ILCD-SBE xmlns:norreq="http://sbeilcd.se/EPD/2017">
                <norreq:Q-Metadata>
                    <norreq:Question>
                        <norreq:QuestionID>QM0501</norreq:QuestionID>
                        <norreq:QuestionGroup>5. Methodology transparency</norreq:QuestionGroup>
                        <norreq:QuestionAnswer>
                            <norreq:YesNo>false</norreq:YesNo>
                        </norreq:QuestionAnswer>
                    </norreq:Question>
                    <norreq:Question>
                        <norreq:QuestionID>QM0502</norreq:QuestionID>
                        <norreq:QuestionGroup>5. Methodology transparency</norreq:QuestionGroup>
                        <norreq:QuestionAnswer>
                            <norreq:YesNo>false</norreq:YesNo>
                        </norreq:QuestionAnswer>
                    </norreq:Question>
                    <norreq:Question>
                        <norreq:QuestionID>QM0503</norreq:QuestionID>
                        <norreq:QuestionGroup>5. Methodology transparency</norreq:QuestionGroup>
                        <norreq:QuestionAnswer>
                            <norreq:YesNo>false</norreq:YesNo>
                        </norreq:QuestionAnswer>
                    </norreq:Question>
                    <norreq:Question>
                        <norreq:QuestionID>QM0504</norreq:QuestionID>
                        <norreq:QuestionGroup>5. Methodology transparency</norreq:QuestionGroup>
                        <norreq:QuestionAnswer>
                            <norreq:YesNo>false</norreq:YesNo>
                        </norreq:QuestionAnswer>
                    </norreq:Question>
                    <norreq:Question>
                        <norreq:QuestionID>QM0505</norreq:QuestionID>
                        <norreq:QuestionGroup>5. Methodology transparency</norreq:QuestionGroup>
                        <norreq:QuestionAnswer>
                            <norreq:YesNo>false</norreq:YesNo>
                        </norreq:QuestionAnswer>
                    </norreq:Question>
                    <norreq:Question>
                        <norreq:QuestionID>QM0506</norreq:QuestionID>
                        <norreq:QuestionGroup>5. Methodology transparency</norreq:QuestionGroup>
                        <norreq:QuestionAnswer>
                            <norreq:YesNo>false</norreq:YesNo>
                        </norreq:QuestionAnswer>
                    </norreq:Question>
                    <norreq:Question>
                        <norreq:QuestionID>QM0507</norreq:QuestionID>
                        <norreq:QuestionGroup>5. Methodology transparency</norreq:QuestionGroup>
                        <norreq:QuestionAnswer>
                            <norreq:YesNo>false</norreq:YesNo>
                        </norreq:QuestionAnswer>
                    </norreq:Question>
                    <norreq:Question>
                        <norreq:QuestionID>QM0508</norreq:QuestionID>
                        <norreq:QuestionGroup>5. Methodology transparency</norreq:QuestionGroup>
                        <norreq:QuestionAnswer>
                            <norreq:YesNo>false</norreq:YesNo>
                        </norreq:QuestionAnswer>
                    </norreq:Question>
                    <norreq:Question>
                        <norreq:QuestionID>QM0509</norreq:QuestionID>
                        <norreq:QuestionGroup>5. Methodology transparency</norreq:QuestionGroup>
                        <norreq:QuestionAnswer>
                            <norreq:YesNo>false</norreq:YesNo>
                        </norreq:QuestionAnswer>
                    </norreq:Question>
                </norreq:Q-Metadata>
            </norreq:ILCD-SBE>
        </common:other>
    </modellingAndValidation>
    <administrativeInformation>
        <dataGenerator>
            <common:referenceToPersonOrEntityGeneratingTheDataSet type="contact data set" refObjectId="50fccae1-aef9-4e76-acf5-fe0428976e43" version="00.00.002">
                <common:shortDescription xml:lang="de">IBO Institut für Baubiologie und Bauökologie</common:shortDescription>
            </common:referenceToPersonOrEntityGeneratingTheDataSet>
        </dataGenerator>
        <dataEntryBy>
            <common:timeStamp>2022-03-23T13:10:11.874+01:00</common:timeStamp>
            <common:referenceToDataSetFormat type="source data set" refObjectId="a29449fd-aa2f-4de8-b5d7-4b06b43c6fde" version="00.01.000">
                <common:shortDescription xml:lang="en">EPD Data Format Extensions v1.2</common:shortDescription>
                <common:shortDescription xml:lang="de">EPD-Datenformaterweiterungen v1.2</common:shortDescription>
            </common:referenceToDataSetFormat>
            <common:referenceToDataSetFormat type="source data set" refObjectId="a97a0155-0234-4b87-b4ce-a45da52f2a40" version="01.00.000" uri="http://lca.jrc.ec.europa.eu/lcainfohub/sample_data/ilcd/sources/ILCD_Format_a97a0155-0234-4b87-b4ce-a45da52f2a40_01.00.000.xml">
                <common:shortDescription xml:lang="en">ILCD format</common:shortDescription>
            </common:referenceToDataSetFormat>
            <common:referenceToPersonOrEntityEnteringTheData type="contact data set" refObjectId="42398bec-0af8-444e-9221-d40be4c4f553" version="00.00.006" uri="http://openlca.org/ilcd/resource/contacts/42398bec-0af8-444e-9221-d40be4c4f553">
                <common:shortDescription xml:lang="de">Bau EPD GmbH</common:shortDescription>
                <common:shortDescription xml:lang="en">Richter Sarah</common:shortDescription>
            </common:referenceToPersonOrEntityEnteringTheData>
        </dataEntryBy>
        <publicationAndOwnership>
            <common:dataSetVersion>00.00.025</common:dataSetVersion>
            <common:referenceToRegistrationAuthority type="contact data set" refObjectId="42398bec-0af8-444e-9221-d40be4c4f553" version="00.00.006" uri="http://openlca.org/ilcd/resource/contacts/42398bec-0af8-444e-9221-d40be4c4f553">
                <common:shortDescription xml:lang="de">Bau EPD GmbH</common:shortDescription>
                <common:shortDescription xml:lang="en">Richter Sarah</common:shortDescription>
            </common:referenceToRegistrationAuthority>
            <common:registrationNumber>BAU-EPD-ALUKÖNIGSTAHL-2020-1-ECOINVENT-ADS-ADUP</common:registrationNumber>
            <common:referenceToOwnershipOfDataSet type="contact data set" refObjectId="9131cae7-5c35-4b9f-bbc7-4bf7c38758d2" version="00.00.001">
                <common:shortDescription xml:lang="de">AluKönigStahl GmbH</common:shortDescription>
            </common:referenceToOwnershipOfDataSet>
            <common:copyright>true</common:copyright>
            <common:licenseType>Free of charge for all users and uses</common:licenseType>
            <common:accessRestrictions xml:lang="de">Keine</common:accessRestrictions>
            <common:other>
                <ns9:referenceToPublisher xmlns:ns9="http://www.indata.network/EPD/2019" refObjectId="42398bec-0af8-444e-9221-d40be4c4f553" type="contact data set" uri="http://openlca.org/ilcd/resource/contacts/42398bec-0af8-444e-9221-d40be4c4f553" version="00.00.004">
                    <common:shortDescription xml:lang="en">Richter Sarah</common:shortDescription>
                    <common:shortDescription xml:lang="de">Bau EPD GmbH - DI Sarah Richter</common:shortDescription>
                </ns9:referenceToPublisher>
            </common:other>
        </publicationAndOwnership>
    </administrativeInformation>
    <exchanges>
        <exchange dataSetInternalID="1">
            <referenceToFlowDataSet type="flow data set" refObjectId="6c836eb7-6822-4dfd-9975-729e37bef86c" version="00.00.004">
                <common:shortDescription xml:lang="de">Schüco AWS 70.HI Fenstersystem Rahmenprofil (ohne Dreifachverglasung)</common:shortDescription>
            </referenceToFlowDataSet>
            <meanAmount>1.0</meanAmount>
            <resultingAmount>1.0</resultingAmount>
        </exchange>
        <exchange dataSetInternalID="2">
            <referenceToFlowDataSet type="flow data set" refObjectId="20f32be5-0398-4288-9b6d-accddd195317" version="30.00.000">
                <common:shortDescription xml:lang="en">Use of renewable primary energy (PERE)</common:shortDescription>
                <common:shortDescription xml:lang="de">Erneuerbare Primärenergie als Energieträger (PERE)</common:shortDescription>
                <common:shortDescription xml:lang="es">Uso de energía primaria renovable excluyendo los recursos de energía primaria renovable utilizada como materia prima (PERE)</common:shortDescription>
            </referenceToFlowDataSet>
            <functionType>General reminder flow</functionType>
            <exchangeDirection>Input</exchangeDirection>
            <meanAmount>0.0</meanAmount>
            <common:other>
                <epd:amount xmlns:epd="http://www.iai.kit.edu/EPD/2013" epd:module="C1" epd:scenario="Recycling">0.23175552587419182</epd:amount>
                <epd:amount xmlns:epd="http://www.iai.kit.edu/EPD/2013" epd:module="C2" epd:scenario="Recycling">0.1673501523027087</epd:amount>
                <epd:amount xmlns:epd="http://www.iai.kit.edu/EPD/2013" epd:module="C3" epd:scenario="Recycling">0.19432226295513855</epd:amount>
                <epd:amount xmlns:epd="http://www.iai.kit.edu/EPD/2013" epd:module="C4" epd:scenario="Recycling">0.0</epd:amount>
                <epd:amount xmlns:epd="http://www.iai.kit.edu/EPD/2013" epd:module="D" epd:scenario="Recycling">-733.9981601148806</epd:amount>
                <epd:amount xmlns:epd="http://www.iai.kit.edu/EPD/2013" epd:module="A1"/>
                <epd:amount xmlns:epd="http://www.iai.kit.edu/EPD/2013" epd:module="A1-A3">512.4791979930408</epd:amount>
                <epd:amount xmlns:epd="http://www.iai.kit.edu/EPD/2013" epd:module="A2"/>
                <epd:amount xmlns:epd="http://www.iai.kit.edu/EPD/2013" epd:module="A3"/>
                <epd:amount xmlns:epd="http://www.iai.kit.edu/EPD/2013" epd:module="A4">0.5690480484178644</epd:amount>
                <epd:amount xmlns:epd="http://www.iai.kit.edu/EPD/2013" epd:module="A5">0.23175554283586078</epd:amount>
                <epd:amount xmlns:epd="http://www.iai.kit.edu/EPD/2013" epd:module="B1"/>
                <epd:amount xmlns:epd="http://www.iai.kit.edu/EPD/2013" epd:module="B2"/>
                <epd:amount xmlns:epd="http://www.iai.kit.edu/EPD/2013" epd:module="B3"/>
                <epd:amount xmlns:epd="http://www.iai.kit.edu/EPD/2013" epd:module="B4"/>
                <epd:amount xmlns:epd="http://www.iai.kit.edu/EPD/2013" epd:module="B5"/>
                <epd:amount xmlns:epd="http://www.iai.kit.edu/EPD/2013" epd:module="B6"/>
                <epd:amount xmlns:epd="http://www.iai.kit.edu/EPD/2013" epd:module="B7"/>
                <epd:amount xmlns:epd="http://www.iai.kit.edu/EPD/2013" epd:module="C1"/>
                <epd:amount xmlns:epd="http://www.iai.kit.edu/EPD/2013" epd:module="C2"/>
                <epd:amount xmlns:epd="http://www.iai.kit.edu/EPD/2013" epd:module="C3"/>
                <epd:amount xmlns:epd="http://www.iai.kit.edu/EPD/2013" epd:module="C4"/>
                <epd:amount xmlns:epd="http://www.iai.kit.edu/EPD/2013" epd:module="D"/>
                <epd:referenceToUnitGroupDataSet xmlns:epd="http://www.iai.kit.edu/EPD/2013" refObjectId="93a60a57-a3c8-11da-a746-0800200c9a66" type="unit group data set" uri="../unitgroups/93a60a57-a3c8-11da-a746-0800200c9a66">
                    <common:shortDescription>MJ</common:shortDescription>
                </epd:referenceToUnitGroupDataSet>
            </common:other>
        </exchange>
        <exchange dataSetInternalID="3">
            <referenceToFlowDataSet type="flow data set" refObjectId="fb3ec0de-548d-4508-aea5-00b73bf6f702" version="30.00.000">
                <common:shortDescription xml:lang="en">Use of renewable primary energy resources used as raw materials (PERM)</common:shortDescription>
                <common:shortDescription xml:lang="de">Erneuerbare Primärenergie zur stofflichen Nutzung (PERM)</common:shortDescription>
                <common:shortDescription xml:lang="es">Uso de energía primaria renovable utilizada como materia prima (PERM)</common:shortDescription>
            </referenceToFlowDataSet>
            <functionType>General reminder flow</functionType>
            <exchangeDirection>Input</exchangeDirection>
            <meanAmount>0.0</meanAmount>
            <common:other>
                <epd:amount xmlns:epd="http://www.iai.kit.edu/EPD/2013" epd:module="C1" epd:scenario="Recycling">0.0</epd:amount>
                <epd:amount xmlns:epd="http://www.iai.kit.edu/EPD/2013" epd:module="C2" epd:scenario="Recycling">0.0</epd:amount>
                <epd:amount xmlns:epd="http://www.iai.kit.edu/EPD/2013" epd:module="C3" epd:scenario="Recycling">0.0</epd:amount>
                <epd:amount xmlns:epd="http://www.iai.kit.edu/EPD/2013" epd:module="C4" epd:scenario="Recycling">0.0</epd:amount>
                <epd:amount xmlns:epd="http://www.iai.kit.edu/EPD/2013" epd:module="D" epd:scenario="Recycling">0.0</epd:amount>
                <epd:amount xmlns:epd="http://www.iai.kit.edu/EPD/2013" epd:module="A1"/>
                <epd:amount xmlns:epd="http://www.iai.kit.edu/EPD/2013" epd:module="A1-A3">0.0</epd:amount>
                <epd:amount xmlns:epd="http://www.iai.kit.edu/EPD/2013" epd:module="A2"/>
                <epd:amount xmlns:epd="http://www.iai.kit.edu/EPD/2013" epd:module="A3"/>
                <epd:amount xmlns:epd="http://www.iai.kit.edu/EPD/2013" epd:module="A4">0.0</epd:amount>
                <epd:amount xmlns:epd="http://www.iai.kit.edu/EPD/2013" epd:module="A5">0.0</epd:amount>
                <epd:amount xmlns:epd="http://www.iai.kit.edu/EPD/2013" epd:module="B1"/>
                <epd:amount xmlns:epd="http://www.iai.kit.edu/EPD/2013" epd:module="B2"/>
                <epd:amount xmlns:epd="http://www.iai.kit.edu/EPD/2013" epd:module="B3"/>
                <epd:amount xmlns:epd="http://www.iai.kit.edu/EPD/2013" epd:module="B4"/>
                <epd:amount xmlns:epd="http://www.iai.kit.edu/EPD/2013" epd:module="B5"/>
                <epd:amount xmlns:epd="http://www.iai.kit.edu/EPD/2013" epd:module="B6"/>
                <epd:amount xmlns:epd="http://www.iai.kit.edu/EPD/2013" epd:module="B7"/>
                <epd:amount xmlns:epd="http://www.iai.kit.edu/EPD/2013" epd:module="C1"/>
                <epd:amount xmlns:epd="http://www.iai.kit.edu/EPD/2013" epd:module="C2"/>
                <epd:amount xmlns:epd="http://www.iai.kit.edu/EPD/2013" epd:module="C3"/>
                <epd:amount xmlns:epd="http://www.iai.kit.edu/EPD/2013" epd:module="C4"/>
                <epd:amount xmlns:epd="http://www.iai.kit.edu/EPD/2013" epd:module="D"/>
                <epd:referenceToUnitGroupDataSet xmlns:epd="http://www.iai.kit.edu/EPD/2013" refObjectId="93a60a57-a3c8-11da-a746-0800200c9a66" type="unit group data set" uri="../unitgroups/93a60a57-a3c8-11da-a746-0800200c9a66">
                    <common:shortDescription>MJ</common:shortDescription>
                </epd:referenceToUnitGroupDataSet>
            </common:other>
        </exchange>
        <exchange dataSetInternalID="4">
            <referenceToFlowDataSet type="flow data set" refObjectId="53f97275-fa8a-4cdd-9024-65936002acd0" version="30.00.000">
                <common:shortDescription xml:lang="en">Total use of renewable primary energy resources (PERT)</common:shortDescription>
                <common:shortDescription xml:lang="de">Total erneuerbare Primärenergie (PERT)</common:shortDescription>
                <common:shortDescription xml:lang="es">Uso total de la energía primaria renovable (energía primaria y recursos de energía primaria renovable utilizada como materia prima) (PERT)</common:shortDescription>
            </referenceToFlowDataSet>
            <functionType>General reminder flow</functionType>
            <exchangeDirection>Input</exchangeDirection>
            <meanAmount>0.0</meanAmount>
            <common:other>
                <epd:amount xmlns:epd="http://www.iai.kit.edu/EPD/2013" epd:module="C1" epd:scenario="Recycling">0.23175552587419182</epd:amount>
                <epd:amount xmlns:epd="http://www.iai.kit.edu/EPD/2013" epd:module="C2" epd:scenario="Recycling">0.1673501523027087</epd:amount>
                <epd:amount xmlns:epd="http://www.iai.kit.edu/EPD/2013" epd:module="C3" epd:scenario="Recycling">0.19432226295513855</epd:amount>
                <epd:amount xmlns:epd="http://www.iai.kit.edu/EPD/2013" epd:module="C4" epd:scenario="Recycling">0.0</epd:amount>
                <epd:amount xmlns:epd="http://www.iai.kit.edu/EPD/2013" epd:module="D" epd:scenario="Recycling">-733.9981601148806</epd:amount>
                <epd:amount xmlns:epd="http://www.iai.kit.edu/EPD/2013" epd:module="A1"/>
                <epd:amount xmlns:epd="http://www.iai.kit.edu/EPD/2013" epd:module="A1-A3">512.4791979930408</epd:amount>
                <epd:amount xmlns:epd="http://www.iai.kit.edu/EPD/2013" epd:module="A2"/>
                <epd:amount xmlns:epd="http://www.iai.kit.edu/EPD/2013" epd:module="A3"/>
                <epd:amount xmlns:epd="http://www.iai.kit.edu/EPD/2013" epd:module="A4">0.5690480484178644</epd:amount>
                <epd:amount xmlns:epd="http://www.iai.kit.edu/EPD/2013" epd:module="A5">0.23175554283586078</epd:amount>
                <epd:amount xmlns:epd="http://www.iai.kit.edu/EPD/2013" epd:module="B1"/>
                <epd:amount xmlns:epd="http://www.iai.kit.edu/EPD/2013" epd:module="B2"/>
                <epd:amount xmlns:epd="http://www.iai.kit.edu/EPD/2013" epd:module="B3"/>
                <epd:amount xmlns:epd="http://www.iai.kit.edu/EPD/2013" epd:module="B4"/>
                <epd:amount xmlns:epd="http://www.iai.kit.edu/EPD/2013" epd:module="B5"/>
                <epd:amount xmlns:epd="http://www.iai.kit.edu/EPD/2013" epd:module="B6"/>
                <epd:amount xmlns:epd="http://www.iai.kit.edu/EPD/2013" epd:module="B7"/>
                <epd:amount xmlns:epd="http://www.iai.kit.edu/EPD/2013" epd:module="C1"/>
                <epd:amount xmlns:epd="http://www.iai.kit.edu/EPD/2013" epd:module="C2"/>
                <epd:amount xmlns:epd="http://www.iai.kit.edu/EPD/2013" epd:module="C3"/>
                <epd:amount xmlns:epd="http://www.iai.kit.edu/EPD/2013" epd:module="C4"/>
                <epd:amount xmlns:epd="http://www.iai.kit.edu/EPD/2013" epd:module="D"/>
                <epd:referenceToUnitGroupDataSet xmlns:epd="http://www.iai.kit.edu/EPD/2013" refObjectId="93a60a57-a3c8-11da-a746-0800200c9a66" type="unit group data set" uri="../unitgroups/93a60a57-a3c8-11da-a746-0800200c9a66">
                    <common:shortDescription>MJ</common:shortDescription>
                </epd:referenceToUnitGroupDataSet>
            </common:other>
        </exchange>
        <exchange dataSetInternalID="5">
            <referenceToFlowDataSet type="flow data set" refObjectId="ac857178-2b45-46ec-892a-a9a4332f0372" version="30.00.000">
                <common:shortDescription xml:lang="en">Use of non renewable primary energy (PENRE)</common:shortDescription>
                <common:shortDescription xml:lang="de">Nicht-erneuerbare Primärenergie als Energieträger (PENRE)</common:shortDescription>
                <common:shortDescription xml:lang="es">Uso de energía primaria no renovable, excluyendo los recursos de energía primaria no renovable utilizada como materia prima (PENRE)</common:shortDescription>
            </referenceToFlowDataSet>
            <functionType>General reminder flow</functionType>
            <exchangeDirection>Input</exchangeDirection>
            <meanAmount>0.0</meanAmount>
            <common:other>
                <epd:amount xmlns:epd="http://www.iai.kit.edu/EPD/2013" epd:module="C1" epd:scenario="Recycling">41.41115931730407</epd:amount>
                <epd:amount xmlns:epd="http://www.iai.kit.edu/EPD/2013" epd:module="C2" epd:scenario="Recycling">16.80175035126179</epd:amount>
                <epd:amount xmlns:epd="http://www.iai.kit.edu/EPD/2013" epd:module="C3" epd:scenario="Recycling">6.298224148405893</epd:amount>
                <epd:amount xmlns:epd="http://www.iai.kit.edu/EPD/2013" epd:module="C4" epd:scenario="Recycling">0.0</epd:amount>
                <epd:amount xmlns:epd="http://www.iai.kit.edu/EPD/2013" epd:module="D" epd:scenario="Recycling">-1737.0591869986054</epd:amount>
                <epd:amount xmlns:epd="http://www.iai.kit.edu/EPD/2013" epd:module="A1"/>
                <epd:amount xmlns:epd="http://www.iai.kit.edu/EPD/2013" epd:module="A1-A3">4356.557464479517</epd:amount>
                <epd:amount xmlns:epd="http://www.iai.kit.edu/EPD/2013" epd:module="A2"/>
                <epd:amount xmlns:epd="http://www.iai.kit.edu/EPD/2013" epd:module="A3"/>
                <epd:amount xmlns:epd="http://www.iai.kit.edu/EPD/2013" epd:module="A4">57.131723702535965</epd:amount>
                <epd:amount xmlns:epd="http://www.iai.kit.edu/EPD/2013" epd:module="A5">41.41115479419236</epd:amount>
                <epd:amount xmlns:epd="http://www.iai.kit.edu/EPD/2013" epd:module="B1"/>
                <epd:amount xmlns:epd="http://www.iai.kit.edu/EPD/2013" epd:module="B2"/>
                <epd:amount xmlns:epd="http://www.iai.kit.edu/EPD/2013" epd:module="B3"/>
                <epd:amount xmlns:epd="http://www.iai.kit.edu/EPD/2013" epd:module="B4"/>
                <epd:amount xmlns:epd="http://www.iai.kit.edu/EPD/2013" epd:module="B5"/>
                <epd:amount xmlns:epd="http://www.iai.kit.edu/EPD/2013" epd:module="B6"/>
                <epd:amount xmlns:epd="http://www.iai.kit.edu/EPD/2013" epd:module="B7"/>
                <epd:amount xmlns:epd="http://www.iai.kit.edu/EPD/2013" epd:module="C1"/>
                <epd:amount xmlns:epd="http://www.iai.kit.edu/EPD/2013" epd:module="C2"/>
                <epd:amount xmlns:epd="http://www.iai.kit.edu/EPD/2013" epd:module="C3"/>
                <epd:amount xmlns:epd="http://www.iai.kit.edu/EPD/2013" epd:module="C4"/>
                <epd:amount xmlns:epd="http://www.iai.kit.edu/EPD/2013" epd:module="D"/>
                <epd:referenceToUnitGroupDataSet xmlns:epd="http://www.iai.kit.edu/EPD/2013" refObjectId="93a60a57-a3c8-11da-a746-0800200c9a66" type="unit group data set" uri="../unitgroups/93a60a57-a3c8-11da-a746-0800200c9a66">
                    <common:shortDescription>MJ</common:shortDescription>
                </epd:referenceToUnitGroupDataSet>
            </common:other>
        </exchange>
        <exchange dataSetInternalID="6">
            <referenceToFlowDataSet type="flow data set" refObjectId="1421caa0-679d-4bf4-b282-0eb850ccae27" version="30.00.000">
                <common:shortDescription xml:lang="en">Use of non renewable primary energy resources used as raw materials (PENRM)</common:shortDescription>
                <common:shortDescription xml:lang="de">Nicht-erneuerbare Primärenergie zur stofflichen Nutzung (PENRM)</common:shortDescription>
                <common:shortDescription xml:lang="es">Uso de la energía primaria no renovable utilizada como materia prima (PENRM)</common:shortDescription>
            </referenceToFlowDataSet>
            <functionType>General reminder flow</functionType>
            <exchangeDirection>Input</exchangeDirection>
            <meanAmount>0.0</meanAmount>
            <common:other>
                <epd:amount xmlns:epd="http://www.iai.kit.edu/EPD/2013" epd:module="C1" epd:scenario="Recycling">0.0</epd:amount>
                <epd:amount xmlns:epd="http://www.iai.kit.edu/EPD/2013" epd:module="C2" epd:scenario="Recycling">0.0</epd:amount>
                <epd:amount xmlns:epd="http://www.iai.kit.edu/EPD/2013" epd:module="C3" epd:scenario="Recycling">0.0</epd:amount>
                <epd:amount xmlns:epd="http://www.iai.kit.edu/EPD/2013" epd:module="C4" epd:scenario="Recycling">0.0</epd:amount>
                <epd:amount xmlns:epd="http://www.iai.kit.edu/EPD/2013" epd:module="D" epd:scenario="Recycling">0.0</epd:amount>
                <epd:amount xmlns:epd="http://www.iai.kit.edu/EPD/2013" epd:module="A1"/>
                <epd:amount xmlns:epd="http://www.iai.kit.edu/EPD/2013" epd:module="A1-A3">327.37643773386907</epd:amount>
                <epd:amount xmlns:epd="http://www.iai.kit.edu/EPD/2013" epd:module="A2"/>
                <epd:amount xmlns:epd="http://www.iai.kit.edu/EPD/2013" epd:module="A3"/>
                <epd:amount xmlns:epd="http://www.iai.kit.edu/EPD/2013" epd:module="A4">0.0</epd:amount>
                <epd:amount xmlns:epd="http://www.iai.kit.edu/EPD/2013" epd:module="A5">0.0</epd:amount>
                <epd:amount xmlns:epd="http://www.iai.kit.edu/EPD/2013" epd:module="B1"/>
                <epd:amount xmlns:epd="http://www.iai.kit.edu/EPD/2013" epd:module="B2"/>
                <epd:amount xmlns:epd="http://www.iai.kit.edu/EPD/2013" epd:module="B3"/>
                <epd:amount xmlns:epd="http://www.iai.kit.edu/EPD/2013" epd:module="B4"/>
                <epd:amount xmlns:epd="http://www.iai.kit.edu/EPD/2013" epd:module="B5"/>
                <epd:amount xmlns:epd="http://www.iai.kit.edu/EPD/2013" epd:module="B6"/>
                <epd:amount xmlns:epd="http://www.iai.kit.edu/EPD/2013" epd:module="B7"/>
                <epd:amount xmlns:epd="http://www.iai.kit.edu/EPD/2013" epd:module="C1"/>
                <epd:amount xmlns:epd="http://www.iai.kit.edu/EPD/2013" epd:module="C2"/>
                <epd:amount xmlns:epd="http://www.iai.kit.edu/EPD/2013" epd:module="C3"/>
                <epd:amount xmlns:epd="http://www.iai.kit.edu/EPD/2013" epd:module="C4"/>
                <epd:amount xmlns:epd="http://www.iai.kit.edu/EPD/2013" epd:module="D"/>
                <epd:referenceToUnitGroupDataSet xmlns:epd="http://www.iai.kit.edu/EPD/2013" refObjectId="93a60a57-a3c8-11da-a746-0800200c9a66" type="unit group data set" uri="../unitgroups/93a60a57-a3c8-11da-a746-0800200c9a66">
                    <common:shortDescription>MJ</common:shortDescription>
                </epd:referenceToUnitGroupDataSet>
            </common:other>
        </exchange>
        <exchange dataSetInternalID="7">
            <referenceToFlowDataSet type="flow data set" refObjectId="06159210-646b-4c8d-8583-da9b3b95a6c1" version="30.00.000">
                <common:shortDescription xml:lang="en">Total use of non renewable primary energy resource (PENRT)</common:shortDescription>
                <common:shortDescription xml:lang="de">Total nicht erneuerbare Primärenergie (PENRT)</common:shortDescription>
                <common:shortDescription xml:lang="es">Uso total de la energía primaria no renovable (energía primaria y recursos de energía primaria renovable utilizada como materia prima) (PENRT)</common:shortDescription>
            </referenceToFlowDataSet>
            <functionType>General reminder flow</functionType>
            <exchangeDirection>Input</exchangeDirection>
            <meanAmount>0.0</meanAmount>
            <common:other>
                <epd:amount xmlns:epd="http://www.iai.kit.edu/EPD/2013" epd:module="C1" epd:scenario="Recycling">41.41115931730407</epd:amount>
                <epd:amount xmlns:epd="http://www.iai.kit.edu/EPD/2013" epd:module="C2" epd:scenario="Recycling">16.80175035126179</epd:amount>
                <epd:amount xmlns:epd="http://www.iai.kit.edu/EPD/2013" epd:module="C3" epd:scenario="Recycling">6.298224148405893</epd:amount>
                <epd:amount xmlns:epd="http://www.iai.kit.edu/EPD/2013" epd:module="C4" epd:scenario="Recycling">0.0</epd:amount>
                <epd:amount xmlns:epd="http://www.iai.kit.edu/EPD/2013" epd:module="D" epd:scenario="Recycling">-1737.0591869986054</epd:amount>
                <epd:amount xmlns:epd="http://www.iai.kit.edu/EPD/2013" epd:module="A1"/>
                <epd:amount xmlns:epd="http://www.iai.kit.edu/EPD/2013" epd:module="A1-A3">4683.933902213385</epd:amount>
                <epd:amount xmlns:epd="http://www.iai.kit.edu/EPD/2013" epd:module="A2"/>
                <epd:amount xmlns:epd="http://www.iai.kit.edu/EPD/2013" epd:module="A3"/>
                <epd:amount xmlns:epd="http://www.iai.kit.edu/EPD/2013" epd:module="A4">57.131723702535965</epd:amount>
                <epd:amount xmlns:epd="http://www.iai.kit.edu/EPD/2013" epd:module="A5">41.41115479419236</epd:amount>
                <epd:amount xmlns:epd="http://www.iai.kit.edu/EPD/2013" epd:module="B1"/>
                <epd:amount xmlns:epd="http://www.iai.kit.edu/EPD/2013" epd:module="B2"/>
                <epd:amount xmlns:epd="http://www.iai.kit.edu/EPD/2013" epd:module="B3"/>
                <epd:amount xmlns:epd="http://www.iai.kit.edu/EPD/2013" epd:module="B4"/>
                <epd:amount xmlns:epd="http://www.iai.kit.edu/EPD/2013" epd:module="B5"/>
                <epd:amount xmlns:epd="http://www.iai.kit.edu/EPD/2013" epd:module="B6"/>
                <epd:amount xmlns:epd="http://www.iai.kit.edu/EPD/2013" epd:module="B7"/>
                <epd:amount xmlns:epd="http://www.iai.kit.edu/EPD/2013" epd:module="C1"/>
                <epd:amount xmlns:epd="http://www.iai.kit.edu/EPD/2013" epd:module="C2"/>
                <epd:amount xmlns:epd="http://www.iai.kit.edu/EPD/2013" epd:module="C3"/>
                <epd:amount xmlns:epd="http://www.iai.kit.edu/EPD/2013" epd:module="C4"/>
                <epd:amount xmlns:epd="http://www.iai.kit.edu/EPD/2013" epd:module="D"/>
                <epd:referenceToUnitGroupDataSet xmlns:epd="http://www.iai.kit.edu/EPD/2013" refObjectId="93a60a57-a3c8-11da-a746-0800200c9a66" type="unit group data set" uri="../unitgroups/93a60a57-a3c8-11da-a746-0800200c9a66">
                    <common:shortDescription>MJ</common:shortDescription>
                </epd:referenceToUnitGroupDataSet>
            </common:other>
        </exchange>
        <exchange dataSetInternalID="8">
            <referenceToFlowDataSet type="flow data set" refObjectId="c6a1f35f-2d09-4f54-8dfb-97e502e1ce92" version="30.00.000">
                <common:shortDescription xml:lang="en">Use of secondary material (SM)</common:shortDescription>
                <common:shortDescription xml:lang="de">Einsatz von Sekundärstoffen (SM)</common:shortDescription>
                <common:shortDescription xml:lang="es">Uso de materiales secundarios (SM)</common:shortDescription>
            </referenceToFlowDataSet>
            <functionType>General reminder flow</functionType>
            <exchangeDirection>Input</exchangeDirection>
            <meanAmount>0.0</meanAmount>
            <common:other>
                <epd:amount xmlns:epd="http://www.iai.kit.edu/EPD/2013" epd:module="C1" epd:scenario="Recycling">0.0</epd:amount>
                <epd:amount xmlns:epd="http://www.iai.kit.edu/EPD/2013" epd:module="C2" epd:scenario="Recycling">0.0</epd:amount>
                <epd:amount xmlns:epd="http://www.iai.kit.edu/EPD/2013" epd:module="C3" epd:scenario="Recycling">0.0</epd:amount>
                <epd:amount xmlns:epd="http://www.iai.kit.edu/EPD/2013" epd:module="C4" epd:scenario="Recycling">0.0</epd:amount>
                <epd:amount xmlns:epd="http://www.iai.kit.edu/EPD/2013" epd:module="D" epd:scenario="Recycling">0.0</epd:amount>
                <epd:amount xmlns:epd="http://www.iai.kit.edu/EPD/2013" epd:module="A1"/>
                <epd:amount xmlns:epd="http://www.iai.kit.edu/EPD/2013" epd:module="A1-A3">11.956146528036673</epd:amount>
                <epd:amount xmlns:epd="http://www.iai.kit.edu/EPD/2013" epd:module="A2"/>
                <epd:amount xmlns:epd="http://www.iai.kit.edu/EPD/2013" epd:module="A3"/>
                <epd:amount xmlns:epd="http://www.iai.kit.edu/EPD/2013" epd:module="A4">0.0</epd:amount>
                <epd:amount xmlns:epd="http://www.iai.kit.edu/EPD/2013" epd:module="A5">0.0</epd:amount>
                <epd:amount xmlns:epd="http://www.iai.kit.edu/EPD/2013" epd:module="B1"/>
                <epd:amount xmlns:epd="http://www.iai.kit.edu/EPD/2013" epd:module="B2"/>
                <epd:amount xmlns:epd="http://www.iai.kit.edu/EPD/2013" epd:module="B3"/>
                <epd:amount xmlns:epd="http://www.iai.kit.edu/EPD/2013" epd:module="B4"/>
                <epd:amount xmlns:epd="http://www.iai.kit.edu/EPD/2013" epd:module="B5"/>
                <epd:amount xmlns:epd="http://www.iai.kit.edu/EPD/2013" epd:module="B6"/>
                <epd:amount xmlns:epd="http://www.iai.kit.edu/EPD/2013" epd:module="B7"/>
                <epd:amount xmlns:epd="http://www.iai.kit.edu/EPD/2013" epd:module="C1"/>
                <epd:amount xmlns:epd="http://www.iai.kit.edu/EPD/2013" epd:module="C2"/>
                <epd:amount xmlns:epd="http://www.iai.kit.edu/EPD/2013" epd:module="C3"/>
                <epd:amount xmlns:epd="http://www.iai.kit.edu/EPD/2013" epd:module="C4"/>
                <epd:amount xmlns:epd="http://www.iai.kit.edu/EPD/2013" epd:module="D"/>
                <epd:referenceToUnitGroupDataSet xmlns:epd="http://www.iai.kit.edu/EPD/2013" refObjectId="ad38d542-3fe9-439d-9b95-2f5f7752acaf" type="unit group data set" uri="../unitgroups/ad38d542-3fe9-439d-9b95-2f5f7752acaf">
                    <common:shortDescription>kg</common:shortDescription>
                </epd:referenceToUnitGroupDataSet>
            </common:other>
        </exchange>
        <exchange dataSetInternalID="9">
            <referenceToFlowDataSet type="flow data set" refObjectId="64333088-a55f-4aa2-9a31-c10b07816787" version="30.00.000">
                <common:shortDescription xml:lang="en">Use of renewable secondary fuels (RSF)</common:shortDescription>
                <common:shortDescription xml:lang="de">Erneuerbare Sekundärbrennstoffe (RSF)</common:shortDescription>
                <common:shortDescription xml:lang="es">Uso de combustibles secundarios renovables (RSF)</common:shortDescription>
            </referenceToFlowDataSet>
            <functionType>General reminder flow</functionType>
            <exchangeDirection>Input</exchangeDirection>
            <meanAmount>0.0</meanAmount>
            <common:other>
                <epd:amount xmlns:epd="http://www.iai.kit.edu/EPD/2013" epd:module="C1" epd:scenario="Recycling">0.0</epd:amount>
                <epd:amount xmlns:epd="http://www.iai.kit.edu/EPD/2013" epd:module="C2" epd:scenario="Recycling">0.0</epd:amount>
                <epd:amount xmlns:epd="http://www.iai.kit.edu/EPD/2013" epd:module="C3" epd:scenario="Recycling">0.0</epd:amount>
                <epd:amount xmlns:epd="http://www.iai.kit.edu/EPD/2013" epd:module="C4" epd:scenario="Recycling">0.0</epd:amount>
                <epd:amount xmlns:epd="http://www.iai.kit.edu/EPD/2013" epd:module="D" epd:scenario="Recycling">0.0</epd:amount>
                <epd:amount xmlns:epd="http://www.iai.kit.edu/EPD/2013" epd:module="A1"/>
                <epd:amount xmlns:epd="http://www.iai.kit.edu/EPD/2013" epd:module="A1-A3">0.0</epd:amount>
                <epd:amount xmlns:epd="http://www.iai.kit.edu/EPD/2013" epd:module="A2"/>
                <epd:amount xmlns:epd="http://www.iai.kit.edu/EPD/2013" epd:module="A3"/>
                <epd:amount xmlns:epd="http://www.iai.kit.edu/EPD/2013" epd:module="A4">0.0</epd:amount>
                <epd:amount xmlns:epd="http://www.iai.kit.edu/EPD/2013" epd:module="A5">0.0</epd:amount>
                <epd:amount xmlns:epd="http://www.iai.kit.edu/EPD/2013" epd:module="B1"/>
                <epd:amount xmlns:epd="http://www.iai.kit.edu/EPD/2013" epd:module="B2"/>
                <epd:amount xmlns:epd="http://www.iai.kit.edu/EPD/2013" epd:module="B3"/>
                <epd:amount xmlns:epd="http://www.iai.kit.edu/EPD/2013" epd:module="B4"/>
                <epd:amount xmlns:epd="http://www.iai.kit.edu/EPD/2013" epd:module="B5"/>
                <epd:amount xmlns:epd="http://www.iai.kit.edu/EPD/2013" epd:module="B6"/>
                <epd:amount xmlns:epd="http://www.iai.kit.edu/EPD/2013" epd:module="B7"/>
                <epd:amount xmlns:epd="http://www.iai.kit.edu/EPD/2013" epd:module="C1"/>
                <epd:amount xmlns:epd="http://www.iai.kit.edu/EPD/2013" epd:module="C2"/>
                <epd:amount xmlns:epd="http://www.iai.kit.edu/EPD/2013" epd:module="C3"/>
                <epd:amount xmlns:epd="http://www.iai.kit.edu/EPD/2013" epd:module="C4"/>
                <epd:amount xmlns:epd="http://www.iai.kit.edu/EPD/2013" epd:module="D"/>
                <epd:referenceToUnitGroupDataSet xmlns:epd="http://www.iai.kit.edu/EPD/2013" refObjectId="93a60a57-a3c8-11da-a746-0800200c9a66" type="unit group data set" uri="../unitgroups/93a60a57-a3c8-11da-a746-0800200c9a66">
                    <common:shortDescription>MJ</common:shortDescription>
                </epd:referenceToUnitGroupDataSet>
            </common:other>
        </exchange>
        <exchange dataSetInternalID="10">
            <referenceToFlowDataSet type="flow data set" refObjectId="89def144-d39a-4287-b86f-efde453ddcb2" version="30.00.000">
                <common:shortDescription xml:lang="en">Use of non renewable secondary fuels (NRSF)</common:shortDescription>
                <common:shortDescription xml:lang="de">Nicht erneuerbare Sekundärbrennstoffe (NRSF)</common:shortDescription>
                <common:shortDescription xml:lang="es">Uso de combustibles secundarios no renovables (NRSF)</common:shortDescription>
            </referenceToFlowDataSet>
            <functionType>General reminder flow</functionType>
            <exchangeDirection>Input</exchangeDirection>
            <meanAmount>0.0</meanAmount>
            <common:other>
                <epd:amount xmlns:epd="http://www.iai.kit.edu/EPD/2013" epd:module="C1" epd:scenario="Recycling">0.0</epd:amount>
                <epd:amount xmlns:epd="http://www.iai.kit.edu/EPD/2013" epd:module="C2" epd:scenario="Recycling">0.0</epd:amount>
                <epd:amount xmlns:epd="http://www.iai.kit.edu/EPD/2013" epd:module="C3" epd:scenario="Recycling">0.0</epd:amount>
                <epd:amount xmlns:epd="http://www.iai.kit.edu/EPD/2013" epd:module="C4" epd:scenario="Recycling">0.0</epd:amount>
                <epd:amount xmlns:epd="http://www.iai.kit.edu/EPD/2013" epd:module="D" epd:scenario="Recycling">0.0</epd:amount>
                <epd:amount xmlns:epd="http://www.iai.kit.edu/EPD/2013" epd:module="A1"/>
                <epd:amount xmlns:epd="http://www.iai.kit.edu/EPD/2013" epd:module="A1-A3">0.0</epd:amount>
                <epd:amount xmlns:epd="http://www.iai.kit.edu/EPD/2013" epd:module="A2"/>
                <epd:amount xmlns:epd="http://www.iai.kit.edu/EPD/2013" epd:module="A3"/>
                <epd:amount xmlns:epd="http://www.iai.kit.edu/EPD/2013" epd:module="A4">0.0</epd:amount>
                <epd:amount xmlns:epd="http://www.iai.kit.edu/EPD/2013" epd:module="A5">0.0</epd:amount>
                <epd:amount xmlns:epd="http://www.iai.kit.edu/EPD/2013" epd:module="B1"/>
                <epd:amount xmlns:epd="http://www.iai.kit.edu/EPD/2013" epd:module="B2"/>
                <epd:amount xmlns:epd="http://www.iai.kit.edu/EPD/2013" epd:module="B3"/>
                <epd:amount xmlns:epd="http://www.iai.kit.edu/EPD/2013" epd:module="B4"/>
                <epd:amount xmlns:epd="http://www.iai.kit.edu/EPD/2013" epd:module="B5"/>
                <epd:amount xmlns:epd="http://www.iai.kit.edu/EPD/2013" epd:module="B6"/>
                <epd:amount xmlns:epd="http://www.iai.kit.edu/EPD/2013" epd:module="B7"/>
                <epd:amount xmlns:epd="http://www.iai.kit.edu/EPD/2013" epd:module="C1"/>
                <epd:amount xmlns:epd="http://www.iai.kit.edu/EPD/2013" epd:module="C2"/>
                <epd:amount xmlns:epd="http://www.iai.kit.edu/EPD/2013" epd:module="C3"/>
                <epd:amount xmlns:epd="http://www.iai.kit.edu/EPD/2013" epd:module="C4"/>
                <epd:amount xmlns:epd="http://www.iai.kit.edu/EPD/2013" epd:module="D"/>
                <epd:referenceToUnitGroupDataSet xmlns:epd="http://www.iai.kit.edu/EPD/2013" refObjectId="93a60a57-a3c8-11da-a746-0800200c9a66" type="unit group data set" uri="../unitgroups/93a60a57-a3c8-11da-a746-0800200c9a66">
                    <common:shortDescription>MJ</common:shortDescription>
                </epd:referenceToUnitGroupDataSet>
            </common:other>
        </exchange>
        <exchange dataSetInternalID="11">
            <referenceToFlowDataSet type="flow data set" refObjectId="3cf952c8-f3a4-461d-8c96-96456ca62246" version="30.00.000">
                <common:shortDescription xml:lang="en">Use of net fresh water (FW)</common:shortDescription>
                <common:shortDescription xml:lang="de">Einsatz von Süßwasserressourcen (FW)</common:shortDescription>
                <common:shortDescription xml:lang="es">Uso neto de recursos de agua dulce (FW)</common:shortDescription>
            </referenceToFlowDataSet>
            <functionType>General reminder flow</functionType>
            <exchangeDirection>Input</exchangeDirection>
            <meanAmount>0.0</meanAmount>
            <common:other>
                <epd:amount xmlns:epd="http://www.iai.kit.edu/EPD/2013" epd:module="C1" epd:scenario="Recycling"/>
                <epd:amount xmlns:epd="http://www.iai.kit.edu/EPD/2013" epd:module="C2" epd:scenario="Recycling"/>
                <epd:amount xmlns:epd="http://www.iai.kit.edu/EPD/2013" epd:module="C3" epd:scenario="Recycling"/>
                <epd:amount xmlns:epd="http://www.iai.kit.edu/EPD/2013" epd:module="C4" epd:scenario="Recycling"/>
                <epd:amount xmlns:epd="http://www.iai.kit.edu/EPD/2013" epd:module="D" epd:scenario="Recycling"/>
                <epd:amount xmlns:epd="http://www.iai.kit.edu/EPD/2013" epd:module="A1"/>
                <epd:amount xmlns:epd="http://www.iai.kit.edu/EPD/2013" epd:module="A1-A3"/>
                <epd:amount xmlns:epd="http://www.iai.kit.edu/EPD/2013" epd:module="A2"/>
                <epd:amount xmlns:epd="http://www.iai.kit.edu/EPD/2013" epd:module="A3"/>
                <epd:amount xmlns:epd="http://www.iai.kit.edu/EPD/2013" epd:module="A4"/>
                <epd:amount xmlns:epd="http://www.iai.kit.edu/EPD/2013" epd:module="A5"/>
                <epd:amount xmlns:epd="http://www.iai.kit.edu/EPD/2013" epd:module="B1"/>
                <epd:amount xmlns:epd="http://www.iai.kit.edu/EPD/2013" epd:module="B2"/>
                <epd:amount xmlns:epd="http://www.iai.kit.edu/EPD/2013" epd:module="B3"/>
                <epd:amount xmlns:epd="http://www.iai.kit.edu/EPD/2013" epd:module="B4"/>
                <epd:amount xmlns:epd="http://www.iai.kit.edu/EPD/2013" epd:module="B5"/>
                <epd:amount xmlns:epd="http://www.iai.kit.edu/EPD/2013" epd:module="B6"/>
                <epd:amount xmlns:epd="http://www.iai.kit.edu/EPD/2013" epd:module="B7"/>
                <epd:amount xmlns:epd="http://www.iai.kit.edu/EPD/2013" epd:module="C1"/>
                <epd:amount xmlns:epd="http://www.iai.kit.edu/EPD/2013" epd:module="C2"/>
                <epd:amount xmlns:epd="http://www.iai.kit.edu/EPD/2013" epd:module="C3"/>
                <epd:amount xmlns:epd="http://www.iai.kit.edu/EPD/2013" epd:module="C4"/>
                <epd:amount xmlns:epd="http://www.iai.kit.edu/EPD/2013" epd:module="D"/>
                <epd:referenceToUnitGroupDataSet xmlns:epd="http://www.iai.kit.edu/EPD/2013" refObjectId="cd950537-0a98-4044-9ba7-9f9a68d0a504" type="unit group data set" uri="../unitgroups/cd950537-0a98-4044-9ba7-9f9a68d0a504">
                    <common:shortDescription>m3</common:shortDescription>
                </epd:referenceToUnitGroupDataSet>
            </common:other>
        </exchange>
        <exchange dataSetInternalID="12">
            <referenceToFlowDataSet type="flow data set" refObjectId="430f9e0f-59b2-46a0-8e0d-55e0e84948fc" version="30.00.000">
                <common:shortDescription xml:lang="en">Hazardous waste disposed (HWD)</common:shortDescription>
                <common:shortDescription xml:lang="de">Gefährlicher Abfall zur Deponie (HWD)</common:shortDescription>
                <common:shortDescription xml:lang="es">Residuos peligrosos eliminados (HWD)</common:shortDescription>
            </referenceToFlowDataSet>
            <functionType>General reminder flow</functionType>
            <exchangeDirection>Output</exchangeDirection>
            <meanAmount>0.0</meanAmount>
            <common:other>
                <epd:amount xmlns:epd="http://www.iai.kit.edu/EPD/2013" epd:module="C1" epd:scenario="Recycling">1.846650819049766E-5</epd:amount>
                <epd:amount xmlns:epd="http://www.iai.kit.edu/EPD/2013" epd:module="C2" epd:scenario="Recycling">1.0554189859179979E-5</epd:amount>
                <epd:amount xmlns:epd="http://www.iai.kit.edu/EPD/2013" epd:module="C3" epd:scenario="Recycling">2.3003413970699916E-5</epd:amount>
                <epd:amount xmlns:epd="http://www.iai.kit.edu/EPD/2013" epd:module="C4" epd:scenario="Recycling">0.0</epd:amount>
                <epd:amount xmlns:epd="http://www.iai.kit.edu/EPD/2013" epd:module="D" epd:scenario="Recycling">0.13446655068141336</epd:amount>
                <epd:amount xmlns:epd="http://www.iai.kit.edu/EPD/2013" epd:module="A1"/>
                <epd:amount xmlns:epd="http://www.iai.kit.edu/EPD/2013" epd:module="A1-A3">0.13435465619692638</epd:amount>
                <epd:amount xmlns:epd="http://www.iai.kit.edu/EPD/2013" epd:module="A2"/>
                <epd:amount xmlns:epd="http://www.iai.kit.edu/EPD/2013" epd:module="A3"/>
                <epd:amount xmlns:epd="http://www.iai.kit.edu/EPD/2013" epd:module="A4">3.588787283065013E-5</epd:amount>
                <epd:amount xmlns:epd="http://www.iai.kit.edu/EPD/2013" epd:module="A5">1.8466508755886624E-5</epd:amount>
                <epd:amount xmlns:epd="http://www.iai.kit.edu/EPD/2013" epd:module="B1"/>
                <epd:amount xmlns:epd="http://www.iai.kit.edu/EPD/2013" epd:module="B2"/>
                <epd:amount xmlns:epd="http://www.iai.kit.edu/EPD/2013" epd:module="B3"/>
                <epd:amount xmlns:epd="http://www.iai.kit.edu/EPD/2013" epd:module="B4"/>
                <epd:amount xmlns:epd="http://www.iai.kit.edu/EPD/2013" epd:module="B5"/>
                <epd:amount xmlns:epd="http://www.iai.kit.edu/EPD/2013" epd:module="B6"/>
                <epd:amount xmlns:epd="http://www.iai.kit.edu/EPD/2013" epd:module="B7"/>
                <epd:amount xmlns:epd="http://www.iai.kit.edu/EPD/2013" epd:module="C1"/>
                <epd:amount xmlns:epd="http://www.iai.kit.edu/EPD/2013" epd:module="C2"/>
                <epd:amount xmlns:epd="http://www.iai.kit.edu/EPD/2013" epd:module="C3"/>
                <epd:amount xmlns:epd="http://www.iai.kit.edu/EPD/2013" epd:module="C4"/>
                <epd:amount xmlns:epd="http://www.iai.kit.edu/EPD/2013" epd:module="D"/>
                <epd:referenceToUnitGroupDataSet xmlns:epd="http://www.iai.kit.edu/EPD/2013" refObjectId="ad38d542-3fe9-439d-9b95-2f5f7752acaf" type="unit group data set" uri="../unitgroups/ad38d542-3fe9-439d-9b95-2f5f7752acaf">
                    <common:shortDescription>kg</common:shortDescription>
                </epd:referenceToUnitGroupDataSet>
            </common:other>
        </exchange>
        <exchange dataSetInternalID="13">
            <referenceToFlowDataSet type="flow data set" refObjectId="b29ef66b-e286-4afa-949f-62f1a7b4d7fa" version="30.00.000">
                <common:shortDescription xml:lang="en">Non hazardous waste dispose (NHWD)</common:shortDescription>
                <common:shortDescription xml:lang="de">Entsorgter nicht gefährlicher Abfall (NHWD)</common:shortDescription>
                <common:shortDescription xml:lang="es">Residuos no peligrosos eliminados (NHWD)</common:shortDescription>
            </referenceToFlowDataSet>
            <functionType>General reminder flow</functionType>
            <exchangeDirection>Output</exchangeDirection>
            <meanAmount>0.0</meanAmount>
            <common:other>
                <epd:amount xmlns:epd="http://www.iai.kit.edu/EPD/2013" epd:module="C1" epd:scenario="Recycling">0.04514434010059884</epd:amount>
                <epd:amount xmlns:epd="http://www.iai.kit.edu/EPD/2013" epd:module="C2" epd:scenario="Recycling">0.7848123502942548</epd:amount>
                <epd:amount xmlns:epd="http://www.iai.kit.edu/EPD/2013" epd:module="C3" epd:scenario="Recycling">0.8583655399527773</epd:amount>
                <epd:amount xmlns:epd="http://www.iai.kit.edu/EPD/2013" epd:module="C4" epd:scenario="Recycling">0.0</epd:amount>
                <epd:amount xmlns:epd="http://www.iai.kit.edu/EPD/2013" epd:module="D" epd:scenario="Recycling">-35.59267601452577</epd:amount>
                <epd:amount xmlns:epd="http://www.iai.kit.edu/EPD/2013" epd:module="A1"/>
                <epd:amount xmlns:epd="http://www.iai.kit.edu/EPD/2013" epd:module="A1-A3">64.32738960689282</epd:amount>
                <epd:amount xmlns:epd="http://www.iai.kit.edu/EPD/2013" epd:module="A2"/>
                <epd:amount xmlns:epd="http://www.iai.kit.edu/EPD/2013" epd:module="A3"/>
                <epd:amount xmlns:epd="http://www.iai.kit.edu/EPD/2013" epd:module="A4">2.668631726767469</epd:amount>
                <epd:amount xmlns:epd="http://www.iai.kit.edu/EPD/2013" epd:module="A5">0.045144336708265044</epd:amount>
                <epd:amount xmlns:epd="http://www.iai.kit.edu/EPD/2013" epd:module="B1"/>
                <epd:amount xmlns:epd="http://www.iai.kit.edu/EPD/2013" epd:module="B2"/>
                <epd:amount xmlns:epd="http://www.iai.kit.edu/EPD/2013" epd:module="B3"/>
                <epd:amount xmlns:epd="http://www.iai.kit.edu/EPD/2013" epd:module="B4"/>
                <epd:amount xmlns:epd="http://www.iai.kit.edu/EPD/2013" epd:module="B5"/>
                <epd:amount xmlns:epd="http://www.iai.kit.edu/EPD/2013" epd:module="B6"/>
                <epd:amount xmlns:epd="http://www.iai.kit.edu/EPD/2013" epd:module="B7"/>
                <epd:amount xmlns:epd="http://www.iai.kit.edu/EPD/2013" epd:module="C1"/>
                <epd:amount xmlns:epd="http://www.iai.kit.edu/EPD/2013" epd:module="C2"/>
                <epd:amount xmlns:epd="http://www.iai.kit.edu/EPD/2013" epd:module="C3"/>
                <epd:amount xmlns:epd="http://www.iai.kit.edu/EPD/2013" epd:module="C4"/>
                <epd:amount xmlns:epd="http://www.iai.kit.edu/EPD/2013" epd:module="D"/>
                <epd:referenceToUnitGroupDataSet xmlns:epd="http://www.iai.kit.edu/EPD/2013" refObjectId="ad38d542-3fe9-439d-9b95-2f5f7752acaf" type="unit group data set" uri="../unitgroups/ad38d542-3fe9-439d-9b95-2f5f7752acaf">
                    <common:shortDescription>kg</common:shortDescription>
                </epd:referenceToUnitGroupDataSet>
            </common:other>
        </exchange>
        <exchange dataSetInternalID="14">
            <referenceToFlowDataSet type="flow data set" refObjectId="3449546e-52ad-4b39-b809-9fb77cea8ff6" version="30.00.000">
                <common:shortDescription xml:lang="en">Radioactive waste disposed (RWD)</common:shortDescription>
                <common:shortDescription xml:lang="de">Entsorgter radioaktiver Abfall (RWD)</common:shortDescription>
                <common:shortDescription xml:lang="es">Residuos radiactivos eliminados (RWD)</common:shortDescription>
            </referenceToFlowDataSet>
            <functionType>General reminder flow</functionType>
            <exchangeDirection>Output</exchangeDirection>
            <meanAmount>0.0</meanAmount>
            <common:other>
                <epd:amount xmlns:epd="http://www.iai.kit.edu/EPD/2013" epd:module="C1" epd:scenario="Recycling">5.742653447009699E-4</epd:amount>
                <epd:amount xmlns:epd="http://www.iai.kit.edu/EPD/2013" epd:module="C2" epd:scenario="Recycling">2.2668153307793228E-4</epd:amount>
                <epd:amount xmlns:epd="http://www.iai.kit.edu/EPD/2013" epd:module="C3" epd:scenario="Recycling">3.2385409331289786E-5</epd:amount>
                <epd:amount xmlns:epd="http://www.iai.kit.edu/EPD/2013" epd:module="C4" epd:scenario="Recycling">0.0</epd:amount>
                <epd:amount xmlns:epd="http://www.iai.kit.edu/EPD/2013" epd:module="D" epd:scenario="Recycling">-0.0186171261201552</epd:amount>
                <epd:amount xmlns:epd="http://www.iai.kit.edu/EPD/2013" epd:module="A1"/>
                <epd:amount xmlns:epd="http://www.iai.kit.edu/EPD/2013" epd:module="A1-A3">0.019197984773483563</epd:amount>
                <epd:amount xmlns:epd="http://www.iai.kit.edu/EPD/2013" epd:module="A2"/>
                <epd:amount xmlns:epd="http://www.iai.kit.edu/EPD/2013" epd:module="A3"/>
                <epd:amount xmlns:epd="http://www.iai.kit.edu/EPD/2013" epd:module="A4">7.70795114018002E-4</epd:amount>
                <epd:amount xmlns:epd="http://www.iai.kit.edu/EPD/2013" epd:module="A5">5.742652881620734E-4</epd:amount>
                <epd:amount xmlns:epd="http://www.iai.kit.edu/EPD/2013" epd:module="B1"/>
                <epd:amount xmlns:epd="http://www.iai.kit.edu/EPD/2013" epd:module="B2"/>
                <epd:amount xmlns:epd="http://www.iai.kit.edu/EPD/2013" epd:module="B3"/>
                <epd:amount xmlns:epd="http://www.iai.kit.edu/EPD/2013" epd:module="B4"/>
                <epd:amount xmlns:epd="http://www.iai.kit.edu/EPD/2013" epd:module="B5"/>
                <epd:amount xmlns:epd="http://www.iai.kit.edu/EPD/2013" epd:module="B6"/>
                <epd:amount xmlns:epd="http://www.iai.kit.edu/EPD/2013" epd:module="B7"/>
                <epd:amount xmlns:epd="http://www.iai.kit.edu/EPD/2013" epd:module="C1"/>
                <epd:amount xmlns:epd="http://www.iai.kit.edu/EPD/2013" epd:module="C2"/>
                <epd:amount xmlns:epd="http://www.iai.kit.edu/EPD/2013" epd:module="C3"/>
                <epd:amount xmlns:epd="http://www.iai.kit.edu/EPD/2013" epd:module="C4"/>
                <epd:amount xmlns:epd="http://www.iai.kit.edu/EPD/2013" epd:module="D"/>
                <epd:referenceToUnitGroupDataSet xmlns:epd="http://www.iai.kit.edu/EPD/2013" refObjectId="ad38d542-3fe9-439d-9b95-2f5f7752acaf" type="unit group data set" uri="../unitgroups/ad38d542-3fe9-439d-9b95-2f5f7752acaf">
                    <common:shortDescription>kg</common:shortDescription>
                </epd:referenceToUnitGroupDataSet>
            </common:other>
        </exchange>
        <exchange dataSetInternalID="15">
            <referenceToFlowDataSet type="flow data set" refObjectId="a2b32f97-3fc7-4af2-b209-525bc6426f33" version="30.00.000">
                <common:shortDescription xml:lang="en">Components for re-use (CRU)</common:shortDescription>
                <common:shortDescription xml:lang="de">Komponenten für die Wiederverwendung (CRU)</common:shortDescription>
                <common:shortDescription xml:lang="es">Componentes para su reutilización (CRU)</common:shortDescription>
            </referenceToFlowDataSet>
            <functionType>General reminder flow</functionType>
            <exchangeDirection>Output</exchangeDirection>
            <meanAmount>0.0</meanAmount>
            <common:other>
                <epd:amount xmlns:epd="http://www.iai.kit.edu/EPD/2013" epd:module="C1" epd:scenario="Recycling">0.0</epd:amount>
                <epd:amount xmlns:epd="http://www.iai.kit.edu/EPD/2013" epd:module="C2" epd:scenario="Recycling">0.0</epd:amount>
                <epd:amount xmlns:epd="http://www.iai.kit.edu/EPD/2013" epd:module="C3" epd:scenario="Recycling">0.0</epd:amount>
                <epd:amount xmlns:epd="http://www.iai.kit.edu/EPD/2013" epd:module="C4" epd:scenario="Recycling">0.0</epd:amount>
                <epd:amount xmlns:epd="http://www.iai.kit.edu/EPD/2013" epd:module="D" epd:scenario="Recycling">0.0</epd:amount>
                <epd:amount xmlns:epd="http://www.iai.kit.edu/EPD/2013" epd:module="A1"/>
                <epd:amount xmlns:epd="http://www.iai.kit.edu/EPD/2013" epd:module="A1-A3">0.0</epd:amount>
                <epd:amount xmlns:epd="http://www.iai.kit.edu/EPD/2013" epd:module="A2"/>
                <epd:amount xmlns:epd="http://www.iai.kit.edu/EPD/2013" epd:module="A3"/>
                <epd:amount xmlns:epd="http://www.iai.kit.edu/EPD/2013" epd:module="A4">0.0</epd:amount>
                <epd:amount xmlns:epd="http://www.iai.kit.edu/EPD/2013" epd:module="A5">0.0</epd:amount>
                <epd:amount xmlns:epd="http://www.iai.kit.edu/EPD/2013" epd:module="B1"/>
                <epd:amount xmlns:epd="http://www.iai.kit.edu/EPD/2013" epd:module="B2"/>
                <epd:amount xmlns:epd="http://www.iai.kit.edu/EPD/2013" epd:module="B3"/>
                <epd:amount xmlns:epd="http://www.iai.kit.edu/EPD/2013" epd:module="B4"/>
                <epd:amount xmlns:epd="http://www.iai.kit.edu/EPD/2013" epd:module="B5"/>
                <epd:amount xmlns:epd="http://www.iai.kit.edu/EPD/2013" epd:module="B6"/>
                <epd:amount xmlns:epd="http://www.iai.kit.edu/EPD/2013" epd:module="B7"/>
                <epd:amount xmlns:epd="http://www.iai.kit.edu/EPD/2013" epd:module="C1"/>
                <epd:amount xmlns:epd="http://www.iai.kit.edu/EPD/2013" epd:module="C2"/>
                <epd:amount xmlns:epd="http://www.iai.kit.edu/EPD/2013" epd:module="C3"/>
                <epd:amount xmlns:epd="http://www.iai.kit.edu/EPD/2013" epd:module="C4"/>
                <epd:amount xmlns:epd="http://www.iai.kit.edu/EPD/2013" epd:module="D"/>
                <epd:referenceToUnitGroupDataSet xmlns:epd="http://www.iai.kit.edu/EPD/2013" refObjectId="ad38d542-3fe9-439d-9b95-2f5f7752acaf" type="unit group data set" uri="../unitgroups/ad38d542-3fe9-439d-9b95-2f5f7752acaf">
                    <common:shortDescription>kg</common:shortDescription>
                </epd:referenceToUnitGroupDataSet>
            </common:other>
        </exchange>
        <exchange dataSetInternalID="16">
            <referenceToFlowDataSet type="flow data set" refObjectId="d7fe48a5-4103-49c8-9aae-b0b5dfdbd6ae" version="30.00.000">
                <common:shortDescription xml:lang="en">Materials for recycling (MFR)</common:shortDescription>
                <common:shortDescription xml:lang="de">Stoffe zum Recycling (MFR)</common:shortDescription>
                <common:shortDescription xml:lang="es">Materiales para el reciclaje (MFR)</common:shortDescription>
            </referenceToFlowDataSet>
            <functionType>General reminder flow</functionType>
            <exchangeDirection>Output</exchangeDirection>
            <meanAmount>0.0</meanAmount>
            <common:other>
                <epd:amount xmlns:epd="http://www.iai.kit.edu/EPD/2013" epd:module="C1" epd:scenario="Recycling">0.0</epd:amount>
                <epd:amount xmlns:epd="http://www.iai.kit.edu/EPD/2013" epd:module="C2" epd:scenario="Recycling">0.0</epd:amount>
                <epd:amount xmlns:epd="http://www.iai.kit.edu/EPD/2013" epd:module="C3" epd:scenario="Recycling">31.95228035292655</epd:amount>
                <epd:amount xmlns:epd="http://www.iai.kit.edu/EPD/2013" epd:module="C4" epd:scenario="Recycling">0.0</epd:amount>
                <epd:amount xmlns:epd="http://www.iai.kit.edu/EPD/2013" epd:module="D" epd:scenario="Recycling">-31.95228035292655</epd:amount>
                <epd:amount xmlns:epd="http://www.iai.kit.edu/EPD/2013" epd:module="A1"/>
                <epd:amount xmlns:epd="http://www.iai.kit.edu/EPD/2013" epd:module="A1-A3">0.0</epd:amount>
                <epd:amount xmlns:epd="http://www.iai.kit.edu/EPD/2013" epd:module="A2"/>
                <epd:amount xmlns:epd="http://www.iai.kit.edu/EPD/2013" epd:module="A3"/>
                <epd:amount xmlns:epd="http://www.iai.kit.edu/EPD/2013" epd:module="A4">0.0</epd:amount>
                <epd:amount xmlns:epd="http://www.iai.kit.edu/EPD/2013" epd:module="A5">0.0</epd:amount>
                <epd:amount xmlns:epd="http://www.iai.kit.edu/EPD/2013" epd:module="B1"/>
                <epd:amount xmlns:epd="http://www.iai.kit.edu/EPD/2013" epd:module="B2"/>
                <epd:amount xmlns:epd="http://www.iai.kit.edu/EPD/2013" epd:module="B3"/>
                <epd:amount xmlns:epd="http://www.iai.kit.edu/EPD/2013" epd:module="B4"/>
                <epd:amount xmlns:epd="http://www.iai.kit.edu/EPD/2013" epd:module="B5"/>
                <epd:amount xmlns:epd="http://www.iai.kit.edu/EPD/2013" epd:module="B6"/>
                <epd:amount xmlns:epd="http://www.iai.kit.edu/EPD/2013" epd:module="B7"/>
                <epd:amount xmlns:epd="http://www.iai.kit.edu/EPD/2013" epd:module="C1"/>
                <epd:amount xmlns:epd="http://www.iai.kit.edu/EPD/2013" epd:module="C2"/>
                <epd:amount xmlns:epd="http://www.iai.kit.edu/EPD/2013" epd:module="C3"/>
                <epd:amount xmlns:epd="http://www.iai.kit.edu/EPD/2013" epd:module="C4"/>
                <epd:amount xmlns:epd="http://www.iai.kit.edu/EPD/2013" epd:module="D"/>
                <epd:referenceToUnitGroupDataSet xmlns:epd="http://www.iai.kit.edu/EPD/2013" refObjectId="ad38d542-3fe9-439d-9b95-2f5f7752acaf" type="unit group data set" uri="../unitgroups/ad38d542-3fe9-439d-9b95-2f5f7752acaf">
                    <common:shortDescription>kg</common:shortDescription>
                </epd:referenceToUnitGroupDataSet>
            </common:other>
        </exchange>
        <exchange dataSetInternalID="17">
            <referenceToFlowDataSet type="flow data set" refObjectId="59a9181c-3aaf-46ee-8b13-2b3723b6e447" version="30.00.000">
                <common:shortDescription xml:lang="en">Materials for energy recovery (MER)</common:shortDescription>
                <common:shortDescription xml:lang="de">Stoffe für die Energierückgewinnung (MER)</common:shortDescription>
                <common:shortDescription xml:lang="es">Materiales para valorización energética (recuperación de energía) (MER)</common:shortDescription>
            </referenceToFlowDataSet>
            <functionType>General reminder flow</functionType>
            <exchangeDirection>Output</exchangeDirection>
            <meanAmount>0.0</meanAmount>
            <common:other>
                <epd:amount xmlns:epd="http://www.iai.kit.edu/EPD/2013" epd:module="C1" epd:scenario="Recycling">0.0</epd:amount>
                <epd:amount xmlns:epd="http://www.iai.kit.edu/EPD/2013" epd:module="C2" epd:scenario="Recycling">0.0</epd:amount>
                <epd:amount xmlns:epd="http://www.iai.kit.edu/EPD/2013" epd:module="C3" epd:scenario="Recycling">10.592284219101668</epd:amount>
                <epd:amount xmlns:epd="http://www.iai.kit.edu/EPD/2013" epd:module="C4" epd:scenario="Recycling">0.0</epd:amount>
                <epd:amount xmlns:epd="http://www.iai.kit.edu/EPD/2013" epd:module="D" epd:scenario="Recycling">-10.592284219101668</epd:amount>
                <epd:amount xmlns:epd="http://www.iai.kit.edu/EPD/2013" epd:module="A1"/>
                <epd:amount xmlns:epd="http://www.iai.kit.edu/EPD/2013" epd:module="A1-A3">0.0</epd:amount>
                <epd:amount xmlns:epd="http://www.iai.kit.edu/EPD/2013" epd:module="A2"/>
                <epd:amount xmlns:epd="http://www.iai.kit.edu/EPD/2013" epd:module="A3"/>
                <epd:amount xmlns:epd="http://www.iai.kit.edu/EPD/2013" epd:module="A4">0.0</epd:amount>
                <epd:amount xmlns:epd="http://www.iai.kit.edu/EPD/2013" epd:module="A5">0.0</epd:amount>
                <epd:amount xmlns:epd="http://www.iai.kit.edu/EPD/2013" epd:module="B1"/>
                <epd:amount xmlns:epd="http://www.iai.kit.edu/EPD/2013" epd:module="B2"/>
                <epd:amount xmlns:epd="http://www.iai.kit.edu/EPD/2013" epd:module="B3"/>
                <epd:amount xmlns:epd="http://www.iai.kit.edu/EPD/2013" epd:module="B4"/>
                <epd:amount xmlns:epd="http://www.iai.kit.edu/EPD/2013" epd:module="B5"/>
                <epd:amount xmlns:epd="http://www.iai.kit.edu/EPD/2013" epd:module="B6"/>
                <epd:amount xmlns:epd="http://www.iai.kit.edu/EPD/2013" epd:module="B7"/>
                <epd:amount xmlns:epd="http://www.iai.kit.edu/EPD/2013" epd:module="C1"/>
                <epd:amount xmlns:epd="http://www.iai.kit.edu/EPD/2013" epd:module="C2"/>
                <epd:amount xmlns:epd="http://www.iai.kit.edu/EPD/2013" epd:module="C3"/>
                <epd:amount xmlns:epd="http://www.iai.kit.edu/EPD/2013" epd:module="C4"/>
                <epd:amount xmlns:epd="http://www.iai.kit.edu/EPD/2013" epd:module="D"/>
                <epd:referenceToUnitGroupDataSet xmlns:epd="http://www.iai.kit.edu/EPD/2013" refObjectId="ad38d542-3fe9-439d-9b95-2f5f7752acaf" type="unit group data set" uri="../unitgroups/ad38d542-3fe9-439d-9b95-2f5f7752acaf">
                    <common:shortDescription>kg</common:shortDescription>
                </epd:referenceToUnitGroupDataSet>
            </common:other>
        </exchange>
        <exchange dataSetInternalID="18">
            <referenceToFlowDataSet type="flow data set" refObjectId="4da0c987-2b76-40d6-9e9e-82a017aaaf29" version="30.00.000">
                <common:shortDescription xml:lang="en">Exported electrical energy (EEE)</common:shortDescription>
                <common:shortDescription xml:lang="de">Exportierte elektrische Energie (EEE)</common:shortDescription>
                <common:shortDescription xml:lang="es">Energía exportada electrica (EEE)</common:shortDescription>
            </referenceToFlowDataSet>
            <functionType>General reminder flow</functionType>
            <exchangeDirection>Output</exchangeDirection>
            <meanAmount>0.0</meanAmount>
            <common:other>
                <epd:amount xmlns:epd="http://www.iai.kit.edu/EPD/2013" epd:module="C1" epd:scenario="Recycling">0.0</epd:amount>
                <epd:amount xmlns:epd="http://www.iai.kit.edu/EPD/2013" epd:module="C2" epd:scenario="Recycling">0.0</epd:amount>
                <epd:amount xmlns:epd="http://www.iai.kit.edu/EPD/2013" epd:module="C3" epd:scenario="Recycling">18.551331471585915</epd:amount>
                <epd:amount xmlns:epd="http://www.iai.kit.edu/EPD/2013" epd:module="C4" epd:scenario="Recycling">0.0</epd:amount>
                <epd:amount xmlns:epd="http://www.iai.kit.edu/EPD/2013" epd:module="D" epd:scenario="Recycling">-18.551331471585915</epd:amount>
                <epd:amount xmlns:epd="http://www.iai.kit.edu/EPD/2013" epd:module="A1"/>
                <epd:amount xmlns:epd="http://www.iai.kit.edu/EPD/2013" epd:module="A1-A3">0.0</epd:amount>
                <epd:amount xmlns:epd="http://www.iai.kit.edu/EPD/2013" epd:module="A2"/>
                <epd:amount xmlns:epd="http://www.iai.kit.edu/EPD/2013" epd:module="A3"/>
                <epd:amount xmlns:epd="http://www.iai.kit.edu/EPD/2013" epd:module="A4">0.0</epd:amount>
                <epd:amount xmlns:epd="http://www.iai.kit.edu/EPD/2013" epd:module="A5">0.0</epd:amount>
                <epd:amount xmlns:epd="http://www.iai.kit.edu/EPD/2013" epd:module="B1"/>
                <epd:amount xmlns:epd="http://www.iai.kit.edu/EPD/2013" epd:module="B2"/>
                <epd:amount xmlns:epd="http://www.iai.kit.edu/EPD/2013" epd:module="B3"/>
                <epd:amount xmlns:epd="http://www.iai.kit.edu/EPD/2013" epd:module="B4"/>
                <epd:amount xmlns:epd="http://www.iai.kit.edu/EPD/2013" epd:module="B5"/>
                <epd:amount xmlns:epd="http://www.iai.kit.edu/EPD/2013" epd:module="B6"/>
                <epd:amount xmlns:epd="http://www.iai.kit.edu/EPD/2013" epd:module="B7"/>
                <epd:amount xmlns:epd="http://www.iai.kit.edu/EPD/2013" epd:module="C1"/>
                <epd:amount xmlns:epd="http://www.iai.kit.edu/EPD/2013" epd:module="C2"/>
                <epd:amount xmlns:epd="http://www.iai.kit.edu/EPD/2013" epd:module="C3"/>
                <epd:amount xmlns:epd="http://www.iai.kit.edu/EPD/2013" epd:module="C4"/>
                <epd:amount xmlns:epd="http://www.iai.kit.edu/EPD/2013" epd:module="D"/>
                <epd:referenceToUnitGroupDataSet xmlns:epd="http://www.iai.kit.edu/EPD/2013" refObjectId="93a60a57-a3c8-11da-a746-0800200c9a66" type="unit group data set" uri="../unitgroups/93a60a57-a3c8-11da-a746-0800200c9a66">
                    <common:shortDescription>MJ</common:shortDescription>
                </epd:referenceToUnitGroupDataSet>
            </common:other>
        </exchange>
        <exchange dataSetInternalID="19">
            <referenceToFlowDataSet type="flow data set" refObjectId="98daf38a-7a79-46d3-9a37-2b7bd0955810" version="30.00.000">
                <common:shortDescription xml:lang="en">Exported thermal energy (EET)</common:shortDescription>
                <common:shortDescription xml:lang="de">Exportierte thermische Energie (EET)</common:shortDescription>
                <common:shortDescription xml:lang="es">Energía exportada termal (EET)</common:shortDescription>
            </referenceToFlowDataSet>
            <functionType>General reminder flow</functionType>
            <exchangeDirection>Output</exchangeDirection>
            <meanAmount>0.0</meanAmount>
            <common:other>
                <epd:amount xmlns:epd="http://www.iai.kit.edu/EPD/2013" epd:module="C1" epd:scenario="Recycling">0.0</epd:amount>
                <epd:amount xmlns:epd="http://www.iai.kit.edu/EPD/2013" epd:module="C2" epd:scenario="Recycling">0.0</epd:amount>
                <epd:amount xmlns:epd="http://www.iai.kit.edu/EPD/2013" epd:module="C3" epd:scenario="Recycling">163.68821886693453</epd:amount>
                <epd:amount xmlns:epd="http://www.iai.kit.edu/EPD/2013" epd:module="C4" epd:scenario="Recycling">0.0</epd:amount>
                <epd:amount xmlns:epd="http://www.iai.kit.edu/EPD/2013" epd:module="D" epd:scenario="Recycling">-163.68821886693453</epd:amount>
                <epd:amount xmlns:epd="http://www.iai.kit.edu/EPD/2013" epd:module="A1"/>
                <epd:amount xmlns:epd="http://www.iai.kit.edu/EPD/2013" epd:module="A1-A3">0.0</epd:amount>
                <epd:amount xmlns:epd="http://www.iai.kit.edu/EPD/2013" epd:module="A2"/>
                <epd:amount xmlns:epd="http://www.iai.kit.edu/EPD/2013" epd:module="A3"/>
                <epd:amount xmlns:epd="http://www.iai.kit.edu/EPD/2013" epd:module="A4">0.0</epd:amount>
                <epd:amount xmlns:epd="http://www.iai.kit.edu/EPD/2013" epd:module="A5">0.0</epd:amount>
                <epd:amount xmlns:epd="http://www.iai.kit.edu/EPD/2013" epd:module="B1"/>
                <epd:amount xmlns:epd="http://www.iai.kit.edu/EPD/2013" epd:module="B2"/>
                <epd:amount xmlns:epd="http://www.iai.kit.edu/EPD/2013" epd:module="B3"/>
                <epd:amount xmlns:epd="http://www.iai.kit.edu/EPD/2013" epd:module="B4"/>
                <epd:amount xmlns:epd="http://www.iai.kit.edu/EPD/2013" epd:module="B5"/>
                <epd:amount xmlns:epd="http://www.iai.kit.edu/EPD/2013" epd:module="B6"/>
                <epd:amount xmlns:epd="http://www.iai.kit.edu/EPD/2013" epd:module="B7"/>
                <epd:amount xmlns:epd="http://www.iai.kit.edu/EPD/2013" epd:module="C1"/>
                <epd:amount xmlns:epd="http://www.iai.kit.edu/EPD/2013" epd:module="C2"/>
                <epd:amount xmlns:epd="http://www.iai.kit.edu/EPD/2013" epd:module="C3"/>
                <epd:amount xmlns:epd="http://www.iai.kit.edu/EPD/2013" epd:module="C4"/>
                <epd:amount xmlns:epd="http://www.iai.kit.edu/EPD/2013" epd:module="D"/>
                <epd:referenceToUnitGroupDataSet xmlns:epd="http://www.iai.kit.edu/EPD/2013" refObjectId="93a60a57-a3c8-11da-a746-0800200c9a66" type="unit group data set" uri="../unitgroups/93a60a57-a3c8-11da-a746-0800200c9a66">
                    <common:shortDescription>MJ</common:shortDescription>
                </epd:referenceToUnitGroupDataSet>
            </common:other>
        </exchange>
    </exchanges>
    <LCIAResults>
        <LCIAResult>
            <referenceToLCIAMethodDataSet type="LCIA method data set" refObjectId="77e416eb-a363-4258-a04e-171d843a6460" version="00.01.000">
                <common:shortDescription xml:lang="en">Global warming potential (GWP)</common:shortDescription>
                <common:shortDescription xml:lang="de">Globales Erwärmungspotenzial (GWP)</common:shortDescription>
                <common:shortDescription xml:lang="es">Potencial de calentamiento global (GWP)</common:shortDescription>
            </referenceToLCIAMethodDataSet>
            <meanAmount>0.0</meanAmount>
            <common:other>
                <epd:amount xmlns:epd="http://www.iai.kit.edu/EPD/2013" epd:module="C1" epd:scenario="Recycling">2.828426987768808</epd:amount>
                <epd:amount xmlns:epd="http://www.iai.kit.edu/EPD/2013" epd:module="C2" epd:scenario="Recycling">1.0796456768749487</epd:amount>
                <epd:amount xmlns:epd="http://www.iai.kit.edu/EPD/2013" epd:module="C3" epd:scenario="Recycling">31.4252758101708</epd:amount>
                <epd:amount xmlns:epd="http://www.iai.kit.edu/EPD/2013" epd:module="C4" epd:scenario="Recycling">0.0</epd:amount>
                <epd:amount xmlns:epd="http://www.iai.kit.edu/EPD/2013" epd:module="D" epd:scenario="Recycling">-131.71952280352926</epd:amount>
                <epd:amount xmlns:epd="http://www.iai.kit.edu/EPD/2013" epd:module="A1"/>
                <epd:amount xmlns:epd="http://www.iai.kit.edu/EPD/2013" epd:module="A1-A3">392.7808135882247</epd:amount>
                <epd:amount xmlns:epd="http://www.iai.kit.edu/EPD/2013" epd:module="A2"/>
                <epd:amount xmlns:epd="http://www.iai.kit.edu/EPD/2013" epd:module="A3"/>
                <epd:amount xmlns:epd="http://www.iai.kit.edu/EPD/2013" epd:module="A4">3.6713543692903268</epd:amount>
                <epd:amount xmlns:epd="http://www.iai.kit.edu/EPD/2013" epd:module="A5">2.8283390132459907</epd:amount>
                <epd:amount xmlns:epd="http://www.iai.kit.edu/EPD/2013" epd:module="B1"/>
                <epd:amount xmlns:epd="http://www.iai.kit.edu/EPD/2013" epd:module="B2"/>
                <epd:amount xmlns:epd="http://www.iai.kit.edu/EPD/2013" epd:module="B3"/>
                <epd:amount xmlns:epd="http://www.iai.kit.edu/EPD/2013" epd:module="B4"/>
                <epd:amount xmlns:epd="http://www.iai.kit.edu/EPD/2013" epd:module="B5"/>
                <epd:amount xmlns:epd="http://www.iai.kit.edu/EPD/2013" epd:module="B6"/>
                <epd:amount xmlns:epd="http://www.iai.kit.edu/EPD/2013" epd:module="B7"/>
                <epd:amount xmlns:epd="http://www.iai.kit.edu/EPD/2013" epd:module="C1"/>
                <epd:amount xmlns:epd="http://www.iai.kit.edu/EPD/2013" epd:module="C2"/>
                <epd:amount xmlns:epd="http://www.iai.kit.edu/EPD/2013" epd:module="C3"/>
                <epd:amount xmlns:epd="http://www.iai.kit.edu/EPD/2013" epd:module="C4"/>
                <epd:amount xmlns:epd="http://www.iai.kit.edu/EPD/2013" epd:module="D"/>
                <epd:referenceToUnitGroupDataSet xmlns:epd="http://www.iai.kit.edu/EPD/2013" refObjectId="1ebf3012-d0db-4de2-aefd-ef30cedb0be1" type="unit group data set" uri="../unitgroups/1ebf3012-d0db-4de2-aefd-ef30cedb0be1">
                    <common:shortDescription>kg CO2-Äqv.</common:shortDescription>
                </epd:referenceToUnitGroupDataSet>
            </common:other>
        </LCIAResult>
        <LCIAResult>
            <referenceToLCIAMethodDataSet type="LCIA method data set" refObjectId="06dcd26f-025f-401a-a7c1-5e457eb54637" version="00.01.000">
                <common:shortDescription xml:lang="en">Depletion potential of the stratospheric ozone layer (ODP)</common:shortDescription>
                <common:shortDescription xml:lang="de">Abbau Potential der stratosphärischen Ozonschicht (ODP)</common:shortDescription>
                <common:shortDescription xml:lang="es">Potencial de agotamiento de la capa de ozono estratosférico (ODP)</common:shortDescription>
            </referenceToLCIAMethodDataSet>
            <meanAmount>0.0</meanAmount>
            <common:other>
                <epd:amount xmlns:epd="http://www.iai.kit.edu/EPD/2013" epd:module="C1" epd:scenario="Recycling">5.136753685143879E-7</epd:amount>
                <epd:amount xmlns:epd="http://www.iai.kit.edu/EPD/2013" epd:module="C2" epd:scenario="Recycling">2.0158855315015688E-7</epd:amount>
                <epd:amount xmlns:epd="http://www.iai.kit.edu/EPD/2013" epd:module="C3" epd:scenario="Recycling">7.315215642820651E-8</epd:amount>
                <epd:amount xmlns:epd="http://www.iai.kit.edu/EPD/2013" epd:module="C4" epd:scenario="Recycling">0.0</epd:amount>
                <epd:amount xmlns:epd="http://www.iai.kit.edu/EPD/2013" epd:module="D" epd:scenario="Recycling">-1.1106014836446985E-5</epd:amount>
                <epd:amount xmlns:epd="http://www.iai.kit.edu/EPD/2013" epd:module="A1"/>
                <epd:amount xmlns:epd="http://www.iai.kit.edu/EPD/2013" epd:module="A1-A3">1.7209528257597724E-5</epd:amount>
                <epd:amount xmlns:epd="http://www.iai.kit.edu/EPD/2013" epd:module="A2"/>
                <epd:amount xmlns:epd="http://www.iai.kit.edu/EPD/2013" epd:module="A3"/>
                <epd:amount xmlns:epd="http://www.iai.kit.edu/EPD/2013" epd:module="A4">6.854703431201939E-7</epd:amount>
                <epd:amount xmlns:epd="http://www.iai.kit.edu/EPD/2013" epd:module="A5">5.136753911299465E-7</epd:amount>
                <epd:amount xmlns:epd="http://www.iai.kit.edu/EPD/2013" epd:module="B1"/>
                <epd:amount xmlns:epd="http://www.iai.kit.edu/EPD/2013" epd:module="B2"/>
                <epd:amount xmlns:epd="http://www.iai.kit.edu/EPD/2013" epd:module="B3"/>
                <epd:amount xmlns:epd="http://www.iai.kit.edu/EPD/2013" epd:module="B4"/>
                <epd:amount xmlns:epd="http://www.iai.kit.edu/EPD/2013" epd:module="B5"/>
                <epd:amount xmlns:epd="http://www.iai.kit.edu/EPD/2013" epd:module="B6"/>
                <epd:amount xmlns:epd="http://www.iai.kit.edu/EPD/2013" epd:module="B7"/>
                <epd:amount xmlns:epd="http://www.iai.kit.edu/EPD/2013" epd:module="C1"/>
                <epd:amount xmlns:epd="http://www.iai.kit.edu/EPD/2013" epd:module="C2"/>
                <epd:amount xmlns:epd="http://www.iai.kit.edu/EPD/2013" epd:module="C3"/>
                <epd:amount xmlns:epd="http://www.iai.kit.edu/EPD/2013" epd:module="C4"/>
                <epd:amount xmlns:epd="http://www.iai.kit.edu/EPD/2013" epd:module="D"/>
                <epd:referenceToUnitGroupDataSet xmlns:epd="http://www.iai.kit.edu/EPD/2013" refObjectId="88054749-b0a6-47ea-a82b-dc5b29326512" type="unit group data set" uri="../unitgroups/88054749-b0a6-47ea-a82b-dc5b29326512">
                    <common:shortDescription>kg R11 eq.</common:shortDescription>
                </epd:referenceToUnitGroupDataSet>
            </common:other>
        </LCIAResult>
        <LCIAResult>
            <referenceToLCIAMethodDataSet type="LCIA method data set" refObjectId="b4274add-93b7-4905-a5e4-2e878c4e4216" version="00.01.000">
                <common:shortDescription xml:lang="en">Acidification potential of soil and water (AP)</common:shortDescription>
                <common:shortDescription xml:lang="de">Versauerungspotenzial von Boden und Wasser (AP)</common:shortDescription>
                <common:shortDescription xml:lang="es">Potencial de acidificación del suelo y de los recursos de agua (AP)</common:shortDescription>
            </referenceToLCIAMethodDataSet>
            <meanAmount>0.0</meanAmount>
            <common:other>
                <epd:amount xmlns:epd="http://www.iai.kit.edu/EPD/2013" epd:module="C1" epd:scenario="Recycling">0.021496587088903944</epd:amount>
                <epd:amount xmlns:epd="http://www.iai.kit.edu/EPD/2013" epd:module="C2" epd:scenario="Recycling">0.005521482669702808</epd:amount>
                <epd:amount xmlns:epd="http://www.iai.kit.edu/EPD/2013" epd:module="C3" epd:scenario="Recycling">0.005693285282299822</epd:amount>
                <epd:amount xmlns:epd="http://www.iai.kit.edu/EPD/2013" epd:module="C4" epd:scenario="Recycling">0.0</epd:amount>
                <epd:amount xmlns:epd="http://www.iai.kit.edu/EPD/2013" epd:module="D" epd:scenario="Recycling">-0.931514556839678</epd:amount>
                <epd:amount xmlns:epd="http://www.iai.kit.edu/EPD/2013" epd:module="A1"/>
                <epd:amount xmlns:epd="http://www.iai.kit.edu/EPD/2013" epd:module="A1-A3">2.2128344400259587</epd:amount>
                <epd:amount xmlns:epd="http://www.iai.kit.edu/EPD/2013" epd:module="A2"/>
                <epd:amount xmlns:epd="http://www.iai.kit.edu/EPD/2013" epd:module="A3"/>
                <epd:amount xmlns:epd="http://www.iai.kit.edu/EPD/2013" epd:module="A4">0.01877493861281537</epd:amount>
                <epd:amount xmlns:epd="http://www.iai.kit.edu/EPD/2013" epd:module="A5">0.021496575781124662</epd:amount>
                <epd:amount xmlns:epd="http://www.iai.kit.edu/EPD/2013" epd:module="B1"/>
                <epd:amount xmlns:epd="http://www.iai.kit.edu/EPD/2013" epd:module="B2"/>
                <epd:amount xmlns:epd="http://www.iai.kit.edu/EPD/2013" epd:module="B3"/>
                <epd:amount xmlns:epd="http://www.iai.kit.edu/EPD/2013" epd:module="B4"/>
                <epd:amount xmlns:epd="http://www.iai.kit.edu/EPD/2013" epd:module="B5"/>
                <epd:amount xmlns:epd="http://www.iai.kit.edu/EPD/2013" epd:module="B6"/>
                <epd:amount xmlns:epd="http://www.iai.kit.edu/EPD/2013" epd:module="B7"/>
                <epd:amount xmlns:epd="http://www.iai.kit.edu/EPD/2013" epd:module="C1"/>
                <epd:amount xmlns:epd="http://www.iai.kit.edu/EPD/2013" epd:module="C2"/>
                <epd:amount xmlns:epd="http://www.iai.kit.edu/EPD/2013" epd:module="C3"/>
                <epd:amount xmlns:epd="http://www.iai.kit.edu/EPD/2013" epd:module="C4"/>
                <epd:amount xmlns:epd="http://www.iai.kit.edu/EPD/2013" epd:module="D"/>
                <epd:referenceToUnitGroupDataSet xmlns:epd="http://www.iai.kit.edu/EPD/2013" refObjectId="bc50c624-a9bc-45b1-a9b0-e6b10d00476f" type="unit group data set" uri="../unitgroups/bc50c624-a9bc-45b1-a9b0-e6b10d00476f">
                    <common:shortDescription>kg SO2-Äqv.</common:shortDescription>
                </epd:referenceToUnitGroupDataSet>
            </common:other>
        </LCIAResult>
        <LCIAResult>
            <referenceToLCIAMethodDataSet type="LCIA method data set" refObjectId="f58827d0-b407-4ec6-be75-8b69efb98a0f" version="00.01.000">
                <common:shortDescription xml:lang="en">Eutrophication potential (EP)</common:shortDescription>
                <common:shortDescription xml:lang="de">Eutrophierungspotenzial (EP)</common:shortDescription>
                <common:shortDescription xml:lang="es">Potencial de eutrofización (EP)</common:shortDescription>
            </referenceToLCIAMethodDataSet>
            <meanAmount>0.0</meanAmount>
            <common:other>
                <epd:amount xmlns:epd="http://www.iai.kit.edu/EPD/2013" epd:module="C1" epd:scenario="Recycling">0.005005742263228089</epd:amount>
                <epd:amount xmlns:epd="http://www.iai.kit.edu/EPD/2013" epd:module="C2" epd:scenario="Recycling">0.001334502837514169</epd:amount>
                <epd:amount xmlns:epd="http://www.iai.kit.edu/EPD/2013" epd:module="C3" epd:scenario="Recycling">0.004026969850738025</epd:amount>
                <epd:amount xmlns:epd="http://www.iai.kit.edu/EPD/2013" epd:module="C4" epd:scenario="Recycling">0.0</epd:amount>
                <epd:amount xmlns:epd="http://www.iai.kit.edu/EPD/2013" epd:module="D" epd:scenario="Recycling">-0.3327021457271861</epd:amount>
                <epd:amount xmlns:epd="http://www.iai.kit.edu/EPD/2013" epd:module="A1"/>
                <epd:amount xmlns:epd="http://www.iai.kit.edu/EPD/2013" epd:module="A1-A3">0.7031917070543886</epd:amount>
                <epd:amount xmlns:epd="http://www.iai.kit.edu/EPD/2013" epd:module="A2"/>
                <epd:amount xmlns:epd="http://www.iai.kit.edu/EPD/2013" epd:module="A3"/>
                <epd:amount xmlns:epd="http://www.iai.kit.edu/EPD/2013" epd:module="A4">0.004537768234536971</epd:amount>
                <epd:amount xmlns:epd="http://www.iai.kit.edu/EPD/2013" epd:module="A5">0.005005739662438855</epd:amount>
                <epd:amount xmlns:epd="http://www.iai.kit.edu/EPD/2013" epd:module="B1"/>
                <epd:amount xmlns:epd="http://www.iai.kit.edu/EPD/2013" epd:module="B2"/>
                <epd:amount xmlns:epd="http://www.iai.kit.edu/EPD/2013" epd:module="B3"/>
                <epd:amount xmlns:epd="http://www.iai.kit.edu/EPD/2013" epd:module="B4"/>
                <epd:amount xmlns:epd="http://www.iai.kit.edu/EPD/2013" epd:module="B5"/>
                <epd:amount xmlns:epd="http://www.iai.kit.edu/EPD/2013" epd:module="B6"/>
                <epd:amount xmlns:epd="http://www.iai.kit.edu/EPD/2013" epd:module="B7"/>
                <epd:amount xmlns:epd="http://www.iai.kit.edu/EPD/2013" epd:module="C1"/>
                <epd:amount xmlns:epd="http://www.iai.kit.edu/EPD/2013" epd:module="C2"/>
                <epd:amount xmlns:epd="http://www.iai.kit.edu/EPD/2013" epd:module="C3"/>
                <epd:amount xmlns:epd="http://www.iai.kit.edu/EPD/2013" epd:module="C4"/>
                <epd:amount xmlns:epd="http://www.iai.kit.edu/EPD/2013" epd:module="D"/>
                <epd:referenceToUnitGroupDataSet xmlns:epd="http://www.iai.kit.edu/EPD/2013" refObjectId="67b5401d-873c-485f-bcf3-6ae83b918822" type="unit group data set" uri="../unitgroups/67b5401d-873c-485f-bcf3-6ae83b918822">
                    <common:shortDescription>kg Phosphat-Äqv.</common:shortDescription>
                </epd:referenceToUnitGroupDataSet>
            </common:other>
        </LCIAResult>
        <LCIAResult>
            <referenceToLCIAMethodDataSet type="LCIA method data set" refObjectId="1e84a202-dae6-42aa-9e9d-71ea48b8be00" version="00.01.000">
                <common:shortDescription xml:lang="en">Formation potential of tropospheric ozone (POCP)</common:shortDescription>
                <common:shortDescription xml:lang="de">Bildungspotential für troposphärisches Ozon (POCP)</common:shortDescription>
                <common:shortDescription xml:lang="es">Potencial de formación de ozono troposférico (POCP)</common:shortDescription>
            </referenceToLCIAMethodDataSet>
            <meanAmount>0.0</meanAmount>
            <common:other>
                <epd:amount xmlns:epd="http://www.iai.kit.edu/EPD/2013" epd:module="C1" epd:scenario="Recycling">0.002614095042294119</epd:amount>
                <epd:amount xmlns:epd="http://www.iai.kit.edu/EPD/2013" epd:module="C2" epd:scenario="Recycling">6.060896760188672E-4</epd:amount>
                <epd:amount xmlns:epd="http://www.iai.kit.edu/EPD/2013" epd:module="C3" epd:scenario="Recycling">2.0250524695193515E-4</epd:amount>
                <epd:amount xmlns:epd="http://www.iai.kit.edu/EPD/2013" epd:module="C4" epd:scenario="Recycling">0.0</epd:amount>
                <epd:amount xmlns:epd="http://www.iai.kit.edu/EPD/2013" epd:module="D" epd:scenario="Recycling">-0.08967396752412907</epd:amount>
                <epd:amount xmlns:epd="http://www.iai.kit.edu/EPD/2013" epd:module="A1"/>
                <epd:amount xmlns:epd="http://www.iai.kit.edu/EPD/2013" epd:module="A1-A3">0.1924334955055714</epd:amount>
                <epd:amount xmlns:epd="http://www.iai.kit.edu/EPD/2013" epd:module="A2"/>
                <epd:amount xmlns:epd="http://www.iai.kit.edu/EPD/2013" epd:module="A3"/>
                <epd:amount xmlns:epd="http://www.iai.kit.edu/EPD/2013" epd:module="A4">0.0020609131086040755</epd:amount>
                <epd:amount xmlns:epd="http://www.iai.kit.edu/EPD/2013" epd:module="A5">0.002614094476905155</epd:amount>
                <epd:amount xmlns:epd="http://www.iai.kit.edu/EPD/2013" epd:module="B1"/>
                <epd:amount xmlns:epd="http://www.iai.kit.edu/EPD/2013" epd:module="B2"/>
                <epd:amount xmlns:epd="http://www.iai.kit.edu/EPD/2013" epd:module="B3"/>
                <epd:amount xmlns:epd="http://www.iai.kit.edu/EPD/2013" epd:module="B4"/>
                <epd:amount xmlns:epd="http://www.iai.kit.edu/EPD/2013" epd:module="B5"/>
                <epd:amount xmlns:epd="http://www.iai.kit.edu/EPD/2013" epd:module="B6"/>
                <epd:amount xmlns:epd="http://www.iai.kit.edu/EPD/2013" epd:module="B7"/>
                <epd:amount xmlns:epd="http://www.iai.kit.edu/EPD/2013" epd:module="C1"/>
                <epd:amount xmlns:epd="http://www.iai.kit.edu/EPD/2013" epd:module="C2"/>
                <epd:amount xmlns:epd="http://www.iai.kit.edu/EPD/2013" epd:module="C3"/>
                <epd:amount xmlns:epd="http://www.iai.kit.edu/EPD/2013" epd:module="C4"/>
                <epd:amount xmlns:epd="http://www.iai.kit.edu/EPD/2013" epd:module="D"/>
                <epd:referenceToUnitGroupDataSet xmlns:epd="http://www.iai.kit.edu/EPD/2013" refObjectId="01c26c17-9a76-406e-8295-f17b55fd909e" type="unit group data set" uri="../unitgroups/01c26c17-9a76-406e-8295-f17b55fd909e">
                    <common:shortDescription>kg Ethen-Äqv.</common:shortDescription>
                </epd:referenceToUnitGroupDataSet>
            </common:other>
        </LCIAResult>
        <LCIAResult>
            <referenceToLCIAMethodDataSet type="LCIA method data set" refObjectId="f7c73bb9-ab1a-4249-9c6d-379a0de6f67e" version="00.01.000">
                <common:shortDescription xml:lang="en">Abiotic depletion potential for non fossil resources (ADPE)</common:shortDescription>
                <common:shortDescription xml:lang="de">Potenzial für den abiotischen Abbau nicht fossiler Ressourcen (ADPE)</common:shortDescription>
                <common:shortDescription xml:lang="es">Potencial de agotamiento de recursos abióticos para recursos no fósiles (ADPE)</common:shortDescription>
            </referenceToLCIAMethodDataSet>
            <meanAmount>0.0</meanAmount>
            <common:other>
                <epd:amount xmlns:epd="http://www.iai.kit.edu/EPD/2013" epd:module="C1" epd:scenario="Recycling">9.55223241408116E-7</epd:amount>
                <epd:amount xmlns:epd="http://www.iai.kit.edu/EPD/2013" epd:module="C2" epd:scenario="Recycling">3.2408119169687643E-6</epd:amount>
                <epd:amount xmlns:epd="http://www.iai.kit.edu/EPD/2013" epd:module="C3" epd:scenario="Recycling">7.990024577827486E-7</epd:amount>
                <epd:amount xmlns:epd="http://www.iai.kit.edu/EPD/2013" epd:module="C4" epd:scenario="Recycling">0.0</epd:amount>
                <epd:amount xmlns:epd="http://www.iai.kit.edu/EPD/2013" epd:module="D" epd:scenario="Recycling">-0.016015163000704193</epd:amount>
                <epd:amount xmlns:epd="http://www.iai.kit.edu/EPD/2013" epd:module="A1"/>
                <epd:amount xmlns:epd="http://www.iai.kit.edu/EPD/2013" epd:module="A1-A3">0.027600821530107837</epd:amount>
                <epd:amount xmlns:epd="http://www.iai.kit.edu/EPD/2013" epd:module="A2"/>
                <epd:amount xmlns:epd="http://www.iai.kit.edu/EPD/2013" epd:module="A3"/>
                <epd:amount xmlns:epd="http://www.iai.kit.edu/EPD/2013" epd:module="A4">1.1019874175644204E-5</epd:amount>
                <epd:amount xmlns:epd="http://www.iai.kit.edu/EPD/2013" epd:module="A5">9.55223241408116E-7</epd:amount>
                <epd:amount xmlns:epd="http://www.iai.kit.edu/EPD/2013" epd:module="B1"/>
                <epd:amount xmlns:epd="http://www.iai.kit.edu/EPD/2013" epd:module="B2"/>
                <epd:amount xmlns:epd="http://www.iai.kit.edu/EPD/2013" epd:module="B3"/>
                <epd:amount xmlns:epd="http://www.iai.kit.edu/EPD/2013" epd:module="B4"/>
                <epd:amount xmlns:epd="http://www.iai.kit.edu/EPD/2013" epd:module="B5"/>
                <epd:amount xmlns:epd="http://www.iai.kit.edu/EPD/2013" epd:module="B6"/>
                <epd:amount xmlns:epd="http://www.iai.kit.edu/EPD/2013" epd:module="B7"/>
                <epd:amount xmlns:epd="http://www.iai.kit.edu/EPD/2013" epd:module="C1"/>
                <epd:amount xmlns:epd="http://www.iai.kit.edu/EPD/2013" epd:module="C2"/>
                <epd:amount xmlns:epd="http://www.iai.kit.edu/EPD/2013" epd:module="C3"/>
                <epd:amount xmlns:epd="http://www.iai.kit.edu/EPD/2013" epd:module="C4"/>
                <epd:amount xmlns:epd="http://www.iai.kit.edu/EPD/2013" epd:module="D"/>
                <epd:referenceToUnitGroupDataSet xmlns:epd="http://www.iai.kit.edu/EPD/2013" refObjectId="54ccd2d9-a32a-4fc2-923d-f2c8c93e89d4" type="unit group data set" uri="../unitgroups/54ccd2d9-a32a-4fc2-923d-f2c8c93e89d4">
                    <common:shortDescription>kg Sb-Äqv.</common:shortDescription>
                </epd:referenceToUnitGroupDataSet>
            </common:other>
        </LCIAResult>
        <LCIAResult>
            <referenceToLCIAMethodDataSet type="LCIA method data set" refObjectId="804ebcdf-309d-4098-8ed8-fdaf2f389981" version="00.01.000">
                <common:shortDescription xml:lang="en">Abiotic depletion potential for fossil resources (ADPF)</common:shortDescription>
                <common:shortDescription xml:lang="de">Potenzial für den abiotischen Abbau fossiler Brennstoffe (ADPF)</common:shortDescription>
                <common:shortDescription xml:lang="es">Potencial de agotamiento de recursos abióticos para recursos fósiles (ADPF)</common:shortDescription>
            </referenceToLCIAMethodDataSet>
            <meanAmount>0.0</meanAmount>
            <common:other>
                <epd:amount xmlns:epd="http://www.iai.kit.edu/EPD/2013" epd:module="C1" epd:scenario="Recycling">41.02841190798658</epd:amount>
                <epd:amount xmlns:epd="http://www.iai.kit.edu/EPD/2013" epd:module="C2" epd:scenario="Recycling">16.536217685818748</epd:amount>
                <epd:amount xmlns:epd="http://www.iai.kit.edu/EPD/2013" epd:module="C3" epd:scenario="Recycling">6.100861604738825</epd:amount>
                <epd:amount xmlns:epd="http://www.iai.kit.edu/EPD/2013" epd:module="C4" epd:scenario="Recycling">0.0</epd:amount>
                <epd:amount xmlns:epd="http://www.iai.kit.edu/EPD/2013" epd:module="D" epd:scenario="Recycling">-1194.2433860790081</epd:amount>
                <epd:amount xmlns:epd="http://www.iai.kit.edu/EPD/2013" epd:module="A1"/>
                <epd:amount xmlns:epd="http://www.iai.kit.edu/EPD/2013" epd:module="A1-A3">4295.484925369012</epd:amount>
                <epd:amount xmlns:epd="http://www.iai.kit.edu/EPD/2013" epd:module="A2"/>
                <epd:amount xmlns:epd="http://www.iai.kit.edu/EPD/2013" epd:module="A3"/>
                <epd:amount xmlns:epd="http://www.iai.kit.edu/EPD/2013" epd:module="A4">56.22882296933991</epd:amount>
                <epd:amount xmlns:epd="http://www.iai.kit.edu/EPD/2013" epd:module="A5">41.028407384874875</epd:amount>
                <epd:amount xmlns:epd="http://www.iai.kit.edu/EPD/2013" epd:module="B1"/>
                <epd:amount xmlns:epd="http://www.iai.kit.edu/EPD/2013" epd:module="B2"/>
                <epd:amount xmlns:epd="http://www.iai.kit.edu/EPD/2013" epd:module="B3"/>
                <epd:amount xmlns:epd="http://www.iai.kit.edu/EPD/2013" epd:module="B4"/>
                <epd:amount xmlns:epd="http://www.iai.kit.edu/EPD/2013" epd:module="B5"/>
                <epd:amount xmlns:epd="http://www.iai.kit.edu/EPD/2013" epd:module="B6"/>
                <epd:amount xmlns:epd="http://www.iai.kit.edu/EPD/2013" epd:module="B7"/>
                <epd:amount xmlns:epd="http://www.iai.kit.edu/EPD/2013" epd:module="C1"/>
                <epd:amount xmlns:epd="http://www.iai.kit.edu/EPD/2013" epd:module="C2"/>
                <epd:amount xmlns:epd="http://www.iai.kit.edu/EPD/2013" epd:module="C3"/>
                <epd:amount xmlns:epd="http://www.iai.kit.edu/EPD/2013" epd:module="C4"/>
                <epd:amount xmlns:epd="http://www.iai.kit.edu/EPD/2013" epd:module="D"/>
                <epd:referenceToUnitGroupDataSet xmlns:epd="http://www.iai.kit.edu/EPD/2013" refObjectId="93a60a57-a3c8-11da-a746-0800200c9a66" type="unit group data set" uri="../unitgroups/93a60a57-a3c8-11da-a746-0800200c9a66">
                    <common:shortDescription>MJ</common:shortDescription>
                </epd:referenceToUnitGroupDataSet>
            </common:other>
        </LCIAResult>
    </LCIAResults>
</processDataSet>
