<?xml-stylesheet type='text/xsl' href='../../stylesheets/epd2html.xsl'?>
<processDataSet xmlns:xsi="http://www.w3.org/2001/XMLSchema-instance" xmlns="http://lca.jrc.it/ILCD/Process" xsi:schemaLocation="http://lca.jrc.it/ILCD/Process ../../schemas/EPD_DataSet.xsd" locations="../ILCDLocations.xml" version="1.1">
  <processInformation>
    <dataSetInformation>
      <common:UUID xmlns:common="http://lca.jrc.it/ILCD/Common">704177f4-78cd-47a3-b71c-07899df86615</common:UUID>
      <name>
        <baseName xmlns:epd="http://www.iai.kit.edu/EPD/2013" xmlns:common="http://lca.jrc.it/ILCD/Common" xml:lang="en">Polystyrene foam filling (cement bound)</baseName>
        <baseName xmlns:epd="http://www.iai.kit.edu/EPD/2013" xmlns:common="http://lca.jrc.it/ILCD/Common" xml:lang="de">Schüttung aus Polystyrolschaumstoff-Partikeln (zementgebunden)</baseName>
      </name>
      <classificationInformation>
        <common:classification xmlns:common="http://lca.jrc.it/ILCD/Common" name="oekobau.dat">
          <common:class level="0" classId="2">Dämmstoffe</common:class>
          <common:class level="1" classId="2.2">Expandiertes Polystyrol (EPS)</common:class>
          <common:class level="2" classId="2.2.01">EPS weiß</common:class>
        </common:classification>
      </classificationInformation>
      <common:generalComment xmlns:common="http://lca.jrc.it/ILCD/Common" xmlns:epd="http://www.iai.kit.edu/EPD/2013" xml:lang="en">This data set has been modeled according to the European Standard EN 15804 for Sustainable Building. Results are depicted in modules that allow the structured expression of results over the entire life cycle.</common:generalComment>
      <common:generalComment xmlns:common="http://lca.jrc.it/ILCD/Common" xmlns:epd="http://www.iai.kit.edu/EPD/2013" xml:lang="de">Dieser Datensatz wurde nach dem European Standard EN 15804 für Nachhaltiges Bauen modelliert. Ergebnisse werden in Modulen abgebildet, die den strukturierten Ausdruck von Ergebnissen über den gesamten Lebenszyklus zulassen.</common:generalComment>
      <common:other xmlns:common="http://lca.jrc.it/ILCD/Common">
        <epd:safetyMargins xmlns:epd="http://www.iai.kit.edu/EPD/2013">
          <epd:margins>10</epd:margins>
          <epd:description xml:lang="en">Product system almost completely covered. Good technological, temporal and geographic representativeness.</epd:description>
          <epd:description xml:lang="de">Produktsystem weitgehend vollständig abgebildet. Gute technologische, zeitliche und geographische Repräsentativität.</epd:description>
        </epd:safetyMargins>
      </common:other>
    </dataSetInformation>
    <quantitativeReference type="Reference flow(s)">
      <referenceToReferenceFlow>101140</referenceToReferenceFlow>
    </quantitativeReference>
    <time>
      <common:referenceYear xmlns:common="http://lca.jrc.it/ILCD/Common">2018</common:referenceYear>
      <common:dataSetValidUntil xmlns:common="http://lca.jrc.it/ILCD/Common">2022</common:dataSetValidUntil>
      <common:timeRepresentativenessDescription xmlns:common="http://lca.jrc.it/ILCD/Common" xmlns:epd="http://www.iai.kit.edu/EPD/2013" xml:lang="en">annual average</common:timeRepresentativenessDescription>
      <common:timeRepresentativenessDescription xmlns:common="http://lca.jrc.it/ILCD/Common" xmlns:epd="http://www.iai.kit.edu/EPD/2013" xml:lang="de">Jährlicher Durchschnitt</common:timeRepresentativenessDescription>
    </time>
    <geography>
      <locationOfOperationSupplyOrProduction location="DE">
        <descriptionOfRestrictions xmlns:epd="http://www.iai.kit.edu/EPD/2013" xmlns:common="http://lca.jrc.it/ILCD/Common" xml:lang="en">The data set represents the country specific situation in Germany, focusing on the main technologies, the region specific characteristics and / or import statistics.</descriptionOfRestrictions>
        <descriptionOfRestrictions xmlns:epd="http://www.iai.kit.edu/EPD/2013" xmlns:common="http://lca.jrc.it/ILCD/Common" xml:lang="de">Der Datensatz bildet die länderspezifische Situation in Deutschland ab. Dabei werden Haupttechnologien, spezifische regionale Charakteristiken und ggf. Importstatistiken berücksichtigt.</descriptionOfRestrictions>
      </locationOfOperationSupplyOrProduction>
    </geography>
    <technology>
      <technologyDescriptionAndIncludedProcesses xmlns:common="http://lca.jrc.it/ILCD/Common" xmlns:epd="http://www.iai.kit.edu/EPD/2013" xml:lang="en">Usually, EPS particles are produced for fillings by grinding production waste (for example from EPS plate production). Since the price differences per unit of volume  for EPS plates and EPS filling are negligibly small, no economic allocation of the environmental burden between main product and by-product was applied. Instead, balancing was applied for 100% primary material. Other raw materials include cement and sand. The mixture is mixed with water and installed similar to a cement screed. The production of EPS and the use of cement dominate the life cycle assessment (together &gt; 80% of the GWP).


Background system:
Electricity: Electricity from renewable and non- renewable powerplants is modelled so that it represents a countrys specific consumption mix including transmission / distribution losses, own consumption, imports, emissions and efficiency standards, and energy carrier properties. Several factors are taken into account. (1) Energy carrier production - The exploration, mining / production, processing, and transportation of energy carrier supply chains are modelled for each country. The models account for differences among countries in production and processing, including crude oil production technologies, flaring rates, production efficiencies, emissions, etc. (2) Energy carrier supply - Each countrys specific energy carrier supply is modelled, taking into account domestic supply versus imports from abroad. Energy carrier properties (e.g. carbon and energy content), which can vary depending from where an energy carrier is sourced, are adjusted accordingly. (3) Power plants - Models are created to represent energy carrier-specific power plants and electricity generation facilities specific to different renewable energy resources. Energy carrier production and supply models are used to represent power plant inputs. Combined heat and power (CHP) plants are also considered. (4) Electricity grid - Models representing the electricity generation facilities are combined into a larger model that reflects a countrys consumption mix. The larger model accounts for a countrys production mix, internal consumption (e.g. pumped storage for hydro power), transmission / distribution losses, and imported electricity. The country model is also adjusted according to national power plant emission and efficiency standards, as well as the countrys share of electricity plants versus CHP facilities.
Thermal energy, process steam: The thermal energy and process steam supply is modelled to reflect each countrys emission standards and typical energy carriers (e.g., coal, natural gas, etc.) Both thermal energy and process steam are assumed to be produced at heat plants. Thermal energy datasets assume energy carrier inputs are converted to thermal energy with 100% efficiency; process steam datasets assume conversion efficiencies of 85%, 90% to 95%. The energy carriers used for the generation of thermal energy and process steam are modelled according to each countrys import situation (see electricity above).
Transportation: All relevant and known transportation processes are included. Ocean-going and inland ship transport as well as rail, truck and pipeline transport of bulk commodities are considered.
Energy carriers: The energy carriers and their respective properties are modelled according to the specific supply situation (see electricity above).
Refinery products: Diesel fuel, gasoline, technical gases, fuel oils, lubricants and residues such as bitumen are modelled with a parameterised country-specific refinery model. The refinery model aims to represent each countrys refining processes (e.g. emissions levels, internal energy consumption, etc.), as well as the countrys product output spectrum, which can vary significantly among countries. The supply of crude oil is likewise modelled according to the country-specific situation and accounts for differences in resource properties (e.g., crude oil energy content).</technologyDescriptionAndIncludedProcesses>
      <technologyDescriptionAndIncludedProcesses xmlns:common="http://lca.jrc.it/ILCD/Common" xmlns:epd="http://www.iai.kit.edu/EPD/2013" xml:lang="de">In der Regel werden EPS-Partikel für Schüttungen durch Zerkleinerung von Produktionsabfällen (z.B. aus der EPS Plattenproduktion) hergestellt. Da die Preisunterschiede für beispielsweise EPS Platten und EPS Schüttung je Volumeneinheit vernachlässigbar klein sind wurde hier auf eine ökonomische Allokation der Umweltlasten zwischen Haupt- und Nebenprodukt verzichtet. Stattdessen wurde mit 100% Primärmaterial bilanziert. Weitere Rohstoffe sind Zement und Sand. Das Gemisch wird mit Wasser vermischt und ähnlich einem Zementestrich eingebaut. Die Herstellung von EPS und der Zementeinsatz dominieren die Ökobilanz (zusammen &gt;80% des GWP).


Hintergrundsystem:
Strom: Die Stromerzeugung wird entsprechend der länderspezifischen Randbedingungen modelliert. Die landesspezifische Analyse beinhaltet:
1.: Spezifische Kraftwerke der verschiedenen fossilen Energieträger und der Einsatz erneuerbarer Energien sind entsprechend der länderspezifischen Energieträgermixe modelliert. Die Analyse bezieht Stromimporte aus den Nachbarländern, Transmissions-und Verteilungsverluste und den Eigenverbrauch im Kraftwerk und bei der Verteilung bzw. Speicherung, z. B. durch Pumpspeicherwerke, ein.
2.: Die landes-/regionalspezifischen Technologiestandards sowie die Erzeugung in Elektrizitätskraftwerken und/oder in speziellen Kraftwerken mit Kraft-Wärme-Kopplung (KWK) sind berücksichtigt. 
3.: Die länderspezifische Energieträgerbereitstellung (mit Anteil der Importe und/oder Eigenversorgung) einschließlich der Energieträger-Eigenschaften (z. B. Elementar- und Energiegehalte) werden berücksichtigt. 
4.: Die Förderung, Produktion, Verarbeitung und Transportprozesse werden entsprechend der Situation im jeweiligen Stromerzeugerland modelliert. Die unterschiedlichen Produktions- und Verarbeitungsverfahren (Emissionen und Wirkungsgrade) in den verschiedenen Energieerzeugerländern werden einbezogen, z. B. Rohöl-Veredelungsverfahren oder Abfackel-Raten an den Ölplattformen.
Thermische Energie, Prozessdampf: Die Erzeugung von Dampf und thermischer Energie in Heizkraftwerken wird entsprechend der landesspezifischen Situation (Emissionsgrenzwerte, Energieträgerbasis) modelliert.
Der Wirkungsgrad für die thermische Energieerzeugung beträgt per Definition 100% des Energieträgereinsatzes. Für Prozessdampf liegt der Wirkungsgrad im Bereich von 85-95%. Die zur Heizenergie-Erzeugung verwendeten Energieträger werden entsprechend der nationalen Situation modelliert (siehe Kapitel Strom oben).
Transporte: Alle relevanten und bekannten Transportprozesse in Form von See- und Binnenschiffsverkehr sowie Bahn-, Lkw- und der Leitungstransport sind enthalten.
Energieträger: Die Energieträger werden entsprechend der spezifischen Versorgungslage modelliert (siehe Kapitel Strom oben). 
Raffinerieprodukte: Diesel, Benzin, technische Gase, Heizöl, Schmierstoffe und Rückstände, wie Bitumen, werden mit einem parametrierten länderspezifische Raffineriemodell modelliert. Das Raffinerie-Modell bezieht die länderspezifischen Veredelungsverfahren (z. B. Emissionspegel, interner Energieverbrauch etc.) und das länderspezifische Produktspektrum ein, das sich je nach Land stark unterscheiden kann. Die Rohöl-Förderung wird gemäß der länderspezifischen Situation mit den jeweiligen Energieträger-Eigenschaften modelliert.</technologyDescriptionAndIncludedProcesses>
      <technologicalApplicability xmlns:common="http://lca.jrc.it/ILCD/Common" xmlns:epd="http://www.iai.kit.edu/EPD/2013" xml:lang="en">Bound fills of polystyrene foam (EPS) are used as a insulation and leveling layer, especially in old buildings. With an appropriate structure (load-distributing layer over the fill) loads of up to 5 kN/m² can be removed through the fill. Fill hights from 4-50 cm can be introduced in one work step.</technologicalApplicability>
      <technologicalApplicability xmlns:common="http://lca.jrc.it/ILCD/Common" xmlns:epd="http://www.iai.kit.edu/EPD/2013" xml:lang="de">Gebundene Schüttungen aus Polystyrolschaumstoff (EPS) werden als Dämm- und Ausgleichsschicht vorallem im Altbau eingesetzt. Bei entsprechendem Aufbau (lastverteilende Schicht über der Schüttung) können Lasten bis etwa 5 kN/m² durch die Schüttung abgetragen werden. Es können Schütthöhen von 4 - 50cm in einem Arbeitsschritt eingebracht werden.</technologicalApplicability>
    </technology>
  </processInformation>
  <modellingAndValidation>
    <LCIMethodAndAllocation>
      <typeOfDataSet>EPD</typeOfDataSet>
      <common:other xmlns:common="http://lca.jrc.it/ILCD/Common">
        <epd:subType xmlns:epd="http://www.iai.kit.edu/EPD/2013">generic dataset</epd:subType>
      </common:other>
    </LCIMethodAndAllocation>
    <dataSourcesTreatmentAndRepresentativeness>
      <referenceToDataSource refObjectId="61875b4e-7249-444b-8691-e4a04e6d3c47" version="39.00.000" type="source data set" uri="../sources/61875b4e-7249-444b-8691-e4a04e6d3c47.xml">
        <common:shortDescription xmlns:common="http://lca.jrc.it/ILCD/Common" xmlns:epd="http://www.iai.kit.edu/EPD/2013" xml:lang="en">GaBi databases</common:shortDescription>
        <common:shortDescription xmlns:common="http://lca.jrc.it/ILCD/Common" xmlns:epd="http://www.iai.kit.edu/EPD/2013" xml:lang="de">GaBi databases</common:shortDescription>
      </referenceToDataSource>
      <referenceToDataSource refObjectId="cb50c596-16b4-44e4-b1aa-319319a79fb5" version="39.00.000" type="source data set" uri="../sources/cb50c596-16b4-44e4-b1aa-319319a79fb5.xml">
        <common:shortDescription xmlns:common="http://lca.jrc.it/ILCD/Common" xmlns:epd="http://www.iai.kit.edu/EPD/2013" xml:lang="en">GaBi Database Edition 2020, SP40</common:shortDescription>
        <common:shortDescription xmlns:common="http://lca.jrc.it/ILCD/Common" xmlns:epd="http://www.iai.kit.edu/EPD/2013" xml:lang="de">GaBi Database Edition 2020, SP40</common:shortDescription>
      </referenceToDataSource>
      <referenceToDataSource refObjectId="28d74cc0-db8b-4d7e-bc44-5f6d56ce0c4a" version="39.00.000" type="source data set" uri="../sources/28d74cc0-db8b-4d7e-bc44-5f6d56ce0c4a.xml">
        <common:shortDescription xmlns:common="http://lca.jrc.it/ILCD/Common" xmlns:epd="http://www.iai.kit.edu/EPD/2013" xml:lang="en">GaBi database (all versions)</common:shortDescription>
        <common:shortDescription xmlns:common="http://lca.jrc.it/ILCD/Common" xmlns:epd="http://www.iai.kit.edu/EPD/2013" xml:lang="de">GaBi database (all versions)</common:shortDescription>
      </referenceToDataSource>
      <useAdviceForDataSet xmlns:common="http://lca.jrc.it/ILCD/Common" xmlns:epd="http://www.iai.kit.edu/EPD/2013" xml:lang="en">This dataset refers to 1 m³ polystyrene foam filling. Cement is used as binding agent. Dry bulk density 350 kg/m³, thermal conductivity 0.1 - 0.15 W/mK. The dataset can be used for approximate estimation of other bulk densities of 300 - 400 kg.

The data set represents a cradle to gate inventory. It can be used to characterise the supply chain situation of the respective commodity in a representative manner. Combination with individual unit processes using this commodity enables the generation of user-specific (product) LCAs.</useAdviceForDataSet>
      <useAdviceForDataSet xmlns:common="http://lca.jrc.it/ILCD/Common" xmlns:epd="http://www.iai.kit.edu/EPD/2013" xml:lang="de">Dieser Datensatz bezieht sich auf 1 m³ Schüttung aus Polystyrolschaumstoff-Partikeln. Als Bindemittel wird Zement eingesetzt. Trockenrohdichte 350 kg/m³, Wärmeleitfähigkeit 0,1 - 0,15 W/mK. Der Datensatz kann für die näherungsweise Abschätzung anderer Schüttdichten von 300 - 400 kg verwendet werden.

Der Datensatz repräsentiert ein Cradle to Gate Inventar. Er kann verwendet werden, um die Lieferkette des jeweiligen Produktes in einer repräsentativen Weise zu charakterisieren. Die Kombination mit einzelnen Einheitenprozessen und diesem Produkt ermöglicht die Erstellung von anwenderspezifischen (Produkt-) LCAs</useAdviceForDataSet>
    </dataSourcesTreatmentAndRepresentativeness>
    <validation>
      <review type="Dependent internal review">
        <common:referenceToNameOfReviewerAndInstitution xmlns:common="http://lca.jrc.it/ILCD/Common" refObjectId="d7fa0337-f279-430d-becf-7f3111a85010" version="39.00.000" type="contact data set" uri="../contacts/d7fa0337-f279-430d-becf-7f3111a85010.xml">
          <common:shortDescription xmlns:epd="http://www.iai.kit.edu/EPD/2013" xml:lang="en">thinkstep</common:shortDescription>
          <common:shortDescription xmlns:epd="http://www.iai.kit.edu/EPD/2013" xml:lang="de">thinkstep</common:shortDescription>
        </common:referenceToNameOfReviewerAndInstitution>
        <common:referenceToNameOfReviewerAndInstitution xmlns:common="http://lca.jrc.it/ILCD/Common" refObjectId="de53c560-d6a9-11da-a94d-0800200c9a66" version="39.00.000" type="contact data set" uri="../contacts/de53c560-d6a9-11da-a94d-0800200c9a66.xml">
          <common:shortDescription xmlns:epd="http://www.iai.kit.edu/EPD/2013" xml:lang="en">IABP-GaBi</common:shortDescription>
          <common:shortDescription xmlns:epd="http://www.iai.kit.edu/EPD/2013" xml:lang="de">IABP-GaBi</common:shortDescription>
        </common:referenceToNameOfReviewerAndInstitution>
        <common:referenceToNameOfReviewerAndInstitution xmlns:common="http://lca.jrc.it/ILCD/Common" refObjectId="c0a9feeb-48d1-4c8f-9e8f-3ada7c0294c7" version="39.00.000" type="contact data set" uri="../contacts/c0a9feeb-48d1-4c8f-9e8f-3ada7c0294c7.xml">
          <common:shortDescription xmlns:epd="http://www.iai.kit.edu/EPD/2013" xml:lang="en">IBP-GaBi</common:shortDescription>
          <common:shortDescription xmlns:epd="http://www.iai.kit.edu/EPD/2013" xml:lang="de">IBP-GaBi</common:shortDescription>
        </common:referenceToNameOfReviewerAndInstitution>
      </review>
      <review type="Independent external review">
        <common:referenceToNameOfReviewerAndInstitution xmlns:common="http://lca.jrc.it/ILCD/Common" refObjectId="8f1306f0-7b83-4f36-a537-aa83f0498266" version="39.00.000" type="contact data set" uri="../contacts/8f1306f0-7b83-4f36-a537-aa83f0498266.xml">
          <common:shortDescription xmlns:epd="http://www.iai.kit.edu/EPD/2013" xml:lang="en">GaBi user forum</common:shortDescription>
          <common:shortDescription xmlns:epd="http://www.iai.kit.edu/EPD/2013" xml:lang="de">GaBi user forum</common:shortDescription>
        </common:referenceToNameOfReviewerAndInstitution>
        <common:referenceToNameOfReviewerAndInstitution xmlns:common="http://lca.jrc.it/ILCD/Common" refObjectId="851d996c-b88d-45ce-983a-b00ed0393ffb" version="39.00.000" type="contact data set" uri="../contacts/851d996c-b88d-45ce-983a-b00ed0393ffb.xml">
          <common:shortDescription xmlns:epd="http://www.iai.kit.edu/EPD/2013" xml:lang="en">GaBi bug forum</common:shortDescription>
          <common:shortDescription xmlns:epd="http://www.iai.kit.edu/EPD/2013" xml:lang="de">GaBi bug forum</common:shortDescription>
        </common:referenceToNameOfReviewerAndInstitution>
        <common:referenceToNameOfReviewerAndInstitution xmlns:common="http://lca.jrc.it/ILCD/Common" refObjectId="47511c41-5096-4dcf-be4f-dbb0c1c5cffc" version="39.00.000" type="contact data set" uri="../contacts/47511c41-5096-4dcf-be4f-dbb0c1c5cffc.xml">
          <common:shortDescription xmlns:epd="http://www.iai.kit.edu/EPD/2013" xml:lang="en">GaBi user community</common:shortDescription>
          <common:shortDescription xmlns:epd="http://www.iai.kit.edu/EPD/2013" xml:lang="de">GaBi user community</common:shortDescription>
        </common:referenceToNameOfReviewerAndInstitution>
      </review>
    </validation>
    <complianceDeclarations>
      <compliance>
        <common:referenceToComplianceSystem xmlns:common="http://lca.jrc.it/ILCD/Common" refObjectId="b00f9ec0-7874-11e3-981f-0800200c9a66" version="02.00.000" type="source data set" uri="../sources/b00f9ec0-7874-11e3-981f-0800200c9a66.xml">
          <common:shortDescription xmlns:epd="http://www.iai.kit.edu/EPD/2013" xml:lang="en">DIN EN 15804</common:shortDescription>
          <common:shortDescription xmlns:epd="http://www.iai.kit.edu/EPD/2013" xml:lang="de">DIN EN 15804</common:shortDescription>
        </common:referenceToComplianceSystem>
        <common:approvalOfOverallCompliance xmlns:common="http://lca.jrc.it/ILCD/Common">Fully compliant</common:approvalOfOverallCompliance>
      </compliance>
    </complianceDeclarations>
  </modellingAndValidation>
  <administrativeInformation>
    <dataEntryBy>
      <common:timeStamp xmlns:common="http://lca.jrc.it/ILCD/Common">2019-12-04T10:06:41+01:00</common:timeStamp>
      <common:referenceToDataSetFormat xmlns:common="http://lca.jrc.it/ILCD/Common" refObjectId="a97a0155-0234-4b87-b4ce-a45da52f2a40" version="03.00.000" type="source data set" uri="../sources/a97a0155-0234-4b87-b4ce-a45da52f2a40.xml">
        <common:shortDescription xmlns:epd="http://www.iai.kit.edu/EPD/2013" xml:lang="en">ILCD format 1.1</common:shortDescription>
        <common:shortDescription xmlns:epd="http://www.iai.kit.edu/EPD/2013" xml:lang="de">ILCD format 1.1</common:shortDescription>
      </common:referenceToDataSetFormat>
      <common:referenceToDataSetFormat xmlns:common="http://lca.jrc.it/ILCD/Common" refObjectId="cba73800-7874-11e3-981f-0800200c9a66" version="02.00.000" type="source data set" uri="../sources/cba73800-7874-11e3-981f-0800200c9a66.xml">
        <common:shortDescription xmlns:epd="http://www.iai.kit.edu/EPD/2013" xml:lang="en">EPD Data Format Extensions</common:shortDescription>
        <common:shortDescription xmlns:epd="http://www.iai.kit.edu/EPD/2013" xml:lang="de">EPD-Datenformaterweiterungen</common:shortDescription>
      </common:referenceToDataSetFormat>
      <common:referenceToPersonOrEntityEnteringTheData xmlns:common="http://lca.jrc.it/ILCD/Common" refObjectId="d7fa0337-f279-430d-becf-7f3111a85010" version="39.00.000" type="contact data set" uri="../contacts/d7fa0337-f279-430d-becf-7f3111a85010.xml">
        <common:shortDescription xmlns:epd="http://www.iai.kit.edu/EPD/2013" xml:lang="en">thinkstep</common:shortDescription>
        <common:shortDescription xmlns:epd="http://www.iai.kit.edu/EPD/2013" xml:lang="de">thinkstep</common:shortDescription>
      </common:referenceToPersonOrEntityEnteringTheData>
    </dataEntryBy>
    <publicationAndOwnership>
      <common:dataSetVersion xmlns:common="http://lca.jrc.it/ILCD/Common">20.19.120</common:dataSetVersion>
      <common:permanentDataSetURI xmlns:common="http://lca.jrc.it/ILCD/Common"/>
      <common:referenceToOwnershipOfDataSet xmlns:common="http://lca.jrc.it/ILCD/Common" refObjectId="d7fa0337-f279-430d-becf-7f3111a85010" version="39.00.000" type="contact data set" uri="../contacts/d7fa0337-f279-430d-becf-7f3111a85010.xml">
        <common:shortDescription xmlns:epd="http://www.iai.kit.edu/EPD/2013" xml:lang="en">thinkstep</common:shortDescription>
        <common:shortDescription xmlns:epd="http://www.iai.kit.edu/EPD/2013" xml:lang="de">thinkstep</common:shortDescription>
      </common:referenceToOwnershipOfDataSet>
      <common:copyright xmlns:common="http://lca.jrc.it/ILCD/Common">true</common:copyright>
    </publicationAndOwnership>
  </administrativeInformation>
  <exchanges>
    <exchange dataSetInternalID="101140">
      <referenceToFlowDataSet refObjectId="8dbd12dd-69f6-41ed-a4c7-0289655c7ecf" version="39.00.000" type="flow data set" uri="../flows/8dbd12dd-69f6-41ed-a4c7-0289655c7ecf.xml">
        <common:shortDescription xmlns:common="http://lca.jrc.it/ILCD/Common" xmlns:epd="http://www.iai.kit.edu/EPD/2013" xml:lang="en">Polystyrene foam filling (cement bound) [m3]</common:shortDescription>
        <common:shortDescription xmlns:common="http://lca.jrc.it/ILCD/Common" xmlns:epd="http://www.iai.kit.edu/EPD/2013" xml:lang="de">Schüttung aus Polystyrolschaumstoff-Partikeln (zementgebunden) [m3]</common:shortDescription>
      </referenceToFlowDataSet>
      <meanAmount>1</meanAmount>
    </exchange>
    <exchange dataSetInternalID="101141">
      <referenceToFlowDataSet refObjectId="20f32be5-0398-4288-9b6d-accddd195317" version="39.00.000" type="flow data set" uri="../flows/20f32be5-0398-4288-9b6d-accddd195317.xml">
        <common:shortDescription xmlns:common="http://lca.jrc.it/ILCD/Common" xmlns:epd="http://www.iai.kit.edu/EPD/2013" xml:lang="en">Use of renewable primary energy (PERE)</common:shortDescription>
        <common:shortDescription xmlns:common="http://lca.jrc.it/ILCD/Common" xmlns:epd="http://www.iai.kit.edu/EPD/2013" xml:lang="de">Erneuerbare Primärenergie als Energieträger (PERE)</common:shortDescription>
      </referenceToFlowDataSet>
      <functionType>General reminder flow</functionType>
      <exchangeDirection>Input</exchangeDirection>
      <common:other xmlns:common="http://lca.jrc.it/ILCD/Common">
        <epd:amount xmlns:epd="http://www.iai.kit.edu/EPD/2013" epd:module="A1-A3">111.134910832947</epd:amount>
        <epd:referenceToUnitGroupDataSet xmlns:epd="http://www.iai.kit.edu/EPD/2013" refObjectId="93a60a57-a3c8-11da-a746-0800200c9a66" version="03.00.000" type="unit group data set" uri="../unitgroups/93a60a57-a3c8-11da-a746-0800200c9a66.xml">
          <common:shortDescription xml:lang="en">MJ</common:shortDescription>
          <common:shortDescription xml:lang="de">MJ</common:shortDescription>
        </epd:referenceToUnitGroupDataSet>
        <epd:amount xmlns:epd="http://www.iai.kit.edu/EPD/2013" epd:module="C1">0</epd:amount>
        <epd:amount xmlns:epd="http://www.iai.kit.edu/EPD/2013" epd:module="C2">0.0559328081883679</epd:amount>
        <epd:amount xmlns:epd="http://www.iai.kit.edu/EPD/2013" epd:module="C3">3.35621716827408</epd:amount>
        <epd:amount xmlns:epd="http://www.iai.kit.edu/EPD/2013" epd:module="D">-181.187238694297</epd:amount>
      </common:other>
    </exchange>
    <exchange dataSetInternalID="101142">
      <referenceToFlowDataSet refObjectId="fb3ec0de-548d-4508-aea5-00b73bf6f702" version="39.00.000" type="flow data set" uri="../flows/fb3ec0de-548d-4508-aea5-00b73bf6f702.xml">
        <common:shortDescription xmlns:common="http://lca.jrc.it/ILCD/Common" xmlns:epd="http://www.iai.kit.edu/EPD/2013" xml:lang="en">Primary energy resources used as raw materials (PERM)</common:shortDescription>
        <common:shortDescription xmlns:common="http://lca.jrc.it/ILCD/Common" xmlns:epd="http://www.iai.kit.edu/EPD/2013" xml:lang="de">Erneuerbare Primärenergie zur stofflichen Nutzung (PERM)</common:shortDescription>
      </referenceToFlowDataSet>
      <functionType>General reminder flow</functionType>
      <exchangeDirection>Input</exchangeDirection>
      <common:other xmlns:common="http://lca.jrc.it/ILCD/Common">
        <epd:amount xmlns:epd="http://www.iai.kit.edu/EPD/2013" epd:module="A1-A3">0</epd:amount>
        <epd:referenceToUnitGroupDataSet xmlns:epd="http://www.iai.kit.edu/EPD/2013" refObjectId="93a60a57-a3c8-11da-a746-0800200c9a66" version="03.00.000" type="unit group data set" uri="../unitgroups/93a60a57-a3c8-11da-a746-0800200c9a66.xml">
          <common:shortDescription xml:lang="en">MJ</common:shortDescription>
          <common:shortDescription xml:lang="de">MJ</common:shortDescription>
        </epd:referenceToUnitGroupDataSet>
        <epd:amount xmlns:epd="http://www.iai.kit.edu/EPD/2013" epd:module="C1">0</epd:amount>
        <epd:amount xmlns:epd="http://www.iai.kit.edu/EPD/2013" epd:module="C2">0</epd:amount>
        <epd:amount xmlns:epd="http://www.iai.kit.edu/EPD/2013" epd:module="C3">0</epd:amount>
        <epd:amount xmlns:epd="http://www.iai.kit.edu/EPD/2013" epd:module="D">0</epd:amount>
      </common:other>
    </exchange>
    <exchange dataSetInternalID="101143">
      <referenceToFlowDataSet refObjectId="53f97275-fa8a-4cdd-9024-65936002acd0" version="39.00.000" type="flow data set" uri="../flows/53f97275-fa8a-4cdd-9024-65936002acd0.xml">
        <common:shortDescription xmlns:common="http://lca.jrc.it/ILCD/Common" xmlns:epd="http://www.iai.kit.edu/EPD/2013" xml:lang="en">Total use of renewable primary energy resources (PERT)</common:shortDescription>
        <common:shortDescription xmlns:common="http://lca.jrc.it/ILCD/Common" xmlns:epd="http://www.iai.kit.edu/EPD/2013" xml:lang="de">Total erneuerbare Primärenergie (PERT)</common:shortDescription>
      </referenceToFlowDataSet>
      <functionType>General reminder flow</functionType>
      <exchangeDirection>Input</exchangeDirection>
      <common:other xmlns:common="http://lca.jrc.it/ILCD/Common">
        <epd:amount xmlns:epd="http://www.iai.kit.edu/EPD/2013" epd:module="A1-A3">111.134910832947</epd:amount>
        <epd:referenceToUnitGroupDataSet xmlns:epd="http://www.iai.kit.edu/EPD/2013" refObjectId="93a60a57-a3c8-11da-a746-0800200c9a66" version="03.00.000" type="unit group data set" uri="../unitgroups/93a60a57-a3c8-11da-a746-0800200c9a66.xml">
          <common:shortDescription xml:lang="en">MJ</common:shortDescription>
          <common:shortDescription xml:lang="de">MJ</common:shortDescription>
        </epd:referenceToUnitGroupDataSet>
        <epd:amount xmlns:epd="http://www.iai.kit.edu/EPD/2013" epd:module="C1">0</epd:amount>
        <epd:amount xmlns:epd="http://www.iai.kit.edu/EPD/2013" epd:module="C2">0.0559328081883679</epd:amount>
        <epd:amount xmlns:epd="http://www.iai.kit.edu/EPD/2013" epd:module="C3">3.35621716827408</epd:amount>
        <epd:amount xmlns:epd="http://www.iai.kit.edu/EPD/2013" epd:module="D">-181.187238694297</epd:amount>
      </common:other>
    </exchange>
    <exchange dataSetInternalID="101144">
      <referenceToFlowDataSet refObjectId="ac857178-2b45-46ec-892a-a9a4332f0372" version="39.00.000" type="flow data set" uri="../flows/ac857178-2b45-46ec-892a-a9a4332f0372.xml">
        <common:shortDescription xmlns:common="http://lca.jrc.it/ILCD/Common" xmlns:epd="http://www.iai.kit.edu/EPD/2013" xml:lang="en">Use of non-renewable primary energy (PENRE)</common:shortDescription>
        <common:shortDescription xmlns:common="http://lca.jrc.it/ILCD/Common" xmlns:epd="http://www.iai.kit.edu/EPD/2013" xml:lang="de">Nicht-erneuerbare Primärenergie als Energieträger (PENRE)</common:shortDescription>
      </referenceToFlowDataSet>
      <functionType>General reminder flow</functionType>
      <exchangeDirection>Input</exchangeDirection>
      <common:other xmlns:common="http://lca.jrc.it/ILCD/Common">
        <epd:amount xmlns:epd="http://www.iai.kit.edu/EPD/2013" epd:module="A1-A3">1750.42110680765</epd:amount>
        <epd:referenceToUnitGroupDataSet xmlns:epd="http://www.iai.kit.edu/EPD/2013" refObjectId="93a60a57-a3c8-11da-a746-0800200c9a66" version="03.00.000" type="unit group data set" uri="../unitgroups/93a60a57-a3c8-11da-a746-0800200c9a66.xml">
          <common:shortDescription xml:lang="en">MJ</common:shortDescription>
          <common:shortDescription xml:lang="de">MJ</common:shortDescription>
        </epd:referenceToUnitGroupDataSet>
        <epd:amount xmlns:epd="http://www.iai.kit.edu/EPD/2013" epd:module="C1">0</epd:amount>
        <epd:amount xmlns:epd="http://www.iai.kit.edu/EPD/2013" epd:module="C2">0.960780423154212</epd:amount>
        <epd:amount xmlns:epd="http://www.iai.kit.edu/EPD/2013" epd:module="C3">1269.10466961705</epd:amount>
        <epd:amount xmlns:epd="http://www.iai.kit.edu/EPD/2013" epd:module="D">-633.97068627241</epd:amount>
      </common:other>
    </exchange>
    <exchange dataSetInternalID="101145">
      <referenceToFlowDataSet refObjectId="1421caa0-679d-4bf4-b282-0eb850ccae27" version="39.00.000" type="flow data set" uri="../flows/1421caa0-679d-4bf4-b282-0eb850ccae27.xml">
        <common:shortDescription xmlns:common="http://lca.jrc.it/ILCD/Common" xmlns:epd="http://www.iai.kit.edu/EPD/2013" xml:lang="en">Non-renewable primary energy resources used as raw materials (PENRM)</common:shortDescription>
        <common:shortDescription xmlns:common="http://lca.jrc.it/ILCD/Common" xmlns:epd="http://www.iai.kit.edu/EPD/2013" xml:lang="de">Nicht-erneuerbare Primärenergie zur stofflichen Nutzung (PENRM)</common:shortDescription>
      </referenceToFlowDataSet>
      <functionType>General reminder flow</functionType>
      <exchangeDirection>Input</exchangeDirection>
      <common:other xmlns:common="http://lca.jrc.it/ILCD/Common">
        <epd:amount xmlns:epd="http://www.iai.kit.edu/EPD/2013" epd:module="A1-A3">1253.56</epd:amount>
        <epd:referenceToUnitGroupDataSet xmlns:epd="http://www.iai.kit.edu/EPD/2013" refObjectId="93a60a57-a3c8-11da-a746-0800200c9a66" version="03.00.000" type="unit group data set" uri="../unitgroups/93a60a57-a3c8-11da-a746-0800200c9a66.xml">
          <common:shortDescription xml:lang="en">MJ</common:shortDescription>
          <common:shortDescription xml:lang="de">MJ</common:shortDescription>
        </epd:referenceToUnitGroupDataSet>
        <epd:amount xmlns:epd="http://www.iai.kit.edu/EPD/2013" epd:module="C1">0</epd:amount>
        <epd:amount xmlns:epd="http://www.iai.kit.edu/EPD/2013" epd:module="C2">0</epd:amount>
        <epd:amount xmlns:epd="http://www.iai.kit.edu/EPD/2013" epd:module="C3">-1253.56</epd:amount>
        <epd:amount xmlns:epd="http://www.iai.kit.edu/EPD/2013" epd:module="D">0</epd:amount>
      </common:other>
    </exchange>
    <exchange dataSetInternalID="101146">
      <referenceToFlowDataSet refObjectId="06159210-646b-4c8d-8583-da9b3b95a6c1" version="39.00.000" type="flow data set" uri="../flows/06159210-646b-4c8d-8583-da9b3b95a6c1.xml">
        <common:shortDescription xmlns:common="http://lca.jrc.it/ILCD/Common" xmlns:epd="http://www.iai.kit.edu/EPD/2013" xml:lang="en">Total use of non-renewable primary energy resources (PENRT)</common:shortDescription>
        <common:shortDescription xmlns:common="http://lca.jrc.it/ILCD/Common" xmlns:epd="http://www.iai.kit.edu/EPD/2013" xml:lang="de">Total nicht erneuerbare Primärenergie (PENRT)</common:shortDescription>
      </referenceToFlowDataSet>
      <functionType>General reminder flow</functionType>
      <exchangeDirection>Input</exchangeDirection>
      <common:other xmlns:common="http://lca.jrc.it/ILCD/Common">
        <epd:amount xmlns:epd="http://www.iai.kit.edu/EPD/2013" epd:module="A1-A3">3003.98110680765</epd:amount>
        <epd:referenceToUnitGroupDataSet xmlns:epd="http://www.iai.kit.edu/EPD/2013" refObjectId="93a60a57-a3c8-11da-a746-0800200c9a66" version="03.00.000" type="unit group data set" uri="../unitgroups/93a60a57-a3c8-11da-a746-0800200c9a66.xml">
          <common:shortDescription xml:lang="en">MJ</common:shortDescription>
          <common:shortDescription xml:lang="de">MJ</common:shortDescription>
        </epd:referenceToUnitGroupDataSet>
        <epd:amount xmlns:epd="http://www.iai.kit.edu/EPD/2013" epd:module="C1">0</epd:amount>
        <epd:amount xmlns:epd="http://www.iai.kit.edu/EPD/2013" epd:module="C2">0.960780423154212</epd:amount>
        <epd:amount xmlns:epd="http://www.iai.kit.edu/EPD/2013" epd:module="C3">15.5446696170509</epd:amount>
        <epd:amount xmlns:epd="http://www.iai.kit.edu/EPD/2013" epd:module="D">-633.97068627241</epd:amount>
      </common:other>
    </exchange>
    <exchange dataSetInternalID="101147">
      <referenceToFlowDataSet refObjectId="c6a1f35f-2d09-4f54-8dfb-97e502e1ce92" version="39.00.000" type="flow data set" uri="../flows/c6a1f35f-2d09-4f54-8dfb-97e502e1ce92.xml">
        <common:shortDescription xmlns:common="http://lca.jrc.it/ILCD/Common" xmlns:epd="http://www.iai.kit.edu/EPD/2013" xml:lang="en">Input of secondary material (SM)</common:shortDescription>
        <common:shortDescription xmlns:common="http://lca.jrc.it/ILCD/Common" xmlns:epd="http://www.iai.kit.edu/EPD/2013" xml:lang="de">Einsatz von Sekundärstoffen (SM)</common:shortDescription>
      </referenceToFlowDataSet>
      <functionType>General reminder flow</functionType>
      <exchangeDirection>Input</exchangeDirection>
      <common:other xmlns:common="http://lca.jrc.it/ILCD/Common">
        <epd:amount xmlns:epd="http://www.iai.kit.edu/EPD/2013" epd:module="A1-A3">0</epd:amount>
        <epd:referenceToUnitGroupDataSet xmlns:epd="http://www.iai.kit.edu/EPD/2013" refObjectId="93a60a57-a4c8-11da-a746-0800200c9a66" version="03.00.000" type="unit group data set" uri="../unitgroups/93a60a57-a4c8-11da-a746-0800200c9a66.xml">
          <common:shortDescription xml:lang="en">kg</common:shortDescription>
          <common:shortDescription xml:lang="de">kg</common:shortDescription>
        </epd:referenceToUnitGroupDataSet>
        <epd:amount xmlns:epd="http://www.iai.kit.edu/EPD/2013" epd:module="C1">0</epd:amount>
        <epd:amount xmlns:epd="http://www.iai.kit.edu/EPD/2013" epd:module="C2">0</epd:amount>
        <epd:amount xmlns:epd="http://www.iai.kit.edu/EPD/2013" epd:module="C3">0</epd:amount>
        <epd:amount xmlns:epd="http://www.iai.kit.edu/EPD/2013" epd:module="D">0</epd:amount>
      </common:other>
    </exchange>
    <exchange dataSetInternalID="101148">
      <referenceToFlowDataSet refObjectId="64333088-a55f-4aa2-9a31-c10b07816787" version="39.00.000" type="flow data set" uri="../flows/64333088-a55f-4aa2-9a31-c10b07816787.xml">
        <common:shortDescription xmlns:common="http://lca.jrc.it/ILCD/Common" xmlns:epd="http://www.iai.kit.edu/EPD/2013" xml:lang="en">Use of renewable secondary fuels (RSF)</common:shortDescription>
        <common:shortDescription xmlns:common="http://lca.jrc.it/ILCD/Common" xmlns:epd="http://www.iai.kit.edu/EPD/2013" xml:lang="de">Erneuerbare Sekundärbrennstoffe (RSF)</common:shortDescription>
      </referenceToFlowDataSet>
      <functionType>General reminder flow</functionType>
      <exchangeDirection>Input</exchangeDirection>
      <common:other xmlns:common="http://lca.jrc.it/ILCD/Common">
        <epd:amount xmlns:epd="http://www.iai.kit.edu/EPD/2013" epd:module="A1-A3">0</epd:amount>
        <epd:referenceToUnitGroupDataSet xmlns:epd="http://www.iai.kit.edu/EPD/2013" refObjectId="93a60a57-a3c8-11da-a746-0800200c9a66" version="03.00.000" type="unit group data set" uri="../unitgroups/93a60a57-a3c8-11da-a746-0800200c9a66.xml">
          <common:shortDescription xml:lang="en">MJ</common:shortDescription>
          <common:shortDescription xml:lang="de">MJ</common:shortDescription>
        </epd:referenceToUnitGroupDataSet>
        <epd:amount xmlns:epd="http://www.iai.kit.edu/EPD/2013" epd:module="C1">0</epd:amount>
        <epd:amount xmlns:epd="http://www.iai.kit.edu/EPD/2013" epd:module="C2">0</epd:amount>
        <epd:amount xmlns:epd="http://www.iai.kit.edu/EPD/2013" epd:module="C3">0</epd:amount>
        <epd:amount xmlns:epd="http://www.iai.kit.edu/EPD/2013" epd:module="D">0</epd:amount>
      </common:other>
    </exchange>
    <exchange dataSetInternalID="101149">
      <referenceToFlowDataSet refObjectId="89def144-d39a-4287-b86f-efde453ddcb2" version="39.00.000" type="flow data set" uri="../flows/89def144-d39a-4287-b86f-efde453ddcb2.xml">
        <common:shortDescription xmlns:common="http://lca.jrc.it/ILCD/Common" xmlns:epd="http://www.iai.kit.edu/EPD/2013" xml:lang="en">Use of non renewable secondary fuels (NRSF)</common:shortDescription>
        <common:shortDescription xmlns:common="http://lca.jrc.it/ILCD/Common" xmlns:epd="http://www.iai.kit.edu/EPD/2013" xml:lang="de">Nicht erneuerbare Sekundärbrennstoffe (NRSF)</common:shortDescription>
      </referenceToFlowDataSet>
      <functionType>General reminder flow</functionType>
      <exchangeDirection>Input</exchangeDirection>
      <common:other xmlns:common="http://lca.jrc.it/ILCD/Common">
        <epd:amount xmlns:epd="http://www.iai.kit.edu/EPD/2013" epd:module="A1-A3">0</epd:amount>
        <epd:referenceToUnitGroupDataSet xmlns:epd="http://www.iai.kit.edu/EPD/2013" refObjectId="93a60a57-a3c8-11da-a746-0800200c9a66" version="03.00.000" type="unit group data set" uri="../unitgroups/93a60a57-a3c8-11da-a746-0800200c9a66.xml">
          <common:shortDescription xml:lang="en">MJ</common:shortDescription>
          <common:shortDescription xml:lang="de">MJ</common:shortDescription>
        </epd:referenceToUnitGroupDataSet>
        <epd:amount xmlns:epd="http://www.iai.kit.edu/EPD/2013" epd:module="C1">0</epd:amount>
        <epd:amount xmlns:epd="http://www.iai.kit.edu/EPD/2013" epd:module="C2">0</epd:amount>
        <epd:amount xmlns:epd="http://www.iai.kit.edu/EPD/2013" epd:module="C3">0</epd:amount>
        <epd:amount xmlns:epd="http://www.iai.kit.edu/EPD/2013" epd:module="D">0</epd:amount>
      </common:other>
    </exchange>
    <exchange dataSetInternalID="101150">
      <referenceToFlowDataSet refObjectId="3cf952c8-f3a4-461d-8c96-96456ca62246" version="39.00.000" type="flow data set" uri="../flows/3cf952c8-f3a4-461d-8c96-96456ca62246.xml">
        <common:shortDescription xmlns:common="http://lca.jrc.it/ILCD/Common" xmlns:epd="http://www.iai.kit.edu/EPD/2013" xml:lang="en">Use of net fresh water (FW)</common:shortDescription>
        <common:shortDescription xmlns:common="http://lca.jrc.it/ILCD/Common" xmlns:epd="http://www.iai.kit.edu/EPD/2013" xml:lang="de">Einsatz von Süßwasserressourcen (FW)</common:shortDescription>
      </referenceToFlowDataSet>
      <functionType>General reminder flow</functionType>
      <exchangeDirection>Input</exchangeDirection>
      <common:other xmlns:common="http://lca.jrc.it/ILCD/Common">
        <epd:amount xmlns:epd="http://www.iai.kit.edu/EPD/2013" epd:module="A1-A3">0.4631552795242</epd:amount>
        <epd:referenceToUnitGroupDataSet xmlns:epd="http://www.iai.kit.edu/EPD/2013" refObjectId="93a60a57-a3c8-12da-a746-0800200c9a66" version="03.00.000" type="unit group data set" uri="../unitgroups/93a60a57-a3c8-12da-a746-0800200c9a66.xml">
          <common:shortDescription xml:lang="en">m3</common:shortDescription>
          <common:shortDescription xml:lang="de">m3</common:shortDescription>
        </epd:referenceToUnitGroupDataSet>
        <epd:amount xmlns:epd="http://www.iai.kit.edu/EPD/2013" epd:module="C1">0</epd:amount>
        <epd:amount xmlns:epd="http://www.iai.kit.edu/EPD/2013" epd:module="C2">5.0092523500794E-5</epd:amount>
        <epd:amount xmlns:epd="http://www.iai.kit.edu/EPD/2013" epd:module="C3">0.196990431279461</epd:amount>
        <epd:amount xmlns:epd="http://www.iai.kit.edu/EPD/2013" epd:module="D">-0.0845198935518813</epd:amount>
      </common:other>
    </exchange>
    <exchange dataSetInternalID="101151">
      <referenceToFlowDataSet refObjectId="430f9e0f-59b2-46a0-8e0d-55e0e84948fc" version="39.00.000" type="flow data set" uri="../flows/430f9e0f-59b2-46a0-8e0d-55e0e84948fc.xml">
        <common:shortDescription xmlns:common="http://lca.jrc.it/ILCD/Common" xmlns:epd="http://www.iai.kit.edu/EPD/2013" xml:lang="en">Hazardous waste disposed (HWD)</common:shortDescription>
        <common:shortDescription xmlns:common="http://lca.jrc.it/ILCD/Common" xmlns:epd="http://www.iai.kit.edu/EPD/2013" xml:lang="de">Gefährlicher Abfall zur Deponie (HWD)</common:shortDescription>
      </referenceToFlowDataSet>
      <functionType>General reminder flow</functionType>
      <exchangeDirection>Output</exchangeDirection>
      <common:other xmlns:common="http://lca.jrc.it/ILCD/Common">
        <epd:amount xmlns:epd="http://www.iai.kit.edu/EPD/2013" epd:module="A1-A3">1.61569299130839E-6</epd:amount>
        <epd:referenceToUnitGroupDataSet xmlns:epd="http://www.iai.kit.edu/EPD/2013" refObjectId="93a60a57-a4c8-11da-a746-0800200c9a66" version="03.00.000" type="unit group data set" uri="../unitgroups/93a60a57-a4c8-11da-a746-0800200c9a66.xml">
          <common:shortDescription xml:lang="en">kg</common:shortDescription>
          <common:shortDescription xml:lang="de">kg</common:shortDescription>
        </epd:referenceToUnitGroupDataSet>
        <epd:amount xmlns:epd="http://www.iai.kit.edu/EPD/2013" epd:module="C1">0</epd:amount>
        <epd:amount xmlns:epd="http://www.iai.kit.edu/EPD/2013" epd:module="C2">3.59033622956235E-8</epd:amount>
        <epd:amount xmlns:epd="http://www.iai.kit.edu/EPD/2013" epd:module="C3">1.50792643436502E-8</epd:amount>
        <epd:amount xmlns:epd="http://www.iai.kit.edu/EPD/2013" epd:module="D">-3.35138552797119E-7</epd:amount>
      </common:other>
    </exchange>
    <exchange dataSetInternalID="101152">
      <referenceToFlowDataSet refObjectId="b29ef66b-e286-4afa-949f-62f1a7b4d7fa" version="39.00.000" type="flow data set" uri="../flows/b29ef66b-e286-4afa-949f-62f1a7b4d7fa.xml">
        <common:shortDescription xmlns:common="http://lca.jrc.it/ILCD/Common" xmlns:epd="http://www.iai.kit.edu/EPD/2013" xml:lang="en">Non-hazardous waste disposed (NHWD)</common:shortDescription>
        <common:shortDescription xmlns:common="http://lca.jrc.it/ILCD/Common" xmlns:epd="http://www.iai.kit.edu/EPD/2013" xml:lang="de">Entsorgter nicht gefährlicher Abfall (NHWD)</common:shortDescription>
      </referenceToFlowDataSet>
      <functionType>General reminder flow</functionType>
      <exchangeDirection>Output</exchangeDirection>
      <common:other xmlns:common="http://lca.jrc.it/ILCD/Common">
        <epd:amount xmlns:epd="http://www.iai.kit.edu/EPD/2013" epd:module="A1-A3">7.29625763395209</epd:amount>
        <epd:referenceToUnitGroupDataSet xmlns:epd="http://www.iai.kit.edu/EPD/2013" refObjectId="93a60a57-a4c8-11da-a746-0800200c9a66" version="03.00.000" type="unit group data set" uri="../unitgroups/93a60a57-a4c8-11da-a746-0800200c9a66.xml">
          <common:shortDescription xml:lang="en">kg</common:shortDescription>
          <common:shortDescription xml:lang="de">kg</common:shortDescription>
        </epd:referenceToUnitGroupDataSet>
        <epd:amount xmlns:epd="http://www.iai.kit.edu/EPD/2013" epd:module="C1">0</epd:amount>
        <epd:amount xmlns:epd="http://www.iai.kit.edu/EPD/2013" epd:module="C2">0.000168633754673258</epd:amount>
        <epd:amount xmlns:epd="http://www.iai.kit.edu/EPD/2013" epd:module="C3">0.627934314464901</epd:amount>
        <epd:amount xmlns:epd="http://www.iai.kit.edu/EPD/2013" epd:module="D">-0.298238199675133</epd:amount>
      </common:other>
    </exchange>
    <exchange dataSetInternalID="101153">
      <referenceToFlowDataSet refObjectId="3449546e-52ad-4b39-b809-9fb77cea8ff6" version="39.00.000" type="flow data set" uri="../flows/3449546e-52ad-4b39-b809-9fb77cea8ff6.xml">
        <common:shortDescription xmlns:common="http://lca.jrc.it/ILCD/Common" xmlns:epd="http://www.iai.kit.edu/EPD/2013" xml:lang="en">Radioactive waste disposed (RWD)</common:shortDescription>
        <common:shortDescription xmlns:common="http://lca.jrc.it/ILCD/Common" xmlns:epd="http://www.iai.kit.edu/EPD/2013" xml:lang="de">Entsorgter radioaktiver Abfall (RWD)</common:shortDescription>
      </referenceToFlowDataSet>
      <functionType>General reminder flow</functionType>
      <exchangeDirection>Output</exchangeDirection>
      <common:other xmlns:common="http://lca.jrc.it/ILCD/Common">
        <epd:amount xmlns:epd="http://www.iai.kit.edu/EPD/2013" epd:module="A1-A3">0.0186601375721765</epd:amount>
        <epd:referenceToUnitGroupDataSet xmlns:epd="http://www.iai.kit.edu/EPD/2013" refObjectId="93a60a57-a4c8-11da-a746-0800200c9a66" version="03.00.000" type="unit group data set" uri="../unitgroups/93a60a57-a4c8-11da-a746-0800200c9a66.xml">
          <common:shortDescription xml:lang="en">kg</common:shortDescription>
          <common:shortDescription xml:lang="de">kg</common:shortDescription>
        </epd:referenceToUnitGroupDataSet>
        <epd:amount xmlns:epd="http://www.iai.kit.edu/EPD/2013" epd:module="C1">0</epd:amount>
        <epd:amount xmlns:epd="http://www.iai.kit.edu/EPD/2013" epd:module="C2">1.01150437888051E-6</epd:amount>
        <epd:amount xmlns:epd="http://www.iai.kit.edu/EPD/2013" epd:module="C3">0.000486239627700979</epd:amount>
        <epd:amount xmlns:epd="http://www.iai.kit.edu/EPD/2013" epd:module="D">-0.0218901821137732</epd:amount>
      </common:other>
    </exchange>
    <exchange dataSetInternalID="101154">
      <referenceToFlowDataSet refObjectId="a2b32f97-3fc7-4af2-b209-525bc6426f33" version="39.00.000" type="flow data set" uri="../flows/a2b32f97-3fc7-4af2-b209-525bc6426f33.xml">
        <common:shortDescription xmlns:common="http://lca.jrc.it/ILCD/Common" xmlns:epd="http://www.iai.kit.edu/EPD/2013" xml:lang="en">Components for re-use (CRU)</common:shortDescription>
        <common:shortDescription xmlns:common="http://lca.jrc.it/ILCD/Common" xmlns:epd="http://www.iai.kit.edu/EPD/2013" xml:lang="de">Komponenten für die Wiederverwendung (CRU)</common:shortDescription>
      </referenceToFlowDataSet>
      <functionType>General reminder flow</functionType>
      <exchangeDirection>Output</exchangeDirection>
      <common:other xmlns:common="http://lca.jrc.it/ILCD/Common">
        <epd:amount xmlns:epd="http://www.iai.kit.edu/EPD/2013" epd:module="A1-A3">0</epd:amount>
        <epd:referenceToUnitGroupDataSet xmlns:epd="http://www.iai.kit.edu/EPD/2013" refObjectId="93a60a57-a4c8-11da-a746-0800200c9a66" version="03.00.000" type="unit group data set" uri="../unitgroups/93a60a57-a4c8-11da-a746-0800200c9a66.xml">
          <common:shortDescription xml:lang="en">kg</common:shortDescription>
          <common:shortDescription xml:lang="de">kg</common:shortDescription>
        </epd:referenceToUnitGroupDataSet>
        <epd:amount xmlns:epd="http://www.iai.kit.edu/EPD/2013" epd:module="C1">0</epd:amount>
        <epd:amount xmlns:epd="http://www.iai.kit.edu/EPD/2013" epd:module="C2">0</epd:amount>
        <epd:amount xmlns:epd="http://www.iai.kit.edu/EPD/2013" epd:module="C3">0</epd:amount>
        <epd:amount xmlns:epd="http://www.iai.kit.edu/EPD/2013" epd:module="D">0</epd:amount>
      </common:other>
    </exchange>
    <exchange dataSetInternalID="101155">
      <referenceToFlowDataSet refObjectId="d7fe48a5-4103-49c8-9aae-b0b5dfdbd6ae" version="39.00.000" type="flow data set" uri="../flows/d7fe48a5-4103-49c8-9aae-b0b5dfdbd6ae.xml">
        <common:shortDescription xmlns:common="http://lca.jrc.it/ILCD/Common" xmlns:epd="http://www.iai.kit.edu/EPD/2013" xml:lang="en">Materials for Recycling (MFR)</common:shortDescription>
        <common:shortDescription xmlns:common="http://lca.jrc.it/ILCD/Common" xmlns:epd="http://www.iai.kit.edu/EPD/2013" xml:lang="de">Stoffe zum Recycling (MFR)</common:shortDescription>
      </referenceToFlowDataSet>
      <functionType>General reminder flow</functionType>
      <exchangeDirection>Output</exchangeDirection>
      <common:other xmlns:common="http://lca.jrc.it/ILCD/Common">
        <epd:amount xmlns:epd="http://www.iai.kit.edu/EPD/2013" epd:module="A1-A3">0</epd:amount>
        <epd:referenceToUnitGroupDataSet xmlns:epd="http://www.iai.kit.edu/EPD/2013" refObjectId="93a60a57-a4c8-11da-a746-0800200c9a66" version="03.00.000" type="unit group data set" uri="../unitgroups/93a60a57-a4c8-11da-a746-0800200c9a66.xml">
          <common:shortDescription xml:lang="en">kg</common:shortDescription>
          <common:shortDescription xml:lang="de">kg</common:shortDescription>
        </epd:referenceToUnitGroupDataSet>
        <epd:amount xmlns:epd="http://www.iai.kit.edu/EPD/2013" epd:module="C1">0</epd:amount>
        <epd:amount xmlns:epd="http://www.iai.kit.edu/EPD/2013" epd:module="C2">0</epd:amount>
        <epd:amount xmlns:epd="http://www.iai.kit.edu/EPD/2013" epd:module="C3">0</epd:amount>
        <epd:amount xmlns:epd="http://www.iai.kit.edu/EPD/2013" epd:module="D">0</epd:amount>
      </common:other>
    </exchange>
    <exchange dataSetInternalID="101156">
      <referenceToFlowDataSet refObjectId="59a9181c-3aaf-46ee-8b13-2b3723b6e447" version="39.00.000" type="flow data set" uri="../flows/59a9181c-3aaf-46ee-8b13-2b3723b6e447.xml">
        <common:shortDescription xmlns:common="http://lca.jrc.it/ILCD/Common" xmlns:epd="http://www.iai.kit.edu/EPD/2013" xml:lang="en">Material for Energy Recovery (MER)</common:shortDescription>
        <common:shortDescription xmlns:common="http://lca.jrc.it/ILCD/Common" xmlns:epd="http://www.iai.kit.edu/EPD/2013" xml:lang="de">Stoffe für die Energierückgewinnung (MER)</common:shortDescription>
      </referenceToFlowDataSet>
      <functionType>General reminder flow</functionType>
      <exchangeDirection>Output</exchangeDirection>
      <common:other xmlns:common="http://lca.jrc.it/ILCD/Common">
        <epd:amount xmlns:epd="http://www.iai.kit.edu/EPD/2013" epd:module="A1-A3">0</epd:amount>
        <epd:referenceToUnitGroupDataSet xmlns:epd="http://www.iai.kit.edu/EPD/2013" refObjectId="93a60a57-a4c8-11da-a746-0800200c9a66" version="03.00.000" type="unit group data set" uri="../unitgroups/93a60a57-a4c8-11da-a746-0800200c9a66.xml">
          <common:shortDescription xml:lang="en">kg</common:shortDescription>
          <common:shortDescription xml:lang="de">kg</common:shortDescription>
        </epd:referenceToUnitGroupDataSet>
        <epd:amount xmlns:epd="http://www.iai.kit.edu/EPD/2013" epd:module="C1">30.8</epd:amount>
        <epd:amount xmlns:epd="http://www.iai.kit.edu/EPD/2013" epd:module="C2">0</epd:amount>
        <epd:amount xmlns:epd="http://www.iai.kit.edu/EPD/2013" epd:module="C3">0</epd:amount>
        <epd:amount xmlns:epd="http://www.iai.kit.edu/EPD/2013" epd:module="D">0</epd:amount>
      </common:other>
    </exchange>
    <exchange dataSetInternalID="101157">
      <referenceToFlowDataSet refObjectId="4da0c987-2b76-40d6-9e9e-82a017aaaf29" version="39.00.000" type="flow data set" uri="../flows/4da0c987-2b76-40d6-9e9e-82a017aaaf29.xml">
        <common:shortDescription xmlns:common="http://lca.jrc.it/ILCD/Common" xmlns:epd="http://www.iai.kit.edu/EPD/2013" xml:lang="en">Exported electrical energy (EEE)</common:shortDescription>
        <common:shortDescription xmlns:common="http://lca.jrc.it/ILCD/Common" xmlns:epd="http://www.iai.kit.edu/EPD/2013" xml:lang="de">Exportierte elektrische Energie (EEE)</common:shortDescription>
      </referenceToFlowDataSet>
      <functionType>General reminder flow</functionType>
      <exchangeDirection>Output</exchangeDirection>
      <common:other xmlns:common="http://lca.jrc.it/ILCD/Common">
        <epd:amount xmlns:epd="http://www.iai.kit.edu/EPD/2013" epd:module="A1-A3">0</epd:amount>
        <epd:referenceToUnitGroupDataSet xmlns:epd="http://www.iai.kit.edu/EPD/2013" refObjectId="93a60a57-a3c8-11da-a746-0800200c9a66" version="03.00.000" type="unit group data set" uri="../unitgroups/93a60a57-a3c8-11da-a746-0800200c9a66.xml">
          <common:shortDescription xml:lang="en">MJ</common:shortDescription>
          <common:shortDescription xml:lang="de">MJ</common:shortDescription>
        </epd:referenceToUnitGroupDataSet>
        <epd:amount xmlns:epd="http://www.iai.kit.edu/EPD/2013" epd:module="C1">0</epd:amount>
        <epd:amount xmlns:epd="http://www.iai.kit.edu/EPD/2013" epd:module="C2">0</epd:amount>
        <epd:amount xmlns:epd="http://www.iai.kit.edu/EPD/2013" epd:module="C3">159.261703112585</epd:amount>
        <epd:amount xmlns:epd="http://www.iai.kit.edu/EPD/2013" epd:module="D">0</epd:amount>
      </common:other>
    </exchange>
    <exchange dataSetInternalID="101158">
      <referenceToFlowDataSet refObjectId="98daf38a-7a79-46d3-9a37-2b7bd0955810" version="39.00.000" type="flow data set" uri="../flows/98daf38a-7a79-46d3-9a37-2b7bd0955810.xml">
        <common:shortDescription xmlns:common="http://lca.jrc.it/ILCD/Common" xmlns:epd="http://www.iai.kit.edu/EPD/2013" xml:lang="en">Exported thermal energy (EET)</common:shortDescription>
        <common:shortDescription xmlns:common="http://lca.jrc.it/ILCD/Common" xmlns:epd="http://www.iai.kit.edu/EPD/2013" xml:lang="de">Exportierte thermische Energie (EET)</common:shortDescription>
      </referenceToFlowDataSet>
      <functionType>General reminder flow</functionType>
      <exchangeDirection>Output</exchangeDirection>
      <common:other xmlns:common="http://lca.jrc.it/ILCD/Common">
        <epd:amount xmlns:epd="http://www.iai.kit.edu/EPD/2013" epd:module="A1-A3">0</epd:amount>
        <epd:referenceToUnitGroupDataSet xmlns:epd="http://www.iai.kit.edu/EPD/2013" refObjectId="93a60a57-a3c8-11da-a746-0800200c9a66" version="03.00.000" type="unit group data set" uri="../unitgroups/93a60a57-a3c8-11da-a746-0800200c9a66.xml">
          <common:shortDescription xml:lang="en">MJ</common:shortDescription>
          <common:shortDescription xml:lang="de">MJ</common:shortDescription>
        </epd:referenceToUnitGroupDataSet>
        <epd:amount xmlns:epd="http://www.iai.kit.edu/EPD/2013" epd:module="C1">0</epd:amount>
        <epd:amount xmlns:epd="http://www.iai.kit.edu/EPD/2013" epd:module="C2">0</epd:amount>
        <epd:amount xmlns:epd="http://www.iai.kit.edu/EPD/2013" epd:module="C3">367.241835962426</epd:amount>
        <epd:amount xmlns:epd="http://www.iai.kit.edu/EPD/2013" epd:module="D">0</epd:amount>
      </common:other>
    </exchange>
  </exchanges>
  <LCIAResults>
    <LCIAResult>
      <referenceToLCIAMethodDataSet refObjectId="77e416eb-a363-4258-a04e-171d843a6460" version="39.00.000" type="LCIA method data set" uri="../lciamethods/77e416eb-a363-4258-a04e-171d843a6460.xml">
        <common:shortDescription xmlns:common="http://lca.jrc.it/ILCD/Common" xmlns:epd="http://www.iai.kit.edu/EPD/2013" xml:lang="en">Global warming potential (GWP)</common:shortDescription>
        <common:shortDescription xmlns:common="http://lca.jrc.it/ILCD/Common" xmlns:epd="http://www.iai.kit.edu/EPD/2013" xml:lang="de">Globales Erwärmungspotenzial (GWP)</common:shortDescription>
      </referenceToLCIAMethodDataSet>
      <common:other xmlns:common="http://lca.jrc.it/ILCD/Common">
        <epd:amount xmlns:epd="http://www.iai.kit.edu/EPD/2013" epd:module="A1-A3">160.082599300968</epd:amount>
        <epd:amount xmlns:epd="http://www.iai.kit.edu/EPD/2013" epd:module="C1">0</epd:amount>
        <epd:amount xmlns:epd="http://www.iai.kit.edu/EPD/2013" epd:module="C2">0.0714832573692925</epd:amount>
        <epd:amount xmlns:epd="http://www.iai.kit.edu/EPD/2013" epd:module="C3">103.432381620612</epd:amount>
        <epd:amount xmlns:epd="http://www.iai.kit.edu/EPD/2013" epd:module="D">-43.3216698220366</epd:amount>
        <epd:referenceToUnitGroupDataSet xmlns:epd="http://www.iai.kit.edu/EPD/2013" refObjectId="1ebf3012-d0db-4de2-aefd-ef30cedb0be1" version="39.00.000" type="unit group data set" uri="../unitgroups/1ebf3012-d0db-4de2-aefd-ef30cedb0be1.xml">
          <common:shortDescription xml:lang="en">kg CO2 eq.</common:shortDescription>
          <common:shortDescription xml:lang="de">kg CO2 Äquiv.</common:shortDescription>
        </epd:referenceToUnitGroupDataSet>
      </common:other>
    </LCIAResult>
    <LCIAResult>
      <referenceToLCIAMethodDataSet refObjectId="06dcd26f-025f-401a-a7c1-5e457eb54637" version="39.00.000" type="LCIA method data set" uri="../lciamethods/06dcd26f-025f-401a-a7c1-5e457eb54637.xml">
        <common:shortDescription xmlns:common="http://lca.jrc.it/ILCD/Common" xmlns:epd="http://www.iai.kit.edu/EPD/2013" xml:lang="en">Ozone Depletion Potential (ODP)</common:shortDescription>
        <common:shortDescription xmlns:common="http://lca.jrc.it/ILCD/Common" xmlns:epd="http://www.iai.kit.edu/EPD/2013" xml:lang="de">Abbaupotenzial der stratosphärischen Ozonschicht (ODP)</common:shortDescription>
      </referenceToLCIAMethodDataSet>
      <common:other xmlns:common="http://lca.jrc.it/ILCD/Common">
        <epd:amount xmlns:epd="http://www.iai.kit.edu/EPD/2013" epd:module="A1-A3">5.83396145444922E-13</epd:amount>
        <epd:amount xmlns:epd="http://www.iai.kit.edu/EPD/2013" epd:module="C1">0</epd:amount>
        <epd:amount xmlns:epd="http://www.iai.kit.edu/EPD/2013" epd:module="C2">2.36612406132284E-17</epd:amount>
        <epd:amount xmlns:epd="http://www.iai.kit.edu/EPD/2013" epd:module="C3">1.89925677989868E-14</epd:amount>
        <epd:amount xmlns:epd="http://www.iai.kit.edu/EPD/2013" epd:module="D">-1.00187965932754E-12</epd:amount>
        <epd:referenceToUnitGroupDataSet xmlns:epd="http://www.iai.kit.edu/EPD/2013" refObjectId="88054749-b0a6-47ea-a82b-dc5b29326512" version="39.00.000" type="unit group data set" uri="../unitgroups/88054749-b0a6-47ea-a82b-dc5b29326512.xml">
          <common:shortDescription xml:lang="en">kg R11 eq.</common:shortDescription>
          <common:shortDescription xml:lang="de">kg R11 Äquiv.</common:shortDescription>
        </epd:referenceToUnitGroupDataSet>
      </common:other>
    </LCIAResult>
    <LCIAResult>
      <referenceToLCIAMethodDataSet refObjectId="b4274add-93b7-4905-a5e4-2e878c4e4216" version="39.00.000" type="LCIA method data set" uri="../lciamethods/b4274add-93b7-4905-a5e4-2e878c4e4216.xml">
        <common:shortDescription xmlns:common="http://lca.jrc.it/ILCD/Common" xmlns:epd="http://www.iai.kit.edu/EPD/2013" xml:lang="en">Acidification potential (AP)</common:shortDescription>
        <common:shortDescription xmlns:common="http://lca.jrc.it/ILCD/Common" xmlns:epd="http://www.iai.kit.edu/EPD/2013" xml:lang="de">Versauerungspotential (AP)</common:shortDescription>
      </referenceToLCIAMethodDataSet>
      <common:other xmlns:common="http://lca.jrc.it/ILCD/Common">
        <epd:amount xmlns:epd="http://www.iai.kit.edu/EPD/2013" epd:module="A1-A3">0.165966953174548</epd:amount>
        <epd:amount xmlns:epd="http://www.iai.kit.edu/EPD/2013" epd:module="C1">0</epd:amount>
        <epd:amount xmlns:epd="http://www.iai.kit.edu/EPD/2013" epd:module="C2">0.000144388475424029</epd:amount>
        <epd:amount xmlns:epd="http://www.iai.kit.edu/EPD/2013" epd:module="C3">0.00821342434171675</epd:amount>
        <epd:amount xmlns:epd="http://www.iai.kit.edu/EPD/2013" epd:module="D">-0.0365646734129771</epd:amount>
        <epd:referenceToUnitGroupDataSet xmlns:epd="http://www.iai.kit.edu/EPD/2013" refObjectId="bc50c624-a9bc-45b1-a9b0-e6b10d00476f" version="39.00.000" type="unit group data set" uri="../unitgroups/bc50c624-a9bc-45b1-a9b0-e6b10d00476f.xml">
          <common:shortDescription xml:lang="en">kg SO2 eq.</common:shortDescription>
          <common:shortDescription xml:lang="de">kg SO2 Äquiv.</common:shortDescription>
        </epd:referenceToUnitGroupDataSet>
      </common:other>
    </LCIAResult>
    <LCIAResult>
      <referenceToLCIAMethodDataSet refObjectId="f58827d0-b407-4ec6-be75-8b69efb98a0f" version="39.00.000" type="LCIA method data set" uri="../lciamethods/f58827d0-b407-4ec6-be75-8b69efb98a0f.xml">
        <common:shortDescription xmlns:common="http://lca.jrc.it/ILCD/Common" xmlns:epd="http://www.iai.kit.edu/EPD/2013" xml:lang="en">Eutrophication potential (EP)</common:shortDescription>
        <common:shortDescription xmlns:common="http://lca.jrc.it/ILCD/Common" xmlns:epd="http://www.iai.kit.edu/EPD/2013" xml:lang="de">Eutrophierungspotential (EP)</common:shortDescription>
      </referenceToLCIAMethodDataSet>
      <common:other xmlns:common="http://lca.jrc.it/ILCD/Common">
        <epd:amount xmlns:epd="http://www.iai.kit.edu/EPD/2013" epd:module="A1-A3">0.022538416863773</epd:amount>
        <epd:amount xmlns:epd="http://www.iai.kit.edu/EPD/2013" epd:module="C1">0</epd:amount>
        <epd:amount xmlns:epd="http://www.iai.kit.edu/EPD/2013" epd:module="C2">3.43251324685386E-5</epd:amount>
        <epd:amount xmlns:epd="http://www.iai.kit.edu/EPD/2013" epd:module="C3">0.00185421065000863</epd:amount>
        <epd:amount xmlns:epd="http://www.iai.kit.edu/EPD/2013" epd:module="D">-0.00692879637429199</epd:amount>
        <epd:referenceToUnitGroupDataSet xmlns:epd="http://www.iai.kit.edu/EPD/2013" refObjectId="67b5401d-873c-485f-bcf3-6ae83b918822" version="39.00.000" type="unit group data set" uri="../unitgroups/67b5401d-873c-485f-bcf3-6ae83b918822.xml">
          <common:shortDescription xml:lang="en">kg Phosphate eq.</common:shortDescription>
          <common:shortDescription xml:lang="de">kg Phosphat Äquiv.</common:shortDescription>
        </epd:referenceToUnitGroupDataSet>
      </common:other>
    </LCIAResult>
    <LCIAResult>
      <referenceToLCIAMethodDataSet refObjectId="1e84a202-dae6-42aa-9e9d-71ea48b8be00" version="39.00.000" type="LCIA method data set" uri="../lciamethods/1e84a202-dae6-42aa-9e9d-71ea48b8be00.xml">
        <common:shortDescription xmlns:common="http://lca.jrc.it/ILCD/Common" xmlns:epd="http://www.iai.kit.edu/EPD/2013" xml:lang="en">Photochemical Ozone Creation Potential (POCP)</common:shortDescription>
        <common:shortDescription xmlns:common="http://lca.jrc.it/ILCD/Common" xmlns:epd="http://www.iai.kit.edu/EPD/2013" xml:lang="de">Bildungspotenzial für troposphärisches Ozon (POCP)</common:shortDescription>
      </referenceToLCIAMethodDataSet>
      <common:other xmlns:common="http://lca.jrc.it/ILCD/Common">
        <epd:amount xmlns:epd="http://www.iai.kit.edu/EPD/2013" epd:module="A1-A3">0.492607816958189</epd:amount>
        <epd:amount xmlns:epd="http://www.iai.kit.edu/EPD/2013" epd:module="C1">0</epd:amount>
        <epd:amount xmlns:epd="http://www.iai.kit.edu/EPD/2013" epd:module="C2">-4.71913289329807E-5</epd:amount>
        <epd:amount xmlns:epd="http://www.iai.kit.edu/EPD/2013" epd:module="C3">0.000607381420736732</epd:amount>
        <epd:amount xmlns:epd="http://www.iai.kit.edu/EPD/2013" epd:module="D">-0.00372504916744812</epd:amount>
        <epd:referenceToUnitGroupDataSet xmlns:epd="http://www.iai.kit.edu/EPD/2013" refObjectId="01c26c17-9a76-406e-8295-f17b55fd909e" version="39.00.000" type="unit group data set" uri="../unitgroups/01c26c17-9a76-406e-8295-f17b55fd909e.xml">
          <common:shortDescription xml:lang="en">kg Ethene eq.</common:shortDescription>
          <common:shortDescription xml:lang="de">kg Ethen Äquiv.</common:shortDescription>
        </epd:referenceToUnitGroupDataSet>
      </common:other>
    </LCIAResult>
    <LCIAResult>
      <referenceToLCIAMethodDataSet refObjectId="f7c73bb9-ab1a-4249-9c6d-379a0de6f67e" version="39.00.000" type="LCIA method data set" uri="../lciamethods/f7c73bb9-ab1a-4249-9c6d-379a0de6f67e.xml">
        <common:shortDescription xmlns:common="http://lca.jrc.it/ILCD/Common" xmlns:epd="http://www.iai.kit.edu/EPD/2013" xml:lang="en">Abiotic depletion potential for non fossil resources (ADPE)</common:shortDescription>
        <common:shortDescription xmlns:common="http://lca.jrc.it/ILCD/Common" xmlns:epd="http://www.iai.kit.edu/EPD/2013" xml:lang="de">Potenzial für den abiotischen Abbau nicht fossiler Ressourcen (ADPE)</common:shortDescription>
      </referenceToLCIAMethodDataSet>
      <common:other xmlns:common="http://lca.jrc.it/ILCD/Common">
        <epd:amount xmlns:epd="http://www.iai.kit.edu/EPD/2013" epd:module="A1-A3">1.22928245273535E-5</epd:amount>
        <epd:amount xmlns:epd="http://www.iai.kit.edu/EPD/2013" epd:module="C1">0</epd:amount>
        <epd:amount xmlns:epd="http://www.iai.kit.edu/EPD/2013" epd:module="C2">6.01537621389297E-9</epd:amount>
        <epd:amount xmlns:epd="http://www.iai.kit.edu/EPD/2013" epd:module="C3">2.02808914572278E-7</epd:amount>
        <epd:amount xmlns:epd="http://www.iai.kit.edu/EPD/2013" epd:module="D">-1.07576835421628E-5</epd:amount>
        <epd:referenceToUnitGroupDataSet xmlns:epd="http://www.iai.kit.edu/EPD/2013" refObjectId="54ccd2d9-a32a-4fc2-923d-f2c8c93e89d4" version="39.00.000" type="unit group data set" uri="../unitgroups/54ccd2d9-a32a-4fc2-923d-f2c8c93e89d4.xml">
          <common:shortDescription xml:lang="en">kg Sb eq.</common:shortDescription>
          <common:shortDescription xml:lang="de">kg Sb Äquiv.</common:shortDescription>
        </epd:referenceToUnitGroupDataSet>
      </common:other>
    </LCIAResult>
    <LCIAResult>
      <referenceToLCIAMethodDataSet refObjectId="804ebcdf-309d-4098-8ed8-fdaf2f389981" version="39.00.000" type="LCIA method data set" uri="../lciamethods/804ebcdf-309d-4098-8ed8-fdaf2f389981.xml">
        <common:shortDescription xmlns:common="http://lca.jrc.it/ILCD/Common" xmlns:epd="http://www.iai.kit.edu/EPD/2013" xml:lang="en">Abiotic depletion potential for fossil resources (ADPF)</common:shortDescription>
        <common:shortDescription xmlns:common="http://lca.jrc.it/ILCD/Common" xmlns:epd="http://www.iai.kit.edu/EPD/2013" xml:lang="de">Potenzial für den abiotischen Abbau fossiler Brennstoffe (ADPF)</common:shortDescription>
      </referenceToLCIAMethodDataSet>
      <common:other xmlns:common="http://lca.jrc.it/ILCD/Common">
        <epd:amount xmlns:epd="http://www.iai.kit.edu/EPD/2013" epd:module="A1-A3">2956.88803911614</epd:amount>
        <epd:amount xmlns:epd="http://www.iai.kit.edu/EPD/2013" epd:module="C1">0</epd:amount>
        <epd:amount xmlns:epd="http://www.iai.kit.edu/EPD/2013" epd:module="C2">0.958195258587056</epd:amount>
        <epd:amount xmlns:epd="http://www.iai.kit.edu/EPD/2013" epd:module="C3">14.3172894480688</epd:amount>
        <epd:amount xmlns:epd="http://www.iai.kit.edu/EPD/2013" epd:module="D">-578.709113588759</epd:amount>
        <epd:referenceToUnitGroupDataSet xmlns:epd="http://www.iai.kit.edu/EPD/2013" refObjectId="93a60a57-a3c8-11da-a746-0800200c9a66" version="03.00.000" type="unit group data set" uri="../unitgroups/93a60a57-a3c8-11da-a746-0800200c9a66.xml">
          <common:shortDescription xml:lang="en">MJ</common:shortDescription>
          <common:shortDescription xml:lang="de">MJ</common:shortDescription>
        </epd:referenceToUnitGroupDataSet>
      </common:other>
    </LCIAResult>
  </LCIAResults>
</processDataSet>