<?xml version="1.0" encoding="utf-8"?>
<processDataSet xmlns:epd="http://www.iai.kit.edu/EPD/2013" xmlns:epd2="http://www.indata.network/EPD/2019" xmlns:common="http://lca.jrc.it/ILCD/Common" xsi:schemaLocation="http://lca.jrc.it/ILCD/Process ../../schemas/EPD_DataSet.xsd" epd2:epd-version="1.2" version="1.1" locations="../ILCDLocations.xml" xmlns:xsi="http://www.w3.org/2001/XMLSchema-instance" xmlns="http://lca.jrc.it/ILCD/Process">
<processInformation>
<dataSetInformation>
<common:UUID>81635c6b-192e-4661-9f82-f63f335c4047</common:UUID>
<name>
<baseName xml:lang="de">GUTEX Thermofibre</baseName>
<baseName xml:lang="en">GUTEX Thermofibre</baseName>
<functionalUnitFlowProperties xml:lang="de" />
</name>
<classificationInformation>
<common:classification name="OEKOBAU.DAT">
<common:class level="0" classId="2">Dämmstoffe</common:class>
<common:class level="1" classId="2.10">Holzfasern</common:class>
<common:class level="2" classId="2.10.01">Holzfaserdämmplatte</common:class>
</common:classification>
<common:classification name="IBUCategories">
<common:class level="0">01 Grundstoffe und Vorprodukte</common:class>
<common:class level="1">Produkte für Beton, Mörtel und Einpressmörtel</common:class>
<common:class level="2">Betonzusatzmittel</common:class>
</common:classification>
</classificationInformation>
<common:generalComment xml:lang="de">GUTEX Thermofibre sind lose Holzfasern, die nach /ETA-12/0181/ getrocknet in vorkomprimierten Gebinden bereitgestellt werden.Die Holzfasern werden aus Nadelholz-Hackschnitzeln durch mechanische Zerkleinerung hergestellt.Die Einblasrohdichte vom Anwendungsbereich ab und beträgt im Mittel ca. 35 kg/m³.</common:generalComment>
<common:generalComment xml:lang="en">GUTEX Thermofibre are loose wood fibres which are dried and made available in pre-compressed units according to /ETA-12/0181/. The wood fibres are manufactured from mechanically-crushed coniferous wood chips. The blow-in gross density depends on the area of application and is on average approx. 35 kg/m³.</common:generalComment>
</dataSetInformation>
<quantitativeReference>
<referenceToReferenceFlow>0</referenceToReferenceFlow>
</quantitativeReference>
<time>
<common:referenceYear>2019</common:referenceYear>
<common:dataSetValidUntil>2024</common:dataSetValidUntil>
<common:other>
<epd2:publicationDateOfEPD>2019-04-18</epd2:publicationDateOfEPD>
</common:other>
</time>
<geography>
<locationOfOperationSupplyOrProduction location="RER" />
</geography>
<technology>
<technologyDescriptionAndIncludedProcesses xml:lang="de">Ausgangsbasis für die Produktherstellung sind angelieferte Hackschnitzel von regionalen Sägewerken, die unter Feuchte- und Wärmeeinfluss zu Holzfasern aufgeschlossen werden. Anschließend werden die Fasern getrocknet und in einem Abfüllprozess zu gleichbleibend großen und schweren Gebinden verpackt. Der Produktionsstandort arbeitet auf Basis eines zertifizierten Qualitätsmanagements (/ISO 9001/). 
Technische Daten: 
Leistungswerte des Produkts entsprechend der Leistungserklärung (GX-01-0029-02) in Bezug auf dessen wesentliche Merkmale gemäß /ETA-12/0181/ vom 21.06.2017. 
Deklarierte Einheit: 
Die deklarierte Einheit der ökologischen Betrachtung ist die Bereitstellung von 1 kg GUTEX Thermofibre.  Hinweis: für die Bilanzierung auf Gebäudeebene sind je nach Anwendungsfall unterschiedliche Dichten anzunehmen (siehe Kapitel 2.3).</technologyDescriptionAndIncludedProcesses>
<technologyDescriptionAndIncludedProcesses xml:lang="en">Product manufacturing is based on wood chips supplied by regional sawmills which are broken down into wood fibres when exposed to moisture and heat. Then the fibres are dried and packed as units of the same size and weight in a filling process. The production site works on the basis of certified quality management (/ISO 9001/). 
Technical data: 
The product’s performance values correspond with the Declaration of Performance (GX-01-0029-02) in terms of its essential properties in accordance with /ETA-12/0181/ dated 21.06.2017. 
Declared unit: 
The declared unit of this ecological analysis is the provision of 1 kg GUTEX Thermofibre. Note: Depending on the respective application, various densities can be assumed for analysis at building level (see section 2.3).</technologyDescriptionAndIncludedProcesses>
<technologicalApplicability xml:lang="de">Der Wärmedämmstoff dient zur Herstellung von nicht druckbelastbaren Dämmschichten durch maschinelle Verarbeitung an der Anwendungsstelle.Folgende Anwendungsbereiche sind möglich:- Raumausfüllende Dämmung in geschlossenen Hohlräumen von Außen- und Innenwänden- Dämmung in geschlossenen Hohlräumen zwischen Sparren und Holzbalken - Freiliegende Dämmung auf horizontalen oder mäßig geneigten Flächen- Dämmung nicht begehbarer, jedoch zugänglicher oberster Geschossdecken- Hohlraumdämmung zwischen Lagerhölzern im Fußbodenbereich und vergleichbaren Unterkonstruktionen</technologicalApplicability>
<technologicalApplicability xml:lang="en">This thermal insulation serves towards manufacturing thermal layers which are not resistant to compression by mechanically processing them at the place of application. The following areas of application are possible: - Expansive insulation in closed cavities in exterior and interior walls - Insulation in closed cavities between rafters and wood beams - Exposed insulation in horizontal or slightly inclined areas - Insulation of top storey ceilings which are accessible but cannot be walked on - Cavity insulation between sleepers in the floor area and comparable supporting constructions</technologicalApplicability>
</technology>
</processInformation>
<modellingAndValidation>
<LCIMethodAndAllocation>
<typeOfDataSet>EPD</typeOfDataSet>
<referenceToLCAMethodDetails type="source data set" refObjectId="b843bfc3-e165-4031-a99e-b51371d5260b">
<common:shortDescription xml:lang="de">Betonzusatzmittel.pdf</common:shortDescription>
</referenceToLCAMethodDetails>
<common:other>
<epd:subType xmlns="http://www.iai.kit.edu/EPD/2013">specific dataset</epd:subType>
</common:other>
</LCIMethodAndAllocation>
<dataSourcesTreatmentAndRepresentativeness>
<referenceToDataSource type="source data set" refObjectId="28d74cc0-db8b-4d7e-bc44-5f6d56ce0c4a">
<common:shortDescription xml:lang="de">GaBi Database (all versions)</common:shortDescription>
</referenceToDataSource>
<referenceToDataSource type="source data set" refObjectId="d8181616-4417-4dbd-9614-09937353f17a">
<common:shortDescription xml:lang="de">GaBi database SP33 2017</common:shortDescription>
</referenceToDataSource>
<useAdviceForDataSet xml:lang="de">Gültigkeitsbereich: 
Diese Umwelt-Produktdeklaration gilt für die im Werk Gutenburg (s. Herstelleradresse) produzierte lose Holzfaserdämmung GUTEX Thermofibre. 
Systemgrenze: 
Der Deklarationstyp entspricht einer EPD „von der Wiege bis Werkstor - mit Optionen“. Inhalte sind das Stadium der Produktion, also von der Bereitstellung der Rohstoffe bis zum Werkstor der Produktion (cradle-to-gate, Module A1-A3), sowie die Entsorgung der Produktverpackung in Modul A5 und Teile des Endes des Lebensweges (Modul C2-C4). Darüber hinaus erfolgt eine Betrachtung des potenziellen Nutzens und der Lasten über den Lebensweg des Produktes hinaus (Modul D).Im Einzelnen werden in Modul A1 die Bereitstellung des Holz-Rohstoffes in Form von Hackschnitzeln aus dem Forst und die Bereitstellung der Zusätze bilanziert. Die Transporte dieser Stoffe werden in Modul A2 berücksichtigt. Modul A3 umfasst die Bereitstellung der Brennstoffe, Betriebsmittel und des Stromes sowie die Herstellungsprozesse vor Ort. Diese sind im Wesentlichen die Zerfaserung, die Fasertrocknung, das Zugeben der Zusätze sowie die Verpackung der Produkte.Modul A5 beinhaltet ausschließlich die Entsorgung der Verpackungsmaterialien.Modul C2 berücksichtigt den Transport zum Entsorger, Modul C3 die Aufbereitung und Sortierung des Altholzes. Zudem werden gemäß /EN 16485/ die CO2-Äquivalente des in Produkt und Verpackung befindlichen Kohlenstoffs sowie die im Produkt und seiner Verpackung enthaltene erneuerbare und nicht erneuerbare Primärenergie (PERM und PENRM) als Abgänge in Modul C3 verbucht. Die sich aus der thermischen Verwertung des Produkts ergebenden Lasten und Potenziale am Ende seines Lebensweges, sowie der potenzielle Nutzen durch Substitution fossiler Brennstoffe im Zuge der Energieerzeugung bei thermischer Verwertung der Produktverpackung, werden in Modul D bilanziert.</useAdviceForDataSet>
<useAdviceForDataSet xml:lang="en">Scope: 
This Environmental Product Declaration is valid for loose GUTEX Thermofibre wood fibre insulation boards produced in the Gutenburg plant (see manufacturer&apos;s address). 
System boundary: 
The Declaration complies with an EPD &quot;from cradle to gate, with options&quot;. It includes the production stage, i.e. from provision of the raw materials through to production (cradle-to-gate, Modules A1-A3), disposal of product packaging in Module A5, and parts of the end-of-life stage (Modules C2-C4). It also contains an analysis of the potential benefits and loads over and beyond the product&apos;s entire life cycle (Module D). The provision of wood as a raw material in the form of wood chips from forestry and the provision of additives are analysed in Module A1. Transport of these substances is considered in Module A2. Module A3 comprises the provision of fuels, resources and electricity as well as the production processes on site. These are essentially defibring, fibre drying, adding additives as well as packing the products. Module A5 exclusively concerns the disposal of packaging materials. Module C2 considers transport to the disposal company and Module C3 is concerned with preparing and sorting waste wood.  In accordance with /EN 16485/, Module C3 also includes as outflows the CO2 equivalents of the carbon in the product and packaging as well as the renewable and non-renewable primary energy (PERM and PENRM) contained in the product and its packaging. The loads and potentials arising from thermal recycling of the product at its end of life and the potential benefits by substituting fossil fuels in the course of generating energy during thermal recycling of the product packaging are analysed in Module D.</useAdviceForDataSet>
<common:other>
<epd2:referenceToOriginalEPD type="source data set" refObjectId="2ad4df9e-5d80-4d07-bfd7-34ade7d72cde">
<common:shortDescription xml:lang="de">GUTEX Thermofibre.pdf</common:shortDescription>
</epd2:referenceToOriginalEPD>
</common:other>
</dataSourcesTreatmentAndRepresentativeness>
<validation>
<review type="Accredited third party review">
<common:referenceToNameOfReviewerAndInstitution uri="../contacts/d111dbec-b024-4be5-86c5-752d6eb2cf95.xml" type="contact data set" refObjectId="d111dbec-b024-4be5-86c5-752d6eb2cf95">
<common:shortDescription xml:lang="de">Institut Bauen und Umwelt e. V.</common:shortDescription>
</common:referenceToNameOfReviewerAndInstitution>
</review>
</validation>
<complianceDeclarations>
<compliance>
<common:referenceToComplianceSystem uri="../sources/b00f9ec0-7874-11e3-981f-0800200c9a66.xml" type="source data set" refObjectId="b00f9ec0-7874-11e3-981f-0800200c9a66">
<common:shortDescription xml:lang="de">DIN EN 15804</common:shortDescription>
</common:referenceToComplianceSystem>
</compliance>
<compliance>
<common:referenceToComplianceSystem uri="../sources/4f2eb655-6e44-4874-a95a-e28f5442cd4d.xml" type="source data set" refObjectId="4f2eb655-6e44-4874-a95a-e28f5442cd4d">
<common:shortDescription xml:lang="de">ISO 14025</common:shortDescription>
</common:referenceToComplianceSystem>
</compliance>
</complianceDeclarations>
</modellingAndValidation>
<administrativeInformation>
<common:commissionerAndGoal>
<common:referenceToCommissioner uri="../contacts/7391944b-7c1d-4888-9cb0-5279215dc906.xml" type="contact data set" refObjectId="7391944b-7c1d-4888-9cb0-5279215dc906">
<common:shortDescription xml:lang="de">GUTEX Holzfaserplattenwerk H. Henselmann GmbH + Co KG</common:shortDescription>
</common:referenceToCommissioner>
</common:commissionerAndGoal>
<dataGenerator>
<common:referenceToPersonOrEntityGeneratingTheDataSet uri="../contacts/de5ed5e4-e8c5-494d-9e3e-e4fe0f039a02.xml" type="contact data set" refObjectId="de5ed5e4-e8c5-494d-9e3e-e4fe0f039a02">
<common:shortDescription xml:lang="de">Thünen-Institut für Holzforschung</common:shortDescription>
</common:referenceToPersonOrEntityGeneratingTheDataSet>
</dataGenerator>
<dataEntryBy>
<common:timeStamp>2019-04-18T14:54:05.644</common:timeStamp>
<common:referenceToDataSetFormat uri="../sources/a97a0155-0234-4b87-b4ce-a45da52f2a40.xml" type="source data set" refObjectId="a97a0155-0234-4b87-b4ce-a45da52f2a40">
<common:shortDescription xml:lang="de">ILCD Format</common:shortDescription>
</common:referenceToDataSetFormat>
<common:referenceToDataSetFormat uri="../sources/a29449fd-aa2f-4de8-b5d7-4b06b43c6fde.xml" type="source data set" refObjectId="a29449fd-aa2f-4de8-b5d7-4b06b43c6fde">
<common:shortDescription xml:lang="de">EPD-Datenformaterweiterungen v1.2</common:shortDescription>
<common:shortDescription xml:lang="en">EPD Data Format Extensions v1.2</common:shortDescription>
</common:referenceToDataSetFormat>
</dataEntryBy>
<publicationAndOwnership>
<common:dataSetVersion>00.01.000</common:dataSetVersion>
<common:referenceToRegistrationAuthority uri="../contacts/d111dbec-b024-4be5-86c5-752d6eb2cf95.xml" type="contact data set" refObjectId="d111dbec-b024-4be5-86c5-752d6eb2cf95">
<common:shortDescription xml:lang="de">Institut Bauen und Umwelt e. V.</common:shortDescription>
</common:referenceToRegistrationAuthority>
<common:registrationNumber>EPD-GTX-20190018-IBA1-DE</common:registrationNumber>
<common:referenceToOwnershipOfDataSet uri="../contacts/7391944b-7c1d-4888-9cb0-5279215dc906.xml" type="contact data set" refObjectId="7391944b-7c1d-4888-9cb0-5279215dc906">
<common:shortDescription xml:lang="de">GUTEX Holzfaserplattenwerk H. Henselmann GmbH + Co KG</common:shortDescription>
</common:referenceToOwnershipOfDataSet>
<common:copyright>true</common:copyright>
<common:licenseType>Free of charge for all users and uses</common:licenseType>
<common:accessRestrictions xml:lang="en">None</common:accessRestrictions>
<common:other>
<epd2:referenceToPublisher type="contact data set" refObjectId="d111dbec-b024-4be5-86c5-752d6eb2cf95" uri="../contacts/d111dbec-b024-4be5-86c5-752d6eb2cf95.xml">
<common:shortDescription xml:lang="de">Institut Bauen und Umwelt e. V.</common:shortDescription>
</epd2:referenceToPublisher>
</common:other>
</publicationAndOwnership>
</administrativeInformation>
<exchanges>
<exchange dataSetInternalID="0">
<referenceToFlowDataSet uri="../flows/0b882bb8-7de5-bb70-8532-73c07c1a6f8b.xml" type="flow data set" refObjectId="0b882bb8-7de5-bb70-8532-73c07c1a6f8b">
<common:shortDescription xml:lang="de">GUTEX Thermofibre ()</common:shortDescription>
</referenceToFlowDataSet>
<meanAmount>1</meanAmount>
<referencesToDataSource />
</exchange>
<exchange dataSetInternalID="1">
<referenceToFlowDataSet uri="../flows/20f32be5-0398-4288-9b6d-accddd195317.xml" type="flow data set" refObjectId="20f32be5-0398-4288-9b6d-accddd195317">
<common:shortDescription xml:lang="de">Erneuerbare Primärenergie als Energieträger (PERE)</common:shortDescription>
<common:shortDescription xml:lang="en">Renewable primary energy as energy carrier (PERE)</common:shortDescription>
</referenceToFlowDataSet>
<functionType>General reminder flow</functionType>
<exchangeDirection>Input</exchangeDirection>
<common:other>
<epd:referenceToUnitGroupDataSet uri="../unitgroups/93a60a57-a3c8-11da-a746-0800200c9a66.xml" type="unit group data set" refObjectId="93a60a57-a3c8-11da-a746-0800200c9a66">
<common:shortDescription xml:lang="de">MJ</common:shortDescription>
</epd:referenceToUnitGroupDataSet>
<epd:amount epd:module="A1">0.107751841936278</epd:amount>
<epd:amount epd:module="A2">0.00475656092381496</epd:amount>
<epd:amount epd:module="A3">0.76770069334249</epd:amount>
<epd:amount epd:module="A5">1.07399555927417</epd:amount>
<epd:amount epd:module="C2">0.00060767306525912</epd:amount>
<epd:amount epd:module="C3">0</epd:amount>
<epd:amount epd:module="D">13.9214144109742</epd:amount>
</common:other>
</exchange>
<exchange dataSetInternalID="2">
<referenceToFlowDataSet uri="../flows/fb3ec0de-548d-4508-aea5-00b73bf6f702.xml" type="flow data set" refObjectId="fb3ec0de-548d-4508-aea5-00b73bf6f702">
<common:shortDescription xml:lang="de">Erneuerbare Primärenergie zur stofflichen Nutzung (PERM)</common:shortDescription>
<common:shortDescription xml:lang="en">Renewable primary energy resources as material utilization (PERM)</common:shortDescription>
</referenceToFlowDataSet>
<functionType>General reminder flow</functionType>
<exchangeDirection>Input</exchangeDirection>
<common:other>
<epd:referenceToUnitGroupDataSet uri="../unitgroups/93a60a57-a3c8-11da-a746-0800200c9a66.xml" type="unit group data set" refObjectId="93a60a57-a3c8-11da-a746-0800200c9a66">
<common:shortDescription xml:lang="de">MJ</common:shortDescription>
</epd:referenceToUnitGroupDataSet>
<epd:amount epd:module="A1">17.054835</epd:amount>
<epd:amount epd:module="A2">0</epd:amount>
<epd:amount epd:module="A3">1.06850985</epd:amount>
<epd:amount epd:module="A5">-1.06850985</epd:amount>
<epd:amount epd:module="C2">0</epd:amount>
<epd:amount epd:module="C3">-17.054835</epd:amount>
<epd:amount epd:module="D">0</epd:amount>
</common:other>
</exchange>
<exchange dataSetInternalID="3">
<referenceToFlowDataSet uri="../flows/53f97275-fa8a-4cdd-9024-65936002acd0.xml" type="flow data set" refObjectId="53f97275-fa8a-4cdd-9024-65936002acd0">
<common:shortDescription xml:lang="de">Total erneuerbare Primärenergie (PERT)</common:shortDescription>
<common:shortDescription xml:lang="en">Total use of renewable primary energy resources (PERT)</common:shortDescription>
</referenceToFlowDataSet>
<functionType>General reminder flow</functionType>
<exchangeDirection>Input</exchangeDirection>
<common:other>
<epd:referenceToUnitGroupDataSet uri="../unitgroups/93a60a57-a3c8-11da-a746-0800200c9a66.xml" type="unit group data set" refObjectId="93a60a57-a3c8-11da-a746-0800200c9a66">
<common:shortDescription xml:lang="de">MJ</common:shortDescription>
</epd:referenceToUnitGroupDataSet>
<epd:amount epd:module="A1">17.1625868419363</epd:amount>
<epd:amount epd:module="A2">0.00475656092381496</epd:amount>
<epd:amount epd:module="A3">1.83621054334249</epd:amount>
<epd:amount epd:module="A5">0.00548570927417136</epd:amount>
<epd:amount epd:module="C2">0.00060767306525912</epd:amount>
<epd:amount epd:module="C3">-17.054835</epd:amount>
<epd:amount epd:module="D">13.9214144109742</epd:amount>
</common:other>
</exchange>
<exchange dataSetInternalID="4">
<referenceToFlowDataSet uri="../flows/ac857178-2b45-46ec-892a-a9a4332f0372.xml" type="flow data set" refObjectId="ac857178-2b45-46ec-892a-a9a4332f0372">
<common:shortDescription xml:lang="de">Nicht-erneuerbare Primärenergie als Energieträger (PENRE)</common:shortDescription>
<common:shortDescription xml:lang="en">Non renewable primary energy as energy carrier (PENRE)</common:shortDescription>
</referenceToFlowDataSet>
<functionType>General reminder flow</functionType>
<exchangeDirection>Input</exchangeDirection>
<common:other>
<epd:referenceToUnitGroupDataSet uri="../unitgroups/93a60a57-a3c8-11da-a746-0800200c9a66.xml" type="unit group data set" refObjectId="93a60a57-a3c8-11da-a746-0800200c9a66">
<common:shortDescription xml:lang="de">MJ</common:shortDescription>
</epd:referenceToUnitGroupDataSet>
<epd:amount epd:module="A1">0.674381873471067</epd:amount>
<epd:amount epd:module="A2">0.100690246875709</epd:amount>
<epd:amount epd:module="A3">8.36718258648612</epd:amount>
<epd:amount epd:module="A5">0.357205074513335</epd:amount>
<epd:amount epd:module="C2">0.0128636533707184</epd:amount>
<epd:amount epd:module="C3">0</epd:amount>
<epd:amount epd:module="D">-14.221056821034</epd:amount>
</common:other>
</exchange>
<exchange dataSetInternalID="5">
<referenceToFlowDataSet uri="../flows/1421caa0-679d-4bf4-b282-0eb850ccae27.xml" type="flow data set" refObjectId="1421caa0-679d-4bf4-b282-0eb850ccae27">
<common:shortDescription xml:lang="de">Nicht-erneuerbare Primärenergie zur stofflichen Nutzung (PENRM)</common:shortDescription>
<common:shortDescription xml:lang="en">Non renewable primary energy as material utilization (PENRM)</common:shortDescription>
</referenceToFlowDataSet>
<functionType>General reminder flow</functionType>
<exchangeDirection>Input</exchangeDirection>
<common:other>
<epd:referenceToUnitGroupDataSet uri="../unitgroups/93a60a57-a3c8-11da-a746-0800200c9a66.xml" type="unit group data set" refObjectId="93a60a57-a3c8-11da-a746-0800200c9a66">
<common:shortDescription xml:lang="de">MJ</common:shortDescription>
</epd:referenceToUnitGroupDataSet>
<epd:amount epd:module="A1">0.35</epd:amount>
<epd:amount epd:module="A2">0</epd:amount>
<epd:amount epd:module="A3">0.32616</epd:amount>
<epd:amount epd:module="A5">-0.32616</epd:amount>
<epd:amount epd:module="C2">0</epd:amount>
<epd:amount epd:module="C3">-0.35</epd:amount>
<epd:amount epd:module="D">0</epd:amount>
</common:other>
</exchange>
<exchange dataSetInternalID="6">
<referenceToFlowDataSet uri="../flows/06159210-646b-4c8d-8583-da9b3b95a6c1.xml" type="flow data set" refObjectId="06159210-646b-4c8d-8583-da9b3b95a6c1">
<common:shortDescription xml:lang="de">Total nicht erneuerbare Primärenergie (PENRT)</common:shortDescription>
<common:shortDescription xml:lang="en">Total use of non renewable primary energy resources (PENRT)</common:shortDescription>
</referenceToFlowDataSet>
<functionType>General reminder flow</functionType>
<exchangeDirection>Input</exchangeDirection>
<common:other>
<epd:referenceToUnitGroupDataSet uri="../unitgroups/93a60a57-a3c8-11da-a746-0800200c9a66.xml" type="unit group data set" refObjectId="93a60a57-a3c8-11da-a746-0800200c9a66">
<common:shortDescription xml:lang="de">MJ</common:shortDescription>
</epd:referenceToUnitGroupDataSet>
<epd:amount epd:module="A1">1.02438187347107</epd:amount>
<epd:amount epd:module="A2">0.100690246875709</epd:amount>
<epd:amount epd:module="A3">8.69334258648612</epd:amount>
<epd:amount epd:module="A5">0.031045074513335</epd:amount>
<epd:amount epd:module="C2">0.0128636533707184</epd:amount>
<epd:amount epd:module="C3">-0.35</epd:amount>
<epd:amount epd:module="D">-14.221056821034</epd:amount>
</common:other>
</exchange>
<exchange dataSetInternalID="7">
<referenceToFlowDataSet uri="../flows/c6a1f35f-2d09-4f54-8dfb-97e502e1ce92.xml" type="flow data set" refObjectId="c6a1f35f-2d09-4f54-8dfb-97e502e1ce92">
<common:shortDescription xml:lang="de">Einsatz von Sekundärstoffen (SM)</common:shortDescription>
<common:shortDescription xml:lang="en">Use of secondary material (SM)</common:shortDescription>
</referenceToFlowDataSet>
<functionType>General reminder flow</functionType>
<exchangeDirection>Input</exchangeDirection>
<common:other>
<epd:referenceToUnitGroupDataSet uri="../unitgroups/ad38d542-3fe9-439d-9b95-2f5f7752acaf.xml" type="unit group data set" refObjectId="ad38d542-3fe9-439d-9b95-2f5f7752acaf">
<common:shortDescription xml:lang="de">kg</common:shortDescription>
</epd:referenceToUnitGroupDataSet>
<epd:amount epd:module="A1">0</epd:amount>
<epd:amount epd:module="A2">0</epd:amount>
<epd:amount epd:module="A3">0</epd:amount>
<epd:amount epd:module="A5">0</epd:amount>
<epd:amount epd:module="C2">0</epd:amount>
<epd:amount epd:module="C3">0</epd:amount>
<epd:amount epd:module="D">0</epd:amount>
</common:other>
</exchange>
<exchange dataSetInternalID="8">
<referenceToFlowDataSet uri="../flows/64333088-a55f-4aa2-9a31-c10b07816787.xml" type="flow data set" refObjectId="64333088-a55f-4aa2-9a31-c10b07816787">
<common:shortDescription xml:lang="de">Erneuerbare Sekundärbrennstoffe (RSF)</common:shortDescription>
<common:shortDescription xml:lang="en">Use of renewable secondary fuels (RSF)</common:shortDescription>
</referenceToFlowDataSet>
<functionType>General reminder flow</functionType>
<exchangeDirection>Input</exchangeDirection>
<common:other>
<epd:referenceToUnitGroupDataSet uri="../unitgroups/93a60a57-a3c8-11da-a746-0800200c9a66.xml" type="unit group data set" refObjectId="93a60a57-a3c8-11da-a746-0800200c9a66">
<common:shortDescription xml:lang="de">MJ</common:shortDescription>
</epd:referenceToUnitGroupDataSet>
<epd:amount epd:module="A1">0</epd:amount>
<epd:amount epd:module="A2">0</epd:amount>
<epd:amount epd:module="A3">0</epd:amount>
<epd:amount epd:module="A5">0</epd:amount>
<epd:amount epd:module="C2">0</epd:amount>
<epd:amount epd:module="C3">0</epd:amount>
<epd:amount epd:module="D">17.054835</epd:amount>
</common:other>
</exchange>
<exchange dataSetInternalID="9">
<referenceToFlowDataSet uri="../flows/89def144-d39a-4287-b86f-efde453ddcb2.xml" type="flow data set" refObjectId="89def144-d39a-4287-b86f-efde453ddcb2">
<common:shortDescription xml:lang="de">Nicht erneuerbare Sekundärbrennstoffe (NRSF)</common:shortDescription>
<common:shortDescription xml:lang="en">Use of non renewable secondary fuels (NRSF)</common:shortDescription>
</referenceToFlowDataSet>
<functionType>General reminder flow</functionType>
<exchangeDirection>Input</exchangeDirection>
<common:other>
<epd:referenceToUnitGroupDataSet uri="../unitgroups/93a60a57-a3c8-11da-a746-0800200c9a66.xml" type="unit group data set" refObjectId="93a60a57-a3c8-11da-a746-0800200c9a66">
<common:shortDescription xml:lang="de">MJ</common:shortDescription>
</epd:referenceToUnitGroupDataSet>
<epd:amount epd:module="A1">0</epd:amount>
<epd:amount epd:module="A2">0</epd:amount>
<epd:amount epd:module="A3">0</epd:amount>
<epd:amount epd:module="A5">0</epd:amount>
<epd:amount epd:module="C2">0</epd:amount>
<epd:amount epd:module="C3">0</epd:amount>
<epd:amount epd:module="D">0.35</epd:amount>
</common:other>
</exchange>
<exchange dataSetInternalID="10">
<referenceToFlowDataSet uri="../flows/3cf952c8-f3a4-461d-8c96-96456ca62246.xml" type="flow data set" refObjectId="3cf952c8-f3a4-461d-8c96-96456ca62246">
<common:shortDescription xml:lang="de">Einsatz von Süßwasserressourcen (FW)</common:shortDescription>
<common:shortDescription xml:lang="en">Use of net fresh water (FW)</common:shortDescription>
</referenceToFlowDataSet>
<functionType>General reminder flow</functionType>
<exchangeDirection>Input</exchangeDirection>
<common:other>
<epd:referenceToUnitGroupDataSet uri="../unitgroups/cd950537-0a98-4044-9ba7-9f9a68d0a504.xml" type="unit group data set" refObjectId="cd950537-0a98-4044-9ba7-9f9a68d0a504">
<common:shortDescription xml:lang="de">m^3</common:shortDescription>
</epd:referenceToUnitGroupDataSet>
<epd:amount epd:module="A1">0.00106958168111957</epd:amount>
<epd:amount epd:module="A2">9.35293509270743E-06</epd:amount>
<epd:amount epd:module="A3">0.00376481416784709</epd:amount>
<epd:amount epd:module="A5">0.000299024143269734</epd:amount>
<epd:amount epd:module="C2">1.19488151796793E-06</epd:amount>
<epd:amount epd:module="C3">0</epd:amount>
<epd:amount epd:module="D">0.00191355737659486</epd:amount>
</common:other>
</exchange>
<exchange dataSetInternalID="11">
<referenceToFlowDataSet uri="../flows/430f9e0f-59b2-46a0-8e0d-55e0e84948fc.xml" type="flow data set" refObjectId="430f9e0f-59b2-46a0-8e0d-55e0e84948fc">
<common:shortDescription xml:lang="de">Gefährlicher Abfall zur Deponie (HWD)</common:shortDescription>
<common:shortDescription xml:lang="en">Hazardous waste disposed (HWD)</common:shortDescription>
</referenceToFlowDataSet>
<functionType>General reminder flow</functionType>
<exchangeDirection>Output</exchangeDirection>
<common:other>
<epd:referenceToUnitGroupDataSet uri="../unitgroups/ad38d542-3fe9-439d-9b95-2f5f7752acaf.xml" type="unit group data set" refObjectId="ad38d542-3fe9-439d-9b95-2f5f7752acaf">
<common:shortDescription xml:lang="de">kg</common:shortDescription>
</epd:referenceToUnitGroupDataSet>
<epd:amount epd:module="A1">0</epd:amount>
<epd:amount epd:module="A2">0</epd:amount>
<epd:amount epd:module="A3">0</epd:amount>
<epd:amount epd:module="A5">0</epd:amount>
<epd:amount epd:module="C2">0</epd:amount>
<epd:amount epd:module="C3">0</epd:amount>
<epd:amount epd:module="D">0</epd:amount>
</common:other>
</exchange>
<exchange dataSetInternalID="12">
<referenceToFlowDataSet uri="../flows/b29ef66b-e286-4afa-949f-62f1a7b4d7fa.xml" type="flow data set" refObjectId="b29ef66b-e286-4afa-949f-62f1a7b4d7fa">
<common:shortDescription xml:lang="de">Entsorgter nicht gefährlicher Abfall (NHWD)</common:shortDescription>
<common:shortDescription xml:lang="en">Non hazardous waste disposed (NHWD)</common:shortDescription>
</referenceToFlowDataSet>
<functionType>General reminder flow</functionType>
<exchangeDirection>Output</exchangeDirection>
<common:other>
<epd:referenceToUnitGroupDataSet uri="../unitgroups/ad38d542-3fe9-439d-9b95-2f5f7752acaf.xml" type="unit group data set" refObjectId="ad38d542-3fe9-439d-9b95-2f5f7752acaf">
<common:shortDescription xml:lang="de">kg</common:shortDescription>
</epd:referenceToUnitGroupDataSet>
<epd:amount epd:module="A1">0</epd:amount>
<epd:amount epd:module="A2">0</epd:amount>
<epd:amount epd:module="A3">0.0001812</epd:amount>
<epd:amount epd:module="A5">0</epd:amount>
<epd:amount epd:module="C2">0</epd:amount>
<epd:amount epd:module="C3">0</epd:amount>
<epd:amount epd:module="D">0</epd:amount>
</common:other>
</exchange>
<exchange dataSetInternalID="13">
<referenceToFlowDataSet uri="../flows/3449546e-52ad-4b39-b809-9fb77cea8ff6.xml" type="flow data set" refObjectId="3449546e-52ad-4b39-b809-9fb77cea8ff6">
<common:shortDescription xml:lang="de">Entsorgter radioaktiver Abfall (RWD)</common:shortDescription>
<common:shortDescription xml:lang="en">Radioactive waste disposed (RWD)</common:shortDescription>
</referenceToFlowDataSet>
<functionType>General reminder flow</functionType>
<exchangeDirection>Output</exchangeDirection>
<common:other>
<epd:referenceToUnitGroupDataSet uri="../unitgroups/ad38d542-3fe9-439d-9b95-2f5f7752acaf.xml" type="unit group data set" refObjectId="ad38d542-3fe9-439d-9b95-2f5f7752acaf">
<common:shortDescription xml:lang="de">kg</common:shortDescription>
</epd:referenceToUnitGroupDataSet>
<epd:amount epd:module="A1">1.67379899713912E-05</epd:amount>
<epd:amount epd:module="A2">1.37542388641441E-07</epd:amount>
<epd:amount epd:module="A3">2.15142932674038E-05</epd:amount>
<epd:amount epd:module="A5">1.26688634200577E-06</epd:amount>
<epd:amount epd:module="C2">1.75716880846278E-08</epd:amount>
<epd:amount epd:module="C3">0</epd:amount>
<epd:amount epd:module="D">-0.000668049448653602</epd:amount>
</common:other>
</exchange>
<exchange dataSetInternalID="14">
<referenceToFlowDataSet uri="../flows/a2b32f97-3fc7-4af2-b209-525bc6426f33.xml" type="flow data set" refObjectId="a2b32f97-3fc7-4af2-b209-525bc6426f33">
<common:shortDescription xml:lang="de">Komponenten für die Wiederverwendung (CRU)</common:shortDescription>
<common:shortDescription xml:lang="en">Components for re-use (CRU)</common:shortDescription>
</referenceToFlowDataSet>
<functionType>General reminder flow</functionType>
<exchangeDirection>Output</exchangeDirection>
<common:other>
<epd:referenceToUnitGroupDataSet uri="../unitgroups/ad38d542-3fe9-439d-9b95-2f5f7752acaf.xml" type="unit group data set" refObjectId="ad38d542-3fe9-439d-9b95-2f5f7752acaf">
<common:shortDescription xml:lang="de">kg</common:shortDescription>
</epd:referenceToUnitGroupDataSet>
<epd:amount epd:module="A1">0</epd:amount>
<epd:amount epd:module="A2">0</epd:amount>
<epd:amount epd:module="A3">0</epd:amount>
<epd:amount epd:module="A5">0</epd:amount>
<epd:amount epd:module="C2">0</epd:amount>
<epd:amount epd:module="C3">0</epd:amount>
<epd:amount epd:module="D">0</epd:amount>
</common:other>
</exchange>
<exchange dataSetInternalID="15">
<referenceToFlowDataSet uri="../flows/d7fe48a5-4103-49c8-9aae-b0b5dfdbd6ae.xml" type="flow data set" refObjectId="d7fe48a5-4103-49c8-9aae-b0b5dfdbd6ae">
<common:shortDescription xml:lang="de">Stoffe zum Recycling (MFR)</common:shortDescription>
<common:shortDescription xml:lang="en">Materials for recycling (MFR)</common:shortDescription>
</referenceToFlowDataSet>
<functionType>General reminder flow</functionType>
<exchangeDirection>Output</exchangeDirection>
<common:other>
<epd:referenceToUnitGroupDataSet uri="../unitgroups/ad38d542-3fe9-439d-9b95-2f5f7752acaf.xml" type="unit group data set" refObjectId="ad38d542-3fe9-439d-9b95-2f5f7752acaf">
<common:shortDescription xml:lang="de">kg</common:shortDescription>
</epd:referenceToUnitGroupDataSet>
<epd:amount epd:module="A1">0</epd:amount>
<epd:amount epd:module="A2">0</epd:amount>
<epd:amount epd:module="A3">0</epd:amount>
<epd:amount epd:module="A5">0</epd:amount>
<epd:amount epd:module="C2">0</epd:amount>
<epd:amount epd:module="C3">0</epd:amount>
<epd:amount epd:module="D">0</epd:amount>
</common:other>
</exchange>
<exchange dataSetInternalID="16">
<referenceToFlowDataSet uri="../flows/59a9181c-3aaf-46ee-8b13-2b3723b6e447.xml" type="flow data set" refObjectId="59a9181c-3aaf-46ee-8b13-2b3723b6e447">
<common:shortDescription xml:lang="de">Stoffe für die Energierückgewinnung (MER)</common:shortDescription>
<common:shortDescription xml:lang="en">Materials for energy recovery (MER)</common:shortDescription>
</referenceToFlowDataSet>
<functionType>General reminder flow</functionType>
<exchangeDirection>Output</exchangeDirection>
<common:other>
<epd:referenceToUnitGroupDataSet uri="../unitgroups/ad38d542-3fe9-439d-9b95-2f5f7752acaf.xml" type="unit group data set" refObjectId="ad38d542-3fe9-439d-9b95-2f5f7752acaf">
<common:shortDescription xml:lang="de">kg</common:shortDescription>
</epd:referenceToUnitGroupDataSet>
<epd:amount epd:module="A1">0</epd:amount>
<epd:amount epd:module="A2">0</epd:amount>
<epd:amount epd:module="A3">0</epd:amount>
<epd:amount epd:module="A5">0</epd:amount>
<epd:amount epd:module="C2">0</epd:amount>
<epd:amount epd:module="C3">1</epd:amount>
<epd:amount epd:module="D">0</epd:amount>
</common:other>
</exchange>
<exchange dataSetInternalID="17">
<referenceToFlowDataSet uri="../flows/4da0c987-2b76-40d6-9e9e-82a017aaaf29.xml" type="flow data set" refObjectId="4da0c987-2b76-40d6-9e9e-82a017aaaf29">
<common:shortDescription xml:lang="de">Exportierte elektrische Energie (EEE)</common:shortDescription>
<common:shortDescription xml:lang="en">Exported electrical energy (EEE)</common:shortDescription>
</referenceToFlowDataSet>
<functionType>General reminder flow</functionType>
<exchangeDirection>Output</exchangeDirection>
<common:other>
<epd:referenceToUnitGroupDataSet uri="../unitgroups/93a60a57-a3c8-11da-a746-0800200c9a66.xml" type="unit group data set" refObjectId="93a60a57-a3c8-11da-a746-0800200c9a66">
<common:shortDescription xml:lang="de">MJ</common:shortDescription>
</epd:referenceToUnitGroupDataSet>
<epd:amount epd:module="A1">0</epd:amount>
<epd:amount epd:module="A2">0</epd:amount>
<epd:amount epd:module="A3">0</epd:amount>
<epd:amount epd:module="A5">0.168128</epd:amount>
<epd:amount epd:module="C2">0</epd:amount>
<epd:amount epd:module="C3">0</epd:amount>
<epd:amount epd:module="D">0</epd:amount>
</common:other>
</exchange>
<exchange dataSetInternalID="18">
<referenceToFlowDataSet uri="../flows/98daf38a-7a79-46d3-9a37-2b7bd0955810.xml" type="flow data set" refObjectId="98daf38a-7a79-46d3-9a37-2b7bd0955810">
<common:shortDescription xml:lang="de">Exportierte thermische Energie (EET)</common:shortDescription>
<common:shortDescription xml:lang="en">Exported thermal energy (EET)</common:shortDescription>
</referenceToFlowDataSet>
<functionType>General reminder flow</functionType>
<exchangeDirection>Output</exchangeDirection>
<common:other>
<epd:referenceToUnitGroupDataSet uri="../unitgroups/93a60a57-a3c8-11da-a746-0800200c9a66.xml" type="unit group data set" refObjectId="93a60a57-a3c8-11da-a746-0800200c9a66">
<common:shortDescription xml:lang="de">MJ</common:shortDescription>
</epd:referenceToUnitGroupDataSet>
<epd:amount epd:module="A1">0</epd:amount>
<epd:amount epd:module="A2">0</epd:amount>
<epd:amount epd:module="A3">0</epd:amount>
<epd:amount epd:module="A5">0.409573</epd:amount>
<epd:amount epd:module="C2">0</epd:amount>
<epd:amount epd:module="C3">0</epd:amount>
<epd:amount epd:module="D">0</epd:amount>
</common:other>
</exchange>
</exchanges>
<LCIAResults>
<LCIAResult>
<referenceToLCIAMethodDataSet uri="../lciamethods/77e416eb-a363-4258-a04e-171d843a6460.xml" type="LCIA method data set" refObjectId="77e416eb-a363-4258-a04e-171d843a6460">
<common:shortDescription xml:lang="de">Globales Erwärmungspotenzial (GWP)</common:shortDescription>
<common:shortDescription xml:lang="en">Global warming potential (GWP)</common:shortDescription>
</referenceToLCIAMethodDataSet>
<common:other>
<epd:referenceToUnitGroupDataSet uri="../unitgroups/1ebf3012-d0db-4de2-aefd-ef30cedb0be1.xml" type="unit group data set" refObjectId="1ebf3012-d0db-4de2-aefd-ef30cedb0be1">
<common:shortDescription xml:lang="de">kg CO_(2)-Äq.</common:shortDescription>
</epd:referenceToUnitGroupDataSet>
<epd:amount epd:module="A1">-1.55088555546345</epd:amount>
<epd:amount epd:module="A2">0.00716957692171316</epd:amount>
<epd:amount epd:module="A3">0.398240381161323</epd:amount>
<epd:amount epd:module="A5">0.125663087616322</epd:amount>
<epd:amount epd:module="C2">0.000915947226243908</epd:amount>
<epd:amount epd:module="C3">1.62132</epd:amount>
<epd:amount epd:module="D">-0.940770338880926</epd:amount>
</common:other>
</LCIAResult>
<LCIAResult>
<referenceToLCIAMethodDataSet uri="../lciamethods/06dcd26f-025f-401a-a7c1-5e457eb54637.xml" type="LCIA method data set" refObjectId="06dcd26f-025f-401a-a7c1-5e457eb54637">
<common:shortDescription xml:lang="de">Abbau Potential der stratosphärischen Ozonschicht (ODP)</common:shortDescription>
<common:shortDescription xml:lang="en">Depletion potential of the stratospheric ozone layer (ODP)</common:shortDescription>
</referenceToLCIAMethodDataSet>
<common:other>
<epd:referenceToUnitGroupDataSet uri="../unitgroups/88054749-b0a6-47ea-a82b-dc5b29326512.xml" type="unit group data set" refObjectId="88054749-b0a6-47ea-a82b-dc5b29326512">
<common:shortDescription xml:lang="de">kg CFC11-Äq.</common:shortDescription>
</epd:referenceToUnitGroupDataSet>
<epd:amount epd:module="A1">5.90159844555185E-14</epd:amount>
<epd:amount epd:module="A2">3.69823944050707E-15</epd:amount>
<epd:amount epd:module="A3">1.45020345464212E-13</epd:amount>
<epd:amount epd:module="A5">7.74506949483874E-15</epd:amount>
<epd:amount epd:module="C2">4.72467510218004E-16</epd:amount>
<epd:amount epd:module="C3">0</epd:amount>
<epd:amount epd:module="D">-2.14159084281947E-12</epd:amount>
</common:other>
</LCIAResult>
<LCIAResult>
<referenceToLCIAMethodDataSet uri="../lciamethods/b4274add-93b7-4905-a5e4-2e878c4e4216.xml" type="LCIA method data set" refObjectId="b4274add-93b7-4905-a5e4-2e878c4e4216">
<common:shortDescription xml:lang="de">Versauerungspotenzial von Boden und Wasser (AP)</common:shortDescription>
<common:shortDescription xml:lang="en">Acidification potential of land and water (AP)</common:shortDescription>
</referenceToLCIAMethodDataSet>
<common:other>
<epd:referenceToUnitGroupDataSet uri="../unitgroups/bc50c624-a9bc-45b1-a9b0-e6b10d00476f.xml" type="unit group data set" refObjectId="bc50c624-a9bc-45b1-a9b0-e6b10d00476f">
<common:shortDescription xml:lang="de">kg SO_(2)-Äq.</common:shortDescription>
</epd:referenceToUnitGroupDataSet>
<epd:amount epd:module="A1">0.000249203567868116</epd:amount>
<epd:amount epd:module="A2">3.02803907771505E-05</epd:amount>
<epd:amount epd:module="A3">0.000363794896787626</epd:amount>
<epd:amount epd:module="A5">1.51492088964266E-05</epd:amount>
<epd:amount epd:module="C2">3.86846256686584E-06</epd:amount>
<epd:amount epd:module="C3">0</epd:amount>
<epd:amount epd:module="D">-0.00100538185431334</epd:amount>
</common:other>
</LCIAResult>
<LCIAResult>
<referenceToLCIAMethodDataSet uri="../lciamethods/f58827d0-b407-4ec6-be75-8b69efb98a0f.xml" type="LCIA method data set" refObjectId="f58827d0-b407-4ec6-be75-8b69efb98a0f">
<common:shortDescription xml:lang="de">Eutrophierungspotenzial (EP)</common:shortDescription>
<common:shortDescription xml:lang="en">Eutrophication potential (EP)</common:shortDescription>
</referenceToLCIAMethodDataSet>
<common:other>
<epd:referenceToUnitGroupDataSet uri="../unitgroups/67b5401d-873c-485f-bcf3-6ae83b918822.xml" type="unit group data set" refObjectId="67b5401d-873c-485f-bcf3-6ae83b918822">
<common:shortDescription xml:lang="de">kg PO_(4)^(3)-Äq.</common:shortDescription>
</epd:referenceToUnitGroupDataSet>
<epd:amount epd:module="A1">5.7049715856621E-05</epd:amount>
<epd:amount epd:module="A2">7.54503329255179E-06</epd:amount>
<epd:amount epd:module="A3">5.43298845613657E-05</epd:amount>
<epd:amount epd:module="A5">2.57092082524955E-06</epd:amount>
<epd:amount epd:module="C2">9.63913546321144E-07</epd:amount>
<epd:amount epd:module="C3">0</epd:amount>
<epd:amount epd:module="D">-0.000151532011258883</epd:amount>
</common:other>
</LCIAResult>
<LCIAResult>
<referenceToLCIAMethodDataSet uri="../lciamethods/1e84a202-dae6-42aa-9e9d-71ea48b8be00.xml" type="LCIA method data set" refObjectId="1e84a202-dae6-42aa-9e9d-71ea48b8be00">
<common:shortDescription xml:lang="de">Bildungspotential für troposphärisches Ozon (POCP)</common:shortDescription>
<common:shortDescription xml:lang="en">Formation potential of tropospheric ozone photochemical oxidants (POCP)</common:shortDescription>
</referenceToLCIAMethodDataSet>
<common:other>
<epd:referenceToUnitGroupDataSet uri="../unitgroups/01c26c17-9a76-406e-8295-f17b55fd909e.xml" type="unit group data set" refObjectId="01c26c17-9a76-406e-8295-f17b55fd909e">
<common:shortDescription xml:lang="de">kg Ethen-Äq.</common:shortDescription>
</epd:referenceToUnitGroupDataSet>
<epd:amount epd:module="A1">1.90911361836949E-06</epd:amount>
<epd:amount epd:module="A2">-1.23186752737577E-05</epd:amount>
<epd:amount epd:module="A3">6.37933414132589E-05</epd:amount>
<epd:amount epd:module="A5">8.74356335673992E-07</epd:amount>
<epd:amount epd:module="C2">-1.57376879712753E-06</epd:amount>
<epd:amount epd:module="C3">0</epd:amount>
<epd:amount epd:module="D">-0.000103014939708578</epd:amount>
</common:other>
</LCIAResult>
<LCIAResult>
<referenceToLCIAMethodDataSet uri="../lciamethods/f7c73bb9-ab1a-4249-9c6d-379a0de6f67e.xml" type="LCIA method data set" refObjectId="f7c73bb9-ab1a-4249-9c6d-379a0de6f67e">
<common:shortDescription xml:lang="de">Potenzial für den abiotischen Abbau nicht fossiler Ressourcen (ADPE)</common:shortDescription>
<common:shortDescription xml:lang="en">Abiotic depletion potential for non fossil resources (ADPE)</common:shortDescription>
</referenceToLCIAMethodDataSet>
<common:other>
<epd:referenceToUnitGroupDataSet uri="../unitgroups/54ccd2d9-a32a-4fc2-923d-f2c8c93e89d4.xml" type="unit group data set" refObjectId="54ccd2d9-a32a-4fc2-923d-f2c8c93e89d4">
<common:shortDescription xml:lang="de">kg Sb-Äq.</common:shortDescription>
</epd:referenceToUnitGroupDataSet>
<epd:amount epd:module="A1">1.68810219524782E-08</epd:amount>
<epd:amount epd:module="A2">4.44082292387051E-10</epd:amount>
<epd:amount epd:module="A3">1.10972146619267E-07</epd:amount>
<epd:amount epd:module="A5">2.8041064811527E-09</epd:amount>
<epd:amount epd:module="C2">5.67336048385353E-11</epd:amount>
<epd:amount epd:module="C3">0</epd:amount>
<epd:amount epd:module="D">-2.9073394558994E-07</epd:amount>
</common:other>
</LCIAResult>
<LCIAResult>
<referenceToLCIAMethodDataSet uri="../lciamethods/804ebcdf-309d-4098-8ed8-fdaf2f389981.xml" type="LCIA method data set" refObjectId="804ebcdf-309d-4098-8ed8-fdaf2f389981">
<common:shortDescription xml:lang="de">Potenzial für den abiotischen Abbau fossiler Brennstoffe (ADPF)</common:shortDescription>
<common:shortDescription xml:lang="en">Abiotic depletion potential for fossil resources (ADPF)</common:shortDescription>
</referenceToLCIAMethodDataSet>
<common:other>
<epd:referenceToUnitGroupDataSet uri="../unitgroups/93a60a57-a3c8-11da-a746-0800200c9a66.xml" type="unit group data set" refObjectId="93a60a57-a3c8-11da-a746-0800200c9a66">
<common:shortDescription xml:lang="de">MJ</common:shortDescription>
</epd:referenceToUnitGroupDataSet>
<epd:amount epd:module="A1">0.982151505405637</epd:amount>
<epd:amount epd:module="A2">0.100338197287191</epd:amount>
<epd:amount epd:module="A3">8.31291078497245</epd:amount>
<epd:amount epd:module="A5">0.0278517201651431</epd:amount>
<epd:amount epd:module="C2">0.0128186773773474</epd:amount>
<epd:amount epd:module="C3">0</epd:amount>
<epd:amount epd:module="D">-12.8866993835012</epd:amount>
</common:other>
</LCIAResult>
</LCIAResults>
</processDataSet>