<?xml version="1.0" encoding="utf-8"?>
<processDataSet xmlns:epd="http://www.iai.kit.edu/EPD/2013" xmlns:epd2="http://www.indata.network/EPD/2019" xmlns:common="http://lca.jrc.it/ILCD/Common" xsi:schemaLocation="http://lca.jrc.it/ILCD/Process ../../schemas/EPD_DataSet.xsd" epd2:epd-version="1.2" version="1.1" locations="../ILCDLocations.xml" xmlns:xsi="http://www.w3.org/2001/XMLSchema-instance" xmlns="http://lca.jrc.it/ILCD/Process">
<processInformation>
<dataSetInformation>
<common:UUID>98abfafd-b08c-4eb4-8d02-67d66e0ecc1d</common:UUID>
<name>
<baseName xml:lang="en">THERMATEX Basic &amp; Standard, Pontarlier</baseName>
<functionalUnitFlowProperties xml:lang="en" />
</name>
<classificationInformation>
<common:classification name="OEKOBAU.DAT">
<common:class level="0" classId="1">Mineralische Baustoffe</common:class>
<common:class level="1" classId="1.3">Steine und Elemente</common:class>
<common:class level="2" classId="1.3.15">Deckenplatten</common:class>
</common:classification>
<common:classification name="IBUCategories">
<common:class level="0">02 Building products</common:class>
<common:class level="1">Internal and external wall and ceiling finishes</common:class>
<common:class level="2">Mineral panels</common:class>
</common:classification>
</classificationInformation>
<common:generalComment xml:lang="en">The ceiling tiles are manufactured using a wet felt process and consist of biosoluble mineral wool, perlite, clay and starch. The ceiling tiles meet the requirements of DIN 18177 and EN 13964.The AMF and Armstrong mineral tiles are available in a wide range of different surface designs and product properties. Depending on the design, the ceiling tiles are available in different formats and edge finishes.This EPD applies to the following products:Basic Range:Armstrong Bajkal, Armstrong Feria, Armstrong Savanna, Armstrong Aleria L, Armstrong Atlas, Armstrong Retail, Armstrong Scala, Armstrong Oasis, Armstrong Etna, ECOMIN Orbit, ECOMIN Orbit micro, ECOMIN Planet, ECOMIN FiligranStandard Range:Armstrong Bioguard Plain, Armstrong Plain, Armstrong Casa, Armstrong Cortega, Armstrong Dune, Armstrong Dune NG, Armstrong Dune eVo, Armstrong Dune eVo dB, Armstrong Dune Supreme, Armstrong Retail, Armstrong Sahara, Armstrong Sahara Max, Armstrong Tatra, Armstrong Cortega, Armstrong Fine Fissured, THERMATEX Schlicht, THERMATEX Star, THERMATEX Mercure, THERMATEX Feinstratos, THERMATEX Feinstrator micro, THERMATEX Fresko, THERMATEX FeinfreskoPlease be aware of the limited representativity of the declared impacts for the products Sahara A1 and Dune NG.</common:generalComment>
</dataSetInformation>
<quantitativeReference>
<referenceToReferenceFlow>0</referenceToReferenceFlow>
</quantitativeReference>
<time>
<common:referenceYear>2021</common:referenceYear>
<common:dataSetValidUntil>2026</common:dataSetValidUntil>
<common:other>
<epd2:publicationDateOfEPD>2021-05-25</epd2:publicationDateOfEPD>
</common:other>
</time>
<geography>
<locationOfOperationSupplyOrProduction location="FR" />
</geography>
<technology>
<technologyDescriptionAndIncludedProcesses xml:lang="en">The mineral tiles are produced in the traditional wet process (wet-felt). The raw materials are mixed with water to form a homogeneous suspension, which is pumped onto a belt conveyor (Fourdrinier). The water is removed mechanically (gravity and vacuum) and by evaporation in the drying oven. As far as possible, the process water is reused. It is treated accordingly and fed back into the process water circuit. Depending on the desired appearance the panels can be sanded, colour-treated, patterned, eroded or embossed. Production waste and dust are reused in the process in the sense of an internal cycle. The manufacturing plant is certified according to ISO 9001, ISO 14001 and OHSAS 18001. 
Technical data: 
Mineral boards (wet-felt) are regulated by EN 13964 and have corresponding labelling and declaration of performance. The following data provide an overview of results: 
Declared unit: 
This EPD refers to a declared unit of 1 m² THERMATEX/Armstrong Standard Range ceiling tiles with an average surface weight of 3,25 kg/m².</technologyDescriptionAndIncludedProcesses>
<technologicalApplicability xml:lang="en">Mineral tiles (wet-felt) are typically used as lay in for suspended ceiling constructions. They are primarily used as optical cladding, but also for sound absorption and sound insulation, for fire resistance and against fire spreading, for cleanrooms and high hygiene requirements.</technologicalApplicability>
</technology>
</processInformation>
<modellingAndValidation>
<LCIMethodAndAllocation>
<typeOfDataSet>EPD</typeOfDataSet>
<referenceToLCAMethodDetails type="source data set" refObjectId="e54a04a9-6f7a-42d8-b593-6dfc37bc16b5">
<common:shortDescription xml:lang="en">Mineral panels.pdf</common:shortDescription>
</referenceToLCAMethodDetails>
<common:other>
<epd:subType xmlns="http://www.iai.kit.edu/EPD/2013">average dataset</epd:subType>
</common:other>
</LCIMethodAndAllocation>
<dataSourcesTreatmentAndRepresentativeness>
<referenceToDataSource type="source data set" refObjectId="28d74cc0-db8b-4d7e-bc44-5f6d56ce0c4a">
<common:shortDescription xml:lang="en">GaBi Database (all versions)</common:shortDescription>
</referenceToDataSource>
<referenceToDataSource type="source data set" refObjectId="0115289e-52f0-4920-bc7e-57b1c96aec8d">
<common:shortDescription xml:lang="en">GaBi database SP40 2020</common:shortDescription>
</referenceToDataSource>
<useAdviceForDataSet xml:lang="en">Scope: 
This document refers to 1 m² THERMATEX/ARMSTRONG Standard Range mineral ceiling tiles with an average recipe and an average surface weight of 3,25 kg/m², manufactured at the production facility in Pontarlier, France under the brand names THERMATEX and ARMSTRONG. 
System boundary: 
The life cycle assessment of average THERMATEX/Armstrong Standard Range mineral ceiling tiles includes a cradle-to-gate analysis of the products’ environmental impacts with options. Subsequent life cycle phases are part of the analysis: Module A1–A3 | Production stage The production stage includes the upstream burdens of raw material supply, their transports and the manufacturing plant of Knauf Ceiling Solutions located in Pontarlier (France). Mineral ceiling tiles are produced in the wet-felt process. Main raw material inputs, therefore, refer to mineral wool, perlite, clay and starch. The production site is supplied with electricity from the French power grid and thermal energy from natural gas.Module A4 | Transport from the gate to the siteModule A4 includes transport to the construction site. For this purpose, transport by truck over a distance of 470 km is used as a representative scenario.Module A5 | Assembly at the site   For installation in the building, a scenario of 5 % loss is declared in this EPD. The losses during installation in the building are strongly dependent on the building geometry and the specific application. Thus, the percentage of waste can vary greatly in the building context and must be adjusted accordingly at the building level according to the actual conditions. In addition to the losses during installation in the building, Module A5 includes the environmental impacts from the End-of-Life of the packaging of the products.  Module C1 | Deconstruction and demolitionDisassembly of the product is done either manually or using smaller tools. Referring energy demand is considered to be negligible.Modul C2 | Transport to disposalThe transport to the disposal of the material is estimated declaring a 50 km radius to the landfill. In reality, this scenario may vary depending on the actual location of deconstruction and referring waste treatment. Module C3 | Waste processingThe declared scenario assumes landfilling of the product. Referring environmental impacts are accounted for in module C4. Module C4 | DisposalModule C4 refers to the emissions from the disposal of the mineral ceiling tiles. The chosen scenario, therefore, includes the environmental burdens of landfilling of the product.  Module D | Benefits and loads beyond the system boundaryThe declared scenario assumes landfilling of the product. Referring environmental impacts are accounted for in module C4. Module D declares the substitution potential from energy recovery of the incineration of packaging waste in module A5.</useAdviceForDataSet>
<common:other>
<epd2:referenceToOriginalEPD type="source data set" refObjectId="c967f032-9d13-449b-9d0e-68e5d1f4acbb">
<common:shortDescription xml:lang="en">THERMATEX Basic &amp; Standard, Pontarlier.pdf</common:shortDescription>
</epd2:referenceToOriginalEPD>
</common:other>
</dataSourcesTreatmentAndRepresentativeness>
<validation>
<review type="Accredited third party review">
<common:referenceToNameOfReviewerAndInstitution uri="../contacts/d111dbec-b024-4be5-86c5-752d6eb2cf95.xml" type="contact data set" refObjectId="d111dbec-b024-4be5-86c5-752d6eb2cf95">
<common:shortDescription xml:lang="en">Institut Bauen und Umwelt e. V.</common:shortDescription>
</common:referenceToNameOfReviewerAndInstitution>
</review>
</validation>
<complianceDeclarations>
<compliance>
<common:referenceToComplianceSystem uri="../sources/c0016b33-8cf7-415c-ac6e-deba0d21440d.xml" type="source data set" refObjectId="c0016b33-8cf7-415c-ac6e-deba0d21440d">
<common:shortDescription xml:lang="en">DIN EN 15804+A2</common:shortDescription>
</common:referenceToComplianceSystem>
</compliance>
<compliance>
<common:referenceToComplianceSystem uri="../sources/4f2eb655-6e44-4874-a95a-e28f5442cd4d.xml" type="source data set" refObjectId="4f2eb655-6e44-4874-a95a-e28f5442cd4d">
<common:shortDescription xml:lang="en">ISO 14025</common:shortDescription>
</common:referenceToComplianceSystem>
</compliance>
</complianceDeclarations>
</modellingAndValidation>
<administrativeInformation>
<common:commissionerAndGoal>
<common:referenceToCommissioner uri="../contacts/385ff54b-8ba2-4ffd-83b7-61566c1c205b.xml" type="contact data set" refObjectId="385ff54b-8ba2-4ffd-83b7-61566c1c205b">
<common:shortDescription xml:lang="en">Knauf Ceiling Solutions GmbH &amp; Co. KG</common:shortDescription>
</common:referenceToCommissioner>
</common:commissionerAndGoal>
<dataGenerator>
<common:referenceToPersonOrEntityGeneratingTheDataSet uri="../contacts/ad8ad627-3991-42b7-a7ca-5a3fe0a34c28.xml" type="contact data set" refObjectId="ad8ad627-3991-42b7-a7ca-5a3fe0a34c28">
<common:shortDescription xml:lang="en">Daxner &amp; Merl GmbH</common:shortDescription>
</common:referenceToPersonOrEntityGeneratingTheDataSet>
</dataGenerator>
<dataEntryBy>
<common:timeStamp>2021-05-25T13:00:49.976</common:timeStamp>
<common:referenceToDataSetFormat uri="../sources/a97a0155-0234-4b87-b4ce-a45da52f2a40.xml" type="source data set" refObjectId="a97a0155-0234-4b87-b4ce-a45da52f2a40">
<common:shortDescription xml:lang="en">ILCD Format</common:shortDescription>
</common:referenceToDataSetFormat>
<common:referenceToDataSetFormat uri="../sources/a29449fd-aa2f-4de8-b5d7-4b06b43c6fde.xml" type="source data set" refObjectId="a29449fd-aa2f-4de8-b5d7-4b06b43c6fde">
<common:shortDescription xml:lang="de">EPD-Datenformaterweiterungen v1.2</common:shortDescription>
<common:shortDescription xml:lang="en">EPD Data Format Extensions v1.2</common:shortDescription>
</common:referenceToDataSetFormat>
</dataEntryBy>
<publicationAndOwnership>
<common:dataSetVersion>00.01.000</common:dataSetVersion>
<common:referenceToRegistrationAuthority uri="../contacts/d111dbec-b024-4be5-86c5-752d6eb2cf95.xml" type="contact data set" refObjectId="d111dbec-b024-4be5-86c5-752d6eb2cf95">
<common:shortDescription xml:lang="en">Institut Bauen und Umwelt e. V.</common:shortDescription>
</common:referenceToRegistrationAuthority>
<common:registrationNumber>EPD-KNA-20210114-IBD1-EN</common:registrationNumber>
<common:referenceToOwnershipOfDataSet uri="../contacts/385ff54b-8ba2-4ffd-83b7-61566c1c205b.xml" type="contact data set" refObjectId="385ff54b-8ba2-4ffd-83b7-61566c1c205b">
<common:shortDescription xml:lang="en">Knauf Ceiling Solutions GmbH &amp; Co. KG</common:shortDescription>
</common:referenceToOwnershipOfDataSet>
<common:copyright>true</common:copyright>
<common:licenseType>Free of charge for all users and uses</common:licenseType>
<common:accessRestrictions xml:lang="en">None</common:accessRestrictions>
<common:other>
<epd2:referenceToPublisher type="contact data set" refObjectId="d111dbec-b024-4be5-86c5-752d6eb2cf95" uri="../contacts/d111dbec-b024-4be5-86c5-752d6eb2cf95.xml">
<common:shortDescription xml:lang="en">Institut Bauen und Umwelt e. V.</common:shortDescription>
</epd2:referenceToPublisher>
</common:other>
</publicationAndOwnership>
</administrativeInformation>
<exchanges>
<exchange dataSetInternalID="0">
<referenceToFlowDataSet uri="../flows/58b13413-5e7d-fa45-39d2-7f7ec86cbf01.xml" type="flow data set" refObjectId="58b13413-5e7d-fa45-39d2-7f7ec86cbf01">
<common:shortDescription xml:lang="en">THERMATEX/Armstrong Standard Range mineral ceiling tiles ()</common:shortDescription>
</referenceToFlowDataSet>
<meanAmount>1</meanAmount>
<referencesToDataSource />
</exchange>
<exchange dataSetInternalID="1">
<referenceToFlowDataSet uri="../flows/20f32be5-0398-4288-9b6d-accddd195317.xml" type="flow data set" refObjectId="20f32be5-0398-4288-9b6d-accddd195317">
<common:shortDescription xml:lang="en">Renewable primary energy as energy carrier (PERE)</common:shortDescription>
</referenceToFlowDataSet>
<functionType>General reminder flow</functionType>
<exchangeDirection>Input</exchangeDirection>
<common:other>
<epd:referenceToUnitGroupDataSet uri="../unitgroups/93a60a57-a3c8-11da-a746-0800200c9a66.xml" type="unit group data set" refObjectId="93a60a57-a3c8-11da-a746-0800200c9a66">
<common:shortDescription xml:lang="en">MJ</common:shortDescription>
</epd:referenceToUnitGroupDataSet>
<epd:amount epd:module="A1-A3">0.276025497363291</epd:amount>
<epd:amount epd:module="A4">0.096883484920352</epd:amount>
<epd:amount epd:module="A5">0.01870230964947</epd:amount>
<epd:amount epd:module="C1">0</epd:amount>
<epd:amount epd:module="C2">0.0103067537149311</epd:amount>
<epd:amount epd:module="C3">0</epd:amount>
<epd:amount epd:module="C4">0.0846819938547441</epd:amount>
<epd:amount epd:module="D">-0.0267316578433764</epd:amount>
</common:other>
</exchange>
<exchange dataSetInternalID="2">
<referenceToFlowDataSet uri="../flows/fb3ec0de-548d-4508-aea5-00b73bf6f702.xml" type="flow data set" refObjectId="fb3ec0de-548d-4508-aea5-00b73bf6f702">
<common:shortDescription xml:lang="en">Renewable primary energy resources as material utilization (PERM)</common:shortDescription>
</referenceToFlowDataSet>
<functionType>General reminder flow</functionType>
<exchangeDirection>Input</exchangeDirection>
<common:other>
<epd:referenceToUnitGroupDataSet uri="../unitgroups/93a60a57-a3c8-11da-a746-0800200c9a66.xml" type="unit group data set" refObjectId="93a60a57-a3c8-11da-a746-0800200c9a66">
<common:shortDescription xml:lang="en">MJ</common:shortDescription>
</epd:referenceToUnitGroupDataSet>
<epd:amount epd:module="A1-A3">9.51</epd:amount>
<epd:amount epd:module="A4">0</epd:amount>
<epd:amount epd:module="A5">0.4755</epd:amount>
<epd:amount epd:module="C1">0</epd:amount>
<epd:amount epd:module="C2">0</epd:amount>
<epd:amount epd:module="C3">0</epd:amount>
<epd:amount epd:module="C4">0</epd:amount>
<epd:amount epd:module="D">0</epd:amount>
</common:other>
</exchange>
<exchange dataSetInternalID="3">
<referenceToFlowDataSet uri="../flows/53f97275-fa8a-4cdd-9024-65936002acd0.xml" type="flow data set" refObjectId="53f97275-fa8a-4cdd-9024-65936002acd0">
<common:shortDescription xml:lang="en">Total use of renewable primary energy resources (PERT)</common:shortDescription>
</referenceToFlowDataSet>
<functionType>General reminder flow</functionType>
<exchangeDirection>Input</exchangeDirection>
<common:other>
<epd:referenceToUnitGroupDataSet uri="../unitgroups/93a60a57-a3c8-11da-a746-0800200c9a66.xml" type="unit group data set" refObjectId="93a60a57-a3c8-11da-a746-0800200c9a66">
<common:shortDescription xml:lang="en">MJ</common:shortDescription>
</epd:referenceToUnitGroupDataSet>
<epd:amount epd:module="A1-A3">9.78602549736329</epd:amount>
<epd:amount epd:module="A4">0.096883484920352</epd:amount>
<epd:amount epd:module="A5">0.49420230964947</epd:amount>
<epd:amount epd:module="C1">0</epd:amount>
<epd:amount epd:module="C2">0.0103067537149311</epd:amount>
<epd:amount epd:module="C3">0</epd:amount>
<epd:amount epd:module="C4">0.0846819938547441</epd:amount>
<epd:amount epd:module="D">-0.0267316578433764</epd:amount>
</common:other>
</exchange>
<exchange dataSetInternalID="4">
<referenceToFlowDataSet uri="../flows/ac857178-2b45-46ec-892a-a9a4332f0372.xml" type="flow data set" refObjectId="ac857178-2b45-46ec-892a-a9a4332f0372">
<common:shortDescription xml:lang="en">Non renewable primary energy as energy carrier (PENRE)</common:shortDescription>
</referenceToFlowDataSet>
<functionType>General reminder flow</functionType>
<exchangeDirection>Input</exchangeDirection>
<common:other>
<epd:referenceToUnitGroupDataSet uri="../unitgroups/93a60a57-a3c8-11da-a746-0800200c9a66.xml" type="unit group data set" refObjectId="93a60a57-a3c8-11da-a746-0800200c9a66">
<common:shortDescription xml:lang="en">MJ</common:shortDescription>
</epd:referenceToUnitGroupDataSet>
<epd:amount epd:module="A1-A3">73.6545155091879</epd:amount>
<epd:amount epd:module="A4">1.1985025505461</epd:amount>
<epd:amount epd:module="A5">3.71859612624744</epd:amount>
<epd:amount epd:module="C1">0</epd:amount>
<epd:amount epd:module="C2">0.127500271334691</epd:amount>
<epd:amount epd:module="C3">0</epd:amount>
<epd:amount epd:module="C4">0.647025413141811</epd:amount>
<epd:amount epd:module="D">-0.25763694027588</epd:amount>
</common:other>
</exchange>
<exchange dataSetInternalID="5">
<referenceToFlowDataSet uri="../flows/1421caa0-679d-4bf4-b282-0eb850ccae27.xml" type="flow data set" refObjectId="1421caa0-679d-4bf4-b282-0eb850ccae27">
<common:shortDescription xml:lang="en">Non renewable primary energy as material utilization (PENRM)</common:shortDescription>
</referenceToFlowDataSet>
<functionType>General reminder flow</functionType>
<exchangeDirection>Input</exchangeDirection>
<common:other>
<epd:referenceToUnitGroupDataSet uri="../unitgroups/93a60a57-a3c8-11da-a746-0800200c9a66.xml" type="unit group data set" refObjectId="93a60a57-a3c8-11da-a746-0800200c9a66">
<common:shortDescription xml:lang="en">MJ</common:shortDescription>
</epd:referenceToUnitGroupDataSet>
<epd:amount epd:module="A1-A3">0.38</epd:amount>
<epd:amount epd:module="A4">0</epd:amount>
<epd:amount epd:module="A5">0.019</epd:amount>
<epd:amount epd:module="C1">0</epd:amount>
<epd:amount epd:module="C2">0</epd:amount>
<epd:amount epd:module="C3">0</epd:amount>
<epd:amount epd:module="C4">0</epd:amount>
<epd:amount epd:module="D">0</epd:amount>
</common:other>
</exchange>
<exchange dataSetInternalID="6">
<referenceToFlowDataSet uri="../flows/06159210-646b-4c8d-8583-da9b3b95a6c1.xml" type="flow data set" refObjectId="06159210-646b-4c8d-8583-da9b3b95a6c1">
<common:shortDescription xml:lang="en">Total use of non renewable primary energy resources (PENRT)</common:shortDescription>
</referenceToFlowDataSet>
<functionType>General reminder flow</functionType>
<exchangeDirection>Input</exchangeDirection>
<common:other>
<epd:referenceToUnitGroupDataSet uri="../unitgroups/93a60a57-a3c8-11da-a746-0800200c9a66.xml" type="unit group data set" refObjectId="93a60a57-a3c8-11da-a746-0800200c9a66">
<common:shortDescription xml:lang="en">MJ</common:shortDescription>
</epd:referenceToUnitGroupDataSet>
<epd:amount epd:module="A1-A3">74.0345155091879</epd:amount>
<epd:amount epd:module="A4">1.1985025505461</epd:amount>
<epd:amount epd:module="A5">3.73759612624744</epd:amount>
<epd:amount epd:module="C1">0</epd:amount>
<epd:amount epd:module="C2">0.127500271334691</epd:amount>
<epd:amount epd:module="C3">0</epd:amount>
<epd:amount epd:module="C4">0.647025413141811</epd:amount>
<epd:amount epd:module="D">-0.25763694027588</epd:amount>
</common:other>
</exchange>
<exchange dataSetInternalID="7">
<referenceToFlowDataSet uri="../flows/c6a1f35f-2d09-4f54-8dfb-97e502e1ce92.xml" type="flow data set" refObjectId="c6a1f35f-2d09-4f54-8dfb-97e502e1ce92">
<common:shortDescription xml:lang="en">Use of secondary material (SM)</common:shortDescription>
</referenceToFlowDataSet>
<functionType>General reminder flow</functionType>
<exchangeDirection>Input</exchangeDirection>
<common:other>
<epd:referenceToUnitGroupDataSet uri="../unitgroups/ad38d542-3fe9-439d-9b95-2f5f7752acaf.xml" type="unit group data set" refObjectId="ad38d542-3fe9-439d-9b95-2f5f7752acaf">
<common:shortDescription xml:lang="en">kg</common:shortDescription>
</epd:referenceToUnitGroupDataSet>
<epd:amount epd:module="A1-A3">0.438465913995615</epd:amount>
<epd:amount epd:module="A4">0</epd:amount>
<epd:amount epd:module="A5">0.0219232956997807</epd:amount>
<epd:amount epd:module="C1">0</epd:amount>
<epd:amount epd:module="C2">0</epd:amount>
<epd:amount epd:module="C3">0</epd:amount>
<epd:amount epd:module="C4">0</epd:amount>
<epd:amount epd:module="D">0</epd:amount>
</common:other>
</exchange>
<exchange dataSetInternalID="8">
<referenceToFlowDataSet uri="../flows/64333088-a55f-4aa2-9a31-c10b07816787.xml" type="flow data set" refObjectId="64333088-a55f-4aa2-9a31-c10b07816787">
<common:shortDescription xml:lang="en">Use of renewable secondary fuels (RSF)</common:shortDescription>
</referenceToFlowDataSet>
<functionType>General reminder flow</functionType>
<exchangeDirection>Input</exchangeDirection>
<common:other>
<epd:referenceToUnitGroupDataSet uri="../unitgroups/93a60a57-a3c8-11da-a746-0800200c9a66.xml" type="unit group data set" refObjectId="93a60a57-a3c8-11da-a746-0800200c9a66">
<common:shortDescription xml:lang="en">MJ</common:shortDescription>
</epd:referenceToUnitGroupDataSet>
<epd:amount epd:module="A1-A3">0</epd:amount>
<epd:amount epd:module="A4">0</epd:amount>
<epd:amount epd:module="A5">0</epd:amount>
<epd:amount epd:module="C1">0</epd:amount>
<epd:amount epd:module="C2">0</epd:amount>
<epd:amount epd:module="C3">0</epd:amount>
<epd:amount epd:module="C4">0</epd:amount>
<epd:amount epd:module="D">0</epd:amount>
</common:other>
</exchange>
<exchange dataSetInternalID="9">
<referenceToFlowDataSet uri="../flows/89def144-d39a-4287-b86f-efde453ddcb2.xml" type="flow data set" refObjectId="89def144-d39a-4287-b86f-efde453ddcb2">
<common:shortDescription xml:lang="en">Use of non renewable secondary fuels (NRSF)</common:shortDescription>
</referenceToFlowDataSet>
<functionType>General reminder flow</functionType>
<exchangeDirection>Input</exchangeDirection>
<common:other>
<epd:referenceToUnitGroupDataSet uri="../unitgroups/93a60a57-a3c8-11da-a746-0800200c9a66.xml" type="unit group data set" refObjectId="93a60a57-a3c8-11da-a746-0800200c9a66">
<common:shortDescription xml:lang="en">MJ</common:shortDescription>
</epd:referenceToUnitGroupDataSet>
<epd:amount epd:module="A1-A3">0</epd:amount>
<epd:amount epd:module="A4">0</epd:amount>
<epd:amount epd:module="A5">0</epd:amount>
<epd:amount epd:module="C1">0</epd:amount>
<epd:amount epd:module="C2">0</epd:amount>
<epd:amount epd:module="C3">0</epd:amount>
<epd:amount epd:module="C4">0</epd:amount>
<epd:amount epd:module="D">0</epd:amount>
</common:other>
</exchange>
<exchange dataSetInternalID="10">
<referenceToFlowDataSet uri="../flows/3cf952c8-f3a4-461d-8c96-96456ca62246.xml" type="flow data set" refObjectId="3cf952c8-f3a4-461d-8c96-96456ca62246">
<common:shortDescription xml:lang="en">Use of net fresh water (FW)</common:shortDescription>
</referenceToFlowDataSet>
<functionType>General reminder flow</functionType>
<exchangeDirection>Input</exchangeDirection>
<common:other>
<epd:referenceToUnitGroupDataSet uri="../unitgroups/cd950537-0a98-4044-9ba7-9f9a68d0a504.xml" type="unit group data set" refObjectId="cd950537-0a98-4044-9ba7-9f9a68d0a504">
<common:shortDescription xml:lang="en">m^3</common:shortDescription>
</epd:referenceToUnitGroupDataSet>
<epd:amount epd:module="A1-A3">0.00354726224291646</epd:amount>
<epd:amount epd:module="A4">0.000155066384910133</epd:amount>
<epd:amount epd:module="A5">0.000248114955860329</epd:amount>
<epd:amount epd:module="C1">0</epd:amount>
<epd:amount epd:module="C2">1.64964239266097E-05</epd:amount>
<epd:amount epd:module="C3">0</epd:amount>
<epd:amount epd:module="C4">0.000163087489095201</epd:amount>
<epd:amount epd:module="D">-6.28995712238373E-05</epd:amount>
</common:other>
</exchange>
<exchange dataSetInternalID="11">
<referenceToFlowDataSet uri="../flows/430f9e0f-59b2-46a0-8e0d-55e0e84948fc.xml" type="flow data set" refObjectId="430f9e0f-59b2-46a0-8e0d-55e0e84948fc">
<common:shortDescription xml:lang="en">Hazardous waste disposed (HWD)</common:shortDescription>
</referenceToFlowDataSet>
<functionType>General reminder flow</functionType>
<exchangeDirection>Output</exchangeDirection>
<common:other>
<epd:referenceToUnitGroupDataSet uri="../unitgroups/ad38d542-3fe9-439d-9b95-2f5f7752acaf.xml" type="unit group data set" refObjectId="ad38d542-3fe9-439d-9b95-2f5f7752acaf">
<common:shortDescription xml:lang="en">kg</common:shortDescription>
</epd:referenceToUnitGroupDataSet>
<epd:amount epd:module="A1-A3">2.04640971566512E-06</epd:amount>
<epd:amount epd:module="A4">1.50152855467901E-07</epd:amount>
<epd:amount epd:module="A5">1.02816000408864E-07</epd:amount>
<epd:amount epd:module="C1">0</epd:amount>
<epd:amount epd:module="C2">1.59737080285001E-08</epd:amount>
<epd:amount epd:module="C3">0</epd:amount>
<epd:amount epd:module="C4">9.86263973786257E-09</epd:amount>
<epd:amount epd:module="D">-5.91739531494341E-11</epd:amount>
</common:other>
</exchange>
<exchange dataSetInternalID="12">
<referenceToFlowDataSet uri="../flows/b29ef66b-e286-4afa-949f-62f1a7b4d7fa.xml" type="flow data set" refObjectId="b29ef66b-e286-4afa-949f-62f1a7b4d7fa">
<common:shortDescription xml:lang="en">Non hazardous waste disposed (NHWD)</common:shortDescription>
</referenceToFlowDataSet>
<functionType>General reminder flow</functionType>
<exchangeDirection>Output</exchangeDirection>
<common:other>
<epd:referenceToUnitGroupDataSet uri="../unitgroups/ad38d542-3fe9-439d-9b95-2f5f7752acaf.xml" type="unit group data set" refObjectId="ad38d542-3fe9-439d-9b95-2f5f7752acaf">
<common:shortDescription xml:lang="en">kg</common:shortDescription>
</epd:referenceToUnitGroupDataSet>
<epd:amount epd:module="A1-A3">0.259838052001931</epd:amount>
<epd:amount epd:module="A4">0.000255709943192411</epd:amount>
<epd:amount epd:module="A5">0.175767076310596</epd:amount>
<epd:amount epd:module="C1">0</epd:amount>
<epd:amount epd:module="C2">2.72031854460012E-05</epd:amount>
<epd:amount epd:module="C3">0</epd:amount>
<epd:amount epd:module="C4">3.25321000480489</epd:amount>
<epd:amount epd:module="D">-7.23274695020559E-05</epd:amount>
</common:other>
</exchange>
<exchange dataSetInternalID="13">
<referenceToFlowDataSet uri="../flows/3449546e-52ad-4b39-b809-9fb77cea8ff6.xml" type="flow data set" refObjectId="3449546e-52ad-4b39-b809-9fb77cea8ff6">
<common:shortDescription xml:lang="en">Radioactive waste disposed (RWD)</common:shortDescription>
</referenceToFlowDataSet>
<functionType>General reminder flow</functionType>
<exchangeDirection>Output</exchangeDirection>
<common:other>
<epd:referenceToUnitGroupDataSet uri="../unitgroups/ad38d542-3fe9-439d-9b95-2f5f7752acaf.xml" type="unit group data set" refObjectId="ad38d542-3fe9-439d-9b95-2f5f7752acaf">
<common:shortDescription xml:lang="en">kg</common:shortDescription>
</epd:referenceToUnitGroupDataSet>
<epd:amount epd:module="A1-A3">0.00422437780315668</epd:amount>
<epd:amount epd:module="A4">5.78501617888143E-06</epd:amount>
<epd:amount epd:module="A5">0.000211792236678849</epd:amount>
<epd:amount epd:module="C1">0</epd:amount>
<epd:amount epd:module="C2">6.15427253072493E-07</epd:amount>
<epd:amount epd:module="C3">0</epd:amount>
<epd:amount epd:module="C4">7.34917795589329E-06</epd:amount>
<epd:amount epd:module="D">-4.6661268542335E-05</epd:amount>
</common:other>
</exchange>
<exchange dataSetInternalID="14">
<referenceToFlowDataSet uri="../flows/a2b32f97-3fc7-4af2-b209-525bc6426f33.xml" type="flow data set" refObjectId="a2b32f97-3fc7-4af2-b209-525bc6426f33">
<common:shortDescription xml:lang="en">Components for re-use (CRU)</common:shortDescription>
</referenceToFlowDataSet>
<functionType>General reminder flow</functionType>
<exchangeDirection>Output</exchangeDirection>
<common:other>
<epd:referenceToUnitGroupDataSet uri="../unitgroups/ad38d542-3fe9-439d-9b95-2f5f7752acaf.xml" type="unit group data set" refObjectId="ad38d542-3fe9-439d-9b95-2f5f7752acaf">
<common:shortDescription xml:lang="en">kg</common:shortDescription>
</epd:referenceToUnitGroupDataSet>
<epd:amount epd:module="A1-A3">0</epd:amount>
<epd:amount epd:module="A4">0</epd:amount>
<epd:amount epd:module="A5">0</epd:amount>
<epd:amount epd:module="C1">0</epd:amount>
<epd:amount epd:module="C2">0</epd:amount>
<epd:amount epd:module="C3">0</epd:amount>
<epd:amount epd:module="C4">0</epd:amount>
<epd:amount epd:module="D">0</epd:amount>
</common:other>
</exchange>
<exchange dataSetInternalID="15">
<referenceToFlowDataSet uri="../flows/d7fe48a5-4103-49c8-9aae-b0b5dfdbd6ae.xml" type="flow data set" refObjectId="d7fe48a5-4103-49c8-9aae-b0b5dfdbd6ae">
<common:shortDescription xml:lang="en">Materials for recycling (MFR)</common:shortDescription>
</referenceToFlowDataSet>
<functionType>General reminder flow</functionType>
<exchangeDirection>Output</exchangeDirection>
<common:other>
<epd:referenceToUnitGroupDataSet uri="../unitgroups/ad38d542-3fe9-439d-9b95-2f5f7752acaf.xml" type="unit group data set" refObjectId="ad38d542-3fe9-439d-9b95-2f5f7752acaf">
<common:shortDescription xml:lang="en">kg</common:shortDescription>
</epd:referenceToUnitGroupDataSet>
<epd:amount epd:module="A1-A3">0</epd:amount>
<epd:amount epd:module="A4">0</epd:amount>
<epd:amount epd:module="A5">0.1435419132</epd:amount>
<epd:amount epd:module="C1">0</epd:amount>
<epd:amount epd:module="C2">0</epd:amount>
<epd:amount epd:module="C3">0</epd:amount>
<epd:amount epd:module="C4">0</epd:amount>
<epd:amount epd:module="D">0</epd:amount>
</common:other>
</exchange>
<exchange dataSetInternalID="16">
<referenceToFlowDataSet uri="../flows/59a9181c-3aaf-46ee-8b13-2b3723b6e447.xml" type="flow data set" refObjectId="59a9181c-3aaf-46ee-8b13-2b3723b6e447">
<common:shortDescription xml:lang="en">Materials for energy recovery (MER)</common:shortDescription>
</referenceToFlowDataSet>
<functionType>General reminder flow</functionType>
<exchangeDirection>Output</exchangeDirection>
<common:other>
<epd:referenceToUnitGroupDataSet uri="../unitgroups/ad38d542-3fe9-439d-9b95-2f5f7752acaf.xml" type="unit group data set" refObjectId="ad38d542-3fe9-439d-9b95-2f5f7752acaf">
<common:shortDescription xml:lang="en">kg</common:shortDescription>
</epd:referenceToUnitGroupDataSet>
<epd:amount epd:module="A1-A3">0</epd:amount>
<epd:amount epd:module="A4">0</epd:amount>
<epd:amount epd:module="A5">0</epd:amount>
<epd:amount epd:module="C1">0</epd:amount>
<epd:amount epd:module="C2">0</epd:amount>
<epd:amount epd:module="C3">0</epd:amount>
<epd:amount epd:module="C4">0</epd:amount>
<epd:amount epd:module="D">0</epd:amount>
</common:other>
</exchange>
<exchange dataSetInternalID="17">
<referenceToFlowDataSet uri="../flows/4da0c987-2b76-40d6-9e9e-82a017aaaf29.xml" type="flow data set" refObjectId="4da0c987-2b76-40d6-9e9e-82a017aaaf29">
<common:shortDescription xml:lang="en">Exported electrical energy (EEE)</common:shortDescription>
</referenceToFlowDataSet>
<functionType>General reminder flow</functionType>
<exchangeDirection>Output</exchangeDirection>
<common:other>
<epd:referenceToUnitGroupDataSet uri="../unitgroups/93a60a57-a3c8-11da-a746-0800200c9a66.xml" type="unit group data set" refObjectId="93a60a57-a3c8-11da-a746-0800200c9a66">
<common:shortDescription xml:lang="en">MJ</common:shortDescription>
</epd:referenceToUnitGroupDataSet>
<epd:amount epd:module="A1-A3">0</epd:amount>
<epd:amount epd:module="A4">0</epd:amount>
<epd:amount epd:module="A5">0.0617834011802684</epd:amount>
<epd:amount epd:module="C1">0</epd:amount>
<epd:amount epd:module="C2">0</epd:amount>
<epd:amount epd:module="C3">0</epd:amount>
<epd:amount epd:module="C4">0</epd:amount>
<epd:amount epd:module="D">0</epd:amount>
</common:other>
</exchange>
<exchange dataSetInternalID="18">
<referenceToFlowDataSet uri="../flows/98daf38a-7a79-46d3-9a37-2b7bd0955810.xml" type="flow data set" refObjectId="98daf38a-7a79-46d3-9a37-2b7bd0955810">
<common:shortDescription xml:lang="en">Exported thermal energy (EET)</common:shortDescription>
</referenceToFlowDataSet>
<functionType>General reminder flow</functionType>
<exchangeDirection>Output</exchangeDirection>
<common:other>
<epd:referenceToUnitGroupDataSet uri="../unitgroups/93a60a57-a3c8-11da-a746-0800200c9a66.xml" type="unit group data set" refObjectId="93a60a57-a3c8-11da-a746-0800200c9a66">
<common:shortDescription xml:lang="en">MJ</common:shortDescription>
</epd:referenceToUnitGroupDataSet>
<epd:amount epd:module="A1-A3">0</epd:amount>
<epd:amount epd:module="A4">0</epd:amount>
<epd:amount epd:module="A5">0.109859375567535</epd:amount>
<epd:amount epd:module="C1">0</epd:amount>
<epd:amount epd:module="C2">0</epd:amount>
<epd:amount epd:module="C3">0</epd:amount>
<epd:amount epd:module="C4">0</epd:amount>
<epd:amount epd:module="D">0</epd:amount>
</common:other>
</exchange>
</exchanges>
<LCIAResults>
<LCIAResult>
<referenceToLCIAMethodDataSet uri="../lciamethods/6a37f984-a4b3-458a-a20a-64418c145fa2.xml" type="LCIA method data set" refObjectId="6a37f984-a4b3-458a-a20a-64418c145fa2">
<common:shortDescription xml:lang="en">Global Warming Potential total (GWP-total)</common:shortDescription>
</referenceToLCIAMethodDataSet>
<common:other>
<epd:referenceToUnitGroupDataSet uri="../unitgroups/1ebf3012-d0db-4de2-aefd-ef30cedb0be1.xml" type="unit group data set" refObjectId="1ebf3012-d0db-4de2-aefd-ef30cedb0be1">
<common:shortDescription xml:lang="en">kg CO_(2)-Äq.</common:shortDescription>
</epd:referenceToUnitGroupDataSet>
<epd:amount epd:module="A1-A3">3.21043334114011</epd:amount>
<epd:amount epd:module="A4">0.0911233814738622</epd:amount>
<epd:amount epd:module="A5">0.223293661285667</epd:amount>
<epd:amount epd:module="C1">0</epd:amount>
<epd:amount epd:module="C2">0.00969397675253854</epd:amount>
<epd:amount epd:module="C3">0</epd:amount>
<epd:amount epd:module="C4">0.67602778025063</epd:amount>
<epd:amount epd:module="D">-0.00894787017545527</epd:amount>
</common:other>
</LCIAResult>
<LCIAResult>
<referenceToLCIAMethodDataSet uri="../lciamethods/5f635281-343e-44fb-83df-1971b155e6b6.xml" type="LCIA method data set" refObjectId="5f635281-343e-44fb-83df-1971b155e6b6">
<common:shortDescription xml:lang="en">Global Warming Potential fossil fuels (GWP-fossil)</common:shortDescription>
</referenceToLCIAMethodDataSet>
<common:other>
<epd:referenceToUnitGroupDataSet uri="../unitgroups/1ebf3012-d0db-4de2-aefd-ef30cedb0be1.xml" type="unit group data set" refObjectId="1ebf3012-d0db-4de2-aefd-ef30cedb0be1">
<common:shortDescription xml:lang="en">kg CO_(2)-Äq.</common:shortDescription>
</epd:referenceToUnitGroupDataSet>
<epd:amount epd:module="A1-A3">3.83412630538217</epd:amount>
<epd:amount epd:module="A4">0.0922853177223197</epd:amount>
<epd:amount epd:module="A5">0.223140986026049</epd:amount>
<epd:amount epd:module="C1">0</epd:amount>
<epd:amount epd:module="C2">0.00981758699173614</epd:amount>
<epd:amount epd:module="C3">0</epd:amount>
<epd:amount epd:module="C4">0.0492935955334327</epd:amount>
<epd:amount epd:module="D">-0.00894414864456802</epd:amount>
</common:other>
</LCIAResult>
<LCIAResult>
<referenceToLCIAMethodDataSet uri="../lciamethods/2356e1ab-0185-4db5-86e5-16de51c7485c.xml" type="LCIA method data set" refObjectId="2356e1ab-0185-4db5-86e5-16de51c7485c">
<common:shortDescription xml:lang="en">Global Warming Potential biogenic (GWP-biogenic)</common:shortDescription>
</referenceToLCIAMethodDataSet>
<common:other>
<epd:referenceToUnitGroupDataSet uri="../unitgroups/1ebf3012-d0db-4de2-aefd-ef30cedb0be1.xml" type="unit group data set" refObjectId="1ebf3012-d0db-4de2-aefd-ef30cedb0be1">
<common:shortDescription xml:lang="en">kg CO_(2)-Äq.</common:shortDescription>
</epd:referenceToUnitGroupDataSet>
<epd:amount epd:module="A1-A3">-0.625890567861835</epd:amount>
<epd:amount epd:module="A4">-0.00226043979594102</epd:amount>
<epd:amount epd:module="A5">3.55427553278553E-05</epd:amount>
<epd:amount epd:module="C1">0</epd:amount>
<epd:amount epd:module="C2">-0.000240472318717131</epd:amount>
<epd:amount epd:module="C3">0</epd:amount>
<epd:amount epd:module="C4">0.626592306272346</epd:amount>
<epd:amount epd:module="D">-1.11217358930043E-06</epd:amount>
</common:other>
</LCIAResult>
<LCIAResult>
<referenceToLCIAMethodDataSet uri="../lciamethods/4331bbdb-978a-490d-8707-eeb047f01a55.xml" type="LCIA method data set" refObjectId="4331bbdb-978a-490d-8707-eeb047f01a55">
<common:shortDescription xml:lang="en">Global Warming Potential luluc (GWP-luluc)</common:shortDescription>
</referenceToLCIAMethodDataSet>
<common:other>
<epd:referenceToUnitGroupDataSet uri="../unitgroups/1ebf3012-d0db-4de2-aefd-ef30cedb0be1.xml" type="unit group data set" refObjectId="1ebf3012-d0db-4de2-aefd-ef30cedb0be1">
<common:shortDescription xml:lang="en">kg CO_(2)-Äq.</common:shortDescription>
</epd:referenceToUnitGroupDataSet>
<epd:amount epd:module="A1-A3">0.00219760361977268</epd:amount>
<epd:amount epd:module="A4">0.00109850354748356</epd:amount>
<epd:amount epd:module="A5">0.000117132504290438</epd:amount>
<epd:amount epd:module="C1">0</epd:amount>
<epd:amount epd:module="C2">0.000116862079519527</epd:amount>
<epd:amount epd:module="C3">0</epd:amount>
<epd:amount epd:module="C4">0.000141878444851561</epd:amount>
<epd:amount epd:module="D">-2.6093572979501E-06</epd:amount>
</common:other>
</LCIAResult>
<LCIAResult>
<referenceToLCIAMethodDataSet uri="../lciamethods/b5c629d6-def3-11e6-bf01-fe55135034f3.xml" type="LCIA method data set" refObjectId="b5c629d6-def3-11e6-bf01-fe55135034f3">
<common:shortDescription xml:lang="en">Depletion potential of the stratospheric ozone layer (ODP)</common:shortDescription>
</referenceToLCIAMethodDataSet>
<common:other>
<epd:referenceToUnitGroupDataSet uri="../unitgroups/d9e957c9-7309-4474-bf3a-7777df6c4e5b.xml" type="unit group data set" refObjectId="d9e957c9-7309-4474-bf3a-7777df6c4e5b">
<common:shortDescription xml:lang="en">kg CFC11-Äq.</common:shortDescription>
</epd:referenceToUnitGroupDataSet>
<epd:amount epd:module="A1-A3">8.75192744896768E-11</epd:amount>
<epd:amount epd:module="A4">1.48588916901759E-17</epd:amount>
<epd:amount epd:module="A5">4.37597488341661E-12</epd:amount>
<epd:amount epd:module="C1">0</epd:amount>
<epd:amount epd:module="C2">1.58073315852935E-18</epd:amount>
<epd:amount epd:module="C3">0</epd:amount>
<epd:amount epd:module="C4">1.8267335036982E-16</epd:amount>
<epd:amount epd:module="D">-6.96287999308472E-17</epd:amount>
</common:other>
</LCIAResult>
<LCIAResult>
<referenceToLCIAMethodDataSet uri="../lciamethods/b5c611c6-def3-11e6-bf01-fe55135034f3.xml" type="LCIA method data set" refObjectId="b5c611c6-def3-11e6-bf01-fe55135034f3">
<common:shortDescription xml:lang="en">Acidification potential of land and water (AP)</common:shortDescription>
</referenceToLCIAMethodDataSet>
<common:other>
<epd:referenceToUnitGroupDataSet uri="../unitgroups/42e089ac-92bf-4bf2-8ca1-5fc40d18f2ed.xml" type="unit group data set" refObjectId="42e089ac-92bf-4bf2-8ca1-5fc40d18f2ed">
<common:shortDescription xml:lang="en">mol H^(+)-Äq.</common:shortDescription>
</epd:referenceToUnitGroupDataSet>
<epd:amount epd:module="A1-A3">0.00954554292621546</epd:amount>
<epd:amount epd:module="A4">0.00032923071949057</epd:amount>
<epd:amount epd:module="A5">0.000497876269534564</epd:amount>
<epd:amount epd:module="C1">0</epd:amount>
<epd:amount epd:module="C2">3.50245446266564E-05</epd:amount>
<epd:amount epd:module="C3">0</epd:amount>
<epd:amount epd:module="C4">0.000353655693087454</epd:amount>
<epd:amount epd:module="D">-8.34701085366493E-06</epd:amount>
</common:other>
</LCIAResult>
<LCIAResult>
<referenceToLCIAMethodDataSet uri="../lciamethods/b53ec18f-7377-4ad3-86eb-cc3f4f276b2b.xml" type="LCIA method data set" refObjectId="b53ec18f-7377-4ad3-86eb-cc3f4f276b2b">
<common:shortDescription xml:lang="en">Eutrophication potential aquatic freshwater (EP-freshwater)</common:shortDescription>
</referenceToLCIAMethodDataSet>
<common:other>
<epd:referenceToUnitGroupDataSet uri="../unitgroups/0429039d-a61d-4590-ba67-aa4a20a810a1.xml" type="unit group data set" refObjectId="0429039d-a61d-4590-ba67-aa4a20a810a1">
<common:shortDescription xml:lang="en">kg PO_(4)-Äq.</common:shortDescription>
</epd:referenceToUnitGroupDataSet>
<epd:amount epd:module="A1-A3">6.89376225635703E-05</epd:amount>
<epd:amount epd:module="A4">6.35483771830097E-07</epd:amount>
<epd:amount epd:module="A5">3.45140778546707E-06</epd:amount>
<epd:amount epd:module="C1">0</epd:amount>
<epd:amount epd:module="C2">6.76046565776698E-08</epd:amount>
<epd:amount epd:module="C3">0</epd:amount>
<epd:amount epd:module="C4">8.46591873264746E-08</epd:amount>
<epd:amount epd:module="D">-5.66269068161987E-09</epd:amount>
</common:other>
</LCIAResult>
<LCIAResult>
<referenceToLCIAMethodDataSet uri="../lciamethods/b5c619fa-def3-11e6-bf01-fe55135034f3.xml" type="LCIA method data set" refObjectId="b5c619fa-def3-11e6-bf01-fe55135034f3">
<common:shortDescription xml:lang="en">Eutrophication potential aquatic marine (EP-marine)</common:shortDescription>
</referenceToLCIAMethodDataSet>
<common:other>
<epd:referenceToUnitGroupDataSet uri="../unitgroups/d05bb823-ecdf-4686-8c40-bf1d9257859f.xml" type="unit group data set" refObjectId="d05bb823-ecdf-4686-8c40-bf1d9257859f">
<common:shortDescription xml:lang="en">kg N-Äq.</common:shortDescription>
</epd:referenceToUnitGroupDataSet>
<epd:amount epd:module="A1-A3">0.00301200170363847</epd:amount>
<epd:amount epd:module="A4">0.000143613649636156</epd:amount>
<epd:amount epd:module="A5">0.000155759452660726</epd:amount>
<epd:amount epd:module="C1">0</epd:amount>
<epd:amount epd:module="C2">1.52780478336336E-05</epd:amount>
<epd:amount epd:module="C3">0</epd:amount>
<epd:amount epd:module="C4">9.1023218879338E-05</epd:amount>
<epd:amount epd:module="D">-3.00878404022698E-06</epd:amount>
</common:other>
</LCIAResult>
<LCIAResult>
<referenceToLCIAMethodDataSet uri="../lciamethods/b5c614d2-def3-11e6-bf01-fe55135034f3.xml" type="LCIA method data set" refObjectId="b5c614d2-def3-11e6-bf01-fe55135034f3">
<common:shortDescription xml:lang="en">Eutrophication potential terrestrial (EP-terrestrial)</common:shortDescription>
</referenceToLCIAMethodDataSet>
<common:other>
<epd:referenceToUnitGroupDataSet uri="../unitgroups/71b4d617-0ec9-4d3f-b65e-e438940c2401.xml" type="unit group data set" refObjectId="71b4d617-0ec9-4d3f-b65e-e438940c2401">
<common:shortDescription xml:lang="en">mol N-Äq.</common:shortDescription>
</epd:referenceToUnitGroupDataSet>
<epd:amount epd:module="A1-A3">0.0333650842229374</epd:amount>
<epd:amount epd:module="A4">0.00164142466528227</epd:amount>
<epd:amount epd:module="A5">0.00173182726176972</epd:amount>
<epd:amount epd:module="C1">0</epd:amount>
<epd:amount epd:module="C2">0.000174619645242795</epd:amount>
<epd:amount epd:module="C3">0</epd:amount>
<epd:amount epd:module="C4">0.0010001902667828</epd:amount>
<epd:amount epd:module="D">-3.20076843748016E-05</epd:amount>
</common:other>
</LCIAResult>
<LCIAResult>
<referenceToLCIAMethodDataSet uri="../lciamethods/b5c610fe-def3-11e6-bf01-fe55135034f3.xml" type="LCIA method data set" refObjectId="b5c610fe-def3-11e6-bf01-fe55135034f3">
<common:shortDescription xml:lang="en">Formation potential of tropospheric ozone photochemical oxidants (POCP)</common:shortDescription>
</referenceToLCIAMethodDataSet>
<common:other>
<epd:referenceToUnitGroupDataSet uri="../unitgroups/d27c25f8-fbc1-44c6-b47b-4adbae4199c6.xml" type="unit group data set" refObjectId="d27c25f8-fbc1-44c6-b47b-4adbae4199c6">
<common:shortDescription xml:lang="en">kg NMVOC-Äq.</common:shortDescription>
</epd:referenceToUnitGroupDataSet>
<epd:amount epd:module="A1-A3">0.00601425290160131</epd:amount>
<epd:amount epd:module="A4">0.000278894482869317</epd:amount>
<epd:amount epd:module="A5">0.000316306618219443</epd:amount>
<epd:amount epd:module="C1">0</epd:amount>
<epd:amount epd:module="C2">2.96696258371614E-05</epd:amount>
<epd:amount epd:module="C3">0</epd:amount>
<epd:amount epd:module="C4">0.000275642597389722</epd:amount>
<epd:amount epd:module="D">-8.59400509789987E-06</epd:amount>
</common:other>
</LCIAResult>
<LCIAResult>
<referenceToLCIAMethodDataSet uri="../lciamethods/b2ad6494-c78d-11e6-9d9d-cec0c932ce01.xml" type="LCIA method data set" refObjectId="b2ad6494-c78d-11e6-9d9d-cec0c932ce01">
<common:shortDescription xml:lang="en">Abiotic depletion potential for non fossil resources (ADPE)</common:shortDescription>
</referenceToLCIAMethodDataSet>
<common:other>
<epd:referenceToUnitGroupDataSet uri="../unitgroups/54ccd2d9-a32a-4fc2-923d-f2c8c93e89d4.xml" type="unit group data set" refObjectId="54ccd2d9-a32a-4fc2-923d-f2c8c93e89d4">
<common:shortDescription xml:lang="en">kg Sb-Äq.</common:shortDescription>
</epd:referenceToUnitGroupDataSet>
<epd:amount epd:module="A1-A3">4.08904637139366E-07</epd:amount>
<epd:amount epd:module="A4">8.6296466256809E-09</epd:amount>
<epd:amount epd:module="A5">2.06985510142299E-08</epd:amount>
<epd:amount epd:module="C1">0</epd:amount>
<epd:amount epd:module="C2">9.18047513370309E-10</epd:amount>
<epd:amount epd:module="C3">0</epd:amount>
<epd:amount epd:module="C4">4.4263032290273E-09</epd:amount>
<epd:amount epd:module="D">-1.22683758594474E-09</epd:amount>
</common:other>
</LCIAResult>
<LCIAResult>
<referenceToLCIAMethodDataSet uri="../lciamethods/b2ad6110-c78d-11e6-9d9d-cec0c932ce01.xml" type="LCIA method data set" refObjectId="b2ad6110-c78d-11e6-9d9d-cec0c932ce01">
<common:shortDescription xml:lang="en">Abiotic depletion potential for fossil resources (ADPF)</common:shortDescription>
</referenceToLCIAMethodDataSet>
<common:other>
<epd:referenceToUnitGroupDataSet uri="../unitgroups/93a60a57-a3c8-11da-a746-0800200c9a66.xml" type="unit group data set" refObjectId="93a60a57-a3c8-11da-a746-0800200c9a66">
<common:shortDescription xml:lang="en">MJ</common:shortDescription>
</epd:referenceToUnitGroupDataSet>
<epd:amount epd:module="A1-A3">74.0108542699163</epd:amount>
<epd:amount epd:module="A4">1.19099246212747</epd:amount>
<epd:amount epd:module="A5">3.73639649236873</epd:amount>
<epd:amount epd:module="C1">0</epd:amount>
<epd:amount epd:module="C2">0.126701325758242</epd:amount>
<epd:amount epd:module="C3">0</epd:amount>
<epd:amount epd:module="C4">0.646721093211453</epd:amount>
<epd:amount epd:module="D">-0.25762139009758</epd:amount>
</common:other>
</LCIAResult>
<LCIAResult>
<referenceToLCIAMethodDataSet uri="../lciamethods/b2ad66ce-c78d-11e6-9d9d-cec0c932ce01.xml" type="LCIA method data set" refObjectId="b2ad66ce-c78d-11e6-9d9d-cec0c932ce01">
<common:shortDescription xml:lang="en">Water use (WDP)</common:shortDescription>
</referenceToLCIAMethodDataSet>
<common:other>
<epd:referenceToUnitGroupDataSet uri="../unitgroups/6ae2df01-888e-46c8-b17d-49fa3869b476.xml" type="unit group data set" refObjectId="6ae2df01-888e-46c8-b17d-49fa3869b476">
<common:shortDescription xml:lang="en">m^(3) world-Äq. deprived</common:shortDescription>
</epd:referenceToUnitGroupDataSet>
<epd:amount epd:module="A1-A3">0.13666418641677</epd:amount>
<epd:amount epd:module="A4">0.00135706431441161</epd:amount>
<epd:amount epd:module="A5">0.00976395324314727</epd:amount>
<epd:amount epd:module="C1">0</epd:amount>
<epd:amount epd:module="C2">0.000144368544086339</epd:amount>
<epd:amount epd:module="C3">0</epd:amount>
<epd:amount epd:module="C4">0.00516660645239393</epd:amount>
<epd:amount epd:module="D">-0.000551694385854062</epd:amount>
</common:other>
</LCIAResult>
<LCIAResult>
<referenceToLCIAMethodDataSet uri="../lciamethods/b5c602c6-def3-11e6-bf01-fe55135034f3.xml" type="LCIA method data set" refObjectId="b5c602c6-def3-11e6-bf01-fe55135034f3">
<common:shortDescription xml:lang="en">Incidence of disease due to PM emissions (PM)</common:shortDescription>
</referenceToLCIAMethodDataSet>
<common:other>
<epd:referenceToUnitGroupDataSet uri="../unitgroups/3883559b-648f-4afc-8ba2-0bd24f3affa3.xml" type="unit group data set" refObjectId="3883559b-648f-4afc-8ba2-0bd24f3affa3">
<common:shortDescription xml:lang="en">Disease incidence</common:shortDescription>
</epd:referenceToUnitGroupDataSet>
<epd:amount epd:module="A1-A3">1.08205894031203E-07</epd:amount>
<epd:amount epd:module="A4">1.92193205592905E-09</epd:amount>
<epd:amount epd:module="A5">5.64647999383121E-09</epd:amount>
<epd:amount epd:module="C1">0</epd:amount>
<epd:amount epd:module="C2">2.04460857013729E-10</epd:amount>
<epd:amount epd:module="C3">0</epd:amount>
<epd:amount epd:module="C4">4.37798835100832E-09</epd:amount>
<epd:amount epd:module="D">-7.06735137965751E-11</epd:amount>
</common:other>
</LCIAResult>
<LCIAResult>
<referenceToLCIAMethodDataSet uri="../lciamethods/b5c632be-def3-11e6-bf01-fe55135034f3.xml" type="LCIA method data set" refObjectId="b5c632be-def3-11e6-bf01-fe55135034f3">
<common:shortDescription xml:lang="en">Human exposure efficiency relative to U235 (IR)</common:shortDescription>
</referenceToLCIAMethodDataSet>
<common:other>
<epd:referenceToUnitGroupDataSet uri="../unitgroups/456b05bf-1415-44a9-9993-02452f554c09.xml" type="unit group data set" refObjectId="456b05bf-1415-44a9-9993-02452f554c09">
<common:shortDescription xml:lang="en">kBq U235-Äq.</common:shortDescription>
</epd:referenceToUnitGroupDataSet>
<epd:amount epd:module="A1-A3">1.03651942298536</epd:amount>
<epd:amount epd:module="A4">0.00133639836524542</epd:amount>
<epd:amount epd:module="A5">0.0518963154613197</epd:amount>
<epd:amount epd:module="C1">0</epd:amount>
<epd:amount epd:module="C2">0.000142170038855896</epd:amount>
<epd:amount epd:module="C3">0</epd:amount>
<epd:amount epd:module="C4">0.000755229621593912</epd:amount>
<epd:amount epd:module="D">-0.011885162876702</epd:amount>
</common:other>
</LCIAResult>
<LCIAResult>
<referenceToLCIAMethodDataSet uri="../lciamethods/ee1082d1-b0f7-43ca-a1f0-21e2a4a74511.xml" type="LCIA method data set" refObjectId="ee1082d1-b0f7-43ca-a1f0-21e2a4a74511">
<common:shortDescription xml:lang="en">Comparative toxic unit for ecosystems (ETP-fw)</common:shortDescription>
</referenceToLCIAMethodDataSet>
<common:other>
<epd:referenceToUnitGroupDataSet uri="../unitgroups/aa959ded-f1eb-4efb-9c5c-2d60be36b3e6.xml" type="unit group data set" refObjectId="aa959ded-f1eb-4efb-9c5c-2d60be36b3e6">
<common:shortDescription xml:lang="en">CTUe</common:shortDescription>
</epd:referenceToUnitGroupDataSet>
<epd:amount epd:module="A1-A3">23.9393382709841</epd:amount>
<epd:amount epd:module="A4">0.987386754740411</epd:amount>
<epd:amount epd:module="A5">1.21705019087016</epd:amount>
<epd:amount epd:module="C1">0</epd:amount>
<epd:amount epd:module="C2">0.10504114412132</epd:amount>
<epd:amount epd:module="C3">0</epd:amount>
<epd:amount epd:module="C4">0.369529111021925</epd:amount>
<epd:amount epd:module="D">-0.068584535408613</epd:amount>
</common:other>
</LCIAResult>
<LCIAResult>
<referenceToLCIAMethodDataSet uri="../lciamethods/2299222a-bbd8-474f-9d4f-4dd1f18aea7c.xml" type="LCIA method data set" refObjectId="2299222a-bbd8-474f-9d4f-4dd1f18aea7c">
<common:shortDescription xml:lang="en">Comparative toxic unit for humans (carcinogenic) (HTP-c)</common:shortDescription>
</referenceToLCIAMethodDataSet>
<common:other>
<epd:referenceToUnitGroupDataSet uri="../unitgroups/d4c9523e-2d7e-49fd-8469-998f547d3a70.xml" type="unit group data set" refObjectId="d4c9523e-2d7e-49fd-8469-998f547d3a70">
<common:shortDescription xml:lang="en">CTUh</common:shortDescription>
</epd:referenceToUnitGroupDataSet>
<epd:amount epd:module="A1-A3">1.29266965559163E-09</epd:amount>
<epd:amount epd:module="A4">2.21270725811122E-11</epd:amount>
<epd:amount epd:module="A5">6.75562308235808E-11</epd:amount>
<epd:amount epd:module="C1">0</epd:amount>
<epd:amount epd:module="C2">2.35394389160768E-12</epd:amount>
<epd:amount epd:module="C3">0</epd:amount>
<epd:amount epd:module="C4">5.4761717544653E-11</epd:amount>
<epd:amount epd:module="D">-1.47409237636533E-12</epd:amount>
</common:other>
</LCIAResult>
<LCIAResult>
<referenceToLCIAMethodDataSet uri="../lciamethods/3af763a5-b7a1-48c9-9cee-1f223481fcef.xml" type="LCIA method data set" refObjectId="3af763a5-b7a1-48c9-9cee-1f223481fcef">
<common:shortDescription xml:lang="en">Comparative toxic unit for humans (noncarcinogenic) (HTP-nc)</common:shortDescription>
</referenceToLCIAMethodDataSet>
<common:other>
<epd:referenceToUnitGroupDataSet uri="../unitgroups/d4c9523e-2d7e-49fd-8469-998f547d3a70.xml" type="unit group data set" refObjectId="d4c9523e-2d7e-49fd-8469-998f547d3a70">
<common:shortDescription xml:lang="en">CTUh</common:shortDescription>
</epd:referenceToUnitGroupDataSet>
<epd:amount epd:module="A1-A3">3.39509043953425E-08</epd:amount>
<epd:amount epd:module="A4">1.43031847137717E-09</epd:amount>
<epd:amount epd:module="A5">2.00490586668877E-09</epd:amount>
<epd:amount epd:module="C1">0</epd:amount>
<epd:amount epd:module="C2">1.5216153950821E-10</epd:amount>
<epd:amount epd:module="C3">0</epd:amount>
<epd:amount epd:module="C4">6.03273503411166E-09</epd:amount>
<epd:amount epd:module="D">-5.42131305765975E-11</epd:amount>
</common:other>
</LCIAResult>
<LCIAResult>
<referenceToLCIAMethodDataSet uri="../lciamethods/b2ad6890-c78d-11e6-9d9d-cec0c932ce01.xml" type="LCIA method data set" refObjectId="b2ad6890-c78d-11e6-9d9d-cec0c932ce01">
<common:shortDescription xml:lang="en">Soil quality index (SQP)</common:shortDescription>
</referenceToLCIAMethodDataSet>
<common:other>
<epd:referenceToUnitGroupDataSet uri="../unitgroups/f130951c-e67f-4f7f-8dd4-665de3974e18.xml" type="unit group data set" refObjectId="f130951c-e67f-4f7f-8dd4-665de3974e18">
<common:shortDescription xml:lang="en">SQP</common:shortDescription>
</epd:referenceToUnitGroupDataSet>
<epd:amount epd:module="A1-A3">65.6606946741081</epd:amount>
<epd:amount epd:module="A4">0.845245985129872</epd:amount>
<epd:amount epd:module="A5">3.29077404751209</epd:amount>
<epd:amount epd:module="C1">0</epd:amount>
<epd:amount epd:module="C2">0.0899197856521146</epd:amount>
<epd:amount epd:module="C3">0</epd:amount>
<epd:amount epd:module="C4">0.134820667079778</epd:amount>
<epd:amount epd:module="D">-0.0128357532524181</epd:amount>
</common:other>
</LCIAResult>
</LCIAResults>
</processDataSet>