<?xml version="1.0" encoding="utf-8"?>
<processDataSet xmlns:epd="http://www.iai.kit.edu/EPD/2013" xmlns:epd2="http://www.indata.network/EPD/2019" xmlns:common="http://lca.jrc.it/ILCD/Common" xsi:schemaLocation="http://lca.jrc.it/ILCD/Process ../../schemas/EPD_DataSet.xsd" epd2:epd-version="1.2" version="1.1" locations="../ILCDLocations.xml" xmlns:xsi="http://www.w3.org/2001/XMLSchema-instance" xmlns="http://lca.jrc.it/ILCD/Process">
<processInformation>
<dataSetInformation>
<common:UUID>ada6f16c-96d9-48a3-a5fd-80f03fb45025</common:UUID>
<name>
<baseName xml:lang="en">AF/ArmaFlex insulation for industrial and building installation</baseName>
<functionalUnitFlowProperties xml:lang="en" />
</name>
<classificationInformation>
<common:classification name="OEKOBAU.DAT">
<common:class level="0" classId="2">Dämmstoffe</common:class>
<common:class level="1" classId="2.19">Kautschuk</common:class>
<common:class level="2" classId="2.19.01">Schaum</common:class>
</common:classification>
<common:classification name="IBUCategories">
<common:class level="0">02 Building products</common:class>
<common:class level="1">Thermal insulation products</common:class>
<common:class level="2">Insulating materials made of foam plastics</common:class>
</common:classification>
</classificationInformation>
<common:generalComment xml:lang="en">AF/ArmaFlex is the professional, highly-flexible, closed-cell elastomeric foam insulation (FEF) for continuous energy saving and condensation control purposes. The combination of very low thermal conductivity and extremely high resistance to water vapour transmission prevents long-term energy losses and water vapour ingress and reduces the risk of corrosion under insulation.</common:generalComment>
</dataSetInformation>
<quantitativeReference>
<referenceToReferenceFlow>0</referenceToReferenceFlow>
</quantitativeReference>
<time>
<common:referenceYear>2021</common:referenceYear>
<common:dataSetValidUntil>2026</common:dataSetValidUntil>
<common:other>
<epd2:publicationDateOfEPD>2021-03-12</epd2:publicationDateOfEPD>
</common:other>
</time>
<geography>
<locationOfOperationSupplyOrProduction location="RER" />
</geography>
<technology>
<technologyDescriptionAndIncludedProcesses xml:lang="en">ArmaFlex products are manufactured in a pressureless, continuous and discontinuous production process. In the first step, a homogenous compound is produced with rubber, additives, ancillary materials, blowing and vulcanization agents. This is done on the rolling mill or in the internal mixer followed by the rolling mill. Rubber extruders are used to process the compounds to produce raw profiles with defined dimensions. Here exact compliance with the dimensions for the raw profile is crucial for the dimensional accuracy of the foamed product. In the case of the discontinuous, pressureless production process, the raw profiles are cut to length and then foamed in a hot-air oven. In the case of the continuous, pressureless process, the extruded profile is fed directly onto a vulcanization line whose energy source may be hot air, for example. In foam production, vulcanization and blowing processes run alongside each other. Both reactions are regulated by temperature control. Recipe and temperature control determine the properties of the foam. Quality assurance: EC Certificate of conformity no. 0543 of the Gütegemeinschaft Hartschaum e.V. Celle. Quality management system in accordance with EN ISO 9001. 
Declared unit: 
The declaration refers to 1 m³ insulation product. For the LCA calculations the average density per product brand is used. As additional information and support for installers the thermal conductivity coefficient (lambda-value) and R-value per 20 cm thickness per product brand are given.</technologyDescriptionAndIncludedProcesses>
<technologicalApplicability xml:lang="en">AF/ArmaFlex is used to insulate pipes, air ducts and vessels including fittings and flanges of industrial installations and building equipment.Condensation control, energy saving and noise control in refrigeration and air conditioning equipment and process plants.Energy saving according to local energy- saving laws, prevention of heat loss and noise reduction of heating and plumbing systems.Condensation control and noise reduction in service-water and waste-water systems. Condensation control, energy saving and noise control in refrigeration and air- conditioning equipment in the ship-building sector.</technologicalApplicability>
</technology>
</processInformation>
<modellingAndValidation>
<LCIMethodAndAllocation>
<typeOfDataSet>EPD</typeOfDataSet>
<referenceToLCAMethodDetails type="source data set" refObjectId="8749df65-b86a-42d3-8a1c-cbedf118dcd8">
<common:shortDescription xml:lang="en">Insulating materials made of foam plastics.pdf</common:shortDescription>
</referenceToLCAMethodDetails>
<common:other>
<epd:subType xmlns="http://www.iai.kit.edu/EPD/2013">average dataset</epd:subType>
</common:other>
</LCIMethodAndAllocation>
<dataSourcesTreatmentAndRepresentativeness>
<referenceToDataSource type="source data set" refObjectId="28d74cc0-db8b-4d7e-bc44-5f6d56ce0c4a">
<common:shortDescription xml:lang="en">GaBi Database (all versions)</common:shortDescription>
</referenceToDataSource>
<referenceToDataSource type="source data set" refObjectId="0115289e-52f0-4920-bc7e-57b1c96aec8d">
<common:shortDescription xml:lang="en">GaBi database SP40 2020</common:shortDescription>
</referenceToDataSource>
<useAdviceForDataSet xml:lang="en">Scope: 
Product line AF/ArmaFlex  Insulation material for industrial and building installations vulcanized in tubes and sheets. This declaration is an Environmental Product Declaration according to ISO 14025  describing the average environmental performance of the product produced in Germany, Spain and Poland. The average has been calculated based on site specific annual production volumes.  As the installation of the product is not restricted to countries where the products have been produced the validity of this EPD is considered at least EU wide. 
System boundary: 
The data collection refers to the yearly production in 2019. The following life cycle stages are considered: Type of EPD: Cradle-to-Gate with options.Production A1-A3:       The LCA calculation covers the production of the raw materials (supply chain – A1), the mixing of raw materials according to the respective recipes (MasterBatch) exclusively done in Münster, Germany, the transport (A2) of the MasterBatches to the production facility for foaming and the foaming process (A3) in Germany, Spain, Poland or Great Britain, including the packaging material. Transport A4:   Average values for the transport from factory gate to construction site are assumed. Installation A5:             The installation considers the production of off-cuts, incineration of these off-cuts and the disposal scenario for the packaging material. Auxiliaries like adhesives or tapes or energy for installation are not considered. End-of-life C2, C3:      An incineration scenario for the used and demolished product, including an assumption for the transport to disposal, is covered. Benefits for the next product system D:        Credits for electrical and thermal energy resulting from the waste incineration process of the off-cut material and packaging (A5) and the product (C3) are declared in module D.</useAdviceForDataSet>
<common:other>
<epd2:referenceToOriginalEPD type="source data set" refObjectId="ad176212-8f47-46c7-8dc9-1e4f8569b489">
<common:shortDescription xml:lang="en">AF/ArmaFlex insulation for industrial and building installation.pdf</common:shortDescription>
</epd2:referenceToOriginalEPD>
</common:other>
</dataSourcesTreatmentAndRepresentativeness>
<validation>
<review type="Accredited third party review">
<common:referenceToNameOfReviewerAndInstitution uri="../contacts/d111dbec-b024-4be5-86c5-752d6eb2cf95.xml" type="contact data set" refObjectId="d111dbec-b024-4be5-86c5-752d6eb2cf95">
<common:shortDescription xml:lang="en">Institut Bauen und Umwelt e. V.</common:shortDescription>
</common:referenceToNameOfReviewerAndInstitution>
</review>
</validation>
<complianceDeclarations>
<compliance>
<common:referenceToComplianceSystem uri="../sources/c0016b33-8cf7-415c-ac6e-deba0d21440d.xml" type="source data set" refObjectId="c0016b33-8cf7-415c-ac6e-deba0d21440d">
<common:shortDescription xml:lang="en">DIN EN 15804+A2</common:shortDescription>
</common:referenceToComplianceSystem>
</compliance>
<compliance>
<common:referenceToComplianceSystem uri="../sources/4f2eb655-6e44-4874-a95a-e28f5442cd4d.xml" type="source data set" refObjectId="4f2eb655-6e44-4874-a95a-e28f5442cd4d">
<common:shortDescription xml:lang="en">ISO 14025</common:shortDescription>
</common:referenceToComplianceSystem>
</compliance>
</complianceDeclarations>
</modellingAndValidation>
<administrativeInformation>
<common:commissionerAndGoal>
<common:referenceToCommissioner uri="../contacts/18c28240-f641-4369-863f-867fe05620be.xml" type="contact data set" refObjectId="18c28240-f641-4369-863f-867fe05620be">
<common:shortDescription xml:lang="en">Armacell GmbH</common:shortDescription>
</common:referenceToCommissioner>
</common:commissionerAndGoal>
<dataGenerator>
<common:referenceToPersonOrEntityGeneratingTheDataSet uri="../contacts/623edf96-39d1-4e6f-9892-674c7228546b.xml" type="contact data set" refObjectId="623edf96-39d1-4e6f-9892-674c7228546b">
<common:shortDescription xml:lang="en">Sphera Solutions GmbH</common:shortDescription>
</common:referenceToPersonOrEntityGeneratingTheDataSet>
</dataGenerator>
<dataEntryBy>
<common:timeStamp>2021-03-12T18:01:28.309</common:timeStamp>
<common:referenceToDataSetFormat uri="../sources/a97a0155-0234-4b87-b4ce-a45da52f2a40.xml" type="source data set" refObjectId="a97a0155-0234-4b87-b4ce-a45da52f2a40">
<common:shortDescription xml:lang="en">ILCD Format</common:shortDescription>
</common:referenceToDataSetFormat>
<common:referenceToDataSetFormat uri="../sources/a29449fd-aa2f-4de8-b5d7-4b06b43c6fde.xml" type="source data set" refObjectId="a29449fd-aa2f-4de8-b5d7-4b06b43c6fde">
<common:shortDescription xml:lang="de">EPD-Datenformaterweiterungen v1.2</common:shortDescription>
<common:shortDescription xml:lang="en">EPD Data Format Extensions v1.2</common:shortDescription>
</common:referenceToDataSetFormat>
</dataEntryBy>
<publicationAndOwnership>
<common:dataSetVersion>00.02.000</common:dataSetVersion>
<common:referenceToPrecedingDataSetVersion uri="../processes/586187c4-0ab9-4286-b91c-1b06c863b435.xml" type="process data set" refObjectId="586187c4-0ab9-4286-b91c-1b06c863b435">
<common:shortDescription xml:lang="en">AF/Armaflex insulation for industrial and building installation</common:shortDescription>
</common:referenceToPrecedingDataSetVersion>
<common:referenceToRegistrationAuthority uri="../contacts/d111dbec-b024-4be5-86c5-752d6eb2cf95.xml" type="contact data set" refObjectId="d111dbec-b024-4be5-86c5-752d6eb2cf95">
<common:shortDescription xml:lang="en">Institut Bauen und Umwelt e. V.</common:shortDescription>
</common:referenceToRegistrationAuthority>
<common:registrationNumber>EPD-ARM-20200219-IBB1-EN</common:registrationNumber>
<common:referenceToOwnershipOfDataSet uri="../contacts/18c28240-f641-4369-863f-867fe05620be.xml" type="contact data set" refObjectId="18c28240-f641-4369-863f-867fe05620be">
<common:shortDescription xml:lang="en">Armacell GmbH</common:shortDescription>
</common:referenceToOwnershipOfDataSet>
<common:copyright>true</common:copyright>
<common:licenseType>Free of charge for all users and uses</common:licenseType>
<common:accessRestrictions xml:lang="en">None</common:accessRestrictions>
<common:other>
<epd2:referenceToPublisher type="contact data set" refObjectId="d111dbec-b024-4be5-86c5-752d6eb2cf95" uri="../contacts/d111dbec-b024-4be5-86c5-752d6eb2cf95.xml">
<common:shortDescription xml:lang="en">Institut Bauen und Umwelt e. V.</common:shortDescription>
</epd2:referenceToPublisher>
</common:other>
</publicationAndOwnership>
</administrativeInformation>
<exchanges>
<exchange dataSetInternalID="0">
<referenceToFlowDataSet uri="../flows/2e83aa56-a0d4-1e77-0a4f-8c8b702c43c7.xml" type="flow data set" refObjectId="2e83aa56-a0d4-1e77-0a4f-8c8b702c43c7">
<common:shortDescription xml:lang="en"> AF/ArmaFlex insulation for industrial and building installation ( AF/ArmaFlex insulation for industrial and building installation)</common:shortDescription>
</referenceToFlowDataSet>
<meanAmount>1</meanAmount>
<referencesToDataSource />
</exchange>
<exchange dataSetInternalID="1">
<referenceToFlowDataSet uri="../flows/20f32be5-0398-4288-9b6d-accddd195317.xml" type="flow data set" refObjectId="20f32be5-0398-4288-9b6d-accddd195317">
<common:shortDescription xml:lang="en">Renewable primary energy as energy carrier (PERE)</common:shortDescription>
</referenceToFlowDataSet>
<functionType>General reminder flow</functionType>
<exchangeDirection>Input</exchangeDirection>
<common:other>
<epd:referenceToUnitGroupDataSet uri="../unitgroups/93a60a57-a3c8-11da-a746-0800200c9a66.xml" type="unit group data set" refObjectId="93a60a57-a3c8-11da-a746-0800200c9a66">
<common:shortDescription xml:lang="en">MJ</common:shortDescription>
</epd:referenceToUnitGroupDataSet>
<epd:amount epd:module="A1-A3">1585.85</epd:amount>
<epd:amount epd:module="A4">2.84</epd:amount>
<epd:amount epd:module="A5">122.25</epd:amount>
<epd:amount epd:module="C2">0.186</epd:amount>
<epd:amount epd:module="C3">52.1</epd:amount>
<epd:amount epd:module="D">-141</epd:amount>
</common:other>
</exchange>
<exchange dataSetInternalID="2">
<referenceToFlowDataSet uri="../flows/fb3ec0de-548d-4508-aea5-00b73bf6f702.xml" type="flow data set" refObjectId="fb3ec0de-548d-4508-aea5-00b73bf6f702">
<common:shortDescription xml:lang="en">Renewable primary energy resources as material utilization (PERM)</common:shortDescription>
</referenceToFlowDataSet>
<functionType>General reminder flow</functionType>
<exchangeDirection>Input</exchangeDirection>
<common:other>
<epd:referenceToUnitGroupDataSet uri="../unitgroups/93a60a57-a3c8-11da-a746-0800200c9a66.xml" type="unit group data set" refObjectId="93a60a57-a3c8-11da-a746-0800200c9a66">
<common:shortDescription xml:lang="en">MJ</common:shortDescription>
</epd:referenceToUnitGroupDataSet>
<epd:amount epd:module="A1-A3">104.15</epd:amount>
<epd:amount epd:module="A4">0</epd:amount>
<epd:amount epd:module="A5">-104.15</epd:amount>
<epd:amount epd:module="C2">0</epd:amount>
<epd:amount epd:module="C3">0</epd:amount>
<epd:amount epd:module="D">0</epd:amount>
</common:other>
</exchange>
<exchange dataSetInternalID="3">
<referenceToFlowDataSet uri="../flows/53f97275-fa8a-4cdd-9024-65936002acd0.xml" type="flow data set" refObjectId="53f97275-fa8a-4cdd-9024-65936002acd0">
<common:shortDescription xml:lang="en">Total use of renewable primary energy resources (PERT)</common:shortDescription>
</referenceToFlowDataSet>
<functionType>General reminder flow</functionType>
<exchangeDirection>Input</exchangeDirection>
<common:other>
<epd:referenceToUnitGroupDataSet uri="../unitgroups/93a60a57-a3c8-11da-a746-0800200c9a66.xml" type="unit group data set" refObjectId="93a60a57-a3c8-11da-a746-0800200c9a66">
<common:shortDescription xml:lang="en">MJ</common:shortDescription>
</epd:referenceToUnitGroupDataSet>
<epd:amount epd:module="A1-A3">1690</epd:amount>
<epd:amount epd:module="A4">2.84</epd:amount>
<epd:amount epd:module="A5">18.1</epd:amount>
<epd:amount epd:module="C2">0.186</epd:amount>
<epd:amount epd:module="C3">52.1</epd:amount>
<epd:amount epd:module="D">-141</epd:amount>
</common:other>
</exchange>
<exchange dataSetInternalID="4">
<referenceToFlowDataSet uri="../flows/ac857178-2b45-46ec-892a-a9a4332f0372.xml" type="flow data set" refObjectId="ac857178-2b45-46ec-892a-a9a4332f0372">
<common:shortDescription xml:lang="en">Non renewable primary energy as energy carrier (PENRE)</common:shortDescription>
</referenceToFlowDataSet>
<functionType>General reminder flow</functionType>
<exchangeDirection>Input</exchangeDirection>
<common:other>
<epd:referenceToUnitGroupDataSet uri="../unitgroups/93a60a57-a3c8-11da-a746-0800200c9a66.xml" type="unit group data set" refObjectId="93a60a57-a3c8-11da-a746-0800200c9a66">
<common:shortDescription xml:lang="en">MJ</common:shortDescription>
</epd:referenceToUnitGroupDataSet>
<epd:amount epd:module="A1-A3">3514.84</epd:amount>
<epd:amount epd:module="A4">50.5</epd:amount>
<epd:amount epd:module="A5">57.91</epd:amount>
<epd:amount epd:module="C2">3.32</epd:amount>
<epd:amount epd:module="C3">1148.75</epd:amount>
<epd:amount epd:module="D">-646</epd:amount>
</common:other>
</exchange>
<exchange dataSetInternalID="5">
<referenceToFlowDataSet uri="../flows/1421caa0-679d-4bf4-b282-0eb850ccae27.xml" type="flow data set" refObjectId="1421caa0-679d-4bf4-b282-0eb850ccae27">
<common:shortDescription xml:lang="en">Non renewable primary energy as material utilization (PENRM)</common:shortDescription>
</referenceToFlowDataSet>
<functionType>General reminder flow</functionType>
<exchangeDirection>Input</exchangeDirection>
<common:other>
<epd:referenceToUnitGroupDataSet uri="../unitgroups/93a60a57-a3c8-11da-a746-0800200c9a66.xml" type="unit group data set" refObjectId="93a60a57-a3c8-11da-a746-0800200c9a66">
<common:shortDescription xml:lang="en">MJ</common:shortDescription>
</epd:referenceToUnitGroupDataSet>
<epd:amount epd:module="A1-A3">905.16</epd:amount>
<epd:amount epd:module="A4">0</epd:amount>
<epd:amount epd:module="A5">-7.41</epd:amount>
<epd:amount epd:module="C2">0</epd:amount>
<epd:amount epd:module="C3">-897.75</epd:amount>
<epd:amount epd:module="D">0</epd:amount>
</common:other>
</exchange>
<exchange dataSetInternalID="6">
<referenceToFlowDataSet uri="../flows/06159210-646b-4c8d-8583-da9b3b95a6c1.xml" type="flow data set" refObjectId="06159210-646b-4c8d-8583-da9b3b95a6c1">
<common:shortDescription xml:lang="en">Total use of non renewable primary energy resources (PENRT)</common:shortDescription>
</referenceToFlowDataSet>
<functionType>General reminder flow</functionType>
<exchangeDirection>Input</exchangeDirection>
<common:other>
<epd:referenceToUnitGroupDataSet uri="../unitgroups/93a60a57-a3c8-11da-a746-0800200c9a66.xml" type="unit group data set" refObjectId="93a60a57-a3c8-11da-a746-0800200c9a66">
<common:shortDescription xml:lang="en">MJ</common:shortDescription>
</epd:referenceToUnitGroupDataSet>
<epd:amount epd:module="A1-A3">4420</epd:amount>
<epd:amount epd:module="A4">50.5</epd:amount>
<epd:amount epd:module="A5">50.5</epd:amount>
<epd:amount epd:module="C2">3.32</epd:amount>
<epd:amount epd:module="C3">251</epd:amount>
<epd:amount epd:module="D">-646</epd:amount>
</common:other>
</exchange>
<exchange dataSetInternalID="7">
<referenceToFlowDataSet uri="../flows/c6a1f35f-2d09-4f54-8dfb-97e502e1ce92.xml" type="flow data set" refObjectId="c6a1f35f-2d09-4f54-8dfb-97e502e1ce92">
<common:shortDescription xml:lang="en">Use of secondary material (SM)</common:shortDescription>
</referenceToFlowDataSet>
<functionType>General reminder flow</functionType>
<exchangeDirection>Input</exchangeDirection>
<common:other>
<epd:referenceToUnitGroupDataSet uri="../unitgroups/ad38d542-3fe9-439d-9b95-2f5f7752acaf.xml" type="unit group data set" refObjectId="ad38d542-3fe9-439d-9b95-2f5f7752acaf">
<common:shortDescription xml:lang="en">kg</common:shortDescription>
</epd:referenceToUnitGroupDataSet>
<epd:amount epd:module="A1-A3">47.22</epd:amount>
<epd:amount epd:module="A4">0</epd:amount>
<epd:amount epd:module="A5">0</epd:amount>
<epd:amount epd:module="C2">0</epd:amount>
<epd:amount epd:module="C3">0</epd:amount>
<epd:amount epd:module="D">0</epd:amount>
</common:other>
</exchange>
<exchange dataSetInternalID="8">
<referenceToFlowDataSet uri="../flows/64333088-a55f-4aa2-9a31-c10b07816787.xml" type="flow data set" refObjectId="64333088-a55f-4aa2-9a31-c10b07816787">
<common:shortDescription xml:lang="en">Use of renewable secondary fuels (RSF)</common:shortDescription>
</referenceToFlowDataSet>
<functionType>General reminder flow</functionType>
<exchangeDirection>Input</exchangeDirection>
<common:other>
<epd:referenceToUnitGroupDataSet uri="../unitgroups/93a60a57-a3c8-11da-a746-0800200c9a66.xml" type="unit group data set" refObjectId="93a60a57-a3c8-11da-a746-0800200c9a66">
<common:shortDescription xml:lang="en">MJ</common:shortDescription>
</epd:referenceToUnitGroupDataSet>
<epd:amount epd:module="A1-A3">0</epd:amount>
<epd:amount epd:module="A4">0</epd:amount>
<epd:amount epd:module="A5">0</epd:amount>
<epd:amount epd:module="C2">0</epd:amount>
<epd:amount epd:module="C3">0</epd:amount>
<epd:amount epd:module="D">0</epd:amount>
</common:other>
</exchange>
<exchange dataSetInternalID="9">
<referenceToFlowDataSet uri="../flows/89def144-d39a-4287-b86f-efde453ddcb2.xml" type="flow data set" refObjectId="89def144-d39a-4287-b86f-efde453ddcb2">
<common:shortDescription xml:lang="en">Use of non renewable secondary fuels (NRSF)</common:shortDescription>
</referenceToFlowDataSet>
<functionType>General reminder flow</functionType>
<exchangeDirection>Input</exchangeDirection>
<common:other>
<epd:referenceToUnitGroupDataSet uri="../unitgroups/93a60a57-a3c8-11da-a746-0800200c9a66.xml" type="unit group data set" refObjectId="93a60a57-a3c8-11da-a746-0800200c9a66">
<common:shortDescription xml:lang="en">MJ</common:shortDescription>
</epd:referenceToUnitGroupDataSet>
<epd:amount epd:module="A1-A3">0</epd:amount>
<epd:amount epd:module="A4">0</epd:amount>
<epd:amount epd:module="A5">0</epd:amount>
<epd:amount epd:module="C2">0</epd:amount>
<epd:amount epd:module="C3">0</epd:amount>
<epd:amount epd:module="D">0</epd:amount>
</common:other>
</exchange>
<exchange dataSetInternalID="10">
<referenceToFlowDataSet uri="../flows/3cf952c8-f3a4-461d-8c96-96456ca62246.xml" type="flow data set" refObjectId="3cf952c8-f3a4-461d-8c96-96456ca62246">
<common:shortDescription xml:lang="en">Use of net fresh water (FW)</common:shortDescription>
</referenceToFlowDataSet>
<functionType>General reminder flow</functionType>
<exchangeDirection>Input</exchangeDirection>
<common:other>
<epd:referenceToUnitGroupDataSet uri="../unitgroups/cd950537-0a98-4044-9ba7-9f9a68d0a504.xml" type="unit group data set" refObjectId="cd950537-0a98-4044-9ba7-9f9a68d0a504">
<common:shortDescription xml:lang="en">m^3</common:shortDescription>
</epd:referenceToUnitGroupDataSet>
<epd:amount epd:module="A1-A3">1.71</epd:amount>
<epd:amount epd:module="A4">0.00329</epd:amount>
<epd:amount epd:module="A5">0.0564</epd:amount>
<epd:amount epd:module="C2">0.000216</epd:amount>
<epd:amount epd:module="C3">0.276</epd:amount>
<epd:amount epd:module="D">-0.163</epd:amount>
</common:other>
</exchange>
<exchange dataSetInternalID="11">
<referenceToFlowDataSet uri="../flows/430f9e0f-59b2-46a0-8e0d-55e0e84948fc.xml" type="flow data set" refObjectId="430f9e0f-59b2-46a0-8e0d-55e0e84948fc">
<common:shortDescription xml:lang="en">Hazardous waste disposed (HWD)</common:shortDescription>
</referenceToFlowDataSet>
<functionType>General reminder flow</functionType>
<exchangeDirection>Output</exchangeDirection>
<common:other>
<epd:referenceToUnitGroupDataSet uri="../unitgroups/ad38d542-3fe9-439d-9b95-2f5f7752acaf.xml" type="unit group data set" refObjectId="ad38d542-3fe9-439d-9b95-2f5f7752acaf">
<common:shortDescription xml:lang="en">kg</common:shortDescription>
</epd:referenceToUnitGroupDataSet>
<epd:amount epd:module="A1-A3">2.87E-05</epd:amount>
<epd:amount epd:module="A4">2.35E-06</epd:amount>
<epd:amount epd:module="A5">3.29E-07</epd:amount>
<epd:amount epd:module="C2">1.54E-07</epd:amount>
<epd:amount epd:module="C3">1.14E-06</epd:amount>
<epd:amount epd:module="D">-2.57E-07</epd:amount>
</common:other>
</exchange>
<exchange dataSetInternalID="12">
<referenceToFlowDataSet uri="../flows/b29ef66b-e286-4afa-949f-62f1a7b4d7fa.xml" type="flow data set" refObjectId="b29ef66b-e286-4afa-949f-62f1a7b4d7fa">
<common:shortDescription xml:lang="en">Non hazardous waste disposed (NHWD)</common:shortDescription>
</referenceToFlowDataSet>
<functionType>General reminder flow</functionType>
<exchangeDirection>Output</exchangeDirection>
<common:other>
<epd:referenceToUnitGroupDataSet uri="../unitgroups/ad38d542-3fe9-439d-9b95-2f5f7752acaf.xml" type="unit group data set" refObjectId="ad38d542-3fe9-439d-9b95-2f5f7752acaf">
<common:shortDescription xml:lang="en">kg</common:shortDescription>
</epd:referenceToUnitGroupDataSet>
<epd:amount epd:module="A1-A3">24.5</epd:amount>
<epd:amount epd:module="A4">0.00773</epd:amount>
<epd:amount epd:module="A5">1.23</epd:amount>
<epd:amount epd:module="C2">0.000508</epd:amount>
<epd:amount epd:module="C3">83.5</epd:amount>
<epd:amount epd:module="D">-0.298</epd:amount>
</common:other>
</exchange>
<exchange dataSetInternalID="13">
<referenceToFlowDataSet uri="../flows/3449546e-52ad-4b39-b809-9fb77cea8ff6.xml" type="flow data set" refObjectId="3449546e-52ad-4b39-b809-9fb77cea8ff6">
<common:shortDescription xml:lang="en">Radioactive waste disposed (RWD)</common:shortDescription>
</referenceToFlowDataSet>
<functionType>General reminder flow</functionType>
<exchangeDirection>Output</exchangeDirection>
<common:other>
<epd:referenceToUnitGroupDataSet uri="../unitgroups/ad38d542-3fe9-439d-9b95-2f5f7752acaf.xml" type="unit group data set" refObjectId="ad38d542-3fe9-439d-9b95-2f5f7752acaf">
<common:shortDescription xml:lang="en">kg</common:shortDescription>
</epd:referenceToUnitGroupDataSet>
<epd:amount epd:module="A1-A3">0.105</epd:amount>
<epd:amount epd:module="A4">6.25E-05</epd:amount>
<epd:amount epd:module="A5">0.00131</epd:amount>
<epd:amount epd:module="C2">4.11E-06</epd:amount>
<epd:amount epd:module="C3">0.00797</epd:amount>
<epd:amount epd:module="D">-0.048</epd:amount>
</common:other>
</exchange>
<exchange dataSetInternalID="14">
<referenceToFlowDataSet uri="../flows/a2b32f97-3fc7-4af2-b209-525bc6426f33.xml" type="flow data set" refObjectId="a2b32f97-3fc7-4af2-b209-525bc6426f33">
<common:shortDescription xml:lang="en">Components for re-use (CRU)</common:shortDescription>
</referenceToFlowDataSet>
<functionType>General reminder flow</functionType>
<exchangeDirection>Output</exchangeDirection>
<common:other>
<epd:referenceToUnitGroupDataSet uri="../unitgroups/ad38d542-3fe9-439d-9b95-2f5f7752acaf.xml" type="unit group data set" refObjectId="ad38d542-3fe9-439d-9b95-2f5f7752acaf">
<common:shortDescription xml:lang="en">kg</common:shortDescription>
</epd:referenceToUnitGroupDataSet>
<epd:amount epd:module="A1-A3">0</epd:amount>
<epd:amount epd:module="A4">0</epd:amount>
<epd:amount epd:module="A5">0</epd:amount>
<epd:amount epd:module="C2">0</epd:amount>
<epd:amount epd:module="C3">0</epd:amount>
<epd:amount epd:module="D">0</epd:amount>
</common:other>
</exchange>
<exchange dataSetInternalID="15">
<referenceToFlowDataSet uri="../flows/d7fe48a5-4103-49c8-9aae-b0b5dfdbd6ae.xml" type="flow data set" refObjectId="d7fe48a5-4103-49c8-9aae-b0b5dfdbd6ae">
<common:shortDescription xml:lang="en">Materials for recycling (MFR)</common:shortDescription>
</referenceToFlowDataSet>
<functionType>General reminder flow</functionType>
<exchangeDirection>Output</exchangeDirection>
<common:other>
<epd:referenceToUnitGroupDataSet uri="../unitgroups/ad38d542-3fe9-439d-9b95-2f5f7752acaf.xml" type="unit group data set" refObjectId="ad38d542-3fe9-439d-9b95-2f5f7752acaf">
<common:shortDescription xml:lang="en">kg</common:shortDescription>
</epd:referenceToUnitGroupDataSet>
<epd:amount epd:module="A1-A3">0</epd:amount>
<epd:amount epd:module="A4">0</epd:amount>
<epd:amount epd:module="A5">40.2</epd:amount>
<epd:amount epd:module="C2">0</epd:amount>
<epd:amount epd:module="C3">0</epd:amount>
<epd:amount epd:module="D">0</epd:amount>
</common:other>
</exchange>
<exchange dataSetInternalID="16">
<referenceToFlowDataSet uri="../flows/59a9181c-3aaf-46ee-8b13-2b3723b6e447.xml" type="flow data set" refObjectId="59a9181c-3aaf-46ee-8b13-2b3723b6e447">
<common:shortDescription xml:lang="en">Materials for energy recovery (MER)</common:shortDescription>
</referenceToFlowDataSet>
<functionType>General reminder flow</functionType>
<exchangeDirection>Output</exchangeDirection>
<common:other>
<epd:referenceToUnitGroupDataSet uri="../unitgroups/ad38d542-3fe9-439d-9b95-2f5f7752acaf.xml" type="unit group data set" refObjectId="ad38d542-3fe9-439d-9b95-2f5f7752acaf">
<common:shortDescription xml:lang="en">kg</common:shortDescription>
</epd:referenceToUnitGroupDataSet>
<epd:amount epd:module="A1-A3">0</epd:amount>
<epd:amount epd:module="A4">0</epd:amount>
<epd:amount epd:module="A5">0</epd:amount>
<epd:amount epd:module="C2">0</epd:amount>
<epd:amount epd:module="C3">0</epd:amount>
<epd:amount epd:module="D">0</epd:amount>
</common:other>
</exchange>
<exchange dataSetInternalID="17">
<referenceToFlowDataSet uri="../flows/4da0c987-2b76-40d6-9e9e-82a017aaaf29.xml" type="flow data set" refObjectId="4da0c987-2b76-40d6-9e9e-82a017aaaf29">
<common:shortDescription xml:lang="en">Exported electrical energy (EEE)</common:shortDescription>
</referenceToFlowDataSet>
<functionType>General reminder flow</functionType>
<exchangeDirection>Output</exchangeDirection>
<common:other>
<epd:referenceToUnitGroupDataSet uri="../unitgroups/93a60a57-a3c8-11da-a746-0800200c9a66.xml" type="unit group data set" refObjectId="93a60a57-a3c8-11da-a746-0800200c9a66">
<common:shortDescription xml:lang="en">MJ</common:shortDescription>
</epd:referenceToUnitGroupDataSet>
<epd:amount epd:module="A1-A3">0</epd:amount>
<epd:amount epd:module="A4">0</epd:amount>
<epd:amount epd:module="A5">21.9</epd:amount>
<epd:amount epd:module="C2">0</epd:amount>
<epd:amount epd:module="C3">137</epd:amount>
<epd:amount epd:module="D">0</epd:amount>
</common:other>
</exchange>
<exchange dataSetInternalID="18">
<referenceToFlowDataSet uri="../flows/98daf38a-7a79-46d3-9a37-2b7bd0955810.xml" type="flow data set" refObjectId="98daf38a-7a79-46d3-9a37-2b7bd0955810">
<common:shortDescription xml:lang="en">Exported thermal energy (EET)</common:shortDescription>
</referenceToFlowDataSet>
<functionType>General reminder flow</functionType>
<exchangeDirection>Output</exchangeDirection>
<common:other>
<epd:referenceToUnitGroupDataSet uri="../unitgroups/93a60a57-a3c8-11da-a746-0800200c9a66.xml" type="unit group data set" refObjectId="93a60a57-a3c8-11da-a746-0800200c9a66">
<common:shortDescription xml:lang="en">MJ</common:shortDescription>
</epd:referenceToUnitGroupDataSet>
<epd:amount epd:module="A1-A3">0</epd:amount>
<epd:amount epd:module="A4">0</epd:amount>
<epd:amount epd:module="A5">39.4</epd:amount>
<epd:amount epd:module="C2">0</epd:amount>
<epd:amount epd:module="C3">250</epd:amount>
<epd:amount epd:module="D">0</epd:amount>
</common:other>
</exchange>
</exchanges>
<LCIAResults>
<LCIAResult>
<referenceToLCIAMethodDataSet uri="../lciamethods/6a37f984-a4b3-458a-a20a-64418c145fa2.xml" type="LCIA method data set" refObjectId="6a37f984-a4b3-458a-a20a-64418c145fa2">
<common:shortDescription xml:lang="en">Global Warming Potential total (GWP-total)</common:shortDescription>
</referenceToLCIAMethodDataSet>
<common:other>
<epd:referenceToUnitGroupDataSet uri="../unitgroups/1ebf3012-d0db-4de2-aefd-ef30cedb0be1.xml" type="unit group data set" refObjectId="1ebf3012-d0db-4de2-aefd-ef30cedb0be1">
<common:shortDescription xml:lang="en">kg CO_(2)-Äq.</common:shortDescription>
</epd:referenceToUnitGroupDataSet>
<epd:amount epd:module="A1-A3">194</epd:amount>
<epd:amount epd:module="A4">3.82</epd:amount>
<epd:amount epd:module="A5">81.8</epd:amount>
<epd:amount epd:module="C2">0.25</epd:amount>
<epd:amount epd:module="C3">136</epd:amount>
<epd:amount epd:module="D">-38.2</epd:amount>
</common:other>
</LCIAResult>
<LCIAResult>
<referenceToLCIAMethodDataSet uri="../lciamethods/5f635281-343e-44fb-83df-1971b155e6b6.xml" type="LCIA method data set" refObjectId="5f635281-343e-44fb-83df-1971b155e6b6">
<common:shortDescription xml:lang="en">Global Warming Potential fossil fuels (GWP-fossil)</common:shortDescription>
</referenceToLCIAMethodDataSet>
<common:other>
<epd:referenceToUnitGroupDataSet uri="../unitgroups/1ebf3012-d0db-4de2-aefd-ef30cedb0be1.xml" type="unit group data set" refObjectId="1ebf3012-d0db-4de2-aefd-ef30cedb0be1">
<common:shortDescription xml:lang="en">kg CO_(2)-Äq.</common:shortDescription>
</epd:referenceToUnitGroupDataSet>
<epd:amount epd:module="A1-A3">267</epd:amount>
<epd:amount epd:module="A4">3.79</epd:amount>
<epd:amount epd:module="A5">4.72</epd:amount>
<epd:amount epd:module="C2">0.249</epd:amount>
<epd:amount epd:module="C3">136</epd:amount>
<epd:amount epd:module="D">-38.1</epd:amount>
</common:other>
</LCIAResult>
<LCIAResult>
<referenceToLCIAMethodDataSet uri="../lciamethods/2356e1ab-0185-4db5-86e5-16de51c7485c.xml" type="LCIA method data set" refObjectId="2356e1ab-0185-4db5-86e5-16de51c7485c">
<common:shortDescription xml:lang="en">Global Warming Potential biogenic (GWP-biogenic)</common:shortDescription>
</referenceToLCIAMethodDataSet>
<common:other>
<epd:referenceToUnitGroupDataSet uri="../unitgroups/1ebf3012-d0db-4de2-aefd-ef30cedb0be1.xml" type="unit group data set" refObjectId="1ebf3012-d0db-4de2-aefd-ef30cedb0be1">
<common:shortDescription xml:lang="en">kg CO_(2)-Äq.</common:shortDescription>
</epd:referenceToUnitGroupDataSet>
<epd:amount epd:module="A1-A3">-74.3</epd:amount>
<epd:amount epd:module="A4">-0.00648</epd:amount>
<epd:amount epd:module="A5">77.1</epd:amount>
<epd:amount epd:module="C2">-0.000425</epd:amount>
<epd:amount epd:module="C3">-0.0595</epd:amount>
<epd:amount epd:module="D">-0.0893</epd:amount>
</common:other>
</LCIAResult>
<LCIAResult>
<referenceToLCIAMethodDataSet uri="../lciamethods/4331bbdb-978a-490d-8707-eeb047f01a55.xml" type="LCIA method data set" refObjectId="4331bbdb-978a-490d-8707-eeb047f01a55">
<common:shortDescription xml:lang="en">Global Warming Potential luluc (GWP-luluc)</common:shortDescription>
</referenceToLCIAMethodDataSet>
<common:other>
<epd:referenceToUnitGroupDataSet uri="../unitgroups/1ebf3012-d0db-4de2-aefd-ef30cedb0be1.xml" type="unit group data set" refObjectId="1ebf3012-d0db-4de2-aefd-ef30cedb0be1">
<common:shortDescription xml:lang="en">kg CO_(2)-Äq.</common:shortDescription>
</epd:referenceToUnitGroupDataSet>
<epd:amount epd:module="A1-A3">0.543</epd:amount>
<epd:amount epd:module="A4">0.0307</epd:amount>
<epd:amount epd:module="A5">0.00617</epd:amount>
<epd:amount epd:module="C2">0.00202</epd:amount>
<epd:amount epd:module="C3">0.0277</epd:amount>
<epd:amount epd:module="D">-0.0266</epd:amount>
</common:other>
</LCIAResult>
<LCIAResult>
<referenceToLCIAMethodDataSet uri="../lciamethods/b5c629d6-def3-11e6-bf01-fe55135034f3.xml" type="LCIA method data set" refObjectId="b5c629d6-def3-11e6-bf01-fe55135034f3">
<common:shortDescription xml:lang="en">Depletion potential of the stratospheric ozone layer (ODP)</common:shortDescription>
</referenceToLCIAMethodDataSet>
<common:other>
<epd:referenceToUnitGroupDataSet uri="../unitgroups/d9e957c9-7309-4474-bf3a-7777df6c4e5b.xml" type="unit group data set" refObjectId="d9e957c9-7309-4474-bf3a-7777df6c4e5b">
<common:shortDescription xml:lang="en">kg CFC11-Äq.</common:shortDescription>
</epd:referenceToUnitGroupDataSet>
<epd:amount epd:module="A1-A3">1.44E-09</epd:amount>
<epd:amount epd:module="A4">4.56E-16</epd:amount>
<epd:amount epd:module="A5">1.47E-11</epd:amount>
<epd:amount epd:module="C2">2.99E-17</epd:amount>
<epd:amount epd:module="C3">2.07E-13</epd:amount>
<epd:amount epd:module="D">-3.96E-13</epd:amount>
</common:other>
</LCIAResult>
<LCIAResult>
<referenceToLCIAMethodDataSet uri="../lciamethods/b5c611c6-def3-11e6-bf01-fe55135034f3.xml" type="LCIA method data set" refObjectId="b5c611c6-def3-11e6-bf01-fe55135034f3">
<common:shortDescription xml:lang="en">Acidification potential of land and water (AP)</common:shortDescription>
</referenceToLCIAMethodDataSet>
<common:other>
<epd:referenceToUnitGroupDataSet uri="../unitgroups/42e089ac-92bf-4bf2-8ca1-5fc40d18f2ed.xml" type="unit group data set" refObjectId="42e089ac-92bf-4bf2-8ca1-5fc40d18f2ed">
<common:shortDescription xml:lang="en">mol H^(+)-Äq.</common:shortDescription>
</epd:referenceToUnitGroupDataSet>
<epd:amount epd:module="A1-A3">1.32</epd:amount>
<epd:amount epd:module="A4">0.0114</epd:amount>
<epd:amount epd:module="A5">0.0162</epd:amount>
<epd:amount epd:module="C2">0.000746</epd:amount>
<epd:amount epd:module="C3">0.0405</epd:amount>
<epd:amount epd:module="D">-0.0532</epd:amount>
</common:other>
</LCIAResult>
<LCIAResult>
<referenceToLCIAMethodDataSet uri="../lciamethods/b53ec18f-7377-4ad3-86eb-cc3f4f276b2b.xml" type="LCIA method data set" refObjectId="b53ec18f-7377-4ad3-86eb-cc3f4f276b2b">
<common:shortDescription xml:lang="en">Eutrophication potential aquatic freshwater (EP-freshwater)</common:shortDescription>
</referenceToLCIAMethodDataSet>
<common:other>
<epd:referenceToUnitGroupDataSet uri="../unitgroups/0429039d-a61d-4590-ba67-aa4a20a810a1.xml" type="unit group data set" refObjectId="0429039d-a61d-4590-ba67-aa4a20a810a1">
<common:shortDescription xml:lang="en">kg PO_(4)-Äq.</common:shortDescription>
</epd:referenceToUnitGroupDataSet>
<epd:amount epd:module="A1-A3">0.00273</epd:amount>
<epd:amount epd:module="A4">1.15E-05</epd:amount>
<epd:amount epd:module="A5">2.81E-05</epd:amount>
<epd:amount epd:module="C2">7.56E-07</epd:amount>
<epd:amount epd:module="C3">3.49E-05</epd:amount>
<epd:amount epd:module="D">-4.89E-05</epd:amount>
</common:other>
</LCIAResult>
<LCIAResult>
<referenceToLCIAMethodDataSet uri="../lciamethods/b5c619fa-def3-11e6-bf01-fe55135034f3.xml" type="LCIA method data set" refObjectId="b5c619fa-def3-11e6-bf01-fe55135034f3">
<common:shortDescription xml:lang="en">Eutrophication potential aquatic marine (EP-marine)</common:shortDescription>
</referenceToLCIAMethodDataSet>
<common:other>
<epd:referenceToUnitGroupDataSet uri="../unitgroups/d05bb823-ecdf-4686-8c40-bf1d9257859f.xml" type="unit group data set" refObjectId="d05bb823-ecdf-4686-8c40-bf1d9257859f">
<common:shortDescription xml:lang="en">kg N-Äq.</common:shortDescription>
</epd:referenceToUnitGroupDataSet>
<epd:amount epd:module="A1-A3">0.178</epd:amount>
<epd:amount epd:module="A4">0.00506</epd:amount>
<epd:amount epd:module="A5">0.00263</epd:amount>
<epd:amount epd:module="C2">0.000332</epd:amount>
<epd:amount epd:module="C3">0.0134</epd:amount>
<epd:amount epd:module="D">-0.0138</epd:amount>
</common:other>
</LCIAResult>
<LCIAResult>
<referenceToLCIAMethodDataSet uri="../lciamethods/b5c614d2-def3-11e6-bf01-fe55135034f3.xml" type="LCIA method data set" refObjectId="b5c614d2-def3-11e6-bf01-fe55135034f3">
<common:shortDescription xml:lang="en">Eutrophication potential terrestrial (EP-terrestrial)</common:shortDescription>
</referenceToLCIAMethodDataSet>
<common:other>
<epd:referenceToUnitGroupDataSet uri="../unitgroups/71b4d617-0ec9-4d3f-b65e-e438940c2401.xml" type="unit group data set" refObjectId="71b4d617-0ec9-4d3f-b65e-e438940c2401">
<common:shortDescription xml:lang="en">mol N-Äq.</common:shortDescription>
</epd:referenceToUnitGroupDataSet>
<epd:amount epd:module="A1-A3">1.72</epd:amount>
<epd:amount epd:module="A4">0.0567</epd:amount>
<epd:amount epd:module="A5">0.0296</epd:amount>
<epd:amount epd:module="C2">0.00372</epd:amount>
<epd:amount epd:module="C3">0.164</epd:amount>
<epd:amount epd:module="D">-0.148</epd:amount>
</common:other>
</LCIAResult>
<LCIAResult>
<referenceToLCIAMethodDataSet uri="../lciamethods/b5c610fe-def3-11e6-bf01-fe55135034f3.xml" type="LCIA method data set" refObjectId="b5c610fe-def3-11e6-bf01-fe55135034f3">
<common:shortDescription xml:lang="en">Formation potential of tropospheric ozone photochemical oxidants (POCP)</common:shortDescription>
</referenceToLCIAMethodDataSet>
<common:other>
<epd:referenceToUnitGroupDataSet uri="../unitgroups/d27c25f8-fbc1-44c6-b47b-4adbae4199c6.xml" type="unit group data set" refObjectId="d27c25f8-fbc1-44c6-b47b-4adbae4199c6">
<common:shortDescription xml:lang="en">kg NMVOC-Äq.</common:shortDescription>
</epd:referenceToUnitGroupDataSet>
<epd:amount epd:module="A1-A3">0.762</epd:amount>
<epd:amount epd:module="A4">0.01</epd:amount>
<epd:amount epd:module="A5">0.0101</epd:amount>
<epd:amount epd:module="C2">0.000656</epd:amount>
<epd:amount epd:module="C3">0.0379</epd:amount>
<epd:amount epd:module="D">-0.0396</epd:amount>
</common:other>
</LCIAResult>
<LCIAResult>
<referenceToLCIAMethodDataSet uri="../lciamethods/b2ad6494-c78d-11e6-9d9d-cec0c932ce01.xml" type="LCIA method data set" refObjectId="b2ad6494-c78d-11e6-9d9d-cec0c932ce01">
<common:shortDescription xml:lang="en">Abiotic depletion potential for non fossil resources (ADPE)</common:shortDescription>
</referenceToLCIAMethodDataSet>
<common:other>
<epd:referenceToUnitGroupDataSet uri="../unitgroups/54ccd2d9-a32a-4fc2-923d-f2c8c93e89d4.xml" type="unit group data set" refObjectId="54ccd2d9-a32a-4fc2-923d-f2c8c93e89d4">
<common:shortDescription xml:lang="en">kg Sb-Äq.</common:shortDescription>
</epd:referenceToUnitGroupDataSet>
<epd:amount epd:module="A1-A3">4410</epd:amount>
<epd:amount epd:module="A4">50.5</epd:amount>
<epd:amount epd:module="A5">50.4</epd:amount>
<epd:amount epd:module="C2">3.31</epd:amount>
<epd:amount epd:module="C3">251</epd:amount>
<epd:amount epd:module="D">-646</epd:amount>
</common:other>
</LCIAResult>
<LCIAResult>
<referenceToLCIAMethodDataSet uri="../lciamethods/b2ad6110-c78d-11e6-9d9d-cec0c932ce01.xml" type="LCIA method data set" refObjectId="b2ad6110-c78d-11e6-9d9d-cec0c932ce01">
<common:shortDescription xml:lang="en">Abiotic depletion potential for fossil resources (ADPF)</common:shortDescription>
</referenceToLCIAMethodDataSet>
<common:other>
<epd:referenceToUnitGroupDataSet uri="../unitgroups/93a60a57-a3c8-11da-a746-0800200c9a66.xml" type="unit group data set" refObjectId="93a60a57-a3c8-11da-a746-0800200c9a66">
<common:shortDescription xml:lang="en">MJ</common:shortDescription>
</epd:referenceToUnitGroupDataSet>
<epd:amount epd:module="A1-A3">1.27</epd:amount>
<epd:amount epd:module="A4">2.72E-07</epd:amount>
<epd:amount epd:module="A5">0.0132</epd:amount>
<epd:amount epd:module="C2">1.78E-08</epd:amount>
<epd:amount epd:module="C3">2.98E-06</epd:amount>
<epd:amount epd:module="D">-6.23E-06</epd:amount>
</common:other>
</LCIAResult>
<LCIAResult>
<referenceToLCIAMethodDataSet uri="../lciamethods/b2ad66ce-c78d-11e6-9d9d-cec0c932ce01.xml" type="LCIA method data set" refObjectId="b2ad66ce-c78d-11e6-9d9d-cec0c932ce01">
<common:shortDescription xml:lang="en">Water use (WDP)</common:shortDescription>
</referenceToLCIAMethodDataSet>
<common:other>
<epd:referenceToUnitGroupDataSet uri="../unitgroups/6ae2df01-888e-46c8-b17d-49fa3869b476.xml" type="unit group data set" refObjectId="6ae2df01-888e-46c8-b17d-49fa3869b476">
<common:shortDescription xml:lang="en">m^(3) world-Äq. deprived</common:shortDescription>
</epd:referenceToUnitGroupDataSet>
<epd:amount epd:module="A1-A3">30.9</epd:amount>
<epd:amount epd:module="A4">0.0339</epd:amount>
<epd:amount epd:module="A5">1.97</epd:amount>
<epd:amount epd:module="C2">0.00222</epd:amount>
<epd:amount epd:module="C3">10.5</epd:amount>
<epd:amount epd:module="D">-3.93</epd:amount>
</common:other>
</LCIAResult>
<LCIAResult>
<referenceToLCIAMethodDataSet uri="../lciamethods/b5c602c6-def3-11e6-bf01-fe55135034f3.xml" type="LCIA method data set" refObjectId="b5c602c6-def3-11e6-bf01-fe55135034f3">
<common:shortDescription xml:lang="en">Incidence of disease due to PM emissions (PM)</common:shortDescription>
</referenceToLCIAMethodDataSet>
<common:other>
<epd:referenceToUnitGroupDataSet uri="../unitgroups/3883559b-648f-4afc-8ba2-0bd24f3affa3.xml" type="unit group data set" refObjectId="3883559b-648f-4afc-8ba2-0bd24f3affa3">
<common:shortDescription xml:lang="en">Disease incidence</common:shortDescription>
</epd:referenceToUnitGroupDataSet>
<epd:amount epd:module="A1-A3">7.6E-05</epd:amount>
<epd:amount epd:module="A4">6.3E-08</epd:amount>
<epd:amount epd:module="A5">8.07E-07</epd:amount>
<epd:amount epd:module="C2">4.13E-09</epd:amount>
<epd:amount epd:module="C3">9.74E-07</epd:amount>
<epd:amount epd:module="D">-4.52E-07</epd:amount>
</common:other>
</LCIAResult>
<LCIAResult>
<referenceToLCIAMethodDataSet uri="../lciamethods/b5c632be-def3-11e6-bf01-fe55135034f3.xml" type="LCIA method data set" refObjectId="b5c632be-def3-11e6-bf01-fe55135034f3">
<common:shortDescription xml:lang="en">Human exposure efficiency relative to U235 (IR)</common:shortDescription>
</referenceToLCIAMethodDataSet>
<common:other>
<epd:referenceToUnitGroupDataSet uri="../unitgroups/456b05bf-1415-44a9-9993-02452f554c09.xml" type="unit group data set" refObjectId="456b05bf-1415-44a9-9993-02452f554c09">
<common:shortDescription xml:lang="en">kBq U235-Äq.</common:shortDescription>
</epd:referenceToUnitGroupDataSet>
<epd:amount epd:module="A1-A3">10.5</epd:amount>
<epd:amount epd:module="A4">0.00904</epd:amount>
<epd:amount epd:module="A5">0.142</epd:amount>
<epd:amount epd:module="C2">0.000594</epd:amount>
<epd:amount epd:module="C3">0.809</epd:amount>
<epd:amount epd:module="D">-7.87</epd:amount>
</common:other>
</LCIAResult>
<LCIAResult>
<referenceToLCIAMethodDataSet uri="../lciamethods/ee1082d1-b0f7-43ca-a1f0-21e2a4a74511.xml" type="LCIA method data set" refObjectId="ee1082d1-b0f7-43ca-a1f0-21e2a4a74511">
<common:shortDescription xml:lang="en">Comparative toxic unit for ecosystems (ETP-fw)</common:shortDescription>
</referenceToLCIAMethodDataSet>
<common:other>
<epd:referenceToUnitGroupDataSet uri="../unitgroups/aa959ded-f1eb-4efb-9c5c-2d60be36b3e6.xml" type="unit group data set" refObjectId="aa959ded-f1eb-4efb-9c5c-2d60be36b3e6">
<common:shortDescription xml:lang="en">CTUe</common:shortDescription>
</epd:referenceToUnitGroupDataSet>
<epd:amount epd:module="A1-A3">4850</epd:amount>
<epd:amount epd:module="A4">35.7</epd:amount>
<epd:amount epd:module="A5">50.1</epd:amount>
<epd:amount epd:module="C2">2.34</epd:amount>
<epd:amount epd:module="C3">208</epd:amount>
<epd:amount epd:module="D">-139</epd:amount>
</common:other>
</LCIAResult>
<LCIAResult>
<referenceToLCIAMethodDataSet uri="../lciamethods/2299222a-bbd8-474f-9d4f-4dd1f18aea7c.xml" type="LCIA method data set" refObjectId="2299222a-bbd8-474f-9d4f-4dd1f18aea7c">
<common:shortDescription xml:lang="en">Comparative toxic unit for humans (carcinogenic) (HTP-c)</common:shortDescription>
</referenceToLCIAMethodDataSet>
<common:other>
<epd:referenceToUnitGroupDataSet uri="../unitgroups/d4c9523e-2d7e-49fd-8469-998f547d3a70.xml" type="unit group data set" refObjectId="d4c9523e-2d7e-49fd-8469-998f547d3a70">
<common:shortDescription xml:lang="en">CTUh</common:shortDescription>
</epd:referenceToUnitGroupDataSet>
<epd:amount epd:module="A1-A3">9.12E-08</epd:amount>
<epd:amount epd:module="A4">7.47E-10</epd:amount>
<epd:amount epd:module="A5">1.11E-09</epd:amount>
<epd:amount epd:module="C2">4.9E-11</epd:amount>
<epd:amount epd:module="C3">8.23E-09</epd:amount>
<epd:amount epd:module="D">-6.03E-09</epd:amount>
</common:other>
</LCIAResult>
<LCIAResult>
<referenceToLCIAMethodDataSet uri="../lciamethods/3af763a5-b7a1-48c9-9cee-1f223481fcef.xml" type="LCIA method data set" refObjectId="3af763a5-b7a1-48c9-9cee-1f223481fcef">
<common:shortDescription xml:lang="en">Comparative toxic unit for humans (noncarcinogenic) (HTP-nc)</common:shortDescription>
</referenceToLCIAMethodDataSet>
<common:other>
<epd:referenceToUnitGroupDataSet uri="../unitgroups/d4c9523e-2d7e-49fd-8469-998f547d3a70.xml" type="unit group data set" refObjectId="d4c9523e-2d7e-49fd-8469-998f547d3a70">
<common:shortDescription xml:lang="en">CTUh</common:shortDescription>
</epd:referenceToUnitGroupDataSet>
<epd:amount epd:module="A1-A3">1.22E-05</epd:amount>
<epd:amount epd:module="A4">4.35E-08</epd:amount>
<epd:amount epd:module="A5">1.37E-07</epd:amount>
<epd:amount epd:module="C2">2.85E-09</epd:amount>
<epd:amount epd:module="C3">8.75E-07</epd:amount>
<epd:amount epd:module="D">-2.24E-07</epd:amount>
</common:other>
</LCIAResult>
<LCIAResult>
<referenceToLCIAMethodDataSet uri="../lciamethods/b2ad6890-c78d-11e6-9d9d-cec0c932ce01.xml" type="LCIA method data set" refObjectId="b2ad6890-c78d-11e6-9d9d-cec0c932ce01">
<common:shortDescription xml:lang="en">Soil quality index (SQP)</common:shortDescription>
</referenceToLCIAMethodDataSet>
<common:other>
<epd:referenceToUnitGroupDataSet uri="../unitgroups/f130951c-e67f-4f7f-8dd4-665de3974e18.xml" type="unit group data set" refObjectId="f130951c-e67f-4f7f-8dd4-665de3974e18">
<common:shortDescription xml:lang="en">SQP</common:shortDescription>
</epd:referenceToUnitGroupDataSet>
<epd:amount epd:module="A1-A3">4990</epd:amount>
<epd:amount epd:module="A4">17.7</epd:amount>
<epd:amount epd:module="A5">51.9</epd:amount>
<epd:amount epd:module="C2">1.16</epd:amount>
<epd:amount epd:module="C3">57</epd:amount>
<epd:amount epd:module="D">-101</epd:amount>
</common:other>
</LCIAResult>
</LCIAResults>
</processDataSet>