<?xml version="1.0" encoding="utf-8"?>
<processDataSet xmlns:epd="http://www.iai.kit.edu/EPD/2013" xmlns:epd2="http://www.indata.network/EPD/2019" xmlns:common="http://lca.jrc.it/ILCD/Common" xsi:schemaLocation="http://lca.jrc.it/ILCD/Process ../../schemas/EPD_DataSet.xsd" epd2:epd-version="1.2" version="1.1" locations="../ILCDLocations.xml" xmlns:xsi="http://www.w3.org/2001/XMLSchema-instance" xmlns="http://lca.jrc.it/ILCD/Process">
<processInformation>
<dataSetInformation>
<common:UUID>b4705987-f28c-4a66-8d0a-43a8942ba594</common:UUID>
<name>
<baseName xml:lang="en">SINIAT Standard and High Density plasterboards</baseName>
<functionalUnitFlowProperties xml:lang="en" />
</name>
<classificationInformation>
<common:classification name="OEKOBAU.DAT">
<common:class level="0" classId="1">Mineralische Baustoffe</common:class>
<common:class level="1" classId="1.3">Steine und Elemente</common:class>
<common:class level="2" classId="1.3.13">Gipsplatten</common:class>
</common:classification>
<common:classification name="IBUCategories">
<common:class level="0">02 Building products</common:class>
<common:class level="1">Gypsum products</common:class>
<common:class level="2">Plasterboard</common:class>
</common:classification>
</classificationInformation>
<common:generalComment xml:lang="en">Siniat plasterboards covered by this EPD are used in interior construction as a dry system where standard performances (type A) or increased density (type D) and impact resistance (type I) are required.This EPD refers to 1 m² of PregyPlac/PregyPlac Plus BA13 plasterboard.The following table presents the thickness and weight of the products covered by this EPD:For the placing on the market of the product in the EU/EFTA (with the exception of Switzerland) Regulation (EU) No. 305/2011 (CPR) applies. The product needs a declaration of performance taking into consideration /EN 520:2009/ Gypsum plasterboards - Definitions, requirements and test methods, and the CE-marking. For the application and use the respective national provisions apply.</common:generalComment>
<common:other>
<epd:scenarios>
<epd:scenario epd:default="true" epd:name="S1">
<epd:description xml:lang="en">100% recycling</epd:description>
</epd:scenario>
<epd:scenario epd:name="S2">
<epd:description xml:lang="en">Scenario 2</epd:description>
</epd:scenario>
</epd:scenarios>
</common:other>
</dataSetInformation>
<quantitativeReference>
<referenceToReferenceFlow>0</referenceToReferenceFlow>
</quantitativeReference>
<time>
<common:referenceYear>2019</common:referenceYear>
<common:dataSetValidUntil>2024</common:dataSetValidUntil>
<common:other>
<epd2:publicationDateOfEPD>2019-04-15</epd2:publicationDateOfEPD>
</common:other>
</time>
<geography>
<locationOfOperationSupplyOrProduction location="IT" />
</geography>
<technology>
<technologyDescriptionAndIncludedProcesses xml:lang="en">The manufacturing process is illustrated in the figure below. A preliminary stage consists in calcining the gypsum (natural gypsum + recycled gypsum) in a kiln to obtain the stucco, which is a calcium sulphate hemi hydrate. Plasterboards are then manufactured in a continuous automated production process by pouring from a mixer a slurry of stucco, water and additives, in-between two layers of a liner, composed of paper 100% recycled. The continuous laminated board is calibrated into a forming plate and transported on a conveyor belt to the knife, while the setting of the slurry occurs and the mechanical bond forms at the gypsum-paper interface. After cutting, the boards are introduced in a multilayer drier to remove the excess of water and increase strength. At the drier out-feed the boards are trimmed to the nominal length, pilled up on stacking units. The quality characteristics of the boards are controlled before storing pallets in the warehouse. The management system operated by the site is in compliance with the UNI EN ISO 9001:2015. 
Technical data: 
Detailed technical information is available in the specific product data sheets at www.siniat.it.For the reference product PregyPlac/PregyPlac Plus BA13:Performance data of the product in accordance with the declaration of performance with respect to its essential characteristics according to/EN 520:2009/ Gypsum plasterboards - Definitions, requirements and test methods apply. Visit www.siniat.it for detailed technical documentation. 
Declared unit: 
The LCA results presented in this EPD are related to 1 m² of PregyPlac (Plus) BA13 installed in the building, which is 12.5 mm thick and weights 8.5 kg approximately.</technologyDescriptionAndIncludedProcesses>
<technologicalApplicability xml:lang="en">Siniat plasterboards covered by this EPD are used in all construction types (residential, non-residential, new or refurbished), ranging from complex high-tech systems to easy to install products, assuring several levels of performance. They can be used for partitions and the lining of walls, ceilings.They are suitable for any type of coating (wallpaper, paint, tiles).</technologicalApplicability>
<referenceToTechnologyFlowDiagrammOrPicture uri="../sources/90fc18d2-fc27-4cda-adb5-91e40f5cec38.xml" type="source data set" refObjectId="90fc18d2-fc27-4cda-adb5-91e40f5cec38">
<common:shortDescription xml:lang="en">Capture5.JPG</common:shortDescription>
</referenceToTechnologyFlowDiagrammOrPicture>
</technology>
</processInformation>
<modellingAndValidation>
<LCIMethodAndAllocation>
<typeOfDataSet>EPD</typeOfDataSet>
<referenceToLCAMethodDetails type="source data set" refObjectId="cee35981-7998-4aab-b066-51600da29be0">
<common:shortDescription xml:lang="en">Plasterboard.pdf</common:shortDescription>
</referenceToLCAMethodDetails>
<common:other>
<epd:subType xmlns="http://www.iai.kit.edu/EPD/2013">average dataset</epd:subType>
</common:other>
</LCIMethodAndAllocation>
<dataSourcesTreatmentAndRepresentativeness>
<referenceToDataSource type="source data set" refObjectId="b497a91f-e14b-4b69-8f28-f50eb1576766">
<common:shortDescription xml:lang="en">ecoinvent database (all versions)</common:shortDescription>
</referenceToDataSource>
<referenceToDataSource type="source data set" refObjectId="db59e0c6-db9a-4d9a-8637-67b8ed42415c">
<common:shortDescription xml:lang="en">ecoinvent 3.4 database</common:shortDescription>
</referenceToDataSource>
<useAdviceForDataSet xml:lang="en">Scope: 
The EPD applies for : PregyFlex BA6; PregyPlac BA10; PregyPlac Plus BA10; PregyPlac BA13; PregyPlac Plus BA13; SyniaPlac 4BA13; PregyPlac BA15; PregyPlac BA18; PregyDur I BA13; PregyDurWhite BA13; WhiteAir BA13; PregySoundboard BA13. The EPD presents environmental impacts valid for PregyPlac/PregyPlac Plus BA13. The environmental impacts for other covered products can be obtained by multiplying the presented results by the corresponding conversion factor presented in the table in 3.1 of this EPD. This EPD was developed from data collected at the Siniat plasterboard factory located in Corfinio, producing 100 % of the total production of these products sold in the Italian market. The EPD is a cradle-to-gate with options EPD and covers Siniat plasterboards sold on the Italian market. 
System boundary: 
This EPD is a cradle-to-gate with options EPD, covering the following life cycle stages:-  plasterboards manufacturing (modules A1-A3), including the production of components, their transport to the manufacturing site, as well as impacts due to energy consumption, air and water emissions, as well as waste treatment and packaging material production, -  transport of the plasterboards from manufacturing to building site (module A4), -  installation (module A5), including the production of auxiliaries (screw, joint tape and coating). Due to the many possible applications of plasterboards, frames or suspended-ceiling systems are excluded from the system boundary, -  emissions during the use phase (modules B1). No emissions occur during Siniat plasterboards use phase, -  end-of-life (modules C1-C4), including impacts from manual deconstruction, transport of waste to treatment facility, and waste processing and waste disposal. Two scenarios were considered : For scenario 1 (100% landfill), the system boundaries include transport to the treatment facility (C2), sorting of screws (C3) and landfill (C4). For scenario 2 (100% recovery), the system boundaries include transport to the treatment facility (C2), sorting of gypsum, cardboard and other waste (C3), and landfill of other auxiliaries (joint tape, sealant).- benefits and loads beyond the system boundaries (D). This module is included only for end-of-life scenario 2.</useAdviceForDataSet>
<common:other>
<epd2:referenceToOriginalEPD type="source data set" refObjectId="13a0b0ef-e01b-477a-b025-d65c2b0645ea">
<common:shortDescription xml:lang="en">SINIAT Standard and High Density plasterboards .pdf</common:shortDescription>
</epd2:referenceToOriginalEPD>
</common:other>
</dataSourcesTreatmentAndRepresentativeness>
<validation>
<review type="Accredited third party review">
<common:referenceToNameOfReviewerAndInstitution uri="../contacts/d111dbec-b024-4be5-86c5-752d6eb2cf95.xml" type="contact data set" refObjectId="d111dbec-b024-4be5-86c5-752d6eb2cf95">
<common:shortDescription xml:lang="en">Institut Bauen und Umwelt e. V.</common:shortDescription>
</common:referenceToNameOfReviewerAndInstitution>
</review>
</validation>
<complianceDeclarations>
<compliance>
<common:referenceToComplianceSystem uri="../sources/b00f9ec0-7874-11e3-981f-0800200c9a66.xml" type="source data set" refObjectId="b00f9ec0-7874-11e3-981f-0800200c9a66">
<common:shortDescription xml:lang="en">DIN EN 15804</common:shortDescription>
</common:referenceToComplianceSystem>
</compliance>
<compliance>
<common:referenceToComplianceSystem uri="../sources/4f2eb655-6e44-4874-a95a-e28f5442cd4d.xml" type="source data set" refObjectId="4f2eb655-6e44-4874-a95a-e28f5442cd4d">
<common:shortDescription xml:lang="en">ISO 14025</common:shortDescription>
</common:referenceToComplianceSystem>
</compliance>
</complianceDeclarations>
</modellingAndValidation>
<administrativeInformation>
<common:commissionerAndGoal>
<common:referenceToCommissioner uri="../contacts/9f15c029-1fb0-467d-8dd1-92b013e91ca8.xml" type="contact data set" refObjectId="9f15c029-1fb0-467d-8dd1-92b013e91ca8">
<common:shortDescription xml:lang="en">Etex Building Performance International</common:shortDescription>
</common:referenceToCommissioner>
</common:commissionerAndGoal>
<dataGenerator>
<common:referenceToPersonOrEntityGeneratingTheDataSet uri="../contacts/9f15c029-1fb0-467d-8dd1-92b013e91ca8.xml" type="contact data set" refObjectId="9f15c029-1fb0-467d-8dd1-92b013e91ca8">
<common:shortDescription xml:lang="en">Etex Building Performance International</common:shortDescription>
</common:referenceToPersonOrEntityGeneratingTheDataSet>
</dataGenerator>
<dataEntryBy>
<common:timeStamp>2019-04-15T08:35:44.736</common:timeStamp>
<common:referenceToDataSetFormat uri="../sources/a97a0155-0234-4b87-b4ce-a45da52f2a40.xml" type="source data set" refObjectId="a97a0155-0234-4b87-b4ce-a45da52f2a40">
<common:shortDescription xml:lang="en">ILCD Format</common:shortDescription>
</common:referenceToDataSetFormat>
<common:referenceToDataSetFormat uri="../sources/a29449fd-aa2f-4de8-b5d7-4b06b43c6fde.xml" type="source data set" refObjectId="a29449fd-aa2f-4de8-b5d7-4b06b43c6fde">
<common:shortDescription xml:lang="de">EPD-Datenformaterweiterungen v1.2</common:shortDescription>
<common:shortDescription xml:lang="en">EPD Data Format Extensions v1.2</common:shortDescription>
</common:referenceToDataSetFormat>
</dataEntryBy>
<publicationAndOwnership>
<common:dataSetVersion>00.01.000</common:dataSetVersion>
<common:referenceToRegistrationAuthority uri="../contacts/d111dbec-b024-4be5-86c5-752d6eb2cf95.xml" type="contact data set" refObjectId="d111dbec-b024-4be5-86c5-752d6eb2cf95">
<common:shortDescription xml:lang="en">Institut Bauen und Umwelt e. V.</common:shortDescription>
</common:referenceToRegistrationAuthority>
<common:registrationNumber>EPD-ETX-20180169-ICA1-EN</common:registrationNumber>
<common:referenceToOwnershipOfDataSet uri="../contacts/9f15c029-1fb0-467d-8dd1-92b013e91ca8.xml" type="contact data set" refObjectId="9f15c029-1fb0-467d-8dd1-92b013e91ca8">
<common:shortDescription xml:lang="en">Etex Building Performance International</common:shortDescription>
</common:referenceToOwnershipOfDataSet>
<common:copyright>true</common:copyright>
<common:licenseType>Free of charge for all users and uses</common:licenseType>
<common:accessRestrictions xml:lang="en">None</common:accessRestrictions>
<common:other>
<epd2:referenceToPublisher type="contact data set" refObjectId="d111dbec-b024-4be5-86c5-752d6eb2cf95" uri="../contacts/d111dbec-b024-4be5-86c5-752d6eb2cf95.xml">
<common:shortDescription xml:lang="en">Institut Bauen und Umwelt e. V.</common:shortDescription>
</epd2:referenceToPublisher>
</common:other>
</publicationAndOwnership>
</administrativeInformation>
<exchanges>
<exchange dataSetInternalID="0">
<referenceToFlowDataSet uri="../flows/f38c4d82-8d10-9131-180c-2660fed1c682.xml" type="flow data set" refObjectId="f38c4d82-8d10-9131-180c-2660fed1c682">
<common:shortDescription xml:lang="en">PregyPlac (Plus) BA13 ()</common:shortDescription>
</referenceToFlowDataSet>
<meanAmount>1</meanAmount>
<referencesToDataSource />
</exchange>
<exchange dataSetInternalID="1">
<referenceToFlowDataSet uri="../flows/20f32be5-0398-4288-9b6d-accddd195317.xml" type="flow data set" refObjectId="20f32be5-0398-4288-9b6d-accddd195317">
<common:shortDescription xml:lang="en">Renewable primary energy as energy carrier (PERE)</common:shortDescription>
</referenceToFlowDataSet>
<functionType>General reminder flow</functionType>
<exchangeDirection>Input</exchangeDirection>
<common:other>
<epd:referenceToUnitGroupDataSet uri="../unitgroups/93a60a57-a3c8-11da-a746-0800200c9a66.xml" type="unit group data set" refObjectId="93a60a57-a3c8-11da-a746-0800200c9a66">
<common:shortDescription xml:lang="en">MJ</common:shortDescription>
</epd:referenceToUnitGroupDataSet>
<epd:amount epd:module="A1-A3">2.71107117358134</epd:amount>
<epd:amount epd:module="A4">0.0915997331541788</epd:amount>
<epd:amount epd:module="A5">0.639745133342212</epd:amount>
<epd:amount epd:module="B1">0</epd:amount>
<epd:amount epd:module="C1">0</epd:amount>
<epd:amount epd:module="C2" epd:scenario="S1">0.04985237106816</epd:amount>
<epd:amount epd:module="C2" epd:scenario="S2">0.04985237106816</epd:amount>
<epd:amount epd:module="C3" epd:scenario="S1">9.697628E-05</epd:amount>
<epd:amount epd:module="C3" epd:scenario="S2">0.06371341596</epd:amount>
<epd:amount epd:module="C4" epd:scenario="S1">0.033477051626322</epd:amount>
<epd:amount epd:module="C4" epd:scenario="S2">0.001471251966322</epd:amount>
<epd:amount epd:module="D">1.0048590256842</epd:amount>
</common:other>
</exchange>
<exchange dataSetInternalID="2">
<referenceToFlowDataSet uri="../flows/fb3ec0de-548d-4508-aea5-00b73bf6f702.xml" type="flow data set" refObjectId="fb3ec0de-548d-4508-aea5-00b73bf6f702">
<common:shortDescription xml:lang="en">Renewable primary energy resources as material utilization (PERM)</common:shortDescription>
</referenceToFlowDataSet>
<functionType>General reminder flow</functionType>
<exchangeDirection>Input</exchangeDirection>
<common:other>
<epd:referenceToUnitGroupDataSet uri="../unitgroups/93a60a57-a3c8-11da-a746-0800200c9a66.xml" type="unit group data set" refObjectId="93a60a57-a3c8-11da-a746-0800200c9a66">
<common:shortDescription xml:lang="en">MJ</common:shortDescription>
</epd:referenceToUnitGroupDataSet>
<epd:amount epd:module="A1-A3">1.46947431031901</epd:amount>
<epd:amount epd:module="A4">0</epd:amount>
<epd:amount epd:module="A5">0.0734737155159505</epd:amount>
<epd:amount epd:module="B1">0</epd:amount>
<epd:amount epd:module="C1">0</epd:amount>
<epd:amount epd:module="C2" epd:scenario="S1">0</epd:amount>
<epd:amount epd:module="C2" epd:scenario="S2">0</epd:amount>
<epd:amount epd:module="C3" epd:scenario="S1">0</epd:amount>
<epd:amount epd:module="C3" epd:scenario="S2">0</epd:amount>
<epd:amount epd:module="C4" epd:scenario="S1">0</epd:amount>
<epd:amount epd:module="C4" epd:scenario="S2">0</epd:amount>
<epd:amount epd:module="D">0</epd:amount>
</common:other>
</exchange>
<exchange dataSetInternalID="3">
<referenceToFlowDataSet uri="../flows/53f97275-fa8a-4cdd-9024-65936002acd0.xml" type="flow data set" refObjectId="53f97275-fa8a-4cdd-9024-65936002acd0">
<common:shortDescription xml:lang="en">Total use of renewable primary energy resources (PERT)</common:shortDescription>
</referenceToFlowDataSet>
<functionType>General reminder flow</functionType>
<exchangeDirection>Input</exchangeDirection>
<common:other>
<epd:referenceToUnitGroupDataSet uri="../unitgroups/93a60a57-a3c8-11da-a746-0800200c9a66.xml" type="unit group data set" refObjectId="93a60a57-a3c8-11da-a746-0800200c9a66">
<common:shortDescription xml:lang="en">MJ</common:shortDescription>
</epd:referenceToUnitGroupDataSet>
<epd:amount epd:module="A1-A3">4.18054548390035</epd:amount>
<epd:amount epd:module="A4">0.0915997331541788</epd:amount>
<epd:amount epd:module="A5">0.713218848858163</epd:amount>
<epd:amount epd:module="B1">0</epd:amount>
<epd:amount epd:module="C1">0</epd:amount>
<epd:amount epd:module="C2" epd:scenario="S1">0.04985237106816</epd:amount>
<epd:amount epd:module="C2" epd:scenario="S2">0.04985237106816</epd:amount>
<epd:amount epd:module="C3" epd:scenario="S1">9.697628E-05</epd:amount>
<epd:amount epd:module="C3" epd:scenario="S2">0.06371341596</epd:amount>
<epd:amount epd:module="C4" epd:scenario="S1">0.033477051626322</epd:amount>
<epd:amount epd:module="C4" epd:scenario="S2">0.001471251966322</epd:amount>
<epd:amount epd:module="D">1.0048590256842</epd:amount>
</common:other>
</exchange>
<exchange dataSetInternalID="4">
<referenceToFlowDataSet uri="../flows/ac857178-2b45-46ec-892a-a9a4332f0372.xml" type="flow data set" refObjectId="ac857178-2b45-46ec-892a-a9a4332f0372">
<common:shortDescription xml:lang="en">Non renewable primary energy as energy carrier (PENRE)</common:shortDescription>
</referenceToFlowDataSet>
<functionType>General reminder flow</functionType>
<exchangeDirection>Input</exchangeDirection>
<common:other>
<epd:referenceToUnitGroupDataSet uri="../unitgroups/93a60a57-a3c8-11da-a746-0800200c9a66.xml" type="unit group data set" refObjectId="93a60a57-a3c8-11da-a746-0800200c9a66">
<common:shortDescription xml:lang="en">MJ</common:shortDescription>
</epd:referenceToUnitGroupDataSet>
<epd:amount epd:module="A1-A3">35.0457124265697</epd:amount>
<epd:amount epd:module="A4">4.07725492415789</epd:amount>
<epd:amount epd:module="A5">3.26957765264775</epd:amount>
<epd:amount epd:module="B1">0</epd:amount>
<epd:amount epd:module="C1">0</epd:amount>
<epd:amount epd:module="C2" epd:scenario="S1">2.255022832528</epd:amount>
<epd:amount epd:module="C2" epd:scenario="S2">2.255022832528</epd:amount>
<epd:amount epd:module="C3" epd:scenario="S1">0.002245671875</epd:amount>
<epd:amount epd:module="C3" epd:scenario="S2">1.475406421875</epd:amount>
<epd:amount epd:module="C4" epd:scenario="S1">1.318582303605</epd:amount>
<epd:amount epd:module="C4" epd:scenario="S2">0.057949153605</epd:amount>
<epd:amount epd:module="D">-0.458581897555979</epd:amount>
</common:other>
</exchange>
<exchange dataSetInternalID="5">
<referenceToFlowDataSet uri="../flows/1421caa0-679d-4bf4-b282-0eb850ccae27.xml" type="flow data set" refObjectId="1421caa0-679d-4bf4-b282-0eb850ccae27">
<common:shortDescription xml:lang="en">Non renewable primary energy as material utilization (PENRM)</common:shortDescription>
</referenceToFlowDataSet>
<functionType>General reminder flow</functionType>
<exchangeDirection>Input</exchangeDirection>
<common:other>
<epd:referenceToUnitGroupDataSet uri="../unitgroups/93a60a57-a3c8-11da-a746-0800200c9a66.xml" type="unit group data set" refObjectId="93a60a57-a3c8-11da-a746-0800200c9a66">
<common:shortDescription xml:lang="en">MJ</common:shortDescription>
</epd:referenceToUnitGroupDataSet>
<epd:amount epd:module="A1-A3">0</epd:amount>
<epd:amount epd:module="A4">0</epd:amount>
<epd:amount epd:module="A5">0</epd:amount>
<epd:amount epd:module="B1">0</epd:amount>
<epd:amount epd:module="C1">0</epd:amount>
<epd:amount epd:module="C2" epd:scenario="S1">0</epd:amount>
<epd:amount epd:module="C2" epd:scenario="S2">0</epd:amount>
<epd:amount epd:module="C3" epd:scenario="S1">0</epd:amount>
<epd:amount epd:module="C3" epd:scenario="S2">0</epd:amount>
<epd:amount epd:module="C4" epd:scenario="S1">0</epd:amount>
<epd:amount epd:module="C4" epd:scenario="S2">0</epd:amount>
<epd:amount epd:module="D">0</epd:amount>
</common:other>
</exchange>
<exchange dataSetInternalID="6">
<referenceToFlowDataSet uri="../flows/06159210-646b-4c8d-8583-da9b3b95a6c1.xml" type="flow data set" refObjectId="06159210-646b-4c8d-8583-da9b3b95a6c1">
<common:shortDescription xml:lang="en">Total use of non renewable primary energy resources (PENRT)</common:shortDescription>
</referenceToFlowDataSet>
<functionType>General reminder flow</functionType>
<exchangeDirection>Input</exchangeDirection>
<common:other>
<epd:referenceToUnitGroupDataSet uri="../unitgroups/93a60a57-a3c8-11da-a746-0800200c9a66.xml" type="unit group data set" refObjectId="93a60a57-a3c8-11da-a746-0800200c9a66">
<common:shortDescription xml:lang="en">MJ</common:shortDescription>
</epd:referenceToUnitGroupDataSet>
<epd:amount epd:module="A1-A3">35.0457124265697</epd:amount>
<epd:amount epd:module="A4">4.07725492415789</epd:amount>
<epd:amount epd:module="A5">3.26957765264775</epd:amount>
<epd:amount epd:module="B1">0</epd:amount>
<epd:amount epd:module="C1">0</epd:amount>
<epd:amount epd:module="C2" epd:scenario="S1">2.255022832528</epd:amount>
<epd:amount epd:module="C2" epd:scenario="S2">2.255022832528</epd:amount>
<epd:amount epd:module="C3" epd:scenario="S1">0.002245671875</epd:amount>
<epd:amount epd:module="C3" epd:scenario="S2">1.475406421875</epd:amount>
<epd:amount epd:module="C4" epd:scenario="S1">1.318582303605</epd:amount>
<epd:amount epd:module="C4" epd:scenario="S2">0.057949153605</epd:amount>
<epd:amount epd:module="D">-0.458581897555979</epd:amount>
</common:other>
</exchange>
<exchange dataSetInternalID="7">
<referenceToFlowDataSet uri="../flows/c6a1f35f-2d09-4f54-8dfb-97e502e1ce92.xml" type="flow data set" refObjectId="c6a1f35f-2d09-4f54-8dfb-97e502e1ce92">
<common:shortDescription xml:lang="en">Use of secondary material (SM)</common:shortDescription>
</referenceToFlowDataSet>
<functionType>General reminder flow</functionType>
<exchangeDirection>Input</exchangeDirection>
<common:other>
<epd:referenceToUnitGroupDataSet uri="../unitgroups/ad38d542-3fe9-439d-9b95-2f5f7752acaf.xml" type="unit group data set" refObjectId="ad38d542-3fe9-439d-9b95-2f5f7752acaf">
<common:shortDescription xml:lang="en">kg</common:shortDescription>
</epd:referenceToUnitGroupDataSet>
<epd:amount epd:module="A1-A3">3.31226816159315</epd:amount>
<epd:amount epd:module="A4">0</epd:amount>
<epd:amount epd:module="A5">0.165613408079657</epd:amount>
<epd:amount epd:module="B1">0</epd:amount>
<epd:amount epd:module="C1">0</epd:amount>
<epd:amount epd:module="C2" epd:scenario="S1">0</epd:amount>
<epd:amount epd:module="C2" epd:scenario="S2">0</epd:amount>
<epd:amount epd:module="C3" epd:scenario="S1">0</epd:amount>
<epd:amount epd:module="C3" epd:scenario="S2">0</epd:amount>
<epd:amount epd:module="C4" epd:scenario="S1">0</epd:amount>
<epd:amount epd:module="C4" epd:scenario="S2">0</epd:amount>
<epd:amount epd:module="D">4.2449694780195</epd:amount>
</common:other>
</exchange>
<exchange dataSetInternalID="8">
<referenceToFlowDataSet uri="../flows/64333088-a55f-4aa2-9a31-c10b07816787.xml" type="flow data set" refObjectId="64333088-a55f-4aa2-9a31-c10b07816787">
<common:shortDescription xml:lang="en">Use of renewable secondary fuels (RSF)</common:shortDescription>
</referenceToFlowDataSet>
<functionType>General reminder flow</functionType>
<exchangeDirection>Input</exchangeDirection>
<common:other>
<epd:referenceToUnitGroupDataSet uri="../unitgroups/93a60a57-a3c8-11da-a746-0800200c9a66.xml" type="unit group data set" refObjectId="93a60a57-a3c8-11da-a746-0800200c9a66">
<common:shortDescription xml:lang="en">MJ</common:shortDescription>
</epd:referenceToUnitGroupDataSet>
<epd:amount epd:module="A1-A3">0</epd:amount>
<epd:amount epd:module="A4">0</epd:amount>
<epd:amount epd:module="A5">0</epd:amount>
<epd:amount epd:module="B1">0</epd:amount>
<epd:amount epd:module="C1">0</epd:amount>
<epd:amount epd:module="C2" epd:scenario="S1">0</epd:amount>
<epd:amount epd:module="C2" epd:scenario="S2">0</epd:amount>
<epd:amount epd:module="C3" epd:scenario="S1">0</epd:amount>
<epd:amount epd:module="C3" epd:scenario="S2">0</epd:amount>
<epd:amount epd:module="C4" epd:scenario="S1">0</epd:amount>
<epd:amount epd:module="C4" epd:scenario="S2">0</epd:amount>
<epd:amount epd:module="D">0</epd:amount>
</common:other>
</exchange>
<exchange dataSetInternalID="9">
<referenceToFlowDataSet uri="../flows/89def144-d39a-4287-b86f-efde453ddcb2.xml" type="flow data set" refObjectId="89def144-d39a-4287-b86f-efde453ddcb2">
<common:shortDescription xml:lang="en">Use of non renewable secondary fuels (NRSF)</common:shortDescription>
</referenceToFlowDataSet>
<functionType>General reminder flow</functionType>
<exchangeDirection>Input</exchangeDirection>
<common:other>
<epd:referenceToUnitGroupDataSet uri="../unitgroups/93a60a57-a3c8-11da-a746-0800200c9a66.xml" type="unit group data set" refObjectId="93a60a57-a3c8-11da-a746-0800200c9a66">
<common:shortDescription xml:lang="en">MJ</common:shortDescription>
</epd:referenceToUnitGroupDataSet>
<epd:amount epd:module="A1-A3">0</epd:amount>
<epd:amount epd:module="A4">0</epd:amount>
<epd:amount epd:module="A5">0</epd:amount>
<epd:amount epd:module="B1">0</epd:amount>
<epd:amount epd:module="C1">0</epd:amount>
<epd:amount epd:module="C2" epd:scenario="S1">0</epd:amount>
<epd:amount epd:module="C2" epd:scenario="S2">0</epd:amount>
<epd:amount epd:module="C3" epd:scenario="S1">0</epd:amount>
<epd:amount epd:module="C3" epd:scenario="S2">0</epd:amount>
<epd:amount epd:module="C4" epd:scenario="S1">0</epd:amount>
<epd:amount epd:module="C4" epd:scenario="S2">0</epd:amount>
<epd:amount epd:module="D">0</epd:amount>
</common:other>
</exchange>
<exchange dataSetInternalID="10">
<referenceToFlowDataSet uri="../flows/3cf952c8-f3a4-461d-8c96-96456ca62246.xml" type="flow data set" refObjectId="3cf952c8-f3a4-461d-8c96-96456ca62246">
<common:shortDescription xml:lang="en">Use of net fresh water (FW)</common:shortDescription>
</referenceToFlowDataSet>
<functionType>General reminder flow</functionType>
<exchangeDirection>Input</exchangeDirection>
<common:other>
<epd:referenceToUnitGroupDataSet uri="../unitgroups/cd950537-0a98-4044-9ba7-9f9a68d0a504.xml" type="unit group data set" refObjectId="cd950537-0a98-4044-9ba7-9f9a68d0a504">
<common:shortDescription xml:lang="en">m^3</common:shortDescription>
</epd:referenceToUnitGroupDataSet>
<epd:amount epd:module="A1-A3">0.00775792518922143</epd:amount>
<epd:amount epd:module="A4">0.000992467538361625</epd:amount>
<epd:amount epd:module="A5">0.00176571799551911</epd:amount>
<epd:amount epd:module="B1">0</epd:amount>
<epd:amount epd:module="C1">0</epd:amount>
<epd:amount epd:module="C2" epd:scenario="S1">0.0005436710313168</epd:amount>
<epd:amount epd:module="C2" epd:scenario="S2">0.0005436710313168</epd:amount>
<epd:amount epd:module="C3" epd:scenario="S1">5.272914875E-07</epd:amount>
<epd:amount epd:module="C3" epd:scenario="S2">0.0003464305072875</epd:amount>
<epd:amount epd:module="C4" epd:scenario="S1">0.0014462795601786</epd:amount>
<epd:amount epd:module="C4" epd:scenario="S2">6.35612021786E-05</epd:amount>
<epd:amount epd:module="D">0.000178250306710183</epd:amount>
</common:other>
</exchange>
<exchange dataSetInternalID="11">
<referenceToFlowDataSet uri="../flows/430f9e0f-59b2-46a0-8e0d-55e0e84948fc.xml" type="flow data set" refObjectId="430f9e0f-59b2-46a0-8e0d-55e0e84948fc">
<common:shortDescription xml:lang="en">Hazardous waste disposed (HWD)</common:shortDescription>
</referenceToFlowDataSet>
<functionType>General reminder flow</functionType>
<exchangeDirection>Output</exchangeDirection>
<common:other>
<epd:referenceToUnitGroupDataSet uri="../unitgroups/ad38d542-3fe9-439d-9b95-2f5f7752acaf.xml" type="unit group data set" refObjectId="ad38d542-3fe9-439d-9b95-2f5f7752acaf">
<common:shortDescription xml:lang="en">kg</common:shortDescription>
</epd:referenceToUnitGroupDataSet>
<epd:amount epd:module="A1-A3">0.0270974872323152</epd:amount>
<epd:amount epd:module="A4">0.00460738812864899</epd:amount>
<epd:amount epd:module="A5">0.00290819435301546</epd:amount>
<epd:amount epd:module="B1">0</epd:amount>
<epd:amount epd:module="C1">0</epd:amount>
<epd:amount epd:module="C2" epd:scenario="S1">0.002476515715504</epd:amount>
<epd:amount epd:module="C2" epd:scenario="S2">0.002476515715504</epd:amount>
<epd:amount epd:module="C3" epd:scenario="S1">5.63173775E-07</epd:amount>
<epd:amount epd:module="C3" epd:scenario="S2">0.000370005170175</epd:amount>
<epd:amount epd:module="C4" epd:scenario="S1">0.00066415808494386</epd:amount>
<epd:amount epd:module="C4" epd:scenario="S2">2.918846914386E-05</epd:amount>
<epd:amount epd:module="D">-3.57572437478722E-05</epd:amount>
</common:other>
</exchange>
<exchange dataSetInternalID="12">
<referenceToFlowDataSet uri="../flows/b29ef66b-e286-4afa-949f-62f1a7b4d7fa.xml" type="flow data set" refObjectId="b29ef66b-e286-4afa-949f-62f1a7b4d7fa">
<common:shortDescription xml:lang="en">Non hazardous waste disposed (NHWD)</common:shortDescription>
</referenceToFlowDataSet>
<functionType>General reminder flow</functionType>
<exchangeDirection>Output</exchangeDirection>
<common:other>
<epd:referenceToUnitGroupDataSet uri="../unitgroups/ad38d542-3fe9-439d-9b95-2f5f7752acaf.xml" type="unit group data set" refObjectId="ad38d542-3fe9-439d-9b95-2f5f7752acaf">
<common:shortDescription xml:lang="en">kg</common:shortDescription>
</epd:referenceToUnitGroupDataSet>
<epd:amount epd:module="A1-A3">0.260361514730392</epd:amount>
<epd:amount epd:module="A4">0.268112134683102</epd:amount>
<epd:amount epd:module="A5">0.480774233993113</epd:amount>
<epd:amount epd:module="B1">0</epd:amount>
<epd:amount epd:module="C1">0</epd:amount>
<epd:amount epd:module="C2" epd:scenario="S1">0.14907752182208</epd:amount>
<epd:amount epd:module="C2" epd:scenario="S2">0.14907752182208</epd:amount>
<epd:amount epd:module="C3" epd:scenario="S1">7.62154775E-06</epd:amount>
<epd:amount epd:module="C3" epd:scenario="S2">0.00500735687175</epd:amount>
<epd:amount epd:module="C4" epd:scenario="S1">8.580111752412</epd:amount>
<epd:amount epd:module="C4" epd:scenario="S2">0.377079392412</epd:amount>
<epd:amount epd:module="D">0.00298780671576455</epd:amount>
</common:other>
</exchange>
<exchange dataSetInternalID="13">
<referenceToFlowDataSet uri="../flows/3449546e-52ad-4b39-b809-9fb77cea8ff6.xml" type="flow data set" refObjectId="3449546e-52ad-4b39-b809-9fb77cea8ff6">
<common:shortDescription xml:lang="en">Radioactive waste disposed (RWD)</common:shortDescription>
</referenceToFlowDataSet>
<functionType>General reminder flow</functionType>
<exchangeDirection>Output</exchangeDirection>
<common:other>
<epd:referenceToUnitGroupDataSet uri="../unitgroups/ad38d542-3fe9-439d-9b95-2f5f7752acaf.xml" type="unit group data set" refObjectId="ad38d542-3fe9-439d-9b95-2f5f7752acaf">
<common:shortDescription xml:lang="en">kg</common:shortDescription>
</epd:referenceToUnitGroupDataSet>
<epd:amount epd:module="A1-A3">5.13765087647887E-05</epd:amount>
<epd:amount epd:module="A4">2.53223489100713E-05</epd:amount>
<epd:amount epd:module="A5">7.89194060433963E-06</epd:amount>
<epd:amount epd:module="B1">0</epd:amount>
<epd:amount epd:module="C1">0</epd:amount>
<epd:amount epd:module="C2" epd:scenario="S1">1.410171634104E-05</epd:amount>
<epd:amount epd:module="C2" epd:scenario="S2">1.410171634104E-05</epd:amount>
<epd:amount epd:module="C3" epd:scenario="S1">2.627957125E-08</epd:amount>
<epd:amount epd:module="C3" epd:scenario="S2">1.726567831125E-05</epd:amount>
<epd:amount epd:module="C4" epd:scenario="S1">8.539532962731E-06</epd:amount>
<epd:amount epd:module="C4" epd:scenario="S2">3.75296032731E-07</epd:amount>
<epd:amount epd:module="D">-2.10002852200667E-06</epd:amount>
</common:other>
</exchange>
<exchange dataSetInternalID="14">
<referenceToFlowDataSet uri="../flows/a2b32f97-3fc7-4af2-b209-525bc6426f33.xml" type="flow data set" refObjectId="a2b32f97-3fc7-4af2-b209-525bc6426f33">
<common:shortDescription xml:lang="en">Components for re-use (CRU)</common:shortDescription>
</referenceToFlowDataSet>
<functionType>General reminder flow</functionType>
<exchangeDirection>Output</exchangeDirection>
<common:other>
<epd:referenceToUnitGroupDataSet uri="../unitgroups/ad38d542-3fe9-439d-9b95-2f5f7752acaf.xml" type="unit group data set" refObjectId="ad38d542-3fe9-439d-9b95-2f5f7752acaf">
<common:shortDescription xml:lang="en">kg</common:shortDescription>
</epd:referenceToUnitGroupDataSet>
<epd:amount epd:module="A1-A3">0</epd:amount>
<epd:amount epd:module="A4">0</epd:amount>
<epd:amount epd:module="A5">0</epd:amount>
<epd:amount epd:module="B1">0</epd:amount>
<epd:amount epd:module="C1">0</epd:amount>
<epd:amount epd:module="C2" epd:scenario="S1">0</epd:amount>
<epd:amount epd:module="C2" epd:scenario="S2">0</epd:amount>
<epd:amount epd:module="C3" epd:scenario="S1">0</epd:amount>
<epd:amount epd:module="C3" epd:scenario="S2">0</epd:amount>
<epd:amount epd:module="C4" epd:scenario="S1">0</epd:amount>
<epd:amount epd:module="C4" epd:scenario="S2">0</epd:amount>
<epd:amount epd:module="D">0</epd:amount>
</common:other>
</exchange>
<exchange dataSetInternalID="15">
<referenceToFlowDataSet uri="../flows/d7fe48a5-4103-49c8-9aae-b0b5dfdbd6ae.xml" type="flow data set" refObjectId="d7fe48a5-4103-49c8-9aae-b0b5dfdbd6ae">
<common:shortDescription xml:lang="en">Materials for recycling (MFR)</common:shortDescription>
</referenceToFlowDataSet>
<functionType>General reminder flow</functionType>
<exchangeDirection>Output</exchangeDirection>
<common:other>
<epd:referenceToUnitGroupDataSet uri="../unitgroups/ad38d542-3fe9-439d-9b95-2f5f7752acaf.xml" type="unit group data set" refObjectId="ad38d542-3fe9-439d-9b95-2f5f7752acaf">
<common:shortDescription xml:lang="en">kg</common:shortDescription>
</epd:referenceToUnitGroupDataSet>
<epd:amount epd:module="A1-A3">0</epd:amount>
<epd:amount epd:module="A4">0</epd:amount>
<epd:amount epd:module="A5">0.20671890677753</epd:amount>
<epd:amount epd:module="B1">0</epd:amount>
<epd:amount epd:module="C1">0</epd:amount>
<epd:amount epd:module="C2" epd:scenario="S1">0</epd:amount>
<epd:amount epd:module="C2" epd:scenario="S2">0</epd:amount>
<epd:amount epd:module="C3" epd:scenario="S1">0.01125</epd:amount>
<epd:amount epd:module="C3" epd:scenario="S2">7.39125</epd:amount>
<epd:amount epd:module="C4" epd:scenario="S1">0</epd:amount>
<epd:amount epd:module="C4" epd:scenario="S2">0</epd:amount>
<epd:amount epd:module="D">0</epd:amount>
</common:other>
</exchange>
<exchange dataSetInternalID="16">
<referenceToFlowDataSet uri="../flows/59a9181c-3aaf-46ee-8b13-2b3723b6e447.xml" type="flow data set" refObjectId="59a9181c-3aaf-46ee-8b13-2b3723b6e447">
<common:shortDescription xml:lang="en">Materials for energy recovery (MER)</common:shortDescription>
</referenceToFlowDataSet>
<functionType>General reminder flow</functionType>
<exchangeDirection>Output</exchangeDirection>
<common:other>
<epd:referenceToUnitGroupDataSet uri="../unitgroups/ad38d542-3fe9-439d-9b95-2f5f7752acaf.xml" type="unit group data set" refObjectId="ad38d542-3fe9-439d-9b95-2f5f7752acaf">
<common:shortDescription xml:lang="en">kg</common:shortDescription>
</epd:referenceToUnitGroupDataSet>
<epd:amount epd:module="A1-A3">0</epd:amount>
<epd:amount epd:module="A4">0</epd:amount>
<epd:amount epd:module="A5">0</epd:amount>
<epd:amount epd:module="B1">0</epd:amount>
<epd:amount epd:module="C1">0</epd:amount>
<epd:amount epd:module="C2" epd:scenario="S1">0</epd:amount>
<epd:amount epd:module="C2" epd:scenario="S2">0</epd:amount>
<epd:amount epd:module="C3" epd:scenario="S1">0</epd:amount>
<epd:amount epd:module="C3" epd:scenario="S2">0</epd:amount>
<epd:amount epd:module="C4" epd:scenario="S1">0</epd:amount>
<epd:amount epd:module="C4" epd:scenario="S2">0</epd:amount>
<epd:amount epd:module="D">0</epd:amount>
</common:other>
</exchange>
<exchange dataSetInternalID="17">
<referenceToFlowDataSet uri="../flows/4da0c987-2b76-40d6-9e9e-82a017aaaf29.xml" type="flow data set" refObjectId="4da0c987-2b76-40d6-9e9e-82a017aaaf29">
<common:shortDescription xml:lang="en">Exported electrical energy (EEE)</common:shortDescription>
</referenceToFlowDataSet>
<functionType>General reminder flow</functionType>
<exchangeDirection>Output</exchangeDirection>
<common:other>
<epd:referenceToUnitGroupDataSet uri="../unitgroups/93a60a57-a3c8-11da-a746-0800200c9a66.xml" type="unit group data set" refObjectId="93a60a57-a3c8-11da-a746-0800200c9a66">
<common:shortDescription xml:lang="en">MJ</common:shortDescription>
</epd:referenceToUnitGroupDataSet>
<epd:amount epd:module="A1-A3">0</epd:amount>
<epd:amount epd:module="A4">0</epd:amount>
<epd:amount epd:module="A5">0</epd:amount>
<epd:amount epd:module="B1">0</epd:amount>
<epd:amount epd:module="C1">0</epd:amount>
<epd:amount epd:module="C2" epd:scenario="S1">0</epd:amount>
<epd:amount epd:module="C2" epd:scenario="S2">0</epd:amount>
<epd:amount epd:module="C3" epd:scenario="S1">0</epd:amount>
<epd:amount epd:module="C3" epd:scenario="S2">0</epd:amount>
<epd:amount epd:module="C4" epd:scenario="S1">0</epd:amount>
<epd:amount epd:module="C4" epd:scenario="S2">0</epd:amount>
<epd:amount epd:module="D">0</epd:amount>
</common:other>
</exchange>
<exchange dataSetInternalID="18">
<referenceToFlowDataSet uri="../flows/98daf38a-7a79-46d3-9a37-2b7bd0955810.xml" type="flow data set" refObjectId="98daf38a-7a79-46d3-9a37-2b7bd0955810">
<common:shortDescription xml:lang="en">Exported thermal energy (EET)</common:shortDescription>
</referenceToFlowDataSet>
<functionType>General reminder flow</functionType>
<exchangeDirection>Output</exchangeDirection>
<common:other>
<epd:referenceToUnitGroupDataSet uri="../unitgroups/93a60a57-a3c8-11da-a746-0800200c9a66.xml" type="unit group data set" refObjectId="93a60a57-a3c8-11da-a746-0800200c9a66">
<common:shortDescription xml:lang="en">MJ</common:shortDescription>
</epd:referenceToUnitGroupDataSet>
<epd:amount epd:module="A1-A3">0</epd:amount>
<epd:amount epd:module="A4">0</epd:amount>
<epd:amount epd:module="A5">0</epd:amount>
<epd:amount epd:module="B1">0</epd:amount>
<epd:amount epd:module="C1">0</epd:amount>
<epd:amount epd:module="C2" epd:scenario="S1">0</epd:amount>
<epd:amount epd:module="C2" epd:scenario="S2">0</epd:amount>
<epd:amount epd:module="C3" epd:scenario="S1">0</epd:amount>
<epd:amount epd:module="C3" epd:scenario="S2">0</epd:amount>
<epd:amount epd:module="C4" epd:scenario="S1">0</epd:amount>
<epd:amount epd:module="C4" epd:scenario="S2">0</epd:amount>
<epd:amount epd:module="D">0</epd:amount>
</common:other>
</exchange>
</exchanges>
<LCIAResults>
<LCIAResult>
<referenceToLCIAMethodDataSet uri="../lciamethods/77e416eb-a363-4258-a04e-171d843a6460.xml" type="LCIA method data set" refObjectId="77e416eb-a363-4258-a04e-171d843a6460">
<common:shortDescription xml:lang="en">Global warming potential (GWP)</common:shortDescription>
</referenceToLCIAMethodDataSet>
<common:other>
<epd:referenceToUnitGroupDataSet uri="../unitgroups/1ebf3012-d0db-4de2-aefd-ef30cedb0be1.xml" type="unit group data set" refObjectId="1ebf3012-d0db-4de2-aefd-ef30cedb0be1">
<common:shortDescription xml:lang="en">kg CO_(2)-Äq.</common:shortDescription>
</epd:referenceToUnitGroupDataSet>
<epd:amount epd:module="A1-A3">1.96528725094384</epd:amount>
<epd:amount epd:module="A4">0.254459120203534</epd:amount>
<epd:amount epd:module="A5">0.197590582551817</epd:amount>
<epd:amount epd:module="B1">0</epd:amount>
<epd:amount epd:module="C1">0</epd:amount>
<epd:amount epd:module="C2" epd:scenario="S1">0.14075216415488</epd:amount>
<epd:amount epd:module="C2" epd:scenario="S2">0.14075216415488</epd:amount>
<epd:amount epd:module="C3" epd:scenario="S1">4.760716375E-05</epd:amount>
<epd:amount epd:module="C3" epd:scenario="S2">0.03127790658375</epd:amount>
<epd:amount epd:module="C4" epd:scenario="S1">0.045469778565978</epd:amount>
<epd:amount epd:module="C4" epd:scenario="S2">0.001998309225978</epd:amount>
<epd:amount epd:module="D">-0.0375350102735811</epd:amount>
</common:other>
</LCIAResult>
<LCIAResult>
<referenceToLCIAMethodDataSet uri="../lciamethods/06dcd26f-025f-401a-a7c1-5e457eb54637.xml" type="LCIA method data set" refObjectId="06dcd26f-025f-401a-a7c1-5e457eb54637">
<common:shortDescription xml:lang="en">Depletion potential of the stratospheric ozone layer (ODP)</common:shortDescription>
</referenceToLCIAMethodDataSet>
<common:other>
<epd:referenceToUnitGroupDataSet uri="../unitgroups/88054749-b0a6-47ea-a82b-dc5b29326512.xml" type="unit group data set" refObjectId="88054749-b0a6-47ea-a82b-dc5b29326512">
<common:shortDescription xml:lang="en">kg CFC11-Äq.</common:shortDescription>
</epd:referenceToUnitGroupDataSet>
<epd:amount epd:module="A1-A3">2.47693149156594E-07</epd:amount>
<epd:amount epd:module="A4">4.46630034942567E-08</epd:amount>
<epd:amount epd:module="A5">2.09354149635827E-08</epd:amount>
<epd:amount epd:module="B1">0</epd:amount>
<epd:amount epd:module="C1">0</epd:amount>
<epd:amount epd:module="C2" epd:scenario="S1">2.485534627504E-08</epd:amount>
<epd:amount epd:module="C2" epd:scenario="S2">2.485534627504E-08</epd:amount>
<epd:amount epd:module="C3" epd:scenario="S1">1.939947125E-11</epd:amount>
<epd:amount epd:module="C3" epd:scenario="S2">1.274545261125E-08</epd:amount>
<epd:amount epd:module="C4" epd:scenario="S1">1.5165434822772E-08</epd:amount>
<epd:amount epd:module="C4" epd:scenario="S2">6.66491662772E-10</epd:amount>
<epd:amount epd:module="D">-6.36471259989548E-09</epd:amount>
</common:other>
</LCIAResult>
<LCIAResult>
<referenceToLCIAMethodDataSet uri="../lciamethods/b4274add-93b7-4905-a5e4-2e878c4e4216.xml" type="LCIA method data set" refObjectId="b4274add-93b7-4905-a5e4-2e878c4e4216">
<common:shortDescription xml:lang="en">Acidification potential of land and water (AP)</common:shortDescription>
</referenceToLCIAMethodDataSet>
<common:other>
<epd:referenceToUnitGroupDataSet uri="../unitgroups/bc50c624-a9bc-45b1-a9b0-e6b10d00476f.xml" type="unit group data set" refObjectId="bc50c624-a9bc-45b1-a9b0-e6b10d00476f">
<common:shortDescription xml:lang="en">kg SO_(2)-Äq.</common:shortDescription>
</epd:referenceToUnitGroupDataSet>
<epd:amount epd:module="A1-A3">0.00387810418181067</epd:amount>
<epd:amount epd:module="A4">0.00104828322795355</epd:amount>
<epd:amount epd:module="A5">0.000619320401547924</epd:amount>
<epd:amount epd:module="B1">0</epd:amount>
<epd:amount epd:module="C1">0</epd:amount>
<epd:amount epd:module="C2" epd:scenario="S1">0.0005781751339008</epd:amount>
<epd:amount epd:module="C2" epd:scenario="S2">0.0005781751339008</epd:amount>
<epd:amount epd:module="C3" epd:scenario="S1">3.491517625E-07</epd:amount>
<epd:amount epd:module="C3" epd:scenario="S2">0.0002293927079625</epd:amount>
<epd:amount epd:module="C4" epd:scenario="S1">0.00033857607023346</epd:amount>
<epd:amount epd:module="C4" epd:scenario="S2">1.487976643346E-05</epd:amount>
<epd:amount epd:module="D">-0.00024491425620345</epd:amount>
</common:other>
</LCIAResult>
<LCIAResult>
<referenceToLCIAMethodDataSet uri="../lciamethods/f58827d0-b407-4ec6-be75-8b69efb98a0f.xml" type="LCIA method data set" refObjectId="f58827d0-b407-4ec6-be75-8b69efb98a0f">
<common:shortDescription xml:lang="en">Eutrophication potential (EP)</common:shortDescription>
</referenceToLCIAMethodDataSet>
<common:other>
<epd:referenceToUnitGroupDataSet uri="../unitgroups/67b5401d-873c-485f-bcf3-6ae83b918822.xml" type="unit group data set" refObjectId="67b5401d-873c-485f-bcf3-6ae83b918822">
<common:shortDescription xml:lang="en">kg PO_(4)^(3)-Äq.</common:shortDescription>
</epd:referenceToUnitGroupDataSet>
<epd:amount epd:module="A1-A3">0.000947264410582756</epd:amount>
<epd:amount epd:module="A4">0.000272020700929614</epd:amount>
<epd:amount epd:module="A5">0.000111093294816411</epd:amount>
<epd:amount epd:module="B1">0</epd:amount>
<epd:amount epd:module="C1">0</epd:amount>
<epd:amount epd:module="C2" epd:scenario="S1">0.00014900164270912</epd:amount>
<epd:amount epd:module="C2" epd:scenario="S2">0.00014900164270912</epd:amount>
<epd:amount epd:module="C3" epd:scenario="S1">7.3401545E-08</epd:amount>
<epd:amount epd:module="C3" epd:scenario="S2">4.8224815065E-05</epd:amount>
<epd:amount epd:module="C4" epd:scenario="S1">5.8390192482198E-05</epd:amount>
<epd:amount epd:module="C4" epd:scenario="S2">2.566136542198E-06</epd:amount>
<epd:amount epd:module="D">-5.19306452274637E-05</epd:amount>
</common:other>
</LCIAResult>
<LCIAResult>
<referenceToLCIAMethodDataSet uri="../lciamethods/1e84a202-dae6-42aa-9e9d-71ea48b8be00.xml" type="LCIA method data set" refObjectId="1e84a202-dae6-42aa-9e9d-71ea48b8be00">
<common:shortDescription xml:lang="en">Formation potential of tropospheric ozone photochemical oxidants (POCP)</common:shortDescription>
</referenceToLCIAMethodDataSet>
<common:other>
<epd:referenceToUnitGroupDataSet uri="../unitgroups/01c26c17-9a76-406e-8295-f17b55fd909e.xml" type="unit group data set" refObjectId="01c26c17-9a76-406e-8295-f17b55fd909e">
<common:shortDescription xml:lang="en">kg Ethen-Äq.</common:shortDescription>
</epd:referenceToUnitGroupDataSet>
<epd:amount epd:module="A1-A3">0.000563365849307516</epd:amount>
<epd:amount epd:module="A4">0.000137971053028916</epd:amount>
<epd:amount epd:module="A5">7.17684826688591E-05</epd:amount>
<epd:amount epd:module="B1">0</epd:amount>
<epd:amount epd:module="C1">0</epd:amount>
<epd:amount epd:module="C2" epd:scenario="S1">7.584652891936E-05</epd:amount>
<epd:amount epd:module="C2" epd:scenario="S2">7.584652891936E-05</epd:amount>
<epd:amount epd:module="C3" epd:scenario="S1">3.702100875E-08</epd:amount>
<epd:amount epd:module="C3" epd:scenario="S2">2.432280274875E-05</epd:amount>
<epd:amount epd:module="C4" epd:scenario="S1">4.2155889961992E-05</epd:amount>
<epd:amount epd:module="C4" epd:scenario="S2">1.852670201992E-06</epd:amount>
<epd:amount epd:module="D">-2.06235810279714E-05</epd:amount>
</common:other>
</LCIAResult>
<LCIAResult>
<referenceToLCIAMethodDataSet uri="../lciamethods/f7c73bb9-ab1a-4249-9c6d-379a0de6f67e.xml" type="LCIA method data set" refObjectId="f7c73bb9-ab1a-4249-9c6d-379a0de6f67e">
<common:shortDescription xml:lang="en">Abiotic depletion potential for non fossil resources (ADPE)</common:shortDescription>
</referenceToLCIAMethodDataSet>
<common:other>
<epd:referenceToUnitGroupDataSet uri="../unitgroups/54ccd2d9-a32a-4fc2-923d-f2c8c93e89d4.xml" type="unit group data set" refObjectId="54ccd2d9-a32a-4fc2-923d-f2c8c93e89d4">
<common:shortDescription xml:lang="en">kg Sb-Äq.</common:shortDescription>
</epd:referenceToUnitGroupDataSet>
<epd:amount epd:module="A1-A3">1.73641600233038E-05</epd:amount>
<epd:amount epd:module="A4">3.07196070912028E-06</epd:amount>
<epd:amount epd:module="A5">1.22959423403614E-06</epd:amount>
<epd:amount epd:module="B1">0</epd:amount>
<epd:amount epd:module="C1">0</epd:amount>
<epd:amount epd:module="C2" epd:scenario="S1">1.6367519135504E-06</epd:amount>
<epd:amount epd:module="C2" epd:scenario="S2">1.6367519135504E-06</epd:amount>
<epd:amount epd:module="C3" epd:scenario="S1">8.99294125E-11</epd:amount>
<epd:amount epd:module="C3" epd:scenario="S2">5.90836240125E-08</epd:amount>
<epd:amount epd:module="C4" epd:scenario="S1">5.7417914852268E-08</epd:amount>
<epd:amount epd:module="C4" epd:scenario="S2">2.523406812268E-09</epd:amount>
<epd:amount epd:module="D">-1.57164241533279E-07</epd:amount>
</common:other>
</LCIAResult>
<LCIAResult>
<referenceToLCIAMethodDataSet uri="../lciamethods/804ebcdf-309d-4098-8ed8-fdaf2f389981.xml" type="LCIA method data set" refObjectId="804ebcdf-309d-4098-8ed8-fdaf2f389981">
<common:shortDescription xml:lang="en">Abiotic depletion potential for fossil resources (ADPF)</common:shortDescription>
</referenceToLCIAMethodDataSet>
<common:other>
<epd:referenceToUnitGroupDataSet uri="../unitgroups/93a60a57-a3c8-11da-a746-0800200c9a66.xml" type="unit group data set" refObjectId="93a60a57-a3c8-11da-a746-0800200c9a66">
<common:shortDescription xml:lang="en">MJ</common:shortDescription>
</epd:referenceToUnitGroupDataSet>
<epd:amount epd:module="A1-A3">33.6360100415654</epd:amount>
<epd:amount epd:module="A4">3.94162535543687</epd:amount>
<epd:amount epd:module="A5">3.03410803847883</epd:amount>
<epd:amount epd:module="B1">0</epd:amount>
<epd:amount epd:module="C1">0</epd:amount>
<epd:amount epd:module="C2" epd:scenario="S1">2.180785161552</epd:amount>
<epd:amount epd:module="C2" epd:scenario="S2">2.180785161552</epd:amount>
<epd:amount epd:module="C3" epd:scenario="S1">0.000687328125</epd:amount>
<epd:amount epd:module="C3" epd:scenario="S2">0.451574578125</epd:amount>
<epd:amount epd:module="C4" epd:scenario="S1">1.2993203832918</epd:amount>
<epd:amount epd:module="C4" epd:scenario="S2">0.0571026292918</epd:amount>
<epd:amount epd:module="D">-0.538665054861864</epd:amount>
</common:other>
</LCIAResult>
</LCIAResults>
</processDataSet>