<?xml version="1.0" encoding="utf-8"?>
<processDataSet xmlns:epd="http://www.iai.kit.edu/EPD/2013" xmlns:common="http://lca.jrc.it/ILCD/Common" xsi:schemaLocation="http://lca.jrc.it/ILCD/Process ../../schemas/EPD_DataSet.xsd" version="1.1" locations="../ILCDLocations.xml" xmlns:xsi="http://www.w3.org/2001/XMLSchema-instance" xmlns="http://lca.jrc.it/ILCD/Process">
<processInformation>
<dataSetInformation>
<common:UUID>b8352556-534e-495c-a2c7-be994ba56a94</common:UUID>
<name>
<baseName xml:lang="en">Cork floor tiles according to EN 12104</baseName>
<functionalUnitFlowProperties xml:lang="en" />
</name>
<classificationInformation>
<common:classification name="OEKOBAU.DAT">
<common:class level="0" classId="3">Holz</common:class>
<common:class level="1" classId="3.3">Holzböden</common:class>
<common:class level="2" classId="3.3.03">Kork</common:class>
</common:classification>
<common:classification name="IBUCategories">
<common:class level="0">02 Building products</common:class>
<common:class level="1">Floor coverings</common:class>
<common:class level="2">Floor coverings</common:class>
</common:classification>
</classificationInformation>
<common:generalComment xml:lang="en">Resilient floor coverings are an entire product family of flexible flooring solutions available in sheet, tiles and planks. It is classified in heterogeneous or homogeneous composition based on plastics, linoleum, cork or rubber. Resilient floor coverings can provide different functionalities (acoustic, static control, slip resistance, easy maintenance etc.) to match a wide range of domestic, commercial and industrial applications. It is available in an enormous range of patterns and colours fitting with inspiration and decorative needs. Cork floor tiles are produced of cork and binders. The cork is produced by stripping the bark from cork oak trees every nine years. Primarily this cork is treated in a boiling process and used for wine cork stoppers. Leftovers from the wine cork stoppers industry and bark cork trees from pruning are granulate in different sizes. For the flooring production the cork granules are mixed with an adhesive. This mixture is cured under temperature and pressure. The cork flooring surface is finally decorated with colour and finished with a UV varnish in order to guarantee wear resistance of the surface.</common:generalComment>
<common:other>
<epd:scenarios>
<epd:scenario epd:name="S1">
<epd:description xml:lang="en">100% incineration</epd:description>
</epd:scenario>
<epd:scenario epd:name="S2">
<epd:description xml:lang="en">100% landfilling</epd:description>
</epd:scenario>
</epd:scenarios>
</common:other>
</dataSetInformation>
<quantitativeReference>
<referenceToReferenceFlow>0</referenceToReferenceFlow>
</quantitativeReference>
<time>
<common:referenceYear>2019</common:referenceYear>
<common:dataSetValidUntil>2024</common:dataSetValidUntil>
</time>
<geography>
<locationOfOperationSupplyOrProduction location="RER" />
</geography>
<technology>
<technologyDescriptionAndIncludedProcesses xml:lang="en">Resilient floor coverings are an entire product family of flexible flooring solutions available in sheet, tiles and planks. It is classified in heterogeneous or homogeneous composition based on plastics, linoleum, cork or rubber. Resilient floor coverings can provide different functionalities (acoustic, static control, slip resistance, easy maintenance etc.) to match a wide range of domestic, commercial and industrial applications. It is available in an enormous range of patterns and colours fitting with inspiration and decorative needs. Cork floor tiles are produced of cork and binders. The cork is produced by stripping the bark from cork oak trees every nine years. Primarily this cork is treated in a boiling process and used for wine cork stoppers. Leftovers from the wine cork stoppers industry and bark cork trees from pruning are granulate in different sizes. For the flooring production the cork granules are mixed with an adhesive. This mixture is cured under temperature and pressure. The cork flooring surface is finally decorated with colour and finished with a UV varnish in order to guarantee wear resistance of the surface. 
Technical data: 
The following table contains the construction data of the declared product group: 
Declared unit: 
1m² of floor covering.</technologyDescriptionAndIncludedProcesses>
<technologicalApplicability xml:lang="en">According to /EN ISO 10874/ the area of application for resilient floor coverings is indicated by use classes. The declared product group covers the use class 23.</technologicalApplicability>
</technology>
</processInformation>
<modellingAndValidation>
<LCIMethodAndAllocation>
<typeOfDataSet>EPD</typeOfDataSet>
<referenceToLCAMethodDetails type="source data set" refObjectId="87b9ef69-fd47-4188-9fbb-8ec484dd7006">
<common:shortDescription xml:lang="en">Floor coverings.pdf</common:shortDescription>
</referenceToLCAMethodDetails>
<common:other>
<epd:subType xmlns="http://www.iai.kit.edu/EPD/2013">average dataset</epd:subType>
</common:other>
</LCIMethodAndAllocation>
<dataSourcesTreatmentAndRepresentativeness>
<referenceToDataSource type="source data set" refObjectId="688c0033-f749-4eb2-acb7-d756783797c9">
<common:shortDescription xml:lang="en">Cork floor tiles according to EN 12104.pdf</common:shortDescription>
</referenceToDataSource>
<referenceToDataSource type="source data set" refObjectId="28d74cc0-db8b-4d7e-bc44-5f6d56ce0c4a">
<common:shortDescription xml:lang="en">GaBi Database (all versions)</common:shortDescription>
</referenceToDataSource>
<referenceToDataSource type="source data set" refObjectId="d8181616-4417-4dbd-9614-09937353f17a">
<common:shortDescription xml:lang="en">GaBi database SP33 2017</common:shortDescription>
</referenceToDataSource>
<useAdviceForDataSet xml:lang="en">Scope: 
In this EPD cork floor tiles are declared. The application of this EPD is restricted to cork floor tiles produced by the members of the European Resilient Flooring Manufacturers’ Institute (ERFMI). Data are based upon production during 2017 in Europe. Data have been provided by one company of ERFMI which represent 100% of ERFMI members. 
System boundary: 
Type of EPD: cradle to graveModules A1-A3 include processes that provide materials and energy input for the system, manufacturing and transport processes up to the factory gate, as well as waste processing.Module A4 includes transport of the floor covering to the place of installation.Module A5 includes the production of offcuts and adhesive for the installation of the floor covering, and incineration of offcuts and packaging material.Module B2 is including provision of cleaning agent, energy and water consumption for the cleaning of the floor covering incl. waste water  treatment. The LCA results in this EPD are declared for a one-year usage.Module C1 considers electricity supply for the deconstruction of the flooring.Module C2 includes transportation of the postconsumer waste to waste processing.End of life scenarios are declared for:100% incineration in a waste incineration plant (WIP) (Scenario 1, C3/1)100% landfilling (Scenario 2, C4/2)Module D declares potential benefits from all net flows given in module A5 and C3 (for incineration and related energy substitution) that leave the product boundary system after having passed the end-of-waste state.Module D is declared for each scenario separately.</useAdviceForDataSet>
</dataSourcesTreatmentAndRepresentativeness>
<validation>
<review type="Accredited third party review">
<common:referenceToNameOfReviewerAndInstitution uri="../contacts/d111dbec-b024-4be5-86c5-752d6eb2cf95.xml" type="contact data set" refObjectId="d111dbec-b024-4be5-86c5-752d6eb2cf95">
<common:shortDescription xml:lang="en">Institut Bauen und Umwelt e. V.</common:shortDescription>
</common:referenceToNameOfReviewerAndInstitution>
</review>
</validation>
<complianceDeclarations>
<compliance>
<common:referenceToComplianceSystem uri="../sources/b00f9ec0-7874-11e3-981f-0800200c9a66.xml" type="source data set" refObjectId="b00f9ec0-7874-11e3-981f-0800200c9a66">
<common:shortDescription xml:lang="en">DIN EN 15804</common:shortDescription>
</common:referenceToComplianceSystem>
</compliance>
<compliance>
<common:referenceToComplianceSystem uri="../sources/4f2eb655-6e44-4874-a95a-e28f5442cd4d.xml" type="source data set" refObjectId="4f2eb655-6e44-4874-a95a-e28f5442cd4d">
<common:shortDescription xml:lang="en">ISO 14025</common:shortDescription>
</common:referenceToComplianceSystem>
</compliance>
</complianceDeclarations>
</modellingAndValidation>
<administrativeInformation>
<dataEntryBy>
<common:timeStamp>2019-03-05T14:58:39.44</common:timeStamp>
<common:referenceToDataSetFormat uri="../sources/a97a0155-0234-4b87-b4ce-a45da52f2a40.xml" type="source data set" refObjectId="a97a0155-0234-4b87-b4ce-a45da52f2a40">
<common:shortDescription xml:lang="en">ILCD Format 1.1</common:shortDescription>
</common:referenceToDataSetFormat>
<common:referenceToDataSetFormat uri="../sources/cba73800-7874-11e3-981f-0800200c9a66.xml" type="source data set" refObjectId="cba73800-7874-11e3-981f-0800200c9a66">
<common:shortDescription xml:lang="en">EPD Data Format Extensions</common:shortDescription>
</common:referenceToDataSetFormat>
<common:referenceToPersonOrEntityEnteringTheData uri="../contacts/623edf96-39d1-4e6f-9892-674c7228546b.xml" type="contact data set" refObjectId="623edf96-39d1-4e6f-9892-674c7228546b">
<common:shortDescription xml:lang="en">thinkstep AG</common:shortDescription>
</common:referenceToPersonOrEntityEnteringTheData>
</dataEntryBy>
<publicationAndOwnership>
<common:dataSetVersion>00.03.000</common:dataSetVersion>
<common:referenceToRegistrationAuthority uri="../contacts/d111dbec-b024-4be5-86c5-752d6eb2cf95.xml" type="contact data set" refObjectId="d111dbec-b024-4be5-86c5-752d6eb2cf95">
<common:shortDescription xml:lang="en">Institut Bauen und Umwelt e. V.</common:shortDescription>
</common:referenceToRegistrationAuthority>
<common:registrationNumber>EPD-ERF-20180184-CCI1-EN</common:registrationNumber>
<common:referenceToOwnershipOfDataSet uri="../contacts/3b24532d-7001-4793-b5c3-0f0c4bb35f4e.xml" type="contact data set" refObjectId="3b24532d-7001-4793-b5c3-0f0c4bb35f4e">
<common:shortDescription xml:lang="en">ERFMI vzw, European Resilient Flooring Manufacturers' Institute</common:shortDescription>
</common:referenceToOwnershipOfDataSet>
<common:copyright>true</common:copyright>
</publicationAndOwnership>
</administrativeInformation>
<exchanges>
<exchange dataSetInternalID="0">
<referenceToFlowDataSet uri="../flows/f3993b52-6274-e302-a0ed-3cda2fc881d3.xml" type="flow data set" refObjectId="f3993b52-6274-e302-a0ed-3cda2fc881d3">
<common:shortDescription xml:lang="en">cork floor tiles (2.0 kg/m²) (cork floor tiles (2.0 kg/m²))</common:shortDescription>
</referenceToFlowDataSet>
<meanAmount>1</meanAmount>
<referencesToDataSource />
</exchange>
<exchange dataSetInternalID="1">
<referenceToFlowDataSet uri="../flows/20f32be5-0398-4288-9b6d-accddd195317.xml" type="flow data set" refObjectId="20f32be5-0398-4288-9b6d-accddd195317">
<common:shortDescription xml:lang="en">Renewable primary energy as energy carrier (PERE)</common:shortDescription>
</referenceToFlowDataSet>
<functionType>General reminder flow</functionType>
<exchangeDirection>Input</exchangeDirection>
<referencesToDataSource />
<common:other>
<epd:referenceToUnitGroupDataSet uri="../unitgroups/93a60a57-a3c8-11da-a746-0800200c9a66.xml" type="unit group data set" refObjectId="93a60a57-a3c8-11da-a746-0800200c9a66">
<common:shortDescription xml:lang="en">MJ</common:shortDescription>
</epd:referenceToUnitGroupDataSet>
<epd:amount epd:module="A1-A3">28.8126</epd:amount>
<epd:amount epd:module="A4">0.166688</epd:amount>
<epd:amount epd:module="A5">7.69892</epd:amount>
<epd:amount epd:module="B2">1.59</epd:amount>
<epd:amount epd:module="C1">0.0854</epd:amount>
<epd:amount epd:module="C2">0.0139</epd:amount>
<epd:amount epd:module="C3">30.533</epd:amount>
<epd:amount epd:module="C4">0.157</epd:amount>
<epd:amount epd:module="D" epd:scenario="S1">-3.341</epd:amount>
<epd:amount epd:module="D" epd:scenario="S2">-0.654</epd:amount>
</common:other>
</exchange>
<exchange dataSetInternalID="2">
<referenceToFlowDataSet uri="../flows/fb3ec0de-548d-4508-aea5-00b73bf6f702.xml" type="flow data set" refObjectId="fb3ec0de-548d-4508-aea5-00b73bf6f702">
<common:shortDescription xml:lang="en">Renewable primary energy resources as material utilization (PERM)</common:shortDescription>
</referenceToFlowDataSet>
<functionType>General reminder flow</functionType>
<exchangeDirection>Input</exchangeDirection>
<referencesToDataSource />
<common:other>
<epd:referenceToUnitGroupDataSet uri="../unitgroups/93a60a57-a3c8-11da-a746-0800200c9a66.xml" type="unit group data set" refObjectId="93a60a57-a3c8-11da-a746-0800200c9a66">
<common:shortDescription xml:lang="en">MJ</common:shortDescription>
</epd:referenceToUnitGroupDataSet>
<epd:amount epd:module="A1-A3">30.4</epd:amount>
<epd:amount epd:module="A4">0</epd:amount>
<epd:amount epd:module="A5">-2.472</epd:amount>
<epd:amount epd:module="B2">0</epd:amount>
<epd:amount epd:module="C1">0</epd:amount>
<epd:amount epd:module="C2">0</epd:amount>
<epd:amount epd:module="C3">-30.4</epd:amount>
<epd:amount epd:module="C4">0</epd:amount>
<epd:amount epd:module="D" epd:scenario="S1">0</epd:amount>
<epd:amount epd:module="D" epd:scenario="S2">0</epd:amount>
</common:other>
</exchange>
<exchange dataSetInternalID="3">
<referenceToFlowDataSet uri="../flows/53f97275-fa8a-4cdd-9024-65936002acd0.xml" type="flow data set" refObjectId="53f97275-fa8a-4cdd-9024-65936002acd0">
<common:shortDescription xml:lang="en">Total use of renewable primary energy resources (PERT)</common:shortDescription>
</referenceToFlowDataSet>
<functionType>General reminder flow</functionType>
<exchangeDirection>Input</exchangeDirection>
<referencesToDataSource />
<common:other>
<epd:referenceToUnitGroupDataSet uri="../unitgroups/93a60a57-a3c8-11da-a746-0800200c9a66.xml" type="unit group data set" refObjectId="93a60a57-a3c8-11da-a746-0800200c9a66">
<common:shortDescription xml:lang="en">MJ</common:shortDescription>
</epd:referenceToUnitGroupDataSet>
<epd:amount epd:module="A1-A3">59.2126</epd:amount>
<epd:amount epd:module="A4">0.166688</epd:amount>
<epd:amount epd:module="A5">5.22692</epd:amount>
<epd:amount epd:module="B2">1.59</epd:amount>
<epd:amount epd:module="C1">0.0854</epd:amount>
<epd:amount epd:module="C2">0.0139</epd:amount>
<epd:amount epd:module="C3">0.133</epd:amount>
<epd:amount epd:module="C4">0.157</epd:amount>
<epd:amount epd:module="D" epd:scenario="S1">-3.341</epd:amount>
<epd:amount epd:module="D" epd:scenario="S2">-0.654</epd:amount>
</common:other>
</exchange>
<exchange dataSetInternalID="4">
<referenceToFlowDataSet uri="../flows/ac857178-2b45-46ec-892a-a9a4332f0372.xml" type="flow data set" refObjectId="ac857178-2b45-46ec-892a-a9a4332f0372">
<common:shortDescription xml:lang="en">Non renewable primary energy as energy carrier (PENRE)</common:shortDescription>
</referenceToFlowDataSet>
<functionType>General reminder flow</functionType>
<exchangeDirection>Input</exchangeDirection>
<referencesToDataSource />
<common:other>
<epd:referenceToUnitGroupDataSet uri="../unitgroups/93a60a57-a3c8-11da-a746-0800200c9a66.xml" type="unit group data set" refObjectId="93a60a57-a3c8-11da-a746-0800200c9a66">
<common:shortDescription xml:lang="en">MJ</common:shortDescription>
</epd:referenceToUnitGroupDataSet>
<epd:amount epd:module="A1-A3">28.2228</epd:amount>
<epd:amount epd:module="A4">3.02212</epd:amount>
<epd:amount epd:module="A5">11.9054</epd:amount>
<epd:amount epd:module="B2">5.13</epd:amount>
<epd:amount epd:module="C1">0.227</epd:amount>
<epd:amount epd:module="C2">0.252</epd:amount>
<epd:amount epd:module="C3">9.598</epd:amount>
<epd:amount epd:module="C4">2.11</epd:amount>
<epd:amount epd:module="D" epd:scenario="S1">-17.18</epd:amount>
<epd:amount epd:module="D" epd:scenario="S2">-3.37</epd:amount>
</common:other>
</exchange>
<exchange dataSetInternalID="5">
<referenceToFlowDataSet uri="../flows/1421caa0-679d-4bf4-b282-0eb850ccae27.xml" type="flow data set" refObjectId="1421caa0-679d-4bf4-b282-0eb850ccae27">
<common:shortDescription xml:lang="en">Non renewable primary energy as material utilization (PENRM)</common:shortDescription>
</referenceToFlowDataSet>
<functionType>General reminder flow</functionType>
<exchangeDirection>Input</exchangeDirection>
<referencesToDataSource />
<common:other>
<epd:referenceToUnitGroupDataSet uri="../unitgroups/93a60a57-a3c8-11da-a746-0800200c9a66.xml" type="unit group data set" refObjectId="93a60a57-a3c8-11da-a746-0800200c9a66">
<common:shortDescription xml:lang="en">MJ</common:shortDescription>
</epd:referenceToUnitGroupDataSet>
<epd:amount epd:module="A1-A3">8.6</epd:amount>
<epd:amount epd:module="A4">0</epd:amount>
<epd:amount epd:module="A5">-0.52</epd:amount>
<epd:amount epd:module="B2">0</epd:amount>
<epd:amount epd:module="C1">0</epd:amount>
<epd:amount epd:module="C2">0</epd:amount>
<epd:amount epd:module="C3">-8.6</epd:amount>
<epd:amount epd:module="C4">0</epd:amount>
<epd:amount epd:module="D" epd:scenario="S1">0</epd:amount>
<epd:amount epd:module="D" epd:scenario="S2">0</epd:amount>
</common:other>
</exchange>
<exchange dataSetInternalID="6">
<referenceToFlowDataSet uri="../flows/06159210-646b-4c8d-8583-da9b3b95a6c1.xml" type="flow data set" refObjectId="06159210-646b-4c8d-8583-da9b3b95a6c1">
<common:shortDescription xml:lang="en">Total use of non renewable primary energy resources (PENRT)</common:shortDescription>
</referenceToFlowDataSet>
<functionType>General reminder flow</functionType>
<exchangeDirection>Input</exchangeDirection>
<referencesToDataSource />
<common:other>
<epd:referenceToUnitGroupDataSet uri="../unitgroups/93a60a57-a3c8-11da-a746-0800200c9a66.xml" type="unit group data set" refObjectId="93a60a57-a3c8-11da-a746-0800200c9a66">
<common:shortDescription xml:lang="en">MJ</common:shortDescription>
</epd:referenceToUnitGroupDataSet>
<epd:amount epd:module="A1-A3">36.8228</epd:amount>
<epd:amount epd:module="A4">3.02212</epd:amount>
<epd:amount epd:module="A5">11.3854</epd:amount>
<epd:amount epd:module="B2">5.13</epd:amount>
<epd:amount epd:module="C1">0.227</epd:amount>
<epd:amount epd:module="C2">0.252</epd:amount>
<epd:amount epd:module="C3">0.998</epd:amount>
<epd:amount epd:module="C4">2.11</epd:amount>
<epd:amount epd:module="D" epd:scenario="S1">-17.18</epd:amount>
<epd:amount epd:module="D" epd:scenario="S2">-3.37</epd:amount>
</common:other>
</exchange>
<exchange dataSetInternalID="7">
<referenceToFlowDataSet uri="../flows/c6a1f35f-2d09-4f54-8dfb-97e502e1ce92.xml" type="flow data set" refObjectId="c6a1f35f-2d09-4f54-8dfb-97e502e1ce92">
<common:shortDescription xml:lang="en">Use of secondary material (SM)</common:shortDescription>
</referenceToFlowDataSet>
<functionType>General reminder flow</functionType>
<exchangeDirection>Input</exchangeDirection>
<referencesToDataSource />
<common:other>
<epd:referenceToUnitGroupDataSet uri="../unitgroups/ad38d542-3fe9-439d-9b95-2f5f7752acaf.xml" type="unit group data set" refObjectId="ad38d542-3fe9-439d-9b95-2f5f7752acaf">
<common:shortDescription xml:lang="en">kg</common:shortDescription>
</epd:referenceToUnitGroupDataSet>
<epd:amount epd:module="A1-A3">0.483721</epd:amount>
<epd:amount epd:module="A4">0</epd:amount>
<epd:amount epd:module="A5">0.0227931</epd:amount>
<epd:amount epd:module="B2">0</epd:amount>
<epd:amount epd:module="C1">0</epd:amount>
<epd:amount epd:module="C2">0</epd:amount>
<epd:amount epd:module="C3">0</epd:amount>
<epd:amount epd:module="C4">0</epd:amount>
<epd:amount epd:module="D" epd:scenario="S1">0</epd:amount>
<epd:amount epd:module="D" epd:scenario="S2">0</epd:amount>
</common:other>
</exchange>
<exchange dataSetInternalID="8">
<referenceToFlowDataSet uri="../flows/64333088-a55f-4aa2-9a31-c10b07816787.xml" type="flow data set" refObjectId="64333088-a55f-4aa2-9a31-c10b07816787">
<common:shortDescription xml:lang="en">Use of renewable secondary fuels (RSF)</common:shortDescription>
</referenceToFlowDataSet>
<functionType>General reminder flow</functionType>
<exchangeDirection>Input</exchangeDirection>
<referencesToDataSource />
<common:other>
<epd:referenceToUnitGroupDataSet uri="../unitgroups/93a60a57-a3c8-11da-a746-0800200c9a66.xml" type="unit group data set" refObjectId="93a60a57-a3c8-11da-a746-0800200c9a66">
<common:shortDescription xml:lang="en">MJ</common:shortDescription>
</epd:referenceToUnitGroupDataSet>
<epd:amount epd:module="A1-A3"></epd:amount>
<epd:amount epd:module="A4"></epd:amount>
<epd:amount epd:module="A5"></epd:amount>
<epd:amount epd:module="B2"></epd:amount>
<epd:amount epd:module="C1"></epd:amount>
<epd:amount epd:module="C2"></epd:amount>
<epd:amount epd:module="C3"></epd:amount>
<epd:amount epd:module="C4"></epd:amount>
<epd:amount epd:module="D" epd:scenario="S1"></epd:amount>
<epd:amount epd:module="D" epd:scenario="S2"></epd:amount>
</common:other>
</exchange>
<exchange dataSetInternalID="9">
<referenceToFlowDataSet uri="../flows/89def144-d39a-4287-b86f-efde453ddcb2.xml" type="flow data set" refObjectId="89def144-d39a-4287-b86f-efde453ddcb2">
<common:shortDescription xml:lang="en">Use of non renewable secondary fuels (NRSF)</common:shortDescription>
</referenceToFlowDataSet>
<functionType>General reminder flow</functionType>
<exchangeDirection>Input</exchangeDirection>
<referencesToDataSource />
<common:other>
<epd:referenceToUnitGroupDataSet uri="../unitgroups/93a60a57-a3c8-11da-a746-0800200c9a66.xml" type="unit group data set" refObjectId="93a60a57-a3c8-11da-a746-0800200c9a66">
<common:shortDescription xml:lang="en">MJ</common:shortDescription>
</epd:referenceToUnitGroupDataSet>
<epd:amount epd:module="A1-A3"></epd:amount>
<epd:amount epd:module="A4"></epd:amount>
<epd:amount epd:module="A5"></epd:amount>
<epd:amount epd:module="B2"></epd:amount>
<epd:amount epd:module="C1"></epd:amount>
<epd:amount epd:module="C2"></epd:amount>
<epd:amount epd:module="C3"></epd:amount>
<epd:amount epd:module="C4"></epd:amount>
<epd:amount epd:module="D" epd:scenario="S1"></epd:amount>
<epd:amount epd:module="D" epd:scenario="S2"></epd:amount>
</common:other>
</exchange>
<exchange dataSetInternalID="10">
<referenceToFlowDataSet uri="../flows/3cf952c8-f3a4-461d-8c96-96456ca62246.xml" type="flow data set" refObjectId="3cf952c8-f3a4-461d-8c96-96456ca62246">
<common:shortDescription xml:lang="en">Use of net fresh water (FW)</common:shortDescription>
</referenceToFlowDataSet>
<functionType>General reminder flow</functionType>
<exchangeDirection>Input</exchangeDirection>
<referencesToDataSource />
<common:other>
<epd:referenceToUnitGroupDataSet uri="../unitgroups/cd950537-0a98-4044-9ba7-9f9a68d0a504.xml" type="unit group data set" refObjectId="cd950537-0a98-4044-9ba7-9f9a68d0a504">
<common:shortDescription xml:lang="en">m^3</common:shortDescription>
</epd:referenceToUnitGroupDataSet>
<epd:amount epd:module="A1-A3">0.0130426</epd:amount>
<epd:amount epd:module="A4">0.000307172</epd:amount>
<epd:amount epd:module="A5">0.00358172</epd:amount>
<epd:amount epd:module="B2">0.00247</epd:amount>
<epd:amount epd:module="C1">0.000116</epd:amount>
<epd:amount epd:module="C2">2.57E-05</epd:amount>
<epd:amount epd:module="C3">0.0082</epd:amount>
<epd:amount epd:module="C4">-5.43E-06</epd:amount>
<epd:amount epd:module="D" epd:scenario="S1">-0.004556</epd:amount>
<epd:amount epd:module="D" epd:scenario="S2">-0.000891</epd:amount>
</common:other>
</exchange>
<exchange dataSetInternalID="11">
<referenceToFlowDataSet uri="../flows/430f9e0f-59b2-46a0-8e0d-55e0e84948fc.xml" type="flow data set" refObjectId="430f9e0f-59b2-46a0-8e0d-55e0e84948fc">
<common:shortDescription xml:lang="en">Hazardous waste disposed (HWD)</common:shortDescription>
</referenceToFlowDataSet>
<functionType>General reminder flow</functionType>
<exchangeDirection>Output</exchangeDirection>
<referencesToDataSource />
<common:other>
<epd:referenceToUnitGroupDataSet uri="../unitgroups/ad38d542-3fe9-439d-9b95-2f5f7752acaf.xml" type="unit group data set" refObjectId="ad38d542-3fe9-439d-9b95-2f5f7752acaf">
<common:shortDescription xml:lang="en">kg</common:shortDescription>
</epd:referenceToUnitGroupDataSet>
<epd:amount epd:module="A1-A3">1.39632E-07</epd:amount>
<epd:amount epd:module="A4">1.74742E-07</epd:amount>
<epd:amount epd:module="A5">3.90991E-08</epd:amount>
<epd:amount epd:module="B2">2.43E-09</epd:amount>
<epd:amount epd:module="C1">1.07E-10</epd:amount>
<epd:amount epd:module="C2">1.46E-08</epd:amount>
<epd:amount epd:module="C3">5.64E-10</epd:amount>
<epd:amount epd:module="C4">9.03E-09</epd:amount>
<epd:amount epd:module="D" epd:scenario="S1">-7.008E-09</epd:amount>
<epd:amount epd:module="D" epd:scenario="S2">-1.37E-09</epd:amount>
</common:other>
</exchange>
<exchange dataSetInternalID="12">
<referenceToFlowDataSet uri="../flows/b29ef66b-e286-4afa-949f-62f1a7b4d7fa.xml" type="flow data set" refObjectId="b29ef66b-e286-4afa-949f-62f1a7b4d7fa">
<common:shortDescription xml:lang="en">Non hazardous waste disposed (NHWD)</common:shortDescription>
</referenceToFlowDataSet>
<functionType>General reminder flow</functionType>
<exchangeDirection>Output</exchangeDirection>
<referencesToDataSource />
<common:other>
<epd:referenceToUnitGroupDataSet uri="../unitgroups/ad38d542-3fe9-439d-9b95-2f5f7752acaf.xml" type="unit group data set" refObjectId="ad38d542-3fe9-439d-9b95-2f5f7752acaf">
<common:shortDescription xml:lang="en">kg</common:shortDescription>
</epd:referenceToUnitGroupDataSet>
<epd:amount epd:module="A1-A3">0.0254935</epd:amount>
<epd:amount epd:module="A4">0.000253163</epd:amount>
<epd:amount epd:module="A5">0.00983763</epd:amount>
<epd:amount epd:module="B2">0.00838</epd:amount>
<epd:amount epd:module="C1">0.00016</epd:amount>
<epd:amount epd:module="C2">2.11E-05</epd:amount>
<epd:amount epd:module="C3">0.00764</epd:amount>
<epd:amount epd:module="C4">1.99</epd:amount>
<epd:amount epd:module="D" epd:scenario="S1">-0.007406</epd:amount>
<epd:amount epd:module="D" epd:scenario="S2">-0.00145</epd:amount>
</common:other>
</exchange>
<exchange dataSetInternalID="13">
<referenceToFlowDataSet uri="../flows/3449546e-52ad-4b39-b809-9fb77cea8ff6.xml" type="flow data set" refObjectId="3449546e-52ad-4b39-b809-9fb77cea8ff6">
<common:shortDescription xml:lang="en">Radioactive waste disposed (RWD)</common:shortDescription>
</referenceToFlowDataSet>
<functionType>General reminder flow</functionType>
<exchangeDirection>Output</exchangeDirection>
<referencesToDataSource />
<common:other>
<epd:referenceToUnitGroupDataSet uri="../unitgroups/ad38d542-3fe9-439d-9b95-2f5f7752acaf.xml" type="unit group data set" refObjectId="ad38d542-3fe9-439d-9b95-2f5f7752acaf">
<common:shortDescription xml:lang="en">kg</common:shortDescription>
</epd:referenceToUnitGroupDataSet>
<epd:amount epd:module="A1-A3">0.000450877</epd:amount>
<epd:amount epd:module="A4">4.13602E-06</epd:amount>
<epd:amount epd:module="A5">0.000130702</epd:amount>
<epd:amount epd:module="B2">0.000702</epd:amount>
<epd:amount epd:module="C1">3.77E-05</epd:amount>
<epd:amount epd:module="C2">3.46E-07</epd:amount>
<epd:amount epd:module="C3">5.29E-05</epd:amount>
<epd:amount epd:module="C4">3E-05</epd:amount>
<epd:amount epd:module="D" epd:scenario="S1">-0.001469</epd:amount>
<epd:amount epd:module="D" epd:scenario="S2">-0.000287</epd:amount>
</common:other>
</exchange>
<exchange dataSetInternalID="14">
<referenceToFlowDataSet uri="../flows/a2b32f97-3fc7-4af2-b209-525bc6426f33.xml" type="flow data set" refObjectId="a2b32f97-3fc7-4af2-b209-525bc6426f33">
<common:shortDescription xml:lang="en">Components for re-use (CRU)</common:shortDescription>
</referenceToFlowDataSet>
<functionType>General reminder flow</functionType>
<exchangeDirection>Output</exchangeDirection>
<referencesToDataSource />
<common:other>
<epd:referenceToUnitGroupDataSet uri="../unitgroups/ad38d542-3fe9-439d-9b95-2f5f7752acaf.xml" type="unit group data set" refObjectId="ad38d542-3fe9-439d-9b95-2f5f7752acaf">
<common:shortDescription xml:lang="en">kg</common:shortDescription>
</epd:referenceToUnitGroupDataSet>
<epd:amount epd:module="A1-A3"></epd:amount>
<epd:amount epd:module="A4"></epd:amount>
<epd:amount epd:module="A5"></epd:amount>
<epd:amount epd:module="B2"></epd:amount>
<epd:amount epd:module="C1"></epd:amount>
<epd:amount epd:module="C2"></epd:amount>
<epd:amount epd:module="C3"></epd:amount>
<epd:amount epd:module="C4"></epd:amount>
<epd:amount epd:module="D" epd:scenario="S1"></epd:amount>
<epd:amount epd:module="D" epd:scenario="S2"></epd:amount>
</common:other>
</exchange>
<exchange dataSetInternalID="15">
<referenceToFlowDataSet uri="../flows/d7fe48a5-4103-49c8-9aae-b0b5dfdbd6ae.xml" type="flow data set" refObjectId="d7fe48a5-4103-49c8-9aae-b0b5dfdbd6ae">
<common:shortDescription xml:lang="en">Materials for recycling (MFR)</common:shortDescription>
</referenceToFlowDataSet>
<functionType>General reminder flow</functionType>
<exchangeDirection>Output</exchangeDirection>
<referencesToDataSource />
<common:other>
<epd:referenceToUnitGroupDataSet uri="../unitgroups/ad38d542-3fe9-439d-9b95-2f5f7752acaf.xml" type="unit group data set" refObjectId="ad38d542-3fe9-439d-9b95-2f5f7752acaf">
<common:shortDescription xml:lang="en">kg</common:shortDescription>
</epd:referenceToUnitGroupDataSet>
<epd:amount epd:module="A1-A3"></epd:amount>
<epd:amount epd:module="A4"></epd:amount>
<epd:amount epd:module="A5"></epd:amount>
<epd:amount epd:module="B2"></epd:amount>
<epd:amount epd:module="C1"></epd:amount>
<epd:amount epd:module="C2"></epd:amount>
<epd:amount epd:module="C3"></epd:amount>
<epd:amount epd:module="C4"></epd:amount>
<epd:amount epd:module="D" epd:scenario="S1"></epd:amount>
<epd:amount epd:module="D" epd:scenario="S2"></epd:amount>
</common:other>
</exchange>
<exchange dataSetInternalID="16">
<referenceToFlowDataSet uri="../flows/59a9181c-3aaf-46ee-8b13-2b3723b6e447.xml" type="flow data set" refObjectId="59a9181c-3aaf-46ee-8b13-2b3723b6e447">
<common:shortDescription xml:lang="en">Materials for energy recovery (MER)</common:shortDescription>
</referenceToFlowDataSet>
<functionType>General reminder flow</functionType>
<exchangeDirection>Output</exchangeDirection>
<referencesToDataSource />
<common:other>
<epd:referenceToUnitGroupDataSet uri="../unitgroups/ad38d542-3fe9-439d-9b95-2f5f7752acaf.xml" type="unit group data set" refObjectId="ad38d542-3fe9-439d-9b95-2f5f7752acaf">
<common:shortDescription xml:lang="en">kg</common:shortDescription>
</epd:referenceToUnitGroupDataSet>
<epd:amount epd:module="A1-A3"></epd:amount>
<epd:amount epd:module="A4"></epd:amount>
<epd:amount epd:module="A5"></epd:amount>
<epd:amount epd:module="B2"></epd:amount>
<epd:amount epd:module="C1"></epd:amount>
<epd:amount epd:module="C2"></epd:amount>
<epd:amount epd:module="C3"></epd:amount>
<epd:amount epd:module="C4"></epd:amount>
<epd:amount epd:module="D" epd:scenario="S1">2</epd:amount>
<epd:amount epd:module="D" epd:scenario="S2"></epd:amount>
</common:other>
</exchange>
<exchange dataSetInternalID="17">
<referenceToFlowDataSet uri="../flows/4da0c987-2b76-40d6-9e9e-82a017aaaf29.xml" type="flow data set" refObjectId="4da0c987-2b76-40d6-9e9e-82a017aaaf29">
<common:shortDescription xml:lang="en">Exported electrical energy (EEE)</common:shortDescription>
</referenceToFlowDataSet>
<functionType>General reminder flow</functionType>
<exchangeDirection>Output</exchangeDirection>
<referencesToDataSource />
<common:other>
<epd:referenceToUnitGroupDataSet uri="../unitgroups/93a60a57-a3c8-11da-a746-0800200c9a66.xml" type="unit group data set" refObjectId="93a60a57-a3c8-11da-a746-0800200c9a66">
<common:shortDescription xml:lang="en">MJ</common:shortDescription>
</epd:referenceToUnitGroupDataSet>
<epd:amount epd:module="A1-A3"></epd:amount>
<epd:amount epd:module="A4"></epd:amount>
<epd:amount epd:module="A5">0.184088</epd:amount>
<epd:amount epd:module="B2"></epd:amount>
<epd:amount epd:module="C1"></epd:amount>
<epd:amount epd:module="C2"></epd:amount>
<epd:amount epd:module="C3">4.09</epd:amount>
<epd:amount epd:module="C4"></epd:amount>
<epd:amount epd:module="D" epd:scenario="S1"></epd:amount>
<epd:amount epd:module="D" epd:scenario="S2"></epd:amount>
</common:other>
</exchange>
<exchange dataSetInternalID="18">
<referenceToFlowDataSet uri="../flows/98daf38a-7a79-46d3-9a37-2b7bd0955810.xml" type="flow data set" refObjectId="98daf38a-7a79-46d3-9a37-2b7bd0955810">
<common:shortDescription xml:lang="en">Exported thermal energy (EET)</common:shortDescription>
</referenceToFlowDataSet>
<functionType>General reminder flow</functionType>
<exchangeDirection>Output</exchangeDirection>
<referencesToDataSource />
<common:other>
<epd:referenceToUnitGroupDataSet uri="../unitgroups/93a60a57-a3c8-11da-a746-0800200c9a66.xml" type="unit group data set" refObjectId="93a60a57-a3c8-11da-a746-0800200c9a66">
<common:shortDescription xml:lang="en">MJ</common:shortDescription>
</epd:referenceToUnitGroupDataSet>
<epd:amount epd:module="A1-A3"></epd:amount>
<epd:amount epd:module="A4"></epd:amount>
<epd:amount epd:module="A5">0.327043</epd:amount>
<epd:amount epd:module="B2"></epd:amount>
<epd:amount epd:module="C1"></epd:amount>
<epd:amount epd:module="C2"></epd:amount>
<epd:amount epd:module="C3">7.27</epd:amount>
<epd:amount epd:module="C4"></epd:amount>
<epd:amount epd:module="D" epd:scenario="S1"></epd:amount>
<epd:amount epd:module="D" epd:scenario="S2"></epd:amount>
</common:other>
</exchange>
</exchanges>
<LCIAResults>
<LCIAResult>
<referenceToLCIAMethodDataSet uri="../flows/77e416eb-a363-4258-a04e-171d843a6460.xml" type="LCIA method data set" refObjectId="77e416eb-a363-4258-a04e-171d843a6460">
<common:shortDescription xml:lang="en">Global warming potential (GWP)</common:shortDescription>
</referenceToLCIAMethodDataSet>
<common:other>
<epd:referenceToUnitGroupDataSet uri="../unitgroups/1ebf3012-d0db-4de2-aefd-ef30cedb0be1.xml" type="unit group data set" refObjectId="1ebf3012-d0db-4de2-aefd-ef30cedb0be1">
<common:shortDescription xml:lang="en">kg CO_(2)-Äq.</common:shortDescription>
</epd:referenceToUnitGroupDataSet>
<epd:amount epd:module="A1-A3">-2.74067</epd:amount>
<epd:amount epd:module="A4">0.221947</epd:amount>
<epd:amount epd:module="A5">0.817816</epd:amount>
<epd:amount epd:module="B2">0.284</epd:amount>
<epd:amount epd:module="C1">0.0124</epd:amount>
<epd:amount epd:module="C2">0.0185</epd:amount>
<epd:amount epd:module="C3">3.59</epd:amount>
<epd:amount epd:module="C4">0.14</epd:amount>
<epd:amount epd:module="D" epd:scenario="S1">-0.9809</epd:amount>
<epd:amount epd:module="D" epd:scenario="S2">-0.193</epd:amount>
</common:other>
</LCIAResult>
<LCIAResult>
<referenceToLCIAMethodDataSet uri="../flows/06dcd26f-025f-401a-a7c1-5e457eb54637.xml" type="LCIA method data set" refObjectId="06dcd26f-025f-401a-a7c1-5e457eb54637">
<common:shortDescription xml:lang="en">Depletion potential of the stratospheric ozone layer (ODP)</common:shortDescription>
</referenceToLCIAMethodDataSet>
<common:other>
<epd:referenceToUnitGroupDataSet uri="../unitgroups/88054749-b0a6-47ea-a82b-dc5b29326512.xml" type="unit group data set" refObjectId="88054749-b0a6-47ea-a82b-dc5b29326512">
<common:shortDescription xml:lang="en">kg CFC11-Äq.</common:shortDescription>
</epd:referenceToUnitGroupDataSet>
<epd:amount epd:module="A1-A3">4.56639E-12</epd:amount>
<epd:amount epd:module="A4">6.04627E-15</epd:amount>
<epd:amount epd:module="A5">1.07119E-12</epd:amount>
<epd:amount epd:module="B2">1.03E-12</epd:amount>
<epd:amount epd:module="C1">5.53E-14</epd:amount>
<epd:amount epd:module="C2">5.05E-16</epd:amount>
<epd:amount epd:module="C3">7.57E-14</epd:amount>
<epd:amount epd:module="C4">3.79E-14</epd:amount>
<epd:amount epd:module="D" epd:scenario="S1">-2.155E-12</epd:amount>
<epd:amount epd:module="D" epd:scenario="S2">-4.21E-13</epd:amount>
</common:other>
</LCIAResult>
<LCIAResult>
<referenceToLCIAMethodDataSet uri="../flows/b4274add-93b7-4905-a5e4-2e878c4e4216.xml" type="LCIA method data set" refObjectId="b4274add-93b7-4905-a5e4-2e878c4e4216">
<common:shortDescription xml:lang="en">Acidification potential of land and water (AP)</common:shortDescription>
</referenceToLCIAMethodDataSet>
<common:other>
<epd:referenceToUnitGroupDataSet uri="../unitgroups/bc50c624-a9bc-45b1-a9b0-e6b10d00476f.xml" type="unit group data set" refObjectId="bc50c624-a9bc-45b1-a9b0-e6b10d00476f">
<common:shortDescription xml:lang="en">kg SO_(2)-Äq.</common:shortDescription>
</epd:referenceToUnitGroupDataSet>
<epd:amount epd:module="A1-A3">0.00483763</epd:amount>
<epd:amount epd:module="A4">0.000483157</epd:amount>
<epd:amount epd:module="A5">0.000921038</epd:amount>
<epd:amount epd:module="B2">0.000728</epd:amount>
<epd:amount epd:module="C1">3.53E-05</epd:amount>
<epd:amount epd:module="C2">4.04E-05</epd:amount>
<epd:amount epd:module="C3">0.00118</epd:amount>
<epd:amount epd:module="C4">0.000384</epd:amount>
<epd:amount epd:module="D" epd:scenario="S1">-0.00166</epd:amount>
<epd:amount epd:module="D" epd:scenario="S2">-0.000325</epd:amount>
</common:other>
</LCIAResult>
<LCIAResult>
<referenceToLCIAMethodDataSet uri="../flows/f58827d0-b407-4ec6-be75-8b69efb98a0f.xml" type="LCIA method data set" refObjectId="f58827d0-b407-4ec6-be75-8b69efb98a0f">
<common:shortDescription xml:lang="en">Eutrophication potential (EP)</common:shortDescription>
</referenceToLCIAMethodDataSet>
<common:other>
<epd:referenceToUnitGroupDataSet uri="../unitgroups/67b5401d-873c-485f-bcf3-6ae83b918822.xml" type="unit group data set" refObjectId="67b5401d-873c-485f-bcf3-6ae83b918822">
<common:shortDescription xml:lang="en">kg PO_(4)^(3)-Äq.</common:shortDescription>
</epd:referenceToUnitGroupDataSet>
<epd:amount epd:module="A1-A3">0.00127882</epd:amount>
<epd:amount epd:module="A4">0.00012217</epd:amount>
<epd:amount epd:module="A5">0.000220909</epd:amount>
<epd:amount epd:module="B2">9.38E-05</epd:amount>
<epd:amount epd:module="C1">3.31E-06</epd:amount>
<epd:amount epd:module="C2">1.02E-05</epd:amount>
<epd:amount epd:module="C3">0.000294</epd:amount>
<epd:amount epd:module="C4">0.000392</epd:amount>
<epd:amount epd:module="D" epd:scenario="S1">-0.0001791</epd:amount>
<epd:amount epd:module="D" epd:scenario="S2">-3.51E-05</epd:amount>
</common:other>
</LCIAResult>
<LCIAResult>
<referenceToLCIAMethodDataSet uri="../flows/1e84a202-dae6-42aa-9e9d-71ea48b8be00.xml" type="LCIA method data set" refObjectId="1e84a202-dae6-42aa-9e9d-71ea48b8be00">
<common:shortDescription xml:lang="en">Formation potential of tropospheric ozone photochemical oxidants (POCP)</common:shortDescription>
</referenceToLCIAMethodDataSet>
<common:other>
<epd:referenceToUnitGroupDataSet uri="../unitgroups/01c26c17-9a76-406e-8295-f17b55fd909e.xml" type="unit group data set" refObjectId="01c26c17-9a76-406e-8295-f17b55fd909e">
<common:shortDescription xml:lang="en">kg Ethen-Äq.</common:shortDescription>
</epd:referenceToUnitGroupDataSet>
<epd:amount epd:module="A1-A3">0.000670238</epd:amount>
<epd:amount epd:module="A4">-0.000158042</epd:amount>
<epd:amount epd:module="A5">0.000116285</epd:amount>
<epd:amount epd:module="B2">5.93E-05</epd:amount>
<epd:amount epd:module="C1">2.21E-06</epd:amount>
<epd:amount epd:module="C2">-1.32E-05</epd:amount>
<epd:amount epd:module="C3">7.52E-05</epd:amount>
<epd:amount epd:module="C4">4.19E-05</epd:amount>
<epd:amount epd:module="D" epd:scenario="S1">-0.0001296</epd:amount>
<epd:amount epd:module="D" epd:scenario="S2">-2.54E-05</epd:amount>
</common:other>
</LCIAResult>
<LCIAResult>
<referenceToLCIAMethodDataSet uri="../flows/f7c73bb9-ab1a-4249-9c6d-379a0de6f67e.xml" type="LCIA method data set" refObjectId="f7c73bb9-ab1a-4249-9c6d-379a0de6f67e">
<common:shortDescription xml:lang="en">Abiotic depletion potential for non fossil resources (ADPE)</common:shortDescription>
</referenceToLCIAMethodDataSet>
<common:other>
<epd:referenceToUnitGroupDataSet uri="../unitgroups/54ccd2d9-a32a-4fc2-923d-f2c8c93e89d4.xml" type="unit group data set" refObjectId="54ccd2d9-a32a-4fc2-923d-f2c8c93e89d4">
<common:shortDescription xml:lang="en">kg Sb-Äq.</common:shortDescription>
</epd:referenceToUnitGroupDataSet>
<epd:amount epd:module="A1-A3">3.01962E-06</epd:amount>
<epd:amount epd:module="A4">1.81691E-08</epd:amount>
<epd:amount epd:module="A5">2.69933E-07</epd:amount>
<epd:amount epd:module="B2">1.64E-07</epd:amount>
<epd:amount epd:module="C1">6.61E-09</epd:amount>
<epd:amount epd:module="C2">1.52E-09</epd:amount>
<epd:amount epd:module="C3">3.74E-08</epd:amount>
<epd:amount epd:module="C4">3.08E-08</epd:amount>
<epd:amount epd:module="D" epd:scenario="S1">-2.798E-07</epd:amount>
<epd:amount epd:module="D" epd:scenario="S2">-5.48E-08</epd:amount>
</common:other>
</LCIAResult>
<LCIAResult>
<referenceToLCIAMethodDataSet uri="../flows/804ebcdf-309d-4098-8ed8-fdaf2f389981.xml" type="LCIA method data set" refObjectId="804ebcdf-309d-4098-8ed8-fdaf2f389981">
<common:shortDescription xml:lang="en">Abiotic depletion potential for fossil resources (ADPF)</common:shortDescription>
</referenceToLCIAMethodDataSet>
<common:other>
<epd:referenceToUnitGroupDataSet uri="../unitgroups/93a60a57-a3c8-11da-a746-0800200c9a66.xml" type="unit group data set" refObjectId="93a60a57-a3c8-11da-a746-0800200c9a66">
<common:shortDescription xml:lang="en">MJ</common:shortDescription>
</epd:referenceToUnitGroupDataSet>
<epd:amount epd:module="A1-A3">35.6841</epd:amount>
<epd:amount epd:module="A4">3.01151</epd:amount>
<epd:amount epd:module="A5">11.0541</epd:amount>
<epd:amount epd:module="B2">3.36</epd:amount>
<epd:amount epd:module="C1">0.133</epd:amount>
<epd:amount epd:module="C2">0.252</epd:amount>
<epd:amount epd:module="C3">0.865</epd:amount>
<epd:amount epd:module="C4">2.04</epd:amount>
<epd:amount epd:module="D" epd:scenario="S1">-13.47</epd:amount>
<epd:amount epd:module="D" epd:scenario="S2">-2.65</epd:amount>
</common:other>
</LCIAResult>
</LCIAResults>
</processDataSet>