<?xml version="1.0" encoding="utf-8"?>
<?xml-stylesheet version="1.0" href="../../stylesheets/epd2html.xsl" type="text/xsl"?>
<processDataSet xmlns="http://lca.jrc.it/ILCD/Process" xmlns:common="http://lca.jrc.it/ILCD/Common" xmlns:epd="http://www.iai.kit.edu/EPD/2013" xmlns:epd2="http://www.indata.network/EPD/2019" xmlns:xsi="http://www.w3.org/2001/XMLSchema-instance" xsi:schemaLocation="http://lca.jrc.it/ILCD/Process ../../schemas/EPD_DataSet.xsd" locations="../ILCDLocations.xml" epd2:epd-version="1.2" version="1.1">
  <processInformation>
    <dataSetInformation>
      <common:UUID>cc54d8cb-f26c-41ea-a152-8b28f7fb5b1d</common:UUID>
      <name>
        <baseName xml:lang="en">Melamin resin foam</baseName>
        <baseName xml:lang="de">Melaminharz-Schaum</baseName>
        <functionalUnitFlowProperties xml:lang="en">10 kg/m3</functionalUnitFlowProperties>
      </name>
      <classificationInformation>
        <common:classification name="oekobau.dat">
          <common:class level="0" classId="2">Dämmstoffe</common:class>
          <common:class level="1" classId="2.17">Melaminharz</common:class>
          <common:class level="2" classId="2.17.01">Schaum</common:class>
        </common:classification>
      </classificationInformation>
      <common:generalComment xml:lang="en">This data set has been modeled according to the European Standard EN 15804+A2 for Sustainable Building. Results are depicted in modules that allow the structured expression of results over the entire life cycle.</common:generalComment>
      <common:generalComment xml:lang="de">Dieser Datensatz wurde nach dem European Standard EN 15804+A2 für Nachhaltiges Bauen modelliert. Ergebnisse werden in Modulen abgebildet, die den strukturierten Ausdruck von Ergebnissen über den gesamten Lebenszyklus zulassen.</common:generalComment>
      <common:other>
        <epd:safetyMargins>
          <epd:margins>20</epd:margins>
          <epd:description xml:lang="en">Product system depicted except for a few missing processes / flows. Technological, temporal and geographic representativeness partly given.</epd:description>
          <epd:description xml:lang="de">Produktsystem bis auf wenige Prozesse/Flüsse abgebildet. Technologische, zeitliche und geographische Repräsentativität teilweise gegeben.</epd:description>
        </epd:safetyMargins>
      </common:other>
    </dataSetInformation>
    <quantitativeReference type="Reference flow(s)">
      <referenceToReferenceFlow>108835</referenceToReferenceFlow>
    </quantitativeReference>
    <time>
      <common:referenceYear>2021</common:referenceYear>
      <common:dataSetValidUntil>2022</common:dataSetValidUntil>
      <common:timeRepresentativenessDescription xml:lang="en">Annual average</common:timeRepresentativenessDescription>
      <common:timeRepresentativenessDescription xml:lang="de">Jährlicher Durchschnitt</common:timeRepresentativenessDescription>
    </time>
    <geography>
      <locationOfOperationSupplyOrProduction location="DE">
        <descriptionOfRestrictions xml:lang="en">The data set represents the country specific situation in Germany, focusing on the main technologies, the region specific characteristics and / or import statistics.</descriptionOfRestrictions>
        <descriptionOfRestrictions xml:lang="de">Der Datensatz bildet die länderspezifische Situation in Deutschland ab. Dabei werden Haupttechnologien, spezifische regionale Charakteristiken und ggf. Importstatistiken berücksichtigt.</descriptionOfRestrictions>
      </locationOfOperationSupplyOrProduction>
    </geography>
    <technology>
      <technologyDescriptionAndIncludedProcesses xml:lang="en">The life cycle analysis of melamine resin foam includes the life cycle phases cradle to gate, i.e. manufacturing of raw and auxiliary materials as well as the melamine resin foam production incl. operation of the production plant and waste water treatment. Melamine is produced from urea in a one-step, low-pressure (0,7 MPa), catalytic vapor-phase process. Urea is converted into melamine using silica-alumina as a catalyst fluidized by preheated ammonia at a reaction temperature of  400 °C. Melamine leaves the reactor in the gaseous form together with ammonia and carbon dioxide. The mixture is quenched with recycled mother liquor (from the following crystallization step), separating ammonia and carbon dioxide from the product. Melamine precipitates from the gas stream and is collected at the bottom of a scrubber. It is purified by crystallization and an activated carbon treatment. Surplus ammonia is recovered and recycled to the reactor. The system boundary is cutted melamine resin foam block at the factory gate (ready for shipment) covered with a cover mat. Transports from the factory to the construction site are not taken into account and have to be incorporated in a system approach.

In module C1, a manual dismantling (no loads) is assumed, collecting losses are neglected.
The transport in module C2 to the recycling plant takes place with a truck (50km).
Module C3 takes into account the grinding and thermal treatment (combustion) of the material. When calculating combustion emissions and credits, the specific calorific value of each material and the material composition are taken into account.
In module D credits for the substitution of electricity (German electricity mix) and thermal energy (from natural gas) are given.</technologyDescriptionAndIncludedProcesses>
      <technologyDescriptionAndIncludedProcesses xml:lang="de">Dieser Datensatz von Melaminharzschaumstoff beinhaltet die Lebenszyklus-Phasen Cradle to gate: von der Rohstoff- und Hilfsstoffherstellung sowie die Melaminharzschaumstoff-Produktion inklusive Betreiben der Produktionsanlage und Abwasseraufbereitung. Melamin wird aus Harnstoff schrittweise unter niedrigem Druck (0,7 MPa) in einem katalytischem Dampfphasenverfahren produziert. Harnstoff wird in Melamin umgewandelt, indem man Aluminiumoxid als Fließkatalysatoren durch vorgeheiztes Ammonium bei einer Reaktionstemperatur von 400 °C Ammonium- und Kohlendioxid verwendet. Melamin verlässt den Reaktor im gasförmigen Zustand zusammen mit Ammoniak und Kohlendioxid. Die Mischung wird  mit recycelter Mutterlauge abgekühlt (ab nachfolgender Kristallisation) und separiert Ammonium- und Kohlendioxid vom Produkt. Melamin ..... aus dem Gasstrom und wird am Boden eines Dampfsiebs gesammelt. Es wird durch Kristallisation und eine Filterung über Aktivkohle gereinigt. Überschüssiges Ammonium wird zurückgewonnen und im Reaktor wiederverwertet. Die Systemgrenze sind geschnittene Melaminharzschaumstoff-Blöcke, die am Fabriktor (bereit zum Transport), mit einer Abdeckfolie abgedeckt werden. Transporte von der Fabrik zur Baustelle werden nicht berücksichtigt und müssen in ein Konzept eingearbeitet werden. 

In Modul C1 wird ein manueller Rückbau (lastenfrei) angenommen. Sammelverluste werden vernachlässigt.
Der Transport in Modul C2 zur Verwertungsanlage erfolgt mit einem LKW (50km). 
In Modul C3 wird die Zerkleinerung und thermische Behandlung (Verbrennung) des Materials berücksichtigt. Bei der Berechnung der Verbrennungsemissionen und Gutschriften wird der spezifische Heizwert des jeweiligen Materials sowie die Materialzusammensetzung berücksichtigt.
In Modul D erfolgen Gutschriften für die Substitution von Strom (deutscher Strommix) und thermischer Energie (aus Erdgas).</technologyDescriptionAndIncludedProcesses>
      <technologicalApplicability xml:lang="en">This product can be used in construction.</technologicalApplicability>
      <technologicalApplicability xml:lang="de">Dieses Produkt kann im Baubereich verwendet werden.</technologicalApplicability>
      <referenceToTechnologyFlowDiagrammOrPicture refObjectId="7e36c650-015a-41b0-9dd7-c076a048aed9" version="21.01.000" type="source data set" uri="../sources/7e36c650-015a-41b0-9dd7-c076a048aed9.xml">
        <common:shortDescription xml:lang="en">intermediates_melamine.gif</common:shortDescription>
      </referenceToTechnologyFlowDiagrammOrPicture>
    </technology>
  </processInformation>
  <modellingAndValidation>
    <LCIMethodAndAllocation>
      <typeOfDataSet>EPD</typeOfDataSet>
      <common:other>
        <epd:subType>generic dataset</epd:subType>
      </common:other>
    </LCIMethodAndAllocation>
    <dataSourcesTreatmentAndRepresentativeness>
      <referenceToDataSource refObjectId="d2732231-5fbd-11db-b0de-0800200c9a66" version="21.01.000" type="source data set" uri="../sources/d2732231-5fbd-11db-b0de-0800200c9a66.xml">
        <common:shortDescription xml:lang="en">ULLMANN'S Encyclopedia of Industrial Chemistry</common:shortDescription>
      </referenceToDataSource>
      <referenceToDataSource refObjectId="e3bd9bbf-2c3c-42aa-8892-fd13f1065ca5" version="21.01.000" type="source data set" uri="../sources/e3bd9bbf-2c3c-42aa-8892-fd13f1065ca5.xml">
        <common:shortDescription xml:lang="en">Documentation of data quality management</common:shortDescription>
      </referenceToDataSource>
      <referenceToDataSource refObjectId="1cece811-7501-44d4-8067-9259bd5cb835" version="00.01.000" type="source data set" uri="../sources/1cece811-7501-44d4-8067-9259bd5cb835.xml">
        <common:shortDescription xml:lang="en">GaBi Database Edition 2021, CUP2021.01</common:shortDescription>
      </referenceToDataSource>
      <referenceToDataSource refObjectId="28d74cc0-db8b-4d7e-bc44-5f6d56ce0c4a" version="00.03.002" type="source data set" uri="../sources/28d74cc0-db8b-4d7e-bc44-5f6d56ce0c4a.xml">
        <common:shortDescription xml:lang="en">GaBi database (all versions)</common:shortDescription>
      </referenceToDataSource>
      <useAdviceForDataSet xml:lang="en">The data set represents a cradle to gate inventory. It can be used to characterise the supply chain situation of the respective commodity in a representative manner. Combination with individual unit processes using this commodity enables the generation of user-specific (product) LCAs.</useAdviceForDataSet>
      <useAdviceForDataSet xml:lang="de">Der Datensatz repräsentiert ein Cradle to Gate Inventar. Er kann verwendet werden, um die Lieferkette des jeweiligen Produktes in einer repräsentativen Weise zu charakterisieren. Die Kombination mit einzelnen Einheitenprozessen und diesem Produkt ermöglicht die Erstellung von anwenderspezifischen (Produkt-) LCAs.</useAdviceForDataSet>
    </dataSourcesTreatmentAndRepresentativeness>
    <validation>
      <review type="Dependent internal review">
        <common:referenceToNameOfReviewerAndInstitution refObjectId="d7fa0337-f279-430d-becf-7f3111a85010" version="21.01.000" type="contact data set" uri="../contacts/d7fa0337-f279-430d-becf-7f3111a85010.xml">
          <common:shortDescription xml:lang="en">Sphera Solutions GmbH</common:shortDescription>
        </common:referenceToNameOfReviewerAndInstitution>
      </review>
      <review type="Independent external review">
        <common:referenceToNameOfReviewerAndInstitution refObjectId="8f1306f0-7b83-4f36-a537-aa83f0498266" version="21.01.000" type="contact data set" uri="../contacts/8f1306f0-7b83-4f36-a537-aa83f0498266.xml">
          <common:shortDescription xml:lang="en">GaBi user forum</common:shortDescription>
        </common:referenceToNameOfReviewerAndInstitution>
      </review>
    </validation>
    <complianceDeclarations>
      <compliance>
        <common:referenceToComplianceSystem refObjectId="c0016b33-8cf7-415c-ac6e-deba0d21440d" version="00.01.000" type="source data set" uri="../sources/c0016b33-8cf7-415c-ac6e-deba0d21440d.xml">
          <common:shortDescription xml:lang="de">EN 15804+A2</common:shortDescription>
          <common:shortDescription xml:lang="en">EN 15804+A2</common:shortDescription>
        </common:referenceToComplianceSystem>
        <common:approvalOfOverallCompliance>Fully compliant</common:approvalOfOverallCompliance>
      </compliance>
    </complianceDeclarations>
  </modellingAndValidation>
  <administrativeInformation>
    <dataEntryBy>
      <common:timeStamp>2021-04-28T21:02:46+01:00</common:timeStamp>
      <common:referenceToDataSetFormat refObjectId="a97a0155-0234-4b87-b4ce-a45da52f2a40" version="01.00.000" type="source data set" uri="../sources/a97a0155-0234-4b87-b4ce-a45da52f2a40.xml">
        <common:shortDescription xml:lang="de">ILCD format 1.1</common:shortDescription>
        <common:shortDescription xml:lang="en">ILCD format 1.1</common:shortDescription>
      </common:referenceToDataSetFormat>
      <common:referenceToDataSetFormat refObjectId="a29449fd-aa2f-4de8-b5d7-4b06b43c6fde" version="00.01.000" type="source data set" uri="../sources/a29449fd-aa2f-4de8-b5d7-4b06b43c6fde.xml">
        <common:shortDescription xml:lang="de">EPD-Datenformaterweiterungen v1.2</common:shortDescription>
        <common:shortDescription xml:lang="en">EPD Data Format Extensions v1.2</common:shortDescription>
      </common:referenceToDataSetFormat>
      <common:referenceToPersonOrEntityEnteringTheData refObjectId="d7fa0337-f279-430d-becf-7f3111a85010" version="21.01.000" type="contact data set" uri="../contacts/d7fa0337-f279-430d-becf-7f3111a85010.xml">
        <common:shortDescription xml:lang="en">Sphera Solutions GmbH</common:shortDescription>
      </common:referenceToPersonOrEntityEnteringTheData>
    </dataEntryBy>
    <publicationAndOwnership>
      <common:dataSetVersion>20.21.060</common:dataSetVersion>
      <common:referenceToPrecedingDataSetVersion refObjectId="cc54d8cb-f26c-41ea-a152-8b28f7fb5b1d" type="process data set" uri="https://www.oekobaudat.de/OEKOBAU.DAT/datasetdetail/process.xhtml?uuid=cc54d8cb-f26c-41ea-a152-8b28f7fb5b1d&amp;stock=OBD_2020_II&amp;lang=de">
        <common:shortDescription xml:lang="en">Melamin resin foam</common:shortDescription>
      </common:referenceToPrecedingDataSetVersion>
      <common:referenceToOwnershipOfDataSet refObjectId="d7fa0337-f279-430d-becf-7f3111a85010" version="21.01.000" type="contact data set" uri="../contacts/d7fa0337-f279-430d-becf-7f3111a85010.xml">
        <common:shortDescription xml:lang="en">Sphera Solutions GmbH</common:shortDescription>
      </common:referenceToOwnershipOfDataSet>
      <common:copyright>true</common:copyright>
      <common:licenseType>Free of charge for all users and uses</common:licenseType>
      <common:accessRestrictions xml:lang="en">The license conditions as stated on https://www.oekobaudat.de/ apply.</common:accessRestrictions>
      <common:accessRestrictions xml:lang="de">Es gelten die Lizenzbedingungen wie sie auf https://www.oekobaudat.de/ genannt sind.</common:accessRestrictions>
      <common:other>
        <epd2:referenceToPublisher refObjectId="f11651e0-7877-11e3-981f-0800200c9a66" version="00.01.000" type="contact data set" uri="../contacts/f11651e0-7877-11e3-981f-0800200c9a66.xml">
          <common:shortDescription xml:lang="en">BBSR</common:shortDescription>
        </epd2:referenceToPublisher>
      </common:other>
    </publicationAndOwnership>
  </administrativeInformation>
  <exchanges>
    <exchange dataSetInternalID="108835">
      <referenceToFlowDataSet refObjectId="4a7ef8e0-2d94-4d2e-bebf-1b201bd519be" version="21.01.000" type="flow data set" uri="../flows/4a7ef8e0-2d94-4d2e-bebf-1b201bd519be.xml">
        <common:shortDescription xml:lang="en">Melamin resin foam</common:shortDescription>
        <common:shortDescription xml:lang="de">Melaminharz-Schaum</common:shortDescription>
      </referenceToFlowDataSet>
      <meanAmount>1</meanAmount>
    </exchange>
    <exchange dataSetInternalID="108836">
      <referenceToFlowDataSet refObjectId="20f32be5-0398-4288-9b6d-accddd195317" version="21.01.000" type="flow data set" uri="../flows/20f32be5-0398-4288-9b6d-accddd195317.xml">
        <common:shortDescription xml:lang="en">Use of renewable primary energy as energy carrier (PERE)</common:shortDescription>
        <common:shortDescription xml:lang="de">Erneuerbare Primärenergie als Energieträger (PERE)</common:shortDescription>
      </referenceToFlowDataSet>
      <functionType>General reminder flow</functionType>
      <exchangeDirection>Input</exchangeDirection>
      <common:other>
        <epd:amount epd:module="A1-A3">8.46283807423303</epd:amount>
        <epd:referenceToUnitGroupDataSet refObjectId="93a60a57-a3c8-11da-a746-0800200c9a66" version="03.00.000" type="unit group data set" uri="../unitgroups/93a60a57-a3c8-11da-a746-0800200c9a66.xml">
          <common:shortDescription xml:lang="en">MJ</common:shortDescription>
        </epd:referenceToUnitGroupDataSet>
        <epd:amount epd:module="C2">0.00218616422722423</epd:amount>
        <epd:amount epd:module="C3">0.202676599220102</epd:amount>
        <epd:amount epd:module="D">-2.7748500820144</epd:amount>
      </common:other>
    </exchange>
    <exchange dataSetInternalID="108837">
      <referenceToFlowDataSet refObjectId="fb3ec0de-548d-4508-aea5-00b73bf6f702" version="21.01.000" type="flow data set" uri="../flows/fb3ec0de-548d-4508-aea5-00b73bf6f702.xml">
        <common:shortDescription xml:lang="en">Use of renewable primary energy resources used as raw materials (PERM)</common:shortDescription>
        <common:shortDescription xml:lang="de">Erneuerbare Primärenergie zur stofflichen Nutzung (PERM)</common:shortDescription>
      </referenceToFlowDataSet>
      <functionType>General reminder flow</functionType>
      <exchangeDirection>Input</exchangeDirection>
      <common:other>
        <epd:amount epd:module="A1-A3">0</epd:amount>
        <epd:referenceToUnitGroupDataSet refObjectId="93a60a57-a3c8-11da-a746-0800200c9a66" version="03.00.000" type="unit group data set" uri="../unitgroups/93a60a57-a3c8-11da-a746-0800200c9a66.xml">
          <common:shortDescription xml:lang="en">MJ</common:shortDescription>
        </epd:referenceToUnitGroupDataSet>
        <epd:amount epd:module="C2">0</epd:amount>
        <epd:amount epd:module="C3">0</epd:amount>
        <epd:amount epd:module="D">0</epd:amount>
      </common:other>
    </exchange>
    <exchange dataSetInternalID="108838">
      <referenceToFlowDataSet refObjectId="53f97275-fa8a-4cdd-9024-65936002acd0" version="21.01.000" type="flow data set" uri="../flows/53f97275-fa8a-4cdd-9024-65936002acd0.xml">
        <common:shortDescription xml:lang="en">Total use of renewable primary energy (PERT)</common:shortDescription>
        <common:shortDescription xml:lang="de">Total erneuerbare Primärenergie (PERT)</common:shortDescription>
      </referenceToFlowDataSet>
      <functionType>General reminder flow</functionType>
      <exchangeDirection>Input</exchangeDirection>
      <common:other>
        <epd:amount epd:module="A1-A3">8.46283807423303</epd:amount>
        <epd:referenceToUnitGroupDataSet refObjectId="93a60a57-a3c8-11da-a746-0800200c9a66" version="03.00.000" type="unit group data set" uri="../unitgroups/93a60a57-a3c8-11da-a746-0800200c9a66.xml">
          <common:shortDescription xml:lang="en">MJ</common:shortDescription>
        </epd:referenceToUnitGroupDataSet>
        <epd:amount epd:module="C2">0.00218616422722423</epd:amount>
        <epd:amount epd:module="C3">0.202676599220102</epd:amount>
        <epd:amount epd:module="D">-2.7748500820144</epd:amount>
      </common:other>
    </exchange>
    <exchange dataSetInternalID="108839">
      <referenceToFlowDataSet refObjectId="ac857178-2b45-46ec-892a-a9a4332f0372" version="21.01.000" type="flow data set" uri="../flows/ac857178-2b45-46ec-892a-a9a4332f0372.xml">
        <common:shortDescription xml:lang="en">Use of non renewable primary energy as energy carrier (PENRE)</common:shortDescription>
        <common:shortDescription xml:lang="de">Nicht-erneuerbare Primärenergie als Energieträger (PENRE)</common:shortDescription>
      </referenceToFlowDataSet>
      <functionType>General reminder flow</functionType>
      <exchangeDirection>Input</exchangeDirection>
      <common:other>
        <epd:amount epd:module="A1-A3">109.14437888923</epd:amount>
        <epd:referenceToUnitGroupDataSet refObjectId="93a60a57-a3c8-11da-a746-0800200c9a66" version="03.00.000" type="unit group data set" uri="../unitgroups/93a60a57-a3c8-11da-a746-0800200c9a66.xml">
          <common:shortDescription xml:lang="en">MJ</common:shortDescription>
        </epd:referenceToUnitGroupDataSet>
        <epd:amount epd:module="C2">0.0376676831118714</epd:amount>
        <epd:amount epd:module="C3">21.090044653388</epd:amount>
        <epd:amount epd:module="D">-8.20700833907719</epd:amount>
      </common:other>
    </exchange>
    <exchange dataSetInternalID="108840">
      <referenceToFlowDataSet refObjectId="1421caa0-679d-4bf4-b282-0eb850ccae27" version="21.01.000" type="flow data set" uri="../flows/1421caa0-679d-4bf4-b282-0eb850ccae27.xml">
        <common:shortDescription xml:lang="en">Use of non renewable primary energy resources used as raw materials (PENRM)</common:shortDescription>
        <common:shortDescription xml:lang="de">Nicht-erneuerbare Primärenergie zur stofflichen Nutzung (PENRM)</common:shortDescription>
      </referenceToFlowDataSet>
      <functionType>General reminder flow</functionType>
      <exchangeDirection>Input</exchangeDirection>
      <common:other>
        <epd:amount epd:module="A1-A3">17</epd:amount>
        <epd:referenceToUnitGroupDataSet refObjectId="93a60a57-a3c8-11da-a746-0800200c9a66" version="03.00.000" type="unit group data set" uri="../unitgroups/93a60a57-a3c8-11da-a746-0800200c9a66.xml">
          <common:shortDescription xml:lang="en">MJ</common:shortDescription>
        </epd:referenceToUnitGroupDataSet>
        <epd:amount epd:module="C2">0</epd:amount>
        <epd:amount epd:module="C3">-17</epd:amount>
        <epd:amount epd:module="D">0</epd:amount>
      </common:other>
    </exchange>
    <exchange dataSetInternalID="108841">
      <referenceToFlowDataSet refObjectId="06159210-646b-4c8d-8583-da9b3b95a6c1" version="21.01.000" type="flow data set" uri="../flows/06159210-646b-4c8d-8583-da9b3b95a6c1.xml">
        <common:shortDescription xml:lang="en">Total use of non renewable primary energy resource (PENRT)</common:shortDescription>
        <common:shortDescription xml:lang="de">Total nicht-erneuerbare Primärenergie (PENRT)</common:shortDescription>
      </referenceToFlowDataSet>
      <functionType>General reminder flow</functionType>
      <exchangeDirection>Input</exchangeDirection>
      <common:other>
        <epd:amount epd:module="A1-A3">126.14437888923</epd:amount>
        <epd:referenceToUnitGroupDataSet refObjectId="93a60a57-a3c8-11da-a746-0800200c9a66" version="03.00.000" type="unit group data set" uri="../unitgroups/93a60a57-a3c8-11da-a746-0800200c9a66.xml">
          <common:shortDescription xml:lang="en">MJ</common:shortDescription>
        </epd:referenceToUnitGroupDataSet>
        <epd:amount epd:module="C2">0.0376676831118714</epd:amount>
        <epd:amount epd:module="C3">4.09004465338802</epd:amount>
        <epd:amount epd:module="D">-8.20700833907719</epd:amount>
      </common:other>
    </exchange>
    <exchange dataSetInternalID="108842">
      <referenceToFlowDataSet refObjectId="c6a1f35f-2d09-4f54-8dfb-97e502e1ce92" version="21.01.000" type="flow data set" uri="../flows/c6a1f35f-2d09-4f54-8dfb-97e502e1ce92.xml">
        <common:shortDescription xml:lang="en">Use of secondary material (SM)</common:shortDescription>
        <common:shortDescription xml:lang="de">Einsatz von Sekundärstoffen (SM)</common:shortDescription>
      </referenceToFlowDataSet>
      <functionType>General reminder flow</functionType>
      <exchangeDirection>Input</exchangeDirection>
      <common:other>
        <epd:amount epd:module="A1-A3">0</epd:amount>
        <epd:referenceToUnitGroupDataSet refObjectId="93a60a57-a4c8-11da-a746-0800200c9a66" version="03.00.000" type="unit group data set" uri="../unitgroups/93a60a57-a4c8-11da-a746-0800200c9a66.xml">
          <common:shortDescription xml:lang="en">kg</common:shortDescription>
        </epd:referenceToUnitGroupDataSet>
        <epd:amount epd:module="C2">0</epd:amount>
        <epd:amount epd:module="C3">0</epd:amount>
        <epd:amount epd:module="D">0</epd:amount>
      </common:other>
    </exchange>
    <exchange dataSetInternalID="108843">
      <referenceToFlowDataSet refObjectId="64333088-a55f-4aa2-9a31-c10b07816787" version="21.01.000" type="flow data set" uri="../flows/64333088-a55f-4aa2-9a31-c10b07816787.xml">
        <common:shortDescription xml:lang="en">Use of renewable secondary fuels (SF)</common:shortDescription>
        <common:shortDescription xml:lang="de">Erneuerbare Sekundärbrennstoffe (SF)</common:shortDescription>
      </referenceToFlowDataSet>
      <functionType>General reminder flow</functionType>
      <exchangeDirection>Input</exchangeDirection>
      <common:other>
        <epd:amount epd:module="A1-A3">0</epd:amount>
        <epd:referenceToUnitGroupDataSet refObjectId="93a60a57-a3c8-11da-a746-0800200c9a66" version="03.00.000" type="unit group data set" uri="../unitgroups/93a60a57-a3c8-11da-a746-0800200c9a66.xml">
          <common:shortDescription xml:lang="en">MJ</common:shortDescription>
        </epd:referenceToUnitGroupDataSet>
        <epd:amount epd:module="C2">0</epd:amount>
        <epd:amount epd:module="C3">0</epd:amount>
        <epd:amount epd:module="D">0</epd:amount>
      </common:other>
    </exchange>
    <exchange dataSetInternalID="108844">
      <referenceToFlowDataSet refObjectId="89def144-d39a-4287-b86f-efde453ddcb2" version="21.01.000" type="flow data set" uri="../flows/89def144-d39a-4287-b86f-efde453ddcb2.xml">
        <common:shortDescription xml:lang="en">Use of non renewable secondary fuels (NRSF)</common:shortDescription>
        <common:shortDescription xml:lang="de">Nicht erneuerbare Sekundärbrennstoffe (NRSF)</common:shortDescription>
      </referenceToFlowDataSet>
      <functionType>General reminder flow</functionType>
      <exchangeDirection>Input</exchangeDirection>
      <common:other>
        <epd:amount epd:module="A1-A3">0</epd:amount>
        <epd:referenceToUnitGroupDataSet refObjectId="93a60a57-a3c8-11da-a746-0800200c9a66" version="03.00.000" type="unit group data set" uri="../unitgroups/93a60a57-a3c8-11da-a746-0800200c9a66.xml">
          <common:shortDescription xml:lang="en">MJ</common:shortDescription>
        </epd:referenceToUnitGroupDataSet>
        <epd:amount epd:module="C2">0</epd:amount>
        <epd:amount epd:module="C3">0</epd:amount>
        <epd:amount epd:module="D">0</epd:amount>
      </common:other>
    </exchange>
    <exchange dataSetInternalID="108845">
      <referenceToFlowDataSet refObjectId="3cf952c8-f3a4-461d-8c96-96456ca62246" version="21.01.000" type="flow data set" uri="../flows/3cf952c8-f3a4-461d-8c96-96456ca62246.xml">
        <common:shortDescription xml:lang="en">Net use of fresh water (FW)</common:shortDescription>
        <common:shortDescription xml:lang="de">Nettoeinsatz von Süßwasserressourcen (FW)</common:shortDescription>
      </referenceToFlowDataSet>
      <functionType>General reminder flow</functionType>
      <exchangeDirection>Input</exchangeDirection>
      <common:other>
        <epd:amount epd:module="A1-A3">0.0227199781911751</epd:amount>
        <epd:referenceToUnitGroupDataSet refObjectId="93a60a57-a3c8-12da-a746-0800200c9a66" version="03.00.000" type="unit group data set" uri="../unitgroups/93a60a57-a3c8-12da-a746-0800200c9a66.xml">
          <common:shortDescription xml:lang="en">m3</common:shortDescription>
        </epd:referenceToUnitGroupDataSet>
        <epd:amount epd:module="C2">1.94295422447495E-6</epd:amount>
        <epd:amount epd:module="C3">0.00352523710757077</epd:amount>
        <epd:amount epd:module="D">-0.00103224552526426</epd:amount>
      </common:other>
    </exchange>
    <exchange dataSetInternalID="108846">
      <referenceToFlowDataSet refObjectId="430f9e0f-59b2-46a0-8e0d-55e0e84948fc" version="21.01.000" type="flow data set" uri="../flows/430f9e0f-59b2-46a0-8e0d-55e0e84948fc.xml">
        <common:shortDescription xml:lang="en">Hazardous waste disposed (HWD)</common:shortDescription>
        <common:shortDescription xml:lang="de">Gefährlicher Abfall zur Deponie (HWD)</common:shortDescription>
      </referenceToFlowDataSet>
      <functionType>General reminder flow</functionType>
      <exchangeDirection>Output</exchangeDirection>
      <common:other>
        <epd:amount epd:module="A1-A3">3.41514915936814E-8</epd:amount>
        <epd:referenceToUnitGroupDataSet refObjectId="93a60a57-a4c8-11da-a746-0800200c9a66" version="03.00.000" type="unit group data set" uri="../unitgroups/93a60a57-a4c8-11da-a746-0800200c9a66.xml">
          <common:shortDescription xml:lang="en">kg</common:shortDescription>
        </epd:referenceToUnitGroupDataSet>
        <epd:amount epd:module="C2">1.57438728108957E-12</epd:amount>
        <epd:amount epd:module="C3">1.51307721422E-10</epd:amount>
        <epd:amount epd:module="D">-2.84920126628823E-9</epd:amount>
      </common:other>
    </exchange>
    <exchange dataSetInternalID="108847">
      <referenceToFlowDataSet refObjectId="b29ef66b-e286-4afa-949f-62f1a7b4d7fa" version="21.01.000" type="flow data set" uri="../flows/b29ef66b-e286-4afa-949f-62f1a7b4d7fa.xml">
        <common:shortDescription xml:lang="en">Non harzardous waste disposed (NHWD)</common:shortDescription>
        <common:shortDescription xml:lang="de">Entsorgter nicht gefährlicher Abfall (NHWD)</common:shortDescription>
      </referenceToFlowDataSet>
      <functionType>General reminder flow</functionType>
      <exchangeDirection>Output</exchangeDirection>
      <common:other>
        <epd:amount epd:module="A1-A3">0.151005575200788</epd:amount>
        <epd:referenceToUnitGroupDataSet refObjectId="93a60a57-a4c8-11da-a746-0800200c9a66" version="03.00.000" type="unit group data set" uri="../unitgroups/93a60a57-a4c8-11da-a746-0800200c9a66.xml">
          <common:shortDescription xml:lang="en">kg</common:shortDescription>
        </epd:referenceToUnitGroupDataSet>
        <epd:amount epd:module="C2">6.08042485415762E-6</epd:amount>
        <epd:amount epd:module="C3">0.149612906934147</epd:amount>
        <epd:amount epd:module="D">-0.00432860763474544</epd:amount>
      </common:other>
    </exchange>
    <exchange dataSetInternalID="108848">
      <referenceToFlowDataSet refObjectId="3449546e-52ad-4b39-b809-9fb77cea8ff6" version="21.01.000" type="flow data set" uri="../flows/3449546e-52ad-4b39-b809-9fb77cea8ff6.xml">
        <common:shortDescription xml:lang="en">Radioactive waste disposed (RWD)</common:shortDescription>
        <common:shortDescription xml:lang="de">Entsorgter radioaktiver Abfall (RWD)</common:shortDescription>
      </referenceToFlowDataSet>
      <functionType>General reminder flow</functionType>
      <exchangeDirection>Output</exchangeDirection>
      <common:other>
        <epd:amount epd:module="A1-A3">0.000921016733267031</epd:amount>
        <epd:referenceToUnitGroupDataSet refObjectId="93a60a57-a4c8-11da-a746-0800200c9a66" version="03.00.000" type="unit group data set" uri="../unitgroups/93a60a57-a4c8-11da-a746-0800200c9a66.xml">
          <common:shortDescription xml:lang="en">kg</common:shortDescription>
        </epd:referenceToUnitGroupDataSet>
        <epd:amount epd:module="C2">3.61470627671868E-8</epd:amount>
        <epd:amount epd:module="C3">2.45381663925974E-5</epd:amount>
        <epd:amount epd:module="D">-0.000298438226281391</epd:amount>
      </common:other>
    </exchange>
    <exchange dataSetInternalID="108849">
      <referenceToFlowDataSet refObjectId="a2b32f97-3fc7-4af2-b209-525bc6426f33" version="21.01.000" type="flow data set" uri="../flows/a2b32f97-3fc7-4af2-b209-525bc6426f33.xml">
        <common:shortDescription xml:lang="en">Components for re-use (CRU)</common:shortDescription>
        <common:shortDescription xml:lang="de">Komponenten für die Wiederverwendung (CRU)</common:shortDescription>
      </referenceToFlowDataSet>
      <functionType>General reminder flow</functionType>
      <exchangeDirection>Output</exchangeDirection>
      <common:other>
        <epd:amount epd:module="A1-A3">0</epd:amount>
        <epd:referenceToUnitGroupDataSet refObjectId="93a60a57-a4c8-11da-a746-0800200c9a66" version="03.00.000" type="unit group data set" uri="../unitgroups/93a60a57-a4c8-11da-a746-0800200c9a66.xml">
          <common:shortDescription xml:lang="en">kg</common:shortDescription>
        </epd:referenceToUnitGroupDataSet>
        <epd:amount epd:module="C2">0</epd:amount>
        <epd:amount epd:module="C3">0</epd:amount>
        <epd:amount epd:module="D">0</epd:amount>
      </common:other>
    </exchange>
    <exchange dataSetInternalID="108850">
      <referenceToFlowDataSet refObjectId="d7fe48a5-4103-49c8-9aae-b0b5dfdbd6ae" version="21.01.000" type="flow data set" uri="../flows/d7fe48a5-4103-49c8-9aae-b0b5dfdbd6ae.xml">
        <common:shortDescription xml:lang="en">Materials for recycling  (MFR)</common:shortDescription>
        <common:shortDescription xml:lang="de">Stoffe zum Recycling (MFR)</common:shortDescription>
      </referenceToFlowDataSet>
      <functionType>General reminder flow</functionType>
      <exchangeDirection>Output</exchangeDirection>
      <common:other>
        <epd:amount epd:module="A1-A3">0</epd:amount>
        <epd:referenceToUnitGroupDataSet refObjectId="93a60a57-a4c8-11da-a746-0800200c9a66" version="03.00.000" type="unit group data set" uri="../unitgroups/93a60a57-a4c8-11da-a746-0800200c9a66.xml">
          <common:shortDescription xml:lang="en">kg</common:shortDescription>
        </epd:referenceToUnitGroupDataSet>
        <epd:amount epd:module="C2">0</epd:amount>
        <epd:amount epd:module="C3">0</epd:amount>
        <epd:amount epd:module="D">0</epd:amount>
      </common:other>
    </exchange>
    <exchange dataSetInternalID="108851">
      <referenceToFlowDataSet refObjectId="59a9181c-3aaf-46ee-8b13-2b3723b6e447" version="21.01.000" type="flow data set" uri="../flows/59a9181c-3aaf-46ee-8b13-2b3723b6e447.xml">
        <common:shortDescription xml:lang="en">Materials for energy recovery (MER)</common:shortDescription>
        <common:shortDescription xml:lang="de">Stoffe für die Energierückgewinnung (MER)</common:shortDescription>
      </referenceToFlowDataSet>
      <functionType>General reminder flow</functionType>
      <exchangeDirection>Output</exchangeDirection>
      <common:other>
        <epd:amount epd:module="A1-A3">0</epd:amount>
        <epd:referenceToUnitGroupDataSet refObjectId="93a60a57-a4c8-11da-a746-0800200c9a66" version="03.00.000" type="unit group data set" uri="../unitgroups/93a60a57-a4c8-11da-a746-0800200c9a66.xml">
          <common:shortDescription xml:lang="en">kg</common:shortDescription>
        </epd:referenceToUnitGroupDataSet>
        <epd:amount epd:module="C2">0</epd:amount>
        <epd:amount epd:module="C3">1</epd:amount>
        <epd:amount epd:module="D">0</epd:amount>
      </common:other>
    </exchange>
    <exchange dataSetInternalID="108852">
      <referenceToFlowDataSet refObjectId="4da0c987-2b76-40d6-9e9e-82a017aaaf29" version="21.01.000" type="flow data set" uri="../flows/4da0c987-2b76-40d6-9e9e-82a017aaaf29.xml">
        <common:shortDescription xml:lang="en">Exported electrical energy (EEE)</common:shortDescription>
        <common:shortDescription xml:lang="de">Exportierte elektrische Energie (EEE)</common:shortDescription>
      </referenceToFlowDataSet>
      <functionType>General reminder flow</functionType>
      <exchangeDirection>Output</exchangeDirection>
      <common:other>
        <epd:amount epd:module="A1-A3">0</epd:amount>
        <epd:referenceToUnitGroupDataSet refObjectId="93a60a57-a3c8-11da-a746-0800200c9a66" version="03.00.000" type="unit group data set" uri="../unitgroups/93a60a57-a3c8-11da-a746-0800200c9a66.xml">
          <common:shortDescription xml:lang="en">MJ</common:shortDescription>
        </epd:referenceToUnitGroupDataSet>
        <epd:amount epd:module="C2">0</epd:amount>
        <epd:amount epd:module="C3">2.22290915704752</epd:amount>
        <epd:amount epd:module="D">0</epd:amount>
      </common:other>
    </exchange>
    <exchange dataSetInternalID="108853">
      <referenceToFlowDataSet refObjectId="98daf38a-7a79-46d3-9a37-2b7bd0955810" version="21.01.000" type="flow data set" uri="../flows/98daf38a-7a79-46d3-9a37-2b7bd0955810.xml">
        <common:shortDescription xml:lang="en">Exported thermal energy (EET)</common:shortDescription>
        <common:shortDescription xml:lang="de">Exportierte thermische Energie (EET)</common:shortDescription>
      </referenceToFlowDataSet>
      <functionType>General reminder flow</functionType>
      <exchangeDirection>Output</exchangeDirection>
      <common:other>
        <epd:amount epd:module="A1-A3">0</epd:amount>
        <epd:referenceToUnitGroupDataSet refObjectId="93a60a57-a3c8-11da-a746-0800200c9a66" version="03.00.000" type="unit group data set" uri="../unitgroups/93a60a57-a3c8-11da-a746-0800200c9a66.xml">
          <common:shortDescription xml:lang="en">MJ</common:shortDescription>
        </epd:referenceToUnitGroupDataSet>
        <epd:amount epd:module="C2">0</epd:amount>
        <epd:amount epd:module="C3">5.10362831011177</epd:amount>
        <epd:amount epd:module="D">0</epd:amount>
      </common:other>
    </exchange>
  </exchanges>
  <LCIAResults>
    <LCIAResult>
      <referenceToLCIAMethodDataSet refObjectId="6a37f984-a4b3-458a-a20a-64418c145fa2" version="21.01.000" type="LCIA method data set" uri="../lciamethods/6a37f984-a4b3-458a-a20a-64418c145fa2.xml">
        <common:shortDescription xml:lang="en">Global Warming Potential - total (GWP-total)</common:shortDescription>
        <common:shortDescription xml:lang="de">Globales Erwärmungspotenzial - total (GWP-total)</common:shortDescription>
      </referenceToLCIAMethodDataSet>
      <common:other>
        <epd:amount epd:module="A1-A3">6.83074542037476</epd:amount>
        <epd:amount epd:module="C2">0.00286116039368676</epd:amount>
        <epd:amount epd:module="C3">1.44126963457891</epd:amount>
        <epd:amount epd:module="D">-0.528137779004067</epd:amount>
        <epd:referenceToUnitGroupDataSet refObjectId="1ebf3012-d0db-4de2-aefd-ef30cedb0be1" version="25.00.000" type="unit group data set" uri="../unitgroups/1ebf3012-d0db-4de2-aefd-ef30cedb0be1.xml">
          <common:shortDescription xml:lang="en">kg CO2 eq.</common:shortDescription>
        </epd:referenceToUnitGroupDataSet>
      </common:other>
    </LCIAResult>
    <LCIAResult>
      <referenceToLCIAMethodDataSet refObjectId="5f635281-343e-44fb-83df-1971b155e6b6" version="21.01.000" type="LCIA method data set" uri="../lciamethods/5f635281-343e-44fb-83df-1971b155e6b6.xml">
        <common:shortDescription xml:lang="en">Global Warming Potential - fossil fuels (GWP-fossil)</common:shortDescription>
        <common:shortDescription xml:lang="de">Globales Erwärmungspotenzial - fossil (GWP-fossil)</common:shortDescription>
      </referenceToLCIAMethodDataSet>
      <common:other>
        <epd:amount epd:module="A1-A3">6.76355177220745</epd:amount>
        <epd:amount epd:module="C2">0.00284173285565002</epd:amount>
        <epd:amount epd:module="C3">1.44102037032622</epd:amount>
        <epd:amount epd:module="D">-0.521749741314557</epd:amount>
        <epd:referenceToUnitGroupDataSet refObjectId="1ebf3012-d0db-4de2-aefd-ef30cedb0be1" version="25.00.000" type="unit group data set" uri="../unitgroups/1ebf3012-d0db-4de2-aefd-ef30cedb0be1.xml">
          <common:shortDescription xml:lang="en">kg CO2 eq.</common:shortDescription>
        </epd:referenceToUnitGroupDataSet>
      </common:other>
    </LCIAResult>
    <LCIAResult>
      <referenceToLCIAMethodDataSet refObjectId="2356e1ab-0185-4db5-86e5-16de51c7485c" version="21.01.000" type="LCIA method data set" uri="../lciamethods/2356e1ab-0185-4db5-86e5-16de51c7485c.xml">
        <common:shortDescription xml:lang="en">Global Warming Potential - biogenic (GWP-biogenic)</common:shortDescription>
        <common:shortDescription xml:lang="de">Globales Erwärmungspotenzial - biogen (GWP-biogenic)</common:shortDescription>
      </referenceToLCIAMethodDataSet>
      <common:other>
        <epd:amount epd:module="A1-A3">0.0646869215612166</epd:amount>
        <epd:amount epd:module="C2">1.17715755154072E-6</epd:amount>
        <epd:amount epd:module="C3">0.000157116848691208</epd:amount>
        <epd:amount epd:module="D">-0.00562149928580943</epd:amount>
        <epd:referenceToUnitGroupDataSet refObjectId="1ebf3012-d0db-4de2-aefd-ef30cedb0be1" version="25.00.000" type="unit group data set" uri="../unitgroups/1ebf3012-d0db-4de2-aefd-ef30cedb0be1.xml">
          <common:shortDescription xml:lang="en">kg CO2 eq.</common:shortDescription>
        </epd:referenceToUnitGroupDataSet>
      </common:other>
    </LCIAResult>
    <LCIAResult>
      <referenceToLCIAMethodDataSet refObjectId="4331bbdb-978a-490d-8707-eeb047f01a55" version="21.01.000" type="LCIA method data set" uri="../lciamethods/4331bbdb-978a-490d-8707-eeb047f01a55.xml">
        <common:shortDescription xml:lang="en">Global Warming Potential - land use and land use change (GWP-luluc)</common:shortDescription>
        <common:shortDescription xml:lang="de">Globales Erwärmungspotenzial - luluc (GWP-luluc)</common:shortDescription>
      </referenceToLCIAMethodDataSet>
      <common:other>
        <epd:amount epd:module="A1-A3">0.00250672660609273</epd:amount>
        <epd:amount epd:module="C2">1.82503804851983E-5</epd:amount>
        <epd:amount epd:module="C3">9.21474040043077E-5</epd:amount>
        <epd:amount epd:module="D">-0.000766538403700838</epd:amount>
        <epd:referenceToUnitGroupDataSet refObjectId="1ebf3012-d0db-4de2-aefd-ef30cedb0be1" version="25.00.000" type="unit group data set" uri="../unitgroups/1ebf3012-d0db-4de2-aefd-ef30cedb0be1.xml">
          <common:shortDescription xml:lang="en">kg CO2 eq.</common:shortDescription>
        </epd:referenceToUnitGroupDataSet>
      </common:other>
    </LCIAResult>
    <LCIAResult>
      <referenceToLCIAMethodDataSet refObjectId="b5c629d6-def3-11e6-bf01-fe55135034f3" version="21.01.000" type="LCIA method data set" uri="../lciamethods/b5c629d6-def3-11e6-bf01-fe55135034f3.xml">
        <common:shortDescription xml:lang="en">Depletion potenzial of the stratospheric ozone layer (ODP)</common:shortDescription>
        <common:shortDescription xml:lang="de">Abbaupotenzial der stratosphärischen Ozonschicht (ODP)</common:shortDescription>
      </referenceToLCIAMethodDataSet>
      <common:other>
        <epd:amount epd:module="A1-A3">2.47774628607028E-14</epd:amount>
        <epd:amount epd:module="C2">7.27125388284495E-19</epd:amount>
        <epd:amount epd:module="C3">8.22066140200319E-16</epd:amount>
        <epd:amount epd:module="D">-1.21138379929496E-14</epd:amount>
        <epd:referenceToUnitGroupDataSet refObjectId="d9e957c9-7309-4474-bf3a-7777df6c4e5b" version="25.00.000" type="unit group data set" uri="../unitgroups/d9e957c9-7309-4474-bf3a-7777df6c4e5b.xml">
          <common:shortDescription xml:lang="en">kg CFC-11 eq.</common:shortDescription>
        </epd:referenceToUnitGroupDataSet>
      </common:other>
    </LCIAResult>
    <LCIAResult>
      <referenceToLCIAMethodDataSet refObjectId="b5c611c6-def3-11e6-bf01-fe55135034f3" version="21.01.000" type="LCIA method data set" uri="../lciamethods/b5c611c6-def3-11e6-bf01-fe55135034f3.xml">
        <common:shortDescription xml:lang="en">Acidifcation potential, Accumulated Exceedance (AP)</common:shortDescription>
        <common:shortDescription xml:lang="de">Versauerungspotenzial, kumulierte Überschreitung (AP)</common:shortDescription>
      </referenceToLCIAMethodDataSet>
      <common:other>
        <epd:amount epd:module="A1-A3">0.00666236016535696</epd:amount>
        <epd:amount epd:module="C2">8.05696368805402E-6</epd:amount>
        <epd:amount epd:module="C3">0.000251066130995848</epd:amount>
        <epd:amount epd:module="D">-0.000535368660511783</epd:amount>
        <epd:referenceToUnitGroupDataSet refObjectId="42e089ac-92bf-4bf2-8ca1-5fc40d18f2ed" version="00.01.000" type="unit group data set" uri="../unitgroups/42e089ac-92bf-4bf2-8ca1-5fc40d18f2ed.xml">
          <common:shortDescription xml:lang="en">Mole of H+ eq.</common:shortDescription>
        </epd:referenceToUnitGroupDataSet>
      </common:other>
    </LCIAResult>
    <LCIAResult>
      <referenceToLCIAMethodDataSet refObjectId="b53ec18f-7377-4ad3-86eb-cc3f4f276b2b" version="21.01.000" type="LCIA method data set" uri="../lciamethods/b53ec18f-7377-4ad3-86eb-cc3f4f276b2b.xml">
        <common:shortDescription xml:lang="en">Eutrophication potential - freshwater (EP-freshwater)</common:shortDescription>
        <common:shortDescription xml:lang="de">Eutrophierungspotenzial - Süßwasser (EP-freshwater)</common:shortDescription>
      </referenceToLCIAMethodDataSet>
      <common:other>
        <epd:amount epd:module="A1-A3">8.52603218621021E-6</epd:amount>
        <epd:amount epd:module="C2">5.84435170815817E-9</epd:amount>
        <epd:amount epd:module="C3">1.18386933602184E-7</epd:amount>
        <epd:amount epd:module="D">-1.27531960369185E-6</epd:amount>
        <epd:referenceToUnitGroupDataSet refObjectId="0429039d-a61d-4590-ba67-aa4a20a810a1" version="25.00.000" type="unit group data set" uri="../unitgroups/0429039d-a61d-4590-ba67-aa4a20a810a1.xml">
          <common:shortDescription xml:lang="en">kg P eq.</common:shortDescription>
        </epd:referenceToUnitGroupDataSet>
      </common:other>
    </LCIAResult>
    <LCIAResult>
      <referenceToLCIAMethodDataSet refObjectId="b5c619fa-def3-11e6-bf01-fe55135034f3" version="21.01.000" type="LCIA method data set" uri="../lciamethods/b5c619fa-def3-11e6-bf01-fe55135034f3.xml">
        <common:shortDescription xml:lang="en">Eutrophication potential - marine (EP-marine)</common:shortDescription>
        <common:shortDescription xml:lang="de">Eutrophierungspotenzial - Salzwasser (EP-marine)</common:shortDescription>
      </referenceToLCIAMethodDataSet>
      <common:other>
        <epd:amount epd:module="A1-A3">0.00750770676370691</epd:amount>
        <epd:amount epd:module="C2">3.71167285756776E-6</epd:amount>
        <epd:amount epd:module="C3">5.67629125410902E-5</epd:amount>
        <epd:amount epd:module="D">-0.000196908963178276</epd:amount>
        <epd:referenceToUnitGroupDataSet refObjectId="d05bb823-ecdf-4686-8c40-bf1d9257859f" version="00.00.003" type="unit group data set" uri="../unitgroups/d05bb823-ecdf-4686-8c40-bf1d9257859f.xml">
          <common:shortDescription xml:lang="en">kg N eq.</common:shortDescription>
        </epd:referenceToUnitGroupDataSet>
      </common:other>
    </LCIAResult>
    <LCIAResult>
      <referenceToLCIAMethodDataSet refObjectId="b5c614d2-def3-11e6-bf01-fe55135034f3" version="21.01.000" type="LCIA method data set" uri="../lciamethods/b5c614d2-def3-11e6-bf01-fe55135034f3.xml">
        <common:shortDescription xml:lang="en">Eutrophication potential - terrestrial (EP-terrestrial)</common:shortDescription>
        <common:shortDescription xml:lang="de">Eutrophierungspotenzial - Land (EP-terrestrial)</common:shortDescription>
      </referenceToLCIAMethodDataSet>
      <common:other>
        <epd:amount epd:module="A1-A3">0.0246854869131876</epd:amount>
        <epd:amount epd:module="C2">4.152687055456E-5</epd:amount>
        <epd:amount epd:module="C3">0.00115583469498389</epd:amount>
        <epd:amount epd:module="D">-0.0020977799114459</epd:amount>
        <epd:referenceToUnitGroupDataSet refObjectId="71b4d617-0ec9-4d3f-b65e-e438940c2401" version="00.00.003" type="unit group data set" uri="../unitgroups/71b4d617-0ec9-4d3f-b65e-e438940c2401.xml">
          <common:shortDescription xml:lang="en">Mole of N eq.</common:shortDescription>
        </epd:referenceToUnitGroupDataSet>
      </common:other>
    </LCIAResult>
    <LCIAResult>
      <referenceToLCIAMethodDataSet refObjectId="b5c610fe-def3-11e6-bf01-fe55135034f3" version="21.01.000" type="LCIA method data set" uri="../lciamethods/b5c610fe-def3-11e6-bf01-fe55135034f3.xml">
        <common:shortDescription xml:lang="en">Photochemical Ozone Creation Potential  (POCP)</common:shortDescription>
        <common:shortDescription xml:lang="de">Bildungspotenzial für troposphärisches Ozon (POCP)</common:shortDescription>
      </referenceToLCIAMethodDataSet>
      <common:other>
        <epd:amount epd:module="A1-A3">0.00693653530705119</epd:amount>
        <epd:amount epd:module="C2">7.23784941161807E-6</epd:amount>
        <epd:amount epd:module="C3">0.000157932811838593</epd:amount>
        <epd:amount epd:module="D">-0.000515712453282876</epd:amount>
        <epd:referenceToUnitGroupDataSet refObjectId="d27c25f8-fbc1-44c6-b47b-4adbae4199c6" version="00.00.003" type="unit group data set" uri="../unitgroups/d27c25f8-fbc1-44c6-b47b-4adbae4199c6.xml">
          <common:shortDescription xml:lang="en">kg NMVOC eq.</common:shortDescription>
        </epd:referenceToUnitGroupDataSet>
      </common:other>
    </LCIAResult>
    <LCIAResult>
      <referenceToLCIAMethodDataSet refObjectId="b2ad6494-c78d-11e6-9d9d-cec0c932ce01" version="21.01.000" type="LCIA method data set" uri="../lciamethods/b2ad6494-c78d-11e6-9d9d-cec0c932ce01.xml">
        <common:shortDescription xml:lang="en">Abiotic depletion potential - non-fossil resources (ADPE)</common:shortDescription>
        <common:shortDescription xml:lang="de">Potenzial für die Verknappung abiotischer Ressourcen  nicht fossile Ressourcen (ADPE)</common:shortDescription>
      </referenceToLCIAMethodDataSet>
      <common:other>
        <epd:amount epd:module="A1-A3">8.12230787549436E-6</epd:amount>
        <epd:amount epd:module="C2">2.47191200372629E-10</epd:amount>
        <epd:amount epd:module="C3">1.11143778454605E-8</epd:amount>
        <epd:amount epd:module="D">-1.63656377929334E-7</epd:amount>
        <epd:referenceToUnitGroupDataSet refObjectId="54ccd2d9-a32a-4fc2-923d-f2c8c93e89d4" version="25.00.000" type="unit group data set" uri="../unitgroups/54ccd2d9-a32a-4fc2-923d-f2c8c93e89d4.xml">
          <common:shortDescription xml:lang="en">kg Sb eq.</common:shortDescription>
        </epd:referenceToUnitGroupDataSet>
      </common:other>
    </LCIAResult>
    <LCIAResult>
      <referenceToLCIAMethodDataSet refObjectId="b2ad6110-c78d-11e6-9d9d-cec0c932ce01" version="21.01.000" type="LCIA method data set" uri="../lciamethods/b2ad6110-c78d-11e6-9d9d-cec0c932ce01.xml">
        <common:shortDescription xml:lang="en">Abiotic depletion potential - fossil resources (ADPF)</common:shortDescription>
        <common:shortDescription xml:lang="de">Potenzial für die Verknappung abiotischer Ressourcen  fossile Brennstoffe (ADPF)</common:shortDescription>
      </referenceToLCIAMethodDataSet>
      <common:other>
        <epd:amount epd:module="A1-A3">129.535859604253</epd:amount>
        <epd:amount epd:module="C2">0.0376661111022794</epd:amount>
        <epd:amount epd:module="C3">0.689877661538729</epd:amount>
        <epd:amount epd:module="D">-8.2058323878605</epd:amount>
        <epd:referenceToUnitGroupDataSet refObjectId="93a60a57-a3c8-11da-a746-0800200c9a66" version="02.00.000" type="unit group data set" uri="../unitgroups/93a60a57-a3c8-11da-a746-0800200c9a66.xml">
          <common:shortDescription xml:lang="en">MJ</common:shortDescription>
        </epd:referenceToUnitGroupDataSet>
      </common:other>
    </LCIAResult>
    <LCIAResult>
      <referenceToLCIAMethodDataSet refObjectId="b2ad66ce-c78d-11e6-9d9d-cec0c932ce01" version="21.01.000" type="LCIA method data set" uri="../lciamethods/b2ad66ce-c78d-11e6-9d9d-cec0c932ce01.xml">
        <common:shortDescription xml:lang="en">Water (user) deprivation potential (WDP)</common:shortDescription>
        <common:shortDescription xml:lang="de">Wasser-Entzugspotenzial (Benutzer) (WDP)</common:shortDescription>
      </referenceToLCIAMethodDataSet>
      <common:other>
        <epd:amount epd:module="A1-A3">0.149079580167243</epd:amount>
        <epd:amount epd:module="C2">1.10467905878249E-5</epd:amount>
        <epd:amount epd:module="C3">0.147298099794283</epd:amount>
        <epd:amount epd:module="D">-0.00626662492672303</epd:amount>
        <epd:referenceToUnitGroupDataSet refObjectId="6ae2df01-888e-46c8-b17d-49fa3869b476" version="00.00.003" type="unit group data set" uri="../unitgroups/6ae2df01-888e-46c8-b17d-49fa3869b476.xml">
          <common:shortDescription xml:lang="en">m³ world equiv.</common:shortDescription>
        </epd:referenceToUnitGroupDataSet>
      </common:other>
    </LCIAResult>
  </LCIAResults>
</processDataSet>
