<?xml version="1.0" encoding="utf-8"?>
<?xml-stylesheet version="1.0" href="../../stylesheets/epd2html.xsl" type="text/xsl"?>
<processDataSet xmlns="http://lca.jrc.it/ILCD/Process" xmlns:common="http://lca.jrc.it/ILCD/Common" xmlns:epd="http://www.iai.kit.edu/EPD/2013" xmlns:epd2="http://www.indata.network/EPD/2019" xmlns:xsi="http://www.w3.org/2001/XMLSchema-instance" xsi:schemaLocation="http://lca.jrc.it/ILCD/Process ../../schemas/EPD_DataSet.xsd" locations="../ILCDLocations.xml" epd2:epd-version="1.2" version="1.1">
  <processInformation>
    <dataSetInformation>
      <common:UUID>d8d0942a-0c4e-49e0-bd78-abc84a41fd80</common:UUID>
      <name>
        <baseName xml:lang="en">Stainless steel drinking water pipe</baseName>
        <baseName xml:lang="de">Edelstahl-Trinkwasserrohr</baseName>
        <functionalUnitFlowProperties xml:lang="en">Stainless steel pipe</functionalUnitFlowProperties>
      </name>
      <classificationInformation>
        <common:classification name="oekobau.dat">
          <common:class level="0" classId="4">Metalle</common:class>
          <common:class level="1" classId="4.2">Edelstahl</common:class>
          <common:class level="2" classId="4.2.03">Edelstahl Trinkwasserrohre</common:class>
        </common:classification>
      </classificationInformation>
      <common:generalComment xml:lang="en">This data set has been modeled according to the European Standard EN 15804+A2 for Sustainable Building. Results are depicted in modules that allow the structured expression of results over the entire life cycle.</common:generalComment>
      <common:generalComment xml:lang="de">Dieser Datensatz wurde nach dem European Standard EN 15804+A2 für Nachhaltiges Bauen modelliert. Ergebnisse werden in Modulen abgebildet, die den strukturierten Ausdruck von Ergebnissen über den gesamten Lebenszyklus zulassen.</common:generalComment>
      <common:other>
        <epd:safetyMargins>
          <epd:margins>10</epd:margins>
          <epd:description xml:lang="en">Product system almost completely covered. Good technological, temporal and geographic representativeness.</epd:description>
          <epd:description xml:lang="de">Produktsystem weitgehend vollständig abgebildet. Gute technologische, zeitliche und geographische Repräsentativität.</epd:description>
        </epd:safetyMargins>
      </common:other>
    </dataSetInformation>
    <quantitativeReference type="Reference flow(s)">
      <referenceToReferenceFlow>103990</referenceToReferenceFlow>
    </quantitativeReference>
    <time>
      <common:referenceYear>2021</common:referenceYear>
      <common:dataSetValidUntil>2022</common:dataSetValidUntil>
      <common:timeRepresentativenessDescription xml:lang="en">Annual average</common:timeRepresentativenessDescription>
      <common:timeRepresentativenessDescription xml:lang="de">Jährlicher Durchschnitt</common:timeRepresentativenessDescription>
    </time>
    <geography>
      <locationOfOperationSupplyOrProduction location="DE">
        <descriptionOfRestrictions xml:lang="en">The data set represents the country specific situation in Germany, focusing on the main technologies, the region specific characteristics and / or import statistics.</descriptionOfRestrictions>
        <descriptionOfRestrictions xml:lang="de">Der Datensatz bildet die länderspezifische Situation in Deutschland ab. Dabei werden Haupttechnologien, spezifische regionale Charakteristiken und ggf. Importstatistiken berücksichtigt.</descriptionOfRestrictions>
      </locationOfOperationSupplyOrProduction>
    </geography>
    <technology>
      <technologyDescriptionAndIncludedProcesses xml:lang="en">The dataset describes the production of a stainless steel drinking water pipe made of stainless steel (cold rolled). In so doing, the process of bending the steel sheet, the production of the welding seam as well as all necessary materials and energy expenditures have been considered. Transports from the factory to the building site are not considered and must be included according to the system boundaries.
The main process step is the melting of stainless steel scrap in the electric arc furnace (EAF), thus the consumed energy is mainly electric power. The major feed stock for the EAF is stainless steel scrap, which may comprise of scrap from inside the steelworks (e.g. cut-offs), cut-offs from steel product manufacturers (e.g. vehicle builders) and post-consumer scrap (e.g. end of life products). As in the integrated steel plant including blast furnaces and converters, a slag is formed from lime to collect undesirable components in the steel. Thus lime is an additive as well as coal (carbon) as reducing agent and alloying elements. Oxygen lances and / or oxy-fuel burners are used to assist in the early stages of melting.  For every material fraction the transport is considered in the data set.   For the production of carbon steel and low alloyed steels, following main operations are performed: raw material handling and storage, furnace charging with/without scrap preheating, EAF scrap melting, steel and slag tapping, ladle furnace treatments for quality adjustment, slag handling and finally continuous casting.   For high alloyed respectively stainless steels, the operation sequence is more complex and tailor-made for the end-products. In addition to the mentioned operations for carbon steels various ladle treatments (secondary metallurgy) are carried out like desulphurisation, degassing for the elimination of dissolved gases like nitrogen and hydrogen, decarburisation (AOD=Argon-Oxygen-Decarburisation or VOD=Vacuum-Oxygen-Decarburisation).  The following operations are two rolling processes: the hot strip mill and the cold rolling mill. In the hot rolling mill the slab is reshaped above the recrystallization temperature. The qualities obtained in this process are e.g. strength and surface quality. During the rolling process the material passes through the furnace and the rolling line. In the furnace the metal is preheated by natural gas. There is no need for an additional warming, if the hot slabs are directly charged into the rolling mill. The forming is done in various rolling frames until the final shape is obtained. The steel scrap in this process are directly recycled.  In the cold rolling mill the material is reshaped below the recrystallization temperature. Thereby a enhanced surface quality, an improved dimensional accuracy as well as a higher strength are achieved. The different process steps are: pickling, the rolling line and the heat treatment.

In the disposal phase, mechanical dismantling is accounted for in module C1 for steel products (excavator), for all other metals a manual dismantling is assumed (no loads). Collecting losses are neglected. It is assumed that all metals reach the end of the waste status immediately after dismantling. This means that the loads for processing and the credits for the substitution of primary material are shown in Module D.
The transport in module C2 to the treatment plant takes place with a truck (50km).
Module D includes loads for sorting, remelting, slag treatment, landfill, filtration of dusts and dross treatment. Credits are given for the net scrap amount (amount returned minus secondary material content, minus processing losses) for the average material mix (from different alloys).</technologyDescriptionAndIncludedProcesses>
      <technologyDescriptionAndIncludedProcesses xml:lang="de">Der Datensatz wird die Herstellung einer Trinkwasserleitung aus rostfreiem Stahl (kaltgewalzt). Dabei wird das Verfahren zum Biegen des Stahlblechs, die Herstellung der Schweißnaht sowie alle notwendigen Materialien sowie der gesamte Energieaufwand berücksichtigt. Transporte von der Fabrik zur Baustelle werden nicht berücksichtigt und müssen entsprechend den Systemgrenzen einbezogen werden.
Der Hauptverfahrensschritt ist hierbei die Schmelzung von Edelstahlschrott im Elektrolichtbogenofen (EAF), folglich besteht der Energieverbrauch hauptsächlich aus elektrischer Leistung/Energie. Das Hauptausgangsmaterial für die Lichtbögenöfen  ist  Eisenmetallschrott, der den Schrott innerhalb der Stahlwerke (z. B. Ausschuss), Ausschuss von Stahlproduktherstellern (z. B. Fahrzeugbauer) und Verbraucherschrott (z. B. Altprodukte/End-of-Life-Produkte) einschließt. Wie in dem integrierten Hütten-/Stahlwerk inklusive Hochöfen und Konvertern, wird Schlacke aus Kalk gebildet, um unerwünschte Komponenten im Stahl zu sammeln. Dementsprechend ist Kalk ein Zusatzstoff, ebenso wie  Kohle  (Kohlenstoff) ein Reduktionsmittel ist. Sauerstofflanzen und/oder Sauerstoffbrenner werden zur Unterstützung in frühen Stadien des Schmelzens verwendet. Für jede Metallfraktion wird der Transport im Datensatz berücksichtigt. Für die Herstellung  von Karbonstahl  und niedriglegierten Stahlen werden die folgenden Operationen durchgeführt: Rohmaterial-Verarbeitung und -Lagerung, Hochofenbeschickung mit/ohne Schrottvorwärmung, Schrott-Einschmelzung im Lichtbogenofen, Stahl- und Schlacken-Abstechen, Stahlbehandlung zur Qualitätsanpassung, Schlacketransporte und schließlich Strangguss. Für hochlegierte bzw. rostfreie Stähle ist die Arbeitsfolge komplexer und für Endprodukte maßgeschneidert. Zusätzlich zu den genannten Operationen für Kohlenstoffstähle werden verschiedene Pfannenbehandlungen (Sekundärmetallurgie) wie Entschwefelung, Entgasen zur Entfernung von gelösten Gasen wie Stickstoff und Wasserstoff, Entkohlung (AOD = Argon-Sauerstoff-Entkohlung oder VOD = Vakuum-Sauerstoff-Entkohlung) ausgeführt. Die folgenden Funktionen sind zwei Walzverfahren: das Warmbandwalzwerk und das Kaltwalzwerk. Im Warmwalzwerk wird die Platte oberhalb der Rekristallisationstemperatur verformt. Die in diesem Verfahren erhaltenen Eigenschaften sind z.B. Festigkeit und Oberflächenqualität. Während des Walzprozesses durchläuft das Material durch Ofen und die Walzlinie. Im Ofen wird das Metall durch Erdgas vorgewärmt. Es besteht keine Notwendigkeit für eine zusätzliche Erwärmung, wenn die heißen Platten direkt in das Walzwerk geladen werden. Das Formen läuft in verschiedenen Walzrahmen ab, bis die endgültige Form erhalten wird. Der Stahlschrott in diesem Prozess wird direkt recycelt. Im Kaltwalzwerk wird das Material unterhalb der Rekristallisationstemperatur verformt. Dadurch werden eine verbesserte Oberflächenqualität, eine verbesserte Maßgenauigkeit sowie eine höhere Festigkeit erzielt. Die verschiedenen Verfahrensschritte sind: Beizen, die Walzlinie und Wärmebehandlung.
 
In der Entsorgungsphase wird in Modul C1 für Stahlprodukte ein maschineller Rückbau bilanziert (Bagger). Für alle anderen Metalle erfolgt ein manueller Rückbau (lastenfrei). Sammelverluste werden vernachlässigt. Es wird angenommen, dass alle Metalle das Ende der Abfalleigenschaft direkt nach dem Ausbau erreichen. Das heißt die Lasten für die Aufbereitung und die Gutschriften für die Substitution von Primärmaterial werden in Modul D ausgewiesen.
Der Transport in Modul C2 zur Aufbereitungsanlage erfolgt mit einem LKW (50km). 
In Modul D sind die Lasten für die Sortierung, Umschmelzen, Schlackebehandlung, Deponierung von Reststoffen, Behandlung von Filterstäuben und Krätzebehandlung enthalten. Die Gutschriften werden für die Nettoschrottmenge (zurückgebaute Menge abzüglich ggfs. enthaltenes Sekundärmaterial, abzüglich Aufbereitungsverluste) für den durchschnittlich vorhandenen Materialmix (aus verschiedenen Legierungen) vergeben.</technologyDescriptionAndIncludedProcesses>
      <technologicalApplicability xml:lang="en">This product can be used in construction.</technologicalApplicability>
      <technologicalApplicability xml:lang="de">Dieses Produkt kann im Baubereich verwendet werden.</technologicalApplicability>
      <referenceToTechnologyPictogramme refObjectId="97f20a4b-d27c-4239-86d7-2aa20dad8c8b" version="21.01.000" type="source data set" uri="../sources/97f20a4b-d27c-4239-86d7-2aa20dad8c8b.xml">
        <common:shortDescription xml:lang="en">metals_glo_stainless steel production.jpg</common:shortDescription>
      </referenceToTechnologyPictogramme>
    </technology>
  </processInformation>
  <modellingAndValidation>
    <LCIMethodAndAllocation>
      <typeOfDataSet>EPD</typeOfDataSet>
      <common:other>
        <epd:subType>generic dataset</epd:subType>
      </common:other>
    </LCIMethodAndAllocation>
    <dataSourcesTreatmentAndRepresentativeness>
      <referenceToDataSource refObjectId="e3bd9bbf-2c3c-42aa-8892-fd13f1065ca5" version="21.01.000" type="source data set" uri="../sources/e3bd9bbf-2c3c-42aa-8892-fd13f1065ca5.xml">
        <common:shortDescription xml:lang="en">Documentation of data quality management</common:shortDescription>
      </referenceToDataSource>
      <referenceToDataSource refObjectId="1cece811-7501-44d4-8067-9259bd5cb835" version="00.01.000" type="source data set" uri="../sources/1cece811-7501-44d4-8067-9259bd5cb835.xml">
        <common:shortDescription xml:lang="en">GaBi Database Edition 2021, CUP2021.01</common:shortDescription>
      </referenceToDataSource>
      <referenceToDataSource refObjectId="28d74cc0-db8b-4d7e-bc44-5f6d56ce0c4a" version="00.03.002" type="source data set" uri="../sources/28d74cc0-db8b-4d7e-bc44-5f6d56ce0c4a.xml">
        <common:shortDescription xml:lang="en">GaBi database (all versions)</common:shortDescription>
      </referenceToDataSource>
      <useAdviceForDataSet xml:lang="en">The data set represents a cradle to gate inventory. It can be used to characterise the supply chain situation of the respective commodity in a representative manner. Combination with individual unit processes using this commodity enables the generation of user-specific (product) LCAs.</useAdviceForDataSet>
      <useAdviceForDataSet xml:lang="de">Der Datensatz repräsentiert ein Cradle to Gate Inventar. Er kann verwendet werden, um die Lieferkette des jeweiligen Produktes in einer repräsentativen Weise zu charakterisieren. Die Kombination mit einzelnen Einheitenprozessen und diesem Produkt ermöglicht die Erstellung von anwenderspezifischen (Produkt-) LCAs.</useAdviceForDataSet>
    </dataSourcesTreatmentAndRepresentativeness>
    <validation>
      <review type="Dependent internal review">
        <common:referenceToNameOfReviewerAndInstitution refObjectId="d7fa0337-f279-430d-becf-7f3111a85010" version="21.01.000" type="contact data set" uri="../contacts/d7fa0337-f279-430d-becf-7f3111a85010.xml">
          <common:shortDescription xml:lang="en">Sphera Solutions GmbH</common:shortDescription>
        </common:referenceToNameOfReviewerAndInstitution>
      </review>
      <review type="Independent external review">
        <common:referenceToNameOfReviewerAndInstitution refObjectId="8f1306f0-7b83-4f36-a537-aa83f0498266" version="21.01.000" type="contact data set" uri="../contacts/8f1306f0-7b83-4f36-a537-aa83f0498266.xml">
          <common:shortDescription xml:lang="en">GaBi user forum</common:shortDescription>
        </common:referenceToNameOfReviewerAndInstitution>
      </review>
    </validation>
    <complianceDeclarations>
      <compliance>
        <common:referenceToComplianceSystem refObjectId="c0016b33-8cf7-415c-ac6e-deba0d21440d" version="00.01.000" type="source data set" uri="../sources/c0016b33-8cf7-415c-ac6e-deba0d21440d.xml">
          <common:shortDescription xml:lang="de">EN 15804+A2</common:shortDescription>
          <common:shortDescription xml:lang="en">EN 15804+A2</common:shortDescription>
        </common:referenceToComplianceSystem>
        <common:approvalOfOverallCompliance>Fully compliant</common:approvalOfOverallCompliance>
      </compliance>
    </complianceDeclarations>
  </modellingAndValidation>
  <administrativeInformation>
    <dataEntryBy>
      <common:timeStamp>2021-04-28T21:03:12+01:00</common:timeStamp>
      <common:referenceToDataSetFormat refObjectId="a97a0155-0234-4b87-b4ce-a45da52f2a40" version="01.00.000" type="source data set" uri="../sources/a97a0155-0234-4b87-b4ce-a45da52f2a40.xml">
        <common:shortDescription xml:lang="de">ILCD format 1.1</common:shortDescription>
        <common:shortDescription xml:lang="en">ILCD format 1.1</common:shortDescription>
      </common:referenceToDataSetFormat>
      <common:referenceToDataSetFormat refObjectId="a29449fd-aa2f-4de8-b5d7-4b06b43c6fde" version="00.01.000" type="source data set" uri="../sources/a29449fd-aa2f-4de8-b5d7-4b06b43c6fde.xml">
        <common:shortDescription xml:lang="de">EPD-Datenformaterweiterungen v1.2</common:shortDescription>
        <common:shortDescription xml:lang="en">EPD Data Format Extensions v1.2</common:shortDescription>
      </common:referenceToDataSetFormat>
      <common:referenceToPersonOrEntityEnteringTheData refObjectId="d7fa0337-f279-430d-becf-7f3111a85010" version="21.01.000" type="contact data set" uri="../contacts/d7fa0337-f279-430d-becf-7f3111a85010.xml">
        <common:shortDescription xml:lang="en">Sphera Solutions GmbH</common:shortDescription>
      </common:referenceToPersonOrEntityEnteringTheData>
    </dataEntryBy>
    <publicationAndOwnership>
      <common:dataSetVersion>20.21.060</common:dataSetVersion>
      <common:referenceToPrecedingDataSetVersion refObjectId="d8d0942a-0c4e-49e0-bd78-abc84a41fd80" type="process data set" uri="https://www.oekobaudat.de/OEKOBAU.DAT/datasetdetail/process.xhtml?uuid=d8d0942a-0c4e-49e0-bd78-abc84a41fd80&amp;stock=OBD_2020_II&amp;lang=de">
        <common:shortDescription xml:lang="en">Stainless steel drinking water pipe</common:shortDescription>
      </common:referenceToPrecedingDataSetVersion>
      <common:referenceToOwnershipOfDataSet refObjectId="d7fa0337-f279-430d-becf-7f3111a85010" version="21.01.000" type="contact data set" uri="../contacts/d7fa0337-f279-430d-becf-7f3111a85010.xml">
        <common:shortDescription xml:lang="en">Sphera Solutions GmbH</common:shortDescription>
      </common:referenceToOwnershipOfDataSet>
      <common:copyright>true</common:copyright>
      <common:licenseType>Free of charge for all users and uses</common:licenseType>
      <common:accessRestrictions xml:lang="en">The license conditions as stated on https://www.oekobaudat.de/ apply.</common:accessRestrictions>
      <common:accessRestrictions xml:lang="de">Es gelten die Lizenzbedingungen wie sie auf https://www.oekobaudat.de/ genannt sind.</common:accessRestrictions>
      <common:other>
        <epd2:referenceToPublisher refObjectId="f11651e0-7877-11e3-981f-0800200c9a66" version="00.01.000" type="contact data set" uri="../contacts/f11651e0-7877-11e3-981f-0800200c9a66.xml">
          <common:shortDescription xml:lang="en">BBSR</common:shortDescription>
        </epd2:referenceToPublisher>
      </common:other>
    </publicationAndOwnership>
  </administrativeInformation>
  <exchanges>
    <exchange dataSetInternalID="103990">
      <referenceToFlowDataSet refObjectId="9eeecef3-a893-477b-a8e1-6f7480233f30" version="21.01.000" type="flow data set" uri="../flows/9eeecef3-a893-477b-a8e1-6f7480233f30.xml">
        <common:shortDescription xml:lang="en">Stainless steel drinking water pipe</common:shortDescription>
        <common:shortDescription xml:lang="de">Edelstahl-Trinkwasserrohr</common:shortDescription>
      </referenceToFlowDataSet>
      <meanAmount>1</meanAmount>
    </exchange>
    <exchange dataSetInternalID="103991">
      <referenceToFlowDataSet refObjectId="20f32be5-0398-4288-9b6d-accddd195317" version="21.01.000" type="flow data set" uri="../flows/20f32be5-0398-4288-9b6d-accddd195317.xml">
        <common:shortDescription xml:lang="en">Use of renewable primary energy as energy carrier (PERE)</common:shortDescription>
        <common:shortDescription xml:lang="de">Erneuerbare Primärenergie als Energieträger (PERE)</common:shortDescription>
      </referenceToFlowDataSet>
      <functionType>General reminder flow</functionType>
      <exchangeDirection>Input</exchangeDirection>
      <common:other>
        <epd:amount epd:module="A1-A3">10.2730926128474</epd:amount>
        <epd:referenceToUnitGroupDataSet refObjectId="93a60a57-a3c8-11da-a746-0800200c9a66" version="03.00.000" type="unit group data set" uri="../unitgroups/93a60a57-a3c8-11da-a746-0800200c9a66.xml">
          <common:shortDescription xml:lang="en">MJ</common:shortDescription>
        </epd:referenceToUnitGroupDataSet>
        <epd:amount epd:module="C1">0</epd:amount>
        <epd:amount epd:module="C2">0.00200398387495554</epd:amount>
        <epd:amount epd:module="D">-2.84380704835545</epd:amount>
      </common:other>
    </exchange>
    <exchange dataSetInternalID="103992">
      <referenceToFlowDataSet refObjectId="fb3ec0de-548d-4508-aea5-00b73bf6f702" version="21.01.000" type="flow data set" uri="../flows/fb3ec0de-548d-4508-aea5-00b73bf6f702.xml">
        <common:shortDescription xml:lang="en">Use of renewable primary energy resources used as raw materials (PERM)</common:shortDescription>
        <common:shortDescription xml:lang="de">Erneuerbare Primärenergie zur stofflichen Nutzung (PERM)</common:shortDescription>
      </referenceToFlowDataSet>
      <functionType>General reminder flow</functionType>
      <exchangeDirection>Input</exchangeDirection>
      <common:other>
        <epd:amount epd:module="A1-A3">0</epd:amount>
        <epd:referenceToUnitGroupDataSet refObjectId="93a60a57-a3c8-11da-a746-0800200c9a66" version="03.00.000" type="unit group data set" uri="../unitgroups/93a60a57-a3c8-11da-a746-0800200c9a66.xml">
          <common:shortDescription xml:lang="en">MJ</common:shortDescription>
        </epd:referenceToUnitGroupDataSet>
        <epd:amount epd:module="C1">0</epd:amount>
        <epd:amount epd:module="C2">0</epd:amount>
        <epd:amount epd:module="D">0</epd:amount>
      </common:other>
    </exchange>
    <exchange dataSetInternalID="103993">
      <referenceToFlowDataSet refObjectId="53f97275-fa8a-4cdd-9024-65936002acd0" version="21.01.000" type="flow data set" uri="../flows/53f97275-fa8a-4cdd-9024-65936002acd0.xml">
        <common:shortDescription xml:lang="en">Total use of renewable primary energy (PERT)</common:shortDescription>
        <common:shortDescription xml:lang="de">Total erneuerbare Primärenergie (PERT)</common:shortDescription>
      </referenceToFlowDataSet>
      <functionType>General reminder flow</functionType>
      <exchangeDirection>Input</exchangeDirection>
      <common:other>
        <epd:amount epd:module="A1-A3">10.2730926128474</epd:amount>
        <epd:referenceToUnitGroupDataSet refObjectId="93a60a57-a3c8-11da-a746-0800200c9a66" version="03.00.000" type="unit group data set" uri="../unitgroups/93a60a57-a3c8-11da-a746-0800200c9a66.xml">
          <common:shortDescription xml:lang="en">MJ</common:shortDescription>
        </epd:referenceToUnitGroupDataSet>
        <epd:amount epd:module="C1">0</epd:amount>
        <epd:amount epd:module="C2">0.00200398387495554</epd:amount>
        <epd:amount epd:module="D">-2.84380704835545</epd:amount>
      </common:other>
    </exchange>
    <exchange dataSetInternalID="103994">
      <referenceToFlowDataSet refObjectId="ac857178-2b45-46ec-892a-a9a4332f0372" version="21.01.000" type="flow data set" uri="../flows/ac857178-2b45-46ec-892a-a9a4332f0372.xml">
        <common:shortDescription xml:lang="en">Use of non renewable primary energy as energy carrier (PENRE)</common:shortDescription>
        <common:shortDescription xml:lang="de">Nicht-erneuerbare Primärenergie als Energieträger (PENRE)</common:shortDescription>
      </referenceToFlowDataSet>
      <functionType>General reminder flow</functionType>
      <exchangeDirection>Input</exchangeDirection>
      <common:other>
        <epd:amount epd:module="A1-A3">46.032853657649</epd:amount>
        <epd:referenceToUnitGroupDataSet refObjectId="93a60a57-a3c8-11da-a746-0800200c9a66" version="03.00.000" type="unit group data set" uri="../unitgroups/93a60a57-a3c8-11da-a746-0800200c9a66.xml">
          <common:shortDescription xml:lang="en">MJ</common:shortDescription>
        </epd:referenceToUnitGroupDataSet>
        <epd:amount epd:module="C1">0</epd:amount>
        <epd:amount epd:module="C2">0.0345287095192154</epd:amount>
        <epd:amount epd:module="D">-14.2687187280768</epd:amount>
      </common:other>
    </exchange>
    <exchange dataSetInternalID="103995">
      <referenceToFlowDataSet refObjectId="1421caa0-679d-4bf4-b282-0eb850ccae27" version="21.01.000" type="flow data set" uri="../flows/1421caa0-679d-4bf4-b282-0eb850ccae27.xml">
        <common:shortDescription xml:lang="en">Use of non renewable primary energy resources used as raw materials (PENRM)</common:shortDescription>
        <common:shortDescription xml:lang="de">Nicht-erneuerbare Primärenergie zur stofflichen Nutzung (PENRM)</common:shortDescription>
      </referenceToFlowDataSet>
      <functionType>General reminder flow</functionType>
      <exchangeDirection>Input</exchangeDirection>
      <common:other>
        <epd:amount epd:module="A1-A3">0</epd:amount>
        <epd:referenceToUnitGroupDataSet refObjectId="93a60a57-a3c8-11da-a746-0800200c9a66" version="03.00.000" type="unit group data set" uri="../unitgroups/93a60a57-a3c8-11da-a746-0800200c9a66.xml">
          <common:shortDescription xml:lang="en">MJ</common:shortDescription>
        </epd:referenceToUnitGroupDataSet>
        <epd:amount epd:module="C1">0</epd:amount>
        <epd:amount epd:module="C2">0</epd:amount>
        <epd:amount epd:module="D">0</epd:amount>
      </common:other>
    </exchange>
    <exchange dataSetInternalID="103996">
      <referenceToFlowDataSet refObjectId="06159210-646b-4c8d-8583-da9b3b95a6c1" version="21.01.000" type="flow data set" uri="../flows/06159210-646b-4c8d-8583-da9b3b95a6c1.xml">
        <common:shortDescription xml:lang="en">Total use of non renewable primary energy resource (PENRT)</common:shortDescription>
        <common:shortDescription xml:lang="de">Total nicht-erneuerbare Primärenergie (PENRT)</common:shortDescription>
      </referenceToFlowDataSet>
      <functionType>General reminder flow</functionType>
      <exchangeDirection>Input</exchangeDirection>
      <common:other>
        <epd:amount epd:module="A1-A3">46.032853657649</epd:amount>
        <epd:referenceToUnitGroupDataSet refObjectId="93a60a57-a3c8-11da-a746-0800200c9a66" version="03.00.000" type="unit group data set" uri="../unitgroups/93a60a57-a3c8-11da-a746-0800200c9a66.xml">
          <common:shortDescription xml:lang="en">MJ</common:shortDescription>
        </epd:referenceToUnitGroupDataSet>
        <epd:amount epd:module="C1">0</epd:amount>
        <epd:amount epd:module="C2">0.0345287095192154</epd:amount>
        <epd:amount epd:module="D">-14.2687187280768</epd:amount>
      </common:other>
    </exchange>
    <exchange dataSetInternalID="103997">
      <referenceToFlowDataSet refObjectId="c6a1f35f-2d09-4f54-8dfb-97e502e1ce92" version="21.01.000" type="flow data set" uri="../flows/c6a1f35f-2d09-4f54-8dfb-97e502e1ce92.xml">
        <common:shortDescription xml:lang="en">Use of secondary material (SM)</common:shortDescription>
        <common:shortDescription xml:lang="de">Einsatz von Sekundärstoffen (SM)</common:shortDescription>
      </referenceToFlowDataSet>
      <functionType>General reminder flow</functionType>
      <exchangeDirection>Input</exchangeDirection>
      <common:other>
        <epd:amount epd:module="A1-A3">0.777241498481604</epd:amount>
        <epd:referenceToUnitGroupDataSet refObjectId="93a60a57-a4c8-11da-a746-0800200c9a66" version="03.00.000" type="unit group data set" uri="../unitgroups/93a60a57-a4c8-11da-a746-0800200c9a66.xml">
          <common:shortDescription xml:lang="en">kg</common:shortDescription>
        </epd:referenceToUnitGroupDataSet>
        <epd:amount epd:module="C1">0</epd:amount>
        <epd:amount epd:module="C2">0</epd:amount>
        <epd:amount epd:module="D">0</epd:amount>
      </common:other>
    </exchange>
    <exchange dataSetInternalID="103998">
      <referenceToFlowDataSet refObjectId="64333088-a55f-4aa2-9a31-c10b07816787" version="21.01.000" type="flow data set" uri="../flows/64333088-a55f-4aa2-9a31-c10b07816787.xml">
        <common:shortDescription xml:lang="en">Use of renewable secondary fuels (SF)</common:shortDescription>
        <common:shortDescription xml:lang="de">Erneuerbare Sekundärbrennstoffe (SF)</common:shortDescription>
      </referenceToFlowDataSet>
      <functionType>General reminder flow</functionType>
      <exchangeDirection>Input</exchangeDirection>
      <common:other>
        <epd:amount epd:module="A1-A3">0</epd:amount>
        <epd:referenceToUnitGroupDataSet refObjectId="93a60a57-a3c8-11da-a746-0800200c9a66" version="03.00.000" type="unit group data set" uri="../unitgroups/93a60a57-a3c8-11da-a746-0800200c9a66.xml">
          <common:shortDescription xml:lang="en">MJ</common:shortDescription>
        </epd:referenceToUnitGroupDataSet>
        <epd:amount epd:module="C1">0</epd:amount>
        <epd:amount epd:module="C2">0</epd:amount>
        <epd:amount epd:module="D">0</epd:amount>
      </common:other>
    </exchange>
    <exchange dataSetInternalID="103999">
      <referenceToFlowDataSet refObjectId="89def144-d39a-4287-b86f-efde453ddcb2" version="21.01.000" type="flow data set" uri="../flows/89def144-d39a-4287-b86f-efde453ddcb2.xml">
        <common:shortDescription xml:lang="en">Use of non renewable secondary fuels (NRSF)</common:shortDescription>
        <common:shortDescription xml:lang="de">Nicht erneuerbare Sekundärbrennstoffe (NRSF)</common:shortDescription>
      </referenceToFlowDataSet>
      <functionType>General reminder flow</functionType>
      <exchangeDirection>Input</exchangeDirection>
      <common:other>
        <epd:amount epd:module="A1-A3">0</epd:amount>
        <epd:referenceToUnitGroupDataSet refObjectId="93a60a57-a3c8-11da-a746-0800200c9a66" version="03.00.000" type="unit group data set" uri="../unitgroups/93a60a57-a3c8-11da-a746-0800200c9a66.xml">
          <common:shortDescription xml:lang="en">MJ</common:shortDescription>
        </epd:referenceToUnitGroupDataSet>
        <epd:amount epd:module="C1">0</epd:amount>
        <epd:amount epd:module="C2">0</epd:amount>
        <epd:amount epd:module="D">0</epd:amount>
      </common:other>
    </exchange>
    <exchange dataSetInternalID="104000">
      <referenceToFlowDataSet refObjectId="3cf952c8-f3a4-461d-8c96-96456ca62246" version="21.01.000" type="flow data set" uri="../flows/3cf952c8-f3a4-461d-8c96-96456ca62246.xml">
        <common:shortDescription xml:lang="en">Net use of fresh water (FW)</common:shortDescription>
        <common:shortDescription xml:lang="de">Nettoeinsatz von Süßwasserressourcen (FW)</common:shortDescription>
      </referenceToFlowDataSet>
      <functionType>General reminder flow</functionType>
      <exchangeDirection>Input</exchangeDirection>
      <common:other>
        <epd:amount epd:module="A1-A3">0.0215345073567934</epd:amount>
        <epd:referenceToUnitGroupDataSet refObjectId="93a60a57-a3c8-12da-a746-0800200c9a66" version="03.00.000" type="unit group data set" uri="../unitgroups/93a60a57-a3c8-12da-a746-0800200c9a66.xml">
          <common:shortDescription xml:lang="en">m3</common:shortDescription>
        </epd:referenceToUnitGroupDataSet>
        <epd:amount epd:module="C1">0</epd:amount>
        <epd:amount epd:module="C2">1.78104137243537E-6</epd:amount>
        <epd:amount epd:module="D">-0.0182028165387471</epd:amount>
      </common:other>
    </exchange>
    <exchange dataSetInternalID="104001">
      <referenceToFlowDataSet refObjectId="430f9e0f-59b2-46a0-8e0d-55e0e84948fc" version="21.01.000" type="flow data set" uri="../flows/430f9e0f-59b2-46a0-8e0d-55e0e84948fc.xml">
        <common:shortDescription xml:lang="en">Hazardous waste disposed (HWD)</common:shortDescription>
        <common:shortDescription xml:lang="de">Gefährlicher Abfall zur Deponie (HWD)</common:shortDescription>
      </referenceToFlowDataSet>
      <functionType>General reminder flow</functionType>
      <exchangeDirection>Output</exchangeDirection>
      <common:other>
        <epd:amount epd:module="A1-A3">7.07308218589233E-9</epd:amount>
        <epd:referenceToUnitGroupDataSet refObjectId="93a60a57-a4c8-11da-a746-0800200c9a66" version="03.00.000" type="unit group data set" uri="../unitgroups/93a60a57-a4c8-11da-a746-0800200c9a66.xml">
          <common:shortDescription xml:lang="en">kg</common:shortDescription>
        </epd:referenceToUnitGroupDataSet>
        <epd:amount epd:module="C1">0</epd:amount>
        <epd:amount epd:module="C2">1.44318834099877E-12</epd:amount>
        <epd:amount epd:module="D">-1.11558454198739E-9</epd:amount>
      </common:other>
    </exchange>
    <exchange dataSetInternalID="104002">
      <referenceToFlowDataSet refObjectId="b29ef66b-e286-4afa-949f-62f1a7b4d7fa" version="21.01.000" type="flow data set" uri="../flows/b29ef66b-e286-4afa-949f-62f1a7b4d7fa.xml">
        <common:shortDescription xml:lang="en">Non harzardous waste disposed (NHWD)</common:shortDescription>
        <common:shortDescription xml:lang="de">Entsorgter nicht gefährlicher Abfall (NHWD)</common:shortDescription>
      </referenceToFlowDataSet>
      <functionType>General reminder flow</functionType>
      <exchangeDirection>Output</exchangeDirection>
      <common:other>
        <epd:amount epd:module="A1-A3">0.49001507030949</epd:amount>
        <epd:referenceToUnitGroupDataSet refObjectId="93a60a57-a4c8-11da-a746-0800200c9a66" version="03.00.000" type="unit group data set" uri="../unitgroups/93a60a57-a4c8-11da-a746-0800200c9a66.xml">
          <common:shortDescription xml:lang="en">kg</common:shortDescription>
        </epd:referenceToUnitGroupDataSet>
        <epd:amount epd:module="C1">0</epd:amount>
        <epd:amount epd:module="C2">5.57372278297782E-6</epd:amount>
        <epd:amount epd:module="D">-0.102051296732741</epd:amount>
      </common:other>
    </exchange>
    <exchange dataSetInternalID="104003">
      <referenceToFlowDataSet refObjectId="3449546e-52ad-4b39-b809-9fb77cea8ff6" version="21.01.000" type="flow data set" uri="../flows/3449546e-52ad-4b39-b809-9fb77cea8ff6.xml">
        <common:shortDescription xml:lang="en">Radioactive waste disposed (RWD)</common:shortDescription>
        <common:shortDescription xml:lang="de">Entsorgter radioaktiver Abfall (RWD)</common:shortDescription>
      </referenceToFlowDataSet>
      <functionType>General reminder flow</functionType>
      <exchangeDirection>Output</exchangeDirection>
      <common:other>
        <epd:amount epd:module="A1-A3">0.00106916550718061</epd:amount>
        <epd:referenceToUnitGroupDataSet refObjectId="93a60a57-a4c8-11da-a746-0800200c9a66" version="03.00.000" type="unit group data set" uri="../unitgroups/93a60a57-a4c8-11da-a746-0800200c9a66.xml">
          <common:shortDescription xml:lang="en">kg</common:shortDescription>
        </epd:referenceToUnitGroupDataSet>
        <epd:amount epd:module="C1">0</epd:amount>
        <epd:amount epd:module="C2">3.31348075365879E-8</epd:amount>
        <epd:amount epd:module="D">-7.06021703788859E-5</epd:amount>
      </common:other>
    </exchange>
    <exchange dataSetInternalID="104004">
      <referenceToFlowDataSet refObjectId="a2b32f97-3fc7-4af2-b209-525bc6426f33" version="21.01.000" type="flow data set" uri="../flows/a2b32f97-3fc7-4af2-b209-525bc6426f33.xml">
        <common:shortDescription xml:lang="en">Components for re-use (CRU)</common:shortDescription>
        <common:shortDescription xml:lang="de">Komponenten für die Wiederverwendung (CRU)</common:shortDescription>
      </referenceToFlowDataSet>
      <functionType>General reminder flow</functionType>
      <exchangeDirection>Output</exchangeDirection>
      <common:other>
        <epd:amount epd:module="A1-A3">0</epd:amount>
        <epd:referenceToUnitGroupDataSet refObjectId="93a60a57-a4c8-11da-a746-0800200c9a66" version="03.00.000" type="unit group data set" uri="../unitgroups/93a60a57-a4c8-11da-a746-0800200c9a66.xml">
          <common:shortDescription xml:lang="en">kg</common:shortDescription>
        </epd:referenceToUnitGroupDataSet>
        <epd:amount epd:module="C1">0</epd:amount>
        <epd:amount epd:module="C2">0</epd:amount>
        <epd:amount epd:module="D">0</epd:amount>
      </common:other>
    </exchange>
    <exchange dataSetInternalID="104005">
      <referenceToFlowDataSet refObjectId="d7fe48a5-4103-49c8-9aae-b0b5dfdbd6ae" version="21.01.000" type="flow data set" uri="../flows/d7fe48a5-4103-49c8-9aae-b0b5dfdbd6ae.xml">
        <common:shortDescription xml:lang="en">Materials for recycling  (MFR)</common:shortDescription>
        <common:shortDescription xml:lang="de">Stoffe zum Recycling (MFR)</common:shortDescription>
      </referenceToFlowDataSet>
      <functionType>General reminder flow</functionType>
      <exchangeDirection>Output</exchangeDirection>
      <common:other>
        <epd:amount epd:module="A1-A3">0</epd:amount>
        <epd:referenceToUnitGroupDataSet refObjectId="93a60a57-a4c8-11da-a746-0800200c9a66" version="03.00.000" type="unit group data set" uri="../unitgroups/93a60a57-a4c8-11da-a746-0800200c9a66.xml">
          <common:shortDescription xml:lang="en">kg</common:shortDescription>
        </epd:referenceToUnitGroupDataSet>
        <epd:amount epd:module="C1">1</epd:amount>
        <epd:amount epd:module="C2">0</epd:amount>
        <epd:amount epd:module="D">0</epd:amount>
      </common:other>
    </exchange>
    <exchange dataSetInternalID="104006">
      <referenceToFlowDataSet refObjectId="59a9181c-3aaf-46ee-8b13-2b3723b6e447" version="21.01.000" type="flow data set" uri="../flows/59a9181c-3aaf-46ee-8b13-2b3723b6e447.xml">
        <common:shortDescription xml:lang="en">Materials for energy recovery (MER)</common:shortDescription>
        <common:shortDescription xml:lang="de">Stoffe für die Energierückgewinnung (MER)</common:shortDescription>
      </referenceToFlowDataSet>
      <functionType>General reminder flow</functionType>
      <exchangeDirection>Output</exchangeDirection>
      <common:other>
        <epd:amount epd:module="A1-A3">0</epd:amount>
        <epd:referenceToUnitGroupDataSet refObjectId="93a60a57-a4c8-11da-a746-0800200c9a66" version="03.00.000" type="unit group data set" uri="../unitgroups/93a60a57-a4c8-11da-a746-0800200c9a66.xml">
          <common:shortDescription xml:lang="en">kg</common:shortDescription>
        </epd:referenceToUnitGroupDataSet>
        <epd:amount epd:module="C1">0</epd:amount>
        <epd:amount epd:module="C2">0</epd:amount>
        <epd:amount epd:module="D">0</epd:amount>
      </common:other>
    </exchange>
    <exchange dataSetInternalID="104007">
      <referenceToFlowDataSet refObjectId="4da0c987-2b76-40d6-9e9e-82a017aaaf29" version="21.01.000" type="flow data set" uri="../flows/4da0c987-2b76-40d6-9e9e-82a017aaaf29.xml">
        <common:shortDescription xml:lang="en">Exported electrical energy (EEE)</common:shortDescription>
        <common:shortDescription xml:lang="de">Exportierte elektrische Energie (EEE)</common:shortDescription>
      </referenceToFlowDataSet>
      <functionType>General reminder flow</functionType>
      <exchangeDirection>Output</exchangeDirection>
      <common:other>
        <epd:amount epd:module="A1-A3">0</epd:amount>
        <epd:referenceToUnitGroupDataSet refObjectId="93a60a57-a3c8-11da-a746-0800200c9a66" version="03.00.000" type="unit group data set" uri="../unitgroups/93a60a57-a3c8-11da-a746-0800200c9a66.xml">
          <common:shortDescription xml:lang="en">MJ</common:shortDescription>
        </epd:referenceToUnitGroupDataSet>
        <epd:amount epd:module="C1">0</epd:amount>
        <epd:amount epd:module="C2">0</epd:amount>
        <epd:amount epd:module="D">0</epd:amount>
      </common:other>
    </exchange>
    <exchange dataSetInternalID="104008">
      <referenceToFlowDataSet refObjectId="98daf38a-7a79-46d3-9a37-2b7bd0955810" version="21.01.000" type="flow data set" uri="../flows/98daf38a-7a79-46d3-9a37-2b7bd0955810.xml">
        <common:shortDescription xml:lang="en">Exported thermal energy (EET)</common:shortDescription>
        <common:shortDescription xml:lang="de">Exportierte thermische Energie (EET)</common:shortDescription>
      </referenceToFlowDataSet>
      <functionType>General reminder flow</functionType>
      <exchangeDirection>Output</exchangeDirection>
      <common:other>
        <epd:amount epd:module="A1-A3">0</epd:amount>
        <epd:referenceToUnitGroupDataSet refObjectId="93a60a57-a3c8-11da-a746-0800200c9a66" version="03.00.000" type="unit group data set" uri="../unitgroups/93a60a57-a3c8-11da-a746-0800200c9a66.xml">
          <common:shortDescription xml:lang="en">MJ</common:shortDescription>
        </epd:referenceToUnitGroupDataSet>
        <epd:amount epd:module="C1">0</epd:amount>
        <epd:amount epd:module="C2">0</epd:amount>
        <epd:amount epd:module="D">0</epd:amount>
      </common:other>
    </exchange>
  </exchanges>
  <LCIAResults>
    <LCIAResult>
      <referenceToLCIAMethodDataSet refObjectId="6a37f984-a4b3-458a-a20a-64418c145fa2" version="21.01.000" type="LCIA method data set" uri="../lciamethods/6a37f984-a4b3-458a-a20a-64418c145fa2.xml">
        <common:shortDescription xml:lang="en">Global Warming Potential - total (GWP-total)</common:shortDescription>
        <common:shortDescription xml:lang="de">Globales Erwärmungspotenzial - total (GWP-total)</common:shortDescription>
      </referenceToLCIAMethodDataSet>
      <common:other>
        <epd:amount epd:module="A1-A3">3.82742795449012</epd:amount>
        <epd:amount epd:module="C1">0</epd:amount>
        <epd:amount epd:module="C2">0.00262282845734216</epd:amount>
        <epd:amount epd:module="D">-1.2394126762896</epd:amount>
        <epd:referenceToUnitGroupDataSet refObjectId="1ebf3012-d0db-4de2-aefd-ef30cedb0be1" version="25.00.000" type="unit group data set" uri="../unitgroups/1ebf3012-d0db-4de2-aefd-ef30cedb0be1.xml">
          <common:shortDescription xml:lang="en">kg CO2 eq.</common:shortDescription>
        </epd:referenceToUnitGroupDataSet>
      </common:other>
    </LCIAResult>
    <LCIAResult>
      <referenceToLCIAMethodDataSet refObjectId="5f635281-343e-44fb-83df-1971b155e6b6" version="21.01.000" type="LCIA method data set" uri="../lciamethods/5f635281-343e-44fb-83df-1971b155e6b6.xml">
        <common:shortDescription xml:lang="en">Global Warming Potential - fossil fuels (GWP-fossil)</common:shortDescription>
        <common:shortDescription xml:lang="de">Globales Erwärmungspotenzial - fossil (GWP-fossil)</common:shortDescription>
      </referenceToLCIAMethodDataSet>
      <common:other>
        <epd:amount epd:module="A1-A3">3.81485419254218</epd:amount>
        <epd:amount epd:module="C1">0</epd:amount>
        <epd:amount epd:module="C2">0.00260492178434586</epd:amount>
        <epd:amount epd:module="D">-1.24319982464104</epd:amount>
        <epd:referenceToUnitGroupDataSet refObjectId="1ebf3012-d0db-4de2-aefd-ef30cedb0be1" version="25.00.000" type="unit group data set" uri="../unitgroups/1ebf3012-d0db-4de2-aefd-ef30cedb0be1.xml">
          <common:shortDescription xml:lang="en">kg CO2 eq.</common:shortDescription>
        </epd:referenceToUnitGroupDataSet>
      </common:other>
    </LCIAResult>
    <LCIAResult>
      <referenceToLCIAMethodDataSet refObjectId="2356e1ab-0185-4db5-86e5-16de51c7485c" version="21.01.000" type="LCIA method data set" uri="../lciamethods/2356e1ab-0185-4db5-86e5-16de51c7485c.xml">
        <common:shortDescription xml:lang="en">Global Warming Potential - biogenic (GWP-biogenic)</common:shortDescription>
        <common:shortDescription xml:lang="de">Globales Erwärmungspotenzial - biogen (GWP-biogenic)</common:shortDescription>
      </referenceToLCIAMethodDataSet>
      <common:other>
        <epd:amount epd:module="A1-A3">0.00804028648364694</epd:amount>
        <epd:amount epd:module="C1">0</epd:amount>
        <epd:amount epd:module="C2">1.17715755154072E-6</epd:amount>
        <epd:amount epd:module="D">0.00604567652079358</epd:amount>
        <epd:referenceToUnitGroupDataSet refObjectId="1ebf3012-d0db-4de2-aefd-ef30cedb0be1" version="25.00.000" type="unit group data set" uri="../unitgroups/1ebf3012-d0db-4de2-aefd-ef30cedb0be1.xml">
          <common:shortDescription xml:lang="en">kg CO2 eq.</common:shortDescription>
        </epd:referenceToUnitGroupDataSet>
      </common:other>
    </LCIAResult>
    <LCIAResult>
      <referenceToLCIAMethodDataSet refObjectId="4331bbdb-978a-490d-8707-eeb047f01a55" version="21.01.000" type="LCIA method data set" uri="../lciamethods/4331bbdb-978a-490d-8707-eeb047f01a55.xml">
        <common:shortDescription xml:lang="en">Global Warming Potential - land use and land use change (GWP-luluc)</common:shortDescription>
        <common:shortDescription xml:lang="de">Globales Erwärmungspotenzial - luluc (GWP-luluc)</common:shortDescription>
      </referenceToLCIAMethodDataSet>
      <common:other>
        <epd:amount epd:module="A1-A3">0.00453347546430275</epd:amount>
        <epd:amount epd:module="C1">0</epd:amount>
        <epd:amount epd:module="C2">1.67295154447651E-5</epd:amount>
        <epd:amount epd:module="D">-0.00225852816935362</epd:amount>
        <epd:referenceToUnitGroupDataSet refObjectId="1ebf3012-d0db-4de2-aefd-ef30cedb0be1" version="25.00.000" type="unit group data set" uri="../unitgroups/1ebf3012-d0db-4de2-aefd-ef30cedb0be1.xml">
          <common:shortDescription xml:lang="en">kg CO2 eq.</common:shortDescription>
        </epd:referenceToUnitGroupDataSet>
      </common:other>
    </LCIAResult>
    <LCIAResult>
      <referenceToLCIAMethodDataSet refObjectId="b5c629d6-def3-11e6-bf01-fe55135034f3" version="21.01.000" type="LCIA method data set" uri="../lciamethods/b5c629d6-def3-11e6-bf01-fe55135034f3.xml">
        <common:shortDescription xml:lang="en">Depletion potenzial of the stratospheric ozone layer (ODP)</common:shortDescription>
        <common:shortDescription xml:lang="de">Abbaupotenzial der stratosphärischen Ozonschicht (ODP)</common:shortDescription>
      </referenceToLCIAMethodDataSet>
      <common:other>
        <epd:amount epd:module="A1-A3">3.307254296018E-14</epd:amount>
        <epd:amount epd:module="C1">0</epd:amount>
        <epd:amount epd:module="C2">6.66531605927454E-19</epd:amount>
        <epd:amount epd:module="D">-2.26493157306373E-15</epd:amount>
        <epd:referenceToUnitGroupDataSet refObjectId="d9e957c9-7309-4474-bf3a-7777df6c4e5b" version="25.00.000" type="unit group data set" uri="../unitgroups/d9e957c9-7309-4474-bf3a-7777df6c4e5b.xml">
          <common:shortDescription xml:lang="en">kg CFC-11 eq.</common:shortDescription>
        </epd:referenceToUnitGroupDataSet>
      </common:other>
    </LCIAResult>
    <LCIAResult>
      <referenceToLCIAMethodDataSet refObjectId="b5c611c6-def3-11e6-bf01-fe55135034f3" version="21.01.000" type="LCIA method data set" uri="../lciamethods/b5c611c6-def3-11e6-bf01-fe55135034f3.xml">
        <common:shortDescription xml:lang="en">Acidifcation potential, Accumulated Exceedance (AP)</common:shortDescription>
        <common:shortDescription xml:lang="de">Versauerungspotenzial, kumulierte Überschreitung (AP)</common:shortDescription>
      </referenceToLCIAMethodDataSet>
      <common:other>
        <epd:amount epd:module="A1-A3">0.024641641289989</epd:amount>
        <epd:amount epd:module="C1">0</epd:amount>
        <epd:amount epd:module="C2">7.38555004738285E-6</epd:amount>
        <epd:amount epd:module="D">-0.00529309691045134</epd:amount>
        <epd:referenceToUnitGroupDataSet refObjectId="42e089ac-92bf-4bf2-8ca1-5fc40d18f2ed" version="00.01.000" type="unit group data set" uri="../unitgroups/42e089ac-92bf-4bf2-8ca1-5fc40d18f2ed.xml">
          <common:shortDescription xml:lang="en">Mole of H+ eq.</common:shortDescription>
        </epd:referenceToUnitGroupDataSet>
      </common:other>
    </LCIAResult>
    <LCIAResult>
      <referenceToLCIAMethodDataSet refObjectId="b53ec18f-7377-4ad3-86eb-cc3f4f276b2b" version="21.01.000" type="LCIA method data set" uri="../lciamethods/b53ec18f-7377-4ad3-86eb-cc3f4f276b2b.xml">
        <common:shortDescription xml:lang="en">Eutrophication potential - freshwater (EP-freshwater)</common:shortDescription>
        <common:shortDescription xml:lang="de">Eutrophierungspotenzial - Süßwasser (EP-freshwater)</common:shortDescription>
      </referenceToLCIAMethodDataSet>
      <common:other>
        <epd:amount epd:module="A1-A3">6.17247388451685E-6</epd:amount>
        <epd:amount epd:module="C1">0</epd:amount>
        <epd:amount epd:module="C2">5.35732239914499E-9</epd:amount>
        <epd:amount epd:module="D">-1.01833010885684E-6</epd:amount>
        <epd:referenceToUnitGroupDataSet refObjectId="0429039d-a61d-4590-ba67-aa4a20a810a1" version="25.00.000" type="unit group data set" uri="../unitgroups/0429039d-a61d-4590-ba67-aa4a20a810a1.xml">
          <common:shortDescription xml:lang="en">kg P eq.</common:shortDescription>
        </epd:referenceToUnitGroupDataSet>
      </common:other>
    </LCIAResult>
    <LCIAResult>
      <referenceToLCIAMethodDataSet refObjectId="b5c619fa-def3-11e6-bf01-fe55135034f3" version="21.01.000" type="LCIA method data set" uri="../lciamethods/b5c619fa-def3-11e6-bf01-fe55135034f3.xml">
        <common:shortDescription xml:lang="en">Eutrophication potential - marine (EP-marine)</common:shortDescription>
        <common:shortDescription xml:lang="de">Eutrophierungspotenzial - Salzwasser (EP-marine)</common:shortDescription>
      </referenceToLCIAMethodDataSet>
      <common:other>
        <epd:amount epd:module="A1-A3">0.00268218805207641</epd:amount>
        <epd:amount epd:module="C1">0</epd:amount>
        <epd:amount epd:module="C2">3.40236678610378E-6</epd:amount>
        <epd:amount epd:module="D">-0.000813353720947192</epd:amount>
        <epd:referenceToUnitGroupDataSet refObjectId="d05bb823-ecdf-4686-8c40-bf1d9257859f" version="00.00.003" type="unit group data set" uri="../unitgroups/d05bb823-ecdf-4686-8c40-bf1d9257859f.xml">
          <common:shortDescription xml:lang="en">kg N eq.</common:shortDescription>
        </epd:referenceToUnitGroupDataSet>
      </common:other>
    </LCIAResult>
    <LCIAResult>
      <referenceToLCIAMethodDataSet refObjectId="b5c614d2-def3-11e6-bf01-fe55135034f3" version="21.01.000" type="LCIA method data set" uri="../lciamethods/b5c614d2-def3-11e6-bf01-fe55135034f3.xml">
        <common:shortDescription xml:lang="en">Eutrophication potential - terrestrial (EP-terrestrial)</common:shortDescription>
        <common:shortDescription xml:lang="de">Eutrophierungspotenzial - Land (EP-terrestrial)</common:shortDescription>
      </referenceToLCIAMethodDataSet>
      <common:other>
        <epd:amount epd:module="A1-A3">0.0294770443178331</epd:amount>
        <epd:amount epd:module="C1">0</epd:amount>
        <epd:amount epd:module="C2">3.80662980083467E-5</epd:amount>
        <epd:amount epd:module="D">-0.00881246872735845</epd:amount>
        <epd:referenceToUnitGroupDataSet refObjectId="71b4d617-0ec9-4d3f-b65e-e438940c2401" version="00.00.003" type="unit group data set" uri="../unitgroups/71b4d617-0ec9-4d3f-b65e-e438940c2401.xml">
          <common:shortDescription xml:lang="en">Mole of N eq.</common:shortDescription>
        </epd:referenceToUnitGroupDataSet>
      </common:other>
    </LCIAResult>
    <LCIAResult>
      <referenceToLCIAMethodDataSet refObjectId="b5c610fe-def3-11e6-bf01-fe55135034f3" version="21.01.000" type="LCIA method data set" uri="../lciamethods/b5c610fe-def3-11e6-bf01-fe55135034f3.xml">
        <common:shortDescription xml:lang="en">Photochemical Ozone Creation Potential  (POCP)</common:shortDescription>
        <common:shortDescription xml:lang="de">Bildungspotenzial für troposphärisches Ozon (POCP)</common:shortDescription>
      </referenceToLCIAMethodDataSet>
      <common:other>
        <epd:amount epd:module="A1-A3">0.0082754638574091</epd:amount>
        <epd:amount epd:module="C1">0</epd:amount>
        <epd:amount epd:module="C2">6.63469529398323E-6</epd:amount>
        <epd:amount epd:module="D">-0.00244367542503009</epd:amount>
        <epd:referenceToUnitGroupDataSet refObjectId="d27c25f8-fbc1-44c6-b47b-4adbae4199c6" version="00.00.003" type="unit group data set" uri="../unitgroups/d27c25f8-fbc1-44c6-b47b-4adbae4199c6.xml">
          <common:shortDescription xml:lang="en">kg NMVOC eq.</common:shortDescription>
        </epd:referenceToUnitGroupDataSet>
      </common:other>
    </LCIAResult>
    <LCIAResult>
      <referenceToLCIAMethodDataSet refObjectId="b2ad6494-c78d-11e6-9d9d-cec0c932ce01" version="21.01.000" type="LCIA method data set" uri="../lciamethods/b2ad6494-c78d-11e6-9d9d-cec0c932ce01.xml">
        <common:shortDescription xml:lang="en">Abiotic depletion potential - non-fossil resources (ADPE)</common:shortDescription>
        <common:shortDescription xml:lang="de">Potenzial für die Verknappung abiotischer Ressourcen  nicht fossile Ressourcen (ADPE)</common:shortDescription>
      </referenceToLCIAMethodDataSet>
      <common:other>
        <epd:amount epd:module="A1-A3">0.000151952165199665</epd:amount>
        <epd:amount epd:module="C1">0</epd:amount>
        <epd:amount epd:module="C2">2.2659193367491E-10</epd:amount>
        <epd:amount epd:module="D">-3.56748809293571E-5</epd:amount>
        <epd:referenceToUnitGroupDataSet refObjectId="54ccd2d9-a32a-4fc2-923d-f2c8c93e89d4" version="25.00.000" type="unit group data set" uri="../unitgroups/54ccd2d9-a32a-4fc2-923d-f2c8c93e89d4.xml">
          <common:shortDescription xml:lang="en">kg Sb eq.</common:shortDescription>
        </epd:referenceToUnitGroupDataSet>
      </common:other>
    </LCIAResult>
    <LCIAResult>
      <referenceToLCIAMethodDataSet refObjectId="b2ad6110-c78d-11e6-9d9d-cec0c932ce01" version="21.01.000" type="LCIA method data set" uri="../lciamethods/b2ad6110-c78d-11e6-9d9d-cec0c932ce01.xml">
        <common:shortDescription xml:lang="en">Abiotic depletion potential - fossil resources (ADPF)</common:shortDescription>
        <common:shortDescription xml:lang="de">Potenzial für die Verknappung abiotischer Ressourcen  fossile Brennstoffe (ADPF)</common:shortDescription>
      </referenceToLCIAMethodDataSet>
      <common:other>
        <epd:amount epd:module="A1-A3">46.0161202075784</epd:amount>
        <epd:amount epd:module="C1">0</epd:amount>
        <epd:amount epd:module="C2">0.0345272685104228</epd:amount>
        <epd:amount epd:module="D">-14.2469868411299</epd:amount>
        <epd:referenceToUnitGroupDataSet refObjectId="93a60a57-a3c8-11da-a746-0800200c9a66" version="02.00.000" type="unit group data set" uri="../unitgroups/93a60a57-a3c8-11da-a746-0800200c9a66.xml">
          <common:shortDescription xml:lang="en">MJ</common:shortDescription>
        </epd:referenceToUnitGroupDataSet>
      </common:other>
    </LCIAResult>
    <LCIAResult>
      <referenceToLCIAMethodDataSet refObjectId="b2ad66ce-c78d-11e6-9d9d-cec0c932ce01" version="21.01.000" type="LCIA method data set" uri="../lciamethods/b2ad66ce-c78d-11e6-9d9d-cec0c932ce01.xml">
        <common:shortDescription xml:lang="en">Water (user) deprivation potential (WDP)</common:shortDescription>
        <common:shortDescription xml:lang="de">Wasser-Entzugspotenzial (Benutzer) (WDP)</common:shortDescription>
      </referenceToLCIAMethodDataSet>
      <common:other>
        <epd:amount epd:module="A1-A3">0.665988521765474</epd:amount>
        <epd:amount epd:module="C1">0</epd:amount>
        <epd:amount epd:module="C2">1.01262247055061E-5</epd:amount>
        <epd:amount epd:module="D">-0.47057556845019</epd:amount>
        <epd:referenceToUnitGroupDataSet refObjectId="6ae2df01-888e-46c8-b17d-49fa3869b476" version="00.00.003" type="unit group data set" uri="../unitgroups/6ae2df01-888e-46c8-b17d-49fa3869b476.xml">
          <common:shortDescription xml:lang="en">m³ world equiv.</common:shortDescription>
        </epd:referenceToUnitGroupDataSet>
      </common:other>
    </LCIAResult>
  </LCIAResults>
</processDataSet>
