<?xml version="1.0" encoding="utf-8"?>
<processDataSet xmlns:epd="http://www.iai.kit.edu/EPD/2013" xmlns:epd2="http://www.indata.network/EPD/2019" xmlns:common="http://lca.jrc.it/ILCD/Common" xsi:schemaLocation="http://lca.jrc.it/ILCD/Process ../../schemas/EPD_DataSet.xsd" epd2:epd-version="1.2" version="1.1" locations="../ILCDLocations.xml" xmlns:xsi="http://www.w3.org/2001/XMLSchema-instance" xmlns="http://lca.jrc.it/ILCD/Process">
<processInformation>
<dataSetInformation>
<common:UUID>db56f54d-1f0e-47a4-9d64-91767b016c91</common:UUID>
<name>
<baseName xml:lang="en">Galvanized steel suspended ceiling panel</baseName>
<functionalUnitFlowProperties xml:lang="en" />
</name>
<classificationInformation>
<common:classification name="OEKOBAU.DAT">
<common:class level="0" classId="1">Mineralische Baustoffe</common:class>
<common:class level="1" classId="1.3">Steine und Elemente</common:class>
<common:class level="2" classId="1.3.15">Deckenplatten</common:class>
</common:classification>
<common:classification name="IBUCategories">
<common:class level="0">02 Building products</common:class>
<common:class level="1">Internal and external wall and ceiling finishes</common:class>
<common:class level="2">Metal ceilings</common:class>
</common:classification>
</classificationInformation>
<common:generalComment xml:lang="en">Steel ceiling systems are manufactured from folded, roll-formed and partially punched steel as complete ceiling kits or as individual components. The ceiling kit comprises the membrane component, e.g. tile panels or plank panel ceilings, as well as substructure for suspending the metal ceiling. The substructure is usually made of steel. It can have various suspension heights and its design is governed by the form, functional requirements and weight of the membrane components. For the use and application of the product the respective national provisions at the place of use apply, in Germany for example the building codes of the federal states and the corresponding national specifications. The ceiling systems are manufactured by considering /TS EN 13964/ and /TS EN ISO 9224/.</common:generalComment>
</dataSetInformation>
<quantitativeReference>
<referenceToReferenceFlow>0</referenceToReferenceFlow>
</quantitativeReference>
<time>
<common:referenceYear>2019</common:referenceYear>
<common:dataSetValidUntil>2024</common:dataSetValidUntil>
<common:other>
<epd2:publicationDateOfEPD>2019-07-25</epd2:publicationDateOfEPD>
</common:other>
</time>
<geography>
<locationOfOperationSupplyOrProduction location="TR" />
</geography>
<technology>
<technologyDescriptionAndIncludedProcesses xml:lang="en">The system components for metal ceilings are manufactured in a continuous manufacturing process. The sheet of steel comes mainly in coils, perforated (optional), punched (aligned as an option), bended, welded (optional) and cut to size. Where the membrane components do not comprise pre-coated material, they are usually powder or spray-painted after the cleaning process. A layer of acoustic tissue can then be applied to the back using a heating process. Adding heat activates a hot-melt adhesive embedded in the tissue, which causes it to adhere to the back of the panel. Punching and perforation waste is gathered, collected by local disposal companies and redirected to the recycling facilities. All production steps are carried out in accordance with the requirements and test guidelines outlined in /TS EN 13964/. Galvanized steel ceiling panel production in the factory is included the stages supply of raw material from stock, cutting, bending, dying, packaging and stockpiling in sequence. 
Technical data: 
Butem Metal ceiling system made of steel is manufactured under the warranty of the /ISO 9001/ Quality Management System to comply with the product requirement specifications. The manufacturing system has /OHSAS 18001/ Occupational Health and Safety and /ISO 14001/ Environmental Management systems.  Depending on the project requirements; Butem Metal can supply additional acoustic enhancement materials, which provides sound absorption value as follows: The weighted sound absorption coefficient (αw) value: aw= 0.35 in accordance with /TS EN ISO 11654/. 
Declared unit: 
The declared unit is 1 m2 of 1 galvanized steel ceiling panel with the average thickness of 0.5 mm. The area weights for each product in steel product group varies depend on sheet thicknesses; accordingly the average thickness is accepted as 0.5 mm. All declared products are produced in the same production procedure with some minor differences like using several membrane elements for certain products or geometrical shape of the final product.</technologyDescriptionAndIncludedProcesses>
<technologicalApplicability xml:lang="en">The metal ceiling systems made of steel outlined in this LCA study are used in interior and exterior designs as rectangular panels, strip panel ceilings, square tiles, chilled ceilings, expanded metal ceilings, ceiling grids, special geometrical design panels or canopy ceilings, all functioning as cladding of the interior ceiling. It is also a low VOC emitted interior product in compliance with /CDPH - CA Section 01350 v1.2/. Metal ceiling systems made of steel are produced in accordance with customer&apos;s requirements. In addition, metal ceiling panels can provide sound absorption.</technologicalApplicability>
</technology>
</processInformation>
<modellingAndValidation>
<LCIMethodAndAllocation>
<typeOfDataSet>EPD</typeOfDataSet>
<referenceToLCAMethodDetails type="source data set" refObjectId="22d3989b-bcdc-4f7f-a4d7-12a90dd40c4a">
<common:shortDescription xml:lang="en">Metal ceilings.pdf</common:shortDescription>
</referenceToLCAMethodDetails>
<common:other>
<epd:subType xmlns="http://www.iai.kit.edu/EPD/2013">average dataset</epd:subType>
</common:other>
</LCIMethodAndAllocation>
<dataSourcesTreatmentAndRepresentativeness>
<referenceToDataSource type="source data set" refObjectId="28d74cc0-db8b-4d7e-bc44-5f6d56ce0c4a">
<common:shortDescription xml:lang="en">GaBi Database (all versions)</common:shortDescription>
</referenceToDataSource>
<referenceToDataSource type="source data set" refObjectId="8cb50bdc-0299-4a4c-9a4e-4c62917018c7">
<common:shortDescription xml:lang="en">GaBi database SP29 2016</common:shortDescription>
</referenceToDataSource>
<useAdviceForDataSet xml:lang="en">Scope: 
Within this study a life cycle analysis according to /ISO14040/44/ is performed for galvanized suspended ceiling panel manufactured by Butem Metal at the production plant in Istanbul, Turkey. The EPD for Butem Metal for galvanized suspended ceiling panel is an average EPD which represents the life cycle analysis of the product group. The area weights for each product in steel product group varies depend on sheet thicknesses; accordingly the average thickness is accepted as 0.5 mm. 
System boundary: 
This is a cradle-to-gate Life Cycle Analysis study. The product stage information modules A1, A2, and A3 are considered. In addition to the product stage, Module A5 is also considered within LCA scope. In detail, this LCA study includes production of raw material extraction and processing (A1), transport of the raw materials (A2) and transport the packaging materials to the manufacturer (A2), manufacturing of the product with the stages supply of raw material from stock, cutting, bending, dying, packaging and stockpiling (A3), recycling of recyclable waste generated during manufacturing (A3), and disposal of packaging materials (A5).</useAdviceForDataSet>
<common:other>
<epd2:referenceToOriginalEPD type="source data set" refObjectId="ded8c7da-a47b-4139-95b7-88440d3f4670">
<common:shortDescription xml:lang="en">Galvanized steel suspended ceiling panel.pdf</common:shortDescription>
</epd2:referenceToOriginalEPD>
</common:other>
</dataSourcesTreatmentAndRepresentativeness>
<validation>
<review type="Accredited third party review">
<common:referenceToNameOfReviewerAndInstitution uri="../contacts/d111dbec-b024-4be5-86c5-752d6eb2cf95.xml" type="contact data set" refObjectId="d111dbec-b024-4be5-86c5-752d6eb2cf95">
<common:shortDescription xml:lang="en">Institut Bauen und Umwelt e. V.</common:shortDescription>
</common:referenceToNameOfReviewerAndInstitution>
</review>
</validation>
<complianceDeclarations>
<compliance>
<common:referenceToComplianceSystem uri="../sources/b00f9ec0-7874-11e3-981f-0800200c9a66.xml" type="source data set" refObjectId="b00f9ec0-7874-11e3-981f-0800200c9a66">
<common:shortDescription xml:lang="en">DIN EN 15804</common:shortDescription>
</common:referenceToComplianceSystem>
</compliance>
<compliance>
<common:referenceToComplianceSystem uri="../sources/4f2eb655-6e44-4874-a95a-e28f5442cd4d.xml" type="source data set" refObjectId="4f2eb655-6e44-4874-a95a-e28f5442cd4d">
<common:shortDescription xml:lang="en">ISO 14025</common:shortDescription>
</common:referenceToComplianceSystem>
</compliance>
</complianceDeclarations>
</modellingAndValidation>
<administrativeInformation>
<common:commissionerAndGoal>
<common:referenceToCommissioner uri="../contacts/5f121287-5e89-49b6-a78e-855a8656bda9.xml" type="contact data set" refObjectId="5f121287-5e89-49b6-a78e-855a8656bda9">
<common:shortDescription xml:lang="en">Butem Metal Form San. Ve Tic. A.S.</common:shortDescription>
</common:referenceToCommissioner>
</common:commissionerAndGoal>
<dataGenerator>
<common:referenceToPersonOrEntityGeneratingTheDataSet uri="../contacts/2d275d1d-89ba-497c-8901-386703315b42.xml" type="contact data set" refObjectId="2d275d1d-89ba-497c-8901-386703315b42">
<common:shortDescription xml:lang="en">ERKE Sustainable Building Design LCC.</common:shortDescription>
</common:referenceToPersonOrEntityGeneratingTheDataSet>
</dataGenerator>
<dataEntryBy>
<common:timeStamp>2019-07-25T09:01:12.58</common:timeStamp>
<common:referenceToDataSetFormat uri="../sources/a97a0155-0234-4b87-b4ce-a45da52f2a40.xml" type="source data set" refObjectId="a97a0155-0234-4b87-b4ce-a45da52f2a40">
<common:shortDescription xml:lang="en">ILCD Format</common:shortDescription>
</common:referenceToDataSetFormat>
<common:referenceToDataSetFormat uri="../sources/a29449fd-aa2f-4de8-b5d7-4b06b43c6fde.xml" type="source data set" refObjectId="a29449fd-aa2f-4de8-b5d7-4b06b43c6fde">
<common:shortDescription xml:lang="de">EPD-Datenformaterweiterungen v1.2</common:shortDescription>
<common:shortDescription xml:lang="en">EPD Data Format Extensions v1.2</common:shortDescription>
</common:referenceToDataSetFormat>
</dataEntryBy>
<publicationAndOwnership>
<common:dataSetVersion>00.01.000</common:dataSetVersion>
<common:referenceToRegistrationAuthority uri="../contacts/d111dbec-b024-4be5-86c5-752d6eb2cf95.xml" type="contact data set" refObjectId="d111dbec-b024-4be5-86c5-752d6eb2cf95">
<common:shortDescription xml:lang="en">Institut Bauen und Umwelt e. V.</common:shortDescription>
</common:referenceToRegistrationAuthority>
<common:registrationNumber>EPD-BUT-20190023-IAC2-EN</common:registrationNumber>
<common:referenceToOwnershipOfDataSet uri="../contacts/5f121287-5e89-49b6-a78e-855a8656bda9.xml" type="contact data set" refObjectId="5f121287-5e89-49b6-a78e-855a8656bda9">
<common:shortDescription xml:lang="en">Butem Metal Form San. Ve Tic. A.S.</common:shortDescription>
</common:referenceToOwnershipOfDataSet>
<common:copyright>true</common:copyright>
<common:licenseType>Free of charge for all users and uses</common:licenseType>
<common:accessRestrictions xml:lang="en">None</common:accessRestrictions>
<common:other>
<epd2:referenceToPublisher type="contact data set" refObjectId="d111dbec-b024-4be5-86c5-752d6eb2cf95" uri="../contacts/d111dbec-b024-4be5-86c5-752d6eb2cf95.xml">
<common:shortDescription xml:lang="en">Institut Bauen und Umwelt e. V.</common:shortDescription>
</epd2:referenceToPublisher>
</common:other>
</publicationAndOwnership>
</administrativeInformation>
<exchanges>
<exchange dataSetInternalID="0">
<referenceToFlowDataSet uri="../flows/91466d3e-8586-1689-c746-b035b73225d2.xml" type="flow data set" refObjectId="91466d3e-8586-1689-c746-b035b73225d2">
<common:shortDescription xml:lang="en">Steel Suspended Ceiling Panel ()</common:shortDescription>
</referenceToFlowDataSet>
<meanAmount>1</meanAmount>
<referencesToDataSource />
</exchange>
<exchange dataSetInternalID="1">
<referenceToFlowDataSet uri="../flows/20f32be5-0398-4288-9b6d-accddd195317.xml" type="flow data set" refObjectId="20f32be5-0398-4288-9b6d-accddd195317">
<common:shortDescription xml:lang="en">Renewable primary energy as energy carrier (PERE)</common:shortDescription>
</referenceToFlowDataSet>
<functionType>General reminder flow</functionType>
<exchangeDirection>Input</exchangeDirection>
<common:other>
<epd:referenceToUnitGroupDataSet uri="../unitgroups/93a60a57-a3c8-11da-a746-0800200c9a66.xml" type="unit group data set" refObjectId="93a60a57-a3c8-11da-a746-0800200c9a66">
<common:shortDescription xml:lang="en">MJ</common:shortDescription>
</epd:referenceToUnitGroupDataSet>
<epd:amount epd:module="A1-A3">14.19</epd:amount>
<epd:amount epd:module="A5">0.0168</epd:amount>
</common:other>
</exchange>
<exchange dataSetInternalID="2">
<referenceToFlowDataSet uri="../flows/fb3ec0de-548d-4508-aea5-00b73bf6f702.xml" type="flow data set" refObjectId="fb3ec0de-548d-4508-aea5-00b73bf6f702">
<common:shortDescription xml:lang="en">Renewable primary energy resources as material utilization (PERM)</common:shortDescription>
</referenceToFlowDataSet>
<functionType>General reminder flow</functionType>
<exchangeDirection>Input</exchangeDirection>
<common:other>
<epd:referenceToUnitGroupDataSet uri="../unitgroups/93a60a57-a3c8-11da-a746-0800200c9a66.xml" type="unit group data set" refObjectId="93a60a57-a3c8-11da-a746-0800200c9a66">
<common:shortDescription xml:lang="en">MJ</common:shortDescription>
</epd:referenceToUnitGroupDataSet>
<epd:amount epd:module="A1-A3"></epd:amount>
<epd:amount epd:module="A5"></epd:amount>
</common:other>
</exchange>
<exchange dataSetInternalID="3">
<referenceToFlowDataSet uri="../flows/53f97275-fa8a-4cdd-9024-65936002acd0.xml" type="flow data set" refObjectId="53f97275-fa8a-4cdd-9024-65936002acd0">
<common:shortDescription xml:lang="en">Total use of renewable primary energy resources (PERT)</common:shortDescription>
</referenceToFlowDataSet>
<functionType>General reminder flow</functionType>
<exchangeDirection>Input</exchangeDirection>
<common:other>
<epd:referenceToUnitGroupDataSet uri="../unitgroups/93a60a57-a3c8-11da-a746-0800200c9a66.xml" type="unit group data set" refObjectId="93a60a57-a3c8-11da-a746-0800200c9a66">
<common:shortDescription xml:lang="en">MJ</common:shortDescription>
</epd:referenceToUnitGroupDataSet>
<epd:amount epd:module="A1-A3">14.19</epd:amount>
<epd:amount epd:module="A5">0.0168</epd:amount>
</common:other>
</exchange>
<exchange dataSetInternalID="4">
<referenceToFlowDataSet uri="../flows/ac857178-2b45-46ec-892a-a9a4332f0372.xml" type="flow data set" refObjectId="ac857178-2b45-46ec-892a-a9a4332f0372">
<common:shortDescription xml:lang="en">Non renewable primary energy as energy carrier (PENRE)</common:shortDescription>
</referenceToFlowDataSet>
<functionType>General reminder flow</functionType>
<exchangeDirection>Input</exchangeDirection>
<common:other>
<epd:referenceToUnitGroupDataSet uri="../unitgroups/93a60a57-a3c8-11da-a746-0800200c9a66.xml" type="unit group data set" refObjectId="93a60a57-a3c8-11da-a746-0800200c9a66">
<common:shortDescription xml:lang="en">MJ</common:shortDescription>
</epd:referenceToUnitGroupDataSet>
<epd:amount epd:module="A1-A3">221.37</epd:amount>
<epd:amount epd:module="A5">0.133</epd:amount>
</common:other>
</exchange>
<exchange dataSetInternalID="5">
<referenceToFlowDataSet uri="../flows/1421caa0-679d-4bf4-b282-0eb850ccae27.xml" type="flow data set" refObjectId="1421caa0-679d-4bf4-b282-0eb850ccae27">
<common:shortDescription xml:lang="en">Non renewable primary energy as material utilization (PENRM)</common:shortDescription>
</referenceToFlowDataSet>
<functionType>General reminder flow</functionType>
<exchangeDirection>Input</exchangeDirection>
<common:other>
<epd:referenceToUnitGroupDataSet uri="../unitgroups/93a60a57-a3c8-11da-a746-0800200c9a66.xml" type="unit group data set" refObjectId="93a60a57-a3c8-11da-a746-0800200c9a66">
<common:shortDescription xml:lang="en">MJ</common:shortDescription>
</epd:referenceToUnitGroupDataSet>
<epd:amount epd:module="A1-A3"></epd:amount>
<epd:amount epd:module="A5"></epd:amount>
</common:other>
</exchange>
<exchange dataSetInternalID="6">
<referenceToFlowDataSet uri="../flows/06159210-646b-4c8d-8583-da9b3b95a6c1.xml" type="flow data set" refObjectId="06159210-646b-4c8d-8583-da9b3b95a6c1">
<common:shortDescription xml:lang="en">Total use of non renewable primary energy resources (PENRT)</common:shortDescription>
</referenceToFlowDataSet>
<functionType>General reminder flow</functionType>
<exchangeDirection>Input</exchangeDirection>
<common:other>
<epd:referenceToUnitGroupDataSet uri="../unitgroups/93a60a57-a3c8-11da-a746-0800200c9a66.xml" type="unit group data set" refObjectId="93a60a57-a3c8-11da-a746-0800200c9a66">
<common:shortDescription xml:lang="en">MJ</common:shortDescription>
</epd:referenceToUnitGroupDataSet>
<epd:amount epd:module="A1-A3">221.37</epd:amount>
<epd:amount epd:module="A5">0.133</epd:amount>
</common:other>
</exchange>
<exchange dataSetInternalID="7">
<referenceToFlowDataSet uri="../flows/c6a1f35f-2d09-4f54-8dfb-97e502e1ce92.xml" type="flow data set" refObjectId="c6a1f35f-2d09-4f54-8dfb-97e502e1ce92">
<common:shortDescription xml:lang="en">Use of secondary material (SM)</common:shortDescription>
</referenceToFlowDataSet>
<functionType>General reminder flow</functionType>
<exchangeDirection>Input</exchangeDirection>
<common:other>
<epd:referenceToUnitGroupDataSet uri="../unitgroups/ad38d542-3fe9-439d-9b95-2f5f7752acaf.xml" type="unit group data set" refObjectId="ad38d542-3fe9-439d-9b95-2f5f7752acaf">
<common:shortDescription xml:lang="en">kg</common:shortDescription>
</epd:referenceToUnitGroupDataSet>
<epd:amount epd:module="A1-A3"></epd:amount>
<epd:amount epd:module="A5"></epd:amount>
</common:other>
</exchange>
<exchange dataSetInternalID="8">
<referenceToFlowDataSet uri="../flows/64333088-a55f-4aa2-9a31-c10b07816787.xml" type="flow data set" refObjectId="64333088-a55f-4aa2-9a31-c10b07816787">
<common:shortDescription xml:lang="en">Use of renewable secondary fuels (RSF)</common:shortDescription>
</referenceToFlowDataSet>
<functionType>General reminder flow</functionType>
<exchangeDirection>Input</exchangeDirection>
<common:other>
<epd:referenceToUnitGroupDataSet uri="../unitgroups/93a60a57-a3c8-11da-a746-0800200c9a66.xml" type="unit group data set" refObjectId="93a60a57-a3c8-11da-a746-0800200c9a66">
<common:shortDescription xml:lang="en">MJ</common:shortDescription>
</epd:referenceToUnitGroupDataSet>
<epd:amount epd:module="A1-A3"></epd:amount>
<epd:amount epd:module="A5"></epd:amount>
</common:other>
</exchange>
<exchange dataSetInternalID="9">
<referenceToFlowDataSet uri="../flows/89def144-d39a-4287-b86f-efde453ddcb2.xml" type="flow data set" refObjectId="89def144-d39a-4287-b86f-efde453ddcb2">
<common:shortDescription xml:lang="en">Use of non renewable secondary fuels (NRSF)</common:shortDescription>
</referenceToFlowDataSet>
<functionType>General reminder flow</functionType>
<exchangeDirection>Input</exchangeDirection>
<common:other>
<epd:referenceToUnitGroupDataSet uri="../unitgroups/93a60a57-a3c8-11da-a746-0800200c9a66.xml" type="unit group data set" refObjectId="93a60a57-a3c8-11da-a746-0800200c9a66">
<common:shortDescription xml:lang="en">MJ</common:shortDescription>
</epd:referenceToUnitGroupDataSet>
<epd:amount epd:module="A1-A3"></epd:amount>
<epd:amount epd:module="A5"></epd:amount>
</common:other>
</exchange>
<exchange dataSetInternalID="10">
<referenceToFlowDataSet uri="../flows/3cf952c8-f3a4-461d-8c96-96456ca62246.xml" type="flow data set" refObjectId="3cf952c8-f3a4-461d-8c96-96456ca62246">
<common:shortDescription xml:lang="en">Use of net fresh water (FW)</common:shortDescription>
</referenceToFlowDataSet>
<functionType>General reminder flow</functionType>
<exchangeDirection>Input</exchangeDirection>
<common:other>
<epd:referenceToUnitGroupDataSet uri="../unitgroups/cd950537-0a98-4044-9ba7-9f9a68d0a504.xml" type="unit group data set" refObjectId="cd950537-0a98-4044-9ba7-9f9a68d0a504">
<common:shortDescription xml:lang="en">m^3</common:shortDescription>
</epd:referenceToUnitGroupDataSet>
<epd:amount epd:module="A1-A3">11.1</epd:amount>
<epd:amount epd:module="A5">0.0146</epd:amount>
</common:other>
</exchange>
<exchange dataSetInternalID="11">
<referenceToFlowDataSet uri="../flows/430f9e0f-59b2-46a0-8e0d-55e0e84948fc.xml" type="flow data set" refObjectId="430f9e0f-59b2-46a0-8e0d-55e0e84948fc">
<common:shortDescription xml:lang="en">Hazardous waste disposed (HWD)</common:shortDescription>
</referenceToFlowDataSet>
<functionType>General reminder flow</functionType>
<exchangeDirection>Output</exchangeDirection>
<common:other>
<epd:referenceToUnitGroupDataSet uri="../unitgroups/ad38d542-3fe9-439d-9b95-2f5f7752acaf.xml" type="unit group data set" refObjectId="ad38d542-3fe9-439d-9b95-2f5f7752acaf">
<common:shortDescription xml:lang="en">kg</common:shortDescription>
</epd:referenceToUnitGroupDataSet>
<epd:amount epd:module="A1-A3">3.86E-07</epd:amount>
<epd:amount epd:module="A5">2.95E-10</epd:amount>
</common:other>
</exchange>
<exchange dataSetInternalID="12">
<referenceToFlowDataSet uri="../flows/b29ef66b-e286-4afa-949f-62f1a7b4d7fa.xml" type="flow data set" refObjectId="b29ef66b-e286-4afa-949f-62f1a7b4d7fa">
<common:shortDescription xml:lang="en">Non hazardous waste disposed (NHWD)</common:shortDescription>
</referenceToFlowDataSet>
<functionType>General reminder flow</functionType>
<exchangeDirection>Output</exchangeDirection>
<common:other>
<epd:referenceToUnitGroupDataSet uri="../unitgroups/ad38d542-3fe9-439d-9b95-2f5f7752acaf.xml" type="unit group data set" refObjectId="ad38d542-3fe9-439d-9b95-2f5f7752acaf">
<common:shortDescription xml:lang="en">kg</common:shortDescription>
</epd:referenceToUnitGroupDataSet>
<epd:amount epd:module="A1-A3">94.6</epd:amount>
<epd:amount epd:module="A5">0.0254</epd:amount>
</common:other>
</exchange>
<exchange dataSetInternalID="13">
<referenceToFlowDataSet uri="../flows/3449546e-52ad-4b39-b809-9fb77cea8ff6.xml" type="flow data set" refObjectId="3449546e-52ad-4b39-b809-9fb77cea8ff6">
<common:shortDescription xml:lang="en">Radioactive waste disposed (RWD)</common:shortDescription>
</referenceToFlowDataSet>
<functionType>General reminder flow</functionType>
<exchangeDirection>Output</exchangeDirection>
<common:other>
<epd:referenceToUnitGroupDataSet uri="../unitgroups/ad38d542-3fe9-439d-9b95-2f5f7752acaf.xml" type="unit group data set" refObjectId="ad38d542-3fe9-439d-9b95-2f5f7752acaf">
<common:shortDescription xml:lang="en">kg</common:shortDescription>
</epd:referenceToUnitGroupDataSet>
<epd:amount epd:module="A1-A3">0.00312</epd:amount>
<epd:amount epd:module="A5">8.05E-06</epd:amount>
</common:other>
</exchange>
<exchange dataSetInternalID="14">
<referenceToFlowDataSet uri="../flows/a2b32f97-3fc7-4af2-b209-525bc6426f33.xml" type="flow data set" refObjectId="a2b32f97-3fc7-4af2-b209-525bc6426f33">
<common:shortDescription xml:lang="en">Components for re-use (CRU)</common:shortDescription>
</referenceToFlowDataSet>
<functionType>General reminder flow</functionType>
<exchangeDirection>Output</exchangeDirection>
<common:other>
<epd:referenceToUnitGroupDataSet uri="../unitgroups/ad38d542-3fe9-439d-9b95-2f5f7752acaf.xml" type="unit group data set" refObjectId="ad38d542-3fe9-439d-9b95-2f5f7752acaf">
<common:shortDescription xml:lang="en">kg</common:shortDescription>
</epd:referenceToUnitGroupDataSet>
<epd:amount epd:module="A1-A3"></epd:amount>
<epd:amount epd:module="A5"></epd:amount>
</common:other>
</exchange>
<exchange dataSetInternalID="15">
<referenceToFlowDataSet uri="../flows/d7fe48a5-4103-49c8-9aae-b0b5dfdbd6ae.xml" type="flow data set" refObjectId="d7fe48a5-4103-49c8-9aae-b0b5dfdbd6ae">
<common:shortDescription xml:lang="en">Materials for recycling (MFR)</common:shortDescription>
</referenceToFlowDataSet>
<functionType>General reminder flow</functionType>
<exchangeDirection>Output</exchangeDirection>
<common:other>
<epd:referenceToUnitGroupDataSet uri="../unitgroups/ad38d542-3fe9-439d-9b95-2f5f7752acaf.xml" type="unit group data set" refObjectId="ad38d542-3fe9-439d-9b95-2f5f7752acaf">
<common:shortDescription xml:lang="en">kg</common:shortDescription>
</epd:referenceToUnitGroupDataSet>
<epd:amount epd:module="A1-A3"></epd:amount>
<epd:amount epd:module="A5"></epd:amount>
</common:other>
</exchange>
<exchange dataSetInternalID="16">
<referenceToFlowDataSet uri="../flows/59a9181c-3aaf-46ee-8b13-2b3723b6e447.xml" type="flow data set" refObjectId="59a9181c-3aaf-46ee-8b13-2b3723b6e447">
<common:shortDescription xml:lang="en">Materials for energy recovery (MER)</common:shortDescription>
</referenceToFlowDataSet>
<functionType>General reminder flow</functionType>
<exchangeDirection>Output</exchangeDirection>
<common:other>
<epd:referenceToUnitGroupDataSet uri="../unitgroups/ad38d542-3fe9-439d-9b95-2f5f7752acaf.xml" type="unit group data set" refObjectId="ad38d542-3fe9-439d-9b95-2f5f7752acaf">
<common:shortDescription xml:lang="en">kg</common:shortDescription>
</epd:referenceToUnitGroupDataSet>
<epd:amount epd:module="A1-A3"></epd:amount>
<epd:amount epd:module="A5"></epd:amount>
</common:other>
</exchange>
<exchange dataSetInternalID="17">
<referenceToFlowDataSet uri="../flows/4da0c987-2b76-40d6-9e9e-82a017aaaf29.xml" type="flow data set" refObjectId="4da0c987-2b76-40d6-9e9e-82a017aaaf29">
<common:shortDescription xml:lang="en">Exported electrical energy (EEE)</common:shortDescription>
</referenceToFlowDataSet>
<functionType>General reminder flow</functionType>
<exchangeDirection>Output</exchangeDirection>
<common:other>
<epd:referenceToUnitGroupDataSet uri="../unitgroups/93a60a57-a3c8-11da-a746-0800200c9a66.xml" type="unit group data set" refObjectId="93a60a57-a3c8-11da-a746-0800200c9a66">
<common:shortDescription xml:lang="en">MJ</common:shortDescription>
</epd:referenceToUnitGroupDataSet>
<epd:amount epd:module="A1-A3"></epd:amount>
<epd:amount epd:module="A5"></epd:amount>
</common:other>
</exchange>
<exchange dataSetInternalID="18">
<referenceToFlowDataSet uri="../flows/98daf38a-7a79-46d3-9a37-2b7bd0955810.xml" type="flow data set" refObjectId="98daf38a-7a79-46d3-9a37-2b7bd0955810">
<common:shortDescription xml:lang="en">Exported thermal energy (EET)</common:shortDescription>
</referenceToFlowDataSet>
<functionType>General reminder flow</functionType>
<exchangeDirection>Output</exchangeDirection>
<common:other>
<epd:referenceToUnitGroupDataSet uri="../unitgroups/93a60a57-a3c8-11da-a746-0800200c9a66.xml" type="unit group data set" refObjectId="93a60a57-a3c8-11da-a746-0800200c9a66">
<common:shortDescription xml:lang="en">MJ</common:shortDescription>
</epd:referenceToUnitGroupDataSet>
<epd:amount epd:module="A1-A3"></epd:amount>
<epd:amount epd:module="A5"></epd:amount>
</common:other>
</exchange>
</exchanges>
<LCIAResults>
<LCIAResult>
<referenceToLCIAMethodDataSet uri="../lciamethods/77e416eb-a363-4258-a04e-171d843a6460.xml" type="LCIA method data set" refObjectId="77e416eb-a363-4258-a04e-171d843a6460">
<common:shortDescription xml:lang="en">Global warming potential (GWP)</common:shortDescription>
</referenceToLCIAMethodDataSet>
<common:other>
<epd:referenceToUnitGroupDataSet uri="../unitgroups/1ebf3012-d0db-4de2-aefd-ef30cedb0be1.xml" type="unit group data set" refObjectId="1ebf3012-d0db-4de2-aefd-ef30cedb0be1">
<common:shortDescription xml:lang="en">kg CO_(2)-Äq.</common:shortDescription>
</epd:referenceToUnitGroupDataSet>
<epd:amount epd:module="A1-A3">18</epd:amount>
<epd:amount epd:module="A5">0.0188</epd:amount>
</common:other>
</LCIAResult>
<LCIAResult>
<referenceToLCIAMethodDataSet uri="../lciamethods/06dcd26f-025f-401a-a7c1-5e457eb54637.xml" type="LCIA method data set" refObjectId="06dcd26f-025f-401a-a7c1-5e457eb54637">
<common:shortDescription xml:lang="en">Depletion potential of the stratospheric ozone layer (ODP)</common:shortDescription>
</referenceToLCIAMethodDataSet>
<common:other>
<epd:referenceToUnitGroupDataSet uri="../unitgroups/88054749-b0a6-47ea-a82b-dc5b29326512.xml" type="unit group data set" refObjectId="88054749-b0a6-47ea-a82b-dc5b29326512">
<common:shortDescription xml:lang="en">kg CFC11-Äq.</common:shortDescription>
</epd:referenceToUnitGroupDataSet>
<epd:amount epd:module="A1-A3">3.65E-10</epd:amount>
<epd:amount epd:module="A5">2.01E-12</epd:amount>
</common:other>
</LCIAResult>
<LCIAResult>
<referenceToLCIAMethodDataSet uri="../lciamethods/b4274add-93b7-4905-a5e4-2e878c4e4216.xml" type="LCIA method data set" refObjectId="b4274add-93b7-4905-a5e4-2e878c4e4216">
<common:shortDescription xml:lang="en">Acidification potential of land and water (AP)</common:shortDescription>
</referenceToLCIAMethodDataSet>
<common:other>
<epd:referenceToUnitGroupDataSet uri="../unitgroups/bc50c624-a9bc-45b1-a9b0-e6b10d00476f.xml" type="unit group data set" refObjectId="bc50c624-a9bc-45b1-a9b0-e6b10d00476f">
<common:shortDescription xml:lang="en">kg SO_(2)-Äq.</common:shortDescription>
</epd:referenceToUnitGroupDataSet>
<epd:amount epd:module="A1-A3">0.0681</epd:amount>
<epd:amount epd:module="A5">7.73E-05</epd:amount>
</common:other>
</LCIAResult>
<LCIAResult>
<referenceToLCIAMethodDataSet uri="../lciamethods/f58827d0-b407-4ec6-be75-8b69efb98a0f.xml" type="LCIA method data set" refObjectId="f58827d0-b407-4ec6-be75-8b69efb98a0f">
<common:shortDescription xml:lang="en">Eutrophication potential (EP)</common:shortDescription>
</referenceToLCIAMethodDataSet>
<common:other>
<epd:referenceToUnitGroupDataSet uri="../unitgroups/67b5401d-873c-485f-bcf3-6ae83b918822.xml" type="unit group data set" refObjectId="67b5401d-873c-485f-bcf3-6ae83b918822">
<common:shortDescription xml:lang="en">kg PO_(4)^(3)-Äq.</common:shortDescription>
</epd:referenceToUnitGroupDataSet>
<epd:amount epd:module="A1-A3">0.00547</epd:amount>
<epd:amount epd:module="A5">1.47E-05</epd:amount>
</common:other>
</LCIAResult>
<LCIAResult>
<referenceToLCIAMethodDataSet uri="../lciamethods/1e84a202-dae6-42aa-9e9d-71ea48b8be00.xml" type="LCIA method data set" refObjectId="1e84a202-dae6-42aa-9e9d-71ea48b8be00">
<common:shortDescription xml:lang="en">Formation potential of tropospheric ozone photochemical oxidants (POCP)</common:shortDescription>
</referenceToLCIAMethodDataSet>
<common:other>
<epd:referenceToUnitGroupDataSet uri="../unitgroups/01c26c17-9a76-406e-8295-f17b55fd909e.xml" type="unit group data set" refObjectId="01c26c17-9a76-406e-8295-f17b55fd909e">
<common:shortDescription xml:lang="en">kg Ethen-Äq.</common:shortDescription>
</epd:referenceToUnitGroupDataSet>
<epd:amount epd:module="A1-A3">0.00847</epd:amount>
<epd:amount epd:module="A5">6.12E-06</epd:amount>
</common:other>
</LCIAResult>
<LCIAResult>
<referenceToLCIAMethodDataSet uri="../lciamethods/f7c73bb9-ab1a-4249-9c6d-379a0de6f67e.xml" type="LCIA method data set" refObjectId="f7c73bb9-ab1a-4249-9c6d-379a0de6f67e">
<common:shortDescription xml:lang="en">Abiotic depletion potential for non fossil resources (ADPE)</common:shortDescription>
</referenceToLCIAMethodDataSet>
<common:other>
<epd:referenceToUnitGroupDataSet uri="../unitgroups/54ccd2d9-a32a-4fc2-923d-f2c8c93e89d4.xml" type="unit group data set" refObjectId="54ccd2d9-a32a-4fc2-923d-f2c8c93e89d4">
<common:shortDescription xml:lang="en">kg Sb-Äq.</common:shortDescription>
</epd:referenceToUnitGroupDataSet>
<epd:amount epd:module="A1-A3">0.0014</epd:amount>
<epd:amount epd:module="A5">7.45E-09</epd:amount>
</common:other>
</LCIAResult>
<LCIAResult>
<referenceToLCIAMethodDataSet uri="../lciamethods/804ebcdf-309d-4098-8ed8-fdaf2f389981.xml" type="LCIA method data set" refObjectId="804ebcdf-309d-4098-8ed8-fdaf2f389981">
<common:shortDescription xml:lang="en">Abiotic depletion potential for fossil resources (ADPF)</common:shortDescription>
</referenceToLCIAMethodDataSet>
<common:other>
<epd:referenceToUnitGroupDataSet uri="../unitgroups/93a60a57-a3c8-11da-a746-0800200c9a66.xml" type="unit group data set" refObjectId="93a60a57-a3c8-11da-a746-0800200c9a66">
<common:shortDescription xml:lang="en">MJ</common:shortDescription>
</epd:referenceToUnitGroupDataSet>
<epd:amount epd:module="A1-A3">213</epd:amount>
<epd:amount epd:module="A5">0.113</epd:amount>
</common:other>
</LCIAResult>
</LCIAResults>
</processDataSet>