<?xml version="1.0" encoding="utf-8"?>
<processDataSet xmlns:epd="http://www.iai.kit.edu/EPD/2013" xmlns:epd2="http://www.indata.network/EPD/2019" xmlns:common="http://lca.jrc.it/ILCD/Common" xsi:schemaLocation="http://lca.jrc.it/ILCD/Process ../../schemas/EPD_DataSet.xsd" epd2:epd-version="1.2" version="1.1" locations="../ILCDLocations.xml" xmlns:xsi="http://www.w3.org/2001/XMLSchema-instance" xmlns="http://lca.jrc.it/ILCD/Process">
<processInformation>
<dataSetInformation>
<common:UUID>e2535897-e47e-4165-8f8a-131389936ec9</common:UUID>
<name>
<baseName xml:lang="de">Elastische Bodenbeläge</baseName>
<baseName xml:lang="en">Resilient floor coverings</baseName>
<functionalUnitFlowProperties xml:lang="de" />
</name>
<classificationInformation>
<common:classification name="OEKOBAU.DAT">
<common:class level="0" classId="3">Holz</common:class>
<common:class level="1" classId="3.3">Holzböden</common:class>
<common:class level="2" classId="3.3.04">Mehrschichtig modulare Bodenbeläge</common:class>
</common:classification>
<common:classification name="IBUCategories">
<common:class level="0">02 Bauprodukte</common:class>
<common:class level="1">Bodenbeläge</common:class>
<common:class level="2">Bodenbeläge</common:class>
</common:classification>
</classificationInformation>
<common:generalComment xml:lang="de">Modular ONEDer mehrschichtige Aufbau der Modular ONE Böden zeichnet sich durch die Beschichtung des Dekorpapieres mit dem weichmacherfreien Werkstoff Polypropylen aus. Diese Beschichtung lässt eine authentische Strukturierung des Dekorpapieres zu und ermöglicht so die naturgetreue Nachbildung echter Holzoberflächen. Trägermaterial der Modular ONE Böden ist eine feuchtraumgeeignete hochdichte Faserplatte, die dem Boden eine flexible Festigkeit gibt und dank Spezialbeschichtung eine Wasserresistenz des Bodens von bis zu 4 Stunden bei stehendem Wasser garantiert.Eco Balance PURÄhnlich wie beim Modular ONE Boden handelt es sich bei Eco Balance PUR um eine kaschierte Hochdichte Faserplatte. Die Dekorschicht besteht aus dem weichmacherfreien Werkstoff Polyurethan, welcher aus nachwachsenden Rohstoffen hergestellt wird. Diese Beschichtung lässt eine authentische Strukturierung des Dekorpapieres zu und ermöglicht so die naturgetreue Nachbildung echter Holzoberflächen.</common:generalComment>
<common:generalComment xml:lang="en">Modular ONEThe multi-layered structure of the Modular ONE flooring is characterised by the coating of decor paper with the plasticiser-free material polypropylene. This coating allows for an authentic structuring of the decor paper and thus enables the realistic reproduction of real wood surfaces.  The core material of the Modular ONE flooring is a high-density fibreboard, which is specially adapted for wet rooms. It gives the floor a flexible strength and thanks to its special coating guarantees water resistance of the flooring for up to 4 hours in the case of standing water.Eco Balance PUR Similar to the Modular ONE flooring, Eco Balance PUR is a coated high-density fibreboard. The decor layer consists of the plasticiser-free material polyurethane, which is produced from renewable resources. This coating allows for an authentic structuring of the decor paper and thus enables the realistic reproduction of real wood surfaces.</common:generalComment>
</dataSetInformation>
<quantitativeReference>
<referenceToReferenceFlow>0</referenceToReferenceFlow>
</quantitativeReference>
<time>
<common:referenceYear>2019</common:referenceYear>
<common:dataSetValidUntil>2024</common:dataSetValidUntil>
<common:other>
<epd2:publicationDateOfEPD>2019-03-06</epd2:publicationDateOfEPD>
</common:other>
</time>
<geography>
<locationOfOperationSupplyOrProduction location="DE" />
</geography>
<technology>
<technologyDescriptionAndIncludedProcesses xml:lang="de">The HDF core board, the wear layer, and the cork backing are pressed together using a glue. The planks are then provided with a longitudinal and transverse profile. After quality control of the individual flooring elements, they are packed in halfshell cartons and shrink-wrapped in PE film. These individual packaging units are stacked on pallets according to the different formats and made available in the warehouse for subsequent delivery. All processes are continually checked and documented as part of the in-house Factory Production Control (FPC) 
Deklarierte Einheit: 
Die Deklarierte Einheit ist ein Quadratmeter (1 m²) elastische Bodenbeläge inkl. Verpackungsmaterialien.Für die gegenständige Deklaration wurden zur Durchschnittsbildung die durchschnittlichen Verkaufsanteile eines Halbjahres bestehend aus den Produkten Eco Balance PUR und Modular ONE herangezogen. Die im Durchschnitt enthaltenen Varianten unterscheiden sich in Bezug auf das Material der Nutzschicht (PUR bzw. PP).</technologyDescriptionAndIncludedProcesses>
<technologyDescriptionAndIncludedProcesses xml:lang="en">The HDF core board, the wear layer, and the cork backing are pressed together using a glue. The planks are then provided with a longitudinal and transverse profile. After quality control of the individual flooring elements, they are packed in half-shell cartons and shrink-wrapped in PE film. These individual packaging units are stacked on pallets according to the different formats and made available in the warehouse for subsequent delivery. All processes are continually checked and documented as part of the in-house Factory Production Control (FPC). 
Declared unit: 
The declared unit is one square metre (1 m²) of resilient floor coverings including packaging material.The average sales shares over 6 months for the Eco Balance PUR and Modular ONE products were used to calculate the average for this declaration. The variants contained in the average differ with regard to the wear layer material (PUR or PP).</technologyDescriptionAndIncludedProcesses>
<technologicalApplicability xml:lang="de">Elastische Bodenbeläge sind geeignet für eine private und gewerbliche Nutzung im Innenbereich. Sie werden entweder auf Estrich oder bestehenden anderen Unterböden in Verbindung mit geeigneten Unterlagen (Dämmunterlagen) schwimmend verlegt oder vollflächig auf dem Estrich verklebt. Die Grundsätze ordnungsgemäßer Verlegung können der beiliegenden Verlege-Anleitung bzw. dem „Ratgeber Elastische Bodenbeläge“ entnommen werden.</technologicalApplicability>
<technologicalApplicability xml:lang="en">Resilient floor coverings are suitable for private and commercial indoor use. They are either laid floating on screed or other existing subfloors in conjunction with suitable underlays (insulating underlays) or glued to the full surface of the screed. The principles of proper installation are available in the enclosed installation instructions or in the &quot;Resilient floor coverings advice section&quot;.</technologicalApplicability>
</technology>
</processInformation>
<modellingAndValidation>
<LCIMethodAndAllocation>
<typeOfDataSet>EPD</typeOfDataSet>
<referenceToLCAMethodDetails type="source data set" refObjectId="c2e770a8-abc6-4fa6-9213-462cad661576">
<common:shortDescription xml:lang="de">Bodenbeläge.pdf</common:shortDescription>
</referenceToLCAMethodDetails>
<common:other>
<epd:subType xmlns="http://www.iai.kit.edu/EPD/2013">average dataset</epd:subType>
</common:other>
</LCIMethodAndAllocation>
<dataSourcesTreatmentAndRepresentativeness>
<referenceToDataSource type="source data set" refObjectId="28d74cc0-db8b-4d7e-bc44-5f6d56ce0c4a">
<common:shortDescription xml:lang="de">GaBi Database (all versions)</common:shortDescription>
</referenceToDataSource>
<referenceToDataSource type="source data set" refObjectId="feda7597-12a1-4bd5-93ef-4d8120877b78">
<common:shortDescription xml:lang="de">GaBi database SP35 2018</common:shortDescription>
</referenceToDataSource>
<useAdviceForDataSet xml:lang="de">Gültigkeitsbereich: 
Die vorliegende EPD bezieht sich auf Herstellung, Transport, Installation und Entsorgung eines durchschnittlichen Quadratmeters elastischer Bodenbeläge von Parador. Die technischen Eigenschaften werden in Kapitel 2.3 dargestellt. Produktionsstandort des Produkts ist Coesfeld in Deutschland. 
Systemgrenze: 
Typ der EPD: Wiege bis Werkstor mit Optionen.Module A1-3, A4 und A5 Das Produktstadium (A1-3) beginnt mit der Berücksichtigung der Produktion der notwendigen Rohstoffe und Energien inklusive aller entsprechenden Vorketten sowie der tatsächlichen Beschaffungstransporte. Weiterhin wurde die gesamte Herstellungsphase abgebildet, inkl. der Behandlung von Produktionsabfällen bis zum Erreichen des End-of-Waste Status (EoW). Ferner wurden sowohl die Distributionstransporte ab Coesfeld / DE (A4) als auch der bei der Installation (A5) entstehende Verpackungsabfall berücksichtigt. Produktverluste sowie Strom verbrauchende Werkzeuge, Hilfsstoffe, und Installationsmaterialen wurden in A5 hingegen nicht berücksichtigt.Module C2-C3 Die Module beinhalten die Umweltwirkungen für die Behandlung der Abfallfraktionen bis zum Erreichen des End-of-Waste Status (EoW) inklusive der zugehörigen Transporte am Ende des Produktlebenswegs.Modul DAusweisung der Lasten und Nutzen des Produktes außerhalb der Systemgrenze. Diese bestehen aus Energie-Gutschriften aus der thermischen Verwertung (C3) in Form vom durchschnittlichen europäischen Strommix bzw. thermischer Energie aus Erdgas.</useAdviceForDataSet>
<useAdviceForDataSet xml:lang="en">Scope: 
This EPD relates to the manufacture, transport, installation, and disposal of an average square metre of Parador resilient floor coverings. The technical characteristics are described in chapter 2.3. The product is manufactured in Coesfeld, Germany. The owner of the declaration is liable for the underlying information and evidence; IBU is not liable for manufacturer information, ecological assessment data, and verification. 
System boundary: 
Type of EPD: Cradle to factory gate with options. Modules A1-3, A4, and A5  The product stage (A1-3) begins with considering the production of the necessary raw materials and energies, including all corresponding upstream chains and the actual procurement transports. Furthermore, the entire manufacturing phase was mapped, including treatment of production waste until end-of-waste status (EoW) was reached. In addition, both the distribution transports from Coesfeld / DE (A4) and the packaging waste generated during installation (A5) were taken into account. Product losses as well as power consuming tools, auxiliary materials, and installation materials were not considered in A5. Modules C2-C3  The modules include the environmental impacts for the treatment of the waste categories until end-of-waste status (EoW) is reached, including the associated transports at the end of the product life cycle. Module DIdentification of the benefits and costs of the product outside the system boundary. These consist of energy credits from thermal utilisation (C3) in the form of the average European electricity mix or thermal energy from natural gas.</useAdviceForDataSet>
<common:other>
<epd2:referenceToOriginalEPD type="source data set" refObjectId="2527dd3d-6e75-491f-b87a-3931e9d6343f">
<common:shortDescription xml:lang="de">Elastische Bodenbeläge.pdf</common:shortDescription>
</epd2:referenceToOriginalEPD>
</common:other>
</dataSourcesTreatmentAndRepresentativeness>
<validation>
<review type="Accredited third party review">
<common:referenceToNameOfReviewerAndInstitution uri="../contacts/d111dbec-b024-4be5-86c5-752d6eb2cf95.xml" type="contact data set" refObjectId="d111dbec-b024-4be5-86c5-752d6eb2cf95">
<common:shortDescription xml:lang="de">Institut Bauen und Umwelt e. V.</common:shortDescription>
</common:referenceToNameOfReviewerAndInstitution>
</review>
</validation>
<complianceDeclarations>
<compliance>
<common:referenceToComplianceSystem uri="../sources/b00f9ec0-7874-11e3-981f-0800200c9a66.xml" type="source data set" refObjectId="b00f9ec0-7874-11e3-981f-0800200c9a66">
<common:shortDescription xml:lang="de">DIN EN 15804</common:shortDescription>
</common:referenceToComplianceSystem>
</compliance>
<compliance>
<common:referenceToComplianceSystem uri="../sources/4f2eb655-6e44-4874-a95a-e28f5442cd4d.xml" type="source data set" refObjectId="4f2eb655-6e44-4874-a95a-e28f5442cd4d">
<common:shortDescription xml:lang="de">ISO 14025</common:shortDescription>
</common:referenceToComplianceSystem>
</compliance>
</complianceDeclarations>
</modellingAndValidation>
<administrativeInformation>
<common:commissionerAndGoal>
<common:referenceToCommissioner uri="../contacts/0861a318-be95-448b-b08e-751d226e2c2c.xml" type="contact data set" refObjectId="0861a318-be95-448b-b08e-751d226e2c2c">
<common:shortDescription xml:lang="de">Parador GmbH</common:shortDescription>
</common:referenceToCommissioner>
</common:commissionerAndGoal>
<dataGenerator>
<common:referenceToPersonOrEntityGeneratingTheDataSet uri="../contacts/6b539b8a-10e3-4004-8ccc-a79f169aa339.xml" type="contact data set" refObjectId="6b539b8a-10e3-4004-8ccc-a79f169aa339">
<common:shortDescription xml:lang="de">brands and values GmbH</common:shortDescription>
</common:referenceToPersonOrEntityGeneratingTheDataSet>
</dataGenerator>
<dataEntryBy>
<common:timeStamp>2019-03-06T14:08:26.971</common:timeStamp>
<common:referenceToDataSetFormat uri="../sources/a97a0155-0234-4b87-b4ce-a45da52f2a40.xml" type="source data set" refObjectId="a97a0155-0234-4b87-b4ce-a45da52f2a40">
<common:shortDescription xml:lang="de">ILCD Format</common:shortDescription>
</common:referenceToDataSetFormat>
<common:referenceToDataSetFormat uri="../sources/a29449fd-aa2f-4de8-b5d7-4b06b43c6fde.xml" type="source data set" refObjectId="a29449fd-aa2f-4de8-b5d7-4b06b43c6fde">
<common:shortDescription xml:lang="de">EPD-Datenformaterweiterungen v1.2</common:shortDescription>
<common:shortDescription xml:lang="en">EPD Data Format Extensions v1.2</common:shortDescription>
</common:referenceToDataSetFormat>
</dataEntryBy>
<publicationAndOwnership>
<common:dataSetVersion>00.04.000</common:dataSetVersion>
<common:referenceToRegistrationAuthority uri="../contacts/d111dbec-b024-4be5-86c5-752d6eb2cf95.xml" type="contact data set" refObjectId="d111dbec-b024-4be5-86c5-752d6eb2cf95">
<common:shortDescription xml:lang="de">Institut Bauen und Umwelt e. V.</common:shortDescription>
</common:referenceToRegistrationAuthority>
<common:registrationNumber>EPD-PAR-20180164-IBC1-DE</common:registrationNumber>
<common:referenceToOwnershipOfDataSet uri="../contacts/0861a318-be95-448b-b08e-751d226e2c2c.xml" type="contact data set" refObjectId="0861a318-be95-448b-b08e-751d226e2c2c">
<common:shortDescription xml:lang="de">Parador GmbH</common:shortDescription>
</common:referenceToOwnershipOfDataSet>
<common:copyright>true</common:copyright>
<common:licenseType>Free of charge for all users and uses</common:licenseType>
<common:accessRestrictions xml:lang="en">None</common:accessRestrictions>
<common:other>
<epd2:referenceToPublisher type="contact data set" refObjectId="d111dbec-b024-4be5-86c5-752d6eb2cf95" uri="../contacts/d111dbec-b024-4be5-86c5-752d6eb2cf95.xml">
<common:shortDescription xml:lang="de">Institut Bauen und Umwelt e. V.</common:shortDescription>
</epd2:referenceToPublisher>
</common:other>
</publicationAndOwnership>
</administrativeInformation>
<exchanges>
<exchange dataSetInternalID="0">
<referenceToFlowDataSet uri="../flows/14b1585f-9a40-0a6b-9908-cf3b7997c917.xml" type="flow data set" refObjectId="14b1585f-9a40-0a6b-9908-cf3b7997c917">
<common:shortDescription xml:lang="de">Elastische Bodenbeläge (Elastische Bodenbeläge)</common:shortDescription>
</referenceToFlowDataSet>
<meanAmount>1</meanAmount>
<referencesToDataSource />
</exchange>
<exchange dataSetInternalID="1">
<referenceToFlowDataSet uri="../flows/20f32be5-0398-4288-9b6d-accddd195317.xml" type="flow data set" refObjectId="20f32be5-0398-4288-9b6d-accddd195317">
<common:shortDescription xml:lang="de">Erneuerbare Primärenergie als Energieträger (PERE)</common:shortDescription>
<common:shortDescription xml:lang="en">Renewable primary energy as energy carrier (PERE)</common:shortDescription>
</referenceToFlowDataSet>
<functionType>General reminder flow</functionType>
<exchangeDirection>Input</exchangeDirection>
<common:other>
<epd:referenceToUnitGroupDataSet uri="../unitgroups/93a60a57-a3c8-11da-a746-0800200c9a66.xml" type="unit group data set" refObjectId="93a60a57-a3c8-11da-a746-0800200c9a66">
<common:shortDescription xml:lang="de">MJ</common:shortDescription>
</epd:referenceToUnitGroupDataSet>
<epd:amount epd:module="A1-A3">-2.74000000000001</epd:amount>
<epd:amount epd:module="A4">0.24942</epd:amount>
<epd:amount epd:module="A5">1.4972209</epd:amount>
<epd:amount epd:module="C2">0.030559</epd:amount>
<epd:amount epd:module="C3">129.74974</epd:amount>
<epd:amount epd:module="D">-11.554</epd:amount>
</common:other>
</exchange>
<exchange dataSetInternalID="2">
<referenceToFlowDataSet uri="../flows/fb3ec0de-548d-4508-aea5-00b73bf6f702.xml" type="flow data set" refObjectId="fb3ec0de-548d-4508-aea5-00b73bf6f702">
<common:shortDescription xml:lang="de">Erneuerbare Primärenergie zur stofflichen Nutzung (PERM)</common:shortDescription>
<common:shortDescription xml:lang="en">Renewable primary energy resources as material utilization (PERM)</common:shortDescription>
</referenceToFlowDataSet>
<functionType>General reminder flow</functionType>
<exchangeDirection>Input</exchangeDirection>
<common:other>
<epd:referenceToUnitGroupDataSet uri="../unitgroups/93a60a57-a3c8-11da-a746-0800200c9a66.xml" type="unit group data set" refObjectId="93a60a57-a3c8-11da-a746-0800200c9a66">
<common:shortDescription xml:lang="de">MJ</common:shortDescription>
</epd:referenceToUnitGroupDataSet>
<epd:amount epd:module="A1-A3">130.8</epd:amount>
<epd:amount epd:module="A4">0</epd:amount>
<epd:amount epd:module="A5">-1.49</epd:amount>
<epd:amount epd:module="C2">0</epd:amount>
<epd:amount epd:module="C3">-129.31</epd:amount>
<epd:amount epd:module="D">0</epd:amount>
</common:other>
</exchange>
<exchange dataSetInternalID="3">
<referenceToFlowDataSet uri="../flows/53f97275-fa8a-4cdd-9024-65936002acd0.xml" type="flow data set" refObjectId="53f97275-fa8a-4cdd-9024-65936002acd0">
<common:shortDescription xml:lang="de">Total erneuerbare Primärenergie (PERT)</common:shortDescription>
<common:shortDescription xml:lang="en">Total use of renewable primary energy resources (PERT)</common:shortDescription>
</referenceToFlowDataSet>
<functionType>General reminder flow</functionType>
<exchangeDirection>Input</exchangeDirection>
<common:other>
<epd:referenceToUnitGroupDataSet uri="../unitgroups/93a60a57-a3c8-11da-a746-0800200c9a66.xml" type="unit group data set" refObjectId="93a60a57-a3c8-11da-a746-0800200c9a66">
<common:shortDescription xml:lang="de">MJ</common:shortDescription>
</epd:referenceToUnitGroupDataSet>
<epd:amount epd:module="A1-A3">128.06</epd:amount>
<epd:amount epd:module="A4">0.24942</epd:amount>
<epd:amount epd:module="A5">0.0072209</epd:amount>
<epd:amount epd:module="C2">0.030559</epd:amount>
<epd:amount epd:module="C3">0.43974</epd:amount>
<epd:amount epd:module="D">-11.554</epd:amount>
</common:other>
</exchange>
<exchange dataSetInternalID="4">
<referenceToFlowDataSet uri="../flows/ac857178-2b45-46ec-892a-a9a4332f0372.xml" type="flow data set" refObjectId="ac857178-2b45-46ec-892a-a9a4332f0372">
<common:shortDescription xml:lang="de">Nicht-erneuerbare Primärenergie als Energieträger (PENRE)</common:shortDescription>
<common:shortDescription xml:lang="en">Non renewable primary energy as energy carrier (PENRE)</common:shortDescription>
</referenceToFlowDataSet>
<functionType>General reminder flow</functionType>
<exchangeDirection>Input</exchangeDirection>
<common:other>
<epd:referenceToUnitGroupDataSet uri="../unitgroups/93a60a57-a3c8-11da-a746-0800200c9a66.xml" type="unit group data set" refObjectId="93a60a57-a3c8-11da-a746-0800200c9a66">
<common:shortDescription xml:lang="de">MJ</common:shortDescription>
</epd:referenceToUnitGroupDataSet>
<epd:amount epd:module="A1-A3">104.45</epd:amount>
<epd:amount epd:module="A4">4.7786</epd:amount>
<epd:amount epd:module="A5">0.521769</epd:amount>
<epd:amount epd:module="C2">0.58548</epd:amount>
<epd:amount epd:module="C3">11.2002</epd:amount>
<epd:amount epd:module="D">-60.087</epd:amount>
</common:other>
</exchange>
<exchange dataSetInternalID="5">
<referenceToFlowDataSet uri="../flows/1421caa0-679d-4bf4-b282-0eb850ccae27.xml" type="flow data set" refObjectId="1421caa0-679d-4bf4-b282-0eb850ccae27">
<common:shortDescription xml:lang="de">Nicht-erneuerbare Primärenergie zur stofflichen Nutzung (PENRM)</common:shortDescription>
<common:shortDescription xml:lang="en">Non renewable primary energy as material utilization (PENRM)</common:shortDescription>
</referenceToFlowDataSet>
<functionType>General reminder flow</functionType>
<exchangeDirection>Input</exchangeDirection>
<common:other>
<epd:referenceToUnitGroupDataSet uri="../unitgroups/93a60a57-a3c8-11da-a746-0800200c9a66.xml" type="unit group data set" refObjectId="93a60a57-a3c8-11da-a746-0800200c9a66">
<common:shortDescription xml:lang="de">MJ</common:shortDescription>
</epd:referenceToUnitGroupDataSet>
<epd:amount epd:module="A1-A3">8.37</epd:amount>
<epd:amount epd:module="A4">0</epd:amount>
<epd:amount epd:module="A5">-0.47</epd:amount>
<epd:amount epd:module="C2">0</epd:amount>
<epd:amount epd:module="C3">-7.9</epd:amount>
<epd:amount epd:module="D">0</epd:amount>
</common:other>
</exchange>
<exchange dataSetInternalID="6">
<referenceToFlowDataSet uri="../flows/06159210-646b-4c8d-8583-da9b3b95a6c1.xml" type="flow data set" refObjectId="06159210-646b-4c8d-8583-da9b3b95a6c1">
<common:shortDescription xml:lang="de">Total nicht erneuerbare Primärenergie (PENRT)</common:shortDescription>
<common:shortDescription xml:lang="en">Total use of non renewable primary energy resources (PENRT)</common:shortDescription>
</referenceToFlowDataSet>
<functionType>General reminder flow</functionType>
<exchangeDirection>Input</exchangeDirection>
<common:other>
<epd:referenceToUnitGroupDataSet uri="../unitgroups/93a60a57-a3c8-11da-a746-0800200c9a66.xml" type="unit group data set" refObjectId="93a60a57-a3c8-11da-a746-0800200c9a66">
<common:shortDescription xml:lang="de">MJ</common:shortDescription>
</epd:referenceToUnitGroupDataSet>
<epd:amount epd:module="A1-A3">112.82</epd:amount>
<epd:amount epd:module="A4">4.7786</epd:amount>
<epd:amount epd:module="A5">0.051769</epd:amount>
<epd:amount epd:module="C2">0.58548</epd:amount>
<epd:amount epd:module="C3">3.3002</epd:amount>
<epd:amount epd:module="D">-60.087</epd:amount>
</common:other>
</exchange>
<exchange dataSetInternalID="7">
<referenceToFlowDataSet uri="../flows/c6a1f35f-2d09-4f54-8dfb-97e502e1ce92.xml" type="flow data set" refObjectId="c6a1f35f-2d09-4f54-8dfb-97e502e1ce92">
<common:shortDescription xml:lang="de">Einsatz von Sekundärstoffen (SM)</common:shortDescription>
<common:shortDescription xml:lang="en">Use of secondary material (SM)</common:shortDescription>
</referenceToFlowDataSet>
<functionType>General reminder flow</functionType>
<exchangeDirection>Input</exchangeDirection>
<common:other>
<epd:referenceToUnitGroupDataSet uri="../unitgroups/ad38d542-3fe9-439d-9b95-2f5f7752acaf.xml" type="unit group data set" refObjectId="ad38d542-3fe9-439d-9b95-2f5f7752acaf">
<common:shortDescription xml:lang="de">kg</common:shortDescription>
</epd:referenceToUnitGroupDataSet>
<epd:amount epd:module="A1-A3">6.419</epd:amount>
<epd:amount epd:module="A4">0</epd:amount>
<epd:amount epd:module="A5">0</epd:amount>
<epd:amount epd:module="C2">0</epd:amount>
<epd:amount epd:module="C3">0</epd:amount>
<epd:amount epd:module="D">0</epd:amount>
</common:other>
</exchange>
<exchange dataSetInternalID="8">
<referenceToFlowDataSet uri="../flows/64333088-a55f-4aa2-9a31-c10b07816787.xml" type="flow data set" refObjectId="64333088-a55f-4aa2-9a31-c10b07816787">
<common:shortDescription xml:lang="de">Erneuerbare Sekundärbrennstoffe (RSF)</common:shortDescription>
<common:shortDescription xml:lang="en">Use of renewable secondary fuels (RSF)</common:shortDescription>
</referenceToFlowDataSet>
<functionType>General reminder flow</functionType>
<exchangeDirection>Input</exchangeDirection>
<common:other>
<epd:referenceToUnitGroupDataSet uri="../unitgroups/93a60a57-a3c8-11da-a746-0800200c9a66.xml" type="unit group data set" refObjectId="93a60a57-a3c8-11da-a746-0800200c9a66">
<common:shortDescription xml:lang="de">MJ</common:shortDescription>
</epd:referenceToUnitGroupDataSet>
<epd:amount epd:module="A1-A3">0</epd:amount>
<epd:amount epd:module="A4">0</epd:amount>
<epd:amount epd:module="A5">0</epd:amount>
<epd:amount epd:module="C2">0</epd:amount>
<epd:amount epd:module="C3">0</epd:amount>
<epd:amount epd:module="D">0</epd:amount>
</common:other>
</exchange>
<exchange dataSetInternalID="9">
<referenceToFlowDataSet uri="../flows/89def144-d39a-4287-b86f-efde453ddcb2.xml" type="flow data set" refObjectId="89def144-d39a-4287-b86f-efde453ddcb2">
<common:shortDescription xml:lang="de">Nicht erneuerbare Sekundärbrennstoffe (NRSF)</common:shortDescription>
<common:shortDescription xml:lang="en">Use of non renewable secondary fuels (NRSF)</common:shortDescription>
</referenceToFlowDataSet>
<functionType>General reminder flow</functionType>
<exchangeDirection>Input</exchangeDirection>
<common:other>
<epd:referenceToUnitGroupDataSet uri="../unitgroups/93a60a57-a3c8-11da-a746-0800200c9a66.xml" type="unit group data set" refObjectId="93a60a57-a3c8-11da-a746-0800200c9a66">
<common:shortDescription xml:lang="de">MJ</common:shortDescription>
</epd:referenceToUnitGroupDataSet>
<epd:amount epd:module="A1-A3">0</epd:amount>
<epd:amount epd:module="A4">0</epd:amount>
<epd:amount epd:module="A5">0</epd:amount>
<epd:amount epd:module="C2">0</epd:amount>
<epd:amount epd:module="C3">0</epd:amount>
<epd:amount epd:module="D">0</epd:amount>
</common:other>
</exchange>
<exchange dataSetInternalID="10">
<referenceToFlowDataSet uri="../flows/3cf952c8-f3a4-461d-8c96-96456ca62246.xml" type="flow data set" refObjectId="3cf952c8-f3a4-461d-8c96-96456ca62246">
<common:shortDescription xml:lang="de">Einsatz von Süßwasserressourcen (FW)</common:shortDescription>
<common:shortDescription xml:lang="en">Use of net fresh water (FW)</common:shortDescription>
</referenceToFlowDataSet>
<functionType>General reminder flow</functionType>
<exchangeDirection>Input</exchangeDirection>
<common:other>
<epd:referenceToUnitGroupDataSet uri="../unitgroups/cd950537-0a98-4044-9ba7-9f9a68d0a504.xml" type="unit group data set" refObjectId="cd950537-0a98-4044-9ba7-9f9a68d0a504">
<common:shortDescription xml:lang="de">m^3</common:shortDescription>
</epd:referenceToUnitGroupDataSet>
<epd:amount epd:module="A1-A3">0.4732</epd:amount>
<epd:amount epd:module="A4">0.00045932</epd:amount>
<epd:amount epd:module="A5">0.00044279</epd:amount>
<epd:amount epd:module="C2">5.6277E-05</epd:amount>
<epd:amount epd:module="C3">0.027183</epd:amount>
<epd:amount epd:module="D">-0.015752</epd:amount>
</common:other>
</exchange>
<exchange dataSetInternalID="11">
<referenceToFlowDataSet uri="../flows/430f9e0f-59b2-46a0-8e0d-55e0e84948fc.xml" type="flow data set" refObjectId="430f9e0f-59b2-46a0-8e0d-55e0e84948fc">
<common:shortDescription xml:lang="de">Gefährlicher Abfall zur Deponie (HWD)</common:shortDescription>
<common:shortDescription xml:lang="en">Hazardous waste disposed (HWD)</common:shortDescription>
</referenceToFlowDataSet>
<functionType>General reminder flow</functionType>
<exchangeDirection>Output</exchangeDirection>
<common:other>
<epd:referenceToUnitGroupDataSet uri="../unitgroups/ad38d542-3fe9-439d-9b95-2f5f7752acaf.xml" type="unit group data set" refObjectId="ad38d542-3fe9-439d-9b95-2f5f7752acaf">
<common:shortDescription xml:lang="de">kg</common:shortDescription>
</epd:referenceToUnitGroupDataSet>
<epd:amount epd:module="A1-A3">1.4838E-06</epd:amount>
<epd:amount epd:module="A4">2.5197E-07</epd:amount>
<epd:amount epd:module="A5">5.4291E-10</epd:amount>
<epd:amount epd:module="C2">3.0872E-08</epd:amount>
<epd:amount epd:module="C3">6.5804E-08</epd:amount>
<epd:amount epd:module="D">-2.4469E-08</epd:amount>
</common:other>
</exchange>
<exchange dataSetInternalID="12">
<referenceToFlowDataSet uri="../flows/b29ef66b-e286-4afa-949f-62f1a7b4d7fa.xml" type="flow data set" refObjectId="b29ef66b-e286-4afa-949f-62f1a7b4d7fa">
<common:shortDescription xml:lang="de">Entsorgter nicht gefährlicher Abfall (NHWD)</common:shortDescription>
<common:shortDescription xml:lang="en">Non hazardous waste disposed (NHWD)</common:shortDescription>
</referenceToFlowDataSet>
<functionType>General reminder flow</functionType>
<exchangeDirection>Output</exchangeDirection>
<common:other>
<epd:referenceToUnitGroupDataSet uri="../unitgroups/ad38d542-3fe9-439d-9b95-2f5f7752acaf.xml" type="unit group data set" refObjectId="ad38d542-3fe9-439d-9b95-2f5f7752acaf">
<common:shortDescription xml:lang="de">kg</common:shortDescription>
</epd:referenceToUnitGroupDataSet>
<epd:amount epd:module="A1-A3">0.069436</epd:amount>
<epd:amount epd:module="A4">0.00038375</epd:amount>
<epd:amount epd:module="A5">0.0031632</epd:amount>
<epd:amount epd:module="C2">4.7019E-05</epd:amount>
<epd:amount epd:module="C3">0.048355</epd:amount>
<epd:amount epd:module="D">-0.025703</epd:amount>
</common:other>
</exchange>
<exchange dataSetInternalID="13">
<referenceToFlowDataSet uri="../flows/3449546e-52ad-4b39-b809-9fb77cea8ff6.xml" type="flow data set" refObjectId="3449546e-52ad-4b39-b809-9fb77cea8ff6">
<common:shortDescription xml:lang="de">Entsorgter radioaktiver Abfall (RWD)</common:shortDescription>
<common:shortDescription xml:lang="en">Radioactive waste disposed (RWD)</common:shortDescription>
</referenceToFlowDataSet>
<functionType>General reminder flow</functionType>
<exchangeDirection>Output</exchangeDirection>
<common:other>
<epd:referenceToUnitGroupDataSet uri="../unitgroups/ad38d542-3fe9-439d-9b95-2f5f7752acaf.xml" type="unit group data set" refObjectId="ad38d542-3fe9-439d-9b95-2f5f7752acaf">
<common:shortDescription xml:lang="de">kg</common:shortDescription>
</epd:referenceToUnitGroupDataSet>
<epd:amount epd:module="A1-A3">0.0053041</epd:amount>
<epd:amount epd:module="A4">9.9847E-06</epd:amount>
<epd:amount epd:module="A5">2.6707E-06</epd:amount>
<epd:amount epd:module="C2">1.2234E-06</epd:amount>
<epd:amount epd:module="C3">0.00017339</epd:amount>
<epd:amount epd:module="D">-0.0050791</epd:amount>
</common:other>
</exchange>
<exchange dataSetInternalID="14">
<referenceToFlowDataSet uri="../flows/a2b32f97-3fc7-4af2-b209-525bc6426f33.xml" type="flow data set" refObjectId="a2b32f97-3fc7-4af2-b209-525bc6426f33">
<common:shortDescription xml:lang="de">Komponenten für die Wiederverwendung (CRU)</common:shortDescription>
<common:shortDescription xml:lang="en">Components for re-use (CRU)</common:shortDescription>
</referenceToFlowDataSet>
<functionType>General reminder flow</functionType>
<exchangeDirection>Output</exchangeDirection>
<common:other>
<epd:referenceToUnitGroupDataSet uri="../unitgroups/ad38d542-3fe9-439d-9b95-2f5f7752acaf.xml" type="unit group data set" refObjectId="ad38d542-3fe9-439d-9b95-2f5f7752acaf">
<common:shortDescription xml:lang="de">kg</common:shortDescription>
</epd:referenceToUnitGroupDataSet>
<epd:amount epd:module="A1-A3">0</epd:amount>
<epd:amount epd:module="A4">0</epd:amount>
<epd:amount epd:module="A5">0</epd:amount>
<epd:amount epd:module="C2">0</epd:amount>
<epd:amount epd:module="C3">0</epd:amount>
<epd:amount epd:module="D">0</epd:amount>
</common:other>
</exchange>
<exchange dataSetInternalID="15">
<referenceToFlowDataSet uri="../flows/d7fe48a5-4103-49c8-9aae-b0b5dfdbd6ae.xml" type="flow data set" refObjectId="d7fe48a5-4103-49c8-9aae-b0b5dfdbd6ae">
<common:shortDescription xml:lang="de">Stoffe zum Recycling (MFR)</common:shortDescription>
<common:shortDescription xml:lang="en">Materials for recycling (MFR)</common:shortDescription>
</referenceToFlowDataSet>
<functionType>General reminder flow</functionType>
<exchangeDirection>Output</exchangeDirection>
<common:other>
<epd:referenceToUnitGroupDataSet uri="../unitgroups/ad38d542-3fe9-439d-9b95-2f5f7752acaf.xml" type="unit group data set" refObjectId="ad38d542-3fe9-439d-9b95-2f5f7752acaf">
<common:shortDescription xml:lang="de">kg</common:shortDescription>
</epd:referenceToUnitGroupDataSet>
<epd:amount epd:module="A1-A3">0</epd:amount>
<epd:amount epd:module="A4">0</epd:amount>
<epd:amount epd:module="A5">0</epd:amount>
<epd:amount epd:module="C2">0</epd:amount>
<epd:amount epd:module="C3">0</epd:amount>
<epd:amount epd:module="D">0</epd:amount>
</common:other>
</exchange>
<exchange dataSetInternalID="16">
<referenceToFlowDataSet uri="../flows/59a9181c-3aaf-46ee-8b13-2b3723b6e447.xml" type="flow data set" refObjectId="59a9181c-3aaf-46ee-8b13-2b3723b6e447">
<common:shortDescription xml:lang="de">Stoffe für die Energierückgewinnung (MER)</common:shortDescription>
<common:shortDescription xml:lang="en">Materials for energy recovery (MER)</common:shortDescription>
</referenceToFlowDataSet>
<functionType>General reminder flow</functionType>
<exchangeDirection>Output</exchangeDirection>
<common:other>
<epd:referenceToUnitGroupDataSet uri="../unitgroups/ad38d542-3fe9-439d-9b95-2f5f7752acaf.xml" type="unit group data set" refObjectId="ad38d542-3fe9-439d-9b95-2f5f7752acaf">
<common:shortDescription xml:lang="de">kg</common:shortDescription>
</epd:referenceToUnitGroupDataSet>
<epd:amount epd:module="A1-A3">0</epd:amount>
<epd:amount epd:module="A4">0</epd:amount>
<epd:amount epd:module="A5">0</epd:amount>
<epd:amount epd:module="C2">0</epd:amount>
<epd:amount epd:module="C3">0</epd:amount>
<epd:amount epd:module="D">0</epd:amount>
</common:other>
</exchange>
<exchange dataSetInternalID="17">
<referenceToFlowDataSet uri="../flows/4da0c987-2b76-40d6-9e9e-82a017aaaf29.xml" type="flow data set" refObjectId="4da0c987-2b76-40d6-9e9e-82a017aaaf29">
<common:shortDescription xml:lang="de">Exportierte elektrische Energie (EEE)</common:shortDescription>
<common:shortDescription xml:lang="en">Exported electrical energy (EEE)</common:shortDescription>
</referenceToFlowDataSet>
<functionType>General reminder flow</functionType>
<exchangeDirection>Output</exchangeDirection>
<common:other>
<epd:referenceToUnitGroupDataSet uri="../unitgroups/93a60a57-a3c8-11da-a746-0800200c9a66.xml" type="unit group data set" refObjectId="93a60a57-a3c8-11da-a746-0800200c9a66">
<common:shortDescription xml:lang="de">MJ</common:shortDescription>
</epd:referenceToUnitGroupDataSet>
<epd:amount epd:module="A1-A3">0</epd:amount>
<epd:amount epd:module="A4">0</epd:amount>
<epd:amount epd:module="A5">0.27</epd:amount>
<epd:amount epd:module="C2">0</epd:amount>
<epd:amount epd:module="C3">14.27</epd:amount>
<epd:amount epd:module="D">0</epd:amount>
</common:other>
</exchange>
<exchange dataSetInternalID="18">
<referenceToFlowDataSet uri="../flows/98daf38a-7a79-46d3-9a37-2b7bd0955810.xml" type="flow data set" refObjectId="98daf38a-7a79-46d3-9a37-2b7bd0955810">
<common:shortDescription xml:lang="de">Exportierte thermische Energie (EET)</common:shortDescription>
<common:shortDescription xml:lang="en">Exported thermal energy (EET)</common:shortDescription>
</referenceToFlowDataSet>
<functionType>General reminder flow</functionType>
<exchangeDirection>Output</exchangeDirection>
<common:other>
<epd:referenceToUnitGroupDataSet uri="../unitgroups/93a60a57-a3c8-11da-a746-0800200c9a66.xml" type="unit group data set" refObjectId="93a60a57-a3c8-11da-a746-0800200c9a66">
<common:shortDescription xml:lang="de">MJ</common:shortDescription>
</epd:referenceToUnitGroupDataSet>
<epd:amount epd:module="A1-A3">0.66</epd:amount>
<epd:amount epd:module="A4">0</epd:amount>
<epd:amount epd:module="A5">0.48</epd:amount>
<epd:amount epd:module="C2">0</epd:amount>
<epd:amount epd:module="C3">26.03</epd:amount>
<epd:amount epd:module="D">0</epd:amount>
</common:other>
</exchange>
</exchanges>
<LCIAResults>
<LCIAResult>
<referenceToLCIAMethodDataSet uri="../lciamethods/77e416eb-a363-4258-a04e-171d843a6460.xml" type="LCIA method data set" refObjectId="77e416eb-a363-4258-a04e-171d843a6460">
<common:shortDescription xml:lang="de">Globales Erwärmungspotenzial (GWP)</common:shortDescription>
<common:shortDescription xml:lang="en">Global warming potential (GWP)</common:shortDescription>
</referenceToLCIAMethodDataSet>
<common:other>
<epd:referenceToUnitGroupDataSet uri="../unitgroups/1ebf3012-d0db-4de2-aefd-ef30cedb0be1.xml" type="unit group data set" refObjectId="1ebf3012-d0db-4de2-aefd-ef30cedb0be1">
<common:shortDescription xml:lang="de">kg CO_(2)-Äq.</common:shortDescription>
</epd:referenceToUnitGroupDataSet>
<epd:amount epd:module="A1-A3">-4.3791</epd:amount>
<epd:amount epd:module="A4">0.35069</epd:amount>
<epd:amount epd:module="A5">0.16138</epd:amount>
<epd:amount epd:module="C2">0.04281</epd:amount>
<epd:amount epd:module="C3">11.882</epd:amount>
<epd:amount epd:module="D">-3.4329</epd:amount>
</common:other>
</LCIAResult>
<LCIAResult>
<referenceToLCIAMethodDataSet uri="../lciamethods/06dcd26f-025f-401a-a7c1-5e457eb54637.xml" type="LCIA method data set" refObjectId="06dcd26f-025f-401a-a7c1-5e457eb54637">
<common:shortDescription xml:lang="de">Abbau Potential der stratosphärischen Ozonschicht (ODP)</common:shortDescription>
<common:shortDescription xml:lang="en">Depletion potential of the stratospheric ozone layer (ODP)</common:shortDescription>
</referenceToLCIAMethodDataSet>
<common:other>
<epd:referenceToUnitGroupDataSet uri="../unitgroups/88054749-b0a6-47ea-a82b-dc5b29326512.xml" type="unit group data set" refObjectId="88054749-b0a6-47ea-a82b-dc5b29326512">
<common:shortDescription xml:lang="de">kg CFC11-Äq.</common:shortDescription>
</epd:referenceToUnitGroupDataSet>
<epd:amount epd:module="A1-A3">3.5488E-07</epd:amount>
<epd:amount epd:module="A4">1.453E-14</epd:amount>
<epd:amount epd:module="A5">3.8231E-15</epd:amount>
<epd:amount epd:module="C2">1.7803E-15</epd:amount>
<epd:amount epd:module="C3">4.4672E-11</epd:amount>
<epd:amount epd:module="D">-7.451E-12</epd:amount>
</common:other>
</LCIAResult>
<LCIAResult>
<referenceToLCIAMethodDataSet uri="../lciamethods/b4274add-93b7-4905-a5e4-2e878c4e4216.xml" type="LCIA method data set" refObjectId="b4274add-93b7-4905-a5e4-2e878c4e4216">
<common:shortDescription xml:lang="de">Versauerungspotenzial von Boden und Wasser (AP)</common:shortDescription>
<common:shortDescription xml:lang="en">Acidification potential of land and water (AP)</common:shortDescription>
</referenceToLCIAMethodDataSet>
<common:other>
<epd:referenceToUnitGroupDataSet uri="../unitgroups/bc50c624-a9bc-45b1-a9b0-e6b10d00476f.xml" type="unit group data set" refObjectId="bc50c624-a9bc-45b1-a9b0-e6b10d00476f">
<common:shortDescription xml:lang="de">kg SO_(2)-Äq.</common:shortDescription>
</epd:referenceToUnitGroupDataSet>
<epd:amount epd:module="A1-A3">0.018477</epd:amount>
<epd:amount epd:module="A4">0.0008531</epd:amount>
<epd:amount epd:module="A5">2.9733E-05</epd:amount>
<epd:amount epd:module="C2">0.00011126</epd:amount>
<epd:amount epd:module="C3">0.0038286</epd:amount>
<epd:amount epd:module="D">-0.005764</epd:amount>
</common:other>
</LCIAResult>
<LCIAResult>
<referenceToLCIAMethodDataSet uri="../lciamethods/f58827d0-b407-4ec6-be75-8b69efb98a0f.xml" type="LCIA method data set" refObjectId="f58827d0-b407-4ec6-be75-8b69efb98a0f">
<common:shortDescription xml:lang="de">Eutrophierungspotenzial (EP)</common:shortDescription>
<common:shortDescription xml:lang="en">Eutrophication potential (EP)</common:shortDescription>
</referenceToLCIAMethodDataSet>
<common:other>
<epd:referenceToUnitGroupDataSet uri="../unitgroups/67b5401d-873c-485f-bcf3-6ae83b918822.xml" type="unit group data set" refObjectId="67b5401d-873c-485f-bcf3-6ae83b918822">
<common:shortDescription xml:lang="de">kg PO_(4)^(3)-Äq.</common:shortDescription>
</epd:referenceToUnitGroupDataSet>
<epd:amount epd:module="A1-A3">0.0064704</epd:amount>
<epd:amount epd:module="A4">0.0002153</epd:amount>
<epd:amount epd:module="A5">5.8079E-06</epd:amount>
<epd:amount epd:module="C2">2.8006E-05</epd:amount>
<epd:amount epd:module="C3">0.00094626</epd:amount>
<epd:amount epd:module="D">-0.00062359</epd:amount>
</common:other>
</LCIAResult>
<LCIAResult>
<referenceToLCIAMethodDataSet uri="../lciamethods/1e84a202-dae6-42aa-9e9d-71ea48b8be00.xml" type="LCIA method data set" refObjectId="1e84a202-dae6-42aa-9e9d-71ea48b8be00">
<common:shortDescription xml:lang="de">Bildungspotential für troposphärisches Ozon (POCP)</common:shortDescription>
<common:shortDescription xml:lang="en">Formation potential of tropospheric ozone photochemical oxidants (POCP)</common:shortDescription>
</referenceToLCIAMethodDataSet>
<common:other>
<epd:referenceToUnitGroupDataSet uri="../unitgroups/01c26c17-9a76-406e-8295-f17b55fd909e.xml" type="unit group data set" refObjectId="01c26c17-9a76-406e-8295-f17b55fd909e">
<common:shortDescription xml:lang="de">kg Ethen-Äq.</common:shortDescription>
</epd:referenceToUnitGroupDataSet>
<epd:amount epd:module="A1-A3">0.0044306</epd:amount>
<epd:amount epd:module="A4">-0.00028967</epd:amount>
<epd:amount epd:module="A5">1.3197E-06</epd:amount>
<epd:amount epd:module="C2">-3.8955E-05</epd:amount>
<epd:amount epd:module="C3">0.00024333</epd:amount>
<epd:amount epd:module="D">-0.00045177</epd:amount>
</common:other>
</LCIAResult>
<LCIAResult>
<referenceToLCIAMethodDataSet uri="../lciamethods/f7c73bb9-ab1a-4249-9c6d-379a0de6f67e.xml" type="LCIA method data set" refObjectId="f7c73bb9-ab1a-4249-9c6d-379a0de6f67e">
<common:shortDescription xml:lang="de">Potenzial für den abiotischen Abbau nicht fossiler Ressourcen (ADPE)</common:shortDescription>
<common:shortDescription xml:lang="en">Abiotic depletion potential for non fossil resources (ADPE)</common:shortDescription>
</referenceToLCIAMethodDataSet>
<common:other>
<epd:referenceToUnitGroupDataSet uri="../unitgroups/54ccd2d9-a32a-4fc2-923d-f2c8c93e89d4.xml" type="unit group data set" refObjectId="54ccd2d9-a32a-4fc2-923d-f2c8c93e89d4">
<common:shortDescription xml:lang="de">kg Sb-Äq.</common:shortDescription>
</epd:referenceToUnitGroupDataSet>
<epd:amount epd:module="A1-A3">1.0903E-05</epd:amount>
<epd:amount epd:module="A4">3.096E-08</epd:amount>
<epd:amount epd:module="A5">2.8032E-09</epd:amount>
<epd:amount epd:module="C2">3.7933E-09</epd:amount>
<epd:amount epd:module="C3">1.4204E-07</epd:amount>
<epd:amount epd:module="D">-9.694E-07</epd:amount>
</common:other>
</LCIAResult>
<LCIAResult>
<referenceToLCIAMethodDataSet uri="../lciamethods/804ebcdf-309d-4098-8ed8-fdaf2f389981.xml" type="LCIA method data set" refObjectId="804ebcdf-309d-4098-8ed8-fdaf2f389981">
<common:shortDescription xml:lang="de">Potenzial für den abiotischen Abbau fossiler Brennstoffe (ADPF)</common:shortDescription>
<common:shortDescription xml:lang="en">Abiotic depletion potential for fossil resources (ADPF)</common:shortDescription>
</referenceToLCIAMethodDataSet>
<common:other>
<epd:referenceToUnitGroupDataSet uri="../unitgroups/93a60a57-a3c8-11da-a746-0800200c9a66.xml" type="unit group data set" refObjectId="93a60a57-a3c8-11da-a746-0800200c9a66">
<common:shortDescription xml:lang="de">MJ</common:shortDescription>
</epd:referenceToUnitGroupDataSet>
<epd:amount epd:module="A1-A3">93.89</epd:amount>
<epd:amount epd:module="A4">4.7531</epd:amount>
<epd:amount epd:module="A5">0.045036</epd:amount>
<epd:amount epd:module="C2">0.58236</epd:amount>
<epd:amount epd:module="C3">2.8627</epd:amount>
<epd:amount epd:module="D">-47.286</epd:amount>
</common:other>
</LCIAResult>
</LCIAResults>
</processDataSet>