<?xml version="1.0" encoding="utf-8"?>
<?xml-stylesheet version="1.0" href="../../stylesheets/epd2html.xsl" type="text/xsl"?>
<processDataSet xmlns="http://lca.jrc.it/ILCD/Process" xmlns:common="http://lca.jrc.it/ILCD/Common" xmlns:epd="http://www.iai.kit.edu/EPD/2013" xmlns:epd2="http://www.indata.network/EPD/2019" xmlns:xsi="http://www.w3.org/2001/XMLSchema-instance" xsi:schemaLocation="http://lca.jrc.it/ILCD/Process ../../schemas/EPD_DataSet.xsd" locations="../ILCDLocations.xml" epd2:epd-version="1.2" version="1.1">
  <processInformation>
    <dataSetInformation>
      <common:UUID>e9920105-0f1a-4452-9a08-47289dc04116</common:UUID>
      <name>
        <baseName xml:lang="en">Anodization of aluminium</baseName>
        <baseName xml:lang="de">Eloxieren von Aluminiumblech</baseName>
        <functionalUnitFlowProperties xml:lang="en">aluminium anodizing</functionalUnitFlowProperties>
      </name>
      <classificationInformation>
        <common:classification name="oekobau.dat">
          <common:class level="0" classId="4">Metalle</common:class>
          <common:class level="1" classId="4.7">Oberflächenbehandlung und Beschichtung von Metallen</common:class>
          <common:class level="2" classId="4.7.01">Anodisieren von Aluminium</common:class>
        </common:classification>
      </classificationInformation>
      <common:generalComment xml:lang="en">This data set has been modeled according to the European Standard EN 15804+A2 for Sustainable Building. Results are depicted in modules that allow the structured expression of results over the entire life cycle.</common:generalComment>
      <common:generalComment xml:lang="de">Dieser Datensatz wurde nach dem European Standard EN 15804+A2 für Nachhaltiges Bauen modelliert. Ergebnisse werden in Modulen abgebildet, die den strukturierten Ausdruck von Ergebnissen über den gesamten Lebenszyklus zulassen.</common:generalComment>
      <common:other>
        <epd:safetyMargins>
          <epd:margins>10</epd:margins>
          <epd:description xml:lang="en">Product system almost completely covered. Good technological, temporal and geographic representativeness.</epd:description>
          <epd:description xml:lang="de">Produktsystem weitgehend vollständig abgebildet. Gute technologische, zeitliche und geographische Repräsentativität.</epd:description>
        </epd:safetyMargins>
      </common:other>
    </dataSetInformation>
    <quantitativeReference type="Reference flow(s)">
      <referenceToReferenceFlow>107429</referenceToReferenceFlow>
    </quantitativeReference>
    <time>
      <common:referenceYear>2021</common:referenceYear>
      <common:dataSetValidUntil>2022</common:dataSetValidUntil>
      <common:timeRepresentativenessDescription xml:lang="en">Annual average</common:timeRepresentativenessDescription>
      <common:timeRepresentativenessDescription xml:lang="de">Jährlicher Durchschnitt</common:timeRepresentativenessDescription>
    </time>
    <geography>
      <locationOfOperationSupplyOrProduction location="DE">
        <descriptionOfRestrictions xml:lang="en">The data set represents the country specific situation in Germany, focusing on the main technologies, the region specific characteristics and / or import statistics.</descriptionOfRestrictions>
        <descriptionOfRestrictions xml:lang="de">Der Datensatz bildet die länderspezifische Situation in Deutschland ab. Dabei werden Haupttechnologien, spezifische regionale Charakteristiken und ggf. Importstatistiken berücksichtigt.</descriptionOfRestrictions>
      </locationOfOperationSupplyOrProduction>
    </geography>
    <technology>
      <technologyDescriptionAndIncludedProcesses xml:lang="en">The dataset includes the process of anodizing of a 2 square meters aluminium profile. Not included is the production of the aluminium extrusion profile, which should be calculated separately. Anodizing is an electrolytic passivation process which increases the thickness of a natural oxide layer on surface of a metal part. The metal is cleaned with a cleaning agent and etched with sodium hydroxides or acids. To grow the aluminium, an electrolysis takes place. Direct current is passed through an electrolytic solution, the aluminium serves as an anode. The cathode consists of carbon, lead, nickel, stainless or other material which is unreactive during the electrolysis. The cathode produces hydrogen, the aluminium anode oxygen forming aluminium oxide. The electrolytic solution chosen depends on which kind of oxide layer has to be produced. Barrier oxide is grown in almost neutral solutions where aluminium oxide is hardly soluble, porous oxide in acidic solutions in which the oxide can also be dissolved. The most widely used solution is dilute sulphuric acid.</technologyDescriptionAndIncludedProcesses>
      <technologyDescriptionAndIncludedProcesses xml:lang="de">Der Datenbestand umfasst den Prozess der Eloxierung eines 2 Quadratmeter großen Aluminiumprofils. Nicht eingeschlossen ist die Herstellung des Aluminium- Strangpressprofils, die separat berechnet werden sollte. Eloxieren ist ein elektrolytisches Passivierungsverfahren, das die Dicke einer natürlichen Oxidschicht auf der Oberfläche eines Metallteils erhöht. Das Metall wird mit einem Reinigungsmittel gereinigt und mit Natriumhydroxid oder Säuren geätzt. Um das Aluminium wachsen zu lassen, findet eine Elektrolyse statt. Gleichstrom wird durch eine elektrolytische Lösung geleitet, das Aluminium dient als Anode. Die Kathode besteht aus Kohlenstoff, Blei, Nickel, rostfreiem Stahl oder anderen Materialien, die während der Elektrolyse nicht reaktiv sind. Die Kathode produziert Wasserstoff, die Aluminiumanoden Sauerstoff bildendes Aluminiumoxid. Die Wahl der Elektrolytlösung hängt davon ab, welche Art von Oxidschicht erzeugt werden soll. Eine oxydische Sperrschicht wächst in fast neutralen Lösungen an, wo Aluminiumoxid kaum löslich ist, poröses Oxid in sauren Lösungen, in denen das Oxid auch gelöst werden kann. Die am weitesten verbreitete Lösung ist verdünnte Schwefelsäure.</technologyDescriptionAndIncludedProcesses>
      <technologicalApplicability xml:lang="en">This product can be used in construction.</technologicalApplicability>
      <technologicalApplicability xml:lang="de">Dieses Produkt kann im Baubereich verwendet werden.</technologicalApplicability>
      <referenceToTechnologyFlowDiagrammOrPicture refObjectId="109ad646-3ef6-4a09-b071-a77f6969f670" version="21.01.000" type="source data set" uri="../sources/109ad646-3ef6-4a09-b071-a77f6969f670.xml">
        <common:shortDescription xml:lang="en">construction_de_aluminium sheet anodised.jpg</common:shortDescription>
      </referenceToTechnologyFlowDiagrammOrPicture>
    </technology>
  </processInformation>
  <modellingAndValidation>
    <LCIMethodAndAllocation>
      <typeOfDataSet>EPD</typeOfDataSet>
      <common:other>
        <epd:subType>generic dataset</epd:subType>
      </common:other>
    </LCIMethodAndAllocation>
    <dataSourcesTreatmentAndRepresentativeness>
      <referenceToDataSource refObjectId="afde213e-7582-4c88-a6bd-318de5d1c36f" version="21.01.000" type="source data set" uri="../sources/afde213e-7582-4c88-a6bd-318de5d1c36f.xml">
        <common:shortDescription xml:lang="en">IBU-Declaration DBC/IVK/VdL; Dispersion based façade paint (EPD-DIV-20140152-IBG1-DE), 2014</common:shortDescription>
      </referenceToDataSource>
      <referenceToDataSource refObjectId="036f89bf-c411-4cec-bc63-6488d4c95943" version="21.01.000" type="source data set" uri="../sources/036f89bf-c411-4cec-bc63-6488d4c95943.xml">
        <common:shortDescription xml:lang="en">IBU-Declaration DBC/IVK/VdL; Reactive resin EP, aqueous/unfilled (EPD-DIV-2012121-E), 2012</common:shortDescription>
      </referenceToDataSource>
      <referenceToDataSource refObjectId="e3bd9bbf-2c3c-42aa-8892-fd13f1065ca5" version="21.01.000" type="source data set" uri="../sources/e3bd9bbf-2c3c-42aa-8892-fd13f1065ca5.xml">
        <common:shortDescription xml:lang="en">Documentation of data quality management</common:shortDescription>
      </referenceToDataSource>
      <referenceToDataSource refObjectId="1cece811-7501-44d4-8067-9259bd5cb835" version="00.01.000" type="source data set" uri="../sources/1cece811-7501-44d4-8067-9259bd5cb835.xml">
        <common:shortDescription xml:lang="en">GaBi Database Edition 2021, CUP2021.01</common:shortDescription>
      </referenceToDataSource>
      <referenceToDataSource refObjectId="28d74cc0-db8b-4d7e-bc44-5f6d56ce0c4a" version="00.03.002" type="source data set" uri="../sources/28d74cc0-db8b-4d7e-bc44-5f6d56ce0c4a.xml">
        <common:shortDescription xml:lang="en">GaBi database (all versions)</common:shortDescription>
      </referenceToDataSource>
      <useAdviceForDataSet xml:lang="en">The data set represents a cradle to gate inventory. It can be used to characterise the supply chain situation of the respective commodity in a representative manner. Combination with individual unit processes using this commodity enables the generation of user-specific (product) LCAs.</useAdviceForDataSet>
      <useAdviceForDataSet xml:lang="de">Der Datensatz repräsentiert ein Cradle to Gate Inventar. Er kann verwendet werden, um die Lieferkette des jeweiligen Produktes in einer repräsentativen Weise zu charakterisieren. Die Kombination mit einzelnen Einheitenprozessen und diesem Produkt ermöglicht die Erstellung von anwenderspezifischen (Produkt-) LCAs.</useAdviceForDataSet>
    </dataSourcesTreatmentAndRepresentativeness>
    <validation>
      <review type="Dependent internal review">
        <common:referenceToNameOfReviewerAndInstitution refObjectId="d7fa0337-f279-430d-becf-7f3111a85010" version="21.01.000" type="contact data set" uri="../contacts/d7fa0337-f279-430d-becf-7f3111a85010.xml">
          <common:shortDescription xml:lang="en">Sphera Solutions GmbH</common:shortDescription>
        </common:referenceToNameOfReviewerAndInstitution>
      </review>
      <review type="Independent external review">
        <common:referenceToNameOfReviewerAndInstitution refObjectId="8f1306f0-7b83-4f36-a537-aa83f0498266" version="21.01.000" type="contact data set" uri="../contacts/8f1306f0-7b83-4f36-a537-aa83f0498266.xml">
          <common:shortDescription xml:lang="en">GaBi user forum</common:shortDescription>
        </common:referenceToNameOfReviewerAndInstitution>
      </review>
    </validation>
    <complianceDeclarations>
      <compliance>
        <common:referenceToComplianceSystem refObjectId="c0016b33-8cf7-415c-ac6e-deba0d21440d" version="00.01.000" type="source data set" uri="../sources/c0016b33-8cf7-415c-ac6e-deba0d21440d.xml">
          <common:shortDescription xml:lang="de">EN 15804+A2</common:shortDescription>
          <common:shortDescription xml:lang="en">EN 15804+A2</common:shortDescription>
        </common:referenceToComplianceSystem>
        <common:approvalOfOverallCompliance>Fully compliant</common:approvalOfOverallCompliance>
      </compliance>
    </complianceDeclarations>
  </modellingAndValidation>
  <administrativeInformation>
    <dataEntryBy>
      <common:timeStamp>2021-04-28T21:02:14+01:00</common:timeStamp>
      <common:referenceToDataSetFormat refObjectId="a97a0155-0234-4b87-b4ce-a45da52f2a40" version="01.00.000" type="source data set" uri="../sources/a97a0155-0234-4b87-b4ce-a45da52f2a40.xml">
        <common:shortDescription xml:lang="de">ILCD format 1.1</common:shortDescription>
        <common:shortDescription xml:lang="en">ILCD format 1.1</common:shortDescription>
      </common:referenceToDataSetFormat>
      <common:referenceToDataSetFormat refObjectId="a29449fd-aa2f-4de8-b5d7-4b06b43c6fde" version="00.01.000" type="source data set" uri="../sources/a29449fd-aa2f-4de8-b5d7-4b06b43c6fde.xml">
        <common:shortDescription xml:lang="de">EPD-Datenformaterweiterungen v1.2</common:shortDescription>
        <common:shortDescription xml:lang="en">EPD Data Format Extensions v1.2</common:shortDescription>
      </common:referenceToDataSetFormat>
      <common:referenceToPersonOrEntityEnteringTheData refObjectId="d7fa0337-f279-430d-becf-7f3111a85010" version="21.01.000" type="contact data set" uri="../contacts/d7fa0337-f279-430d-becf-7f3111a85010.xml">
        <common:shortDescription xml:lang="en">Sphera Solutions GmbH</common:shortDescription>
      </common:referenceToPersonOrEntityEnteringTheData>
    </dataEntryBy>
    <publicationAndOwnership>
      <common:dataSetVersion>20.21.060</common:dataSetVersion>
      <common:referenceToPrecedingDataSetVersion refObjectId="e9920105-0f1a-4452-9a08-47289dc04116" type="process data set" uri="https://www.oekobaudat.de/OEKOBAU.DAT/datasetdetail/process.xhtml?uuid=e9920105-0f1a-4452-9a08-47289dc04116&amp;stock=OBD_2020_II&amp;lang=de">
        <common:shortDescription xml:lang="en">Anodization of aluminium</common:shortDescription>
      </common:referenceToPrecedingDataSetVersion>
      <common:referenceToOwnershipOfDataSet refObjectId="d7fa0337-f279-430d-becf-7f3111a85010" version="21.01.000" type="contact data set" uri="../contacts/d7fa0337-f279-430d-becf-7f3111a85010.xml">
        <common:shortDescription xml:lang="en">Sphera Solutions GmbH</common:shortDescription>
      </common:referenceToOwnershipOfDataSet>
      <common:copyright>true</common:copyright>
      <common:licenseType>Free of charge for all users and uses</common:licenseType>
      <common:accessRestrictions xml:lang="en">The license conditions as stated on https://www.oekobaudat.de/ apply.</common:accessRestrictions>
      <common:accessRestrictions xml:lang="de">Es gelten die Lizenzbedingungen wie sie auf https://www.oekobaudat.de/ genannt sind.</common:accessRestrictions>
      <common:other>
        <epd2:referenceToPublisher refObjectId="f11651e0-7877-11e3-981f-0800200c9a66" version="00.01.000" type="contact data set" uri="../contacts/f11651e0-7877-11e3-981f-0800200c9a66.xml">
          <common:shortDescription xml:lang="en">BBSR</common:shortDescription>
        </epd2:referenceToPublisher>
      </common:other>
    </publicationAndOwnership>
  </administrativeInformation>
  <exchanges>
    <exchange dataSetInternalID="107429">
      <referenceToFlowDataSet refObjectId="8e7910f1-1daf-4f69-bded-c57d8fc622f8" version="21.01.000" type="flow data set" uri="../flows/8e7910f1-1daf-4f69-bded-c57d8fc622f8.xml">
        <common:shortDescription xml:lang="en">Anodization of aluminium</common:shortDescription>
        <common:shortDescription xml:lang="de">Eloxieren von Aluminiumblech</common:shortDescription>
      </referenceToFlowDataSet>
      <meanAmount>1</meanAmount>
    </exchange>
    <exchange dataSetInternalID="107430">
      <referenceToFlowDataSet refObjectId="20f32be5-0398-4288-9b6d-accddd195317" version="21.01.000" type="flow data set" uri="../flows/20f32be5-0398-4288-9b6d-accddd195317.xml">
        <common:shortDescription xml:lang="en">Use of renewable primary energy as energy carrier (PERE)</common:shortDescription>
        <common:shortDescription xml:lang="de">Erneuerbare Primärenergie als Energieträger (PERE)</common:shortDescription>
      </referenceToFlowDataSet>
      <functionType>General reminder flow</functionType>
      <exchangeDirection>Input</exchangeDirection>
      <common:other>
        <epd:amount epd:module="A1-A3">37.384619539242</epd:amount>
        <epd:referenceToUnitGroupDataSet refObjectId="93a60a57-a3c8-11da-a746-0800200c9a66" version="03.00.000" type="unit group data set" uri="../unitgroups/93a60a57-a3c8-11da-a746-0800200c9a66.xml">
          <common:shortDescription xml:lang="en">MJ</common:shortDescription>
        </epd:referenceToUnitGroupDataSet>
      </common:other>
    </exchange>
    <exchange dataSetInternalID="107431">
      <referenceToFlowDataSet refObjectId="fb3ec0de-548d-4508-aea5-00b73bf6f702" version="21.01.000" type="flow data set" uri="../flows/fb3ec0de-548d-4508-aea5-00b73bf6f702.xml">
        <common:shortDescription xml:lang="en">Use of renewable primary energy resources used as raw materials (PERM)</common:shortDescription>
        <common:shortDescription xml:lang="de">Erneuerbare Primärenergie zur stofflichen Nutzung (PERM)</common:shortDescription>
      </referenceToFlowDataSet>
      <functionType>General reminder flow</functionType>
      <exchangeDirection>Input</exchangeDirection>
      <common:other>
        <epd:amount epd:module="A1-A3">0</epd:amount>
        <epd:referenceToUnitGroupDataSet refObjectId="93a60a57-a3c8-11da-a746-0800200c9a66" version="03.00.000" type="unit group data set" uri="../unitgroups/93a60a57-a3c8-11da-a746-0800200c9a66.xml">
          <common:shortDescription xml:lang="en">MJ</common:shortDescription>
        </epd:referenceToUnitGroupDataSet>
      </common:other>
    </exchange>
    <exchange dataSetInternalID="107432">
      <referenceToFlowDataSet refObjectId="53f97275-fa8a-4cdd-9024-65936002acd0" version="21.01.000" type="flow data set" uri="../flows/53f97275-fa8a-4cdd-9024-65936002acd0.xml">
        <common:shortDescription xml:lang="en">Total use of renewable primary energy (PERT)</common:shortDescription>
        <common:shortDescription xml:lang="de">Total erneuerbare Primärenergie (PERT)</common:shortDescription>
      </referenceToFlowDataSet>
      <functionType>General reminder flow</functionType>
      <exchangeDirection>Input</exchangeDirection>
      <common:other>
        <epd:amount epd:module="A1-A3">37.384619539242</epd:amount>
        <epd:referenceToUnitGroupDataSet refObjectId="93a60a57-a3c8-11da-a746-0800200c9a66" version="03.00.000" type="unit group data set" uri="../unitgroups/93a60a57-a3c8-11da-a746-0800200c9a66.xml">
          <common:shortDescription xml:lang="en">MJ</common:shortDescription>
        </epd:referenceToUnitGroupDataSet>
      </common:other>
    </exchange>
    <exchange dataSetInternalID="107433">
      <referenceToFlowDataSet refObjectId="ac857178-2b45-46ec-892a-a9a4332f0372" version="21.01.000" type="flow data set" uri="../flows/ac857178-2b45-46ec-892a-a9a4332f0372.xml">
        <common:shortDescription xml:lang="en">Use of non renewable primary energy as energy carrier (PENRE)</common:shortDescription>
        <common:shortDescription xml:lang="de">Nicht-erneuerbare Primärenergie als Energieträger (PENRE)</common:shortDescription>
      </referenceToFlowDataSet>
      <functionType>General reminder flow</functionType>
      <exchangeDirection>Input</exchangeDirection>
      <common:other>
        <epd:amount epd:module="A1-A3">89.2937785279157</epd:amount>
        <epd:referenceToUnitGroupDataSet refObjectId="93a60a57-a3c8-11da-a746-0800200c9a66" version="03.00.000" type="unit group data set" uri="../unitgroups/93a60a57-a3c8-11da-a746-0800200c9a66.xml">
          <common:shortDescription xml:lang="en">MJ</common:shortDescription>
        </epd:referenceToUnitGroupDataSet>
      </common:other>
    </exchange>
    <exchange dataSetInternalID="107434">
      <referenceToFlowDataSet refObjectId="1421caa0-679d-4bf4-b282-0eb850ccae27" version="21.01.000" type="flow data set" uri="../flows/1421caa0-679d-4bf4-b282-0eb850ccae27.xml">
        <common:shortDescription xml:lang="en">Use of non renewable primary energy resources used as raw materials (PENRM)</common:shortDescription>
        <common:shortDescription xml:lang="de">Nicht-erneuerbare Primärenergie zur stofflichen Nutzung (PENRM)</common:shortDescription>
      </referenceToFlowDataSet>
      <functionType>General reminder flow</functionType>
      <exchangeDirection>Input</exchangeDirection>
      <common:other>
        <epd:amount epd:module="A1-A3">0</epd:amount>
        <epd:referenceToUnitGroupDataSet refObjectId="93a60a57-a3c8-11da-a746-0800200c9a66" version="03.00.000" type="unit group data set" uri="../unitgroups/93a60a57-a3c8-11da-a746-0800200c9a66.xml">
          <common:shortDescription xml:lang="en">MJ</common:shortDescription>
        </epd:referenceToUnitGroupDataSet>
      </common:other>
    </exchange>
    <exchange dataSetInternalID="107435">
      <referenceToFlowDataSet refObjectId="06159210-646b-4c8d-8583-da9b3b95a6c1" version="21.01.000" type="flow data set" uri="../flows/06159210-646b-4c8d-8583-da9b3b95a6c1.xml">
        <common:shortDescription xml:lang="en">Total use of non renewable primary energy resource (PENRT)</common:shortDescription>
        <common:shortDescription xml:lang="de">Total nicht-erneuerbare Primärenergie (PENRT)</common:shortDescription>
      </referenceToFlowDataSet>
      <functionType>General reminder flow</functionType>
      <exchangeDirection>Input</exchangeDirection>
      <common:other>
        <epd:amount epd:module="A1-A3">89.2937785279157</epd:amount>
        <epd:referenceToUnitGroupDataSet refObjectId="93a60a57-a3c8-11da-a746-0800200c9a66" version="03.00.000" type="unit group data set" uri="../unitgroups/93a60a57-a3c8-11da-a746-0800200c9a66.xml">
          <common:shortDescription xml:lang="en">MJ</common:shortDescription>
        </epd:referenceToUnitGroupDataSet>
      </common:other>
    </exchange>
    <exchange dataSetInternalID="107436">
      <referenceToFlowDataSet refObjectId="c6a1f35f-2d09-4f54-8dfb-97e502e1ce92" version="21.01.000" type="flow data set" uri="../flows/c6a1f35f-2d09-4f54-8dfb-97e502e1ce92.xml">
        <common:shortDescription xml:lang="en">Use of secondary material (SM)</common:shortDescription>
        <common:shortDescription xml:lang="de">Einsatz von Sekundärstoffen (SM)</common:shortDescription>
      </referenceToFlowDataSet>
      <functionType>General reminder flow</functionType>
      <exchangeDirection>Input</exchangeDirection>
      <common:other>
        <epd:amount epd:module="A1-A3">0</epd:amount>
        <epd:referenceToUnitGroupDataSet refObjectId="93a60a57-a4c8-11da-a746-0800200c9a66" version="03.00.000" type="unit group data set" uri="../unitgroups/93a60a57-a4c8-11da-a746-0800200c9a66.xml">
          <common:shortDescription xml:lang="en">kg</common:shortDescription>
        </epd:referenceToUnitGroupDataSet>
      </common:other>
    </exchange>
    <exchange dataSetInternalID="107437">
      <referenceToFlowDataSet refObjectId="64333088-a55f-4aa2-9a31-c10b07816787" version="21.01.000" type="flow data set" uri="../flows/64333088-a55f-4aa2-9a31-c10b07816787.xml">
        <common:shortDescription xml:lang="en">Use of renewable secondary fuels (SF)</common:shortDescription>
        <common:shortDescription xml:lang="de">Erneuerbare Sekundärbrennstoffe (SF)</common:shortDescription>
      </referenceToFlowDataSet>
      <functionType>General reminder flow</functionType>
      <exchangeDirection>Input</exchangeDirection>
      <common:other>
        <epd:amount epd:module="A1-A3">0</epd:amount>
        <epd:referenceToUnitGroupDataSet refObjectId="93a60a57-a3c8-11da-a746-0800200c9a66" version="03.00.000" type="unit group data set" uri="../unitgroups/93a60a57-a3c8-11da-a746-0800200c9a66.xml">
          <common:shortDescription xml:lang="en">MJ</common:shortDescription>
        </epd:referenceToUnitGroupDataSet>
      </common:other>
    </exchange>
    <exchange dataSetInternalID="107438">
      <referenceToFlowDataSet refObjectId="89def144-d39a-4287-b86f-efde453ddcb2" version="21.01.000" type="flow data set" uri="../flows/89def144-d39a-4287-b86f-efde453ddcb2.xml">
        <common:shortDescription xml:lang="en">Use of non renewable secondary fuels (NRSF)</common:shortDescription>
        <common:shortDescription xml:lang="de">Nicht erneuerbare Sekundärbrennstoffe (NRSF)</common:shortDescription>
      </referenceToFlowDataSet>
      <functionType>General reminder flow</functionType>
      <exchangeDirection>Input</exchangeDirection>
      <common:other>
        <epd:amount epd:module="A1-A3">0</epd:amount>
        <epd:referenceToUnitGroupDataSet refObjectId="93a60a57-a3c8-11da-a746-0800200c9a66" version="03.00.000" type="unit group data set" uri="../unitgroups/93a60a57-a3c8-11da-a746-0800200c9a66.xml">
          <common:shortDescription xml:lang="en">MJ</common:shortDescription>
        </epd:referenceToUnitGroupDataSet>
      </common:other>
    </exchange>
    <exchange dataSetInternalID="107439">
      <referenceToFlowDataSet refObjectId="3cf952c8-f3a4-461d-8c96-96456ca62246" version="21.01.000" type="flow data set" uri="../flows/3cf952c8-f3a4-461d-8c96-96456ca62246.xml">
        <common:shortDescription xml:lang="en">Net use of fresh water (FW)</common:shortDescription>
        <common:shortDescription xml:lang="de">Nettoeinsatz von Süßwasserressourcen (FW)</common:shortDescription>
      </referenceToFlowDataSet>
      <functionType>General reminder flow</functionType>
      <exchangeDirection>Input</exchangeDirection>
      <common:other>
        <epd:amount epd:module="A1-A3">0.0179569759715205</epd:amount>
        <epd:referenceToUnitGroupDataSet refObjectId="93a60a57-a3c8-12da-a746-0800200c9a66" version="03.00.000" type="unit group data set" uri="../unitgroups/93a60a57-a3c8-12da-a746-0800200c9a66.xml">
          <common:shortDescription xml:lang="en">m3</common:shortDescription>
        </epd:referenceToUnitGroupDataSet>
      </common:other>
    </exchange>
    <exchange dataSetInternalID="107440">
      <referenceToFlowDataSet refObjectId="430f9e0f-59b2-46a0-8e0d-55e0e84948fc" version="21.01.000" type="flow data set" uri="../flows/430f9e0f-59b2-46a0-8e0d-55e0e84948fc.xml">
        <common:shortDescription xml:lang="en">Hazardous waste disposed (HWD)</common:shortDescription>
        <common:shortDescription xml:lang="de">Gefährlicher Abfall zur Deponie (HWD)</common:shortDescription>
      </referenceToFlowDataSet>
      <functionType>General reminder flow</functionType>
      <exchangeDirection>Output</exchangeDirection>
      <common:other>
        <epd:amount epd:module="A1-A3">3.06951263000728E-8</epd:amount>
        <epd:referenceToUnitGroupDataSet refObjectId="93a60a57-a4c8-11da-a746-0800200c9a66" version="03.00.000" type="unit group data set" uri="../unitgroups/93a60a57-a4c8-11da-a746-0800200c9a66.xml">
          <common:shortDescription xml:lang="en">kg</common:shortDescription>
        </epd:referenceToUnitGroupDataSet>
      </common:other>
    </exchange>
    <exchange dataSetInternalID="107441">
      <referenceToFlowDataSet refObjectId="b29ef66b-e286-4afa-949f-62f1a7b4d7fa" version="21.01.000" type="flow data set" uri="../flows/b29ef66b-e286-4afa-949f-62f1a7b4d7fa.xml">
        <common:shortDescription xml:lang="en">Non harzardous waste disposed (NHWD)</common:shortDescription>
        <common:shortDescription xml:lang="de">Entsorgter nicht gefährlicher Abfall (NHWD)</common:shortDescription>
      </referenceToFlowDataSet>
      <functionType>General reminder flow</functionType>
      <exchangeDirection>Output</exchangeDirection>
      <common:other>
        <epd:amount epd:module="A1-A3">0.295417512743817</epd:amount>
        <epd:referenceToUnitGroupDataSet refObjectId="93a60a57-a4c8-11da-a746-0800200c9a66" version="03.00.000" type="unit group data set" uri="../unitgroups/93a60a57-a4c8-11da-a746-0800200c9a66.xml">
          <common:shortDescription xml:lang="en">kg</common:shortDescription>
        </epd:referenceToUnitGroupDataSet>
      </common:other>
    </exchange>
    <exchange dataSetInternalID="107442">
      <referenceToFlowDataSet refObjectId="3449546e-52ad-4b39-b809-9fb77cea8ff6" version="21.01.000" type="flow data set" uri="../flows/3449546e-52ad-4b39-b809-9fb77cea8ff6.xml">
        <common:shortDescription xml:lang="en">Radioactive waste disposed (RWD)</common:shortDescription>
        <common:shortDescription xml:lang="de">Entsorgter radioaktiver Abfall (RWD)</common:shortDescription>
      </referenceToFlowDataSet>
      <functionType>General reminder flow</functionType>
      <exchangeDirection>Output</exchangeDirection>
      <common:other>
        <epd:amount epd:module="A1-A3">0.0040543793808044</epd:amount>
        <epd:referenceToUnitGroupDataSet refObjectId="93a60a57-a4c8-11da-a746-0800200c9a66" version="03.00.000" type="unit group data set" uri="../unitgroups/93a60a57-a4c8-11da-a746-0800200c9a66.xml">
          <common:shortDescription xml:lang="en">kg</common:shortDescription>
        </epd:referenceToUnitGroupDataSet>
      </common:other>
    </exchange>
    <exchange dataSetInternalID="107443">
      <referenceToFlowDataSet refObjectId="a2b32f97-3fc7-4af2-b209-525bc6426f33" version="21.01.000" type="flow data set" uri="../flows/a2b32f97-3fc7-4af2-b209-525bc6426f33.xml">
        <common:shortDescription xml:lang="en">Components for re-use (CRU)</common:shortDescription>
        <common:shortDescription xml:lang="de">Komponenten für die Wiederverwendung (CRU)</common:shortDescription>
      </referenceToFlowDataSet>
      <functionType>General reminder flow</functionType>
      <exchangeDirection>Output</exchangeDirection>
      <common:other>
        <epd:amount epd:module="A1-A3">0</epd:amount>
        <epd:referenceToUnitGroupDataSet refObjectId="93a60a57-a4c8-11da-a746-0800200c9a66" version="03.00.000" type="unit group data set" uri="../unitgroups/93a60a57-a4c8-11da-a746-0800200c9a66.xml">
          <common:shortDescription xml:lang="en">kg</common:shortDescription>
        </epd:referenceToUnitGroupDataSet>
      </common:other>
    </exchange>
    <exchange dataSetInternalID="107444">
      <referenceToFlowDataSet refObjectId="d7fe48a5-4103-49c8-9aae-b0b5dfdbd6ae" version="21.01.000" type="flow data set" uri="../flows/d7fe48a5-4103-49c8-9aae-b0b5dfdbd6ae.xml">
        <common:shortDescription xml:lang="en">Materials for recycling  (MFR)</common:shortDescription>
        <common:shortDescription xml:lang="de">Stoffe zum Recycling (MFR)</common:shortDescription>
      </referenceToFlowDataSet>
      <functionType>General reminder flow</functionType>
      <exchangeDirection>Output</exchangeDirection>
      <common:other>
        <epd:amount epd:module="A1-A3">0</epd:amount>
        <epd:referenceToUnitGroupDataSet refObjectId="93a60a57-a4c8-11da-a746-0800200c9a66" version="03.00.000" type="unit group data set" uri="../unitgroups/93a60a57-a4c8-11da-a746-0800200c9a66.xml">
          <common:shortDescription xml:lang="en">kg</common:shortDescription>
        </epd:referenceToUnitGroupDataSet>
      </common:other>
    </exchange>
    <exchange dataSetInternalID="107445">
      <referenceToFlowDataSet refObjectId="59a9181c-3aaf-46ee-8b13-2b3723b6e447" version="21.01.000" type="flow data set" uri="../flows/59a9181c-3aaf-46ee-8b13-2b3723b6e447.xml">
        <common:shortDescription xml:lang="en">Materials for energy recovery (MER)</common:shortDescription>
        <common:shortDescription xml:lang="de">Stoffe für die Energierückgewinnung (MER)</common:shortDescription>
      </referenceToFlowDataSet>
      <functionType>General reminder flow</functionType>
      <exchangeDirection>Output</exchangeDirection>
      <common:other>
        <epd:amount epd:module="A1-A3">0</epd:amount>
        <epd:referenceToUnitGroupDataSet refObjectId="93a60a57-a4c8-11da-a746-0800200c9a66" version="03.00.000" type="unit group data set" uri="../unitgroups/93a60a57-a4c8-11da-a746-0800200c9a66.xml">
          <common:shortDescription xml:lang="en">kg</common:shortDescription>
        </epd:referenceToUnitGroupDataSet>
      </common:other>
    </exchange>
    <exchange dataSetInternalID="107446">
      <referenceToFlowDataSet refObjectId="4da0c987-2b76-40d6-9e9e-82a017aaaf29" version="21.01.000" type="flow data set" uri="../flows/4da0c987-2b76-40d6-9e9e-82a017aaaf29.xml">
        <common:shortDescription xml:lang="en">Exported electrical energy (EEE)</common:shortDescription>
        <common:shortDescription xml:lang="de">Exportierte elektrische Energie (EEE)</common:shortDescription>
      </referenceToFlowDataSet>
      <functionType>General reminder flow</functionType>
      <exchangeDirection>Output</exchangeDirection>
      <common:other>
        <epd:amount epd:module="A1-A3">0</epd:amount>
        <epd:referenceToUnitGroupDataSet refObjectId="93a60a57-a3c8-11da-a746-0800200c9a66" version="03.00.000" type="unit group data set" uri="../unitgroups/93a60a57-a3c8-11da-a746-0800200c9a66.xml">
          <common:shortDescription xml:lang="en">MJ</common:shortDescription>
        </epd:referenceToUnitGroupDataSet>
      </common:other>
    </exchange>
    <exchange dataSetInternalID="107447">
      <referenceToFlowDataSet refObjectId="98daf38a-7a79-46d3-9a37-2b7bd0955810" version="21.01.000" type="flow data set" uri="../flows/98daf38a-7a79-46d3-9a37-2b7bd0955810.xml">
        <common:shortDescription xml:lang="en">Exported thermal energy (EET)</common:shortDescription>
        <common:shortDescription xml:lang="de">Exportierte thermische Energie (EET)</common:shortDescription>
      </referenceToFlowDataSet>
      <functionType>General reminder flow</functionType>
      <exchangeDirection>Output</exchangeDirection>
      <common:other>
        <epd:amount epd:module="A1-A3">0</epd:amount>
        <epd:referenceToUnitGroupDataSet refObjectId="93a60a57-a3c8-11da-a746-0800200c9a66" version="03.00.000" type="unit group data set" uri="../unitgroups/93a60a57-a3c8-11da-a746-0800200c9a66.xml">
          <common:shortDescription xml:lang="en">MJ</common:shortDescription>
        </epd:referenceToUnitGroupDataSet>
      </common:other>
    </exchange>
  </exchanges>
  <LCIAResults>
    <LCIAResult>
      <referenceToLCIAMethodDataSet refObjectId="6a37f984-a4b3-458a-a20a-64418c145fa2" version="21.01.000" type="LCIA method data set" uri="../lciamethods/6a37f984-a4b3-458a-a20a-64418c145fa2.xml">
        <common:shortDescription xml:lang="en">Global Warming Potential - total (GWP-total)</common:shortDescription>
        <common:shortDescription xml:lang="de">Globales Erwärmungspotenzial - total (GWP-total)</common:shortDescription>
      </referenceToLCIAMethodDataSet>
      <common:other>
        <epd:amount epd:module="A1-A3">5.73104326991599</epd:amount>
        <epd:referenceToUnitGroupDataSet refObjectId="1ebf3012-d0db-4de2-aefd-ef30cedb0be1" version="25.00.000" type="unit group data set" uri="../unitgroups/1ebf3012-d0db-4de2-aefd-ef30cedb0be1.xml">
          <common:shortDescription xml:lang="en">kg CO2 eq.</common:shortDescription>
        </epd:referenceToUnitGroupDataSet>
      </common:other>
    </LCIAResult>
    <LCIAResult>
      <referenceToLCIAMethodDataSet refObjectId="5f635281-343e-44fb-83df-1971b155e6b6" version="21.01.000" type="LCIA method data set" uri="../lciamethods/5f635281-343e-44fb-83df-1971b155e6b6.xml">
        <common:shortDescription xml:lang="en">Global Warming Potential - fossil fuels (GWP-fossil)</common:shortDescription>
        <common:shortDescription xml:lang="de">Globales Erwärmungspotenzial - fossil (GWP-fossil)</common:shortDescription>
      </referenceToLCIAMethodDataSet>
      <common:other>
        <epd:amount epd:module="A1-A3">5.66549915239061</epd:amount>
        <epd:referenceToUnitGroupDataSet refObjectId="1ebf3012-d0db-4de2-aefd-ef30cedb0be1" version="25.00.000" type="unit group data set" uri="../unitgroups/1ebf3012-d0db-4de2-aefd-ef30cedb0be1.xml">
          <common:shortDescription xml:lang="en">kg CO2 eq.</common:shortDescription>
        </epd:referenceToUnitGroupDataSet>
      </common:other>
    </LCIAResult>
    <LCIAResult>
      <referenceToLCIAMethodDataSet refObjectId="2356e1ab-0185-4db5-86e5-16de51c7485c" version="21.01.000" type="LCIA method data set" uri="../lciamethods/2356e1ab-0185-4db5-86e5-16de51c7485c.xml">
        <common:shortDescription xml:lang="en">Global Warming Potential - biogenic (GWP-biogenic)</common:shortDescription>
        <common:shortDescription xml:lang="de">Globales Erwärmungspotenzial - biogen (GWP-biogenic)</common:shortDescription>
      </referenceToLCIAMethodDataSet>
      <common:other>
        <epd:amount epd:module="A1-A3">0.0550058927222081</epd:amount>
        <epd:referenceToUnitGroupDataSet refObjectId="1ebf3012-d0db-4de2-aefd-ef30cedb0be1" version="25.00.000" type="unit group data set" uri="../unitgroups/1ebf3012-d0db-4de2-aefd-ef30cedb0be1.xml">
          <common:shortDescription xml:lang="en">kg CO2 eq.</common:shortDescription>
        </epd:referenceToUnitGroupDataSet>
      </common:other>
    </LCIAResult>
    <LCIAResult>
      <referenceToLCIAMethodDataSet refObjectId="4331bbdb-978a-490d-8707-eeb047f01a55" version="21.01.000" type="LCIA method data set" uri="../lciamethods/4331bbdb-978a-490d-8707-eeb047f01a55.xml">
        <common:shortDescription xml:lang="en">Global Warming Potential - land use and land use change (GWP-luluc)</common:shortDescription>
        <common:shortDescription xml:lang="de">Globales Erwärmungspotenzial - luluc (GWP-luluc)</common:shortDescription>
      </referenceToLCIAMethodDataSet>
      <common:other>
        <epd:amount epd:module="A1-A3">0.0105382248031712</epd:amount>
        <epd:referenceToUnitGroupDataSet refObjectId="1ebf3012-d0db-4de2-aefd-ef30cedb0be1" version="25.00.000" type="unit group data set" uri="../unitgroups/1ebf3012-d0db-4de2-aefd-ef30cedb0be1.xml">
          <common:shortDescription xml:lang="en">kg CO2 eq.</common:shortDescription>
        </epd:referenceToUnitGroupDataSet>
      </common:other>
    </LCIAResult>
    <LCIAResult>
      <referenceToLCIAMethodDataSet refObjectId="b5c629d6-def3-11e6-bf01-fe55135034f3" version="21.01.000" type="LCIA method data set" uri="../lciamethods/b5c629d6-def3-11e6-bf01-fe55135034f3.xml">
        <common:shortDescription xml:lang="en">Depletion potenzial of the stratospheric ozone layer (ODP)</common:shortDescription>
        <common:shortDescription xml:lang="de">Abbaupotenzial der stratosphärischen Ozonschicht (ODP)</common:shortDescription>
      </referenceToLCIAMethodDataSet>
      <common:other>
        <epd:amount epd:module="A1-A3">1.62749344890691E-13</epd:amount>
        <epd:referenceToUnitGroupDataSet refObjectId="d9e957c9-7309-4474-bf3a-7777df6c4e5b" version="25.00.000" type="unit group data set" uri="../unitgroups/d9e957c9-7309-4474-bf3a-7777df6c4e5b.xml">
          <common:shortDescription xml:lang="en">kg CFC-11 eq.</common:shortDescription>
        </epd:referenceToUnitGroupDataSet>
      </common:other>
    </LCIAResult>
    <LCIAResult>
      <referenceToLCIAMethodDataSet refObjectId="b5c611c6-def3-11e6-bf01-fe55135034f3" version="21.01.000" type="LCIA method data set" uri="../lciamethods/b5c611c6-def3-11e6-bf01-fe55135034f3.xml">
        <common:shortDescription xml:lang="en">Acidifcation potential, Accumulated Exceedance (AP)</common:shortDescription>
        <common:shortDescription xml:lang="de">Versauerungspotenzial, kumulierte Überschreitung (AP)</common:shortDescription>
      </referenceToLCIAMethodDataSet>
      <common:other>
        <epd:amount epd:module="A1-A3">0.0096864442897525</epd:amount>
        <epd:referenceToUnitGroupDataSet refObjectId="42e089ac-92bf-4bf2-8ca1-5fc40d18f2ed" version="00.01.000" type="unit group data set" uri="../unitgroups/42e089ac-92bf-4bf2-8ca1-5fc40d18f2ed.xml">
          <common:shortDescription xml:lang="en">Mole of H+ eq.</common:shortDescription>
        </epd:referenceToUnitGroupDataSet>
      </common:other>
    </LCIAResult>
    <LCIAResult>
      <referenceToLCIAMethodDataSet refObjectId="b53ec18f-7377-4ad3-86eb-cc3f4f276b2b" version="21.01.000" type="LCIA method data set" uri="../lciamethods/b53ec18f-7377-4ad3-86eb-cc3f4f276b2b.xml">
        <common:shortDescription xml:lang="en">Eutrophication potential - freshwater (EP-freshwater)</common:shortDescription>
        <common:shortDescription xml:lang="de">Eutrophierungspotenzial - Süßwasser (EP-freshwater)</common:shortDescription>
      </referenceToLCIAMethodDataSet>
      <common:other>
        <epd:amount epd:module="A1-A3">2.19423593434661E-5</epd:amount>
        <epd:referenceToUnitGroupDataSet refObjectId="0429039d-a61d-4590-ba67-aa4a20a810a1" version="25.00.000" type="unit group data set" uri="../unitgroups/0429039d-a61d-4590-ba67-aa4a20a810a1.xml">
          <common:shortDescription xml:lang="en">kg P eq.</common:shortDescription>
        </epd:referenceToUnitGroupDataSet>
      </common:other>
    </LCIAResult>
    <LCIAResult>
      <referenceToLCIAMethodDataSet refObjectId="b5c619fa-def3-11e6-bf01-fe55135034f3" version="21.01.000" type="LCIA method data set" uri="../lciamethods/b5c619fa-def3-11e6-bf01-fe55135034f3.xml">
        <common:shortDescription xml:lang="en">Eutrophication potential - marine (EP-marine)</common:shortDescription>
        <common:shortDescription xml:lang="de">Eutrophierungspotenzial - Salzwasser (EP-marine)</common:shortDescription>
      </referenceToLCIAMethodDataSet>
      <common:other>
        <epd:amount epd:module="A1-A3">0.00417536651519458</epd:amount>
        <epd:referenceToUnitGroupDataSet refObjectId="d05bb823-ecdf-4686-8c40-bf1d9257859f" version="00.00.003" type="unit group data set" uri="../unitgroups/d05bb823-ecdf-4686-8c40-bf1d9257859f.xml">
          <common:shortDescription xml:lang="en">kg N eq.</common:shortDescription>
        </epd:referenceToUnitGroupDataSet>
      </common:other>
    </LCIAResult>
    <LCIAResult>
      <referenceToLCIAMethodDataSet refObjectId="b5c614d2-def3-11e6-bf01-fe55135034f3" version="21.01.000" type="LCIA method data set" uri="../lciamethods/b5c614d2-def3-11e6-bf01-fe55135034f3.xml">
        <common:shortDescription xml:lang="en">Eutrophication potential - terrestrial (EP-terrestrial)</common:shortDescription>
        <common:shortDescription xml:lang="de">Eutrophierungspotenzial - Land (EP-terrestrial)</common:shortDescription>
      </referenceToLCIAMethodDataSet>
      <common:other>
        <epd:amount epd:module="A1-A3">0.0259340629997643</epd:amount>
        <epd:referenceToUnitGroupDataSet refObjectId="71b4d617-0ec9-4d3f-b65e-e438940c2401" version="00.00.003" type="unit group data set" uri="../unitgroups/71b4d617-0ec9-4d3f-b65e-e438940c2401.xml">
          <common:shortDescription xml:lang="en">Mole of N eq.</common:shortDescription>
        </epd:referenceToUnitGroupDataSet>
      </common:other>
    </LCIAResult>
    <LCIAResult>
      <referenceToLCIAMethodDataSet refObjectId="b5c610fe-def3-11e6-bf01-fe55135034f3" version="21.01.000" type="LCIA method data set" uri="../lciamethods/b5c610fe-def3-11e6-bf01-fe55135034f3.xml">
        <common:shortDescription xml:lang="en">Photochemical Ozone Creation Potential  (POCP)</common:shortDescription>
        <common:shortDescription xml:lang="de">Bildungspotenzial für troposphärisches Ozon (POCP)</common:shortDescription>
      </referenceToLCIAMethodDataSet>
      <common:other>
        <epd:amount epd:module="A1-A3">0.00652056588126886</epd:amount>
        <epd:referenceToUnitGroupDataSet refObjectId="d27c25f8-fbc1-44c6-b47b-4adbae4199c6" version="00.00.003" type="unit group data set" uri="../unitgroups/d27c25f8-fbc1-44c6-b47b-4adbae4199c6.xml">
          <common:shortDescription xml:lang="en">kg NMVOC eq.</common:shortDescription>
        </epd:referenceToUnitGroupDataSet>
      </common:other>
    </LCIAResult>
    <LCIAResult>
      <referenceToLCIAMethodDataSet refObjectId="b2ad6494-c78d-11e6-9d9d-cec0c932ce01" version="21.01.000" type="LCIA method data set" uri="../lciamethods/b2ad6494-c78d-11e6-9d9d-cec0c932ce01.xml">
        <common:shortDescription xml:lang="en">Abiotic depletion potential - non-fossil resources (ADPE)</common:shortDescription>
        <common:shortDescription xml:lang="de">Potenzial für die Verknappung abiotischer Ressourcen  nicht fossile Ressourcen (ADPE)</common:shortDescription>
      </referenceToLCIAMethodDataSet>
      <common:other>
        <epd:amount epd:module="A1-A3">2.10916931274296E-6</epd:amount>
        <epd:referenceToUnitGroupDataSet refObjectId="54ccd2d9-a32a-4fc2-923d-f2c8c93e89d4" version="25.00.000" type="unit group data set" uri="../unitgroups/54ccd2d9-a32a-4fc2-923d-f2c8c93e89d4.xml">
          <common:shortDescription xml:lang="en">kg Sb eq.</common:shortDescription>
        </epd:referenceToUnitGroupDataSet>
      </common:other>
    </LCIAResult>
    <LCIAResult>
      <referenceToLCIAMethodDataSet refObjectId="b2ad6110-c78d-11e6-9d9d-cec0c932ce01" version="21.01.000" type="LCIA method data set" uri="../lciamethods/b2ad6110-c78d-11e6-9d9d-cec0c932ce01.xml">
        <common:shortDescription xml:lang="en">Abiotic depletion potential - fossil resources (ADPF)</common:shortDescription>
        <common:shortDescription xml:lang="de">Potenzial für die Verknappung abiotischer Ressourcen  fossile Brennstoffe (ADPF)</common:shortDescription>
      </referenceToLCIAMethodDataSet>
      <common:other>
        <epd:amount epd:module="A1-A3">89.2775415548986</epd:amount>
        <epd:referenceToUnitGroupDataSet refObjectId="93a60a57-a3c8-11da-a746-0800200c9a66" version="02.00.000" type="unit group data set" uri="../unitgroups/93a60a57-a3c8-11da-a746-0800200c9a66.xml">
          <common:shortDescription xml:lang="en">MJ</common:shortDescription>
        </epd:referenceToUnitGroupDataSet>
      </common:other>
    </LCIAResult>
    <LCIAResult>
      <referenceToLCIAMethodDataSet refObjectId="b2ad66ce-c78d-11e6-9d9d-cec0c932ce01" version="21.01.000" type="LCIA method data set" uri="../lciamethods/b2ad66ce-c78d-11e6-9d9d-cec0c932ce01.xml">
        <common:shortDescription xml:lang="en">Water (user) deprivation potential (WDP)</common:shortDescription>
        <common:shortDescription xml:lang="de">Wasser-Entzugspotenzial (Benutzer) (WDP)</common:shortDescription>
      </referenceToLCIAMethodDataSet>
      <common:other>
        <epd:amount epd:module="A1-A3">0.202405538942687</epd:amount>
        <epd:referenceToUnitGroupDataSet refObjectId="6ae2df01-888e-46c8-b17d-49fa3869b476" version="00.00.003" type="unit group data set" uri="../unitgroups/6ae2df01-888e-46c8-b17d-49fa3869b476.xml">
          <common:shortDescription xml:lang="en">m³ world equiv.</common:shortDescription>
        </epd:referenceToUnitGroupDataSet>
      </common:other>
    </LCIAResult>
  </LCIAResults>
</processDataSet>
