<?xml version="1.0" encoding="utf-8"?>
<processDataSet xmlns:epd="http://www.iai.kit.edu/EPD/2013" xmlns:epd2="http://www.indata.network/EPD/2019" xmlns:common="http://lca.jrc.it/ILCD/Common" xsi:schemaLocation="http://lca.jrc.it/ILCD/Process ../../schemas/EPD_DataSet.xsd" epd2:epd-version="1.2" version="1.1" locations="../ILCDLocations.xml" xmlns:xsi="http://www.w3.org/2001/XMLSchema-instance" xmlns="http://lca.jrc.it/ILCD/Process">
<processInformation>
<dataSetInformation>
<common:UUID>f43d4177-5694-4384-b485-3c47988583cb</common:UUID>
<name>
<baseName xml:lang="de">Butyl Dichtungsbahn NovoProof® (FAI)</baseName>
<baseName xml:lang="en">Butyl waterproofing membrane NovoProof® FAI</baseName>
<functionalUnitFlowProperties xml:lang="de" />
</name>
<classificationInformation>
<common:classification name="OEKOBAU.DAT">
<common:class level="0" classId="6">Kunststoffe</common:class>
<common:class level="1" classId="6.3">Dachbahnen</common:class>
<common:class level="2" classId="6.3.03">Elastomer-Dachbahnen</common:class>
</common:classification>
<common:classification name="IBUCategories">
<common:class level="0">02 Bauprodukte</common:class>
<common:class level="1">Abdichtungen</common:class>
<common:class level="2">Dach- und Dichtungsbahnsysteme aus Kunststoffen und Elastomeren</common:class>
</common:classification>
</classificationInformation>
<common:generalComment xml:lang="de">NovoProof®-Dichtungssysteme bestehen aus voll vernetzten Elastomerbahnen auf Basis von Butyl (IIR).   Die NovoProof® Familie umfasst vielfältige Varianten. Hier wird folgende Variante betrachtet: NovoProof® FAI Homogene Butyl-Bauwerksdichtung  Die Durchschnittsbildung basiert auf den entsprechenden Produktionsmengen für das Kalenderjahr 2014.</common:generalComment>
<common:generalComment xml:lang="en">NovoProof® waterproofing systems comprise fully cross-linked elastomer sheets based on butyl (IIR).    The NovoProof® family comprises numerous variants. The following variants are considered here:NovoProof® FAI Homogeneous butyl waterproofing sheet  Averaging is based on the corresponding production volumes for the 2014 calendar year. Directive (EU) No. 305/2011 (CPR) applies for placing the product on the market in the EU/EFTA. The product requires a Declaration of Performance taking consideration of - DIN EN 13859-2:2014 Flexible sheets for waterproofing – Definitions and characteristics of underlays – Part 2: Underlays for walls;  - and CE marking. Use is governed by the respective national regulations.</common:generalComment>
<common:other>
<epd:scenarios>
<epd:scenario epd:name="S1">
<epd:description xml:lang="de">Recycling</epd:description>
<epd:description xml:lang="en">recycling</epd:description>
</epd:scenario>
<epd:scenario epd:name="S2">
<epd:description xml:lang="de">thermische Verwertung</epd:description>
<epd:description xml:lang="en">thermal utilisation</epd:description>
</epd:scenario>
</epd:scenarios>
</common:other>
</dataSetInformation>
<quantitativeReference>
<referenceToReferenceFlow>0</referenceToReferenceFlow>
</quantitativeReference>
<time>
<common:referenceYear>2017</common:referenceYear>
<common:dataSetValidUntil>2022</common:dataSetValidUntil>
<common:other>
<epd2:publicationDateOfEPD>2017-09-11</epd2:publicationDateOfEPD>
</common:other>
</time>
<geography>
<locationOfOperationSupplyOrProduction location="DE" />
</geography>
<technology>
<technologyDescriptionAndIncludedProcesses xml:lang="de">Grundlage der Produktion von Gummimischungen als Werkstoff für die Herstellung von Butyl Dichtungsbahnen ist eine Rezeptur, die die eingesetzten Rohstoffe qualitativ als auch quantitativ festschreibt. Der Herstellprozess in Wadern-Büschfeld ist ein klassischer Batchprozess. Die benötigten Rohstoffe werden gemäß der Rezepturrechner gesteuert in automatische Waagen dosiert und über geeignete Fördereinrichtungen in einem Innenmischer bereitgestellt. Das Ergebnis des Mischprozesses ist eine homogene Rohgummimischung. Produktionsbegleitend werden die Qualitätsmerkmale wie zum Beispiel Festigkeit, Dehnung, Härte, Dichte, Rheometer-Kurve an allen fertigen Rohmischungen geprüft. Die so hergestellte Rohgummimischung wird in nächstem Schritt auf einer Roller-Head-Anlage weiterverarbeitet. Der kontinuierliche Produktionsprozess beginnt mit der Extrusion, dabei wird das Material mithilfe von Breitspritzkopf und Kalander auf die gewünschte Dicke (0,6 – 2,5 mm) und Breite (max. 1400 mm) gebracht. Danach durchläuft die unvulkanisierte Bahn Prägewalzen. Bei der Butyl-Dichtungsbahn wird der Schriftzug „IIR“ mit eingeprägt. Im weiteren Prozessverlauf wird die so geformte Bahn in einem Heißluftkanal in einem kontinuierlichen Prozess vulkanisiert (vernetzt). Nach der Vulkanisation wird die Bahn über eine Abkühlstrecke auf Raumtemperatur gebracht und als Rollenware aufgewickelt. Bei Bedarf können die Bahnen vorkonfektioniert werden. Die Entwicklung und Herstellung erfolgt gemäß den Anforderungen des Qualitätsmanagementsystems nach /DIN EN ISO 9001:2008/. Die Qualität der fertigen Produkte wird regelmäßig durch die werkseigene Produktionskontrolle und durch externe Qualitätsüberwachungen gesichert. 
Technische Daten: 
Leistungswerte des Produkts entsprechend der Leistungserklärung in Bezug auf dessen Wesentliche Merkmale gemäß - DIN EN 13859-2:2014 „Abdichtungsbahnen – Definitionen und Eigenschaften von Unterdeck- und Unterspannbahnen – Teil 2: Unterdeck- und Unterspannbahnen für WändeNovoProof® FAI 
Deklarierte Einheit: 
Die deklarierte Einheit ist 1 m² der verklebten NovoProof Dichtungsbahn FAI, inklusive Verpackungsmaterialien und Befestigungsmaterial (Klebstoff).</technologyDescriptionAndIncludedProcesses>
<technologyDescriptionAndIncludedProcesses xml:lang="en">The production of rubber compound as a material for manufacturing butyl waterproofing membranes is based on a formula which specifies the quality and quantity of raw materials used. The manufacturing process in Wadern-Büschfeld is a classic batch process. The requisite raw materials are portioned in accordance with the formula calculator into automatic weighing machines and conveyed to an internal mixer using suitable conveying equipment. The mixing process results in a homogenous rubber compound. During production, quality characteristics such as strength, elasticity, hardness, density and rheometer curve are tested on all finished compounds. The rubber compound is then processed on a roller-head plant. The continuous production process commences with extrusion, whereby the material achieves the desired thickness (0.6 - 2.5 mm) and width (max. 1400 mm) using a wide extrusion die and calender. The uncured sheet is run through embossing rolls where the letters “IIR” are embossed on the butyl waterproofing membranes. Another stage of the process involves curing the sheets in a continuous hot air channel (cross-linking). Curing is followed by the sheets achieving room temperature over a cooling conveyor zone and winding onto rolls. If necessary, the sheets can be pre-assembled. Development and manufacturing are in line with the requirements of the quality management system according to /DIN EN ISO 9001:2008/. The quality of the finished products is regularly assured in the form of factory production control and external quality Monitoring. 
Technical data: 
The product’s performance values correspond with the Declaration of Performance in terms of its essential properties in accordance with DIN EN 13859-2:2014 Flexible sheets for waterproofing - Definitions and characteristics of underlays - Part 2: Underlays for walls.NovoProof® FAI 
Declared unit: 
The declared unit is 1 m² adhered NovoProof® waterproofing membrane FAI, including packaging and fastening materials (adhesive).</technologyDescriptionAndIncludedProcesses>
<technologicalApplicability xml:lang="de">NovoProof® FAI wird zur dauerelastischen, luft- und wasserdampfdichten Abdichtung von Fenster- und Fassadenanschlüsse eingesetzt. Die Bahn wird dabei mit der Innenwand und/oder Fenster verklebt.</technologicalApplicability>
<technologicalApplicability xml:lang="en">NovoProof® FAI is used for establishing permanently resilient, airtight and vapour-tight waterproofing of window connections and facade joints. The sheet is adhered to the internal wall and/or window.</technologicalApplicability>
</technology>
</processInformation>
<modellingAndValidation>
<LCIMethodAndAllocation>
<typeOfDataSet>EPD</typeOfDataSet>
<referenceToLCAMethodDetails type="source data set" refObjectId="ed4b4d7c-d224-4afb-a79e-1d06f2d70f66">
<common:shortDescription xml:lang="de">Dach- und Dichtungsbahnsysteme aus Kunststoffen und Elastomeren.pdf</common:shortDescription>
</referenceToLCAMethodDetails>
<common:other>
<epd:subType xmlns="http://www.iai.kit.edu/EPD/2013">average dataset</epd:subType>
</common:other>
</LCIMethodAndAllocation>
<dataSourcesTreatmentAndRepresentativeness>
<referenceToDataSource type="source data set" refObjectId="28d74cc0-db8b-4d7e-bc44-5f6d56ce0c4a">
<common:shortDescription xml:lang="de">GaBi Database (all versions)</common:shortDescription>
</referenceToDataSource>
<referenceToDataSource type="source data set" refObjectId="9422129a-7992-4eaf-aa17-0fca36af4512">
<common:shortDescription xml:lang="de">GaBi database SP27 2015</common:shortDescription>
</referenceToDataSource>
<useAdviceForDataSet xml:lang="de">Gültigkeitsbereich: 
Die vorliegende EPD bezieht sich auf den gesamten Lebensweg einer Durchschnittsdichtungsbahn von SaarGummi Construction Deutschland der Variante FAI. Die unterschiedlichen technischen Eigenschaften werden in Kapitel 2.3 dargestellt. Die Produkte werden am SaarGummi Construction Deutschland Produktionsstandort in Wadern-Büschfeld, Deutschland, produziert. 
Systemgrenze: 
Typ der EPD: Wiege bis Werkstor – mit OptionenModule A1-A3 Die Herstellungsphase enthält die Produktion der notwendigen Rohstoffe inklusive aller Vorketten sowie der notwendigen Beschaffungstransporte. Für die Produktion der deklarierten Einheit wurden auch die hierfür notwendige elektrische und thermische Energie sowie Hilfs- und Betriebsstoffe inklusive deren Vorketten betrachtet. Anfallende Abfälle und Abwässer werden bis zu deren vollständigen Beseitigung berücksichtigt. Modul A4 Dieses Modul betrachtet die ökologischen Auswirkungen des Transportes der deklarierten Einheit vom Werkstor bis zur Baustelle. Modul A5 Hier wurden die entstehenden Umweltwirkungen bei der Entsorgung der Produktverpackungsmaterialien berücksichtigt. In diesem wird der Installationsaufwand betrachtet. Module C2-3 Die Module beinhalten die Umweltwirkungen der Abfallbehandlung am Ende der Produktnutzung sowie die zugehörigen Transporte. In Szenario 1 wird hier der Aufwand für das Aufbereiten, in Szenario 2 der Aufwand für die Verbrennung der Dichtungsbahn modelliert.Modul D Die aus der Abfallbehandlung (aus A5 und C3) resultierenden Wertströme, die wiederum potenziell als energetischer (Verbrennung mit Energierückgewinnung, Szenario 2) oder werkstofflicher Input (Recycling, Szenario 1) für ein nachgelagertes Produktsystem dienen können, werden hier als Gutschriften ausgewiesen.</useAdviceForDataSet>
<useAdviceForDataSet xml:lang="en">Scope: 
This EPD refers to the entire life cycle of an average FAI SaarGummi Construction Deutschland waterproofing membrane. The various technical characteristics are depicted in section 2.3.  The products are manufactured at the SaarGummi Construction Deutschland production facility in Wadern-Büschfeld, Germany.This document is translated from the German Environmental Product Declaration into English. It is based on the German original version EPD-DUR-20170092-IBD1-DE. The verifier has no influence on the quality of the translation. 
System boundary: 
Type of EPD: Cradle to gate – with options Modules A1-A3 The manufacturing stage involves production of the requisite raw materials including all of the upstream chains as well as the requisite procurement transport. Production of the declared unit also considered the requisite electrical and thermal energy as well as auxiliaries and consumables, including their upstream chains. Waste and waste water incurred are considered until full disposal thereof.  Module A4 This module considers the ecological impact of transporting the declared unit from the plant gate to the construction site.  Module A5 The environmental impacts incurred during the disposal of product packaging materials were taken into consideration here. Efforts associated with installation are also considered.  Modules C2-3 These modules include the environmental impacts of waste treatment at the end of life and the associated transports. In scenario 1, the efforts associated with processing are modelled while scenario 2 involves the efforts associated with incineration of the waterproofing membranes. Module D The value streams arising from waste treatment (from A5 and C3) which can in turn serve as energetic (incineration with energy recovery, scenario 2) or material input (recycling, scenario 1) for a downstream product system are indicated as credits here.</useAdviceForDataSet>
<common:other>
<epd2:referenceToOriginalEPD type="source data set" refObjectId="df326652-cec1-482f-b246-48a2da279930">
<common:shortDescription xml:lang="de">Butyl Dichtungsbahn NovoProof® (FAI).pdf</common:shortDescription>
</epd2:referenceToOriginalEPD>
</common:other>
</dataSourcesTreatmentAndRepresentativeness>
<validation>
<review type="Accredited third party review">
<common:referenceToNameOfReviewerAndInstitution uri="../contacts/d111dbec-b024-4be5-86c5-752d6eb2cf95.xml" type="contact data set" refObjectId="d111dbec-b024-4be5-86c5-752d6eb2cf95">
<common:shortDescription xml:lang="de">Institut Bauen und Umwelt e. V.</common:shortDescription>
</common:referenceToNameOfReviewerAndInstitution>
</review>
</validation>
<complianceDeclarations>
<compliance>
<common:referenceToComplianceSystem uri="../sources/b00f9ec0-7874-11e3-981f-0800200c9a66.xml" type="source data set" refObjectId="b00f9ec0-7874-11e3-981f-0800200c9a66">
<common:shortDescription xml:lang="de">DIN EN 15804</common:shortDescription>
</common:referenceToComplianceSystem>
</compliance>
<compliance>
<common:referenceToComplianceSystem uri="../sources/4f2eb655-6e44-4874-a95a-e28f5442cd4d.xml" type="source data set" refObjectId="4f2eb655-6e44-4874-a95a-e28f5442cd4d">
<common:shortDescription xml:lang="de">ISO 14025</common:shortDescription>
</common:referenceToComplianceSystem>
</compliance>
</complianceDeclarations>
</modellingAndValidation>
<administrativeInformation>
<common:commissionerAndGoal>
<common:referenceToCommissioner uri="../contacts/4a6cdd71-2102-450e-baf8-768352fb9821.xml" type="contact data set" refObjectId="4a6cdd71-2102-450e-baf8-768352fb9821">
<common:shortDescription xml:lang="de">CQLT SaarGummi Deutschland GmbH</common:shortDescription>
</common:referenceToCommissioner>
</common:commissionerAndGoal>
<dataGenerator>
<common:referenceToPersonOrEntityGeneratingTheDataSet uri="../contacts/6b539b8a-10e3-4004-8ccc-a79f169aa339.xml" type="contact data set" refObjectId="6b539b8a-10e3-4004-8ccc-a79f169aa339">
<common:shortDescription xml:lang="de">brands and values GmbH</common:shortDescription>
</common:referenceToPersonOrEntityGeneratingTheDataSet>
</dataGenerator>
<dataEntryBy>
<common:timeStamp>2017-09-11T10:14:48.81</common:timeStamp>
<common:referenceToDataSetFormat uri="../sources/a97a0155-0234-4b87-b4ce-a45da52f2a40.xml" type="source data set" refObjectId="a97a0155-0234-4b87-b4ce-a45da52f2a40">
<common:shortDescription xml:lang="de">ILCD Format</common:shortDescription>
</common:referenceToDataSetFormat>
<common:referenceToDataSetFormat uri="../sources/a29449fd-aa2f-4de8-b5d7-4b06b43c6fde.xml" type="source data set" refObjectId="a29449fd-aa2f-4de8-b5d7-4b06b43c6fde">
<common:shortDescription xml:lang="de">EPD-Datenformaterweiterungen v1.2</common:shortDescription>
<common:shortDescription xml:lang="en">EPD Data Format Extensions v1.2</common:shortDescription>
</common:referenceToDataSetFormat>
</dataEntryBy>
<publicationAndOwnership>
<common:dataSetVersion>00.14.000</common:dataSetVersion>
<common:referenceToRegistrationAuthority uri="../contacts/d111dbec-b024-4be5-86c5-752d6eb2cf95.xml" type="contact data set" refObjectId="d111dbec-b024-4be5-86c5-752d6eb2cf95">
<common:shortDescription xml:lang="de">Institut Bauen und Umwelt e. V.</common:shortDescription>
</common:referenceToRegistrationAuthority>
<common:registrationNumber>EPD-DUR-20170092-IBD1-DE</common:registrationNumber>
<common:referenceToOwnershipOfDataSet uri="../contacts/4a6cdd71-2102-450e-baf8-768352fb9821.xml" type="contact data set" refObjectId="4a6cdd71-2102-450e-baf8-768352fb9821">
<common:shortDescription xml:lang="de">CQLT SaarGummi Deutschland GmbH</common:shortDescription>
</common:referenceToOwnershipOfDataSet>
<common:copyright>true</common:copyright>
<common:licenseType>Free of charge for all users and uses</common:licenseType>
<common:accessRestrictions xml:lang="en">None</common:accessRestrictions>
<common:other>
<epd2:referenceToPublisher type="contact data set" refObjectId="d111dbec-b024-4be5-86c5-752d6eb2cf95" uri="../contacts/d111dbec-b024-4be5-86c5-752d6eb2cf95.xml">
<common:shortDescription xml:lang="de">Institut Bauen und Umwelt e. V.</common:shortDescription>
</epd2:referenceToPublisher>
</common:other>
</publicationAndOwnership>
</administrativeInformation>
<exchanges>
<exchange dataSetInternalID="0">
<referenceToFlowDataSet uri="../flows/c3def748-fd11-c94b-1e39-8fc3d6a20afe.xml" type="flow data set" refObjectId="c3def748-fd11-c94b-1e39-8fc3d6a20afe">
<common:shortDescription xml:lang="de">1 m² Durchschnittsdichtungsbahn (FAI) inkl. Verpackungsmaterialien und Befestigungsmitteln (1 m² Durchschnittsdichtungsbahn (FAI) inkl. Verpackungsmaterialien und Befestigungsmitteln)</common:shortDescription>
</referenceToFlowDataSet>
<meanAmount>1</meanAmount>
<referencesToDataSource />
</exchange>
<exchange dataSetInternalID="1">
<referenceToFlowDataSet uri="../flows/20f32be5-0398-4288-9b6d-accddd195317.xml" type="flow data set" refObjectId="20f32be5-0398-4288-9b6d-accddd195317">
<common:shortDescription xml:lang="de">Erneuerbare Primärenergie als Energieträger (PERE)</common:shortDescription>
<common:shortDescription xml:lang="en">Renewable primary energy as energy carrier (PERE)</common:shortDescription>
</referenceToFlowDataSet>
<functionType>General reminder flow</functionType>
<exchangeDirection>Input</exchangeDirection>
<common:other>
<epd:referenceToUnitGroupDataSet uri="../unitgroups/93a60a57-a3c8-11da-a746-0800200c9a66.xml" type="unit group data set" refObjectId="93a60a57-a3c8-11da-a746-0800200c9a66">
<common:shortDescription xml:lang="de">MJ</common:shortDescription>
</epd:referenceToUnitGroupDataSet>
<epd:amount epd:module="A1-A3">7.17932</epd:amount>
<epd:amount epd:module="A4">0.0209726</epd:amount>
<epd:amount epd:module="A5">0.523367</epd:amount>
<epd:amount epd:module="C2">0.0126979</epd:amount>
<epd:amount epd:module="C3" epd:scenario="S1">0.0420622</epd:amount>
<epd:amount epd:module="C3" epd:scenario="S2">0.0628688</epd:amount>
<epd:amount epd:module="D" epd:scenario="S1">-1.86103</epd:amount>
<epd:amount epd:module="D" epd:scenario="S2">-0.0572284</epd:amount>
</common:other>
</exchange>
<exchange dataSetInternalID="2">
<referenceToFlowDataSet uri="../flows/fb3ec0de-548d-4508-aea5-00b73bf6f702.xml" type="flow data set" refObjectId="fb3ec0de-548d-4508-aea5-00b73bf6f702">
<common:shortDescription xml:lang="de">Erneuerbare Primärenergie zur stofflichen Nutzung (PERM)</common:shortDescription>
<common:shortDescription xml:lang="en">Renewable primary energy resources as material utilization (PERM)</common:shortDescription>
</referenceToFlowDataSet>
<functionType>General reminder flow</functionType>
<exchangeDirection>Input</exchangeDirection>
<common:other>
<epd:referenceToUnitGroupDataSet uri="../unitgroups/93a60a57-a3c8-11da-a746-0800200c9a66.xml" type="unit group data set" refObjectId="93a60a57-a3c8-11da-a746-0800200c9a66">
<common:shortDescription xml:lang="de">MJ</common:shortDescription>
</epd:referenceToUnitGroupDataSet>
<epd:amount epd:module="A1-A3">0.0845</epd:amount>
<epd:amount epd:module="A4">0</epd:amount>
<epd:amount epd:module="A5">-0.097</epd:amount>
<epd:amount epd:module="C2">0</epd:amount>
<epd:amount epd:module="C3" epd:scenario="S1">0</epd:amount>
<epd:amount epd:module="C3" epd:scenario="S2">0</epd:amount>
<epd:amount epd:module="D" epd:scenario="S1">0</epd:amount>
<epd:amount epd:module="D" epd:scenario="S2">0</epd:amount>
</common:other>
</exchange>
<exchange dataSetInternalID="3">
<referenceToFlowDataSet uri="../flows/53f97275-fa8a-4cdd-9024-65936002acd0.xml" type="flow data set" refObjectId="53f97275-fa8a-4cdd-9024-65936002acd0">
<common:shortDescription xml:lang="de">Total erneuerbare Primärenergie (PERT)</common:shortDescription>
<common:shortDescription xml:lang="en">Total use of renewable primary energy resources (PERT)</common:shortDescription>
</referenceToFlowDataSet>
<functionType>General reminder flow</functionType>
<exchangeDirection>Input</exchangeDirection>
<common:other>
<epd:referenceToUnitGroupDataSet uri="../unitgroups/93a60a57-a3c8-11da-a746-0800200c9a66.xml" type="unit group data set" refObjectId="93a60a57-a3c8-11da-a746-0800200c9a66">
<common:shortDescription xml:lang="de">MJ</common:shortDescription>
</epd:referenceToUnitGroupDataSet>
<epd:amount epd:module="A1-A3">7.26382</epd:amount>
<epd:amount epd:module="A4">0.0209726</epd:amount>
<epd:amount epd:module="A5">0.426367</epd:amount>
<epd:amount epd:module="C2">0.0126979</epd:amount>
<epd:amount epd:module="C3" epd:scenario="S1">0.0420622</epd:amount>
<epd:amount epd:module="C3" epd:scenario="S2">0.0628688</epd:amount>
<epd:amount epd:module="D" epd:scenario="S1">-1.86103</epd:amount>
<epd:amount epd:module="D" epd:scenario="S2">-0.0572284</epd:amount>
</common:other>
</exchange>
<exchange dataSetInternalID="4">
<referenceToFlowDataSet uri="../flows/ac857178-2b45-46ec-892a-a9a4332f0372.xml" type="flow data set" refObjectId="ac857178-2b45-46ec-892a-a9a4332f0372">
<common:shortDescription xml:lang="de">Nicht-erneuerbare Primärenergie als Energieträger (PENRE)</common:shortDescription>
<common:shortDescription xml:lang="en">Non renewable primary energy as energy carrier (PENRE)</common:shortDescription>
</referenceToFlowDataSet>
<functionType>General reminder flow</functionType>
<exchangeDirection>Input</exchangeDirection>
<common:other>
<epd:referenceToUnitGroupDataSet uri="../unitgroups/93a60a57-a3c8-11da-a746-0800200c9a66.xml" type="unit group data set" refObjectId="93a60a57-a3c8-11da-a746-0800200c9a66">
<common:shortDescription xml:lang="de">MJ</common:shortDescription>
</epd:referenceToUnitGroupDataSet>
<epd:amount epd:module="A1-A3">49.8623</epd:amount>
<epd:amount epd:module="A4">0.370327</epd:amount>
<epd:amount epd:module="A5">15.8517</epd:amount>
<epd:amount epd:module="C2">0.224216</epd:amount>
<epd:amount epd:module="C3" epd:scenario="S1">27.170222</epd:amount>
<epd:amount epd:module="C3" epd:scenario="S2">0.720722</epd:amount>
<epd:amount epd:module="D" epd:scenario="S1">-34.2612</epd:amount>
<epd:amount epd:module="D" epd:scenario="S2">-24.3871</epd:amount>
</common:other>
</exchange>
<exchange dataSetInternalID="5">
<referenceToFlowDataSet uri="../flows/1421caa0-679d-4bf4-b282-0eb850ccae27.xml" type="flow data set" refObjectId="1421caa0-679d-4bf4-b282-0eb850ccae27">
<common:shortDescription xml:lang="de">Nicht-erneuerbare Primärenergie zur stofflichen Nutzung (PENRM)</common:shortDescription>
<common:shortDescription xml:lang="en">Non renewable primary energy as material utilization (PENRM)</common:shortDescription>
</referenceToFlowDataSet>
<functionType>General reminder flow</functionType>
<exchangeDirection>Input</exchangeDirection>
<common:other>
<epd:referenceToUnitGroupDataSet uri="../unitgroups/93a60a57-a3c8-11da-a746-0800200c9a66.xml" type="unit group data set" refObjectId="93a60a57-a3c8-11da-a746-0800200c9a66">
<common:shortDescription xml:lang="de">MJ</common:shortDescription>
</epd:referenceToUnitGroupDataSet>
<epd:amount epd:module="A1-A3">40.121</epd:amount>
<epd:amount epd:module="A4">0</epd:amount>
<epd:amount epd:module="A5">-1.77</epd:amount>
<epd:amount epd:module="C2">0</epd:amount>
<epd:amount epd:module="C3" epd:scenario="S1">-27.02</epd:amount>
<epd:amount epd:module="C3" epd:scenario="S2">-27.02</epd:amount>
<epd:amount epd:module="D" epd:scenario="S1">-27.02</epd:amount>
<epd:amount epd:module="D" epd:scenario="S2">0</epd:amount>
</common:other>
</exchange>
<exchange dataSetInternalID="6">
<referenceToFlowDataSet uri="../flows/06159210-646b-4c8d-8583-da9b3b95a6c1.xml" type="flow data set" refObjectId="06159210-646b-4c8d-8583-da9b3b95a6c1">
<common:shortDescription xml:lang="de">Total nicht erneuerbare Primärenergie (PENRT)</common:shortDescription>
<common:shortDescription xml:lang="en">Total use of non renewable primary energy resources (PENRT)</common:shortDescription>
</referenceToFlowDataSet>
<functionType>General reminder flow</functionType>
<exchangeDirection>Input</exchangeDirection>
<common:other>
<epd:referenceToUnitGroupDataSet uri="../unitgroups/93a60a57-a3c8-11da-a746-0800200c9a66.xml" type="unit group data set" refObjectId="93a60a57-a3c8-11da-a746-0800200c9a66">
<common:shortDescription xml:lang="de">MJ</common:shortDescription>
</epd:referenceToUnitGroupDataSet>
<epd:amount epd:module="A1-A3">89.9833</epd:amount>
<epd:amount epd:module="A4">0.370327</epd:amount>
<epd:amount epd:module="A5">14.0817</epd:amount>
<epd:amount epd:module="C2">0.224216</epd:amount>
<epd:amount epd:module="C3" epd:scenario="S1">0.150222</epd:amount>
<epd:amount epd:module="C3" epd:scenario="S2">0.720743</epd:amount>
<epd:amount epd:module="D" epd:scenario="S1">-61.2812</epd:amount>
<epd:amount epd:module="D" epd:scenario="S2">-24.3871</epd:amount>
</common:other>
</exchange>
<exchange dataSetInternalID="7">
<referenceToFlowDataSet uri="../flows/c6a1f35f-2d09-4f54-8dfb-97e502e1ce92.xml" type="flow data set" refObjectId="c6a1f35f-2d09-4f54-8dfb-97e502e1ce92">
<common:shortDescription xml:lang="de">Einsatz von Sekundärstoffen (SM)</common:shortDescription>
<common:shortDescription xml:lang="en">Use of secondary material (SM)</common:shortDescription>
</referenceToFlowDataSet>
<functionType>General reminder flow</functionType>
<exchangeDirection>Input</exchangeDirection>
<common:other>
<epd:referenceToUnitGroupDataSet uri="../unitgroups/ad38d542-3fe9-439d-9b95-2f5f7752acaf.xml" type="unit group data set" refObjectId="ad38d542-3fe9-439d-9b95-2f5f7752acaf">
<common:shortDescription xml:lang="de">kg</common:shortDescription>
</epd:referenceToUnitGroupDataSet>
<epd:amount epd:module="A1-A3">0</epd:amount>
<epd:amount epd:module="A4">0</epd:amount>
<epd:amount epd:module="A5">0</epd:amount>
<epd:amount epd:module="C2">0</epd:amount>
<epd:amount epd:module="C3" epd:scenario="S1">0</epd:amount>
<epd:amount epd:module="C3" epd:scenario="S2">0</epd:amount>
<epd:amount epd:module="D" epd:scenario="S1">0.599</epd:amount>
<epd:amount epd:module="D" epd:scenario="S2">0</epd:amount>
</common:other>
</exchange>
<exchange dataSetInternalID="8">
<referenceToFlowDataSet uri="../flows/64333088-a55f-4aa2-9a31-c10b07816787.xml" type="flow data set" refObjectId="64333088-a55f-4aa2-9a31-c10b07816787">
<common:shortDescription xml:lang="de">Erneuerbare Sekundärbrennstoffe (RSF)</common:shortDescription>
<common:shortDescription xml:lang="en">Use of renewable secondary fuels (RSF)</common:shortDescription>
</referenceToFlowDataSet>
<functionType>General reminder flow</functionType>
<exchangeDirection>Input</exchangeDirection>
<common:other>
<epd:referenceToUnitGroupDataSet uri="../unitgroups/93a60a57-a3c8-11da-a746-0800200c9a66.xml" type="unit group data set" refObjectId="93a60a57-a3c8-11da-a746-0800200c9a66">
<common:shortDescription xml:lang="de">MJ</common:shortDescription>
</epd:referenceToUnitGroupDataSet>
<epd:amount epd:module="A1-A3">0</epd:amount>
<epd:amount epd:module="A4">0</epd:amount>
<epd:amount epd:module="A5">0</epd:amount>
<epd:amount epd:module="C2">0</epd:amount>
<epd:amount epd:module="C3" epd:scenario="S1">0</epd:amount>
<epd:amount epd:module="C3" epd:scenario="S2">0</epd:amount>
<epd:amount epd:module="D" epd:scenario="S1">0</epd:amount>
<epd:amount epd:module="D" epd:scenario="S2">0</epd:amount>
</common:other>
</exchange>
<exchange dataSetInternalID="9">
<referenceToFlowDataSet uri="../flows/89def144-d39a-4287-b86f-efde453ddcb2.xml" type="flow data set" refObjectId="89def144-d39a-4287-b86f-efde453ddcb2">
<common:shortDescription xml:lang="de">Nicht erneuerbare Sekundärbrennstoffe (NRSF)</common:shortDescription>
<common:shortDescription xml:lang="en">Use of non renewable secondary fuels (NRSF)</common:shortDescription>
</referenceToFlowDataSet>
<functionType>General reminder flow</functionType>
<exchangeDirection>Input</exchangeDirection>
<common:other>
<epd:referenceToUnitGroupDataSet uri="../unitgroups/93a60a57-a3c8-11da-a746-0800200c9a66.xml" type="unit group data set" refObjectId="93a60a57-a3c8-11da-a746-0800200c9a66">
<common:shortDescription xml:lang="de">MJ</common:shortDescription>
</epd:referenceToUnitGroupDataSet>
<epd:amount epd:module="A1-A3">0</epd:amount>
<epd:amount epd:module="A4">0</epd:amount>
<epd:amount epd:module="A5">0</epd:amount>
<epd:amount epd:module="C2">0</epd:amount>
<epd:amount epd:module="C3" epd:scenario="S1">0</epd:amount>
<epd:amount epd:module="C3" epd:scenario="S2">0</epd:amount>
<epd:amount epd:module="D" epd:scenario="S1">0</epd:amount>
<epd:amount epd:module="D" epd:scenario="S2">0</epd:amount>
</common:other>
</exchange>
<exchange dataSetInternalID="10">
<referenceToFlowDataSet uri="../flows/3cf952c8-f3a4-461d-8c96-96456ca62246.xml" type="flow data set" refObjectId="3cf952c8-f3a4-461d-8c96-96456ca62246">
<common:shortDescription xml:lang="de">Einsatz von Süßwasserressourcen (FW)</common:shortDescription>
<common:shortDescription xml:lang="en">Use of net fresh water (FW)</common:shortDescription>
</referenceToFlowDataSet>
<functionType>General reminder flow</functionType>
<exchangeDirection>Input</exchangeDirection>
<common:other>
<epd:referenceToUnitGroupDataSet uri="../unitgroups/cd950537-0a98-4044-9ba7-9f9a68d0a504.xml" type="unit group data set" refObjectId="cd950537-0a98-4044-9ba7-9f9a68d0a504">
<common:shortDescription xml:lang="de">m^3</common:shortDescription>
</epd:referenceToUnitGroupDataSet>
<epd:amount epd:module="A1-A3">0.472994</epd:amount>
<epd:amount epd:module="A4">5.25318E-05</epd:amount>
<epd:amount epd:module="A5">0.0205873</epd:amount>
<epd:amount epd:module="C2">3.18056E-05</epd:amount>
<epd:amount epd:module="C3" epd:scenario="S1">6.48931E-05</epd:amount>
<epd:amount epd:module="C3" epd:scenario="S2">0.00654256</epd:amount>
<epd:amount epd:module="D" epd:scenario="S1">-0.00719157</epd:amount>
<epd:amount epd:module="D" epd:scenario="S2">-0.00079997</epd:amount>
</common:other>
</exchange>
<exchange dataSetInternalID="11">
<referenceToFlowDataSet uri="../flows/430f9e0f-59b2-46a0-8e0d-55e0e84948fc.xml" type="flow data set" refObjectId="430f9e0f-59b2-46a0-8e0d-55e0e84948fc">
<common:shortDescription xml:lang="de">Gefährlicher Abfall zur Deponie (HWD)</common:shortDescription>
<common:shortDescription xml:lang="en">Hazardous waste disposed (HWD)</common:shortDescription>
</referenceToFlowDataSet>
<functionType>General reminder flow</functionType>
<exchangeDirection>Output</exchangeDirection>
<common:other>
<epd:referenceToUnitGroupDataSet uri="../unitgroups/ad38d542-3fe9-439d-9b95-2f5f7752acaf.xml" type="unit group data set" refObjectId="ad38d542-3fe9-439d-9b95-2f5f7752acaf">
<common:shortDescription xml:lang="de">kg</common:shortDescription>
</epd:referenceToUnitGroupDataSet>
<epd:amount epd:module="A1-A3">1.86987E-07</epd:amount>
<epd:amount epd:module="A4">2.80057E-08</epd:amount>
<epd:amount epd:module="A5">7.67312E-09</epd:amount>
<epd:amount epd:module="C2">1.69561E-08</epd:amount>
<epd:amount epd:module="C3" epd:scenario="S1">9.53736E-11</epd:amount>
<epd:amount epd:module="C3" epd:scenario="S2">5.08683E-09</epd:amount>
<epd:amount epd:module="D" epd:scenario="S1">-2.97164E-07</epd:amount>
<epd:amount epd:module="D" epd:scenario="S2">-4.35766E-09</epd:amount>
</common:other>
</exchange>
<exchange dataSetInternalID="12">
<referenceToFlowDataSet uri="../flows/b29ef66b-e286-4afa-949f-62f1a7b4d7fa.xml" type="flow data set" refObjectId="b29ef66b-e286-4afa-949f-62f1a7b4d7fa">
<common:shortDescription xml:lang="de">Entsorgter nicht gefährlicher Abfall (NHWD)</common:shortDescription>
<common:shortDescription xml:lang="en">Non hazardous waste disposed (NHWD)</common:shortDescription>
</referenceToFlowDataSet>
<functionType>General reminder flow</functionType>
<exchangeDirection>Output</exchangeDirection>
<common:other>
<epd:referenceToUnitGroupDataSet uri="../unitgroups/ad38d542-3fe9-439d-9b95-2f5f7752acaf.xml" type="unit group data set" refObjectId="ad38d542-3fe9-439d-9b95-2f5f7752acaf">
<common:shortDescription xml:lang="de">kg</common:shortDescription>
</epd:referenceToUnitGroupDataSet>
<epd:amount epd:module="A1-A3">0.0262244</epd:amount>
<epd:amount epd:module="A4">3.11181E-05</epd:amount>
<epd:amount epd:module="A5">0.00393291</epd:amount>
<epd:amount epd:module="C2">1.88406E-05</epd:amount>
<epd:amount epd:module="C3" epd:scenario="S1">9.06663E-05</epd:amount>
<epd:amount epd:module="C3" epd:scenario="S2">5.65217E-06</epd:amount>
<epd:amount epd:module="D" epd:scenario="S1">-0.0247106</epd:amount>
<epd:amount epd:module="D" epd:scenario="S2">-0.00262891</epd:amount>
</common:other>
</exchange>
<exchange dataSetInternalID="13">
<referenceToFlowDataSet uri="../flows/3449546e-52ad-4b39-b809-9fb77cea8ff6.xml" type="flow data set" refObjectId="3449546e-52ad-4b39-b809-9fb77cea8ff6">
<common:shortDescription xml:lang="de">Entsorgter radioaktiver Abfall (RWD)</common:shortDescription>
<common:shortDescription xml:lang="en">Radioactive waste disposed (RWD)</common:shortDescription>
</referenceToFlowDataSet>
<functionType>General reminder flow</functionType>
<exchangeDirection>Output</exchangeDirection>
<common:other>
<epd:referenceToUnitGroupDataSet uri="../unitgroups/ad38d542-3fe9-439d-9b95-2f5f7752acaf.xml" type="unit group data set" refObjectId="ad38d542-3fe9-439d-9b95-2f5f7752acaf">
<common:shortDescription xml:lang="de">kg</common:shortDescription>
</epd:referenceToUnitGroupDataSet>
<epd:amount epd:module="A1-A3">0.0016922</epd:amount>
<epd:amount epd:module="A4">5.29466E-07</epd:amount>
<epd:amount epd:module="A5">0.00015954</epd:amount>
<epd:amount epd:module="C2">3.20567E-07</epd:amount>
<epd:amount epd:module="C3" epd:scenario="S1">2.26654E-05</epd:amount>
<epd:amount epd:module="C3" epd:scenario="S2">9.617E-08</epd:amount>
<epd:amount epd:module="D" epd:scenario="S1">-0.000442876</epd:amount>
<epd:amount epd:module="D" epd:scenario="S2">-1.30679E-05</epd:amount>
</common:other>
</exchange>
<exchange dataSetInternalID="14">
<referenceToFlowDataSet uri="../flows/a2b32f97-3fc7-4af2-b209-525bc6426f33.xml" type="flow data set" refObjectId="a2b32f97-3fc7-4af2-b209-525bc6426f33">
<common:shortDescription xml:lang="de">Komponenten für die Wiederverwendung (CRU)</common:shortDescription>
<common:shortDescription xml:lang="en">Components for re-use (CRU)</common:shortDescription>
</referenceToFlowDataSet>
<functionType>General reminder flow</functionType>
<exchangeDirection>Output</exchangeDirection>
<common:other>
<epd:referenceToUnitGroupDataSet uri="../unitgroups/ad38d542-3fe9-439d-9b95-2f5f7752acaf.xml" type="unit group data set" refObjectId="ad38d542-3fe9-439d-9b95-2f5f7752acaf">
<common:shortDescription xml:lang="de">kg</common:shortDescription>
</epd:referenceToUnitGroupDataSet>
<epd:amount epd:module="A1-A3">0</epd:amount>
<epd:amount epd:module="A4">0</epd:amount>
<epd:amount epd:module="A5">0</epd:amount>
<epd:amount epd:module="C2">0</epd:amount>
<epd:amount epd:module="C3" epd:scenario="S1">0</epd:amount>
<epd:amount epd:module="C3" epd:scenario="S2">0</epd:amount>
<epd:amount epd:module="D" epd:scenario="S1">0</epd:amount>
<epd:amount epd:module="D" epd:scenario="S2">0</epd:amount>
</common:other>
</exchange>
<exchange dataSetInternalID="15">
<referenceToFlowDataSet uri="../flows/d7fe48a5-4103-49c8-9aae-b0b5dfdbd6ae.xml" type="flow data set" refObjectId="d7fe48a5-4103-49c8-9aae-b0b5dfdbd6ae">
<common:shortDescription xml:lang="de">Stoffe zum Recycling (MFR)</common:shortDescription>
<common:shortDescription xml:lang="en">Materials for recycling (MFR)</common:shortDescription>
</referenceToFlowDataSet>
<functionType>General reminder flow</functionType>
<exchangeDirection>Output</exchangeDirection>
<common:other>
<epd:referenceToUnitGroupDataSet uri="../unitgroups/ad38d542-3fe9-439d-9b95-2f5f7752acaf.xml" type="unit group data set" refObjectId="ad38d542-3fe9-439d-9b95-2f5f7752acaf">
<common:shortDescription xml:lang="de">kg</common:shortDescription>
</epd:referenceToUnitGroupDataSet>
<epd:amount epd:module="A1-A3">0</epd:amount>
<epd:amount epd:module="A4">0</epd:amount>
<epd:amount epd:module="A5">0</epd:amount>
<epd:amount epd:module="C2">0</epd:amount>
<epd:amount epd:module="C3" epd:scenario="S1">1.1875</epd:amount>
<epd:amount epd:module="C3" epd:scenario="S2">0</epd:amount>
<epd:amount epd:module="D" epd:scenario="S1">0</epd:amount>
<epd:amount epd:module="D" epd:scenario="S2">0</epd:amount>
</common:other>
</exchange>
<exchange dataSetInternalID="16">
<referenceToFlowDataSet uri="../flows/59a9181c-3aaf-46ee-8b13-2b3723b6e447.xml" type="flow data set" refObjectId="59a9181c-3aaf-46ee-8b13-2b3723b6e447">
<common:shortDescription xml:lang="de">Stoffe für die Energierückgewinnung (MER)</common:shortDescription>
<common:shortDescription xml:lang="en">Materials for energy recovery (MER)</common:shortDescription>
</referenceToFlowDataSet>
<functionType>General reminder flow</functionType>
<exchangeDirection>Output</exchangeDirection>
<common:other>
<epd:referenceToUnitGroupDataSet uri="../unitgroups/ad38d542-3fe9-439d-9b95-2f5f7752acaf.xml" type="unit group data set" refObjectId="ad38d542-3fe9-439d-9b95-2f5f7752acaf">
<common:shortDescription xml:lang="de">kg</common:shortDescription>
</epd:referenceToUnitGroupDataSet>
<epd:amount epd:module="A1-A3">0</epd:amount>
<epd:amount epd:module="A4">0</epd:amount>
<epd:amount epd:module="A5">0</epd:amount>
<epd:amount epd:module="C2">0</epd:amount>
<epd:amount epd:module="C3" epd:scenario="S1">0</epd:amount>
<epd:amount epd:module="C3" epd:scenario="S2">0</epd:amount>
<epd:amount epd:module="D" epd:scenario="S1">0</epd:amount>
<epd:amount epd:module="D" epd:scenario="S2">0</epd:amount>
</common:other>
</exchange>
<exchange dataSetInternalID="17">
<referenceToFlowDataSet uri="../flows/4da0c987-2b76-40d6-9e9e-82a017aaaf29.xml" type="flow data set" refObjectId="4da0c987-2b76-40d6-9e9e-82a017aaaf29">
<common:shortDescription xml:lang="de">Exportierte elektrische Energie (EEE)</common:shortDescription>
<common:shortDescription xml:lang="en">Exported electrical energy (EEE)</common:shortDescription>
</referenceToFlowDataSet>
<functionType>General reminder flow</functionType>
<exchangeDirection>Output</exchangeDirection>
<common:other>
<epd:referenceToUnitGroupDataSet uri="../unitgroups/93a60a57-a3c8-11da-a746-0800200c9a66.xml" type="unit group data set" refObjectId="93a60a57-a3c8-11da-a746-0800200c9a66">
<common:shortDescription xml:lang="de">MJ</common:shortDescription>
</epd:referenceToUnitGroupDataSet>
<epd:amount epd:module="A1-A3">0</epd:amount>
<epd:amount epd:module="A4">0</epd:amount>
<epd:amount epd:module="A5">0.294</epd:amount>
<epd:amount epd:module="C2">0</epd:amount>
<epd:amount epd:module="C3" epd:scenario="S1">0</epd:amount>
<epd:amount epd:module="C3" epd:scenario="S2">4.59</epd:amount>
<epd:amount epd:module="D" epd:scenario="S1">0</epd:amount>
<epd:amount epd:module="D" epd:scenario="S2">0</epd:amount>
</common:other>
</exchange>
<exchange dataSetInternalID="18">
<referenceToFlowDataSet uri="../flows/98daf38a-7a79-46d3-9a37-2b7bd0955810.xml" type="flow data set" refObjectId="98daf38a-7a79-46d3-9a37-2b7bd0955810">
<common:shortDescription xml:lang="de">Exportierte thermische Energie (EET)</common:shortDescription>
<common:shortDescription xml:lang="en">Exported thermal energy (EET)</common:shortDescription>
</referenceToFlowDataSet>
<functionType>General reminder flow</functionType>
<exchangeDirection>Output</exchangeDirection>
<common:other>
<epd:referenceToUnitGroupDataSet uri="../unitgroups/93a60a57-a3c8-11da-a746-0800200c9a66.xml" type="unit group data set" refObjectId="93a60a57-a3c8-11da-a746-0800200c9a66">
<common:shortDescription xml:lang="de">MJ</common:shortDescription>
</epd:referenceToUnitGroupDataSet>
<epd:amount epd:module="A1-A3">0</epd:amount>
<epd:amount epd:module="A4">0</epd:amount>
<epd:amount epd:module="A5">0.676</epd:amount>
<epd:amount epd:module="C2">0</epd:amount>
<epd:amount epd:module="C3" epd:scenario="S1">0</epd:amount>
<epd:amount epd:module="C3" epd:scenario="S2">11.076</epd:amount>
<epd:amount epd:module="D" epd:scenario="S1">0</epd:amount>
<epd:amount epd:module="D" epd:scenario="S2">0</epd:amount>
</common:other>
</exchange>
</exchanges>
<LCIAResults>
<LCIAResult>
<referenceToLCIAMethodDataSet uri="../lciamethods/77e416eb-a363-4258-a04e-171d843a6460.xml" type="LCIA method data set" refObjectId="77e416eb-a363-4258-a04e-171d843a6460">
<common:shortDescription xml:lang="de">Globales Erwärmungspotenzial (GWP)</common:shortDescription>
<common:shortDescription xml:lang="en">Global warming potential (GWP)</common:shortDescription>
</referenceToLCIAMethodDataSet>
<common:other>
<epd:referenceToUnitGroupDataSet uri="../unitgroups/1ebf3012-d0db-4de2-aefd-ef30cedb0be1.xml" type="unit group data set" refObjectId="1ebf3012-d0db-4de2-aefd-ef30cedb0be1">
<common:shortDescription xml:lang="de">kg CO_(2)-Äq.</common:shortDescription>
</epd:referenceToUnitGroupDataSet>
<epd:amount epd:module="A1-A3">3.71219</epd:amount>
<epd:amount epd:module="A4">0.0267871</epd:amount>
<epd:amount epd:module="A5">0.694583</epd:amount>
<epd:amount epd:module="C2">0.016226</epd:amount>
<epd:amount epd:module="C3" epd:scenario="S1">0.00861801</epd:amount>
<epd:amount epd:module="C3" epd:scenario="S2">2.58857</epd:amount>
<epd:amount epd:module="D" epd:scenario="S1">-2.21734</epd:amount>
<epd:amount epd:module="D" epd:scenario="S2">-1.49982</epd:amount>
</common:other>
</LCIAResult>
<LCIAResult>
<referenceToLCIAMethodDataSet uri="../lciamethods/06dcd26f-025f-401a-a7c1-5e457eb54637.xml" type="LCIA method data set" refObjectId="06dcd26f-025f-401a-a7c1-5e457eb54637">
<common:shortDescription xml:lang="de">Abbau Potential der stratosphärischen Ozonschicht (ODP)</common:shortDescription>
<common:shortDescription xml:lang="en">Depletion potential of the stratospheric ozone layer (ODP)</common:shortDescription>
</referenceToLCIAMethodDataSet>
<common:other>
<epd:referenceToUnitGroupDataSet uri="../unitgroups/88054749-b0a6-47ea-a82b-dc5b29326512.xml" type="unit group data set" refObjectId="88054749-b0a6-47ea-a82b-dc5b29326512">
<common:shortDescription xml:lang="de">kg CFC11-Äq.</common:shortDescription>
</epd:referenceToUnitGroupDataSet>
<epd:amount epd:module="A1-A3">2.49198E-07</epd:amount>
<epd:amount epd:module="A4">1.23126E-13</epd:amount>
<epd:amount epd:module="A5">1.09708E-08</epd:amount>
<epd:amount epd:module="C2">7.45468E-14</epd:amount>
<epd:amount epd:module="C3" epd:scenario="S1">6.11946E-12</epd:amount>
<epd:amount epd:module="C3" epd:scenario="S2">5.55734E-10</epd:amount>
<epd:amount epd:module="D" epd:scenario="S1">-2.59062E-11</epd:amount>
<epd:amount epd:module="D" epd:scenario="S2">-6.71559E-13</epd:amount>
</common:other>
</LCIAResult>
<LCIAResult>
<referenceToLCIAMethodDataSet uri="../lciamethods/b4274add-93b7-4905-a5e4-2e878c4e4216.xml" type="LCIA method data set" refObjectId="b4274add-93b7-4905-a5e4-2e878c4e4216">
<common:shortDescription xml:lang="de">Versauerungspotenzial von Boden und Wasser (AP)</common:shortDescription>
<common:shortDescription xml:lang="en">Acidification potential of land and water (AP)</common:shortDescription>
</referenceToLCIAMethodDataSet>
<common:other>
<epd:referenceToUnitGroupDataSet uri="../unitgroups/bc50c624-a9bc-45b1-a9b0-e6b10d00476f.xml" type="unit group data set" refObjectId="bc50c624-a9bc-45b1-a9b0-e6b10d00476f">
<common:shortDescription xml:lang="de">kg SO_(2)-Äq.</common:shortDescription>
</epd:referenceToUnitGroupDataSet>
<epd:amount epd:module="A1-A3">0.00836794</epd:amount>
<epd:amount epd:module="A4">0.000116657</epd:amount>
<epd:amount epd:module="A5">0.000952976</epd:amount>
<epd:amount epd:module="C2">0.000101378</epd:amount>
<epd:amount epd:module="C3" epd:scenario="S1">2.39954E-05</epd:amount>
<epd:amount epd:module="C3" epd:scenario="S2">0.000198207</epd:amount>
<epd:amount epd:module="D" epd:scenario="S1">-0.00278884</epd:amount>
<epd:amount epd:module="D" epd:scenario="S2">-0.00101631</epd:amount>
</common:other>
</LCIAResult>
<LCIAResult>
<referenceToLCIAMethodDataSet uri="../lciamethods/f58827d0-b407-4ec6-be75-8b69efb98a0f.xml" type="LCIA method data set" refObjectId="f58827d0-b407-4ec6-be75-8b69efb98a0f">
<common:shortDescription xml:lang="de">Eutrophierungspotenzial (EP)</common:shortDescription>
<common:shortDescription xml:lang="en">Eutrophication potential (EP)</common:shortDescription>
</referenceToLCIAMethodDataSet>
<common:other>
<epd:referenceToUnitGroupDataSet uri="../unitgroups/67b5401d-873c-485f-bcf3-6ae83b918822.xml" type="unit group data set" refObjectId="67b5401d-873c-485f-bcf3-6ae83b918822">
<common:shortDescription xml:lang="de">kg PO_(4)^(3)-Äq.</common:shortDescription>
</epd:referenceToUnitGroupDataSet>
<epd:amount epd:module="A1-A3">0.000942306</epd:amount>
<epd:amount epd:module="A4">2.85897E-05</epd:amount>
<epd:amount epd:module="A5">0.000104595</epd:amount>
<epd:amount epd:module="C2">2.54186E-05</epd:amount>
<epd:amount epd:module="C3" epd:scenario="S1">2.14693E-06</epd:amount>
<epd:amount epd:module="C3" epd:scenario="S2">4.33667E-05</epd:amount>
<epd:amount epd:module="D" epd:scenario="S1">-0.000334858</epd:amount>
<epd:amount epd:module="D" epd:scenario="S2">-0.000152232</epd:amount>
</common:other>
</LCIAResult>
<LCIAResult>
<referenceToLCIAMethodDataSet uri="../lciamethods/1e84a202-dae6-42aa-9e9d-71ea48b8be00.xml" type="LCIA method data set" refObjectId="1e84a202-dae6-42aa-9e9d-71ea48b8be00">
<common:shortDescription xml:lang="de">Bildungspotential für troposphärisches Ozon (POCP)</common:shortDescription>
<common:shortDescription xml:lang="en">Formation potential of tropospheric ozone photochemical oxidants (POCP)</common:shortDescription>
</referenceToLCIAMethodDataSet>
<common:other>
<epd:referenceToUnitGroupDataSet uri="../unitgroups/01c26c17-9a76-406e-8295-f17b55fd909e.xml" type="unit group data set" refObjectId="01c26c17-9a76-406e-8295-f17b55fd909e">
<common:shortDescription xml:lang="de">kg Ethen-Äq.</common:shortDescription>
</epd:referenceToUnitGroupDataSet>
<epd:amount epd:module="A1-A3">0.00091133</epd:amount>
<epd:amount epd:module="A4">-3.99434E-05</epd:amount>
<epd:amount epd:module="A5">0.000169796</epd:amount>
<epd:amount epd:module="C2">-4.24951E-05</epd:amount>
<epd:amount epd:module="C3" epd:scenario="S1">1.65385E-06</epd:amount>
<epd:amount epd:module="C3" epd:scenario="S2">2.25994E-05</epd:amount>
<epd:amount epd:module="D" epd:scenario="S1">-0.000484782</epd:amount>
<epd:amount epd:module="D" epd:scenario="S2">-0.000190775</epd:amount>
</common:other>
</LCIAResult>
<LCIAResult>
<referenceToLCIAMethodDataSet uri="../lciamethods/f7c73bb9-ab1a-4249-9c6d-379a0de6f67e.xml" type="LCIA method data set" refObjectId="f7c73bb9-ab1a-4249-9c6d-379a0de6f67e">
<common:shortDescription xml:lang="de">Potenzial für den abiotischen Abbau nicht fossiler Ressourcen (ADPE)</common:shortDescription>
<common:shortDescription xml:lang="en">Abiotic depletion potential for non fossil resources (ADPE)</common:shortDescription>
</referenceToLCIAMethodDataSet>
<common:other>
<epd:referenceToUnitGroupDataSet uri="../unitgroups/54ccd2d9-a32a-4fc2-923d-f2c8c93e89d4.xml" type="unit group data set" refObjectId="54ccd2d9-a32a-4fc2-923d-f2c8c93e89d4">
<common:shortDescription xml:lang="de">kg Sb-Äq.</common:shortDescription>
</epd:referenceToUnitGroupDataSet>
<epd:amount epd:module="A1-A3">1.25134E-05</epd:amount>
<epd:amount epd:module="A4">1.78385E-09</epd:amount>
<epd:amount epd:module="A5">5.8029E-07</epd:amount>
<epd:amount epd:module="C2">1.08004E-09</epd:amount>
<epd:amount epd:module="C3" epd:scenario="S1">2.81434E-09</epd:amount>
<epd:amount epd:module="C3" epd:scenario="S2">-1.83977E-08</epd:amount>
<epd:amount epd:module="D" epd:scenario="S1">-1.61286E-06</epd:amount>
<epd:amount epd:module="D" epd:scenario="S2">-6.99001E-08</epd:amount>
</common:other>
</LCIAResult>
<LCIAResult>
<referenceToLCIAMethodDataSet uri="../lciamethods/804ebcdf-309d-4098-8ed8-fdaf2f389981.xml" type="LCIA method data set" refObjectId="804ebcdf-309d-4098-8ed8-fdaf2f389981">
<common:shortDescription xml:lang="de">Potenzial für den abiotischen Abbau fossiler Brennstoffe (ADPF)</common:shortDescription>
<common:shortDescription xml:lang="en">Abiotic depletion potential for fossil resources (ADPF)</common:shortDescription>
</referenceToLCIAMethodDataSet>
<common:other>
<epd:referenceToUnitGroupDataSet uri="../unitgroups/93a60a57-a3c8-11da-a746-0800200c9a66.xml" type="unit group data set" refObjectId="93a60a57-a3c8-11da-a746-0800200c9a66">
<common:shortDescription xml:lang="de">MJ</common:shortDescription>
</epd:referenceToUnitGroupDataSet>
<epd:amount epd:module="A1-A3">85.2044</epd:amount>
<epd:amount epd:module="A4">0.36897</epd:amount>
<epd:amount epd:module="A5">13.6656</epd:amount>
<epd:amount epd:module="C2">0.223394</epd:amount>
<epd:amount epd:module="C3" epd:scenario="S1">0.0933598</epd:amount>
<epd:amount epd:module="C3" epd:scenario="S2">0.642542</epd:amount>
<epd:amount epd:module="D" epd:scenario="S1">-60.1653</epd:amount>
<epd:amount epd:module="D" epd:scenario="S2">-24.354</epd:amount>
</common:other>
</LCIAResult>
</LCIAResults>
</processDataSet>